<?xml version="1.0"?>

<!-- 
	DO NOT EDIT THIS FILE
	=====================
	
	This file is compiled from sources under [modularized](https://github.com/acoli-repo/olia/tree/master/modularized). 
	Please see [modularized/Makefile](https://github.com/acoli-repo/olia/tree/master/modularized/Makefile) for the procedure and 
	edit only the component ontologies.
	
	CHANGES APPLIED DIRECTLY TO THIS FILE MAY BE OVERWRITTEN 
	ANY TIME AND WITHOUT NOTICE.
-->

<?xml version="1.0" encoding="utf-8"?>
<rdf:RDF xmlns:owl="http://www.w3.org/2002/07/owl#" xmlns:rdf="http://www.w3.org/1999/02/22-rdf-syntax-ns#" xmlns:rdfs="http://www.w3.org/2000/01/rdf-schema#" xmlns:skos="http://www.w3.org/2004/02/skos/core#" xmlns:terms="http://purl.org/dc/terms/" xmlns:xml="http://www.w3.org/XML/1998/namespace" xmlns:xsd="http://www.w3.org/2001/XMLSchema#" xmlns="http://purl.org/olia/discourse/olia_discourse.owl#" xml:base="#">
  <rdf:Description rdf:about="http://purl.org/olia/discourse/olia_discourse.owl">
    <rdf:type rdf:resource="http://www.w3.org/2002/07/owl#Ontology"/>
  </rdf:Description>
  <rdf:Description rdf:about="http://purl.org/olia/discourse/olia_discourse.owl">
    <owl:imports rdf:resource="http://purl.org/olia/system.owl"/>
  </rdf:Description>
  <rdf:Description rdf:about="http://purl.org/olia/discourse/olia_discourse.owl">
    <owl:imports rdf:resource="http://purl.org/olia/olia-top.owl"/>
  </rdf:Description>
  <rdf:Description rdf:about="http://purl.org/olia/discourse/olia_discourse.owl">
    <rdfs:comment>OLiA Discourse: OLiA sub-vocabulary for discourse annotation, i.e.
	- discourse relations (coherence relations)
	- discourse structure
	- coreference and bridging
	- information structure

	This ontology does not extend to
	- lexical semantics (covered by extensive specialized vocabularies, e.g., WordNet, FrameNet, for which RDF instantiations already exist)
	- semantic roles (covered covered by specialized vocabularies, e.g., FrameNet, for which RDF instantiations already exist)
	- implicit semantic roles (do not require a specialized vocabulary, this is merely the intersentential application of semantic roles)
	- dialog acts (yet to come)
	- speech acts (yet to come)
	- syntax, morphosyntax, morphology (OLiA Reference Model)
	- SDRT (SDRT was initially excluded as SDRT corpora had not been available at the time when the OLiA Discourse Extensions were created)

	Selected References for Information Structure:
	- Caroline Féry, Gisbert Fanselow and Manfred Krifka (2007), Introduction, in: Féry C., G. Fanselow and M. Krifka (eds.), Interdisciplinary Studies on Information Structure 6: The Notions of Information Structure, p. 1–12
	- Tom Güldemann, Ines Fiedler, Yukiko Morimoto, Kirill Prokhorov (2010), Preposed verb doubling and predicate-centered focus. paper presented at the International Conference of the SFB 632 "Information Structure", July 9th, 2010

	References for Discourse Structure
	- annotation scheme of the RST Discourse Treebank (RSTDTB, Carlson and Marcu 2001) and general RST documentation (Mann and Thompson 1988, Mann and Taboada 2010)
	- annotation scheme of the Penn Discourse Treebank (PDTB, Prasad et al. 2007) and its adaptions for Hindi (Oza et al. 2009, HDRB), Italian (Tonelli et al. 2010, LUNA) and Arabic (Al-Saif and Markert 2010, LADTB)
	- annotation scheme of the Penn Discourse Graphbank (Wolf et al. 2003, http://www.ldc.upenn.edu/Catalog/docs/LDC2005T08/database-documentation.pdf)
	- Harry Bunt and Rashmi Prasad, ISO DR-Core (ISO 24617-8): Core Concepts for the Annotation of Discourse Relations, paper presented at ISA-12 (Note: the original ISO documentation must not be republished, so we ground all our efforts on this summary.)

	Ch. Chiarcos, christian.chiarcos@web.de</rdfs:comment>
  </rdf:Description>
  <rdf:Description rdf:about="http://purl.org/olia/discourse/olia_discourse.owl">
    <owl:versionInfo>
	2008-05-23 OLiA-InfoStruct (experimental) created, for information structure and coreference only
	
    2010-07-09 OLiA-InfoStruct (experimental) extended with respect to Féry et al. (2007)
	
    2010-07-09 OLiA-InfoStruct (experimental): subclasses of predicate-centered focus introduced in accordance with Güldemann et al. (2010)
	
    2010-10-14 OLiA-InfoStruct (experimental): subclassification of Focus and StructuralFocusType modified as suggested by Ines Fiedler (pers. comm.)
	
    2012-02-10 OLiA-InfoStruct (experimental): Sourceforge commit
	
    2014-03-20 OLiA-InfoStruct (experimental) merged with OLiA-Discourse

	


    2010-05-21 OLiA-Discourse (experimental) (experimental) created, for discourse relations and discourse structure only
	
    2010-05-21 OLiA-Discourse (experimental): RST
	
    2010-05-26 OLiA-Discourse (experimental): PDTB, RST revised
	
    2010-05-27 OLiA-Discourse (experimental): PDGB
	
    2010-05-28 OLiA-Discourse (experimental): PDTB-derived schemes
	
    2010-05-30 OLiA-Discourse (experimental): first version
	
    2012-02-10 OLiA-Discourse (experimental): Sourceforge commit
	
    2014-03-20 OLiA-Discourse (experimental): *Category to *Unit, TextOrganizationalUnit to TextStructuralUnit
	
    2014-03-21 OLiA-Discourse (experimental): DiscourseFunction, hasDiscourseFunction, PresentationalRelation, SubjectMatterRelation, EntityTypes, RelationCue
	
    2021-07-27 OLiA-Discourse (experimental): ISO discourse relations (integration primarily based on their PDTB mapping), annotation property inverseOf. Some restructuring.
	
    2021-10-11 OLiA-Discourse (experimental): minor adjustments for OWL validation
	
    2021-10-26 OLiA-Discourse (experimental): TopicContinuityRelation redefined as subclass of Expansion. This is based on the treatment of Progression in C-TED (where a novel subclass 
    EXPANSION.Progression has been introduced).
    
    2021-11-30 OLiA-Discourse (experimental): Extensions and refinement for the SemDok ontology. The ontology is part of a discourse parser. Although this is no longer available, it provides an insightful model of RST-based ontology modelling of discourse relations. For SemDok, cf. Bärenfänger, M., Lüngen, H., Hilbert, M., &amp; Lobin, H. (2010). The role of logical and generic document structure in relational discourse analysis. Kühnlein, Peter/Benz, Anton/Sidner, Candace L.: Constraints in discourse, 2, 81-104.
    
    2022-05-23 OLiA-Discourse (experimental): rdfs:labels added (automatically)

    2022-07-22 OLiA-Discourse (experimental): OWL validation

    2022-10-13 OLiA-Discourse (experimental): EntityType classification extended to common NER schemes (based on NERD ontology)

    2024-11-25 OLiA-Discourse (experimental) deprecated; integrated into modularized OLiA Reference Model

</owl:versionInfo>
  </rdf:Description>
  <rdf:Description rdf:about="http://purl.org/olia/discourse/olia_discourse.owl#inverseOf">
    <rdf:type rdf:resource="http://www.w3.org/2002/07/owl#AnnotationProperty"/>
  </rdf:Description>
  <rdf:Description rdf:about="http://purl.org/olia/discourse/olia_discourse.owl#inverseOf">
    <rdfs:comment>if two asymmetric discourse relations are equivalent in their definition and differ only in their nuclearity, they should be connected by this relation. This is used systematically to capture the dependencies between argument roles in ISO.</rdfs:comment>
  </rdf:Description>
  <rdf:Description rdf:about="http://purl.org/olia/discourse/olia_discourse.owl#inverseOf">
    <rdfs:label xml:lang="en">inverse of</rdfs:label>
  </rdf:Description>
  <rdf:Description rdf:about="http://www.w3.org/2000/01/rdf-schema#comment">
    <rdf:type rdf:resource="http://www.w3.org/2002/07/owl#AnnotationProperty"/>
  </rdf:Description>
  <rdf:Description rdf:about="http://www.w3.org/2002/07/owl#imports">
    <rdf:type rdf:resource="http://www.w3.org/2002/07/owl#AnnotationProperty"/>
  </rdf:Description>
  <rdf:Description rdf:about="http://www.w3.org/2002/07/owl#versionInfo">
    <rdf:type rdf:resource="http://www.w3.org/2002/07/owl#AnnotationProperty"/>
  </rdf:Description>
  <rdf:Description rdf:about="http://www.w3.org/2004/02/skos/core#prefLabel">
    <rdf:type rdf:resource="http://www.w3.org/2002/07/owl#AnnotationProperty"/>
  </rdf:Description>
  <rdf:Description rdf:about="http://purl.org/olia/discourse/olia_discourse.owl#denotates">
    <rdf:type rdf:resource="http://www.w3.org/2002/07/owl#ObjectProperty"/>
  </rdf:Description>
  <rdf:Description rdf:about="http://purl.org/olia/discourse/olia_discourse.owl#denotates">
    <rdfs:domain rdf:resource="http://purl.org/olia/discourse/olia_discourse.owl#Markable"/>
  </rdf:Description>
  <rdf:Description rdf:about="http://purl.org/olia/discourse/olia_discourse.owl#denotates">
    <rdfs:range rdf:resource="http://purl.org/olia/olia-top.owl#DiscourseEntity"/>
  </rdf:Description>
  <rdf:Description rdf:about="http://purl.org/olia/discourse/olia_discourse.owl#denotates">
    <rdfs:comment>Relation between linguistic expressions and their semantic content.</rdfs:comment>
  </rdf:Description>
  <rdf:Description rdf:about="http://purl.org/olia/discourse/olia_discourse.owl#denotates">
    <rdfs:label xml:lang="en">denotates</rdfs:label>
  </rdf:Description>
  <rdf:Description rdf:about="http://purl.org/olia/discourse/olia_discourse.owl#hasAttributionSource">
    <rdf:type rdf:resource="http://www.w3.org/2002/07/owl#ObjectProperty"/>
  </rdf:Description>
  <rdf:Description rdf:about="http://purl.org/olia/discourse/olia_discourse.owl#hasAttributionSource">
    <rdfs:subPropertyOf rdf:resource="http://purl.org/olia/discourse/olia_discourse.owl#hasPragmaticFeature"/>
  </rdf:Description>
  <rdf:Description rdf:nodeID="genid1">
    <rdf:type rdf:resource="http://www.w3.org/2002/07/owl#Class"/>
  </rdf:Description>
  <rdf:Description rdf:nodeID="genid2">
    <rdf:first rdf:resource="http://purl.org/olia/discourse/olia_discourse.owl#DiscourseRelation"/>
  </rdf:Description>
  <rdf:Description rdf:nodeID="genid3">
    <rdf:first rdf:resource="http://purl.org/olia/discourse/olia_discourse.owl#DiscourseSegment"/>
  </rdf:Description>
  <rdf:Description rdf:nodeID="genid2">
    <rdf:rest rdf:nodeID="genid3"/>
  </rdf:Description>
  <rdf:Description rdf:nodeID="genid3">
    <rdf:rest rdf:resource="http://www.w3.org/1999/02/22-rdf-syntax-ns#nil"/>
  </rdf:Description>
  <rdf:Description rdf:nodeID="genid1">
    <owl:unionOf rdf:nodeID="genid2"/>
  </rdf:Description>
  <rdf:Description rdf:about="http://purl.org/olia/discourse/olia_discourse.owl#hasAttributionSource">
    <rdfs:domain rdf:nodeID="genid1"/>
  </rdf:Description>
  <rdf:Description rdf:about="http://purl.org/olia/discourse/olia_discourse.owl#hasAttributionSource">
    <rdfs:range rdf:resource="http://purl.org/olia/discourse/olia_discourse.owl#AttributionSource"/>
  </rdf:Description>
  <rdf:Description rdf:about="http://purl.org/olia/discourse/olia_discourse.owl#hasAttributionSource">
    <rdfs:label xml:lang="en">has attribution source</rdfs:label>
  </rdf:Description>
  <rdf:Description rdf:about="http://purl.org/olia/discourse/olia_discourse.owl#hasBridgingType">
    <rdf:type rdf:resource="http://www.w3.org/2002/07/owl#ObjectProperty"/>
  </rdf:Description>
  <rdf:Description rdf:about="http://purl.org/olia/discourse/olia_discourse.owl#hasBridgingType">
    <rdfs:subPropertyOf rdf:resource="http://purl.org/olia/discourse/olia_discourse.owl#hasPragmaticFeature"/>
  </rdf:Description>
  <rdf:Description rdf:nodeID="genid4">
    <rdf:type rdf:resource="http://www.w3.org/2002/07/owl#Class"/>
  </rdf:Description>
  <rdf:Description rdf:nodeID="genid5">
    <rdf:first rdf:resource="http://purl.org/olia/discourse/olia_discourse.owl#BridgingRelation"/>
  </rdf:Description>
  <rdf:Description rdf:nodeID="genid6">
    <rdf:first rdf:resource="http://purl.org/olia/discourse/olia_discourse.owl#ReferringExpression"/>
  </rdf:Description>
  <rdf:Description rdf:nodeID="genid5">
    <rdf:rest rdf:nodeID="genid6"/>
  </rdf:Description>
  <rdf:Description rdf:nodeID="genid6">
    <rdf:rest rdf:resource="http://www.w3.org/1999/02/22-rdf-syntax-ns#nil"/>
  </rdf:Description>
  <rdf:Description rdf:nodeID="genid4">
    <owl:unionOf rdf:nodeID="genid5"/>
  </rdf:Description>
  <rdf:Description rdf:about="http://purl.org/olia/discourse/olia_discourse.owl#hasBridgingType">
    <rdfs:domain rdf:nodeID="genid4"/>
  </rdf:Description>
  <rdf:Description rdf:about="http://purl.org/olia/discourse/olia_discourse.owl#hasBridgingType">
    <rdfs:range rdf:resource="http://purl.org/olia/discourse/olia_discourse.owl#BridgingType"/>
  </rdf:Description>
  <rdf:Description rdf:about="http://purl.org/olia/discourse/olia_discourse.owl#hasBridgingType">
    <rdfs:label xml:lang="en">has bridging type</rdfs:label>
  </rdf:Description>
  <rdf:Description rdf:about="http://purl.org/olia/discourse/olia_discourse.owl#hasDefiniteness">
    <rdf:type rdf:resource="http://www.w3.org/2002/07/owl#ObjectProperty"/>
  </rdf:Description>
  <rdf:Description rdf:about="http://purl.org/olia/discourse/olia_discourse.owl#hasDefiniteness">
    <rdfs:subPropertyOf rdf:resource="http://purl.org/olia/discourse/olia_discourse.owl#hasSemanticFeature"/>
  </rdf:Description>
  <rdf:Description rdf:about="http://purl.org/olia/discourse/olia_discourse.owl#hasDefiniteness">
    <rdfs:label xml:lang="en">has definiteness</rdfs:label>
  </rdf:Description>
  <rdf:Description rdf:about="http://purl.org/olia/discourse/olia_discourse.owl#hasPragmaticFeature">
    <rdf:type rdf:resource="http://www.w3.org/2002/07/owl#ObjectProperty"/>
  </rdf:Description>
  <rdf:Description rdf:nodeID="genid7">
    <rdf:type rdf:resource="http://www.w3.org/2002/07/owl#Class"/>
  </rdf:Description>
  <rdf:Description rdf:nodeID="genid8">
    <rdf:first rdf:resource="http://purl.org/olia/olia-top.owl#DiscourseEntity"/>
  </rdf:Description>
  <rdf:Description rdf:nodeID="genid9">
    <rdf:first rdf:resource="http://purl.org/olia/discourse/olia_discourse.owl#Markable"/>
  </rdf:Description>
  <rdf:Description rdf:nodeID="genid8">
    <rdf:rest rdf:nodeID="genid9"/>
  </rdf:Description>
  <rdf:Description rdf:nodeID="genid10">
    <rdf:first rdf:resource="http://purl.org/olia/discourse/olia_discourse.owl#PragmaticRelation"/>
  </rdf:Description>
  <rdf:Description rdf:nodeID="genid9">
    <rdf:rest rdf:nodeID="genid10"/>
  </rdf:Description>
  <rdf:Description rdf:nodeID="genid10">
    <rdf:rest rdf:resource="http://www.w3.org/1999/02/22-rdf-syntax-ns#nil"/>
  </rdf:Description>
  <rdf:Description rdf:nodeID="genid7">
    <owl:unionOf rdf:nodeID="genid8"/>
  </rdf:Description>
  <rdf:Description rdf:about="http://purl.org/olia/discourse/olia_discourse.owl#hasPragmaticFeature">
    <rdfs:domain rdf:nodeID="genid7"/>
  </rdf:Description>
  <rdf:Description rdf:about="http://purl.org/olia/discourse/olia_discourse.owl#hasPragmaticFeature">
    <rdfs:range rdf:resource="http://purl.org/olia/olia-top.owl#PragmaticFeature"/>
  </rdf:Description>
  <rdf:Description rdf:about="http://purl.org/olia/discourse/olia_discourse.owl#hasPragmaticFeature">
    <rdfs:comment>Relation between discourse entities and pragmatic features, and (mediated by the denotates relationship) between markables and pragmatic features.</rdfs:comment>
  </rdf:Description>
  <rdf:Description rdf:about="http://purl.org/olia/discourse/olia_discourse.owl#hasPragmaticFeature">
    <rdfs:label xml:lang="en">has pragmatic feature</rdfs:label>
  </rdf:Description>
  <rdf:Description rdf:about="http://purl.org/olia/discourse/olia_discourse.owl#hasDiscourseFunction">
    <rdf:type rdf:resource="http://www.w3.org/2002/07/owl#ObjectProperty"/>
  </rdf:Description>
  <rdf:Description rdf:about="http://purl.org/olia/discourse/olia_discourse.owl#hasDiscourseFunction">
    <rdfs:subPropertyOf rdf:resource="http://purl.org/olia/discourse/olia_discourse.owl#hasPragmaticFeature"/>
  </rdf:Description>
  <rdf:Description rdf:about="http://purl.org/olia/discourse/olia_discourse.owl#hasDiscourseFunction">
    <rdfs:domain rdf:resource="http://purl.org/olia/discourse/olia_discourse.owl#DiscourseRelation"/>
  </rdf:Description>
  <rdf:Description rdf:about="http://purl.org/olia/discourse/olia_discourse.owl#hasDiscourseFunction">
    <rdfs:range rdf:resource="http://purl.org/olia/discourse/olia_discourse.owl#DiscourseFunction"/>
  </rdf:Description>
  <rdf:Description rdf:about="http://purl.org/olia/discourse/olia_discourse.owl#hasDiscourseFunction">
    <rdfs:label xml:lang="en">has discourse function</rdfs:label>
  </rdf:Description>
  <rdf:Description rdf:about="http://purl.org/olia/discourse/olia_discourse.owl#hasDiscourseStructuralPattern">
    <rdf:type rdf:resource="http://www.w3.org/2002/07/owl#ObjectProperty"/>
  </rdf:Description>
  <rdf:Description rdf:about="http://purl.org/olia/discourse/olia_discourse.owl#hasDiscourseStructuralPattern">
    <rdfs:subPropertyOf rdf:resource="http://purl.org/olia/discourse/olia_discourse.owl#hasPragmaticFeature"/>
  </rdf:Description>
  <rdf:Description rdf:about="http://purl.org/olia/discourse/olia_discourse.owl#hasDiscourseStructuralPattern">
    <rdfs:domain rdf:resource="http://purl.org/olia/discourse/olia_discourse.owl#DiscourseRelation"/>
  </rdf:Description>
  <rdf:Description rdf:about="http://purl.org/olia/discourse/olia_discourse.owl#hasDiscourseStructuralPattern">
    <rdfs:range rdf:resource="http://purl.org/olia/discourse/olia_discourse.owl#DiscourseStructuralPattern"/>
  </rdf:Description>
  <rdf:Description rdf:about="http://purl.org/olia/discourse/olia_discourse.owl#hasDiscourseStructuralPattern">
    <rdfs:label xml:lang="en">has discourse structural pattern</rdfs:label>
  </rdf:Description>
  <rdf:Description rdf:about="http://purl.org/olia/discourse/olia_discourse.owl#hasEntityType">
    <rdf:type rdf:resource="http://www.w3.org/2002/07/owl#ObjectProperty"/>
  </rdf:Description>
  <rdf:Description rdf:about="http://purl.org/olia/discourse/olia_discourse.owl#hasEntityType">
    <rdfs:subPropertyOf rdf:resource="http://purl.org/olia/discourse/olia_discourse.owl#hasSemanticFeature"/>
  </rdf:Description>
  <rdf:Description rdf:about="http://purl.org/olia/discourse/olia_discourse.owl#hasEntityType">
    <rdfs:label xml:lang="en">has entity type</rdfs:label>
  </rdf:Description>
  <rdf:Description rdf:about="http://purl.org/olia/discourse/olia_discourse.owl#hasFactuality">
    <rdf:type rdf:resource="http://www.w3.org/2002/07/owl#ObjectProperty"/>
  </rdf:Description>
  <rdf:Description rdf:about="http://purl.org/olia/discourse/olia_discourse.owl#hasFactuality">
    <rdfs:subPropertyOf rdf:resource="http://purl.org/olia/discourse/olia_discourse.owl#hasSemanticFeature"/>
  </rdf:Description>
  <rdf:Description rdf:about="http://purl.org/olia/discourse/olia_discourse.owl#hasFactuality">
    <rdfs:label xml:lang="en">has factuality</rdfs:label>
  </rdf:Description>
  <rdf:Description rdf:about="http://purl.org/olia/discourse/olia_discourse.owl#hasInformationStatus">
    <rdf:type rdf:resource="http://www.w3.org/2002/07/owl#ObjectProperty"/>
  </rdf:Description>
  <rdf:Description rdf:about="http://purl.org/olia/discourse/olia_discourse.owl#hasInformationStatus">
    <rdfs:subPropertyOf rdf:resource="http://purl.org/olia/discourse/olia_discourse.owl#hasPragmaticFeature"/>
  </rdf:Description>
  <rdf:Description rdf:nodeID="genid11">
    <rdf:type rdf:resource="http://www.w3.org/2002/07/owl#Class"/>
  </rdf:Description>
  <rdf:Description rdf:nodeID="genid12">
    <rdf:first rdf:resource="http://purl.org/olia/discourse/olia_discourse.owl#DiscourseReferent"/>
  </rdf:Description>
  <rdf:Description rdf:nodeID="genid13">
    <rdf:first rdf:resource="http://purl.org/olia/discourse/olia_discourse.owl#ReferringExpression"/>
  </rdf:Description>
  <rdf:Description rdf:nodeID="genid12">
    <rdf:rest rdf:nodeID="genid13"/>
  </rdf:Description>
  <rdf:Description rdf:nodeID="genid13">
    <rdf:rest rdf:resource="http://www.w3.org/1999/02/22-rdf-syntax-ns#nil"/>
  </rdf:Description>
  <rdf:Description rdf:nodeID="genid11">
    <owl:unionOf rdf:nodeID="genid12"/>
  </rdf:Description>
  <rdf:Description rdf:about="http://purl.org/olia/discourse/olia_discourse.owl#hasInformationStatus">
    <rdfs:domain rdf:nodeID="genid11"/>
  </rdf:Description>
  <rdf:Description rdf:about="http://purl.org/olia/discourse/olia_discourse.owl#hasInformationStatus">
    <rdfs:range rdf:resource="http://purl.org/olia/discourse/olia_discourse.owl#InformationStatus"/>
  </rdf:Description>
  <rdf:Description rdf:about="http://purl.org/olia/discourse/olia_discourse.owl#hasInformationStatus">
    <rdfs:comment>Relation between discourse referents and information status, and (mediated by the denotates relationship) between referring expressions and information status.</rdfs:comment>
  </rdf:Description>
  <rdf:Description rdf:about="http://purl.org/olia/discourse/olia_discourse.owl#hasInformationStatus">
    <rdfs:label xml:lang="en">has information status</rdfs:label>
  </rdf:Description>
  <rdf:Description rdf:about="http://purl.org/olia/discourse/olia_discourse.owl#hasPolarity">
    <rdf:type rdf:resource="http://www.w3.org/2002/07/owl#ObjectProperty"/>
  </rdf:Description>
  <rdf:Description rdf:about="http://purl.org/olia/discourse/olia_discourse.owl#hasPolarity">
    <rdfs:subPropertyOf rdf:resource="http://purl.org/olia/discourse/olia_discourse.owl#hasSemanticFeature"/>
  </rdf:Description>
  <rdf:Description rdf:about="http://purl.org/olia/discourse/olia_discourse.owl#hasPolarity">
    <rdfs:label xml:lang="en">has polarity</rdfs:label>
  </rdf:Description>
  <rdf:Description rdf:about="http://purl.org/olia/discourse/olia_discourse.owl#hasReferentType">
    <rdf:type rdf:resource="http://www.w3.org/2002/07/owl#ObjectProperty"/>
  </rdf:Description>
  <rdf:Description rdf:about="http://purl.org/olia/discourse/olia_discourse.owl#hasReferentType">
    <rdfs:subPropertyOf rdf:resource="http://purl.org/olia/system.owl#hasFeature"/>
  </rdf:Description>
  <rdf:Description rdf:about="http://purl.org/olia/discourse/olia_discourse.owl#hasReferentType">
    <rdfs:range rdf:resource="http://purl.org/olia/olia-top.owl#ReferentTypeFeature"/>
  </rdf:Description>
  <rdf:Description rdf:about="http://purl.org/olia/discourse/olia_discourse.owl#hasReferentType">
    <owl:versionInfo>http://www.isocat.org/datcat/DC-1376 (referentType)</owl:versionInfo>
  </rdf:Description>
  <rdf:Description rdf:about="http://purl.org/olia/discourse/olia_discourse.owl#hasReferentiality">
    <rdf:type rdf:resource="http://www.w3.org/2002/07/owl#ObjectProperty"/>
  </rdf:Description>
  <rdf:Description rdf:about="http://purl.org/olia/discourse/olia_discourse.owl#hasReferentiality">
    <rdfs:subPropertyOf rdf:resource="http://purl.org/olia/discourse/olia_discourse.owl#hasSemanticFeature"/>
  </rdf:Description>
  <rdf:Description rdf:about="http://purl.org/olia/discourse/olia_discourse.owl#hasReferentiality">
    <rdfs:label xml:lang="en">has referentiality</rdfs:label>
  </rdf:Description>
  <rdf:Description rdf:about="http://purl.org/olia/discourse/olia_discourse.owl#hasRegister">
    <rdf:type rdf:resource="http://www.w3.org/2002/07/owl#ObjectProperty"/>
  </rdf:Description>
  <rdf:Description rdf:about="http://purl.org/olia/discourse/olia_discourse.owl#hasRegister">
    <rdfs:subPropertyOf rdf:resource="http://purl.org/olia/system.owl#hasFeature"/>
  </rdf:Description>
  <rdf:Description rdf:about="http://purl.org/olia/discourse/olia_discourse.owl#hasRegister">
    <rdfs:range rdf:resource="http://purl.org/olia/olia-top.owl#RegisterFeature"/>
  </rdf:Description>
  <rdf:Description rdf:about="http://purl.org/olia/discourse/olia_discourse.owl#hasRegister">
    <rdfs:comment>
                            Classification indicating the relative level of language individually assigned to a lexeme or term or to a text type.
                                (ISO12620; http://www.isocat.org/datcat/DC-1988)
                            </rdfs:comment>
  </rdf:Description>
  <rdf:Description rdf:about="http://purl.org/olia/discourse/olia_discourse.owl#hasRegister">
    <owl:versionInfo>http://www.isocat.org/datcat/DC-1988</owl:versionInfo>
  </rdf:Description>
  <rdf:Description rdf:about="http://purl.org/olia/discourse/olia_discourse.owl#hasSemanticFeature">
    <rdf:type rdf:resource="http://www.w3.org/2002/07/owl#ObjectProperty"/>
  </rdf:Description>
  <rdf:Description rdf:about="http://purl.org/olia/discourse/olia_discourse.owl#hasSemanticFeature">
    <rdfs:label xml:lang="en">has semantic feature</rdfs:label>
  </rdf:Description>
  <rdf:Description rdf:about="http://purl.org/olia/discourse/olia_discourse.owl#hasSource">
    <rdf:type rdf:resource="http://www.w3.org/2002/07/owl#ObjectProperty"/>
  </rdf:Description>
  <rdf:Description rdf:about="http://purl.org/olia/discourse/olia_discourse.owl#hasSource">
    <rdfs:subPropertyOf rdf:resource="http://www.w3.org/2002/07/owl#topObjectProperty"/>
  </rdf:Description>
  <rdf:Description rdf:about="http://purl.org/olia/discourse/olia_discourse.owl#hasSource">
    <rdfs:domain rdf:resource="http://purl.org/olia/discourse/olia_discourse.owl#PragmaticRelation"/>
  </rdf:Description>
  <rdf:Description rdf:nodeID="genid14">
    <rdf:type rdf:resource="http://www.w3.org/2002/07/owl#Class"/>
  </rdf:Description>
  <rdf:Description rdf:nodeID="genid15">
    <rdf:first rdf:resource="http://purl.org/olia/discourse/olia_discourse.owl#PragmaticUnit"/>
  </rdf:Description>
  <rdf:Description rdf:nodeID="genid16">
    <rdf:first rdf:resource="http://purl.org/olia/system.owl#UnitOfAnnotation"/>
  </rdf:Description>
  <rdf:Description rdf:nodeID="genid15">
    <rdf:rest rdf:nodeID="genid16"/>
  </rdf:Description>
  <rdf:Description rdf:nodeID="genid16">
    <rdf:rest rdf:resource="http://www.w3.org/1999/02/22-rdf-syntax-ns#nil"/>
  </rdf:Description>
  <rdf:Description rdf:nodeID="genid14">
    <owl:unionOf rdf:nodeID="genid15"/>
  </rdf:Description>
  <rdf:Description rdf:about="http://purl.org/olia/discourse/olia_discourse.owl#hasSource">
    <rdfs:range rdf:nodeID="genid14"/>
  </rdf:Description>
  <rdf:Description rdf:about="http://purl.org/olia/discourse/olia_discourse.owl#hasSource">
    <rdfs:label xml:lang="en">has source</rdfs:label>
  </rdf:Description>
  <rdf:Description rdf:about="http://purl.org/olia/discourse/olia_discourse.owl#hasStructuralFocusType">
    <rdf:type rdf:resource="http://www.w3.org/2002/07/owl#ObjectProperty"/>
  </rdf:Description>
  <rdf:Description rdf:about="http://purl.org/olia/discourse/olia_discourse.owl#hasStructuralFocusType">
    <rdfs:subPropertyOf rdf:resource="http://purl.org/olia/discourse/olia_discourse.owl#hasPragmaticFeature"/>
  </rdf:Description>
  <rdf:Description rdf:about="http://purl.org/olia/discourse/olia_discourse.owl#hasStructuralFocusType">
    <rdfs:domain rdf:resource="http://purl.org/olia/discourse/olia_discourse.owl#Focus"/>
  </rdf:Description>
  <rdf:Description rdf:about="http://purl.org/olia/discourse/olia_discourse.owl#hasStructuralFocusType">
    <rdfs:range rdf:resource="http://purl.org/olia/discourse/olia_discourse.owl#StructuralFocusType"/>
  </rdf:Description>
  <rdf:Description rdf:about="http://purl.org/olia/discourse/olia_discourse.owl#hasStructuralFocusType">
    <rdfs:label xml:lang="en">has structural focus type</rdfs:label>
  </rdf:Description>
  <rdf:Description rdf:about="http://purl.org/olia/discourse/olia_discourse.owl#hasTarget">
    <rdf:type rdf:resource="http://www.w3.org/2002/07/owl#ObjectProperty"/>
  </rdf:Description>
  <rdf:Description rdf:about="http://purl.org/olia/discourse/olia_discourse.owl#hasTarget">
    <rdfs:subPropertyOf rdf:resource="http://www.w3.org/2002/07/owl#topObjectProperty"/>
  </rdf:Description>
  <rdf:Description rdf:about="http://purl.org/olia/discourse/olia_discourse.owl#hasTarget">
    <rdfs:domain rdf:resource="http://purl.org/olia/discourse/olia_discourse.owl#PragmaticRelation"/>
  </rdf:Description>
  <rdf:Description rdf:nodeID="genid17">
    <rdf:type rdf:resource="http://www.w3.org/2002/07/owl#Class"/>
  </rdf:Description>
  <rdf:Description rdf:nodeID="genid18">
    <rdf:first rdf:resource="http://purl.org/olia/discourse/olia_discourse.owl#PragmaticUnit"/>
  </rdf:Description>
  <rdf:Description rdf:nodeID="genid19">
    <rdf:first rdf:resource="http://purl.org/olia/system.owl#UnitOfAnnotation"/>
  </rdf:Description>
  <rdf:Description rdf:nodeID="genid18">
    <rdf:rest rdf:nodeID="genid19"/>
  </rdf:Description>
  <rdf:Description rdf:nodeID="genid19">
    <rdf:rest rdf:resource="http://www.w3.org/1999/02/22-rdf-syntax-ns#nil"/>
  </rdf:Description>
  <rdf:Description rdf:nodeID="genid17">
    <owl:unionOf rdf:nodeID="genid18"/>
  </rdf:Description>
  <rdf:Description rdf:about="http://purl.org/olia/discourse/olia_discourse.owl#hasTarget">
    <rdfs:range rdf:nodeID="genid17"/>
  </rdf:Description>
  <rdf:Description rdf:about="http://purl.org/olia/discourse/olia_discourse.owl#hasTarget">
    <rdfs:label xml:lang="en">has target</rdfs:label>
  </rdf:Description>
  <rdf:Description rdf:about="http://purl.org/olia/discourse/olia_discourse.owl#hasUsage">
    <rdf:type rdf:resource="http://www.w3.org/2002/07/owl#ObjectProperty"/>
  </rdf:Description>
  <rdf:Description rdf:about="http://purl.org/olia/discourse/olia_discourse.owl#hasUsage">
    <rdfs:subPropertyOf rdf:resource="http://purl.org/olia/system.owl#hasFeature"/>
  </rdf:Description>
  <rdf:Description rdf:about="http://purl.org/olia/discourse/olia_discourse.owl#hasUsage">
    <rdfs:range rdf:resource="http://purl.org/olia/olia-top.owl#UsageAndFrequencyFeature"/>
  </rdf:Description>
  <rdf:Description rdf:about="http://purl.org/olia/discourse/olia_discourse.owl#hasUsage">
    <rdfs:comment>
                            The relative commonness with which a term occurs.
                                (ISO12620; http://www.isocat.org/datcat/DC-1965)
                            </rdfs:comment>
  </rdf:Description>
  <rdf:Description rdf:about="http://purl.org/olia/discourse/olia_discourse.owl#hasUsage">
    <owl:versionInfo>http://www.isocat.org/datcat/DC-1965</owl:versionInfo>
  </rdf:Description>
  <rdf:Description rdf:about="http://www.w3.org/2002/07/owl#topObjectProperty">
    <rdf:type rdf:resource="http://www.w3.org/2002/07/owl#ObjectProperty"/>
  </rdf:Description>
  <rdf:Description rdf:about="http://purl.org/olia/olia-top.owl#DiscourseEntity">
    <rdf:type rdf:resource="http://www.w3.org/2002/07/owl#Class"/>
  </rdf:Description>
  <rdf:Description rdf:about="http://purl.org/olia/olia-top.owl#DiscourseEntity">
    <rdfs:subClassOf rdf:resource="http://purl.org/olia/discourse/olia_discourse.owl#PragmaticUnit"/>
  </rdf:Description>
  <rdf:Description rdf:about="http://purl.org/olia/olia-top.owl#DiscourseEntity">
    <rdfs:comment>A cognitive and informational unit a hearer needs to construct in order to interpret a given stretch of discourse correctly.</rdfs:comment>
  </rdf:Description>
  <rdf:Description rdf:about="http://purl.org/olia/olia-top.owl#DiscourseEntity">
    <rdfs:comment>Often, discourse entity is used as a synonym of discourse referent (e.g., Prince 1982), but here, a more general definition is adopted for the generalization over discourse referents, propositions and discourse segments.</rdfs:comment>
  </rdf:Description>
  <rdf:Description rdf:about="http://purl.org/olia/olia-top.owl#DiscourseEntity">
    <rdfs:label xml:lang="en">discourse entity</rdfs:label>
  </rdf:Description>
  <rdf:Description rdf:about="http://purl.org/olia/olia-top.owl#LinguisticConcept">
    <rdf:type rdf:resource="http://www.w3.org/2002/07/owl#Class"/>
  </rdf:Description>
  <rdf:Description rdf:about="http://purl.org/olia/olia-top.owl#NarrativeType">
    <rdf:type rdf:resource="http://www.w3.org/2002/07/owl#Class"/>
  </rdf:Description>
  <rdf:Description rdf:about="http://purl.org/olia/olia-top.owl#NarrativeType">
    <rdfs:subClassOf rdf:resource="http://purl.org/olia/olia-top.owl#PragmaticFeature"/>
  </rdf:Description>
  <rdf:Description rdf:about="http://purl.org/olia/olia-top.owl#PragmaticFeature">
    <rdf:type rdf:resource="http://www.w3.org/2002/07/owl#Class"/>
  </rdf:Description>
  <rdf:Description rdf:about="http://purl.org/olia/olia-top.owl#PragmaticFeature">
    <rdfs:subClassOf rdf:resource="http://purl.org/olia/olia-top.owl#LinguisticConcept"/>
  </rdf:Description>
  <rdf:Description rdf:about="http://purl.org/olia/olia-top.owl#PragmaticFeature">
    <rdfs:subClassOf rdf:resource="http://purl.org/olia/system.owl#Feature"/>
  </rdf:Description>
  <rdf:Description rdf:about="http://purl.org/olia/olia-top.owl#PragmaticFeature">
    <rdfs:comment xml:lang="en">Note that "pragmatics" is used in a broad sense as opposed to semantics, hence discourse annotations are in its scope.</rdfs:comment>
  </rdf:Description>
  <rdf:Description rdf:about="http://purl.org/olia/olia-top.owl#PragmaticFeature">
    <rdfs:label xml:lang="en">pragmatic feature</rdfs:label>
  </rdf:Description>
  <rdf:Description rdf:about="http://purl.org/olia/olia-top.owl#ReferentTypeFeature">
    <rdf:type rdf:resource="http://www.w3.org/2002/07/owl#Class"/>
  </rdf:Description>
  <rdf:Description rdf:about="http://purl.org/olia/olia-top.owl#ReferentTypeFeature">
    <rdfs:subClassOf rdf:resource="http://purl.org/olia/olia-top.owl#PragmaticFeature"/>
  </rdf:Description>
  <rdf:Description rdf:about="http://purl.org/olia/olia-top.owl#RegisterFeature">
    <rdf:type rdf:resource="http://www.w3.org/2002/07/owl#Class"/>
  </rdf:Description>
  <rdf:Description rdf:about="http://purl.org/olia/olia-top.owl#RegisterFeature">
    <rdfs:subClassOf rdf:resource="http://purl.org/olia/olia-top.owl#PragmaticFeature"/>
  </rdf:Description>
  <rdf:Description rdf:about="http://purl.org/olia/olia-top.owl#TextStructuralUnit">
    <rdf:type rdf:resource="http://www.w3.org/2002/07/owl#Class"/>
  </rdf:Description>
  <rdf:Description rdf:about="http://purl.org/olia/olia-top.owl#TextStructuralUnit">
    <rdfs:subClassOf rdf:resource="http://purl.org/olia/olia-top.owl#LinguisticConcept"/>
  </rdf:Description>
  <rdf:Description rdf:about="http://purl.org/olia/olia-top.owl#TextStructuralUnit">
    <rdfs:comment>
            Text structure relates to the physical features of text as it is laid out for reading. This includes the arrangement of sentences and paragraphs, and other aspects of the ordering of information in reading materials.
            (https://psychology.wikia.org/wiki/Text_structure)
        </rdfs:comment>
  </rdf:Description>
  <rdf:Description rdf:about="http://purl.org/olia/olia-top.owl#TextStructuralUnit">
    <rdfs:comment>Structural elements of the organization of a text, such as a title, author, signature block, or the body of the text itself.
(Carlson and Marcu 2001, definition of "Schema" in Rhetorical Structure Theory, cf. Mann and Thompson 1988)</rdfs:comment>
  </rdf:Description>
  <rdf:Description rdf:about="http://purl.org/olia/olia-top.owl#TextStructuralUnit">
    <rdfs:label>RST Schema</rdfs:label>
  </rdf:Description>
  <rdf:Description rdf:about="http://purl.org/olia/olia-top.owl#TextStructuralUnit">
    <rdfs:label xml:lang="en">text structural unit</rdfs:label>
  </rdf:Description>
  <rdf:Description rdf:about="http://purl.org/olia/olia-top.owl#TextStructuralUnit">
    <rdfs:label>text-structural unit</rdfs:label>
  </rdf:Description>
  <rdf:Description rdf:about="http://purl.org/olia/olia-top.owl#TextStructuralUnit">
    <owl:versionInfo>extended to also serve as generalization over Boilerplate, Headline etc.</owl:versionInfo>
  </rdf:Description>
  <rdf:Description rdf:about="http://purl.org/olia/olia-top.owl#TextStructuralUnit">
    <owl:versionInfo>subClasses adopted from classification of RST schemata by Marcu and Carlson (2001)</owl:versionInfo>
  </rdf:Description>
  <rdf:Description rdf:about="http://purl.org/olia/olia-top.owl#UsageAndFrequencyFeature">
    <rdf:type rdf:resource="http://www.w3.org/2002/07/owl#Class"/>
  </rdf:Description>
  <rdf:Description rdf:about="http://purl.org/olia/olia-top.owl#UsageAndFrequencyFeature">
    <rdfs:subClassOf rdf:resource="http://purl.org/olia/olia-top.owl#PragmaticFeature"/>
  </rdf:Description>
  <rdf:Description rdf:about="http://purl.org/olia/discourse/olia_discourse.owl#AboutnessTopic">
    <rdf:type rdf:resource="http://www.w3.org/2002/07/owl#Class"/>
  </rdf:Description>
  <rdf:Description rdf:about="http://purl.org/olia/discourse/olia_discourse.owl#AboutnessTopic">
    <rdfs:subClassOf rdf:resource="http://purl.org/olia/discourse/olia_discourse.owl#Topic"/>
  </rdf:Description>
  <rdf:Description rdf:about="http://purl.org/olia/discourse/olia_discourse.owl#AboutnessTopic">
    <rdfs:comment>The entity that an utterance is construed about. (Reinhart 1982, Lambrecht 1994)</rdfs:comment>
  </rdf:Description>
  <rdf:Description rdf:about="http://purl.org/olia/discourse/olia_discourse.owl#AboutnessTopic">
    <rdfs:label xml:lang="en">aboutness topic</rdfs:label>
  </rdf:Description>
  <rdf:Description rdf:about="http://purl.org/olia/discourse/olia_discourse.owl#Abstract">
    <rdf:type rdf:resource="http://www.w3.org/2002/07/owl#Class"/>
  </rdf:Description>
  <rdf:Description rdf:about="http://purl.org/olia/discourse/olia_discourse.owl#Abstract">
    <rdfs:subClassOf rdf:resource="http://purl.org/olia/olia-top.owl#TextStructuralUnit"/>
  </rdf:Description>
  <rdf:Description rdf:about="http://purl.org/olia/discourse/olia_discourse.owl#Abstract">
    <rdfs:comment>When a separate section of a document contains an abstract or summary of the
document, this schema should be used. If, within the text of the article, a sentence or paragraph
adequately summarizes the document, then the relation SUMMARY-S or SUMMARY-N should be
selected. The schema ABSTRACT is reserved for a summary which is separate from the body of the
text itself. (Carlson and Marcu 2001)</rdfs:comment>
  </rdf:Description>
  <rdf:Description rdf:about="http://purl.org/olia/discourse/olia_discourse.owl#Abstract">
    <rdfs:label xml:lang="en">abstract</rdfs:label>
  </rdf:Description>
  <rdf:Description rdf:about="http://purl.org/olia/discourse/olia_discourse.owl#AbstractEntity">
    <rdf:type rdf:resource="http://www.w3.org/2002/07/owl#Class"/>
  </rdf:Description>
  <rdf:Description rdf:about="http://purl.org/olia/discourse/olia_discourse.owl#AbstractEntity">
    <rdfs:subClassOf rdf:resource="http://purl.org/olia/discourse/olia_discourse.owl#EntityType"/>
  </rdf:Description>
  <rdf:Description rdf:about="http://purl.org/olia/discourse/olia_discourse.owl#AbstractEntity">
    <rdfs:comment xml:lang="en">Categories specified for referring expressions (Poesio &amp; Artstein 2006): Abstract, Animate, Concrete, Person, Plan, Space, Time

It is not quite clear how Poesio and Artstein defined the category, but we assume that is applies to situations rather than entities proper. According, nerd:Event is assumed to be a sub-class.</rdfs:comment>
  </rdf:Description>
  <rdf:Description rdf:about="http://purl.org/olia/discourse/olia_discourse.owl#AbstractEntity">
    <rdfs:label xml:lang="en">abstract entity</rdfs:label>
  </rdf:Description>
  <rdf:Description rdf:about="http://purl.org/olia/discourse/olia_discourse.owl#Accessible">
    <rdf:type rdf:resource="http://www.w3.org/2002/07/owl#Class"/>
  </rdf:Description>
  <rdf:Description rdf:about="http://purl.org/olia/discourse/olia_discourse.owl#Accessible">
    <rdfs:subClassOf rdf:resource="http://purl.org/olia/discourse/olia_discourse.owl#InformationStatus"/>
  </rdf:Description>
  <rdf:Description rdf:about="http://purl.org/olia/discourse/olia_discourse.owl#Accessible">
    <rdfs:comment>A referent is accessible if it has not been previously mentioned, but the hearer has a representation of the referent at the moment the referring expression is encountered. (Prince 1988: "discourse-new, but hearer old")</rdfs:comment>
  </rdf:Description>
  <rdf:Description rdf:about="http://purl.org/olia/discourse/olia_discourse.owl#Accessible">
    <rdfs:label xml:lang="en">accessible</rdfs:label>
  </rdf:Description>
  <rdf:Description rdf:about="http://purl.org/olia/discourse/olia_discourse.owl#Achievement">
    <rdf:type rdf:resource="http://www.w3.org/2002/07/owl#Class"/>
  </rdf:Description>
  <rdf:Description rdf:about="http://purl.org/olia/discourse/olia_discourse.owl#Achievement">
    <rdfs:subClassOf rdf:resource="http://purl.org/olia/discourse/olia_discourse.owl#Consequence"/>
  </rdf:Description>
  <rdf:Description rdf:about="http://purl.org/olia/discourse/olia_discourse.owl#Achievement">
    <inverseOf rdf:resource="http://purl.org/olia/discourse/Means"/>
  </rdf:Description>
  <rdf:Description rdf:about="http://purl.org/olia/discourse/olia_discourse.owl#Achievement">
    <rdfs:comment>ISO Manner is an asymmetric discourse relation in which the means (Arg1) is a way in which the achievement (Arg2) comes about or occurs.

Corresponds to ISO Manner with argument achievement. Nucleus is the means.</rdfs:comment>
  </rdf:Description>
  <rdf:Description rdf:about="http://purl.org/olia/discourse/olia_discourse.owl#Achievement">
    <rdfs:label xml:lang="en">achievement</rdfs:label>
  </rdf:Description>
  <rdf:Description rdf:about="http://purl.org/olia/discourse/olia_discourse.owl#Active">
    <rdf:type rdf:resource="http://www.w3.org/2002/07/owl#Class"/>
  </rdf:Description>
  <rdf:Description rdf:about="http://purl.org/olia/discourse/olia_discourse.owl#Active">
    <rdfs:subClassOf rdf:resource="http://purl.org/olia/discourse/olia_discourse.owl#Given"/>
  </rdf:Description>
  <rdf:Description rdf:about="http://purl.org/olia/discourse/olia_discourse.owl#Active">
    <rdfs:comment>A referent is active if it belongs to a small group of given referents which are particularly salient ("in the focus/center of attention"), typically indicated by pronouns (Chafe 1976, cf. Gundel et al. 1993 "in focus", Levelt 1989 "in focus").</rdfs:comment>
  </rdf:Description>
  <rdf:Description rdf:about="http://purl.org/olia/discourse/olia_discourse.owl#Active">
    <rdfs:label xml:lang="en">active</rdfs:label>
  </rdf:Description>
  <rdf:Description rdf:about="http://purl.org/olia/discourse/olia_discourse.owl#Address">
    <rdf:type rdf:resource="http://www.w3.org/2002/07/owl#Class"/>
  </rdf:Description>
  <rdf:Description rdf:about="http://purl.org/olia/discourse/olia_discourse.owl#Address">
    <rdfs:subClassOf rdf:resource="http://purl.org/olia/discourse/olia_discourse.owl#ManufacturedObject"/>
  </rdf:Description>
  <rdf:Description rdf:about="http://purl.org/olia/discourse/olia_discourse.owl#Address">
    <rdfs:comment xml:lang="en">introduced as a generalization over various NERD "products" that denote different forms of or are parts of an address.</rdfs:comment>
  </rdf:Description>
  <rdf:Description rdf:about="http://purl.org/olia/discourse/olia_discourse.owl#AdministrativeRegion">
    <rdf:type rdf:resource="http://www.w3.org/2002/07/owl#Class"/>
  </rdf:Description>
  <rdf:Description rdf:about="http://purl.org/olia/discourse/olia_discourse.owl#AdministrativeRegion">
    <rdfs:subClassOf rdf:resource="http://purl.org/olia/discourse/olia_discourse.owl#PoliticalUnit"/>
  </rdf:Description>
  <rdf:Description rdf:about="http://purl.org/olia/discourse/olia_discourse.owl#AdministrativeRegion">
    <rdfs:comment xml:lang="en">for nerd:AdministrativeRegion</rdfs:comment>
  </rdf:Description>
  <rdf:Description rdf:about="http://purl.org/olia/discourse/olia_discourse.owl#AdministrativeRegion">
    <rdfs:label xml:lang="en">administrative division</rdfs:label>
  </rdf:Description>
  <rdf:Description rdf:about="http://purl.org/olia/discourse/olia_discourse.owl#AdministrativeRegion">
    <rdfs:label xml:lang="en">gouvernmental jurisdiction</rdfs:label>
  </rdf:Description>
  <rdf:Description rdf:about="http://purl.org/olia/discourse/olia_discourse.owl#AdministrativeRegion">
    <skos:prefLabel xml:lang="en">administrative region</skos:prefLabel>
  </rdf:Description>
  <rdf:Description rdf:about="http://purl.org/olia/discourse/olia_discourse.owl#AdverbialFocus">
    <rdf:type rdf:resource="http://www.w3.org/2002/07/owl#Class"/>
  </rdf:Description>
  <rdf:Description rdf:about="http://purl.org/olia/discourse/olia_discourse.owl#AdverbialFocus">
    <rdfs:subClassOf rdf:resource="http://purl.org/olia/discourse/olia_discourse.owl#ArgumentFocus"/>
  </rdf:Description>
  <rdf:Description rdf:about="http://purl.org/olia/discourse/olia_discourse.owl#AdverbialFocus">
    <rdfs:comment>Narrow focus on an adverbial. (Fiedler)</rdfs:comment>
  </rdf:Description>
  <rdf:Description rdf:about="http://purl.org/olia/discourse/olia_discourse.owl#AdverbialFocus">
    <rdfs:label xml:lang="en">adverbial focus</rdfs:label>
  </rdf:Description>
  <rdf:Description rdf:about="http://purl.org/olia/discourse/olia_discourse.owl#Aircraft">
    <rdf:type rdf:resource="http://www.w3.org/2002/07/owl#Class"/>
  </rdf:Description>
  <rdf:Description rdf:about="http://purl.org/olia/discourse/olia_discourse.owl#Aircraft">
    <rdfs:subClassOf rdf:resource="http://purl.org/olia/discourse/olia_discourse.owl#Vehicle"/>
  </rdf:Description>
  <rdf:Description rdf:about="http://purl.org/olia/discourse/olia_discourse.owl#Aircraft">
    <rdfs:comment xml:lang="en">for nerd:Aircraft</rdfs:comment>
  </rdf:Description>
  <rdf:Description rdf:about="http://purl.org/olia/discourse/olia_discourse.owl#Airline">
    <rdf:type rdf:resource="http://www.w3.org/2002/07/owl#Class"/>
  </rdf:Description>
  <rdf:Description rdf:about="http://purl.org/olia/discourse/olia_discourse.owl#Airline">
    <rdfs:subClassOf rdf:resource="http://purl.org/olia/discourse/olia_discourse.owl#Company"/>
  </rdf:Description>
  <rdf:Description rdf:about="http://purl.org/olia/discourse/olia_discourse.owl#Airline">
    <rdfs:comment xml:lang="en">for nerd:Airline, classified as Company here, but in NERD a subclass of Organozation</rdfs:comment>
  </rdf:Description>
  <rdf:Description rdf:about="http://purl.org/olia/discourse/olia_discourse.owl#Airport">
    <rdf:type rdf:resource="http://www.w3.org/2002/07/owl#Class"/>
  </rdf:Description>
  <rdf:Description rdf:about="http://purl.org/olia/discourse/olia_discourse.owl#Airport">
    <rdfs:subClassOf rdf:resource="http://purl.org/olia/discourse/olia_discourse.owl#ArchitecturalFeature"/>
  </rdf:Description>
  <rdf:Description rdf:about="http://purl.org/olia/discourse/olia_discourse.owl#Airport">
    <rdfs:comment xml:lang="en">for nerd:Airport</rdfs:comment>
  </rdf:Description>
  <rdf:Description rdf:about="http://purl.org/olia/discourse/olia_discourse.owl#Album">
    <rdf:type rdf:resource="http://www.w3.org/2002/07/owl#Class"/>
  </rdf:Description>
  <rdf:Description rdf:about="http://purl.org/olia/discourse/olia_discourse.owl#Album">
    <rdfs:subClassOf rdf:resource="http://purl.org/olia/discourse/olia_discourse.owl#MediaProduct"/>
  </rdf:Description>
  <rdf:Description rdf:about="http://purl.org/olia/discourse/olia_discourse.owl#Album">
    <rdfs:comment xml:lang="en">for nerd:Album sub nerd:Product</rdfs:comment>
  </rdf:Description>
  <rdf:Description rdf:about="http://purl.org/olia/discourse/olia_discourse.owl#Alternative">
    <rdf:type rdf:resource="http://www.w3.org/2002/07/owl#Class"/>
  </rdf:Description>
  <rdf:Description rdf:about="http://purl.org/olia/discourse/olia_discourse.owl#Alternative">
    <rdfs:subClassOf rdf:resource="http://purl.org/olia/discourse/olia_discourse.owl#Expansion"/>
  </rdf:Description>
  <rdf:Description rdf:about="http://purl.org/olia/discourse/olia_discourse.owl#Alternative">
    <rdfs:comment>The connective indicates that its two arguments denote alternative situations. (Prasad et al. 2007)</rdfs:comment>
  </rdf:Description>
  <rdf:Description rdf:about="http://purl.org/olia/discourse/olia_discourse.owl#Alternative">
    <rdfs:label xml:lang="en">alternative</rdfs:label>
  </rdf:Description>
  <rdf:Description rdf:about="http://purl.org/olia/discourse/olia_discourse.owl#AlternativeLexicalization">
    <rdf:type rdf:resource="http://www.w3.org/2002/07/owl#Class"/>
  </rdf:Description>
  <rdf:Description rdf:about="http://purl.org/olia/discourse/olia_discourse.owl#AlternativeLexicalization">
    <rdfs:subClassOf rdf:resource="http://purl.org/olia/discourse/olia_discourse.owl#RelationCue"/>
  </rdf:Description>
  <rdf:Description rdf:about="http://purl.org/olia/discourse/olia_discourse.owl#AlternativeLexicalization">
    <rdfs:comment>Alternative lexicalization: a discourse relation is inferred, but insertion of an
Implicit connective leads to redundancy in its expression due to the relation being alternatively
lexicalized by some other expression.

These are cases where a discourse relation is inferred between adjacent sentences but where providing
an Implicit connective leads to redundancy in the expression of the relation. This is because the
relation is alternatively lexicalized by some “non-connective expression”. Such expressions include
(1) those which have two parts, one referring to the relation and another anaphorically to Arg1; (2)
those which have just one part referring anaphorically to Arg1; (3) those which have just one part
referring to the relation.</rdfs:comment>
  </rdf:Description>
  <rdf:Description rdf:about="http://purl.org/olia/discourse/olia_discourse.owl#AlternativeLexicalization">
    <rdfs:label xml:lang="en">alternative lexicalization</rdfs:label>
  </rdf:Description>
  <rdf:Description rdf:about="http://purl.org/olia/discourse/olia_discourse.owl#Ambassador">
    <rdf:type rdf:resource="http://www.w3.org/2002/07/owl#Class"/>
  </rdf:Description>
  <rdf:Description rdf:about="http://purl.org/olia/discourse/olia_discourse.owl#Ambassador">
    <rdfs:subClassOf rdf:resource="http://purl.org/olia/discourse/olia_discourse.owl#Politician"/>
  </rdf:Description>
  <rdf:Description rdf:about="http://purl.org/olia/discourse/olia_discourse.owl#Ambassador">
    <rdfs:comment xml:lang="en">for nerd:Ambassador, originally sub Person, here sub Politician; cf. extractic:AMBASSADOR</rdfs:comment>
  </rdf:Description>
  <rdf:Description rdf:about="http://purl.org/olia/discourse/olia_discourse.owl#Amount">
    <rdf:type rdf:resource="http://www.w3.org/2002/07/owl#Class"/>
  </rdf:Description>
  <rdf:Description rdf:about="http://purl.org/olia/discourse/olia_discourse.owl#Amount">
    <rdfs:subClassOf rdf:resource="http://purl.org/olia/discourse/olia_discourse.owl#EntityType"/>
  </rdf:Description>
  <rdf:Description rdf:about="http://purl.org/olia/discourse/olia_discourse.owl#Amount">
    <rdfs:comment xml:lang="en">for NERD core class Amount</rdfs:comment>
  </rdf:Description>
  <rdf:Description rdf:about="http://purl.org/olia/discourse/olia_discourse.owl#Analogy_RST">
    <rdf:type rdf:resource="http://www.w3.org/2002/07/owl#Class"/>
  </rdf:Description>
  <rdf:Description rdf:about="http://purl.org/olia/discourse/olia_discourse.owl#Analogy_RST">
    <rdfs:subClassOf rdf:resource="http://purl.org/olia/discourse/olia_discourse.owl#NonContrastiveComparison"/>
  </rdf:Description>
  <rdf:Description rdf:about="http://purl.org/olia/discourse/olia_discourse.owl#Analogy_RST">
    <rdfs:comment>In an ANALOGY relation, two textual spans, often quite dissimilar, are set in correspondence in some respects. An analogy contains an inference that if two or more things agree with one another in some respects, they will probably agree in other respects.
(Carlson and Marcu 2001)</rdfs:comment>
  </rdf:Description>
  <rdf:Description rdf:about="http://purl.org/olia/discourse/olia_discourse.owl#Analogy_RST">
    <rdfs:label xml:lang="en">analogy (RST)</rdfs:label>
  </rdf:Description>
  <rdf:Description rdf:about="http://purl.org/olia/discourse/olia_discourse.owl#AnaphoricRelation">
    <rdf:type rdf:resource="http://www.w3.org/2002/07/owl#Class"/>
  </rdf:Description>
  <rdf:Description rdf:about="http://purl.org/olia/discourse/olia_discourse.owl#AnaphoricRelation">
    <rdfs:subClassOf rdf:resource="http://purl.org/olia/discourse/olia_discourse.owl#PragmaticRelation"/>
  </rdf:Description>
  <rdf:Description rdf:about="http://purl.org/olia/discourse/olia_discourse.owl#AnaphoricRelation">
    <rdfs:label xml:lang="en">anaphoric relation</rdfs:label>
  </rdf:Description>
  <rdf:Description rdf:about="http://purl.org/olia/discourse/olia_discourse.owl#Animal">
    <rdf:type rdf:resource="http://www.w3.org/2002/07/owl#Class"/>
  </rdf:Description>
  <rdf:Description rdf:about="http://purl.org/olia/discourse/olia_discourse.owl#Animal">
    <rdfs:subClassOf rdf:resource="http://purl.org/olia/discourse/olia_discourse.owl#AnimateEntity"/>
  </rdf:Description>
  <rdf:Description rdf:about="http://purl.org/olia/discourse/olia_discourse.owl#Animal">
    <rdfs:comment xml:lang="en">for NERD core class Animal</rdfs:comment>
  </rdf:Description>
  <rdf:Description rdf:about="http://purl.org/olia/discourse/olia_discourse.owl#AnimateEntity">
    <rdf:type rdf:resource="http://www.w3.org/2002/07/owl#Class"/>
  </rdf:Description>
  <rdf:Description rdf:about="http://purl.org/olia/discourse/olia_discourse.owl#AnimateEntity">
    <rdfs:subClassOf rdf:resource="http://purl.org/olia/discourse/olia_discourse.owl#ConcreteEntity"/>
  </rdf:Description>
  <rdf:Description rdf:about="http://purl.org/olia/discourse/olia_discourse.owl#AnimateEntity">
    <rdfs:label xml:lang="en">animate entity</rdfs:label>
  </rdf:Description>
  <rdf:Description rdf:about="http://purl.org/olia/discourse/olia_discourse.owl#Antithesis">
    <rdf:type rdf:resource="http://www.w3.org/2002/07/owl#Class"/>
  </rdf:Description>
  <rdf:Description rdf:nodeID="genid20">
    <rdf:type rdf:resource="http://www.w3.org/2002/07/owl#Class"/>
  </rdf:Description>
  <rdf:Description rdf:nodeID="genid21">
    <rdf:first rdf:resource="http://purl.org/olia/discourse/olia_discourse.owl#Contrast"/>
  </rdf:Description>
  <rdf:Description rdf:nodeID="genid22">
    <rdf:first rdf:resource="http://purl.org/olia/discourse/olia_discourse.owl#HypotacticDiscourseRelation"/>
  </rdf:Description>
  <rdf:Description rdf:nodeID="genid21">
    <rdf:rest rdf:nodeID="genid22"/>
  </rdf:Description>
  <rdf:Description rdf:nodeID="genid22">
    <rdf:rest rdf:resource="http://www.w3.org/1999/02/22-rdf-syntax-ns#nil"/>
  </rdf:Description>
  <rdf:Description rdf:nodeID="genid20">
    <owl:intersectionOf rdf:nodeID="genid21"/>
  </rdf:Description>
  <rdf:Description rdf:about="http://purl.org/olia/discourse/olia_discourse.owl#Antithesis">
    <owl:equivalentClass rdf:nodeID="genid20"/>
  </rdf:Description>
  <rdf:Description rdf:about="http://purl.org/olia/discourse/olia_discourse.owl#Antithesis">
    <rdfs:subClassOf rdf:resource="http://purl.org/olia/discourse/olia_discourse.owl#Contrast"/>
  </rdf:Description>
  <rdf:Description rdf:about="http://purl.org/olia/discourse/olia_discourse.owl#Antithesis">
    <rdfs:subClassOf rdf:resource="http://purl.org/olia/discourse/olia_discourse.owl#PresentationalRelation"/>
  </rdf:Description>
  <rdf:Description rdf:about="http://purl.org/olia/discourse/olia_discourse.owl#Antithesis">
    <rdfs:comment>RST: The situation presented in the nucleus comes in contrast with the situation presented in the satellite. The contrast may happen in only one or few respects, while everything else can remain the same in other respects. An ANTITHESIS relation is
always mononuclear -- it is a contrastive relation that distinguishes clearly between the nuclearity of its arguments. It differs from the mononuclear CONCESSION relation, which is characterized by a violated expectation. (Carlson and Marcu 2001)

Markers are "although", "however", and "while".

Axiomatization follows SemDok</rdfs:comment>
  </rdf:Description>
  <rdf:Description rdf:about="http://purl.org/olia/discourse/olia_discourse.owl#Antithesis">
    <rdfs:label>antithesis</rdfs:label>
  </rdf:Description>
  <rdf:Description rdf:about="http://purl.org/olia/discourse/olia_discourse.owl#Antithesis">
    <rdfs:label xml:lang="en">antithesis</rdfs:label>
  </rdf:Description>
  <rdf:Description rdf:about="http://purl.org/olia/discourse/olia_discourse.owl#Antithesis">
    <owl:versionInfo>Supersedes Antithesis_RST. Also used in SemDok.</owl:versionInfo>
  </rdf:Description>
  <rdf:Description rdf:about="http://purl.org/olia/discourse/olia_discourse.owl#Antithesis_RST">
    <rdf:type rdf:resource="http://www.w3.org/2002/07/owl#Class"/>
  </rdf:Description>
  <rdf:Description rdf:about="http://purl.org/olia/discourse/olia_discourse.owl#Antithesis_RST">
    <rdfs:subClassOf rdf:resource="http://purl.org/olia/discourse/olia_discourse.owl#Antithesis"/>
  </rdf:Description>
  <rdf:Description rdf:about="http://purl.org/olia/discourse/olia_discourse.owl#Antithesis_RST">
    <rdfs:comment>superseded by Antithesis, maintained only for backward-compatibility.</rdfs:comment>
  </rdf:Description>
  <rdf:Description rdf:about="http://purl.org/olia/discourse/olia_discourse.owl#Antithesis_RST">
    <rdfs:label xml:lang="en">antithesis (RST)</rdfs:label>
  </rdf:Description>
  <rdf:Description rdf:about="http://purl.org/olia/discourse/olia_discourse.owl#Antithesis_RST">
    <owl:deprecated rdf:datatype="http://www.w3.org/2001/XMLSchema#boolean">true</owl:deprecated>
  </rdf:Description>
  <rdf:Description rdf:about="http://purl.org/olia/discourse/olia_discourse.owl#Apellation">
    <rdf:type rdf:resource="http://www.w3.org/2002/07/owl#Class"/>
  </rdf:Description>
  <rdf:Description rdf:about="http://purl.org/olia/discourse/olia_discourse.owl#Apellation">
    <rdfs:subClassOf rdf:resource="http://purl.org/olia/discourse/olia_discourse.owl#Identifier"/>
  </rdf:Description>
  <rdf:Description rdf:about="http://purl.org/olia/discourse/olia_discourse.owl#Apellation">
    <rdfs:comment>A designation that represents an individual concept. (Sue Ellen Wright, http://www.isocat.org/datcat/DC-347)
      
      A verbal designation of an individual, unique concept, e. g. Mount Everest, Nobel Prize (https://en.wikipedia.org/wiki/Appellation_(disambiguation))
                            </rdfs:comment>
  </rdf:Description>
  <rdf:Description rdf:about="http://purl.org/olia/discourse/olia_discourse.owl#Apellation">
    <rdfs:label>apellation</rdfs:label>
  </rdf:Description>
  <rdf:Description rdf:about="http://purl.org/olia/discourse/olia_discourse.owl#Apellation">
    <owl:versionInfo>http://www.isocat.org/datcat/DC-347</owl:versionInfo>
  </rdf:Description>
  <rdf:Description rdf:about="http://purl.org/olia/discourse/olia_discourse.owl#Architect">
    <rdf:type rdf:resource="http://www.w3.org/2002/07/owl#Class"/>
  </rdf:Description>
  <rdf:Description rdf:about="http://purl.org/olia/discourse/olia_discourse.owl#Architect">
    <rdfs:subClassOf rdf:resource="http://purl.org/olia/discourse/olia_discourse.owl#Person"/>
  </rdf:Description>
  <rdf:Description rdf:about="http://purl.org/olia/discourse/olia_discourse.owl#Architect">
    <rdfs:comment xml:lang="en">for nerd:Architect. As this is not supported by an external extractor, it is deprecated.</rdfs:comment>
  </rdf:Description>
  <rdf:Description rdf:about="http://purl.org/olia/discourse/olia_discourse.owl#Architect">
    <owl:deprecated rdf:datatype="http://www.w3.org/2001/XMLSchema#boolean">true</owl:deprecated>
  </rdf:Description>
  <rdf:Description rdf:about="http://purl.org/olia/discourse/olia_discourse.owl#ArchitecturalFeature">
    <rdf:type rdf:resource="http://www.w3.org/2002/07/owl#Class"/>
  </rdf:Description>
  <rdf:Description rdf:about="http://purl.org/olia/discourse/olia_discourse.owl#ArchitecturalFeature">
    <rdfs:subClassOf rdf:resource="http://purl.org/olia/discourse/olia_discourse.owl#Space"/>
  </rdf:Description>
  <rdf:Description rdf:about="http://purl.org/olia/discourse/olia_discourse.owl#ArchitecturalFeature">
    <rdfs:comment xml:lang="en">introduced as generalization over nerd:Space subclasses that describe buildings, groups of buldings or functional spaces within cities (e.g., park, which results from landscape architecture). Unlike GeographicalFeatures (which are mostly natural) and PoliticalUnits (which are abstract), architectural features result from manual construction efforts. Note that we include roads (as a result of planned human activity, and often, construction, but not channels (all waterways are considered geographical; a channel is a natural body of water that is only redirected by means of a manual construction).</rdfs:comment>
  </rdf:Description>
  <rdf:Description rdf:about="http://purl.org/olia/discourse/olia_discourse.owl#ArgumentFocus">
    <rdf:type rdf:resource="http://www.w3.org/2002/07/owl#Class"/>
  </rdf:Description>
  <rdf:Description rdf:about="http://purl.org/olia/discourse/olia_discourse.owl#ArgumentFocus">
    <rdfs:subClassOf rdf:resource="http://purl.org/olia/discourse/olia_discourse.owl#NarrowFocus"/>
  </rdf:Description>
  <rdf:Description rdf:about="http://purl.org/olia/discourse/olia_discourse.owl#ArgumentFocus">
    <rdfs:comment>Narrow focus on one single non-verbal constituent in the focus.
Corresponding to "narrow focus"  (van Valin &amp; Lapolla 1997), or "argument focus" (Lambrecht 1994). "Term focus" as suggested by Güldemann &amp; Fiedler would be more precise (adverbials also fall in this group, but no verbs).</rdfs:comment>
  </rdf:Description>
  <rdf:Description rdf:about="http://purl.org/olia/discourse/olia_discourse.owl#ArgumentFocus">
    <rdfs:label xml:lang="en">argument focus</rdfs:label>
  </rdf:Description>
  <rdf:Description rdf:about="http://purl.org/olia/discourse/olia_discourse.owl#ArticleTopLevelSchema">
    <rdf:type rdf:resource="http://www.w3.org/2002/07/owl#Class"/>
  </rdf:Description>
  <rdf:Description rdf:about="http://purl.org/olia/discourse/olia_discourse.owl#ArticleTopLevelSchema">
    <rdfs:subClassOf rdf:resource="http://purl.org/olia/discourse/olia_discourse.owl#TextualOrganization_RST"/>
  </rdf:Description>
  <rdf:Description rdf:about="http://purl.org/olia/discourse/olia_discourse.owl#ArticleTopLevelSchema">
    <rdfs:comment>cf. SemDok ArticleTopLevelSchema</rdfs:comment>
  </rdf:Description>
  <rdf:Description rdf:about="http://purl.org/olia/discourse/olia_discourse.owl#ArticleTopLevelSchema">
    <rdfs:label xml:lang="en">article top level schema</rdfs:label>
  </rdf:Description>
  <rdf:Description rdf:about="http://purl.org/olia/discourse/olia_discourse.owl#ArticleTopLevelSchema">
    <rdfs:label>article top-level schema</rdfs:label>
  </rdf:Description>
  <rdf:Description rdf:about="http://purl.org/olia/discourse/olia_discourse.owl#Artist">
    <rdf:type rdf:resource="http://www.w3.org/2002/07/owl#Class"/>
  </rdf:Description>
  <rdf:Description rdf:about="http://purl.org/olia/discourse/olia_discourse.owl#Artist">
    <rdfs:subClassOf rdf:resource="http://purl.org/olia/discourse/olia_discourse.owl#Person"/>
  </rdf:Description>
  <rdf:Description rdf:about="http://purl.org/olia/discourse/olia_discourse.owl#Artist">
    <rdfs:comment xml:lang="en">for nerd:Artist, zemanata:artist</rdfs:comment>
  </rdf:Description>
  <rdf:Description rdf:about="http://purl.org/olia/discourse/olia_discourse.owl#Assertion">
    <rdf:type rdf:resource="http://www.w3.org/2002/07/owl#Class"/>
  </rdf:Description>
  <rdf:Description rdf:about="http://purl.org/olia/discourse/olia_discourse.owl#Assertion">
    <rdfs:subClassOf rdf:resource="http://purl.org/olia/discourse/olia_discourse.owl#PropositionalFactuality"/>
  </rdf:Description>
  <rdf:Description rdf:about="http://purl.org/olia/discourse/olia_discourse.owl#Assertion">
    <rdfs:comment>Assertion proposition AOs are associated with a communication type of attribution (“Comm” for short), conveyed by standard verbs of communication (Levin, 1993) such as say, mention, claim, argue, explain etc.
(Prasad et al. 2007)</rdfs:comment>
  </rdf:Description>
  <rdf:Description rdf:about="http://purl.org/olia/discourse/olia_discourse.owl#Assertion">
    <rdfs:label xml:lang="en">assertion</rdfs:label>
  </rdf:Description>
  <rdf:Description rdf:about="http://purl.org/olia/discourse/olia_discourse.owl#Assessment">
    <rdf:type rdf:resource="http://www.w3.org/2002/07/owl#Class"/>
  </rdf:Description>
  <rdf:Description rdf:about="http://purl.org/olia/discourse/olia_discourse.owl#Assessment">
    <rdfs:subClassOf rdf:resource="http://purl.org/olia/discourse/olia_discourse.owl#Expansion"/>
  </rdf:Description>
  <rdf:Description rdf:about="http://purl.org/olia/discourse/olia_discourse.owl#Assessment">
    <rdfs:comment>Assessment is introduced here as a generalization over RST relations like COMMENT, EVALUATION, INTERPRETATION etc. where a subjective, objective or neutral assessment of the information represented in the nucleus is expressed in the satellite. (Ch. Chiarcos)

It corresponds to SemDok InterpretativeEvaluation, except that assessment is underspecified with respect to nuclearity whereas .</rdfs:comment>
  </rdf:Description>
  <rdf:Description rdf:about="http://purl.org/olia/discourse/olia_discourse.owl#Assessment">
    <rdfs:label xml:lang="en">assessment</rdfs:label>
  </rdf:Description>
  <rdf:Description rdf:about="http://purl.org/olia/discourse/olia_discourse.owl#Assessment">
    <rdfs:label>interpretative evaluation</rdfs:label>
  </rdf:Description>
  <rdf:Description rdf:about="http://purl.org/olia/discourse/olia_discourse.owl#Assessment">
    <skos:prefLabel>assessment</skos:prefLabel>
  </rdf:Description>
  <rdf:Description rdf:about="http://purl.org/olia/discourse/olia_discourse.owl#Astronaut">
    <rdf:type rdf:resource="http://www.w3.org/2002/07/owl#Class"/>
  </rdf:Description>
  <rdf:Description rdf:about="http://purl.org/olia/discourse/olia_discourse.owl#Astronaut">
    <rdfs:subClassOf rdf:resource="http://purl.org/olia/discourse/olia_discourse.owl#Person"/>
  </rdf:Description>
  <rdf:Description rdf:about="http://purl.org/olia/discourse/olia_discourse.owl#Astronaut">
    <rdfs:comment xml:lang="en">for nerd:Astronaut. As this is not supported by an external extractor, it is deprecated.</rdfs:comment>
  </rdf:Description>
  <rdf:Description rdf:about="http://purl.org/olia/discourse/olia_discourse.owl#Astronaut">
    <owl:deprecated rdf:datatype="http://www.w3.org/2001/XMLSchema#boolean">true</owl:deprecated>
  </rdf:Description>
  <rdf:Description rdf:about="http://purl.org/olia/discourse/olia_discourse.owl#AsynchronousRelation">
    <rdf:type rdf:resource="http://www.w3.org/2002/07/owl#Class"/>
  </rdf:Description>
  <rdf:Description rdf:about="http://purl.org/olia/discourse/olia_discourse.owl#AsynchronousRelation">
    <rdfs:subClassOf rdf:resource="http://purl.org/olia/discourse/olia_discourse.owl#TemporalRelation"/>
  </rdf:Description>
  <rdf:Description rdf:about="http://purl.org/olia/discourse/olia_discourse.owl#AsynchronousRelation">
    <rdfs:comment>The situations described in the two arguments are temporally ordered. (Prasad et al. 2007)</rdfs:comment>
  </rdf:Description>
  <rdf:Description rdf:about="http://purl.org/olia/discourse/olia_discourse.owl#AsynchronousRelation">
    <rdfs:label xml:lang="en">asynchronous relation</rdfs:label>
  </rdf:Description>
  <rdf:Description rdf:about="http://purl.org/olia/discourse/olia_discourse.owl#AsynchronousRelation">
    <rdfs:label>temporal sequence</rdfs:label>
  </rdf:Description>
  <rdf:Description rdf:about="http://purl.org/olia/discourse/olia_discourse.owl#Athlete">
    <rdf:type rdf:resource="http://www.w3.org/2002/07/owl#Class"/>
  </rdf:Description>
  <rdf:Description rdf:about="http://purl.org/olia/discourse/olia_discourse.owl#Athlete">
    <rdfs:subClassOf rdf:resource="http://purl.org/olia/discourse/olia_discourse.owl#Person"/>
  </rdf:Description>
  <rdf:Description rdf:about="http://purl.org/olia/discourse/olia_discourse.owl#Athlete">
    <rdfs:comment xml:lang="en">introduced as generalization over nerd:SoccerPlayer, nerd:TennisPlayer. As these are, however, not supported by an external extractor, it is deprecated.</rdfs:comment>
  </rdf:Description>
  <rdf:Description rdf:about="http://purl.org/olia/discourse/olia_discourse.owl#Athlete">
    <owl:deprecated rdf:datatype="http://www.w3.org/2001/XMLSchema#boolean">true</owl:deprecated>
  </rdf:Description>
  <rdf:Description rdf:about="http://purl.org/olia/discourse/olia_discourse.owl#Attribution">
    <rdf:type rdf:resource="http://www.w3.org/2002/07/owl#Class"/>
  </rdf:Description>
  <rdf:Description rdf:about="http://purl.org/olia/discourse/olia_discourse.owl#Attribution">
    <rdfs:subClassOf rdf:resource="http://purl.org/olia/discourse/olia_discourse.owl#TextualOrganizationalRelation"/>
  </rdf:Description>
  <rdf:Description rdf:about="http://purl.org/olia/discourse/olia_discourse.owl#Attribution">
    <rdfs:comment>The relation of attribution is a relation of “ownership” between abstract objects and individuals
or agents. That is, attribution has to do with ascribing beliefs and assertions expressed in text to
the agent(s) holding or making them (Riloff and Wiebe, 2003; Wiebe et al., 2004, 2005).
(Prasad et al. 2007)

Instances of reported speech, both direct and indirect, should be marked for
the rhetorical relation of ATTRIBUTION. The satellite is the source of the attribution (a clause con-
taining a reporting verb, or a phrase beginning with according to), and the nucleus is the content
of the reported message (which must be in a separate clause). The ATTRIBUTION relation is also
used with cognitive predicates, to include feelings, thoughts, hopes, etc.
(Carlson and Marcu 2001)

The Satellite attributes the Nucleus to a source.
(Wolf et al. 2003)

Note that SemDok groups Attribution and Citation with Support and thus not a textual, but a presentational relation. However, we adopt the PDTB perspective in that attribution is to be modelled separately, and in accordance with its usage in text, consider it a textual device rather than a presentational relation.

cf. SemDok Attribution</rdfs:comment>
  </rdf:Description>
  <rdf:Description rdf:about="http://purl.org/olia/discourse/olia_discourse.owl#Attribution">
    <rdfs:label xml:lang="en">attribution</rdfs:label>
  </rdf:Description>
  <rdf:Description rdf:about="http://purl.org/olia/discourse/olia_discourse.owl#AttributionSource">
    <rdf:type rdf:resource="http://www.w3.org/2002/07/owl#Class"/>
  </rdf:Description>
  <rdf:Description rdf:about="http://purl.org/olia/discourse/olia_discourse.owl#AttributionSource">
    <rdfs:subClassOf rdf:resource="http://purl.org/olia/olia-top.owl#PragmaticFeature"/>
  </rdf:Description>
  <rdf:Description rdf:about="http://purl.org/olia/discourse/olia_discourse.owl#AttributionSource">
    <rdfs:comment>Classification of Attribute relations with respect to different types of agents that act as source of Attribution. (Prasad et al. 2007)</rdfs:comment>
  </rdf:Description>
  <rdf:Description rdf:about="http://purl.org/olia/discourse/olia_discourse.owl#AttributionSource">
    <rdfs:label xml:lang="en">attribution source</rdfs:label>
  </rdf:Description>
  <rdf:Description rdf:about="http://purl.org/olia/discourse/olia_discourse.owl#Author">
    <rdf:type rdf:resource="http://www.w3.org/2002/07/owl#Class"/>
  </rdf:Description>
  <rdf:Description rdf:about="http://purl.org/olia/discourse/olia_discourse.owl#Author">
    <rdfs:subClassOf rdf:resource="http://purl.org/olia/olia-top.owl#TextStructuralUnit"/>
  </rdf:Description>
  <rdf:Description rdf:about="http://purl.org/olia/discourse/olia_discourse.owl#Author">
    <rdfs:comment>Most of the time, the WSJ articles in our corpus did not include title and
author information. However, in a small number of cases, a line about the author was included at
the end of the text. In such cases, the schema Author was used to link this with the rest of the text. (Carlson and Marcu 2001)</rdfs:comment>
  </rdf:Description>
  <rdf:Description rdf:about="http://purl.org/olia/discourse/olia_discourse.owl#Author">
    <rdfs:label xml:lang="en">author</rdfs:label>
  </rdf:Description>
  <rdf:Description rdf:about="http://purl.org/olia/discourse/olia_discourse.owl#AuthorAttributionSource">
    <rdf:type rdf:resource="http://www.w3.org/2002/07/owl#Class"/>
  </rdf:Description>
  <rdf:Description rdf:about="http://purl.org/olia/discourse/olia_discourse.owl#AuthorAttributionSource">
    <rdfs:subClassOf rdf:resource="http://purl.org/olia/discourse/olia_discourse.owl#AttributionSource"/>
  </rdf:Description>
  <rdf:Description rdf:about="http://purl.org/olia/discourse/olia_discourse.owl#AuthorAttributionSource">
    <rdfs:comment>Source is writer of text (Prasad et al. 2007)</rdfs:comment>
  </rdf:Description>
  <rdf:Description rdf:about="http://purl.org/olia/discourse/olia_discourse.owl#AuthorAttributionSource">
    <rdfs:label xml:lang="en">author attribution source</rdfs:label>
  </rdf:Description>
  <rdf:Description rdf:about="http://purl.org/olia/discourse/olia_discourse.owl#Automobile">
    <rdf:type rdf:resource="http://www.w3.org/2002/07/owl#Class"/>
  </rdf:Description>
  <rdf:Description rdf:about="http://purl.org/olia/discourse/olia_discourse.owl#Automobile">
    <rdfs:subClassOf rdf:resource="http://purl.org/olia/discourse/olia_discourse.owl#Vehicle"/>
  </rdf:Description>
  <rdf:Description rdf:about="http://purl.org/olia/discourse/olia_discourse.owl#Automobile">
    <rdfs:comment xml:lang="en">for nerd:Automobile</rdfs:comment>
  </rdf:Description>
  <rdf:Description rdf:about="http://purl.org/olia/discourse/olia_discourse.owl#Automobile">
    <rdfs:label xml:lang="en">automobile model</rdfs:label>
  </rdf:Description>
  <rdf:Description rdf:about="http://purl.org/olia/discourse/olia_discourse.owl#Automobile">
    <skos:prefLabel xml:lang="en">automobile</skos:prefLabel>
  </rdf:Description>
  <rdf:Description rdf:about="http://purl.org/olia/discourse/olia_discourse.owl#Background">
    <rdf:type rdf:resource="http://www.w3.org/2002/07/owl#Class"/>
  </rdf:Description>
  <rdf:Description rdf:about="http://purl.org/olia/discourse/olia_discourse.owl#Background">
    <rdfs:subClassOf rdf:resource="http://purl.org/olia/discourse/olia_discourse.owl#Expansion"/>
  </rdf:Description>
  <rdf:Description rdf:about="http://purl.org/olia/discourse/olia_discourse.owl#Background">
    <rdfs:subClassOf rdf:resource="http://purl.org/olia/discourse/olia_discourse.owl#PresentationalRelation"/>
  </rdf:Description>
  <rdf:Description rdf:about="http://purl.org/olia/discourse/olia_discourse.owl#Background">
    <rdfs:comment>EXPANSION.Background applies when the argument that is syntactically associated with the connective describes prior eventualities which are background information of the other argument. (Al-Saif and Markert 2010)

cf. RST Background: In a BACKGROUND relation, the satellite establishes the context or the grounds with respect to which the nucleus is to be interpreted. Understanding the satellite helps the reader understand the nucleus. (Carlson and Marcu 2001)

We follow SemDok in assuming that Background is an interpersonal (presentational) relation.</rdfs:comment>
  </rdf:Description>
  <rdf:Description rdf:about="http://purl.org/olia/discourse/olia_discourse.owl#Background">
    <rdfs:label xml:lang="en">background</rdfs:label>
  </rdf:Description>
  <rdf:Description rdf:about="http://purl.org/olia/discourse/olia_discourse.owl#Background_RST">
    <rdf:type rdf:resource="http://www.w3.org/2002/07/owl#Class"/>
  </rdf:Description>
  <rdf:Description rdf:about="http://purl.org/olia/discourse/olia_discourse.owl#Background_RST">
    <rdfs:subClassOf rdf:resource="http://purl.org/olia/discourse/olia_discourse.owl#Background"/>
  </rdf:Description>
  <rdf:Description rdf:about="http://purl.org/olia/discourse/olia_discourse.owl#Background_RST">
    <rdfs:comment>In a BACKGROUND relation, the satellite establishes the context or the grounds
with respect to which the nucleus is to be interpreted. Understanding the satellite helps the reader
understand the nucleus. The satellite IS NOT the cause/reason/motivation of the situation pre-
sented in the nucleus. The reader/writer intentions are irrelevant in determining whether such a
relation holds. In contrast with the CIRCUMSTANCE relation, the information or the context of the
BACKGROUND relation is not always specified clearly or delimited sharply. Hence, the CIRCUM-
STANCE relation is stronger than BACKGROUND.
(Carlson and Marcu 2001)

Equivalent to SemDok Background. The superclass Background is more generic than the SemDok class in that it also covers the SemDok class Preparation. However, SemDoc concepts are undefined, so details are hard to make out.</rdfs:comment>
  </rdf:Description>
  <rdf:Description rdf:about="http://purl.org/olia/discourse/olia_discourse.owl#Background_RST">
    <rdfs:label xml:lang="en">background (RST)</rdfs:label>
  </rdf:Description>
  <rdf:Description rdf:about="http://purl.org/olia/discourse/olia_discourse.owl#Band">
    <rdf:type rdf:resource="http://www.w3.org/2002/07/owl#Class"/>
  </rdf:Description>
  <rdf:Description rdf:about="http://purl.org/olia/discourse/olia_discourse.owl#Band">
    <rdfs:subClassOf rdf:resource="http://purl.org/olia/discourse/olia_discourse.owl#MusicalEnsemble"/>
  </rdf:Description>
  <rdf:Description rdf:about="http://purl.org/olia/discourse/olia_discourse.owl#Band">
    <rdfs:comment xml:lang="en">for nerd:Band</rdfs:comment>
  </rdf:Description>
  <rdf:Description rdf:about="http://purl.org/olia/discourse/olia_discourse.owl#Band">
    <rdfs:label xml:lang="en">music group</rdfs:label>
  </rdf:Description>
  <rdf:Description rdf:about="http://purl.org/olia/discourse/olia_discourse.owl#Band">
    <skos:prefLabel xml:lang="en">band</skos:prefLabel>
  </rdf:Description>
  <rdf:Description rdf:about="http://purl.org/olia/discourse/olia_discourse.owl#Belief">
    <rdf:type rdf:resource="http://www.w3.org/2002/07/owl#Class"/>
  </rdf:Description>
  <rdf:Description rdf:about="http://purl.org/olia/discourse/olia_discourse.owl#Belief">
    <rdfs:subClassOf rdf:resource="http://purl.org/olia/discourse/olia_discourse.owl#PropositionalFactuality"/>
  </rdf:Description>
  <rdf:Description rdf:about="http://purl.org/olia/discourse/olia_discourse.owl#Belief">
    <rdfs:comment>Belief proposition AOs are associated with a “belief” type of attribution, conveyed by propositional attitude verbs (Hintikka, 1971) such as believe, think, expect, suppose, imagine, etc.
(Prasad et al. 2007, for PDTB)</rdfs:comment>
  </rdf:Description>
  <rdf:Description rdf:about="http://purl.org/olia/discourse/olia_discourse.owl#Belief">
    <rdfs:label xml:lang="en">belief</rdfs:label>
  </rdf:Description>
  <rdf:Description rdf:about="http://purl.org/olia/discourse/olia_discourse.owl#BenchLevelRegister">
    <rdf:type rdf:resource="http://www.w3.org/2002/07/owl#Class"/>
  </rdf:Description>
  <rdf:Description rdf:about="http://purl.org/olia/discourse/olia_discourse.owl#BenchLevelRegister">
    <rdfs:subClassOf rdf:resource="http://purl.org/olia/olia-top.owl#RegisterFeature"/>
  </rdf:Description>
  <rdf:Description rdf:about="http://purl.org/olia/discourse/olia_discourse.owl#BenchLevelRegister">
    <rdfs:comment>
                            Register of terms used in applications-oriented as opposed to theoretical or academic levels of language.
                                (ISO12620; http://www.isocat.org/datcat/DC-1989, http://www.isocat.org/datcat/DC-427)
                            </rdfs:comment>
  </rdf:Description>
  <rdf:Description rdf:about="http://purl.org/olia/discourse/olia_discourse.owl#BenchLevelRegister">
    <rdfs:label>bench-level register</rdfs:label>
  </rdf:Description>
  <rdf:Description rdf:about="http://purl.org/olia/discourse/olia_discourse.owl#BenchLevelRegister">
    <rdfs:label>shop term</rdfs:label>
  </rdf:Description>
  <rdf:Description rdf:about="http://purl.org/olia/discourse/olia_discourse.owl#BenchLevelRegister">
    <owl:versionInfo>http://www.isocat.org/datcat/DC-1989, http://www.isocat.org/datcat/DC-427</owl:versionInfo>
  </rdf:Description>
  <rdf:Description rdf:about="http://purl.org/olia/discourse/olia_discourse.owl#BenchLevelRegister">
    <owl:versionInfo>subClassOf register (dcif:conceptualDomain)</owl:versionInfo>
  </rdf:Description>
  <rdf:Description rdf:about="http://purl.org/olia/discourse/olia_discourse.owl#Bird">
    <rdf:type rdf:resource="http://www.w3.org/2002/07/owl#Class"/>
  </rdf:Description>
  <rdf:Description rdf:about="http://purl.org/olia/discourse/olia_discourse.owl#Bird">
    <rdfs:subClassOf rdf:resource="http://purl.org/olia/discourse/olia_discourse.owl#Animal"/>
  </rdf:Description>
  <rdf:Description rdf:about="http://purl.org/olia/discourse/olia_discourse.owl#Bird">
    <rdfs:comment xml:lang="en">for nerd:Bird and extractiv:BIRD</rdfs:comment>
  </rdf:Description>
  <rdf:Description rdf:about="http://purl.org/olia/discourse/olia_discourse.owl#Boilerplate">
    <rdf:type rdf:resource="http://www.w3.org/2002/07/owl#Class"/>
  </rdf:Description>
  <rdf:Description rdf:about="http://purl.org/olia/discourse/olia_discourse.owl#Boilerplate">
    <rdfs:subClassOf rdf:resource="http://purl.org/olia/olia-top.owl#TextStructuralUnit"/>
  </rdf:Description>
  <rdf:Description rdf:about="http://purl.org/olia/discourse/olia_discourse.owl#Boilerplate">
    <rdfs:comment>A fixed chunk of recurring text. (Sue Ellen Wright, http://www.isocat.org/datcat/DC-343)
    
    Boilerplate text, or simply boilerplate, is any written text (copy) that can be reused in new contexts or applications without significant changes to the original. The term is used in reference to statements, contracts and computer code ... In contract law, the term "boilerplate language" or "boilerplate clause" describes the parts of a contract that are considered standard. (https://en.wikipedia.org/wiki/Boilerplate_text)
    </rdfs:comment>
  </rdf:Description>
  <rdf:Description rdf:about="http://purl.org/olia/discourse/olia_discourse.owl#Boilerplate">
    <rdfs:label xml:lang="de">Textbaustein</rdfs:label>
  </rdf:Description>
  <rdf:Description rdf:about="http://purl.org/olia/discourse/olia_discourse.owl#Boilerplate">
    <rdfs:label>boilerplate</rdfs:label>
  </rdf:Description>
  <rdf:Description rdf:about="http://purl.org/olia/discourse/olia_discourse.owl#Boilerplate">
    <rdfs:label xml:lang="en">boilerplate text</rdfs:label>
  </rdf:Description>
  <rdf:Description rdf:about="http://purl.org/olia/discourse/olia_discourse.owl#Boilerplate">
    <rdfs:label xml:lang="en">standard text</rdfs:label>
  </rdf:Description>
  <rdf:Description rdf:about="http://purl.org/olia/discourse/olia_discourse.owl#Boilerplate">
    <owl:versionInfo>http://www.isocat.org/datcat/DC-343</owl:versionInfo>
  </rdf:Description>
  <rdf:Description rdf:about="http://purl.org/olia/discourse/olia_discourse.owl#Book">
    <rdf:type rdf:resource="http://www.w3.org/2002/07/owl#Class"/>
  </rdf:Description>
  <rdf:Description rdf:about="http://purl.org/olia/discourse/olia_discourse.owl#Book">
    <rdfs:subClassOf rdf:resource="http://purl.org/olia/discourse/olia_discourse.owl#MediaProduct"/>
  </rdf:Description>
  <rdf:Description rdf:about="http://purl.org/olia/discourse/olia_discourse.owl#Book">
    <rdfs:comment xml:lang="en">for nerd:Book sub nerd;Product</rdfs:comment>
  </rdf:Description>
  <rdf:Description rdf:about="http://purl.org/olia/discourse/olia_discourse.owl#Bridge">
    <rdf:type rdf:resource="http://www.w3.org/2002/07/owl#Class"/>
  </rdf:Description>
  <rdf:Description rdf:about="http://purl.org/olia/discourse/olia_discourse.owl#Bridge">
    <rdfs:subClassOf rdf:resource="http://purl.org/olia/discourse/olia_discourse.owl#ArchitecturalFeature"/>
  </rdf:Description>
  <rdf:Description rdf:about="http://purl.org/olia/discourse/olia_discourse.owl#Bridge">
    <rdfs:comment xml:lang="en">for nerd:Bridge</rdfs:comment>
  </rdf:Description>
  <rdf:Description rdf:about="http://purl.org/olia/discourse/olia_discourse.owl#BridgingRelation">
    <rdf:type rdf:resource="http://www.w3.org/2002/07/owl#Class"/>
  </rdf:Description>
  <rdf:Description rdf:about="http://purl.org/olia/discourse/olia_discourse.owl#BridgingRelation">
    <rdfs:subClassOf rdf:resource="http://purl.org/olia/discourse/olia_discourse.owl#PragmaticRelation"/>
  </rdf:Description>
  <rdf:Description rdf:about="http://purl.org/olia/discourse/olia_discourse.owl#BridgingRelation">
    <rdfs:comment>cf. SemDok BridgingRelation</rdfs:comment>
  </rdf:Description>
  <rdf:Description rdf:about="http://purl.org/olia/discourse/olia_discourse.owl#BridgingRelation">
    <rdfs:label>bridging relation</rdfs:label>
  </rdf:Description>
  <rdf:Description rdf:about="http://purl.org/olia/discourse/olia_discourse.owl#BridgingRelation">
    <rdfs:label xml:lang="en">bridging relation</rdfs:label>
  </rdf:Description>
  <rdf:Description rdf:about="http://purl.org/olia/discourse/olia_discourse.owl#BridgingType">
    <rdf:type rdf:resource="http://www.w3.org/2002/07/owl#Class"/>
  </rdf:Description>
  <rdf:Description rdf:about="http://purl.org/olia/discourse/olia_discourse.owl#BridgingType">
    <rdfs:subClassOf rdf:resource="http://purl.org/olia/olia-top.owl#PragmaticFeature"/>
  </rdf:Description>
  <rdf:Description rdf:about="http://purl.org/olia/discourse/olia_discourse.owl#BridgingType">
    <rdfs:comment>Types of textual inference, presupposes Inferrable InformationStatus</rdfs:comment>
  </rdf:Description>
  <rdf:Description rdf:about="http://purl.org/olia/discourse/olia_discourse.owl#BridgingType">
    <rdfs:label xml:lang="en">bridging type</rdfs:label>
  </rdf:Description>
  <rdf:Description rdf:about="http://purl.org/olia/discourse/olia_discourse.owl#Broadcast">
    <rdf:type rdf:resource="http://www.w3.org/2002/07/owl#Class"/>
  </rdf:Description>
  <rdf:Description rdf:about="http://purl.org/olia/discourse/olia_discourse.owl#Broadcast">
    <rdfs:subClassOf rdf:resource="http://purl.org/olia/discourse/olia_discourse.owl#BroadcastingOrganization"/>
  </rdf:Description>
  <rdf:Description rdf:about="http://purl.org/olia/discourse/olia_discourse.owl#Broadcast">
    <rdfs:comment xml:lang="en">for nerd:Broadcast sub nerd:Organization

Note: As there is no definition given, it is not fully clear what this is supposed to mean. I assume this means Broadcast*er*, not the Broadcast itself, but if so, RatioStation and TVStation should be sub-classes. Because of the unclear semantics and the lack of a link within NERD, this is marked as deprecated.</rdfs:comment>
  </rdf:Description>
  <rdf:Description rdf:about="http://purl.org/olia/discourse/olia_discourse.owl#Broadcast">
    <owl:deprecated rdf:datatype="http://www.w3.org/2001/XMLSchema#boolean">true</owl:deprecated>
  </rdf:Description>
  <rdf:Description rdf:about="http://purl.org/olia/discourse/olia_discourse.owl#BroadcastingOrganization">
    <rdf:type rdf:resource="http://www.w3.org/2002/07/owl#Class"/>
  </rdf:Description>
  <rdf:Description rdf:about="http://purl.org/olia/discourse/olia_discourse.owl#BroadcastingOrganization">
    <rdfs:subClassOf rdf:resource="http://purl.org/olia/discourse/olia_discourse.owl#Organization"/>
  </rdf:Description>
  <rdf:Description rdf:about="http://purl.org/olia/discourse/olia_discourse.owl#BroadcastingOrganization">
    <rdfs:comment xml:lang="en">Generalization over nerd:TVStation and nerd:RadioStation. nerd:Broadcast may have meant the same, but it has unclear semantics in NERD.</rdfs:comment>
  </rdf:Description>
  <rdf:Description rdf:about="http://purl.org/olia/discourse/olia_discourse.owl#Canal">
    <rdf:type rdf:resource="http://www.w3.org/2002/07/owl#Class"/>
  </rdf:Description>
  <rdf:Description rdf:about="http://purl.org/olia/discourse/olia_discourse.owl#Canal">
    <rdfs:subClassOf rdf:resource="http://purl.org/olia/discourse/olia_discourse.owl#GeographicalFeature"/>
  </rdf:Description>
  <rdf:Description rdf:about="http://purl.org/olia/discourse/olia_discourse.owl#Canal">
    <rdfs:comment xml:lang="en">for nerd:Canal</rdfs:comment>
  </rdf:Description>
  <rdf:Description rdf:about="http://purl.org/olia/discourse/olia_discourse.owl#Cause">
    <rdf:type rdf:resource="http://www.w3.org/2002/07/owl#Class"/>
  </rdf:Description>
  <rdf:Description rdf:about="http://purl.org/olia/discourse/olia_discourse.owl#Cause">
    <rdfs:subClassOf rdf:resource="http://purl.org/olia/discourse/olia_discourse.owl#Contigency"/>
  </rdf:Description>
  <rdf:Description rdf:about="http://purl.org/olia/discourse/olia_discourse.owl#Cause">
    <rdfs:comment>As the semantics/pragmatics differentiation of PDTB relations does not exactly correspond to the subject-matter/presentational distinction in RST, Cause is introduced as a generalization over SemanticCause and PragmaticCause.

This generalization is in line with (and inspired by) the ISO Core DRels (Bunt and Prasad, ISA-12).</rdfs:comment>
  </rdf:Description>
  <rdf:Description rdf:about="http://purl.org/olia/discourse/olia_discourse.owl#Cause">
    <rdfs:label xml:lang="en">cause</rdfs:label>
  </rdf:Description>
  <rdf:Description rdf:about="http://purl.org/olia/discourse/olia_discourse.owl#CausePrecedesEffect_PDTB">
    <rdf:type rdf:resource="http://www.w3.org/2002/07/owl#Class"/>
  </rdf:Description>
  <rdf:Description rdf:about="http://purl.org/olia/discourse/olia_discourse.owl#CausePrecedesEffect_PDTB">
    <rdfs:subClassOf rdf:resource="http://purl.org/olia/discourse/olia_discourse.owl#Result"/>
  </rdf:Description>
  <rdf:Description rdf:about="http://purl.org/olia/discourse/olia_discourse.owl#CausePrecedesEffect_PDTB">
    <rdfs:comment>PDTB "Result": The situation in Arg2 is the effect brought about by the situation described in Arg1. (Prasad et al. 2007)</rdfs:comment>
  </rdf:Description>
  <rdf:Description rdf:about="http://purl.org/olia/discourse/olia_discourse.owl#CausePrecedesEffect_PDTB">
    <rdfs:label xml:lang="en">cause precedes effect (PDTB)</rdfs:label>
  </rdf:Description>
  <rdf:Description rdf:about="http://purl.org/olia/discourse/olia_discourse.owl#CausePrecedesEffect_PDTB">
    <rdfs:label>result</rdfs:label>
  </rdf:Description>
  <rdf:Description rdf:about="http://purl.org/olia/discourse/olia_discourse.owl#CauseResult_RST">
    <rdf:type rdf:resource="http://www.w3.org/2002/07/owl#Class"/>
  </rdf:Description>
  <rdf:Description rdf:about="http://purl.org/olia/discourse/olia_discourse.owl#CauseResult_RST">
    <rdfs:subClassOf rdf:resource="http://purl.org/olia/discourse/olia_discourse.owl#Cause"/>
  </rdf:Description>
  <rdf:Description rdf:about="http://purl.org/olia/discourse/olia_discourse.owl#CauseResult_RST">
    <rdfs:subClassOf rdf:resource="http://purl.org/olia/discourse/olia_discourse.owl#ParatacticDiscourseRelation"/>
  </rdf:Description>
  <rdf:Description rdf:about="http://purl.org/olia/discourse/olia_discourse.owl#CauseResult_RST">
    <rdfs:subClassOf rdf:resource="http://purl.org/olia/discourse/olia_discourse.owl#SubjectMatterRelation"/>
  </rdf:Description>
  <rdf:Description rdf:about="http://purl.org/olia/discourse/olia_discourse.owl#CauseResult_RST">
    <rdfs:comment>This is a causal relation in which two EDUs, one representing the cause and the other representing the result, are of equal importance or weight. The multinuclear relations CAUSE-RESULT and CONSEQUENCE are similar. The former should be selected when the causality is perceived as being more direct, while the latter is reserved for a more indirect causal connection.
(Carlson and Marcu 2001)

Corresponds to SemDok CauseResult-multi</rdfs:comment>
  </rdf:Description>
  <rdf:Description rdf:about="http://purl.org/olia/discourse/olia_discourse.owl#CauseResult_RST">
    <rdfs:label xml:lang="en">cause result (RST)</rdfs:label>
  </rdf:Description>
  <rdf:Description rdf:about="http://purl.org/olia/discourse/olia_discourse.owl#Cause_RST">
    <rdf:type rdf:resource="http://www.w3.org/2002/07/owl#Class"/>
  </rdf:Description>
  <rdf:Description rdf:about="http://purl.org/olia/discourse/olia_discourse.owl#Cause_RST">
    <rdfs:subClassOf rdf:resource="http://purl.org/olia/discourse/olia_discourse.owl#HypotacticDiscourseRelation"/>
  </rdf:Description>
  <rdf:Description rdf:about="http://purl.org/olia/discourse/olia_discourse.owl#Cause_RST">
    <rdfs:subClassOf rdf:resource="http://purl.org/olia/discourse/olia_discourse.owl#Reason"/>
  </rdf:Description>
  <rdf:Description rdf:about="http://purl.org/olia/discourse/olia_discourse.owl#Cause_RST">
    <rdfs:comment>RST "CAUSE": The situation presented in the nucleus is the cause of the situation presented in
the satellite. The cause, which is the nucleus, is the most important part. The satellite represents
the result of the action. The intention of the writer is to emphasize the cause. When the result is
the nucleus, the mononuclear relation RESULT should be selected. When it is not clear whether the
cause or result is more important, select the multinuclear relation CAUSE-RESULT.
(Carlson and Marcu 2001)</rdfs:comment>
  </rdf:Description>
  <rdf:Description rdf:about="http://purl.org/olia/discourse/olia_discourse.owl#Cause_RST">
    <rdfs:label xml:lang="en">cause (RST)</rdfs:label>
  </rdf:Description>
  <rdf:Description rdf:about="http://purl.org/olia/discourse/olia_discourse.owl#Celebrity">
    <rdf:type rdf:resource="http://www.w3.org/2002/07/owl#Class"/>
  </rdf:Description>
  <rdf:Description rdf:about="http://purl.org/olia/discourse/olia_discourse.owl#Celebrity">
    <rdfs:subClassOf rdf:resource="http://purl.org/olia/discourse/olia_discourse.owl#Person"/>
  </rdf:Description>
  <rdf:Description rdf:about="http://purl.org/olia/discourse/olia_discourse.owl#Celebrity">
    <rdfs:comment xml:lang="en">for nerd:Celebrity. As this is not supported by an external extractor, it is deprecated.</rdfs:comment>
  </rdf:Description>
  <rdf:Description rdf:about="http://purl.org/olia/discourse/olia_discourse.owl#Celebrity">
    <owl:deprecated rdf:datatype="http://www.w3.org/2001/XMLSchema#boolean">true</owl:deprecated>
  </rdf:Description>
  <rdf:Description rdf:about="http://purl.org/olia/discourse/olia_discourse.owl#ChosenAlternative_PDTB">
    <rdf:type rdf:resource="http://www.w3.org/2002/07/owl#Class"/>
  </rdf:Description>
  <rdf:Description rdf:about="http://purl.org/olia/discourse/olia_discourse.owl#ChosenAlternative_PDTB">
    <rdfs:subClassOf rdf:resource="http://purl.org/olia/discourse/olia_discourse.owl#FavouredAlternative"/>
  </rdf:Description>
  <rdf:Description rdf:about="http://purl.org/olia/discourse/olia_discourse.owl#ChosenAlternative_PDTB">
    <rdfs:comment>The connective indicates that two alternatives are evoked in the discourse but only one is taken. (Prasad et al. 2007)</rdfs:comment>
  </rdf:Description>
  <rdf:Description rdf:about="http://purl.org/olia/discourse/olia_discourse.owl#ChosenAlternative_PDTB">
    <rdfs:label xml:lang="en">chosen alternative (PDTB)</rdfs:label>
  </rdf:Description>
  <rdf:Description rdf:about="http://purl.org/olia/discourse/olia_discourse.owl#Circumstance">
    <rdf:type rdf:resource="http://www.w3.org/2002/07/owl#Class"/>
  </rdf:Description>
  <rdf:Description rdf:about="http://purl.org/olia/discourse/olia_discourse.owl#Circumstance">
    <rdfs:subClassOf rdf:resource="http://purl.org/olia/discourse/olia_discourse.owl#Background"/>
  </rdf:Description>
  <rdf:Description rdf:about="http://purl.org/olia/discourse/olia_discourse.owl#Circumstance">
    <rdfs:subClassOf rdf:resource="http://purl.org/olia/discourse/olia_discourse.owl#SubjectMatterRelation"/>
  </rdf:Description>
  <rdf:Description rdf:about="http://purl.org/olia/discourse/olia_discourse.owl#Circumstance">
    <rdfs:subClassOf rdf:resource="http://purl.org/olia/discourse/olia_discourse.owl#SynchronousRelation"/>
  </rdf:Description>
  <rdf:Description rdf:about="http://purl.org/olia/discourse/olia_discourse.owl#Circumstance">
    <rdfs:comment>The situation presented in the satellite provides the context in which the situation presented in the nucleus should be interpreted. The satellite IS NOT the cause/reason/motivation of the situation presented in the nucleus. (Carlson and Marcu 2001)
S is not unrealized; S sets a framework in the subject matter within which R is intended to interpret N (Mann and Taboada 2010)

Note that this is not an RST-specific relation because of its use in SemDok. Axiomatization follows SemDok</rdfs:comment>
  </rdf:Description>
  <rdf:Description rdf:about="http://purl.org/olia/discourse/olia_discourse.owl#Circumstance">
    <rdfs:label xml:lang="en">circumstance</rdfs:label>
  </rdf:Description>
  <rdf:Description rdf:about="http://purl.org/olia/discourse/olia_discourse.owl#Circumstance">
    <owl:versionInfo>Defined as a SynchronousRelation because of its association with the discourse marker "while", cf. Prasad et al. (2007)</owl:versionInfo>
  </rdf:Description>
  <rdf:Description rdf:about="http://purl.org/olia/discourse/olia_discourse.owl#Circumstance_RST">
    <rdf:type rdf:resource="http://www.w3.org/2002/07/owl#Class"/>
  </rdf:Description>
  <rdf:Description rdf:about="http://purl.org/olia/discourse/olia_discourse.owl#Circumstance_RST">
    <rdfs:subClassOf rdf:resource="http://purl.org/olia/discourse/olia_discourse.owl#Circumstance"/>
  </rdf:Description>
  <rdf:Description rdf:about="http://purl.org/olia/discourse/olia_discourse.owl#Circumstance_RST">
    <rdfs:comment>superseded by Circumstance, maintained for backward compatibility</rdfs:comment>
  </rdf:Description>
  <rdf:Description rdf:about="http://purl.org/olia/discourse/olia_discourse.owl#Circumstance_RST">
    <rdfs:label>circumstance (RST)</rdfs:label>
  </rdf:Description>
  <rdf:Description rdf:about="http://purl.org/olia/discourse/olia_discourse.owl#Circumstance_RST">
    <rdfs:label xml:lang="en">circumstance (RST)</rdfs:label>
  </rdf:Description>
  <rdf:Description rdf:about="http://purl.org/olia/discourse/olia_discourse.owl#Circumstance_RST">
    <owl:deprecated rdf:datatype="http://www.w3.org/2001/XMLSchema#boolean">true</owl:deprecated>
  </rdf:Description>
  <rdf:Description rdf:about="http://purl.org/olia/discourse/olia_discourse.owl#Citation">
    <rdf:type rdf:resource="http://www.w3.org/2002/07/owl#Class"/>
  </rdf:Description>
  <rdf:Description rdf:about="http://purl.org/olia/discourse/olia_discourse.owl#Citation">
    <rdfs:subClassOf rdf:resource="http://purl.org/olia/olia-top.owl#TextStructuralUnit"/>
  </rdf:Description>
  <rdf:Description rdf:about="http://purl.org/olia/discourse/olia_discourse.owl#Citation">
    <rdfs:comment>introduced for SemDok Citation. However, we consider Citation not as a rhetorical relation, but as a structural element in the text that can serve different purposes (discourse relations). These purposes correspond to the subclasses of Citation in SemDok, and these subclasses are thus in the intersection between OLiA Citation and the discourse relation that corresponds to their respective function,</rdfs:comment>
  </rdf:Description>
  <rdf:Description rdf:about="http://purl.org/olia/discourse/olia_discourse.owl#Citation">
    <rdfs:label xml:lang="en">citation</rdfs:label>
  </rdf:Description>
  <rdf:Description rdf:about="http://purl.org/olia/discourse/olia_discourse.owl#CitationAttribution">
    <rdf:type rdf:resource="http://www.w3.org/2002/07/owl#Class"/>
  </rdf:Description>
  <rdf:Description rdf:about="http://purl.org/olia/discourse/olia_discourse.owl#CitationAttribution">
    <rdfs:subClassOf rdf:resource="http://purl.org/olia/discourse/olia_discourse.owl#Attribution"/>
  </rdf:Description>
  <rdf:Description rdf:about="http://purl.org/olia/discourse/olia_discourse.owl#CitationAttribution">
    <rdfs:subClassOf rdf:resource="http://purl.org/olia/discourse/olia_discourse.owl#Citation"/>
  </rdf:Description>
  <rdf:Description rdf:about="http://purl.org/olia/discourse/olia_discourse.owl#CitationAttribution">
    <rdfs:comment>cf. SemDok Citation-attribution</rdfs:comment>
  </rdf:Description>
  <rdf:Description rdf:about="http://purl.org/olia/discourse/olia_discourse.owl#CitationAttribution">
    <rdfs:label xml:lang="en">citation attribution</rdfs:label>
  </rdf:Description>
  <rdf:Description rdf:about="http://purl.org/olia/discourse/olia_discourse.owl#CitationAttribution">
    <rdfs:label>citation/attribution</rdfs:label>
  </rdf:Description>
  <rdf:Description rdf:about="http://purl.org/olia/discourse/olia_discourse.owl#CitationEvidence">
    <rdf:type rdf:resource="http://www.w3.org/2002/07/owl#Class"/>
  </rdf:Description>
  <rdf:Description rdf:about="http://purl.org/olia/discourse/olia_discourse.owl#CitationEvidence">
    <rdfs:subClassOf rdf:resource="http://purl.org/olia/discourse/olia_discourse.owl#Citation"/>
  </rdf:Description>
  <rdf:Description rdf:about="http://purl.org/olia/discourse/olia_discourse.owl#CitationEvidence">
    <rdfs:subClassOf rdf:resource="http://purl.org/olia/discourse/olia_discourse.owl#Evidence"/>
  </rdf:Description>
  <rdf:Description rdf:about="http://purl.org/olia/discourse/olia_discourse.owl#CitationEvidence">
    <rdfs:comment>cf. SemDok Citation-evidence</rdfs:comment>
  </rdf:Description>
  <rdf:Description rdf:about="http://purl.org/olia/discourse/olia_discourse.owl#CitationEvidence">
    <rdfs:label xml:lang="en">citation evidence</rdfs:label>
  </rdf:Description>
  <rdf:Description rdf:about="http://purl.org/olia/discourse/olia_discourse.owl#CitationEvidence">
    <rdfs:label>citation/evidence</rdfs:label>
  </rdf:Description>
  <rdf:Description rdf:about="http://purl.org/olia/discourse/olia_discourse.owl#CitationSelf">
    <rdf:type rdf:resource="http://www.w3.org/2002/07/owl#Class"/>
  </rdf:Description>
  <rdf:Description rdf:about="http://purl.org/olia/discourse/olia_discourse.owl#CitationSelf">
    <rdfs:subClassOf rdf:resource="http://purl.org/olia/discourse/olia_discourse.owl#Citation"/>
  </rdf:Description>
  <rdf:Description rdf:about="http://purl.org/olia/discourse/olia_discourse.owl#CitationSelf">
    <rdfs:subClassOf rdf:resource="http://purl.org/olia/discourse/olia_discourse.owl#Support"/>
  </rdf:Description>
  <rdf:Description rdf:about="http://purl.org/olia/discourse/olia_discourse.owl#CitationSelf">
    <rdfs:comment>SemDok Citation-self, subclass of Support</rdfs:comment>
  </rdf:Description>
  <rdf:Description rdf:about="http://purl.org/olia/discourse/olia_discourse.owl#CitationSelf">
    <rdfs:label xml:lang="en">citation self</rdfs:label>
  </rdf:Description>
  <rdf:Description rdf:about="http://purl.org/olia/discourse/olia_discourse.owl#CitationSelf">
    <rdfs:label>citation/self</rdfs:label>
  </rdf:Description>
  <rdf:Description rdf:about="http://purl.org/olia/discourse/olia_discourse.owl#City">
    <rdf:type rdf:resource="http://www.w3.org/2002/07/owl#Class"/>
  </rdf:Description>
  <rdf:Description rdf:about="http://purl.org/olia/discourse/olia_discourse.owl#City">
    <rdfs:subClassOf rdf:resource="http://purl.org/olia/discourse/olia_discourse.owl#PoliticalUnit"/>
  </rdf:Description>
  <rdf:Description rdf:about="http://purl.org/olia/discourse/olia_discourse.owl#City">
    <rdfs:comment xml:lang="en">for nerd:City</rdfs:comment>
  </rdf:Description>
  <rdf:Description rdf:about="http://purl.org/olia/discourse/olia_discourse.owl#CoherenceRelation">
    <rdf:type rdf:resource="http://www.w3.org/2002/07/owl#Class"/>
  </rdf:Description>
  <rdf:Description rdf:about="http://purl.org/olia/discourse/olia_discourse.owl#CoherenceRelation">
    <rdfs:subClassOf rdf:resource="http://purl.org/olia/discourse/olia_discourse.owl#DiscourseRelation"/>
  </rdf:Description>
  <rdf:Description rdf:about="http://purl.org/olia/discourse/olia_discourse.owl#CoherenceRelation">
    <owl:disjointWith rdf:resource="http://purl.org/olia/discourse/olia_discourse.owl#EntityBasedRelation"/>
  </rdf:Description>
  <rdf:Description rdf:about="http://purl.org/olia/discourse/olia_discourse.owl#CoherenceRelation">
    <owl:disjointWith rdf:resource="http://purl.org/olia/discourse/olia_discourse.owl#TextualOrganizationalRelation"/>
  </rdf:Description>
  <rdf:Description rdf:about="http://purl.org/olia/discourse/olia_discourse.owl#CoherenceRelation">
    <rdfs:comment>CoherenceRelation is used here as a synonym of PDTB "coherence relation". RST "discourse relation", however, is broader.</rdfs:comment>
  </rdf:Description>
  <rdf:Description rdf:about="http://purl.org/olia/discourse/olia_discourse.owl#CoherenceRelation">
    <rdfs:label>coherence relation</rdfs:label>
  </rdf:Description>
  <rdf:Description rdf:about="http://purl.org/olia/discourse/olia_discourse.owl#CoherenceRelation">
    <rdfs:label xml:lang="en">coherence relation</rdfs:label>
  </rdf:Description>
  <rdf:Description rdf:about="http://purl.org/olia/discourse/olia_discourse.owl#ColumnTitle">
    <rdf:type rdf:resource="http://www.w3.org/2002/07/owl#Class"/>
  </rdf:Description>
  <rdf:Description rdf:about="http://purl.org/olia/discourse/olia_discourse.owl#ColumnTitle">
    <rdfs:subClassOf rdf:resource="http://purl.org/olia/olia-top.owl#TextStructuralUnit"/>
  </rdf:Description>
  <rdf:Description rdf:about="http://purl.org/olia/discourse/olia_discourse.owl#ColumnTitle">
    <rdfs:comment>This schema refers to the name of a regularly featured column in the paper,
and should be used when the paper begins by presenting a TITLE, COLUMN-TITLE and AUTHOR.
(Carlson and Marcu 2001)</rdfs:comment>
  </rdf:Description>
  <rdf:Description rdf:about="http://purl.org/olia/discourse/olia_discourse.owl#ColumnTitle">
    <rdfs:label xml:lang="en">column title</rdfs:label>
  </rdf:Description>
  <rdf:Description rdf:about="http://purl.org/olia/discourse/olia_discourse.owl#ComicsCharacter">
    <rdf:type rdf:resource="http://www.w3.org/2002/07/owl#Class"/>
  </rdf:Description>
  <rdf:Description rdf:about="http://purl.org/olia/discourse/olia_discourse.owl#ComicsCharacter">
    <rdfs:subClassOf rdf:resource="http://purl.org/olia/discourse/olia_discourse.owl#Person"/>
  </rdf:Description>
  <rdf:Description rdf:about="http://purl.org/olia/discourse/olia_discourse.owl#ComicsCharacter">
    <rdfs:comment xml:lang="en">for nerd:ComicsCharacter. As this is not supported by an external extractor, it is deprecated.</rdfs:comment>
  </rdf:Description>
  <rdf:Description rdf:about="http://purl.org/olia/discourse/olia_discourse.owl#ComicsCharacter">
    <owl:deprecated rdf:datatype="http://www.w3.org/2001/XMLSchema#boolean">true</owl:deprecated>
  </rdf:Description>
  <rdf:Description rdf:about="http://purl.org/olia/discourse/olia_discourse.owl#CommentTopic">
    <rdf:type rdf:resource="http://www.w3.org/2002/07/owl#Class"/>
  </rdf:Description>
  <rdf:Description rdf:about="http://purl.org/olia/discourse/olia_discourse.owl#CommentTopic">
    <rdfs:subClassOf rdf:resource="http://purl.org/olia/discourse/olia_discourse.owl#TopicContinuityRelation"/>
  </rdf:Description>
  <rdf:Description rdf:about="http://purl.org/olia/discourse/olia_discourse.owl#CommentTopic">
    <rdfs:comment>introduced in analogy with TopicComment as generalization over CommentTopic_RST</rdfs:comment>
  </rdf:Description>
  <rdf:Description rdf:about="http://purl.org/olia/discourse/olia_discourse.owl#CommentTopic">
    <rdfs:label xml:lang="en">comment topic</rdfs:label>
  </rdf:Description>
  <rdf:Description rdf:about="http://purl.org/olia/discourse/olia_discourse.owl#CommentTopic_RST">
    <rdf:type rdf:resource="http://www.w3.org/2002/07/owl#Class"/>
  </rdf:Description>
  <rdf:Description rdf:about="http://purl.org/olia/discourse/olia_discourse.owl#CommentTopic_RST">
    <rdfs:subClassOf rdf:resource="http://purl.org/olia/discourse/olia_discourse.owl#CommentTopic"/>
  </rdf:Description>
  <rdf:Description rdf:about="http://purl.org/olia/discourse/olia_discourse.owl#CommentTopic_RST">
    <rdfs:subClassOf rdf:resource="http://purl.org/olia/discourse/olia_discourse.owl#ParatacticDiscourseRelation"/>
  </rdf:Description>
  <rdf:Description rdf:about="http://purl.org/olia/discourse/olia_discourse.owl#CommentTopic_RST">
    <rdfs:comment>A specific remark is made on a topic or statement, after which the topic itself is identified. This relation is always multinuclear, as both spans are necessary to understand the context. When the spans occur in the reverse order, with the topic preceding the comment, the relation TOPIC-COMMENT is selected. While COMMENT-TOPIC is not a frequently used device in English, it is seen in news reporting, for example, when someone makes a statement, after which a reference is given to help the reader interpret the context of the statement.
(Carlson and Marcu 2001)</rdfs:comment>
  </rdf:Description>
  <rdf:Description rdf:about="http://purl.org/olia/discourse/olia_discourse.owl#CommentTopic_RST">
    <rdfs:label xml:lang="en">comment topic (RST)</rdfs:label>
  </rdf:Description>
  <rdf:Description rdf:about="http://purl.org/olia/discourse/olia_discourse.owl#Comment_RST">
    <rdf:type rdf:resource="http://www.w3.org/2002/07/owl#Class"/>
  </rdf:Description>
  <rdf:Description rdf:about="http://purl.org/olia/discourse/olia_discourse.owl#Comment_RST">
    <rdfs:subClassOf rdf:resource="http://purl.org/olia/discourse/olia_discourse.owl#Assessment"/>
  </rdf:Description>
  <rdf:Description rdf:about="http://purl.org/olia/discourse/olia_discourse.owl#Comment_RST">
    <rdfs:comment>In a COMMENT relation, the satellite constitutes a subjective remark on a previous segment of the text. It is not an evaluation or an interpretation. The comment is usually presented from a perspective that is outside of the elements in focus in the nucleus.
(Carlson and Marcu 2001)</rdfs:comment>
  </rdf:Description>
  <rdf:Description rdf:about="http://purl.org/olia/discourse/olia_discourse.owl#Comment_RST">
    <rdfs:label xml:lang="en">comment (RST)</rdfs:label>
  </rdf:Description>
  <rdf:Description rdf:about="http://purl.org/olia/discourse/olia_discourse.owl#CommonlyUsed">
    <rdf:type rdf:resource="http://www.w3.org/2002/07/owl#Class"/>
  </rdf:Description>
  <rdf:Description rdf:about="http://purl.org/olia/discourse/olia_discourse.owl#CommonlyUsed">
    <rdfs:subClassOf rdf:resource="http://purl.org/olia/discourse/olia_discourse.owl#Possible"/>
  </rdf:Description>
  <rdf:Description rdf:about="http://purl.org/olia/discourse/olia_discourse.owl#CommonlyUsed">
    <rdfs:comment>
                            Said of a term that appears frequently.
                                (ISO12620; http://www.isocat.org/datcat/DC-1984)
                            </rdfs:comment>
  </rdf:Description>
  <rdf:Description rdf:about="http://purl.org/olia/discourse/olia_discourse.owl#CommonlyUsed">
    <rdfs:label>commonly used</rdfs:label>
  </rdf:Description>
  <rdf:Description rdf:about="http://purl.org/olia/discourse/olia_discourse.owl#CommonlyUsed">
    <owl:versionInfo>http://www.isocat.org/datcat/DC-1984</owl:versionInfo>
  </rdf:Description>
  <rdf:Description rdf:about="http://purl.org/olia/discourse/olia_discourse.owl#CommonlyUsed">
    <owl:versionInfo>subClassOf frequency (dcif:conceptualDomain)</owl:versionInfo>
  </rdf:Description>
  <rdf:Description rdf:about="http://purl.org/olia/discourse/olia_discourse.owl#Company">
    <rdf:type rdf:resource="http://www.w3.org/2002/07/owl#Class"/>
  </rdf:Description>
  <rdf:Description rdf:about="http://purl.org/olia/discourse/olia_discourse.owl#Company">
    <rdfs:subClassOf rdf:resource="http://purl.org/olia/discourse/olia_discourse.owl#Organization"/>
  </rdf:Description>
  <rdf:Description rdf:about="http://purl.org/olia/discourse/olia_discourse.owl#Company">
    <rdfs:comment xml:lang="en">for nerd:Company</rdfs:comment>
  </rdf:Description>
  <rdf:Description rdf:about="http://purl.org/olia/discourse/olia_discourse.owl#Company">
    <rdfs:label xml:lang="en">company name</rdfs:label>
  </rdf:Description>
  <rdf:Description rdf:about="http://purl.org/olia/discourse/olia_discourse.owl#Company">
    <skos:prefLabel xml:lang="en">company</skos:prefLabel>
  </rdf:Description>
  <rdf:Description rdf:about="http://purl.org/olia/discourse/olia_discourse.owl#Comparison">
    <rdf:type rdf:resource="http://www.w3.org/2002/07/owl#Class"/>
  </rdf:Description>
  <rdf:Description rdf:about="http://purl.org/olia/discourse/olia_discourse.owl#Comparison">
    <rdfs:subClassOf rdf:resource="http://purl.org/olia/discourse/olia_discourse.owl#CoherenceRelation"/>
  </rdf:Description>
  <rdf:Description rdf:about="http://purl.org/olia/discourse/olia_discourse.owl#Comparison">
    <rdfs:comment>The connective indicates that a discourse relation is established between Arg1 and Arg2 in order to highlight prominent differences between the two situations. Semantically, the truth of both arguments is independent of the connective or the established relation. (Prasad et al. 2007)

cf. Resemblance (Wolf et al. 2003): Resemblance relations establish commonalities and contrasts between corresponding (sets of) discourse entities or properties (Kehler (2002)). Corresponding (sets of) discourse entities or
properties are usually syntactically and / or semantically parallel.</rdfs:comment>
  </rdf:Description>
  <rdf:Description rdf:about="http://purl.org/olia/discourse/olia_discourse.owl#Comparison">
    <rdfs:label xml:lang="en">comparison</rdfs:label>
  </rdf:Description>
  <rdf:Description rdf:about="http://purl.org/olia/discourse/olia_discourse.owl#Comparison_RST">
    <rdf:type rdf:resource="http://www.w3.org/2002/07/owl#Class"/>
  </rdf:Description>
  <rdf:Description rdf:about="http://purl.org/olia/discourse/olia_discourse.owl#Comparison_RST">
    <rdfs:subClassOf rdf:resource="http://purl.org/olia/discourse/olia_discourse.owl#NonContrastiveComparison"/>
  </rdf:Description>
  <rdf:Description rdf:about="http://purl.org/olia/discourse/olia_discourse.owl#Comparison_RST">
    <rdfs:comment>Two textual spans are compared along some dimension, which can be abstract. The relations can convey that some abstract entities that pertain to the comparison relation are similar, different, greater-than, less-than, etc. In the case of a comparison
relation, the spans, entities, etc. are not in contrast. (Carlson and Marcu 2001)</rdfs:comment>
  </rdf:Description>
  <rdf:Description rdf:about="http://purl.org/olia/discourse/olia_discourse.owl#Comparison_RST">
    <rdfs:label xml:lang="en">comparison (RST)</rdfs:label>
  </rdf:Description>
  <rdf:Description rdf:about="http://purl.org/olia/discourse/olia_discourse.owl#ComplexDiscourseSegment">
    <rdf:type rdf:resource="http://www.w3.org/2002/07/owl#Class"/>
  </rdf:Description>
  <rdf:Description rdf:about="http://purl.org/olia/discourse/olia_discourse.owl#ComplexDiscourseSegment">
    <rdfs:subClassOf rdf:resource="http://purl.org/olia/discourse/olia_discourse.owl#DiscourseSegment"/>
  </rdf:Description>
  <rdf:Description rdf:about="http://purl.org/olia/discourse/olia_discourse.owl#ComplexDiscourseSegment">
    <rdfs:comment>from SemDok

SemDok also defines three sub-classes: CDS-block, CDS-div, CDS-doc. It seems these refer to the structure of XML documents, and without definitions, these have not been adopted here.</rdfs:comment>
  </rdf:Description>
  <rdf:Description rdf:about="http://purl.org/olia/discourse/olia_discourse.owl#ComplexDiscourseSegment">
    <rdfs:label>complex discourse segment</rdfs:label>
  </rdf:Description>
  <rdf:Description rdf:about="http://purl.org/olia/discourse/olia_discourse.owl#ComplexDiscourseSegment">
    <rdfs:label xml:lang="en">complex discourse segment</rdfs:label>
  </rdf:Description>
  <rdf:Description rdf:about="http://purl.org/olia/discourse/olia_discourse.owl#Concession">
    <rdf:type rdf:resource="http://www.w3.org/2002/07/owl#Class"/>
  </rdf:Description>
  <rdf:Description rdf:about="http://purl.org/olia/discourse/olia_discourse.owl#Concession">
    <rdfs:subClassOf rdf:resource="http://purl.org/olia/discourse/olia_discourse.owl#ContrastiveComparison"/>
  </rdf:Description>
  <rdf:Description rdf:nodeID="genid23">
    <rdf:type rdf:resource="http://www.w3.org/2002/07/owl#Class"/>
  </rdf:Description>
  <rdf:Description rdf:nodeID="genid24">
    <rdf:first rdf:resource="http://purl.org/olia/discourse/olia_discourse.owl#ContrastiveComparison"/>
  </rdf:Description>
  <rdf:Description rdf:nodeID="genid25">
    <rdf:first rdf:resource="http://purl.org/olia/discourse/olia_discourse.owl#HypotacticDiscourseRelation"/>
  </rdf:Description>
  <rdf:Description rdf:nodeID="genid24">
    <rdf:rest rdf:nodeID="genid25"/>
  </rdf:Description>
  <rdf:Description rdf:nodeID="genid26">
    <rdf:first rdf:resource="http://purl.org/olia/discourse/olia_discourse.owl#PresentationalRelation"/>
  </rdf:Description>
  <rdf:Description rdf:nodeID="genid25">
    <rdf:rest rdf:nodeID="genid26"/>
  </rdf:Description>
  <rdf:Description rdf:nodeID="genid26">
    <rdf:rest rdf:resource="http://www.w3.org/1999/02/22-rdf-syntax-ns#nil"/>
  </rdf:Description>
  <rdf:Description rdf:nodeID="genid23">
    <owl:intersectionOf rdf:nodeID="genid24"/>
  </rdf:Description>
  <rdf:Description rdf:about="http://purl.org/olia/discourse/olia_discourse.owl#Concession">
    <rdfs:subClassOf rdf:nodeID="genid23"/>
  </rdf:Description>
  <rdf:Description rdf:about="http://purl.org/olia/discourse/olia_discourse.owl#Concession">
    <rdfs:comment>One of the arguments describes a situation A which causes C, while the other asserts (or implies) the complement of C.
(Prasad et al. 2007)

The situation indicated in the nucleus is contrary to expectation in the light of the information presented in the satellite. In other words, a CONCESSION relation is always characterized by a violated expectation. In some cases, which text span is the
satellite and which is the nucleus do not depend on the semantics of the spans, but rather on the intention of the writer.
(Carlson and Marcu 2001)

A typical marker is "although" (in PTDB and RSTDTB).

Axiomatization follows SemDok Concession (subclass of Contrast). We follow SemDok in assuming that Concession is always hypotactic (mononuclear), although this is not explicit in the PDTB definitions.</rdfs:comment>
  </rdf:Description>
  <rdf:Description rdf:about="http://purl.org/olia/discourse/olia_discourse.owl#Concession">
    <rdfs:label>concession</rdfs:label>
  </rdf:Description>
  <rdf:Description rdf:about="http://purl.org/olia/discourse/olia_discourse.owl#Concession">
    <rdfs:label xml:lang="en">concession</rdfs:label>
  </rdf:Description>
  <rdf:Description rdf:about="http://purl.org/olia/discourse/olia_discourse.owl#Concession">
    <rdfs:label>violated expectation</rdfs:label>
  </rdf:Description>
  <rdf:Description rdf:about="http://purl.org/olia/discourse/olia_discourse.owl#Conclusion_RST">
    <rdf:type rdf:resource="http://www.w3.org/2002/07/owl#Class"/>
  </rdf:Description>
  <rdf:Description rdf:about="http://purl.org/olia/discourse/olia_discourse.owl#Conclusion_RST">
    <rdfs:subClassOf rdf:resource="http://purl.org/olia/discourse/olia_discourse.owl#Contigency"/>
  </rdf:Description>
  <rdf:Description rdf:nodeID="genid27">
    <rdf:type rdf:resource="http://www.w3.org/2002/07/owl#Class"/>
  </rdf:Description>
  <rdf:Description rdf:nodeID="genid28">
    <rdf:first rdf:resource="http://purl.org/olia/discourse/olia_discourse.owl#Cause"/>
  </rdf:Description>
  <rdf:Description rdf:nodeID="genid29">
    <rdf:first rdf:resource="http://purl.org/olia/discourse/olia_discourse.owl#Condition"/>
  </rdf:Description>
  <rdf:Description rdf:nodeID="genid28">
    <rdf:rest rdf:nodeID="genid29"/>
  </rdf:Description>
  <rdf:Description rdf:nodeID="genid29">
    <rdf:rest rdf:resource="http://www.w3.org/1999/02/22-rdf-syntax-ns#nil"/>
  </rdf:Description>
  <rdf:Description rdf:nodeID="genid27">
    <owl:unionOf rdf:nodeID="genid28"/>
  </rdf:Description>
  <rdf:Description rdf:about="http://purl.org/olia/discourse/olia_discourse.owl#Conclusion_RST">
    <rdfs:subClassOf rdf:nodeID="genid27"/>
  </rdf:Description>
  <rdf:Description rdf:about="http://purl.org/olia/discourse/olia_discourse.owl#Conclusion_RST">
    <rdfs:comment>In a CONCLUSION relation, the satellite presents a final statement that wraps up the situation presented in the nucleus. A CONCLUSION satellite is a reasoned judgment, inference, necessary consequence, or final decision with respect to the situation presented in the nucleus. When the nucleus and satellite are of equal importance, select the multinuclear CONCLUSION.
(Carlson and Marcu 2001)</rdfs:comment>
  </rdf:Description>
  <rdf:Description rdf:about="http://purl.org/olia/discourse/olia_discourse.owl#Conclusion_RST">
    <rdfs:label xml:lang="en">conclusion (RST)</rdfs:label>
  </rdf:Description>
  <rdf:Description rdf:about="http://purl.org/olia/discourse/olia_discourse.owl#ConcreteEntity">
    <rdf:type rdf:resource="http://www.w3.org/2002/07/owl#Class"/>
  </rdf:Description>
  <rdf:Description rdf:about="http://purl.org/olia/discourse/olia_discourse.owl#ConcreteEntity">
    <rdfs:subClassOf rdf:resource="http://purl.org/olia/discourse/olia_discourse.owl#EntityType"/>
  </rdf:Description>
  <rdf:Description rdf:about="http://purl.org/olia/discourse/olia_discourse.owl#ConcreteEntity">
    <rdfs:comment>Categories specified for referring expressions (Poesio &amp; Artstein 2006): Abstract, Animate, Concrete, Person, Plan, Space, Time</rdfs:comment>
  </rdf:Description>
  <rdf:Description rdf:about="http://purl.org/olia/discourse/olia_discourse.owl#ConcreteEntity">
    <rdfs:label xml:lang="en">concrete entity</rdfs:label>
  </rdf:Description>
  <rdf:Description rdf:about="http://purl.org/olia/discourse/olia_discourse.owl#Condition">
    <rdf:type rdf:resource="http://www.w3.org/2002/07/owl#Class"/>
  </rdf:Description>
  <rdf:Description rdf:about="http://purl.org/olia/discourse/olia_discourse.owl#Condition">
    <rdfs:subClassOf rdf:resource="http://purl.org/olia/discourse/olia_discourse.owl#Contigency"/>
  </rdf:Description>
  <rdf:Description rdf:about="http://purl.org/olia/discourse/olia_discourse.owl#Condition">
    <rdfs:comment>Note that Condition is undefined with respect to nuclearity. Mononuclear relations are Consequence (condition is nucleus) and Pragmatic / Semantic Condition (condition is satellite).

RST-DTB: In a CONDITION relation, the truth of the proposition associated with the nucleus is a consequence of the fulfillment of the condition in the satellite. The satellite presents a situation that is not realized. (Carlson and Marcu 2001)

PDGB: the event described in the Nucleus can only take place if the event described in the Satellite also takes place (before or simultaneously with the event described in the Nucleus)
(Wolf et al. 2003)

PDTB: As the semantics/pragmatics differentiation of PDTB relations does not exactly correspond to the subject-matter/presentational distinction in RST, Condition was originally introduced as a generalization over SemanticCondition and PragmaticCondition. Both SemanticCondition and PragmaticCondition take the condition to be the satellite.

ISO: Condition and Negative Condition describe the relation between both arguments, the RST/PDTB/PDGB condition relations correspond to an ISO (Negative) Condition with argument (Negated) Antecedent.</rdfs:comment>
  </rdf:Description>
  <rdf:Description rdf:about="http://purl.org/olia/discourse/olia_discourse.owl#Condition">
    <rdfs:label xml:lang="en">condition</rdfs:label>
  </rdf:Description>
  <rdf:Description rdf:about="http://purl.org/olia/discourse/olia_discourse.owl#Conjunction">
    <rdf:type rdf:resource="http://www.w3.org/2002/07/owl#Class"/>
  </rdf:Description>
  <rdf:Description rdf:about="http://purl.org/olia/discourse/olia_discourse.owl#Conjunction">
    <rdfs:subClassOf rdf:resource="http://purl.org/olia/discourse/olia_discourse.owl#Expansion"/>
  </rdf:Description>
  <rdf:Description rdf:about="http://purl.org/olia/discourse/olia_discourse.owl#Conjunction">
    <rdfs:subClassOf rdf:resource="http://purl.org/olia/discourse/olia_discourse.owl#ParatacticDiscourseRelation"/>
  </rdf:Description>
  <rdf:Description rdf:about="http://purl.org/olia/discourse/olia_discourse.owl#Conjunction">
    <rdfs:comment>The situation described in Arg2 provides additional, discourse new, information that is related to the situation described in Arg1. Typical connectives for “Conjunction” are also, in addition, additionally, further, etc. (Prasad et al. 2007)

The items are conjoined to form a unit in which each item plays a comparable role. (Mann and Taboada 2010)

We follow Bunt and Prasad (ISA-12) in assuming that (ISO) conjunction is a superclass of (PDTB) list. HOWEVER, in terms of the PDTB v2.0 definitions, both are more likely to be taken as sibling concepts.</rdfs:comment>
  </rdf:Description>
  <rdf:Description rdf:about="http://purl.org/olia/discourse/olia_discourse.owl#Conjunction">
    <rdfs:label xml:lang="en">conjunction</rdfs:label>
  </rdf:Description>
  <rdf:Description rdf:about="http://purl.org/olia/discourse/olia_discourse.owl#Conjunctive_PDTB">
    <rdf:type rdf:resource="http://www.w3.org/2002/07/owl#Class"/>
  </rdf:Description>
  <rdf:Description rdf:about="http://purl.org/olia/discourse/olia_discourse.owl#Conjunctive_PDTB">
    <rdfs:subClassOf rdf:resource="http://purl.org/olia/discourse/olia_discourse.owl#Alternative"/>
  </rdf:Description>
  <rdf:Description rdf:about="http://purl.org/olia/discourse/olia_discourse.owl#Conjunctive_PDTB">
    <rdfs:comment>The connective indicates that both alternatives hold or are possible. (Prasad et al. 2007)</rdfs:comment>
  </rdf:Description>
  <rdf:Description rdf:about="http://purl.org/olia/discourse/olia_discourse.owl#Conjunctive_PDTB">
    <rdfs:label xml:lang="en">conjunctive (PDTB)</rdfs:label>
  </rdf:Description>
  <rdf:Description rdf:about="http://purl.org/olia/discourse/olia_discourse.owl#Consequence">
    <rdf:type rdf:resource="http://www.w3.org/2002/07/owl#Class"/>
  </rdf:Description>
  <rdf:Description rdf:about="http://purl.org/olia/discourse/olia_discourse.owl#Consequence">
    <rdfs:subClassOf rdf:resource="http://purl.org/olia/discourse/olia_discourse.owl#Condition"/>
  </rdf:Description>
  <rdf:Description rdf:about="http://purl.org/olia/discourse/olia_discourse.owl#Consequence">
    <rdfs:subClassOf rdf:resource="http://purl.org/olia/discourse/olia_discourse.owl#SubjectMatterRelation"/>
  </rdf:Description>
  <rdf:Description rdf:about="http://purl.org/olia/discourse/olia_discourse.owl#Consequence">
    <rdfs:comment>ISO DR-Core: Condition or Negated Condition, argument Consequent

This is an annotation that marks a condition at the consequent rather than the condition, itself. We expect such a relation to require both a consequent and a condition, and that the type of condition is marked at the condition rather at the consequent. Accordinly, Consequence does not have further subclasses, but should be coupled with Condition annotations.

Axiomatization follows SemDok Consequence</rdfs:comment>
  </rdf:Description>
  <rdf:Description rdf:about="http://purl.org/olia/discourse/olia_discourse.owl#Consequence">
    <rdfs:label>consequence</rdfs:label>
  </rdf:Description>
  <rdf:Description rdf:about="http://purl.org/olia/discourse/olia_discourse.owl#Consequence">
    <rdfs:label xml:lang="en">consequence</rdfs:label>
  </rdf:Description>
  <rdf:Description rdf:about="http://purl.org/olia/discourse/olia_discourse.owl#Consequence">
    <rdfs:label>consequent</rdfs:label>
  </rdf:Description>
  <rdf:Description rdf:about="http://purl.org/olia/discourse/olia_discourse.owl#Consequence_RST">
    <rdf:type rdf:resource="http://www.w3.org/2002/07/owl#Class"/>
  </rdf:Description>
  <rdf:Description rdf:about="http://purl.org/olia/discourse/olia_discourse.owl#Consequence_RST">
    <rdfs:subClassOf rdf:resource="http://purl.org/olia/discourse/olia_discourse.owl#Consequence"/>
  </rdf:Description>
  <rdf:Description rdf:about="http://purl.org/olia/discourse/olia_discourse.owl#Consequence_RST">
    <rdfs:comment>In a consequence relation, the situation presented in one span is a consequence of the situation presented in the other span. (Carlson and Marcu 2001)

SemDok distinguishes three subtypes, which, however, only differ in nuclearity.</rdfs:comment>
  </rdf:Description>
  <rdf:Description rdf:about="http://purl.org/olia/discourse/olia_discourse.owl#Consequence_RST">
    <rdfs:label>consequence (RST)</rdfs:label>
  </rdf:Description>
  <rdf:Description rdf:about="http://purl.org/olia/discourse/olia_discourse.owl#Consequence_RST">
    <rdfs:label xml:lang="en">consequence (RST)</rdfs:label>
  </rdf:Description>
  <rdf:Description rdf:about="http://purl.org/olia/discourse/olia_discourse.owl#ContextualVariation">
    <rdf:type rdf:resource="http://www.w3.org/2002/07/owl#Class"/>
  </rdf:Description>
  <rdf:Description rdf:about="http://purl.org/olia/discourse/olia_discourse.owl#ContextualVariation">
    <rdfs:subClassOf rdf:resource="http://purl.org/olia/discourse/olia_discourse.owl#Possible"/>
  </rdf:Description>
  <rdf:Description rdf:about="http://purl.org/olia/discourse/olia_discourse.owl#ContextualVariation">
    <rdfs:comment>Variation on a particular usage or immediate proximity of words.</rdfs:comment>
  </rdf:Description>
  <rdf:Description rdf:about="http://purl.org/olia/discourse/olia_discourse.owl#ContextualVariation">
    <rdfs:isDefinedBy>http://www.isocat.org/datcat/DC-1977</rdfs:isDefinedBy>
  </rdf:Description>
  <rdf:Description rdf:about="http://purl.org/olia/discourse/olia_discourse.owl#Contigency">
    <rdf:type rdf:resource="http://www.w3.org/2002/07/owl#Class"/>
  </rdf:Description>
  <rdf:Description rdf:about="http://purl.org/olia/discourse/olia_discourse.owl#Contigency">
    <rdfs:subClassOf rdf:resource="http://purl.org/olia/discourse/olia_discourse.owl#CoherenceRelation"/>
  </rdf:Description>
  <rdf:Description rdf:about="http://purl.org/olia/discourse/olia_discourse.owl#Contigency">
    <rdfs:comment>The situations are (assumed to be) related by an abstract notion of recurrence or habituality (Carlson and Marcu 2001), often, one of the situations described in Arg1 and Arg2 causally influences the other. (Prasad et al. 2007).

cf. Wolf et al.'s "Cause-Effect": Cause-Effect relations establish a causal inference path between discourse segments.

Roughly corresponding to SemDok CauseResult. However, this is limited to ideational relations (subject-matter relations), whereas here, we follow PDTB to also include presentaitonal (interpersonal) relations (PragmaticCause).</rdfs:comment>
  </rdf:Description>
  <rdf:Description rdf:about="http://purl.org/olia/discourse/olia_discourse.owl#Contigency">
    <rdfs:label>cause-result</rdfs:label>
  </rdf:Description>
  <rdf:Description rdf:about="http://purl.org/olia/discourse/olia_discourse.owl#Contigency">
    <rdfs:label xml:lang="en">contigency</rdfs:label>
  </rdf:Description>
  <rdf:Description rdf:about="http://purl.org/olia/discourse/olia_discourse.owl#Contigency">
    <skos:prefLabel>contingency</skos:prefLabel>
  </rdf:Description>
  <rdf:Description rdf:about="http://purl.org/olia/discourse/olia_discourse.owl#Contigency_RST">
    <rdf:type rdf:resource="http://www.w3.org/2002/07/owl#Class"/>
  </rdf:Description>
  <rdf:Description rdf:about="http://purl.org/olia/discourse/olia_discourse.owl#Contigency_RST">
    <rdfs:subClassOf rdf:resource="http://purl.org/olia/discourse/olia_discourse.owl#HabitualCooccurrence"/>
  </rdf:Description>
  <rdf:Description rdf:about="http://purl.org/olia/discourse/olia_discourse.owl#Contigency_RST">
    <rdfs:comment>In a CONTINGENCY relation, the satellite suggests an abstract notion of recurrence or habituality. Hence, the expression of time, place, or condition is not the primary focus.
(Carlson and Marcu 2001)</rdfs:comment>
  </rdf:Description>
  <rdf:Description rdf:about="http://purl.org/olia/discourse/olia_discourse.owl#Contigency_RST">
    <rdfs:label xml:lang="en">contigency (RST)</rdfs:label>
  </rdf:Description>
  <rdf:Description rdf:about="http://purl.org/olia/discourse/olia_discourse.owl#Continent">
    <rdf:type rdf:resource="http://www.w3.org/2002/07/owl#Class"/>
  </rdf:Description>
  <rdf:Description rdf:about="http://purl.org/olia/discourse/olia_discourse.owl#Continent">
    <rdfs:subClassOf rdf:resource="http://purl.org/olia/discourse/olia_discourse.owl#GeographicalFeature"/>
  </rdf:Description>
  <rdf:Description rdf:about="http://purl.org/olia/discourse/olia_discourse.owl#Continent">
    <rdfs:comment xml:lang="en">for nerd:Continent</rdfs:comment>
  </rdf:Description>
  <rdf:Description rdf:about="http://purl.org/olia/discourse/olia_discourse.owl#ContraExpectation">
    <rdf:type rdf:resource="http://www.w3.org/2002/07/owl#Class"/>
  </rdf:Description>
  <rdf:Description rdf:about="http://purl.org/olia/discourse/olia_discourse.owl#ContraExpectation">
    <rdfs:subClassOf rdf:resource="http://purl.org/olia/discourse/olia_discourse.owl#Concession"/>
  </rdf:Description>
  <rdf:Description rdf:about="http://purl.org/olia/discourse/olia_discourse.owl#ContraExpectation">
    <inverseOf rdf:resource="http://purl.org/olia/discourse/Expectation"/>
  </rdf:Description>
  <rdf:Description rdf:about="http://purl.org/olia/discourse/olia_discourse.owl#ContraExpectation">
    <rdfs:comment>expectation denier</rdfs:comment>
  </rdf:Description>
  <rdf:Description rdf:about="http://purl.org/olia/discourse/olia_discourse.owl#ContraExpectation">
    <rdfs:comment>PDTB COMPARISON/Concession/contra-expectation: Arg1 creates an expectation that Arg2 denies. (Prasad et al. 2007)

ISO DR-Core: Concession, argument expectation-denier (Bunt &amp; Prasad, ISA-12)</rdfs:comment>
  </rdf:Description>
  <rdf:Description rdf:about="http://purl.org/olia/discourse/olia_discourse.owl#ContraExpectation">
    <rdfs:label xml:lang="en">contra expectation</rdfs:label>
  </rdf:Description>
  <rdf:Description rdf:about="http://purl.org/olia/discourse/olia_discourse.owl#ContraExpectation">
    <rdfs:label>contra-expectation</rdfs:label>
  </rdf:Description>
  <rdf:Description rdf:about="http://purl.org/olia/discourse/olia_discourse.owl#ContraExpectation">
    <rdfs:label>contraexpectation</rdfs:label>
  </rdf:Description>
  <rdf:Description rdf:about="http://purl.org/olia/discourse/olia_discourse.owl#ContraExpectation">
    <rdfs:label>counterexpectation</rdfs:label>
  </rdf:Description>
  <rdf:Description rdf:about="http://purl.org/olia/discourse/olia_discourse.owl#Contrast">
    <rdf:type rdf:resource="http://www.w3.org/2002/07/owl#Class"/>
  </rdf:Description>
  <rdf:Description rdf:about="http://purl.org/olia/discourse/olia_discourse.owl#Contrast">
    <rdfs:subClassOf rdf:resource="http://purl.org/olia/discourse/olia_discourse.owl#ContrastiveComparison"/>
  </rdf:Description>
  <rdf:Description rdf:about="http://purl.org/olia/discourse/olia_discourse.owl#Contrast">
    <rdfs:comment>The situations presented in the arguments come in contrast with each other along some dimension. The contrast may happen in only one or few respects, while everything else can remain the same in other respects. Typically, a CONTRAST relation includes a contrastive discourse cue, such as "but", "however", "while". (Carlson and Marcu 2001)

Distinguished from PDTB "Contrast" as a generalization over PDTB "Contrast" and "Pragmatic Contrast" (Ch. Chiarcos), This definition is in line with the ISO relation "Contrast" and corresponds to it notably in the exclusion of Concessions,</rdfs:comment>
  </rdf:Description>
  <rdf:Description rdf:about="http://purl.org/olia/discourse/olia_discourse.owl#Contrast">
    <rdfs:label xml:lang="en">contrast</rdfs:label>
  </rdf:Description>
  <rdf:Description rdf:about="http://purl.org/olia/discourse/olia_discourse.owl#Contrast">
    <skos:prefLabel>contrast</skos:prefLabel>
  </rdf:Description>
  <rdf:Description rdf:about="http://purl.org/olia/discourse/olia_discourse.owl#Contrast_RST">
    <rdf:type rdf:resource="http://www.w3.org/2002/07/owl#Class"/>
  </rdf:Description>
  <rdf:Description rdf:nodeID="genid30">
    <rdf:type rdf:resource="http://www.w3.org/2002/07/owl#Class"/>
  </rdf:Description>
  <rdf:Description rdf:nodeID="genid31">
    <rdf:first rdf:resource="http://purl.org/olia/discourse/olia_discourse.owl#Contrast"/>
  </rdf:Description>
  <rdf:Description rdf:nodeID="genid32">
    <rdf:first rdf:resource="http://purl.org/olia/discourse/olia_discourse.owl#ParatacticDiscourseRelation"/>
  </rdf:Description>
  <rdf:Description rdf:nodeID="genid31">
    <rdf:rest rdf:nodeID="genid32"/>
  </rdf:Description>
  <rdf:Description rdf:nodeID="genid32">
    <rdf:rest rdf:resource="http://www.w3.org/1999/02/22-rdf-syntax-ns#nil"/>
  </rdf:Description>
  <rdf:Description rdf:nodeID="genid30">
    <owl:intersectionOf rdf:nodeID="genid31"/>
  </rdf:Description>
  <rdf:Description rdf:about="http://purl.org/olia/discourse/olia_discourse.owl#Contrast_RST">
    <owl:equivalentClass rdf:nodeID="genid30"/>
  </rdf:Description>
  <rdf:Description rdf:about="http://purl.org/olia/discourse/olia_discourse.owl#Contrast_RST">
    <rdfs:comment>In a CONTRAST relation, two or more nuclei come in contrast with each other along some dimension. The contrast may happen in only one or few respects, while everything else can remain the same in other respects. Typically, a CONTRAST relation includes a contrastive discourse cue, such as but, however, while, whereas a COMPARISON does not.
(Carlson and Marcu 2001)

No more than two nuclei; the situations in these two nuclei are (a) comprehended as the same in many respects (b) comprehended as differing in a few respects and (c) compared with respect to one or more of these differences (Mann and Taboada 2010).

Corresponds to SemDok Contrast-multi</rdfs:comment>
  </rdf:Description>
  <rdf:Description rdf:about="http://purl.org/olia/discourse/olia_discourse.owl#Contrast_RST">
    <rdfs:label>contrast</rdfs:label>
  </rdf:Description>
  <rdf:Description rdf:about="http://purl.org/olia/discourse/olia_discourse.owl#Contrast_RST">
    <rdfs:label>contrast (RST)</rdfs:label>
  </rdf:Description>
  <rdf:Description rdf:about="http://purl.org/olia/discourse/olia_discourse.owl#Contrast_RST">
    <rdfs:label xml:lang="en">contrast (RST)</rdfs:label>
  </rdf:Description>
  <rdf:Description rdf:about="http://purl.org/olia/discourse/olia_discourse.owl#Contrast_RST">
    <skos:prefLabel>contrast (multi)</skos:prefLabel>
  </rdf:Description>
  <rdf:Description rdf:about="http://purl.org/olia/discourse/olia_discourse.owl#ContrastiveComparison">
    <rdf:type rdf:resource="http://www.w3.org/2002/07/owl#Class"/>
  </rdf:Description>
  <rdf:Description rdf:about="http://purl.org/olia/discourse/olia_discourse.owl#ContrastiveComparison">
    <rdfs:subClassOf rdf:resource="http://purl.org/olia/discourse/olia_discourse.owl#Comparison"/>
  </rdf:Description>
  <rdf:Description rdf:about="http://purl.org/olia/discourse/olia_discourse.owl#ContrastiveComparison">
    <rdfs:comment>Generalization over RST/PDTB contrast and concession.

Cf. Contrast as defined by Wolf et al. (2003): Infer a set of entities from DS0, E(DS0), and a set of entities from DS1, E(DS1). Then infer contrasts between members of E(DS0) and E(DS1).
• Contrast-1 is a contrast between corresponding predicates in DS0 and DS1. The
arguments of these contrasting predicates are identical.
• Contrast-2 is a contrast between the arguments of corresponding predicates in DS0
and DS1. The predicates over these contrasting arguments are identical.

Corresponds to SemDok Contrast (generalization over Concession, Antithesis and Contrast).</rdfs:comment>
  </rdf:Description>
  <rdf:Description rdf:about="http://purl.org/olia/discourse/olia_discourse.owl#ContrastiveComparison">
    <rdfs:label>contrast</rdfs:label>
  </rdf:Description>
  <rdf:Description rdf:about="http://purl.org/olia/discourse/olia_discourse.owl#ContrastiveComparison">
    <rdfs:label xml:lang="en">contrastive comparison</rdfs:label>
  </rdf:Description>
  <rdf:Description rdf:about="http://purl.org/olia/discourse/olia_discourse.owl#ContrastiveComparison">
    <skos:prefLabel>contrastive comparison</skos:prefLabel>
  </rdf:Description>
  <rdf:Description rdf:about="http://purl.org/olia/discourse/olia_discourse.owl#ContrastiveFocus">
    <rdf:type rdf:resource="http://www.w3.org/2002/07/owl#Class"/>
  </rdf:Description>
  <rdf:Description rdf:about="http://purl.org/olia/discourse/olia_discourse.owl#ContrastiveFocus">
    <rdfs:subClassOf rdf:resource="http://purl.org/olia/discourse/olia_discourse.owl#DenotationFocus"/>
  </rdf:Description>
  <rdf:Description rdf:about="http://purl.org/olia/discourse/olia_discourse.owl#ContrastiveFocus">
    <rdfs:comment>The contrastive focus (cf) is that element of the sentence that evokes a notion of contrast to (an element of) another utterance. (SFB632 guidelines)

Contrastive focus may also extend over different domains of an utterance. In alternative questions and the answers to them it covers the whole CP. E.g.

WORDS: Is it raining or not ? CFocus: [ _cf It is raining] or [ _cf not]. WORDS: Yes , it is . NFocus: Yes, [ _nf it is]. CFocus: Yes, [ _cf it is]. (5.3)

Also referred to as "identificational focus", or "alternative focus".</rdfs:comment>
  </rdf:Description>
  <rdf:Description rdf:about="http://purl.org/olia/discourse/olia_discourse.owl#ContrastiveFocus">
    <rdfs:label xml:lang="en">contrastive focus</rdfs:label>
  </rdf:Description>
  <rdf:Description rdf:about="http://purl.org/olia/discourse/olia_discourse.owl#Coordination">
    <rdf:type rdf:resource="http://www.w3.org/2002/07/owl#Class"/>
  </rdf:Description>
  <rdf:Description rdf:about="http://purl.org/olia/discourse/olia_discourse.owl#Coordination">
    <rdfs:subClassOf rdf:resource="http://purl.org/olia/discourse/olia_discourse.owl#List"/>
  </rdf:Description>
  <rdf:Description rdf:about="http://purl.org/olia/discourse/olia_discourse.owl#Coordination">
    <rdfs:comment>cf. SemDok List-coordination. No definition provided, but this could be meant for cases of (otherwise uninterpreted) syntactic coordination between discourse units.</rdfs:comment>
  </rdf:Description>
  <rdf:Description rdf:about="http://purl.org/olia/discourse/olia_discourse.owl#Coordination">
    <rdfs:label>coordination</rdfs:label>
  </rdf:Description>
  <rdf:Description rdf:about="http://purl.org/olia/discourse/olia_discourse.owl#Coordination">
    <rdfs:label xml:lang="en">coordination</rdfs:label>
  </rdf:Description>
  <rdf:Description rdf:about="http://purl.org/olia/discourse/olia_discourse.owl#Coordination">
    <skos:prefLabel>list/coordination</skos:prefLabel>
  </rdf:Description>
  <rdf:Description rdf:about="http://purl.org/olia/discourse/olia_discourse.owl#Country">
    <rdf:type rdf:resource="http://www.w3.org/2002/07/owl#Class"/>
  </rdf:Description>
  <rdf:Description rdf:about="http://purl.org/olia/discourse/olia_discourse.owl#Country">
    <rdfs:subClassOf rdf:resource="http://purl.org/olia/discourse/olia_discourse.owl#PoliticalUnit"/>
  </rdf:Description>
  <rdf:Description rdf:about="http://purl.org/olia/discourse/olia_discourse.owl#Country">
    <rdfs:comment xml:lang="en">for nerd:Country</rdfs:comment>
  </rdf:Description>
  <rdf:Description rdf:about="http://purl.org/olia/discourse/olia_discourse.owl#Criminal">
    <rdf:type rdf:resource="http://www.w3.org/2002/07/owl#Class"/>
  </rdf:Description>
  <rdf:Description rdf:about="http://purl.org/olia/discourse/olia_discourse.owl#Criminal">
    <rdfs:subClassOf rdf:resource="http://purl.org/olia/discourse/olia_discourse.owl#Person"/>
  </rdf:Description>
  <rdf:Description rdf:about="http://purl.org/olia/discourse/olia_discourse.owl#Criminal">
    <rdfs:comment xml:lang="en">for nerd:Criminal and extractiv:CRIMINAL</rdfs:comment>
  </rdf:Description>
  <rdf:Description rdf:about="http://purl.org/olia/discourse/olia_discourse.owl#Date">
    <rdf:type rdf:resource="http://www.w3.org/2002/07/owl#Class"/>
  </rdf:Description>
  <rdf:Description rdf:about="http://purl.org/olia/discourse/olia_discourse.owl#Date">
    <rdfs:subClassOf rdf:resource="http://purl.org/olia/olia-top.owl#TextStructuralUnit"/>
  </rdf:Description>
  <rdf:Description rdf:about="http://purl.org/olia/discourse/olia_discourse.owl#Date">
    <rdfs:comment>When a date is provided at the beginning of the document, and it refers to the
rest of the article, the DATE schema should be used. It may also be used for subsections of the
document. It should be linked to a TEXT or SECTIONTEXT schema.  (Carlson and Marcu 2001)</rdfs:comment>
  </rdf:Description>
  <rdf:Description rdf:about="http://purl.org/olia/discourse/olia_discourse.owl#Date">
    <rdfs:label xml:lang="en">date</rdfs:label>
  </rdf:Description>
  <rdf:Description rdf:about="http://purl.org/olia/discourse/olia_discourse.owl#Definite">
    <rdf:type rdf:resource="http://www.w3.org/2002/07/owl#Class"/>
  </rdf:Description>
  <rdf:Description rdf:about="http://purl.org/olia/discourse/olia_discourse.owl#Definite">
    <rdfs:subClassOf rdf:resource="http://purl.org/olia/discourse/olia_discourse.owl#Definiteness"/>
  </rdf:Description>
  <rdf:Description rdf:about="http://purl.org/olia/discourse/olia_discourse.owl#Definite">
    <rdfs:label xml:lang="en">definite</rdfs:label>
  </rdf:Description>
  <rdf:Description rdf:about="http://purl.org/olia/discourse/olia_discourse.owl#Definiteness">
    <rdf:type rdf:resource="http://www.w3.org/2002/07/owl#Class"/>
  </rdf:Description>
  <rdf:Description rdf:about="http://purl.org/olia/discourse/olia_discourse.owl#Definiteness">
    <rdfs:subClassOf rdf:resource="http://purl.org/olia/discourse/olia_discourse.owl#SemanticFeature"/>
  </rdf:Description>
  <rdf:Description rdf:about="http://purl.org/olia/discourse/olia_discourse.owl#Definiteness">
    <rdfs:comment>(Semantic) definiteness means that an expression is morphosyntactically marked as hearer-known (definite or pronominal) and the hearer can infer exactly one entity to which this description applies at the current point in discourse, either because it is unique (Russel 1937), or it is the most salient entity in the current situation to which the referring expression may apply (Lewis 1979, v. Heusinger 1996). In particular, most pronuns are also definite as they refer to one particular antecedent.</rdfs:comment>
  </rdf:Description>
  <rdf:Description rdf:about="http://purl.org/olia/discourse/olia_discourse.owl#Definiteness">
    <rdfs:label xml:lang="en">definiteness</rdfs:label>
  </rdf:Description>
  <rdf:Description rdf:about="http://purl.org/olia/discourse/olia_discourse.owl#Definition">
    <rdf:type rdf:resource="http://www.w3.org/2002/07/owl#Class"/>
  </rdf:Description>
  <rdf:Description rdf:about="http://purl.org/olia/discourse/olia_discourse.owl#Definition">
    <rdfs:subClassOf rdf:resource="http://purl.org/olia/discourse/olia_discourse.owl#Assessment"/>
  </rdf:Description>
  <rdf:Description rdf:about="http://purl.org/olia/discourse/olia_discourse.owl#Definition">
    <rdfs:comment>Introduced as generalization over Definition_RST and ElaborationDefinition (from SemDok). In fact, these may just be equivalent.</rdfs:comment>
  </rdf:Description>
  <rdf:Description rdf:about="http://purl.org/olia/discourse/olia_discourse.owl#Definition">
    <rdfs:label xml:lang="en">definition</rdfs:label>
  </rdf:Description>
  <rdf:Description rdf:about="http://purl.org/olia/discourse/olia_discourse.owl#Definition_RST">
    <rdf:type rdf:resource="http://www.w3.org/2002/07/owl#Class"/>
  </rdf:Description>
  <rdf:Description rdf:about="http://purl.org/olia/discourse/olia_discourse.owl#Definition_RST">
    <rdfs:subClassOf rdf:resource="http://purl.org/olia/discourse/olia_discourse.owl#Definition"/>
  </rdf:Description>
  <rdf:Description rdf:about="http://purl.org/olia/discourse/olia_discourse.owl#Definition_RST">
    <rdfs:comment>In a DEFINITION relation, the satellite gives a definition of the nucleus.
(Carlson and Marcu 2001)</rdfs:comment>
  </rdf:Description>
  <rdf:Description rdf:about="http://purl.org/olia/discourse/olia_discourse.owl#Definition_RST">
    <rdfs:label xml:lang="en">definition (RST)</rdfs:label>
  </rdf:Description>
  <rdf:Description rdf:about="http://purl.org/olia/discourse/olia_discourse.owl#DenotationFocus">
    <rdf:type rdf:resource="http://www.w3.org/2002/07/owl#Class"/>
  </rdf:Description>
  <rdf:Description rdf:about="http://purl.org/olia/discourse/olia_discourse.owl#DenotationFocus">
    <rdfs:subClassOf rdf:resource="http://purl.org/olia/discourse/olia_discourse.owl#Focus"/>
  </rdf:Description>
  <rdf:Description rdf:about="http://purl.org/olia/discourse/olia_discourse.owl#DenotationFocus">
    <rdfs:comment>Krifka distinguishes between ‘expression focus’ and ‘denotation focus.’ Differences in meaning are only found in the latter kind of focus, on which we concentrate here.

...

Some semantic uses of focus are focus-sensitive particles (socalled
‘association with focus’ cases), negations, reason clauses and restrictors of quantifiers.

It is important to understand which subclasses of focus can be expressed by grammatical means, even if the distinction is only realized in a small group of languages. In the SFB annotation guidelines, ‘focus’ is subcategorized into new and contrastive.
(Féry et al. 2007)</rdfs:comment>
  </rdf:Description>
  <rdf:Description rdf:about="http://purl.org/olia/discourse/olia_discourse.owl#DenotationFocus">
    <rdfs:label xml:lang="en">denotation focus</rdfs:label>
  </rdf:Description>
  <rdf:Description rdf:about="http://purl.org/olia/discourse/olia_discourse.owl#Deprecated">
    <rdf:type rdf:resource="http://www.w3.org/2002/07/owl#Class"/>
  </rdf:Description>
  <rdf:Description rdf:about="http://purl.org/olia/discourse/olia_discourse.owl#Deprecated">
    <rdfs:subClassOf rdf:resource="http://purl.org/olia/discourse/olia_discourse.owl#TemporallyDefinedUsage"/>
  </rdf:Description>
  <rdf:Description rdf:about="http://purl.org/olia/discourse/olia_discourse.owl#Deprecated">
    <rdfs:comment>Deprecated Term: A term rated according to the scale of a term acceptability rating as undesired. (Sue Ellen Wright, http://www.isocat.org/datcat/DC-378)
      
      Superseded Term: A term that is no longer preferred or admitted. (Sue Ellen Wright, http://www.isocat.org/datcat/DC-379)
      
      Obsolete Form: A term or lexeme which is no longer in common use. (Sue Ellen Wright, http://www.isocat.org/datcat/DC-506)
      </rdfs:comment>
  </rdf:Description>
  <rdf:Description rdf:about="http://purl.org/olia/discourse/olia_discourse.owl#Deprecated">
    <rdfs:isDefinedBy>http://www.isocat.org/datcat/DC-378, http://www.isocat.org/datcat/DC-379</rdfs:isDefinedBy>
  </rdf:Description>
  <rdf:Description rdf:about="http://purl.org/olia/discourse/olia_discourse.owl#Deprecated">
    <rdfs:label>deprecated</rdfs:label>
  </rdf:Description>
  <rdf:Description rdf:about="http://purl.org/olia/discourse/olia_discourse.owl#Deprecated">
    <rdfs:label>deprecated term</rdfs:label>
  </rdf:Description>
  <rdf:Description rdf:about="http://purl.org/olia/discourse/olia_discourse.owl#Deprecated">
    <rdfs:label>obsolete</rdfs:label>
  </rdf:Description>
  <rdf:Description rdf:about="http://purl.org/olia/discourse/olia_discourse.owl#Deprecated">
    <rdfs:label>obsolete form</rdfs:label>
  </rdf:Description>
  <rdf:Description rdf:about="http://purl.org/olia/discourse/olia_discourse.owl#Deprecated">
    <rdfs:label>superseded</rdfs:label>
  </rdf:Description>
  <rdf:Description rdf:about="http://purl.org/olia/discourse/olia_discourse.owl#Deprecated">
    <rdfs:label>superseded term</rdfs:label>
  </rdf:Description>
  <rdf:Description rdf:about="http://purl.org/olia/discourse/olia_discourse.owl#DeterminateAttribution">
    <rdf:type rdf:resource="http://www.w3.org/2002/07/owl#Class"/>
  </rdf:Description>
  <rdf:Description rdf:about="http://purl.org/olia/discourse/olia_discourse.owl#DeterminateAttribution">
    <rdfs:subClassOf rdf:resource="http://purl.org/olia/discourse/olia_discourse.owl#Attribution"/>
  </rdf:Description>
  <rdf:Description rdf:about="http://purl.org/olia/discourse/olia_discourse.owl#DeterminateAttribution">
    <rdfs:comment>Classification of Attribute relations with respect to their "determinacy", which signals a context that cancels what would otherwise be an entailment of attribution.
The determinacy feature captures the fact that the attribution over a relation or argument can itself be cancelled in particular contexts, such as within negated, conditional, and infinitive contexts.
Determinate contexts are simply marked by the default “Null”. (Prasad et al. 2007)
</rdfs:comment>
  </rdf:Description>
  <rdf:Description rdf:about="http://purl.org/olia/discourse/olia_discourse.owl#DeterminateAttribution">
    <rdfs:label xml:lang="en">determinate attribution</rdfs:label>
  </rdf:Description>
  <rdf:Description rdf:about="http://purl.org/olia/discourse/olia_discourse.owl#DialectRegister">
    <rdf:type rdf:resource="http://www.w3.org/2002/07/owl#Class"/>
  </rdf:Description>
  <rdf:Description rdf:about="http://purl.org/olia/discourse/olia_discourse.owl#DialectRegister">
    <rdfs:subClassOf rdf:resource="http://purl.org/olia/olia-top.owl#RegisterFeature"/>
  </rdf:Description>
  <rdf:Description rdf:about="http://purl.org/olia/discourse/olia_discourse.owl#DialectRegister">
    <rdfs:comment>
                            Register that is specific to a dialect.
                                (http://www.isocat.org/datcat/DC-1990)
                            </rdfs:comment>
  </rdf:Description>
  <rdf:Description rdf:about="http://purl.org/olia/discourse/olia_discourse.owl#DialectRegister">
    <rdfs:label>dialect register</rdfs:label>
  </rdf:Description>
  <rdf:Description rdf:about="http://purl.org/olia/discourse/olia_discourse.owl#DialectRegister">
    <owl:versionInfo>http://www.isocat.org/datcat/DC-1990</owl:versionInfo>
  </rdf:Description>
  <rdf:Description rdf:about="http://purl.org/olia/discourse/olia_discourse.owl#DialectRegister">
    <owl:versionInfo>subClassOf register (dcif:conceptualDomain)</owl:versionInfo>
  </rdf:Description>
  <rdf:Description rdf:about="http://purl.org/olia/discourse/olia_discourse.owl#DialogRelation">
    <rdf:type rdf:resource="http://www.w3.org/2002/07/owl#Class"/>
  </rdf:Description>
  <rdf:Description rdf:about="http://purl.org/olia/discourse/olia_discourse.owl#DialogRelation">
    <rdfs:subClassOf rdf:resource="http://purl.org/olia/discourse/olia_discourse.owl#DiscourseRelation"/>
  </rdf:Description>
  <rdf:Description rdf:about="http://purl.org/olia/discourse/olia_discourse.owl#DialogRelation">
    <rdfs:subClassOf rdf:resource="http://purl.org/olia/discourse/olia_discourse.owl#PresentationalRelation"/>
  </rdf:Description>
  <rdf:Description rdf:about="http://purl.org/olia/discourse/olia_discourse.owl#DialogRelation">
    <rdfs:comment>added as generalization over ISO FunctionalDependence (response from one interlocutor) and FeedbackDependence (questions, answers and meta communication). Extended to quasi-dialoguous relations (rhetorical questions).
Note that PDTB, CCR and RST don't cover dialogue acts.

Likewise, SemDok doesn't address dialogs. However, dialog relations clearly have an interpersonal function. Because of the modelling of dialog relations as interpersonal, this entails that they are presentational.</rdfs:comment>
  </rdf:Description>
  <rdf:Description rdf:about="http://purl.org/olia/discourse/olia_discourse.owl#DialogRelation">
    <rdfs:label xml:lang="en">dialog relation</rdfs:label>
  </rdf:Description>
  <rdf:Description rdf:about="http://purl.org/olia/discourse/olia_discourse.owl#DirectSpeech">
    <rdf:type rdf:resource="http://www.w3.org/2002/07/owl#Class"/>
  </rdf:Description>
  <rdf:Description rdf:about="http://purl.org/olia/discourse/olia_discourse.owl#DirectSpeech">
    <rdfs:subClassOf rdf:resource="http://purl.org/olia/olia-top.owl#NarrativeType"/>
  </rdf:Description>
  <rdf:Description rdf:about="http://purl.org/olia/discourse/olia_discourse.owl#DirectSpeech">
    <rdfs:comment>added in accordance with TIGER</rdfs:comment>
  </rdf:Description>
  <rdf:Description rdf:about="http://purl.org/olia/discourse/olia_discourse.owl#DirectSpeech">
    <owl:versionInfo>added in accordance with TIGER</owl:versionInfo>
  </rdf:Description>
  <rdf:Description rdf:about="http://purl.org/olia/discourse/olia_discourse.owl#DiscourseAdverbial">
    <rdf:type rdf:resource="http://www.w3.org/2002/07/owl#Class"/>
  </rdf:Description>
  <rdf:Description rdf:about="http://purl.org/olia/discourse/olia_discourse.owl#DiscourseAdverbial">
    <rdfs:subClassOf rdf:resource="http://purl.org/olia/discourse/olia_discourse.owl#ExplicitConnective"/>
  </rdf:Description>
  <rdf:Description rdf:about="http://purl.org/olia/discourse/olia_discourse.owl#DiscourseAdverbial">
    <rdfs:comment>adopted from SemDok</rdfs:comment>
  </rdf:Description>
  <rdf:Description rdf:about="http://purl.org/olia/discourse/olia_discourse.owl#DiscourseAdverbial">
    <rdfs:label>discourse adverbial</rdfs:label>
  </rdf:Description>
  <rdf:Description rdf:about="http://purl.org/olia/discourse/olia_discourse.owl#DiscourseAdverbial">
    <rdfs:label xml:lang="en">discourse adverbial</rdfs:label>
  </rdf:Description>
  <rdf:Description rdf:about="http://purl.org/olia/discourse/olia_discourse.owl#DiscourseFunction">
    <rdf:type rdf:resource="http://www.w3.org/2002/07/owl#Class"/>
  </rdf:Description>
  <rdf:Description rdf:about="http://purl.org/olia/discourse/olia_discourse.owl#DiscourseFunction">
    <rdfs:subClassOf rdf:resource="http://purl.org/olia/olia-top.owl#PragmaticFeature"/>
  </rdf:Description>
  <rdf:Description rdf:about="http://purl.org/olia/discourse/olia_discourse.owl#DiscourseFunction">
    <rdfs:label xml:lang="en">discourse function</rdfs:label>
  </rdf:Description>
  <rdf:Description rdf:about="http://purl.org/olia/discourse/olia_discourse.owl#DiscourseReferent">
    <rdf:type rdf:resource="http://www.w3.org/2002/07/owl#Class"/>
  </rdf:Description>
  <rdf:Description rdf:about="http://purl.org/olia/discourse/olia_discourse.owl#DiscourseReferent">
    <rdfs:subClassOf rdf:resource="http://purl.org/olia/olia-top.owl#DiscourseEntity"/>
  </rdf:Description>
  <rdf:Description rdf:nodeID="genid33">
    <rdf:type rdf:resource="http://www.w3.org/2002/07/owl#Restriction"/>
  </rdf:Description>
  <rdf:Description rdf:nodeID="genid33">
    <owl:onProperty rdf:resource="http://purl.org/olia/discourse/olia_discourse.owl#hasInformationStatus"/>
  </rdf:Description>
  <rdf:Description rdf:nodeID="genid33">
    <owl:cardinality rdf:datatype="http://www.w3.org/2001/XMLSchema#nonNegativeInteger">1</owl:cardinality>
  </rdf:Description>
  <rdf:Description rdf:about="http://purl.org/olia/discourse/olia_discourse.owl#DiscourseReferent">
    <rdfs:subClassOf rdf:nodeID="genid33"/>
  </rdf:Description>
  <rdf:Description rdf:about="http://purl.org/olia/discourse/olia_discourse.owl#DiscourseReferent">
    <rdfs:comment>A prototypical object that is referred to in discourse (Karttunen 1972).</rdfs:comment>
  </rdf:Description>
  <rdf:Description rdf:about="http://purl.org/olia/discourse/olia_discourse.owl#DiscourseReferent">
    <rdfs:label xml:lang="en">discourse referent</rdfs:label>
  </rdf:Description>
  <rdf:Description rdf:about="http://purl.org/olia/discourse/olia_discourse.owl#DiscourseRelation">
    <rdf:type rdf:resource="http://www.w3.org/2002/07/owl#Class"/>
  </rdf:Description>
  <rdf:Description rdf:about="http://purl.org/olia/discourse/olia_discourse.owl#DiscourseRelation">
    <rdfs:subClassOf rdf:resource="http://purl.org/olia/discourse/olia_discourse.owl#PragmaticRelation"/>
  </rdf:Description>
  <rdf:Description rdf:about="http://purl.org/olia/discourse/olia_discourse.owl#DiscourseRelation">
    <rdfs:comment>corresponds to SemDok RhetoricalRelation (but not DiscourseRelation)</rdfs:comment>
  </rdf:Description>
  <rdf:Description rdf:about="http://purl.org/olia/discourse/olia_discourse.owl#DiscourseRelation">
    <rdfs:comment>Relation between discourse segments. (Mann and Thompson 1988)
In order to distangle discourse-syntactic (paratactic/hypotactic) and functional-semantic aspects, DiscourseRelation is distinguished from DiscourseStructuralPattern: DiscourseRelations defined discourse relations in terms of their communicative function and underlying semantics. An RST antithesis, for example, is thus to be defined both as a ContrastRelation (subclass of DiscourseRelation) and as a HypotacticDiscourseRelation (subclass of DiscourseStructuralPattern).

Note that Attribution is modelled here as a relation (as in RST), not as a feature (as in PDTB).</rdfs:comment>
  </rdf:Description>
  <rdf:Description rdf:about="http://purl.org/olia/discourse/olia_discourse.owl#DiscourseRelation">
    <rdfs:label>discourse relation</rdfs:label>
  </rdf:Description>
  <rdf:Description rdf:about="http://purl.org/olia/discourse/olia_discourse.owl#DiscourseRelation">
    <rdfs:label xml:lang="en">discourse relation</rdfs:label>
  </rdf:Description>
  <rdf:Description rdf:about="http://purl.org/olia/discourse/olia_discourse.owl#DiscourseRelation">
    <rdfs:label>rhetorical relation</rdfs:label>
  </rdf:Description>
  <rdf:Description rdf:about="http://purl.org/olia/discourse/olia_discourse.owl#DiscourseRelation">
    <owl:versionInfo>The taxonomy of DiscourseRelations follows roughly the Penn Discourse Treebank (Prasad et al. 2007), with additions in accordance to the Hindi Discourse Relation Bank (HDRB, Oza et al. 2009), the Italian LUNA corpus (Tonelli et al. 2010), the Leeds Arabic Discourse Treebank  (LADTB, Al-Saif and Markert  2010) and an alignment with Carlson and Marcu's (2001) RST relations and with Wolf et al.'s (2003, PDGB) coherence relations. Unaligned relations are marked by suffixes RST (for classical RST and RDTDTB relations) on the one hand and PDTB, HDRB, LUNA and LADTB on the other hand. No indices are used are used if a relation can be confirmed for at least two families of annotation schemes (PDTB, RSTDTB, PDGB).

We provide two, intersection subclassifications of discourse relations:
- ideational, interpersonal and textual (following SemDoc, i.e., the RST tradition)
- entity relations and (other) coherence relations (following PDTB)

With the following overlaps:
- entity relations are ideational relations
- interpersonal relations are coherence relations
- textual relations (not addressed in PDTB) are disjoint from both entity and coherence relations

However, the RST-style classification is encoded via subclasses of discourse function, the PDTB-style classification (along with additional concepts for textual patterns and dialog relations) is encoded via subclasses of discourse relation.</owl:versionInfo>
  </rdf:Description>
  <rdf:Description rdf:about="http://purl.org/olia/discourse/olia_discourse.owl#DiscourseSegment">
    <rdf:type rdf:resource="http://www.w3.org/2002/07/owl#Class"/>
  </rdf:Description>
  <rdf:Description rdf:about="http://purl.org/olia/discourse/olia_discourse.owl#DiscourseSegment">
    <rdfs:subClassOf rdf:resource="http://purl.org/olia/olia-top.owl#DiscourseEntity"/>
  </rdf:Description>
  <rdf:Description rdf:about="http://purl.org/olia/discourse/olia_discourse.owl#DiscourseSegment">
    <rdfs:comment>cf. SemDok DiscourseSegment</rdfs:comment>
  </rdf:Description>
  <rdf:Description rdf:about="http://purl.org/olia/discourse/olia_discourse.owl#DiscourseSegment">
    <rdfs:comment>roughly corresponds to the notion of "Arguments" in PDTB:

Argument of a Relation, e.g., a connective. Syntactically characterized as Simple clauses, certain VP coordinations (the conjunction in a coordinated verb phase is not annotated as a distinct discourse connective, but one or more verb phrases within the coordinated structure can be annotated as the argument of another connective), certain nominalizations, anaphoric expressions denoting abstract objects  (like "this", or "that" or "so"), responses to questions
(Prasad et al. 2007)</rdfs:comment>
  </rdf:Description>
  <rdf:Description rdf:about="http://purl.org/olia/discourse/olia_discourse.owl#DiscourseSegment">
    <rdfs:comment>Cognitive representation representing a longer stretch of discourse (Grosz and Sidner 1986), defined by a particular "discourse segment purpose" (Grosz and Sidner 1986), a specific propositional content of the relation between dependent DiscourseSegments, or the propositional content of the text contained in a minimal discourse segment (Mann and Thompson 1988). DiscourseSegments are interconnected by DiscourseRelations in a hierarchical and sequential structure.</rdfs:comment>
  </rdf:Description>
  <rdf:Description rdf:about="http://purl.org/olia/discourse/olia_discourse.owl#DiscourseSegment">
    <rdfs:comment>Discourse segment (discourse unit) is a segment of discourse that represents either an elementary discourse unit (e.g., a clause, proposition) or a complex discourse unit (constituted by several discourse units). Depending on theory, discourse segments reflect the scope of quantifiers and discourse connectives (Kamp 1982, Asher and Lascarides 2003), turn- or paragraph-like structures (Grosz and Sidner 1986) or range and domain of discourse relations (cf. Mann and Thompson 1988, Carlson et al. 2003).</rdfs:comment>
  </rdf:Description>
  <rdf:Description rdf:about="http://purl.org/olia/discourse/olia_discourse.owl#DiscourseSegment">
    <rdfs:comment>Near-synonyms in RST literature are "discourse unit" (Carlsson et al. 2003) and "text span" (Mann and Thompson 1988).</rdfs:comment>
  </rdf:Description>
  <rdf:Description rdf:about="http://purl.org/olia/discourse/olia_discourse.owl#DiscourseSegment">
    <rdfs:label>argument (PDTB)</rdfs:label>
  </rdf:Description>
  <rdf:Description rdf:about="http://purl.org/olia/discourse/olia_discourse.owl#DiscourseSegment">
    <rdfs:label>discourse segment</rdfs:label>
  </rdf:Description>
  <rdf:Description rdf:about="http://purl.org/olia/discourse/olia_discourse.owl#DiscourseSegment">
    <rdfs:label xml:lang="en">discourse segment</rdfs:label>
  </rdf:Description>
  <rdf:Description rdf:about="http://purl.org/olia/discourse/olia_discourse.owl#DiscourseSegment">
    <rdfs:label>discourse unit</rdfs:label>
  </rdf:Description>
  <rdf:Description rdf:about="http://purl.org/olia/discourse/olia_discourse.owl#DiscourseSegment">
    <rdfs:label>node (PDGB)</rdfs:label>
  </rdf:Description>
  <rdf:Description rdf:about="http://purl.org/olia/discourse/olia_discourse.owl#DiscourseStructuralPattern">
    <rdf:type rdf:resource="http://www.w3.org/2002/07/owl#Class"/>
  </rdf:Description>
  <rdf:Description rdf:about="http://purl.org/olia/discourse/olia_discourse.owl#DiscourseStructuralPattern">
    <rdfs:subClassOf rdf:resource="http://purl.org/olia/olia-top.owl#PragmaticFeature"/>
  </rdf:Description>
  <rdf:Description rdf:about="http://purl.org/olia/discourse/olia_discourse.owl#DiscourseStructuralPattern">
    <rdfs:comment>The feature DiscourseStructuralPattern was introduced to characterize discourse relations according to their "discourse-syntactic" function as opposed to their functional-semantic function (that is formalized in DiscourseRelation). We distinguish paratactic (SDRT: coordinating, RST: multinuclear) and hypotactic (SDRT: subordinating, RST: mononuclear) relations.</rdfs:comment>
  </rdf:Description>
  <rdf:Description rdf:about="http://purl.org/olia/discourse/olia_discourse.owl#DiscourseStructuralPattern">
    <rdfs:label xml:lang="en">discourse structural pattern</rdfs:label>
  </rdf:Description>
  <rdf:Description rdf:about="http://purl.org/olia/discourse/olia_discourse.owl#DisfavouredAlternative">
    <rdf:type rdf:resource="http://www.w3.org/2002/07/owl#Class"/>
  </rdf:Description>
  <rdf:Description rdf:about="http://purl.org/olia/discourse/olia_discourse.owl#DisfavouredAlternative">
    <rdfs:subClassOf rdf:resource="http://purl.org/olia/discourse/olia_discourse.owl#Alternative"/>
  </rdf:Description>
  <rdf:Description rdf:about="http://purl.org/olia/discourse/olia_discourse.owl#DisfavouredAlternative">
    <inverseOf rdf:resource="http://purl.org/olia/discourse/FavouredAlternative"/>
  </rdf:Description>
  <rdf:Description rdf:about="http://purl.org/olia/discourse/olia_discourse.owl#DisfavouredAlternative">
    <rdfs:comment>ISO Substitution with argument disfavoured alternative,</rdfs:comment>
  </rdf:Description>
  <rdf:Description rdf:about="http://purl.org/olia/discourse/olia_discourse.owl#DisfavouredAlternative">
    <rdfs:label>disfavoured alternative</rdfs:label>
  </rdf:Description>
  <rdf:Description rdf:about="http://purl.org/olia/discourse/olia_discourse.owl#DisfavouredAlternative">
    <rdfs:label xml:lang="en">disfavoured alternative</rdfs:label>
  </rdf:Description>
  <rdf:Description rdf:about="http://purl.org/olia/discourse/olia_discourse.owl#Disjunctive">
    <rdf:type rdf:resource="http://www.w3.org/2002/07/owl#Class"/>
  </rdf:Description>
  <rdf:Description rdf:about="http://purl.org/olia/discourse/olia_discourse.owl#Disjunctive">
    <rdfs:subClassOf rdf:resource="http://purl.org/olia/discourse/olia_discourse.owl#Alternative"/>
  </rdf:Description>
  <rdf:Description rdf:about="http://purl.org/olia/discourse/olia_discourse.owl#Disjunctive">
    <rdfs:subClassOf rdf:resource="http://purl.org/olia/discourse/olia_discourse.owl#ParatacticDiscourseRelation"/>
  </rdf:Description>
  <rdf:Description rdf:about="http://purl.org/olia/discourse/olia_discourse.owl#Disjunctive">
    <rdfs:comment>PDTB: Two situations are evoked in the discourse but only one of them holds. (Prasad et al. 2007)
Note that PDTB distinguishes Disjunction and Disjunctive.

RST-DTB: DISJUNCTION is a multinuclear relation whose elements can be listed as alternatives, either positive or negative. (Carlson and Marcu 2001)

RST: An item presents a (not necessarily exclusive) alternative for the other(s). (Mann and Taboada 2010)</rdfs:comment>
  </rdf:Description>
  <rdf:Description rdf:about="http://purl.org/olia/discourse/olia_discourse.owl#Disjunctive">
    <rdfs:label>disjunction</rdfs:label>
  </rdf:Description>
  <rdf:Description rdf:about="http://purl.org/olia/discourse/olia_discourse.owl#Disjunctive">
    <rdfs:label>disjunctive</rdfs:label>
  </rdf:Description>
  <rdf:Description rdf:about="http://purl.org/olia/discourse/olia_discourse.owl#Disjunctive">
    <rdfs:label xml:lang="en">disjunctive</rdfs:label>
  </rdf:Description>
  <rdf:Description rdf:about="http://purl.org/olia/discourse/olia_discourse.owl#Document">
    <rdf:type rdf:resource="http://www.w3.org/2002/07/owl#Class"/>
  </rdf:Description>
  <rdf:Description rdf:about="http://purl.org/olia/discourse/olia_discourse.owl#Document">
    <rdfs:subClassOf rdf:resource="http://purl.org/olia/olia-top.owl#TextStructuralUnit"/>
  </rdf:Description>
  <rdf:Description rdf:about="http://purl.org/olia/discourse/olia_discourse.owl#Document">
    <rdfs:comment>introduced for SemDok CDS-doc</rdfs:comment>
  </rdf:Description>
  <rdf:Description rdf:about="http://purl.org/olia/discourse/olia_discourse.owl#Document">
    <rdfs:label>document</rdfs:label>
  </rdf:Description>
  <rdf:Description rdf:about="http://purl.org/olia/discourse/olia_discourse.owl#Document">
    <rdfs:label xml:lang="en">document</rdfs:label>
  </rdf:Description>
  <rdf:Description rdf:about="http://purl.org/olia/discourse/olia_discourse.owl#Drug">
    <rdf:type rdf:resource="http://www.w3.org/2002/07/owl#Class"/>
  </rdf:Description>
  <rdf:Description rdf:about="http://purl.org/olia/discourse/olia_discourse.owl#Drug">
    <rdfs:subClassOf rdf:resource="http://purl.org/olia/discourse/olia_discourse.owl#ManufacturedObject"/>
  </rdf:Description>
  <rdf:Description rdf:about="http://purl.org/olia/discourse/olia_discourse.owl#Drug">
    <rdfs:comment xml:lang="en">for nerd:Drug</rdfs:comment>
  </rdf:Description>
  <rdf:Description rdf:about="http://purl.org/olia/discourse/olia_discourse.owl#EducationalInstitution">
    <rdf:type rdf:resource="http://www.w3.org/2002/07/owl#Class"/>
  </rdf:Description>
  <rdf:Description rdf:about="http://purl.org/olia/discourse/olia_discourse.owl#EducationalInstitution">
    <rdfs:subClassOf rdf:resource="http://purl.org/olia/discourse/olia_discourse.owl#Organization"/>
  </rdf:Description>
  <rdf:Description rdf:about="http://purl.org/olia/discourse/olia_discourse.owl#EducationalInstitution">
    <rdfs:comment xml:lang="en">for nerd:EducationalInstitution</rdfs:comment>
  </rdf:Description>
  <rdf:Description rdf:about="http://purl.org/olia/discourse/olia_discourse.owl#EducationalInstitution">
    <rdfs:label xml:lang="en">educational ORG</rdfs:label>
  </rdf:Description>
  <rdf:Description rdf:about="http://purl.org/olia/discourse/olia_discourse.owl#EducationalInstitution">
    <rdfs:label xml:lang="en">educational organization</rdfs:label>
  </rdf:Description>
  <rdf:Description rdf:about="http://purl.org/olia/discourse/olia_discourse.owl#EducationalInstitution">
    <skos:prefLabel xml:lang="en">educational institution</skos:prefLabel>
  </rdf:Description>
  <rdf:Description rdf:about="http://purl.org/olia/discourse/olia_discourse.owl#EffectPrecedesCause_PDTB">
    <rdf:type rdf:resource="http://www.w3.org/2002/07/owl#Class"/>
  </rdf:Description>
  <rdf:Description rdf:about="http://purl.org/olia/discourse/olia_discourse.owl#EffectPrecedesCause_PDTB">
    <rdfs:subClassOf rdf:resource="http://purl.org/olia/discourse/olia_discourse.owl#Reason"/>
  </rdf:Description>
  <rdf:Description rdf:about="http://purl.org/olia/discourse/olia_discourse.owl#EffectPrecedesCause_PDTB">
    <rdfs:comment>PDTB "Reason": The situation described in Arg2 is the cause and the situation described in Arg1 is the effect. (Prasad et al. 2007)</rdfs:comment>
  </rdf:Description>
  <rdf:Description rdf:about="http://purl.org/olia/discourse/olia_discourse.owl#EffectPrecedesCause_PDTB">
    <rdfs:label xml:lang="en">effect precedes cause (PDTB)</rdfs:label>
  </rdf:Description>
  <rdf:Description rdf:about="http://purl.org/olia/discourse/olia_discourse.owl#EffectPrecedesCause_PDTB">
    <rdfs:label>reason</rdfs:label>
  </rdf:Description>
  <rdf:Description rdf:about="http://purl.org/olia/discourse/olia_discourse.owl#Elaboration">
    <rdf:type rdf:resource="http://www.w3.org/2002/07/owl#Class"/>
  </rdf:Description>
  <rdf:Description rdf:about="http://purl.org/olia/discourse/olia_discourse.owl#Elaboration">
    <rdfs:subClassOf rdf:resource="http://purl.org/olia/discourse/olia_discourse.owl#EntityBasedRelation"/>
  </rdf:Description>
  <rdf:Description rdf:about="http://purl.org/olia/discourse/olia_discourse.owl#Elaboration">
    <rdfs:subClassOf rdf:resource="http://purl.org/olia/discourse/olia_discourse.owl#HypotacticDiscourseRelation"/>
  </rdf:Description>
  <rdf:Description rdf:about="http://purl.org/olia/discourse/olia_discourse.owl#Elaboration">
    <rdfs:comment>R recognizes S as providing additional detail for N. R identifies the element of subject matter for which detail is provided. (Mann and Taboada 2010)
Infer a set of coherent entities, E(DS0, DS1) from DS0 and DS1. The members of E(DS0, DS1) are centered around a common event or entity, e01. (Wolf et al. 2003)

A classical discourse relation that has been applied to different kinds of dependency relations, e.g., between a set and its member(s), an abstraction and its instance(s), whole and part, process and step, object and attribute, or generalization and specific.
Since Knott et al. (2001), it seems generally accepted that elaboration is to be circumscribed by entity-based coherence, e.g., EntRel relationships as defined by Prasad et al. (2007): "no discourse relation can be inferred and where the second sentence only serves to provide some further description of an entity in the first sentence".

Although Elaboration is thus closely entangled with anaphora and textual inferences, both phenomena are to be modelled separately: Elaboration is a relationship between discourse segments, whereas anaphora and bridging are relationships between discourse referents.

The subclassification of Elaboration follows SemDok. Note that we do not express directionSatellite value "left" as we do not explicitly encode positioning. 

Our modelling follows Webber and Knott (2001) in assuming that elaboration is *always* mediated by an entity relation. However, in some cases relations grouped under elaboration in one framework are grouped with other discourse relations in the PDTB tradition (e.g., ElaborationSpecification is Elaboration in RST and SemDok, but a special case of Specification/Expansion in PDTB). In these cases, we provide double classification.</rdfs:comment>
  </rdf:Description>
  <rdf:Description rdf:about="http://purl.org/olia/discourse/olia_discourse.owl#Elaboration">
    <rdfs:label xml:lang="en">elaboration</rdfs:label>
  </rdf:Description>
  <rdf:Description rdf:about="http://purl.org/olia/discourse/olia_discourse.owl#ElaborationAdditional_RST">
    <rdf:type rdf:resource="http://www.w3.org/2002/07/owl#Class"/>
  </rdf:Description>
  <rdf:Description rdf:about="http://purl.org/olia/discourse/olia_discourse.owl#ElaborationAdditional_RST">
    <rdfs:subClassOf rdf:resource="http://purl.org/olia/discourse/olia_discourse.owl#ElaborationSpecification"/>
  </rdf:Description>
  <rdf:Description rdf:about="http://purl.org/olia/discourse/olia_discourse.owl#ElaborationAdditional_RST">
    <rdfs:comment>In an ELABORATION-ADDITIONAL relation, the satellite gives additional infor-
mation or detail about the situation presented in the nucleus. This relation is extremely common at
all levels of the discourse structure, and is especially popular to show relations across large spans of information. It is the default for the family of elaboration relations, and should be used when
none of the other, more specific, elaboration relations apply.

When an elaborating satellite is an embedded unit, the relation ELABORATION-ADDI-
TIONAL-E is used. Generally, the embedded satellite of this relation is separated from the nucleus
by a comma and represents a nonrestrictive relative clause, whereas an ELABORATION-OBJECT-
ATTRIBUTE-E represents a restrictive relative clause
(Carlson and Marcu 2001)</rdfs:comment>
  </rdf:Description>
  <rdf:Description rdf:about="http://purl.org/olia/discourse/olia_discourse.owl#ElaborationAdditional_RST">
    <rdfs:label xml:lang="en">elaboration additional (RST)</rdfs:label>
  </rdf:Description>
  <rdf:Description rdf:about="http://purl.org/olia/discourse/olia_discourse.owl#ElaborationAssign">
    <rdf:type rdf:resource="http://www.w3.org/2002/07/owl#Class"/>
  </rdf:Description>
  <rdf:Description rdf:about="http://purl.org/olia/discourse/olia_discourse.owl#ElaborationAssign">
    <rdfs:subClassOf rdf:resource="http://purl.org/olia/discourse/olia_discourse.owl#ElaborationSpecification"/>
  </rdf:Description>
  <rdf:Description rdf:about="http://purl.org/olia/discourse/olia_discourse.owl#ElaborationAssign">
    <rdfs:comment>SemDok Elaboration-assign.
Note that we skipped the subclass Elaboration-assign-other, as its definition is unclear.</rdfs:comment>
  </rdf:Description>
  <rdf:Description rdf:about="http://purl.org/olia/discourse/olia_discourse.owl#ElaborationAssign">
    <rdfs:label xml:lang="en">elaboration assign</rdfs:label>
  </rdf:Description>
  <rdf:Description rdf:about="http://purl.org/olia/discourse/olia_discourse.owl#ElaborationAssignAbbreviation">
    <rdf:type rdf:resource="http://www.w3.org/2002/07/owl#Class"/>
  </rdf:Description>
  <rdf:Description rdf:about="http://purl.org/olia/discourse/olia_discourse.owl#ElaborationAssignAbbreviation">
    <rdfs:subClassOf rdf:resource="http://purl.org/olia/discourse/olia_discourse.owl#ElaborationAssign"/>
  </rdf:Description>
  <rdf:Description rdf:about="http://purl.org/olia/discourse/olia_discourse.owl#ElaborationAssignAbbreviation">
    <rdfs:comment>SemDok ElaborationAssignAbbreviation</rdfs:comment>
  </rdf:Description>
  <rdf:Description rdf:about="http://purl.org/olia/discourse/olia_discourse.owl#ElaborationAssignAbbreviation">
    <rdfs:label xml:lang="en">elaboration assign abbreviation</rdfs:label>
  </rdf:Description>
  <rdf:Description rdf:about="http://purl.org/olia/discourse/olia_discourse.owl#ElaborationClassInstance">
    <rdf:type rdf:resource="http://www.w3.org/2002/07/owl#Class"/>
  </rdf:Description>
  <rdf:Description rdf:about="http://purl.org/olia/discourse/olia_discourse.owl#ElaborationClassInstance">
    <rdfs:subClassOf rdf:resource="http://purl.org/olia/discourse/olia_discourse.owl#ElaborationDerivation"/>
  </rdf:Description>
  <rdf:Description rdf:about="http://purl.org/olia/discourse/olia_discourse.owl#ElaborationClassInstance">
    <rdfs:comment>Elaboration-class-instance</rdfs:comment>
  </rdf:Description>
  <rdf:Description rdf:about="http://purl.org/olia/discourse/olia_discourse.owl#ElaborationClassInstance">
    <rdfs:label xml:lang="en">elaboration class instance</rdfs:label>
  </rdf:Description>
  <rdf:Description rdf:about="http://purl.org/olia/discourse/olia_discourse.owl#ElaborationClassSubclass">
    <rdf:type rdf:resource="http://www.w3.org/2002/07/owl#Class"/>
  </rdf:Description>
  <rdf:Description rdf:about="http://purl.org/olia/discourse/olia_discourse.owl#ElaborationClassSubclass">
    <rdfs:subClassOf rdf:resource="http://purl.org/olia/discourse/olia_discourse.owl#ElaborationDerivation"/>
  </rdf:Description>
  <rdf:Description rdf:about="http://purl.org/olia/discourse/olia_discourse.owl#ElaborationClassSubclass">
    <rdfs:comment>SemDok Elaboration-class-subclass</rdfs:comment>
  </rdf:Description>
  <rdf:Description rdf:about="http://purl.org/olia/discourse/olia_discourse.owl#ElaborationClassSubclass">
    <rdfs:label xml:lang="en">elaboration class subclass</rdfs:label>
  </rdf:Description>
  <rdf:Description rdf:about="http://purl.org/olia/discourse/olia_discourse.owl#ElaborationContinuation">
    <rdf:type rdf:resource="http://www.w3.org/2002/07/owl#Class"/>
  </rdf:Description>
  <rdf:Description rdf:about="http://purl.org/olia/discourse/olia_discourse.owl#ElaborationContinuation">
    <rdfs:subClassOf rdf:resource="http://purl.org/olia/discourse/olia_discourse.owl#ElaborationIdentity"/>
  </rdf:Description>
  <rdf:Description rdf:about="http://purl.org/olia/discourse/olia_discourse.owl#ElaborationContinuation">
    <rdfs:subClassOf rdf:resource="http://purl.org/olia/discourse/olia_discourse.owl#TopicContinuityRelation"/>
  </rdf:Description>
  <rdf:Description rdf:about="http://purl.org/olia/discourse/olia_discourse.owl#ElaborationContinuation">
    <rdfs:comment>SemDok Elaboration-continuation. We omitted the subclass Elaboration-continuation-other because it is unclear how this is defined. Its subclasses are, however, preserved.

SemDok treats all topic continuity relations as subclasses of elaboration, but this comes with the assumption of hypotactic relation, whereas other topic continuity relations in RST are paratactic or underdefined (see TopicContinuityRelation). We thus add these SemDok elaborations as subclasses of TopicContinuityRelation rather than merging them into a single concept.</rdfs:comment>
  </rdf:Description>
  <rdf:Description rdf:about="http://purl.org/olia/discourse/olia_discourse.owl#ElaborationContinuation">
    <rdfs:label xml:lang="en">elaboration continuation</rdfs:label>
  </rdf:Description>
  <rdf:Description rdf:about="http://purl.org/olia/discourse/olia_discourse.owl#ElaborationDefinition">
    <rdf:type rdf:resource="http://www.w3.org/2002/07/owl#Class"/>
  </rdf:Description>
  <rdf:Description rdf:about="http://purl.org/olia/discourse/olia_discourse.owl#ElaborationDefinition">
    <rdfs:subClassOf rdf:resource="http://purl.org/olia/discourse/olia_discourse.owl#Definition"/>
  </rdf:Description>
  <rdf:Description rdf:about="http://purl.org/olia/discourse/olia_discourse.owl#ElaborationDefinition">
    <rdfs:subClassOf rdf:resource="http://purl.org/olia/discourse/olia_discourse.owl#Elaboration"/>
  </rdf:Description>
  <rdf:Description rdf:about="http://purl.org/olia/discourse/olia_discourse.owl#ElaborationDefinition">
    <rdfs:comment>from SemDok Elaboration-definition, no definition given

We assume that this is (near-) identical to RST Definition.</rdfs:comment>
  </rdf:Description>
  <rdf:Description rdf:about="http://purl.org/olia/discourse/olia_discourse.owl#ElaborationDefinition">
    <rdfs:label xml:lang="en">elaboration definition</rdfs:label>
  </rdf:Description>
  <rdf:Description rdf:about="http://purl.org/olia/discourse/olia_discourse.owl#ElaborationDerivation">
    <rdf:type rdf:resource="http://www.w3.org/2002/07/owl#Class"/>
  </rdf:Description>
  <rdf:Description rdf:about="http://purl.org/olia/discourse/olia_discourse.owl#ElaborationDerivation">
    <rdfs:subClassOf rdf:resource="http://purl.org/olia/discourse/olia_discourse.owl#Elaboration"/>
  </rdf:Description>
  <rdf:Description rdf:about="http://purl.org/olia/discourse/olia_discourse.owl#ElaborationDerivation">
    <rdfs:comment>for SemDok Elaboration-derivation</rdfs:comment>
  </rdf:Description>
  <rdf:Description rdf:about="http://purl.org/olia/discourse/olia_discourse.owl#ElaborationDerivation">
    <rdfs:label xml:lang="en">elaboration derivation</rdfs:label>
  </rdf:Description>
  <rdf:Description rdf:about="http://purl.org/olia/discourse/olia_discourse.owl#ElaborationDrift">
    <rdf:type rdf:resource="http://www.w3.org/2002/07/owl#Class"/>
  </rdf:Description>
  <rdf:Description rdf:about="http://purl.org/olia/discourse/olia_discourse.owl#ElaborationDrift">
    <rdfs:subClassOf rdf:resource="http://purl.org/olia/discourse/olia_discourse.owl#ElaborationContinuation"/>
  </rdf:Description>
  <rdf:Description rdf:about="http://purl.org/olia/discourse/olia_discourse.owl#ElaborationDrift">
    <rdfs:subClassOf rdf:resource="http://purl.org/olia/discourse/olia_discourse.owl#TopicDrift"/>
  </rdf:Description>
  <rdf:Description rdf:about="http://purl.org/olia/discourse/olia_discourse.owl#ElaborationDrift">
    <rdfs:comment>SemDok Elaboration-drift</rdfs:comment>
  </rdf:Description>
  <rdf:Description rdf:about="http://purl.org/olia/discourse/olia_discourse.owl#ElaborationDrift">
    <rdfs:label xml:lang="en">elaboration drift</rdfs:label>
  </rdf:Description>
  <rdf:Description rdf:about="http://purl.org/olia/discourse/olia_discourse.owl#ElaborationExample">
    <rdf:type rdf:resource="http://www.w3.org/2002/07/owl#Class"/>
  </rdf:Description>
  <rdf:Description rdf:about="http://purl.org/olia/discourse/olia_discourse.owl#ElaborationExample">
    <rdfs:subClassOf rdf:resource="http://purl.org/olia/discourse/olia_discourse.owl#Elaboration"/>
  </rdf:Description>
  <rdf:Description rdf:about="http://purl.org/olia/discourse/olia_discourse.owl#ElaborationExample">
    <rdfs:subClassOf rdf:resource="http://purl.org/olia/discourse/olia_discourse.owl#Example"/>
  </rdf:Description>
  <rdf:Description rdf:about="http://purl.org/olia/discourse/olia_discourse.owl#ElaborationExample">
    <rdfs:comment>SemDok Elaboration-example

We assume that this is a mononuclear subclass of Example.</rdfs:comment>
  </rdf:Description>
  <rdf:Description rdf:about="http://purl.org/olia/discourse/olia_discourse.owl#ElaborationExample">
    <rdfs:label xml:lang="en">elaboration example</rdfs:label>
  </rdf:Description>
  <rdf:Description rdf:about="http://purl.org/olia/discourse/olia_discourse.owl#ElaborationGenericSpecific_RST">
    <rdf:type rdf:resource="http://www.w3.org/2002/07/owl#Class"/>
  </rdf:Description>
  <rdf:Description rdf:about="http://purl.org/olia/discourse/olia_discourse.owl#ElaborationGenericSpecific_RST">
    <rdfs:subClassOf rdf:resource="http://purl.org/olia/discourse/olia_discourse.owl#ElaborationSpecification"/>
  </rdf:Description>
  <rdf:Description rdf:about="http://purl.org/olia/discourse/olia_discourse.owl#ElaborationGenericSpecific_RST">
    <rdfs:comment>ELABORATION-GENERAL-SPECIFIC: The satellite provides specific information to help define a very general con-
cept introduced in the nucleus.
(Carlson et al. 2001)</rdfs:comment>
  </rdf:Description>
  <rdf:Description rdf:about="http://purl.org/olia/discourse/olia_discourse.owl#ElaborationGenericSpecific_RST">
    <rdfs:label xml:lang="en">elaboration generic specific (RST)</rdfs:label>
  </rdf:Description>
  <rdf:Description rdf:about="http://purl.org/olia/discourse/olia_discourse.owl#ElaborationIdentity">
    <rdf:type rdf:resource="http://www.w3.org/2002/07/owl#Class"/>
  </rdf:Description>
  <rdf:Description rdf:about="http://purl.org/olia/discourse/olia_discourse.owl#ElaborationIdentity">
    <rdfs:subClassOf rdf:resource="http://purl.org/olia/discourse/olia_discourse.owl#Elaboration"/>
  </rdf:Description>
  <rdf:Description rdf:about="http://purl.org/olia/discourse/olia_discourse.owl#ElaborationIdentity">
    <rdfs:comment>SemDok Elaboration-identity</rdfs:comment>
  </rdf:Description>
  <rdf:Description rdf:about="http://purl.org/olia/discourse/olia_discourse.owl#ElaborationIdentity">
    <rdfs:label xml:lang="en">elaboration identity</rdfs:label>
  </rdf:Description>
  <rdf:Description rdf:about="http://purl.org/olia/discourse/olia_discourse.owl#ElaborationIntegration">
    <rdf:type rdf:resource="http://www.w3.org/2002/07/owl#Class"/>
  </rdf:Description>
  <rdf:Description rdf:about="http://purl.org/olia/discourse/olia_discourse.owl#ElaborationIntegration">
    <rdfs:subClassOf rdf:resource="http://purl.org/olia/discourse/olia_discourse.owl#Elaboration"/>
  </rdf:Description>
  <rdf:Description rdf:about="http://purl.org/olia/discourse/olia_discourse.owl#ElaborationIntegration">
    <rdfs:subClassOf rdf:resource="http://purl.org/olia/discourse/olia_discourse.owl#Generalization"/>
  </rdf:Description>
  <rdf:Description rdf:about="http://purl.org/olia/discourse/olia_discourse.owl#ElaborationIntegration">
    <rdfs:comment>SemDok Elaboration-integration

No definition is given. By analogy with ElaborationWholePart, we assume that this may stand for ElaborationPartWhole, but this is unconfirmed. Based on this interpretation, however, we define it as subclass of Generalization.

As a SemDok Elaboration, this is a subject-matter relation. This seems to be the main difference to SemDok Summary, which is interpersonal.</rdfs:comment>
  </rdf:Description>
  <rdf:Description rdf:about="http://purl.org/olia/discourse/olia_discourse.owl#ElaborationIntegration">
    <rdfs:label xml:lang="en">elaboration integration</rdfs:label>
  </rdf:Description>
  <rdf:Description rdf:about="http://purl.org/olia/discourse/olia_discourse.owl#ElaborationObjectAttribute_RST">
    <rdf:type rdf:resource="http://www.w3.org/2002/07/owl#Class"/>
  </rdf:Description>
  <rdf:Description rdf:about="http://purl.org/olia/discourse/olia_discourse.owl#ElaborationObjectAttribute_RST">
    <rdfs:subClassOf rdf:resource="http://purl.org/olia/discourse/olia_discourse.owl#ElaborationSpecification"/>
  </rdf:Description>
  <rdf:Description rdf:about="http://purl.org/olia/discourse/olia_discourse.owl#ElaborationObjectAttribute_RST">
    <rdfs:comment>ELABORATION-OBJECT-ATTRIBUTE is a relation involving a clause, usually a
postmodifier of a noun phrase, that is required to give meaning to an animate or inanimate object.
The modifying clause is the satellite, and the object it modifies is the nucleus. The satellite is
intrinsic to the meaning of the nucleus, and/or essential to understanding the context, and is
almost always an embedded unit. This relation is almost always embedded

In embedded units, ELABORATION-OBJECT-ATTRIBUTE-E is much more common than
ELABORATION-ADDITIONAL-E. The way to distinguish between ELABORATION-OBJECT-
ATTRIBUTE-E and ELABORATION-ADDITIONAL-E is that the former is intrinsic to the object it is
modifying in the nucleus, while the latter is extrinsic, i.e. it contains information that is incidental
and which could be omitted without loss of understanding. Usually, an ELABORATION-ADDI-
TIONAL-E is separated from the nucleus by a comma and represents a nonrestrictive relative
clause, whereas an ELABORATION-OBJECT-ATTRIBUTE-E represents a restrictive relative clause.
(Carlson and Marcu 2001)</rdfs:comment>
  </rdf:Description>
  <rdf:Description rdf:about="http://purl.org/olia/discourse/olia_discourse.owl#ElaborationObjectAttribute_RST">
    <rdfs:label xml:lang="en">elaboration object attribute (RST)</rdfs:label>
  </rdf:Description>
  <rdf:Description rdf:about="http://purl.org/olia/discourse/olia_discourse.owl#ElaborationOfDetail_PDGB">
    <rdf:type rdf:resource="http://www.w3.org/2002/07/owl#Class"/>
  </rdf:Description>
  <rdf:Description rdf:about="http://purl.org/olia/discourse/olia_discourse.owl#ElaborationOfDetail_PDGB">
    <rdfs:subClassOf rdf:resource="http://purl.org/olia/discourse/olia_discourse.owl#ElaborationSpecification"/>
  </rdf:Description>
  <rdf:Description rdf:about="http://purl.org/olia/discourse/olia_discourse.owl#ElaborationOfDetail_PDGB">
    <rdfs:subClassOf rdf:resource="http://purl.org/olia/discourse/olia_discourse.owl#TemporalRelation"/>
  </rdf:Description>
  <rdf:Description rdf:about="http://purl.org/olia/discourse/olia_discourse.owl#ElaborationOfDetail_PDGB">
    <rdfs:comment>The Satellite gives details about an entity involved in the event described by the
Nucleus. The details cannot be captured by any of the relations above.
(Wolf et al. 2003)</rdfs:comment>
  </rdf:Description>
  <rdf:Description rdf:about="http://purl.org/olia/discourse/olia_discourse.owl#ElaborationOfDetail_PDGB">
    <rdfs:label xml:lang="en">elaboration of detail (PDGB)</rdfs:label>
  </rdf:Description>
  <rdf:Description rdf:about="http://purl.org/olia/discourse/olia_discourse.owl#ElaborationOfLocation_PDGB">
    <rdf:type rdf:resource="http://www.w3.org/2002/07/owl#Class"/>
  </rdf:Description>
  <rdf:Description rdf:about="http://purl.org/olia/discourse/olia_discourse.owl#ElaborationOfLocation_PDGB">
    <rdfs:subClassOf rdf:resource="http://purl.org/olia/discourse/olia_discourse.owl#ElaborationSpecification"/>
  </rdf:Description>
  <rdf:Description rdf:about="http://purl.org/olia/discourse/olia_discourse.owl#ElaborationOfLocation_PDGB">
    <rdfs:comment>The Satellite gives information about the location where the Nucleus took place
(Wolf et al. 2003)</rdfs:comment>
  </rdf:Description>
  <rdf:Description rdf:about="http://purl.org/olia/discourse/olia_discourse.owl#ElaborationOfLocation_PDGB">
    <rdfs:label xml:lang="en">elaboration of location (PDGB)</rdfs:label>
  </rdf:Description>
  <rdf:Description rdf:about="http://purl.org/olia/discourse/olia_discourse.owl#ElaborationOfNumber_PDGB">
    <rdf:type rdf:resource="http://www.w3.org/2002/07/owl#Class"/>
  </rdf:Description>
  <rdf:Description rdf:about="http://purl.org/olia/discourse/olia_discourse.owl#ElaborationOfNumber_PDGB">
    <rdfs:subClassOf rdf:resource="http://purl.org/olia/discourse/olia_discourse.owl#ElaborationSpecification"/>
  </rdf:Description>
  <rdf:Description rdf:about="http://purl.org/olia/discourse/olia_discourse.owl#ElaborationOfNumber_PDGB">
    <rdfs:subClassOf rdf:resource="http://purl.org/olia/discourse/olia_discourse.owl#TemporalRelation"/>
  </rdf:Description>
  <rdf:Description rdf:about="http://purl.org/olia/discourse/olia_discourse.owl#ElaborationOfNumber_PDGB">
    <rdfs:comment>The Satellite gives information about the time at which the Nucleus took place (???)
(Wolf et al. 2003)</rdfs:comment>
  </rdf:Description>
  <rdf:Description rdf:about="http://purl.org/olia/discourse/olia_discourse.owl#ElaborationOfNumber_PDGB">
    <rdfs:label xml:lang="en">elaboration of number (PDGB)</rdfs:label>
  </rdf:Description>
  <rdf:Description rdf:about="http://purl.org/olia/discourse/olia_discourse.owl#ElaborationOfOrganization_PDGB">
    <rdf:type rdf:resource="http://www.w3.org/2002/07/owl#Class"/>
  </rdf:Description>
  <rdf:Description rdf:about="http://purl.org/olia/discourse/olia_discourse.owl#ElaborationOfOrganization_PDGB">
    <rdfs:subClassOf rdf:resource="http://purl.org/olia/discourse/olia_discourse.owl#ElaborationSpecification"/>
  </rdf:Description>
  <rdf:Description rdf:about="http://purl.org/olia/discourse/olia_discourse.owl#ElaborationOfOrganization_PDGB">
    <rdfs:comment>The Satellite gives information about an organization involved in the event
described by the Nucleus
(Wolf et al. 2003)</rdfs:comment>
  </rdf:Description>
  <rdf:Description rdf:about="http://purl.org/olia/discourse/olia_discourse.owl#ElaborationOfOrganization_PDGB">
    <rdfs:label xml:lang="en">elaboration of organization (PDGB)</rdfs:label>
  </rdf:Description>
  <rdf:Description rdf:about="http://purl.org/olia/discourse/olia_discourse.owl#ElaborationOfPerson_PDGB">
    <rdf:type rdf:resource="http://www.w3.org/2002/07/owl#Class"/>
  </rdf:Description>
  <rdf:Description rdf:about="http://purl.org/olia/discourse/olia_discourse.owl#ElaborationOfPerson_PDGB">
    <rdfs:subClassOf rdf:resource="http://purl.org/olia/discourse/olia_discourse.owl#ElaborationSpecification"/>
  </rdf:Description>
  <rdf:Description rdf:about="http://purl.org/olia/discourse/olia_discourse.owl#ElaborationOfPerson_PDGB">
    <rdfs:comment>The Satellite gives information about a person involved in the event described by the
Nucleus
(Wolf et al. 2003)</rdfs:comment>
  </rdf:Description>
  <rdf:Description rdf:about="http://purl.org/olia/discourse/olia_discourse.owl#ElaborationOfPerson_PDGB">
    <rdfs:label xml:lang="en">elaboration of person (PDGB)</rdfs:label>
  </rdf:Description>
  <rdf:Description rdf:about="http://purl.org/olia/discourse/olia_discourse.owl#ElaborationOfTime_PDGB">
    <rdf:type rdf:resource="http://www.w3.org/2002/07/owl#Class"/>
  </rdf:Description>
  <rdf:Description rdf:about="http://purl.org/olia/discourse/olia_discourse.owl#ElaborationOfTime_PDGB">
    <rdfs:subClassOf rdf:resource="http://purl.org/olia/discourse/olia_discourse.owl#ElaborationSpecification"/>
  </rdf:Description>
  <rdf:Description rdf:about="http://purl.org/olia/discourse/olia_discourse.owl#ElaborationOfTime_PDGB">
    <rdfs:subClassOf rdf:resource="http://purl.org/olia/discourse/olia_discourse.owl#TemporalRelation"/>
  </rdf:Description>
  <rdf:Description rdf:about="http://purl.org/olia/discourse/olia_discourse.owl#ElaborationOfTime_PDGB">
    <rdfs:comment>The Satellite gives information about the time at which the Nucleus took place
(Wolf et al. 2003)</rdfs:comment>
  </rdf:Description>
  <rdf:Description rdf:about="http://purl.org/olia/discourse/olia_discourse.owl#ElaborationOfTime_PDGB">
    <rdfs:label xml:lang="en">elaboration of time (PDGB)</rdfs:label>
  </rdf:Description>
  <rdf:Description rdf:about="http://purl.org/olia/discourse/olia_discourse.owl#ElaborationPartWhole_RST">
    <rdf:type rdf:resource="http://www.w3.org/2002/07/owl#Class"/>
  </rdf:Description>
  <rdf:Description rdf:about="http://purl.org/olia/discourse/olia_discourse.owl#ElaborationPartWhole_RST">
    <rdfs:subClassOf rdf:resource="http://purl.org/olia/discourse/olia_discourse.owl#ElaborationIntegration"/>
  </rdf:Description>
  <rdf:Description rdf:about="http://purl.org/olia/discourse/olia_discourse.owl#ElaborationPartWhole_RST">
    <rdfs:comment>In an ELABORATION-PART-WHOLE relation, the satellite specifies or elaborates
on a portion or part of the nucleus. Since this relation is most often appropriate for representing
parts of objects, it is only occasionally found to hold between EDUs. Most typically, this would be
in a parenthetical modifier. It is distinguished from ELABORATION-SET-MEMBER, in which each
member is representative of the entire set in a similar way.
(Carlson and Marcu 2001)</rdfs:comment>
  </rdf:Description>
  <rdf:Description rdf:about="http://purl.org/olia/discourse/olia_discourse.owl#ElaborationPartWhole_RST">
    <rdfs:label xml:lang="en">elaboration part whole (RST)</rdfs:label>
  </rdf:Description>
  <rdf:Description rdf:about="http://purl.org/olia/discourse/olia_discourse.owl#ElaborationProcessStep">
    <rdf:type rdf:resource="http://www.w3.org/2002/07/owl#Class"/>
  </rdf:Description>
  <rdf:Description rdf:about="http://purl.org/olia/discourse/olia_discourse.owl#ElaborationProcessStep">
    <rdfs:subClassOf rdf:resource="http://purl.org/olia/discourse/olia_discourse.owl#ElaborationDerivation"/>
  </rdf:Description>
  <rdf:Description rdf:about="http://purl.org/olia/discourse/olia_discourse.owl#ElaborationProcessStep">
    <rdfs:comment>ELABORATION-PROCESS-STEP: In this elaboration relation, the nucleus introduces an activity or event (a pro-
cess). The satellite then enumerates the steps involved in carrying out the process, usually in chro-
nological order. Thus, the steps are most often represented in a multinuclear SEQUENCE
relationship.
(Carlson and Marcu 2001)

SemDok Elaboration-process-step</rdfs:comment>
  </rdf:Description>
  <rdf:Description rdf:about="http://purl.org/olia/discourse/olia_discourse.owl#ElaborationProcessStep">
    <rdfs:label xml:lang="en">elaboration process step</rdfs:label>
  </rdf:Description>
  <rdf:Description rdf:about="http://purl.org/olia/discourse/olia_discourse.owl#ElaborationProcessStep_RST">
    <rdf:type rdf:resource="http://www.w3.org/2002/07/owl#Class"/>
  </rdf:Description>
  <rdf:Description rdf:about="http://purl.org/olia/discourse/olia_discourse.owl#ElaborationProcessStep_RST">
    <rdfs:subClassOf rdf:resource="http://purl.org/olia/discourse/olia_discourse.owl#ElaborationProcessStep"/>
  </rdf:Description>
  <rdf:Description rdf:about="http://purl.org/olia/discourse/olia_discourse.owl#ElaborationProcessStep_RST">
    <rdfs:label xml:lang="en">elaboration process step (RST)</rdfs:label>
  </rdf:Description>
  <rdf:Description rdf:about="http://purl.org/olia/discourse/olia_discourse.owl#ElaborationProcessStep_RST">
    <owl:deprecated rdf:datatype="http://www.w3.org/2001/XMLSchema#boolean">true</owl:deprecated>
  </rdf:Description>
  <rdf:Description rdf:about="http://purl.org/olia/discourse/olia_discourse.owl#ElaborationRestatement">
    <rdf:type rdf:resource="http://www.w3.org/2002/07/owl#Class"/>
  </rdf:Description>
  <rdf:Description rdf:about="http://purl.org/olia/discourse/olia_discourse.owl#ElaborationRestatement">
    <rdfs:subClassOf rdf:resource="http://purl.org/olia/discourse/olia_discourse.owl#Elaboration"/>
  </rdf:Description>
  <rdf:Description rdf:about="http://purl.org/olia/discourse/olia_discourse.owl#ElaborationRestatement">
    <rdfs:subClassOf rdf:resource="http://purl.org/olia/discourse/olia_discourse.owl#EquivalentRestatement"/>
  </rdf:Description>
  <rdf:Description rdf:about="http://purl.org/olia/discourse/olia_discourse.owl#ElaborationRestatement">
    <rdfs:comment>SemDok Elaboration-Restatement

Apparently, this is a mononuclear version of Restatement as found in other frameworks.</rdfs:comment>
  </rdf:Description>
  <rdf:Description rdf:about="http://purl.org/olia/discourse/olia_discourse.owl#ElaborationRestatement">
    <rdfs:label xml:lang="en">elaboration restatement</rdfs:label>
  </rdf:Description>
  <rdf:Description rdf:about="http://purl.org/olia/discourse/olia_discourse.owl#ElaborationSetMember">
    <rdf:type rdf:resource="http://www.w3.org/2002/07/owl#Class"/>
  </rdf:Description>
  <rdf:Description rdf:about="http://purl.org/olia/discourse/olia_discourse.owl#ElaborationSetMember">
    <rdfs:subClassOf rdf:resource="http://purl.org/olia/discourse/olia_discourse.owl#ElaborationDerivation"/>
  </rdf:Description>
  <rdf:Description rdf:about="http://purl.org/olia/discourse/olia_discourse.owl#ElaborationSetMember">
    <rdfs:comment>ELABORATION-SET-MEMBER: In this elaboration relation, the nucleus introduces a finite set (which may be
generic or a named entity) or a list of information. The satellite then specifically elaborates on at
least one member of the set. Typically, the members themselves are represented in a multinuclear
LIST relationship.
(Carlson and Marcu 2001)

SemDok Elaboration-set-member</rdfs:comment>
  </rdf:Description>
  <rdf:Description rdf:about="http://purl.org/olia/discourse/olia_discourse.owl#ElaborationSetMember">
    <rdfs:label xml:lang="en">elaboration set member</rdfs:label>
  </rdf:Description>
  <rdf:Description rdf:about="http://purl.org/olia/discourse/olia_discourse.owl#ElaborationSetMember_RST">
    <rdf:type rdf:resource="http://www.w3.org/2002/07/owl#Class"/>
  </rdf:Description>
  <rdf:Description rdf:about="http://purl.org/olia/discourse/olia_discourse.owl#ElaborationSetMember_RST">
    <rdfs:subClassOf rdf:resource="http://purl.org/olia/discourse/olia_discourse.owl#ElaborationSetMember"/>
  </rdf:Description>
  <rdf:Description rdf:about="http://purl.org/olia/discourse/olia_discourse.owl#ElaborationSetMember_RST">
    <rdfs:label xml:lang="en">elaboration set member (RST)</rdfs:label>
  </rdf:Description>
  <rdf:Description rdf:about="http://purl.org/olia/discourse/olia_discourse.owl#ElaborationSetMember_RST">
    <owl:deprecated rdf:datatype="http://www.w3.org/2001/XMLSchema#boolean">true</owl:deprecated>
  </rdf:Description>
  <rdf:Description rdf:about="http://purl.org/olia/discourse/olia_discourse.owl#ElaborationSpecification">
    <rdf:type rdf:resource="http://www.w3.org/2002/07/owl#Class"/>
  </rdf:Description>
  <rdf:Description rdf:about="http://purl.org/olia/discourse/olia_discourse.owl#ElaborationSpecification">
    <rdfs:subClassOf rdf:resource="http://purl.org/olia/discourse/olia_discourse.owl#ElaborationIdentity"/>
  </rdf:Description>
  <rdf:Description rdf:about="http://purl.org/olia/discourse/olia_discourse.owl#ElaborationSpecification">
    <rdfs:subClassOf rdf:resource="http://purl.org/olia/discourse/olia_discourse.owl#Specification"/>
  </rdf:Description>
  <rdf:Description rdf:about="http://purl.org/olia/discourse/olia_discourse.owl#ElaborationSpecification">
    <rdfs:comment>SemDok Elaboration-specification

Apparently, this is a mononuclear version of Specification.</rdfs:comment>
  </rdf:Description>
  <rdf:Description rdf:about="http://purl.org/olia/discourse/olia_discourse.owl#ElaborationSpecification">
    <rdfs:label xml:lang="en">elaboration specification</rdfs:label>
  </rdf:Description>
  <rdf:Description rdf:about="http://purl.org/olia/discourse/olia_discourse.owl#ElaborationThemeRheme">
    <rdf:type rdf:resource="http://www.w3.org/2002/07/owl#Class"/>
  </rdf:Description>
  <rdf:Description rdf:about="http://purl.org/olia/discourse/olia_discourse.owl#ElaborationThemeRheme">
    <rdfs:subClassOf rdf:resource="http://purl.org/olia/discourse/olia_discourse.owl#ElaborationContinuation"/>
  </rdf:Description>
  <rdf:Description rdf:about="http://purl.org/olia/discourse/olia_discourse.owl#ElaborationThemeRheme">
    <rdfs:subClassOf rdf:resource="http://purl.org/olia/discourse/olia_discourse.owl#TopicComment"/>
  </rdf:Description>
  <rdf:Description rdf:about="http://purl.org/olia/discourse/olia_discourse.owl#ElaborationThemeRheme">
    <rdfs:comment>SemDok Elaboration-theme-rheme</rdfs:comment>
  </rdf:Description>
  <rdf:Description rdf:about="http://purl.org/olia/discourse/olia_discourse.owl#ElaborationThemeRheme">
    <rdfs:label xml:lang="en">elaboration theme rheme</rdfs:label>
  </rdf:Description>
  <rdf:Description rdf:about="http://purl.org/olia/discourse/olia_discourse.owl#ElaborationThemeTheme">
    <rdf:type rdf:resource="http://www.w3.org/2002/07/owl#Class"/>
  </rdf:Description>
  <rdf:Description rdf:about="http://purl.org/olia/discourse/olia_discourse.owl#ElaborationThemeTheme">
    <rdfs:subClassOf rdf:resource="http://purl.org/olia/discourse/olia_discourse.owl#ElaborationContinuation"/>
  </rdf:Description>
  <rdf:Description rdf:about="http://purl.org/olia/discourse/olia_discourse.owl#ElaborationThemeTheme">
    <rdfs:comment>SemDok Elaboration-theme-theme

Unfortunately, SemDok doesn't provide definitions, so it is unclear whether this is meant to be comparable to TopicShift. At least, it would be surprising to see that modelled as an Elaboration.</rdfs:comment>
  </rdf:Description>
  <rdf:Description rdf:about="http://purl.org/olia/discourse/olia_discourse.owl#ElaborationThemeTheme">
    <rdfs:label xml:lang="en">elaboration theme theme</rdfs:label>
  </rdf:Description>
  <rdf:Description rdf:about="http://purl.org/olia/discourse/olia_discourse.owl#ElaborationWholePart">
    <rdf:type rdf:resource="http://www.w3.org/2002/07/owl#Class"/>
  </rdf:Description>
  <rdf:Description rdf:about="http://purl.org/olia/discourse/olia_discourse.owl#ElaborationWholePart">
    <rdfs:subClassOf rdf:resource="http://purl.org/olia/discourse/olia_discourse.owl#ElaborationDerivation"/>
  </rdf:Description>
  <rdf:Description rdf:about="http://purl.org/olia/discourse/olia_discourse.owl#ElaborationWholePart">
    <rdfs:comment>SemDok Elaboration-whole-part</rdfs:comment>
  </rdf:Description>
  <rdf:Description rdf:about="http://purl.org/olia/discourse/olia_discourse.owl#ElaborationWholePart">
    <rdfs:label xml:lang="en">elaboration whole part</rdfs:label>
  </rdf:Description>
  <rdf:Description rdf:about="http://purl.org/olia/discourse/olia_discourse.owl#ElementOf">
    <rdf:type rdf:resource="http://www.w3.org/2002/07/owl#Class"/>
  </rdf:Description>
  <rdf:Description rdf:about="http://purl.org/olia/discourse/olia_discourse.owl#ElementOf">
    <rdfs:subClassOf rdf:resource="http://purl.org/olia/discourse/olia_discourse.owl#Set"/>
  </rdf:Description>
  <rdf:Description rdf:about="http://purl.org/olia/discourse/olia_discourse.owl#ElementOf">
    <rdfs:label xml:lang="en">element of</rdfs:label>
  </rdf:Description>
  <rdf:Description rdf:about="http://purl.org/olia/discourse/olia_discourse.owl#ElementaryDiscourseUnit">
    <rdf:type rdf:resource="http://www.w3.org/2002/07/owl#Class"/>
  </rdf:Description>
  <rdf:Description rdf:about="http://purl.org/olia/discourse/olia_discourse.owl#ElementaryDiscourseUnit">
    <rdfs:subClassOf rdf:resource="http://purl.org/olia/discourse/olia_discourse.owl#DiscourseSegment"/>
  </rdf:Description>
  <rdf:Description rdf:about="http://purl.org/olia/discourse/olia_discourse.owl#ElementaryDiscourseUnit">
    <rdfs:comment>cf. SemDok ElementaryDiscourseSegment</rdfs:comment>
  </rdf:Description>
  <rdf:Description rdf:about="http://purl.org/olia/discourse/olia_discourse.owl#ElementaryDiscourseUnit">
    <rdfs:comment xml:lang="en">edu</rdfs:comment>
  </rdf:Description>
  <rdf:Description rdf:about="http://purl.org/olia/discourse/olia_discourse.owl#ElementaryDiscourseUnit">
    <rdfs:comment>A discourse segment that does not contain dependent discourse segments. Elementary element of discourse structure defined by a variety of grammatical criteria (Carlsson et al. 2003).</rdfs:comment>
  </rdf:Description>
  <rdf:Description rdf:about="http://purl.org/olia/discourse/olia_discourse.owl#ElementaryDiscourseUnit">
    <rdfs:comment>An elementary discourse unit is a terminal element in a hierarchical model of discourse structure.
(Note that here, the term "discourse segment" is used, as discourse unit is potentially ambiguous in comparison with "discourse entity".)

(cf. Carlson et al. 2003)</rdfs:comment>
  </rdf:Description>
  <rdf:Description rdf:about="http://purl.org/olia/discourse/olia_discourse.owl#ElementaryDiscourseUnit">
    <rdfs:label>elementary discourse segment</rdfs:label>
  </rdf:Description>
  <rdf:Description rdf:about="http://purl.org/olia/discourse/olia_discourse.owl#ElementaryDiscourseUnit">
    <rdfs:label xml:lang="en">elementary discourse unit</rdfs:label>
  </rdf:Description>
  <rdf:Description rdf:about="http://purl.org/olia/discourse/olia_discourse.owl#ElementaryDiscourseUnit">
    <rdfs:label xml:lang="en">minimal discourse unit</rdfs:label>
  </rdf:Description>
  <rdf:Description rdf:about="http://purl.org/olia/discourse/olia_discourse.owl#EmailAddress">
    <rdf:type rdf:resource="http://www.w3.org/2002/07/owl#Class"/>
  </rdf:Description>
  <rdf:Description rdf:about="http://purl.org/olia/discourse/olia_discourse.owl#EmailAddress">
    <rdfs:subClassOf rdf:resource="http://purl.org/olia/discourse/olia_discourse.owl#Address"/>
  </rdf:Description>
  <rdf:Description rdf:about="http://purl.org/olia/discourse/olia_discourse.owl#EmailAddress">
    <rdfs:comment xml:lang="en">for nerd:EmailAddress, sub nerd:Product</rdfs:comment>
  </rdf:Description>
  <rdf:Description rdf:about="http://purl.org/olia/discourse/olia_discourse.owl#EmailAddress">
    <rdfs:label xml:lang="en">email</rdfs:label>
  </rdf:Description>
  <rdf:Description rdf:about="http://purl.org/olia/discourse/olia_discourse.owl#EmailAddress">
    <skos:prefLabel xml:lang="en">email address</skos:prefLabel>
  </rdf:Description>
  <rdf:Description rdf:about="http://purl.org/olia/discourse/olia_discourse.owl#Enablement">
    <rdf:type rdf:resource="http://www.w3.org/2002/07/owl#Class"/>
  </rdf:Description>
  <rdf:Description rdf:about="http://purl.org/olia/discourse/olia_discourse.owl#Enablement">
    <rdfs:subClassOf rdf:resource="http://purl.org/olia/discourse/olia_discourse.owl#PragmaticCause"/>
  </rdf:Description>
  <rdf:Description rdf:about="http://purl.org/olia/discourse/olia_discourse.owl#Enablement">
    <inverseOf rdf:resource="http://purl.org/olia/discourse/Goal"/>
  </rdf:Description>
  <rdf:Description rdf:about="http://purl.org/olia/discourse/olia_discourse.owl#Enablement">
    <rdfs:comment>ISO Purpose with argument enablement. The nucleus is the the goal (intended result).</rdfs:comment>
  </rdf:Description>
  <rdf:Description rdf:about="http://purl.org/olia/discourse/olia_discourse.owl#Enablement">
    <rdfs:label>enablement</rdfs:label>
  </rdf:Description>
  <rdf:Description rdf:about="http://purl.org/olia/discourse/olia_discourse.owl#Enablement">
    <rdfs:label xml:lang="en">enablement</rdfs:label>
  </rdf:Description>
  <rdf:Description rdf:about="http://purl.org/olia/discourse/olia_discourse.owl#Enablement_RST">
    <rdf:type rdf:resource="http://www.w3.org/2002/07/owl#Class"/>
  </rdf:Description>
  <rdf:Description rdf:about="http://purl.org/olia/discourse/olia_discourse.owl#Enablement_RST">
    <rdfs:subClassOf rdf:resource="http://purl.org/olia/discourse/olia_discourse.owl#PragmaticCondition"/>
  </rdf:Description>
  <rdf:Description rdf:about="http://purl.org/olia/discourse/olia_discourse.owl#Enablement_RST">
    <rdfs:comment>In an ENABLEMENT relation, the situation presented in the nucleus is unreal-
ized. The action presented in the satellite increases the chances of the situation in the nucleus
being realized.
(Carlson and Marcu 2001)</rdfs:comment>
  </rdf:Description>
  <rdf:Description rdf:about="http://purl.org/olia/discourse/olia_discourse.owl#Enablement_RST">
    <rdfs:label xml:lang="en">enablement (RST)</rdfs:label>
  </rdf:Description>
  <rdf:Description rdf:about="http://purl.org/olia/discourse/olia_discourse.owl#EntityBasedRelation">
    <rdf:type rdf:resource="http://www.w3.org/2002/07/owl#Class"/>
  </rdf:Description>
  <rdf:Description rdf:about="http://purl.org/olia/discourse/olia_discourse.owl#EntityBasedRelation">
    <rdfs:subClassOf rdf:resource="http://purl.org/olia/discourse/olia_discourse.owl#DiscourseRelation"/>
  </rdf:Description>
  <rdf:Description rdf:about="http://purl.org/olia/discourse/olia_discourse.owl#EntityBasedRelation">
    <rdfs:subClassOf rdf:resource="http://purl.org/olia/discourse/olia_discourse.owl#SubjectMatterRelation"/>
  </rdf:Description>
  <rdf:Description rdf:about="http://purl.org/olia/discourse/olia_discourse.owl#EntityBasedRelation">
    <rdfs:comment>No discourse relation can be inferred and where the second sentence only serves to provide some further description of an entity in the first sentence. (Prasad et al. 2007)

Entity relations (which include Elaboration) are grouped with IdeationalRelations in SemDok, hence also a subclass of SubjectMatterRelation.

Note that we follow Webber and Knott (2001) to assume that Elaboration is always an entity relation (even though this entity may be abstract or implicit), however, many types of elaboration (taxonomy following SemDok) are put under Expansion in the PDTB tradition. Entity relations proper are thus only elaborations which have no other discourse relation assigned. These are (only) the sublasses of ElaborationDerivation.</rdfs:comment>
  </rdf:Description>
  <rdf:Description rdf:about="http://purl.org/olia/discourse/olia_discourse.owl#EntityBasedRelation">
    <rdfs:label xml:lang="en">entity based relation</rdfs:label>
  </rdf:Description>
  <rdf:Description rdf:about="http://purl.org/olia/discourse/olia_discourse.owl#EntityType">
    <rdf:type rdf:resource="http://www.w3.org/2002/07/owl#Class"/>
  </rdf:Description>
  <rdf:Description rdf:about="http://purl.org/olia/discourse/olia_discourse.owl#EntityType">
    <rdfs:subClassOf rdf:resource="http://purl.org/olia/discourse/olia_discourse.owl#SemanticFeature"/>
  </rdf:Description>
  <rdf:Description rdf:about="http://purl.org/olia/discourse/olia_discourse.owl#EntityType">
    <rdfs:comment>Categories specified for referring expressions (Poesio &amp; Artstein 2006): Abstract, Animate, Concrete, Person, Plan, Space, Time</rdfs:comment>
  </rdf:Description>
  <rdf:Description rdf:about="http://purl.org/olia/discourse/olia_discourse.owl#EntityType">
    <rdfs:label xml:lang="en">entity type</rdfs:label>
  </rdf:Description>
  <rdf:Description rdf:about="http://purl.org/olia/discourse/olia_discourse.owl#EpistemicCause_HDRB">
    <rdf:type rdf:resource="http://www.w3.org/2002/07/owl#Class"/>
  </rdf:Description>
  <rdf:Description rdf:about="http://purl.org/olia/discourse/olia_discourse.owl#EpistemicCause_HDRB">
    <rdfs:subClassOf rdf:resource="http://purl.org/olia/discourse/olia_discourse.owl#PragmaticCause"/>
  </rdf:Description>
  <rdf:Description rdf:about="http://purl.org/olia/discourse/olia_discourse.owl#EpistemicCause_HDRB">
    <rdfs:comment>An extension of the PDTB scheme suggested by Oza et al. (2009).

Each pragmatic sense at the type level is
further distinguished into three subtypes: “epis-
temic” (Sweetser 1990), “speech-act” (Sweetser
1990), and “propositional”.
(Oza et al. 2009)</rdfs:comment>
  </rdf:Description>
  <rdf:Description rdf:about="http://purl.org/olia/discourse/olia_discourse.owl#EpistemicCause_HDRB">
    <rdfs:label xml:lang="en">epistemic cause (HDRB)</rdfs:label>
  </rdf:Description>
  <rdf:Description rdf:about="http://purl.org/olia/discourse/olia_discourse.owl#EpistemicConcession_HDRB">
    <rdf:type rdf:resource="http://www.w3.org/2002/07/owl#Class"/>
  </rdf:Description>
  <rdf:Description rdf:about="http://purl.org/olia/discourse/olia_discourse.owl#EpistemicConcession_HDRB">
    <rdfs:subClassOf rdf:resource="http://purl.org/olia/discourse/olia_discourse.owl#PragmaticConcession_HDRB"/>
  </rdf:Description>
  <rdf:Description rdf:about="http://purl.org/olia/discourse/olia_discourse.owl#EpistemicConcession_HDRB">
    <rdfs:comment>Suggested as an extension of the PDTB scheme by Oza et al. (2009) and Tonelli et al. (2010).

Each pragmatic sense at the type level is
further distinguished into three subtypes: “epis-
temic” (Sweetser 1990), “speech-act” (Sweetser
1990), and “propositional”.
(Oza et al. 2009)</rdfs:comment>
  </rdf:Description>
  <rdf:Description rdf:about="http://purl.org/olia/discourse/olia_discourse.owl#EpistemicConcession_HDRB">
    <rdfs:label xml:lang="en">epistemic concession (HDRB)</rdfs:label>
  </rdf:Description>
  <rdf:Description rdf:about="http://purl.org/olia/discourse/olia_discourse.owl#EpistemicCondition">
    <rdf:type rdf:resource="http://www.w3.org/2002/07/owl#Class"/>
  </rdf:Description>
  <rdf:Description rdf:about="http://purl.org/olia/discourse/olia_discourse.owl#EpistemicCondition">
    <rdfs:subClassOf rdf:resource="http://purl.org/olia/discourse/olia_discourse.owl#PragmaticCondition"/>
  </rdf:Description>
  <rdf:Description rdf:about="http://purl.org/olia/discourse/olia_discourse.owl#EpistemicCondition">
    <rdfs:label xml:lang="en">epistemic condition</rdfs:label>
  </rdf:Description>
  <rdf:Description rdf:about="http://purl.org/olia/discourse/olia_discourse.owl#EpistemicCondition_HDRB">
    <rdf:type rdf:resource="http://www.w3.org/2002/07/owl#Class"/>
  </rdf:Description>
  <rdf:Description rdf:about="http://purl.org/olia/discourse/olia_discourse.owl#EpistemicCondition_HDRB">
    <rdfs:subClassOf rdf:resource="http://purl.org/olia/discourse/olia_discourse.owl#EpistemicCondition"/>
  </rdf:Description>
  <rdf:Description rdf:about="http://purl.org/olia/discourse/olia_discourse.owl#EpistemicCondition_HDRB">
    <rdfs:comment>An extension of the PDTB scheme suggested by Oza et al. (2009).

Each pragmatic sense at the type level is
further distinguished into three subtypes: “epis-
temic” (Sweetser 1990), “speech-act” (Sweetser
1990), and “propositional”.
(Oza et al. 2009)</rdfs:comment>
  </rdf:Description>
  <rdf:Description rdf:about="http://purl.org/olia/discourse/olia_discourse.owl#EpistemicCondition_HDRB">
    <rdfs:label xml:lang="en">epistemic condition (HDRB)</rdfs:label>
  </rdf:Description>
  <rdf:Description rdf:about="http://purl.org/olia/discourse/olia_discourse.owl#EpistemicCondition_LUNA">
    <rdf:type rdf:resource="http://www.w3.org/2002/07/owl#Class"/>
  </rdf:Description>
  <rdf:Description rdf:about="http://purl.org/olia/discourse/olia_discourse.owl#EpistemicCondition_LUNA">
    <rdfs:subClassOf rdf:resource="http://purl.org/olia/discourse/olia_discourse.owl#EpistemicCondition"/>
  </rdf:Description>
  <rdf:Description rdf:about="http://purl.org/olia/discourse/olia_discourse.owl#EpistemicCondition_LUNA">
    <rdfs:comment>Sara Tonelli, Giuseppe Riccardi, Rashmi Prasad and Aravind Joshi (2010), Annotation of Discourse Relations for Conversational Spoken Dialogs, Proceedings of the Seventh conference on International Language Resources and Evaluation (LREC'10), May, 19-21, Valletta, Malta</rdfs:comment>
  </rdf:Description>
  <rdf:Description rdf:about="http://purl.org/olia/discourse/olia_discourse.owl#EpistemicCondition_LUNA">
    <rdfs:label xml:lang="en">epistemic condition (LUNA)</rdfs:label>
  </rdf:Description>
  <rdf:Description rdf:about="http://purl.org/olia/discourse/olia_discourse.owl#EpistemicContrast_HDRB">
    <rdf:type rdf:resource="http://www.w3.org/2002/07/owl#Class"/>
  </rdf:Description>
  <rdf:Description rdf:about="http://purl.org/olia/discourse/olia_discourse.owl#EpistemicContrast_HDRB">
    <rdfs:subClassOf rdf:resource="http://purl.org/olia/discourse/olia_discourse.owl#PragmaticContrast_PDTB"/>
  </rdf:Description>
  <rdf:Description rdf:about="http://purl.org/olia/discourse/olia_discourse.owl#EpistemicContrast_HDRB">
    <rdfs:comment>Suggested as an extension of the PDTB scheme by Oza et al. (2009).

Each pragmatic sense at the type level is
further distinguished into three subtypes: “epis-
temic” (Sweetser 1990), “speech-act” (Sweetser
1990), and “propositional”.
(Oza et al. 2009)</rdfs:comment>
  </rdf:Description>
  <rdf:Description rdf:about="http://purl.org/olia/discourse/olia_discourse.owl#EpistemicContrast_HDRB">
    <rdfs:label xml:lang="en">epistemic contrast (HDRB)</rdfs:label>
  </rdf:Description>
  <rdf:Description rdf:about="http://purl.org/olia/discourse/olia_discourse.owl#EquivalentRestatement">
    <rdf:type rdf:resource="http://www.w3.org/2002/07/owl#Class"/>
  </rdf:Description>
  <rdf:Description rdf:about="http://purl.org/olia/discourse/olia_discourse.owl#EquivalentRestatement">
    <rdfs:subClassOf rdf:resource="http://purl.org/olia/discourse/olia_discourse.owl#Restatement"/>
  </rdf:Description>
  <rdf:Description rdf:about="http://purl.org/olia/discourse/olia_discourse.owl#EquivalentRestatement">
    <rdfs:comment>PDTB Restatement/equivalence. ISO Restatement (which does not include generalization/specialization relations, as these are in Elaboration, etc).</rdfs:comment>
  </rdf:Description>
  <rdf:Description rdf:about="http://purl.org/olia/discourse/olia_discourse.owl#EquivalentRestatement">
    <rdfs:label xml:lang="en">equivalent restatement</rdfs:label>
  </rdf:Description>
  <rdf:Description rdf:about="http://purl.org/olia/discourse/olia_discourse.owl#EquivalentRestatement_PDTB">
    <rdf:type rdf:resource="http://www.w3.org/2002/07/owl#Class"/>
  </rdf:Description>
  <rdf:Description rdf:about="http://purl.org/olia/discourse/olia_discourse.owl#EquivalentRestatement_PDTB">
    <rdfs:subClassOf rdf:resource="http://purl.org/olia/discourse/olia_discourse.owl#EquivalentRestatement"/>
  </rdf:Description>
  <rdf:Description rdf:about="http://purl.org/olia/discourse/olia_discourse.owl#EquivalentRestatement_PDTB">
    <rdfs:comment>Arg1 and Arg2 describe the same situation from different perspectives. (Prasad et al. 2007)</rdfs:comment>
  </rdf:Description>
  <rdf:Description rdf:about="http://purl.org/olia/discourse/olia_discourse.owl#EquivalentRestatement_PDTB">
    <rdfs:label>equivalence</rdfs:label>
  </rdf:Description>
  <rdf:Description rdf:about="http://purl.org/olia/discourse/olia_discourse.owl#EquivalentRestatement_PDTB">
    <rdfs:label xml:lang="en">equivalent restatement (PDTB)</rdfs:label>
  </rdf:Description>
  <rdf:Description rdf:about="http://purl.org/olia/discourse/olia_discourse.owl#Evaluation">
    <rdf:type rdf:resource="http://www.w3.org/2002/07/owl#Class"/>
  </rdf:Description>
  <rdf:Description rdf:about="http://purl.org/olia/discourse/olia_discourse.owl#Evaluation">
    <rdfs:subClassOf rdf:resource="http://purl.org/olia/discourse/olia_discourse.owl#Assessment"/>
  </rdf:Description>
  <rdf:Description rdf:about="http://purl.org/olia/discourse/olia_discourse.owl#Evaluation">
    <rdfs:comment>In an evaluation relationship, one span assesses the situation presented in the other
span of the relationship on a scale of good to bad. An evaluation can be an appraisal, estimation,
rating, interpretation, or assessment of a situation. The evaluation can be the viewpoint of the
writer or another agent in the text.
(Carlson and Marcu 2001)

Cf. SemDok Evaluation</rdfs:comment>
  </rdf:Description>
  <rdf:Description rdf:about="http://purl.org/olia/discourse/olia_discourse.owl#Evaluation">
    <rdfs:label xml:lang="en">evaluation</rdfs:label>
  </rdf:Description>
  <rdf:Description rdf:about="http://purl.org/olia/discourse/olia_discourse.owl#Evaluation_RST">
    <rdf:type rdf:resource="http://www.w3.org/2002/07/owl#Class"/>
  </rdf:Description>
  <rdf:Description rdf:about="http://purl.org/olia/discourse/olia_discourse.owl#Evaluation_RST">
    <rdfs:subClassOf rdf:resource="http://purl.org/olia/discourse/olia_discourse.owl#Evaluation"/>
  </rdf:Description>
  <rdf:Description rdf:about="http://purl.org/olia/discourse/olia_discourse.owl#Evaluation_RST">
    <rdfs:label xml:lang="en">evaluation (RST)</rdfs:label>
  </rdf:Description>
  <rdf:Description rdf:about="http://purl.org/olia/discourse/olia_discourse.owl#Evaluation_RST">
    <owl:deprecated rdf:datatype="http://www.w3.org/2001/XMLSchema#boolean">true</owl:deprecated>
  </rdf:Description>
  <rdf:Description rdf:about="http://purl.org/olia/discourse/olia_discourse.owl#Event">
    <rdf:type rdf:resource="http://www.w3.org/2002/07/owl#Class"/>
  </rdf:Description>
  <rdf:Description rdf:about="http://purl.org/olia/discourse/olia_discourse.owl#Event">
    <rdfs:subClassOf rdf:resource="http://purl.org/olia/discourse/olia_discourse.owl#AbstractEntity"/>
  </rdf:Description>
  <rdf:Description rdf:about="http://purl.org/olia/discourse/olia_discourse.owl#Event">
    <rdfs:comment xml:lang="en">introduced for nerd:Event, a NERD core class.</rdfs:comment>
  </rdf:Description>
  <rdf:Description rdf:about="http://purl.org/olia/discourse/olia_discourse.owl#EventualFactuality">
    <rdf:type rdf:resource="http://www.w3.org/2002/07/owl#Class"/>
  </rdf:Description>
  <rdf:Description rdf:about="http://purl.org/olia/discourse/olia_discourse.owl#EventualFactuality">
    <rdfs:subClassOf rdf:resource="http://purl.org/olia/discourse/olia_discourse.owl#Factuality"/>
  </rdf:Description>
  <rdf:Description rdf:about="http://purl.org/olia/discourse/olia_discourse.owl#EventualFactuality">
    <rdfs:comment>When eventuality AOs occur with attribution, it conveys an agent’s intention/attitude towards a considered event, state or action. Eventuality AOs occur with “control” types of attribution (“Ctrl” for short), conveyed by any of three different classes of control verbs (Sag and Pollard, 1991). The
first kind is anchored by a verb of influence like persuade, permit, order, and involve one agent influencing another agent to perform (or not perform) an action. The second kind is anchored by a verb of commitment like promise, agree, try, intend, refuse, decline, and involve an agent committing
to perform (or not perform) an action. The third kind is anchored by a verb of orientation like want, expect, wish, yearn, and involve desire, expectation, or some similar mental orientation towards some state(s) of affairs. These sub-distinctions are not encoded in the annotation, but we have used the definitions as a guide for identifying these predicates.
(Prasad et al. 2007, for PDTB)</rdfs:comment>
  </rdf:Description>
  <rdf:Description rdf:about="http://purl.org/olia/discourse/olia_discourse.owl#EventualFactuality">
    <rdfs:label xml:lang="en">eventual factuality</rdfs:label>
  </rdf:Description>
  <rdf:Description rdf:about="http://purl.org/olia/discourse/olia_discourse.owl#EventualFactuality">
    <rdfs:label>eventuality</rdfs:label>
  </rdf:Description>
  <rdf:Description rdf:about="http://purl.org/olia/discourse/olia_discourse.owl#Evidence">
    <rdf:type rdf:resource="http://www.w3.org/2002/07/owl#Class"/>
  </rdf:Description>
  <rdf:Description rdf:about="http://purl.org/olia/discourse/olia_discourse.owl#Evidence">
    <rdfs:subClassOf rdf:resource="http://purl.org/olia/discourse/olia_discourse.owl#Support"/>
  </rdf:Description>
  <rdf:Description rdf:about="http://purl.org/olia/discourse/olia_discourse.owl#Evidence">
    <rdfs:comment>Generalization over RST Evidence, SemDok Citation-evidence and SemDok Evidence</rdfs:comment>
  </rdf:Description>
  <rdf:Description rdf:about="http://purl.org/olia/discourse/olia_discourse.owl#Evidence">
    <rdfs:label xml:lang="en">evidence</rdfs:label>
  </rdf:Description>
  <rdf:Description rdf:about="http://purl.org/olia/discourse/olia_discourse.owl#Evidence_RST">
    <rdf:type rdf:resource="http://www.w3.org/2002/07/owl#Class"/>
  </rdf:Description>
  <rdf:Description rdf:about="http://purl.org/olia/discourse/olia_discourse.owl#Evidence_RST">
    <rdfs:subClassOf rdf:resource="http://purl.org/olia/discourse/olia_discourse.owl#Evidence"/>
  </rdf:Description>
  <rdf:Description rdf:about="http://purl.org/olia/discourse/olia_discourse.owl#Evidence_RST">
    <rdfs:comment>In an EVIDENCE relation, the situation presented in the satellite provides evi-
dence or justification for the situation presented in the nucleus. Usually EVIDENCE relations per-
tain to actions and situations that are independent of the will of an animate agent. Evidence is data
on which judgment of a conclusion may be based, and is presented by the writer or an agent in the
article to convince the reader of a point. An evidence satellite increases the chance of the reader
accepting the information presented in the nucleus.
(Carlson and Marcu 2001)</rdfs:comment>
  </rdf:Description>
  <rdf:Description rdf:about="http://purl.org/olia/discourse/olia_discourse.owl#Evidence_RST">
    <rdfs:label xml:lang="en">evidence (RST)</rdfs:label>
  </rdf:Description>
  <rdf:Description rdf:about="http://purl.org/olia/discourse/olia_discourse.owl#Example">
    <rdf:type rdf:resource="http://www.w3.org/2002/07/owl#Class"/>
  </rdf:Description>
  <rdf:Description rdf:about="http://purl.org/olia/discourse/olia_discourse.owl#Example">
    <rdfs:subClassOf rdf:resource="http://purl.org/olia/discourse/olia_discourse.owl#Instantiation"/>
  </rdf:Description>
  <rdf:Description rdf:about="http://purl.org/olia/discourse/olia_discourse.owl#Example">
    <rdfs:comment>RST "Example": The satellite provides an example with respect to the information presented in
the nucleus. If the example is a member of a set which may be enumerable but not all of whose
elements are known or specified, then choose the relation EXAMPLE. If the example is a member of an enumerable set whose elements are known or specified, select the relation ELABORATION-SET-
MEMBER.
(Carlson and Marcu 2001)

Infer a set of entities from DS0, E(DS0), and a set of entities from DS1, E(DS1). Then
find some element in E(DS1) that is a member or subset of the corresponding
element in E(DS0).
• Infer a set of entities from DS0, E(DS0), and a set of entities from DS1, E(DS1). Then
find some element in E(DS1) that is a new instantiation of an entity in E(DS0).
(Wolf et al. 2003)

cf. Al-Saif and Markert (2010) "Exemplification" in the LADTB corpus</rdfs:comment>
  </rdf:Description>
  <rdf:Description rdf:about="http://purl.org/olia/discourse/olia_discourse.owl#Example">
    <rdfs:label xml:lang="en">example</rdfs:label>
  </rdf:Description>
  <rdf:Description rdf:about="http://purl.org/olia/discourse/olia_discourse.owl#Exception">
    <rdf:type rdf:resource="http://www.w3.org/2002/07/owl#Class"/>
  </rdf:Description>
  <rdf:Description rdf:about="http://purl.org/olia/discourse/olia_discourse.owl#Exception">
    <rdfs:subClassOf rdf:resource="http://purl.org/olia/discourse/olia_discourse.owl#Expansion"/>
  </rdf:Description>
  <rdf:Description rdf:about="http://purl.org/olia/discourse/olia_discourse.owl#Exception">
    <rdfs:comment>PDTB Exception, ISO Exception</rdfs:comment>
  </rdf:Description>
  <rdf:Description rdf:about="http://purl.org/olia/discourse/olia_discourse.owl#Exception">
    <rdfs:label xml:lang="en">exception</rdfs:label>
  </rdf:Description>
  <rdf:Description rdf:about="http://purl.org/olia/discourse/olia_discourse.owl#Exception_PDTB">
    <rdf:type rdf:resource="http://www.w3.org/2002/07/owl#Class"/>
  </rdf:Description>
  <rdf:Description rdf:about="http://purl.org/olia/discourse/olia_discourse.owl#Exception_PDTB">
    <rdfs:subClassOf rdf:resource="http://purl.org/olia/discourse/olia_discourse.owl#Exception"/>
  </rdf:Description>
  <rdf:Description rdf:about="http://purl.org/olia/discourse/olia_discourse.owl#Exception_PDTB">
    <rdfs:comment>Arg2 specifies an exception to the generalization specified by Arg1. In other words, Arg1 is false because Arg2 is true, but if Arg2 were false, Arg1 would be true. (Prasad et al. 2007)</rdfs:comment>
  </rdf:Description>
  <rdf:Description rdf:about="http://purl.org/olia/discourse/olia_discourse.owl#Exception_PDTB">
    <rdfs:label xml:lang="en">exception (PDTB)</rdfs:label>
  </rdf:Description>
  <rdf:Description rdf:about="http://purl.org/olia/discourse/olia_discourse.owl#Expansion">
    <rdf:type rdf:resource="http://www.w3.org/2002/07/owl#Class"/>
  </rdf:Description>
  <rdf:Description rdf:about="http://purl.org/olia/discourse/olia_discourse.owl#Expansion">
    <rdfs:subClassOf rdf:resource="http://purl.org/olia/discourse/olia_discourse.owl#CoherenceRelation"/>
  </rdf:Description>
  <rdf:Description rdf:about="http://purl.org/olia/discourse/olia_discourse.owl#Expansion">
    <rdfs:comment>Relations which expand the discourse and move its narrative or exposition forward. (Prasad et al. 2007)

Note that Expansion in the sense of ISO has been equated by Bunt &amp; Prasad (ISA-12) with PDTB EntRel rather than PDTB Expansion. We follow this assessment</rdfs:comment>
  </rdf:Description>
  <rdf:Description rdf:about="http://purl.org/olia/discourse/olia_discourse.owl#Expansion">
    <rdfs:label xml:lang="en">expansion</rdfs:label>
  </rdf:Description>
  <rdf:Description rdf:about="http://purl.org/olia/discourse/olia_discourse.owl#Expectation">
    <rdf:type rdf:resource="http://www.w3.org/2002/07/owl#Class"/>
  </rdf:Description>
  <rdf:Description rdf:about="http://purl.org/olia/discourse/olia_discourse.owl#Expectation">
    <rdfs:subClassOf rdf:resource="http://purl.org/olia/discourse/olia_discourse.owl#Concession"/>
  </rdf:Description>
  <rdf:Description rdf:about="http://purl.org/olia/discourse/olia_discourse.owl#Expectation">
    <inverseOf rdf:resource="http://purl.org/olia/discourse/ContaExpectation"/>
  </rdf:Description>
  <rdf:Description rdf:about="http://purl.org/olia/discourse/olia_discourse.owl#Expectation">
    <rdfs:comment>PDTB COMPARISON/Concession/expectation: Arg2 creates an expectation that Arg1 denies. (Prasad et al. 2007)

ISO Core-DR: Concession, argument Expectation-raiser (Bunt &amp; Prasad, ISA-12)</rdfs:comment>
  </rdf:Description>
  <rdf:Description rdf:about="http://purl.org/olia/discourse/olia_discourse.owl#Expectation">
    <rdfs:label>expectation</rdfs:label>
  </rdf:Description>
  <rdf:Description rdf:about="http://purl.org/olia/discourse/olia_discourse.owl#Expectation">
    <rdfs:label xml:lang="en">expectation</rdfs:label>
  </rdf:Description>
  <rdf:Description rdf:about="http://purl.org/olia/discourse/olia_discourse.owl#Explanation">
    <rdf:type rdf:resource="http://www.w3.org/2002/07/owl#Class"/>
  </rdf:Description>
  <rdf:Description rdf:about="http://purl.org/olia/discourse/olia_discourse.owl#Explanation">
    <rdfs:subClassOf rdf:resource="http://purl.org/olia/discourse/olia_discourse.owl#PragmaticCause"/>
  </rdf:Description>
  <rdf:Description rdf:about="http://purl.org/olia/discourse/olia_discourse.owl#Explanation">
    <rdfs:comment>An EXPLANATION-ARGUMENTATIVE relation usually pertain to actions and situations that are independent of the will of an animate agent.The satellite provides a factual explanation for the situation presented in the nucleus. (Carlson and Marcu 2001)

Explanation: Infer a causal relation between DS0 and DS1. (Wolf et al. 2003)</rdfs:comment>
  </rdf:Description>
  <rdf:Description rdf:about="http://purl.org/olia/discourse/olia_discourse.owl#Explanation">
    <rdfs:label xml:lang="en">explanation</rdfs:label>
  </rdf:Description>
  <rdf:Description rdf:about="http://purl.org/olia/discourse/olia_discourse.owl#ExplicitConnective">
    <rdf:type rdf:resource="http://www.w3.org/2002/07/owl#Class"/>
  </rdf:Description>
  <rdf:Description rdf:about="http://purl.org/olia/discourse/olia_discourse.owl#ExplicitConnective">
    <rdfs:subClassOf rdf:resource="http://purl.org/olia/discourse/olia_discourse.owl#RelationCue"/>
  </rdf:Description>
  <rdf:Description rdf:about="http://purl.org/olia/discourse/olia_discourse.owl#ExplicitConnective">
    <rdfs:comment>Explicit discourse connectives ... are drawn primarily from well-defined syntactic classes, i.e., Subordinating conjunctions (e.g., because, when, since, although), Coordinating conjunctions (e.g., and, or, nor):, (ADVP and PP) adverbials (e.g., however, otherwise, then, as a result, for example).
(Prasad et al. 2007, PDTB)</rdfs:comment>
  </rdf:Description>
  <rdf:Description rdf:about="http://purl.org/olia/discourse/olia_discourse.owl#ExplicitConnective">
    <rdfs:label xml:lang="en">explicit connective</rdfs:label>
  </rdf:Description>
  <rdf:Description rdf:about="http://purl.org/olia/discourse/olia_discourse.owl#ExpressionFocus">
    <rdf:type rdf:resource="http://www.w3.org/2002/07/owl#Class"/>
  </rdf:Description>
  <rdf:Description rdf:about="http://purl.org/olia/discourse/olia_discourse.owl#ExpressionFocus">
    <rdfs:subClassOf rdf:resource="http://purl.org/olia/discourse/olia_discourse.owl#Focus"/>
  </rdf:Description>
  <rdf:Description rdf:about="http://purl.org/olia/discourse/olia_discourse.owl#ExpressionFocus">
    <rdfs:comment>Krifka distinguishes between ‘expression focus’ and ‘denotation focus.’ Differences in meaning are only found in the latter kind of focus, on which we concentrate here.

The pragmatic use of focus (or ‘management of CG’) does not
involve any change in the truth-value of the sentence. Only the semantic use of focus (or ‘content of CG’) has such an effect. Pragmatic uses of focus include answers to wh-questions, corrections, confirmations, parallel expressions and delimitations.

(Féry et al. 2007)</rdfs:comment>
  </rdf:Description>
  <rdf:Description rdf:about="http://purl.org/olia/discourse/olia_discourse.owl#ExpressionFocus">
    <rdfs:label xml:lang="en">expression focus</rdfs:label>
  </rdf:Description>
  <rdf:Description rdf:about="http://purl.org/olia/discourse/olia_discourse.owl#Extra">
    <rdf:type rdf:resource="http://www.w3.org/2002/07/owl#Class"/>
  </rdf:Description>
  <rdf:Description rdf:about="http://purl.org/olia/discourse/olia_discourse.owl#Extra">
    <rdfs:subClassOf rdf:resource="http://purl.org/olia/discourse/olia_discourse.owl#TextualOrganizationalRelation"/>
  </rdf:Description>
  <rdf:Description rdf:about="http://purl.org/olia/discourse/olia_discourse.owl#Extra">
    <rdfs:comment>cf. SemDok Extra (undefined)</rdfs:comment>
  </rdf:Description>
  <rdf:Description rdf:about="http://purl.org/olia/discourse/olia_discourse.owl#Extra">
    <rdfs:label>extra</rdfs:label>
  </rdf:Description>
  <rdf:Description rdf:about="http://purl.org/olia/discourse/olia_discourse.owl#Extra">
    <rdfs:label xml:lang="en">extra</rdfs:label>
  </rdf:Description>
  <rdf:Description rdf:about="http://purl.org/olia/discourse/olia_discourse.owl#FacetiousRegister">
    <rdf:type rdf:resource="http://www.w3.org/2002/07/owl#Class"/>
  </rdf:Description>
  <rdf:Description rdf:about="http://purl.org/olia/discourse/olia_discourse.owl#FacetiousRegister">
    <rdfs:subClassOf rdf:resource="http://purl.org/olia/olia-top.owl#RegisterFeature"/>
  </rdf:Description>
  <rdf:Description rdf:about="http://purl.org/olia/discourse/olia_discourse.owl#FacetiousRegister">
    <rdfs:comment>
                            Register related to an expression that is intended to be clever and funny but that is really silly and annoying.
                                (Longma DCE; http://www.isocat.org/datcat/DC-1991)
                            </rdfs:comment>
  </rdf:Description>
  <rdf:Description rdf:about="http://purl.org/olia/discourse/olia_discourse.owl#FacetiousRegister">
    <rdfs:label>facecious register</rdfs:label>
  </rdf:Description>
  <rdf:Description rdf:about="http://purl.org/olia/discourse/olia_discourse.owl#FacetiousRegister">
    <owl:versionInfo>http://www.isocat.org/datcat/DC-1991</owl:versionInfo>
  </rdf:Description>
  <rdf:Description rdf:about="http://purl.org/olia/discourse/olia_discourse.owl#FacetiousRegister">
    <owl:versionInfo>subClassOf register (dcif:conceptualDomain)</owl:versionInfo>
  </rdf:Description>
  <rdf:Description rdf:about="http://purl.org/olia/discourse/olia_discourse.owl#FactiveFactuality">
    <rdf:type rdf:resource="http://www.w3.org/2002/07/owl#Class"/>
  </rdf:Description>
  <rdf:Description rdf:about="http://purl.org/olia/discourse/olia_discourse.owl#FactiveFactuality">
    <rdfs:subClassOf rdf:resource="http://purl.org/olia/discourse/olia_discourse.owl#Factuality"/>
  </rdf:Description>
  <rdf:Description rdf:about="http://purl.org/olia/discourse/olia_discourse.owl#FactiveFactuality">
    <rdfs:comment>Facts AOs involve attribution to an agent of an evaluation towards or knowledge of a proposition whose truth is taken for granted (i.e., presupposed). Fact AOs are associated with a “factive” type of attribution (“Ftv” for short), conveyed by “factive” and “semi-factive verbs” (Kiparsky and Kiparsky, 1971; Karttunen, 1971) such as regret, forget, remember, know, see, hear, etc.
(Prasad et al. 2007, PDTB)</rdfs:comment>
  </rdf:Description>
  <rdf:Description rdf:about="http://purl.org/olia/discourse/olia_discourse.owl#FactiveFactuality">
    <rdfs:label>fact</rdfs:label>
  </rdf:Description>
  <rdf:Description rdf:about="http://purl.org/olia/discourse/olia_discourse.owl#FactiveFactuality">
    <rdfs:label>factive</rdfs:label>
  </rdf:Description>
  <rdf:Description rdf:about="http://purl.org/olia/discourse/olia_discourse.owl#FactiveFactuality">
    <rdfs:label xml:lang="en">factive factuality</rdfs:label>
  </rdf:Description>
  <rdf:Description rdf:about="http://purl.org/olia/discourse/olia_discourse.owl#FactualCondition">
    <rdf:type rdf:resource="http://www.w3.org/2002/07/owl#Class"/>
  </rdf:Description>
  <rdf:Description rdf:about="http://purl.org/olia/discourse/olia_discourse.owl#FactualCondition">
    <rdfs:subClassOf rdf:resource="http://purl.org/olia/discourse/olia_discourse.owl#SemanticCondition"/>
  </rdf:Description>
  <rdf:Description rdf:about="http://purl.org/olia/discourse/olia_discourse.owl#FactualCondition">
    <rdfs:label xml:lang="en">factual condition</rdfs:label>
  </rdf:Description>
  <rdf:Description rdf:about="http://purl.org/olia/discourse/olia_discourse.owl#FactualCondition_HDRB">
    <rdf:type rdf:resource="http://www.w3.org/2002/07/owl#Class"/>
  </rdf:Description>
  <rdf:Description rdf:about="http://purl.org/olia/discourse/olia_discourse.owl#FactualCondition_HDRB">
    <rdfs:subClassOf rdf:resource="http://purl.org/olia/discourse/olia_discourse.owl#FactualCondition"/>
  </rdf:Description>
  <rdf:Description rdf:about="http://purl.org/olia/discourse/olia_discourse.owl#FactualCondition_HDRB">
    <rdfs:comment>Oza et al. (2009) suggested to abandon the PDTB distinction between FactualPastCondition and FactualPresentCondition.</rdfs:comment>
  </rdf:Description>
  <rdf:Description rdf:about="http://purl.org/olia/discourse/olia_discourse.owl#FactualCondition_HDRB">
    <rdfs:label xml:lang="en">factual condition (HDRB)</rdfs:label>
  </rdf:Description>
  <rdf:Description rdf:about="http://purl.org/olia/discourse/olia_discourse.owl#FactualCondition_HDRB">
    <rdfs:label>merge with factual condition</rdfs:label>
  </rdf:Description>
  <rdf:Description rdf:about="http://purl.org/olia/discourse/olia_discourse.owl#FactualPastCondition_PDTB">
    <rdf:type rdf:resource="http://www.w3.org/2002/07/owl#Class"/>
  </rdf:Description>
  <rdf:Description rdf:about="http://purl.org/olia/discourse/olia_discourse.owl#FactualPastCondition_PDTB">
    <rdfs:subClassOf rdf:resource="http://purl.org/olia/discourse/olia_discourse.owl#FactualCondition"/>
  </rdf:Description>
  <rdf:Description rdf:about="http://purl.org/olia/discourse/olia_discourse.owl#FactualPastCondition_PDTB">
    <rdfs:comment>Arg2 describes a situation that is assumed to have taken place at a time in the past, and in Arg1, a consequence that may subsequently occur assuming Arg2 holds. (Prasad et al. 2007)</rdfs:comment>
  </rdf:Description>
  <rdf:Description rdf:about="http://purl.org/olia/discourse/olia_discourse.owl#FactualPastCondition_PDTB">
    <rdfs:label xml:lang="en">factual past condition (PDTB)</rdfs:label>
  </rdf:Description>
  <rdf:Description rdf:about="http://purl.org/olia/discourse/olia_discourse.owl#FactualPresentCondition_PDTB">
    <rdf:type rdf:resource="http://www.w3.org/2002/07/owl#Class"/>
  </rdf:Description>
  <rdf:Description rdf:about="http://purl.org/olia/discourse/olia_discourse.owl#FactualPresentCondition_PDTB">
    <rdfs:subClassOf rdf:resource="http://purl.org/olia/discourse/olia_discourse.owl#FactualCondition"/>
  </rdf:Description>
  <rdf:Description rdf:about="http://purl.org/olia/discourse/olia_discourse.owl#FactualPresentCondition_PDTB">
    <rdfs:comment>Arg2 is a situation that has either been presented as a fact in the prior discourse or is believed
by somebody other than the speaker/writer. “Factual present” is really a special case of the subtype
“hypothetical”. (Prasad et al. 2007)</rdfs:comment>
  </rdf:Description>
  <rdf:Description rdf:about="http://purl.org/olia/discourse/olia_discourse.owl#FactualPresentCondition_PDTB">
    <rdfs:label xml:lang="en">factual present condition (PDTB)</rdfs:label>
  </rdf:Description>
  <rdf:Description rdf:about="http://purl.org/olia/discourse/olia_discourse.owl#Factuality">
    <rdf:type rdf:resource="http://www.w3.org/2002/07/owl#Class"/>
  </rdf:Description>
  <rdf:Description rdf:about="http://purl.org/olia/discourse/olia_discourse.owl#Factuality">
    <rdfs:subClassOf rdf:resource="http://purl.org/olia/discourse/olia_discourse.owl#SemanticFeature"/>
  </rdf:Description>
  <rdf:Description rdf:about="http://purl.org/olia/discourse/olia_discourse.owl#Factuality">
    <rdfs:comment>PDTB (applied to AttributionObjects)
Classification of Attribute relations with respect to the "Type", i.e., the nature of the relationship between agents and AOs, leading to different inferences about the degree of factuality of the AO (Prasad et al. 2007).</rdfs:comment>
  </rdf:Description>
  <rdf:Description rdf:about="http://purl.org/olia/discourse/olia_discourse.owl#Factuality">
    <rdfs:label xml:lang="en">factuality</rdfs:label>
  </rdf:Description>
  <rdf:Description rdf:about="http://purl.org/olia/discourse/olia_discourse.owl#FavouredAlternative">
    <rdf:type rdf:resource="http://www.w3.org/2002/07/owl#Class"/>
  </rdf:Description>
  <rdf:Description rdf:about="http://purl.org/olia/discourse/olia_discourse.owl#FavouredAlternative">
    <rdfs:subClassOf rdf:resource="http://purl.org/olia/discourse/olia_discourse.owl#Alternative"/>
  </rdf:Description>
  <rdf:Description rdf:about="http://purl.org/olia/discourse/olia_discourse.owl#FavouredAlternative">
    <inverseOf rdf:resource="http://purl.org/olia/discourse/DisfavouredAlternative"/>
  </rdf:Description>
  <rdf:Description rdf:about="http://purl.org/olia/discourse/olia_discourse.owl#FavouredAlternative">
    <rdfs:comment>ISO Substitution with argument favoured alternative</rdfs:comment>
  </rdf:Description>
  <rdf:Description rdf:about="http://purl.org/olia/discourse/olia_discourse.owl#FavouredAlternative">
    <rdfs:label>favoured alternative</rdfs:label>
  </rdf:Description>
  <rdf:Description rdf:about="http://purl.org/olia/discourse/olia_discourse.owl#FavouredAlternative">
    <rdfs:label xml:lang="en">favoured alternative</rdfs:label>
  </rdf:Description>
  <rdf:Description rdf:about="http://purl.org/olia/discourse/olia_discourse.owl#FeedbackAct">
    <rdf:type rdf:resource="http://www.w3.org/2002/07/owl#Class"/>
  </rdf:Description>
  <rdf:Description rdf:about="http://purl.org/olia/discourse/olia_discourse.owl#FeedbackAct">
    <rdfs:subClassOf rdf:resource="http://purl.org/olia/discourse/olia_discourse.owl#UnsolicitedResponse"/>
  </rdf:Description>
  <rdf:Description rdf:about="http://purl.org/olia/discourse/olia_discourse.owl#FeedbackAct">
    <inverseOf rdf:resource="http://purl.org/olia/discourse/FeedbackScope"/>
  </rdf:Description>
  <rdf:Description rdf:about="http://purl.org/olia/discourse/olia_discourse.owl#FeedbackAct">
    <rdfs:comment>Mononuclear relation linking a dialogue act with a responsive communicative function (feedback act) with its scope. The nucleus is the scope.

Corresponds to ISO Feedback Dependence with argument feedback act.</rdfs:comment>
  </rdf:Description>
  <rdf:Description rdf:about="http://purl.org/olia/discourse/olia_discourse.owl#FeedbackAct">
    <rdfs:label>feedback</rdfs:label>
  </rdf:Description>
  <rdf:Description rdf:about="http://purl.org/olia/discourse/olia_discourse.owl#FeedbackAct">
    <rdfs:label xml:lang="en">feedback act</rdfs:label>
  </rdf:Description>
  <rdf:Description rdf:about="http://purl.org/olia/discourse/olia_discourse.owl#FeedbackAct">
    <skos:prefLabel>feedback act</skos:prefLabel>
  </rdf:Description>
  <rdf:Description rdf:about="http://purl.org/olia/discourse/olia_discourse.owl#FeedbackScope">
    <rdf:type rdf:resource="http://www.w3.org/2002/07/owl#Class"/>
  </rdf:Description>
  <rdf:Description rdf:about="http://purl.org/olia/discourse/olia_discourse.owl#FeedbackScope">
    <rdfs:subClassOf rdf:resource="http://purl.org/olia/discourse/olia_discourse.owl#UnsolicitedResponse"/>
  </rdf:Description>
  <rdf:Description rdf:about="http://purl.org/olia/discourse/olia_discourse.owl#FeedbackScope">
    <inverseOf rdf:resource="http://purl.org/olia/discourse/FeedbackAct"/>
  </rdf:Description>
  <rdf:Description rdf:about="http://purl.org/olia/discourse/olia_discourse.owl#FeedbackScope">
    <rdfs:comment>Mononuclear relation linking the scope of a feedback act with the feedback act. The nucleus is the feedback act.

Corresponds to ISO Feedback Dependence with argument Feedback Scope.</rdfs:comment>
  </rdf:Description>
  <rdf:Description rdf:about="http://purl.org/olia/discourse/olia_discourse.owl#FeedbackScope">
    <rdfs:label>feedback scope</rdfs:label>
  </rdf:Description>
  <rdf:Description rdf:about="http://purl.org/olia/discourse/olia_discourse.owl#FeedbackScope">
    <rdfs:label xml:lang="en">feedback scope</rdfs:label>
  </rdf:Description>
  <rdf:Description rdf:about="http://purl.org/olia/discourse/olia_discourse.owl#FictionalCharacter">
    <rdf:type rdf:resource="http://www.w3.org/2002/07/owl#Class"/>
  </rdf:Description>
  <rdf:Description rdf:about="http://purl.org/olia/discourse/olia_discourse.owl#FictionalCharacter">
    <rdfs:subClassOf rdf:resource="http://purl.org/olia/discourse/olia_discourse.owl#Person"/>
  </rdf:Description>
  <rdf:Description rdf:about="http://purl.org/olia/discourse/olia_discourse.owl#FictionalCharacter">
    <rdfs:comment xml:lang="en">for nerd:FictionalCharacter. As this is not supported by an external extractor, it is deprecated.</rdfs:comment>
  </rdf:Description>
  <rdf:Description rdf:about="http://purl.org/olia/discourse/olia_discourse.owl#FictionalCharacter">
    <owl:deprecated rdf:datatype="http://www.w3.org/2001/XMLSchema#boolean">true</owl:deprecated>
  </rdf:Description>
  <rdf:Description rdf:about="http://purl.org/olia/discourse/olia_discourse.owl#Focus">
    <rdf:type rdf:resource="http://www.w3.org/2002/07/owl#Class"/>
  </rdf:Description>
  <rdf:Description rdf:about="http://purl.org/olia/discourse/olia_discourse.owl#Focus">
    <rdfs:subClassOf rdf:resource="http://purl.org/olia/discourse/olia_discourse.owl#PragmaticUnit"/>
  </rdf:Description>
  <rdf:Description rdf:about="http://purl.org/olia/discourse/olia_discourse.owl#Focus">
    <rdfs:comment>Focus indicates the presence of alternatives that are relevant for the
interpretation of linguistic expressions.
(Féry et al. 2007)

That part of an expression which provides the most relevant information in a particular context as opposed to the (not so relevant) rest of information making up the background of the utterance. Typically, focus on a subexpression indicates that it is selected from possible alternatives that are either implicit or given explicitly, whereas the background can be derived from the context of the utterance. (SFB632 Guidelines)

Foci are classified here according to their discourse function (independently from their structural realization).</rdfs:comment>
  </rdf:Description>
  <rdf:Description rdf:about="http://purl.org/olia/discourse/olia_discourse.owl#Focus">
    <rdfs:label xml:lang="en">focus</rdfs:label>
  </rdf:Description>
  <rdf:Description rdf:about="http://purl.org/olia/discourse/olia_discourse.owl#FocusDomain">
    <rdf:type rdf:resource="http://www.w3.org/2002/07/owl#Class"/>
  </rdf:Description>
  <rdf:Description rdf:about="http://purl.org/olia/discourse/olia_discourse.owl#FocusDomain">
    <rdfs:subClassOf rdf:resource="http://purl.org/olia/discourse/olia_discourse.owl#Markable"/>
  </rdf:Description>
  <rdf:Description rdf:about="http://purl.org/olia/discourse/olia_discourse.owl#FocusDomain">
    <rdfs:comment>Structural domain that corresponds to the scope of the focus.
(van Valin &amp; Lapolla 1997)</rdfs:comment>
  </rdf:Description>
  <rdf:Description rdf:about="http://purl.org/olia/discourse/olia_discourse.owl#FocusDomain">
    <rdfs:label xml:lang="en">focus domain</rdfs:label>
  </rdf:Description>
  <rdf:Description rdf:about="http://purl.org/olia/discourse/olia_discourse.owl#Footnote">
    <rdf:type rdf:resource="http://www.w3.org/2002/07/owl#Class"/>
  </rdf:Description>
  <rdf:Description rdf:about="http://purl.org/olia/discourse/olia_discourse.owl#Footnote">
    <rdfs:subClassOf rdf:resource="http://purl.org/olia/olia-top.owl#TextStructuralUnit"/>
  </rdf:Description>
  <rdf:Description rdf:about="http://purl.org/olia/discourse/olia_discourse.owl#Footnote">
    <rdfs:comment>Supplementary information given outside of the body of the text, usually at
the end of a document in this corpus. (Carlson and Marcu 2001)</rdfs:comment>
  </rdf:Description>
  <rdf:Description rdf:about="http://purl.org/olia/discourse/olia_discourse.owl#Footnote">
    <rdfs:label xml:lang="en">footnote</rdfs:label>
  </rdf:Description>
  <rdf:Description rdf:about="http://purl.org/olia/discourse/olia_discourse.owl#FormalRegister">
    <rdf:type rdf:resource="http://www.w3.org/2002/07/owl#Class"/>
  </rdf:Description>
  <rdf:Description rdf:about="http://purl.org/olia/discourse/olia_discourse.owl#FormalRegister">
    <rdfs:subClassOf rdf:resource="http://purl.org/olia/olia-top.owl#RegisterFeature"/>
  </rdf:Description>
  <rdf:Description rdf:about="http://purl.org/olia/discourse/olia_discourse.owl#FormalRegister">
    <rdfs:comment>
                            Formal register.
                                (12620; http://www.isocat.org/datcat/DC-1992)
                            </rdfs:comment>
  </rdf:Description>
  <rdf:Description rdf:about="http://purl.org/olia/discourse/olia_discourse.owl#FormalRegister">
    <rdfs:label>formal register</rdfs:label>
  </rdf:Description>
  <rdf:Description rdf:about="http://purl.org/olia/discourse/olia_discourse.owl#FormalRegister">
    <owl:versionInfo>http://www.isocat.org/datcat/DC-1992</owl:versionInfo>
  </rdf:Description>
  <rdf:Description rdf:about="http://purl.org/olia/discourse/olia_discourse.owl#FormalRegister">
    <owl:versionInfo>subClassOf register (dcif:conceptualDomain)</owl:versionInfo>
  </rdf:Description>
  <rdf:Description rdf:about="http://purl.org/olia/discourse/olia_discourse.owl#FrameSettingTopic">
    <rdf:type rdf:resource="http://www.w3.org/2002/07/owl#Class"/>
  </rdf:Description>
  <rdf:Description rdf:about="http://purl.org/olia/discourse/olia_discourse.owl#FrameSettingTopic">
    <rdfs:subClassOf rdf:resource="http://purl.org/olia/discourse/olia_discourse.owl#Topic"/>
  </rdf:Description>
  <rdf:Description rdf:about="http://purl.org/olia/discourse/olia_discourse.owl#FrameSettingTopic">
    <rdfs:comment>An element that is realized at a particularly prominent (sentence-initial) position and defines a spatio-temporal context with reference to which an utterance is to be interpreted (Erteschik-Shir 1994).</rdfs:comment>
  </rdf:Description>
  <rdf:Description rdf:about="http://purl.org/olia/discourse/olia_discourse.owl#FrameSettingTopic">
    <rdfs:label xml:lang="en">frame setting topic</rdfs:label>
  </rdf:Description>
  <rdf:Description rdf:about="http://purl.org/olia/discourse/olia_discourse.owl#Function">
    <rdf:type rdf:resource="http://www.w3.org/2002/07/owl#Class"/>
  </rdf:Description>
  <rdf:Description rdf:about="http://purl.org/olia/discourse/olia_discourse.owl#Function">
    <rdfs:subClassOf rdf:resource="http://purl.org/olia/discourse/olia_discourse.owl#ConcreteEntity"/>
  </rdf:Description>
  <rdf:Description rdf:about="http://purl.org/olia/discourse/olia_discourse.owl#Function">
    <rdfs:comment xml:lang="en">For nerd:Function (=opencalais:Position, dbo:PersonFunction), a NERD core class that seems to designate ranks and professions, albeit some of these are subsumed under nerd:Person. Because of the unclear definition and the unclear relation with nerd:Person, this is marked as deprecated.</rdfs:comment>
  </rdf:Description>
  <rdf:Description rdf:about="http://purl.org/olia/discourse/olia_discourse.owl#Function">
    <rdfs:label xml:lang="en">FONC</rdfs:label>
  </rdf:Description>
  <rdf:Description rdf:about="http://purl.org/olia/discourse/olia_discourse.owl#Function">
    <rdfs:label xml:lang="en">function</rdfs:label>
  </rdf:Description>
  <rdf:Description rdf:about="http://purl.org/olia/discourse/olia_discourse.owl#Function">
    <rdfs:label xml:lang="en">person function</rdfs:label>
  </rdf:Description>
  <rdf:Description rdf:about="http://purl.org/olia/discourse/olia_discourse.owl#Function">
    <rdfs:label xml:lang="en">position</rdfs:label>
  </rdf:Description>
  <rdf:Description rdf:about="http://purl.org/olia/discourse/olia_discourse.owl#Function">
    <owl:deprecated rdf:datatype="http://www.w3.org/2001/XMLSchema#boolean">true</owl:deprecated>
  </rdf:Description>
  <rdf:Description rdf:about="http://purl.org/olia/discourse/olia_discourse.owl#GeneralCondition_PDTB">
    <rdf:type rdf:resource="http://www.w3.org/2002/07/owl#Class"/>
  </rdf:Description>
  <rdf:Description rdf:about="http://purl.org/olia/discourse/olia_discourse.owl#GeneralCondition_PDTB">
    <rdfs:subClassOf rdf:resource="http://purl.org/olia/discourse/olia_discourse.owl#FactualCondition"/>
  </rdf:Description>
  <rdf:Description rdf:about="http://purl.org/olia/discourse/olia_discourse.owl#GeneralCondition_PDTB">
    <rdfs:comment>Every time that ||Arg2|| holds true , ||Arg1|| is also caused to be true. (Prasad et al. 2007)</rdfs:comment>
  </rdf:Description>
  <rdf:Description rdf:about="http://purl.org/olia/discourse/olia_discourse.owl#GeneralCondition_PDTB">
    <rdfs:label xml:lang="en">general condition (PDTB)</rdfs:label>
  </rdf:Description>
  <rdf:Description rdf:about="http://purl.org/olia/discourse/olia_discourse.owl#Generalization">
    <rdf:type rdf:resource="http://www.w3.org/2002/07/owl#Class"/>
  </rdf:Description>
  <rdf:Description rdf:about="http://purl.org/olia/discourse/olia_discourse.owl#Generalization">
    <rdfs:subClassOf rdf:resource="http://purl.org/olia/discourse/olia_discourse.owl#Restatement"/>
  </rdf:Description>
  <rdf:Description rdf:about="http://purl.org/olia/discourse/olia_discourse.owl#Generalization">
    <inverseOf rdf:resource="http://purl.org/olia/discourse/Specification"/>
  </rdf:Description>
  <rdf:Description rdf:about="http://purl.org/olia/discourse/olia_discourse.owl#Generalization">
    <rdfs:comment>Arg2 summarizes Arg1, or in some cases expresses a conclusion based on Arg1. Typical connectives for “generalization” are in sum, overall, finally, etc. (Prasad et al. 2007)

Infer a set of entities from DS0, E(DS0), and a set of entities from DS1, E(DS1). Then
find some element in E(DS0) that is a member or subset of the corresponding
element in E(DS1).
• Infer a set of entities from DS0, E(DS0), and a set of entities from DS1, E(DS1). Then
find some element in E(DS0) that is a new instantiation of an entity in E(DS1).
(Wolf et al. 2003)</rdfs:comment>
  </rdf:Description>
  <rdf:Description rdf:about="http://purl.org/olia/discourse/olia_discourse.owl#Generalization">
    <rdfs:label xml:lang="en">generalization</rdfs:label>
  </rdf:Description>
  <rdf:Description rdf:about="http://purl.org/olia/discourse/olia_discourse.owl#GenerallyAccessible">
    <rdf:type rdf:resource="http://www.w3.org/2002/07/owl#Class"/>
  </rdf:Description>
  <rdf:Description rdf:about="http://purl.org/olia/discourse/olia_discourse.owl#GenerallyAccessible">
    <rdfs:subClassOf rdf:resource="http://purl.org/olia/discourse/olia_discourse.owl#Accessible"/>
  </rdf:Description>
  <rdf:Description rdf:about="http://purl.org/olia/discourse/olia_discourse.owl#GenerallyAccessible">
    <rdfs:comment>A referent is accessible to a hearer on grounds of the hearer's world knowledge or knowledge the speaker presupposes the hearer to have. (Lambrecht 1994)</rdfs:comment>
  </rdf:Description>
  <rdf:Description rdf:about="http://purl.org/olia/discourse/olia_discourse.owl#GenerallyAccessible">
    <rdfs:label xml:lang="en">generally accessible</rdfs:label>
  </rdf:Description>
  <rdf:Description rdf:about="http://purl.org/olia/discourse/olia_discourse.owl#GeographicalFeature">
    <rdf:type rdf:resource="http://www.w3.org/2002/07/owl#Class"/>
  </rdf:Description>
  <rdf:Description rdf:about="http://purl.org/olia/discourse/olia_discourse.owl#GeographicalFeature">
    <rdfs:subClassOf rdf:resource="http://purl.org/olia/discourse/olia_discourse.owl#Space"/>
  </rdf:Description>
  <rdf:Description rdf:about="http://purl.org/olia/discourse/olia_discourse.owl#GeographicalFeature">
    <rdfs:comment xml:lang="en">introduced as a generalization over nerd:Space subclasses pertaining to natural features and waterways (canals and lakes can be artificial)</rdfs:comment>
  </rdf:Description>
  <rdf:Description rdf:about="http://purl.org/olia/discourse/olia_discourse.owl#GeographicalVariant">
    <rdf:type rdf:resource="http://www.w3.org/2002/07/owl#Class"/>
  </rdf:Description>
  <rdf:Description rdf:about="http://purl.org/olia/discourse/olia_discourse.owl#GeographicalVariant">
    <rdfs:subClassOf rdf:resource="http://purl.org/olia/discourse/olia_discourse.owl#Possible"/>
  </rdf:Description>
  <rdf:Description rdf:about="http://purl.org/olia/discourse/olia_discourse.owl#GeographicalVariant">
    <rdfs:comment>
                            Description of a specific form used in a certain region as opposed to another form used in another region
                                (http://www.isocat.org/datcat/DC-1851)
                            </rdfs:comment>
  </rdf:Description>
  <rdf:Description rdf:about="http://purl.org/olia/discourse/olia_discourse.owl#GeographicalVariant">
    <rdfs:label>geographical variant</rdfs:label>
  </rdf:Description>
  <rdf:Description rdf:about="http://purl.org/olia/discourse/olia_discourse.owl#GeographicalVariant">
    <owl:versionInfo>http://www.isocat.org/datcat/DC-1851</owl:versionInfo>
  </rdf:Description>
  <rdf:Description rdf:about="http://purl.org/olia/discourse/olia_discourse.owl#Given">
    <rdf:type rdf:resource="http://www.w3.org/2002/07/owl#Class"/>
  </rdf:Description>
  <rdf:Description rdf:about="http://purl.org/olia/discourse/olia_discourse.owl#Given">
    <rdfs:subClassOf rdf:resource="http://purl.org/olia/discourse/olia_discourse.owl#InformationStatus"/>
  </rdf:Description>
  <rdf:Description rdf:about="http://purl.org/olia/discourse/olia_discourse.owl#Given">
    <rdfs:comment>A referent is given it is mentioned in the previous discourse, cf. Prince (1982) "textually evoked", Prince (1988) "discourse old".
For given referents, different hierarchies of cognitive states and corresponding referring expressions have been proposed (e.g. Levelt 1989, Ariel 1990, Gundel et al. 1993, Chafe 1996). As these conceptualizations are, however, often incompatible with each other, I only propose one subcategory here, i.e. referents that are particularly prominent (salient, active, in focus).</rdfs:comment>
  </rdf:Description>
  <rdf:Description rdf:about="http://purl.org/olia/discourse/olia_discourse.owl#Given">
    <rdfs:label xml:lang="en">given</rdfs:label>
  </rdf:Description>
  <rdf:Description rdf:about="http://purl.org/olia/discourse/olia_discourse.owl#Goal">
    <rdf:type rdf:resource="http://www.w3.org/2002/07/owl#Class"/>
  </rdf:Description>
  <rdf:Description rdf:about="http://purl.org/olia/discourse/olia_discourse.owl#Goal">
    <rdfs:subClassOf rdf:resource="http://purl.org/olia/discourse/olia_discourse.owl#Result"/>
  </rdf:Description>
  <rdf:Description rdf:about="http://purl.org/olia/discourse/olia_discourse.owl#Goal">
    <inverseOf rdf:resource="http://purl.org/olia/discourse/Enablement"/>
  </rdf:Description>
  <rdf:Description rdf:about="http://purl.org/olia/discourse/olia_discourse.owl#Goal">
    <rdfs:comment>ISO Purpose: Asymmetric relation in which Arg2 is the goal or purpose of Arg1.

Mononuclear relation that corresponds to ISO Purpose with argument goal ("purpose"). The goal is the satellite.

Cf. SemDok Purpose-n</rdfs:comment>
  </rdf:Description>
  <rdf:Description rdf:about="http://purl.org/olia/discourse/olia_discourse.owl#Goal">
    <rdfs:label>goal</rdfs:label>
  </rdf:Description>
  <rdf:Description rdf:about="http://purl.org/olia/discourse/olia_discourse.owl#Goal">
    <rdfs:label xml:lang="en">goal</rdfs:label>
  </rdf:Description>
  <rdf:Description rdf:about="http://purl.org/olia/discourse/olia_discourse.owl#Goal">
    <rdfs:label>purpose</rdfs:label>
  </rdf:Description>
  <rdf:Description rdf:about="http://purl.org/olia/discourse/olia_discourse.owl#Goal">
    <rdfs:label>purpose-n (SemDok)</rdfs:label>
  </rdf:Description>
  <rdf:Description rdf:about="http://purl.org/olia/discourse/olia_discourse.owl#Goal_HDRB">
    <rdf:type rdf:resource="http://www.w3.org/2002/07/owl#Class"/>
  </rdf:Description>
  <rdf:Description rdf:about="http://purl.org/olia/discourse/olia_discourse.owl#Goal_HDRB">
    <rdfs:subClassOf rdf:resource="http://purl.org/olia/discourse/olia_discourse.owl#Goal"/>
  </rdf:Description>
  <rdf:Description rdf:about="http://purl.org/olia/discourse/olia_discourse.owl#Goal_HDRB">
    <rdfs:comment>The “Goal” sense: Under the “Contingency” class, we have added a new type “Goal”, which applies to relations where the situation described in one of the arguments is the goal of the situation described in the other argument (which enables the achievement of the goal).
(Oza et al. 2009, also adopted by Tonelli et al. 2010)</rdfs:comment>
  </rdf:Description>
  <rdf:Description rdf:about="http://purl.org/olia/discourse/olia_discourse.owl#Goal_HDRB">
    <rdfs:label xml:lang="en">goal (HDRB)</rdfs:label>
  </rdf:Description>
  <rdf:Description rdf:about="http://purl.org/olia/discourse/olia_discourse.owl#HabitualCooccurrence">
    <rdf:type rdf:resource="http://www.w3.org/2002/07/owl#Class"/>
  </rdf:Description>
  <rdf:Description rdf:about="http://purl.org/olia/discourse/olia_discourse.owl#HabitualCooccurrence">
    <rdfs:subClassOf rdf:resource="http://purl.org/olia/discourse/olia_discourse.owl#Contigency"/>
  </rdf:Description>
  <rdf:Description rdf:about="http://purl.org/olia/discourse/olia_discourse.owl#HabitualCooccurrence">
    <rdfs:label xml:lang="en">habitual cooccurrence</rdfs:label>
  </rdf:Description>
  <rdf:Description rdf:about="http://purl.org/olia/discourse/olia_discourse.owl#Heading">
    <rdf:type rdf:resource="http://www.w3.org/2002/07/owl#Class"/>
  </rdf:Description>
  <rdf:Description rdf:about="http://purl.org/olia/discourse/olia_discourse.owl#Heading">
    <rdfs:subClassOf rdf:resource="http://purl.org/olia/olia-top.owl#TextStructuralUnit"/>
  </rdf:Description>
  <rdf:Description rdf:about="http://purl.org/olia/discourse/olia_discourse.owl#Heading">
    <rdfs:comment>The WSJ articles in our corpus did not include headings, so this schema was
not used in tagging the corpus. (Carlson and Marcu 2001)</rdfs:comment>
  </rdf:Description>
  <rdf:Description rdf:about="http://purl.org/olia/discourse/olia_discourse.owl#Heading">
    <rdfs:label xml:lang="en">heading</rdfs:label>
  </rdf:Description>
  <rdf:Description rdf:about="http://purl.org/olia/discourse/olia_discourse.owl#Headline">
    <rdf:type rdf:resource="http://www.w3.org/2002/07/owl#Class"/>
  </rdf:Description>
  <rdf:Description rdf:about="http://purl.org/olia/discourse/olia_discourse.owl#Headline">
    <rdfs:subClassOf rdf:resource="http://purl.org/olia/olia-top.owl#TextStructuralUnit"/>
  </rdf:Description>
  <rdf:Description rdf:about="http://purl.org/olia/discourse/olia_discourse.owl#Headline">
    <rdfs:comment>-HLN (headline)
— marks headlines and datelines. Note that headlines and datelines always constitute a unit of text that is structurally independent from the following sentence. 
(Bies et al. 1995)</rdfs:comment>
  </rdf:Description>
  <rdf:Description rdf:about="http://purl.org/olia/discourse/olia_discourse.owl#Headline">
    <owl:versionInfo>PTB bracketing guidelines, Bies et al. 1995</owl:versionInfo>
  </rdf:Description>
  <rdf:Description rdf:about="http://purl.org/olia/discourse/olia_discourse.owl#Holiday">
    <rdf:type rdf:resource="http://www.w3.org/2002/07/owl#Class"/>
  </rdf:Description>
  <rdf:Description rdf:about="http://purl.org/olia/discourse/olia_discourse.owl#Holiday">
    <rdfs:subClassOf rdf:resource="http://purl.org/olia/discourse/olia_discourse.owl#Time"/>
  </rdf:Description>
  <rdf:Description rdf:about="http://purl.org/olia/discourse/olia_discourse.owl#Holiday">
    <rdfs:comment xml:lang="en">introduced for nerd:Holiday, subclass of nerd:Time</rdfs:comment>
  </rdf:Description>
  <rdf:Description rdf:about="http://purl.org/olia/discourse/olia_discourse.owl#Honorific">
    <rdf:type rdf:resource="http://www.w3.org/2002/07/owl#Class"/>
  </rdf:Description>
  <rdf:Description rdf:about="http://purl.org/olia/discourse/olia_discourse.owl#Honorific">
    <rdfs:subClassOf rdf:resource="http://purl.org/olia/discourse/olia_discourse.owl#Possible"/>
  </rdf:Description>
  <rdf:Description rdf:about="http://purl.org/olia/discourse/olia_discourse.owl#Honorific">
    <rdfs:comment>
                            special form of language used when talking about those in positions of social situation
                                (http://www.isocat.org/datcat/DC-2347)
                            </rdfs:comment>
  </rdf:Description>
  <rdf:Description rdf:about="http://purl.org/olia/discourse/olia_discourse.owl#Honorific">
    <rdfs:label>honorific</rdfs:label>
  </rdf:Description>
  <rdf:Description rdf:about="http://purl.org/olia/discourse/olia_discourse.owl#Honorific">
    <owl:versionInfo>http://www.isocat.org/datcat/DC-2347</owl:versionInfo>
  </rdf:Description>
  <rdf:Description rdf:about="http://purl.org/olia/discourse/olia_discourse.owl#Hospital">
    <rdf:type rdf:resource="http://www.w3.org/2002/07/owl#Class"/>
  </rdf:Description>
  <rdf:Description rdf:about="http://purl.org/olia/discourse/olia_discourse.owl#Hospital">
    <rdfs:subClassOf rdf:resource="http://purl.org/olia/discourse/olia_discourse.owl#ArchitecturalFeature"/>
  </rdf:Description>
  <rdf:Description rdf:about="http://purl.org/olia/discourse/olia_discourse.owl#Hospital">
    <rdfs:comment xml:lang="en">for nerd:Hospital</rdfs:comment>
  </rdf:Description>
  <rdf:Description rdf:about="http://purl.org/olia/discourse/olia_discourse.owl#HypotacticDiscourseRelation">
    <rdf:type rdf:resource="http://www.w3.org/2002/07/owl#Class"/>
  </rdf:Description>
  <rdf:Description rdf:about="http://purl.org/olia/discourse/olia_discourse.owl#HypotacticDiscourseRelation">
    <rdfs:subClassOf rdf:resource="http://purl.org/olia/discourse/olia_discourse.owl#DiscourseStructuralPattern"/>
  </rdf:Description>
  <rdf:Description rdf:about="http://purl.org/olia/discourse/olia_discourse.owl#HypotacticDiscourseRelation">
    <owl:disjointWith rdf:resource="http://purl.org/olia/discourse/olia_discourse.owl#ParatacticDiscourseRelation"/>
  </rdf:Description>
  <rdf:Description rdf:about="http://purl.org/olia/discourse/olia_discourse.owl#HypotacticDiscourseRelation">
    <rdfs:comment>Subordinating or Mononuclear Relations (RST):
The most frequent structural pattern is that two spans of text (virtually always adjacent, but exceptions can be found) are related such that one of them has a specific role relative to the other. A paradigm case is a claim followed by evidence for the claim. RST posits an "Evidence" relation between the two spans. It also says that the claim is more essential to the text than the particular evidence, and this essentiality is represented by calling the claim span a nucleus and the evidence span a satellite.
(Mann and Taboada 2010)</rdfs:comment>
  </rdf:Description>
  <rdf:Description rdf:about="http://purl.org/olia/discourse/olia_discourse.owl#HypotacticDiscourseRelation">
    <rdfs:label>asymmetrical coherence relation</rdfs:label>
  </rdf:Description>
  <rdf:Description rdf:about="http://purl.org/olia/discourse/olia_discourse.owl#HypotacticDiscourseRelation">
    <rdfs:label xml:lang="en">hypotactic discourse relation</rdfs:label>
  </rdf:Description>
  <rdf:Description rdf:about="http://purl.org/olia/discourse/olia_discourse.owl#HypotacticDiscourseRelation">
    <rdfs:label>hypotaxis</rdfs:label>
  </rdf:Description>
  <rdf:Description rdf:about="http://purl.org/olia/discourse/olia_discourse.owl#HypotacticDiscourseRelation">
    <rdfs:label>mononuclear</rdfs:label>
  </rdf:Description>
  <rdf:Description rdf:about="http://purl.org/olia/discourse/olia_discourse.owl#HypotacticDiscourseRelation">
    <rdfs:label>mononuclear relation</rdfs:label>
  </rdf:Description>
  <rdf:Description rdf:about="http://purl.org/olia/discourse/olia_discourse.owl#HypotacticDiscourseRelation">
    <rdfs:label>subordination</rdfs:label>
  </rdf:Description>
  <rdf:Description rdf:about="http://purl.org/olia/discourse/olia_discourse.owl#HypotheticalCondition">
    <rdf:type rdf:resource="http://www.w3.org/2002/07/owl#Class"/>
  </rdf:Description>
  <rdf:Description rdf:about="http://purl.org/olia/discourse/olia_discourse.owl#HypotheticalCondition">
    <rdfs:subClassOf rdf:resource="http://purl.org/olia/discourse/olia_discourse.owl#FactualCondition"/>
  </rdf:Description>
  <rdf:Description rdf:about="http://purl.org/olia/discourse/olia_discourse.owl#HypotheticalCondition">
    <rdfs:comment>If Arg2 holds true, Arg1 is caused to hold at some instant in all possible futures. However, Arg1 can be true
in the future independently of Arg2. (Prasad et al. 2007)

In a HYPOTHETICAL relation, the satellite presents a situation that is not fac-
tual, but that one supposes or conjectures to be true. The nucleus presents the consequences that
would arise should the situation come true. (Carlson and Marcu 2001)</rdfs:comment>
  </rdf:Description>
  <rdf:Description rdf:about="http://purl.org/olia/discourse/olia_discourse.owl#HypotheticalCondition">
    <rdfs:label xml:lang="en">hypothetical condition</rdfs:label>
  </rdf:Description>
  <rdf:Description rdf:about="http://purl.org/olia/discourse/olia_discourse.owl#Identifier">
    <rdf:type rdf:resource="http://www.w3.org/2002/07/owl#Class"/>
  </rdf:Description>
  <rdf:Description rdf:about="http://purl.org/olia/discourse/olia_discourse.owl#Identifier">
    <rdfs:subClassOf rdf:resource="http://purl.org/olia/olia-top.owl#DiscourseEntity"/>
  </rdf:Description>
  <rdf:Description rdf:about="http://purl.org/olia/discourse/olia_discourse.owl#Identifier">
    <rdfs:comment>Designation of a unique entity or a singleton concept (CC)</rdfs:comment>
  </rdf:Description>
  <rdf:Description rdf:about="http://purl.org/olia/discourse/olia_discourse.owl#Identifier">
    <rdfs:label>identifier</rdfs:label>
  </rdf:Description>
  <rdf:Description rdf:about="http://purl.org/olia/discourse/olia_discourse.owl#Identifier">
    <owl:versionInfo>introduced as generalization over NamedEntity, Apellation and lexinfo:partNumber</owl:versionInfo>
  </rdf:Description>
  <rdf:Description rdf:about="http://purl.org/olia/discourse/olia_discourse.owl#ImplicitConnective">
    <rdf:type rdf:resource="http://www.w3.org/2002/07/owl#Class"/>
  </rdf:Description>
  <rdf:Description rdf:about="http://purl.org/olia/discourse/olia_discourse.owl#ImplicitConnective">
    <rdfs:subClassOf rdf:resource="http://purl.org/olia/discourse/olia_discourse.owl#ImplicitRelation"/>
  </rdf:Description>
  <rdf:Description rdf:about="http://purl.org/olia/discourse/olia_discourse.owl#ImplicitConnective">
    <rdfs:comment>Implicit discourse connectives (...) are inserted between paragraph-internal adjacent sentence pairs not related explicitly by any of the syntactically-defined set of Explicit connectives. (...) the reader must attempt to infer a discourse relation between the adjacent sentences, and “annotation” consists of inserting a connective expression that best conveys the inferred relation. Connectives inserted in this way to express inferred relations are called Implicit connectives. Multiple discourse relations (Webber et al., 1999) can also be inferred, and are annotated by inserting multiple Implicit connectives.

The goal of annotating Implicit connectives in the PDTB is to capture relations between abstract
objects that are not realized explicitly in the text (by one of a set of the lexically-defined Explicit
connectives) and are left to be inferred by the reader.
(Prasad et al. 2007, PDTB)</rdfs:comment>
  </rdf:Description>
  <rdf:Description rdf:about="http://purl.org/olia/discourse/olia_discourse.owl#ImplicitConnective">
    <rdfs:label xml:lang="en">implicit connective</rdfs:label>
  </rdf:Description>
  <rdf:Description rdf:about="http://purl.org/olia/discourse/olia_discourse.owl#ImplicitRelation">
    <rdf:type rdf:resource="http://www.w3.org/2002/07/owl#Class"/>
  </rdf:Description>
  <rdf:Description rdf:about="http://purl.org/olia/discourse/olia_discourse.owl#ImplicitRelation">
    <rdfs:subClassOf rdf:resource="http://purl.org/olia/discourse/olia_discourse.owl#RelationCue"/>
  </rdf:Description>
  <rdf:Description rdf:about="http://purl.org/olia/discourse/olia_discourse.owl#ImplicitRelation">
    <rdfs:comment>In PDTB: Two kinds of implicit relations are distinguished: ImplicitConnectives (where a connective and an associated relation can be inferred) and EntityRelations (where neither connective nor relation can be inferred but referential coherence is observed). While the former is actually annotated in PDTB, the latter is not, hence no subclass here.

PDTB Entity Relation: no discourse relation can be inferred and where the second sentence only serves to provide some further description of an entity in the first sentence (akin to entity-based coherence (Knott et al., 2001))

Entity-based coherence captures cases where the implicit relation between adjacent sentences is not between their AO
interpretations, but is rather a form of entity-based coherence (Knott et al., 2001) in which the same
entity is realized in both sentences</rdfs:comment>
  </rdf:Description>
  <rdf:Description rdf:about="http://purl.org/olia/discourse/olia_discourse.owl#ImplicitRelation">
    <rdfs:comment>PDTB Entity Relation: no discourse relation can be inferred and where the second sentence only serves to provide some further description of an entity in the first sentence (akin to entity-based coherence (Knott et al., 2001))

Entity-based coherence captures cases where the implicit relation between adjacent sentences is not between their AO
interpretations, but is rather a form of entity-based coherence (Knott et al., 2001) in which the same
entity is realized in both sentences</rdfs:comment>
  </rdf:Description>
  <rdf:Description rdf:about="http://purl.org/olia/discourse/olia_discourse.owl#ImplicitRelation">
    <rdfs:label xml:lang="en">implicit relation</rdfs:label>
  </rdf:Description>
  <rdf:Description rdf:about="http://purl.org/olia/discourse/olia_discourse.owl#ImplicitlyAssertedCondition_PDTB">
    <rdf:type rdf:resource="http://www.w3.org/2002/07/owl#Class"/>
  </rdf:Description>
  <rdf:Description rdf:about="http://purl.org/olia/discourse/olia_discourse.owl#ImplicitlyAssertedCondition_PDTB">
    <rdfs:subClassOf rdf:resource="http://purl.org/olia/discourse/olia_discourse.owl#PragmaticCondition"/>
  </rdf:Description>
  <rdf:Description rdf:about="http://purl.org/olia/discourse/olia_discourse.owl#ImplicitlyAssertedCondition_PDTB">
    <rdfs:comment>Special rhetorical uses of if-constructions when the intepretation of the conditional construction is an implicit assertion. (Prasad et al. 2007)</rdfs:comment>
  </rdf:Description>
  <rdf:Description rdf:about="http://purl.org/olia/discourse/olia_discourse.owl#ImplicitlyAssertedCondition_PDTB">
    <rdfs:label>implicit assertion</rdfs:label>
  </rdf:Description>
  <rdf:Description rdf:about="http://purl.org/olia/discourse/olia_discourse.owl#ImplicitlyAssertedCondition_PDTB">
    <rdfs:label xml:lang="en">implicitly asserted condition (PDTB)</rdfs:label>
  </rdf:Description>
  <rdf:Description rdf:about="http://purl.org/olia/discourse/olia_discourse.owl#Impossible">
    <rdf:type rdf:resource="http://www.w3.org/2002/07/owl#Class"/>
  </rdf:Description>
  <rdf:Description rdf:about="http://purl.org/olia/discourse/olia_discourse.owl#Impossible">
    <rdfs:subClassOf rdf:resource="http://purl.org/olia/olia-top.owl#UsageAndFrequencyFeature"/>
  </rdf:Description>
  <rdf:Description rdf:about="http://purl.org/olia/discourse/olia_discourse.owl#Impossible">
    <rdfs:comment>to denote something that cannot be considered as being correct in a given language</rdfs:comment>
  </rdf:Description>
  <rdf:Description rdf:about="http://purl.org/olia/discourse/olia_discourse.owl#Impossible">
    <rdfs:isDefinedBy>http://www.isocat.org/datcat/DC-1866</rdfs:isDefinedBy>
  </rdf:Description>
  <rdf:Description rdf:about="http://purl.org/olia/discourse/olia_discourse.owl#InHouseRegister">
    <rdf:type rdf:resource="http://www.w3.org/2002/07/owl#Class"/>
  </rdf:Description>
  <rdf:Description rdf:about="http://purl.org/olia/discourse/olia_discourse.owl#InHouseRegister">
    <rdfs:subClassOf rdf:resource="http://purl.org/olia/olia-top.owl#RegisterFeature"/>
  </rdf:Description>
  <rdf:Description rdf:about="http://purl.org/olia/discourse/olia_discourse.owl#InHouseRegister">
    <rdfs:comment>
                            Register of terms that are company-specific and not readily recognized outside this environment.
                                (ISO12620; http://www.isocat.org/datcat/DC-1993)
                            </rdfs:comment>
  </rdf:Description>
  <rdf:Description rdf:about="http://purl.org/olia/discourse/olia_discourse.owl#InHouseRegister">
    <rdfs:label>in house register</rdfs:label>
  </rdf:Description>
  <rdf:Description rdf:about="http://purl.org/olia/discourse/olia_discourse.owl#InHouseRegister">
    <owl:versionInfo>http://www.isocat.org/datcat/DC-1993</owl:versionInfo>
  </rdf:Description>
  <rdf:Description rdf:about="http://purl.org/olia/discourse/olia_discourse.owl#InHouseRegister">
    <owl:versionInfo>subClassOf register (dcif:conceptualDomain)</owl:versionInfo>
  </rdf:Description>
  <rdf:Description rdf:about="http://purl.org/olia/discourse/olia_discourse.owl#Indefinite">
    <rdf:type rdf:resource="http://www.w3.org/2002/07/owl#Class"/>
  </rdf:Description>
  <rdf:Description rdf:about="http://purl.org/olia/discourse/olia_discourse.owl#Indefinite">
    <rdfs:subClassOf rdf:resource="http://purl.org/olia/discourse/olia_discourse.owl#Definiteness"/>
  </rdf:Description>
  <rdf:Description rdf:about="http://purl.org/olia/discourse/olia_discourse.owl#Indefinite">
    <rdfs:label xml:lang="en">indefinite</rdfs:label>
  </rdf:Description>
  <rdf:Description rdf:about="http://purl.org/olia/discourse/olia_discourse.owl#IndeterminateAttribution">
    <rdf:type rdf:resource="http://www.w3.org/2002/07/owl#Class"/>
  </rdf:Description>
  <rdf:Description rdf:about="http://purl.org/olia/discourse/olia_discourse.owl#IndeterminateAttribution">
    <rdfs:subClassOf rdf:resource="http://purl.org/olia/discourse/olia_discourse.owl#Attribution"/>
  </rdf:Description>
  <rdf:Description rdf:about="http://purl.org/olia/discourse/olia_discourse.owl#IndeterminateAttribution">
    <rdfs:comment>Classification of Attribute relations with respect to their "determinacy", which signals a context that cancels what would otherwise be an entailment of attribution.
The determinacy feature captures the fact that the attribution over a relation or argument can itself be cancelled in particular contexts, such as within negated, conditional, and infinitive contexts.

The attribution over a relation or argument can itself be cancelled in particular contexts, such as within negated, conditional, and infinitive contexts. Such indeterminacy is indicated by the value “Indet”. (Prasad et al. 2007)</rdfs:comment>
  </rdf:Description>
  <rdf:Description rdf:about="http://purl.org/olia/discourse/olia_discourse.owl#IndeterminateAttribution">
    <rdfs:label xml:lang="en">indeterminate attribution</rdfs:label>
  </rdf:Description>
  <rdf:Description rdf:about="http://purl.org/olia/discourse/olia_discourse.owl#Inferrable">
    <rdf:type rdf:resource="http://www.w3.org/2002/07/owl#Class"/>
  </rdf:Description>
  <rdf:Description rdf:about="http://purl.org/olia/discourse/olia_discourse.owl#Inferrable">
    <rdfs:subClassOf rdf:resource="http://purl.org/olia/discourse/olia_discourse.owl#Accessible"/>
  </rdf:Description>
  <rdf:Description rdf:about="http://purl.org/olia/discourse/olia_discourse.owl#Inferrable">
    <rdfs:comment>A referent is (textually) inferrable if the hearer constructs a mental representation of the referent on the basis of the earlier realization of another, related referent. Syn. "bridging" (Clark &amp; Clark 1976)</rdfs:comment>
  </rdf:Description>
  <rdf:Description rdf:about="http://purl.org/olia/discourse/olia_discourse.owl#Inferrable">
    <rdfs:label xml:lang="en">inferrable</rdfs:label>
  </rdf:Description>
  <rdf:Description rdf:about="http://purl.org/olia/discourse/olia_discourse.owl#InformationStatus">
    <rdf:type rdf:resource="http://www.w3.org/2002/07/owl#Class"/>
  </rdf:Description>
  <rdf:Description rdf:about="http://purl.org/olia/discourse/olia_discourse.owl#InformationStatus">
    <rdfs:subClassOf rdf:resource="http://purl.org/olia/olia-top.owl#PragmaticFeature"/>
  </rdf:Description>
  <rdf:Description rdf:about="http://purl.org/olia/discourse/olia_discourse.owl#InformationStatus">
    <rdfs:comment>Givenness
A feature X of an expression α is a Givenness feature iff X indicates
whether the denotation of α is present in the CG or not, and/or indicates the degree to which it is present in the immediate CG.
(Féry et al. 2007)</rdfs:comment>
  </rdf:Description>
  <rdf:Description rdf:about="http://purl.org/olia/discourse/olia_discourse.owl#InformationStatus">
    <rdfs:comment>A property of discourse referents, hence referring expressions. This hierarchy is organized following the criteria of hearer new/hearer old and discourse new/discourse old of Prince (1988), the terminology is inspired by Lambrecht (1994) and Chafe (1996).</rdfs:comment>
  </rdf:Description>
  <rdf:Description rdf:about="http://purl.org/olia/discourse/olia_discourse.owl#InformationStatus">
    <rdfs:label xml:lang="en">information status</rdfs:label>
  </rdf:Description>
  <rdf:Description rdf:about="http://purl.org/olia/discourse/olia_discourse.owl#InfrequentlyUsed">
    <rdf:type rdf:resource="http://www.w3.org/2002/07/owl#Class"/>
  </rdf:Description>
  <rdf:Description rdf:about="http://purl.org/olia/discourse/olia_discourse.owl#InfrequentlyUsed">
    <rdfs:subClassOf rdf:resource="http://purl.org/olia/discourse/olia_discourse.owl#Possible"/>
  </rdf:Description>
  <rdf:Description rdf:about="http://purl.org/olia/discourse/olia_discourse.owl#InfrequentlyUsed">
    <rdfs:comment>
                            Said of a term that does not appear frequently.
                                (ISO12620; http://www.isocat.org/datcat/DC-1985)
                            </rdfs:comment>
  </rdf:Description>
  <rdf:Description rdf:about="http://purl.org/olia/discourse/olia_discourse.owl#InfrequentlyUsed">
    <rdfs:label>infrequently used</rdfs:label>
  </rdf:Description>
  <rdf:Description rdf:about="http://purl.org/olia/discourse/olia_discourse.owl#InfrequentlyUsed">
    <owl:versionInfo>http://www.isocat.org/datcat/DC-1985</owl:versionInfo>
  </rdf:Description>
  <rdf:Description rdf:about="http://purl.org/olia/discourse/olia_discourse.owl#InfrequentlyUsed">
    <owl:versionInfo>subClassOf frequency (dcif:conceptualDomain)</owl:versionInfo>
  </rdf:Description>
  <rdf:Description rdf:about="http://purl.org/olia/discourse/olia_discourse.owl#InheritedAttributionSource">
    <rdf:type rdf:resource="http://www.w3.org/2002/07/owl#Class"/>
  </rdf:Description>
  <rdf:Description rdf:about="http://purl.org/olia/discourse/olia_discourse.owl#InheritedAttributionSource">
    <rdfs:subClassOf rdf:resource="http://purl.org/olia/discourse/olia_discourse.owl#AttributionSource"/>
  </rdf:Description>
  <rdf:Description rdf:about="http://purl.org/olia/discourse/olia_discourse.owl#InheritedAttributionSource">
    <rdfs:comment>Since attribution can have scope over an entire relation, arguments can be annotated with a fourth value “Inh”, to indicate that their source value is inherited from the relation. (Prasad et al. 2007)</rdfs:comment>
  </rdf:Description>
  <rdf:Description rdf:about="http://purl.org/olia/discourse/olia_discourse.owl#InheritedAttributionSource">
    <rdfs:label xml:lang="en">inherited attribution source</rdfs:label>
  </rdf:Description>
  <rdf:Description rdf:about="http://purl.org/olia/discourse/olia_discourse.owl#Insect">
    <rdf:type rdf:resource="http://www.w3.org/2002/07/owl#Class"/>
  </rdf:Description>
  <rdf:Description rdf:about="http://purl.org/olia/discourse/olia_discourse.owl#Insect">
    <rdfs:subClassOf rdf:resource="http://purl.org/olia/discourse/olia_discourse.owl#Animal"/>
  </rdf:Description>
  <rdf:Description rdf:about="http://purl.org/olia/discourse/olia_discourse.owl#Insect">
    <rdfs:comment xml:lang="en">for nerd:Insect and extractiv:INSECT</rdfs:comment>
  </rdf:Description>
  <rdf:Description rdf:about="http://purl.org/olia/discourse/olia_discourse.owl#Instantiation">
    <rdf:type rdf:resource="http://www.w3.org/2002/07/owl#Class"/>
  </rdf:Description>
  <rdf:Description rdf:about="http://purl.org/olia/discourse/olia_discourse.owl#Instantiation">
    <rdfs:subClassOf rdf:resource="http://purl.org/olia/discourse/olia_discourse.owl#Expansion"/>
  </rdf:Description>
  <rdf:Description rdf:about="http://purl.org/olia/discourse/olia_discourse.owl#Instantiation">
    <rdfs:comment>Arg1 evokes a set and Arg2 describes it in further detail. Typical connectives often tagged as “Instantiation” are for example,
for instance and specifically. (Prasad et al. 2007)

ISO DR-Core Excemplification, argument Instance</rdfs:comment>
  </rdf:Description>
  <rdf:Description rdf:about="http://purl.org/olia/discourse/olia_discourse.owl#Instantiation">
    <rdfs:label>exemplification</rdfs:label>
  </rdf:Description>
  <rdf:Description rdf:about="http://purl.org/olia/discourse/olia_discourse.owl#Instantiation">
    <rdfs:label>instance</rdfs:label>
  </rdf:Description>
  <rdf:Description rdf:about="http://purl.org/olia/discourse/olia_discourse.owl#Instantiation">
    <rdfs:label>instantiation</rdfs:label>
  </rdf:Description>
  <rdf:Description rdf:about="http://purl.org/olia/discourse/olia_discourse.owl#Instantiation">
    <rdfs:label xml:lang="en">instantiation</rdfs:label>
  </rdf:Description>
  <rdf:Description rdf:about="http://purl.org/olia/discourse/olia_discourse.owl#Internationalism">
    <rdf:type rdf:resource="http://www.w3.org/2002/07/owl#Class"/>
  </rdf:Description>
  <rdf:Description rdf:about="http://purl.org/olia/discourse/olia_discourse.owl#Internationalism">
    <rdfs:subClassOf rdf:resource="http://purl.org/olia/olia-top.owl#RegisterFeature"/>
  </rdf:Description>
  <rdf:Description rdf:about="http://purl.org/olia/discourse/olia_discourse.owl#Internationalism">
    <rdfs:comment>A term that has the same or nearly identical orthographic or phonemic form in many languages. (Sue Ellen Wright, http://www.isocat.org/datcat/DC-320)</rdfs:comment>
  </rdf:Description>
  <rdf:Description rdf:about="http://purl.org/olia/discourse/olia_discourse.owl#Internationalism">
    <rdfs:label>internationalism</rdfs:label>
  </rdf:Description>
  <rdf:Description rdf:about="http://purl.org/olia/discourse/olia_discourse.owl#Internationalism">
    <owl:versionInfo>http://www.isocat.org/datcat/DC-320, TODO: check treatment as register feature</owl:versionInfo>
  </rdf:Description>
  <rdf:Description rdf:about="http://purl.org/olia/discourse/olia_discourse.owl#Interpretation">
    <rdf:type rdf:resource="http://www.w3.org/2002/07/owl#Class"/>
  </rdf:Description>
  <rdf:Description rdf:about="http://purl.org/olia/discourse/olia_discourse.owl#Interpretation">
    <rdfs:subClassOf rdf:resource="http://purl.org/olia/discourse/olia_discourse.owl#Assessment"/>
  </rdf:Description>
  <rdf:Description rdf:about="http://purl.org/olia/discourse/olia_discourse.owl#Interpretation">
    <rdfs:comment>In interpretation relations, one side of the relation gives a different perspective on the situation presented in the other side. It is subjective, presenting the personal opinion of the writer or of a third party. An interpretation can be: 1) an explanation of what is not immediately plain or explicit; 2) an explanation of actions, events, or statements by pointing out or suggesting inner relationships, motives, or by relating particulars to general principles; or 3) an understanding or appreciation of a situation in light of individual belief, judgment, interest, or circumstance.
(Carlson and Marcu 2001)

cf. SemDok Interpretation</rdfs:comment>
  </rdf:Description>
  <rdf:Description rdf:about="http://purl.org/olia/discourse/olia_discourse.owl#Interpretation">
    <rdfs:label xml:lang="en">interpretation</rdfs:label>
  </rdf:Description>
  <rdf:Description rdf:about="http://purl.org/olia/discourse/olia_discourse.owl#Interpretation_RST">
    <rdf:type rdf:resource="http://www.w3.org/2002/07/owl#Class"/>
  </rdf:Description>
  <rdf:Description rdf:about="http://purl.org/olia/discourse/olia_discourse.owl#Interpretation_RST">
    <rdfs:subClassOf rdf:resource="http://purl.org/olia/discourse/olia_discourse.owl#Interpretation"/>
  </rdf:Description>
  <rdf:Description rdf:about="http://purl.org/olia/discourse/olia_discourse.owl#Interpretation_RST">
    <rdfs:label xml:lang="en">interpretation (RST)</rdfs:label>
  </rdf:Description>
  <rdf:Description rdf:about="http://purl.org/olia/discourse/olia_discourse.owl#Interpretation_RST">
    <owl:deprecated rdf:datatype="http://www.w3.org/2001/XMLSchema#boolean">true</owl:deprecated>
  </rdf:Description>
  <rdf:Description rdf:about="http://purl.org/olia/discourse/olia_discourse.owl#InvertedSequence">
    <rdf:type rdf:resource="http://www.w3.org/2002/07/owl#Class"/>
  </rdf:Description>
  <rdf:Description rdf:nodeID="genid34">
    <rdf:type rdf:resource="http://www.w3.org/2002/07/owl#Class"/>
  </rdf:Description>
  <rdf:Description rdf:nodeID="genid35">
    <rdf:first rdf:resource="http://purl.org/olia/discourse/olia_discourse.owl#ListSequence"/>
  </rdf:Description>
  <rdf:Description rdf:nodeID="genid36">
    <rdf:first rdf:resource="http://purl.org/olia/discourse/olia_discourse.owl#SuccessionRelation"/>
  </rdf:Description>
  <rdf:Description rdf:nodeID="genid35">
    <rdf:rest rdf:nodeID="genid36"/>
  </rdf:Description>
  <rdf:Description rdf:nodeID="genid36">
    <rdf:rest rdf:resource="http://www.w3.org/1999/02/22-rdf-syntax-ns#nil"/>
  </rdf:Description>
  <rdf:Description rdf:nodeID="genid34">
    <owl:intersectionOf rdf:nodeID="genid35"/>
  </rdf:Description>
  <rdf:Description rdf:about="http://purl.org/olia/discourse/olia_discourse.owl#InvertedSequence">
    <owl:equivalentClass rdf:nodeID="genid34"/>
  </rdf:Description>
  <rdf:Description rdf:about="http://purl.org/olia/discourse/olia_discourse.owl#InvertedSequence">
    <rdfs:comment>An INVERTED-SEQUENCE is a multinuclear list of events presented in reverse
chronological order.
(Carlson and Marcu 2001)</rdfs:comment>
  </rdf:Description>
  <rdf:Description rdf:about="http://purl.org/olia/discourse/olia_discourse.owl#InvertedSequence">
    <rdfs:label xml:lang="en">inverted sequence</rdfs:label>
  </rdf:Description>
  <rdf:Description rdf:about="http://purl.org/olia/discourse/olia_discourse.owl#IronicRegister">
    <rdf:type rdf:resource="http://www.w3.org/2002/07/owl#Class"/>
  </rdf:Description>
  <rdf:Description rdf:about="http://purl.org/olia/discourse/olia_discourse.owl#IronicRegister">
    <rdfs:subClassOf rdf:resource="http://purl.org/olia/olia-top.owl#RegisterFeature"/>
  </rdf:Description>
  <rdf:Description rdf:about="http://purl.org/olia/discourse/olia_discourse.owl#IronicRegister">
    <rdfs:comment>
                            Register for irony.
                                (12620; http://www.isocat.org/datcat/DC-1994)
                            </rdfs:comment>
  </rdf:Description>
  <rdf:Description rdf:about="http://purl.org/olia/discourse/olia_discourse.owl#IronicRegister">
    <rdfs:label>ironic register</rdfs:label>
  </rdf:Description>
  <rdf:Description rdf:about="http://purl.org/olia/discourse/olia_discourse.owl#IronicRegister">
    <owl:versionInfo>http://www.isocat.org/datcat/DC-1994</owl:versionInfo>
  </rdf:Description>
  <rdf:Description rdf:about="http://purl.org/olia/discourse/olia_discourse.owl#IronicRegister">
    <owl:versionInfo>subClassOf register (dcif:conceptualDomain)</owl:versionInfo>
  </rdf:Description>
  <rdf:Description rdf:about="http://purl.org/olia/discourse/olia_discourse.owl#Island">
    <rdf:type rdf:resource="http://www.w3.org/2002/07/owl#Class"/>
  </rdf:Description>
  <rdf:Description rdf:about="http://purl.org/olia/discourse/olia_discourse.owl#Island">
    <rdfs:subClassOf rdf:resource="http://purl.org/olia/discourse/olia_discourse.owl#GeographicalFeature"/>
  </rdf:Description>
  <rdf:Description rdf:about="http://purl.org/olia/discourse/olia_discourse.owl#Island">
    <rdfs:comment xml:lang="en">for nerd:Island</rdfs:comment>
  </rdf:Description>
  <rdf:Description rdf:about="http://purl.org/olia/discourse/olia_discourse.owl#Joint">
    <rdf:type rdf:resource="http://www.w3.org/2002/07/owl#Class"/>
  </rdf:Description>
  <rdf:Description rdf:about="http://purl.org/olia/discourse/olia_discourse.owl#Joint">
    <rdfs:subClassOf rdf:resource="http://purl.org/olia/discourse/olia_discourse.owl#TextualOrganizationalRelation"/>
  </rdf:Description>
  <rdf:Description rdf:about="http://purl.org/olia/discourse/olia_discourse.owl#Joint">
    <rdfs:comment>generalization over SemDok Joint and RST Joint. As SemDok does not provide definitions, it is unclear whether these are equivalent,</rdfs:comment>
  </rdf:Description>
  <rdf:Description rdf:about="http://purl.org/olia/discourse/olia_discourse.owl#Joint">
    <rdfs:label>joint</rdfs:label>
  </rdf:Description>
  <rdf:Description rdf:about="http://purl.org/olia/discourse/olia_discourse.owl#Joint">
    <rdfs:label xml:lang="en">joint</rdfs:label>
  </rdf:Description>
  <rdf:Description rdf:about="http://purl.org/olia/discourse/olia_discourse.owl#Joint_RST">
    <rdf:type rdf:resource="http://www.w3.org/2002/07/owl#Class"/>
  </rdf:Description>
  <rdf:Description rdf:about="http://purl.org/olia/discourse/olia_discourse.owl#Joint_RST">
    <rdfs:subClassOf rdf:resource="http://purl.org/olia/discourse/olia_discourse.owl#Joint"/>
  </rdf:Description>
  <rdf:Description rdf:about="http://purl.org/olia/discourse/olia_discourse.owl#Joint_RST">
    <rdfs:comment>Joint represents the lack of a rhetorical relation between the nuclei. (Mann and Taboada 2010)</rdfs:comment>
  </rdf:Description>
  <rdf:Description rdf:about="http://purl.org/olia/discourse/olia_discourse.owl#Joint_RST">
    <rdfs:label>joint (RST)</rdfs:label>
  </rdf:Description>
  <rdf:Description rdf:about="http://purl.org/olia/discourse/olia_discourse.owl#Joint_RST">
    <rdfs:label xml:lang="en">joint (RST)</rdfs:label>
  </rdf:Description>
  <rdf:Description rdf:about="http://purl.org/olia/discourse/olia_discourse.owl#Justification">
    <rdf:type rdf:resource="http://www.w3.org/2002/07/owl#Class"/>
  </rdf:Description>
  <rdf:Description rdf:about="http://purl.org/olia/discourse/olia_discourse.owl#Justification">
    <rdfs:subClassOf rdf:resource="http://purl.org/olia/discourse/olia_discourse.owl#Support"/>
  </rdf:Description>
  <rdf:Description rdf:about="http://purl.org/olia/discourse/olia_discourse.owl#Justification">
    <rdfs:comment>Epistemic uses of the connective “because” are labelled as “Pragmatic cause:justification”. (Prasad et al. 2007)
RST "Justify": R's comprehending S increases R's readiness to accept W's right to present N (Mann and Taboada 2010)

Cf. SemDok Justify, subclass of Support.</rdfs:comment>
  </rdf:Description>
  <rdf:Description rdf:about="http://purl.org/olia/discourse/olia_discourse.owl#Justification">
    <rdfs:label>justification</rdfs:label>
  </rdf:Description>
  <rdf:Description rdf:about="http://purl.org/olia/discourse/olia_discourse.owl#Justification">
    <rdfs:label xml:lang="en">justification</rdfs:label>
  </rdf:Description>
  <rdf:Description rdf:about="http://purl.org/olia/discourse/olia_discourse.owl#Justification">
    <rdfs:label>justify</rdfs:label>
  </rdf:Description>
  <rdf:Description rdf:about="http://purl.org/olia/discourse/olia_discourse.owl#Juxtaposition_PDTB">
    <rdf:type rdf:resource="http://www.w3.org/2002/07/owl#Class"/>
  </rdf:Description>
  <rdf:Description rdf:about="http://purl.org/olia/discourse/olia_discourse.owl#Juxtaposition_PDTB">
    <rdfs:subClassOf rdf:resource="http://purl.org/olia/discourse/olia_discourse.owl#SemanticContrast_PDTB"/>
  </rdf:Description>
  <rdf:Description rdf:about="http://purl.org/olia/discourse/olia_discourse.owl#Juxtaposition_PDTB">
    <rdfs:comment>The values assigned to some shared property are taken to be alternatives (e.g., John paid $5
but Mary paid $10.)
(Prasad et al. 2007)</rdfs:comment>
  </rdf:Description>
  <rdf:Description rdf:about="http://purl.org/olia/discourse/olia_discourse.owl#Juxtaposition_PDTB">
    <rdfs:label xml:lang="en">juxtaposition (PDTB)</rdfs:label>
  </rdf:Description>
  <rdf:Description rdf:about="http://purl.org/olia/discourse/olia_discourse.owl#Lake">
    <rdf:type rdf:resource="http://www.w3.org/2002/07/owl#Class"/>
  </rdf:Description>
  <rdf:Description rdf:about="http://purl.org/olia/discourse/olia_discourse.owl#Lake">
    <rdfs:subClassOf rdf:resource="http://purl.org/olia/discourse/olia_discourse.owl#GeographicalFeature"/>
  </rdf:Description>
  <rdf:Description rdf:about="http://purl.org/olia/discourse/olia_discourse.owl#Lake">
    <rdfs:comment xml:lang="en">for nerd:Lake</rdfs:comment>
  </rdf:Description>
  <rdf:Description rdf:about="http://purl.org/olia/discourse/olia_discourse.owl#LegalRegister">
    <rdf:type rdf:resource="http://www.w3.org/2002/07/owl#Class"/>
  </rdf:Description>
  <rdf:Description rdf:about="http://purl.org/olia/discourse/olia_discourse.owl#LegalRegister">
    <rdfs:subClassOf rdf:resource="http://purl.org/olia/olia-top.owl#RegisterFeature"/>
  </rdf:Description>
  <rdf:Description rdf:about="http://purl.org/olia/discourse/olia_discourse.owl#LegalRegister">
    <rdfs:comment>Used for terms that are legally defined and used in legally binding documents.
                                (cf. http://www.isocat.org/datcat/DC-380)
                            </rdfs:comment>
  </rdf:Description>
  <rdf:Description rdf:about="http://purl.org/olia/discourse/olia_discourse.owl#LegalRegister">
    <rdfs:label>legal register</rdfs:label>
  </rdf:Description>
  <rdf:Description rdf:about="http://purl.org/olia/discourse/olia_discourse.owl#LegalRegister">
    <owl:versionInfo>http://www.isocat.org/datcat/DC-380, but rendered as a feature of individual terms, there</owl:versionInfo>
  </rdf:Description>
  <rdf:Description rdf:about="http://purl.org/olia/discourse/olia_discourse.owl#Legislature">
    <rdf:type rdf:resource="http://www.w3.org/2002/07/owl#Class"/>
  </rdf:Description>
  <rdf:Description rdf:about="http://purl.org/olia/discourse/olia_discourse.owl#Legislature">
    <rdfs:subClassOf rdf:resource="http://purl.org/olia/discourse/olia_discourse.owl#PoliticalOrganization"/>
  </rdf:Description>
  <rdf:Description rdf:about="http://purl.org/olia/discourse/olia_discourse.owl#Legislature">
    <rdfs:comment xml:lang="en">for nerd:Legislature</rdfs:comment>
  </rdf:Description>
  <rdf:Description rdf:about="http://purl.org/olia/discourse/olia_discourse.owl#LexicalUnit">
    <rdf:type rdf:resource="http://www.w3.org/2002/07/owl#Class"/>
  </rdf:Description>
  <rdf:Description rdf:about="http://purl.org/olia/discourse/olia_discourse.owl#LexicalUnit">
    <rdfs:subClassOf rdf:resource="http://purl.org/olia/olia-top.owl#LinguisticConcept"/>
  </rdf:Description>
  <rdf:Description rdf:about="http://purl.org/olia/discourse/olia_discourse.owl#Lighthouse">
    <rdf:type rdf:resource="http://www.w3.org/2002/07/owl#Class"/>
  </rdf:Description>
  <rdf:Description rdf:about="http://purl.org/olia/discourse/olia_discourse.owl#Lighthouse">
    <rdfs:subClassOf rdf:resource="http://purl.org/olia/discourse/olia_discourse.owl#ArchitecturalFeature"/>
  </rdf:Description>
  <rdf:Description rdf:about="http://purl.org/olia/discourse/olia_discourse.owl#Lighthouse">
    <rdfs:comment xml:lang="en">for nerd:Lighthouse</rdfs:comment>
  </rdf:Description>
  <rdf:Description rdf:about="http://purl.org/olia/discourse/olia_discourse.owl#List">
    <rdf:type rdf:resource="http://www.w3.org/2002/07/owl#Class"/>
  </rdf:Description>
  <rdf:Description rdf:about="http://purl.org/olia/discourse/olia_discourse.owl#List">
    <rdfs:subClassOf rdf:resource="http://purl.org/olia/discourse/olia_discourse.owl#Conjunction"/>
  </rdf:Description>
  <rdf:Description rdf:about="http://purl.org/olia/discourse/olia_discourse.owl#List">
    <rdfs:subClassOf rdf:resource="http://purl.org/olia/discourse/olia_discourse.owl#ListSequence"/>
  </rdf:Description>
  <rdf:Description rdf:about="http://purl.org/olia/discourse/olia_discourse.owl#List">
    <rdfs:subClassOf rdf:resource="http://purl.org/olia/discourse/olia_discourse.owl#PresentationalRelation"/>
  </rdf:Description>
  <rdf:Description rdf:about="http://purl.org/olia/discourse/olia_discourse.owl#List">
    <rdfs:comment>An item comparable to others linked to it by the List relation. (Mann and Taboada 2010)

Arg1 and Arg2 are members of a list, defined in the prior discourse. “List” does not require the situations specified in Arg1 and Arg2 to be directly related. (Prasad et al. 2007)

A LIST is a multinuclear relation whose elements can be listed, but which are not in a comparison, contrast or other, stronger type of multinuclear relation. A LIST relation usually exhibits some sort of parallel structure between the units involved in the relation. At lower levels of the discourse structure, such as between clauses or sentences, a LIST relation is often selected when there is some sort of parallel syntactic or semantic structure between the units, such as in the examples below. At higher levels of the discourse structure, the relation may be found when there are paragraphs of items enumerated in a similar fashion.
(Carlson and Marcu 2001)

Axiomatization follows SemDok. In particular, we assume that Lists do not follow any natural order, their order thus reflects an (implicit) purpose of the speaker. They are thus interpersonal (presentational) relations.

Note that we skipped the SemDok subclass List-dm_other, as its definition is unclear.</rdfs:comment>
  </rdf:Description>
  <rdf:Description rdf:about="http://purl.org/olia/discourse/olia_discourse.owl#List">
    <rdfs:label xml:lang="en">list</rdfs:label>
  </rdf:Description>
  <rdf:Description rdf:about="http://purl.org/olia/discourse/olia_discourse.owl#ListSequence">
    <rdf:type rdf:resource="http://www.w3.org/2002/07/owl#Class"/>
  </rdf:Description>
  <rdf:Description rdf:about="http://purl.org/olia/discourse/olia_discourse.owl#ListSequence">
    <rdfs:subClassOf rdf:resource="http://purl.org/olia/discourse/olia_discourse.owl#ParatacticDiscourseRelation"/>
  </rdf:Description>
  <rdf:Description rdf:about="http://purl.org/olia/discourse/olia_discourse.owl#ListSequence">
    <rdfs:comment>Introduced as generalization over List and Sequence in analogy with SemDok. However, note that this is not a discourse relation proper, but a specific case of ParatacticDiscourseRelation for which no semantic relation except for paratactic organization can be provided.</rdfs:comment>
  </rdf:Description>
  <rdf:Description rdf:about="http://purl.org/olia/discourse/olia_discourse.owl#ListSequence">
    <rdfs:label xml:lang="en">list sequence</rdfs:label>
  </rdf:Description>
  <rdf:Description rdf:about="http://purl.org/olia/discourse/olia_discourse.owl#ListSequence">
    <rdfs:label>list/sequence</rdfs:label>
  </rdf:Description>
  <rdf:Description rdf:about="http://purl.org/olia/discourse/olia_discourse.owl#Magazine">
    <rdf:type rdf:resource="http://www.w3.org/2002/07/owl#Class"/>
  </rdf:Description>
  <rdf:Description rdf:about="http://purl.org/olia/discourse/olia_discourse.owl#Magazine">
    <rdfs:subClassOf rdf:resource="http://purl.org/olia/discourse/olia_discourse.owl#Newspaper"/>
  </rdf:Description>
  <rdf:Description rdf:about="http://purl.org/olia/discourse/olia_discourse.owl#Magazine">
    <rdfs:comment xml:lang="en">for nerd:Magazine sub nerd:Product</rdfs:comment>
  </rdf:Description>
  <rdf:Description rdf:about="http://purl.org/olia/discourse/olia_discourse.owl#Manner_RST">
    <rdf:type rdf:resource="http://www.w3.org/2002/07/owl#Class"/>
  </rdf:Description>
  <rdf:Description rdf:about="http://purl.org/olia/discourse/olia_discourse.owl#Manner_RST">
    <rdfs:subClassOf rdf:resource="http://purl.org/olia/discourse/olia_discourse.owl#Means"/>
  </rdf:Description>
  <rdf:Description rdf:about="http://purl.org/olia/discourse/olia_discourse.owl#Manner_RST">
    <rdfs:comment>A manner satellite explains the way in which something is done. (It sometimes also expresses some sort of similarity/comparison.) The satellite answers the question “in what manner?” or “in what way?”. A MANNER relation is less “goal-oriented” than a MEANS relation, and often is more of a description of the style of an action.
(Carlson and Marcu 2001)</rdfs:comment>
  </rdf:Description>
  <rdf:Description rdf:about="http://purl.org/olia/discourse/olia_discourse.owl#Manner_RST">
    <rdfs:label xml:lang="en">manner (RST)</rdfs:label>
  </rdf:Description>
  <rdf:Description rdf:about="http://purl.org/olia/discourse/olia_discourse.owl#ManufacturedObject">
    <rdf:type rdf:resource="http://www.w3.org/2002/07/owl#Class"/>
  </rdf:Description>
  <rdf:Description rdf:about="http://purl.org/olia/discourse/olia_discourse.owl#ManufacturedObject">
    <rdfs:subClassOf rdf:resource="http://purl.org/olia/discourse/olia_discourse.owl#Object"/>
  </rdf:Description>
  <rdf:Description rdf:about="http://purl.org/olia/discourse/olia_discourse.owl#ManufacturedObject">
    <rdfs:comment xml:lang="en">NERD seems to have been designed for economic purposes, so all objects (non-animate, concrete entitites) are described as "product". Here, we go with the more neutral term "ManufacturedObject".

for nerd:Product, subclass of nerd:Thing, not a NERD core class.</rdfs:comment>
  </rdf:Description>
  <rdf:Description rdf:about="http://purl.org/olia/discourse/olia_discourse.owl#ManufacturedObject">
    <rdfs:label xml:lang="en">PROD</rdfs:label>
  </rdf:Description>
  <rdf:Description rdf:about="http://purl.org/olia/discourse/olia_discourse.owl#ManufacturedObject">
    <rdfs:label xml:lang="en">consumer product</rdfs:label>
  </rdf:Description>
  <rdf:Description rdf:about="http://purl.org/olia/discourse/olia_discourse.owl#ManufacturedObject">
    <rdfs:label xml:lang="en">product</rdfs:label>
  </rdf:Description>
  <rdf:Description rdf:about="http://purl.org/olia/discourse/olia_discourse.owl#ManufacturedObject">
    <skos:prefLabel xml:lang="en">manufactured object</skos:prefLabel>
  </rdf:Description>
  <rdf:Description rdf:about="http://purl.org/olia/discourse/olia_discourse.owl#MapObject">
    <rdf:type rdf:resource="http://www.w3.org/2002/07/owl#Class"/>
  </rdf:Description>
  <rdf:Description rdf:about="http://purl.org/olia/discourse/olia_discourse.owl#MapObject">
    <rdfs:subClassOf rdf:resource="http://purl.org/olia/system.owl#UnitOfAnnotation"/>
  </rdf:Description>
  <rdf:Description rdf:about="http://purl.org/olia/discourse/olia_discourse.owl#MapObject">
    <rdfs:comment>An object on the map used for deictic references.
Language expressions may also depend on the visual, as opposed to verbal, context. An utterance like Could you pass me the salt? , uttered, e.g.,
at a restaurant, is usually understandable even if salt hasn’t been mentioned
before; the recipient can recover the referent of the expression the salt from the visual context. (An even clearer example is Could you please close
the window? .) We will use the term deictic references to refer to these
expressions.
(Artstein &amp; Poesio, 2006, ARRAU)</rdfs:comment>
  </rdf:Description>
  <rdf:Description rdf:about="http://purl.org/olia/discourse/olia_discourse.owl#MapObject">
    <rdfs:label xml:lang="en">map object</rdfs:label>
  </rdf:Description>
  <rdf:Description rdf:about="http://purl.org/olia/discourse/olia_discourse.owl#Markable">
    <rdf:type rdf:resource="http://www.w3.org/2002/07/owl#Class"/>
  </rdf:Description>
  <rdf:Description rdf:about="http://purl.org/olia/discourse/olia_discourse.owl#Markable">
    <rdfs:subClassOf rdf:resource="http://purl.org/olia/system.owl#UnitOfAnnotation"/>
  </rdf:Description>
  <rdf:Description rdf:about="http://purl.org/olia/discourse/olia_discourse.owl#Markable">
    <rdfs:comment>A markable refers to an element that is subject to annotation. Annotation schemes for coreference annotation *applied to plain text* usually require explicitly defined markables, for example.

The notion of Markable is somewhat problematic in its relation to DiscourseSegment. An RST elementary discourse unit (discourse segment) is basically a markable (almost-arbitrary plain String) together with a label, but an SDRT discourse segment is a structured semantic entity. Here, we remain agnostic. It is thus possible to define a joint subclass of DiscourseSegment and Markable for RST, for example.</rdfs:comment>
  </rdf:Description>
  <rdf:Description rdf:about="http://purl.org/olia/discourse/olia_discourse.owl#Markable">
    <rdfs:label xml:lang="en">markable</rdfs:label>
  </rdf:Description>
  <rdf:Description rdf:about="http://purl.org/olia/discourse/olia_discourse.owl#Mayor">
    <rdf:type rdf:resource="http://www.w3.org/2002/07/owl#Class"/>
  </rdf:Description>
  <rdf:Description rdf:about="http://purl.org/olia/discourse/olia_discourse.owl#Mayor">
    <rdfs:subClassOf rdf:resource="http://purl.org/olia/discourse/olia_discourse.owl#Politician"/>
  </rdf:Description>
  <rdf:Description rdf:about="http://purl.org/olia/discourse/olia_discourse.owl#Mayor">
    <rdfs:comment xml:lang="en">for nerd:Mayor, originally sub Person, here sub Politician. As this is not supported by an external extractor, it is deprecated.</rdfs:comment>
  </rdf:Description>
  <rdf:Description rdf:about="http://purl.org/olia/discourse/olia_discourse.owl#Mayor">
    <owl:deprecated rdf:datatype="http://www.w3.org/2001/XMLSchema#boolean">true</owl:deprecated>
  </rdf:Description>
  <rdf:Description rdf:about="http://purl.org/olia/discourse/olia_discourse.owl#Means">
    <rdf:type rdf:resource="http://www.w3.org/2002/07/owl#Class"/>
  </rdf:Description>
  <rdf:Description rdf:about="http://purl.org/olia/discourse/olia_discourse.owl#Means">
    <rdfs:subClassOf rdf:resource="http://purl.org/olia/discourse/olia_discourse.owl#HypotacticDiscourseRelation"/>
  </rdf:Description>
  <rdf:Description rdf:about="http://purl.org/olia/discourse/olia_discourse.owl#Means">
    <rdfs:subClassOf rdf:resource="http://purl.org/olia/discourse/olia_discourse.owl#PragmaticCondition"/>
  </rdf:Description>
  <rdf:Description rdf:about="http://purl.org/olia/discourse/olia_discourse.owl#Means">
    <rdfs:subClassOf rdf:resource="http://purl.org/olia/discourse/olia_discourse.owl#PresentationalRelation"/>
  </rdf:Description>
  <rdf:Description rdf:about="http://purl.org/olia/discourse/olia_discourse.owl#Means">
    <inverseOf rdf:resource="http://purl.org/olia/discourse/Achievement"/>
  </rdf:Description>
  <rdf:Description rdf:about="http://purl.org/olia/discourse/olia_discourse.owl#Means">
    <rdfs:comment>ISO Manner is an asymmetric discourse relation in which the means (Arg1) is a way in which the achievement (Arg2) comes about or occurs.

Corresponds to ISO Manner with argument means. Nucleus is the achievement.

cf. SemDok Means: mononuclear, interpersonal</rdfs:comment>
  </rdf:Description>
  <rdf:Description rdf:about="http://purl.org/olia/discourse/olia_discourse.owl#Means">
    <rdfs:label>manner</rdfs:label>
  </rdf:Description>
  <rdf:Description rdf:about="http://purl.org/olia/discourse/olia_discourse.owl#Means">
    <rdfs:label xml:lang="en">means</rdfs:label>
  </rdf:Description>
  <rdf:Description rdf:about="http://purl.org/olia/discourse/olia_discourse.owl#Means">
    <skos:prefLabel>means</skos:prefLabel>
  </rdf:Description>
  <rdf:Description rdf:about="http://purl.org/olia/discourse/olia_discourse.owl#Means_RST">
    <rdf:type rdf:resource="http://www.w3.org/2002/07/owl#Class"/>
  </rdf:Description>
  <rdf:Description rdf:about="http://purl.org/olia/discourse/olia_discourse.owl#Means_RST">
    <rdfs:subClassOf rdf:resource="http://purl.org/olia/discourse/olia_discourse.owl#Means"/>
  </rdf:Description>
  <rdf:Description rdf:about="http://purl.org/olia/discourse/olia_discourse.owl#Means_RST">
    <rdfs:comment>A means satellite specifies a method, mechanism, instrument, channel or con-
duit for accomplishing some goal. It should tell you how something was or is to be accomplished.
In other words, the satellite answers a “by which means?”or “how?” question that can be assigned
to the nucleus. It is often indicated by the preposition by.
(Carlson and Marcu 2001)</rdfs:comment>
  </rdf:Description>
  <rdf:Description rdf:about="http://purl.org/olia/discourse/olia_discourse.owl#Means_RST">
    <rdfs:label xml:lang="en">means (RST)</rdfs:label>
  </rdf:Description>
  <rdf:Description rdf:about="http://purl.org/olia/discourse/olia_discourse.owl#MediaProduct">
    <rdf:type rdf:resource="http://www.w3.org/2002/07/owl#Class"/>
  </rdf:Description>
  <rdf:Description rdf:about="http://purl.org/olia/discourse/olia_discourse.owl#MediaProduct">
    <rdfs:subClassOf rdf:resource="http://purl.org/olia/discourse/olia_discourse.owl#ManufacturedObject"/>
  </rdf:Description>
  <rdf:Description rdf:about="http://purl.org/olia/discourse/olia_discourse.owl#MediaProduct">
    <rdfs:comment xml:lang="en">introduced as a generalization over various nerd:Products</rdfs:comment>
  </rdf:Description>
  <rdf:Description rdf:about="http://purl.org/olia/discourse/olia_discourse.owl#MilitaryConflict">
    <rdf:type rdf:resource="http://www.w3.org/2002/07/owl#Class"/>
  </rdf:Description>
  <rdf:Description rdf:about="http://purl.org/olia/discourse/olia_discourse.owl#MilitaryConflict">
    <rdfs:subClassOf rdf:resource="http://purl.org/olia/discourse/olia_discourse.owl#Event"/>
  </rdf:Description>
  <rdf:Description rdf:about="http://purl.org/olia/discourse/olia_discourse.owl#MilitaryConflict">
    <rdfs:comment xml:lang="en">for nerd:MilitaryConflict</rdfs:comment>
  </rdf:Description>
  <rdf:Description rdf:about="http://purl.org/olia/discourse/olia_discourse.owl#MilitaryConflict">
    <rdfs:label xml:lang="en">conflict</rdfs:label>
  </rdf:Description>
  <rdf:Description rdf:about="http://purl.org/olia/discourse/olia_discourse.owl#MilitaryConflict">
    <skos:prefLabel xml:lang="en">military conflict</skos:prefLabel>
  </rdf:Description>
  <rdf:Description rdf:about="http://purl.org/olia/discourse/olia_discourse.owl#ModernUsage">
    <rdf:type rdf:resource="http://www.w3.org/2002/07/owl#Class"/>
  </rdf:Description>
  <rdf:Description rdf:about="http://purl.org/olia/discourse/olia_discourse.owl#ModernUsage">
    <rdfs:subClassOf rdf:resource="http://purl.org/olia/discourse/olia_discourse.owl#TemporallyDefinedUsage"/>
  </rdf:Description>
  <rdf:Description rdf:about="http://purl.org/olia/discourse/olia_discourse.owl#ModernUsage">
    <rdfs:comment>
                            Currently in use.
                                (http://www.isocat.org/datcat/DC-1962)
                            </rdfs:comment>
  </rdf:Description>
  <rdf:Description rdf:about="http://purl.org/olia/discourse/olia_discourse.owl#ModernUsage">
    <rdfs:label>modern</rdfs:label>
  </rdf:Description>
  <rdf:Description rdf:about="http://purl.org/olia/discourse/olia_discourse.owl#ModernUsage">
    <rdfs:label xml:lang="en">modern usage</rdfs:label>
  </rdf:Description>
  <rdf:Description rdf:about="http://purl.org/olia/discourse/olia_discourse.owl#ModernUsage">
    <owl:versionInfo>http://www.isocat.org/datcat/DC-1962 (modern)</owl:versionInfo>
  </rdf:Description>
  <rdf:Description rdf:about="http://purl.org/olia/discourse/olia_discourse.owl#ModernUsage">
    <owl:versionInfo>subClassOf dating (dcif:conceptualDomain)</owl:versionInfo>
  </rdf:Description>
  <rdf:Description rdf:about="http://purl.org/olia/discourse/olia_discourse.owl#Motivation_RST">
    <rdf:type rdf:resource="http://www.w3.org/2002/07/owl#Class"/>
  </rdf:Description>
  <rdf:Description rdf:about="http://purl.org/olia/discourse/olia_discourse.owl#Motivation_RST">
    <rdfs:subClassOf rdf:resource="http://purl.org/olia/discourse/olia_discourse.owl#PragmaticCause"/>
  </rdf:Description>
  <rdf:Description rdf:about="http://purl.org/olia/discourse/olia_discourse.owl#Motivation_RST">
    <rdfs:comment>Comprehending S increases R's desire to perform action in N
(Mann and Taboada 2010)</rdfs:comment>
  </rdf:Description>
  <rdf:Description rdf:about="http://purl.org/olia/discourse/olia_discourse.owl#Motivation_RST">
    <rdfs:label xml:lang="en">motivation (RST)</rdfs:label>
  </rdf:Description>
  <rdf:Description rdf:about="http://purl.org/olia/discourse/olia_discourse.owl#Mountain">
    <rdf:type rdf:resource="http://www.w3.org/2002/07/owl#Class"/>
  </rdf:Description>
  <rdf:Description rdf:about="http://purl.org/olia/discourse/olia_discourse.owl#Mountain">
    <rdfs:subClassOf rdf:resource="http://purl.org/olia/discourse/olia_discourse.owl#GeographicalFeature"/>
  </rdf:Description>
  <rdf:Description rdf:about="http://purl.org/olia/discourse/olia_discourse.owl#Mountain">
    <rdfs:comment xml:lang="en">for nerd:Mountain</rdfs:comment>
  </rdf:Description>
  <rdf:Description rdf:about="http://purl.org/olia/discourse/olia_discourse.owl#Movie">
    <rdf:type rdf:resource="http://www.w3.org/2002/07/owl#Class"/>
  </rdf:Description>
  <rdf:Description rdf:about="http://purl.org/olia/discourse/olia_discourse.owl#Movie">
    <rdfs:subClassOf rdf:resource="http://purl.org/olia/discourse/olia_discourse.owl#MediaProduct"/>
  </rdf:Description>
  <rdf:Description rdf:about="http://purl.org/olia/discourse/olia_discourse.owl#Movie">
    <rdfs:comment xml:lang="en">for nerd:Movie sub nerd:Product</rdfs:comment>
  </rdf:Description>
  <rdf:Description rdf:about="http://purl.org/olia/discourse/olia_discourse.owl#Movie">
    <rdfs:label xml:lang="en">film</rdfs:label>
  </rdf:Description>
  <rdf:Description rdf:about="http://purl.org/olia/discourse/olia_discourse.owl#Movie">
    <rdfs:label xml:lang="en">movie name</rdfs:label>
  </rdf:Description>
  <rdf:Description rdf:about="http://purl.org/olia/discourse/olia_discourse.owl#Movie">
    <skos:prefLabel xml:lang="en">movie</skos:prefLabel>
  </rdf:Description>
  <rdf:Description rdf:about="http://purl.org/olia/discourse/olia_discourse.owl#Museum">
    <rdf:type rdf:resource="http://www.w3.org/2002/07/owl#Class"/>
  </rdf:Description>
  <rdf:Description rdf:about="http://purl.org/olia/discourse/olia_discourse.owl#Museum">
    <rdfs:subClassOf rdf:resource="http://purl.org/olia/discourse/olia_discourse.owl#ArchitecturalFeature"/>
  </rdf:Description>
  <rdf:Description rdf:about="http://purl.org/olia/discourse/olia_discourse.owl#Museum">
    <rdfs:comment xml:lang="en">for nerd:Museum</rdfs:comment>
  </rdf:Description>
  <rdf:Description rdf:about="http://purl.org/olia/discourse/olia_discourse.owl#MusicalArtist">
    <rdf:type rdf:resource="http://www.w3.org/2002/07/owl#Class"/>
  </rdf:Description>
  <rdf:Description rdf:about="http://purl.org/olia/discourse/olia_discourse.owl#MusicalArtist">
    <rdfs:subClassOf rdf:resource="http://purl.org/olia/discourse/olia_discourse.owl#Artist"/>
  </rdf:Description>
  <rdf:Description rdf:about="http://purl.org/olia/discourse/olia_discourse.owl#MusicalArtist">
    <rdfs:comment xml:lang="en">for nerd:MusicalArtist, there subclass of nerd:Person. Cf. yahoo:music_artist</rdfs:comment>
  </rdf:Description>
  <rdf:Description rdf:about="http://purl.org/olia/discourse/olia_discourse.owl#MusicalEnsemble">
    <rdf:type rdf:resource="http://www.w3.org/2002/07/owl#Class"/>
  </rdf:Description>
  <rdf:Description rdf:about="http://purl.org/olia/discourse/olia_discourse.owl#MusicalEnsemble">
    <rdfs:subClassOf rdf:resource="http://purl.org/olia/discourse/olia_discourse.owl#Organization"/>
  </rdf:Description>
  <rdf:Description rdf:about="http://purl.org/olia/discourse/olia_discourse.owl#MusicalEnsemble">
    <rdfs:comment xml:lang="en">introduced as a generalization over nerd:Band and related terms, e.g., orchestra.

A musical ensemble, also known as a music group or musical group, is a group of people who perform instrumental or vocal music, with the ensemble typically known by a distinct name. (https://en.wikipedia.org/wiki/Musical_ensemble)</rdfs:comment>
  </rdf:Description>
  <rdf:Description rdf:about="http://purl.org/olia/discourse/olia_discourse.owl#NamedEntity">
    <rdf:type rdf:resource="http://www.w3.org/2002/07/owl#Class"/>
  </rdf:Description>
  <rdf:Description rdf:about="http://purl.org/olia/discourse/olia_discourse.owl#NamedEntity">
    <rdfs:subClassOf rdf:resource="http://purl.org/olia/discourse/olia_discourse.owl#Identifier"/>
  </rdf:Description>
  <rdf:Description rdf:about="http://purl.org/olia/discourse/olia_discourse.owl#NamedEntity">
    <rdfs:comment>
                            segment of text for which one or many rigid designators stands for the referent
                                (Gil Francopoulo; http://www.isocat.org/datcat/DC-2275)
                            </rdfs:comment>
  </rdf:Description>
  <rdf:Description rdf:about="http://purl.org/olia/discourse/olia_discourse.owl#NamedEntity">
    <rdfs:label>named entity</rdfs:label>
  </rdf:Description>
  <rdf:Description rdf:about="http://purl.org/olia/discourse/olia_discourse.owl#NamedEntity">
    <owl:versionInfo>http://www.isocat.org/datcat/DC-2275, note that the definition refers to the text that designates the entity, not the entity itself; consider renaming to NameOfEntity</owl:versionInfo>
  </rdf:Description>
  <rdf:Description rdf:about="http://purl.org/olia/discourse/olia_discourse.owl#NarrowFocus">
    <rdf:type rdf:resource="http://www.w3.org/2002/07/owl#Class"/>
  </rdf:Description>
  <rdf:Description rdf:about="http://purl.org/olia/discourse/olia_discourse.owl#NarrowFocus">
    <rdfs:subClassOf rdf:resource="http://purl.org/olia/discourse/olia_discourse.owl#StructuralFocusType"/>
  </rdf:Description>
  <rdf:Description rdf:about="http://purl.org/olia/discourse/olia_discourse.owl#NarrowFocus">
    <rdfs:comment>Wide focus and narrow focus represent an often-adopted, coarse-grained subclassification of foci according to their scope. Narrow focus means that one single constituent is in focus, whereas wide focus means that multiple constituents are in focus. (Fiedler &amp; Chiarcos)</rdfs:comment>
  </rdf:Description>
  <rdf:Description rdf:about="http://purl.org/olia/discourse/olia_discourse.owl#NarrowFocus">
    <rdfs:label xml:lang="en">narrow focus</rdfs:label>
  </rdf:Description>
  <rdf:Description rdf:about="http://purl.org/olia/discourse/olia_discourse.owl#NegatedAttribution">
    <rdf:type rdf:resource="http://www.w3.org/2002/07/owl#Class"/>
  </rdf:Description>
  <rdf:Description rdf:nodeID="genid37">
    <rdf:type rdf:resource="http://www.w3.org/2002/07/owl#Class"/>
  </rdf:Description>
  <rdf:Description rdf:nodeID="genid38">
    <rdf:first rdf:resource="http://purl.org/olia/discourse/olia_discourse.owl#Attribution"/>
  </rdf:Description>
  <rdf:Description rdf:nodeID="genid39">
    <rdf:first rdf:resource="http://purl.org/olia/discourse/olia_discourse.owl#NegativePolarity"/>
  </rdf:Description>
  <rdf:Description rdf:nodeID="genid38">
    <rdf:rest rdf:nodeID="genid39"/>
  </rdf:Description>
  <rdf:Description rdf:nodeID="genid41">
    <rdf:first rdf:nodeID="genid40"/>
  </rdf:Description>
  <rdf:Description rdf:nodeID="genid39">
    <rdf:rest rdf:nodeID="genid41"/>
  </rdf:Description>
  <rdf:Description rdf:nodeID="genid40">
    <rdf:type rdf:resource="http://www.w3.org/2002/07/owl#Restriction"/>
  </rdf:Description>
  <rdf:Description rdf:nodeID="genid40">
    <owl:onProperty rdf:resource="http://purl.org/olia/discourse/olia_discourse.owl#hasPolarity"/>
  </rdf:Description>
  <rdf:Description rdf:nodeID="genid40">
    <owl:hasSelf rdf:datatype="http://www.w3.org/2001/XMLSchema#boolean">true</owl:hasSelf>
  </rdf:Description>
  <rdf:Description rdf:nodeID="genid41">
    <rdf:rest rdf:resource="http://www.w3.org/1999/02/22-rdf-syntax-ns#nil"/>
  </rdf:Description>
  <rdf:Description rdf:nodeID="genid37">
    <owl:intersectionOf rdf:nodeID="genid38"/>
  </rdf:Description>
  <rdf:Description rdf:about="http://purl.org/olia/discourse/olia_discourse.owl#NegatedAttribution">
    <owl:equivalentClass rdf:nodeID="genid37"/>
  </rdf:Description>
  <rdf:Description rdf:about="http://purl.org/olia/discourse/olia_discourse.owl#NegatedAttribution">
    <rdfs:subClassOf rdf:resource="http://purl.org/olia/discourse/olia_discourse.owl#Attribution"/>
  </rdf:Description>
  <rdf:Description rdf:nodeID="genid42">
    <rdf:type rdf:resource="http://www.w3.org/2002/07/owl#Class"/>
  </rdf:Description>
  <rdf:Description rdf:nodeID="genid42">
    <owl:complementOf rdf:resource="http://purl.org/olia/discourse/olia_discourse.owl#NonNegatedAttribution"/>
  </rdf:Description>
  <rdf:Description rdf:about="http://purl.org/olia/discourse/olia_discourse.owl#NegatedAttribution">
    <rdfs:subClassOf rdf:nodeID="genid42"/>
  </rdf:Description>
  <rdf:Description rdf:about="http://purl.org/olia/discourse/olia_discourse.owl#NegatedAttribution">
    <rdfs:comment>This relation marks a negative attribution. The negation must be in the satel-
lite, or source, of the attribution in order for the ATTRIBUTION-N relation to hold.
(Carlson and Marcu 2001)

Verbs of attribution are negated on the surface - syntactically (e.g., didn’t say, don’t think) or lexically (e.g., denied), and the negation reverses the polarity of the attributed relation or argument content (Horn, 1978). The interpretation of the contrastive relation denoted by but requires that Arg2 should be interpreted under the scope of negation.
(Prasad et al. 2007)</rdfs:comment>
  </rdf:Description>
  <rdf:Description rdf:about="http://purl.org/olia/discourse/olia_discourse.owl#NegatedAttribution">
    <rdfs:label>negated attribution</rdfs:label>
  </rdf:Description>
  <rdf:Description rdf:about="http://purl.org/olia/discourse/olia_discourse.owl#NegatedAttribution">
    <rdfs:label xml:lang="en">negated attribution</rdfs:label>
  </rdf:Description>
  <rdf:Description rdf:about="http://purl.org/olia/discourse/olia_discourse.owl#NegatedAttribution">
    <rdfs:label>negative attribution</rdfs:label>
  </rdf:Description>
  <rdf:Description rdf:about="http://purl.org/olia/discourse/olia_discourse.owl#NegativeCondition">
    <rdf:type rdf:resource="http://www.w3.org/2002/07/owl#Class"/>
  </rdf:Description>
  <rdf:Description rdf:about="http://purl.org/olia/discourse/olia_discourse.owl#NegativeCondition">
    <rdfs:subClassOf rdf:resource="http://purl.org/olia/discourse/olia_discourse.owl#SemanticCondition"/>
  </rdf:Description>
  <rdf:Description rdf:about="http://purl.org/olia/discourse/olia_discourse.owl#NegativeCondition">
    <rdfs:comment>ISO: Asymmetric relation in which Arg1 is an unrealized situation which, when not realized, would lead to Arg2.

Roughly comparable to UnrealPastCondition and UnrealPresentCondition in PDTB. For HDRB, Oza et al. (2009) suggested to abandon the original tense distinction of PDTB.</rdfs:comment>
  </rdf:Description>
  <rdf:Description rdf:about="http://purl.org/olia/discourse/olia_discourse.owl#NegativeCondition">
    <rdfs:comment>Introduced as a generalization over PDTB FactualPastCondition and FactualPresentCondition in accordance with HDRB. Roughly corresponds to ISO Condition with argument antecedent.</rdfs:comment>
  </rdf:Description>
  <rdf:Description rdf:about="http://purl.org/olia/discourse/olia_discourse.owl#NegativeCondition">
    <rdfs:label>counterfactual</rdfs:label>
  </rdf:Description>
  <rdf:Description rdf:about="http://purl.org/olia/discourse/olia_discourse.owl#NegativeCondition">
    <rdfs:label>negative condition</rdfs:label>
  </rdf:Description>
  <rdf:Description rdf:about="http://purl.org/olia/discourse/olia_discourse.owl#NegativeCondition">
    <rdfs:label xml:lang="en">negative condition</rdfs:label>
  </rdf:Description>
  <rdf:Description rdf:about="http://purl.org/olia/discourse/olia_discourse.owl#NegativePolarity">
    <rdf:type rdf:resource="http://www.w3.org/2002/07/owl#Class"/>
  </rdf:Description>
  <rdf:Description rdf:about="http://purl.org/olia/discourse/olia_discourse.owl#NegativePolarity">
    <rdfs:subClassOf rdf:resource="http://purl.org/olia/discourse/olia_discourse.owl#Polarity"/>
  </rdf:Description>
  <rdf:Description rdf:about="http://purl.org/olia/discourse/olia_discourse.owl#NegativePolarity">
    <owl:disjointWith rdf:resource="http://purl.org/olia/discourse/olia_discourse.owl#UnmarkedPolarity"/>
  </rdf:Description>
  <rdf:Description rdf:about="http://purl.org/olia/discourse/olia_discourse.owl#NegativePolarity">
    <rdfs:comment>The scopal polarity feature is annotated on relations and their arguments to identify cases where verbs
of attribution are negated on the surface - syntactically (e.g., didn’t say, don’t think) or lexically (e.g.,
denied), but where the negation in fact reverses the polarity of the attributed relation or argument
content (Horn, 1978). Example (162) illustrates such a case. The but clause entails an interpretation
such as I think it’s not a main consideration, for which the negation must take narrow scope over the
embedded clause rather than the higher clause. In particular, the interpretation of the contrastive
relation denoted by but requires that Arg2 should be interpreted under the scope of negation.
(162) “Having the dividend increases is a supportive element in the market outlook, but
I don’t think it’s a main consideration,” he says. (0090)

To capture such entailments with surface negations on attribution verbs, an argument of a connective
is marked “Neg” for scopal polarity when the interpretation of the connective requires the surface
negation to take semantic scope over the lower argument. Thus, in Example (162), scopal polarity is
marked as “Neg” for Arg2.
(Prasad et al. 2007)</rdfs:comment>
  </rdf:Description>
  <rdf:Description rdf:about="http://purl.org/olia/discourse/olia_discourse.owl#NegativePolarity">
    <rdfs:label xml:lang="en">negative polarity</rdfs:label>
  </rdf:Description>
  <rdf:Description rdf:about="http://purl.org/olia/discourse/olia_discourse.owl#NeutralRegister">
    <rdf:type rdf:resource="http://www.w3.org/2002/07/owl#Class"/>
  </rdf:Description>
  <rdf:Description rdf:about="http://purl.org/olia/discourse/olia_discourse.owl#NeutralRegister">
    <rdfs:subClassOf rdf:resource="http://purl.org/olia/olia-top.owl#RegisterFeature"/>
  </rdf:Description>
  <rdf:Description rdf:about="http://purl.org/olia/discourse/olia_discourse.owl#NeutralRegister">
    <rdfs:comment>
                            The register appropriate to general texts or discourse.
                                (ISO12620; http://www.isocat.org/datcat/DC-1999)
                            </rdfs:comment>
  </rdf:Description>
  <rdf:Description rdf:about="http://purl.org/olia/discourse/olia_discourse.owl#NeutralRegister">
    <rdfs:label>neutral register</rdfs:label>
  </rdf:Description>
  <rdf:Description rdf:about="http://purl.org/olia/discourse/olia_discourse.owl#NeutralRegister">
    <rdfs:label>standard register</rdfs:label>
  </rdf:Description>
  <rdf:Description rdf:about="http://purl.org/olia/discourse/olia_discourse.owl#NeutralRegister">
    <owl:versionInfo>http://www.isocat.org/datcat/DC-1999</owl:versionInfo>
  </rdf:Description>
  <rdf:Description rdf:about="http://purl.org/olia/discourse/olia_discourse.owl#NeutralRegister">
    <owl:versionInfo>subClassOf register (dcif:conceptualDomain)</owl:versionInfo>
  </rdf:Description>
  <rdf:Description rdf:about="http://purl.org/olia/discourse/olia_discourse.owl#New">
    <rdf:type rdf:resource="http://www.w3.org/2002/07/owl#Class"/>
  </rdf:Description>
  <rdf:Description rdf:about="http://purl.org/olia/discourse/olia_discourse.owl#New">
    <rdfs:subClassOf rdf:resource="http://purl.org/olia/discourse/olia_discourse.owl#InformationStatus"/>
  </rdf:Description>
  <rdf:Description rdf:about="http://purl.org/olia/discourse/olia_discourse.owl#New">
    <rdfs:comment>A referent is new if at a given point in discourse, the hearer does not have a mental representation of this referent. (Prince 1988: "hearer-new")</rdfs:comment>
  </rdf:Description>
  <rdf:Description rdf:about="http://purl.org/olia/discourse/olia_discourse.owl#New">
    <rdfs:label xml:lang="en">new</rdfs:label>
  </rdf:Description>
  <rdf:Description rdf:about="http://purl.org/olia/discourse/olia_discourse.owl#NewInformationFocus">
    <rdf:type rdf:resource="http://www.w3.org/2002/07/owl#Class"/>
  </rdf:Description>
  <rdf:Description rdf:about="http://purl.org/olia/discourse/olia_discourse.owl#NewInformationFocus">
    <rdfs:subClassOf rdf:resource="http://purl.org/olia/discourse/olia_discourse.owl#DenotationFocus"/>
  </rdf:Description>
  <rdf:Description rdf:about="http://purl.org/olia/discourse/olia_discourse.owl#NewInformationFocus">
    <rdfs:comment>New-information focus (nf) is that part of the utterance providing the new and missing information which serves to develop the discourse. (SFB632 Guidelines)

WORDS: Who is reading a book?
NFocus:[ _nf Who] is reading a book?

WORDS: Mary is reading a book.
NFocus: [ _nf Mary] is reading a book. (5.2.1)

Also referred to as "assertive focus" or "completive focus".</rdfs:comment>
  </rdf:Description>
  <rdf:Description rdf:about="http://purl.org/olia/discourse/olia_discourse.owl#NewInformationFocus">
    <rdfs:label xml:lang="en">new information focus</rdfs:label>
  </rdf:Description>
  <rdf:Description rdf:about="http://purl.org/olia/discourse/olia_discourse.owl#Newspaper">
    <rdf:type rdf:resource="http://www.w3.org/2002/07/owl#Class"/>
  </rdf:Description>
  <rdf:Description rdf:about="http://purl.org/olia/discourse/olia_discourse.owl#Newspaper">
    <rdfs:subClassOf rdf:resource="http://purl.org/olia/discourse/olia_discourse.owl#MediaProduct"/>
  </rdf:Description>
  <rdf:Description rdf:about="http://purl.org/olia/discourse/olia_discourse.owl#Newspaper">
    <rdfs:comment xml:lang="en">for nerd:Newspaper sub nerd:Product</rdfs:comment>
  </rdf:Description>
  <rdf:Description rdf:about="http://purl.org/olia/discourse/olia_discourse.owl#NonContrastiveComparison">
    <rdf:type rdf:resource="http://www.w3.org/2002/07/owl#Class"/>
  </rdf:Description>
  <rdf:Description rdf:about="http://purl.org/olia/discourse/olia_discourse.owl#NonContrastiveComparison">
    <rdfs:subClassOf rdf:resource="http://purl.org/olia/discourse/olia_discourse.owl#Comparison"/>
  </rdf:Description>
  <rdf:Description rdf:about="http://purl.org/olia/discourse/olia_discourse.owl#NonContrastiveComparison">
    <rdfs:label xml:lang="en">non contrastive comparison</rdfs:label>
  </rdf:Description>
  <rdf:Description rdf:about="http://purl.org/olia/discourse/olia_discourse.owl#NonNegatedAttribution">
    <rdf:type rdf:resource="http://www.w3.org/2002/07/owl#Class"/>
  </rdf:Description>
  <rdf:Description rdf:nodeID="genid43">
    <rdf:type rdf:resource="http://www.w3.org/2002/07/owl#Class"/>
  </rdf:Description>
  <rdf:Description rdf:nodeID="genid44">
    <rdf:first rdf:resource="http://purl.org/olia/discourse/olia_discourse.owl#Attribution"/>
  </rdf:Description>
  <rdf:Description rdf:nodeID="genid45">
    <rdf:first rdf:resource="http://purl.org/olia/discourse/olia_discourse.owl#UnmarkedPolarity"/>
  </rdf:Description>
  <rdf:Description rdf:nodeID="genid44">
    <rdf:rest rdf:nodeID="genid45"/>
  </rdf:Description>
  <rdf:Description rdf:nodeID="genid47">
    <rdf:first rdf:nodeID="genid46"/>
  </rdf:Description>
  <rdf:Description rdf:nodeID="genid45">
    <rdf:rest rdf:nodeID="genid47"/>
  </rdf:Description>
  <rdf:Description rdf:nodeID="genid46">
    <rdf:type rdf:resource="http://www.w3.org/2002/07/owl#Restriction"/>
  </rdf:Description>
  <rdf:Description rdf:nodeID="genid46">
    <owl:onProperty rdf:resource="http://purl.org/olia/discourse/olia_discourse.owl#hasPolarity"/>
  </rdf:Description>
  <rdf:Description rdf:nodeID="genid46">
    <owl:hasSelf rdf:datatype="http://www.w3.org/2001/XMLSchema#boolean">true</owl:hasSelf>
  </rdf:Description>
  <rdf:Description rdf:nodeID="genid47">
    <rdf:rest rdf:resource="http://www.w3.org/1999/02/22-rdf-syntax-ns#nil"/>
  </rdf:Description>
  <rdf:Description rdf:nodeID="genid43">
    <owl:intersectionOf rdf:nodeID="genid44"/>
  </rdf:Description>
  <rdf:Description rdf:about="http://purl.org/olia/discourse/olia_discourse.owl#NonNegatedAttribution">
    <owl:equivalentClass rdf:nodeID="genid43"/>
  </rdf:Description>
  <rdf:Description rdf:about="http://purl.org/olia/discourse/olia_discourse.owl#NonNegatedAttribution">
    <rdfs:comment>Instances of reported speech, both direct and indirect, should be marked for the rhetorical relation of ATTRIBUTION. The satellite is the source of the attribution (a clause containing a reporting verb, or a phrase beginning with according to), and the nucleus is the content of the reported message (which must be in a separate clause). The ATTRIBUTION relation is also used with cognitive predicates, to include feelings, thoughts, hopes, etc.
(Carlson and Marcu 2001)</rdfs:comment>
  </rdf:Description>
  <rdf:Description rdf:about="http://purl.org/olia/discourse/olia_discourse.owl#NonNegatedAttribution">
    <rdfs:label xml:lang="en">non negated attribution</rdfs:label>
  </rdf:Description>
  <rdf:Description rdf:about="http://purl.org/olia/discourse/olia_discourse.owl#NonProfitOrganization">
    <rdf:type rdf:resource="http://www.w3.org/2002/07/owl#Class"/>
  </rdf:Description>
  <rdf:Description rdf:about="http://purl.org/olia/discourse/olia_discourse.owl#NonProfitOrganization">
    <rdfs:subClassOf rdf:resource="http://purl.org/olia/discourse/olia_discourse.owl#Organization"/>
  </rdf:Description>
  <rdf:Description rdf:about="http://purl.org/olia/discourse/olia_discourse.owl#NonProfitOrganization">
    <rdfs:comment xml:lang="en">for nerd:NonProfitOrganization. As this is not supported by an external extractor, it is deprecated.</rdfs:comment>
  </rdf:Description>
  <rdf:Description rdf:about="http://purl.org/olia/discourse/olia_discourse.owl#NonProfitOrganization">
    <owl:deprecated rdf:datatype="http://www.w3.org/2001/XMLSchema#boolean">true</owl:deprecated>
  </rdf:Description>
  <rdf:Description rdf:about="http://purl.org/olia/discourse/olia_discourse.owl#NonReferring">
    <rdf:type rdf:resource="http://www.w3.org/2002/07/owl#Class"/>
  </rdf:Description>
  <rdf:Description rdf:about="http://purl.org/olia/discourse/olia_discourse.owl#NonReferring">
    <rdfs:subClassOf rdf:resource="http://purl.org/olia/discourse/olia_discourse.owl#Referentiality"/>
  </rdf:Description>
  <rdf:Description rdf:about="http://purl.org/olia/discourse/olia_discourse.owl#NonReferring">
    <rdfs:label xml:lang="en">non referring</rdfs:label>
  </rdf:Description>
  <rdf:Description rdf:about="http://purl.org/olia/discourse/olia_discourse.owl#NonVolitionalCause_RST">
    <rdf:type rdf:resource="http://www.w3.org/2002/07/owl#Class"/>
  </rdf:Description>
  <rdf:Description rdf:about="http://purl.org/olia/discourse/olia_discourse.owl#NonVolitionalCause_RST">
    <rdfs:subClassOf rdf:resource="http://purl.org/olia/discourse/olia_discourse.owl#Cause_RST"/>
  </rdf:Description>
  <rdf:Description rdf:about="http://purl.org/olia/discourse/olia_discourse.owl#NonVolitionalCause_RST">
    <rdfs:comment>S, by means other than motivating a volitional action, caused N; without the presentation of S, R might not know the particular cause of the situation; a presentation of N is more central than S to W's purposes in putting forth the N-S combination. (Mann and Taboada 2010)</rdfs:comment>
  </rdf:Description>
  <rdf:Description rdf:about="http://purl.org/olia/discourse/olia_discourse.owl#NonVolitionalCause_RST">
    <rdfs:label xml:lang="en">non volitional cause (RST)</rdfs:label>
  </rdf:Description>
  <rdf:Description rdf:about="http://purl.org/olia/discourse/olia_discourse.owl#NonVolitionalResult_RST">
    <rdf:type rdf:resource="http://www.w3.org/2002/07/owl#Class"/>
  </rdf:Description>
  <rdf:Description rdf:about="http://purl.org/olia/discourse/olia_discourse.owl#NonVolitionalResult_RST">
    <rdfs:subClassOf rdf:resource="http://purl.org/olia/discourse/olia_discourse.owl#Result_RST"/>
  </rdf:Description>
  <rdf:Description rdf:about="http://purl.org/olia/discourse/olia_discourse.owl#NonVolitionalResult_RST">
    <rdfs:comment>N caused S; presentation of N is more central to W's purposes in putting forth the N-S combination than is the presentation of S.
(Mann and Taboada 2010)</rdfs:comment>
  </rdf:Description>
  <rdf:Description rdf:about="http://purl.org/olia/discourse/olia_discourse.owl#NonVolitionalResult_RST">
    <rdfs:label xml:lang="en">non volitional result (RST)</rdfs:label>
  </rdf:Description>
  <rdf:Description rdf:about="http://purl.org/olia/discourse/olia_discourse.owl#NonspecificAttributionSource">
    <rdf:type rdf:resource="http://www.w3.org/2002/07/owl#Class"/>
  </rdf:Description>
  <rdf:Description rdf:about="http://purl.org/olia/discourse/olia_discourse.owl#NonspecificAttributionSource">
    <rdfs:subClassOf rdf:resource="http://purl.org/olia/discourse/olia_discourse.owl#AttributionSource"/>
  </rdf:Description>
  <rdf:Description rdf:about="http://purl.org/olia/discourse/olia_discourse.owl#NonspecificAttributionSource">
    <rdfs:comment>Source is some arbitrary individual(s) indicated via a non-specific reference in the text.  (Prasad et al. 2007)</rdfs:comment>
  </rdf:Description>
  <rdf:Description rdf:about="http://purl.org/olia/discourse/olia_discourse.owl#NonspecificAttributionSource">
    <rdfs:label xml:lang="en">nonspecific attribution source</rdfs:label>
  </rdf:Description>
  <rdf:Description rdf:about="http://purl.org/olia/discourse/olia_discourse.owl#Object">
    <rdf:type rdf:resource="http://www.w3.org/2002/07/owl#Class"/>
  </rdf:Description>
  <rdf:Description rdf:about="http://purl.org/olia/discourse/olia_discourse.owl#Object">
    <rdfs:subClassOf rdf:resource="http://purl.org/olia/discourse/olia_discourse.owl#ConcreteEntity"/>
  </rdf:Description>
  <rdf:Description rdf:about="http://purl.org/olia/discourse/olia_discourse.owl#Object">
    <rdfs:comment xml:lang="en">introduced as an abstraction over nerd:Product and :ManufacturedObject</rdfs:comment>
  </rdf:Description>
  <rdf:Description rdf:about="http://purl.org/olia/discourse/olia_discourse.owl#ObjectFocus">
    <rdf:type rdf:resource="http://www.w3.org/2002/07/owl#Class"/>
  </rdf:Description>
  <rdf:Description rdf:about="http://purl.org/olia/discourse/olia_discourse.owl#ObjectFocus">
    <rdfs:subClassOf rdf:resource="http://purl.org/olia/discourse/olia_discourse.owl#ArgumentFocus"/>
  </rdf:Description>
  <rdf:Description rdf:about="http://purl.org/olia/discourse/olia_discourse.owl#ObjectFocus">
    <rdfs:comment>Narrow focus on the object argument. (Fiedler)</rdfs:comment>
  </rdf:Description>
  <rdf:Description rdf:about="http://purl.org/olia/discourse/olia_discourse.owl#ObjectFocus">
    <rdfs:label xml:lang="en">object focus</rdfs:label>
  </rdf:Description>
  <rdf:Description rdf:about="http://purl.org/olia/discourse/olia_discourse.owl#OldUsage">
    <rdf:type rdf:resource="http://www.w3.org/2002/07/owl#Class"/>
  </rdf:Description>
  <rdf:Description rdf:about="http://purl.org/olia/discourse/olia_discourse.owl#OldUsage">
    <rdfs:subClassOf rdf:resource="http://purl.org/olia/discourse/olia_discourse.owl#TemporallyDefinedUsage"/>
  </rdf:Description>
  <rdf:Description rdf:about="http://purl.org/olia/discourse/olia_discourse.owl#OldUsage">
    <rdfs:comment>
                            Old: Used in the past.
                                (http://www.isocat.org/datcat/DC-1961)
                                
                            Outdated form: A term or lexeme that has fallen from fashion, but the meaning of which is readily recognizable.(Sue Ellen Wright, http://www.isocat.org/datcat/DC-505)
                            </rdfs:comment>
  </rdf:Description>
  <rdf:Description rdf:about="http://purl.org/olia/discourse/olia_discourse.owl#OldUsage">
    <rdfs:label>old</rdfs:label>
  </rdf:Description>
  <rdf:Description rdf:about="http://purl.org/olia/discourse/olia_discourse.owl#OldUsage">
    <rdfs:label xml:lang="en">old usage</rdfs:label>
  </rdf:Description>
  <rdf:Description rdf:about="http://purl.org/olia/discourse/olia_discourse.owl#OldUsage">
    <rdfs:label>outdated</rdfs:label>
  </rdf:Description>
  <rdf:Description rdf:about="http://purl.org/olia/discourse/olia_discourse.owl#OldUsage">
    <owl:versionInfo>http://www.isocat.org/datcat/DC-1961, http://www.isocat.org/datcat/DC-505</owl:versionInfo>
  </rdf:Description>
  <rdf:Description rdf:about="http://purl.org/olia/discourse/olia_discourse.owl#OldUsage">
    <owl:versionInfo>subClassOf dating (dcif:conceptualDomain)</owl:versionInfo>
  </rdf:Description>
  <rdf:Description rdf:about="http://purl.org/olia/discourse/olia_discourse.owl#OperatingSystem">
    <rdf:type rdf:resource="http://www.w3.org/2002/07/owl#Class"/>
  </rdf:Description>
  <rdf:Description rdf:about="http://purl.org/olia/discourse/olia_discourse.owl#OperatingSystem">
    <rdfs:subClassOf rdf:resource="http://purl.org/olia/discourse/olia_discourse.owl#Software"/>
  </rdf:Description>
  <rdf:Description rdf:about="http://purl.org/olia/discourse/olia_discourse.owl#OperatingSystem">
    <rdfs:comment xml:lang="en">for nerd:OperatingSystem, subclass of nerd:Product</rdfs:comment>
  </rdf:Description>
  <rdf:Description rdf:about="http://purl.org/olia/discourse/olia_discourse.owl#OperatingSystem">
    <rdfs:label xml:lang="en">operating system</rdfs:label>
  </rdf:Description>
  <rdf:Description rdf:about="http://purl.org/olia/discourse/olia_discourse.owl#OperatorFocus">
    <rdf:type rdf:resource="http://www.w3.org/2002/07/owl#Class"/>
  </rdf:Description>
  <rdf:Description rdf:about="http://purl.org/olia/discourse/olia_discourse.owl#OperatorFocus">
    <rdfs:subClassOf rdf:resource="http://purl.org/olia/discourse/olia_discourse.owl#PredicateCenteredFocus"/>
  </rdf:Description>
  <rdf:Description rdf:about="http://purl.org/olia/discourse/olia_discourse.owl#OperatorFocus">
    <rdfs:comment>verb/predicate operator focus includes most importantly "verum" focus (truth value focus, polarity focus)
(Güldemann et al. 2010)</rdfs:comment>
  </rdf:Description>
  <rdf:Description rdf:about="http://purl.org/olia/discourse/olia_discourse.owl#OperatorFocus">
    <rdfs:label xml:lang="en">operator focus</rdfs:label>
  </rdf:Description>
  <rdf:Description rdf:about="http://purl.org/olia/discourse/olia_discourse.owl#Opposition_PDTB">
    <rdf:type rdf:resource="http://www.w3.org/2002/07/owl#Class"/>
  </rdf:Description>
  <rdf:Description rdf:about="http://purl.org/olia/discourse/olia_discourse.owl#Opposition_PDTB">
    <rdfs:subClassOf rdf:resource="http://purl.org/olia/discourse/olia_discourse.owl#SemanticContrast_PDTB"/>
  </rdf:Description>
  <rdf:Description rdf:about="http://purl.org/olia/discourse/olia_discourse.owl#Opposition_PDTB">
    <rdfs:comment>The values assigned to some shared property are the extremes of a gradable scale, e.g., tall-short,
accept-reject etc.
(Prasad et al. 2007)</rdfs:comment>
  </rdf:Description>
  <rdf:Description rdf:about="http://purl.org/olia/discourse/olia_discourse.owl#Opposition_PDTB">
    <rdfs:label xml:lang="en">opposition (PDTB)</rdfs:label>
  </rdf:Description>
  <rdf:Description rdf:about="http://purl.org/olia/discourse/olia_discourse.owl#Organization">
    <rdf:type rdf:resource="http://www.w3.org/2002/07/owl#Class"/>
  </rdf:Description>
  <rdf:Description rdf:about="http://purl.org/olia/discourse/olia_discourse.owl#Organization">
    <rdfs:subClassOf rdf:resource="http://purl.org/olia/discourse/olia_discourse.owl#ConcreteEntity"/>
  </rdf:Description>
  <rdf:Description rdf:about="http://purl.org/olia/discourse/olia_discourse.owl#Organization">
    <rdfs:comment xml:lang="en">for nerd:Organization, a NERD core class. As for organizations, we assume that this refers to organizations that are (or can be registered as) legal persons. In that sense, they are Concrete (because they are defined by a specific legal act)- In NERD, however, these are core concepts.</rdfs:comment>
  </rdf:Description>
  <rdf:Description rdf:about="http://purl.org/olia/discourse/olia_discourse.owl#Organization">
    <rdfs:label xml:lang="en">ORG</rdfs:label>
  </rdf:Description>
  <rdf:Description rdf:about="http://purl.org/olia/discourse/olia_discourse.owl#Organization">
    <skos:prefLabel xml:lang="en">organization</skos:prefLabel>
  </rdf:Description>
  <rdf:Description rdf:about="http://purl.org/olia/discourse/olia_discourse.owl#Other">
    <rdf:type rdf:resource="http://www.w3.org/2002/07/owl#Class"/>
  </rdf:Description>
  <rdf:Description rdf:about="http://purl.org/olia/discourse/olia_discourse.owl#Other">
    <rdfs:subClassOf rdf:resource="http://purl.org/olia/discourse/olia_discourse.owl#SameType"/>
  </rdf:Description>
  <rdf:Description rdf:about="http://purl.org/olia/discourse/olia_discourse.owl#Other">
    <rdfs:comment>A particular type of referent has been introduced before, the current referent specifies a new instantiation of this type, overtly marked by "other" (Poesio &amp; Artstein 2006).</rdfs:comment>
  </rdf:Description>
  <rdf:Description rdf:about="http://purl.org/olia/discourse/olia_discourse.owl#Other">
    <rdfs:label xml:lang="en">other</rdfs:label>
  </rdf:Description>
  <rdf:Description rdf:about="http://purl.org/olia/discourse/olia_discourse.owl#Otherwise_RST">
    <rdf:type rdf:resource="http://www.w3.org/2002/07/owl#Class"/>
  </rdf:Description>
  <rdf:Description rdf:about="http://purl.org/olia/discourse/olia_discourse.owl#Otherwise_RST">
    <rdfs:subClassOf rdf:resource="http://purl.org/olia/discourse/olia_discourse.owl#Alternative"/>
  </rdf:Description>
  <rdf:Description rdf:about="http://purl.org/olia/discourse/olia_discourse.owl#Otherwise_RST">
    <rdfs:comment>This is a mutually exclusive relation between two elements of equal importance. The situations presented by both the satellite and the nucleus are unrealized. Realizing the situation associated with the nucleus will prevent the realization of the consequences associated with the satellite. This relation may also be multinuclear.
(Carlson and Marcu 2001)</rdfs:comment>
  </rdf:Description>
  <rdf:Description rdf:about="http://purl.org/olia/discourse/olia_discourse.owl#Otherwise_RST">
    <rdfs:label xml:lang="en">otherwise (RST)</rdfs:label>
  </rdf:Description>
  <rdf:Description rdf:about="http://purl.org/olia/discourse/olia_discourse.owl#Parallel">
    <rdf:type rdf:resource="http://www.w3.org/2002/07/owl#Class"/>
  </rdf:Description>
  <rdf:Description rdf:about="http://purl.org/olia/discourse/olia_discourse.owl#Parallel">
    <rdfs:subClassOf rdf:resource="http://purl.org/olia/discourse/olia_discourse.owl#NonContrastiveComparison"/>
  </rdf:Description>
  <rdf:Description rdf:about="http://purl.org/olia/discourse/olia_discourse.owl#Parallel">
    <rdfs:comment>Infer a set of entities from DS0, E(DS0), and a set of entities from DS1, E(DS1).
Then infer commonalities between members of E(DS0) and E(DS1).
(Wolf et al. 2003)</rdfs:comment>
  </rdf:Description>
  <rdf:Description rdf:about="http://purl.org/olia/discourse/olia_discourse.owl#Parallel">
    <rdfs:label xml:lang="en">parallel</rdfs:label>
  </rdf:Description>
  <rdf:Description rdf:about="http://purl.org/olia/discourse/olia_discourse.owl#ParatacticDiscourseRelation">
    <rdf:type rdf:resource="http://www.w3.org/2002/07/owl#Class"/>
  </rdf:Description>
  <rdf:Description rdf:about="http://purl.org/olia/discourse/olia_discourse.owl#ParatacticDiscourseRelation">
    <rdfs:subClassOf rdf:resource="http://purl.org/olia/discourse/olia_discourse.owl#DiscourseStructuralPattern"/>
  </rdf:Description>
  <rdf:Description rdf:about="http://purl.org/olia/discourse/olia_discourse.owl#ParatacticDiscourseRelation">
    <rdfs:comment>Coordinating or Multinuclear relations.</rdfs:comment>
  </rdf:Description>
  <rdf:Description rdf:about="http://purl.org/olia/discourse/olia_discourse.owl#ParatacticDiscourseRelation">
    <rdfs:label>coordination</rdfs:label>
  </rdf:Description>
  <rdf:Description rdf:about="http://purl.org/olia/discourse/olia_discourse.owl#ParatacticDiscourseRelation">
    <rdfs:label>multinuclear</rdfs:label>
  </rdf:Description>
  <rdf:Description rdf:about="http://purl.org/olia/discourse/olia_discourse.owl#ParatacticDiscourseRelation">
    <rdfs:label xml:lang="en">paratactic discourse relation</rdfs:label>
  </rdf:Description>
  <rdf:Description rdf:about="http://purl.org/olia/discourse/olia_discourse.owl#ParatacticDiscourseRelation">
    <rdfs:label>parataxis</rdfs:label>
  </rdf:Description>
  <rdf:Description rdf:about="http://purl.org/olia/discourse/olia_discourse.owl#ParatacticDiscourseRelation">
    <rdfs:label>symmetrical coherence relation</rdfs:label>
  </rdf:Description>
  <rdf:Description rdf:about="http://purl.org/olia/discourse/olia_discourse.owl#Park">
    <rdf:type rdf:resource="http://www.w3.org/2002/07/owl#Class"/>
  </rdf:Description>
  <rdf:Description rdf:about="http://purl.org/olia/discourse/olia_discourse.owl#Park">
    <rdfs:subClassOf rdf:resource="http://purl.org/olia/discourse/olia_discourse.owl#ArchitecturalFeature"/>
  </rdf:Description>
  <rdf:Description rdf:about="http://purl.org/olia/discourse/olia_discourse.owl#Park">
    <rdfs:comment xml:lang="en">for nerd:Park</rdfs:comment>
  </rdf:Description>
  <rdf:Description rdf:about="http://purl.org/olia/discourse/olia_discourse.owl#PartOf">
    <rdf:type rdf:resource="http://www.w3.org/2002/07/owl#Class"/>
  </rdf:Description>
  <rdf:Description rdf:about="http://purl.org/olia/discourse/olia_discourse.owl#PartOf">
    <rdfs:subClassOf rdf:resource="http://purl.org/olia/discourse/olia_discourse.owl#PartWhole"/>
  </rdf:Description>
  <rdf:Description rdf:about="http://purl.org/olia/discourse/olia_discourse.owl#PartOf">
    <rdfs:comment>The referent is a part of another referent mentioned before (Poesio &amp; Artstein 2006).</rdfs:comment>
  </rdf:Description>
  <rdf:Description rdf:about="http://purl.org/olia/discourse/olia_discourse.owl#PartOf">
    <rdfs:label xml:lang="en">part of</rdfs:label>
  </rdf:Description>
  <rdf:Description rdf:about="http://purl.org/olia/discourse/olia_discourse.owl#PartWhole">
    <rdf:type rdf:resource="http://www.w3.org/2002/07/owl#Class"/>
  </rdf:Description>
  <rdf:Description rdf:about="http://purl.org/olia/discourse/olia_discourse.owl#PartWhole">
    <rdfs:subClassOf rdf:resource="http://purl.org/olia/discourse/olia_discourse.owl#BridgingType"/>
  </rdf:Description>
  <rdf:Description rdf:about="http://purl.org/olia/discourse/olia_discourse.owl#PartWhole">
    <rdfs:comment>A referent is a subset, an element, or a component of another referent mentioned before. (Stuttgart Guidelines)</rdfs:comment>
  </rdf:Description>
  <rdf:Description rdf:about="http://purl.org/olia/discourse/olia_discourse.owl#PartWhole">
    <rdfs:label xml:lang="en">part whole</rdfs:label>
  </rdf:Description>
  <rdf:Description rdf:about="http://purl.org/olia/discourse/olia_discourse.owl#Person">
    <rdf:type rdf:resource="http://www.w3.org/2002/07/owl#Class"/>
  </rdf:Description>
  <rdf:Description rdf:about="http://purl.org/olia/discourse/olia_discourse.owl#Person">
    <rdfs:subClassOf rdf:resource="http://purl.org/olia/discourse/olia_discourse.owl#AnimateEntity"/>
  </rdf:Description>
  <rdf:Description rdf:about="http://purl.org/olia/discourse/olia_discourse.owl#Person">
    <rdfs:comment xml:lang="en">Categories specified for referring expressions (Poesio &amp; Artstein 2006): Abstract, Animate, Concrete, Person, Plan, Space, Time.

Corresponds to nerd:Person</rdfs:comment>
  </rdf:Description>
  <rdf:Description rdf:about="http://purl.org/olia/discourse/olia_discourse.owl#Person">
    <rdfs:label xml:lang="en">PERS</rdfs:label>
  </rdf:Description>
  <rdf:Description rdf:about="http://purl.org/olia/discourse/olia_discourse.owl#Person">
    <skos:prefLabel xml:lang="en">person</skos:prefLabel>
  </rdf:Description>
  <rdf:Description rdf:about="http://purl.org/olia/discourse/olia_discourse.owl#Personal">
    <rdf:type rdf:resource="http://www.w3.org/2002/07/owl#Class"/>
  </rdf:Description>
  <rdf:Description rdf:about="http://purl.org/olia/discourse/olia_discourse.owl#Personal">
    <rdfs:subClassOf rdf:resource="http://purl.org/olia/olia-top.owl#ReferentTypeFeature"/>
  </rdf:Description>
  <rdf:Description rdf:about="http://purl.org/olia/discourse/olia_discourse.owl#Personal">
    <rdfs:comment>
                            Property that refers to the person.
                                (http://www.isocat.org/datcat/DC-1946)
                            </rdfs:comment>
  </rdf:Description>
  <rdf:Description rdf:about="http://purl.org/olia/discourse/olia_discourse.owl#Personal">
    <rdfs:label>personal</rdfs:label>
  </rdf:Description>
  <rdf:Description rdf:about="http://purl.org/olia/discourse/olia_discourse.owl#Personal">
    <owl:versionInfo>http://www.isocat.org/datcat/DC-1946</owl:versionInfo>
  </rdf:Description>
  <rdf:Description rdf:about="http://purl.org/olia/discourse/olia_discourse.owl#Personal">
    <owl:versionInfo>subClassOf referentType (dcif:conceptualDomain)</owl:versionInfo>
  </rdf:Description>
  <rdf:Description rdf:about="http://purl.org/olia/discourse/olia_discourse.owl#PhoneNumber">
    <rdf:type rdf:resource="http://www.w3.org/2002/07/owl#Class"/>
  </rdf:Description>
  <rdf:Description rdf:about="http://purl.org/olia/discourse/olia_discourse.owl#PhoneNumber">
    <rdfs:subClassOf rdf:resource="http://purl.org/olia/discourse/olia_discourse.owl#Address"/>
  </rdf:Description>
  <rdf:Description rdf:about="http://purl.org/olia/discourse/olia_discourse.owl#PhoneNumber">
    <rdfs:comment xml:lang="en">for nerd:PhoneNumber sub nerd:Product</rdfs:comment>
  </rdf:Description>
  <rdf:Description rdf:about="http://purl.org/olia/discourse/olia_discourse.owl#PlainRestatement_RST">
    <rdf:type rdf:resource="http://www.w3.org/2002/07/owl#Class"/>
  </rdf:Description>
  <rdf:Description rdf:about="http://purl.org/olia/discourse/olia_discourse.owl#PlainRestatement_RST">
    <rdfs:subClassOf rdf:resource="http://purl.org/olia/discourse/olia_discourse.owl#EquivalentRestatement"/>
  </rdf:Description>
  <rdf:Description rdf:about="http://purl.org/olia/discourse/olia_discourse.owl#PlainRestatement_RST">
    <rdfs:comment>A restatement relation is always mononuclear. The satellite and nucleus are of (roughly) comparable size. The satellite reiterates the information presented in the nucleus, typically with slightly different wording. It does not add to or interpret the information.
(Carlson and Marcu 2001)</rdfs:comment>
  </rdf:Description>
  <rdf:Description rdf:about="http://purl.org/olia/discourse/olia_discourse.owl#PlainRestatement_RST">
    <rdfs:label xml:lang="en">plain restatement (RST)</rdfs:label>
  </rdf:Description>
  <rdf:Description rdf:about="http://purl.org/olia/discourse/olia_discourse.owl#Plan">
    <rdf:type rdf:resource="http://www.w3.org/2002/07/owl#Class"/>
  </rdf:Description>
  <rdf:Description rdf:about="http://purl.org/olia/discourse/olia_discourse.owl#Plan">
    <rdfs:subClassOf rdf:resource="http://purl.org/olia/discourse/olia_discourse.owl#EntityType"/>
  </rdf:Description>
  <rdf:Description rdf:about="http://purl.org/olia/discourse/olia_discourse.owl#Plan">
    <rdfs:comment>Categories specified for referring expressions (Poesio &amp; Artstein 2006): Abstract, Animate, Concrete, Person, Plan, Space, Time</rdfs:comment>
  </rdf:Description>
  <rdf:Description rdf:about="http://purl.org/olia/discourse/olia_discourse.owl#Plan">
    <rdfs:label xml:lang="en">plan</rdfs:label>
  </rdf:Description>
  <rdf:Description rdf:about="http://purl.org/olia/discourse/olia_discourse.owl#PointOfOrigin">
    <rdf:type rdf:resource="http://www.w3.org/2002/07/owl#Class"/>
  </rdf:Description>
  <rdf:Description rdf:about="http://purl.org/olia/discourse/olia_discourse.owl#PointOfOrigin">
    <rdfs:subClassOf rdf:resource="http://purl.org/olia/olia-top.owl#TextStructuralUnit"/>
  </rdf:Description>
  <rdf:Description rdf:about="http://purl.org/olia/discourse/olia_discourse.owl#PointOfOrigin">
    <rdfs:comment>POINT-OF-ORIGIN refers to the geographic location in which the events in the
story take place. Use this schema if this information is designated separately at the beginning or
end of the article or section of the article. It should be linked to a TEXT or SECTIONTEXT schema. (Carlson and Marcu 2001)</rdfs:comment>
  </rdf:Description>
  <rdf:Description rdf:about="http://purl.org/olia/discourse/olia_discourse.owl#PointOfOrigin">
    <rdfs:label xml:lang="en">point of origin</rdfs:label>
  </rdf:Description>
  <rdf:Description rdf:about="http://purl.org/olia/discourse/olia_discourse.owl#Polarity">
    <rdf:type rdf:resource="http://www.w3.org/2002/07/owl#Class"/>
  </rdf:Description>
  <rdf:Description rdf:about="http://purl.org/olia/discourse/olia_discourse.owl#Polarity">
    <rdfs:subClassOf rdf:resource="http://purl.org/olia/discourse/olia_discourse.owl#SemanticFeature"/>
  </rdf:Description>
  <rdf:Description rdf:about="http://purl.org/olia/discourse/olia_discourse.owl#Polarity">
    <rdfs:comment>PDTB: applied to attributions

Classification of Attribute relations with respect to their "scopal polarity", marked when surface negated attribution reverses the polarity of the attributed AO.
The scopal polarity feature is annotated on relations and their arguments to identify cases where verbs
of attribution are negated on the surface - syntactically (e.g., didn’t say, don’t think) or lexically (e.g.,
denied), but where the negation in fact reverses the polarity of the attributed relation or argument
content (Horn, 1978).
(Prasad et al. 2007)</rdfs:comment>
  </rdf:Description>
  <rdf:Description rdf:about="http://purl.org/olia/discourse/olia_discourse.owl#Polarity">
    <rdfs:label xml:lang="en">polarity</rdfs:label>
  </rdf:Description>
  <rdf:Description rdf:about="http://purl.org/olia/discourse/olia_discourse.owl#PolarityFocus">
    <rdf:type rdf:resource="http://www.w3.org/2002/07/owl#Class"/>
  </rdf:Description>
  <rdf:Description rdf:about="http://purl.org/olia/discourse/olia_discourse.owl#PolarityFocus">
    <rdfs:subClassOf rdf:resource="http://purl.org/olia/discourse/olia_discourse.owl#OperatorFocus"/>
  </rdf:Description>
  <rdf:Description rdf:about="http://purl.org/olia/discourse/olia_discourse.owl#PolarityFocus">
    <rdfs:comment>"truth value focus", "polarity focus"

Context: I cannot imagine that the princess kissed the slippery frog.
example: Yes, she DID kiss him.
(Güldemann et al. 2010)</rdfs:comment>
  </rdf:Description>
  <rdf:Description rdf:about="http://purl.org/olia/discourse/olia_discourse.owl#PolarityFocus">
    <rdfs:label xml:lang="en">polarity focus</rdfs:label>
  </rdf:Description>
  <rdf:Description rdf:about="http://purl.org/olia/discourse/olia_discourse.owl#PoliticalEvent">
    <rdf:type rdf:resource="http://www.w3.org/2002/07/owl#Class"/>
  </rdf:Description>
  <rdf:Description rdf:about="http://purl.org/olia/discourse/olia_discourse.owl#PoliticalEvent">
    <rdfs:subClassOf rdf:resource="http://purl.org/olia/discourse/olia_discourse.owl#Event"/>
  </rdf:Description>
  <rdf:Description rdf:about="http://purl.org/olia/discourse/olia_discourse.owl#PoliticalEvent">
    <rdfs:comment xml:lang="en">for nerd:PoliticalEvent</rdfs:comment>
  </rdf:Description>
  <rdf:Description rdf:about="http://purl.org/olia/discourse/olia_discourse.owl#PoliticalOrganization">
    <rdf:type rdf:resource="http://www.w3.org/2002/07/owl#Class"/>
  </rdf:Description>
  <rdf:Description rdf:about="http://purl.org/olia/discourse/olia_discourse.owl#PoliticalOrganization">
    <rdfs:subClassOf rdf:resource="http://purl.org/olia/discourse/olia_discourse.owl#Organization"/>
  </rdf:Description>
  <rdf:Description rdf:about="http://purl.org/olia/discourse/olia_discourse.owl#PoliticalOrganization">
    <rdfs:comment xml:lang="en">introduced as generalization over PoliticalParty and nerd:Legislature</rdfs:comment>
  </rdf:Description>
  <rdf:Description rdf:about="http://purl.org/olia/discourse/olia_discourse.owl#PoliticalParty">
    <rdf:type rdf:resource="http://www.w3.org/2002/07/owl#Class"/>
  </rdf:Description>
  <rdf:Description rdf:about="http://purl.org/olia/discourse/olia_discourse.owl#PoliticalParty">
    <rdfs:subClassOf rdf:resource="http://purl.org/olia/discourse/olia_discourse.owl#PoliticalOrganization"/>
  </rdf:Description>
  <rdf:Description rdf:about="http://purl.org/olia/discourse/olia_discourse.owl#PoliticalParty">
    <rdfs:comment xml:lang="en">missing from NERD, however, nerd:PoliticalEvent was subclass of alchemyapi:PoliticalParty. This seems to have been misunderstood.</rdfs:comment>
  </rdf:Description>
  <rdf:Description rdf:about="http://purl.org/olia/discourse/olia_discourse.owl#PoliticalParty">
    <skos:prefLabel xml:lang="en">political party</skos:prefLabel>
  </rdf:Description>
  <rdf:Description rdf:about="http://purl.org/olia/discourse/olia_discourse.owl#PoliticalUnit">
    <rdf:type rdf:resource="http://www.w3.org/2002/07/owl#Class"/>
  </rdf:Description>
  <rdf:Description rdf:about="http://purl.org/olia/discourse/olia_discourse.owl#PoliticalUnit">
    <rdfs:subClassOf rdf:resource="http://purl.org/olia/discourse/olia_discourse.owl#Space"/>
  </rdf:Description>
  <rdf:Description rdf:about="http://purl.org/olia/discourse/olia_discourse.owl#PoliticalUnit">
    <rdfs:comment xml:lang="en">introduced as a generalization over nerd subclasses of Space that have a special political or social function, e.g., city, county, etc.</rdfs:comment>
  </rdf:Description>
  <rdf:Description rdf:about="http://purl.org/olia/discourse/olia_discourse.owl#Politician">
    <rdf:type rdf:resource="http://www.w3.org/2002/07/owl#Class"/>
  </rdf:Description>
  <rdf:Description rdf:about="http://purl.org/olia/discourse/olia_discourse.owl#Politician">
    <rdfs:subClassOf rdf:resource="http://purl.org/olia/discourse/olia_discourse.owl#Person"/>
  </rdf:Description>
  <rdf:Description rdf:about="http://purl.org/olia/discourse/olia_discourse.owl#Politician">
    <rdfs:comment xml:lang="en">for nerd:Politician and zemanta:politician</rdfs:comment>
  </rdf:Description>
  <rdf:Description rdf:about="http://purl.org/olia/discourse/olia_discourse.owl#Possessive">
    <rdf:type rdf:resource="http://www.w3.org/2002/07/owl#Class"/>
  </rdf:Description>
  <rdf:Description rdf:about="http://purl.org/olia/discourse/olia_discourse.owl#Possessive">
    <rdfs:subClassOf rdf:resource="http://purl.org/olia/olia-top.owl#ReferentTypeFeature"/>
  </rdf:Description>
  <rdf:Description rdf:about="http://purl.org/olia/discourse/olia_discourse.owl#Possessive">
    <rdfs:comment>
                            Relative to the possession or association.
                                (www.wordreference.com/English/definition.asp?en=possessive; http://www.isocat.org/datcat/DC-1355)
                            </rdfs:comment>
  </rdf:Description>
  <rdf:Description rdf:about="http://purl.org/olia/discourse/olia_discourse.owl#Possessive">
    <rdfs:label>possessive</rdfs:label>
  </rdf:Description>
  <rdf:Description rdf:about="http://purl.org/olia/discourse/olia_discourse.owl#Possessive">
    <owl:versionInfo>http://www.isocat.org/datcat/DC-1355</owl:versionInfo>
  </rdf:Description>
  <rdf:Description rdf:about="http://purl.org/olia/discourse/olia_discourse.owl#Possessive">
    <owl:versionInfo>subClassOf referentType (dcif:conceptualDomain)</owl:versionInfo>
  </rdf:Description>
  <rdf:Description rdf:about="http://purl.org/olia/discourse/olia_discourse.owl#Possible">
    <rdf:type rdf:resource="http://www.w3.org/2002/07/owl#Class"/>
  </rdf:Description>
  <rdf:Description rdf:about="http://purl.org/olia/discourse/olia_discourse.owl#Possible">
    <rdfs:subClassOf rdf:resource="http://purl.org/olia/olia-top.owl#UsageAndFrequencyFeature"/>
  </rdf:Description>
  <rdf:Description rdf:about="http://purl.org/olia/discourse/olia_discourse.owl#Possible">
    <rdfs:comment>Value that denotes a linguistic situation considered as being correct in the given language</rdfs:comment>
  </rdf:Description>
  <rdf:Description rdf:about="http://purl.org/olia/discourse/olia_discourse.owl#Possible">
    <rdfs:isDefinedBy>http://www.isocat.org/datcat/DC-1865</rdfs:isDefinedBy>
  </rdf:Description>
  <rdf:Description rdf:about="http://purl.org/olia/discourse/olia_discourse.owl#PragmaticCause">
    <rdf:type rdf:resource="http://www.w3.org/2002/07/owl#Class"/>
  </rdf:Description>
  <rdf:Description rdf:about="http://purl.org/olia/discourse/olia_discourse.owl#PragmaticCause">
    <rdfs:subClassOf rdf:resource="http://purl.org/olia/discourse/olia_discourse.owl#Cause"/>
  </rdf:Description>
  <rdf:Description rdf:about="http://purl.org/olia/discourse/olia_discourse.owl#PragmaticCause">
    <rdfs:subClassOf rdf:resource="http://purl.org/olia/discourse/olia_discourse.owl#PresentationalRelation"/>
  </rdf:Description>
  <rdf:Description rdf:about="http://purl.org/olia/discourse/olia_discourse.owl#PragmaticCause">
    <rdfs:comment>Arg1 expresses a claim and Arg2 provides justification for this claim. There is no causal influence between the two situations. (Prasad et al. 2007)</rdfs:comment>
  </rdf:Description>
  <rdf:Description rdf:about="http://purl.org/olia/discourse/olia_discourse.owl#PragmaticCause">
    <rdfs:label xml:lang="en">pragmatic cause</rdfs:label>
  </rdf:Description>
  <rdf:Description rdf:about="http://purl.org/olia/discourse/olia_discourse.owl#PragmaticCause">
    <rdfs:label>Speech-act Cause (LUNA)</rdfs:label>
  </rdf:Description>
  <rdf:Description rdf:about="http://purl.org/olia/discourse/olia_discourse.owl#PragmaticConcession_HDRB">
    <rdf:type rdf:resource="http://www.w3.org/2002/07/owl#Class"/>
  </rdf:Description>
  <rdf:Description rdf:about="http://purl.org/olia/discourse/olia_discourse.owl#PragmaticConcession_HDRB">
    <rdfs:subClassOf rdf:resource="http://purl.org/olia/discourse/olia_discourse.owl#Concession"/>
  </rdf:Description>
  <rdf:Description rdf:about="http://purl.org/olia/discourse/olia_discourse.owl#PragmaticConcession_HDRB">
    <rdfs:comment>Suggested as an extension of the PDTB scheme by Oza et al. (2009).</rdfs:comment>
  </rdf:Description>
  <rdf:Description rdf:about="http://purl.org/olia/discourse/olia_discourse.owl#PragmaticConcession_HDRB">
    <rdfs:label xml:lang="en">pragmatic concession (HDRB)</rdfs:label>
  </rdf:Description>
  <rdf:Description rdf:about="http://purl.org/olia/discourse/olia_discourse.owl#PragmaticConcession_LUNA">
    <rdf:type rdf:resource="http://www.w3.org/2002/07/owl#Class"/>
  </rdf:Description>
  <rdf:Description rdf:about="http://purl.org/olia/discourse/olia_discourse.owl#PragmaticConcession_LUNA">
    <rdfs:subClassOf rdf:resource="http://purl.org/olia/discourse/olia_discourse.owl#PragmaticConcession_HDRB"/>
  </rdf:Description>
  <rdf:Description rdf:about="http://purl.org/olia/discourse/olia_discourse.owl#PragmaticConcession_LUNA">
    <rdfs:comment>In the LUNA corpus (Tonelli et al. 2010), PragmaticConcession is a sibling concept of SpeechActConcession, EpistemicConcession and PropositionalConcession. Apparently, PragmaticConcession_LUNA has more specific semantics than just being a generalization over these types so that it is represented independently here.</rdfs:comment>
  </rdf:Description>
  <rdf:Description rdf:about="http://purl.org/olia/discourse/olia_discourse.owl#PragmaticConcession_LUNA">
    <rdfs:label xml:lang="en">pragmatic concession (LUNA)</rdfs:label>
  </rdf:Description>
  <rdf:Description rdf:about="http://purl.org/olia/discourse/olia_discourse.owl#PragmaticCondition">
    <rdf:type rdf:resource="http://www.w3.org/2002/07/owl#Class"/>
  </rdf:Description>
  <rdf:Description rdf:about="http://purl.org/olia/discourse/olia_discourse.owl#PragmaticCondition">
    <rdfs:subClassOf rdf:resource="http://purl.org/olia/discourse/olia_discourse.owl#Condition"/>
  </rdf:Description>
  <rdf:Description rdf:about="http://purl.org/olia/discourse/olia_discourse.owl#PragmaticCondition">
    <rdfs:comment>Conditional constructions whose interpretation deviates from that of the semantics of “Condition”. Arg1 and Arg2 are causally related. In all cases, Arg1 holds true independently of Arg2.  (Prasad et al. 2007)</rdfs:comment>
  </rdf:Description>
  <rdf:Description rdf:about="http://purl.org/olia/discourse/olia_discourse.owl#PragmaticCondition">
    <rdfs:label xml:lang="en">pragmatic condition</rdfs:label>
  </rdf:Description>
  <rdf:Description rdf:about="http://purl.org/olia/discourse/olia_discourse.owl#PragmaticCondition">
    <rdfs:label>Speech-act Condition (LUNA)</rdfs:label>
  </rdf:Description>
  <rdf:Description rdf:about="http://purl.org/olia/discourse/olia_discourse.owl#PragmaticContrast_PDTB">
    <rdf:type rdf:resource="http://www.w3.org/2002/07/owl#Class"/>
  </rdf:Description>
  <rdf:Description rdf:about="http://purl.org/olia/discourse/olia_discourse.owl#PragmaticContrast_PDTB">
    <rdfs:subClassOf rdf:resource="http://purl.org/olia/discourse/olia_discourse.owl#Contrast"/>
  </rdf:Description>
  <rdf:Description rdf:about="http://purl.org/olia/discourse/olia_discourse.owl#PragmaticContrast_PDTB">
    <rdfs:comment>The connective indicates a contrast between one of the arguments and an inference that can be drawn from the other, in many cases at the speech act level: The contrast is not between the situations described in Arg1 and Arg2.
(Prasad et al. 2007)</rdfs:comment>
  </rdf:Description>
  <rdf:Description rdf:about="http://purl.org/olia/discourse/olia_discourse.owl#PragmaticContrast_PDTB">
    <rdfs:label xml:lang="en">pragmatic contrast (PDTB)</rdfs:label>
  </rdf:Description>
  <rdf:Description rdf:about="http://purl.org/olia/discourse/olia_discourse.owl#PragmaticContrast_PDTB">
    <rdfs:label>Speech-act Contrast (LUNA)</rdfs:label>
  </rdf:Description>
  <rdf:Description rdf:about="http://purl.org/olia/discourse/olia_discourse.owl#PragmaticRelation">
    <rdf:type rdf:resource="http://www.w3.org/2002/07/owl#Class"/>
  </rdf:Description>
  <rdf:Description rdf:about="http://purl.org/olia/discourse/olia_discourse.owl#PragmaticRelation">
    <rdfs:subClassOf rdf:resource="http://purl.org/olia/system.owl#Relation"/>
  </rdf:Description>
  <rdf:Description rdf:nodeID="genid48">
    <rdf:type rdf:resource="http://www.w3.org/2002/07/owl#Class"/>
  </rdf:Description>
  <rdf:Description rdf:nodeID="genid50">
    <rdf:first rdf:nodeID="genid49"/>
  </rdf:Description>
  <rdf:Description rdf:nodeID="genid49">
    <rdf:type rdf:resource="http://www.w3.org/2002/07/owl#Restriction"/>
  </rdf:Description>
  <rdf:Description rdf:nodeID="genid49">
    <owl:onProperty rdf:resource="http://purl.org/olia/discourse/olia_discourse.owl#hasSource"/>
  </rdf:Description>
  <rdf:Description rdf:nodeID="genid49">
    <owl:qualifiedCardinality rdf:datatype="http://www.w3.org/2001/XMLSchema#nonNegativeInteger">1</owl:qualifiedCardinality>
  </rdf:Description>
  <rdf:Description rdf:nodeID="genid49">
    <owl:onClass rdf:resource="http://purl.org/olia/discourse/olia_discourse.owl#PragmaticUnit"/>
  </rdf:Description>
  <rdf:Description rdf:nodeID="genid52">
    <rdf:first rdf:nodeID="genid51"/>
  </rdf:Description>
  <rdf:Description rdf:nodeID="genid50">
    <rdf:rest rdf:nodeID="genid52"/>
  </rdf:Description>
  <rdf:Description rdf:nodeID="genid51">
    <rdf:type rdf:resource="http://www.w3.org/2002/07/owl#Restriction"/>
  </rdf:Description>
  <rdf:Description rdf:nodeID="genid51">
    <owl:onProperty rdf:resource="http://purl.org/olia/discourse/olia_discourse.owl#hasSource"/>
  </rdf:Description>
  <rdf:Description rdf:nodeID="genid51">
    <owl:qualifiedCardinality rdf:datatype="http://www.w3.org/2001/XMLSchema#nonNegativeInteger">1</owl:qualifiedCardinality>
  </rdf:Description>
  <rdf:Description rdf:nodeID="genid51">
    <owl:onClass rdf:resource="http://purl.org/olia/system.owl#UnitOfAnnotation"/>
  </rdf:Description>
  <rdf:Description rdf:nodeID="genid52">
    <rdf:rest rdf:resource="http://www.w3.org/1999/02/22-rdf-syntax-ns#nil"/>
  </rdf:Description>
  <rdf:Description rdf:nodeID="genid48">
    <owl:unionOf rdf:nodeID="genid50"/>
  </rdf:Description>
  <rdf:Description rdf:about="http://purl.org/olia/discourse/olia_discourse.owl#PragmaticRelation">
    <rdfs:subClassOf rdf:nodeID="genid48"/>
  </rdf:Description>
  <rdf:Description rdf:nodeID="genid53">
    <rdf:type rdf:resource="http://www.w3.org/2002/07/owl#Class"/>
  </rdf:Description>
  <rdf:Description rdf:nodeID="genid55">
    <rdf:first rdf:nodeID="genid54"/>
  </rdf:Description>
  <rdf:Description rdf:nodeID="genid54">
    <rdf:type rdf:resource="http://www.w3.org/2002/07/owl#Restriction"/>
  </rdf:Description>
  <rdf:Description rdf:nodeID="genid54">
    <owl:onProperty rdf:resource="http://purl.org/olia/discourse/olia_discourse.owl#hasTarget"/>
  </rdf:Description>
  <rdf:Description rdf:nodeID="genid54">
    <owl:qualifiedCardinality rdf:datatype="http://www.w3.org/2001/XMLSchema#nonNegativeInteger">1</owl:qualifiedCardinality>
  </rdf:Description>
  <rdf:Description rdf:nodeID="genid54">
    <owl:onClass rdf:resource="http://purl.org/olia/discourse/olia_discourse.owl#PragmaticUnit"/>
  </rdf:Description>
  <rdf:Description rdf:nodeID="genid57">
    <rdf:first rdf:nodeID="genid56"/>
  </rdf:Description>
  <rdf:Description rdf:nodeID="genid55">
    <rdf:rest rdf:nodeID="genid57"/>
  </rdf:Description>
  <rdf:Description rdf:nodeID="genid56">
    <rdf:type rdf:resource="http://www.w3.org/2002/07/owl#Restriction"/>
  </rdf:Description>
  <rdf:Description rdf:nodeID="genid56">
    <owl:onProperty rdf:resource="http://purl.org/olia/discourse/olia_discourse.owl#hasTarget"/>
  </rdf:Description>
  <rdf:Description rdf:nodeID="genid56">
    <owl:qualifiedCardinality rdf:datatype="http://www.w3.org/2001/XMLSchema#nonNegativeInteger">1</owl:qualifiedCardinality>
  </rdf:Description>
  <rdf:Description rdf:nodeID="genid56">
    <owl:onClass rdf:resource="http://purl.org/olia/system.owl#UnitOfAnnotation"/>
  </rdf:Description>
  <rdf:Description rdf:nodeID="genid57">
    <rdf:rest rdf:resource="http://www.w3.org/1999/02/22-rdf-syntax-ns#nil"/>
  </rdf:Description>
  <rdf:Description rdf:nodeID="genid53">
    <owl:unionOf rdf:nodeID="genid55"/>
  </rdf:Description>
  <rdf:Description rdf:about="http://purl.org/olia/discourse/olia_discourse.owl#PragmaticRelation">
    <rdfs:subClassOf rdf:nodeID="genid53"/>
  </rdf:Description>
  <rdf:Description rdf:about="http://purl.org/olia/discourse/olia_discourse.owl#PragmaticRelation">
    <rdfs:comment>PragmaticRelations are anaphoric, inferential or discourse-structural links between PragmaticCategories, e.g., DiscourseEntities, or AnnotationUnits.
Here, these are represented by an individual that represents the relation, and two properties hasSource and hasTarget that link is with the individuals that actually are connected by this relationship.

Note that "pragmatics" is used in a broad sense as opposed to semantics, hence discourse annotations are in its scope.</rdfs:comment>
  </rdf:Description>
  <rdf:Description rdf:about="http://purl.org/olia/discourse/olia_discourse.owl#PragmaticRelation">
    <rdfs:comment>cf. SemDok DiscourseRelation, which comprises both BridgingRelation and RhetoricalRelation.</rdfs:comment>
  </rdf:Description>
  <rdf:Description rdf:about="http://purl.org/olia/discourse/olia_discourse.owl#PragmaticRelation">
    <rdfs:label xml:lang="en">pragmatic relation</rdfs:label>
  </rdf:Description>
  <rdf:Description rdf:about="http://purl.org/olia/discourse/olia_discourse.owl#PragmaticUnit">
    <rdf:type rdf:resource="http://www.w3.org/2002/07/owl#Class"/>
  </rdf:Description>
  <rdf:Description rdf:about="http://purl.org/olia/discourse/olia_discourse.owl#PragmaticUnit">
    <rdfs:subClassOf rdf:resource="http://purl.org/olia/olia-top.owl#LinguisticConcept"/>
  </rdf:Description>
  <rdf:Description rdf:about="http://purl.org/olia/discourse/olia_discourse.owl#PragmaticUnit">
    <rdfs:comment>PragmaticCategory covers different information-structural, discourse-structural and classical pragmatic categories, structures and entities.

Note that "pragmatics" is used in a broad sense as opposed to semantics, hence discourse annotations are in its scope.</rdfs:comment>
  </rdf:Description>
  <rdf:Description rdf:about="http://purl.org/olia/discourse/olia_discourse.owl#PragmaticUnit">
    <rdfs:label xml:lang="en">pragmatic unit</rdfs:label>
  </rdf:Description>
  <rdf:Description rdf:about="http://purl.org/olia/discourse/olia_discourse.owl#PrecedenceRelation">
    <rdf:type rdf:resource="http://www.w3.org/2002/07/owl#Class"/>
  </rdf:Description>
  <rdf:Description rdf:about="http://purl.org/olia/discourse/olia_discourse.owl#PrecedenceRelation">
    <rdfs:subClassOf rdf:resource="http://purl.org/olia/discourse/olia_discourse.owl#AsynchronousRelation"/>
  </rdf:Description>
  <rdf:Description rdf:about="http://purl.org/olia/discourse/olia_discourse.owl#PrecedenceRelation">
    <inverseOf rdf:resource="http://purl.org/olia/discourse/SuccessionRelation"/>
  </rdf:Description>
  <rdf:Description rdf:about="http://purl.org/olia/discourse/olia_discourse.owl#PrecedenceRelation">
    <rdfs:comment>The connective indicates that the situation in Arg1 precedes the situation described in Arg2. (Prasad et al. 2007)</rdfs:comment>
  </rdf:Description>
  <rdf:Description rdf:about="http://purl.org/olia/discourse/olia_discourse.owl#PrecedenceRelation">
    <rdfs:label xml:lang="en">precedence relation</rdfs:label>
  </rdf:Description>
  <rdf:Description rdf:about="http://purl.org/olia/discourse/olia_discourse.owl#PredicateCenteredFocus">
    <rdf:type rdf:resource="http://www.w3.org/2002/07/owl#Class"/>
  </rdf:Description>
  <rdf:Description rdf:about="http://purl.org/olia/discourse/olia_discourse.owl#PredicateCenteredFocus">
    <rdfs:subClassOf rdf:resource="http://purl.org/olia/discourse/olia_discourse.owl#NarrowFocus"/>
  </rdf:Description>
  <rdf:Description rdf:about="http://purl.org/olia/discourse/olia_discourse.owl#PredicateCenteredFocus">
    <rdfs:comment>Narrow focus on the predicate. (Fiedler)

predicate is the host of two major functions relating to focus
(a) it instantiates an illocutionary act which relates to different operators
(b) it identifies/selects a state of affairs
(Güldemann et al. 2010)

Not to be confused with "predicate focus", as this is applied here to wide verb phrase focus following Lambrecht (1994)
</rdfs:comment>
  </rdf:Description>
  <rdf:Description rdf:about="http://purl.org/olia/discourse/olia_discourse.owl#PredicateCenteredFocus">
    <rdfs:label xml:lang="en">predicate centered focus</rdfs:label>
  </rdf:Description>
  <rdf:Description rdf:about="http://purl.org/olia/discourse/olia_discourse.owl#PredicateFocus">
    <rdf:type rdf:resource="http://www.w3.org/2002/07/owl#Class"/>
  </rdf:Description>
  <rdf:Description rdf:about="http://purl.org/olia/discourse/olia_discourse.owl#PredicateFocus">
    <rdfs:subClassOf rdf:resource="http://purl.org/olia/discourse/olia_discourse.owl#WideFocus"/>
  </rdf:Description>
  <rdf:Description rdf:about="http://purl.org/olia/discourse/olia_discourse.owl#PredicateFocus">
    <rdfs:comment>Following Lambrecht (1994), predicate focus is wide verb phrase focus. Not to be confused with PredicateCenteredFocus.</rdfs:comment>
  </rdf:Description>
  <rdf:Description rdf:about="http://purl.org/olia/discourse/olia_discourse.owl#PredicateFocus">
    <rdfs:label xml:lang="en">predicate focus</rdfs:label>
  </rdf:Description>
  <rdf:Description rdf:about="http://purl.org/olia/discourse/olia_discourse.owl#Preference_RST">
    <rdf:type rdf:resource="http://www.w3.org/2002/07/owl#Class"/>
  </rdf:Description>
  <rdf:Description rdf:about="http://purl.org/olia/discourse/olia_discourse.owl#Preference_RST">
    <rdfs:subClassOf rdf:resource="http://purl.org/olia/discourse/olia_discourse.owl#NonContrastiveComparison"/>
  </rdf:Description>
  <rdf:Description rdf:about="http://purl.org/olia/discourse/olia_discourse.owl#Preference_RST">
    <rdfs:comment>The relation compares two situations, acts, events, etc., and assigns a clear preference for one of the situations, acts, events, etc. The preferred situation, act, event, etc. is the nucleus.
(Lynn Carlson and Daniel Marcu. 2001. Discourse Tagging Manual. ISI Tech Report ISI-TR-545. July 2001. http://www.isi.edu/~marcu/discourse/tagging-ref-manual.pdf)</rdfs:comment>
  </rdf:Description>
  <rdf:Description rdf:about="http://purl.org/olia/discourse/olia_discourse.owl#Preference_RST">
    <rdfs:label xml:lang="en">preference (RST)</rdfs:label>
  </rdf:Description>
  <rdf:Description rdf:about="http://purl.org/olia/discourse/olia_discourse.owl#Preferred">
    <rdf:type rdf:resource="http://www.w3.org/2002/07/owl#Class"/>
  </rdf:Description>
  <rdf:Description rdf:about="http://purl.org/olia/discourse/olia_discourse.owl#Preferred">
    <rdfs:subClassOf rdf:resource="http://purl.org/olia/discourse/olia_discourse.owl#Possible"/>
  </rdf:Description>
  <rdf:Description rdf:about="http://purl.org/olia/discourse/olia_discourse.owl#Preferred">
    <rdfs:comment>
                            Preferred Term: A term rated according to the scale of a term acceptability rating as the primary term for a given concept.
                                (Sue Ellen Wright, http://www.isocat.org/datcat/DC-376)
                            </rdfs:comment>
  </rdf:Description>
  <rdf:Description rdf:about="http://purl.org/olia/discourse/olia_discourse.owl#Preferred">
    <rdfs:label>preferred</rdfs:label>
  </rdf:Description>
  <rdf:Description rdf:about="http://purl.org/olia/discourse/olia_discourse.owl#Preferred">
    <owl:versionInfo>http://www.isocat.org/datcat/DC-376</owl:versionInfo>
  </rdf:Description>
  <rdf:Description rdf:about="http://purl.org/olia/discourse/olia_discourse.owl#PreferredAlternative_RST">
    <rdf:type rdf:resource="http://www.w3.org/2002/07/owl#Class"/>
  </rdf:Description>
  <rdf:Description rdf:about="http://purl.org/olia/discourse/olia_discourse.owl#PreferredAlternative_RST">
    <rdfs:subClassOf rdf:resource="http://purl.org/olia/discourse/olia_discourse.owl#FavouredAlternative"/>
  </rdf:Description>
  <rdf:Description rdf:about="http://purl.org/olia/discourse/olia_discourse.owl#PreferredAlternative_RST">
    <rdfs:comment>RST-DTB Preference relation: The relation compares two situations, acts, events, etc., and assigns a clear preference for one of the situations, acts, events, etc. The preferred situation, act, event, etc. is the nucleus.
(Carlson and Marcu 2001)</rdfs:comment>
  </rdf:Description>
  <rdf:Description rdf:about="http://purl.org/olia/discourse/olia_discourse.owl#PreferredAlternative_RST">
    <rdfs:label xml:lang="en">preferred alternative (RST)</rdfs:label>
  </rdf:Description>
  <rdf:Description rdf:about="http://purl.org/olia/discourse/olia_discourse.owl#Preparation">
    <rdf:type rdf:resource="http://www.w3.org/2002/07/owl#Class"/>
  </rdf:Description>
  <rdf:Description rdf:about="http://purl.org/olia/discourse/olia_discourse.owl#Preparation">
    <rdfs:subClassOf rdf:resource="http://purl.org/olia/discourse/olia_discourse.owl#Background"/>
  </rdf:Description>
  <rdf:Description rdf:about="http://purl.org/olia/discourse/olia_discourse.owl#Preparation">
    <rdfs:subClassOf rdf:resource="http://purl.org/olia/discourse/olia_discourse.owl#PresentationalRelation"/>
  </rdf:Description>
  <rdf:Description rdf:about="http://purl.org/olia/discourse/olia_discourse.owl#Preparation">
    <rdfs:comment>introduced as generalization over Preparation in RST and SemDok. Axiomatization follows SemDok</rdfs:comment>
  </rdf:Description>
  <rdf:Description rdf:about="http://purl.org/olia/discourse/olia_discourse.owl#Preparation">
    <rdfs:label>preparation</rdfs:label>
  </rdf:Description>
  <rdf:Description rdf:about="http://purl.org/olia/discourse/olia_discourse.owl#Preparation">
    <rdfs:label xml:lang="en">preparation</rdfs:label>
  </rdf:Description>
  <rdf:Description rdf:about="http://purl.org/olia/discourse/olia_discourse.owl#PreparationQuestion">
    <rdf:type rdf:resource="http://www.w3.org/2002/07/owl#Class"/>
  </rdf:Description>
  <rdf:Description rdf:about="http://purl.org/olia/discourse/olia_discourse.owl#PreparationQuestion">
    <owl:equivalentClass rdf:resource="http://purl.org/olia/discourse/olia_discourse.owl#RhetoricalQuestion_RST"/>
  </rdf:Description>
  <rdf:Description rdf:about="http://purl.org/olia/discourse/olia_discourse.owl#PreparationQuestion">
    <rdfs:subClassOf rdf:resource="http://purl.org/olia/discourse/olia_discourse.owl#Preparation"/>
  </rdf:Description>
  <rdf:Description rdf:about="http://purl.org/olia/discourse/olia_discourse.owl#PreparationQuestion">
    <rdfs:comment>for SemDok Preparation-question

I assume that this is basically equivalent with RhetoricalQuestion_RST, but note that SemDok does not provide explicit definitions.</rdfs:comment>
  </rdf:Description>
  <rdf:Description rdf:about="http://purl.org/olia/discourse/olia_discourse.owl#PreparationQuestion">
    <rdfs:label xml:lang="en">preparation question</rdfs:label>
  </rdf:Description>
  <rdf:Description rdf:about="http://purl.org/olia/discourse/olia_discourse.owl#PreparationQuestion">
    <rdfs:label>preparation-question</rdfs:label>
  </rdf:Description>
  <rdf:Description rdf:about="http://purl.org/olia/discourse/olia_discourse.owl#PreparationTitle">
    <rdf:type rdf:resource="http://www.w3.org/2002/07/owl#Class"/>
  </rdf:Description>
  <rdf:Description rdf:about="http://purl.org/olia/discourse/olia_discourse.owl#PreparationTitle">
    <rdfs:subClassOf rdf:resource="http://purl.org/olia/discourse/olia_discourse.owl#Preparation"/>
  </rdf:Description>
  <rdf:Description rdf:about="http://purl.org/olia/discourse/olia_discourse.owl#PreparationTitle">
    <rdfs:subClassOf rdf:resource="http://purl.org/olia/discourse/olia_discourse.owl#Title"/>
  </rdf:Description>
  <rdf:Description rdf:about="http://purl.org/olia/discourse/olia_discourse.owl#PreparationTitle">
    <rdfs:comment>for SemDok Preparation-title</rdfs:comment>
  </rdf:Description>
  <rdf:Description rdf:about="http://purl.org/olia/discourse/olia_discourse.owl#PreparationTitle">
    <rdfs:label xml:lang="en">preparation title</rdfs:label>
  </rdf:Description>
  <rdf:Description rdf:about="http://purl.org/olia/discourse/olia_discourse.owl#PreparationTitle">
    <rdfs:label>preparation-title</rdfs:label>
  </rdf:Description>
  <rdf:Description rdf:about="http://purl.org/olia/discourse/olia_discourse.owl#Preparation_RST">
    <rdf:type rdf:resource="http://www.w3.org/2002/07/owl#Class"/>
  </rdf:Description>
  <rdf:Description rdf:about="http://purl.org/olia/discourse/olia_discourse.owl#Preparation_RST">
    <rdfs:subClassOf rdf:resource="http://purl.org/olia/discourse/olia_discourse.owl#Preparation"/>
  </rdf:Description>
  <rdf:Description rdf:about="http://purl.org/olia/discourse/olia_discourse.owl#Preparation_RST">
    <rdfs:comment>S precedes N in the text; S tends to make R more ready, interested or oriented for reading N
(Mann and Taboada 2010)</rdfs:comment>
  </rdf:Description>
  <rdf:Description rdf:about="http://purl.org/olia/discourse/olia_discourse.owl#Preparation_RST">
    <rdfs:label xml:lang="en">preparation (RST)</rdfs:label>
  </rdf:Description>
  <rdf:Description rdf:about="http://purl.org/olia/discourse/olia_discourse.owl#PresentationalRelation">
    <rdf:type rdf:resource="http://www.w3.org/2002/07/owl#Class"/>
  </rdf:Description>
  <rdf:Description rdf:about="http://purl.org/olia/discourse/olia_discourse.owl#PresentationalRelation">
    <rdfs:subClassOf rdf:resource="http://purl.org/olia/discourse/olia_discourse.owl#DiscourseFunction"/>
  </rdf:Description>
  <rdf:Description rdf:about="http://purl.org/olia/discourse/olia_discourse.owl#PresentationalRelation">
    <owl:disjointWith rdf:resource="http://purl.org/olia/discourse/olia_discourse.owl#SubjectMatterRelation"/>
  </rdf:Description>
  <rdf:Description rdf:about="http://purl.org/olia/discourse/olia_discourse.owl#PresentationalRelation">
    <owl:disjointWith rdf:resource="http://purl.org/olia/discourse/olia_discourse.owl#TextualOrganizationalRelation"/>
  </rdf:Description>
  <rdf:Description rdf:about="http://purl.org/olia/discourse/olia_discourse.owl#PresentationalRelation">
    <rdfs:comment>"[In RST] a distinction is made between Subject-Matter relations and Presentational relations. Subject-Matter relations express parts of the subject matter of the text. The Presentational relations facilitate the presentation process."
(http://www.sfu.ca/rst/01intro/intro.html)</rdfs:comment>
  </rdf:Description>
  <rdf:Description rdf:about="http://purl.org/olia/discourse/olia_discourse.owl#PresentationalRelation">
    <rdfs:comment>cf. SemDok InterpersonalRelation, no definition given there, but the conventional definition alludes to RST "presentational relations".

Conventional definition (https://en.wikipedia.org/wiki/Metafunction#Ideational_function): The interpersonal function refers to the grammatical choices that enable speakers to enact their complex and diverse interpersonal relations. This tenet of systemic functional linguistics is based on the claim that a speaker not only talks about something, but is always talking to and with others.</rdfs:comment>
  </rdf:Description>
  <rdf:Description rdf:about="http://purl.org/olia/discourse/olia_discourse.owl#PresentationalRelation">
    <rdfs:label>interpersonal relation</rdfs:label>
  </rdf:Description>
  <rdf:Description rdf:about="http://purl.org/olia/discourse/olia_discourse.owl#PresentationalRelation">
    <rdfs:label>presentational relation</rdfs:label>
  </rdf:Description>
  <rdf:Description rdf:about="http://purl.org/olia/discourse/olia_discourse.owl#PresentationalRelation">
    <rdfs:label xml:lang="en">presentational relation</rdfs:label>
  </rdf:Description>
  <rdf:Description rdf:about="http://purl.org/olia/discourse/olia_discourse.owl#ProblemSolution">
    <rdf:type rdf:resource="http://www.w3.org/2002/07/owl#Class"/>
  </rdf:Description>
  <rdf:Description rdf:about="http://purl.org/olia/discourse/olia_discourse.owl#ProblemSolution">
    <rdfs:subClassOf rdf:resource="http://purl.org/olia/discourse/olia_discourse.owl#PragmaticCondition"/>
  </rdf:Description>
  <rdf:Description rdf:about="http://purl.org/olia/discourse/olia_discourse.owl#ProblemSolution">
    <rdfs:subClassOf rdf:resource="http://purl.org/olia/discourse/olia_discourse.owl#PresentationalRelation"/>
  </rdf:Description>
  <rdf:Description rdf:about="http://purl.org/olia/discourse/olia_discourse.owl#ProblemSolution">
    <rdfs:comment>Introduced as generalization over Problem-Solution in RST-DTB and SemDok.

In a problem-solution relation, one textual span presents a problem, and the other text span presents a solution. The relation may be mononuclear or multinuclear, depending on the context. (Carlson and Marcu 2001)

RST "Solutionhood": R recognizes N as a solution to the problem presented in S. (Mann and Taboada 2010)</rdfs:comment>
  </rdf:Description>
  <rdf:Description rdf:about="http://purl.org/olia/discourse/olia_discourse.owl#ProblemSolution">
    <rdfs:label xml:lang="en">problem solution</rdfs:label>
  </rdf:Description>
  <rdf:Description rdf:about="http://purl.org/olia/discourse/olia_discourse.owl#ProblemSolution">
    <rdfs:label>solutionhood</rdfs:label>
  </rdf:Description>
  <rdf:Description rdf:about="http://purl.org/olia/discourse/olia_discourse.owl#ProblemSolution">
    <skos:prefLabel>problem-solution</skos:prefLabel>
  </rdf:Description>
  <rdf:Description rdf:about="http://purl.org/olia/discourse/olia_discourse.owl#ProblemSolution_RST">
    <rdf:type rdf:resource="http://www.w3.org/2002/07/owl#Class"/>
  </rdf:Description>
  <rdf:Description rdf:about="http://purl.org/olia/discourse/olia_discourse.owl#ProblemSolution_RST">
    <rdfs:subClassOf rdf:resource="http://purl.org/olia/discourse/olia_discourse.owl#ProblemSolution"/>
  </rdf:Description>
  <rdf:Description rdf:about="http://purl.org/olia/discourse/olia_discourse.owl#ProblemSolution_RST">
    <rdfs:label xml:lang="en">problem solution (RST)</rdfs:label>
  </rdf:Description>
  <rdf:Description rdf:about="http://purl.org/olia/discourse/olia_discourse.owl#ProblemSolution_RST">
    <owl:deprecated rdf:datatype="http://www.w3.org/2001/XMLSchema#boolean">true</owl:deprecated>
  </rdf:Description>
  <rdf:Description rdf:about="http://purl.org/olia/discourse/olia_discourse.owl#ProgrammingLanguage">
    <rdf:type rdf:resource="http://www.w3.org/2002/07/owl#Class"/>
  </rdf:Description>
  <rdf:Description rdf:about="http://purl.org/olia/discourse/olia_discourse.owl#ProgrammingLanguage">
    <rdfs:subClassOf rdf:resource="http://purl.org/olia/discourse/olia_discourse.owl#Software"/>
  </rdf:Description>
  <rdf:Description rdf:about="http://purl.org/olia/discourse/olia_discourse.owl#ProgrammingLanguage">
    <rdfs:comment xml:lang="en">for nerd:ProgrammingLanguage sub nerd:Product. Marked as deprecated as its qualification as a product is hardly justifiable.

after renaming Product to "Manufactured Object", this is a valid concept, again</rdfs:comment>
  </rdf:Description>
  <rdf:Description rdf:about="http://purl.org/olia/discourse/olia_discourse.owl#Proportion_RST">
    <rdf:type rdf:resource="http://www.w3.org/2002/07/owl#Class"/>
  </rdf:Description>
  <rdf:Description rdf:about="http://purl.org/olia/discourse/olia_discourse.owl#Proportion_RST">
    <rdfs:subClassOf rdf:resource="http://purl.org/olia/discourse/olia_discourse.owl#Similarity"/>
  </rdf:Description>
  <rdf:Description rdf:about="http://purl.org/olia/discourse/olia_discourse.owl#Proportion_RST">
    <rdfs:comment>A PROPORTION relation expresses a proportionality or equivalence of tendency or degree between two nuclei. It is always multinuclear.
(Carlson and Marcu 2001)</rdfs:comment>
  </rdf:Description>
  <rdf:Description rdf:about="http://purl.org/olia/discourse/olia_discourse.owl#Proportion_RST">
    <rdfs:label xml:lang="en">proportion (RST)</rdfs:label>
  </rdf:Description>
  <rdf:Description rdf:about="http://purl.org/olia/discourse/olia_discourse.owl#Proposition">
    <rdf:type rdf:resource="http://www.w3.org/2002/07/owl#Class"/>
  </rdf:Description>
  <rdf:Description rdf:about="http://purl.org/olia/discourse/olia_discourse.owl#Proposition">
    <rdfs:subClassOf rdf:resource="http://purl.org/olia/olia-top.owl#DiscourseEntity"/>
  </rdf:Description>
  <rdf:Description rdf:about="http://purl.org/olia/discourse/olia_discourse.owl#Proposition">
    <rdfs:comment>Cognitive representation of the information conveyed in a particular clause or sentence. Not to be confused with "proposition" in semantics (Kintsch REF).</rdfs:comment>
  </rdf:Description>
  <rdf:Description rdf:about="http://purl.org/olia/discourse/olia_discourse.owl#Proposition">
    <rdfs:label xml:lang="en">proposition</rdfs:label>
  </rdf:Description>
  <rdf:Description rdf:about="http://purl.org/olia/discourse/olia_discourse.owl#PropositionalCause_HDRB">
    <rdf:type rdf:resource="http://www.w3.org/2002/07/owl#Class"/>
  </rdf:Description>
  <rdf:Description rdf:about="http://purl.org/olia/discourse/olia_discourse.owl#PropositionalCause_HDRB">
    <rdfs:subClassOf rdf:resource="http://purl.org/olia/discourse/olia_discourse.owl#PragmaticCause"/>
  </rdf:Description>
  <rdf:Description rdf:about="http://purl.org/olia/discourse/olia_discourse.owl#PropositionalCause_HDRB">
    <rdfs:comment>An extension of the PDTB scheme suggested by Oza et al. (2009).

Each pragmatic sense at the type level is
further distinguished into three subtypes: “epis-
temic” (Sweetser 1990), “speech-act” (Sweetser
1990), and “propositional”. The propositional
subtype involves the inference of a complete
proposition. The relation is then taken to hold
between this inferred proposition and the propo-
sitional content of one of the arguments.
(Oza et al. 2009)</rdfs:comment>
  </rdf:Description>
  <rdf:Description rdf:about="http://purl.org/olia/discourse/olia_discourse.owl#PropositionalCause_HDRB">
    <rdfs:label xml:lang="en">propositional cause (HDRB)</rdfs:label>
  </rdf:Description>
  <rdf:Description rdf:about="http://purl.org/olia/discourse/olia_discourse.owl#PropositionalConcession_HDRB">
    <rdf:type rdf:resource="http://www.w3.org/2002/07/owl#Class"/>
  </rdf:Description>
  <rdf:Description rdf:about="http://purl.org/olia/discourse/olia_discourse.owl#PropositionalConcession_HDRB">
    <rdfs:subClassOf rdf:resource="http://purl.org/olia/discourse/olia_discourse.owl#PragmaticConcession_HDRB"/>
  </rdf:Description>
  <rdf:Description rdf:about="http://purl.org/olia/discourse/olia_discourse.owl#PropositionalConcession_HDRB">
    <rdfs:comment>Suggested as an extension of the PDTB scheme by Oza et al. (2009) and Tonelli et al. (2010).

Each pragmatic sense at the type level is
further distinguished into three subtypes: “epis-
temic” (Sweetser 1990), “speech-act” (Sweetser
1990), and “propositional”. The propositional
subtype involves the inference of a complete
proposition. The relation is then taken to hold
between this inferred proposition and the propo-
sitional content of one of the arguments.
(Oza et al. 2009)</rdfs:comment>
  </rdf:Description>
  <rdf:Description rdf:about="http://purl.org/olia/discourse/olia_discourse.owl#PropositionalConcession_HDRB">
    <rdfs:label xml:lang="en">propositional concession (HDRB)</rdfs:label>
  </rdf:Description>
  <rdf:Description rdf:about="http://purl.org/olia/discourse/olia_discourse.owl#PropositionalCondition_HDRB">
    <rdf:type rdf:resource="http://www.w3.org/2002/07/owl#Class"/>
  </rdf:Description>
  <rdf:Description rdf:about="http://purl.org/olia/discourse/olia_discourse.owl#PropositionalCondition_HDRB">
    <rdfs:subClassOf rdf:resource="http://purl.org/olia/discourse/olia_discourse.owl#PragmaticCondition"/>
  </rdf:Description>
  <rdf:Description rdf:about="http://purl.org/olia/discourse/olia_discourse.owl#PropositionalCondition_HDRB">
    <rdfs:comment>An extension of the PDTB scheme suggested by Oza et al. (2009).

Each pragmatic sense at the type level is
further distinguished into three subtypes: “epis-
temic” (Sweetser 1990), “speech-act” (Sweetser
1990), and “propositional”. The propositional
subtype involves the inference of a complete
proposition. The relation is then taken to hold
between this inferred proposition and the propo-
sitional content of one of the arguments.
(Oza et al. 2009)</rdfs:comment>
  </rdf:Description>
  <rdf:Description rdf:about="http://purl.org/olia/discourse/olia_discourse.owl#PropositionalCondition_HDRB">
    <rdfs:label xml:lang="en">propositional condition (HDRB)</rdfs:label>
  </rdf:Description>
  <rdf:Description rdf:about="http://purl.org/olia/discourse/olia_discourse.owl#PropositionalContrast_HDRB">
    <rdf:type rdf:resource="http://www.w3.org/2002/07/owl#Class"/>
  </rdf:Description>
  <rdf:Description rdf:about="http://purl.org/olia/discourse/olia_discourse.owl#PropositionalContrast_HDRB">
    <rdfs:subClassOf rdf:resource="http://purl.org/olia/discourse/olia_discourse.owl#PragmaticContrast_PDTB"/>
  </rdf:Description>
  <rdf:Description rdf:about="http://purl.org/olia/discourse/olia_discourse.owl#PropositionalContrast_HDRB">
    <rdfs:comment>Suggested as an extension of the PDTB scheme by Oza et al. (2009).

Each pragmatic sense at the type level is
further distinguished into three subtypes: “epis-
temic” (Sweetser 1990), “speech-act” (Sweetser
1990), and “propositional”. The propositional
subtype involves the inference of a complete
proposition. The relation is then taken to hold
between this inferred proposition and the propo-
sitional content of one of the arguments.
(Oza et al. 2009)</rdfs:comment>
  </rdf:Description>
  <rdf:Description rdf:about="http://purl.org/olia/discourse/olia_discourse.owl#PropositionalContrast_HDRB">
    <rdfs:label xml:lang="en">propositional contrast (HDRB)</rdfs:label>
  </rdf:Description>
  <rdf:Description rdf:about="http://purl.org/olia/discourse/olia_discourse.owl#PropositionalFactuality">
    <rdf:type rdf:resource="http://www.w3.org/2002/07/owl#Class"/>
  </rdf:Description>
  <rdf:Description rdf:about="http://purl.org/olia/discourse/olia_discourse.owl#PropositionalFactuality">
    <rdfs:subClassOf rdf:resource="http://purl.org/olia/discourse/olia_discourse.owl#Factuality"/>
  </rdf:Description>
  <rdf:Description rdf:about="http://purl.org/olia/discourse/olia_discourse.owl#PropositionalFactuality">
    <rdfs:comment>Proposition AOs involve attribution to an agent of his/her commitment towards the truth of a proposition. A further distinction captures differences in the degree of that commitment, by distinguishing between “assertions” and “beliefs”.
(Prasad et al. 2007, PDTB)</rdfs:comment>
  </rdf:Description>
  <rdf:Description rdf:about="http://purl.org/olia/discourse/olia_discourse.owl#PropositionalFactuality">
    <rdfs:label>proposition</rdfs:label>
  </rdf:Description>
  <rdf:Description rdf:about="http://purl.org/olia/discourse/olia_discourse.owl#PropositionalFactuality">
    <rdfs:label xml:lang="en">propositional factuality</rdfs:label>
  </rdf:Description>
  <rdf:Description rdf:about="http://purl.org/olia/discourse/olia_discourse.owl#Proverb">
    <rdf:type rdf:resource="http://www.w3.org/2002/07/owl#Class"/>
  </rdf:Description>
  <rdf:Description rdf:about="http://purl.org/olia/discourse/olia_discourse.owl#Proverb">
    <rdfs:subClassOf rdf:resource="http://purl.org/olia/discourse/olia_discourse.owl#LexicalUnit"/>
  </rdf:Description>
  <rdf:Description rdf:about="http://purl.org/olia/discourse/olia_discourse.owl#Proverb">
    <rdfs:subClassOf rdf:resource="http://purl.org/olia/discourse/olia_discourse.owl#Utterance"/>
  </rdf:Description>
  <rdf:Description rdf:about="http://purl.org/olia/discourse/olia_discourse.owl#Proverb">
    <rdfs:comment>A brief popular axiom or saying. (Sue Ellen Wright, http://www.isocat.org/datcat/DC-353)</rdfs:comment>
  </rdf:Description>
  <rdf:Description rdf:about="http://purl.org/olia/discourse/olia_discourse.owl#Proverb">
    <owl:versionInfo>http://www.isocat.org/datcat/DC-353</owl:versionInfo>
  </rdf:Description>
  <rdf:Description rdf:about="http://purl.org/olia/discourse/olia_discourse.owl#Purpose-s_SemDok">
    <rdf:type rdf:resource="http://www.w3.org/2002/07/owl#Class"/>
  </rdf:Description>
  <rdf:Description rdf:about="http://purl.org/olia/discourse/olia_discourse.owl#Purpose-s_SemDok">
    <rdfs:subClassOf rdf:resource="http://purl.org/olia/discourse/olia_discourse.owl#HypotacticDiscourseRelation"/>
  </rdf:Description>
  <rdf:Description rdf:about="http://purl.org/olia/discourse/olia_discourse.owl#Purpose-s_SemDok">
    <rdfs:subClassOf rdf:resource="http://purl.org/olia/discourse/olia_discourse.owl#Reason"/>
  </rdf:Description>
  <rdf:Description rdf:about="http://purl.org/olia/discourse/olia_discourse.owl#Purpose-s_SemDok">
    <rdfs:comment>SemDok Purpose-s (Purpose Satellite?)</rdfs:comment>
  </rdf:Description>
  <rdf:Description rdf:about="http://purl.org/olia/discourse/olia_discourse.owl#Purpose-s_SemDok">
    <rdfs:label>purpose-s</rdfs:label>
  </rdf:Description>
  <rdf:Description rdf:about="http://purl.org/olia/discourse/olia_discourse.owl#Purpose-s_SemDok">
    <rdfs:label xml:lang="en">purpose-s (SemDok)</rdfs:label>
  </rdf:Description>
  <rdf:Description rdf:about="http://purl.org/olia/discourse/olia_discourse.owl#Purpose_RST">
    <rdf:type rdf:resource="http://www.w3.org/2002/07/owl#Class"/>
  </rdf:Description>
  <rdf:Description rdf:about="http://purl.org/olia/discourse/olia_discourse.owl#Purpose_RST">
    <rdfs:subClassOf rdf:resource="http://purl.org/olia/discourse/olia_discourse.owl#Goal"/>
  </rdf:Description>
  <rdf:Description rdf:about="http://purl.org/olia/discourse/olia_discourse.owl#Purpose_RST">
    <rdfs:subClassOf rdf:resource="http://purl.org/olia/discourse/olia_discourse.owl#HypotacticDiscourseRelation"/>
  </rdf:Description>
  <rdf:Description rdf:about="http://purl.org/olia/discourse/olia_discourse.owl#Purpose_RST">
    <rdfs:comment>The situation presented in the satellite of a purpose relation is only putative, i.e., it is yet to be achieved. Most often it can be paraphrased as “in order to”. (Carlson and Marcu 2001)

cf. SemDok Purpose-n</rdfs:comment>
  </rdf:Description>
  <rdf:Description rdf:about="http://purl.org/olia/discourse/olia_discourse.owl#Purpose_RST">
    <rdfs:label>purpose</rdfs:label>
  </rdf:Description>
  <rdf:Description rdf:about="http://purl.org/olia/discourse/olia_discourse.owl#Purpose_RST">
    <rdfs:label xml:lang="en">purpose (RST)</rdfs:label>
  </rdf:Description>
  <rdf:Description rdf:about="http://purl.org/olia/discourse/olia_discourse.owl#Purpose_RST">
    <rdfs:label>purpose-n</rdfs:label>
  </rdf:Description>
  <rdf:Description rdf:about="http://purl.org/olia/discourse/olia_discourse.owl#Purpose_RST">
    <skos:prefLabel>purpose (RST)</skos:prefLabel>
  </rdf:Description>
  <rdf:Description rdf:about="http://purl.org/olia/discourse/olia_discourse.owl#QuestionAnswer_RST">
    <rdf:type rdf:resource="http://www.w3.org/2002/07/owl#Class"/>
  </rdf:Description>
  <rdf:Description rdf:about="http://purl.org/olia/discourse/olia_discourse.owl#QuestionAnswer_RST">
    <rdfs:subClassOf rdf:resource="http://purl.org/olia/discourse/olia_discourse.owl#SolicitedResponse"/>
  </rdf:Description>
  <rdf:Description rdf:about="http://purl.org/olia/discourse/olia_discourse.owl#QuestionAnswer_RST">
    <rdfs:comment>In a question-answer relation, one textual span poses a question (not necessarily realized as an interrogative sentence), and the other text span answers the question. The relation may be mononuclear or multinuclear, depending on the context.
(Carlson and Marcu 2001)</rdfs:comment>
  </rdf:Description>
  <rdf:Description rdf:about="http://purl.org/olia/discourse/olia_discourse.owl#QuestionAnswer_RST">
    <rdfs:label xml:lang="en">question answer (RST)</rdfs:label>
  </rdf:Description>
  <rdf:Description rdf:about="http://purl.org/olia/discourse/olia_discourse.owl#QuestionAnswer_RST">
    <owl:versionInfo>TODO: merge with SolicitedResponse</owl:versionInfo>
  </rdf:Description>
  <rdf:Description rdf:about="http://purl.org/olia/discourse/olia_discourse.owl#RadioProgram">
    <rdf:type rdf:resource="http://www.w3.org/2002/07/owl#Class"/>
  </rdf:Description>
  <rdf:Description rdf:about="http://purl.org/olia/discourse/olia_discourse.owl#RadioProgram">
    <rdfs:subClassOf rdf:resource="http://purl.org/olia/discourse/olia_discourse.owl#MediaProduct"/>
  </rdf:Description>
  <rdf:Description rdf:about="http://purl.org/olia/discourse/olia_discourse.owl#RadioProgram">
    <rdfs:comment xml:lang="en">for nerd:RadioProgram sub nerd:Product</rdfs:comment>
  </rdf:Description>
  <rdf:Description rdf:about="http://purl.org/olia/discourse/olia_discourse.owl#RadioStation">
    <rdf:type rdf:resource="http://www.w3.org/2002/07/owl#Class"/>
  </rdf:Description>
  <rdf:Description rdf:about="http://purl.org/olia/discourse/olia_discourse.owl#RadioStation">
    <rdfs:subClassOf rdf:resource="http://purl.org/olia/discourse/olia_discourse.owl#BroadcastingOrganization"/>
  </rdf:Description>
  <rdf:Description rdf:about="http://purl.org/olia/discourse/olia_discourse.owl#RadioStation">
    <rdfs:comment xml:lang="en">for nerd:RadioStation sub nerd:Organization</rdfs:comment>
  </rdf:Description>
  <rdf:Description rdf:about="http://purl.org/olia/discourse/olia_discourse.owl#RarelyUsed">
    <rdf:type rdf:resource="http://www.w3.org/2002/07/owl#Class"/>
  </rdf:Description>
  <rdf:Description rdf:about="http://purl.org/olia/discourse/olia_discourse.owl#RarelyUsed">
    <rdfs:subClassOf rdf:resource="http://purl.org/olia/discourse/olia_discourse.owl#Possible"/>
  </rdf:Description>
  <rdf:Description rdf:about="http://purl.org/olia/discourse/olia_discourse.owl#RarelyUsed">
    <rdfs:comment>
                            Said of a term that is almost never used.
                                (ISO12620; http://www.isocat.org/datcat/DC-1986)
                            </rdfs:comment>
  </rdf:Description>
  <rdf:Description rdf:about="http://purl.org/olia/discourse/olia_discourse.owl#RarelyUsed">
    <rdfs:label>rarely used</rdfs:label>
  </rdf:Description>
  <rdf:Description rdf:about="http://purl.org/olia/discourse/olia_discourse.owl#RarelyUsed">
    <owl:versionInfo>http://www.isocat.org/datcat/DC-1986</owl:versionInfo>
  </rdf:Description>
  <rdf:Description rdf:about="http://purl.org/olia/discourse/olia_discourse.owl#RarelyUsed">
    <owl:versionInfo>subClassOf frequency (dcif:conceptualDomain)</owl:versionInfo>
  </rdf:Description>
  <rdf:Description rdf:about="http://purl.org/olia/discourse/olia_discourse.owl#Reason">
    <rdf:type rdf:resource="http://www.w3.org/2002/07/owl#Class"/>
  </rdf:Description>
  <rdf:Description rdf:about="http://purl.org/olia/discourse/olia_discourse.owl#Reason">
    <rdfs:subClassOf rdf:resource="http://purl.org/olia/discourse/olia_discourse.owl#SemanticCause"/>
  </rdf:Description>
  <rdf:Description rdf:about="http://purl.org/olia/discourse/olia_discourse.owl#Reason">
    <rdfs:comment>PDTB Reason. This is introduced as a generalization over RST Reason because it does not come with assumptions about nuclearity.</rdfs:comment>
  </rdf:Description>
  <rdf:Description rdf:about="http://purl.org/olia/discourse/olia_discourse.owl#Reason">
    <rdfs:label xml:lang="en">reason</rdfs:label>
  </rdf:Description>
  <rdf:Description rdf:about="http://purl.org/olia/discourse/olia_discourse.owl#Reason">
    <skos:prefLabel>reason</skos:prefLabel>
  </rdf:Description>
  <rdf:Description rdf:about="http://purl.org/olia/discourse/olia_discourse.owl#Reason_RST">
    <rdf:type rdf:resource="http://www.w3.org/2002/07/owl#Class"/>
  </rdf:Description>
  <rdf:Description rdf:about="http://purl.org/olia/discourse/olia_discourse.owl#Reason_RST">
    <rdfs:subClassOf rdf:resource="http://purl.org/olia/discourse/olia_discourse.owl#HypotacticDiscourseRelation"/>
  </rdf:Description>
  <rdf:Description rdf:about="http://purl.org/olia/discourse/olia_discourse.owl#Reason_RST">
    <rdfs:subClassOf rdf:resource="http://purl.org/olia/discourse/olia_discourse.owl#Reason"/>
  </rdf:Description>
  <rdf:Description rdf:about="http://purl.org/olia/discourse/olia_discourse.owl#Reason_RST">
    <rdfs:comment>The nucleus must be an action carried out by an animate agent. Only animate agents can have reasons for performing actions. You can paraphrase it as “Satellite is the reason for Nucleus.” (Carlson and Marcu 2001)</rdfs:comment>
  </rdf:Description>
  <rdf:Description rdf:about="http://purl.org/olia/discourse/olia_discourse.owl#Reason_RST">
    <rdfs:label xml:lang="en">reason (RST)</rdfs:label>
  </rdf:Description>
  <rdf:Description rdf:about="http://purl.org/olia/discourse/olia_discourse.owl#Referentiality">
    <rdf:type rdf:resource="http://www.w3.org/2002/07/owl#Class"/>
  </rdf:Description>
  <rdf:Description rdf:about="http://purl.org/olia/discourse/olia_discourse.owl#Referentiality">
    <rdfs:subClassOf rdf:resource="http://purl.org/olia/discourse/olia_discourse.owl#SemanticFeature"/>
  </rdf:Description>
  <rdf:Description rdf:about="http://purl.org/olia/discourse/olia_discourse.owl#Referentiality">
    <rdfs:label xml:lang="en">referentiality</rdfs:label>
  </rdf:Description>
  <rdf:Description rdf:about="http://purl.org/olia/discourse/olia_discourse.owl#Referring">
    <rdf:type rdf:resource="http://www.w3.org/2002/07/owl#Class"/>
  </rdf:Description>
  <rdf:Description rdf:about="http://purl.org/olia/discourse/olia_discourse.owl#Referring">
    <rdfs:subClassOf rdf:resource="http://purl.org/olia/discourse/olia_discourse.owl#Referentiality"/>
  </rdf:Description>
  <rdf:Description rdf:about="http://purl.org/olia/discourse/olia_discourse.owl#Referring">
    <rdfs:label xml:lang="en">referring</rdfs:label>
  </rdf:Description>
  <rdf:Description rdf:about="http://purl.org/olia/discourse/olia_discourse.owl#ReferringExpression">
    <rdf:type rdf:resource="http://www.w3.org/2002/07/owl#Class"/>
  </rdf:Description>
  <rdf:Description rdf:nodeID="genid58">
    <rdf:type rdf:resource="http://www.w3.org/2002/07/owl#Restriction"/>
  </rdf:Description>
  <rdf:Description rdf:nodeID="genid58">
    <owl:onProperty rdf:resource="http://purl.org/olia/discourse/olia_discourse.owl#denotates"/>
  </rdf:Description>
  <rdf:Description rdf:nodeID="genid58">
    <owl:allValuesFrom rdf:resource="http://purl.org/olia/discourse/olia_discourse.owl#DiscourseReferent"/>
  </rdf:Description>
  <rdf:Description rdf:about="http://purl.org/olia/discourse/olia_discourse.owl#ReferringExpression">
    <owl:equivalentClass rdf:nodeID="genid58"/>
  </rdf:Description>
  <rdf:Description rdf:about="http://purl.org/olia/discourse/olia_discourse.owl#ReferringExpression">
    <rdfs:subClassOf rdf:resource="http://purl.org/olia/discourse/olia_discourse.owl#Markable"/>
  </rdf:Description>
  <rdf:Description rdf:about="http://purl.org/olia/discourse/olia_discourse.owl#ReferringExpression">
    <rdfs:label xml:lang="en">referring expression</rdfs:label>
  </rdf:Description>
  <rdf:Description rdf:about="http://purl.org/olia/discourse/olia_discourse.owl#RelationCue">
    <rdf:type rdf:resource="http://www.w3.org/2002/07/owl#Class"/>
  </rdf:Description>
  <rdf:Description rdf:about="http://purl.org/olia/discourse/olia_discourse.owl#RelationCue">
    <rdfs:subClassOf rdf:resource="http://purl.org/olia/system.owl#UnitOfAnnotation"/>
  </rdf:Description>
  <rdf:Description rdf:about="http://purl.org/olia/discourse/olia_discourse.owl#RelationCue">
    <rdfs:comment>In PDTB, Relations are organized according to their structural type (material manifestation). To avoid a terminological clash, these are referred to as RelationCue here.

EntityRelations, however, do not represent a RelationCue as they are not physically materialized, but need to be inferred.</rdfs:comment>
  </rdf:Description>
  <rdf:Description rdf:about="http://purl.org/olia/discourse/olia_discourse.owl#RelationCue">
    <rdfs:comment>relation (PDTB)</rdfs:comment>
  </rdf:Description>
  <rdf:Description rdf:about="http://purl.org/olia/discourse/olia_discourse.owl#RelationCue">
    <rdfs:label>cue word</rdfs:label>
  </rdf:Description>
  <rdf:Description rdf:about="http://purl.org/olia/discourse/olia_discourse.owl#RelationCue">
    <rdfs:label>discourse marker</rdfs:label>
  </rdf:Description>
  <rdf:Description rdf:about="http://purl.org/olia/discourse/olia_discourse.owl#RelationCue">
    <rdfs:label xml:lang="en">relation cue</rdfs:label>
  </rdf:Description>
  <rdf:Description rdf:about="http://purl.org/olia/discourse/olia_discourse.owl#RelationCue">
    <rdfs:seeAlso>semdoc:DiscourseMarker</rdfs:seeAlso>
  </rdf:Description>
  <rdf:Description rdf:about="http://purl.org/olia/discourse/olia_discourse.owl#RelevanceConditional_PDTB">
    <rdf:type rdf:resource="http://www.w3.org/2002/07/owl#Class"/>
  </rdf:Description>
  <rdf:Description rdf:about="http://purl.org/olia/discourse/olia_discourse.owl#RelevanceConditional_PDTB">
    <rdfs:subClassOf rdf:resource="http://purl.org/olia/discourse/olia_discourse.owl#PragmaticCondition"/>
  </rdf:Description>
  <rdf:Description rdf:about="http://purl.org/olia/discourse/olia_discourse.owl#RelevanceConditional_PDTB">
    <rdfs:comment>The conditional clause in the “relevance” conditional (Arg2) provides the context in which the description of the situation in Arg1 is relevant. There is no causal relation between the two arguments. (Prasad et al. 2007)</rdfs:comment>
  </rdf:Description>
  <rdf:Description rdf:about="http://purl.org/olia/discourse/olia_discourse.owl#RelevanceConditional_PDTB">
    <rdfs:label xml:lang="en">relevance conditional (PDTB)</rdfs:label>
  </rdf:Description>
  <rdf:Description rdf:about="http://purl.org/olia/discourse/olia_discourse.owl#RequestForComment">
    <rdf:type rdf:resource="http://www.w3.org/2002/07/owl#Class"/>
  </rdf:Description>
  <rdf:Description rdf:about="http://purl.org/olia/discourse/olia_discourse.owl#RequestForComment">
    <rdfs:subClassOf rdf:resource="http://purl.org/olia/discourse/olia_discourse.owl#SolicitedResponse"/>
  </rdf:Description>
  <rdf:Description rdf:about="http://purl.org/olia/discourse/olia_discourse.owl#RequestForComment">
    <inverseOf rdf:resource="http://purl.org/olia/discourse/ResponseAct"/>
  </rdf:Description>
  <rdf:Description rdf:about="http://purl.org/olia/discourse/olia_discourse.owl#RequestForComment">
    <rdfs:comment>Mononuclear solicited response relation that links the antecedent act, e.g., a question, to the dependent act, i.e., the response. The nucleus is the response.

Corresponds to ISO Functional Dependency with argument role "anteceent act".</rdfs:comment>
  </rdf:Description>
  <rdf:Description rdf:about="http://purl.org/olia/discourse/olia_discourse.owl#RequestForComment">
    <rdfs:label>antecedent act</rdfs:label>
  </rdf:Description>
  <rdf:Description rdf:about="http://purl.org/olia/discourse/olia_discourse.owl#RequestForComment">
    <rdfs:label>question</rdfs:label>
  </rdf:Description>
  <rdf:Description rdf:about="http://purl.org/olia/discourse/olia_discourse.owl#RequestForComment">
    <rdfs:label xml:lang="en">request for comment</rdfs:label>
  </rdf:Description>
  <rdf:Description rdf:about="http://purl.org/olia/discourse/olia_discourse.owl#RequestForComment">
    <skos:prefLabel>request for comment</skos:prefLabel>
  </rdf:Description>
  <rdf:Description rdf:about="http://purl.org/olia/discourse/olia_discourse.owl#ResponseAct">
    <rdf:type rdf:resource="http://www.w3.org/2002/07/owl#Class"/>
  </rdf:Description>
  <rdf:Description rdf:about="http://purl.org/olia/discourse/olia_discourse.owl#ResponseAct">
    <rdfs:subClassOf rdf:resource="http://purl.org/olia/discourse/olia_discourse.owl#SolicitedResponse"/>
  </rdf:Description>
  <rdf:Description rdf:about="http://purl.org/olia/discourse/olia_discourse.owl#ResponseAct">
    <inverseOf rdf:resource="http://purl.org/olia/discourse/RequestForComment"/>
  </rdf:Description>
  <rdf:Description rdf:about="http://purl.org/olia/discourse/olia_discourse.owl#ResponseAct">
    <rdfs:comment>Mononuclear solicited response relation that links the dependent act, e.g., an answer or another response act, to the antececent act, e.g., a question. The nucleus is the antecedent act.

Corresponds to ISO Functional Dependency with argument role "dependent act".</rdfs:comment>
  </rdf:Description>
  <rdf:Description rdf:about="http://purl.org/olia/discourse/olia_discourse.owl#ResponseAct">
    <rdfs:label>answer</rdfs:label>
  </rdf:Description>
  <rdf:Description rdf:about="http://purl.org/olia/discourse/olia_discourse.owl#ResponseAct">
    <rdfs:label>dependent act</rdfs:label>
  </rdf:Description>
  <rdf:Description rdf:about="http://purl.org/olia/discourse/olia_discourse.owl#ResponseAct">
    <rdfs:label>response</rdfs:label>
  </rdf:Description>
  <rdf:Description rdf:about="http://purl.org/olia/discourse/olia_discourse.owl#ResponseAct">
    <rdfs:label xml:lang="en">response act</rdfs:label>
  </rdf:Description>
  <rdf:Description rdf:about="http://purl.org/olia/discourse/olia_discourse.owl#ResponseAct">
    <skos:prefLabel>response act</skos:prefLabel>
  </rdf:Description>
  <rdf:Description rdf:about="http://purl.org/olia/discourse/olia_discourse.owl#Restatement">
    <rdf:type rdf:resource="http://www.w3.org/2002/07/owl#Class"/>
  </rdf:Description>
  <rdf:Description rdf:about="http://purl.org/olia/discourse/olia_discourse.owl#Restatement">
    <rdfs:subClassOf rdf:resource="http://purl.org/olia/discourse/olia_discourse.owl#Expansion"/>
  </rdf:Description>
  <rdf:Description rdf:about="http://purl.org/olia/discourse/olia_discourse.owl#Restatement">
    <rdfs:comment>The semantics of Arg2 restates the semantics of Arg1. It is inferred that the situations described in Arg1 and Arg2 hold true at the same time. (Prasad et al. 2007)
An item is primarily a reexpression of one linked to it (Mann and Taboada 2010).
cf. Al-Saif and Markert (2010) "Reformulation" in the LADTB corpus</rdfs:comment>
  </rdf:Description>
  <rdf:Description rdf:about="http://purl.org/olia/discourse/olia_discourse.owl#Restatement">
    <rdfs:label xml:lang="en">restatement</rdfs:label>
  </rdf:Description>
  <rdf:Description rdf:about="http://purl.org/olia/discourse/olia_discourse.owl#Restatement">
    <rdfs:label>Reformulation (LADTB)</rdfs:label>
  </rdf:Description>
  <rdf:Description rdf:about="http://purl.org/olia/discourse/olia_discourse.owl#Restaurant">
    <rdf:type rdf:resource="http://www.w3.org/2002/07/owl#Class"/>
  </rdf:Description>
  <rdf:Description rdf:about="http://purl.org/olia/discourse/olia_discourse.owl#Restaurant">
    <rdfs:subClassOf rdf:resource="http://purl.org/olia/discourse/olia_discourse.owl#ArchitecturalFeature"/>
  </rdf:Description>
  <rdf:Description rdf:about="http://purl.org/olia/discourse/olia_discourse.owl#Restaurant">
    <rdfs:comment xml:lang="en">for nerd:Restaurant</rdfs:comment>
  </rdf:Description>
  <rdf:Description rdf:about="http://purl.org/olia/discourse/olia_discourse.owl#Result">
    <rdf:type rdf:resource="http://www.w3.org/2002/07/owl#Class"/>
  </rdf:Description>
  <rdf:Description rdf:about="http://purl.org/olia/discourse/olia_discourse.owl#Result">
    <rdfs:subClassOf rdf:resource="http://purl.org/olia/discourse/olia_discourse.owl#Cause"/>
  </rdf:Description>
  <rdf:Description rdf:about="http://purl.org/olia/discourse/olia_discourse.owl#Result">
    <rdfs:comment>Result corresponds to ISO Cause with argument Result.
Note that the other argument can be either a pragmatic cause (Justification) or a semantic cause (Reason), so we expect the difference between different kinds of causes to be expressed in the cause argument.

PDTB Result, also generalizes over RST Result, but doesn't come with constraints on nuclearity.

Corresponds to SemDoc ResultPurpose</rdfs:comment>
  </rdf:Description>
  <rdf:Description rdf:about="http://purl.org/olia/discourse/olia_discourse.owl#Result">
    <rdfs:label xml:lang="en">result</rdfs:label>
  </rdf:Description>
  <rdf:Description rdf:about="http://purl.org/olia/discourse/olia_discourse.owl#Result">
    <rdfs:label>result/purpose</rdfs:label>
  </rdf:Description>
  <rdf:Description rdf:about="http://purl.org/olia/discourse/olia_discourse.owl#Result">
    <skos:prefLabel>result</skos:prefLabel>
  </rdf:Description>
  <rdf:Description rdf:about="http://purl.org/olia/discourse/olia_discourse.owl#Result_RST">
    <rdf:type rdf:resource="http://www.w3.org/2002/07/owl#Class"/>
  </rdf:Description>
  <rdf:Description rdf:about="http://purl.org/olia/discourse/olia_discourse.owl#Result_RST">
    <rdfs:subClassOf rdf:resource="http://purl.org/olia/discourse/olia_discourse.owl#HypotacticDiscourseRelation"/>
  </rdf:Description>
  <rdf:Description rdf:about="http://purl.org/olia/discourse/olia_discourse.owl#Result_RST">
    <rdfs:subClassOf rdf:resource="http://purl.org/olia/discourse/olia_discourse.owl#Result"/>
  </rdf:Description>
  <rdf:Description rdf:about="http://purl.org/olia/discourse/olia_discourse.owl#Result_RST">
    <rdfs:comment>The situation presented in the satellite is the cause of the situation presented in the nucleus. The result, which is the nucleus, is the most important part. Without presenting the satellite, the reader may not know what caused the result in the nucleus. In contrast to a PURPOSE relation, the situation presented in the nucleus of a result relation is factual, i.e., it is achieved. The
intention of the writer is to emphasize the result.
(Carlson and Marcu 2001)

cf. SemDok Result.</rdfs:comment>
  </rdf:Description>
  <rdf:Description rdf:about="http://purl.org/olia/discourse/olia_discourse.owl#Result_RST">
    <rdfs:label>result</rdfs:label>
  </rdf:Description>
  <rdf:Description rdf:about="http://purl.org/olia/discourse/olia_discourse.owl#Result_RST">
    <rdfs:label xml:lang="en">result (RST)</rdfs:label>
  </rdf:Description>
  <rdf:Description rdf:about="http://purl.org/olia/discourse/olia_discourse.owl#Result_RST">
    <skos:prefLabel>result (RST)</skos:prefLabel>
  </rdf:Description>
  <rdf:Description rdf:about="http://purl.org/olia/discourse/olia_discourse.owl#RhetoricalQuestion_RST">
    <rdf:type rdf:resource="http://www.w3.org/2002/07/owl#Class"/>
  </rdf:Description>
  <rdf:Description rdf:about="http://purl.org/olia/discourse/olia_discourse.owl#RhetoricalQuestion_RST">
    <rdfs:subClassOf rdf:resource="http://purl.org/olia/discourse/olia_discourse.owl#RequestForComment"/>
  </rdf:Description>
  <rdf:Description rdf:about="http://purl.org/olia/discourse/olia_discourse.owl#RhetoricalQuestion_RST">
    <rdfs:comment>In a RHETORICAL-QUESTION relation, the satellite poses a question vis-a-vis a segment of the text; the intention of the author is usually not to answer it, but rather, to raise an issue for the reader to consider, or to raise an issue for which the answer should be obvious.
(Carlson and Marcu 2001)</rdfs:comment>
  </rdf:Description>
  <rdf:Description rdf:about="http://purl.org/olia/discourse/olia_discourse.owl#RhetoricalQuestion_RST">
    <rdfs:label xml:lang="en">rhetorical question (RST)</rdfs:label>
  </rdf:Description>
  <rdf:Description rdf:about="http://purl.org/olia/discourse/olia_discourse.owl#River">
    <rdf:type rdf:resource="http://www.w3.org/2002/07/owl#Class"/>
  </rdf:Description>
  <rdf:Description rdf:about="http://purl.org/olia/discourse/olia_discourse.owl#River">
    <rdfs:subClassOf rdf:resource="http://purl.org/olia/discourse/olia_discourse.owl#GeographicalFeature"/>
  </rdf:Description>
  <rdf:Description rdf:about="http://purl.org/olia/discourse/olia_discourse.owl#River">
    <rdfs:comment xml:lang="en">for nerd:River</rdfs:comment>
  </rdf:Description>
  <rdf:Description rdf:about="http://purl.org/olia/discourse/olia_discourse.owl#Road">
    <rdf:type rdf:resource="http://www.w3.org/2002/07/owl#Class"/>
  </rdf:Description>
  <rdf:Description rdf:about="http://purl.org/olia/discourse/olia_discourse.owl#Road">
    <rdfs:subClassOf rdf:resource="http://purl.org/olia/discourse/olia_discourse.owl#ArchitecturalFeature"/>
  </rdf:Description>
  <rdf:Description rdf:about="http://purl.org/olia/discourse/olia_discourse.owl#Road">
    <rdfs:comment xml:lang="en">for nerd:Road</rdfs:comment>
  </rdf:Description>
  <rdf:Description rdf:about="http://purl.org/olia/discourse/olia_discourse.owl#SameType">
    <rdf:type rdf:resource="http://www.w3.org/2002/07/owl#Class"/>
  </rdf:Description>
  <rdf:Description rdf:about="http://purl.org/olia/discourse/olia_discourse.owl#SameType">
    <rdfs:subClassOf rdf:resource="http://purl.org/olia/discourse/olia_discourse.owl#BridgingType"/>
  </rdf:Description>
  <rdf:Description rdf:about="http://purl.org/olia/discourse/olia_discourse.owl#SameType">
    <rdfs:comment>A referent represents another instantiation of the same type of another pre-mentioned referent. (Stuttgart Guidelines)</rdfs:comment>
  </rdf:Description>
  <rdf:Description rdf:about="http://purl.org/olia/discourse/olia_discourse.owl#SameType">
    <rdfs:label xml:lang="en">same type</rdfs:label>
  </rdf:Description>
  <rdf:Description rdf:about="http://purl.org/olia/discourse/olia_discourse.owl#SameUnit_RST">
    <rdf:type rdf:resource="http://www.w3.org/2002/07/owl#Class"/>
  </rdf:Description>
  <rdf:Description rdf:about="http://purl.org/olia/discourse/olia_discourse.owl#SameUnit_RST">
    <rdfs:subClassOf rdf:resource="http://purl.org/olia/discourse/olia_discourse.owl#TextualOrganizationalRelation"/>
  </rdf:Description>
  <rdf:Description rdf:about="http://purl.org/olia/discourse/olia_discourse.owl#SameUnit_RST">
    <rdfs:comment>cf. SemDok SameSegment</rdfs:comment>
  </rdf:Description>
  <rdf:Description rdf:about="http://purl.org/olia/discourse/olia_discourse.owl#SameUnit_RST">
    <rdfs:comment>A pseudo-relation used as a device for linking two discontinuous text fragments that are really a single EDU, but which are broken up by an embedded unit. Examples of embedded units that can break up other EDUs include: relative clauses, other nominal postmodifiers, parentheticals, participial clauses, etc. By convention, this relation is always multinuclear.
(Carlson and Marcu 2001)

If a DS has intervening material; the “Same” relation is no coherence relation, but
a “trick” that allows dealing with DSs nested in other DSs. (Wolf et al. 2003)</rdfs:comment>
  </rdf:Description>
  <rdf:Description rdf:about="http://purl.org/olia/discourse/olia_discourse.owl#SameUnit_RST">
    <rdfs:label>same segment</rdfs:label>
  </rdf:Description>
  <rdf:Description rdf:about="http://purl.org/olia/discourse/olia_discourse.owl#SameUnit_RST">
    <rdfs:label>same unit</rdfs:label>
  </rdf:Description>
  <rdf:Description rdf:about="http://purl.org/olia/discourse/olia_discourse.owl#SameUnit_RST">
    <rdfs:label xml:lang="en">same unit (RST)</rdfs:label>
  </rdf:Description>
  <rdf:Description rdf:about="http://purl.org/olia/discourse/olia_discourse.owl#SchoolNewspaper">
    <rdf:type rdf:resource="http://www.w3.org/2002/07/owl#Class"/>
  </rdf:Description>
  <rdf:Description rdf:about="http://purl.org/olia/discourse/olia_discourse.owl#SchoolNewspaper">
    <rdfs:subClassOf rdf:resource="http://purl.org/olia/discourse/olia_discourse.owl#Newspaper"/>
  </rdf:Description>
  <rdf:Description rdf:about="http://purl.org/olia/discourse/olia_discourse.owl#SchoolNewspaper">
    <rdfs:comment xml:lang="en">for nerd:SchoolNewspaper, but this is a subclass of nerd:Product</rdfs:comment>
  </rdf:Description>
  <rdf:Description rdf:about="http://purl.org/olia/discourse/olia_discourse.owl#SectionText">
    <rdf:type rdf:resource="http://www.w3.org/2002/07/owl#Class"/>
  </rdf:Description>
  <rdf:Description rdf:about="http://purl.org/olia/discourse/olia_discourse.owl#SectionText">
    <rdfs:subClassOf rdf:resource="http://purl.org/olia/olia-top.owl#TextStructuralUnit"/>
  </rdf:Description>
  <rdf:Description rdf:about="http://purl.org/olia/discourse/olia_discourse.owl#SectionText">
    <rdfs:comment>Often, an article will be broken up structurally into distinct sections represent-
ing different topics. In this case, the schema SectionText is used. Most often, each section will be
labeled, so there will be a corresponding SECTIONTITLE and SECTIONTEXT. (Carlson and Marcu 2001)</rdfs:comment>
  </rdf:Description>
  <rdf:Description rdf:about="http://purl.org/olia/discourse/olia_discourse.owl#SectionText">
    <rdfs:label xml:lang="en">section text</rdfs:label>
  </rdf:Description>
  <rdf:Description rdf:about="http://purl.org/olia/discourse/olia_discourse.owl#SectionTitle">
    <rdf:type rdf:resource="http://www.w3.org/2002/07/owl#Class"/>
  </rdf:Description>
  <rdf:Description rdf:about="http://purl.org/olia/discourse/olia_discourse.owl#SectionTitle">
    <rdfs:subClassOf rdf:resource="http://purl.org/olia/olia-top.owl#TextStructuralUnit"/>
  </rdf:Description>
  <rdf:Description rdf:about="http://purl.org/olia/discourse/olia_discourse.owl#SectionTitle">
    <rdfs:comment>Often, an article will be broken up structurally into distinct sections represent-
ing different topics. Most often, each section will be labeled, so there will be a corresponding
SECTIONTITLE and SECTIONTEXT. Usually, the section title occurs on a separate line. (Carlson and Marcu 2001)</rdfs:comment>
  </rdf:Description>
  <rdf:Description rdf:about="http://purl.org/olia/discourse/olia_discourse.owl#SectionTitle">
    <rdfs:label xml:lang="en">section title</rdfs:label>
  </rdf:Description>
  <rdf:Description rdf:about="http://purl.org/olia/discourse/olia_discourse.owl#SemanticAlternative_LUNA">
    <rdf:type rdf:resource="http://www.w3.org/2002/07/owl#Class"/>
  </rdf:Description>
  <rdf:Description rdf:about="http://purl.org/olia/discourse/olia_discourse.owl#SemanticAlternative_LUNA">
    <rdfs:subClassOf rdf:resource="http://purl.org/olia/discourse/olia_discourse.owl#Alternative"/>
  </rdf:Description>
  <rdf:Description rdf:about="http://purl.org/olia/discourse/olia_discourse.owl#SemanticAlternative_LUNA">
    <rdfs:comment>Sara Tonelli, Giuseppe Riccardi, Rashmi Prasad and Aravind Joshi (2010), Annotation of Discourse Relations for Conversational Spoken Dialogs, Proceedings of the Seventh conference on International Language Resources and Evaluation (LREC'10), May, 19-21, Valletta, Malta</rdfs:comment>
  </rdf:Description>
  <rdf:Description rdf:about="http://purl.org/olia/discourse/olia_discourse.owl#SemanticAlternative_LUNA">
    <rdfs:label xml:lang="en">semantic alternative (LUNA)</rdfs:label>
  </rdf:Description>
  <rdf:Description rdf:about="http://purl.org/olia/discourse/olia_discourse.owl#SemanticCause">
    <rdf:type rdf:resource="http://www.w3.org/2002/07/owl#Class"/>
  </rdf:Description>
  <rdf:Description rdf:about="http://purl.org/olia/discourse/olia_discourse.owl#SemanticCause">
    <rdfs:subClassOf rdf:resource="http://purl.org/olia/discourse/olia_discourse.owl#Cause"/>
  </rdf:Description>
  <rdf:Description rdf:about="http://purl.org/olia/discourse/olia_discourse.owl#SemanticCause">
    <rdfs:comment>The situations described in Arg1 and Arg2 are causally influenced and the two are not in a conditional relation. (Prasad et al. 2007)

PDTB Reason. This is introduced as a generalization over RST Reason because it does not come with assumptions about nuclearity.

The classification of causal relations in RST/RSTDTB and PDTB is hard to be aligneable, further, hence original definitions preserved with suffixed relations

Cf. SemDok CausePurpose (but this is limited to HypotacticDiscourseRelations).</rdfs:comment>
  </rdf:Description>
  <rdf:Description rdf:about="http://purl.org/olia/discourse/olia_discourse.owl#SemanticCause">
    <rdfs:label>cause/purpose</rdfs:label>
  </rdf:Description>
  <rdf:Description rdf:about="http://purl.org/olia/discourse/olia_discourse.owl#SemanticCause">
    <rdfs:label>reason</rdfs:label>
  </rdf:Description>
  <rdf:Description rdf:about="http://purl.org/olia/discourse/olia_discourse.owl#SemanticCause">
    <rdfs:label xml:lang="en">semantic cause</rdfs:label>
  </rdf:Description>
  <rdf:Description rdf:about="http://purl.org/olia/discourse/olia_discourse.owl#SemanticCause">
    <skos:prefLabel>semantic cause</skos:prefLabel>
  </rdf:Description>
  <rdf:Description rdf:about="http://purl.org/olia/discourse/olia_discourse.owl#SemanticConcession_HDRB">
    <rdf:type rdf:resource="http://www.w3.org/2002/07/owl#Class"/>
  </rdf:Description>
  <rdf:Description rdf:about="http://purl.org/olia/discourse/olia_discourse.owl#SemanticConcession_HDRB">
    <rdfs:subClassOf rdf:resource="http://purl.org/olia/discourse/olia_discourse.owl#Concession"/>
  </rdf:Description>
  <rdf:Description rdf:about="http://purl.org/olia/discourse/olia_discourse.owl#SemanticConcession_HDRB">
    <rdfs:comment>Suggested as an extension of the PDTB scheme by Oza et al. (2009) and Tonelli et al. (2010).</rdfs:comment>
  </rdf:Description>
  <rdf:Description rdf:about="http://purl.org/olia/discourse/olia_discourse.owl#SemanticConcession_HDRB">
    <rdfs:label xml:lang="en">semantic concession (HDRB)</rdfs:label>
  </rdf:Description>
  <rdf:Description rdf:about="http://purl.org/olia/discourse/olia_discourse.owl#SemanticCondition">
    <rdf:type rdf:resource="http://www.w3.org/2002/07/owl#Class"/>
  </rdf:Description>
  <rdf:Description rdf:about="http://purl.org/olia/discourse/olia_discourse.owl#SemanticCondition">
    <rdfs:subClassOf rdf:resource="http://purl.org/olia/discourse/olia_discourse.owl#Condition"/>
  </rdf:Description>
  <rdf:Description rdf:about="http://purl.org/olia/discourse/olia_discourse.owl#SemanticCondition">
    <rdfs:comment>The situation in Arg2 is taken to be the condition and the situation described in Arg1 is taken to be the consequence, i.e., the situation that holds when the condition is true. Unlike “Cause”, however, the truth value of the arguments of a “Condition” relation cannot be determined independently of the connective. (Prasad et al. 2007)

In a CONDITION relation, the truth of the proposition associated with the nucleus is a consequence of the fulfillment of the condition in the satellite. The satellite presents a situation that is not realized. (Carlson and Marcu 2001)</rdfs:comment>
  </rdf:Description>
  <rdf:Description rdf:about="http://purl.org/olia/discourse/olia_discourse.owl#SemanticCondition">
    <rdfs:label xml:lang="en">semantic condition</rdfs:label>
  </rdf:Description>
  <rdf:Description rdf:about="http://purl.org/olia/discourse/olia_discourse.owl#SemanticCondition">
    <owl:versionInfo>Identified with RST Condition because of its association with the markers "as long as", "until", and "if", cf. Prasad et al. (2007).</owl:versionInfo>
  </rdf:Description>
  <rdf:Description rdf:about="http://purl.org/olia/discourse/olia_discourse.owl#SemanticConjunction_LUNA">
    <rdf:type rdf:resource="http://www.w3.org/2002/07/owl#Class"/>
  </rdf:Description>
  <rdf:Description rdf:about="http://purl.org/olia/discourse/olia_discourse.owl#SemanticConjunction_LUNA">
    <rdfs:subClassOf rdf:resource="http://purl.org/olia/discourse/olia_discourse.owl#Conjunction"/>
  </rdf:Description>
  <rdf:Description rdf:about="http://purl.org/olia/discourse/olia_discourse.owl#SemanticConjunction_LUNA">
    <rdfs:comment>Sara Tonelli, Giuseppe Riccardi, Rashmi Prasad and Aravind Joshi (2010), Annotation of Discourse Relations for Conversational Spoken Dialogs, Proceedings of the Seventh conference on International Language Resources and Evaluation (LREC'10), May, 19-21, Valletta, Malta</rdfs:comment>
  </rdf:Description>
  <rdf:Description rdf:about="http://purl.org/olia/discourse/olia_discourse.owl#SemanticConjunction_LUNA">
    <rdfs:label xml:lang="en">semantic conjunction (LUNA)</rdfs:label>
  </rdf:Description>
  <rdf:Description rdf:about="http://purl.org/olia/discourse/olia_discourse.owl#SemanticContrast_PDTB">
    <rdf:type rdf:resource="http://www.w3.org/2002/07/owl#Class"/>
  </rdf:Description>
  <rdf:Description rdf:about="http://purl.org/olia/discourse/olia_discourse.owl#SemanticContrast_PDTB">
    <rdfs:subClassOf rdf:resource="http://purl.org/olia/discourse/olia_discourse.owl#Contrast"/>
  </rdf:Description>
  <rdf:Description rdf:about="http://purl.org/olia/discourse/olia_discourse.owl#SemanticContrast_PDTB">
    <rdfs:comment>Arg1 and Arg2 share a predicate or property and a difference is highlighted with respect to the values assigned to the shared property. (Prasad et al. 2007)</rdfs:comment>
  </rdf:Description>
  <rdf:Description rdf:about="http://purl.org/olia/discourse/olia_discourse.owl#SemanticContrast_PDTB">
    <rdfs:label xml:lang="en">semantic contrast (PDTB)</rdfs:label>
  </rdf:Description>
  <rdf:Description rdf:about="http://purl.org/olia/discourse/olia_discourse.owl#SemanticFeature">
    <rdf:type rdf:resource="http://www.w3.org/2002/07/owl#Class"/>
  </rdf:Description>
  <rdf:Description rdf:about="http://purl.org/olia/discourse/olia_discourse.owl#SemanticFeature">
    <rdfs:subClassOf rdf:resource="http://purl.org/olia/system.owl#Feature"/>
  </rdf:Description>
  <rdf:Description rdf:about="http://purl.org/olia/discourse/olia_discourse.owl#SemanticFeature">
    <rdfs:comment>The SemanticFeatures enlisted here are drawn from discourse annotations. These are to move to the Reference Model</rdfs:comment>
  </rdf:Description>
  <rdf:Description rdf:about="http://purl.org/olia/discourse/olia_discourse.owl#SemanticFeature">
    <rdfs:label xml:lang="en">semantic feature</rdfs:label>
  </rdf:Description>
  <rdf:Description rdf:about="http://purl.org/olia/discourse/olia_discourse.owl#SemanticGoal_LUNA">
    <rdf:type rdf:resource="http://www.w3.org/2002/07/owl#Class"/>
  </rdf:Description>
  <rdf:Description rdf:about="http://purl.org/olia/discourse/olia_discourse.owl#SemanticGoal_LUNA">
    <rdfs:subClassOf rdf:resource="http://purl.org/olia/discourse/olia_discourse.owl#Goal_HDRB"/>
  </rdf:Description>
  <rdf:Description rdf:about="http://purl.org/olia/discourse/olia_discourse.owl#SemanticGoal_LUNA">
    <rdfs:comment>Sara Tonelli, Giuseppe Riccardi, Rashmi Prasad and Aravind Joshi (2010), Annotation of Discourse Relations for Conversational Spoken Dialogs, Proceedings of the Seventh conference on International Language Resources and Evaluation (LREC'10), May, 19-21, Valletta, Malta</rdfs:comment>
  </rdf:Description>
  <rdf:Description rdf:about="http://purl.org/olia/discourse/olia_discourse.owl#SemanticGoal_LUNA">
    <rdfs:label xml:lang="en">semantic goal (LUNA)</rdfs:label>
  </rdf:Description>
  <rdf:Description rdf:about="http://purl.org/olia/discourse/olia_discourse.owl#Sentence">
    <rdf:type rdf:resource="http://www.w3.org/2002/07/owl#Class"/>
  </rdf:Description>
  <rdf:Description rdf:about="http://purl.org/olia/discourse/olia_discourse.owl#Sentence">
    <rdfs:subClassOf rdf:resource="http://purl.org/olia/olia-top.owl#TextStructuralUnit"/>
  </rdf:Description>
  <rdf:Description rdf:about="http://purl.org/olia/discourse/olia_discourse.owl#Sentence">
    <rdfs:comment>introduced to account for SemDok SententialDiscourseSegment</rdfs:comment>
  </rdf:Description>
  <rdf:Description rdf:about="http://purl.org/olia/discourse/olia_discourse.owl#Sentence">
    <rdfs:label>sentence</rdfs:label>
  </rdf:Description>
  <rdf:Description rdf:about="http://purl.org/olia/discourse/olia_discourse.owl#Sentence">
    <rdfs:label xml:lang="en">sentence</rdfs:label>
  </rdf:Description>
  <rdf:Description rdf:about="http://purl.org/olia/discourse/olia_discourse.owl#SentenceFocus">
    <rdf:type rdf:resource="http://www.w3.org/2002/07/owl#Class"/>
  </rdf:Description>
  <rdf:Description rdf:about="http://purl.org/olia/discourse/olia_discourse.owl#SentenceFocus">
    <rdfs:subClassOf rdf:resource="http://purl.org/olia/discourse/olia_discourse.owl#WideFocus"/>
  </rdf:Description>
  <rdf:Description rdf:about="http://purl.org/olia/discourse/olia_discourse.owl#SentenceFocus">
    <rdfs:comment>The entire sentence is in focus.</rdfs:comment>
  </rdf:Description>
  <rdf:Description rdf:about="http://purl.org/olia/discourse/olia_discourse.owl#SentenceFocus">
    <rdfs:label xml:lang="en">sentence focus</rdfs:label>
  </rdf:Description>
  <rdf:Description rdf:about="http://purl.org/olia/discourse/olia_discourse.owl#SententialDiscourseSegment">
    <rdf:type rdf:resource="http://www.w3.org/2002/07/owl#Class"/>
  </rdf:Description>
  <rdf:Description rdf:nodeID="genid59">
    <rdf:type rdf:resource="http://www.w3.org/2002/07/owl#Class"/>
  </rdf:Description>
  <rdf:Description rdf:nodeID="genid60">
    <rdf:first rdf:resource="http://purl.org/olia/discourse/olia_discourse.owl#DiscourseSegment"/>
  </rdf:Description>
  <rdf:Description rdf:nodeID="genid61">
    <rdf:first rdf:resource="http://purl.org/olia/discourse/olia_discourse.owl#Sentence"/>
  </rdf:Description>
  <rdf:Description rdf:nodeID="genid60">
    <rdf:rest rdf:nodeID="genid61"/>
  </rdf:Description>
  <rdf:Description rdf:nodeID="genid61">
    <rdf:rest rdf:resource="http://www.w3.org/1999/02/22-rdf-syntax-ns#nil"/>
  </rdf:Description>
  <rdf:Description rdf:nodeID="genid59">
    <owl:intersectionOf rdf:nodeID="genid60"/>
  </rdf:Description>
  <rdf:Description rdf:about="http://purl.org/olia/discourse/olia_discourse.owl#SententialDiscourseSegment">
    <owl:equivalentClass rdf:nodeID="genid59"/>
  </rdf:Description>
  <rdf:Description rdf:about="http://purl.org/olia/discourse/olia_discourse.owl#SententialDiscourseSegment">
    <rdfs:subClassOf rdf:resource="http://purl.org/olia/discourse/olia_discourse.owl#DiscourseSegment"/>
  </rdf:Description>
  <rdf:Description rdf:about="http://purl.org/olia/discourse/olia_discourse.owl#SententialDiscourseSegment">
    <rdfs:subClassOf rdf:resource="http://purl.org/olia/discourse/olia_discourse.owl#Sentence"/>
  </rdf:Description>
  <rdf:Description rdf:about="http://purl.org/olia/discourse/olia_discourse.owl#SententialDiscourseSegment">
    <rdfs:comment>from SemDok

It seems, however, that this conflates aspects of discourse structure with surface syntax, so whether this is a valid segment different from discourse segment or complex discourse segment may be debated.</rdfs:comment>
  </rdf:Description>
  <rdf:Description rdf:about="http://purl.org/olia/discourse/olia_discourse.owl#SententialDiscourseSegment">
    <rdfs:label>sentential discourse segment</rdfs:label>
  </rdf:Description>
  <rdf:Description rdf:about="http://purl.org/olia/discourse/olia_discourse.owl#SententialDiscourseSegment">
    <rdfs:label xml:lang="en">sentential discourse segment</rdfs:label>
  </rdf:Description>
  <rdf:Description rdf:about="http://purl.org/olia/discourse/olia_discourse.owl#Sequence">
    <rdf:type rdf:resource="http://www.w3.org/2002/07/owl#Class"/>
  </rdf:Description>
  <rdf:Description rdf:nodeID="genid62">
    <rdf:type rdf:resource="http://www.w3.org/2002/07/owl#Class"/>
  </rdf:Description>
  <rdf:Description rdf:nodeID="genid63">
    <rdf:first rdf:resource="http://purl.org/olia/discourse/olia_discourse.owl#ListSequence"/>
  </rdf:Description>
  <rdf:Description rdf:nodeID="genid64">
    <rdf:first rdf:resource="http://purl.org/olia/discourse/olia_discourse.owl#PrecedenceRelation"/>
  </rdf:Description>
  <rdf:Description rdf:nodeID="genid63">
    <rdf:rest rdf:nodeID="genid64"/>
  </rdf:Description>
  <rdf:Description rdf:nodeID="genid64">
    <rdf:rest rdf:resource="http://www.w3.org/1999/02/22-rdf-syntax-ns#nil"/>
  </rdf:Description>
  <rdf:Description rdf:nodeID="genid62">
    <owl:intersectionOf rdf:nodeID="genid63"/>
  </rdf:Description>
  <rdf:Description rdf:about="http://purl.org/olia/discourse/olia_discourse.owl#Sequence">
    <owl:equivalentClass rdf:nodeID="genid62"/>
  </rdf:Description>
  <rdf:Description rdf:about="http://purl.org/olia/discourse/olia_discourse.owl#Sequence">
    <rdfs:subClassOf rdf:resource="http://purl.org/olia/discourse/olia_discourse.owl#SubjectMatterRelation"/>
  </rdf:Description>
  <rdf:Description rdf:about="http://purl.org/olia/discourse/olia_discourse.owl#Sequence">
    <rdfs:comment>A SEQUENCE is a multinuclear list of events presented in chronological order. (Carlson and Marcu 2001)
There is a succession relationship between the situations in the nuclei (Mann and Taboada 2010).

cf. SemDok Sequence. We follow SemDok in assuming that the difference between Sequence and List is that a sequence has a natural (i.e., spatio-temporal) order and is thus an ideational (subject-matter) relation, whereas a list has no such order and is thus compiled and organized for a particular purpose, i.e., interpersonal (presentational) in nature. This is a design decision that may be reconsidered.</rdfs:comment>
  </rdf:Description>
  <rdf:Description rdf:about="http://purl.org/olia/discourse/olia_discourse.owl#Sequence">
    <rdfs:label xml:lang="en">sequence</rdfs:label>
  </rdf:Description>
  <rdf:Description rdf:about="http://purl.org/olia/discourse/olia_discourse.owl#Set">
    <rdf:type rdf:resource="http://www.w3.org/2002/07/owl#Class"/>
  </rdf:Description>
  <rdf:Description rdf:about="http://purl.org/olia/discourse/olia_discourse.owl#Set">
    <rdfs:subClassOf rdf:resource="http://purl.org/olia/discourse/olia_discourse.owl#PartWhole"/>
  </rdf:Description>
  <rdf:Description rdf:about="http://purl.org/olia/discourse/olia_discourse.owl#Set">
    <rdfs:comment>The referent denotes a subset or an element of a set mentioned before (Poesio &amp; Artstein 2006).</rdfs:comment>
  </rdf:Description>
  <rdf:Description rdf:about="http://purl.org/olia/discourse/olia_discourse.owl#Set">
    <rdfs:label xml:lang="en">set</rdfs:label>
  </rdf:Description>
  <rdf:Description rdf:about="http://purl.org/olia/discourse/olia_discourse.owl#ShoppingMall">
    <rdf:type rdf:resource="http://www.w3.org/2002/07/owl#Class"/>
  </rdf:Description>
  <rdf:Description rdf:about="http://purl.org/olia/discourse/olia_discourse.owl#ShoppingMall">
    <rdfs:subClassOf rdf:resource="http://purl.org/olia/discourse/olia_discourse.owl#ArchitecturalFeature"/>
  </rdf:Description>
  <rdf:Description rdf:about="http://purl.org/olia/discourse/olia_discourse.owl#ShoppingMall">
    <rdfs:comment xml:lang="en">for nerd:ShoppingMall</rdfs:comment>
  </rdf:Description>
  <rdf:Description rdf:about="http://purl.org/olia/discourse/olia_discourse.owl#SignatureBlock">
    <rdf:type rdf:resource="http://www.w3.org/2002/07/owl#Class"/>
  </rdf:Description>
  <rdf:Description rdf:about="http://purl.org/olia/discourse/olia_discourse.owl#SignatureBlock">
    <rdfs:subClassOf rdf:resource="http://purl.org/olia/olia-top.owl#TextStructuralUnit"/>
  </rdf:Description>
  <rdf:Description rdf:about="http://purl.org/olia/discourse/olia_discourse.owl#SignatureBlock">
    <rdfs:comment>A SIGNATURE-BLOCK is a section of the document that may contain a person’s
name, title and company. If these occur on multiple lines, each line should be treated as a separate
EDU, and all should be linked via a LIST relation before the SIGNATURE-BLOCK label is selected.
This occurs in letters to the editor in the WSJ corpus. This schema is linked to the schema TEXT
(if the entire article is a letter) or SECTIONTEXT (if only a portion of the article is a letter). (Carlson and Marcu 2001)</rdfs:comment>
  </rdf:Description>
  <rdf:Description rdf:about="http://purl.org/olia/discourse/olia_discourse.owl#SignatureBlock">
    <rdfs:label xml:lang="en">signature block</rdfs:label>
  </rdf:Description>
  <rdf:Description rdf:about="http://purl.org/olia/discourse/olia_discourse.owl#Similarity">
    <rdf:type rdf:resource="http://www.w3.org/2002/07/owl#Class"/>
  </rdf:Description>
  <rdf:Description rdf:about="http://purl.org/olia/discourse/olia_discourse.owl#Similarity">
    <rdfs:subClassOf rdf:resource="http://purl.org/olia/discourse/olia_discourse.owl#NonContrastiveComparison"/>
  </rdf:Description>
  <rdf:Description rdf:about="http://purl.org/olia/discourse/olia_discourse.owl#Similarity">
    <rdfs:comment>ISO: Similarity is a symmetric discourse relation in which one or more similarities between Arg1 and Arg2 are highlighted with respect
to what each predicates as a whole or to some entities they mention.

COMPARISON.Similarity applies when the connective indicates that the two arguments express similar abstract objects. It is therefore a complement to the contrast relation.
(Al-Saif and Markert 2010, LADTB)

Also applied in the HDRB (Oza et al. 2009).</rdfs:comment>
  </rdf:Description>
  <rdf:Description rdf:about="http://purl.org/olia/discourse/olia_discourse.owl#Similarity">
    <rdfs:label xml:lang="en">similarity</rdfs:label>
  </rdf:Description>
  <rdf:Description rdf:about="http://purl.org/olia/discourse/olia_discourse.owl#SituationallyAccessible">
    <rdf:type rdf:resource="http://www.w3.org/2002/07/owl#Class"/>
  </rdf:Description>
  <rdf:Description rdf:about="http://purl.org/olia/discourse/olia_discourse.owl#SituationallyAccessible">
    <rdfs:subClassOf rdf:resource="http://purl.org/olia/discourse/olia_discourse.owl#Accessible"/>
  </rdf:Description>
  <rdf:Description rdf:about="http://purl.org/olia/discourse/olia_discourse.owl#SituationallyAccessible">
    <rdfs:comment>A referent is situationally accessible, if it has not been mentioned before, but it is prominent in the given situational environment (Lambrecht 1994, Chafe 1996, cf. Prince 1982 "situationally evoked").</rdfs:comment>
  </rdf:Description>
  <rdf:Description rdf:about="http://purl.org/olia/discourse/olia_discourse.owl#SituationallyAccessible">
    <rdfs:label xml:lang="en">situationally accessible</rdfs:label>
  </rdf:Description>
  <rdf:Description rdf:about="http://purl.org/olia/discourse/olia_discourse.owl#SlangRegister">
    <rdf:type rdf:resource="http://www.w3.org/2002/07/owl#Class"/>
  </rdf:Description>
  <rdf:Description rdf:about="http://purl.org/olia/discourse/olia_discourse.owl#SlangRegister">
    <rdfs:subClassOf rdf:resource="http://purl.org/olia/olia-top.owl#RegisterFeature"/>
  </rdf:Description>
  <rdf:Description rdf:about="http://purl.org/olia/discourse/olia_discourse.owl#SlangRegister">
    <rdfs:comment>
                            An extremely informal register of a word, term, or text that is used in spoken and everyday language and less commonly in documents.
                                (ISO12620; http://www.isocat.org/datcat/DC-1995)
                            </rdfs:comment>
  </rdf:Description>
  <rdf:Description rdf:about="http://purl.org/olia/discourse/olia_discourse.owl#SlangRegister">
    <rdfs:label>slang register</rdfs:label>
  </rdf:Description>
  <rdf:Description rdf:about="http://purl.org/olia/discourse/olia_discourse.owl#SlangRegister">
    <owl:versionInfo>http://www.isocat.org/datcat/DC-1995</owl:versionInfo>
  </rdf:Description>
  <rdf:Description rdf:about="http://purl.org/olia/discourse/olia_discourse.owl#SlangRegister">
    <owl:versionInfo>subClassOf register (dcif:conceptualDomain)</owl:versionInfo>
  </rdf:Description>
  <rdf:Description rdf:about="http://purl.org/olia/discourse/olia_discourse.owl#SoccerClub">
    <rdf:type rdf:resource="http://www.w3.org/2002/07/owl#Class"/>
  </rdf:Description>
  <rdf:Description rdf:about="http://purl.org/olia/discourse/olia_discourse.owl#SoccerClub">
    <rdfs:subClassOf rdf:resource="http://purl.org/olia/discourse/olia_discourse.owl#SportsOrganization"/>
  </rdf:Description>
  <rdf:Description rdf:about="http://purl.org/olia/discourse/olia_discourse.owl#SoccerClub">
    <rdfs:comment xml:lang="en">for nerd:SoccerClub sub nerd:Organization. However, this is probably too specific, hence marked as deprecated.</rdfs:comment>
  </rdf:Description>
  <rdf:Description rdf:about="http://purl.org/olia/discourse/olia_discourse.owl#SoccerClub">
    <owl:deprecated rdf:datatype="http://www.w3.org/2001/XMLSchema#boolean">true</owl:deprecated>
  </rdf:Description>
  <rdf:Description rdf:about="http://purl.org/olia/discourse/olia_discourse.owl#SoccerPlayer">
    <rdf:type rdf:resource="http://www.w3.org/2002/07/owl#Class"/>
  </rdf:Description>
  <rdf:Description rdf:about="http://purl.org/olia/discourse/olia_discourse.owl#SoccerPlayer">
    <rdfs:subClassOf rdf:resource="http://purl.org/olia/discourse/olia_discourse.owl#Athlete"/>
  </rdf:Description>
  <rdf:Description rdf:about="http://purl.org/olia/discourse/olia_discourse.owl#SoccerPlayer">
    <rdfs:comment xml:lang="en">for nerd:SoccerPlayer, sub nerd:Person. Probably too specific, hence marked as deprecated.</rdfs:comment>
  </rdf:Description>
  <rdf:Description rdf:about="http://purl.org/olia/discourse/olia_discourse.owl#SoccerPlayer">
    <owl:deprecated rdf:datatype="http://www.w3.org/2001/XMLSchema#boolean">true</owl:deprecated>
  </rdf:Description>
  <rdf:Description rdf:about="http://purl.org/olia/discourse/olia_discourse.owl#Software">
    <rdf:type rdf:resource="http://www.w3.org/2002/07/owl#Class"/>
  </rdf:Description>
  <rdf:Description rdf:about="http://purl.org/olia/discourse/olia_discourse.owl#Software">
    <rdfs:subClassOf rdf:resource="http://purl.org/olia/discourse/olia_discourse.owl#ManufacturedObject"/>
  </rdf:Description>
  <rdf:Description rdf:about="http://purl.org/olia/discourse/olia_discourse.owl#Software">
    <rdfs:comment xml:lang="en">for nerd:Software</rdfs:comment>
  </rdf:Description>
  <rdf:Description rdf:about="http://purl.org/olia/discourse/olia_discourse.owl#SolicitedResponse">
    <rdf:type rdf:resource="http://www.w3.org/2002/07/owl#Class"/>
  </rdf:Description>
  <rdf:Description rdf:about="http://purl.org/olia/discourse/olia_discourse.owl#SolicitedResponse">
    <rdfs:subClassOf rdf:resource="http://purl.org/olia/discourse/olia_discourse.owl#DialogRelation"/>
  </rdf:Description>
  <rdf:Description rdf:about="http://purl.org/olia/discourse/olia_discourse.owl#SolicitedResponse">
    <rdfs:comment>ISO: Functional depenence is an asymmetric relation between a dialogue act with a responsive communicative function (dependent act) and the dialogue act(s) that it responds to (antecedent act).

comment: "functional dependence" is an unfortunate term because both "dependency" and "functional" have very different definitions in linguistic syntax (dependency syntax, functional grammar). As a less ambiguous term, we thus propose "response relation". Moreover, as the difference between feedback and response relations *seems* to be that feedback is unsolicited whereas a response is solicited, this dichothomy is used as a naming pattern, here.</rdfs:comment>
  </rdf:Description>
  <rdf:Description rdf:about="http://purl.org/olia/discourse/olia_discourse.owl#SolicitedResponse">
    <rdfs:label>functional dependence</rdfs:label>
  </rdf:Description>
  <rdf:Description rdf:about="http://purl.org/olia/discourse/olia_discourse.owl#SolicitedResponse">
    <rdfs:label>response relation</rdfs:label>
  </rdf:Description>
  <rdf:Description rdf:about="http://purl.org/olia/discourse/olia_discourse.owl#SolicitedResponse">
    <rdfs:label xml:lang="en">solicited response</rdfs:label>
  </rdf:Description>
  <rdf:Description rdf:about="http://purl.org/olia/discourse/olia_discourse.owl#SolicitedResponse">
    <skos:prefLabel>solicited response</skos:prefLabel>
  </rdf:Description>
  <rdf:Description rdf:about="http://purl.org/olia/discourse/olia_discourse.owl#Song">
    <rdf:type rdf:resource="http://www.w3.org/2002/07/owl#Class"/>
  </rdf:Description>
  <rdf:Description rdf:about="http://purl.org/olia/discourse/olia_discourse.owl#Song">
    <rdfs:subClassOf rdf:resource="http://purl.org/olia/discourse/olia_discourse.owl#MediaProduct"/>
  </rdf:Description>
  <rdf:Description rdf:about="http://purl.org/olia/discourse/olia_discourse.owl#Song">
    <rdfs:comment xml:lang="en">for nerd:Song, zemanta:track</rdfs:comment>
  </rdf:Description>
  <rdf:Description rdf:about="http://purl.org/olia/discourse/olia_discourse.owl#Song">
    <rdfs:label xml:lang="en">track</rdfs:label>
  </rdf:Description>
  <rdf:Description rdf:about="http://purl.org/olia/discourse/olia_discourse.owl#Song">
    <skos:prefLabel xml:lang="en">song</skos:prefLabel>
  </rdf:Description>
  <rdf:Description rdf:about="http://purl.org/olia/discourse/olia_discourse.owl#Source">
    <rdf:type rdf:resource="http://www.w3.org/2002/07/owl#Class"/>
  </rdf:Description>
  <rdf:Description rdf:about="http://purl.org/olia/discourse/olia_discourse.owl#Source">
    <rdfs:subClassOf rdf:resource="http://purl.org/olia/olia-top.owl#TextStructuralUnit"/>
  </rdf:Description>
  <rdf:Description rdf:about="http://purl.org/olia/discourse/olia_discourse.owl#Source">
    <rdfs:comment>The schema SOURCE is used when an article, or section of an article, begins or
ends by noting the source of the information presented in the article. It should be linked to a TEXT
or SECTIONTEXT schema. (Carlson and Marcu 2001)</rdfs:comment>
  </rdf:Description>
  <rdf:Description rdf:about="http://purl.org/olia/discourse/olia_discourse.owl#Source">
    <rdfs:label xml:lang="en">source</rdfs:label>
  </rdf:Description>
  <rdf:Description rdf:about="http://purl.org/olia/discourse/olia_discourse.owl#Space">
    <rdf:type rdf:resource="http://www.w3.org/2002/07/owl#Class"/>
  </rdf:Description>
  <rdf:Description rdf:about="http://purl.org/olia/discourse/olia_discourse.owl#Space">
    <rdfs:subClassOf rdf:resource="http://purl.org/olia/discourse/olia_discourse.owl#EntityType"/>
  </rdf:Description>
  <rdf:Description rdf:about="http://purl.org/olia/discourse/olia_discourse.owl#Space">
    <rdfs:comment xml:lang="en">Categories specified for referring expressions (Poesio &amp; Artstein 2006): Abstract, Animate, Concrete, Person, Plan, Space, Time

corresponds to nerd:Location</rdfs:comment>
  </rdf:Description>
  <rdf:Description rdf:about="http://purl.org/olia/discourse/olia_discourse.owl#Space">
    <rdfs:label xml:lang="en">LOC</rdfs:label>
  </rdf:Description>
  <rdf:Description rdf:about="http://purl.org/olia/discourse/olia_discourse.owl#Space">
    <rdfs:label xml:lang="en">location</rdfs:label>
  </rdf:Description>
  <rdf:Description rdf:about="http://purl.org/olia/discourse/olia_discourse.owl#Space">
    <rdfs:label xml:lang="en">place</rdfs:label>
  </rdf:Description>
  <rdf:Description rdf:about="http://purl.org/olia/discourse/olia_discourse.owl#Space">
    <rdfs:label xml:lang="en">space</rdfs:label>
  </rdf:Description>
  <rdf:Description rdf:about="http://purl.org/olia/discourse/olia_discourse.owl#Spacecraft">
    <rdf:type rdf:resource="http://www.w3.org/2002/07/owl#Class"/>
  </rdf:Description>
  <rdf:Description rdf:about="http://purl.org/olia/discourse/olia_discourse.owl#Spacecraft">
    <rdfs:subClassOf rdf:resource="http://purl.org/olia/discourse/olia_discourse.owl#Vehicle"/>
  </rdf:Description>
  <rdf:Description rdf:about="http://purl.org/olia/discourse/olia_discourse.owl#Spacecraft">
    <rdfs:comment xml:lang="en">for nerd:Spacecraft</rdfs:comment>
  </rdf:Description>
  <rdf:Description rdf:about="http://purl.org/olia/discourse/olia_discourse.owl#SpecializedRestatement_PDTB">
    <rdf:type rdf:resource="http://www.w3.org/2002/07/owl#Class"/>
  </rdf:Description>
  <rdf:Description rdf:about="http://purl.org/olia/discourse/olia_discourse.owl#SpecializedRestatement_PDTB">
    <rdfs:subClassOf rdf:resource="http://purl.org/olia/discourse/olia_discourse.owl#Specification"/>
  </rdf:Description>
  <rdf:Description rdf:about="http://purl.org/olia/discourse/olia_discourse.owl#SpecializedRestatement_PDTB">
    <rdfs:comment>Arg2 describes the situation described in Arg1 in more detail. Typical connectives for “specification” are specifically,
indeed and in fact. (Prasad et al. 2007)</rdfs:comment>
  </rdf:Description>
  <rdf:Description rdf:about="http://purl.org/olia/discourse/olia_discourse.owl#SpecializedRestatement_PDTB">
    <rdfs:label xml:lang="en">specialized restatement (PDTB)</rdfs:label>
  </rdf:Description>
  <rdf:Description rdf:about="http://purl.org/olia/discourse/olia_discourse.owl#SpecializedRestatement_PDTB">
    <rdfs:label>specification</rdfs:label>
  </rdf:Description>
  <rdf:Description rdf:about="http://purl.org/olia/discourse/olia_discourse.owl#Specification">
    <rdf:type rdf:resource="http://www.w3.org/2002/07/owl#Class"/>
  </rdf:Description>
  <rdf:Description rdf:about="http://purl.org/olia/discourse/olia_discourse.owl#Specification">
    <rdfs:subClassOf rdf:resource="http://purl.org/olia/discourse/olia_discourse.owl#Restatement"/>
  </rdf:Description>
  <rdf:Description rdf:about="http://purl.org/olia/discourse/olia_discourse.owl#Specification">
    <inverseOf rdf:resource="http://purl.org/olia/discourse/Generalization"/>
  </rdf:Description>
  <rdf:Description rdf:about="http://purl.org/olia/discourse/olia_discourse.owl#Specification">
    <rdfs:comment>PDTB Specification

ISO Elaboration, argument role SpecificPartOfElaboration</rdfs:comment>
  </rdf:Description>
  <rdf:Description rdf:about="http://purl.org/olia/discourse/olia_discourse.owl#Specification">
    <rdfs:label xml:lang="en">specification</rdfs:label>
  </rdf:Description>
  <rdf:Description rdf:about="http://purl.org/olia/discourse/olia_discourse.owl#SpeechActAlternative_LUNA">
    <rdf:type rdf:resource="http://www.w3.org/2002/07/owl#Class"/>
  </rdf:Description>
  <rdf:Description rdf:about="http://purl.org/olia/discourse/olia_discourse.owl#SpeechActAlternative_LUNA">
    <rdfs:subClassOf rdf:resource="http://purl.org/olia/discourse/olia_discourse.owl#Alternative"/>
  </rdf:Description>
  <rdf:Description rdf:about="http://purl.org/olia/discourse/olia_discourse.owl#SpeechActAlternative_LUNA">
    <rdfs:comment>Sara Tonelli, Giuseppe Riccardi, Rashmi Prasad and Aravind Joshi (2010), Annotation of Discourse Relations for Conversational Spoken Dialogs, Proceedings of the Seventh conference on International Language Resources and Evaluation (LREC'10), May, 19-21, Valletta, Malta</rdfs:comment>
  </rdf:Description>
  <rdf:Description rdf:about="http://purl.org/olia/discourse/olia_discourse.owl#SpeechActAlternative_LUNA">
    <rdfs:label xml:lang="en">speech act alternative (LUNA)</rdfs:label>
  </rdf:Description>
  <rdf:Description rdf:about="http://purl.org/olia/discourse/olia_discourse.owl#SpeechActCause_HDRB">
    <rdf:type rdf:resource="http://www.w3.org/2002/07/owl#Class"/>
  </rdf:Description>
  <rdf:Description rdf:about="http://purl.org/olia/discourse/olia_discourse.owl#SpeechActCause_HDRB">
    <rdfs:subClassOf rdf:resource="http://purl.org/olia/discourse/olia_discourse.owl#PragmaticCause"/>
  </rdf:Description>
  <rdf:Description rdf:about="http://purl.org/olia/discourse/olia_discourse.owl#SpeechActCause_HDRB">
    <rdfs:comment>An extension of the PDTB scheme suggested by Oza et al. (2009).

Each pragmatic sense at the type level is
further distinguished into three subtypes: “epis-
temic” (Sweetser 1990), “speech-act” (Sweetser
1990), and “propositional”.
(Oza et al. 2009)</rdfs:comment>
  </rdf:Description>
  <rdf:Description rdf:about="http://purl.org/olia/discourse/olia_discourse.owl#SpeechActCause_HDRB">
    <rdfs:label xml:lang="en">speech act cause (HDRB)</rdfs:label>
  </rdf:Description>
  <rdf:Description rdf:about="http://purl.org/olia/discourse/olia_discourse.owl#SpeechActConcession_HDRB">
    <rdf:type rdf:resource="http://www.w3.org/2002/07/owl#Class"/>
  </rdf:Description>
  <rdf:Description rdf:about="http://purl.org/olia/discourse/olia_discourse.owl#SpeechActConcession_HDRB">
    <rdfs:subClassOf rdf:resource="http://purl.org/olia/discourse/olia_discourse.owl#PragmaticConcession_HDRB"/>
  </rdf:Description>
  <rdf:Description rdf:about="http://purl.org/olia/discourse/olia_discourse.owl#SpeechActConcession_HDRB">
    <rdfs:comment>Suggested as an extension of the PDTB scheme by Oza et al. (2009) and Tonelli et al. (2010).

Each pragmatic sense at the type level is
further distinguished into three subtypes: “epis-
temic” (Sweetser 1990), “speech-act” (Sweetser
1990), and “propositional”.
(Oza et al. 2009)</rdfs:comment>
  </rdf:Description>
  <rdf:Description rdf:about="http://purl.org/olia/discourse/olia_discourse.owl#SpeechActConcession_HDRB">
    <rdfs:label xml:lang="en">speech act concession (HDRB)</rdfs:label>
  </rdf:Description>
  <rdf:Description rdf:about="http://purl.org/olia/discourse/olia_discourse.owl#SpeechActCondition_HDRB">
    <rdf:type rdf:resource="http://www.w3.org/2002/07/owl#Class"/>
  </rdf:Description>
  <rdf:Description rdf:about="http://purl.org/olia/discourse/olia_discourse.owl#SpeechActCondition_HDRB">
    <rdfs:subClassOf rdf:resource="http://purl.org/olia/discourse/olia_discourse.owl#PragmaticCondition"/>
  </rdf:Description>
  <rdf:Description rdf:about="http://purl.org/olia/discourse/olia_discourse.owl#SpeechActCondition_HDRB">
    <rdfs:comment>An extension of the PDTB scheme suggested by Oza et al. (2009).

Each pragmatic sense at the type level is
further distinguished into three subtypes: “epis-
temic” (Sweetser 1990), “speech-act” (Sweetser
1990), and “propositional”.
(Oza et al. 2009)</rdfs:comment>
  </rdf:Description>
  <rdf:Description rdf:about="http://purl.org/olia/discourse/olia_discourse.owl#SpeechActCondition_HDRB">
    <rdfs:label xml:lang="en">speech act condition (HDRB)</rdfs:label>
  </rdf:Description>
  <rdf:Description rdf:about="http://purl.org/olia/discourse/olia_discourse.owl#SpeechActConjunction_LUNA">
    <rdf:type rdf:resource="http://www.w3.org/2002/07/owl#Class"/>
  </rdf:Description>
  <rdf:Description rdf:about="http://purl.org/olia/discourse/olia_discourse.owl#SpeechActConjunction_LUNA">
    <rdfs:subClassOf rdf:resource="http://purl.org/olia/discourse/olia_discourse.owl#Conjunction"/>
  </rdf:Description>
  <rdf:Description rdf:about="http://purl.org/olia/discourse/olia_discourse.owl#SpeechActConjunction_LUNA">
    <rdfs:comment>Sara Tonelli, Giuseppe Riccardi, Rashmi Prasad and Aravind Joshi (2010), Annotation of Discourse Relations for Conversational Spoken Dialogs, Proceedings of the Seventh conference on International Language Resources and Evaluation (LREC'10), May, 19-21, Valletta, Malta</rdfs:comment>
  </rdf:Description>
  <rdf:Description rdf:about="http://purl.org/olia/discourse/olia_discourse.owl#SpeechActConjunction_LUNA">
    <rdfs:label xml:lang="en">speech act conjunction (LUNA)</rdfs:label>
  </rdf:Description>
  <rdf:Description rdf:about="http://purl.org/olia/discourse/olia_discourse.owl#SpeechActContrast_HDRB">
    <rdf:type rdf:resource="http://www.w3.org/2002/07/owl#Class"/>
  </rdf:Description>
  <rdf:Description rdf:about="http://purl.org/olia/discourse/olia_discourse.owl#SpeechActContrast_HDRB">
    <rdfs:subClassOf rdf:resource="http://purl.org/olia/discourse/olia_discourse.owl#PragmaticContrast_PDTB"/>
  </rdf:Description>
  <rdf:Description rdf:about="http://purl.org/olia/discourse/olia_discourse.owl#SpeechActContrast_HDRB">
    <rdfs:comment>Suggested as an extension of the PDTB scheme by Oza et al. (2009).

Each pragmatic sense at the type level is
further distinguished into three subtypes: “epis-
temic” (Sweetser 1990), “speech-act” (Sweetser
1990), and “propositional”.
(Oza et al. 2009)</rdfs:comment>
  </rdf:Description>
  <rdf:Description rdf:about="http://purl.org/olia/discourse/olia_discourse.owl#SpeechActContrast_HDRB">
    <rdfs:label xml:lang="en">speech act contrast (HDRB)</rdfs:label>
  </rdf:Description>
  <rdf:Description rdf:about="http://purl.org/olia/discourse/olia_discourse.owl#SpeechActGoal_LUNA">
    <rdf:type rdf:resource="http://www.w3.org/2002/07/owl#Class"/>
  </rdf:Description>
  <rdf:Description rdf:about="http://purl.org/olia/discourse/olia_discourse.owl#SpeechActGoal_LUNA">
    <rdfs:subClassOf rdf:resource="http://purl.org/olia/discourse/olia_discourse.owl#Goal_HDRB"/>
  </rdf:Description>
  <rdf:Description rdf:about="http://purl.org/olia/discourse/olia_discourse.owl#SpeechActGoal_LUNA">
    <rdfs:comment>Sara Tonelli, Giuseppe Riccardi, Rashmi Prasad and Aravind Joshi (2010), Annotation of Discourse Relations for Conversational Spoken Dialogs, Proceedings of the Seventh conference on International Language Resources and Evaluation (LREC'10), May, 19-21, Valletta, Malta</rdfs:comment>
  </rdf:Description>
  <rdf:Description rdf:about="http://purl.org/olia/discourse/olia_discourse.owl#SpeechActGoal_LUNA">
    <rdfs:label xml:lang="en">speech act goal (LUNA)</rdfs:label>
  </rdf:Description>
  <rdf:Description rdf:about="http://purl.org/olia/discourse/olia_discourse.owl#SportsEvent">
    <rdf:type rdf:resource="http://www.w3.org/2002/07/owl#Class"/>
  </rdf:Description>
  <rdf:Description rdf:about="http://purl.org/olia/discourse/olia_discourse.owl#SportsEvent">
    <rdfs:subClassOf rdf:resource="http://purl.org/olia/discourse/olia_discourse.owl#Event"/>
  </rdf:Description>
  <rdf:Description rdf:about="http://purl.org/olia/discourse/olia_discourse.owl#SportsEvent">
    <rdfs:comment xml:lang="en">for nerd:SportEvent</rdfs:comment>
  </rdf:Description>
  <rdf:Description rdf:about="http://purl.org/olia/discourse/olia_discourse.owl#SportsEvent">
    <rdfs:label xml:lang="en">sports event</rdfs:label>
  </rdf:Description>
  <rdf:Description rdf:about="http://purl.org/olia/discourse/olia_discourse.owl#SportsEvent">
    <skos:prefLabel xml:lang="en">sport event</skos:prefLabel>
  </rdf:Description>
  <rdf:Description rdf:about="http://purl.org/olia/discourse/olia_discourse.owl#SportsLeague">
    <rdf:type rdf:resource="http://www.w3.org/2002/07/owl#Class"/>
  </rdf:Description>
  <rdf:Description rdf:about="http://purl.org/olia/discourse/olia_discourse.owl#SportsLeague">
    <rdfs:subClassOf rdf:resource="http://purl.org/olia/discourse/olia_discourse.owl#SportsOrganization"/>
  </rdf:Description>
  <rdf:Description rdf:about="http://purl.org/olia/discourse/olia_discourse.owl#SportsLeague">
    <rdfs:comment xml:lang="en">for nerd:SportsLeague sub nerd:Organization</rdfs:comment>
  </rdf:Description>
  <rdf:Description rdf:about="http://purl.org/olia/discourse/olia_discourse.owl#SportsOrganization">
    <rdf:type rdf:resource="http://www.w3.org/2002/07/owl#Class"/>
  </rdf:Description>
  <rdf:Description rdf:about="http://purl.org/olia/discourse/olia_discourse.owl#SportsOrganization">
    <rdfs:subClassOf rdf:resource="http://purl.org/olia/discourse/olia_discourse.owl#Organization"/>
  </rdf:Description>
  <rdf:Description rdf:about="http://purl.org/olia/discourse/olia_discourse.owl#SportsOrganization">
    <rdfs:comment xml:lang="en">introduced as generalization over nerd:SportsLeague, nerd:SportsTeam, nerd:SoccerClub. Note that "sports organization" is somewhat ambiguous. In a broader sense (as adopted here), it refers to any (NERD) organzation concerned with sports, in a stricter sense, it refers to "any organization that serves as the ruling body for an event for one or several sports." (https://www.lawinsider.com/dictionary/sports-organization)</rdfs:comment>
  </rdf:Description>
  <rdf:Description rdf:about="http://purl.org/olia/discourse/olia_discourse.owl#SportsTeam">
    <rdf:type rdf:resource="http://www.w3.org/2002/07/owl#Class"/>
  </rdf:Description>
  <rdf:Description rdf:about="http://purl.org/olia/discourse/olia_discourse.owl#SportsTeam">
    <rdfs:subClassOf rdf:resource="http://purl.org/olia/discourse/olia_discourse.owl#SportsOrganization"/>
  </rdf:Description>
  <rdf:Description rdf:about="http://purl.org/olia/discourse/olia_discourse.owl#SportsTeam">
    <rdfs:comment xml:lang="en">for nerd:SportsTeam sub nerd:Organization</rdfs:comment>
  </rdf:Description>
  <rdf:Description rdf:about="http://purl.org/olia/discourse/olia_discourse.owl#Stadium">
    <rdf:type rdf:resource="http://www.w3.org/2002/07/owl#Class"/>
  </rdf:Description>
  <rdf:Description rdf:about="http://purl.org/olia/discourse/olia_discourse.owl#Stadium">
    <rdfs:subClassOf rdf:resource="http://purl.org/olia/discourse/olia_discourse.owl#ArchitecturalFeature"/>
  </rdf:Description>
  <rdf:Description rdf:about="http://purl.org/olia/discourse/olia_discourse.owl#Stadium">
    <rdfs:comment xml:lang="en">for nerd:Stadium</rdfs:comment>
  </rdf:Description>
  <rdf:Description rdf:about="http://purl.org/olia/discourse/olia_discourse.owl#Standardized">
    <rdf:type rdf:resource="http://www.w3.org/2002/07/owl#Class"/>
  </rdf:Description>
  <rdf:Description rdf:about="http://purl.org/olia/discourse/olia_discourse.owl#Standardized">
    <rdfs:subClassOf rdf:resource="http://purl.org/olia/discourse/olia_discourse.owl#Possible"/>
  </rdf:Description>
  <rdf:Description rdf:about="http://purl.org/olia/discourse/olia_discourse.owl#Standardized">
    <rdfs:comment>
                            Standardized Term: A term that has been standardized by a standardizing body.
                                (Sue Ellen Wright, http://www.isocat.org/datcat/DC-375)
                            </rdfs:comment>
  </rdf:Description>
  <rdf:Description rdf:about="http://purl.org/olia/discourse/olia_discourse.owl#Standardized">
    <rdfs:label>standardized</rdfs:label>
  </rdf:Description>
  <rdf:Description rdf:about="http://purl.org/olia/discourse/olia_discourse.owl#Standardized">
    <owl:versionInfo>http://www.isocat.org/datcat/DC-375</owl:versionInfo>
  </rdf:Description>
  <rdf:Description rdf:about="http://purl.org/olia/discourse/olia_discourse.owl#StateOfAffairFocus">
    <rdf:type rdf:resource="http://www.w3.org/2002/07/owl#Class"/>
  </rdf:Description>
  <rdf:Description rdf:about="http://purl.org/olia/discourse/olia_discourse.owl#StateOfAffairFocus">
    <rdfs:subClassOf rdf:resource="http://purl.org/olia/discourse/olia_discourse.owl#PredicateCenteredFocus"/>
  </rdf:Description>
  <rdf:Description rdf:about="http://purl.org/olia/discourse/olia_discourse.owl#StateOfAffairFocus">
    <rdfs:comment>StateOfAffairFocus, i.e., focus is often (but not necessarily) on a verbal lexeme

e.g.,
Quaestio: What did the princess do with the frog ?
Example: She KISSED him.
(Güldemann et al. 2010)</rdfs:comment>
  </rdf:Description>
  <rdf:Description rdf:about="http://purl.org/olia/discourse/olia_discourse.owl#StateOfAffairFocus">
    <rdfs:label xml:lang="en">state of affair focus</rdfs:label>
  </rdf:Description>
  <rdf:Description rdf:about="http://purl.org/olia/discourse/olia_discourse.owl#StatementResponse_RST">
    <rdf:type rdf:resource="http://www.w3.org/2002/07/owl#Class"/>
  </rdf:Description>
  <rdf:Description rdf:about="http://purl.org/olia/discourse/olia_discourse.owl#StatementResponse_RST">
    <rdfs:subClassOf rdf:resource="http://purl.org/olia/discourse/olia_discourse.owl#Assessment"/>
  </rdf:Description>
  <rdf:Description rdf:about="http://purl.org/olia/discourse/olia_discourse.owl#StatementResponse_RST">
    <rdfs:comment>In a STATEMENT-RESPONSE relation, one textual span presents a statement and the other span makes some sort of response to it. The statement may be one actually spoken by someone or the author’s statement of a situation. Similarly, the response may be one actually spoken or a situational response to what is occurring in the statement portion.
(Carlson and Marcu 2001)</rdfs:comment>
  </rdf:Description>
  <rdf:Description rdf:about="http://purl.org/olia/discourse/olia_discourse.owl#StatementResponse_RST">
    <rdfs:label xml:lang="en">statement response (RST)</rdfs:label>
  </rdf:Description>
  <rdf:Description rdf:about="http://purl.org/olia/discourse/olia_discourse.owl#Station">
    <rdf:type rdf:resource="http://www.w3.org/2002/07/owl#Class"/>
  </rdf:Description>
  <rdf:Description rdf:about="http://purl.org/olia/discourse/olia_discourse.owl#Station">
    <rdfs:subClassOf rdf:resource="http://purl.org/olia/discourse/olia_discourse.owl#ArchitecturalFeature"/>
  </rdf:Description>
  <rdf:Description rdf:about="http://purl.org/olia/discourse/olia_discourse.owl#Station">
    <rdfs:comment xml:lang="en">for nerd:Station</rdfs:comment>
  </rdf:Description>
  <rdf:Description rdf:about="http://purl.org/olia/discourse/olia_discourse.owl#StructuralConnective">
    <rdf:type rdf:resource="http://www.w3.org/2002/07/owl#Class"/>
  </rdf:Description>
  <rdf:Description rdf:about="http://purl.org/olia/discourse/olia_discourse.owl#StructuralConnective">
    <rdfs:subClassOf rdf:resource="http://purl.org/olia/discourse/olia_discourse.owl#ExplicitConnective"/>
  </rdf:Description>
  <rdf:Description rdf:about="http://purl.org/olia/discourse/olia_discourse.owl#StructuralConnective">
    <rdfs:comment>adopted from SemDok</rdfs:comment>
  </rdf:Description>
  <rdf:Description rdf:about="http://purl.org/olia/discourse/olia_discourse.owl#StructuralConnective">
    <rdfs:label>structural connective</rdfs:label>
  </rdf:Description>
  <rdf:Description rdf:about="http://purl.org/olia/discourse/olia_discourse.owl#StructuralConnective">
    <rdfs:label xml:lang="en">structural connective</rdfs:label>
  </rdf:Description>
  <rdf:Description rdf:about="http://purl.org/olia/discourse/olia_discourse.owl#StructuralFocusType">
    <rdf:type rdf:resource="http://www.w3.org/2002/07/owl#Class"/>
  </rdf:Description>
  <rdf:Description rdf:about="http://purl.org/olia/discourse/olia_discourse.owl#StructuralFocusType">
    <rdfs:subClassOf rdf:resource="http://purl.org/olia/olia-top.owl#PragmaticFeature"/>
  </rdf:Description>
  <rdf:Description rdf:about="http://purl.org/olia/discourse/olia_discourse.owl#StructuralFocusType">
    <rdfs:comment>By StructuralFocusType, we mean a classification of foci according to the structural characteristics, i.e., their scope.

The subclassification of StructuralFocusType assumed here follows a suggestion by Ines Fiedler (2010, Oct 14).</rdfs:comment>
  </rdf:Description>
  <rdf:Description rdf:about="http://purl.org/olia/discourse/olia_discourse.owl#StructuralFocusType">
    <rdfs:label xml:lang="en">structural focus type</rdfs:label>
  </rdf:Description>
  <rdf:Description rdf:about="http://purl.org/olia/discourse/olia_discourse.owl#SubSetOf">
    <rdf:type rdf:resource="http://www.w3.org/2002/07/owl#Class"/>
  </rdf:Description>
  <rdf:Description rdf:about="http://purl.org/olia/discourse/olia_discourse.owl#SubSetOf">
    <rdfs:subClassOf rdf:resource="http://purl.org/olia/discourse/olia_discourse.owl#Set"/>
  </rdf:Description>
  <rdf:Description rdf:about="http://purl.org/olia/discourse/olia_discourse.owl#SubSetOf">
    <rdfs:label xml:lang="en">sub set of</rdfs:label>
  </rdf:Description>
  <rdf:Description rdf:about="http://purl.org/olia/discourse/olia_discourse.owl#SubjectFocus">
    <rdf:type rdf:resource="http://www.w3.org/2002/07/owl#Class"/>
  </rdf:Description>
  <rdf:Description rdf:about="http://purl.org/olia/discourse/olia_discourse.owl#SubjectFocus">
    <rdfs:subClassOf rdf:resource="http://purl.org/olia/discourse/olia_discourse.owl#ArgumentFocus"/>
  </rdf:Description>
  <rdf:Description rdf:about="http://purl.org/olia/discourse/olia_discourse.owl#SubjectFocus">
    <rdfs:comment>Narrow focus on the subject argument. (Fiedler)</rdfs:comment>
  </rdf:Description>
  <rdf:Description rdf:about="http://purl.org/olia/discourse/olia_discourse.owl#SubjectFocus">
    <rdfs:label xml:lang="en">subject focus</rdfs:label>
  </rdf:Description>
  <rdf:Description rdf:about="http://purl.org/olia/discourse/olia_discourse.owl#SubjectMatterRelation">
    <rdf:type rdf:resource="http://www.w3.org/2002/07/owl#Class"/>
  </rdf:Description>
  <rdf:Description rdf:about="http://purl.org/olia/discourse/olia_discourse.owl#SubjectMatterRelation">
    <rdfs:subClassOf rdf:resource="http://purl.org/olia/discourse/olia_discourse.owl#DiscourseFunction"/>
  </rdf:Description>
  <rdf:Description rdf:about="http://purl.org/olia/discourse/olia_discourse.owl#SubjectMatterRelation">
    <owl:disjointWith rdf:resource="http://purl.org/olia/discourse/olia_discourse.owl#TextualOrganizationalRelation"/>
  </rdf:Description>
  <rdf:Description rdf:about="http://purl.org/olia/discourse/olia_discourse.owl#SubjectMatterRelation">
    <rdfs:comment>"[In RST] a distinction is made between Subject-Matter relations and Presentational relations. Subject-Matter relations express parts of the subject matter of the text. The Presentational relations facilitate the presentation process."
(http://www.sfu.ca/rst/01intro/intro.html)</rdfs:comment>
  </rdf:Description>
  <rdf:Description rdf:about="http://purl.org/olia/discourse/olia_discourse.owl#SubjectMatterRelation">
    <rdfs:comment>cf. SemDok IdeationalRelation, except for disjointness axions there is no definition given there, but the conventional definition alludes to RST "subject-matter relations".

Conventional definition (https://en.wikipedia.org/wiki/Metafunction#Ideational_function): The ideational function is language concerned with building and maintaining a theory of experience. It includes the experiential function and the logical function. The experiential function refers to the grammatical choices that enable speakers to make meanings about the world around us and inside us ... Halliday describes the logical function as those systems "which set up logical–semantic relationships between one clausal unit and another"</rdfs:comment>
  </rdf:Description>
  <rdf:Description rdf:about="http://purl.org/olia/discourse/olia_discourse.owl#SubjectMatterRelation">
    <rdfs:comment>ideational relation</rdfs:comment>
  </rdf:Description>
  <rdf:Description rdf:about="http://purl.org/olia/discourse/olia_discourse.owl#SubjectMatterRelation">
    <rdfs:comment>subject-matter relation</rdfs:comment>
  </rdf:Description>
  <rdf:Description rdf:about="http://purl.org/olia/discourse/olia_discourse.owl#SubjectMatterRelation">
    <rdfs:label xml:lang="en">subject matter relation</rdfs:label>
  </rdf:Description>
  <rdf:Description rdf:about="http://purl.org/olia/discourse/olia_discourse.owl#SuccessionRelation">
    <rdf:type rdf:resource="http://www.w3.org/2002/07/owl#Class"/>
  </rdf:Description>
  <rdf:Description rdf:about="http://purl.org/olia/discourse/olia_discourse.owl#SuccessionRelation">
    <rdfs:subClassOf rdf:resource="http://purl.org/olia/discourse/olia_discourse.owl#AsynchronousRelation"/>
  </rdf:Description>
  <rdf:Description rdf:about="http://purl.org/olia/discourse/olia_discourse.owl#SuccessionRelation">
    <inverseOf rdf:resource="http://purl.org/olia/discourse/PrecedenceRelation"/>
  </rdf:Description>
  <rdf:Description rdf:about="http://purl.org/olia/discourse/olia_discourse.owl#SuccessionRelation">
    <rdfs:comment>The connective indicates that the situation described in Arg1 follows the situation described in Arg2. (Prasad et al. 2007)</rdfs:comment>
  </rdf:Description>
  <rdf:Description rdf:about="http://purl.org/olia/discourse/olia_discourse.owl#SuccessionRelation">
    <rdfs:label xml:lang="en">succession relation</rdfs:label>
  </rdf:Description>
  <rdf:Description rdf:about="http://purl.org/olia/discourse/olia_discourse.owl#Summary">
    <rdf:type rdf:resource="http://www.w3.org/2002/07/owl#Class"/>
  </rdf:Description>
  <rdf:Description rdf:about="http://purl.org/olia/discourse/olia_discourse.owl#Summary">
    <rdfs:subClassOf rdf:resource="http://purl.org/olia/discourse/olia_discourse.owl#Generalization"/>
  </rdf:Description>
  <rdf:Description rdf:about="http://purl.org/olia/discourse/olia_discourse.owl#Summary">
    <rdfs:subClassOf rdf:resource="http://purl.org/olia/discourse/olia_discourse.owl#HypotacticDiscourseRelation"/>
  </rdf:Description>
  <rdf:Description rdf:about="http://purl.org/olia/discourse/olia_discourse.owl#Summary">
    <rdfs:subClassOf rdf:resource="http://purl.org/olia/discourse/olia_discourse.owl#PresentationalRelation"/>
  </rdf:Description>
  <rdf:Description rdf:about="http://purl.org/olia/discourse/olia_discourse.owl#Summary">
    <rdfs:comment>introduced as generalization over RST Summary and SemDok Summary. Axiomatized according to the latter (mononuclear presentational relation).</rdfs:comment>
  </rdf:Description>
  <rdf:Description rdf:about="http://purl.org/olia/discourse/olia_discourse.owl#Summary">
    <rdfs:label xml:lang="en">summary</rdfs:label>
  </rdf:Description>
  <rdf:Description rdf:about="http://purl.org/olia/discourse/olia_discourse.owl#Summary_RST">
    <rdf:type rdf:resource="http://www.w3.org/2002/07/owl#Class"/>
  </rdf:Description>
  <rdf:Description rdf:about="http://purl.org/olia/discourse/olia_discourse.owl#Summary_RST">
    <rdfs:subClassOf rdf:resource="http://purl.org/olia/discourse/olia_discourse.owl#Summary"/>
  </rdf:Description>
  <rdf:Description rdf:about="http://purl.org/olia/discourse/olia_discourse.owl#Summary_RST">
    <rdfs:comment>In a SUMMARY-S relation, the satellite summarizes the information presented in the nucleus. The emphasis is on the situation presented in the nucleus. The size of the summary (the satellite) is shorter than the size of the nucleus. In an SUMMARY-N relation, the nucleus summarizes the information presented in the satellite. The emphasis is on the summary. The size of the summary (the nucleus) is shorter than the size of the satellite.
(Carlson and Marcu 2001)</rdfs:comment>
  </rdf:Description>
  <rdf:Description rdf:about="http://purl.org/olia/discourse/olia_discourse.owl#Summary_RST">
    <rdfs:label xml:lang="en">summary (RST)</rdfs:label>
  </rdf:Description>
  <rdf:Description rdf:about="http://purl.org/olia/discourse/olia_discourse.owl#Support">
    <rdf:type rdf:resource="http://www.w3.org/2002/07/owl#Class"/>
  </rdf:Description>
  <rdf:Description rdf:about="http://purl.org/olia/discourse/olia_discourse.owl#Support">
    <rdfs:subClassOf rdf:resource="http://purl.org/olia/discourse/olia_discourse.owl#HypotacticDiscourseRelation"/>
  </rdf:Description>
  <rdf:Description rdf:about="http://purl.org/olia/discourse/olia_discourse.owl#Support">
    <rdfs:subClassOf rdf:resource="http://purl.org/olia/discourse/olia_discourse.owl#PragmaticCause"/>
  </rdf:Description>
  <rdf:Description rdf:about="http://purl.org/olia/discourse/olia_discourse.owl#Support">
    <rdfs:subClassOf rdf:resource="http://purl.org/olia/discourse/olia_discourse.owl#PresentationalRelation"/>
  </rdf:Description>
  <rdf:Description rdf:about="http://purl.org/olia/discourse/olia_discourse.owl#Support">
    <rdfs:comment>for SemDok Support, mononuclear interpersonal relation</rdfs:comment>
  </rdf:Description>
  <rdf:Description rdf:about="http://purl.org/olia/discourse/olia_discourse.owl#Support">
    <rdfs:label xml:lang="en">support</rdfs:label>
  </rdf:Description>
  <rdf:Description rdf:about="http://purl.org/olia/discourse/olia_discourse.owl#SynchronousRelation">
    <rdf:type rdf:resource="http://www.w3.org/2002/07/owl#Class"/>
  </rdf:Description>
  <rdf:Description rdf:about="http://purl.org/olia/discourse/olia_discourse.owl#SynchronousRelation">
    <rdfs:subClassOf rdf:resource="http://purl.org/olia/discourse/olia_discourse.owl#TemporalRelation"/>
  </rdf:Description>
  <rdf:Description rdf:about="http://purl.org/olia/discourse/olia_discourse.owl#SynchronousRelation">
    <rdfs:comment>The situations described in Arg1 and Arg2 overlap. (Prasad et al. 2007)</rdfs:comment>
  </rdf:Description>
  <rdf:Description rdf:about="http://purl.org/olia/discourse/olia_discourse.owl#SynchronousRelation">
    <rdfs:label xml:lang="en">synchronous relation</rdfs:label>
  </rdf:Description>
  <rdf:Description rdf:about="http://purl.org/olia/discourse/olia_discourse.owl#TAMFocus">
    <rdf:type rdf:resource="http://www.w3.org/2002/07/owl#Class"/>
  </rdf:Description>
  <rdf:Description rdf:about="http://purl.org/olia/discourse/olia_discourse.owl#TAMFocus">
    <rdfs:subClassOf rdf:resource="http://purl.org/olia/discourse/olia_discourse.owl#OperatorFocus"/>
  </rdf:Description>
  <rdf:Description rdf:about="http://purl.org/olia/discourse/olia_discourse.owl#TAMFocus">
    <rdfs:comment>Focus with scope over a tense, aspect, or mood marker (Fiedler &amp; Chiarcos)

Quaestio: Is the princess kissing the frog (right now) ?
example: She HAS kissed him.
(Güldemann et al. 2010; note: example ambiguous with polarity focus)</rdfs:comment>
  </rdf:Description>
  <rdf:Description rdf:about="http://purl.org/olia/discourse/olia_discourse.owl#TAMFocus">
    <rdfs:label xml:lang="en">t a m focus</rdfs:label>
  </rdf:Description>
  <rdf:Description rdf:about="http://purl.org/olia/discourse/olia_discourse.owl#TVStation">
    <rdf:type rdf:resource="http://www.w3.org/2002/07/owl#Class"/>
  </rdf:Description>
  <rdf:Description rdf:about="http://purl.org/olia/discourse/olia_discourse.owl#TVStation">
    <rdfs:subClassOf rdf:resource="http://purl.org/olia/discourse/olia_discourse.owl#BroadcastingOrganization"/>
  </rdf:Description>
  <rdf:Description rdf:about="http://purl.org/olia/discourse/olia_discourse.owl#TVStation">
    <rdfs:comment xml:lang="en">for nerd:TVStation sub nerd:Organization</rdfs:comment>
  </rdf:Description>
  <rdf:Description rdf:about="http://purl.org/olia/discourse/olia_discourse.owl#TVStation">
    <rdfs:label xml:lang="en">TV network</rdfs:label>
  </rdf:Description>
  <rdf:Description rdf:about="http://purl.org/olia/discourse/olia_discourse.owl#TVStation">
    <skos:prefLabel xml:lang="en">TV station</skos:prefLabel>
  </rdf:Description>
  <rdf:Description rdf:about="http://purl.org/olia/discourse/olia_discourse.owl#TabooRegister">
    <rdf:type rdf:resource="http://www.w3.org/2002/07/owl#Class"/>
  </rdf:Description>
  <rdf:Description rdf:about="http://purl.org/olia/discourse/olia_discourse.owl#TabooRegister">
    <rdfs:subClassOf rdf:resource="http://purl.org/olia/olia-top.owl#RegisterFeature"/>
  </rdf:Description>
  <rdf:Description rdf:about="http://purl.org/olia/discourse/olia_discourse.owl#TabooRegister">
    <rdfs:comment>
                            Register that expresses a situation that people avoid because it is extremely offensive or embarrassing.
                                (ISO12620; http://www.isocat.org/datcat/DC-1996)
                            </rdfs:comment>
  </rdf:Description>
  <rdf:Description rdf:about="http://purl.org/olia/discourse/olia_discourse.owl#TabooRegister">
    <rdfs:label>taboo register</rdfs:label>
  </rdf:Description>
  <rdf:Description rdf:about="http://purl.org/olia/discourse/olia_discourse.owl#TabooRegister">
    <owl:versionInfo>http://www.isocat.org/datcat/DC-1996</owl:versionInfo>
  </rdf:Description>
  <rdf:Description rdf:about="http://purl.org/olia/discourse/olia_discourse.owl#TabooRegister">
    <owl:versionInfo>subClassOf register (dcif:conceptualDomain)</owl:versionInfo>
  </rdf:Description>
  <rdf:Description rdf:about="http://purl.org/olia/discourse/olia_discourse.owl#TechnicalRegister">
    <rdf:type rdf:resource="http://www.w3.org/2002/07/owl#Class"/>
  </rdf:Description>
  <rdf:Description rdf:about="http://purl.org/olia/discourse/olia_discourse.owl#TechnicalRegister">
    <rdfs:subClassOf rdf:resource="http://purl.org/olia/olia-top.owl#RegisterFeature"/>
  </rdf:Description>
  <rdf:Description rdf:about="http://purl.org/olia/discourse/olia_discourse.owl#TechnicalRegister">
    <rdfs:comment>
                            The register appropriate to scientific texts or special languages.
                                (ISO12620; http://www.isocat.org/datcat/DC-1997)
                            </rdfs:comment>
  </rdf:Description>
  <rdf:Description rdf:about="http://purl.org/olia/discourse/olia_discourse.owl#TechnicalRegister">
    <rdfs:label>technical register</rdfs:label>
  </rdf:Description>
  <rdf:Description rdf:about="http://purl.org/olia/discourse/olia_discourse.owl#TechnicalRegister">
    <owl:versionInfo>http://www.isocat.org/datcat/DC-1997</owl:versionInfo>
  </rdf:Description>
  <rdf:Description rdf:about="http://purl.org/olia/discourse/olia_discourse.owl#TechnicalRegister">
    <owl:versionInfo>subClassOf register (dcif:conceptualDomain)</owl:versionInfo>
  </rdf:Description>
  <rdf:Description rdf:about="http://purl.org/olia/discourse/olia_discourse.owl#TemporalAfter">
    <rdf:type rdf:resource="http://www.w3.org/2002/07/owl#Class"/>
  </rdf:Description>
  <rdf:Description rdf:nodeID="genid65">
    <rdf:type rdf:resource="http://www.w3.org/2002/07/owl#Class"/>
  </rdf:Description>
  <rdf:Description rdf:nodeID="genid66">
    <rdf:first rdf:resource="http://purl.org/olia/discourse/olia_discourse.owl#HypotacticDiscourseRelation"/>
  </rdf:Description>
  <rdf:Description rdf:nodeID="genid67">
    <rdf:first rdf:resource="http://purl.org/olia/discourse/olia_discourse.owl#SuccessionRelation"/>
  </rdf:Description>
  <rdf:Description rdf:nodeID="genid66">
    <rdf:rest rdf:nodeID="genid67"/>
  </rdf:Description>
  <rdf:Description rdf:nodeID="genid67">
    <rdf:rest rdf:resource="http://www.w3.org/1999/02/22-rdf-syntax-ns#nil"/>
  </rdf:Description>
  <rdf:Description rdf:nodeID="genid65">
    <owl:intersectionOf rdf:nodeID="genid66"/>
  </rdf:Description>
  <rdf:Description rdf:about="http://purl.org/olia/discourse/olia_discourse.owl#TemporalAfter">
    <owl:equivalentClass rdf:nodeID="genid65"/>
  </rdf:Description>
  <rdf:Description rdf:about="http://purl.org/olia/discourse/olia_discourse.owl#TemporalAfter">
    <rdfs:comment>In a TEMPORAL-AFTER relation, the situation presented in the nucleus (often
realized as a superordinate clause) occurs after the situation presented in the satellite (often real-
ized as a subordinate clause). When the relation is multinuclear, and the spans occur in temporal
order -- i.e., the situation presented in the second segment occurs after the situation presented in
the first segment -- select the multinuclear relation SEQUENCE.
(Carlson and Marcu 2001)</rdfs:comment>
  </rdf:Description>
  <rdf:Description rdf:about="http://purl.org/olia/discourse/olia_discourse.owl#TemporalAfter">
    <rdfs:label xml:lang="en">temporal after</rdfs:label>
  </rdf:Description>
  <rdf:Description rdf:about="http://purl.org/olia/discourse/olia_discourse.owl#TemporalBefore">
    <rdf:type rdf:resource="http://www.w3.org/2002/07/owl#Class"/>
  </rdf:Description>
  <rdf:Description rdf:nodeID="genid68">
    <rdf:type rdf:resource="http://www.w3.org/2002/07/owl#Class"/>
  </rdf:Description>
  <rdf:Description rdf:nodeID="genid69">
    <rdf:first rdf:resource="http://purl.org/olia/discourse/olia_discourse.owl#HypotacticDiscourseRelation"/>
  </rdf:Description>
  <rdf:Description rdf:nodeID="genid70">
    <rdf:first rdf:resource="http://purl.org/olia/discourse/olia_discourse.owl#PrecedenceRelation"/>
  </rdf:Description>
  <rdf:Description rdf:nodeID="genid69">
    <rdf:rest rdf:nodeID="genid70"/>
  </rdf:Description>
  <rdf:Description rdf:nodeID="genid70">
    <rdf:rest rdf:resource="http://www.w3.org/1999/02/22-rdf-syntax-ns#nil"/>
  </rdf:Description>
  <rdf:Description rdf:nodeID="genid68">
    <owl:intersectionOf rdf:nodeID="genid69"/>
  </rdf:Description>
  <rdf:Description rdf:about="http://purl.org/olia/discourse/olia_discourse.owl#TemporalBefore">
    <owl:equivalentClass rdf:nodeID="genid68"/>
  </rdf:Description>
  <rdf:Description rdf:about="http://purl.org/olia/discourse/olia_discourse.owl#TemporalBefore">
    <rdfs:comment>In a TEMPORAL-BEFORE relation, the situation presented in the nucleus (often
realized as a superordinate clause) occurs before or leading up to the situation in the satellite
(often realized as a subordinate clause). When the relation is multinuclear but the spans occur in
reverse temporal order -- i.e., the situation presented in the second span occurs before the situation
presented in the first span -- select the multinuclear relation INVERTED-SEQUENCE. (Carlson and Marcu 2001)</rdfs:comment>
  </rdf:Description>
  <rdf:Description rdf:about="http://purl.org/olia/discourse/olia_discourse.owl#TemporalBefore">
    <rdfs:label xml:lang="en">temporal before</rdfs:label>
  </rdf:Description>
  <rdf:Description rdf:about="http://purl.org/olia/discourse/olia_discourse.owl#TemporalRelation">
    <rdf:type rdf:resource="http://www.w3.org/2002/07/owl#Class"/>
  </rdf:Description>
  <rdf:Description rdf:about="http://purl.org/olia/discourse/olia_discourse.owl#TemporalRelation">
    <rdfs:subClassOf rdf:resource="http://purl.org/olia/discourse/olia_discourse.owl#CoherenceRelation"/>
  </rdf:Description>
  <rdf:Description rdf:about="http://purl.org/olia/discourse/olia_discourse.owl#TemporalRelation">
    <rdfs:comment>The situations described in the arguments are related temporally. (Prasad et al. 2007)

Infer a temporal sequence of the events described by DS0 and DS1. There is no
causal relation between DS0 and DS1. If there is a causal relation, the relation between DS0
and DS1 should be described as a Cause-Effect relation.
(Wolf et al. 2003)</rdfs:comment>
  </rdf:Description>
  <rdf:Description rdf:about="http://purl.org/olia/discourse/olia_discourse.owl#TemporalRelation">
    <rdfs:label xml:lang="en">temporal relation</rdfs:label>
  </rdf:Description>
  <rdf:Description rdf:about="http://purl.org/olia/discourse/olia_discourse.owl#TemporalSameTime">
    <rdf:type rdf:resource="http://www.w3.org/2002/07/owl#Class"/>
  </rdf:Description>
  <rdf:Description rdf:about="http://purl.org/olia/discourse/olia_discourse.owl#TemporalSameTime">
    <rdfs:subClassOf rdf:resource="http://purl.org/olia/discourse/olia_discourse.owl#SynchronousRelation"/>
  </rdf:Description>
  <rdf:Description rdf:about="http://purl.org/olia/discourse/olia_discourse.owl#TemporalSameTime">
    <rdfs:comment>In a TEMPORAL-SAME-TIME relation, the situations presented in the nucleus and satellite occur at approximately the same time, or at least there is an overlap between the two situations. This relation can be mononuclear or multinuclear.
(Carlson and Marcu 2001)</rdfs:comment>
  </rdf:Description>
  <rdf:Description rdf:about="http://purl.org/olia/discourse/olia_discourse.owl#TemporalSameTime">
    <rdfs:label xml:lang="en">temporal same time</rdfs:label>
  </rdf:Description>
  <rdf:Description rdf:about="http://purl.org/olia/discourse/olia_discourse.owl#TemporallyDefinedUsage">
    <rdf:type rdf:resource="http://www.w3.org/2002/07/owl#Class"/>
  </rdf:Description>
  <rdf:Description rdf:about="http://purl.org/olia/discourse/olia_discourse.owl#TemporallyDefinedUsage">
    <rdfs:subClassOf rdf:resource="http://purl.org/olia/discourse/olia_discourse.owl#Possible"/>
  </rdf:Description>
  <rdf:Description rdf:about="http://purl.org/olia/discourse/olia_discourse.owl#TemporallyDefinedUsage">
    <rdfs:comment>Indication specifying whether the usage is old or modern.</rdfs:comment>
  </rdf:Description>
  <rdf:Description rdf:about="http://purl.org/olia/discourse/olia_discourse.owl#TemporallyDefinedUsage">
    <rdfs:isDefinedBy>http://www.isocat.org/datcat/DC-1959</rdfs:isDefinedBy>
  </rdf:Description>
  <rdf:Description rdf:about="http://purl.org/olia/discourse/olia_discourse.owl#TemporallyDefinedUsage">
    <rdfs:label>dating</rdfs:label>
  </rdf:Description>
  <rdf:Description rdf:about="http://purl.org/olia/discourse/olia_discourse.owl#TemporallyDefinedUsage">
    <rdfs:label xml:lang="en">temporally defined usage</rdfs:label>
  </rdf:Description>
  <rdf:Description rdf:about="http://purl.org/olia/discourse/olia_discourse.owl#TennisPlayer">
    <rdf:type rdf:resource="http://www.w3.org/2002/07/owl#Class"/>
  </rdf:Description>
  <rdf:Description rdf:about="http://purl.org/olia/discourse/olia_discourse.owl#TennisPlayer">
    <rdfs:subClassOf rdf:resource="http://purl.org/olia/discourse/olia_discourse.owl#Athlete"/>
  </rdf:Description>
  <rdf:Description rdf:about="http://purl.org/olia/discourse/olia_discourse.owl#TennisPlayer">
    <rdfs:comment xml:lang="en">for nerd:TennisPlayer, sub nerd:Person. Probably too specific, hence marked as deprecated.</rdfs:comment>
  </rdf:Description>
  <rdf:Description rdf:about="http://purl.org/olia/discourse/olia_discourse.owl#TennisPlayer">
    <owl:deprecated rdf:datatype="http://www.w3.org/2001/XMLSchema#boolean">true</owl:deprecated>
  </rdf:Description>
  <rdf:Description rdf:about="http://purl.org/olia/discourse/olia_discourse.owl#Text">
    <rdf:type rdf:resource="http://www.w3.org/2002/07/owl#Class"/>
  </rdf:Description>
  <rdf:Description rdf:about="http://purl.org/olia/discourse/olia_discourse.owl#Text">
    <rdfs:subClassOf rdf:resource="http://purl.org/olia/olia-top.owl#TextStructuralUnit"/>
  </rdf:Description>
  <rdf:Description rdf:about="http://purl.org/olia/discourse/olia_discourse.owl#Text">
    <rdfs:comment>The schema Text is used to link the main body of the text to other structural
elements of the document, such as a FOOTNOTE, SOURCE, HEADING, etc. This schema is used only
if the entire body of the text should be linked to another schema. If only a subsection of the text is
relevant, the schema SECTIONTEXT is used instead. Occasionally, a WSJ document contains more
than one article. In that case, the schema TEXT may be used, for example to link a TITLE and TEXT
for each of the three articles included within a single document (see example below under 13.
Title). (Carlson and Marcu 2001)</rdfs:comment>
  </rdf:Description>
  <rdf:Description rdf:about="http://purl.org/olia/discourse/olia_discourse.owl#Text">
    <rdfs:label xml:lang="en">text</rdfs:label>
  </rdf:Description>
  <rdf:Description rdf:about="http://purl.org/olia/discourse/olia_discourse.owl#TextualOrganization_RST">
    <rdf:type rdf:resource="http://www.w3.org/2002/07/owl#Class"/>
  </rdf:Description>
  <rdf:Description rdf:about="http://purl.org/olia/discourse/olia_discourse.owl#TextualOrganization_RST">
    <rdfs:subClassOf rdf:resource="http://purl.org/olia/discourse/olia_discourse.owl#TextualOrganizationalRelation"/>
  </rdf:Description>
  <rdf:Description rdf:about="http://purl.org/olia/discourse/olia_discourse.owl#TextualOrganization_RST">
    <rdfs:comment>This seems to roughly correspond to SemDok Schema (with sub-class ArticleTopLevelSchema). However, note that a schema is an n-ary relation whereas text-organizational relations are binary.</rdfs:comment>
  </rdf:Description>
  <rdf:Description rdf:about="http://purl.org/olia/discourse/olia_discourse.owl#TextualOrganization_RST">
    <rdfs:comment>TEXTUAL-ORGANIZATION is a multinuclear relation used to link elements of the structure of the text, for example, to link a title with the body of the text, a section title with the text of a section, etc. The role of the relation is primarily that of enforcing a tree structure on the representation.
(Carlson and Marcu 2001)</rdfs:comment>
  </rdf:Description>
  <rdf:Description rdf:about="http://purl.org/olia/discourse/olia_discourse.owl#TextualOrganization_RST">
    <rdfs:label>schema</rdfs:label>
  </rdf:Description>
  <rdf:Description rdf:about="http://purl.org/olia/discourse/olia_discourse.owl#TextualOrganization_RST">
    <rdfs:label>textual organization</rdfs:label>
  </rdf:Description>
  <rdf:Description rdf:about="http://purl.org/olia/discourse/olia_discourse.owl#TextualOrganization_RST">
    <rdfs:label xml:lang="en">textual organization (RST)</rdfs:label>
  </rdf:Description>
  <rdf:Description rdf:about="http://purl.org/olia/discourse/olia_discourse.owl#TextualOrganizationalRelation">
    <rdf:type rdf:resource="http://www.w3.org/2002/07/owl#Class"/>
  </rdf:Description>
  <rdf:Description rdf:about="http://purl.org/olia/discourse/olia_discourse.owl#TextualOrganizationalRelation">
    <rdfs:subClassOf rdf:resource="http://purl.org/olia/discourse/olia_discourse.owl#DiscourseRelation"/>
  </rdf:Description>
  <rdf:Description rdf:about="http://purl.org/olia/discourse/olia_discourse.owl#TextualOrganizationalRelation">
    <rdfs:comment>cf. SemDok TextualRelation</rdfs:comment>
  </rdf:Description>
  <rdf:Description rdf:about="http://purl.org/olia/discourse/olia_discourse.owl#TextualOrganizationalRelation">
    <rdfs:comment>"Pseudo-relations" that represent conventional text-structural relationships between text spans, not strictly speaking discourse relations.</rdfs:comment>
  </rdf:Description>
  <rdf:Description rdf:about="http://purl.org/olia/discourse/olia_discourse.owl#TextualOrganizationalRelation">
    <rdfs:label>textual organizational relation</rdfs:label>
  </rdf:Description>
  <rdf:Description rdf:about="http://purl.org/olia/discourse/olia_discourse.owl#TextualOrganizationalRelation">
    <rdfs:label xml:lang="en">textual organizational relation</rdfs:label>
  </rdf:Description>
  <rdf:Description rdf:about="http://purl.org/olia/discourse/olia_discourse.owl#TextualOrganizationalRelation">
    <rdfs:label>textual relation</rdfs:label>
  </rdf:Description>
  <rdf:Description rdf:about="http://purl.org/olia/discourse/olia_discourse.owl#Time">
    <rdf:type rdf:resource="http://www.w3.org/2002/07/owl#Class"/>
  </rdf:Description>
  <rdf:Description rdf:about="http://purl.org/olia/discourse/olia_discourse.owl#Time">
    <rdfs:subClassOf rdf:resource="http://purl.org/olia/discourse/olia_discourse.owl#EntityType"/>
  </rdf:Description>
  <rdf:Description rdf:about="http://purl.org/olia/discourse/olia_discourse.owl#Time">
    <rdfs:comment xml:lang="en">Categories specified for referring expressions (Poesio &amp; Artstein 2006): Abstract, Animate, Concrete, Person, Plan, Space, Time.
Corresponds to nerd:Time.</rdfs:comment>
  </rdf:Description>
  <rdf:Description rdf:about="http://purl.org/olia/discourse/olia_discourse.owl#Time">
    <rdfs:label xml:lang="en">time</rdfs:label>
  </rdf:Description>
  <rdf:Description rdf:about="http://purl.org/olia/discourse/olia_discourse.owl#Title">
    <rdf:type rdf:resource="http://www.w3.org/2002/07/owl#Class"/>
  </rdf:Description>
  <rdf:Description rdf:about="http://purl.org/olia/discourse/olia_discourse.owl#Title">
    <rdfs:subClassOf rdf:resource="http://purl.org/olia/olia-top.owl#TextStructuralUnit"/>
  </rdf:Description>
  <rdf:Description rdf:about="http://purl.org/olia/discourse/olia_discourse.owl#Title">
    <rdfs:comment>The WSJ documents from the LDC usually did not include titles. However, in
a small number of cases, a WSJ document consisted of more than one article, each of which
included a title. In that case the schemata TITLE and TEXT were used. (Carlson and Marcu 2001)</rdfs:comment>
  </rdf:Description>
  <rdf:Description rdf:about="http://purl.org/olia/discourse/olia_discourse.owl#Title">
    <rdfs:label xml:lang="en">title</rdfs:label>
  </rdf:Description>
  <rdf:Description rdf:about="http://purl.org/olia/discourse/olia_discourse.owl#TitleInRunningText">
    <rdf:type rdf:resource="http://www.w3.org/2002/07/owl#Class"/>
  </rdf:Description>
  <rdf:Description rdf:about="http://purl.org/olia/discourse/olia_discourse.owl#TitleInRunningText">
    <rdfs:subClassOf rdf:resource="http://purl.org/olia/olia-top.owl#TextStructuralUnit"/>
  </rdf:Description>
  <rdf:Description rdf:about="http://purl.org/olia/discourse/olia_discourse.owl#TitleInRunningText">
    <rdfs:comment>-TTL (title)
— is attached to the top node of a title when this title appears inside running text.
-TTL implies -NOM. The internal structure of the title is bracketed as usual. (See section 12 [Titles] for more information about the bracketing of titles.) 
(Bies et al. 1995)</rdfs:comment>
  </rdf:Description>
  <rdf:Description rdf:about="http://purl.org/olia/discourse/olia_discourse.owl#TitleInRunningText">
    <owl:versionInfo>PTB bracketing guidelines, Bies et al. 1995</owl:versionInfo>
  </rdf:Description>
  <rdf:Description rdf:about="http://purl.org/olia/discourse/olia_discourse.owl#Topic">
    <rdf:type rdf:resource="http://www.w3.org/2002/07/owl#Class"/>
  </rdf:Description>
  <rdf:Description rdf:about="http://purl.org/olia/discourse/olia_discourse.owl#Topic">
    <rdfs:subClassOf rdf:resource="http://purl.org/olia/discourse/olia_discourse.owl#PragmaticUnit"/>
  </rdf:Description>
  <rdf:Description rdf:about="http://purl.org/olia/discourse/olia_discourse.owl#Topic">
    <rdfs:comment>The topic constituent identifies the entity or set of entities under which
the information expressed in the comment constituent should be stored in the CG content.

The notion of topic is best understood as a kind of address or file card which specifies the individual or set about which the remainder of the sentence makes a comment (see Reinhart 1981 for such a concept of topicality). It has no truthconditional effect except that it presupposes the existence of that individual. In this sense, the complement of ‘topic’ is ‘comment,’ which can itself be partitioned into a focused and a backgrounded part. Sentences usually have only one topic, but can also have none, or more than one. Following Jacobs (2001), topics can be aboutness or frame-setting topics, and the means to express a topic in the grammar can be pinpointed rather precisely in terms of which syntactic and intonational preferences the topic displays, at least in an intonation language. However, according to Féry’s theses, none of these properties are definitional for topic. Rather they express preferences as to how a ‘good’ topic has to be realized (see also Jacobs 2001 for a similar view).
(Féry et al. 2007)</rdfs:comment>
  </rdf:Description>
  <rdf:Description rdf:about="http://purl.org/olia/discourse/olia_discourse.owl#Topic">
    <rdfs:comment>"Topic" is a prominent notion in pragmatics, though often with varying definitions. For detailed definitions, compare the sub-classes.</rdfs:comment>
  </rdf:Description>
  <rdf:Description rdf:about="http://purl.org/olia/discourse/olia_discourse.owl#Topic">
    <rdfs:label xml:lang="en">topic</rdfs:label>
  </rdf:Description>
  <rdf:Description rdf:about="http://purl.org/olia/discourse/olia_discourse.owl#TopicComment">
    <rdf:type rdf:resource="http://www.w3.org/2002/07/owl#Class"/>
  </rdf:Description>
  <rdf:Description rdf:about="http://purl.org/olia/discourse/olia_discourse.owl#TopicComment">
    <rdfs:subClassOf rdf:resource="http://purl.org/olia/discourse/olia_discourse.owl#TopicContinuityRelation"/>
  </rdf:Description>
  <rdf:Description rdf:about="http://purl.org/olia/discourse/olia_discourse.owl#TopicComment">
    <rdfs:comment>introduced as generalization over TopicComment_RST and ElaborationThemeRheme (from SemDok). These differ in nuclearity.</rdfs:comment>
  </rdf:Description>
  <rdf:Description rdf:about="http://purl.org/olia/discourse/olia_discourse.owl#TopicComment">
    <rdfs:label xml:lang="en">topic comment</rdfs:label>
  </rdf:Description>
  <rdf:Description rdf:about="http://purl.org/olia/discourse/olia_discourse.owl#TopicComment_RST">
    <rdf:type rdf:resource="http://www.w3.org/2002/07/owl#Class"/>
  </rdf:Description>
  <rdf:Description rdf:about="http://purl.org/olia/discourse/olia_discourse.owl#TopicComment_RST">
    <rdfs:subClassOf rdf:resource="http://purl.org/olia/discourse/olia_discourse.owl#ParatacticDiscourseRelation"/>
  </rdf:Description>
  <rdf:Description rdf:about="http://purl.org/olia/discourse/olia_discourse.owl#TopicComment_RST">
    <rdfs:subClassOf rdf:resource="http://purl.org/olia/discourse/olia_discourse.owl#TopicComment"/>
  </rdf:Description>
  <rdf:Description rdf:about="http://purl.org/olia/discourse/olia_discourse.owl#TopicComment_RST">
    <rdfs:comment>A general statement or topic of discussion is introduced, after which a specific
remark is made on the statement or topic. This relation is always multinuclear, as both spans are
necessary to understand the context. When the spans occur in the reverse order, with the comment
preceding the topic, the relation COMMENT-TOPIC is selected.
(Carlson and Marcu 2001)</rdfs:comment>
  </rdf:Description>
  <rdf:Description rdf:about="http://purl.org/olia/discourse/olia_discourse.owl#TopicComment_RST">
    <rdfs:label xml:lang="en">topic comment (RST)</rdfs:label>
  </rdf:Description>
  <rdf:Description rdf:about="http://purl.org/olia/discourse/olia_discourse.owl#TopicContinuityRelation">
    <rdf:type rdf:resource="http://www.w3.org/2002/07/owl#Class"/>
  </rdf:Description>
  <rdf:Description rdf:about="http://purl.org/olia/discourse/olia_discourse.owl#TopicContinuityRelation">
    <rdfs:subClassOf rdf:resource="http://purl.org/olia/discourse/olia_discourse.owl#Expansion"/>
  </rdf:Description>
  <rdf:Description rdf:about="http://purl.org/olia/discourse/olia_discourse.owl#TopicContinuityRelation">
    <rdfs:comment>TopicShift and TopicDrift.</rdfs:comment>
  </rdf:Description>
  <rdf:Description rdf:about="http://purl.org/olia/discourse/olia_discourse.owl#TopicContinuityRelation">
    <rdfs:label>progression</rdfs:label>
  </rdf:Description>
  <rdf:Description rdf:about="http://purl.org/olia/discourse/olia_discourse.owl#TopicContinuityRelation">
    <rdfs:label>topic continuity relation</rdfs:label>
  </rdf:Description>
  <rdf:Description rdf:about="http://purl.org/olia/discourse/olia_discourse.owl#TopicContinuityRelation">
    <rdfs:label xml:lang="en">topic continuity relation</rdfs:label>
  </rdf:Description>
  <rdf:Description rdf:about="http://purl.org/olia/discourse/olia_discourse.owl#TopicContinuityRelation">
    <owl:versionInfo>Introduced as a supercategory for RST-DTB relations topic-shift and topic-drift. Both connect large text spans that were no subject to annotation in PDTB.

Note that C-TED introduced EXPANSION.Progression in an extension of the PDTB 3 schema. As progression in Chinese refers to aspects of topic continuity, this concept, formerly a direct subclass of CoherenceRelation, has been reconceptualized as a subclass of Expansion.</owl:versionInfo>
  </rdf:Description>
  <rdf:Description rdf:about="http://purl.org/olia/discourse/olia_discourse.owl#TopicDrift">
    <rdf:type rdf:resource="http://www.w3.org/2002/07/owl#Class"/>
  </rdf:Description>
  <rdf:Description rdf:about="http://purl.org/olia/discourse/olia_discourse.owl#TopicDrift">
    <rdfs:subClassOf rdf:resource="http://purl.org/olia/discourse/olia_discourse.owl#TopicContinuityRelation"/>
  </rdf:Description>
  <rdf:Description rdf:about="http://purl.org/olia/discourse/olia_discourse.owl#TopicDrift">
    <rdfs:comment>introduced as generalization over ElaborationDrift (from SemDok) and TopicDrift_RST</rdfs:comment>
  </rdf:Description>
  <rdf:Description rdf:about="http://purl.org/olia/discourse/olia_discourse.owl#TopicDrift">
    <rdfs:label xml:lang="en">topic drift</rdfs:label>
  </rdf:Description>
  <rdf:Description rdf:about="http://purl.org/olia/discourse/olia_discourse.owl#TopicDrift_RST">
    <rdf:type rdf:resource="http://www.w3.org/2002/07/owl#Class"/>
  </rdf:Description>
  <rdf:Description rdf:about="http://purl.org/olia/discourse/olia_discourse.owl#TopicDrift_RST">
    <rdfs:subClassOf rdf:resource="http://purl.org/olia/discourse/olia_discourse.owl#TopicDrift"/>
  </rdf:Description>
  <rdf:Description rdf:about="http://purl.org/olia/discourse/olia_discourse.owl#TopicDrift_RST">
    <rdfs:comment>The relation TOPIC-DRIFT is used to link large textual spans when the topic
drifts smoothly from the information presented in the first span to the information presented in the
second. The same elements are in focus in both textual units. While this relation may be either
mononuclear or multinuclear, it is usually multinuclear. Only select mononuclear if the relative
size or importance of one of the spans is less significant than that of the other.
(Carlson and Marcu 2001)</rdfs:comment>
  </rdf:Description>
  <rdf:Description rdf:about="http://purl.org/olia/discourse/olia_discourse.owl#TopicDrift_RST">
    <rdfs:label xml:lang="en">topic drift (RST)</rdfs:label>
  </rdf:Description>
  <rdf:Description rdf:about="http://purl.org/olia/discourse/olia_discourse.owl#TopicExpression">
    <rdf:type rdf:resource="http://www.w3.org/2002/07/owl#Class"/>
  </rdf:Description>
  <rdf:Description rdf:about="http://purl.org/olia/discourse/olia_discourse.owl#TopicExpression">
    <rdfs:subClassOf rdf:resource="http://purl.org/olia/discourse/olia_discourse.owl#Markable"/>
  </rdf:Description>
  <rdf:Description rdf:about="http://purl.org/olia/discourse/olia_discourse.owl#TopicExpression">
    <rdfs:comment>A topic expression is the expression that denotates the topic referent. (Lambrecht 1994)</rdfs:comment>
  </rdf:Description>
  <rdf:Description rdf:about="http://purl.org/olia/discourse/olia_discourse.owl#TopicExpression">
    <rdfs:label xml:lang="en">topic expression</rdfs:label>
  </rdf:Description>
  <rdf:Description rdf:about="http://purl.org/olia/discourse/olia_discourse.owl#TopicShift">
    <rdf:type rdf:resource="http://www.w3.org/2002/07/owl#Class"/>
  </rdf:Description>
  <rdf:Description rdf:about="http://purl.org/olia/discourse/olia_discourse.owl#TopicShift">
    <rdfs:subClassOf rdf:resource="http://purl.org/olia/discourse/olia_discourse.owl#TopicContinuityRelation"/>
  </rdf:Description>
  <rdf:Description rdf:about="http://purl.org/olia/discourse/olia_discourse.owl#TopicShift">
    <rdfs:comment>introduced in analogy to TopicDrift as a generalization over TopicShift_RST.</rdfs:comment>
  </rdf:Description>
  <rdf:Description rdf:about="http://purl.org/olia/discourse/olia_discourse.owl#TopicShift">
    <rdfs:label xml:lang="en">topic shift</rdfs:label>
  </rdf:Description>
  <rdf:Description rdf:about="http://purl.org/olia/discourse/olia_discourse.owl#TopicShift_RST">
    <rdf:type rdf:resource="http://www.w3.org/2002/07/owl#Class"/>
  </rdf:Description>
  <rdf:Description rdf:about="http://purl.org/olia/discourse/olia_discourse.owl#TopicShift_RST">
    <rdfs:subClassOf rdf:resource="http://purl.org/olia/discourse/olia_discourse.owl#TopicShift"/>
  </rdf:Description>
  <rdf:Description rdf:about="http://purl.org/olia/discourse/olia_discourse.owl#TopicShift_RST">
    <rdfs:comment>The relation TOPIC-SHIFT is used to link large textual spans when there is a
sharp change in focus going from one segment to the other. The same elements are NOT in focus
in the two spans. While this relation may be either mononuclear or multinuclear, it is usually
multinuclear. Only select mononuclear if the relative size or importance of one of the spans is less
significant than that of the other.
(Carlson and Marcu 2001)</rdfs:comment>
  </rdf:Description>
  <rdf:Description rdf:about="http://purl.org/olia/discourse/olia_discourse.owl#TopicShift_RST">
    <rdfs:label xml:lang="en">topic shift (RST)</rdfs:label>
  </rdf:Description>
  <rdf:Description rdf:about="http://purl.org/olia/discourse/olia_discourse.owl#URL">
    <rdf:type rdf:resource="http://www.w3.org/2002/07/owl#Class"/>
  </rdf:Description>
  <rdf:Description rdf:about="http://purl.org/olia/discourse/olia_discourse.owl#URL">
    <rdfs:subClassOf rdf:resource="http://purl.org/olia/discourse/olia_discourse.owl#Address"/>
  </rdf:Description>
  <rdf:Description rdf:about="http://purl.org/olia/discourse/olia_discourse.owl#URL">
    <rdfs:comment xml:lang="en">for nerd:URL sub nerd:Product</rdfs:comment>
  </rdf:Description>
  <rdf:Description rdf:about="http://purl.org/olia/discourse/olia_discourse.owl#Unconditional">
    <rdf:type rdf:resource="http://www.w3.org/2002/07/owl#Class"/>
  </rdf:Description>
  <rdf:Description rdf:about="http://purl.org/olia/discourse/olia_discourse.owl#Unconditional">
    <rdfs:subClassOf rdf:resource="http://purl.org/olia/discourse/olia_discourse.owl#Contigency"/>
  </rdf:Description>
  <rdf:Description rdf:about="http://purl.org/olia/discourse/olia_discourse.owl#Unconditional">
    <rdfs:comment>S conceivably could affect the realization of N, N does not depend on S. R recognizes that N does not depend on S.
(Mann and Taboada 2010)

cf. Wolf et al.'s (2003) "ViolatedExpectation": Infer that normally there is a causal relation between DS0 and DS1 but that causal relation is absent between DS0 and DS1.</rdfs:comment>
  </rdf:Description>
  <rdf:Description rdf:about="http://purl.org/olia/discourse/olia_discourse.owl#Unconditional">
    <rdfs:label xml:lang="en">unconditional</rdfs:label>
  </rdf:Description>
  <rdf:Description rdf:about="http://purl.org/olia/discourse/olia_discourse.owl#University">
    <rdf:type rdf:resource="http://www.w3.org/2002/07/owl#Class"/>
  </rdf:Description>
  <rdf:Description rdf:about="http://purl.org/olia/discourse/olia_discourse.owl#University">
    <rdfs:subClassOf rdf:resource="http://purl.org/olia/discourse/olia_discourse.owl#EducationalInstitution"/>
  </rdf:Description>
  <rdf:Description rdf:about="http://purl.org/olia/discourse/olia_discourse.owl#University">
    <rdfs:comment xml:lang="en">for nerd:University, originally subclass of Organization</rdfs:comment>
  </rdf:Description>
  <rdf:Description rdf:about="http://purl.org/olia/discourse/olia_discourse.owl#Unless_RST">
    <rdf:type rdf:resource="http://www.w3.org/2002/07/owl#Class"/>
  </rdf:Description>
  <rdf:Description rdf:about="http://purl.org/olia/discourse/olia_discourse.owl#Unless_RST">
    <rdfs:subClassOf rdf:resource="http://purl.org/olia/discourse/olia_discourse.owl#NegativeCondition"/>
  </rdf:Description>
  <rdf:Description rdf:about="http://purl.org/olia/discourse/olia_discourse.owl#Unless_RST">
    <rdfs:comment>S affects the realization of N; N is realized provided that S is not realized.
(Mann and Taboada 2010)</rdfs:comment>
  </rdf:Description>
  <rdf:Description rdf:about="http://purl.org/olia/discourse/olia_discourse.owl#Unless_RST">
    <rdfs:label xml:lang="en">unless (RST)</rdfs:label>
  </rdf:Description>
  <rdf:Description rdf:about="http://purl.org/olia/discourse/olia_discourse.owl#UnmarkedFactuality">
    <rdf:type rdf:resource="http://www.w3.org/2002/07/owl#Class"/>
  </rdf:Description>
  <rdf:Description rdf:about="http://purl.org/olia/discourse/olia_discourse.owl#UnmarkedFactuality">
    <rdfs:subClassOf rdf:resource="http://purl.org/olia/discourse/olia_discourse.owl#PropositionalFactuality"/>
  </rdf:Description>
  <rdf:Description rdf:about="http://purl.org/olia/discourse/olia_discourse.owl#UnmarkedFactuality">
    <rdfs:comment>In the absence of an independent occurrence of attribution on an argument, as for Arg2 of Example (158), a “Null” value for the type on the argument means that it needs to be derived by independent (here, undefined) considerations under the scope of the relation.

(158) When Mr. Green won a $240,000 verdict in a land condemnation case against the State in June 1983, he says Judge O’Kicki unexpectedly awarded him an additional $100,000. (0267)

Note that unlike the “Inh” value of the source feature, “Null” does not indicate inheritance. In a subordinate clause, for example, while the relation denoted by the subordinating conjunction may be asserted, the clause content itself may be “presupposed”, as seems to be the case in (158). However, we found these differences difficult to determine at times, and consequently leave this undefined in the scheme.
(Prasad et al. 2007, for PDTB)</rdfs:comment>
  </rdf:Description>
  <rdf:Description rdf:about="http://purl.org/olia/discourse/olia_discourse.owl#UnmarkedFactuality">
    <rdfs:label>attribution type null</rdfs:label>
  </rdf:Description>
  <rdf:Description rdf:about="http://purl.org/olia/discourse/olia_discourse.owl#UnmarkedFactuality">
    <rdfs:label xml:lang="en">unmarked factuality</rdfs:label>
  </rdf:Description>
  <rdf:Description rdf:about="http://purl.org/olia/discourse/olia_discourse.owl#UnmarkedPolarity">
    <rdf:type rdf:resource="http://www.w3.org/2002/07/owl#Class"/>
  </rdf:Description>
  <rdf:Description rdf:about="http://purl.org/olia/discourse/olia_discourse.owl#UnmarkedPolarity">
    <rdfs:subClassOf rdf:resource="http://purl.org/olia/discourse/olia_discourse.owl#Polarity"/>
  </rdf:Description>
  <rdf:Description rdf:about="http://purl.org/olia/discourse/olia_discourse.owl#UnmarkedPolarity">
    <rdfs:comment>"Null" marking in PDTB, i.e. Default (or NonNegated)</rdfs:comment>
  </rdf:Description>
  <rdf:Description rdf:about="http://purl.org/olia/discourse/olia_discourse.owl#UnmarkedPolarity">
    <rdfs:label>default polarity</rdfs:label>
  </rdf:Description>
  <rdf:Description rdf:about="http://purl.org/olia/discourse/olia_discourse.owl#UnmarkedPolarity">
    <rdfs:label>positive</rdfs:label>
  </rdf:Description>
  <rdf:Description rdf:about="http://purl.org/olia/discourse/olia_discourse.owl#UnmarkedPolarity">
    <rdfs:label>unmarked polarity</rdfs:label>
  </rdf:Description>
  <rdf:Description rdf:about="http://purl.org/olia/discourse/olia_discourse.owl#UnmarkedPolarity">
    <rdfs:label xml:lang="en">unmarked polarity</rdfs:label>
  </rdf:Description>
  <rdf:Description rdf:about="http://purl.org/olia/discourse/olia_discourse.owl#UnrealCondition_HDRB">
    <rdf:type rdf:resource="http://www.w3.org/2002/07/owl#Class"/>
  </rdf:Description>
  <rdf:Description rdf:about="http://purl.org/olia/discourse/olia_discourse.owl#UnrealCondition_HDRB">
    <rdfs:subClassOf rdf:resource="http://purl.org/olia/discourse/olia_discourse.owl#NegativeCondition"/>
  </rdf:Description>
  <rdf:Description rdf:about="http://purl.org/olia/discourse/olia_discourse.owl#UnrealCondition_HDRB">
    <rdfs:comment>Oza et al. (2009) suggested to abandon the PDTB distinction between UnrealPastCondition and UnrealPresentCondition.</rdfs:comment>
  </rdf:Description>
  <rdf:Description rdf:about="http://purl.org/olia/discourse/olia_discourse.owl#UnrealCondition_HDRB">
    <rdfs:label xml:lang="en">unreal condition (HDRB)</rdfs:label>
  </rdf:Description>
  <rdf:Description rdf:about="http://purl.org/olia/discourse/olia_discourse.owl#UnrealCondition_HDRB">
    <owl:versionInfo>TODO: merge with NegativeCondition</owl:versionInfo>
  </rdf:Description>
  <rdf:Description rdf:about="http://purl.org/olia/discourse/olia_discourse.owl#UnrealPastCondition_PDTB">
    <rdf:type rdf:resource="http://www.w3.org/2002/07/owl#Class"/>
  </rdf:Description>
  <rdf:Description rdf:about="http://purl.org/olia/discourse/olia_discourse.owl#UnrealPastCondition_PDTB">
    <rdfs:subClassOf rdf:resource="http://purl.org/olia/discourse/olia_discourse.owl#UnrealCondition_HDRB"/>
  </rdf:Description>
  <rdf:Description rdf:about="http://purl.org/olia/discourse/olia_discourse.owl#UnrealPastCondition_PDTB">
    <rdfs:comment>Arg2 describes a situation that did not occur in the past and Arg1 expresses what the consequence would have been if it had. It is inferred from the semantics of this subtype of “Condition” that the situations described in Arg1 and Arg2 did not hold. (Prasad et al. 2007)</rdfs:comment>
  </rdf:Description>
  <rdf:Description rdf:about="http://purl.org/olia/discourse/olia_discourse.owl#UnrealPastCondition_PDTB">
    <rdfs:label xml:lang="en">unreal past condition (PDTB)</rdfs:label>
  </rdf:Description>
  <rdf:Description rdf:about="http://purl.org/olia/discourse/olia_discourse.owl#UnrealPresentCondition_PDTB">
    <rdf:type rdf:resource="http://www.w3.org/2002/07/owl#Class"/>
  </rdf:Description>
  <rdf:Description rdf:about="http://purl.org/olia/discourse/olia_discourse.owl#UnrealPresentCondition_PDTB">
    <rdfs:subClassOf rdf:resource="http://purl.org/olia/discourse/olia_discourse.owl#UnrealCondition_HDRB"/>
  </rdf:Description>
  <rdf:Description rdf:about="http://purl.org/olia/discourse/olia_discourse.owl#UnrealPresentCondition_PDTB">
    <rdfs:comment>Arg2 describes a condition that either does not hold at present. Arg1 describes what would also hold if Arg2 were true. “Unreal present” represents the semantics of conditional relations also known in the lingustic literature as present counterfactuals (Iatridou, 2000). The semantics for “unreal present” is a special case of the semantics for hypothetical. (Prasad et al. 2007)</rdfs:comment>
  </rdf:Description>
  <rdf:Description rdf:about="http://purl.org/olia/discourse/olia_discourse.owl#UnrealPresentCondition_PDTB">
    <rdfs:label xml:lang="en">unreal present condition (PDTB)</rdfs:label>
  </rdf:Description>
  <rdf:Description rdf:about="http://purl.org/olia/discourse/olia_discourse.owl#UnsolicitedResponse">
    <rdf:type rdf:resource="http://www.w3.org/2002/07/owl#Class"/>
  </rdf:Description>
  <rdf:Description rdf:about="http://purl.org/olia/discourse/olia_discourse.owl#UnsolicitedResponse">
    <rdfs:subClassOf rdf:resource="http://purl.org/olia/discourse/olia_discourse.owl#DialogRelation"/>
  </rdf:Description>
  <rdf:Description rdf:about="http://purl.org/olia/discourse/olia_discourse.owl#UnsolicitedResponse">
    <rdfs:comment>ISO: Asymmetric relation of a feedback act with its scope: Feedback act is a dialogue act with a responsive communicative function; Feedback scope is the dialogue act(s) that the feedback act responds to.

Comment: Note that "Dependence" implies an ordering here (in analogy with dependency syntax), however, Bunt and Prasad explicitly argue against such an interpretation in their schema (when comparing it with RST nuclearity). As a less ambigous term, we thus introduce the label "feedback relation". Moreover, as the difference between feedback and response relations *seems* to be that feedback is unsolicited whereas a response is solicited, this dichothomy is used as a naming pattern, here.</rdfs:comment>
  </rdf:Description>
  <rdf:Description rdf:about="http://purl.org/olia/discourse/olia_discourse.owl#UnsolicitedResponse">
    <rdfs:label>feedback dependence</rdfs:label>
  </rdf:Description>
  <rdf:Description rdf:about="http://purl.org/olia/discourse/olia_discourse.owl#UnsolicitedResponse">
    <rdfs:label>feedback relation</rdfs:label>
  </rdf:Description>
  <rdf:Description rdf:about="http://purl.org/olia/discourse/olia_discourse.owl#UnsolicitedResponse">
    <rdfs:label>unsolicited response</rdfs:label>
  </rdf:Description>
  <rdf:Description rdf:about="http://purl.org/olia/discourse/olia_discourse.owl#UnsolicitedResponse">
    <rdfs:label xml:lang="en">unsolicited response</rdfs:label>
  </rdf:Description>
  <rdf:Description rdf:about="http://purl.org/olia/discourse/olia_discourse.owl#Utterance">
    <rdf:type rdf:resource="http://www.w3.org/2002/07/owl#Class"/>
  </rdf:Description>
  <rdf:Description rdf:about="http://purl.org/olia/discourse/olia_discourse.owl#Utterance">
    <rdfs:subClassOf rdf:resource="http://purl.org/olia/olia-top.owl#DiscourseEntity"/>
  </rdf:Description>
  <rdf:Description rdf:about="http://purl.org/olia/discourse/olia_discourse.owl#Utterance">
    <rdfs:comment>
                            Complete unit of talk, bounded by the speaker's silence.
                                (www.sil.org/linguistics/GlossaryOfLinguisticTerms/WhatIsAnUtterance.htm; http://www.isocat.org/datcat/DC-1409)
                            </rdfs:comment>
  </rdf:Description>
  <rdf:Description rdf:about="http://purl.org/olia/discourse/olia_discourse.owl#Utterance">
    <rdfs:label>utterance</rdfs:label>
  </rdf:Description>
  <rdf:Description rdf:about="http://purl.org/olia/discourse/olia_discourse.owl#Utterance">
    <owl:versionInfo>http://www.isocat.org/datcat/DC-1409</owl:versionInfo>
  </rdf:Description>
  <rdf:Description rdf:about="http://purl.org/olia/discourse/olia_discourse.owl#Valley">
    <rdf:type rdf:resource="http://www.w3.org/2002/07/owl#Class"/>
  </rdf:Description>
  <rdf:Description rdf:about="http://purl.org/olia/discourse/olia_discourse.owl#Valley">
    <rdfs:subClassOf rdf:resource="http://purl.org/olia/discourse/olia_discourse.owl#GeographicalFeature"/>
  </rdf:Description>
  <rdf:Description rdf:about="http://purl.org/olia/discourse/olia_discourse.owl#Valley">
    <rdfs:comment xml:lang="en">for nerd:Valley</rdfs:comment>
  </rdf:Description>
  <rdf:Description rdf:about="http://purl.org/olia/discourse/olia_discourse.owl#Vehicle">
    <rdf:type rdf:resource="http://www.w3.org/2002/07/owl#Class"/>
  </rdf:Description>
  <rdf:Description rdf:about="http://purl.org/olia/discourse/olia_discourse.owl#Vehicle">
    <rdfs:subClassOf rdf:resource="http://purl.org/olia/discourse/olia_discourse.owl#ManufacturedObject"/>
  </rdf:Description>
  <rdf:Description rdf:about="http://purl.org/olia/discourse/olia_discourse.owl#Vehicle">
    <rdfs:comment xml:lang="en">introduced as a generalization over various nerd:Products that designate means of transportation</rdfs:comment>
  </rdf:Description>
  <rdf:Description rdf:about="http://purl.org/olia/discourse/olia_discourse.owl#VideoGame">
    <rdf:type rdf:resource="http://www.w3.org/2002/07/owl#Class"/>
  </rdf:Description>
  <rdf:Description rdf:about="http://purl.org/olia/discourse/olia_discourse.owl#VideoGame">
    <rdfs:subClassOf rdf:resource="http://purl.org/olia/discourse/olia_discourse.owl#Software"/>
  </rdf:Description>
  <rdf:Description rdf:about="http://purl.org/olia/discourse/olia_discourse.owl#VideoGame">
    <rdfs:comment xml:lang="en">for nerd:VideoGame sub nerd:Product</rdfs:comment>
  </rdf:Description>
  <rdf:Description rdf:about="http://purl.org/olia/discourse/olia_discourse.owl#VideoGame">
    <skos:prefLabel xml:lang="en">video game</skos:prefLabel>
  </rdf:Description>
  <rdf:Description rdf:about="http://purl.org/olia/discourse/olia_discourse.owl#VocativeExpression">
    <rdf:type rdf:resource="http://www.w3.org/2002/07/owl#Class"/>
  </rdf:Description>
  <rdf:Description rdf:about="http://purl.org/olia/discourse/olia_discourse.owl#VocativeExpression">
    <rdfs:subClassOf rdf:resource="http://purl.org/olia/olia-top.owl#DiscourseEntity"/>
  </rdf:Description>
  <rdf:Description rdf:about="http://purl.org/olia/discourse/olia_discourse.owl#VocativeExpression">
    <rdfs:comment>An expression referring to a person to which the utterance is addressed, e.g. Old High German "truhtin",  "meistar" or "fater". The vocative expression typically occurs outside of the clause and not in an argument position selected by the predicate. (Petrova 2008, see http://purl.org/olia/tcodex.owl)</rdfs:comment>
  </rdf:Description>
  <rdf:Description rdf:about="http://purl.org/olia/discourse/olia_discourse.owl#VocativeExpression">
    <rdfs:label>vocative expression</rdfs:label>
  </rdf:Description>
  <rdf:Description rdf:about="http://purl.org/olia/discourse/olia_discourse.owl#VocativeExpression">
    <owl:versionInfo>http://purl.org/olia/tcodex.owl#VocativeForm</owl:versionInfo>
  </rdf:Description>
  <rdf:Description rdf:about="http://purl.org/olia/discourse/olia_discourse.owl#VolitionalCause_RST">
    <rdf:type rdf:resource="http://www.w3.org/2002/07/owl#Class"/>
  </rdf:Description>
  <rdf:Description rdf:about="http://purl.org/olia/discourse/olia_discourse.owl#VolitionalCause_RST">
    <rdfs:subClassOf rdf:resource="http://purl.org/olia/discourse/olia_discourse.owl#Cause_RST"/>
  </rdf:Description>
  <rdf:Description rdf:about="http://purl.org/olia/discourse/olia_discourse.owl#VolitionalCause_RST">
    <rdfs:comment>R recognizes S as a cause for the volitional action in N
(Mann and Taboada 2010)</rdfs:comment>
  </rdf:Description>
  <rdf:Description rdf:about="http://purl.org/olia/discourse/olia_discourse.owl#VolitionalCause_RST">
    <rdfs:label xml:lang="en">volitional cause (RST)</rdfs:label>
  </rdf:Description>
  <rdf:Description rdf:about="http://purl.org/olia/discourse/olia_discourse.owl#VolitionalResult_RST">
    <rdf:type rdf:resource="http://www.w3.org/2002/07/owl#Class"/>
  </rdf:Description>
  <rdf:Description rdf:about="http://purl.org/olia/discourse/olia_discourse.owl#VolitionalResult_RST">
    <rdfs:subClassOf rdf:resource="http://purl.org/olia/discourse/olia_discourse.owl#Result_RST"/>
  </rdf:Description>
  <rdf:Description rdf:about="http://purl.org/olia/discourse/olia_discourse.owl#VolitionalResult_RST">
    <rdfs:comment>R recognizes that N could be a cause for the action or situation in S
(Mann and Taboada 2010)</rdfs:comment>
  </rdf:Description>
  <rdf:Description rdf:about="http://purl.org/olia/discourse/olia_discourse.owl#VolitionalResult_RST">
    <rdfs:label xml:lang="en">volitional result (RST)</rdfs:label>
  </rdf:Description>
  <rdf:Description rdf:about="http://purl.org/olia/discourse/olia_discourse.owl#VulgarRegister">
    <rdf:type rdf:resource="http://www.w3.org/2002/07/owl#Class"/>
  </rdf:Description>
  <rdf:Description rdf:about="http://purl.org/olia/discourse/olia_discourse.owl#VulgarRegister">
    <rdfs:subClassOf rdf:resource="http://purl.org/olia/olia-top.owl#RegisterFeature"/>
  </rdf:Description>
  <rdf:Description rdf:about="http://purl.org/olia/discourse/olia_discourse.owl#VulgarRegister">
    <rdfs:comment>
                            Register of a term or text type that can be characterized as profane or socially unacceptable.
                                (ISO12620; http://www.isocat.org/datcat/DC-1998)
                            </rdfs:comment>
  </rdf:Description>
  <rdf:Description rdf:about="http://purl.org/olia/discourse/olia_discourse.owl#VulgarRegister">
    <rdfs:label>vulgar register</rdfs:label>
  </rdf:Description>
  <rdf:Description rdf:about="http://purl.org/olia/discourse/olia_discourse.owl#VulgarRegister">
    <owl:versionInfo>http://www.isocat.org/datcat/DC-1998</owl:versionInfo>
  </rdf:Description>
  <rdf:Description rdf:about="http://purl.org/olia/discourse/olia_discourse.owl#VulgarRegister">
    <owl:versionInfo>subClassOf register (dcif:conceptualDomain)</owl:versionInfo>
  </rdf:Description>
  <rdf:Description rdf:about="http://purl.org/olia/discourse/olia_discourse.owl#Weapon">
    <rdf:type rdf:resource="http://www.w3.org/2002/07/owl#Class"/>
  </rdf:Description>
  <rdf:Description rdf:about="http://purl.org/olia/discourse/olia_discourse.owl#Weapon">
    <rdfs:subClassOf rdf:resource="http://purl.org/olia/discourse/olia_discourse.owl#ManufacturedObject"/>
  </rdf:Description>
  <rdf:Description rdf:about="http://purl.org/olia/discourse/olia_discourse.owl#Weapon">
    <rdfs:comment xml:lang="en">for nerd:Weapon</rdfs:comment>
  </rdf:Description>
  <rdf:Description rdf:about="http://purl.org/olia/discourse/olia_discourse.owl#Website">
    <rdf:type rdf:resource="http://www.w3.org/2002/07/owl#Class"/>
  </rdf:Description>
  <rdf:Description rdf:about="http://purl.org/olia/discourse/olia_discourse.owl#Website">
    <rdfs:subClassOf rdf:resource="http://purl.org/olia/discourse/olia_discourse.owl#URL"/>
  </rdf:Description>
  <rdf:Description rdf:about="http://purl.org/olia/discourse/olia_discourse.owl#Website">
    <rdfs:comment xml:lang="en">for nerd:Website, sub nerd:Product</rdfs:comment>
  </rdf:Description>
  <rdf:Description rdf:about="http://purl.org/olia/discourse/olia_discourse.owl#WholePart">
    <rdf:type rdf:resource="http://www.w3.org/2002/07/owl#Class"/>
  </rdf:Description>
  <rdf:Description rdf:about="http://purl.org/olia/discourse/olia_discourse.owl#WholePart">
    <rdfs:subClassOf rdf:resource="http://purl.org/olia/discourse/olia_discourse.owl#BridgingType"/>
  </rdf:Description>
  <rdf:Description rdf:about="http://purl.org/olia/discourse/olia_discourse.owl#WholePart">
    <rdfs:comment>A referent represents a superset, a class, type or environment to which another pre-mentioned referent belongs (Stuttgart Guidelines).</rdfs:comment>
  </rdf:Description>
  <rdf:Description rdf:about="http://purl.org/olia/discourse/olia_discourse.owl#WholePart">
    <rdfs:label xml:lang="en">whole part</rdfs:label>
  </rdf:Description>
  <rdf:Description rdf:about="http://purl.org/olia/discourse/olia_discourse.owl#WideFocus">
    <rdf:type rdf:resource="http://www.w3.org/2002/07/owl#Class"/>
  </rdf:Description>
  <rdf:Description rdf:about="http://purl.org/olia/discourse/olia_discourse.owl#WideFocus">
    <rdfs:subClassOf rdf:resource="http://purl.org/olia/discourse/olia_discourse.owl#StructuralFocusType"/>
  </rdf:Description>
  <rdf:Description rdf:about="http://purl.org/olia/discourse/olia_discourse.owl#WideFocus">
    <rdfs:comment>Wide focus and narrow focus represent an often-adopted, coarse-grained subclassification of foci according to their scope. Narrow focus means that one single constituent is in focus, whereas wide focus means that multiple constituents are in focus. (Fiedler &amp; Chiarcos)</rdfs:comment>
  </rdf:Description>
  <rdf:Description rdf:about="http://purl.org/olia/discourse/olia_discourse.owl#WideFocus">
    <rdfs:label xml:lang="en">wide focus</rdfs:label>
  </rdf:Description>
  <rdf:Description rdf:about="http://purl.org/olia/system.owl#UnitOfAnnotation">
    <rdf:type rdf:resource="http://www.w3.org/2002/07/owl#Class"/>
  </rdf:Description>
  <rdf:Description rdf:about="http://purl.org/olia/system.owl#UnitOfAnnotation">
    <rdfs:comment>AnnotationUnit was introduced to account for annotating strings (selected according to certain criteria) directly with discourse information. Where structured elements (e.g., from syntax or semantics) represent the basis of annotation, the annotations should be directly anchored with them.

Here, we are concerned with discourse annotation only. Syntactically or semantically defined units of annotations are thus considered opaque objects, as these are to be described in terms of the OLiA Reference Model.</rdfs:comment>
  </rdf:Description>
  <rdf:Description rdf:about="http://purl.org/olia/system.owl#UnitOfAnnotation">
    <rdfs:label xml:lang="en">annotation unit</rdfs:label>
  </rdf:Description>
  <rdf:Description rdf:about="http://www.w3.org/2002/07/owl#Thing">
    <rdf:type rdf:resource="http://www.w3.org/2002/07/owl#Class"/>
  </rdf:Description>
  <rdf:Description rdf:about="http://purl.org/olia/discourse/olia_discourse.owl#AboutnessTopic">
    <terms:replacedBy rdf:resource="http://purl.org/olia/olia.owl#AboutnessTopic"/>
  </rdf:Description>
  <rdf:Description rdf:about="http://purl.org/olia/discourse/olia_discourse.owl#AboutnessTopic">
    <owl:deprecated rdf:datatype="http://www.w3.org/2001/XMLSchema#boolean">true</owl:deprecated>
  </rdf:Description>
  <rdf:Description rdf:about="http://purl.org/olia/discourse/olia_discourse.owl#Abstract">
    <terms:replacedBy rdf:resource="http://purl.org/olia/olia.owl#Abstract"/>
  </rdf:Description>
  <rdf:Description rdf:about="http://purl.org/olia/discourse/olia_discourse.owl#Abstract">
    <owl:deprecated rdf:datatype="http://www.w3.org/2001/XMLSchema#boolean">true</owl:deprecated>
  </rdf:Description>
  <rdf:Description rdf:about="http://purl.org/olia/discourse/olia_discourse.owl#AbstractEntity">
    <terms:replacedBy rdf:resource="http://purl.org/olia/olia.owl#AbstractEntity"/>
  </rdf:Description>
  <rdf:Description rdf:about="http://purl.org/olia/discourse/olia_discourse.owl#AbstractEntity">
    <owl:deprecated rdf:datatype="http://www.w3.org/2001/XMLSchema#boolean">true</owl:deprecated>
  </rdf:Description>
  <rdf:Description rdf:about="http://purl.org/olia/discourse/olia_discourse.owl#Accessible">
    <terms:replacedBy rdf:resource="http://purl.org/olia/olia.owl#Accessible"/>
  </rdf:Description>
  <rdf:Description rdf:about="http://purl.org/olia/discourse/olia_discourse.owl#Accessible">
    <owl:deprecated rdf:datatype="http://www.w3.org/2001/XMLSchema#boolean">true</owl:deprecated>
  </rdf:Description>
  <rdf:Description rdf:about="http://purl.org/olia/discourse/olia_discourse.owl#Achievement">
    <terms:replacedBy rdf:resource="http://purl.org/olia/olia.owl#Achievement"/>
  </rdf:Description>
  <rdf:Description rdf:about="http://purl.org/olia/discourse/olia_discourse.owl#Achievement">
    <owl:deprecated rdf:datatype="http://www.w3.org/2001/XMLSchema#boolean">true</owl:deprecated>
  </rdf:Description>
  <rdf:Description rdf:about="http://purl.org/olia/discourse/olia_discourse.owl#Active">
    <terms:replacedBy rdf:resource="http://purl.org/olia/olia.owl#Active"/>
  </rdf:Description>
  <rdf:Description rdf:about="http://purl.org/olia/discourse/olia_discourse.owl#Active">
    <owl:deprecated rdf:datatype="http://www.w3.org/2001/XMLSchema#boolean">true</owl:deprecated>
  </rdf:Description>
  <rdf:Description rdf:about="http://purl.org/olia/discourse/olia_discourse.owl#Address">
    <terms:replacedBy rdf:resource="http://purl.org/olia/olia.owl#Address"/>
  </rdf:Description>
  <rdf:Description rdf:about="http://purl.org/olia/discourse/olia_discourse.owl#Address">
    <owl:deprecated rdf:datatype="http://www.w3.org/2001/XMLSchema#boolean">true</owl:deprecated>
  </rdf:Description>
  <rdf:Description rdf:about="http://purl.org/olia/discourse/olia_discourse.owl#AdministrativeRegion">
    <terms:replacedBy rdf:resource="http://purl.org/olia/olia.owl#AdministrativeRegion"/>
  </rdf:Description>
  <rdf:Description rdf:about="http://purl.org/olia/discourse/olia_discourse.owl#AdministrativeRegion">
    <owl:deprecated rdf:datatype="http://www.w3.org/2001/XMLSchema#boolean">true</owl:deprecated>
  </rdf:Description>
  <rdf:Description rdf:about="http://purl.org/olia/discourse/olia_discourse.owl#AdverbialFocus">
    <terms:replacedBy rdf:resource="http://purl.org/olia/olia.owl#AdverbialFocus"/>
  </rdf:Description>
  <rdf:Description rdf:about="http://purl.org/olia/discourse/olia_discourse.owl#AdverbialFocus">
    <owl:deprecated rdf:datatype="http://www.w3.org/2001/XMLSchema#boolean">true</owl:deprecated>
  </rdf:Description>
  <rdf:Description rdf:about="http://purl.org/olia/discourse/olia_discourse.owl#Aircraft">
    <terms:replacedBy rdf:resource="http://purl.org/olia/olia.owl#Aircraft"/>
  </rdf:Description>
  <rdf:Description rdf:about="http://purl.org/olia/discourse/olia_discourse.owl#Aircraft">
    <owl:deprecated rdf:datatype="http://www.w3.org/2001/XMLSchema#boolean">true</owl:deprecated>
  </rdf:Description>
  <rdf:Description rdf:about="http://purl.org/olia/discourse/olia_discourse.owl#Airline">
    <terms:replacedBy rdf:resource="http://purl.org/olia/olia.owl#Airline"/>
  </rdf:Description>
  <rdf:Description rdf:about="http://purl.org/olia/discourse/olia_discourse.owl#Airline">
    <owl:deprecated rdf:datatype="http://www.w3.org/2001/XMLSchema#boolean">true</owl:deprecated>
  </rdf:Description>
  <rdf:Description rdf:about="http://purl.org/olia/discourse/olia_discourse.owl#Airport">
    <terms:replacedBy rdf:resource="http://purl.org/olia/olia.owl#Airport"/>
  </rdf:Description>
  <rdf:Description rdf:about="http://purl.org/olia/discourse/olia_discourse.owl#Airport">
    <owl:deprecated rdf:datatype="http://www.w3.org/2001/XMLSchema#boolean">true</owl:deprecated>
  </rdf:Description>
  <rdf:Description rdf:about="http://purl.org/olia/discourse/olia_discourse.owl#Album">
    <terms:replacedBy rdf:resource="http://purl.org/olia/olia.owl#Album"/>
  </rdf:Description>
  <rdf:Description rdf:about="http://purl.org/olia/discourse/olia_discourse.owl#Album">
    <owl:deprecated rdf:datatype="http://www.w3.org/2001/XMLSchema#boolean">true</owl:deprecated>
  </rdf:Description>
  <rdf:Description rdf:about="http://purl.org/olia/discourse/olia_discourse.owl#Alternative">
    <terms:replacedBy rdf:resource="http://purl.org/olia/olia.owl#Alternative"/>
  </rdf:Description>
  <rdf:Description rdf:about="http://purl.org/olia/discourse/olia_discourse.owl#Alternative">
    <owl:deprecated rdf:datatype="http://www.w3.org/2001/XMLSchema#boolean">true</owl:deprecated>
  </rdf:Description>
  <rdf:Description rdf:about="http://purl.org/olia/discourse/olia_discourse.owl#AlternativeLexicalization">
    <terms:replacedBy rdf:resource="http://purl.org/olia/olia.owl#AlternativeLexicalization"/>
  </rdf:Description>
  <rdf:Description rdf:about="http://purl.org/olia/discourse/olia_discourse.owl#AlternativeLexicalization">
    <owl:deprecated rdf:datatype="http://www.w3.org/2001/XMLSchema#boolean">true</owl:deprecated>
  </rdf:Description>
  <rdf:Description rdf:about="http://purl.org/olia/discourse/olia_discourse.owl#Ambassador">
    <terms:replacedBy rdf:resource="http://purl.org/olia/olia.owl#Ambassador"/>
  </rdf:Description>
  <rdf:Description rdf:about="http://purl.org/olia/discourse/olia_discourse.owl#Ambassador">
    <owl:deprecated rdf:datatype="http://www.w3.org/2001/XMLSchema#boolean">true</owl:deprecated>
  </rdf:Description>
  <rdf:Description rdf:about="http://purl.org/olia/discourse/olia_discourse.owl#Amount">
    <terms:replacedBy rdf:resource="http://purl.org/olia/olia.owl#Amount"/>
  </rdf:Description>
  <rdf:Description rdf:about="http://purl.org/olia/discourse/olia_discourse.owl#Amount">
    <owl:deprecated rdf:datatype="http://www.w3.org/2001/XMLSchema#boolean">true</owl:deprecated>
  </rdf:Description>
  <rdf:Description rdf:about="http://purl.org/olia/discourse/olia_discourse.owl#Analogy_RST">
    <terms:replacedBy rdf:resource="http://purl.org/olia/olia.owl#Analogy_RST"/>
  </rdf:Description>
  <rdf:Description rdf:about="http://purl.org/olia/discourse/olia_discourse.owl#Analogy_RST">
    <owl:deprecated rdf:datatype="http://www.w3.org/2001/XMLSchema#boolean">true</owl:deprecated>
  </rdf:Description>
  <rdf:Description rdf:about="http://purl.org/olia/discourse/olia_discourse.owl#AnaphoricRelation">
    <terms:replacedBy rdf:resource="http://purl.org/olia/olia.owl#AnaphoricRelation"/>
  </rdf:Description>
  <rdf:Description rdf:about="http://purl.org/olia/discourse/olia_discourse.owl#AnaphoricRelation">
    <owl:deprecated rdf:datatype="http://www.w3.org/2001/XMLSchema#boolean">true</owl:deprecated>
  </rdf:Description>
  <rdf:Description rdf:about="http://purl.org/olia/discourse/olia_discourse.owl#Animal">
    <terms:replacedBy rdf:resource="http://purl.org/olia/olia.owl#Animal"/>
  </rdf:Description>
  <rdf:Description rdf:about="http://purl.org/olia/discourse/olia_discourse.owl#Animal">
    <owl:deprecated rdf:datatype="http://www.w3.org/2001/XMLSchema#boolean">true</owl:deprecated>
  </rdf:Description>
  <rdf:Description rdf:about="http://purl.org/olia/discourse/olia_discourse.owl#AnimateEntity">
    <terms:replacedBy rdf:resource="http://purl.org/olia/olia.owl#AnimateEntity"/>
  </rdf:Description>
  <rdf:Description rdf:about="http://purl.org/olia/discourse/olia_discourse.owl#AnimateEntity">
    <owl:deprecated rdf:datatype="http://www.w3.org/2001/XMLSchema#boolean">true</owl:deprecated>
  </rdf:Description>
  <rdf:Description rdf:about="http://purl.org/olia/discourse/olia_discourse.owl#Antithesis">
    <terms:replacedBy rdf:resource="http://purl.org/olia/olia.owl#Antithesis"/>
  </rdf:Description>
  <rdf:Description rdf:about="http://purl.org/olia/discourse/olia_discourse.owl#Antithesis">
    <owl:deprecated rdf:datatype="http://www.w3.org/2001/XMLSchema#boolean">true</owl:deprecated>
  </rdf:Description>
  <rdf:Description rdf:about="http://purl.org/olia/discourse/olia_discourse.owl#Antithesis_RST">
    <terms:replacedBy rdf:resource="http://purl.org/olia/olia.owl#Antithesis_RST"/>
  </rdf:Description>
  <rdf:Description rdf:about="http://purl.org/olia/discourse/olia_discourse.owl#Antithesis_RST">
    <owl:deprecated rdf:datatype="http://www.w3.org/2001/XMLSchema#boolean">true</owl:deprecated>
  </rdf:Description>
  <rdf:Description rdf:about="http://purl.org/olia/discourse/olia_discourse.owl#Apellation">
    <terms:replacedBy rdf:resource="http://purl.org/olia/olia.owl#Apellation"/>
  </rdf:Description>
  <rdf:Description rdf:about="http://purl.org/olia/discourse/olia_discourse.owl#Apellation">
    <owl:deprecated rdf:datatype="http://www.w3.org/2001/XMLSchema#boolean">true</owl:deprecated>
  </rdf:Description>
  <rdf:Description rdf:about="http://purl.org/olia/discourse/olia_discourse.owl#Architect">
    <terms:replacedBy rdf:resource="http://purl.org/olia/olia.owl#Architect"/>
  </rdf:Description>
  <rdf:Description rdf:about="http://purl.org/olia/discourse/olia_discourse.owl#Architect">
    <owl:deprecated rdf:datatype="http://www.w3.org/2001/XMLSchema#boolean">true</owl:deprecated>
  </rdf:Description>
  <rdf:Description rdf:about="http://purl.org/olia/discourse/olia_discourse.owl#ArchitecturalFeature">
    <terms:replacedBy rdf:resource="http://purl.org/olia/olia.owl#ArchitecturalFeature"/>
  </rdf:Description>
  <rdf:Description rdf:about="http://purl.org/olia/discourse/olia_discourse.owl#ArchitecturalFeature">
    <owl:deprecated rdf:datatype="http://www.w3.org/2001/XMLSchema#boolean">true</owl:deprecated>
  </rdf:Description>
  <rdf:Description rdf:about="http://purl.org/olia/discourse/olia_discourse.owl#ArgumentFocus">
    <terms:replacedBy rdf:resource="http://purl.org/olia/olia.owl#ArgumentFocus"/>
  </rdf:Description>
  <rdf:Description rdf:about="http://purl.org/olia/discourse/olia_discourse.owl#ArgumentFocus">
    <owl:deprecated rdf:datatype="http://www.w3.org/2001/XMLSchema#boolean">true</owl:deprecated>
  </rdf:Description>
  <rdf:Description rdf:about="http://purl.org/olia/discourse/olia_discourse.owl#ArticleTopLevelSchema">
    <terms:replacedBy rdf:resource="http://purl.org/olia/olia.owl#ArticleTopLevelSchema"/>
  </rdf:Description>
  <rdf:Description rdf:about="http://purl.org/olia/discourse/olia_discourse.owl#ArticleTopLevelSchema">
    <owl:deprecated rdf:datatype="http://www.w3.org/2001/XMLSchema#boolean">true</owl:deprecated>
  </rdf:Description>
  <rdf:Description rdf:about="http://purl.org/olia/discourse/olia_discourse.owl#Artist">
    <terms:replacedBy rdf:resource="http://purl.org/olia/olia.owl#Artist"/>
  </rdf:Description>
  <rdf:Description rdf:about="http://purl.org/olia/discourse/olia_discourse.owl#Artist">
    <owl:deprecated rdf:datatype="http://www.w3.org/2001/XMLSchema#boolean">true</owl:deprecated>
  </rdf:Description>
  <rdf:Description rdf:about="http://purl.org/olia/discourse/olia_discourse.owl#Assertion">
    <terms:replacedBy rdf:resource="http://purl.org/olia/olia.owl#Assertion"/>
  </rdf:Description>
  <rdf:Description rdf:about="http://purl.org/olia/discourse/olia_discourse.owl#Assertion">
    <owl:deprecated rdf:datatype="http://www.w3.org/2001/XMLSchema#boolean">true</owl:deprecated>
  </rdf:Description>
  <rdf:Description rdf:about="http://purl.org/olia/discourse/olia_discourse.owl#Assessment">
    <terms:replacedBy rdf:resource="http://purl.org/olia/olia.owl#Assessment"/>
  </rdf:Description>
  <rdf:Description rdf:about="http://purl.org/olia/discourse/olia_discourse.owl#Assessment">
    <owl:deprecated rdf:datatype="http://www.w3.org/2001/XMLSchema#boolean">true</owl:deprecated>
  </rdf:Description>
  <rdf:Description rdf:about="http://purl.org/olia/discourse/olia_discourse.owl#Astronaut">
    <terms:replacedBy rdf:resource="http://purl.org/olia/olia.owl#Astronaut"/>
  </rdf:Description>
  <rdf:Description rdf:about="http://purl.org/olia/discourse/olia_discourse.owl#Astronaut">
    <owl:deprecated rdf:datatype="http://www.w3.org/2001/XMLSchema#boolean">true</owl:deprecated>
  </rdf:Description>
  <rdf:Description rdf:about="http://purl.org/olia/discourse/olia_discourse.owl#AsynchronousRelation">
    <terms:replacedBy rdf:resource="http://purl.org/olia/olia.owl#AsynchronousRelation"/>
  </rdf:Description>
  <rdf:Description rdf:about="http://purl.org/olia/discourse/olia_discourse.owl#AsynchronousRelation">
    <owl:deprecated rdf:datatype="http://www.w3.org/2001/XMLSchema#boolean">true</owl:deprecated>
  </rdf:Description>
  <rdf:Description rdf:about="http://purl.org/olia/discourse/olia_discourse.owl#Athlete">
    <terms:replacedBy rdf:resource="http://purl.org/olia/olia.owl#Athlete"/>
  </rdf:Description>
  <rdf:Description rdf:about="http://purl.org/olia/discourse/olia_discourse.owl#Athlete">
    <owl:deprecated rdf:datatype="http://www.w3.org/2001/XMLSchema#boolean">true</owl:deprecated>
  </rdf:Description>
  <rdf:Description rdf:about="http://purl.org/olia/discourse/olia_discourse.owl#Attribution">
    <terms:replacedBy rdf:resource="http://purl.org/olia/olia.owl#Attribution"/>
  </rdf:Description>
  <rdf:Description rdf:about="http://purl.org/olia/discourse/olia_discourse.owl#Attribution">
    <owl:deprecated rdf:datatype="http://www.w3.org/2001/XMLSchema#boolean">true</owl:deprecated>
  </rdf:Description>
  <rdf:Description rdf:about="http://purl.org/olia/discourse/olia_discourse.owl#AttributionSource">
    <terms:replacedBy rdf:resource="http://purl.org/olia/olia.owl#AttributionSource"/>
  </rdf:Description>
  <rdf:Description rdf:about="http://purl.org/olia/discourse/olia_discourse.owl#AttributionSource">
    <owl:deprecated rdf:datatype="http://www.w3.org/2001/XMLSchema#boolean">true</owl:deprecated>
  </rdf:Description>
  <rdf:Description rdf:about="http://purl.org/olia/discourse/olia_discourse.owl#Author">
    <terms:replacedBy rdf:resource="http://purl.org/olia/olia.owl#Author"/>
  </rdf:Description>
  <rdf:Description rdf:about="http://purl.org/olia/discourse/olia_discourse.owl#Author">
    <owl:deprecated rdf:datatype="http://www.w3.org/2001/XMLSchema#boolean">true</owl:deprecated>
  </rdf:Description>
  <rdf:Description rdf:about="http://purl.org/olia/discourse/olia_discourse.owl#AuthorAttributionSource">
    <terms:replacedBy rdf:resource="http://purl.org/olia/olia.owl#AuthorAttributionSource"/>
  </rdf:Description>
  <rdf:Description rdf:about="http://purl.org/olia/discourse/olia_discourse.owl#AuthorAttributionSource">
    <owl:deprecated rdf:datatype="http://www.w3.org/2001/XMLSchema#boolean">true</owl:deprecated>
  </rdf:Description>
  <rdf:Description rdf:about="http://purl.org/olia/discourse/olia_discourse.owl#Automobile">
    <terms:replacedBy rdf:resource="http://purl.org/olia/olia.owl#Automobile"/>
  </rdf:Description>
  <rdf:Description rdf:about="http://purl.org/olia/discourse/olia_discourse.owl#Automobile">
    <owl:deprecated rdf:datatype="http://www.w3.org/2001/XMLSchema#boolean">true</owl:deprecated>
  </rdf:Description>
  <rdf:Description rdf:about="http://purl.org/olia/discourse/olia_discourse.owl#Background">
    <terms:replacedBy rdf:resource="http://purl.org/olia/olia.owl#Background"/>
  </rdf:Description>
  <rdf:Description rdf:about="http://purl.org/olia/discourse/olia_discourse.owl#Background">
    <owl:deprecated rdf:datatype="http://www.w3.org/2001/XMLSchema#boolean">true</owl:deprecated>
  </rdf:Description>
  <rdf:Description rdf:about="http://purl.org/olia/discourse/olia_discourse.owl#Background_RST">
    <terms:replacedBy rdf:resource="http://purl.org/olia/olia.owl#Background_RST"/>
  </rdf:Description>
  <rdf:Description rdf:about="http://purl.org/olia/discourse/olia_discourse.owl#Background_RST">
    <owl:deprecated rdf:datatype="http://www.w3.org/2001/XMLSchema#boolean">true</owl:deprecated>
  </rdf:Description>
  <rdf:Description rdf:about="http://purl.org/olia/discourse/olia_discourse.owl#Band">
    <terms:replacedBy rdf:resource="http://purl.org/olia/olia.owl#Band"/>
  </rdf:Description>
  <rdf:Description rdf:about="http://purl.org/olia/discourse/olia_discourse.owl#Band">
    <owl:deprecated rdf:datatype="http://www.w3.org/2001/XMLSchema#boolean">true</owl:deprecated>
  </rdf:Description>
  <rdf:Description rdf:about="http://purl.org/olia/discourse/olia_discourse.owl#Belief">
    <terms:replacedBy rdf:resource="http://purl.org/olia/olia.owl#Belief"/>
  </rdf:Description>
  <rdf:Description rdf:about="http://purl.org/olia/discourse/olia_discourse.owl#Belief">
    <owl:deprecated rdf:datatype="http://www.w3.org/2001/XMLSchema#boolean">true</owl:deprecated>
  </rdf:Description>
  <rdf:Description rdf:about="http://purl.org/olia/discourse/olia_discourse.owl#BenchLevelRegister">
    <terms:replacedBy rdf:resource="http://purl.org/olia/olia.owl#BenchLevelRegister"/>
  </rdf:Description>
  <rdf:Description rdf:about="http://purl.org/olia/discourse/olia_discourse.owl#BenchLevelRegister">
    <owl:deprecated rdf:datatype="http://www.w3.org/2001/XMLSchema#boolean">true</owl:deprecated>
  </rdf:Description>
  <rdf:Description rdf:about="http://purl.org/olia/discourse/olia_discourse.owl#Bird">
    <terms:replacedBy rdf:resource="http://purl.org/olia/olia.owl#Bird"/>
  </rdf:Description>
  <rdf:Description rdf:about="http://purl.org/olia/discourse/olia_discourse.owl#Bird">
    <owl:deprecated rdf:datatype="http://www.w3.org/2001/XMLSchema#boolean">true</owl:deprecated>
  </rdf:Description>
  <rdf:Description rdf:about="http://purl.org/olia/discourse/olia_discourse.owl#Boilerplate">
    <terms:replacedBy rdf:resource="http://purl.org/olia/olia.owl#Boilerplate"/>
  </rdf:Description>
  <rdf:Description rdf:about="http://purl.org/olia/discourse/olia_discourse.owl#Boilerplate">
    <owl:deprecated rdf:datatype="http://www.w3.org/2001/XMLSchema#boolean">true</owl:deprecated>
  </rdf:Description>
  <rdf:Description rdf:about="http://purl.org/olia/discourse/olia_discourse.owl#Book">
    <terms:replacedBy rdf:resource="http://purl.org/olia/olia.owl#Book"/>
  </rdf:Description>
  <rdf:Description rdf:about="http://purl.org/olia/discourse/olia_discourse.owl#Book">
    <owl:deprecated rdf:datatype="http://www.w3.org/2001/XMLSchema#boolean">true</owl:deprecated>
  </rdf:Description>
  <rdf:Description rdf:about="http://purl.org/olia/discourse/olia_discourse.owl#Bridge">
    <terms:replacedBy rdf:resource="http://purl.org/olia/olia.owl#Bridge"/>
  </rdf:Description>
  <rdf:Description rdf:about="http://purl.org/olia/discourse/olia_discourse.owl#Bridge">
    <owl:deprecated rdf:datatype="http://www.w3.org/2001/XMLSchema#boolean">true</owl:deprecated>
  </rdf:Description>
  <rdf:Description rdf:about="http://purl.org/olia/discourse/olia_discourse.owl#BridgingRelation">
    <terms:replacedBy rdf:resource="http://purl.org/olia/olia.owl#BridgingRelation"/>
  </rdf:Description>
  <rdf:Description rdf:about="http://purl.org/olia/discourse/olia_discourse.owl#BridgingRelation">
    <owl:deprecated rdf:datatype="http://www.w3.org/2001/XMLSchema#boolean">true</owl:deprecated>
  </rdf:Description>
  <rdf:Description rdf:about="http://purl.org/olia/discourse/olia_discourse.owl#BridgingType">
    <terms:replacedBy rdf:resource="http://purl.org/olia/olia.owl#BridgingType"/>
  </rdf:Description>
  <rdf:Description rdf:about="http://purl.org/olia/discourse/olia_discourse.owl#BridgingType">
    <owl:deprecated rdf:datatype="http://www.w3.org/2001/XMLSchema#boolean">true</owl:deprecated>
  </rdf:Description>
  <rdf:Description rdf:about="http://purl.org/olia/discourse/olia_discourse.owl#Broadcast">
    <terms:replacedBy rdf:resource="http://purl.org/olia/olia.owl#Broadcast"/>
  </rdf:Description>
  <rdf:Description rdf:about="http://purl.org/olia/discourse/olia_discourse.owl#Broadcast">
    <owl:deprecated rdf:datatype="http://www.w3.org/2001/XMLSchema#boolean">true</owl:deprecated>
  </rdf:Description>
  <rdf:Description rdf:about="http://purl.org/olia/discourse/olia_discourse.owl#BroadcastingOrganization">
    <terms:replacedBy rdf:resource="http://purl.org/olia/olia.owl#BroadcastingOrganization"/>
  </rdf:Description>
  <rdf:Description rdf:about="http://purl.org/olia/discourse/olia_discourse.owl#BroadcastingOrganization">
    <owl:deprecated rdf:datatype="http://www.w3.org/2001/XMLSchema#boolean">true</owl:deprecated>
  </rdf:Description>
  <rdf:Description rdf:about="http://purl.org/olia/discourse/olia_discourse.owl#Canal">
    <terms:replacedBy rdf:resource="http://purl.org/olia/olia.owl#Canal"/>
  </rdf:Description>
  <rdf:Description rdf:about="http://purl.org/olia/discourse/olia_discourse.owl#Canal">
    <owl:deprecated rdf:datatype="http://www.w3.org/2001/XMLSchema#boolean">true</owl:deprecated>
  </rdf:Description>
  <rdf:Description rdf:about="http://purl.org/olia/discourse/olia_discourse.owl#Cause">
    <terms:replacedBy rdf:resource="http://purl.org/olia/olia.owl#Cause"/>
  </rdf:Description>
  <rdf:Description rdf:about="http://purl.org/olia/discourse/olia_discourse.owl#Cause">
    <owl:deprecated rdf:datatype="http://www.w3.org/2001/XMLSchema#boolean">true</owl:deprecated>
  </rdf:Description>
  <rdf:Description rdf:about="http://purl.org/olia/discourse/olia_discourse.owl#CausePrecedesEffect_PDTB">
    <terms:replacedBy rdf:resource="http://purl.org/olia/olia.owl#CausePrecedesEffect_PDTB"/>
  </rdf:Description>
  <rdf:Description rdf:about="http://purl.org/olia/discourse/olia_discourse.owl#CausePrecedesEffect_PDTB">
    <owl:deprecated rdf:datatype="http://www.w3.org/2001/XMLSchema#boolean">true</owl:deprecated>
  </rdf:Description>
  <rdf:Description rdf:about="http://purl.org/olia/discourse/olia_discourse.owl#CauseResult_RST">
    <terms:replacedBy rdf:resource="http://purl.org/olia/olia.owl#CauseResult_RST"/>
  </rdf:Description>
  <rdf:Description rdf:about="http://purl.org/olia/discourse/olia_discourse.owl#CauseResult_RST">
    <owl:deprecated rdf:datatype="http://www.w3.org/2001/XMLSchema#boolean">true</owl:deprecated>
  </rdf:Description>
  <rdf:Description rdf:about="http://purl.org/olia/discourse/olia_discourse.owl#Cause_RST">
    <terms:replacedBy rdf:resource="http://purl.org/olia/olia.owl#Cause_RST"/>
  </rdf:Description>
  <rdf:Description rdf:about="http://purl.org/olia/discourse/olia_discourse.owl#Cause_RST">
    <owl:deprecated rdf:datatype="http://www.w3.org/2001/XMLSchema#boolean">true</owl:deprecated>
  </rdf:Description>
  <rdf:Description rdf:about="http://purl.org/olia/discourse/olia_discourse.owl#Celebrity">
    <terms:replacedBy rdf:resource="http://purl.org/olia/olia.owl#Celebrity"/>
  </rdf:Description>
  <rdf:Description rdf:about="http://purl.org/olia/discourse/olia_discourse.owl#Celebrity">
    <owl:deprecated rdf:datatype="http://www.w3.org/2001/XMLSchema#boolean">true</owl:deprecated>
  </rdf:Description>
  <rdf:Description rdf:about="http://purl.org/olia/discourse/olia_discourse.owl#ChosenAlternative_PDTB">
    <terms:replacedBy rdf:resource="http://purl.org/olia/olia.owl#ChosenAlternative_PDTB"/>
  </rdf:Description>
  <rdf:Description rdf:about="http://purl.org/olia/discourse/olia_discourse.owl#ChosenAlternative_PDTB">
    <owl:deprecated rdf:datatype="http://www.w3.org/2001/XMLSchema#boolean">true</owl:deprecated>
  </rdf:Description>
  <rdf:Description rdf:about="http://purl.org/olia/discourse/olia_discourse.owl#Circumstance">
    <terms:replacedBy rdf:resource="http://purl.org/olia/olia.owl#Circumstance"/>
  </rdf:Description>
  <rdf:Description rdf:about="http://purl.org/olia/discourse/olia_discourse.owl#Circumstance">
    <owl:deprecated rdf:datatype="http://www.w3.org/2001/XMLSchema#boolean">true</owl:deprecated>
  </rdf:Description>
  <rdf:Description rdf:about="http://purl.org/olia/discourse/olia_discourse.owl#Circumstance_RST">
    <terms:replacedBy rdf:resource="http://purl.org/olia/olia.owl#Circumstance_RST"/>
  </rdf:Description>
  <rdf:Description rdf:about="http://purl.org/olia/discourse/olia_discourse.owl#Circumstance_RST">
    <owl:deprecated rdf:datatype="http://www.w3.org/2001/XMLSchema#boolean">true</owl:deprecated>
  </rdf:Description>
  <rdf:Description rdf:about="http://purl.org/olia/discourse/olia_discourse.owl#Citation">
    <terms:replacedBy rdf:resource="http://purl.org/olia/olia.owl#Citation"/>
  </rdf:Description>
  <rdf:Description rdf:about="http://purl.org/olia/discourse/olia_discourse.owl#Citation">
    <owl:deprecated rdf:datatype="http://www.w3.org/2001/XMLSchema#boolean">true</owl:deprecated>
  </rdf:Description>
  <rdf:Description rdf:about="http://purl.org/olia/discourse/olia_discourse.owl#CitationAttribution">
    <terms:replacedBy rdf:resource="http://purl.org/olia/olia.owl#CitationAttribution"/>
  </rdf:Description>
  <rdf:Description rdf:about="http://purl.org/olia/discourse/olia_discourse.owl#CitationAttribution">
    <owl:deprecated rdf:datatype="http://www.w3.org/2001/XMLSchema#boolean">true</owl:deprecated>
  </rdf:Description>
  <rdf:Description rdf:about="http://purl.org/olia/discourse/olia_discourse.owl#CitationEvidence">
    <terms:replacedBy rdf:resource="http://purl.org/olia/olia.owl#CitationEvidence"/>
  </rdf:Description>
  <rdf:Description rdf:about="http://purl.org/olia/discourse/olia_discourse.owl#CitationEvidence">
    <owl:deprecated rdf:datatype="http://www.w3.org/2001/XMLSchema#boolean">true</owl:deprecated>
  </rdf:Description>
  <rdf:Description rdf:about="http://purl.org/olia/discourse/olia_discourse.owl#CitationSelf">
    <terms:replacedBy rdf:resource="http://purl.org/olia/olia.owl#CitationSelf"/>
  </rdf:Description>
  <rdf:Description rdf:about="http://purl.org/olia/discourse/olia_discourse.owl#CitationSelf">
    <owl:deprecated rdf:datatype="http://www.w3.org/2001/XMLSchema#boolean">true</owl:deprecated>
  </rdf:Description>
  <rdf:Description rdf:about="http://purl.org/olia/discourse/olia_discourse.owl#City">
    <terms:replacedBy rdf:resource="http://purl.org/olia/olia.owl#City"/>
  </rdf:Description>
  <rdf:Description rdf:about="http://purl.org/olia/discourse/olia_discourse.owl#City">
    <owl:deprecated rdf:datatype="http://www.w3.org/2001/XMLSchema#boolean">true</owl:deprecated>
  </rdf:Description>
  <rdf:Description rdf:about="http://purl.org/olia/discourse/olia_discourse.owl#CoherenceRelation">
    <terms:replacedBy rdf:resource="http://purl.org/olia/olia.owl#CoherenceRelation"/>
  </rdf:Description>
  <rdf:Description rdf:about="http://purl.org/olia/discourse/olia_discourse.owl#CoherenceRelation">
    <owl:deprecated rdf:datatype="http://www.w3.org/2001/XMLSchema#boolean">true</owl:deprecated>
  </rdf:Description>
  <rdf:Description rdf:about="http://purl.org/olia/discourse/olia_discourse.owl#ColumnTitle">
    <terms:replacedBy rdf:resource="http://purl.org/olia/olia.owl#ColumnTitle"/>
  </rdf:Description>
  <rdf:Description rdf:about="http://purl.org/olia/discourse/olia_discourse.owl#ColumnTitle">
    <owl:deprecated rdf:datatype="http://www.w3.org/2001/XMLSchema#boolean">true</owl:deprecated>
  </rdf:Description>
  <rdf:Description rdf:about="http://purl.org/olia/discourse/olia_discourse.owl#ComicsCharacter">
    <terms:replacedBy rdf:resource="http://purl.org/olia/olia.owl#ComicsCharacter"/>
  </rdf:Description>
  <rdf:Description rdf:about="http://purl.org/olia/discourse/olia_discourse.owl#ComicsCharacter">
    <owl:deprecated rdf:datatype="http://www.w3.org/2001/XMLSchema#boolean">true</owl:deprecated>
  </rdf:Description>
  <rdf:Description rdf:about="http://purl.org/olia/discourse/olia_discourse.owl#Comment_RST">
    <terms:replacedBy rdf:resource="http://purl.org/olia/olia.owl#Comment_RST"/>
  </rdf:Description>
  <rdf:Description rdf:about="http://purl.org/olia/discourse/olia_discourse.owl#Comment_RST">
    <owl:deprecated rdf:datatype="http://www.w3.org/2001/XMLSchema#boolean">true</owl:deprecated>
  </rdf:Description>
  <rdf:Description rdf:about="http://purl.org/olia/discourse/olia_discourse.owl#CommentTopic">
    <terms:replacedBy rdf:resource="http://purl.org/olia/olia.owl#CommentTopic"/>
  </rdf:Description>
  <rdf:Description rdf:about="http://purl.org/olia/discourse/olia_discourse.owl#CommentTopic">
    <owl:deprecated rdf:datatype="http://www.w3.org/2001/XMLSchema#boolean">true</owl:deprecated>
  </rdf:Description>
  <rdf:Description rdf:about="http://purl.org/olia/discourse/olia_discourse.owl#CommentTopic_RST">
    <terms:replacedBy rdf:resource="http://purl.org/olia/olia.owl#CommentTopic_RST"/>
  </rdf:Description>
  <rdf:Description rdf:about="http://purl.org/olia/discourse/olia_discourse.owl#CommentTopic_RST">
    <owl:deprecated rdf:datatype="http://www.w3.org/2001/XMLSchema#boolean">true</owl:deprecated>
  </rdf:Description>
  <rdf:Description rdf:about="http://purl.org/olia/discourse/olia_discourse.owl#CommonlyUsed">
    <terms:replacedBy rdf:resource="http://purl.org/olia/olia.owl#CommonlyUsed"/>
  </rdf:Description>
  <rdf:Description rdf:about="http://purl.org/olia/discourse/olia_discourse.owl#CommonlyUsed">
    <owl:deprecated rdf:datatype="http://www.w3.org/2001/XMLSchema#boolean">true</owl:deprecated>
  </rdf:Description>
  <rdf:Description rdf:about="http://purl.org/olia/discourse/olia_discourse.owl#Company">
    <terms:replacedBy rdf:resource="http://purl.org/olia/olia.owl#Company"/>
  </rdf:Description>
  <rdf:Description rdf:about="http://purl.org/olia/discourse/olia_discourse.owl#Company">
    <owl:deprecated rdf:datatype="http://www.w3.org/2001/XMLSchema#boolean">true</owl:deprecated>
  </rdf:Description>
  <rdf:Description rdf:about="http://purl.org/olia/discourse/olia_discourse.owl#Comparison">
    <terms:replacedBy rdf:resource="http://purl.org/olia/olia.owl#Comparison"/>
  </rdf:Description>
  <rdf:Description rdf:about="http://purl.org/olia/discourse/olia_discourse.owl#Comparison">
    <owl:deprecated rdf:datatype="http://www.w3.org/2001/XMLSchema#boolean">true</owl:deprecated>
  </rdf:Description>
  <rdf:Description rdf:about="http://purl.org/olia/discourse/olia_discourse.owl#Comparison_RST">
    <terms:replacedBy rdf:resource="http://purl.org/olia/olia.owl#Comparison_RST"/>
  </rdf:Description>
  <rdf:Description rdf:about="http://purl.org/olia/discourse/olia_discourse.owl#Comparison_RST">
    <owl:deprecated rdf:datatype="http://www.w3.org/2001/XMLSchema#boolean">true</owl:deprecated>
  </rdf:Description>
  <rdf:Description rdf:about="http://purl.org/olia/discourse/olia_discourse.owl#ComplexDiscourseSegment">
    <terms:replacedBy rdf:resource="http://purl.org/olia/olia.owl#ComplexDiscourseSegment"/>
  </rdf:Description>
  <rdf:Description rdf:about="http://purl.org/olia/discourse/olia_discourse.owl#ComplexDiscourseSegment">
    <owl:deprecated rdf:datatype="http://www.w3.org/2001/XMLSchema#boolean">true</owl:deprecated>
  </rdf:Description>
  <rdf:Description rdf:about="http://purl.org/olia/discourse/olia_discourse.owl#Concession">
    <terms:replacedBy rdf:resource="http://purl.org/olia/olia.owl#Concession"/>
  </rdf:Description>
  <rdf:Description rdf:about="http://purl.org/olia/discourse/olia_discourse.owl#Concession">
    <owl:deprecated rdf:datatype="http://www.w3.org/2001/XMLSchema#boolean">true</owl:deprecated>
  </rdf:Description>
  <rdf:Description rdf:about="http://purl.org/olia/discourse/olia_discourse.owl#Conclusion_RST">
    <terms:replacedBy rdf:resource="http://purl.org/olia/olia.owl#Conclusion_RST"/>
  </rdf:Description>
  <rdf:Description rdf:about="http://purl.org/olia/discourse/olia_discourse.owl#Conclusion_RST">
    <owl:deprecated rdf:datatype="http://www.w3.org/2001/XMLSchema#boolean">true</owl:deprecated>
  </rdf:Description>
  <rdf:Description rdf:about="http://purl.org/olia/discourse/olia_discourse.owl#ConcreteEntity">
    <terms:replacedBy rdf:resource="http://purl.org/olia/olia.owl#ConcreteEntity"/>
  </rdf:Description>
  <rdf:Description rdf:about="http://purl.org/olia/discourse/olia_discourse.owl#ConcreteEntity">
    <owl:deprecated rdf:datatype="http://www.w3.org/2001/XMLSchema#boolean">true</owl:deprecated>
  </rdf:Description>
  <rdf:Description rdf:about="http://purl.org/olia/discourse/olia_discourse.owl#Condition">
    <terms:replacedBy rdf:resource="http://purl.org/olia/olia.owl#Condition"/>
  </rdf:Description>
  <rdf:Description rdf:about="http://purl.org/olia/discourse/olia_discourse.owl#Condition">
    <owl:deprecated rdf:datatype="http://www.w3.org/2001/XMLSchema#boolean">true</owl:deprecated>
  </rdf:Description>
  <rdf:Description rdf:about="http://purl.org/olia/discourse/olia_discourse.owl#Conjunction">
    <terms:replacedBy rdf:resource="http://purl.org/olia/olia.owl#Conjunction"/>
  </rdf:Description>
  <rdf:Description rdf:about="http://purl.org/olia/discourse/olia_discourse.owl#Conjunction">
    <owl:deprecated rdf:datatype="http://www.w3.org/2001/XMLSchema#boolean">true</owl:deprecated>
  </rdf:Description>
  <rdf:Description rdf:about="http://purl.org/olia/discourse/olia_discourse.owl#Conjunctive_PDTB">
    <terms:replacedBy rdf:resource="http://purl.org/olia/olia.owl#Conjunctive_PDTB"/>
  </rdf:Description>
  <rdf:Description rdf:about="http://purl.org/olia/discourse/olia_discourse.owl#Conjunctive_PDTB">
    <owl:deprecated rdf:datatype="http://www.w3.org/2001/XMLSchema#boolean">true</owl:deprecated>
  </rdf:Description>
  <rdf:Description rdf:about="http://purl.org/olia/discourse/olia_discourse.owl#Consequence">
    <terms:replacedBy rdf:resource="http://purl.org/olia/olia.owl#Consequence"/>
  </rdf:Description>
  <rdf:Description rdf:about="http://purl.org/olia/discourse/olia_discourse.owl#Consequence">
    <owl:deprecated rdf:datatype="http://www.w3.org/2001/XMLSchema#boolean">true</owl:deprecated>
  </rdf:Description>
  <rdf:Description rdf:about="http://purl.org/olia/discourse/olia_discourse.owl#Consequence_RST">
    <terms:replacedBy rdf:resource="http://purl.org/olia/olia.owl#Consequence_RST"/>
  </rdf:Description>
  <rdf:Description rdf:about="http://purl.org/olia/discourse/olia_discourse.owl#Consequence_RST">
    <owl:deprecated rdf:datatype="http://www.w3.org/2001/XMLSchema#boolean">true</owl:deprecated>
  </rdf:Description>
  <rdf:Description rdf:about="http://purl.org/olia/discourse/olia_discourse.owl#ContextualVariation">
    <terms:replacedBy rdf:resource="http://purl.org/olia/olia.owl#ContextualVariation"/>
  </rdf:Description>
  <rdf:Description rdf:about="http://purl.org/olia/discourse/olia_discourse.owl#ContextualVariation">
    <owl:deprecated rdf:datatype="http://www.w3.org/2001/XMLSchema#boolean">true</owl:deprecated>
  </rdf:Description>
  <rdf:Description rdf:about="http://purl.org/olia/discourse/olia_discourse.owl#Contigency">
    <terms:replacedBy rdf:resource="http://purl.org/olia/olia.owl#Contigency"/>
  </rdf:Description>
  <rdf:Description rdf:about="http://purl.org/olia/discourse/olia_discourse.owl#Contigency">
    <owl:deprecated rdf:datatype="http://www.w3.org/2001/XMLSchema#boolean">true</owl:deprecated>
  </rdf:Description>
  <rdf:Description rdf:about="http://purl.org/olia/discourse/olia_discourse.owl#Contigency_RST">
    <terms:replacedBy rdf:resource="http://purl.org/olia/olia.owl#Contigency_RST"/>
  </rdf:Description>
  <rdf:Description rdf:about="http://purl.org/olia/discourse/olia_discourse.owl#Contigency_RST">
    <owl:deprecated rdf:datatype="http://www.w3.org/2001/XMLSchema#boolean">true</owl:deprecated>
  </rdf:Description>
  <rdf:Description rdf:about="http://purl.org/olia/discourse/olia_discourse.owl#Continent">
    <terms:replacedBy rdf:resource="http://purl.org/olia/olia.owl#Continent"/>
  </rdf:Description>
  <rdf:Description rdf:about="http://purl.org/olia/discourse/olia_discourse.owl#Continent">
    <owl:deprecated rdf:datatype="http://www.w3.org/2001/XMLSchema#boolean">true</owl:deprecated>
  </rdf:Description>
  <rdf:Description rdf:about="http://purl.org/olia/discourse/olia_discourse.owl#ContraExpectation">
    <terms:replacedBy rdf:resource="http://purl.org/olia/olia.owl#ContraExpectation"/>
  </rdf:Description>
  <rdf:Description rdf:about="http://purl.org/olia/discourse/olia_discourse.owl#ContraExpectation">
    <owl:deprecated rdf:datatype="http://www.w3.org/2001/XMLSchema#boolean">true</owl:deprecated>
  </rdf:Description>
  <rdf:Description rdf:about="http://purl.org/olia/discourse/olia_discourse.owl#Contrast">
    <terms:replacedBy rdf:resource="http://purl.org/olia/olia.owl#Contrast"/>
  </rdf:Description>
  <rdf:Description rdf:about="http://purl.org/olia/discourse/olia_discourse.owl#Contrast">
    <owl:deprecated rdf:datatype="http://www.w3.org/2001/XMLSchema#boolean">true</owl:deprecated>
  </rdf:Description>
  <rdf:Description rdf:about="http://purl.org/olia/discourse/olia_discourse.owl#ContrastiveComparison">
    <terms:replacedBy rdf:resource="http://purl.org/olia/olia.owl#ContrastiveComparison"/>
  </rdf:Description>
  <rdf:Description rdf:about="http://purl.org/olia/discourse/olia_discourse.owl#ContrastiveComparison">
    <owl:deprecated rdf:datatype="http://www.w3.org/2001/XMLSchema#boolean">true</owl:deprecated>
  </rdf:Description>
  <rdf:Description rdf:about="http://purl.org/olia/discourse/olia_discourse.owl#ContrastiveFocus">
    <terms:replacedBy rdf:resource="http://purl.org/olia/olia.owl#ContrastiveFocus"/>
  </rdf:Description>
  <rdf:Description rdf:about="http://purl.org/olia/discourse/olia_discourse.owl#ContrastiveFocus">
    <owl:deprecated rdf:datatype="http://www.w3.org/2001/XMLSchema#boolean">true</owl:deprecated>
  </rdf:Description>
  <rdf:Description rdf:about="http://purl.org/olia/discourse/olia_discourse.owl#Contrast_RST">
    <terms:replacedBy rdf:resource="http://purl.org/olia/olia.owl#Contrast_RST"/>
  </rdf:Description>
  <rdf:Description rdf:about="http://purl.org/olia/discourse/olia_discourse.owl#Contrast_RST">
    <owl:deprecated rdf:datatype="http://www.w3.org/2001/XMLSchema#boolean">true</owl:deprecated>
  </rdf:Description>
  <rdf:Description rdf:about="http://purl.org/olia/discourse/olia_discourse.owl#Coordination">
    <terms:replacedBy rdf:resource="http://purl.org/olia/olia.owl#Coordination"/>
  </rdf:Description>
  <rdf:Description rdf:about="http://purl.org/olia/discourse/olia_discourse.owl#Coordination">
    <owl:deprecated rdf:datatype="http://www.w3.org/2001/XMLSchema#boolean">true</owl:deprecated>
  </rdf:Description>
  <rdf:Description rdf:about="http://purl.org/olia/discourse/olia_discourse.owl#Country">
    <terms:replacedBy rdf:resource="http://purl.org/olia/olia.owl#Country"/>
  </rdf:Description>
  <rdf:Description rdf:about="http://purl.org/olia/discourse/olia_discourse.owl#Country">
    <owl:deprecated rdf:datatype="http://www.w3.org/2001/XMLSchema#boolean">true</owl:deprecated>
  </rdf:Description>
  <rdf:Description rdf:about="http://purl.org/olia/discourse/olia_discourse.owl#Criminal">
    <terms:replacedBy rdf:resource="http://purl.org/olia/olia.owl#Criminal"/>
  </rdf:Description>
  <rdf:Description rdf:about="http://purl.org/olia/discourse/olia_discourse.owl#Criminal">
    <owl:deprecated rdf:datatype="http://www.w3.org/2001/XMLSchema#boolean">true</owl:deprecated>
  </rdf:Description>
  <rdf:Description rdf:about="http://purl.org/olia/discourse/olia_discourse.owl#Date">
    <terms:replacedBy rdf:resource="http://purl.org/olia/olia.owl#Date"/>
  </rdf:Description>
  <rdf:Description rdf:about="http://purl.org/olia/discourse/olia_discourse.owl#Date">
    <owl:deprecated rdf:datatype="http://www.w3.org/2001/XMLSchema#boolean">true</owl:deprecated>
  </rdf:Description>
  <rdf:Description rdf:about="http://purl.org/olia/discourse/olia_discourse.owl#Definite">
    <terms:replacedBy rdf:resource="http://purl.org/olia/olia.owl#Definite"/>
  </rdf:Description>
  <rdf:Description rdf:about="http://purl.org/olia/discourse/olia_discourse.owl#Definite">
    <owl:deprecated rdf:datatype="http://www.w3.org/2001/XMLSchema#boolean">true</owl:deprecated>
  </rdf:Description>
  <rdf:Description rdf:about="http://purl.org/olia/discourse/olia_discourse.owl#Definiteness">
    <terms:replacedBy rdf:resource="http://purl.org/olia/olia.owl#Definiteness"/>
  </rdf:Description>
  <rdf:Description rdf:about="http://purl.org/olia/discourse/olia_discourse.owl#Definiteness">
    <owl:deprecated rdf:datatype="http://www.w3.org/2001/XMLSchema#boolean">true</owl:deprecated>
  </rdf:Description>
  <rdf:Description rdf:about="http://purl.org/olia/discourse/olia_discourse.owl#Definition">
    <terms:replacedBy rdf:resource="http://purl.org/olia/olia.owl#Definition"/>
  </rdf:Description>
  <rdf:Description rdf:about="http://purl.org/olia/discourse/olia_discourse.owl#Definition">
    <owl:deprecated rdf:datatype="http://www.w3.org/2001/XMLSchema#boolean">true</owl:deprecated>
  </rdf:Description>
  <rdf:Description rdf:about="http://purl.org/olia/discourse/olia_discourse.owl#Definition_RST">
    <terms:replacedBy rdf:resource="http://purl.org/olia/olia.owl#Definition_RST"/>
  </rdf:Description>
  <rdf:Description rdf:about="http://purl.org/olia/discourse/olia_discourse.owl#Definition_RST">
    <owl:deprecated rdf:datatype="http://www.w3.org/2001/XMLSchema#boolean">true</owl:deprecated>
  </rdf:Description>
  <rdf:Description rdf:about="http://purl.org/olia/discourse/olia_discourse.owl#denotates">
    <terms:replacedBy rdf:resource="http://purl.org/olia/olia.owl#denotates"/>
  </rdf:Description>
  <rdf:Description rdf:about="http://purl.org/olia/discourse/olia_discourse.owl#denotates">
    <owl:deprecated rdf:datatype="http://www.w3.org/2001/XMLSchema#boolean">true</owl:deprecated>
  </rdf:Description>
  <rdf:Description rdf:about="http://purl.org/olia/discourse/olia_discourse.owl#DenotationFocus">
    <terms:replacedBy rdf:resource="http://purl.org/olia/olia.owl#DenotationFocus"/>
  </rdf:Description>
  <rdf:Description rdf:about="http://purl.org/olia/discourse/olia_discourse.owl#DenotationFocus">
    <owl:deprecated rdf:datatype="http://www.w3.org/2001/XMLSchema#boolean">true</owl:deprecated>
  </rdf:Description>
  <rdf:Description rdf:about="http://purl.org/olia/discourse/olia_discourse.owl#Deprecated">
    <terms:replacedBy rdf:resource="http://purl.org/olia/olia.owl#Deprecated"/>
  </rdf:Description>
  <rdf:Description rdf:about="http://purl.org/olia/discourse/olia_discourse.owl#Deprecated">
    <owl:deprecated rdf:datatype="http://www.w3.org/2001/XMLSchema#boolean">true</owl:deprecated>
  </rdf:Description>
  <rdf:Description rdf:about="http://purl.org/olia/discourse/olia_discourse.owl#DeterminateAttribution">
    <terms:replacedBy rdf:resource="http://purl.org/olia/olia.owl#DeterminateAttribution"/>
  </rdf:Description>
  <rdf:Description rdf:about="http://purl.org/olia/discourse/olia_discourse.owl#DeterminateAttribution">
    <owl:deprecated rdf:datatype="http://www.w3.org/2001/XMLSchema#boolean">true</owl:deprecated>
  </rdf:Description>
  <rdf:Description rdf:about="http://purl.org/olia/discourse/olia_discourse.owl#DialectRegister">
    <terms:replacedBy rdf:resource="http://purl.org/olia/olia.owl#DialectRegister"/>
  </rdf:Description>
  <rdf:Description rdf:about="http://purl.org/olia/discourse/olia_discourse.owl#DialectRegister">
    <owl:deprecated rdf:datatype="http://www.w3.org/2001/XMLSchema#boolean">true</owl:deprecated>
  </rdf:Description>
  <rdf:Description rdf:about="http://purl.org/olia/discourse/olia_discourse.owl#DialogRelation">
    <terms:replacedBy rdf:resource="http://purl.org/olia/olia.owl#DialogRelation"/>
  </rdf:Description>
  <rdf:Description rdf:about="http://purl.org/olia/discourse/olia_discourse.owl#DialogRelation">
    <owl:deprecated rdf:datatype="http://www.w3.org/2001/XMLSchema#boolean">true</owl:deprecated>
  </rdf:Description>
  <rdf:Description rdf:about="http://purl.org/olia/discourse/olia_discourse.owl#DirectSpeech">
    <terms:replacedBy rdf:resource="http://purl.org/olia/olia.owl#DirectSpeech"/>
  </rdf:Description>
  <rdf:Description rdf:about="http://purl.org/olia/discourse/olia_discourse.owl#DirectSpeech">
    <owl:deprecated rdf:datatype="http://www.w3.org/2001/XMLSchema#boolean">true</owl:deprecated>
  </rdf:Description>
  <rdf:Description rdf:about="http://purl.org/olia/discourse/olia_discourse.owl#DiscourseAdverbial">
    <terms:replacedBy rdf:resource="http://purl.org/olia/olia.owl#DiscourseAdverbial"/>
  </rdf:Description>
  <rdf:Description rdf:about="http://purl.org/olia/discourse/olia_discourse.owl#DiscourseAdverbial">
    <owl:deprecated rdf:datatype="http://www.w3.org/2001/XMLSchema#boolean">true</owl:deprecated>
  </rdf:Description>
  <rdf:Description rdf:about="http://purl.org/olia/discourse/olia_discourse.owl#DiscourseFunction">
    <terms:replacedBy rdf:resource="http://purl.org/olia/olia.owl#DiscourseFunction"/>
  </rdf:Description>
  <rdf:Description rdf:about="http://purl.org/olia/discourse/olia_discourse.owl#DiscourseFunction">
    <owl:deprecated rdf:datatype="http://www.w3.org/2001/XMLSchema#boolean">true</owl:deprecated>
  </rdf:Description>
  <rdf:Description rdf:about="http://purl.org/olia/discourse/olia_discourse.owl#DiscourseReferent">
    <terms:replacedBy rdf:resource="http://purl.org/olia/olia.owl#DiscourseReferent"/>
  </rdf:Description>
  <rdf:Description rdf:about="http://purl.org/olia/discourse/olia_discourse.owl#DiscourseReferent">
    <owl:deprecated rdf:datatype="http://www.w3.org/2001/XMLSchema#boolean">true</owl:deprecated>
  </rdf:Description>
  <rdf:Description rdf:about="http://purl.org/olia/discourse/olia_discourse.owl#DiscourseRelation">
    <terms:replacedBy rdf:resource="http://purl.org/olia/olia.owl#DiscourseRelation"/>
  </rdf:Description>
  <rdf:Description rdf:about="http://purl.org/olia/discourse/olia_discourse.owl#DiscourseRelation">
    <owl:deprecated rdf:datatype="http://www.w3.org/2001/XMLSchema#boolean">true</owl:deprecated>
  </rdf:Description>
  <rdf:Description rdf:about="http://purl.org/olia/discourse/olia_discourse.owl#DiscourseSegment">
    <terms:replacedBy rdf:resource="http://purl.org/olia/olia.owl#DiscourseSegment"/>
  </rdf:Description>
  <rdf:Description rdf:about="http://purl.org/olia/discourse/olia_discourse.owl#DiscourseSegment">
    <owl:deprecated rdf:datatype="http://www.w3.org/2001/XMLSchema#boolean">true</owl:deprecated>
  </rdf:Description>
  <rdf:Description rdf:about="http://purl.org/olia/discourse/olia_discourse.owl#DiscourseStructuralPattern">
    <terms:replacedBy rdf:resource="http://purl.org/olia/olia.owl#DiscourseStructuralPattern"/>
  </rdf:Description>
  <rdf:Description rdf:about="http://purl.org/olia/discourse/olia_discourse.owl#DiscourseStructuralPattern">
    <owl:deprecated rdf:datatype="http://www.w3.org/2001/XMLSchema#boolean">true</owl:deprecated>
  </rdf:Description>
  <rdf:Description rdf:about="http://purl.org/olia/discourse/olia_discourse.owl#DisfavouredAlternative">
    <terms:replacedBy rdf:resource="http://purl.org/olia/olia.owl#DisfavouredAlternative"/>
  </rdf:Description>
  <rdf:Description rdf:about="http://purl.org/olia/discourse/olia_discourse.owl#DisfavouredAlternative">
    <owl:deprecated rdf:datatype="http://www.w3.org/2001/XMLSchema#boolean">true</owl:deprecated>
  </rdf:Description>
  <rdf:Description rdf:about="http://purl.org/olia/discourse/olia_discourse.owl#Disjunctive">
    <terms:replacedBy rdf:resource="http://purl.org/olia/olia.owl#Disjunctive"/>
  </rdf:Description>
  <rdf:Description rdf:about="http://purl.org/olia/discourse/olia_discourse.owl#Disjunctive">
    <owl:deprecated rdf:datatype="http://www.w3.org/2001/XMLSchema#boolean">true</owl:deprecated>
  </rdf:Description>
  <rdf:Description rdf:about="http://purl.org/olia/discourse/olia_discourse.owl#Document">
    <terms:replacedBy rdf:resource="http://purl.org/olia/olia.owl#Document"/>
  </rdf:Description>
  <rdf:Description rdf:about="http://purl.org/olia/discourse/olia_discourse.owl#Document">
    <owl:deprecated rdf:datatype="http://www.w3.org/2001/XMLSchema#boolean">true</owl:deprecated>
  </rdf:Description>
  <rdf:Description rdf:about="http://purl.org/olia/discourse/olia_discourse.owl#Drug">
    <terms:replacedBy rdf:resource="http://purl.org/olia/olia.owl#Drug"/>
  </rdf:Description>
  <rdf:Description rdf:about="http://purl.org/olia/discourse/olia_discourse.owl#Drug">
    <owl:deprecated rdf:datatype="http://www.w3.org/2001/XMLSchema#boolean">true</owl:deprecated>
  </rdf:Description>
  <rdf:Description rdf:about="http://purl.org/olia/discourse/olia_discourse.owl#EducationalInstitution">
    <terms:replacedBy rdf:resource="http://purl.org/olia/olia.owl#EducationalInstitution"/>
  </rdf:Description>
  <rdf:Description rdf:about="http://purl.org/olia/discourse/olia_discourse.owl#EducationalInstitution">
    <owl:deprecated rdf:datatype="http://www.w3.org/2001/XMLSchema#boolean">true</owl:deprecated>
  </rdf:Description>
  <rdf:Description rdf:about="http://purl.org/olia/discourse/olia_discourse.owl#EffectPrecedesCause_PDTB">
    <terms:replacedBy rdf:resource="http://purl.org/olia/olia.owl#EffectPrecedesCause_PDTB"/>
  </rdf:Description>
  <rdf:Description rdf:about="http://purl.org/olia/discourse/olia_discourse.owl#EffectPrecedesCause_PDTB">
    <owl:deprecated rdf:datatype="http://www.w3.org/2001/XMLSchema#boolean">true</owl:deprecated>
  </rdf:Description>
  <rdf:Description rdf:about="http://purl.org/olia/discourse/olia_discourse.owl#Elaboration">
    <terms:replacedBy rdf:resource="http://purl.org/olia/olia.owl#Elaboration"/>
  </rdf:Description>
  <rdf:Description rdf:about="http://purl.org/olia/discourse/olia_discourse.owl#Elaboration">
    <owl:deprecated rdf:datatype="http://www.w3.org/2001/XMLSchema#boolean">true</owl:deprecated>
  </rdf:Description>
  <rdf:Description rdf:about="http://purl.org/olia/discourse/olia_discourse.owl#ElaborationAdditional_RST">
    <terms:replacedBy rdf:resource="http://purl.org/olia/olia.owl#ElaborationAdditional_RST"/>
  </rdf:Description>
  <rdf:Description rdf:about="http://purl.org/olia/discourse/olia_discourse.owl#ElaborationAdditional_RST">
    <owl:deprecated rdf:datatype="http://www.w3.org/2001/XMLSchema#boolean">true</owl:deprecated>
  </rdf:Description>
  <rdf:Description rdf:about="http://purl.org/olia/discourse/olia_discourse.owl#ElaborationAssign">
    <terms:replacedBy rdf:resource="http://purl.org/olia/olia.owl#ElaborationAssign"/>
  </rdf:Description>
  <rdf:Description rdf:about="http://purl.org/olia/discourse/olia_discourse.owl#ElaborationAssign">
    <owl:deprecated rdf:datatype="http://www.w3.org/2001/XMLSchema#boolean">true</owl:deprecated>
  </rdf:Description>
  <rdf:Description rdf:about="http://purl.org/olia/discourse/olia_discourse.owl#ElaborationAssignAbbreviation">
    <terms:replacedBy rdf:resource="http://purl.org/olia/olia.owl#ElaborationAssignAbbreviation"/>
  </rdf:Description>
  <rdf:Description rdf:about="http://purl.org/olia/discourse/olia_discourse.owl#ElaborationAssignAbbreviation">
    <owl:deprecated rdf:datatype="http://www.w3.org/2001/XMLSchema#boolean">true</owl:deprecated>
  </rdf:Description>
  <rdf:Description rdf:about="http://purl.org/olia/discourse/olia_discourse.owl#ElaborationClassInstance">
    <terms:replacedBy rdf:resource="http://purl.org/olia/olia.owl#ElaborationClassInstance"/>
  </rdf:Description>
  <rdf:Description rdf:about="http://purl.org/olia/discourse/olia_discourse.owl#ElaborationClassInstance">
    <owl:deprecated rdf:datatype="http://www.w3.org/2001/XMLSchema#boolean">true</owl:deprecated>
  </rdf:Description>
  <rdf:Description rdf:about="http://purl.org/olia/discourse/olia_discourse.owl#ElaborationClassSubclass">
    <terms:replacedBy rdf:resource="http://purl.org/olia/olia.owl#ElaborationClassSubclass"/>
  </rdf:Description>
  <rdf:Description rdf:about="http://purl.org/olia/discourse/olia_discourse.owl#ElaborationClassSubclass">
    <owl:deprecated rdf:datatype="http://www.w3.org/2001/XMLSchema#boolean">true</owl:deprecated>
  </rdf:Description>
  <rdf:Description rdf:about="http://purl.org/olia/discourse/olia_discourse.owl#ElaborationContinuation">
    <terms:replacedBy rdf:resource="http://purl.org/olia/olia.owl#ElaborationContinuation"/>
  </rdf:Description>
  <rdf:Description rdf:about="http://purl.org/olia/discourse/olia_discourse.owl#ElaborationContinuation">
    <owl:deprecated rdf:datatype="http://www.w3.org/2001/XMLSchema#boolean">true</owl:deprecated>
  </rdf:Description>
  <rdf:Description rdf:about="http://purl.org/olia/discourse/olia_discourse.owl#ElaborationDefinition">
    <terms:replacedBy rdf:resource="http://purl.org/olia/olia.owl#ElaborationDefinition"/>
  </rdf:Description>
  <rdf:Description rdf:about="http://purl.org/olia/discourse/olia_discourse.owl#ElaborationDefinition">
    <owl:deprecated rdf:datatype="http://www.w3.org/2001/XMLSchema#boolean">true</owl:deprecated>
  </rdf:Description>
  <rdf:Description rdf:about="http://purl.org/olia/discourse/olia_discourse.owl#ElaborationDerivation">
    <terms:replacedBy rdf:resource="http://purl.org/olia/olia.owl#ElaborationDerivation"/>
  </rdf:Description>
  <rdf:Description rdf:about="http://purl.org/olia/discourse/olia_discourse.owl#ElaborationDerivation">
    <owl:deprecated rdf:datatype="http://www.w3.org/2001/XMLSchema#boolean">true</owl:deprecated>
  </rdf:Description>
  <rdf:Description rdf:about="http://purl.org/olia/discourse/olia_discourse.owl#ElaborationDrift">
    <terms:replacedBy rdf:resource="http://purl.org/olia/olia.owl#ElaborationDrift"/>
  </rdf:Description>
  <rdf:Description rdf:about="http://purl.org/olia/discourse/olia_discourse.owl#ElaborationDrift">
    <owl:deprecated rdf:datatype="http://www.w3.org/2001/XMLSchema#boolean">true</owl:deprecated>
  </rdf:Description>
  <rdf:Description rdf:about="http://purl.org/olia/discourse/olia_discourse.owl#ElaborationExample">
    <terms:replacedBy rdf:resource="http://purl.org/olia/olia.owl#ElaborationExample"/>
  </rdf:Description>
  <rdf:Description rdf:about="http://purl.org/olia/discourse/olia_discourse.owl#ElaborationExample">
    <owl:deprecated rdf:datatype="http://www.w3.org/2001/XMLSchema#boolean">true</owl:deprecated>
  </rdf:Description>
  <rdf:Description rdf:about="http://purl.org/olia/discourse/olia_discourse.owl#ElaborationGenericSpecific_RST">
    <terms:replacedBy rdf:resource="http://purl.org/olia/olia.owl#ElaborationGenericSpecific_RST"/>
  </rdf:Description>
  <rdf:Description rdf:about="http://purl.org/olia/discourse/olia_discourse.owl#ElaborationGenericSpecific_RST">
    <owl:deprecated rdf:datatype="http://www.w3.org/2001/XMLSchema#boolean">true</owl:deprecated>
  </rdf:Description>
  <rdf:Description rdf:about="http://purl.org/olia/discourse/olia_discourse.owl#ElaborationIdentity">
    <terms:replacedBy rdf:resource="http://purl.org/olia/olia.owl#ElaborationIdentity"/>
  </rdf:Description>
  <rdf:Description rdf:about="http://purl.org/olia/discourse/olia_discourse.owl#ElaborationIdentity">
    <owl:deprecated rdf:datatype="http://www.w3.org/2001/XMLSchema#boolean">true</owl:deprecated>
  </rdf:Description>
  <rdf:Description rdf:about="http://purl.org/olia/discourse/olia_discourse.owl#ElaborationIntegration">
    <terms:replacedBy rdf:resource="http://purl.org/olia/olia.owl#ElaborationIntegration"/>
  </rdf:Description>
  <rdf:Description rdf:about="http://purl.org/olia/discourse/olia_discourse.owl#ElaborationIntegration">
    <owl:deprecated rdf:datatype="http://www.w3.org/2001/XMLSchema#boolean">true</owl:deprecated>
  </rdf:Description>
  <rdf:Description rdf:about="http://purl.org/olia/discourse/olia_discourse.owl#ElaborationObjectAttribute_RST">
    <terms:replacedBy rdf:resource="http://purl.org/olia/olia.owl#ElaborationObjectAttribute_RST"/>
  </rdf:Description>
  <rdf:Description rdf:about="http://purl.org/olia/discourse/olia_discourse.owl#ElaborationObjectAttribute_RST">
    <owl:deprecated rdf:datatype="http://www.w3.org/2001/XMLSchema#boolean">true</owl:deprecated>
  </rdf:Description>
  <rdf:Description rdf:about="http://purl.org/olia/discourse/olia_discourse.owl#ElaborationOfDetail_PDGB">
    <terms:replacedBy rdf:resource="http://purl.org/olia/olia.owl#ElaborationOfDetail_PDGB"/>
  </rdf:Description>
  <rdf:Description rdf:about="http://purl.org/olia/discourse/olia_discourse.owl#ElaborationOfDetail_PDGB">
    <owl:deprecated rdf:datatype="http://www.w3.org/2001/XMLSchema#boolean">true</owl:deprecated>
  </rdf:Description>
  <rdf:Description rdf:about="http://purl.org/olia/discourse/olia_discourse.owl#ElaborationOfLocation_PDGB">
    <terms:replacedBy rdf:resource="http://purl.org/olia/olia.owl#ElaborationOfLocation_PDGB"/>
  </rdf:Description>
  <rdf:Description rdf:about="http://purl.org/olia/discourse/olia_discourse.owl#ElaborationOfLocation_PDGB">
    <owl:deprecated rdf:datatype="http://www.w3.org/2001/XMLSchema#boolean">true</owl:deprecated>
  </rdf:Description>
  <rdf:Description rdf:about="http://purl.org/olia/discourse/olia_discourse.owl#ElaborationOfNumber_PDGB">
    <terms:replacedBy rdf:resource="http://purl.org/olia/olia.owl#ElaborationOfNumber_PDGB"/>
  </rdf:Description>
  <rdf:Description rdf:about="http://purl.org/olia/discourse/olia_discourse.owl#ElaborationOfNumber_PDGB">
    <owl:deprecated rdf:datatype="http://www.w3.org/2001/XMLSchema#boolean">true</owl:deprecated>
  </rdf:Description>
  <rdf:Description rdf:about="http://purl.org/olia/discourse/olia_discourse.owl#ElaborationOfOrganization_PDGB">
    <terms:replacedBy rdf:resource="http://purl.org/olia/olia.owl#ElaborationOfOrganization_PDGB"/>
  </rdf:Description>
  <rdf:Description rdf:about="http://purl.org/olia/discourse/olia_discourse.owl#ElaborationOfOrganization_PDGB">
    <owl:deprecated rdf:datatype="http://www.w3.org/2001/XMLSchema#boolean">true</owl:deprecated>
  </rdf:Description>
  <rdf:Description rdf:about="http://purl.org/olia/discourse/olia_discourse.owl#ElaborationOfPerson_PDGB">
    <terms:replacedBy rdf:resource="http://purl.org/olia/olia.owl#ElaborationOfPerson_PDGB"/>
  </rdf:Description>
  <rdf:Description rdf:about="http://purl.org/olia/discourse/olia_discourse.owl#ElaborationOfPerson_PDGB">
    <owl:deprecated rdf:datatype="http://www.w3.org/2001/XMLSchema#boolean">true</owl:deprecated>
  </rdf:Description>
  <rdf:Description rdf:about="http://purl.org/olia/discourse/olia_discourse.owl#ElaborationOfTime_PDGB">
    <terms:replacedBy rdf:resource="http://purl.org/olia/olia.owl#ElaborationOfTime_PDGB"/>
  </rdf:Description>
  <rdf:Description rdf:about="http://purl.org/olia/discourse/olia_discourse.owl#ElaborationOfTime_PDGB">
    <owl:deprecated rdf:datatype="http://www.w3.org/2001/XMLSchema#boolean">true</owl:deprecated>
  </rdf:Description>
  <rdf:Description rdf:about="http://purl.org/olia/discourse/olia_discourse.owl#ElaborationPartWhole_RST">
    <terms:replacedBy rdf:resource="http://purl.org/olia/olia.owl#ElaborationPartWhole_RST"/>
  </rdf:Description>
  <rdf:Description rdf:about="http://purl.org/olia/discourse/olia_discourse.owl#ElaborationPartWhole_RST">
    <owl:deprecated rdf:datatype="http://www.w3.org/2001/XMLSchema#boolean">true</owl:deprecated>
  </rdf:Description>
  <rdf:Description rdf:about="http://purl.org/olia/discourse/olia_discourse.owl#ElaborationProcessStep">
    <terms:replacedBy rdf:resource="http://purl.org/olia/olia.owl#ElaborationProcessStep"/>
  </rdf:Description>
  <rdf:Description rdf:about="http://purl.org/olia/discourse/olia_discourse.owl#ElaborationProcessStep">
    <owl:deprecated rdf:datatype="http://www.w3.org/2001/XMLSchema#boolean">true</owl:deprecated>
  </rdf:Description>
  <rdf:Description rdf:about="http://purl.org/olia/discourse/olia_discourse.owl#ElaborationProcessStep_RST">
    <terms:replacedBy rdf:resource="http://purl.org/olia/olia.owl#ElaborationProcessStep_RST"/>
  </rdf:Description>
  <rdf:Description rdf:about="http://purl.org/olia/discourse/olia_discourse.owl#ElaborationProcessStep_RST">
    <owl:deprecated rdf:datatype="http://www.w3.org/2001/XMLSchema#boolean">true</owl:deprecated>
  </rdf:Description>
  <rdf:Description rdf:about="http://purl.org/olia/discourse/olia_discourse.owl#ElaborationRestatement">
    <terms:replacedBy rdf:resource="http://purl.org/olia/olia.owl#ElaborationRestatement"/>
  </rdf:Description>
  <rdf:Description rdf:about="http://purl.org/olia/discourse/olia_discourse.owl#ElaborationRestatement">
    <owl:deprecated rdf:datatype="http://www.w3.org/2001/XMLSchema#boolean">true</owl:deprecated>
  </rdf:Description>
  <rdf:Description rdf:about="http://purl.org/olia/discourse/olia_discourse.owl#ElaborationSetMember">
    <terms:replacedBy rdf:resource="http://purl.org/olia/olia.owl#ElaborationSetMember"/>
  </rdf:Description>
  <rdf:Description rdf:about="http://purl.org/olia/discourse/olia_discourse.owl#ElaborationSetMember">
    <owl:deprecated rdf:datatype="http://www.w3.org/2001/XMLSchema#boolean">true</owl:deprecated>
  </rdf:Description>
  <rdf:Description rdf:about="http://purl.org/olia/discourse/olia_discourse.owl#ElaborationSetMember_RST">
    <terms:replacedBy rdf:resource="http://purl.org/olia/olia.owl#ElaborationSetMember_RST"/>
  </rdf:Description>
  <rdf:Description rdf:about="http://purl.org/olia/discourse/olia_discourse.owl#ElaborationSetMember_RST">
    <owl:deprecated rdf:datatype="http://www.w3.org/2001/XMLSchema#boolean">true</owl:deprecated>
  </rdf:Description>
  <rdf:Description rdf:about="http://purl.org/olia/discourse/olia_discourse.owl#ElaborationSpecification">
    <terms:replacedBy rdf:resource="http://purl.org/olia/olia.owl#ElaborationSpecification"/>
  </rdf:Description>
  <rdf:Description rdf:about="http://purl.org/olia/discourse/olia_discourse.owl#ElaborationSpecification">
    <owl:deprecated rdf:datatype="http://www.w3.org/2001/XMLSchema#boolean">true</owl:deprecated>
  </rdf:Description>
  <rdf:Description rdf:about="http://purl.org/olia/discourse/olia_discourse.owl#ElaborationThemeRheme">
    <terms:replacedBy rdf:resource="http://purl.org/olia/olia.owl#ElaborationThemeRheme"/>
  </rdf:Description>
  <rdf:Description rdf:about="http://purl.org/olia/discourse/olia_discourse.owl#ElaborationThemeRheme">
    <owl:deprecated rdf:datatype="http://www.w3.org/2001/XMLSchema#boolean">true</owl:deprecated>
  </rdf:Description>
  <rdf:Description rdf:about="http://purl.org/olia/discourse/olia_discourse.owl#ElaborationThemeTheme">
    <terms:replacedBy rdf:resource="http://purl.org/olia/olia.owl#ElaborationThemeTheme"/>
  </rdf:Description>
  <rdf:Description rdf:about="http://purl.org/olia/discourse/olia_discourse.owl#ElaborationThemeTheme">
    <owl:deprecated rdf:datatype="http://www.w3.org/2001/XMLSchema#boolean">true</owl:deprecated>
  </rdf:Description>
  <rdf:Description rdf:about="http://purl.org/olia/discourse/olia_discourse.owl#ElaborationWholePart">
    <terms:replacedBy rdf:resource="http://purl.org/olia/olia.owl#ElaborationWholePart"/>
  </rdf:Description>
  <rdf:Description rdf:about="http://purl.org/olia/discourse/olia_discourse.owl#ElaborationWholePart">
    <owl:deprecated rdf:datatype="http://www.w3.org/2001/XMLSchema#boolean">true</owl:deprecated>
  </rdf:Description>
  <rdf:Description rdf:about="http://purl.org/olia/discourse/olia_discourse.owl#ElementaryDiscourseUnit">
    <terms:replacedBy rdf:resource="http://purl.org/olia/olia.owl#ElementaryDiscourseUnit"/>
  </rdf:Description>
  <rdf:Description rdf:about="http://purl.org/olia/discourse/olia_discourse.owl#ElementaryDiscourseUnit">
    <owl:deprecated rdf:datatype="http://www.w3.org/2001/XMLSchema#boolean">true</owl:deprecated>
  </rdf:Description>
  <rdf:Description rdf:about="http://purl.org/olia/discourse/olia_discourse.owl#ElementOf">
    <terms:replacedBy rdf:resource="http://purl.org/olia/olia.owl#ElementOf"/>
  </rdf:Description>
  <rdf:Description rdf:about="http://purl.org/olia/discourse/olia_discourse.owl#ElementOf">
    <owl:deprecated rdf:datatype="http://www.w3.org/2001/XMLSchema#boolean">true</owl:deprecated>
  </rdf:Description>
  <rdf:Description rdf:about="http://purl.org/olia/discourse/olia_discourse.owl#EmailAddress">
    <terms:replacedBy rdf:resource="http://purl.org/olia/olia.owl#EmailAddress"/>
  </rdf:Description>
  <rdf:Description rdf:about="http://purl.org/olia/discourse/olia_discourse.owl#EmailAddress">
    <owl:deprecated rdf:datatype="http://www.w3.org/2001/XMLSchema#boolean">true</owl:deprecated>
  </rdf:Description>
  <rdf:Description rdf:about="http://purl.org/olia/discourse/olia_discourse.owl#Enablement">
    <terms:replacedBy rdf:resource="http://purl.org/olia/olia.owl#Enablement"/>
  </rdf:Description>
  <rdf:Description rdf:about="http://purl.org/olia/discourse/olia_discourse.owl#Enablement">
    <owl:deprecated rdf:datatype="http://www.w3.org/2001/XMLSchema#boolean">true</owl:deprecated>
  </rdf:Description>
  <rdf:Description rdf:about="http://purl.org/olia/discourse/olia_discourse.owl#Enablement_RST">
    <terms:replacedBy rdf:resource="http://purl.org/olia/olia.owl#Enablement_RST"/>
  </rdf:Description>
  <rdf:Description rdf:about="http://purl.org/olia/discourse/olia_discourse.owl#Enablement_RST">
    <owl:deprecated rdf:datatype="http://www.w3.org/2001/XMLSchema#boolean">true</owl:deprecated>
  </rdf:Description>
  <rdf:Description rdf:about="http://purl.org/olia/discourse/olia_discourse.owl#EntityBasedRelation">
    <terms:replacedBy rdf:resource="http://purl.org/olia/olia.owl#EntityBasedRelation"/>
  </rdf:Description>
  <rdf:Description rdf:about="http://purl.org/olia/discourse/olia_discourse.owl#EntityBasedRelation">
    <owl:deprecated rdf:datatype="http://www.w3.org/2001/XMLSchema#boolean">true</owl:deprecated>
  </rdf:Description>
  <rdf:Description rdf:about="http://purl.org/olia/discourse/olia_discourse.owl#EntityType">
    <terms:replacedBy rdf:resource="http://purl.org/olia/olia.owl#EntityType"/>
  </rdf:Description>
  <rdf:Description rdf:about="http://purl.org/olia/discourse/olia_discourse.owl#EntityType">
    <owl:deprecated rdf:datatype="http://www.w3.org/2001/XMLSchema#boolean">true</owl:deprecated>
  </rdf:Description>
  <rdf:Description rdf:about="http://purl.org/olia/discourse/olia_discourse.owl#EpistemicCause_HDRB">
    <terms:replacedBy rdf:resource="http://purl.org/olia/olia.owl#EpistemicCause_HDRB"/>
  </rdf:Description>
  <rdf:Description rdf:about="http://purl.org/olia/discourse/olia_discourse.owl#EpistemicCause_HDRB">
    <owl:deprecated rdf:datatype="http://www.w3.org/2001/XMLSchema#boolean">true</owl:deprecated>
  </rdf:Description>
  <rdf:Description rdf:about="http://purl.org/olia/discourse/olia_discourse.owl#EpistemicConcession_HDRB">
    <terms:replacedBy rdf:resource="http://purl.org/olia/olia.owl#EpistemicConcession_HDRB"/>
  </rdf:Description>
  <rdf:Description rdf:about="http://purl.org/olia/discourse/olia_discourse.owl#EpistemicConcession_HDRB">
    <owl:deprecated rdf:datatype="http://www.w3.org/2001/XMLSchema#boolean">true</owl:deprecated>
  </rdf:Description>
  <rdf:Description rdf:about="http://purl.org/olia/discourse/olia_discourse.owl#EpistemicCondition">
    <terms:replacedBy rdf:resource="http://purl.org/olia/olia.owl#EpistemicCondition"/>
  </rdf:Description>
  <rdf:Description rdf:about="http://purl.org/olia/discourse/olia_discourse.owl#EpistemicCondition">
    <owl:deprecated rdf:datatype="http://www.w3.org/2001/XMLSchema#boolean">true</owl:deprecated>
  </rdf:Description>
  <rdf:Description rdf:about="http://purl.org/olia/discourse/olia_discourse.owl#EpistemicCondition_HDRB">
    <terms:replacedBy rdf:resource="http://purl.org/olia/olia.owl#EpistemicCondition_HDRB"/>
  </rdf:Description>
  <rdf:Description rdf:about="http://purl.org/olia/discourse/olia_discourse.owl#EpistemicCondition_HDRB">
    <owl:deprecated rdf:datatype="http://www.w3.org/2001/XMLSchema#boolean">true</owl:deprecated>
  </rdf:Description>
  <rdf:Description rdf:about="http://purl.org/olia/discourse/olia_discourse.owl#EpistemicCondition_LUNA">
    <terms:replacedBy rdf:resource="http://purl.org/olia/olia.owl#EpistemicCondition_LUNA"/>
  </rdf:Description>
  <rdf:Description rdf:about="http://purl.org/olia/discourse/olia_discourse.owl#EpistemicCondition_LUNA">
    <owl:deprecated rdf:datatype="http://www.w3.org/2001/XMLSchema#boolean">true</owl:deprecated>
  </rdf:Description>
  <rdf:Description rdf:about="http://purl.org/olia/discourse/olia_discourse.owl#EpistemicContrast_HDRB">
    <terms:replacedBy rdf:resource="http://purl.org/olia/olia.owl#EpistemicContrast_HDRB"/>
  </rdf:Description>
  <rdf:Description rdf:about="http://purl.org/olia/discourse/olia_discourse.owl#EpistemicContrast_HDRB">
    <owl:deprecated rdf:datatype="http://www.w3.org/2001/XMLSchema#boolean">true</owl:deprecated>
  </rdf:Description>
  <rdf:Description rdf:about="http://purl.org/olia/discourse/olia_discourse.owl#EquivalentRestatement">
    <terms:replacedBy rdf:resource="http://purl.org/olia/olia.owl#EquivalentRestatement"/>
  </rdf:Description>
  <rdf:Description rdf:about="http://purl.org/olia/discourse/olia_discourse.owl#EquivalentRestatement">
    <owl:deprecated rdf:datatype="http://www.w3.org/2001/XMLSchema#boolean">true</owl:deprecated>
  </rdf:Description>
  <rdf:Description rdf:about="http://purl.org/olia/discourse/olia_discourse.owl#EquivalentRestatement_PDTB">
    <terms:replacedBy rdf:resource="http://purl.org/olia/olia.owl#EquivalentRestatement_PDTB"/>
  </rdf:Description>
  <rdf:Description rdf:about="http://purl.org/olia/discourse/olia_discourse.owl#EquivalentRestatement_PDTB">
    <owl:deprecated rdf:datatype="http://www.w3.org/2001/XMLSchema#boolean">true</owl:deprecated>
  </rdf:Description>
  <rdf:Description rdf:about="http://purl.org/olia/discourse/olia_discourse.owl#Evaluation">
    <terms:replacedBy rdf:resource="http://purl.org/olia/olia.owl#Evaluation"/>
  </rdf:Description>
  <rdf:Description rdf:about="http://purl.org/olia/discourse/olia_discourse.owl#Evaluation">
    <owl:deprecated rdf:datatype="http://www.w3.org/2001/XMLSchema#boolean">true</owl:deprecated>
  </rdf:Description>
  <rdf:Description rdf:about="http://purl.org/olia/discourse/olia_discourse.owl#Evaluation_RST">
    <terms:replacedBy rdf:resource="http://purl.org/olia/olia.owl#Evaluation_RST"/>
  </rdf:Description>
  <rdf:Description rdf:about="http://purl.org/olia/discourse/olia_discourse.owl#Evaluation_RST">
    <owl:deprecated rdf:datatype="http://www.w3.org/2001/XMLSchema#boolean">true</owl:deprecated>
  </rdf:Description>
  <rdf:Description rdf:about="http://purl.org/olia/discourse/olia_discourse.owl#Event">
    <terms:replacedBy rdf:resource="http://purl.org/olia/olia.owl#Event"/>
  </rdf:Description>
  <rdf:Description rdf:about="http://purl.org/olia/discourse/olia_discourse.owl#Event">
    <owl:deprecated rdf:datatype="http://www.w3.org/2001/XMLSchema#boolean">true</owl:deprecated>
  </rdf:Description>
  <rdf:Description rdf:about="http://purl.org/olia/discourse/olia_discourse.owl#EventualFactuality">
    <terms:replacedBy rdf:resource="http://purl.org/olia/olia.owl#EventualFactuality"/>
  </rdf:Description>
  <rdf:Description rdf:about="http://purl.org/olia/discourse/olia_discourse.owl#EventualFactuality">
    <owl:deprecated rdf:datatype="http://www.w3.org/2001/XMLSchema#boolean">true</owl:deprecated>
  </rdf:Description>
  <rdf:Description rdf:about="http://purl.org/olia/discourse/olia_discourse.owl#Evidence">
    <terms:replacedBy rdf:resource="http://purl.org/olia/olia.owl#Evidence"/>
  </rdf:Description>
  <rdf:Description rdf:about="http://purl.org/olia/discourse/olia_discourse.owl#Evidence">
    <owl:deprecated rdf:datatype="http://www.w3.org/2001/XMLSchema#boolean">true</owl:deprecated>
  </rdf:Description>
  <rdf:Description rdf:about="http://purl.org/olia/discourse/olia_discourse.owl#Evidence_RST">
    <terms:replacedBy rdf:resource="http://purl.org/olia/olia.owl#Evidence_RST"/>
  </rdf:Description>
  <rdf:Description rdf:about="http://purl.org/olia/discourse/olia_discourse.owl#Evidence_RST">
    <owl:deprecated rdf:datatype="http://www.w3.org/2001/XMLSchema#boolean">true</owl:deprecated>
  </rdf:Description>
  <rdf:Description rdf:about="http://purl.org/olia/discourse/olia_discourse.owl#Example">
    <terms:replacedBy rdf:resource="http://purl.org/olia/olia.owl#Example"/>
  </rdf:Description>
  <rdf:Description rdf:about="http://purl.org/olia/discourse/olia_discourse.owl#Example">
    <owl:deprecated rdf:datatype="http://www.w3.org/2001/XMLSchema#boolean">true</owl:deprecated>
  </rdf:Description>
  <rdf:Description rdf:about="http://purl.org/olia/discourse/olia_discourse.owl#Exception">
    <terms:replacedBy rdf:resource="http://purl.org/olia/olia.owl#Exception"/>
  </rdf:Description>
  <rdf:Description rdf:about="http://purl.org/olia/discourse/olia_discourse.owl#Exception">
    <owl:deprecated rdf:datatype="http://www.w3.org/2001/XMLSchema#boolean">true</owl:deprecated>
  </rdf:Description>
  <rdf:Description rdf:about="http://purl.org/olia/discourse/olia_discourse.owl#Exception_PDTB">
    <terms:replacedBy rdf:resource="http://purl.org/olia/olia.owl#Exception_PDTB"/>
  </rdf:Description>
  <rdf:Description rdf:about="http://purl.org/olia/discourse/olia_discourse.owl#Exception_PDTB">
    <owl:deprecated rdf:datatype="http://www.w3.org/2001/XMLSchema#boolean">true</owl:deprecated>
  </rdf:Description>
  <rdf:Description rdf:about="http://purl.org/olia/discourse/olia_discourse.owl#Expansion">
    <terms:replacedBy rdf:resource="http://purl.org/olia/olia.owl#Expansion"/>
  </rdf:Description>
  <rdf:Description rdf:about="http://purl.org/olia/discourse/olia_discourse.owl#Expansion">
    <owl:deprecated rdf:datatype="http://www.w3.org/2001/XMLSchema#boolean">true</owl:deprecated>
  </rdf:Description>
  <rdf:Description rdf:about="http://purl.org/olia/discourse/olia_discourse.owl#Expectation">
    <terms:replacedBy rdf:resource="http://purl.org/olia/olia.owl#Expectation"/>
  </rdf:Description>
  <rdf:Description rdf:about="http://purl.org/olia/discourse/olia_discourse.owl#Expectation">
    <owl:deprecated rdf:datatype="http://www.w3.org/2001/XMLSchema#boolean">true</owl:deprecated>
  </rdf:Description>
  <rdf:Description rdf:about="http://purl.org/olia/discourse/olia_discourse.owl#Explanation">
    <terms:replacedBy rdf:resource="http://purl.org/olia/olia.owl#Explanation"/>
  </rdf:Description>
  <rdf:Description rdf:about="http://purl.org/olia/discourse/olia_discourse.owl#Explanation">
    <owl:deprecated rdf:datatype="http://www.w3.org/2001/XMLSchema#boolean">true</owl:deprecated>
  </rdf:Description>
  <rdf:Description rdf:about="http://purl.org/olia/discourse/olia_discourse.owl#ExplicitConnective">
    <terms:replacedBy rdf:resource="http://purl.org/olia/olia.owl#ExplicitConnective"/>
  </rdf:Description>
  <rdf:Description rdf:about="http://purl.org/olia/discourse/olia_discourse.owl#ExplicitConnective">
    <owl:deprecated rdf:datatype="http://www.w3.org/2001/XMLSchema#boolean">true</owl:deprecated>
  </rdf:Description>
  <rdf:Description rdf:about="http://purl.org/olia/discourse/olia_discourse.owl#ExpressionFocus">
    <terms:replacedBy rdf:resource="http://purl.org/olia/olia.owl#ExpressionFocus"/>
  </rdf:Description>
  <rdf:Description rdf:about="http://purl.org/olia/discourse/olia_discourse.owl#ExpressionFocus">
    <owl:deprecated rdf:datatype="http://www.w3.org/2001/XMLSchema#boolean">true</owl:deprecated>
  </rdf:Description>
  <rdf:Description rdf:about="http://purl.org/olia/discourse/olia_discourse.owl#Extra">
    <terms:replacedBy rdf:resource="http://purl.org/olia/olia.owl#Extra"/>
  </rdf:Description>
  <rdf:Description rdf:about="http://purl.org/olia/discourse/olia_discourse.owl#Extra">
    <owl:deprecated rdf:datatype="http://www.w3.org/2001/XMLSchema#boolean">true</owl:deprecated>
  </rdf:Description>
  <rdf:Description rdf:about="http://purl.org/olia/discourse/olia_discourse.owl#FacetiousRegister">
    <terms:replacedBy rdf:resource="http://purl.org/olia/olia.owl#FacetiousRegister"/>
  </rdf:Description>
  <rdf:Description rdf:about="http://purl.org/olia/discourse/olia_discourse.owl#FacetiousRegister">
    <owl:deprecated rdf:datatype="http://www.w3.org/2001/XMLSchema#boolean">true</owl:deprecated>
  </rdf:Description>
  <rdf:Description rdf:about="http://purl.org/olia/discourse/olia_discourse.owl#FactiveFactuality">
    <terms:replacedBy rdf:resource="http://purl.org/olia/olia.owl#FactiveFactuality"/>
  </rdf:Description>
  <rdf:Description rdf:about="http://purl.org/olia/discourse/olia_discourse.owl#FactiveFactuality">
    <owl:deprecated rdf:datatype="http://www.w3.org/2001/XMLSchema#boolean">true</owl:deprecated>
  </rdf:Description>
  <rdf:Description rdf:about="http://purl.org/olia/discourse/olia_discourse.owl#FactualCondition">
    <terms:replacedBy rdf:resource="http://purl.org/olia/olia.owl#FactualCondition"/>
  </rdf:Description>
  <rdf:Description rdf:about="http://purl.org/olia/discourse/olia_discourse.owl#FactualCondition">
    <owl:deprecated rdf:datatype="http://www.w3.org/2001/XMLSchema#boolean">true</owl:deprecated>
  </rdf:Description>
  <rdf:Description rdf:about="http://purl.org/olia/discourse/olia_discourse.owl#FactualCondition_HDRB">
    <terms:replacedBy rdf:resource="http://purl.org/olia/olia.owl#FactualCondition_HDRB"/>
  </rdf:Description>
  <rdf:Description rdf:about="http://purl.org/olia/discourse/olia_discourse.owl#FactualCondition_HDRB">
    <owl:deprecated rdf:datatype="http://www.w3.org/2001/XMLSchema#boolean">true</owl:deprecated>
  </rdf:Description>
  <rdf:Description rdf:about="http://purl.org/olia/discourse/olia_discourse.owl#Factuality">
    <terms:replacedBy rdf:resource="http://purl.org/olia/olia.owl#Factuality"/>
  </rdf:Description>
  <rdf:Description rdf:about="http://purl.org/olia/discourse/olia_discourse.owl#Factuality">
    <owl:deprecated rdf:datatype="http://www.w3.org/2001/XMLSchema#boolean">true</owl:deprecated>
  </rdf:Description>
  <rdf:Description rdf:about="http://purl.org/olia/discourse/olia_discourse.owl#FactualPastCondition_PDTB">
    <terms:replacedBy rdf:resource="http://purl.org/olia/olia.owl#FactualPastCondition_PDTB"/>
  </rdf:Description>
  <rdf:Description rdf:about="http://purl.org/olia/discourse/olia_discourse.owl#FactualPastCondition_PDTB">
    <owl:deprecated rdf:datatype="http://www.w3.org/2001/XMLSchema#boolean">true</owl:deprecated>
  </rdf:Description>
  <rdf:Description rdf:about="http://purl.org/olia/discourse/olia_discourse.owl#FactualPresentCondition_PDTB">
    <terms:replacedBy rdf:resource="http://purl.org/olia/olia.owl#FactualPresentCondition_PDTB"/>
  </rdf:Description>
  <rdf:Description rdf:about="http://purl.org/olia/discourse/olia_discourse.owl#FactualPresentCondition_PDTB">
    <owl:deprecated rdf:datatype="http://www.w3.org/2001/XMLSchema#boolean">true</owl:deprecated>
  </rdf:Description>
  <rdf:Description rdf:about="http://purl.org/olia/discourse/olia_discourse.owl#FavouredAlternative">
    <terms:replacedBy rdf:resource="http://purl.org/olia/olia.owl#FavouredAlternative"/>
  </rdf:Description>
  <rdf:Description rdf:about="http://purl.org/olia/discourse/olia_discourse.owl#FavouredAlternative">
    <owl:deprecated rdf:datatype="http://www.w3.org/2001/XMLSchema#boolean">true</owl:deprecated>
  </rdf:Description>
  <rdf:Description rdf:about="http://purl.org/olia/discourse/olia_discourse.owl#FeedbackAct">
    <terms:replacedBy rdf:resource="http://purl.org/olia/olia.owl#FeedbackAct"/>
  </rdf:Description>
  <rdf:Description rdf:about="http://purl.org/olia/discourse/olia_discourse.owl#FeedbackAct">
    <owl:deprecated rdf:datatype="http://www.w3.org/2001/XMLSchema#boolean">true</owl:deprecated>
  </rdf:Description>
  <rdf:Description rdf:about="http://purl.org/olia/discourse/olia_discourse.owl#FeedbackScope">
    <terms:replacedBy rdf:resource="http://purl.org/olia/olia.owl#FeedbackScope"/>
  </rdf:Description>
  <rdf:Description rdf:about="http://purl.org/olia/discourse/olia_discourse.owl#FeedbackScope">
    <owl:deprecated rdf:datatype="http://www.w3.org/2001/XMLSchema#boolean">true</owl:deprecated>
  </rdf:Description>
  <rdf:Description rdf:about="http://purl.org/olia/discourse/olia_discourse.owl#FictionalCharacter">
    <terms:replacedBy rdf:resource="http://purl.org/olia/olia.owl#FictionalCharacter"/>
  </rdf:Description>
  <rdf:Description rdf:about="http://purl.org/olia/discourse/olia_discourse.owl#FictionalCharacter">
    <owl:deprecated rdf:datatype="http://www.w3.org/2001/XMLSchema#boolean">true</owl:deprecated>
  </rdf:Description>
  <rdf:Description rdf:about="http://purl.org/olia/discourse/olia_discourse.owl#Focus">
    <terms:replacedBy rdf:resource="http://purl.org/olia/olia.owl#Focus"/>
  </rdf:Description>
  <rdf:Description rdf:about="http://purl.org/olia/discourse/olia_discourse.owl#Focus">
    <owl:deprecated rdf:datatype="http://www.w3.org/2001/XMLSchema#boolean">true</owl:deprecated>
  </rdf:Description>
  <rdf:Description rdf:about="http://purl.org/olia/discourse/olia_discourse.owl#FocusDomain">
    <terms:replacedBy rdf:resource="http://purl.org/olia/olia.owl#FocusDomain"/>
  </rdf:Description>
  <rdf:Description rdf:about="http://purl.org/olia/discourse/olia_discourse.owl#FocusDomain">
    <owl:deprecated rdf:datatype="http://www.w3.org/2001/XMLSchema#boolean">true</owl:deprecated>
  </rdf:Description>
  <rdf:Description rdf:about="http://purl.org/olia/discourse/olia_discourse.owl#Footnote">
    <terms:replacedBy rdf:resource="http://purl.org/olia/olia.owl#Footnote"/>
  </rdf:Description>
  <rdf:Description rdf:about="http://purl.org/olia/discourse/olia_discourse.owl#Footnote">
    <owl:deprecated rdf:datatype="http://www.w3.org/2001/XMLSchema#boolean">true</owl:deprecated>
  </rdf:Description>
  <rdf:Description rdf:about="http://purl.org/olia/discourse/olia_discourse.owl#FormalRegister">
    <terms:replacedBy rdf:resource="http://purl.org/olia/olia.owl#FormalRegister"/>
  </rdf:Description>
  <rdf:Description rdf:about="http://purl.org/olia/discourse/olia_discourse.owl#FormalRegister">
    <owl:deprecated rdf:datatype="http://www.w3.org/2001/XMLSchema#boolean">true</owl:deprecated>
  </rdf:Description>
  <rdf:Description rdf:about="http://purl.org/olia/discourse/olia_discourse.owl#FrameSettingTopic">
    <terms:replacedBy rdf:resource="http://purl.org/olia/olia.owl#FrameSettingTopic"/>
  </rdf:Description>
  <rdf:Description rdf:about="http://purl.org/olia/discourse/olia_discourse.owl#FrameSettingTopic">
    <owl:deprecated rdf:datatype="http://www.w3.org/2001/XMLSchema#boolean">true</owl:deprecated>
  </rdf:Description>
  <rdf:Description rdf:about="http://purl.org/olia/discourse/olia_discourse.owl#Function">
    <terms:replacedBy rdf:resource="http://purl.org/olia/olia.owl#Function"/>
  </rdf:Description>
  <rdf:Description rdf:about="http://purl.org/olia/discourse/olia_discourse.owl#Function">
    <owl:deprecated rdf:datatype="http://www.w3.org/2001/XMLSchema#boolean">true</owl:deprecated>
  </rdf:Description>
  <rdf:Description rdf:about="http://purl.org/olia/discourse/olia_discourse.owl#GeneralCondition_PDTB">
    <terms:replacedBy rdf:resource="http://purl.org/olia/olia.owl#GeneralCondition_PDTB"/>
  </rdf:Description>
  <rdf:Description rdf:about="http://purl.org/olia/discourse/olia_discourse.owl#GeneralCondition_PDTB">
    <owl:deprecated rdf:datatype="http://www.w3.org/2001/XMLSchema#boolean">true</owl:deprecated>
  </rdf:Description>
  <rdf:Description rdf:about="http://purl.org/olia/discourse/olia_discourse.owl#Generalization">
    <terms:replacedBy rdf:resource="http://purl.org/olia/olia.owl#Generalization"/>
  </rdf:Description>
  <rdf:Description rdf:about="http://purl.org/olia/discourse/olia_discourse.owl#Generalization">
    <owl:deprecated rdf:datatype="http://www.w3.org/2001/XMLSchema#boolean">true</owl:deprecated>
  </rdf:Description>
  <rdf:Description rdf:about="http://purl.org/olia/discourse/olia_discourse.owl#GenerallyAccessible">
    <terms:replacedBy rdf:resource="http://purl.org/olia/olia.owl#GenerallyAccessible"/>
  </rdf:Description>
  <rdf:Description rdf:about="http://purl.org/olia/discourse/olia_discourse.owl#GenerallyAccessible">
    <owl:deprecated rdf:datatype="http://www.w3.org/2001/XMLSchema#boolean">true</owl:deprecated>
  </rdf:Description>
  <rdf:Description rdf:about="http://purl.org/olia/discourse/olia_discourse.owl#GeographicalFeature">
    <terms:replacedBy rdf:resource="http://purl.org/olia/olia.owl#GeographicalFeature"/>
  </rdf:Description>
  <rdf:Description rdf:about="http://purl.org/olia/discourse/olia_discourse.owl#GeographicalFeature">
    <owl:deprecated rdf:datatype="http://www.w3.org/2001/XMLSchema#boolean">true</owl:deprecated>
  </rdf:Description>
  <rdf:Description rdf:about="http://purl.org/olia/discourse/olia_discourse.owl#GeographicalVariant">
    <terms:replacedBy rdf:resource="http://purl.org/olia/olia.owl#GeographicalVariant"/>
  </rdf:Description>
  <rdf:Description rdf:about="http://purl.org/olia/discourse/olia_discourse.owl#GeographicalVariant">
    <owl:deprecated rdf:datatype="http://www.w3.org/2001/XMLSchema#boolean">true</owl:deprecated>
  </rdf:Description>
  <rdf:Description rdf:about="http://purl.org/olia/discourse/olia_discourse.owl#Given">
    <terms:replacedBy rdf:resource="http://purl.org/olia/olia.owl#Given"/>
  </rdf:Description>
  <rdf:Description rdf:about="http://purl.org/olia/discourse/olia_discourse.owl#Given">
    <owl:deprecated rdf:datatype="http://www.w3.org/2001/XMLSchema#boolean">true</owl:deprecated>
  </rdf:Description>
  <rdf:Description rdf:about="http://purl.org/olia/discourse/olia_discourse.owl#Goal">
    <terms:replacedBy rdf:resource="http://purl.org/olia/olia.owl#Goal"/>
  </rdf:Description>
  <rdf:Description rdf:about="http://purl.org/olia/discourse/olia_discourse.owl#Goal">
    <owl:deprecated rdf:datatype="http://www.w3.org/2001/XMLSchema#boolean">true</owl:deprecated>
  </rdf:Description>
  <rdf:Description rdf:about="http://purl.org/olia/discourse/olia_discourse.owl#Goal_HDRB">
    <terms:replacedBy rdf:resource="http://purl.org/olia/olia.owl#Goal_HDRB"/>
  </rdf:Description>
  <rdf:Description rdf:about="http://purl.org/olia/discourse/olia_discourse.owl#Goal_HDRB">
    <owl:deprecated rdf:datatype="http://www.w3.org/2001/XMLSchema#boolean">true</owl:deprecated>
  </rdf:Description>
  <rdf:Description rdf:about="http://purl.org/olia/discourse/olia_discourse.owl#HabitualCooccurrence">
    <terms:replacedBy rdf:resource="http://purl.org/olia/olia.owl#HabitualCooccurrence"/>
  </rdf:Description>
  <rdf:Description rdf:about="http://purl.org/olia/discourse/olia_discourse.owl#HabitualCooccurrence">
    <owl:deprecated rdf:datatype="http://www.w3.org/2001/XMLSchema#boolean">true</owl:deprecated>
  </rdf:Description>
  <rdf:Description rdf:about="http://purl.org/olia/discourse/olia_discourse.owl#hasAttributionSource">
    <terms:replacedBy rdf:resource="http://purl.org/olia/olia.owl#hasAttributionSource"/>
  </rdf:Description>
  <rdf:Description rdf:about="http://purl.org/olia/discourse/olia_discourse.owl#hasAttributionSource">
    <owl:deprecated rdf:datatype="http://www.w3.org/2001/XMLSchema#boolean">true</owl:deprecated>
  </rdf:Description>
  <rdf:Description rdf:about="http://purl.org/olia/discourse/olia_discourse.owl#hasBridgingType">
    <terms:replacedBy rdf:resource="http://purl.org/olia/olia.owl#hasBridgingType"/>
  </rdf:Description>
  <rdf:Description rdf:about="http://purl.org/olia/discourse/olia_discourse.owl#hasBridgingType">
    <owl:deprecated rdf:datatype="http://www.w3.org/2001/XMLSchema#boolean">true</owl:deprecated>
  </rdf:Description>
  <rdf:Description rdf:about="http://purl.org/olia/discourse/olia_discourse.owl#hasDefiniteness">
    <terms:replacedBy rdf:resource="http://purl.org/olia/olia.owl#hasDefiniteness"/>
  </rdf:Description>
  <rdf:Description rdf:about="http://purl.org/olia/discourse/olia_discourse.owl#hasDefiniteness">
    <owl:deprecated rdf:datatype="http://www.w3.org/2001/XMLSchema#boolean">true</owl:deprecated>
  </rdf:Description>
  <rdf:Description rdf:about="http://purl.org/olia/discourse/olia_discourse.owl#hasDiscourseFunction">
    <terms:replacedBy rdf:resource="http://purl.org/olia/olia.owl#hasDiscourseFunction"/>
  </rdf:Description>
  <rdf:Description rdf:about="http://purl.org/olia/discourse/olia_discourse.owl#hasDiscourseFunction">
    <owl:deprecated rdf:datatype="http://www.w3.org/2001/XMLSchema#boolean">true</owl:deprecated>
  </rdf:Description>
  <rdf:Description rdf:about="http://purl.org/olia/discourse/olia_discourse.owl#hasDiscourseStructuralPattern">
    <terms:replacedBy rdf:resource="http://purl.org/olia/olia.owl#hasDiscourseStructuralPattern"/>
  </rdf:Description>
  <rdf:Description rdf:about="http://purl.org/olia/discourse/olia_discourse.owl#hasDiscourseStructuralPattern">
    <owl:deprecated rdf:datatype="http://www.w3.org/2001/XMLSchema#boolean">true</owl:deprecated>
  </rdf:Description>
  <rdf:Description rdf:about="http://purl.org/olia/discourse/olia_discourse.owl#hasEntityType">
    <terms:replacedBy rdf:resource="http://purl.org/olia/olia.owl#hasEntityType"/>
  </rdf:Description>
  <rdf:Description rdf:about="http://purl.org/olia/discourse/olia_discourse.owl#hasEntityType">
    <owl:deprecated rdf:datatype="http://www.w3.org/2001/XMLSchema#boolean">true</owl:deprecated>
  </rdf:Description>
  <rdf:Description rdf:about="http://purl.org/olia/discourse/olia_discourse.owl#hasFactuality">
    <terms:replacedBy rdf:resource="http://purl.org/olia/olia.owl#hasFactuality"/>
  </rdf:Description>
  <rdf:Description rdf:about="http://purl.org/olia/discourse/olia_discourse.owl#hasFactuality">
    <owl:deprecated rdf:datatype="http://www.w3.org/2001/XMLSchema#boolean">true</owl:deprecated>
  </rdf:Description>
  <rdf:Description rdf:about="http://purl.org/olia/discourse/olia_discourse.owl#hasInformationStatus">
    <terms:replacedBy rdf:resource="http://purl.org/olia/olia.owl#hasInformationStatus"/>
  </rdf:Description>
  <rdf:Description rdf:about="http://purl.org/olia/discourse/olia_discourse.owl#hasInformationStatus">
    <owl:deprecated rdf:datatype="http://www.w3.org/2001/XMLSchema#boolean">true</owl:deprecated>
  </rdf:Description>
  <rdf:Description rdf:about="http://purl.org/olia/discourse/olia_discourse.owl#hasPolarity">
    <terms:replacedBy rdf:resource="http://purl.org/olia/olia.owl#hasPolarity"/>
  </rdf:Description>
  <rdf:Description rdf:about="http://purl.org/olia/discourse/olia_discourse.owl#hasPolarity">
    <owl:deprecated rdf:datatype="http://www.w3.org/2001/XMLSchema#boolean">true</owl:deprecated>
  </rdf:Description>
  <rdf:Description rdf:about="http://purl.org/olia/discourse/olia_discourse.owl#hasPragmaticFeature">
    <terms:replacedBy rdf:resource="http://purl.org/olia/olia.owl#hasPragmaticFeature"/>
  </rdf:Description>
  <rdf:Description rdf:about="http://purl.org/olia/discourse/olia_discourse.owl#hasPragmaticFeature">
    <owl:deprecated rdf:datatype="http://www.w3.org/2001/XMLSchema#boolean">true</owl:deprecated>
  </rdf:Description>
  <rdf:Description rdf:about="http://purl.org/olia/discourse/olia_discourse.owl#hasReferentiality">
    <terms:replacedBy rdf:resource="http://purl.org/olia/olia.owl#hasReferentiality"/>
  </rdf:Description>
  <rdf:Description rdf:about="http://purl.org/olia/discourse/olia_discourse.owl#hasReferentiality">
    <owl:deprecated rdf:datatype="http://www.w3.org/2001/XMLSchema#boolean">true</owl:deprecated>
  </rdf:Description>
  <rdf:Description rdf:about="http://purl.org/olia/discourse/olia_discourse.owl#hasReferentType">
    <terms:replacedBy rdf:resource="http://purl.org/olia/olia.owl#hasReferentType"/>
  </rdf:Description>
  <rdf:Description rdf:about="http://purl.org/olia/discourse/olia_discourse.owl#hasReferentType">
    <owl:deprecated rdf:datatype="http://www.w3.org/2001/XMLSchema#boolean">true</owl:deprecated>
  </rdf:Description>
  <rdf:Description rdf:about="http://purl.org/olia/discourse/olia_discourse.owl#hasRegister">
    <terms:replacedBy rdf:resource="http://purl.org/olia/olia.owl#hasRegister"/>
  </rdf:Description>
  <rdf:Description rdf:about="http://purl.org/olia/discourse/olia_discourse.owl#hasRegister">
    <owl:deprecated rdf:datatype="http://www.w3.org/2001/XMLSchema#boolean">true</owl:deprecated>
  </rdf:Description>
  <rdf:Description rdf:about="http://purl.org/olia/discourse/olia_discourse.owl#hasSemanticFeature">
    <terms:replacedBy rdf:resource="http://purl.org/olia/olia.owl#hasSemanticFeature"/>
  </rdf:Description>
  <rdf:Description rdf:about="http://purl.org/olia/discourse/olia_discourse.owl#hasSemanticFeature">
    <owl:deprecated rdf:datatype="http://www.w3.org/2001/XMLSchema#boolean">true</owl:deprecated>
  </rdf:Description>
  <rdf:Description rdf:about="http://purl.org/olia/discourse/olia_discourse.owl#hasSource">
    <terms:replacedBy rdf:resource="http://purl.org/olia/olia.owl#hasSource"/>
  </rdf:Description>
  <rdf:Description rdf:about="http://purl.org/olia/discourse/olia_discourse.owl#hasSource">
    <owl:deprecated rdf:datatype="http://www.w3.org/2001/XMLSchema#boolean">true</owl:deprecated>
  </rdf:Description>
  <rdf:Description rdf:about="http://purl.org/olia/discourse/olia_discourse.owl#hasStructuralFocusType">
    <terms:replacedBy rdf:resource="http://purl.org/olia/olia.owl#hasStructuralFocusType"/>
  </rdf:Description>
  <rdf:Description rdf:about="http://purl.org/olia/discourse/olia_discourse.owl#hasStructuralFocusType">
    <owl:deprecated rdf:datatype="http://www.w3.org/2001/XMLSchema#boolean">true</owl:deprecated>
  </rdf:Description>
  <rdf:Description rdf:about="http://purl.org/olia/discourse/olia_discourse.owl#hasTarget">
    <terms:replacedBy rdf:resource="http://purl.org/olia/olia.owl#hasTarget"/>
  </rdf:Description>
  <rdf:Description rdf:about="http://purl.org/olia/discourse/olia_discourse.owl#hasTarget">
    <owl:deprecated rdf:datatype="http://www.w3.org/2001/XMLSchema#boolean">true</owl:deprecated>
  </rdf:Description>
  <rdf:Description rdf:about="http://purl.org/olia/discourse/olia_discourse.owl#hasUsage">
    <terms:replacedBy rdf:resource="http://purl.org/olia/olia.owl#hasUsage"/>
  </rdf:Description>
  <rdf:Description rdf:about="http://purl.org/olia/discourse/olia_discourse.owl#hasUsage">
    <owl:deprecated rdf:datatype="http://www.w3.org/2001/XMLSchema#boolean">true</owl:deprecated>
  </rdf:Description>
  <rdf:Description rdf:about="http://purl.org/olia/discourse/olia_discourse.owl#Heading">
    <terms:replacedBy rdf:resource="http://purl.org/olia/olia.owl#Heading"/>
  </rdf:Description>
  <rdf:Description rdf:about="http://purl.org/olia/discourse/olia_discourse.owl#Heading">
    <owl:deprecated rdf:datatype="http://www.w3.org/2001/XMLSchema#boolean">true</owl:deprecated>
  </rdf:Description>
  <rdf:Description rdf:about="http://purl.org/olia/discourse/olia_discourse.owl#Headline">
    <terms:replacedBy rdf:resource="http://purl.org/olia/olia.owl#Headline"/>
  </rdf:Description>
  <rdf:Description rdf:about="http://purl.org/olia/discourse/olia_discourse.owl#Headline">
    <owl:deprecated rdf:datatype="http://www.w3.org/2001/XMLSchema#boolean">true</owl:deprecated>
  </rdf:Description>
  <rdf:Description rdf:about="http://purl.org/olia/discourse/olia_discourse.owl#Holiday">
    <terms:replacedBy rdf:resource="http://purl.org/olia/olia.owl#Holiday"/>
  </rdf:Description>
  <rdf:Description rdf:about="http://purl.org/olia/discourse/olia_discourse.owl#Holiday">
    <owl:deprecated rdf:datatype="http://www.w3.org/2001/XMLSchema#boolean">true</owl:deprecated>
  </rdf:Description>
  <rdf:Description rdf:about="http://purl.org/olia/discourse/olia_discourse.owl#Honorific">
    <terms:replacedBy rdf:resource="http://purl.org/olia/olia.owl#Honorific"/>
  </rdf:Description>
  <rdf:Description rdf:about="http://purl.org/olia/discourse/olia_discourse.owl#Honorific">
    <owl:deprecated rdf:datatype="http://www.w3.org/2001/XMLSchema#boolean">true</owl:deprecated>
  </rdf:Description>
  <rdf:Description rdf:about="http://purl.org/olia/discourse/olia_discourse.owl#Hospital">
    <terms:replacedBy rdf:resource="http://purl.org/olia/olia.owl#Hospital"/>
  </rdf:Description>
  <rdf:Description rdf:about="http://purl.org/olia/discourse/olia_discourse.owl#Hospital">
    <owl:deprecated rdf:datatype="http://www.w3.org/2001/XMLSchema#boolean">true</owl:deprecated>
  </rdf:Description>
  <rdf:Description rdf:about="http://purl.org/olia/discourse/olia_discourse.owl#HypotacticDiscourseRelation">
    <terms:replacedBy rdf:resource="http://purl.org/olia/olia.owl#HypotacticDiscourseRelation"/>
  </rdf:Description>
  <rdf:Description rdf:about="http://purl.org/olia/discourse/olia_discourse.owl#HypotacticDiscourseRelation">
    <owl:deprecated rdf:datatype="http://www.w3.org/2001/XMLSchema#boolean">true</owl:deprecated>
  </rdf:Description>
  <rdf:Description rdf:about="http://purl.org/olia/discourse/olia_discourse.owl#HypotheticalCondition">
    <terms:replacedBy rdf:resource="http://purl.org/olia/olia.owl#HypotheticalCondition"/>
  </rdf:Description>
  <rdf:Description rdf:about="http://purl.org/olia/discourse/olia_discourse.owl#HypotheticalCondition">
    <owl:deprecated rdf:datatype="http://www.w3.org/2001/XMLSchema#boolean">true</owl:deprecated>
  </rdf:Description>
  <rdf:Description rdf:about="http://purl.org/olia/discourse/olia_discourse.owl#Identifier">
    <terms:replacedBy rdf:resource="http://purl.org/olia/olia.owl#Identifier"/>
  </rdf:Description>
  <rdf:Description rdf:about="http://purl.org/olia/discourse/olia_discourse.owl#Identifier">
    <owl:deprecated rdf:datatype="http://www.w3.org/2001/XMLSchema#boolean">true</owl:deprecated>
  </rdf:Description>
  <rdf:Description rdf:about="http://purl.org/olia/discourse/olia_discourse.owl#ImplicitConnective">
    <terms:replacedBy rdf:resource="http://purl.org/olia/olia.owl#ImplicitConnective"/>
  </rdf:Description>
  <rdf:Description rdf:about="http://purl.org/olia/discourse/olia_discourse.owl#ImplicitConnective">
    <owl:deprecated rdf:datatype="http://www.w3.org/2001/XMLSchema#boolean">true</owl:deprecated>
  </rdf:Description>
  <rdf:Description rdf:about="http://purl.org/olia/discourse/olia_discourse.owl#ImplicitlyAssertedCondition_PDTB">
    <terms:replacedBy rdf:resource="http://purl.org/olia/olia.owl#ImplicitlyAssertedCondition_PDTB"/>
  </rdf:Description>
  <rdf:Description rdf:about="http://purl.org/olia/discourse/olia_discourse.owl#ImplicitlyAssertedCondition_PDTB">
    <owl:deprecated rdf:datatype="http://www.w3.org/2001/XMLSchema#boolean">true</owl:deprecated>
  </rdf:Description>
  <rdf:Description rdf:about="http://purl.org/olia/discourse/olia_discourse.owl#ImplicitRelation">
    <terms:replacedBy rdf:resource="http://purl.org/olia/olia.owl#ImplicitRelation"/>
  </rdf:Description>
  <rdf:Description rdf:about="http://purl.org/olia/discourse/olia_discourse.owl#ImplicitRelation">
    <owl:deprecated rdf:datatype="http://www.w3.org/2001/XMLSchema#boolean">true</owl:deprecated>
  </rdf:Description>
  <rdf:Description rdf:about="http://purl.org/olia/discourse/olia_discourse.owl#Impossible">
    <terms:replacedBy rdf:resource="http://purl.org/olia/olia.owl#Impossible"/>
  </rdf:Description>
  <rdf:Description rdf:about="http://purl.org/olia/discourse/olia_discourse.owl#Impossible">
    <owl:deprecated rdf:datatype="http://www.w3.org/2001/XMLSchema#boolean">true</owl:deprecated>
  </rdf:Description>
  <rdf:Description rdf:about="http://purl.org/olia/discourse/olia_discourse.owl#Indefinite">
    <terms:replacedBy rdf:resource="http://purl.org/olia/olia.owl#Indefinite"/>
  </rdf:Description>
  <rdf:Description rdf:about="http://purl.org/olia/discourse/olia_discourse.owl#Indefinite">
    <owl:deprecated rdf:datatype="http://www.w3.org/2001/XMLSchema#boolean">true</owl:deprecated>
  </rdf:Description>
  <rdf:Description rdf:about="http://purl.org/olia/discourse/olia_discourse.owl#IndeterminateAttribution">
    <terms:replacedBy rdf:resource="http://purl.org/olia/olia.owl#IndeterminateAttribution"/>
  </rdf:Description>
  <rdf:Description rdf:about="http://purl.org/olia/discourse/olia_discourse.owl#IndeterminateAttribution">
    <owl:deprecated rdf:datatype="http://www.w3.org/2001/XMLSchema#boolean">true</owl:deprecated>
  </rdf:Description>
  <rdf:Description rdf:about="http://purl.org/olia/discourse/olia_discourse.owl#Inferrable">
    <terms:replacedBy rdf:resource="http://purl.org/olia/olia.owl#Inferrable"/>
  </rdf:Description>
  <rdf:Description rdf:about="http://purl.org/olia/discourse/olia_discourse.owl#Inferrable">
    <owl:deprecated rdf:datatype="http://www.w3.org/2001/XMLSchema#boolean">true</owl:deprecated>
  </rdf:Description>
  <rdf:Description rdf:about="http://purl.org/olia/discourse/olia_discourse.owl#InformationStatus">
    <terms:replacedBy rdf:resource="http://purl.org/olia/olia.owl#InformationStatus"/>
  </rdf:Description>
  <rdf:Description rdf:about="http://purl.org/olia/discourse/olia_discourse.owl#InformationStatus">
    <owl:deprecated rdf:datatype="http://www.w3.org/2001/XMLSchema#boolean">true</owl:deprecated>
  </rdf:Description>
  <rdf:Description rdf:about="http://purl.org/olia/discourse/olia_discourse.owl#InfrequentlyUsed">
    <terms:replacedBy rdf:resource="http://purl.org/olia/olia.owl#InfrequentlyUsed"/>
  </rdf:Description>
  <rdf:Description rdf:about="http://purl.org/olia/discourse/olia_discourse.owl#InfrequentlyUsed">
    <owl:deprecated rdf:datatype="http://www.w3.org/2001/XMLSchema#boolean">true</owl:deprecated>
  </rdf:Description>
  <rdf:Description rdf:about="http://purl.org/olia/discourse/olia_discourse.owl#InheritedAttributionSource">
    <terms:replacedBy rdf:resource="http://purl.org/olia/olia.owl#InheritedAttributionSource"/>
  </rdf:Description>
  <rdf:Description rdf:about="http://purl.org/olia/discourse/olia_discourse.owl#InheritedAttributionSource">
    <owl:deprecated rdf:datatype="http://www.w3.org/2001/XMLSchema#boolean">true</owl:deprecated>
  </rdf:Description>
  <rdf:Description rdf:about="http://purl.org/olia/discourse/olia_discourse.owl#InHouseRegister">
    <terms:replacedBy rdf:resource="http://purl.org/olia/olia.owl#InHouseRegister"/>
  </rdf:Description>
  <rdf:Description rdf:about="http://purl.org/olia/discourse/olia_discourse.owl#InHouseRegister">
    <owl:deprecated rdf:datatype="http://www.w3.org/2001/XMLSchema#boolean">true</owl:deprecated>
  </rdf:Description>
  <rdf:Description rdf:about="http://purl.org/olia/discourse/olia_discourse.owl#Insect">
    <terms:replacedBy rdf:resource="http://purl.org/olia/olia.owl#Insect"/>
  </rdf:Description>
  <rdf:Description rdf:about="http://purl.org/olia/discourse/olia_discourse.owl#Insect">
    <owl:deprecated rdf:datatype="http://www.w3.org/2001/XMLSchema#boolean">true</owl:deprecated>
  </rdf:Description>
  <rdf:Description rdf:about="http://purl.org/olia/discourse/olia_discourse.owl#Instantiation">
    <terms:replacedBy rdf:resource="http://purl.org/olia/olia.owl#Instantiation"/>
  </rdf:Description>
  <rdf:Description rdf:about="http://purl.org/olia/discourse/olia_discourse.owl#Instantiation">
    <owl:deprecated rdf:datatype="http://www.w3.org/2001/XMLSchema#boolean">true</owl:deprecated>
  </rdf:Description>
  <rdf:Description rdf:about="http://purl.org/olia/discourse/olia_discourse.owl#Internationalism">
    <terms:replacedBy rdf:resource="http://purl.org/olia/olia.owl#Internationalism"/>
  </rdf:Description>
  <rdf:Description rdf:about="http://purl.org/olia/discourse/olia_discourse.owl#Internationalism">
    <owl:deprecated rdf:datatype="http://www.w3.org/2001/XMLSchema#boolean">true</owl:deprecated>
  </rdf:Description>
  <rdf:Description rdf:about="http://purl.org/olia/discourse/olia_discourse.owl#Interpretation">
    <terms:replacedBy rdf:resource="http://purl.org/olia/olia.owl#Interpretation"/>
  </rdf:Description>
  <rdf:Description rdf:about="http://purl.org/olia/discourse/olia_discourse.owl#Interpretation">
    <owl:deprecated rdf:datatype="http://www.w3.org/2001/XMLSchema#boolean">true</owl:deprecated>
  </rdf:Description>
  <rdf:Description rdf:about="http://purl.org/olia/discourse/olia_discourse.owl#Interpretation_RST">
    <terms:replacedBy rdf:resource="http://purl.org/olia/olia.owl#Interpretation_RST"/>
  </rdf:Description>
  <rdf:Description rdf:about="http://purl.org/olia/discourse/olia_discourse.owl#Interpretation_RST">
    <owl:deprecated rdf:datatype="http://www.w3.org/2001/XMLSchema#boolean">true</owl:deprecated>
  </rdf:Description>
  <rdf:Description rdf:about="http://purl.org/olia/discourse/olia_discourse.owl#inverseOf">
    <terms:replacedBy rdf:resource="http://purl.org/olia/olia.owl#inverseOf"/>
  </rdf:Description>
  <rdf:Description rdf:about="http://purl.org/olia/discourse/olia_discourse.owl#inverseOf">
    <owl:deprecated rdf:datatype="http://www.w3.org/2001/XMLSchema#boolean">true</owl:deprecated>
  </rdf:Description>
  <rdf:Description rdf:about="http://purl.org/olia/discourse/olia_discourse.owl#InvertedSequence">
    <terms:replacedBy rdf:resource="http://purl.org/olia/olia.owl#InvertedSequence"/>
  </rdf:Description>
  <rdf:Description rdf:about="http://purl.org/olia/discourse/olia_discourse.owl#InvertedSequence">
    <owl:deprecated rdf:datatype="http://www.w3.org/2001/XMLSchema#boolean">true</owl:deprecated>
  </rdf:Description>
  <rdf:Description rdf:about="http://purl.org/olia/discourse/olia_discourse.owl#IronicRegister">
    <terms:replacedBy rdf:resource="http://purl.org/olia/olia.owl#IronicRegister"/>
  </rdf:Description>
  <rdf:Description rdf:about="http://purl.org/olia/discourse/olia_discourse.owl#IronicRegister">
    <owl:deprecated rdf:datatype="http://www.w3.org/2001/XMLSchema#boolean">true</owl:deprecated>
  </rdf:Description>
  <rdf:Description rdf:about="http://purl.org/olia/discourse/olia_discourse.owl#Island">
    <terms:replacedBy rdf:resource="http://purl.org/olia/olia.owl#Island"/>
  </rdf:Description>
  <rdf:Description rdf:about="http://purl.org/olia/discourse/olia_discourse.owl#Island">
    <owl:deprecated rdf:datatype="http://www.w3.org/2001/XMLSchema#boolean">true</owl:deprecated>
  </rdf:Description>
  <rdf:Description rdf:about="http://purl.org/olia/discourse/olia_discourse.owl#Joint">
    <terms:replacedBy rdf:resource="http://purl.org/olia/olia.owl#Joint"/>
  </rdf:Description>
  <rdf:Description rdf:about="http://purl.org/olia/discourse/olia_discourse.owl#Joint">
    <owl:deprecated rdf:datatype="http://www.w3.org/2001/XMLSchema#boolean">true</owl:deprecated>
  </rdf:Description>
  <rdf:Description rdf:about="http://purl.org/olia/discourse/olia_discourse.owl#Joint_RST">
    <terms:replacedBy rdf:resource="http://purl.org/olia/olia.owl#Joint_RST"/>
  </rdf:Description>
  <rdf:Description rdf:about="http://purl.org/olia/discourse/olia_discourse.owl#Joint_RST">
    <owl:deprecated rdf:datatype="http://www.w3.org/2001/XMLSchema#boolean">true</owl:deprecated>
  </rdf:Description>
  <rdf:Description rdf:about="http://purl.org/olia/discourse/olia_discourse.owl#Justification">
    <terms:replacedBy rdf:resource="http://purl.org/olia/olia.owl#Justification"/>
  </rdf:Description>
  <rdf:Description rdf:about="http://purl.org/olia/discourse/olia_discourse.owl#Justification">
    <owl:deprecated rdf:datatype="http://www.w3.org/2001/XMLSchema#boolean">true</owl:deprecated>
  </rdf:Description>
  <rdf:Description rdf:about="http://purl.org/olia/discourse/olia_discourse.owl#Juxtaposition_PDTB">
    <terms:replacedBy rdf:resource="http://purl.org/olia/olia.owl#Juxtaposition_PDTB"/>
  </rdf:Description>
  <rdf:Description rdf:about="http://purl.org/olia/discourse/olia_discourse.owl#Juxtaposition_PDTB">
    <owl:deprecated rdf:datatype="http://www.w3.org/2001/XMLSchema#boolean">true</owl:deprecated>
  </rdf:Description>
  <rdf:Description rdf:about="http://purl.org/olia/discourse/olia_discourse.owl#Lake">
    <terms:replacedBy rdf:resource="http://purl.org/olia/olia.owl#Lake"/>
  </rdf:Description>
  <rdf:Description rdf:about="http://purl.org/olia/discourse/olia_discourse.owl#Lake">
    <owl:deprecated rdf:datatype="http://www.w3.org/2001/XMLSchema#boolean">true</owl:deprecated>
  </rdf:Description>
  <rdf:Description rdf:about="http://purl.org/olia/discourse/olia_discourse.owl#LegalRegister">
    <terms:replacedBy rdf:resource="http://purl.org/olia/olia.owl#LegalRegister"/>
  </rdf:Description>
  <rdf:Description rdf:about="http://purl.org/olia/discourse/olia_discourse.owl#LegalRegister">
    <owl:deprecated rdf:datatype="http://www.w3.org/2001/XMLSchema#boolean">true</owl:deprecated>
  </rdf:Description>
  <rdf:Description rdf:about="http://purl.org/olia/discourse/olia_discourse.owl#Legislature">
    <terms:replacedBy rdf:resource="http://purl.org/olia/olia.owl#Legislature"/>
  </rdf:Description>
  <rdf:Description rdf:about="http://purl.org/olia/discourse/olia_discourse.owl#Legislature">
    <owl:deprecated rdf:datatype="http://www.w3.org/2001/XMLSchema#boolean">true</owl:deprecated>
  </rdf:Description>
  <rdf:Description rdf:about="http://purl.org/olia/discourse/olia_discourse.owl#LexicalUnit">
    <terms:replacedBy rdf:resource="http://purl.org/olia/olia.owl#LexicalUnit"/>
  </rdf:Description>
  <rdf:Description rdf:about="http://purl.org/olia/discourse/olia_discourse.owl#LexicalUnit">
    <owl:deprecated rdf:datatype="http://www.w3.org/2001/XMLSchema#boolean">true</owl:deprecated>
  </rdf:Description>
  <rdf:Description rdf:about="http://purl.org/olia/discourse/olia_discourse.owl#Lighthouse">
    <terms:replacedBy rdf:resource="http://purl.org/olia/olia.owl#Lighthouse"/>
  </rdf:Description>
  <rdf:Description rdf:about="http://purl.org/olia/discourse/olia_discourse.owl#Lighthouse">
    <owl:deprecated rdf:datatype="http://www.w3.org/2001/XMLSchema#boolean">true</owl:deprecated>
  </rdf:Description>
  <rdf:Description rdf:about="http://purl.org/olia/discourse/olia_discourse.owl#List">
    <terms:replacedBy rdf:resource="http://purl.org/olia/olia.owl#List"/>
  </rdf:Description>
  <rdf:Description rdf:about="http://purl.org/olia/discourse/olia_discourse.owl#List">
    <owl:deprecated rdf:datatype="http://www.w3.org/2001/XMLSchema#boolean">true</owl:deprecated>
  </rdf:Description>
  <rdf:Description rdf:about="http://purl.org/olia/discourse/olia_discourse.owl#ListSequence">
    <terms:replacedBy rdf:resource="http://purl.org/olia/olia.owl#ListSequence"/>
  </rdf:Description>
  <rdf:Description rdf:about="http://purl.org/olia/discourse/olia_discourse.owl#ListSequence">
    <owl:deprecated rdf:datatype="http://www.w3.org/2001/XMLSchema#boolean">true</owl:deprecated>
  </rdf:Description>
  <rdf:Description rdf:about="http://purl.org/olia/discourse/olia_discourse.owl#Magazine">
    <terms:replacedBy rdf:resource="http://purl.org/olia/olia.owl#Magazine"/>
  </rdf:Description>
  <rdf:Description rdf:about="http://purl.org/olia/discourse/olia_discourse.owl#Magazine">
    <owl:deprecated rdf:datatype="http://www.w3.org/2001/XMLSchema#boolean">true</owl:deprecated>
  </rdf:Description>
  <rdf:Description rdf:about="http://purl.org/olia/discourse/olia_discourse.owl#Manner_RST">
    <terms:replacedBy rdf:resource="http://purl.org/olia/olia.owl#Manner_RST"/>
  </rdf:Description>
  <rdf:Description rdf:about="http://purl.org/olia/discourse/olia_discourse.owl#Manner_RST">
    <owl:deprecated rdf:datatype="http://www.w3.org/2001/XMLSchema#boolean">true</owl:deprecated>
  </rdf:Description>
  <rdf:Description rdf:about="http://purl.org/olia/discourse/olia_discourse.owl#ManufacturedObject">
    <terms:replacedBy rdf:resource="http://purl.org/olia/olia.owl#ManufacturedObject"/>
  </rdf:Description>
  <rdf:Description rdf:about="http://purl.org/olia/discourse/olia_discourse.owl#ManufacturedObject">
    <owl:deprecated rdf:datatype="http://www.w3.org/2001/XMLSchema#boolean">true</owl:deprecated>
  </rdf:Description>
  <rdf:Description rdf:about="http://purl.org/olia/discourse/olia_discourse.owl#MapObject">
    <terms:replacedBy rdf:resource="http://purl.org/olia/olia.owl#MapObject"/>
  </rdf:Description>
  <rdf:Description rdf:about="http://purl.org/olia/discourse/olia_discourse.owl#MapObject">
    <owl:deprecated rdf:datatype="http://www.w3.org/2001/XMLSchema#boolean">true</owl:deprecated>
  </rdf:Description>
  <rdf:Description rdf:about="http://purl.org/olia/discourse/olia_discourse.owl#Markable">
    <terms:replacedBy rdf:resource="http://purl.org/olia/olia.owl#Markable"/>
  </rdf:Description>
  <rdf:Description rdf:about="http://purl.org/olia/discourse/olia_discourse.owl#Markable">
    <owl:deprecated rdf:datatype="http://www.w3.org/2001/XMLSchema#boolean">true</owl:deprecated>
  </rdf:Description>
  <rdf:Description rdf:about="http://purl.org/olia/discourse/olia_discourse.owl#Mayor">
    <terms:replacedBy rdf:resource="http://purl.org/olia/olia.owl#Mayor"/>
  </rdf:Description>
  <rdf:Description rdf:about="http://purl.org/olia/discourse/olia_discourse.owl#Mayor">
    <owl:deprecated rdf:datatype="http://www.w3.org/2001/XMLSchema#boolean">true</owl:deprecated>
  </rdf:Description>
  <rdf:Description rdf:about="http://purl.org/olia/discourse/olia_discourse.owl#Means">
    <terms:replacedBy rdf:resource="http://purl.org/olia/olia.owl#Means"/>
  </rdf:Description>
  <rdf:Description rdf:about="http://purl.org/olia/discourse/olia_discourse.owl#Means">
    <owl:deprecated rdf:datatype="http://www.w3.org/2001/XMLSchema#boolean">true</owl:deprecated>
  </rdf:Description>
  <rdf:Description rdf:about="http://purl.org/olia/discourse/olia_discourse.owl#Means_RST">
    <terms:replacedBy rdf:resource="http://purl.org/olia/olia.owl#Means_RST"/>
  </rdf:Description>
  <rdf:Description rdf:about="http://purl.org/olia/discourse/olia_discourse.owl#Means_RST">
    <owl:deprecated rdf:datatype="http://www.w3.org/2001/XMLSchema#boolean">true</owl:deprecated>
  </rdf:Description>
  <rdf:Description rdf:about="http://purl.org/olia/discourse/olia_discourse.owl#MediaProduct">
    <terms:replacedBy rdf:resource="http://purl.org/olia/olia.owl#MediaProduct"/>
  </rdf:Description>
  <rdf:Description rdf:about="http://purl.org/olia/discourse/olia_discourse.owl#MediaProduct">
    <owl:deprecated rdf:datatype="http://www.w3.org/2001/XMLSchema#boolean">true</owl:deprecated>
  </rdf:Description>
  <rdf:Description rdf:about="http://purl.org/olia/discourse/olia_discourse.owl#MilitaryConflict">
    <terms:replacedBy rdf:resource="http://purl.org/olia/olia.owl#MilitaryConflict"/>
  </rdf:Description>
  <rdf:Description rdf:about="http://purl.org/olia/discourse/olia_discourse.owl#MilitaryConflict">
    <owl:deprecated rdf:datatype="http://www.w3.org/2001/XMLSchema#boolean">true</owl:deprecated>
  </rdf:Description>
  <rdf:Description rdf:about="http://purl.org/olia/discourse/olia_discourse.owl#ModernUsage">
    <terms:replacedBy rdf:resource="http://purl.org/olia/olia.owl#ModernUsage"/>
  </rdf:Description>
  <rdf:Description rdf:about="http://purl.org/olia/discourse/olia_discourse.owl#ModernUsage">
    <owl:deprecated rdf:datatype="http://www.w3.org/2001/XMLSchema#boolean">true</owl:deprecated>
  </rdf:Description>
  <rdf:Description rdf:about="http://purl.org/olia/discourse/olia_discourse.owl#Motivation_RST">
    <terms:replacedBy rdf:resource="http://purl.org/olia/olia.owl#Motivation_RST"/>
  </rdf:Description>
  <rdf:Description rdf:about="http://purl.org/olia/discourse/olia_discourse.owl#Motivation_RST">
    <owl:deprecated rdf:datatype="http://www.w3.org/2001/XMLSchema#boolean">true</owl:deprecated>
  </rdf:Description>
  <rdf:Description rdf:about="http://purl.org/olia/discourse/olia_discourse.owl#Mountain">
    <terms:replacedBy rdf:resource="http://purl.org/olia/olia.owl#Mountain"/>
  </rdf:Description>
  <rdf:Description rdf:about="http://purl.org/olia/discourse/olia_discourse.owl#Mountain">
    <owl:deprecated rdf:datatype="http://www.w3.org/2001/XMLSchema#boolean">true</owl:deprecated>
  </rdf:Description>
  <rdf:Description rdf:about="http://purl.org/olia/discourse/olia_discourse.owl#Movie">
    <terms:replacedBy rdf:resource="http://purl.org/olia/olia.owl#Movie"/>
  </rdf:Description>
  <rdf:Description rdf:about="http://purl.org/olia/discourse/olia_discourse.owl#Movie">
    <owl:deprecated rdf:datatype="http://www.w3.org/2001/XMLSchema#boolean">true</owl:deprecated>
  </rdf:Description>
  <rdf:Description rdf:about="http://purl.org/olia/discourse/olia_discourse.owl#Museum">
    <terms:replacedBy rdf:resource="http://purl.org/olia/olia.owl#Museum"/>
  </rdf:Description>
  <rdf:Description rdf:about="http://purl.org/olia/discourse/olia_discourse.owl#Museum">
    <owl:deprecated rdf:datatype="http://www.w3.org/2001/XMLSchema#boolean">true</owl:deprecated>
  </rdf:Description>
  <rdf:Description rdf:about="http://purl.org/olia/discourse/olia_discourse.owl#MusicalArtist">
    <terms:replacedBy rdf:resource="http://purl.org/olia/olia.owl#MusicalArtist"/>
  </rdf:Description>
  <rdf:Description rdf:about="http://purl.org/olia/discourse/olia_discourse.owl#MusicalArtist">
    <owl:deprecated rdf:datatype="http://www.w3.org/2001/XMLSchema#boolean">true</owl:deprecated>
  </rdf:Description>
  <rdf:Description rdf:about="http://purl.org/olia/discourse/olia_discourse.owl#MusicalEnsemble">
    <terms:replacedBy rdf:resource="http://purl.org/olia/olia.owl#MusicalEnsemble"/>
  </rdf:Description>
  <rdf:Description rdf:about="http://purl.org/olia/discourse/olia_discourse.owl#MusicalEnsemble">
    <owl:deprecated rdf:datatype="http://www.w3.org/2001/XMLSchema#boolean">true</owl:deprecated>
  </rdf:Description>
  <rdf:Description rdf:about="http://purl.org/olia/discourse/olia_discourse.owl#NamedEntity">
    <terms:replacedBy rdf:resource="http://purl.org/olia/olia.owl#NamedEntity"/>
  </rdf:Description>
  <rdf:Description rdf:about="http://purl.org/olia/discourse/olia_discourse.owl#NamedEntity">
    <owl:deprecated rdf:datatype="http://www.w3.org/2001/XMLSchema#boolean">true</owl:deprecated>
  </rdf:Description>
  <rdf:Description rdf:about="http://purl.org/olia/discourse/olia_discourse.owl#NarrowFocus">
    <terms:replacedBy rdf:resource="http://purl.org/olia/olia.owl#NarrowFocus"/>
  </rdf:Description>
  <rdf:Description rdf:about="http://purl.org/olia/discourse/olia_discourse.owl#NarrowFocus">
    <owl:deprecated rdf:datatype="http://www.w3.org/2001/XMLSchema#boolean">true</owl:deprecated>
  </rdf:Description>
  <rdf:Description rdf:about="http://purl.org/olia/discourse/olia_discourse.owl#NegatedAttribution">
    <terms:replacedBy rdf:resource="http://purl.org/olia/olia.owl#NegatedAttribution"/>
  </rdf:Description>
  <rdf:Description rdf:about="http://purl.org/olia/discourse/olia_discourse.owl#NegatedAttribution">
    <owl:deprecated rdf:datatype="http://www.w3.org/2001/XMLSchema#boolean">true</owl:deprecated>
  </rdf:Description>
  <rdf:Description rdf:about="http://purl.org/olia/discourse/olia_discourse.owl#NegativeCondition">
    <terms:replacedBy rdf:resource="http://purl.org/olia/olia.owl#NegativeCondition"/>
  </rdf:Description>
  <rdf:Description rdf:about="http://purl.org/olia/discourse/olia_discourse.owl#NegativeCondition">
    <owl:deprecated rdf:datatype="http://www.w3.org/2001/XMLSchema#boolean">true</owl:deprecated>
  </rdf:Description>
  <rdf:Description rdf:about="http://purl.org/olia/discourse/olia_discourse.owl#NegativePolarity">
    <terms:replacedBy rdf:resource="http://purl.org/olia/olia.owl#NegativePolarity"/>
  </rdf:Description>
  <rdf:Description rdf:about="http://purl.org/olia/discourse/olia_discourse.owl#NegativePolarity">
    <owl:deprecated rdf:datatype="http://www.w3.org/2001/XMLSchema#boolean">true</owl:deprecated>
  </rdf:Description>
  <rdf:Description rdf:about="http://purl.org/olia/discourse/olia_discourse.owl#NeutralRegister">
    <terms:replacedBy rdf:resource="http://purl.org/olia/olia.owl#NeutralRegister"/>
  </rdf:Description>
  <rdf:Description rdf:about="http://purl.org/olia/discourse/olia_discourse.owl#NeutralRegister">
    <owl:deprecated rdf:datatype="http://www.w3.org/2001/XMLSchema#boolean">true</owl:deprecated>
  </rdf:Description>
  <rdf:Description rdf:about="http://purl.org/olia/discourse/olia_discourse.owl#New">
    <terms:replacedBy rdf:resource="http://purl.org/olia/olia.owl#New"/>
  </rdf:Description>
  <rdf:Description rdf:about="http://purl.org/olia/discourse/olia_discourse.owl#New">
    <owl:deprecated rdf:datatype="http://www.w3.org/2001/XMLSchema#boolean">true</owl:deprecated>
  </rdf:Description>
  <rdf:Description rdf:about="http://purl.org/olia/discourse/olia_discourse.owl#NewInformationFocus">
    <terms:replacedBy rdf:resource="http://purl.org/olia/olia.owl#NewInformationFocus"/>
  </rdf:Description>
  <rdf:Description rdf:about="http://purl.org/olia/discourse/olia_discourse.owl#NewInformationFocus">
    <owl:deprecated rdf:datatype="http://www.w3.org/2001/XMLSchema#boolean">true</owl:deprecated>
  </rdf:Description>
  <rdf:Description rdf:about="http://purl.org/olia/discourse/olia_discourse.owl#Newspaper">
    <terms:replacedBy rdf:resource="http://purl.org/olia/olia.owl#Newspaper"/>
  </rdf:Description>
  <rdf:Description rdf:about="http://purl.org/olia/discourse/olia_discourse.owl#Newspaper">
    <owl:deprecated rdf:datatype="http://www.w3.org/2001/XMLSchema#boolean">true</owl:deprecated>
  </rdf:Description>
  <rdf:Description rdf:about="http://purl.org/olia/discourse/olia_discourse.owl#NonContrastiveComparison">
    <terms:replacedBy rdf:resource="http://purl.org/olia/olia.owl#NonContrastiveComparison"/>
  </rdf:Description>
  <rdf:Description rdf:about="http://purl.org/olia/discourse/olia_discourse.owl#NonContrastiveComparison">
    <owl:deprecated rdf:datatype="http://www.w3.org/2001/XMLSchema#boolean">true</owl:deprecated>
  </rdf:Description>
  <rdf:Description rdf:about="http://purl.org/olia/discourse/olia_discourse.owl#NonNegatedAttribution">
    <terms:replacedBy rdf:resource="http://purl.org/olia/olia.owl#NonNegatedAttribution"/>
  </rdf:Description>
  <rdf:Description rdf:about="http://purl.org/olia/discourse/olia_discourse.owl#NonNegatedAttribution">
    <owl:deprecated rdf:datatype="http://www.w3.org/2001/XMLSchema#boolean">true</owl:deprecated>
  </rdf:Description>
  <rdf:Description rdf:about="http://purl.org/olia/discourse/olia_discourse.owl#NonProfitOrganization">
    <terms:replacedBy rdf:resource="http://purl.org/olia/olia.owl#NonProfitOrganization"/>
  </rdf:Description>
  <rdf:Description rdf:about="http://purl.org/olia/discourse/olia_discourse.owl#NonProfitOrganization">
    <owl:deprecated rdf:datatype="http://www.w3.org/2001/XMLSchema#boolean">true</owl:deprecated>
  </rdf:Description>
  <rdf:Description rdf:about="http://purl.org/olia/discourse/olia_discourse.owl#NonReferring">
    <terms:replacedBy rdf:resource="http://purl.org/olia/olia.owl#NonReferring"/>
  </rdf:Description>
  <rdf:Description rdf:about="http://purl.org/olia/discourse/olia_discourse.owl#NonReferring">
    <owl:deprecated rdf:datatype="http://www.w3.org/2001/XMLSchema#boolean">true</owl:deprecated>
  </rdf:Description>
  <rdf:Description rdf:about="http://purl.org/olia/discourse/olia_discourse.owl#NonspecificAttributionSource">
    <terms:replacedBy rdf:resource="http://purl.org/olia/olia.owl#NonspecificAttributionSource"/>
  </rdf:Description>
  <rdf:Description rdf:about="http://purl.org/olia/discourse/olia_discourse.owl#NonspecificAttributionSource">
    <owl:deprecated rdf:datatype="http://www.w3.org/2001/XMLSchema#boolean">true</owl:deprecated>
  </rdf:Description>
  <rdf:Description rdf:about="http://purl.org/olia/discourse/olia_discourse.owl#NonVolitionalCause_RST">
    <terms:replacedBy rdf:resource="http://purl.org/olia/olia.owl#NonVolitionalCause_RST"/>
  </rdf:Description>
  <rdf:Description rdf:about="http://purl.org/olia/discourse/olia_discourse.owl#NonVolitionalCause_RST">
    <owl:deprecated rdf:datatype="http://www.w3.org/2001/XMLSchema#boolean">true</owl:deprecated>
  </rdf:Description>
  <rdf:Description rdf:about="http://purl.org/olia/discourse/olia_discourse.owl#NonVolitionalResult_RST">
    <terms:replacedBy rdf:resource="http://purl.org/olia/olia.owl#NonVolitionalResult_RST"/>
  </rdf:Description>
  <rdf:Description rdf:about="http://purl.org/olia/discourse/olia_discourse.owl#NonVolitionalResult_RST">
    <owl:deprecated rdf:datatype="http://www.w3.org/2001/XMLSchema#boolean">true</owl:deprecated>
  </rdf:Description>
  <rdf:Description rdf:about="http://purl.org/olia/discourse/olia_discourse.owl#Object">
    <terms:replacedBy rdf:resource="http://purl.org/olia/olia.owl#Object"/>
  </rdf:Description>
  <rdf:Description rdf:about="http://purl.org/olia/discourse/olia_discourse.owl#Object">
    <owl:deprecated rdf:datatype="http://www.w3.org/2001/XMLSchema#boolean">true</owl:deprecated>
  </rdf:Description>
  <rdf:Description rdf:about="http://purl.org/olia/discourse/olia_discourse.owl#ObjectFocus">
    <terms:replacedBy rdf:resource="http://purl.org/olia/olia.owl#ObjectFocus"/>
  </rdf:Description>
  <rdf:Description rdf:about="http://purl.org/olia/discourse/olia_discourse.owl#ObjectFocus">
    <owl:deprecated rdf:datatype="http://www.w3.org/2001/XMLSchema#boolean">true</owl:deprecated>
  </rdf:Description>
  <rdf:Description rdf:about="http://purl.org/olia/discourse/olia_discourse.owl#OldUsage">
    <terms:replacedBy rdf:resource="http://purl.org/olia/olia.owl#OldUsage"/>
  </rdf:Description>
  <rdf:Description rdf:about="http://purl.org/olia/discourse/olia_discourse.owl#OldUsage">
    <owl:deprecated rdf:datatype="http://www.w3.org/2001/XMLSchema#boolean">true</owl:deprecated>
  </rdf:Description>
  <rdf:Description rdf:about="http://purl.org/olia/discourse/olia_discourse.owl#OperatingSystem">
    <terms:replacedBy rdf:resource="http://purl.org/olia/olia.owl#OperatingSystem"/>
  </rdf:Description>
  <rdf:Description rdf:about="http://purl.org/olia/discourse/olia_discourse.owl#OperatingSystem">
    <owl:deprecated rdf:datatype="http://www.w3.org/2001/XMLSchema#boolean">true</owl:deprecated>
  </rdf:Description>
  <rdf:Description rdf:about="http://purl.org/olia/discourse/olia_discourse.owl#OperatorFocus">
    <terms:replacedBy rdf:resource="http://purl.org/olia/olia.owl#OperatorFocus"/>
  </rdf:Description>
  <rdf:Description rdf:about="http://purl.org/olia/discourse/olia_discourse.owl#OperatorFocus">
    <owl:deprecated rdf:datatype="http://www.w3.org/2001/XMLSchema#boolean">true</owl:deprecated>
  </rdf:Description>
  <rdf:Description rdf:about="http://purl.org/olia/discourse/olia_discourse.owl#Opposition_PDTB">
    <terms:replacedBy rdf:resource="http://purl.org/olia/olia.owl#Opposition_PDTB"/>
  </rdf:Description>
  <rdf:Description rdf:about="http://purl.org/olia/discourse/olia_discourse.owl#Opposition_PDTB">
    <owl:deprecated rdf:datatype="http://www.w3.org/2001/XMLSchema#boolean">true</owl:deprecated>
  </rdf:Description>
  <rdf:Description rdf:about="http://purl.org/olia/discourse/olia_discourse.owl#Organization">
    <terms:replacedBy rdf:resource="http://purl.org/olia/olia.owl#Organization"/>
  </rdf:Description>
  <rdf:Description rdf:about="http://purl.org/olia/discourse/olia_discourse.owl#Organization">
    <owl:deprecated rdf:datatype="http://www.w3.org/2001/XMLSchema#boolean">true</owl:deprecated>
  </rdf:Description>
  <rdf:Description rdf:about="http://purl.org/olia/discourse/olia_discourse.owl#Other">
    <terms:replacedBy rdf:resource="http://purl.org/olia/olia.owl#Other"/>
  </rdf:Description>
  <rdf:Description rdf:about="http://purl.org/olia/discourse/olia_discourse.owl#Other">
    <owl:deprecated rdf:datatype="http://www.w3.org/2001/XMLSchema#boolean">true</owl:deprecated>
  </rdf:Description>
  <rdf:Description rdf:about="http://purl.org/olia/discourse/olia_discourse.owl#Otherwise_RST">
    <terms:replacedBy rdf:resource="http://purl.org/olia/olia.owl#Otherwise_RST"/>
  </rdf:Description>
  <rdf:Description rdf:about="http://purl.org/olia/discourse/olia_discourse.owl#Otherwise_RST">
    <owl:deprecated rdf:datatype="http://www.w3.org/2001/XMLSchema#boolean">true</owl:deprecated>
  </rdf:Description>
  <rdf:Description rdf:about="http://purl.org/olia/discourse/olia_discourse.owl#Parallel">
    <terms:replacedBy rdf:resource="http://purl.org/olia/olia.owl#Parallel"/>
  </rdf:Description>
  <rdf:Description rdf:about="http://purl.org/olia/discourse/olia_discourse.owl#Parallel">
    <owl:deprecated rdf:datatype="http://www.w3.org/2001/XMLSchema#boolean">true</owl:deprecated>
  </rdf:Description>
  <rdf:Description rdf:about="http://purl.org/olia/discourse/olia_discourse.owl#ParatacticDiscourseRelation">
    <terms:replacedBy rdf:resource="http://purl.org/olia/olia.owl#ParatacticDiscourseRelation"/>
  </rdf:Description>
  <rdf:Description rdf:about="http://purl.org/olia/discourse/olia_discourse.owl#ParatacticDiscourseRelation">
    <owl:deprecated rdf:datatype="http://www.w3.org/2001/XMLSchema#boolean">true</owl:deprecated>
  </rdf:Description>
  <rdf:Description rdf:about="http://purl.org/olia/discourse/olia_discourse.owl#Park">
    <terms:replacedBy rdf:resource="http://purl.org/olia/olia.owl#Park"/>
  </rdf:Description>
  <rdf:Description rdf:about="http://purl.org/olia/discourse/olia_discourse.owl#Park">
    <owl:deprecated rdf:datatype="http://www.w3.org/2001/XMLSchema#boolean">true</owl:deprecated>
  </rdf:Description>
  <rdf:Description rdf:about="http://purl.org/olia/discourse/olia_discourse.owl#PartOf">
    <terms:replacedBy rdf:resource="http://purl.org/olia/olia.owl#PartOf"/>
  </rdf:Description>
  <rdf:Description rdf:about="http://purl.org/olia/discourse/olia_discourse.owl#PartOf">
    <owl:deprecated rdf:datatype="http://www.w3.org/2001/XMLSchema#boolean">true</owl:deprecated>
  </rdf:Description>
  <rdf:Description rdf:about="http://purl.org/olia/discourse/olia_discourse.owl#PartWhole">
    <terms:replacedBy rdf:resource="http://purl.org/olia/olia.owl#PartWhole"/>
  </rdf:Description>
  <rdf:Description rdf:about="http://purl.org/olia/discourse/olia_discourse.owl#PartWhole">
    <owl:deprecated rdf:datatype="http://www.w3.org/2001/XMLSchema#boolean">true</owl:deprecated>
  </rdf:Description>
  <rdf:Description rdf:about="http://purl.org/olia/discourse/olia_discourse.owl#Person">
    <terms:replacedBy rdf:resource="http://purl.org/olia/olia.owl#Person"/>
  </rdf:Description>
  <rdf:Description rdf:about="http://purl.org/olia/discourse/olia_discourse.owl#Person">
    <owl:deprecated rdf:datatype="http://www.w3.org/2001/XMLSchema#boolean">true</owl:deprecated>
  </rdf:Description>
  <rdf:Description rdf:about="http://purl.org/olia/discourse/olia_discourse.owl#Personal">
    <terms:replacedBy rdf:resource="http://purl.org/olia/olia.owl#Personal"/>
  </rdf:Description>
  <rdf:Description rdf:about="http://purl.org/olia/discourse/olia_discourse.owl#Personal">
    <owl:deprecated rdf:datatype="http://www.w3.org/2001/XMLSchema#boolean">true</owl:deprecated>
  </rdf:Description>
  <rdf:Description rdf:about="http://purl.org/olia/discourse/olia_discourse.owl#PhoneNumber">
    <terms:replacedBy rdf:resource="http://purl.org/olia/olia.owl#PhoneNumber"/>
  </rdf:Description>
  <rdf:Description rdf:about="http://purl.org/olia/discourse/olia_discourse.owl#PhoneNumber">
    <owl:deprecated rdf:datatype="http://www.w3.org/2001/XMLSchema#boolean">true</owl:deprecated>
  </rdf:Description>
  <rdf:Description rdf:about="http://purl.org/olia/discourse/olia_discourse.owl#PlainRestatement_RST">
    <terms:replacedBy rdf:resource="http://purl.org/olia/olia.owl#PlainRestatement_RST"/>
  </rdf:Description>
  <rdf:Description rdf:about="http://purl.org/olia/discourse/olia_discourse.owl#PlainRestatement_RST">
    <owl:deprecated rdf:datatype="http://www.w3.org/2001/XMLSchema#boolean">true</owl:deprecated>
  </rdf:Description>
  <rdf:Description rdf:about="http://purl.org/olia/discourse/olia_discourse.owl#Plan">
    <terms:replacedBy rdf:resource="http://purl.org/olia/olia.owl#Plan"/>
  </rdf:Description>
  <rdf:Description rdf:about="http://purl.org/olia/discourse/olia_discourse.owl#Plan">
    <owl:deprecated rdf:datatype="http://www.w3.org/2001/XMLSchema#boolean">true</owl:deprecated>
  </rdf:Description>
  <rdf:Description rdf:about="http://purl.org/olia/discourse/olia_discourse.owl#PointOfOrigin">
    <terms:replacedBy rdf:resource="http://purl.org/olia/olia.owl#PointOfOrigin"/>
  </rdf:Description>
  <rdf:Description rdf:about="http://purl.org/olia/discourse/olia_discourse.owl#PointOfOrigin">
    <owl:deprecated rdf:datatype="http://www.w3.org/2001/XMLSchema#boolean">true</owl:deprecated>
  </rdf:Description>
  <rdf:Description rdf:about="http://purl.org/olia/discourse/olia_discourse.owl#Polarity">
    <terms:replacedBy rdf:resource="http://purl.org/olia/olia.owl#Polarity"/>
  </rdf:Description>
  <rdf:Description rdf:about="http://purl.org/olia/discourse/olia_discourse.owl#Polarity">
    <owl:deprecated rdf:datatype="http://www.w3.org/2001/XMLSchema#boolean">true</owl:deprecated>
  </rdf:Description>
  <rdf:Description rdf:about="http://purl.org/olia/discourse/olia_discourse.owl#PolarityFocus">
    <terms:replacedBy rdf:resource="http://purl.org/olia/olia.owl#PolarityFocus"/>
  </rdf:Description>
  <rdf:Description rdf:about="http://purl.org/olia/discourse/olia_discourse.owl#PolarityFocus">
    <owl:deprecated rdf:datatype="http://www.w3.org/2001/XMLSchema#boolean">true</owl:deprecated>
  </rdf:Description>
  <rdf:Description rdf:about="http://purl.org/olia/discourse/olia_discourse.owl#PoliticalEvent">
    <terms:replacedBy rdf:resource="http://purl.org/olia/olia.owl#PoliticalEvent"/>
  </rdf:Description>
  <rdf:Description rdf:about="http://purl.org/olia/discourse/olia_discourse.owl#PoliticalEvent">
    <owl:deprecated rdf:datatype="http://www.w3.org/2001/XMLSchema#boolean">true</owl:deprecated>
  </rdf:Description>
  <rdf:Description rdf:about="http://purl.org/olia/discourse/olia_discourse.owl#PoliticalOrganization">
    <terms:replacedBy rdf:resource="http://purl.org/olia/olia.owl#PoliticalOrganization"/>
  </rdf:Description>
  <rdf:Description rdf:about="http://purl.org/olia/discourse/olia_discourse.owl#PoliticalOrganization">
    <owl:deprecated rdf:datatype="http://www.w3.org/2001/XMLSchema#boolean">true</owl:deprecated>
  </rdf:Description>
  <rdf:Description rdf:about="http://purl.org/olia/discourse/olia_discourse.owl#PoliticalParty">
    <terms:replacedBy rdf:resource="http://purl.org/olia/olia.owl#PoliticalParty"/>
  </rdf:Description>
  <rdf:Description rdf:about="http://purl.org/olia/discourse/olia_discourse.owl#PoliticalParty">
    <owl:deprecated rdf:datatype="http://www.w3.org/2001/XMLSchema#boolean">true</owl:deprecated>
  </rdf:Description>
  <rdf:Description rdf:about="http://purl.org/olia/discourse/olia_discourse.owl#PoliticalUnit">
    <terms:replacedBy rdf:resource="http://purl.org/olia/olia.owl#PoliticalUnit"/>
  </rdf:Description>
  <rdf:Description rdf:about="http://purl.org/olia/discourse/olia_discourse.owl#PoliticalUnit">
    <owl:deprecated rdf:datatype="http://www.w3.org/2001/XMLSchema#boolean">true</owl:deprecated>
  </rdf:Description>
  <rdf:Description rdf:about="http://purl.org/olia/discourse/olia_discourse.owl#Politician">
    <terms:replacedBy rdf:resource="http://purl.org/olia/olia.owl#Politician"/>
  </rdf:Description>
  <rdf:Description rdf:about="http://purl.org/olia/discourse/olia_discourse.owl#Politician">
    <owl:deprecated rdf:datatype="http://www.w3.org/2001/XMLSchema#boolean">true</owl:deprecated>
  </rdf:Description>
  <rdf:Description rdf:about="http://purl.org/olia/discourse/olia_discourse.owl#Possessive">
    <terms:replacedBy rdf:resource="http://purl.org/olia/olia.owl#Possessive"/>
  </rdf:Description>
  <rdf:Description rdf:about="http://purl.org/olia/discourse/olia_discourse.owl#Possessive">
    <owl:deprecated rdf:datatype="http://www.w3.org/2001/XMLSchema#boolean">true</owl:deprecated>
  </rdf:Description>
  <rdf:Description rdf:about="http://purl.org/olia/discourse/olia_discourse.owl#Possible">
    <terms:replacedBy rdf:resource="http://purl.org/olia/olia.owl#Possible"/>
  </rdf:Description>
  <rdf:Description rdf:about="http://purl.org/olia/discourse/olia_discourse.owl#Possible">
    <owl:deprecated rdf:datatype="http://www.w3.org/2001/XMLSchema#boolean">true</owl:deprecated>
  </rdf:Description>
  <rdf:Description rdf:about="http://purl.org/olia/discourse/olia_discourse.owl#PragmaticCause">
    <terms:replacedBy rdf:resource="http://purl.org/olia/olia.owl#PragmaticCause"/>
  </rdf:Description>
  <rdf:Description rdf:about="http://purl.org/olia/discourse/olia_discourse.owl#PragmaticCause">
    <owl:deprecated rdf:datatype="http://www.w3.org/2001/XMLSchema#boolean">true</owl:deprecated>
  </rdf:Description>
  <rdf:Description rdf:about="http://purl.org/olia/discourse/olia_discourse.owl#PragmaticConcession_HDRB">
    <terms:replacedBy rdf:resource="http://purl.org/olia/olia.owl#PragmaticConcession_HDRB"/>
  </rdf:Description>
  <rdf:Description rdf:about="http://purl.org/olia/discourse/olia_discourse.owl#PragmaticConcession_HDRB">
    <owl:deprecated rdf:datatype="http://www.w3.org/2001/XMLSchema#boolean">true</owl:deprecated>
  </rdf:Description>
  <rdf:Description rdf:about="http://purl.org/olia/discourse/olia_discourse.owl#PragmaticConcession_LUNA">
    <terms:replacedBy rdf:resource="http://purl.org/olia/olia.owl#PragmaticConcession_LUNA"/>
  </rdf:Description>
  <rdf:Description rdf:about="http://purl.org/olia/discourse/olia_discourse.owl#PragmaticConcession_LUNA">
    <owl:deprecated rdf:datatype="http://www.w3.org/2001/XMLSchema#boolean">true</owl:deprecated>
  </rdf:Description>
  <rdf:Description rdf:about="http://purl.org/olia/discourse/olia_discourse.owl#PragmaticCondition">
    <terms:replacedBy rdf:resource="http://purl.org/olia/olia.owl#PragmaticCondition"/>
  </rdf:Description>
  <rdf:Description rdf:about="http://purl.org/olia/discourse/olia_discourse.owl#PragmaticCondition">
    <owl:deprecated rdf:datatype="http://www.w3.org/2001/XMLSchema#boolean">true</owl:deprecated>
  </rdf:Description>
  <rdf:Description rdf:about="http://purl.org/olia/discourse/olia_discourse.owl#PragmaticContrast_PDTB">
    <terms:replacedBy rdf:resource="http://purl.org/olia/olia.owl#PragmaticContrast_PDTB"/>
  </rdf:Description>
  <rdf:Description rdf:about="http://purl.org/olia/discourse/olia_discourse.owl#PragmaticContrast_PDTB">
    <owl:deprecated rdf:datatype="http://www.w3.org/2001/XMLSchema#boolean">true</owl:deprecated>
  </rdf:Description>
  <rdf:Description rdf:about="http://purl.org/olia/discourse/olia_discourse.owl#PragmaticRelation">
    <terms:replacedBy rdf:resource="http://purl.org/olia/olia.owl#PragmaticRelation"/>
  </rdf:Description>
  <rdf:Description rdf:about="http://purl.org/olia/discourse/olia_discourse.owl#PragmaticRelation">
    <owl:deprecated rdf:datatype="http://www.w3.org/2001/XMLSchema#boolean">true</owl:deprecated>
  </rdf:Description>
  <rdf:Description rdf:about="http://purl.org/olia/discourse/olia_discourse.owl#PragmaticUnit">
    <terms:replacedBy rdf:resource="http://purl.org/olia/olia.owl#PragmaticUnit"/>
  </rdf:Description>
  <rdf:Description rdf:about="http://purl.org/olia/discourse/olia_discourse.owl#PragmaticUnit">
    <owl:deprecated rdf:datatype="http://www.w3.org/2001/XMLSchema#boolean">true</owl:deprecated>
  </rdf:Description>
  <rdf:Description rdf:about="http://purl.org/olia/discourse/olia_discourse.owl#PrecedenceRelation">
    <terms:replacedBy rdf:resource="http://purl.org/olia/olia.owl#PrecedenceRelation"/>
  </rdf:Description>
  <rdf:Description rdf:about="http://purl.org/olia/discourse/olia_discourse.owl#PrecedenceRelation">
    <owl:deprecated rdf:datatype="http://www.w3.org/2001/XMLSchema#boolean">true</owl:deprecated>
  </rdf:Description>
  <rdf:Description rdf:about="http://purl.org/olia/discourse/olia_discourse.owl#PredicateCenteredFocus">
    <terms:replacedBy rdf:resource="http://purl.org/olia/olia.owl#PredicateCenteredFocus"/>
  </rdf:Description>
  <rdf:Description rdf:about="http://purl.org/olia/discourse/olia_discourse.owl#PredicateCenteredFocus">
    <owl:deprecated rdf:datatype="http://www.w3.org/2001/XMLSchema#boolean">true</owl:deprecated>
  </rdf:Description>
  <rdf:Description rdf:about="http://purl.org/olia/discourse/olia_discourse.owl#PredicateFocus">
    <terms:replacedBy rdf:resource="http://purl.org/olia/olia.owl#PredicateFocus"/>
  </rdf:Description>
  <rdf:Description rdf:about="http://purl.org/olia/discourse/olia_discourse.owl#PredicateFocus">
    <owl:deprecated rdf:datatype="http://www.w3.org/2001/XMLSchema#boolean">true</owl:deprecated>
  </rdf:Description>
  <rdf:Description rdf:about="http://purl.org/olia/discourse/olia_discourse.owl#Preference_RST">
    <terms:replacedBy rdf:resource="http://purl.org/olia/olia.owl#Preference_RST"/>
  </rdf:Description>
  <rdf:Description rdf:about="http://purl.org/olia/discourse/olia_discourse.owl#Preference_RST">
    <owl:deprecated rdf:datatype="http://www.w3.org/2001/XMLSchema#boolean">true</owl:deprecated>
  </rdf:Description>
  <rdf:Description rdf:about="http://purl.org/olia/discourse/olia_discourse.owl#Preferred">
    <terms:replacedBy rdf:resource="http://purl.org/olia/olia.owl#Preferred"/>
  </rdf:Description>
  <rdf:Description rdf:about="http://purl.org/olia/discourse/olia_discourse.owl#Preferred">
    <owl:deprecated rdf:datatype="http://www.w3.org/2001/XMLSchema#boolean">true</owl:deprecated>
  </rdf:Description>
  <rdf:Description rdf:about="http://purl.org/olia/discourse/olia_discourse.owl#PreferredAlternative_RST">
    <terms:replacedBy rdf:resource="http://purl.org/olia/olia.owl#PreferredAlternative_RST"/>
  </rdf:Description>
  <rdf:Description rdf:about="http://purl.org/olia/discourse/olia_discourse.owl#PreferredAlternative_RST">
    <owl:deprecated rdf:datatype="http://www.w3.org/2001/XMLSchema#boolean">true</owl:deprecated>
  </rdf:Description>
  <rdf:Description rdf:about="http://purl.org/olia/discourse/olia_discourse.owl#Preparation">
    <terms:replacedBy rdf:resource="http://purl.org/olia/olia.owl#Preparation"/>
  </rdf:Description>
  <rdf:Description rdf:about="http://purl.org/olia/discourse/olia_discourse.owl#Preparation">
    <owl:deprecated rdf:datatype="http://www.w3.org/2001/XMLSchema#boolean">true</owl:deprecated>
  </rdf:Description>
  <rdf:Description rdf:about="http://purl.org/olia/discourse/olia_discourse.owl#PreparationQuestion">
    <terms:replacedBy rdf:resource="http://purl.org/olia/olia.owl#PreparationQuestion"/>
  </rdf:Description>
  <rdf:Description rdf:about="http://purl.org/olia/discourse/olia_discourse.owl#PreparationQuestion">
    <owl:deprecated rdf:datatype="http://www.w3.org/2001/XMLSchema#boolean">true</owl:deprecated>
  </rdf:Description>
  <rdf:Description rdf:about="http://purl.org/olia/discourse/olia_discourse.owl#Preparation_RST">
    <terms:replacedBy rdf:resource="http://purl.org/olia/olia.owl#Preparation_RST"/>
  </rdf:Description>
  <rdf:Description rdf:about="http://purl.org/olia/discourse/olia_discourse.owl#Preparation_RST">
    <owl:deprecated rdf:datatype="http://www.w3.org/2001/XMLSchema#boolean">true</owl:deprecated>
  </rdf:Description>
  <rdf:Description rdf:about="http://purl.org/olia/discourse/olia_discourse.owl#PreparationTitle">
    <terms:replacedBy rdf:resource="http://purl.org/olia/olia.owl#PreparationTitle"/>
  </rdf:Description>
  <rdf:Description rdf:about="http://purl.org/olia/discourse/olia_discourse.owl#PreparationTitle">
    <owl:deprecated rdf:datatype="http://www.w3.org/2001/XMLSchema#boolean">true</owl:deprecated>
  </rdf:Description>
  <rdf:Description rdf:about="http://purl.org/olia/discourse/olia_discourse.owl#PresentationalRelation">
    <terms:replacedBy rdf:resource="http://purl.org/olia/olia.owl#PresentationalRelation"/>
  </rdf:Description>
  <rdf:Description rdf:about="http://purl.org/olia/discourse/olia_discourse.owl#PresentationalRelation">
    <owl:deprecated rdf:datatype="http://www.w3.org/2001/XMLSchema#boolean">true</owl:deprecated>
  </rdf:Description>
  <rdf:Description rdf:about="http://purl.org/olia/discourse/olia_discourse.owl#ProblemSolution">
    <terms:replacedBy rdf:resource="http://purl.org/olia/olia.owl#ProblemSolution"/>
  </rdf:Description>
  <rdf:Description rdf:about="http://purl.org/olia/discourse/olia_discourse.owl#ProblemSolution">
    <owl:deprecated rdf:datatype="http://www.w3.org/2001/XMLSchema#boolean">true</owl:deprecated>
  </rdf:Description>
  <rdf:Description rdf:about="http://purl.org/olia/discourse/olia_discourse.owl#ProblemSolution_RST">
    <terms:replacedBy rdf:resource="http://purl.org/olia/olia.owl#ProblemSolution_RST"/>
  </rdf:Description>
  <rdf:Description rdf:about="http://purl.org/olia/discourse/olia_discourse.owl#ProblemSolution_RST">
    <owl:deprecated rdf:datatype="http://www.w3.org/2001/XMLSchema#boolean">true</owl:deprecated>
  </rdf:Description>
  <rdf:Description rdf:about="http://purl.org/olia/discourse/olia_discourse.owl#ProgrammingLanguage">
    <terms:replacedBy rdf:resource="http://purl.org/olia/olia.owl#ProgrammingLanguage"/>
  </rdf:Description>
  <rdf:Description rdf:about="http://purl.org/olia/discourse/olia_discourse.owl#ProgrammingLanguage">
    <owl:deprecated rdf:datatype="http://www.w3.org/2001/XMLSchema#boolean">true</owl:deprecated>
  </rdf:Description>
  <rdf:Description rdf:about="http://purl.org/olia/discourse/olia_discourse.owl#Proportion_RST">
    <terms:replacedBy rdf:resource="http://purl.org/olia/olia.owl#Proportion_RST"/>
  </rdf:Description>
  <rdf:Description rdf:about="http://purl.org/olia/discourse/olia_discourse.owl#Proportion_RST">
    <owl:deprecated rdf:datatype="http://www.w3.org/2001/XMLSchema#boolean">true</owl:deprecated>
  </rdf:Description>
  <rdf:Description rdf:about="http://purl.org/olia/discourse/olia_discourse.owl#Proposition">
    <terms:replacedBy rdf:resource="http://purl.org/olia/olia.owl#Proposition"/>
  </rdf:Description>
  <rdf:Description rdf:about="http://purl.org/olia/discourse/olia_discourse.owl#Proposition">
    <owl:deprecated rdf:datatype="http://www.w3.org/2001/XMLSchema#boolean">true</owl:deprecated>
  </rdf:Description>
  <rdf:Description rdf:about="http://purl.org/olia/discourse/olia_discourse.owl#PropositionalCause_HDRB">
    <terms:replacedBy rdf:resource="http://purl.org/olia/olia.owl#PropositionalCause_HDRB"/>
  </rdf:Description>
  <rdf:Description rdf:about="http://purl.org/olia/discourse/olia_discourse.owl#PropositionalCause_HDRB">
    <owl:deprecated rdf:datatype="http://www.w3.org/2001/XMLSchema#boolean">true</owl:deprecated>
  </rdf:Description>
  <rdf:Description rdf:about="http://purl.org/olia/discourse/olia_discourse.owl#PropositionalConcession_HDRB">
    <terms:replacedBy rdf:resource="http://purl.org/olia/olia.owl#PropositionalConcession_HDRB"/>
  </rdf:Description>
  <rdf:Description rdf:about="http://purl.org/olia/discourse/olia_discourse.owl#PropositionalConcession_HDRB">
    <owl:deprecated rdf:datatype="http://www.w3.org/2001/XMLSchema#boolean">true</owl:deprecated>
  </rdf:Description>
  <rdf:Description rdf:about="http://purl.org/olia/discourse/olia_discourse.owl#PropositionalCondition_HDRB">
    <terms:replacedBy rdf:resource="http://purl.org/olia/olia.owl#PropositionalCondition_HDRB"/>
  </rdf:Description>
  <rdf:Description rdf:about="http://purl.org/olia/discourse/olia_discourse.owl#PropositionalCondition_HDRB">
    <owl:deprecated rdf:datatype="http://www.w3.org/2001/XMLSchema#boolean">true</owl:deprecated>
  </rdf:Description>
  <rdf:Description rdf:about="http://purl.org/olia/discourse/olia_discourse.owl#PropositionalContrast_HDRB">
    <terms:replacedBy rdf:resource="http://purl.org/olia/olia.owl#PropositionalContrast_HDRB"/>
  </rdf:Description>
  <rdf:Description rdf:about="http://purl.org/olia/discourse/olia_discourse.owl#PropositionalContrast_HDRB">
    <owl:deprecated rdf:datatype="http://www.w3.org/2001/XMLSchema#boolean">true</owl:deprecated>
  </rdf:Description>
  <rdf:Description rdf:about="http://purl.org/olia/discourse/olia_discourse.owl#PropositionalFactuality">
    <terms:replacedBy rdf:resource="http://purl.org/olia/olia.owl#PropositionalFactuality"/>
  </rdf:Description>
  <rdf:Description rdf:about="http://purl.org/olia/discourse/olia_discourse.owl#PropositionalFactuality">
    <owl:deprecated rdf:datatype="http://www.w3.org/2001/XMLSchema#boolean">true</owl:deprecated>
  </rdf:Description>
  <rdf:Description rdf:about="http://purl.org/olia/discourse/olia_discourse.owl#Proverb">
    <terms:replacedBy rdf:resource="http://purl.org/olia/olia.owl#Proverb"/>
  </rdf:Description>
  <rdf:Description rdf:about="http://purl.org/olia/discourse/olia_discourse.owl#Proverb">
    <owl:deprecated rdf:datatype="http://www.w3.org/2001/XMLSchema#boolean">true</owl:deprecated>
  </rdf:Description>
  <rdf:Description rdf:about="http://purl.org/olia/discourse/olia_discourse.owl#Purpose_RST">
    <terms:replacedBy rdf:resource="http://purl.org/olia/olia.owl#Purpose_RST"/>
  </rdf:Description>
  <rdf:Description rdf:about="http://purl.org/olia/discourse/olia_discourse.owl#Purpose_RST">
    <owl:deprecated rdf:datatype="http://www.w3.org/2001/XMLSchema#boolean">true</owl:deprecated>
  </rdf:Description>
  <rdf:Description rdf:about="http://purl.org/olia/discourse/olia_discourse.owl#Purpose-s_SemDok">
    <terms:replacedBy rdf:resource="http://purl.org/olia/olia.owl#Purpose-s_SemDok"/>
  </rdf:Description>
  <rdf:Description rdf:about="http://purl.org/olia/discourse/olia_discourse.owl#Purpose-s_SemDok">
    <owl:deprecated rdf:datatype="http://www.w3.org/2001/XMLSchema#boolean">true</owl:deprecated>
  </rdf:Description>
  <rdf:Description rdf:about="http://purl.org/olia/discourse/olia_discourse.owl#QuestionAnswer_RST">
    <terms:replacedBy rdf:resource="http://purl.org/olia/olia.owl#QuestionAnswer_RST"/>
  </rdf:Description>
  <rdf:Description rdf:about="http://purl.org/olia/discourse/olia_discourse.owl#QuestionAnswer_RST">
    <owl:deprecated rdf:datatype="http://www.w3.org/2001/XMLSchema#boolean">true</owl:deprecated>
  </rdf:Description>
  <rdf:Description rdf:about="http://purl.org/olia/discourse/olia_discourse.owl#RadioProgram">
    <terms:replacedBy rdf:resource="http://purl.org/olia/olia.owl#RadioProgram"/>
  </rdf:Description>
  <rdf:Description rdf:about="http://purl.org/olia/discourse/olia_discourse.owl#RadioProgram">
    <owl:deprecated rdf:datatype="http://www.w3.org/2001/XMLSchema#boolean">true</owl:deprecated>
  </rdf:Description>
  <rdf:Description rdf:about="http://purl.org/olia/discourse/olia_discourse.owl#RadioStation">
    <terms:replacedBy rdf:resource="http://purl.org/olia/olia.owl#RadioStation"/>
  </rdf:Description>
  <rdf:Description rdf:about="http://purl.org/olia/discourse/olia_discourse.owl#RadioStation">
    <owl:deprecated rdf:datatype="http://www.w3.org/2001/XMLSchema#boolean">true</owl:deprecated>
  </rdf:Description>
  <rdf:Description rdf:about="http://purl.org/olia/discourse/olia_discourse.owl#RarelyUsed">
    <terms:replacedBy rdf:resource="http://purl.org/olia/olia.owl#RarelyUsed"/>
  </rdf:Description>
  <rdf:Description rdf:about="http://purl.org/olia/discourse/olia_discourse.owl#RarelyUsed">
    <owl:deprecated rdf:datatype="http://www.w3.org/2001/XMLSchema#boolean">true</owl:deprecated>
  </rdf:Description>
  <rdf:Description rdf:about="http://purl.org/olia/discourse/olia_discourse.owl#Reason">
    <terms:replacedBy rdf:resource="http://purl.org/olia/olia.owl#Reason"/>
  </rdf:Description>
  <rdf:Description rdf:about="http://purl.org/olia/discourse/olia_discourse.owl#Reason">
    <owl:deprecated rdf:datatype="http://www.w3.org/2001/XMLSchema#boolean">true</owl:deprecated>
  </rdf:Description>
  <rdf:Description rdf:about="http://purl.org/olia/discourse/olia_discourse.owl#Reason_RST">
    <terms:replacedBy rdf:resource="http://purl.org/olia/olia.owl#Reason_RST"/>
  </rdf:Description>
  <rdf:Description rdf:about="http://purl.org/olia/discourse/olia_discourse.owl#Reason_RST">
    <owl:deprecated rdf:datatype="http://www.w3.org/2001/XMLSchema#boolean">true</owl:deprecated>
  </rdf:Description>
  <rdf:Description rdf:about="http://purl.org/olia/discourse/olia_discourse.owl#Referentiality">
    <terms:replacedBy rdf:resource="http://purl.org/olia/olia.owl#Referentiality"/>
  </rdf:Description>
  <rdf:Description rdf:about="http://purl.org/olia/discourse/olia_discourse.owl#Referentiality">
    <owl:deprecated rdf:datatype="http://www.w3.org/2001/XMLSchema#boolean">true</owl:deprecated>
  </rdf:Description>
  <rdf:Description rdf:about="http://purl.org/olia/discourse/olia_discourse.owl#Referring">
    <terms:replacedBy rdf:resource="http://purl.org/olia/olia.owl#Referring"/>
  </rdf:Description>
  <rdf:Description rdf:about="http://purl.org/olia/discourse/olia_discourse.owl#Referring">
    <owl:deprecated rdf:datatype="http://www.w3.org/2001/XMLSchema#boolean">true</owl:deprecated>
  </rdf:Description>
  <rdf:Description rdf:about="http://purl.org/olia/discourse/olia_discourse.owl#ReferringExpression">
    <terms:replacedBy rdf:resource="http://purl.org/olia/olia.owl#ReferringExpression"/>
  </rdf:Description>
  <rdf:Description rdf:about="http://purl.org/olia/discourse/olia_discourse.owl#ReferringExpression">
    <owl:deprecated rdf:datatype="http://www.w3.org/2001/XMLSchema#boolean">true</owl:deprecated>
  </rdf:Description>
  <rdf:Description rdf:about="http://purl.org/olia/discourse/olia_discourse.owl#RelationCue">
    <terms:replacedBy rdf:resource="http://purl.org/olia/olia.owl#RelationCue"/>
  </rdf:Description>
  <rdf:Description rdf:about="http://purl.org/olia/discourse/olia_discourse.owl#RelationCue">
    <owl:deprecated rdf:datatype="http://www.w3.org/2001/XMLSchema#boolean">true</owl:deprecated>
  </rdf:Description>
  <rdf:Description rdf:about="http://purl.org/olia/discourse/olia_discourse.owl#RelevanceConditional_PDTB">
    <terms:replacedBy rdf:resource="http://purl.org/olia/olia.owl#RelevanceConditional_PDTB"/>
  </rdf:Description>
  <rdf:Description rdf:about="http://purl.org/olia/discourse/olia_discourse.owl#RelevanceConditional_PDTB">
    <owl:deprecated rdf:datatype="http://www.w3.org/2001/XMLSchema#boolean">true</owl:deprecated>
  </rdf:Description>
  <rdf:Description rdf:about="http://purl.org/olia/discourse/olia_discourse.owl#RequestForComment">
    <terms:replacedBy rdf:resource="http://purl.org/olia/olia.owl#RequestForComment"/>
  </rdf:Description>
  <rdf:Description rdf:about="http://purl.org/olia/discourse/olia_discourse.owl#RequestForComment">
    <owl:deprecated rdf:datatype="http://www.w3.org/2001/XMLSchema#boolean">true</owl:deprecated>
  </rdf:Description>
  <rdf:Description rdf:about="http://purl.org/olia/discourse/olia_discourse.owl#ResponseAct">
    <terms:replacedBy rdf:resource="http://purl.org/olia/olia.owl#ResponseAct"/>
  </rdf:Description>
  <rdf:Description rdf:about="http://purl.org/olia/discourse/olia_discourse.owl#ResponseAct">
    <owl:deprecated rdf:datatype="http://www.w3.org/2001/XMLSchema#boolean">true</owl:deprecated>
  </rdf:Description>
  <rdf:Description rdf:about="http://purl.org/olia/discourse/olia_discourse.owl#Restatement">
    <terms:replacedBy rdf:resource="http://purl.org/olia/olia.owl#Restatement"/>
  </rdf:Description>
  <rdf:Description rdf:about="http://purl.org/olia/discourse/olia_discourse.owl#Restatement">
    <owl:deprecated rdf:datatype="http://www.w3.org/2001/XMLSchema#boolean">true</owl:deprecated>
  </rdf:Description>
  <rdf:Description rdf:about="http://purl.org/olia/discourse/olia_discourse.owl#Restaurant">
    <terms:replacedBy rdf:resource="http://purl.org/olia/olia.owl#Restaurant"/>
  </rdf:Description>
  <rdf:Description rdf:about="http://purl.org/olia/discourse/olia_discourse.owl#Restaurant">
    <owl:deprecated rdf:datatype="http://www.w3.org/2001/XMLSchema#boolean">true</owl:deprecated>
  </rdf:Description>
  <rdf:Description rdf:about="http://purl.org/olia/discourse/olia_discourse.owl#Result">
    <terms:replacedBy rdf:resource="http://purl.org/olia/olia.owl#Result"/>
  </rdf:Description>
  <rdf:Description rdf:about="http://purl.org/olia/discourse/olia_discourse.owl#Result">
    <owl:deprecated rdf:datatype="http://www.w3.org/2001/XMLSchema#boolean">true</owl:deprecated>
  </rdf:Description>
  <rdf:Description rdf:about="http://purl.org/olia/discourse/olia_discourse.owl#Result_RST">
    <terms:replacedBy rdf:resource="http://purl.org/olia/olia.owl#Result_RST"/>
  </rdf:Description>
  <rdf:Description rdf:about="http://purl.org/olia/discourse/olia_discourse.owl#Result_RST">
    <owl:deprecated rdf:datatype="http://www.w3.org/2001/XMLSchema#boolean">true</owl:deprecated>
  </rdf:Description>
  <rdf:Description rdf:about="http://purl.org/olia/discourse/olia_discourse.owl#RhetoricalQuestion_RST">
    <terms:replacedBy rdf:resource="http://purl.org/olia/olia.owl#RhetoricalQuestion_RST"/>
  </rdf:Description>
  <rdf:Description rdf:about="http://purl.org/olia/discourse/olia_discourse.owl#RhetoricalQuestion_RST">
    <owl:deprecated rdf:datatype="http://www.w3.org/2001/XMLSchema#boolean">true</owl:deprecated>
  </rdf:Description>
  <rdf:Description rdf:about="http://purl.org/olia/discourse/olia_discourse.owl#River">
    <terms:replacedBy rdf:resource="http://purl.org/olia/olia.owl#River"/>
  </rdf:Description>
  <rdf:Description rdf:about="http://purl.org/olia/discourse/olia_discourse.owl#River">
    <owl:deprecated rdf:datatype="http://www.w3.org/2001/XMLSchema#boolean">true</owl:deprecated>
  </rdf:Description>
  <rdf:Description rdf:about="http://purl.org/olia/discourse/olia_discourse.owl#Road">
    <terms:replacedBy rdf:resource="http://purl.org/olia/olia.owl#Road"/>
  </rdf:Description>
  <rdf:Description rdf:about="http://purl.org/olia/discourse/olia_discourse.owl#Road">
    <owl:deprecated rdf:datatype="http://www.w3.org/2001/XMLSchema#boolean">true</owl:deprecated>
  </rdf:Description>
  <rdf:Description rdf:about="http://purl.org/olia/discourse/olia_discourse.owl#SameType">
    <terms:replacedBy rdf:resource="http://purl.org/olia/olia.owl#SameType"/>
  </rdf:Description>
  <rdf:Description rdf:about="http://purl.org/olia/discourse/olia_discourse.owl#SameType">
    <owl:deprecated rdf:datatype="http://www.w3.org/2001/XMLSchema#boolean">true</owl:deprecated>
  </rdf:Description>
  <rdf:Description rdf:about="http://purl.org/olia/discourse/olia_discourse.owl#SameUnit_RST">
    <terms:replacedBy rdf:resource="http://purl.org/olia/olia.owl#SameUnit_RST"/>
  </rdf:Description>
  <rdf:Description rdf:about="http://purl.org/olia/discourse/olia_discourse.owl#SameUnit_RST">
    <owl:deprecated rdf:datatype="http://www.w3.org/2001/XMLSchema#boolean">true</owl:deprecated>
  </rdf:Description>
  <rdf:Description rdf:about="http://purl.org/olia/discourse/olia_discourse.owl#SchoolNewspaper">
    <terms:replacedBy rdf:resource="http://purl.org/olia/olia.owl#SchoolNewspaper"/>
  </rdf:Description>
  <rdf:Description rdf:about="http://purl.org/olia/discourse/olia_discourse.owl#SchoolNewspaper">
    <owl:deprecated rdf:datatype="http://www.w3.org/2001/XMLSchema#boolean">true</owl:deprecated>
  </rdf:Description>
  <rdf:Description rdf:about="http://purl.org/olia/discourse/olia_discourse.owl#SectionText">
    <terms:replacedBy rdf:resource="http://purl.org/olia/olia.owl#SectionText"/>
  </rdf:Description>
  <rdf:Description rdf:about="http://purl.org/olia/discourse/olia_discourse.owl#SectionText">
    <owl:deprecated rdf:datatype="http://www.w3.org/2001/XMLSchema#boolean">true</owl:deprecated>
  </rdf:Description>
  <rdf:Description rdf:about="http://purl.org/olia/discourse/olia_discourse.owl#SectionTitle">
    <terms:replacedBy rdf:resource="http://purl.org/olia/olia.owl#SectionTitle"/>
  </rdf:Description>
  <rdf:Description rdf:about="http://purl.org/olia/discourse/olia_discourse.owl#SectionTitle">
    <owl:deprecated rdf:datatype="http://www.w3.org/2001/XMLSchema#boolean">true</owl:deprecated>
  </rdf:Description>
  <rdf:Description rdf:about="http://purl.org/olia/discourse/olia_discourse.owl#SemanticAlternative_LUNA">
    <terms:replacedBy rdf:resource="http://purl.org/olia/olia.owl#SemanticAlternative_LUNA"/>
  </rdf:Description>
  <rdf:Description rdf:about="http://purl.org/olia/discourse/olia_discourse.owl#SemanticAlternative_LUNA">
    <owl:deprecated rdf:datatype="http://www.w3.org/2001/XMLSchema#boolean">true</owl:deprecated>
  </rdf:Description>
  <rdf:Description rdf:about="http://purl.org/olia/discourse/olia_discourse.owl#SemanticCause">
    <terms:replacedBy rdf:resource="http://purl.org/olia/olia.owl#SemanticCause"/>
  </rdf:Description>
  <rdf:Description rdf:about="http://purl.org/olia/discourse/olia_discourse.owl#SemanticCause">
    <owl:deprecated rdf:datatype="http://www.w3.org/2001/XMLSchema#boolean">true</owl:deprecated>
  </rdf:Description>
  <rdf:Description rdf:about="http://purl.org/olia/discourse/olia_discourse.owl#SemanticConcession_HDRB">
    <terms:replacedBy rdf:resource="http://purl.org/olia/olia.owl#SemanticConcession_HDRB"/>
  </rdf:Description>
  <rdf:Description rdf:about="http://purl.org/olia/discourse/olia_discourse.owl#SemanticConcession_HDRB">
    <owl:deprecated rdf:datatype="http://www.w3.org/2001/XMLSchema#boolean">true</owl:deprecated>
  </rdf:Description>
  <rdf:Description rdf:about="http://purl.org/olia/discourse/olia_discourse.owl#SemanticCondition">
    <terms:replacedBy rdf:resource="http://purl.org/olia/olia.owl#SemanticCondition"/>
  </rdf:Description>
  <rdf:Description rdf:about="http://purl.org/olia/discourse/olia_discourse.owl#SemanticCondition">
    <owl:deprecated rdf:datatype="http://www.w3.org/2001/XMLSchema#boolean">true</owl:deprecated>
  </rdf:Description>
  <rdf:Description rdf:about="http://purl.org/olia/discourse/olia_discourse.owl#SemanticConjunction_LUNA">
    <terms:replacedBy rdf:resource="http://purl.org/olia/olia.owl#SemanticConjunction_LUNA"/>
  </rdf:Description>
  <rdf:Description rdf:about="http://purl.org/olia/discourse/olia_discourse.owl#SemanticConjunction_LUNA">
    <owl:deprecated rdf:datatype="http://www.w3.org/2001/XMLSchema#boolean">true</owl:deprecated>
  </rdf:Description>
  <rdf:Description rdf:about="http://purl.org/olia/discourse/olia_discourse.owl#SemanticContrast_PDTB">
    <terms:replacedBy rdf:resource="http://purl.org/olia/olia.owl#SemanticContrast_PDTB"/>
  </rdf:Description>
  <rdf:Description rdf:about="http://purl.org/olia/discourse/olia_discourse.owl#SemanticContrast_PDTB">
    <owl:deprecated rdf:datatype="http://www.w3.org/2001/XMLSchema#boolean">true</owl:deprecated>
  </rdf:Description>
  <rdf:Description rdf:about="http://purl.org/olia/discourse/olia_discourse.owl#SemanticFeature">
    <terms:replacedBy rdf:resource="http://purl.org/olia/olia.owl#SemanticFeature"/>
  </rdf:Description>
  <rdf:Description rdf:about="http://purl.org/olia/discourse/olia_discourse.owl#SemanticFeature">
    <owl:deprecated rdf:datatype="http://www.w3.org/2001/XMLSchema#boolean">true</owl:deprecated>
  </rdf:Description>
  <rdf:Description rdf:about="http://purl.org/olia/discourse/olia_discourse.owl#SemanticGoal_LUNA">
    <terms:replacedBy rdf:resource="http://purl.org/olia/olia.owl#SemanticGoal_LUNA"/>
  </rdf:Description>
  <rdf:Description rdf:about="http://purl.org/olia/discourse/olia_discourse.owl#SemanticGoal_LUNA">
    <owl:deprecated rdf:datatype="http://www.w3.org/2001/XMLSchema#boolean">true</owl:deprecated>
  </rdf:Description>
  <rdf:Description rdf:about="http://purl.org/olia/discourse/olia_discourse.owl#Sentence">
    <terms:replacedBy rdf:resource="http://purl.org/olia/olia.owl#Sentence"/>
  </rdf:Description>
  <rdf:Description rdf:about="http://purl.org/olia/discourse/olia_discourse.owl#Sentence">
    <owl:deprecated rdf:datatype="http://www.w3.org/2001/XMLSchema#boolean">true</owl:deprecated>
  </rdf:Description>
  <rdf:Description rdf:about="http://purl.org/olia/discourse/olia_discourse.owl#SentenceFocus">
    <terms:replacedBy rdf:resource="http://purl.org/olia/olia.owl#SentenceFocus"/>
  </rdf:Description>
  <rdf:Description rdf:about="http://purl.org/olia/discourse/olia_discourse.owl#SentenceFocus">
    <owl:deprecated rdf:datatype="http://www.w3.org/2001/XMLSchema#boolean">true</owl:deprecated>
  </rdf:Description>
  <rdf:Description rdf:about="http://purl.org/olia/discourse/olia_discourse.owl#SententialDiscourseSegment">
    <terms:replacedBy rdf:resource="http://purl.org/olia/olia.owl#SententialDiscourseSegment"/>
  </rdf:Description>
  <rdf:Description rdf:about="http://purl.org/olia/discourse/olia_discourse.owl#SententialDiscourseSegment">
    <owl:deprecated rdf:datatype="http://www.w3.org/2001/XMLSchema#boolean">true</owl:deprecated>
  </rdf:Description>
  <rdf:Description rdf:about="http://purl.org/olia/discourse/olia_discourse.owl#Sequence">
    <terms:replacedBy rdf:resource="http://purl.org/olia/olia.owl#Sequence"/>
  </rdf:Description>
  <rdf:Description rdf:about="http://purl.org/olia/discourse/olia_discourse.owl#Sequence">
    <owl:deprecated rdf:datatype="http://www.w3.org/2001/XMLSchema#boolean">true</owl:deprecated>
  </rdf:Description>
  <rdf:Description rdf:about="http://purl.org/olia/discourse/olia_discourse.owl#Set">
    <terms:replacedBy rdf:resource="http://purl.org/olia/olia.owl#Set"/>
  </rdf:Description>
  <rdf:Description rdf:about="http://purl.org/olia/discourse/olia_discourse.owl#Set">
    <owl:deprecated rdf:datatype="http://www.w3.org/2001/XMLSchema#boolean">true</owl:deprecated>
  </rdf:Description>
  <rdf:Description rdf:about="http://purl.org/olia/discourse/olia_discourse.owl#ShoppingMall">
    <terms:replacedBy rdf:resource="http://purl.org/olia/olia.owl#ShoppingMall"/>
  </rdf:Description>
  <rdf:Description rdf:about="http://purl.org/olia/discourse/olia_discourse.owl#ShoppingMall">
    <owl:deprecated rdf:datatype="http://www.w3.org/2001/XMLSchema#boolean">true</owl:deprecated>
  </rdf:Description>
  <rdf:Description rdf:about="http://purl.org/olia/discourse/olia_discourse.owl#SignatureBlock">
    <terms:replacedBy rdf:resource="http://purl.org/olia/olia.owl#SignatureBlock"/>
  </rdf:Description>
  <rdf:Description rdf:about="http://purl.org/olia/discourse/olia_discourse.owl#SignatureBlock">
    <owl:deprecated rdf:datatype="http://www.w3.org/2001/XMLSchema#boolean">true</owl:deprecated>
  </rdf:Description>
  <rdf:Description rdf:about="http://purl.org/olia/discourse/olia_discourse.owl#Similarity">
    <terms:replacedBy rdf:resource="http://purl.org/olia/olia.owl#Similarity"/>
  </rdf:Description>
  <rdf:Description rdf:about="http://purl.org/olia/discourse/olia_discourse.owl#Similarity">
    <owl:deprecated rdf:datatype="http://www.w3.org/2001/XMLSchema#boolean">true</owl:deprecated>
  </rdf:Description>
  <rdf:Description rdf:about="http://purl.org/olia/discourse/olia_discourse.owl#SituationallyAccessible">
    <terms:replacedBy rdf:resource="http://purl.org/olia/olia.owl#SituationallyAccessible"/>
  </rdf:Description>
  <rdf:Description rdf:about="http://purl.org/olia/discourse/olia_discourse.owl#SituationallyAccessible">
    <owl:deprecated rdf:datatype="http://www.w3.org/2001/XMLSchema#boolean">true</owl:deprecated>
  </rdf:Description>
  <rdf:Description rdf:about="http://purl.org/olia/discourse/olia_discourse.owl#SlangRegister">
    <terms:replacedBy rdf:resource="http://purl.org/olia/olia.owl#SlangRegister"/>
  </rdf:Description>
  <rdf:Description rdf:about="http://purl.org/olia/discourse/olia_discourse.owl#SlangRegister">
    <owl:deprecated rdf:datatype="http://www.w3.org/2001/XMLSchema#boolean">true</owl:deprecated>
  </rdf:Description>
  <rdf:Description rdf:about="http://purl.org/olia/discourse/olia_discourse.owl#SoccerClub">
    <terms:replacedBy rdf:resource="http://purl.org/olia/olia.owl#SoccerClub"/>
  </rdf:Description>
  <rdf:Description rdf:about="http://purl.org/olia/discourse/olia_discourse.owl#SoccerClub">
    <owl:deprecated rdf:datatype="http://www.w3.org/2001/XMLSchema#boolean">true</owl:deprecated>
  </rdf:Description>
  <rdf:Description rdf:about="http://purl.org/olia/discourse/olia_discourse.owl#SoccerPlayer">
    <terms:replacedBy rdf:resource="http://purl.org/olia/olia.owl#SoccerPlayer"/>
  </rdf:Description>
  <rdf:Description rdf:about="http://purl.org/olia/discourse/olia_discourse.owl#SoccerPlayer">
    <owl:deprecated rdf:datatype="http://www.w3.org/2001/XMLSchema#boolean">true</owl:deprecated>
  </rdf:Description>
  <rdf:Description rdf:about="http://purl.org/olia/discourse/olia_discourse.owl#Software">
    <terms:replacedBy rdf:resource="http://purl.org/olia/olia.owl#Software"/>
  </rdf:Description>
  <rdf:Description rdf:about="http://purl.org/olia/discourse/olia_discourse.owl#Software">
    <owl:deprecated rdf:datatype="http://www.w3.org/2001/XMLSchema#boolean">true</owl:deprecated>
  </rdf:Description>
  <rdf:Description rdf:about="http://purl.org/olia/discourse/olia_discourse.owl#SolicitedResponse">
    <terms:replacedBy rdf:resource="http://purl.org/olia/olia.owl#SolicitedResponse"/>
  </rdf:Description>
  <rdf:Description rdf:about="http://purl.org/olia/discourse/olia_discourse.owl#SolicitedResponse">
    <owl:deprecated rdf:datatype="http://www.w3.org/2001/XMLSchema#boolean">true</owl:deprecated>
  </rdf:Description>
  <rdf:Description rdf:about="http://purl.org/olia/discourse/olia_discourse.owl#Song">
    <terms:replacedBy rdf:resource="http://purl.org/olia/olia.owl#Song"/>
  </rdf:Description>
  <rdf:Description rdf:about="http://purl.org/olia/discourse/olia_discourse.owl#Song">
    <owl:deprecated rdf:datatype="http://www.w3.org/2001/XMLSchema#boolean">true</owl:deprecated>
  </rdf:Description>
  <rdf:Description rdf:about="http://purl.org/olia/discourse/olia_discourse.owl#Source">
    <terms:replacedBy rdf:resource="http://purl.org/olia/olia.owl#Source"/>
  </rdf:Description>
  <rdf:Description rdf:about="http://purl.org/olia/discourse/olia_discourse.owl#Source">
    <owl:deprecated rdf:datatype="http://www.w3.org/2001/XMLSchema#boolean">true</owl:deprecated>
  </rdf:Description>
  <rdf:Description rdf:about="http://purl.org/olia/discourse/olia_discourse.owl#Space">
    <terms:replacedBy rdf:resource="http://purl.org/olia/olia.owl#Space"/>
  </rdf:Description>
  <rdf:Description rdf:about="http://purl.org/olia/discourse/olia_discourse.owl#Space">
    <owl:deprecated rdf:datatype="http://www.w3.org/2001/XMLSchema#boolean">true</owl:deprecated>
  </rdf:Description>
  <rdf:Description rdf:about="http://purl.org/olia/discourse/olia_discourse.owl#Spacecraft">
    <terms:replacedBy rdf:resource="http://purl.org/olia/olia.owl#Spacecraft"/>
  </rdf:Description>
  <rdf:Description rdf:about="http://purl.org/olia/discourse/olia_discourse.owl#Spacecraft">
    <owl:deprecated rdf:datatype="http://www.w3.org/2001/XMLSchema#boolean">true</owl:deprecated>
  </rdf:Description>
  <rdf:Description rdf:about="http://purl.org/olia/discourse/olia_discourse.owl#SpecializedRestatement_PDTB">
    <terms:replacedBy rdf:resource="http://purl.org/olia/olia.owl#SpecializedRestatement_PDTB"/>
  </rdf:Description>
  <rdf:Description rdf:about="http://purl.org/olia/discourse/olia_discourse.owl#SpecializedRestatement_PDTB">
    <owl:deprecated rdf:datatype="http://www.w3.org/2001/XMLSchema#boolean">true</owl:deprecated>
  </rdf:Description>
  <rdf:Description rdf:about="http://purl.org/olia/discourse/olia_discourse.owl#Specification">
    <terms:replacedBy rdf:resource="http://purl.org/olia/olia.owl#Specification"/>
  </rdf:Description>
  <rdf:Description rdf:about="http://purl.org/olia/discourse/olia_discourse.owl#Specification">
    <owl:deprecated rdf:datatype="http://www.w3.org/2001/XMLSchema#boolean">true</owl:deprecated>
  </rdf:Description>
  <rdf:Description rdf:about="http://purl.org/olia/discourse/olia_discourse.owl#SpeechActAlternative_LUNA">
    <terms:replacedBy rdf:resource="http://purl.org/olia/olia.owl#SpeechActAlternative_LUNA"/>
  </rdf:Description>
  <rdf:Description rdf:about="http://purl.org/olia/discourse/olia_discourse.owl#SpeechActAlternative_LUNA">
    <owl:deprecated rdf:datatype="http://www.w3.org/2001/XMLSchema#boolean">true</owl:deprecated>
  </rdf:Description>
  <rdf:Description rdf:about="http://purl.org/olia/discourse/olia_discourse.owl#SpeechActCause_HDRB">
    <terms:replacedBy rdf:resource="http://purl.org/olia/olia.owl#SpeechActCause_HDRB"/>
  </rdf:Description>
  <rdf:Description rdf:about="http://purl.org/olia/discourse/olia_discourse.owl#SpeechActCause_HDRB">
    <owl:deprecated rdf:datatype="http://www.w3.org/2001/XMLSchema#boolean">true</owl:deprecated>
  </rdf:Description>
  <rdf:Description rdf:about="http://purl.org/olia/discourse/olia_discourse.owl#SpeechActConcession_HDRB">
    <terms:replacedBy rdf:resource="http://purl.org/olia/olia.owl#SpeechActConcession_HDRB"/>
  </rdf:Description>
  <rdf:Description rdf:about="http://purl.org/olia/discourse/olia_discourse.owl#SpeechActConcession_HDRB">
    <owl:deprecated rdf:datatype="http://www.w3.org/2001/XMLSchema#boolean">true</owl:deprecated>
  </rdf:Description>
  <rdf:Description rdf:about="http://purl.org/olia/discourse/olia_discourse.owl#SpeechActCondition_HDRB">
    <terms:replacedBy rdf:resource="http://purl.org/olia/olia.owl#SpeechActCondition_HDRB"/>
  </rdf:Description>
  <rdf:Description rdf:about="http://purl.org/olia/discourse/olia_discourse.owl#SpeechActCondition_HDRB">
    <owl:deprecated rdf:datatype="http://www.w3.org/2001/XMLSchema#boolean">true</owl:deprecated>
  </rdf:Description>
  <rdf:Description rdf:about="http://purl.org/olia/discourse/olia_discourse.owl#SpeechActConjunction_LUNA">
    <terms:replacedBy rdf:resource="http://purl.org/olia/olia.owl#SpeechActConjunction_LUNA"/>
  </rdf:Description>
  <rdf:Description rdf:about="http://purl.org/olia/discourse/olia_discourse.owl#SpeechActConjunction_LUNA">
    <owl:deprecated rdf:datatype="http://www.w3.org/2001/XMLSchema#boolean">true</owl:deprecated>
  </rdf:Description>
  <rdf:Description rdf:about="http://purl.org/olia/discourse/olia_discourse.owl#SpeechActContrast_HDRB">
    <terms:replacedBy rdf:resource="http://purl.org/olia/olia.owl#SpeechActContrast_HDRB"/>
  </rdf:Description>
  <rdf:Description rdf:about="http://purl.org/olia/discourse/olia_discourse.owl#SpeechActContrast_HDRB">
    <owl:deprecated rdf:datatype="http://www.w3.org/2001/XMLSchema#boolean">true</owl:deprecated>
  </rdf:Description>
  <rdf:Description rdf:about="http://purl.org/olia/discourse/olia_discourse.owl#SpeechActGoal_LUNA">
    <terms:replacedBy rdf:resource="http://purl.org/olia/olia.owl#SpeechActGoal_LUNA"/>
  </rdf:Description>
  <rdf:Description rdf:about="http://purl.org/olia/discourse/olia_discourse.owl#SpeechActGoal_LUNA">
    <owl:deprecated rdf:datatype="http://www.w3.org/2001/XMLSchema#boolean">true</owl:deprecated>
  </rdf:Description>
  <rdf:Description rdf:about="http://purl.org/olia/discourse/olia_discourse.owl#SportsEvent">
    <terms:replacedBy rdf:resource="http://purl.org/olia/olia.owl#SportsEvent"/>
  </rdf:Description>
  <rdf:Description rdf:about="http://purl.org/olia/discourse/olia_discourse.owl#SportsEvent">
    <owl:deprecated rdf:datatype="http://www.w3.org/2001/XMLSchema#boolean">true</owl:deprecated>
  </rdf:Description>
  <rdf:Description rdf:about="http://purl.org/olia/discourse/olia_discourse.owl#SportsLeague">
    <terms:replacedBy rdf:resource="http://purl.org/olia/olia.owl#SportsLeague"/>
  </rdf:Description>
  <rdf:Description rdf:about="http://purl.org/olia/discourse/olia_discourse.owl#SportsLeague">
    <owl:deprecated rdf:datatype="http://www.w3.org/2001/XMLSchema#boolean">true</owl:deprecated>
  </rdf:Description>
  <rdf:Description rdf:about="http://purl.org/olia/discourse/olia_discourse.owl#SportsOrganization">
    <terms:replacedBy rdf:resource="http://purl.org/olia/olia.owl#SportsOrganization"/>
  </rdf:Description>
  <rdf:Description rdf:about="http://purl.org/olia/discourse/olia_discourse.owl#SportsOrganization">
    <owl:deprecated rdf:datatype="http://www.w3.org/2001/XMLSchema#boolean">true</owl:deprecated>
  </rdf:Description>
  <rdf:Description rdf:about="http://purl.org/olia/discourse/olia_discourse.owl#SportsTeam">
    <terms:replacedBy rdf:resource="http://purl.org/olia/olia.owl#SportsTeam"/>
  </rdf:Description>
  <rdf:Description rdf:about="http://purl.org/olia/discourse/olia_discourse.owl#SportsTeam">
    <owl:deprecated rdf:datatype="http://www.w3.org/2001/XMLSchema#boolean">true</owl:deprecated>
  </rdf:Description>
  <rdf:Description rdf:about="http://purl.org/olia/discourse/olia_discourse.owl#Stadium">
    <terms:replacedBy rdf:resource="http://purl.org/olia/olia.owl#Stadium"/>
  </rdf:Description>
  <rdf:Description rdf:about="http://purl.org/olia/discourse/olia_discourse.owl#Stadium">
    <owl:deprecated rdf:datatype="http://www.w3.org/2001/XMLSchema#boolean">true</owl:deprecated>
  </rdf:Description>
  <rdf:Description rdf:about="http://purl.org/olia/discourse/olia_discourse.owl#Standardized">
    <terms:replacedBy rdf:resource="http://purl.org/olia/olia.owl#Standardized"/>
  </rdf:Description>
  <rdf:Description rdf:about="http://purl.org/olia/discourse/olia_discourse.owl#Standardized">
    <owl:deprecated rdf:datatype="http://www.w3.org/2001/XMLSchema#boolean">true</owl:deprecated>
  </rdf:Description>
  <rdf:Description rdf:about="http://purl.org/olia/discourse/olia_discourse.owl#StatementResponse_RST">
    <terms:replacedBy rdf:resource="http://purl.org/olia/olia.owl#StatementResponse_RST"/>
  </rdf:Description>
  <rdf:Description rdf:about="http://purl.org/olia/discourse/olia_discourse.owl#StatementResponse_RST">
    <owl:deprecated rdf:datatype="http://www.w3.org/2001/XMLSchema#boolean">true</owl:deprecated>
  </rdf:Description>
  <rdf:Description rdf:about="http://purl.org/olia/discourse/olia_discourse.owl#StateOfAffairFocus">
    <terms:replacedBy rdf:resource="http://purl.org/olia/olia.owl#StateOfAffairFocus"/>
  </rdf:Description>
  <rdf:Description rdf:about="http://purl.org/olia/discourse/olia_discourse.owl#StateOfAffairFocus">
    <owl:deprecated rdf:datatype="http://www.w3.org/2001/XMLSchema#boolean">true</owl:deprecated>
  </rdf:Description>
  <rdf:Description rdf:about="http://purl.org/olia/discourse/olia_discourse.owl#Station">
    <terms:replacedBy rdf:resource="http://purl.org/olia/olia.owl#Station"/>
  </rdf:Description>
  <rdf:Description rdf:about="http://purl.org/olia/discourse/olia_discourse.owl#Station">
    <owl:deprecated rdf:datatype="http://www.w3.org/2001/XMLSchema#boolean">true</owl:deprecated>
  </rdf:Description>
  <rdf:Description rdf:about="http://purl.org/olia/discourse/olia_discourse.owl#StructuralConnective">
    <terms:replacedBy rdf:resource="http://purl.org/olia/olia.owl#StructuralConnective"/>
  </rdf:Description>
  <rdf:Description rdf:about="http://purl.org/olia/discourse/olia_discourse.owl#StructuralConnective">
    <owl:deprecated rdf:datatype="http://www.w3.org/2001/XMLSchema#boolean">true</owl:deprecated>
  </rdf:Description>
  <rdf:Description rdf:about="http://purl.org/olia/discourse/olia_discourse.owl#StructuralFocusType">
    <terms:replacedBy rdf:resource="http://purl.org/olia/olia.owl#StructuralFocusType"/>
  </rdf:Description>
  <rdf:Description rdf:about="http://purl.org/olia/discourse/olia_discourse.owl#StructuralFocusType">
    <owl:deprecated rdf:datatype="http://www.w3.org/2001/XMLSchema#boolean">true</owl:deprecated>
  </rdf:Description>
  <rdf:Description rdf:about="http://purl.org/olia/discourse/olia_discourse.owl#SubjectFocus">
    <terms:replacedBy rdf:resource="http://purl.org/olia/olia.owl#SubjectFocus"/>
  </rdf:Description>
  <rdf:Description rdf:about="http://purl.org/olia/discourse/olia_discourse.owl#SubjectFocus">
    <owl:deprecated rdf:datatype="http://www.w3.org/2001/XMLSchema#boolean">true</owl:deprecated>
  </rdf:Description>
  <rdf:Description rdf:about="http://purl.org/olia/discourse/olia_discourse.owl#SubjectMatterRelation">
    <terms:replacedBy rdf:resource="http://purl.org/olia/olia.owl#SubjectMatterRelation"/>
  </rdf:Description>
  <rdf:Description rdf:about="http://purl.org/olia/discourse/olia_discourse.owl#SubjectMatterRelation">
    <owl:deprecated rdf:datatype="http://www.w3.org/2001/XMLSchema#boolean">true</owl:deprecated>
  </rdf:Description>
  <rdf:Description rdf:about="http://purl.org/olia/discourse/olia_discourse.owl#SubSetOf">
    <terms:replacedBy rdf:resource="http://purl.org/olia/olia.owl#SubSetOf"/>
  </rdf:Description>
  <rdf:Description rdf:about="http://purl.org/olia/discourse/olia_discourse.owl#SubSetOf">
    <owl:deprecated rdf:datatype="http://www.w3.org/2001/XMLSchema#boolean">true</owl:deprecated>
  </rdf:Description>
  <rdf:Description rdf:about="http://purl.org/olia/discourse/olia_discourse.owl#SuccessionRelation">
    <terms:replacedBy rdf:resource="http://purl.org/olia/olia.owl#SuccessionRelation"/>
  </rdf:Description>
  <rdf:Description rdf:about="http://purl.org/olia/discourse/olia_discourse.owl#SuccessionRelation">
    <owl:deprecated rdf:datatype="http://www.w3.org/2001/XMLSchema#boolean">true</owl:deprecated>
  </rdf:Description>
  <rdf:Description rdf:about="http://purl.org/olia/discourse/olia_discourse.owl#Summary">
    <terms:replacedBy rdf:resource="http://purl.org/olia/olia.owl#Summary"/>
  </rdf:Description>
  <rdf:Description rdf:about="http://purl.org/olia/discourse/olia_discourse.owl#Summary">
    <owl:deprecated rdf:datatype="http://www.w3.org/2001/XMLSchema#boolean">true</owl:deprecated>
  </rdf:Description>
  <rdf:Description rdf:about="http://purl.org/olia/discourse/olia_discourse.owl#Summary_RST">
    <terms:replacedBy rdf:resource="http://purl.org/olia/olia.owl#Summary_RST"/>
  </rdf:Description>
  <rdf:Description rdf:about="http://purl.org/olia/discourse/olia_discourse.owl#Summary_RST">
    <owl:deprecated rdf:datatype="http://www.w3.org/2001/XMLSchema#boolean">true</owl:deprecated>
  </rdf:Description>
  <rdf:Description rdf:about="http://purl.org/olia/discourse/olia_discourse.owl#Support">
    <terms:replacedBy rdf:resource="http://purl.org/olia/olia.owl#Support"/>
  </rdf:Description>
  <rdf:Description rdf:about="http://purl.org/olia/discourse/olia_discourse.owl#Support">
    <owl:deprecated rdf:datatype="http://www.w3.org/2001/XMLSchema#boolean">true</owl:deprecated>
  </rdf:Description>
  <rdf:Description rdf:about="http://purl.org/olia/discourse/olia_discourse.owl#SynchronousRelation">
    <terms:replacedBy rdf:resource="http://purl.org/olia/olia.owl#SynchronousRelation"/>
  </rdf:Description>
  <rdf:Description rdf:about="http://purl.org/olia/discourse/olia_discourse.owl#SynchronousRelation">
    <owl:deprecated rdf:datatype="http://www.w3.org/2001/XMLSchema#boolean">true</owl:deprecated>
  </rdf:Description>
  <rdf:Description rdf:about="http://purl.org/olia/discourse/olia_discourse.owl#TabooRegister">
    <terms:replacedBy rdf:resource="http://purl.org/olia/olia.owl#TabooRegister"/>
  </rdf:Description>
  <rdf:Description rdf:about="http://purl.org/olia/discourse/olia_discourse.owl#TabooRegister">
    <owl:deprecated rdf:datatype="http://www.w3.org/2001/XMLSchema#boolean">true</owl:deprecated>
  </rdf:Description>
  <rdf:Description rdf:about="http://purl.org/olia/discourse/olia_discourse.owl#TAMFocus">
    <terms:replacedBy rdf:resource="http://purl.org/olia/olia.owl#TAMFocus"/>
  </rdf:Description>
  <rdf:Description rdf:about="http://purl.org/olia/discourse/olia_discourse.owl#TAMFocus">
    <owl:deprecated rdf:datatype="http://www.w3.org/2001/XMLSchema#boolean">true</owl:deprecated>
  </rdf:Description>
  <rdf:Description rdf:about="http://purl.org/olia/discourse/olia_discourse.owl#TechnicalRegister">
    <terms:replacedBy rdf:resource="http://purl.org/olia/olia.owl#TechnicalRegister"/>
  </rdf:Description>
  <rdf:Description rdf:about="http://purl.org/olia/discourse/olia_discourse.owl#TechnicalRegister">
    <owl:deprecated rdf:datatype="http://www.w3.org/2001/XMLSchema#boolean">true</owl:deprecated>
  </rdf:Description>
  <rdf:Description rdf:about="http://purl.org/olia/discourse/olia_discourse.owl#TemporalAfter">
    <terms:replacedBy rdf:resource="http://purl.org/olia/olia.owl#TemporalAfter"/>
  </rdf:Description>
  <rdf:Description rdf:about="http://purl.org/olia/discourse/olia_discourse.owl#TemporalAfter">
    <owl:deprecated rdf:datatype="http://www.w3.org/2001/XMLSchema#boolean">true</owl:deprecated>
  </rdf:Description>
  <rdf:Description rdf:about="http://purl.org/olia/discourse/olia_discourse.owl#TemporalBefore">
    <terms:replacedBy rdf:resource="http://purl.org/olia/olia.owl#TemporalBefore"/>
  </rdf:Description>
  <rdf:Description rdf:about="http://purl.org/olia/discourse/olia_discourse.owl#TemporalBefore">
    <owl:deprecated rdf:datatype="http://www.w3.org/2001/XMLSchema#boolean">true</owl:deprecated>
  </rdf:Description>
  <rdf:Description rdf:about="http://purl.org/olia/discourse/olia_discourse.owl#TemporallyDefinedUsage">
    <terms:replacedBy rdf:resource="http://purl.org/olia/olia.owl#TemporallyDefinedUsage"/>
  </rdf:Description>
  <rdf:Description rdf:about="http://purl.org/olia/discourse/olia_discourse.owl#TemporallyDefinedUsage">
    <owl:deprecated rdf:datatype="http://www.w3.org/2001/XMLSchema#boolean">true</owl:deprecated>
  </rdf:Description>
  <rdf:Description rdf:about="http://purl.org/olia/discourse/olia_discourse.owl#TemporalRelation">
    <terms:replacedBy rdf:resource="http://purl.org/olia/olia.owl#TemporalRelation"/>
  </rdf:Description>
  <rdf:Description rdf:about="http://purl.org/olia/discourse/olia_discourse.owl#TemporalRelation">
    <owl:deprecated rdf:datatype="http://www.w3.org/2001/XMLSchema#boolean">true</owl:deprecated>
  </rdf:Description>
  <rdf:Description rdf:about="http://purl.org/olia/discourse/olia_discourse.owl#TemporalSameTime">
    <terms:replacedBy rdf:resource="http://purl.org/olia/olia.owl#TemporalSameTime"/>
  </rdf:Description>
  <rdf:Description rdf:about="http://purl.org/olia/discourse/olia_discourse.owl#TemporalSameTime">
    <owl:deprecated rdf:datatype="http://www.w3.org/2001/XMLSchema#boolean">true</owl:deprecated>
  </rdf:Description>
  <rdf:Description rdf:about="http://purl.org/olia/discourse/olia_discourse.owl#TennisPlayer">
    <terms:replacedBy rdf:resource="http://purl.org/olia/olia.owl#TennisPlayer"/>
  </rdf:Description>
  <rdf:Description rdf:about="http://purl.org/olia/discourse/olia_discourse.owl#TennisPlayer">
    <owl:deprecated rdf:datatype="http://www.w3.org/2001/XMLSchema#boolean">true</owl:deprecated>
  </rdf:Description>
  <rdf:Description rdf:about="http://purl.org/olia/discourse/olia_discourse.owl#Text">
    <terms:replacedBy rdf:resource="http://purl.org/olia/olia.owl#Text"/>
  </rdf:Description>
  <rdf:Description rdf:about="http://purl.org/olia/discourse/olia_discourse.owl#Text">
    <owl:deprecated rdf:datatype="http://www.w3.org/2001/XMLSchema#boolean">true</owl:deprecated>
  </rdf:Description>
  <rdf:Description rdf:about="http://purl.org/olia/discourse/olia_discourse.owl#TextualOrganizationalRelation">
    <terms:replacedBy rdf:resource="http://purl.org/olia/olia.owl#TextualOrganizationalRelation"/>
  </rdf:Description>
  <rdf:Description rdf:about="http://purl.org/olia/discourse/olia_discourse.owl#TextualOrganizationalRelation">
    <owl:deprecated rdf:datatype="http://www.w3.org/2001/XMLSchema#boolean">true</owl:deprecated>
  </rdf:Description>
  <rdf:Description rdf:about="http://purl.org/olia/discourse/olia_discourse.owl#TextualOrganization_RST">
    <terms:replacedBy rdf:resource="http://purl.org/olia/olia.owl#TextualOrganization_RST"/>
  </rdf:Description>
  <rdf:Description rdf:about="http://purl.org/olia/discourse/olia_discourse.owl#TextualOrganization_RST">
    <owl:deprecated rdf:datatype="http://www.w3.org/2001/XMLSchema#boolean">true</owl:deprecated>
  </rdf:Description>
  <rdf:Description rdf:about="http://purl.org/olia/discourse/olia_discourse.owl#Time">
    <terms:replacedBy rdf:resource="http://purl.org/olia/olia.owl#Time"/>
  </rdf:Description>
  <rdf:Description rdf:about="http://purl.org/olia/discourse/olia_discourse.owl#Time">
    <owl:deprecated rdf:datatype="http://www.w3.org/2001/XMLSchema#boolean">true</owl:deprecated>
  </rdf:Description>
  <rdf:Description rdf:about="http://purl.org/olia/discourse/olia_discourse.owl#Title">
    <terms:replacedBy rdf:resource="http://purl.org/olia/olia.owl#Title"/>
  </rdf:Description>
  <rdf:Description rdf:about="http://purl.org/olia/discourse/olia_discourse.owl#Title">
    <owl:deprecated rdf:datatype="http://www.w3.org/2001/XMLSchema#boolean">true</owl:deprecated>
  </rdf:Description>
  <rdf:Description rdf:about="http://purl.org/olia/discourse/olia_discourse.owl#TitleInRunningText">
    <terms:replacedBy rdf:resource="http://purl.org/olia/olia.owl#TitleInRunningText"/>
  </rdf:Description>
  <rdf:Description rdf:about="http://purl.org/olia/discourse/olia_discourse.owl#TitleInRunningText">
    <owl:deprecated rdf:datatype="http://www.w3.org/2001/XMLSchema#boolean">true</owl:deprecated>
  </rdf:Description>
  <rdf:Description rdf:about="http://purl.org/olia/discourse/olia_discourse.owl#Topic">
    <terms:replacedBy rdf:resource="http://purl.org/olia/olia.owl#Topic"/>
  </rdf:Description>
  <rdf:Description rdf:about="http://purl.org/olia/discourse/olia_discourse.owl#Topic">
    <owl:deprecated rdf:datatype="http://www.w3.org/2001/XMLSchema#boolean">true</owl:deprecated>
  </rdf:Description>
  <rdf:Description rdf:about="http://purl.org/olia/discourse/olia_discourse.owl#TopicComment">
    <terms:replacedBy rdf:resource="http://purl.org/olia/olia.owl#TopicComment"/>
  </rdf:Description>
  <rdf:Description rdf:about="http://purl.org/olia/discourse/olia_discourse.owl#TopicComment">
    <owl:deprecated rdf:datatype="http://www.w3.org/2001/XMLSchema#boolean">true</owl:deprecated>
  </rdf:Description>
  <rdf:Description rdf:about="http://purl.org/olia/discourse/olia_discourse.owl#TopicComment_RST">
    <terms:replacedBy rdf:resource="http://purl.org/olia/olia.owl#TopicComment_RST"/>
  </rdf:Description>
  <rdf:Description rdf:about="http://purl.org/olia/discourse/olia_discourse.owl#TopicComment_RST">
    <owl:deprecated rdf:datatype="http://www.w3.org/2001/XMLSchema#boolean">true</owl:deprecated>
  </rdf:Description>
  <rdf:Description rdf:about="http://purl.org/olia/discourse/olia_discourse.owl#TopicContinuityRelation">
    <terms:replacedBy rdf:resource="http://purl.org/olia/olia.owl#TopicContinuityRelation"/>
  </rdf:Description>
  <rdf:Description rdf:about="http://purl.org/olia/discourse/olia_discourse.owl#TopicContinuityRelation">
    <owl:deprecated rdf:datatype="http://www.w3.org/2001/XMLSchema#boolean">true</owl:deprecated>
  </rdf:Description>
  <rdf:Description rdf:about="http://purl.org/olia/discourse/olia_discourse.owl#TopicDrift">
    <terms:replacedBy rdf:resource="http://purl.org/olia/olia.owl#TopicDrift"/>
  </rdf:Description>
  <rdf:Description rdf:about="http://purl.org/olia/discourse/olia_discourse.owl#TopicDrift">
    <owl:deprecated rdf:datatype="http://www.w3.org/2001/XMLSchema#boolean">true</owl:deprecated>
  </rdf:Description>
  <rdf:Description rdf:about="http://purl.org/olia/discourse/olia_discourse.owl#TopicDrift_RST">
    <terms:replacedBy rdf:resource="http://purl.org/olia/olia.owl#TopicDrift_RST"/>
  </rdf:Description>
  <rdf:Description rdf:about="http://purl.org/olia/discourse/olia_discourse.owl#TopicDrift_RST">
    <owl:deprecated rdf:datatype="http://www.w3.org/2001/XMLSchema#boolean">true</owl:deprecated>
  </rdf:Description>
  <rdf:Description rdf:about="http://purl.org/olia/discourse/olia_discourse.owl#TopicExpression">
    <terms:replacedBy rdf:resource="http://purl.org/olia/olia.owl#TopicExpression"/>
  </rdf:Description>
  <rdf:Description rdf:about="http://purl.org/olia/discourse/olia_discourse.owl#TopicExpression">
    <owl:deprecated rdf:datatype="http://www.w3.org/2001/XMLSchema#boolean">true</owl:deprecated>
  </rdf:Description>
  <rdf:Description rdf:about="http://purl.org/olia/discourse/olia_discourse.owl#TopicShift">
    <terms:replacedBy rdf:resource="http://purl.org/olia/olia.owl#TopicShift"/>
  </rdf:Description>
  <rdf:Description rdf:about="http://purl.org/olia/discourse/olia_discourse.owl#TopicShift">
    <owl:deprecated rdf:datatype="http://www.w3.org/2001/XMLSchema#boolean">true</owl:deprecated>
  </rdf:Description>
  <rdf:Description rdf:about="http://purl.org/olia/discourse/olia_discourse.owl#TopicShift_RST">
    <terms:replacedBy rdf:resource="http://purl.org/olia/olia.owl#TopicShift_RST"/>
  </rdf:Description>
  <rdf:Description rdf:about="http://purl.org/olia/discourse/olia_discourse.owl#TopicShift_RST">
    <owl:deprecated rdf:datatype="http://www.w3.org/2001/XMLSchema#boolean">true</owl:deprecated>
  </rdf:Description>
  <rdf:Description rdf:about="http://purl.org/olia/discourse/olia_discourse.owl#TVStation">
    <terms:replacedBy rdf:resource="http://purl.org/olia/olia.owl#TVStation"/>
  </rdf:Description>
  <rdf:Description rdf:about="http://purl.org/olia/discourse/olia_discourse.owl#TVStation">
    <owl:deprecated rdf:datatype="http://www.w3.org/2001/XMLSchema#boolean">true</owl:deprecated>
  </rdf:Description>
  <rdf:Description rdf:about="http://purl.org/olia/discourse/olia_discourse.owl#Unconditional">
    <terms:replacedBy rdf:resource="http://purl.org/olia/olia.owl#Unconditional"/>
  </rdf:Description>
  <rdf:Description rdf:about="http://purl.org/olia/discourse/olia_discourse.owl#Unconditional">
    <owl:deprecated rdf:datatype="http://www.w3.org/2001/XMLSchema#boolean">true</owl:deprecated>
  </rdf:Description>
  <rdf:Description rdf:about="http://purl.org/olia/discourse/olia_discourse.owl#University">
    <terms:replacedBy rdf:resource="http://purl.org/olia/olia.owl#University"/>
  </rdf:Description>
  <rdf:Description rdf:about="http://purl.org/olia/discourse/olia_discourse.owl#University">
    <owl:deprecated rdf:datatype="http://www.w3.org/2001/XMLSchema#boolean">true</owl:deprecated>
  </rdf:Description>
  <rdf:Description rdf:about="http://purl.org/olia/discourse/olia_discourse.owl#Unless_RST">
    <terms:replacedBy rdf:resource="http://purl.org/olia/olia.owl#Unless_RST"/>
  </rdf:Description>
  <rdf:Description rdf:about="http://purl.org/olia/discourse/olia_discourse.owl#Unless_RST">
    <owl:deprecated rdf:datatype="http://www.w3.org/2001/XMLSchema#boolean">true</owl:deprecated>
  </rdf:Description>
  <rdf:Description rdf:about="http://purl.org/olia/discourse/olia_discourse.owl#UnmarkedFactuality">
    <terms:replacedBy rdf:resource="http://purl.org/olia/olia.owl#UnmarkedFactuality"/>
  </rdf:Description>
  <rdf:Description rdf:about="http://purl.org/olia/discourse/olia_discourse.owl#UnmarkedFactuality">
    <owl:deprecated rdf:datatype="http://www.w3.org/2001/XMLSchema#boolean">true</owl:deprecated>
  </rdf:Description>
  <rdf:Description rdf:about="http://purl.org/olia/discourse/olia_discourse.owl#UnmarkedPolarity">
    <terms:replacedBy rdf:resource="http://purl.org/olia/olia.owl#UnmarkedPolarity"/>
  </rdf:Description>
  <rdf:Description rdf:about="http://purl.org/olia/discourse/olia_discourse.owl#UnmarkedPolarity">
    <owl:deprecated rdf:datatype="http://www.w3.org/2001/XMLSchema#boolean">true</owl:deprecated>
  </rdf:Description>
  <rdf:Description rdf:about="http://purl.org/olia/discourse/olia_discourse.owl#UnrealCondition_HDRB">
    <terms:replacedBy rdf:resource="http://purl.org/olia/olia.owl#UnrealCondition_HDRB"/>
  </rdf:Description>
  <rdf:Description rdf:about="http://purl.org/olia/discourse/olia_discourse.owl#UnrealCondition_HDRB">
    <owl:deprecated rdf:datatype="http://www.w3.org/2001/XMLSchema#boolean">true</owl:deprecated>
  </rdf:Description>
  <rdf:Description rdf:about="http://purl.org/olia/discourse/olia_discourse.owl#UnrealPastCondition_PDTB">
    <terms:replacedBy rdf:resource="http://purl.org/olia/olia.owl#UnrealPastCondition_PDTB"/>
  </rdf:Description>
  <rdf:Description rdf:about="http://purl.org/olia/discourse/olia_discourse.owl#UnrealPastCondition_PDTB">
    <owl:deprecated rdf:datatype="http://www.w3.org/2001/XMLSchema#boolean">true</owl:deprecated>
  </rdf:Description>
  <rdf:Description rdf:about="http://purl.org/olia/discourse/olia_discourse.owl#UnrealPresentCondition_PDTB">
    <terms:replacedBy rdf:resource="http://purl.org/olia/olia.owl#UnrealPresentCondition_PDTB"/>
  </rdf:Description>
  <rdf:Description rdf:about="http://purl.org/olia/discourse/olia_discourse.owl#UnrealPresentCondition_PDTB">
    <owl:deprecated rdf:datatype="http://www.w3.org/2001/XMLSchema#boolean">true</owl:deprecated>
  </rdf:Description>
  <rdf:Description rdf:about="http://purl.org/olia/discourse/olia_discourse.owl#UnsolicitedResponse">
    <terms:replacedBy rdf:resource="http://purl.org/olia/olia.owl#UnsolicitedResponse"/>
  </rdf:Description>
  <rdf:Description rdf:about="http://purl.org/olia/discourse/olia_discourse.owl#UnsolicitedResponse">
    <owl:deprecated rdf:datatype="http://www.w3.org/2001/XMLSchema#boolean">true</owl:deprecated>
  </rdf:Description>
  <rdf:Description rdf:about="http://purl.org/olia/discourse/olia_discourse.owl#URL">
    <terms:replacedBy rdf:resource="http://purl.org/olia/olia.owl#URL"/>
  </rdf:Description>
  <rdf:Description rdf:about="http://purl.org/olia/discourse/olia_discourse.owl#URL">
    <owl:deprecated rdf:datatype="http://www.w3.org/2001/XMLSchema#boolean">true</owl:deprecated>
  </rdf:Description>
  <rdf:Description rdf:about="http://purl.org/olia/discourse/olia_discourse.owl#Utterance">
    <terms:replacedBy rdf:resource="http://purl.org/olia/olia.owl#Utterance"/>
  </rdf:Description>
  <rdf:Description rdf:about="http://purl.org/olia/discourse/olia_discourse.owl#Utterance">
    <owl:deprecated rdf:datatype="http://www.w3.org/2001/XMLSchema#boolean">true</owl:deprecated>
  </rdf:Description>
  <rdf:Description rdf:about="http://purl.org/olia/discourse/olia_discourse.owl#Valley">
    <terms:replacedBy rdf:resource="http://purl.org/olia/olia.owl#Valley"/>
  </rdf:Description>
  <rdf:Description rdf:about="http://purl.org/olia/discourse/olia_discourse.owl#Valley">
    <owl:deprecated rdf:datatype="http://www.w3.org/2001/XMLSchema#boolean">true</owl:deprecated>
  </rdf:Description>
  <rdf:Description rdf:about="http://purl.org/olia/discourse/olia_discourse.owl#Vehicle">
    <terms:replacedBy rdf:resource="http://purl.org/olia/olia.owl#Vehicle"/>
  </rdf:Description>
  <rdf:Description rdf:about="http://purl.org/olia/discourse/olia_discourse.owl#Vehicle">
    <owl:deprecated rdf:datatype="http://www.w3.org/2001/XMLSchema#boolean">true</owl:deprecated>
  </rdf:Description>
  <rdf:Description rdf:about="http://purl.org/olia/discourse/olia_discourse.owl#VideoGame">
    <terms:replacedBy rdf:resource="http://purl.org/olia/olia.owl#VideoGame"/>
  </rdf:Description>
  <rdf:Description rdf:about="http://purl.org/olia/discourse/olia_discourse.owl#VideoGame">
    <owl:deprecated rdf:datatype="http://www.w3.org/2001/XMLSchema#boolean">true</owl:deprecated>
  </rdf:Description>
  <rdf:Description rdf:about="http://purl.org/olia/discourse/olia_discourse.owl#VocativeExpression">
    <terms:replacedBy rdf:resource="http://purl.org/olia/olia.owl#VocativeExpression"/>
  </rdf:Description>
  <rdf:Description rdf:about="http://purl.org/olia/discourse/olia_discourse.owl#VocativeExpression">
    <owl:deprecated rdf:datatype="http://www.w3.org/2001/XMLSchema#boolean">true</owl:deprecated>
  </rdf:Description>
  <rdf:Description rdf:about="http://purl.org/olia/discourse/olia_discourse.owl#VolitionalCause_RST">
    <terms:replacedBy rdf:resource="http://purl.org/olia/olia.owl#VolitionalCause_RST"/>
  </rdf:Description>
  <rdf:Description rdf:about="http://purl.org/olia/discourse/olia_discourse.owl#VolitionalCause_RST">
    <owl:deprecated rdf:datatype="http://www.w3.org/2001/XMLSchema#boolean">true</owl:deprecated>
  </rdf:Description>
  <rdf:Description rdf:about="http://purl.org/olia/discourse/olia_discourse.owl#VolitionalResult_RST">
    <terms:replacedBy rdf:resource="http://purl.org/olia/olia.owl#VolitionalResult_RST"/>
  </rdf:Description>
  <rdf:Description rdf:about="http://purl.org/olia/discourse/olia_discourse.owl#VolitionalResult_RST">
    <owl:deprecated rdf:datatype="http://www.w3.org/2001/XMLSchema#boolean">true</owl:deprecated>
  </rdf:Description>
  <rdf:Description rdf:about="http://purl.org/olia/discourse/olia_discourse.owl#VulgarRegister">
    <terms:replacedBy rdf:resource="http://purl.org/olia/olia.owl#VulgarRegister"/>
  </rdf:Description>
  <rdf:Description rdf:about="http://purl.org/olia/discourse/olia_discourse.owl#VulgarRegister">
    <owl:deprecated rdf:datatype="http://www.w3.org/2001/XMLSchema#boolean">true</owl:deprecated>
  </rdf:Description>
  <rdf:Description rdf:about="http://purl.org/olia/discourse/olia_discourse.owl#Weapon">
    <terms:replacedBy rdf:resource="http://purl.org/olia/olia.owl#Weapon"/>
  </rdf:Description>
  <rdf:Description rdf:about="http://purl.org/olia/discourse/olia_discourse.owl#Weapon">
    <owl:deprecated rdf:datatype="http://www.w3.org/2001/XMLSchema#boolean">true</owl:deprecated>
  </rdf:Description>
  <rdf:Description rdf:about="http://purl.org/olia/discourse/olia_discourse.owl#Website">
    <terms:replacedBy rdf:resource="http://purl.org/olia/olia.owl#Website"/>
  </rdf:Description>
  <rdf:Description rdf:about="http://purl.org/olia/discourse/olia_discourse.owl#Website">
    <owl:deprecated rdf:datatype="http://www.w3.org/2001/XMLSchema#boolean">true</owl:deprecated>
  </rdf:Description>
  <rdf:Description rdf:about="http://purl.org/olia/discourse/olia_discourse.owl#WholePart">
    <terms:replacedBy rdf:resource="http://purl.org/olia/olia.owl#WholePart"/>
  </rdf:Description>
  <rdf:Description rdf:about="http://purl.org/olia/discourse/olia_discourse.owl#WholePart">
    <owl:deprecated rdf:datatype="http://www.w3.org/2001/XMLSchema#boolean">true</owl:deprecated>
  </rdf:Description>
  <rdf:Description rdf:about="http://purl.org/olia/discourse/olia_discourse.owl#WideFocus">
    <terms:replacedBy rdf:resource="http://purl.org/olia/olia.owl#WideFocus"/>
  </rdf:Description>
  <rdf:Description rdf:about="http://purl.org/olia/discourse/olia_discourse.owl#WideFocus">
    <owl:deprecated rdf:datatype="http://www.w3.org/2001/XMLSchema#boolean">true</owl:deprecated>
  </rdf:Description>
</rdf:RDF>
