<?xml version="1.0"?>
<rdf:RDF xmlns="http://purl.org/olia/olia-top.owl#"
     xml:base="http://purl.org/olia/olia-top.owl"
     xmlns:dcr="http://www.isocat.org/ns/dcr.rdf#"
     xmlns:dct="http://purl.org/dc/terms/"
     xmlns:owl="http://www.w3.org/2002/07/owl#"
     xmlns:rdf="http://www.w3.org/1999/02/22-rdf-syntax-ns#"
     xmlns:xml="http://www.w3.org/XML/1998/namespace"
     xmlns:xsd="http://www.w3.org/2001/XMLSchema#"
     xmlns:rdfs="http://www.w3.org/2000/01/rdf-schema#"
     xmlns:olia_system="http://purl.org/olia/system.owl#">
    <owl:Ontology rdf:about="http://purl.org/olia/olia-top.owl">
        <owl:imports rdf:resource="http://purl.org/olia/system.owl"/>
        <dct:license rdf:resource="https://creativecommons.org/licenses/by/3.0/"/>
        <rdfs:comment>Top categories of the OLiA Reference Model
  2010-01-19 OLiA-Top created 
  
  2010-04-08 OLiA-Top: removed NPFunction (=&gt; SyntacticRole) 
	
  2010-04-13 OLiA-Top: added MorphologicalProcess, MorphologicalFeature, DiscourseFeature (PragmaticFeature), AnimacyFeature, ReferentTypeFeature, RegisterFeature, UsageAndFrequencyFeature
	
  2010-04-14 OLiA-Top: validation, PossessiveFeature removed (see olia:hasOwnerNumber), moved olia:NarrativeType and olia:PolarityFeature here
	
  2010-04-15 OLiA-Top: additions in accordance to the PTB Bracketing Guidelines: NullElement, SentenceTypeFeature (Santorini 1991, Bies et al. 1995)
	
  2010-11-30 OLiA-Top: added TopologicalField in accordance to the TueDa-D/Z annotation guidelines (Telljohann et al. 2009)
	
  2011-07-29 OLiA-Top: replace url by purl
	
  2011-07-31 OLiA-Top: added ProximityFeature
	
  2011-08-03 OLiA-Top: added SpecificityFeature
	
  2011-08-04 OLiA-Top: SubordTypeFeature, CoordTypeFeature deprecated, added NumeralAgreementClass
	
  2011-08-11 OLiA-Top: StrengthFeature recast as MorphologicalFeature rather than MorphosyntacticFeature
	
  2011-08-15 OLiA-Top: EmphasisFeature added
	
  2011-08-15 OLiA-Top: PhonologicalProcess added (for Elision and Apocope, formerly both classified as MorphologicalProcess)
	
  2013-06-25 OLiA-Top: EvidentialityFeature, ClusivityFeature added (from ISOcat), intensity as new label to EmphasisFeature; LexicalRelation for labels for relations holding between lexemes
	
  2013-06-27 OLiA-Top: AgreementFeature (from ISOcat, as superclass of NominalAgreementClass, Person, Gender, Number; not as a relation between words)	
	
  2013-06-28 OLiA-Top: EvaluativeFeature (for ISOcat PreferredEvaluative and PejorativeEvaluative), ModalityFeature (Modality and Mood distinction revised)
	
  2016-04-18 OLiA-Top: fixed minor validity warnings
	
  2016-08-29 OLiA-Top: added MovementFeature as cover term for Rising and Control (for compliance with lexinfo)
	
  2020-02-06 OLiA-Top: fixed use of owl:deprecated
	
  2020-02-24 OLiA-Top: description of Constituent
  
  2022-05-23 OLiA-Top: rdfs:labels added (automatically)
  
  2024-11-25 OLiA-Top: integration of OLiA Discourse: 
    PragmaticRelation, TextStructuralUnit,
    DiscourseFeature =&gt; PragmaticFeature, 
    PragmaticUnit introduced as superclass of DiscourseEntity,

  </rdfs:comment>
        <owl:versionInfo>TODO: check upper level organization, remodel strength as categories (as in DCR), rename UsageAndFrequencyFeature to UsageFeature</owl:versionInfo>
    </owl:Ontology>
    


    <!-- 
    ///////////////////////////////////////////////////////////////////////////////////////
    //
    // Annotation properties
    //
    ///////////////////////////////////////////////////////////////////////////////////////
     -->

    


    <!-- http://purl.org/dc/terms/replaces -->

    <owl:AnnotationProperty rdf:about="http://purl.org/dc/terms/replaces"/>
    


    <!-- 
    ///////////////////////////////////////////////////////////////////////////////////////
    //
    // Classes
    //
    ///////////////////////////////////////////////////////////////////////////////////////
     -->

    


    <!-- http://purl.org/olia/olia-top.owl#AgreementFeature -->

    <owl:Class rdf:about="http://purl.org/olia/olia-top.owl#AgreementFeature">
        <rdfs:subClassOf rdf:resource="http://purl.org/olia/olia-top.owl#MorphosyntacticFeature"/>
        <rdfs:comment>Agreement: Formal relationship whereby a word (or a sub-part of a word) requires a corresponding form of another word (or sub-part of a word) (http://www.isocat.org/datcat/DC-2188)
	  
	  PVAGR: agreement as shown (stem + affix) in inflected forms of a finite verb (http://www.isocat.org/datcat/DC-4973)</rdfs:comment>
        <rdfs:isDefinedBy>http://www.isocat.org/datcat/DC-2188</rdfs:isDefinedBy>
        <rdfs:isDefinedBy>http://www.isocat.org/datcat/DC-4973</rdfs:isDefinedBy>
        <rdfs:label>PVAGR</rdfs:label>
        <rdfs:label>agreement</rdfs:label>
        <rdfs:label xml:lang="en">agreement feature</rdfs:label>
    </owl:Class>
    


    <!-- http://purl.org/olia/olia-top.owl#AnimacyFeature -->

    <owl:Class rdf:about="http://purl.org/olia/olia-top.owl#AnimacyFeature">
        <rdfs:subClassOf rdf:resource="http://purl.org/olia/olia-top.owl#SemanticFeature"/>
        <rdfs:comment>
                            The characteristic of a word indicating that in a given discourse community, its referent is considered to be alive or to possess a quality of volition or consciousness.
                                (ISO12620; http://www.isocat.org/datcat/DC-1902)
      </rdfs:comment>
        <rdfs:label>animacy</rdfs:label>
        <rdfs:label xml:lang="en">animacy feature</rdfs:label>
        <owl:versionInfo>http://www.isocat.org/datcat/DC-1902, extended to cover http://purl.org/olia/mte/multext-east.owl#Humanness</owl:versionInfo>
    </owl:Class>
    


    <!-- http://purl.org/olia/olia-top.owl#AspectFeature -->

    <owl:Class rdf:about="http://purl.org/olia/olia-top.owl#AspectFeature">
        <rdfs:subClassOf rdf:resource="http://purl.org/olia/olia-top.owl#MorphosyntacticFeature"/>
        <rdfs:comment>Category associated to verbs and referring to the way the grammar marks the duration or type of temporal activity. (http://www.isocat.org/datcat/DC-1242)
	  
	  Aspect is a grammatical category associated with verbs that expresses a temporal view of the event or state expressed by the verb. (http://www.sil.org/linguistics/glossaryoflinguisticterms/WhatIsAspect.htm  17.11.06)

The in Eagles optional attribute Aspect is needed for Greek and Slavonic verbs. It corresponds also to the Past Simple/Imperfect distinction of Romance languages. (http://www.ilc.cnr.it/EAGLES96/annotate/node18.html#oav1av  17.11.06)</rdfs:comment>
        <rdfs:isDefinedBy>http://www.isocat.org/datcat/DC-1242</rdfs:isDefinedBy>
        <rdfs:label>aspect</rdfs:label>
        <rdfs:label xml:lang="en">aspect feature</rdfs:label>
    </owl:Class>
    


    <!-- http://purl.org/olia/olia-top.owl#CaseFeature -->

    <owl:Class rdf:about="http://purl.org/olia/olia-top.owl#CaseFeature">
        <rdfs:subClassOf rdf:resource="http://purl.org/olia/olia-top.owl#MorphosyntacticFeature"/>
        <rdfs:comment>Case is a grammatical category determined by the syntactic or semantic function of a noun or pronoun. The term case has traditionally been restricted to apply to only those languages which indicate certain functions by the inflection of nouns, pronouns, or noun phrase constituents, such as adjectives and numerals. (http://www.sil.org/linguistics/glossaryoflinguisticterms/WhatIsCase.htm  17.11.06)</rdfs:comment>
        <rdfs:label xml:lang="en">case feature</rdfs:label>
    </owl:Class>
    


    <!-- http://purl.org/olia/olia-top.owl#ClusivityFeature -->

    <owl:Class rdf:about="http://purl.org/olia/olia-top.owl#ClusivityFeature">
        <rdfs:subClassOf rdf:resource="http://purl.org/olia/olia-top.owl#MorphosyntacticFeature"/>
        <rdfs:comment>The category that encodes &quot;whether the addressee (addressees) are included in or excluded from the set of referents which also contains the speaker&quot;.</rdfs:comment>
        <rdfs:isDefinedBy>http://www.isocat.org/datcat/DC-3031</rdfs:isDefinedBy>
        <rdfs:label>clusivity</rdfs:label>
        <rdfs:label xml:lang="en">clusivity feature</rdfs:label>
    </owl:Class>
    


    <!-- http://purl.org/olia/olia-top.owl#Constituent -->

    <owl:Class rdf:about="http://purl.org/olia/olia-top.owl#Constituent">
        <rdfs:subClassOf rdf:resource="http://purl.org/olia/olia-top.owl#SyntacticCategory"/>
        <rdfs:comment>
	In syntactic theory, a constituent is a unit of words that constitute a unit of multiple independent words. Formally, this can be illustrated by substitution (and other tests):
	&quot;[The dog] bit Peter.&quot;: valid, &quot;the dog&quot; can be replaced by &quot;lions&quot; (etc.).
	&quot;*The [dog bit] Peter.&quot;: non-valid, there is no valid one-word replacement for &quot;dog bit&quot;.
	&quot;The dog [bit Peter].&quot;: valid, &quot;bit Peter&quot; can be replaced by &quot;slept&quot; (etc.)
	
	Note that OLiA takes a theory-independent stance on &quot;constituent&quot;. Constituent thus does not necessarily refer to a syntactic constituent, but to a node in syntax annotation that contains other nodes. This includes elements whose constituency has been debated (verb phrases), but also elements that are (potentially incomplete) phrase candidates (chunks).
	(Christian Chiarcos)
	</rdfs:comment>
        <rdfs:label xml:lang="en">constituent</rdfs:label>
    </owl:Class>
    


    <!-- http://purl.org/olia/olia-top.owl#CoordTypeFeature -->

    <owl:Class rdf:about="http://purl.org/olia/olia-top.owl#CoordTypeFeature">
        <rdfs:subClassOf rdf:resource="http://purl.org/olia/olia-top.owl#MorphosyntacticFeature"/>
        <rdfs:comment>The CoordType attribute subclassifies coordinating conjunctions. (http://www.ilc.cnr.it/EAGLES96/annotate/node18.html#oav1av  17.11.06)</rdfs:comment>
        <rdfs:label xml:lang="en">coord type feature</rdfs:label>
        <owl:deprecated rdf:datatype="http://www.w3.org/2001/XMLSchema#boolean">true</owl:deprecated>
        <owl:versionInfo>Deprecated: reimplemented as subhierarchy of CoordinatingConjunction</owl:versionInfo>
    </owl:Class>
    


    <!-- http://purl.org/olia/olia-top.owl#CountabilityFeature -->

    <owl:Class rdf:about="http://purl.org/olia/olia-top.owl#CountabilityFeature">
        <rdfs:subClassOf rdf:resource="http://purl.org/olia/olia-top.owl#SemanticFeature"/>
        <rdfs:comment>Represents the difference between countable and uncountable nouns, e.g., in English</rdfs:comment>
        <rdfs:label xml:lang="en">countability feature</rdfs:label>
        <owl:versionInfo>EAGLES</owl:versionInfo>
    </owl:Class>
    


    <!-- http://purl.org/olia/olia-top.owl#DefinitenessFeature -->

    <owl:Class rdf:about="http://purl.org/olia/olia-top.owl#DefinitenessFeature">
        <rdfs:subClassOf rdf:resource="http://purl.org/olia/olia-top.owl#MorphosyntacticFeature"/>
        <rdfs:comment>In grammatical theory, definiteness is a feature of noun phrases, distinguishing between entities which are specific and identifiable in a given context (definite noun phrases) and entities which are not (indefinite noun phrases).
(http://en.wikipedia.org/wiki/Definiteness 02.05.07)

	Property about the possiblity to identify an entity. (http://www.isocat.org/datcat/DC-1926)

An in Eagles additional language-specific attribute for nouns/ noun phrases is Definiteness.
(http://www.ilc.cnr.it/EAGLES96/annotate/node19.html#oav2  16.11.06)</rdfs:comment>
        <rdfs:isDefinedBy>http://www.isocat.org/datcat/DC-1926</rdfs:isDefinedBy>
        <rdfs:label>definiteness</rdfs:label>
        <rdfs:label xml:lang="en">definiteness feature</rdfs:label>
    </owl:Class>
    


    <!-- http://purl.org/olia/olia-top.owl#DegreeFeature -->

    <owl:Class rdf:about="http://purl.org/olia/olia-top.owl#DegreeFeature">
        <rdfs:subClassOf rdf:resource="http://purl.org/olia/olia-top.owl#MorphosyntacticFeature"/>
        <rdfs:comment>Property concerning comparison. (http://www.isocat.org/datcat/DC-1419) 
	  
	  The Eagles-recommended attribute Degree applies only to inflectional comparatives and superlatives. In some languages, e.g. Spanish, the number of such adjectives is very small. (http://www.ilc.cnr.it/EAGLES96/annotate/node17.html#recn)</rdfs:comment>
        <rdfs:isDefinedBy>http://www.isocat.org/datcat/DC-1419</rdfs:isDefinedBy>
        <rdfs:label>degree</rdfs:label>
        <rdfs:label xml:lang="en">degree feature</rdfs:label>
    </owl:Class>
    


    <!-- http://purl.org/olia/olia-top.owl#DependencyRelation -->

    <owl:Class rdf:about="http://purl.org/olia/olia-top.owl#DependencyRelation">
        <rdfs:subClassOf rdf:resource="http://purl.org/olia/olia-top.owl#SyntacticRelation"/>
        <rdfs:label xml:lang="en">dependency relation</rdfs:label>
    </owl:Class>
    


    <!-- http://purl.org/olia/olia-top.owl#DiscourseEntity -->

    <owl:Class rdf:about="http://purl.org/olia/olia-top.owl#DiscourseEntity">
        <rdfs:subClassOf rdf:resource="http://purl.org/olia/olia-top.owl#PragmaticUnit"/>
        <rdfs:label xml:lang="en">discourse entity</rdfs:label>
    </owl:Class>
    


    <!-- http://purl.org/olia/olia-top.owl#DominanceRelation -->

    <owl:Class rdf:about="http://purl.org/olia/olia-top.owl#DominanceRelation">
        <rdfs:subClassOf rdf:resource="http://purl.org/olia/olia-top.owl#SyntacticRelation"/>
        <rdfs:label xml:lang="en">dominance relation</rdfs:label>
    </owl:Class>
    


    <!-- http://purl.org/olia/olia-top.owl#EmphasisFeature -->

    <owl:Class rdf:about="http://purl.org/olia/olia-top.owl#EmphasisFeature">
        <rdfs:subClassOf rdf:resource="http://purl.org/olia/olia-top.owl#MorphosyntacticFeature"/>
        <rdfs:comment>Applies to grammatical (morphosyntactic) markers of emphasis for languages where emphatic expressions are distinguished from non-emphatic forms.
      In Irish Gaelic, for example, the unmarked personal pronouns (e.g., sé, é ‘he, him’) is distinguished from the emphatic pronoun (e.g., seisean, eisean ‘he, him’). 
      Beyond pronouns, also nouns can be emphatically marked, e.g., by adding a clitic reflexive element to them. (Mulkern 2007).
      
      (Ann E. Mulkern. Knowing who’s important: Relative discourse salience and Irish pronominal forms. In Nancy A. Hedberg and Ron Zacharski, editors, The Grammar-Pragmatics Interface: Essays in honor of Jeanette K. Gundel, pages 113–142. John Benjamins, Amsterdam and Philadelphia, 2007.)
    </rdfs:comment>
        <rdfs:comment>Quality of being felt very strongly or having a strong effect (intensity, http://www.isocat.org/datcat/DC-2197)</rdfs:comment>
        <rdfs:isDefinedBy>http://www.isocat.org/datcat/DC-2197</rdfs:isDefinedBy>
        <rdfs:label>emphasis</rdfs:label>
        <rdfs:label xml:lang="en">emphasis feature</rdfs:label>
        <rdfs:label>intensity</rdfs:label>
        <owl:versionInfo>adopted from ILPOSTS, there a property of Adverb, Classifier, Demonstrative, Noun, Particle, Adposition, Quantifier, Verb, identified with http://www.isocat.org/datcat/DC-2197 &quot;intensity&quot;</owl:versionInfo>
    </owl:Class>
    


    <!-- http://purl.org/olia/olia-top.owl#EvaluativeFeature -->

    <owl:Class rdf:about="http://purl.org/olia/olia-top.owl#EvaluativeFeature">
        <rdfs:subClassOf rdf:resource="http://purl.org/olia/olia-top.owl#SemanticFeature"/>
        <rdfs:comment>generalization over PreferredEvaluative and PejorativeEvaluative in ISOcat</rdfs:comment>
        <rdfs:label xml:lang="en">evaluative feature</rdfs:label>
    </owl:Class>
    


    <!-- http://purl.org/olia/olia-top.owl#EvidentialityFeature -->

    <owl:Class rdf:about="http://purl.org/olia/olia-top.owl#EvidentialityFeature">
        <rdfs:subClassOf rdf:resource="http://purl.org/olia/olia-top.owl#MorphosyntacticFeature"/>
        <rdfs:comment>Evidentiality denotes the basis that the speaker
                        has for claiming that the event has occurred (or is going to take place).
                        Appear to show a greater number of distinctions in the realis mood
                        (especially in the past tense) than the irrealis mood. [Bhat 1999: 63-64,
                        70]</rdfs:comment>
        <rdfs:isDefinedBy>http://www.isocat.org/datcat/DC-3185</rdfs:isDefinedBy>
        <rdfs:label xml:lang="en">evidentiality feature</rdfs:label>
        <owl:versionInfo>isoCat ID: http://www.isocat.org/datcat/DC-3185</owl:versionInfo>
    </owl:Class>
    


    <!-- http://purl.org/olia/olia-top.owl#GenderFeature -->

    <owl:Class rdf:about="http://purl.org/olia/olia-top.owl#GenderFeature">
        <rdfs:subClassOf rdf:resource="http://purl.org/olia/olia-top.owl#AgreementFeature"/>
        <rdfs:comment>The term gender refers to various forms of expressing biological or sociological gender by inflecting words.  Nouns, pronouns, articles and the adjectives denote the gender of their referent. (http://en.wikipedia.org/wiki/Grammatical_gender  17.11.06)
	
	Category based on (depending on languages) the natural distinction between sex and formal criteria.
    (http://www.isocat.org/datcat/DC-1297)
	</rdfs:comment>
        <rdfs:label xml:lang="en">gender feature</rdfs:label>
    </owl:Class>
    


    <!-- http://purl.org/olia/olia-top.owl#InflectionTypeFeature -->

    <owl:Class rdf:about="http://purl.org/olia/olia-top.owl#InflectionTypeFeature">
        <rdfs:subClassOf rdf:resource="http://purl.org/olia/olia-top.owl#MorphologicalFeature"/>
        <rdfs:comment>InflectionType is in Eagles an optional attribute for adjectives. Weak and Strong are values for adjectival inflection in the Germanic languages German, Dutch and Danish. (http://www.ilc.cnr.it/EAGLES96/annotate/node18.html#oav1av  14.11.06)</rdfs:comment>
        <rdfs:label xml:lang="en">inflection type feature</rdfs:label>
    </owl:Class>
    


    <!-- http://purl.org/olia/olia-top.owl#LexicalRelation -->

    <owl:Class rdf:about="http://purl.org/olia/olia-top.owl#LexicalRelation">
        <rdfs:subClassOf rdf:resource="http://purl.org/olia/olia-top.owl#LinguisticConcept"/>
        <rdfs:label xml:lang="en">lexical relation</rdfs:label>
        <owl:versionInfo>introduced for relation labels such as homonym. These label relations holding between two lexemes.</owl:versionInfo>
    </owl:Class>
    


    <!-- http://purl.org/olia/olia-top.owl#LinguisticConcept -->

    <owl:Class rdf:about="http://purl.org/olia/olia-top.owl#LinguisticConcept">
        <rdfs:comment>The OLiA ontology specifies linguistic concepts on a theoretical basis, as for concepts used in annotations, see system.owl.
There is a great extent of overlap between LinguisticCategories/LinguisticFeatures and Categories/Features as defined in system.owl.</rdfs:comment>
        <rdfs:label xml:lang="en">linguistic concept</rdfs:label>
        <owl:versionInfo>Note that olia_system:LinguisticAnnotation, olia_system:UnitOfAnnotation and olia_system:Feature pertain to the usage of type labels and annotated features according to a particular annotation scheme, whereas, here, category and feature mean linguistic concepts. Thus, an olia:MorphosyntacticCategory (etc.) is not necessarily represented by a olia_system:UnitOfAnnotation.</owl:versionInfo>
    </owl:Class>
    


    <!-- http://purl.org/olia/olia-top.owl#ModalityFeature -->

    <owl:Class rdf:about="http://purl.org/olia/olia-top.owl#ModalityFeature">
        <rdfs:subClassOf rdf:resource="http://purl.org/olia/olia-top.owl#SemanticFeature"/>
        <rdfs:comment>
			Modality is a facet of illocutionary point or general intent of a speaker, 
			or a speaker&apos;s degree of commitment to the expressed proposition&apos;s believability, 
			obligatoriness, desirability or reality.
            (ISO12620; http://www.isocat.org/datcat/DC-1427)

			The term „mood“ is used by some authors in the same sense as „modality“, while 
			others distinguish the two (...) using „mood“ to refer to the contrastive 
			grammatical expressions of different modalities, and thus reserving „modality“ 
			to refer to the meanings so expressed. &gt;A grammatical category is related to 
			a variety of factors affecting the nature of a predication, such as factors include 
			factivity, certainty (evidentials), attitudes, speaker’s knowledge/beliefs/desires, 
			agent’s ability/volitionality, etc.; a set of distinctive forms used to express 
			modality (as verbal inflections or a set of auxiliarys, each signaling a modality). 
			(http://www.uni-erfurt.de/sprachwissenschaft/proxy.php?port=8080&amp;file=lido/servlet/Lido_Servlet Modus 14.05.07)
	</rdfs:comment>
        <rdfs:label>modality</rdfs:label>
        <rdfs:label xml:lang="en">modality feature</rdfs:label>
        <rdfs:label>mood</rdfs:label>
        <owl:versionInfo>2024-11-22 redefined as a SemanticFeature, for modality as a morphosyntactic concept, see MoodFeature</owl:versionInfo>
        <owl:versionInfo>http://www.isocat.org/datcat/DC-1427</owl:versionInfo>
    </owl:Class>
    


    <!-- http://purl.org/olia/olia-top.owl#MoodFeature -->

    <owl:Class rdf:about="http://purl.org/olia/olia-top.owl#MoodFeature">
        <rdfs:subClassOf rdf:resource="http://purl.org/olia/olia-top.owl#MorphosyntacticFeature"/>
        <rdfs:comment>
			Modality is a facet of illocutionary point or general intent of a speaker, 
			or a speaker&apos;s degree of commitment to the expressed proposition&apos;s believability, 
			obligatoriness, desirability or reality.
            (ISO12620; http://www.isocat.org/datcat/DC-1427)

			The term „mood“ is used by some authors in the same sense as „modality“, while 
			others distinguish the two (...) using „mood“ to refer to the contrastive 
			grammatical expressions of different modalities, and thus reserving „modality“ 
			to refer to the meanings so expressed. &gt;A grammatical category is related to 
			a variety of factors affecting the nature of a predication, such as factors include 
			factivity, certainty (evidentials), attitudes, speaker’s knowledge/beliefs/desires, 
			agent’s ability/volitionality, etc.; a set of distinctive forms used to express 
			modality (as verbal inflections or a set of auxiliarys, each signaling a modality). 
			(http://www.uni-erfurt.de/sprachwissenschaft/proxy.php?port=8080&amp;file=lido/servlet/Lido_Servlet Modus 14.05.07)
	</rdfs:comment>
        <rdfs:label>mood</rdfs:label>
        <rdfs:label xml:lang="en">mood feature</rdfs:label>
        <rdfs:label>verb form mood</rdfs:label>
        <owl:versionInfo>http://www.isocat.org/datcat/DC-1427</owl:versionInfo>
    </owl:Class>
    


    <!-- http://purl.org/olia/olia-top.owl#MorphologicalCategory -->

    <owl:Class rdf:about="http://purl.org/olia/olia-top.owl#MorphologicalCategory">
        <rdfs:subClassOf rdf:resource="http://purl.org/olia/olia-top.owl#LinguisticConcept"/>
        <rdfs:label xml:lang="en">morphological category</rdfs:label>
    </owl:Class>
    


    <!-- http://purl.org/olia/olia-top.owl#MorphologicalFeature -->

    <owl:Class rdf:about="http://purl.org/olia/olia-top.owl#MorphologicalFeature">
        <rdfs:subClassOf rdf:resource="http://purl.org/olia/olia-top.owl#LinguisticConcept"/>
        <rdfs:subClassOf rdf:resource="http://purl.org/olia/system.owl#Feature"/>
        <rdfs:comment>
                            Property attached to a given inflected form that usually permits to distinguish this form from the generic lemmatised form of the word.
                                (http://www.isocat.org/datcat/DC-1425)
                            </rdfs:comment>
        <rdfs:label xml:lang="en">morphological feature</rdfs:label>
        <owl:versionInfo>http://www.isocat.org/datcat/DC-1425</owl:versionInfo>
    </owl:Class>
    


    <!-- http://purl.org/olia/olia-top.owl#MorphologicalProcess -->

    <owl:Class rdf:about="http://purl.org/olia/olia-top.owl#MorphologicalProcess">
        <rdfs:subClassOf rdf:resource="http://purl.org/olia/olia-top.owl#LinguisticConcept"/>
        <rdfs:label xml:lang="en">morphological process</rdfs:label>
    </owl:Class>
    


    <!-- http://purl.org/olia/olia-top.owl#MorphosyntacticCategory -->

    <owl:Class rdf:about="http://purl.org/olia/olia-top.owl#MorphosyntacticCategory">
        <owl:equivalentClass rdf:resource="http://purl.org/olia/olia-top.owl#Word"/>
        <rdfs:subClassOf rdf:resource="http://purl.org/olia/olia-top.owl#LinguisticConcept"/>
        <rdfs:comment>partOfSpeech: Term used to describe how a particular word is used in a sentence. (http://www.isocat.org/datcat/DC-1345)</rdfs:comment>
        <rdfs:isDefinedBy>http://www.isocat.org/datcat/DC-1345</rdfs:isDefinedBy>
        <rdfs:label>morphosyntactic category</rdfs:label>
        <rdfs:label xml:lang="en">morphosyntactic category</rdfs:label>
        <rdfs:label>part of speech</rdfs:label>
        <owl:versionInfo>&quot;extended&quot; EAGLES

- saubere Definitionen statt form-basierter Zusammenlegung von Kategorien

- VerbalNoun in der Schnittmenge von NonfiniteVerb und CommonNoun
- Classifier zunächst als top-level-konzept
- AuxiliaryVerb aufgespalten in StrictAuxiliarVerb, ModalVerb, Copula
- neues Konzept Quantifier, da jedoch eher semantisch als syntaktisch definiert, mit Numeral zu einem neuen top-level-node zusammengefasst (entsprechend die Definbition bei Bußmann: Quantor enthält ausdrücklich Numerale, diverse Determinierer und Pronomen)
  
  =&gt; sfb:PRONQUANT -&gt; eagles:Quantifier &amp; eagles:PronounOrDeterminer &amp; !eagles:Numeral
     sfb:PRONQUANT_AT -&gt; eagles:Quantifier &amp; eagles:IndefiniteDeterminer &amp; !eagles:Numeral
     sfb:PRONQUANT_SU -&gt; eagles:Quantifier &amp; eagles:IndefinitePronoun &amp; !eagles:Numeral
  =&gt; Numeral als Subkonzept von Quantifier</owl:versionInfo>
        <owl:versionInfo>TODO: saubere definition statt form-baseierten kategorien</owl:versionInfo>
    </owl:Class>
    


    <!-- http://purl.org/olia/olia-top.owl#MorphosyntacticFeature -->

    <owl:Class rdf:about="http://purl.org/olia/olia-top.owl#MorphosyntacticFeature">
        <rdfs:subClassOf rdf:resource="http://purl.org/olia/olia-top.owl#LinguisticConcept"/>
        <rdfs:subClassOf rdf:resource="http://purl.org/olia/system.owl#Feature"/>
        <rdfs:comment>Morphosyntactic and morphological features.</rdfs:comment>
        <rdfs:label xml:lang="en">morphosyntactic feature</rdfs:label>
    </owl:Class>
    


    <!-- http://purl.org/olia/olia-top.owl#MovementFeature -->

    <owl:Class rdf:about="http://purl.org/olia/olia-top.owl#MovementFeature">
        <rdfs:subClassOf rdf:resource="http://purl.org/olia/olia-top.owl#SyntacticFeature"/>
        <rdfs:comment>
		In generative grammar, syntactic alternations of semantically equivalent utterances are explained by movement operations.
		Even though alternative analyses have been proposed, we keep this conventional term to account for syntactic phenomena such as Raising and Control.
	</rdfs:comment>
        <rdfs:label xml:lang="en">movement feature</rdfs:label>
        <owl:versionInfo>Introduced as part of the lexinfo extension as a cover term for Raising and Control properties of (lexical entries of) syntactic verbs.</owl:versionInfo>
    </owl:Class>
    


    <!-- http://purl.org/olia/olia-top.owl#NarrativeType -->

    <owl:Class rdf:about="http://purl.org/olia/olia-top.owl#NarrativeType">
        <rdfs:subClassOf rdf:resource="http://purl.org/olia/olia-top.owl#PragmaticFeature"/>
        <rdfs:label xml:lang="en">narrative type</rdfs:label>
    </owl:Class>
    


    <!-- http://purl.org/olia/olia-top.owl#NullElement -->

    <owl:Class rdf:about="http://purl.org/olia/olia-top.owl#NullElement">
        <rdfs:subClassOf rdf:resource="http://purl.org/olia/olia-top.owl#SyntacticCategory"/>
        <rdfs:comment>Modelled like tokens, Santorini (1991, Â§4.2), Bies (1995, Â§2.3, Â§2.5)</rdfs:comment>
        <rdfs:label xml:lang="en">null element</rdfs:label>
        <owl:versionInfo>added in accordance with PTB bracketing guidelines ,Santorini (1991, Â§4.2), Bies (1995, Â§2.3, Â§2.5)</owl:versionInfo>
    </owl:Class>
    


    <!-- http://purl.org/olia/olia-top.owl#NumberFeature -->

    <owl:Class rdf:about="http://purl.org/olia/olia-top.owl#NumberFeature">
        <rdfs:subClassOf rdf:resource="http://purl.org/olia/olia-top.owl#AgreementFeature"/>
        <rdfs:comment>
            Grammatical category for the variation in form of nouns, pronouns, and any words agreeing 
			with them, depending on how many persons or things are referred to.
            (www.wordreference.com/English/definition.asp?en=number 12; http://www.isocat.org/datcat/DC-1298)

			A grammatical number is a morphological category characterized by the expression of quantity 
			through inflection or agreement. (http://en.wikipedia.org/wiki/Grammatical_number  17.11.06)</rdfs:comment>
        <rdfs:label xml:lang="en">number feature</rdfs:label>
        <owl:versionInfo>http://www.isocat.org/datcat/DC-1298</owl:versionInfo>
    </owl:Class>
    


    <!-- http://purl.org/olia/olia-top.owl#NumeralAgreementClass -->

    <owl:Class rdf:about="http://purl.org/olia/olia-top.owl#NumeralAgreementClass">
        <rdfs:subClassOf rdf:resource="http://purl.org/olia/olia-top.owl#AgreementFeature"/>
        <rdfs:comment>In most Slavic languages, Numerals and Quantifiers involve specific agreement patterns, e.g., in Russian:&lt;br/&gt;
      
      (a) SingularQuantifier (MTE v4: Numeral/Class=&quot;definite1&quot;): requires noun in nominative singular, e.g., один год &quot;one year&quot;
      (b) PaucalQuantifier (MTE v4: Numeral/Class=&quot;definite234&quot;): requires noun in genitive singular, e.g., два/три/четыре года &quot;two/three/four years&quot;
      (c) PluralQuantifier (MTE v4: Numeral/Class=&quot;definite&quot;):requires noun in genitive plural, e.g., пять/много/сколько/столько лет &quot;five/many/how many/that many years&quot;&lt;br/&gt;
      
      Bulgarian has done away with the distinction between 4 and 5, and generalised the 2-4 form to all numerals (and some other quantifiers), but the others generally keep it.  Also Slovene has a living dual (both Sorbians likewise, but they haven&apos;t been MTEd).&lt;br/&gt;
      
      Some Czech feminine and neuter body parts have preserved dual forms, and if the noun is dual, so are its attributes (adjectives, pronouns).  So 2 differs formally from 3-4. The corresponding agreement pattern is a DualQuantifier (MTE v4: Numeral/Class=&quot;definite2&quot;).
      (Ivan A. Derzhanski &amp; Christian Chiarcos, http://purl.org/olia/mte/multext-east.owl#NumeralAgreementClass)</rdfs:comment>
        <rdfs:label xml:lang="en">numeral agreement class</rdfs:label>
        <owl:versionInfo>http://purl.org/olia/mte/multext-east.owl#NumeralAgreementClass</owl:versionInfo>
    </owl:Class>
    


    <!-- http://purl.org/olia/olia-top.owl#OrthographicEntity -->

    <owl:Class rdf:about="http://purl.org/olia/olia-top.owl#OrthographicEntity">
        <rdfs:subClassOf rdf:resource="http://purl.org/olia/olia-top.owl#LinguisticConcept"/>
        <rdfs:label xml:lang="en">orthographic entity</rdfs:label>
        <owl:versionInfo>introduced to account for DCR space, etc.</owl:versionInfo>
    </owl:Class>
    


    <!-- http://purl.org/olia/olia-top.owl#PersonFeature -->

    <owl:Class rdf:about="http://purl.org/olia/olia-top.owl#PersonFeature">
        <rdfs:subClassOf rdf:resource="http://purl.org/olia/olia-top.owl#AgreementFeature"/>
        <rdfs:comment>The grammatical person is deictic reference to the participant role of a referent, such as the speaker, the addressee, and others. Grammatical person typically defines a language&apos;s set of personal pronouns. It also frequently affects verbs, sometimes nouns, and possessive relationships as well. (http://en.wikipedia.org/wiki/Grammatical_person  17.11.06)
	
	Indication of grammatical person (1st, 2nd, 3rd, etc.) associated with a given inflected form.
    (ISO12620; http://www.isocat.org/datcat/DC-1328)
    </rdfs:comment>
        <rdfs:label xml:lang="en">person feature</rdfs:label>
    </owl:Class>
    


    <!-- http://purl.org/olia/olia-top.owl#PhonologicalProcess -->

    <owl:Class rdf:about="http://purl.org/olia/olia-top.owl#PhonologicalProcess">
        <rdfs:subClassOf rdf:resource="http://purl.org/olia/olia-top.owl#LinguisticConcept"/>
        <rdfs:label xml:lang="en">phonological process</rdfs:label>
    </owl:Class>
    


    <!-- http://purl.org/olia/olia-top.owl#PolarityFeature -->

    <owl:Class rdf:about="http://purl.org/olia/olia-top.owl#PolarityFeature">
        <rdfs:subClassOf rdf:resource="http://purl.org/olia/olia-top.owl#SemanticFeature"/>
        <rdfs:label xml:lang="en">polarity feature</rdfs:label>
    </owl:Class>
    


    <!-- http://purl.org/olia/olia-top.owl#PragmaticFeature -->

    <owl:Class rdf:about="http://purl.org/olia/olia-top.owl#PragmaticFeature">
        <rdfs:subClassOf rdf:resource="http://purl.org/olia/olia-top.owl#LinguisticConcept"/>
        <rdfs:subClassOf rdf:resource="http://purl.org/olia/system.owl#Feature"/>
        <dct:replaces></dct:replaces>
        <rdfs:comment></rdfs:comment>
        <rdfs:label xml:lang="en">discourse feature</rdfs:label>
        <owl:versionInfo>has been renamed from &quot;discourse feature&quot; to &quot;pragmatic feature&quot; in the process of integrating the OLiA Discourse Extensions into the OLiA Reference Model, adopting OLiA Discourse lingo. In general, &quot;pragmatic feature&quot; is considered to be broader and to encompass discourse phenomena, as well. In the 2010 OLiA Discourse extensions, a difference was made between &quot;pragmatic relations&quot; (encompassing anaphoric relations, bridging, etc.) and &quot;discourse relation&quot; (a subclass of pragmatic relation concerned exclusively with aspects of discourse structure)</owl:versionInfo>
    </owl:Class>
    


    <!-- http://purl.org/olia/olia-top.owl#PragmaticRelation -->

    <owl:Class rdf:about="http://purl.org/olia/olia-top.owl#PragmaticRelation">
        <rdfs:subClassOf rdf:resource="http://purl.org/olia/olia-top.owl#LinguisticConcept"/>
        <rdfs:subClassOf rdf:resource="http://purl.org/olia/olia-top.owl#Relation"/>
    </owl:Class>
    


    <!-- http://purl.org/olia/olia-top.owl#PragmaticUnit -->

    <owl:Class rdf:about="http://purl.org/olia/olia-top.owl#PragmaticUnit">
        <rdfs:subClassOf rdf:resource="http://purl.org/olia/olia-top.owl#LinguisticConcept"/>
    </owl:Class>
    


    <!-- http://purl.org/olia/olia-top.owl#ProximityFeature -->

    <owl:Class rdf:about="http://purl.org/olia/olia-top.owl#ProximityFeature">
        <rdfs:subClassOf rdf:resource="http://purl.org/olia/olia-top.owl#MorphosyntacticFeature"/>
        <rdfs:comment>In many Indo-European languages, proximity is a relevant feature of pronominal systems (e.g., Macedonian proximal vs. distal determiners, cf. English this vs. that). 
      In several indigeneous languages of North America, proximity is represented by verbal agreement (then also known as obviation, e.g., Blackfoot third [proximal] and &quot;fourth&quot; [distal 3rd] person).
      As defined here, proximity is considered a morphosyntactic feature, because it applies to morphosyntactic *markers* of proximity.
      (Chiarcos)
    </rdfs:comment>
        <rdfs:label>distance</rdfs:label>
        <rdfs:label>obviation</rdfs:label>
        <rdfs:label>proximity</rdfs:label>
        <rdfs:label xml:lang="en">proximity feature</rdfs:label>
        <owl:versionInfo>distinguishes for distal and proximal determiners, e.g., in Macedonian (MULTEXT-East, see http://purl.org/olia/mte/multext-east.owl#CliticDistalDeterminer and http://purl.org/olia/mte/multext-east.owl#CliticProximalDeterminer)</owl:versionInfo>
    </owl:Class>
    


    <!-- http://purl.org/olia/olia-top.owl#ReduplicationTypeFeature -->

    <owl:Class rdf:about="http://purl.org/olia/olia-top.owl#ReduplicationTypeFeature">
        <rdfs:subClassOf rdf:resource="http://purl.org/olia/olia-top.owl#MorphologicalFeature"/>
        <rdfs:comment>
                            type of reduplication
                                (http://www.isocat.org/datcat/DC-2240)
                            </rdfs:comment>
        <rdfs:label>reduplication type</rdfs:label>
        <rdfs:label xml:lang="en">reduplication type feature</rdfs:label>
        <owl:versionInfo>http://www.isocat.org/datcat/DC-2240 (reduplication type, no values given)</owl:versionInfo>
    </owl:Class>
    


    <!-- http://purl.org/olia/olia-top.owl#ReferentTypeFeature -->

    <owl:Class rdf:about="http://purl.org/olia/olia-top.owl#ReferentTypeFeature">
        <rdfs:subClassOf rdf:resource="http://purl.org/olia/olia-top.owl#PragmaticFeature"/>
        <rdfs:comment>
                            Type of concrete object or concept (the referent) that an expression represents (the reference).
                                (DFKI; http://www.isocat.org/datcat/DC-1376)
                            </rdfs:comment>
        <rdfs:label>referent type</rdfs:label>
        <rdfs:label xml:lang="en">referent type feature</rdfs:label>
        <owl:versionInfo>http://www.isocat.org/datcat/DC-1376 (referent type)</owl:versionInfo>
    </owl:Class>
    


    <!-- http://purl.org/olia/olia-top.owl#ReflexivityFeature -->

    <owl:Class rdf:about="http://purl.org/olia/olia-top.owl#ReflexivityFeature">
        <rdfs:subClassOf rdf:resource="http://purl.org/olia/olia-top.owl#MorphosyntacticFeature"/>
        <rdfs:comment>The optional attribute Reflexivity is applied to main verbs in French, German, Dutch, etc., and determines the selection of &quot;avoir&quot; or &quot;être&quot;, etc., as auxiliary for the Perfect. 
(http://www.ilc.cnr.it/EAGLES96/annotate/node18.html#oav1c 15.11.06)</rdfs:comment>
        <rdfs:label xml:lang="en">reflexivity feature</rdfs:label>
    </owl:Class>
    


    <!-- http://purl.org/olia/olia-top.owl#RegisterFeature -->

    <owl:Class rdf:about="http://purl.org/olia/olia-top.owl#RegisterFeature">
        <rdfs:subClassOf rdf:resource="http://purl.org/olia/olia-top.owl#PragmaticFeature"/>
        <rdfs:comment>
                            Classification indicating the relative level of language individually assigned to a lexeme or term or to a text type.
                                (ISO12620; http://www.isocat.org/datcat/DC-1988)
                            </rdfs:comment>
        <rdfs:label>register</rdfs:label>
        <rdfs:label xml:lang="en">register feature</rdfs:label>
        <owl:versionInfo>http://www.isocat.org/datcat/DC-1988</owl:versionInfo>
    </owl:Class>
    


    <!-- http://purl.org/olia/olia-top.owl#Relation -->

    <owl:Class rdf:about="http://purl.org/olia/olia-top.owl#Relation"/>
    


    <!-- http://purl.org/olia/olia-top.owl#SemanticFeature -->

    <owl:Class rdf:about="http://purl.org/olia/olia-top.owl#SemanticFeature">
        <rdfs:subClassOf rdf:resource="http://purl.org/olia/olia-top.owl#LinguisticConcept"/>
        <rdfs:subClassOf rdf:resource="http://purl.org/olia/system.owl#Feature"/>
        <rdfs:comment></rdfs:comment>
        <rdfs:label xml:lang="en">semantic feature</rdfs:label>
    </owl:Class>
    


    <!-- http://purl.org/olia/olia-top.owl#SemanticRole -->

    <owl:Class rdf:about="http://purl.org/olia/olia-top.owl#SemanticRole">
        <rdfs:subClassOf rdf:resource="http://purl.org/olia/olia-top.owl#SemanticFeature"/>
        <rdfs:comment>
        In linguistics, a theta role or θ-role is the semantic role a noun 
        phrase plays in a sentence. The term Thematic role denotes the same 
        concept. As such it is a semantic rather than a syntactic feature, in 
        contrast to such notions as the subject of a sentence or a 
        prepositional object. 
        (http://en.wikipedia.org/wiki/Subject_(linguistics).
		
		Originally, semantic roles were referred to as &quot;case roles&quot;, leading to
		an unfortunate name clash with grammatical case (e.g. in GOLD CaseValue)
	</rdfs:comment>
        <rdfs:label xml:lang="en">semantic role</rdfs:label>
    </owl:Class>
    


    <!-- http://purl.org/olia/olia-top.owl#SemanticUnit -->

    <owl:Class rdf:about="http://purl.org/olia/olia-top.owl#SemanticUnit">
        <rdfs:subClassOf rdf:resource="http://purl.org/olia/olia-top.owl#LinguisticConcept"/>
        <rdfs:label xml:lang="en">semantic unit</rdfs:label>
    </owl:Class>
    


    <!-- http://purl.org/olia/olia-top.owl#SentenceTypeFeature -->

    <owl:Class rdf:about="http://purl.org/olia/olia-top.owl#SentenceTypeFeature">
        <rdfs:subClassOf rdf:resource="http://purl.org/olia/olia-top.owl#SyntacticFeature"/>
        <rdfs:label xml:lang="en">sentence type feature</rdfs:label>
        <owl:versionInfo>classification of sentences according to their function, e.g., illocutionary act</owl:versionInfo>
    </owl:Class>
    


    <!-- http://purl.org/olia/olia-top.owl#SeparabilityFeature -->

    <owl:Class rdf:about="http://purl.org/olia/olia-top.owl#SeparabilityFeature">
        <rdfs:subClassOf rdf:resource="http://purl.org/olia/olia-top.owl#MorphologicalFeature"/>
        <rdfs:comment>The optional Eagles attribute Separability is relevant for German compound verbs (&quot;fängt ...an&quot;, &quot;anfangen&quot;) and also to phrasal verbs in Danish and English. 
(http://www.ilc.cnr.it/EAGLES96/annotate/node18.html#oav1c 15.11.06)</rdfs:comment>
        <rdfs:label xml:lang="en">separability feature</rdfs:label>
    </owl:Class>
    


    <!-- http://purl.org/olia/olia-top.owl#SpecificityFeature -->

    <owl:Class rdf:about="http://purl.org/olia/olia-top.owl#SpecificityFeature">
        <rdfs:subClassOf rdf:resource="http://purl.org/olia/olia-top.owl#MorphosyntacticFeature"/>
        <rdfs:comment>
      &quot;By ʻspecificʼ and ʻnon-specificʼ I intend the difference between the
      two readings of English indefinites like (3):
      
      (3) Iʼm looking for a deer.
      
      In the specific reading there is a particular deer, say Bambi, that I am
      looking for. In the non-specific reading I will be happy to find any deer.
      Von Heusinger (2002) likes the test in English of inserting ʻcertainʼ after the
      ʻaʼ to fix the specific reading. In either reading of (3) a deer is being
      introduced as a new discourse referent. This is opposed to ʻdefiniteʼ which
      requires a previous pragmatic instantiation as in ʻIʼm looking for the deer.ʼ
      In English both the readings of (3) are indefinite. In Klallam, the specific
      demonstratives are neither definite nor indefinite.&quot;
      (Montler, Timothy. 2007. Klallam demonstratives. Papers ICSNL XLVII. The 42nd International Conference on Salish and Neighbouring Language, pp. 409-425. University of British Columbia Working Papers in Linguistics, Volume 20; on specific vs. nonspecific determiners in Klallam, a Salish language, http://montler.net/papers/KlallamDemons.pdf)
    </rdfs:comment>
        <rdfs:label>genericity</rdfs:label>
        <rdfs:label>specificity</rdfs:label>
        <rdfs:label xml:lang="en">specificity feature</rdfs:label>
        <owl:versionInfo>distinguishes specific and nonspecific determiners, e.g., in Klallam (Salish, see olia:SpecificArticle, olia:NonspecificArticle), or in Persian (http://purl.org/olia/mte/multext-east.owl#CliticSpecificDeterminer)</owl:versionInfo>
    </owl:Class>
    


    <!-- http://purl.org/olia/olia-top.owl#StrengthFeature -->

    <owl:Class rdf:about="http://purl.org/olia/olia-top.owl#StrengthFeature">
        <rdfs:subClassOf rdf:resource="http://purl.org/olia/olia-top.owl#MorphologicalFeature"/>
        <rdfs:label xml:lang="en">strength feature</rdfs:label>
        <owl:versionInfo>In EAGLES, Strength is a language-specific attribute for pronouns and determiners to characterize weak (reduced) and strong (full) forms (http://www.ilc.cnr.it/EAGLES96/annotate/node19.html#oav2av  20.11.06).
      Here, it is extended to full and reduced adjective inflection in Slavic languages (cf. MULTEXT-East). May be renamed to ReductionFeature.</owl:versionInfo>
    </owl:Class>
    


    <!-- http://purl.org/olia/olia-top.owl#SubordTypeFeature -->

    <owl:Class rdf:about="http://purl.org/olia/olia-top.owl#SubordTypeFeature">
        <rdfs:subClassOf rdf:resource="http://purl.org/olia/olia-top.owl#MorphosyntacticFeature"/>
        <rdfs:comment>The SubordType is in Eagles an additional language-specific attribute, applying to subordinating conjunctions only.  (http://www.ilc.cnr.it/EAGLES96/annotate/node19.html#oav2u  17.11.06)</rdfs:comment>
        <rdfs:label xml:lang="en">subord type feature</rdfs:label>
        <owl:deprecated rdf:datatype="http://www.w3.org/2001/XMLSchema#boolean">true</owl:deprecated>
        <owl:versionInfo>Deprecated: reimplemented within SubordinatingConjunction taxonomy</owl:versionInfo>
    </owl:Class>
    


    <!-- http://purl.org/olia/olia-top.owl#SyntacticCategory -->

    <owl:Class rdf:about="http://purl.org/olia/olia-top.owl#SyntacticCategory">
        <rdfs:subClassOf rdf:resource="http://purl.org/olia/olia-top.owl#LinguisticConcept"/>
        <rdfs:label xml:lang="en">syntactic category</rdfs:label>
    </owl:Class>
    


    <!-- http://purl.org/olia/olia-top.owl#SyntacticConstruction -->

    <owl:Class rdf:about="http://purl.org/olia/olia-top.owl#SyntacticConstruction">
        <rdfs:subClassOf rdf:resource="http://purl.org/olia/olia-top.owl#SyntacticCategory"/>
        <rdfs:comment>Syntactic constructions that involve multiple constituents, or that are independent of the concept of constituent, e.g., word order phenomena, non-canonical sentences , ...</rdfs:comment>
        <rdfs:label xml:lang="en">syntactic construction</rdfs:label>
    </owl:Class>
    


    <!-- http://purl.org/olia/olia-top.owl#SyntacticFeature -->

    <owl:Class rdf:about="http://purl.org/olia/olia-top.owl#SyntacticFeature">
        <rdfs:subClassOf rdf:resource="http://purl.org/olia/olia-top.owl#LinguisticConcept"/>
        <rdfs:subClassOf rdf:resource="http://purl.org/olia/system.owl#Feature"/>
        <rdfs:label xml:lang="en">syntactic feature</rdfs:label>
    </owl:Class>
    


    <!-- http://purl.org/olia/olia-top.owl#SyntacticFunction -->

    <owl:Class rdf:about="http://purl.org/olia/olia-top.owl#SyntacticFunction">
        <rdfs:subClassOf rdf:resource="http://purl.org/olia/olia-top.owl#SyntacticFeature"/>
        <rdfs:comment>
			Relation to be used when the syntactic function of a constituent is different from its morphosyntactic type, 
			cf. FormFunctionDiscrepancy in the PTB bracketing guidelines, Bies et al. (1995, §2.2.1)
		</rdfs:comment>
        <rdfs:label xml:lang="en">syntactic function</rdfs:label>
        <owl:versionInfo>Bies et al 1995</owl:versionInfo>
    </owl:Class>
    


    <!-- http://purl.org/olia/olia-top.owl#SyntacticRelation -->

    <owl:Class rdf:about="http://purl.org/olia/olia-top.owl#SyntacticRelation">
        <rdfs:subClassOf rdf:resource="http://purl.org/olia/olia-top.owl#LinguisticConcept"/>
        <rdfs:label xml:lang="en">syntactic relation</rdfs:label>
    </owl:Class>
    


    <!-- http://purl.org/olia/olia-top.owl#SyntacticRole -->

    <owl:Class rdf:about="http://purl.org/olia/olia-top.owl#SyntacticRole">
        <rdfs:subClassOf rdf:resource="http://purl.org/olia/olia-top.owl#SyntacticFeature"/>
        <rdfs:comment>Traditionally, &quot;grammatical relations&quot; or &quot;grammatical roles&quot; are specifically those between the verb (clause) and its arguments/adjunct/complementizer.
      In modern corpus research, however, a broad variety of relations between nominal heads, their arguments, modifiers, etc. are distinguished and the scope of &quot;Grammatical Relation&quot; has extended here to cover these as well.
      (http://purl.org/linguistics/gold/syntacticRole)</rdfs:comment>
        <rdfs:label xml:lang="en">syntactic role</rdfs:label>
    </owl:Class>
    


    <!-- http://purl.org/olia/olia-top.owl#TenseFeature -->

    <owl:Class rdf:about="http://purl.org/olia/olia-top.owl#TenseFeature">
        <rdfs:subClassOf rdf:resource="http://purl.org/olia/olia-top.owl#MorphosyntacticFeature"/>
        <rdfs:comment>verb tense: property referring to the way the grammar marks (via affixes and/or suppletion) the time at which the action denoted by the verb took place. (http://www.isocat.org/datcat/DC-4964)
	  
	  Tense is a grammatical category, typically marked on the verb, that deictically refers to the time of the event or state denoted by the verb in relation to some other temporal reference point. (http://www.sil.org/linguistics/glossaryoflinguisticterms/WhatIsTense.htm  17.11.06)</rdfs:comment>
        <rdfs:isDefinedBy>http://www.isocat.org/datcat/DC-4964</rdfs:isDefinedBy>
        <rdfs:label>tense</rdfs:label>
        <rdfs:label xml:lang="en">tense feature</rdfs:label>
        <rdfs:label>verb tense</rdfs:label>
    </owl:Class>
    


    <!-- http://purl.org/olia/olia-top.owl#TextStructuralUnit -->

    <owl:Class rdf:about="http://purl.org/olia/olia-top.owl#TextStructuralUnit">
        <rdfs:subClassOf rdf:resource="http://purl.org/olia/olia-top.owl#LinguisticConcept"/>
    </owl:Class>
    


    <!-- http://purl.org/olia/olia-top.owl#TopologicalField -->

    <owl:Class rdf:about="http://purl.org/olia/olia-top.owl#TopologicalField">
        <rdfs:subClassOf rdf:resource="http://purl.org/olia/olia-top.owl#SyntacticCategory"/>
        <rdfs:label xml:lang="en">topological field</rdfs:label>
    </owl:Class>
    


    <!-- http://purl.org/olia/olia-top.owl#UsageAndFrequencyFeature -->

    <owl:Class rdf:about="http://purl.org/olia/olia-top.owl#UsageAndFrequencyFeature">
        <rdfs:subClassOf rdf:resource="http://purl.org/olia/olia-top.owl#PragmaticFeature"/>
        <rdfs:comment>
			Frequency: The relative commonness with which a term occurs.
            (ISO12620; http://www.isocat.org/datcat/DC-1965)
            
			Dating: Indication specifying whether the usage is old or modern.
            (http://www.isocat.org/datcat/DC-1959)
	  </rdfs:comment>
        <rdfs:label xml:lang="en">usage and frequency feature</rdfs:label>
        <owl:versionInfo>http://www.isocat.org/datcat/DC-1965 (frequency), http://www.isocat.org/datcat/DC-1959 (dating)</owl:versionInfo>
    </owl:Class>
    


    <!-- http://purl.org/olia/olia-top.owl#ValencyFeature -->

    <owl:Class rdf:about="http://purl.org/olia/olia-top.owl#ValencyFeature">
        <rdfs:subClassOf rdf:resource="http://purl.org/olia/olia-top.owl#SyntacticFeature"/>
        <rdfs:comment>
		Syntactic valency pertains to the number of syntactic arguments a verb requires. 
		Semantic valency pertains to the number of arguments of a semantic predicate.
		If syntactic valency is greater than the semantic valency, an expletive pronoun may be used, 
		cf. van Valin and LaPolla (1997) on the distinction between syntactic valency and semantic valency.
	</rdfs:comment>
        <rdfs:label xml:lang="en">valency feature</rdfs:label>
        <owl:versionInfo>EAGLES</owl:versionInfo>
    </owl:Class>
    


    <!-- http://purl.org/olia/olia-top.owl#VoiceFeature -->

    <owl:Class rdf:about="http://purl.org/olia/olia-top.owl#VoiceFeature">
        <rdfs:subClassOf rdf:resource="http://purl.org/olia/olia-top.owl#SyntacticFeature"/>
        <rdfs:comment>The voice of a verb describes the relationship between the action (or state) that the verb expresses and the participants identified by its arguments (subject, object, etc.). (http://en.wikipedia.org/wiki/Grammatical_voice  17.11.06)</rdfs:comment>
        <rdfs:label xml:lang="en">voice feature</rdfs:label>
        <owl:versionInfo>2024-11-22 redefined as SyntacticFeature (was MorphoyntacticFeature)</owl:versionInfo>
    </owl:Class>
    


    <!-- http://purl.org/olia/olia-top.owl#Word -->

    <owl:Class rdf:about="http://purl.org/olia/olia-top.owl#Word">
        <rdfs:subClassOf rdf:resource="http://purl.org/olia/olia-top.owl#SyntacticCategory"/>
        <rdfs:comment>
		SyntacticWord is the class of syntactic units occupying the lowest position in 
		a syntactic construction. They are the largest units resistant to insertion of 
		new constituents within their boundaries; or they are the smallest constituents 
		that can be moved within a sentence without making the sentence ungrammatical.
		(http://www.linguistics-ontology.org/gold/2008/SyntacticWord)
		
		Linguistic unit composed of at least a part of speech and a lemma.
        (Gil Francopoulo; http://www.isocat.org/datcat/DC-1415)
	</rdfs:comment>
        <rdfs:comment>Terminal nodes of syntactic annotations, termed &quot;Word&quot; here, are the same structural entities that are subject to morphosyntactic (Part of Speech) annotations.
		
		cf. http://www.isocat.org/datcat/DC-1415 &quot;word&quot;: Linguistic unit composed of at least a part of speech and a lemma.</rdfs:comment>
        <rdfs:isDefinedBy>http://www.isocat.org/datcat/DC-1415</rdfs:isDefinedBy>
        <rdfs:label>word</rdfs:label>
        <rdfs:label xml:lang="en">word</rdfs:label>
        <owl:versionInfo>http://www.isocat.org/datcat/DC-1415, cf. GOLD SyntacticWord</owl:versionInfo>
    </owl:Class>
    


    <!-- http://purl.org/olia/system.owl#Feature -->

    <owl:Class rdf:about="http://purl.org/olia/system.owl#Feature"/>
</rdf:RDF>



<!-- Generated by the OWL API (version 4.5.25.2023-02-15T19:15:49Z) https://github.com/owlcs/owlapi -->

