<?xml version="1.0"?>
<rdf:RDF xmlns="http://purl.org/olia/system.owl#"
     xml:base="http://purl.org/olia/system.owl"
     xmlns:dct="http://purl.org/dc/terms/"
     xmlns:owl="http://www.w3.org/2002/07/owl#"
     xmlns:rdf="http://www.w3.org/1999/02/22-rdf-syntax-ns#"
     xmlns:xml="http://www.w3.org/XML/1998/namespace"
     xmlns:xsd="http://www.w3.org/2001/XMLSchema#"
     xmlns:rdfs="http://www.w3.org/2000/01/rdf-schema#"
     xmlns:olia_system="http://purl.org/olia/system.owl#">
    <owl:Ontology rdf:about="http://purl.org/olia/system.owl">
        <dct:license rdf:resource="https://creativecommons.org/licenses/by/3.0/"/>
        <rdfs:comment>OLiA core concepts for linguistic annotations.</rdfs:comment>
        <owl:versionInfo xml:lang="uni-potsdam.de">
      2008-01-13 created
      2010-04-06 removed deprecated Category (equiv UnitOfAnnotation) category
      2010-04-14 added AnnotationProcess (cf. DCR process directory)
      2011-07-15 replaced base url by purl
      2011-07-27 added hasTagMatching with full support for XSLT-style regular expressions
      2013-06-27 added ISOcat reference for LinguisticAnnotation
      2022-05-23 rdfs:labels added (automatically)	  

      Christian Chiarcos, chiarcos</owl:versionInfo>
        <owl:versionInfo>TODO: LinguisticAnnotation disjoint</owl:versionInfo>
    </owl:Ontology>
    


    <!-- 
    ///////////////////////////////////////////////////////////////////////////////////////
    //
    // Annotation properties
    //
    ///////////////////////////////////////////////////////////////////////////////////////
     -->

    


    <!-- http://purl.org/dc/terms/license -->

    <owl:AnnotationProperty rdf:about="http://purl.org/dc/terms/license"/>
    


    <!-- 
    ///////////////////////////////////////////////////////////////////////////////////////
    //
    // Object Properties
    //
    ///////////////////////////////////////////////////////////////////////////////////////
     -->

    


    <!-- http://purl.org/olia/system.owl#hasFeature -->

    <owl:ObjectProperty rdf:about="http://purl.org/olia/system.owl#hasFeature">
        <rdfs:domain rdf:resource="http://purl.org/olia/system.owl#LinguisticAnnotation"/>
        <rdfs:range rdf:resource="http://purl.org/olia/system.owl#Feature"/>
        <rdfs:comment>A UnitOfAnnotation or a Relation can carry Features that express annotations attached to them. By convention, (tags that represent) Features can be linked with Feature individuals, as well. Because of this reflexivity, a predicate like hasDegree(positive) allows to retrieve the individual positive as well. (This is necessary if positive represents a tag on its own, rather than being a property of a complex tag.)</rdfs:comment>
        <rdfs:label xml:lang="en">has feature</rdfs:label>
    </owl:ObjectProperty>
    


    <!-- http://purl.org/olia/system.owl#hasSource -->

    <owl:ObjectProperty rdf:about="http://purl.org/olia/system.owl#hasSource">
        <rdfs:domain rdf:resource="http://purl.org/olia/system.owl#Relation"/>
        <rdfs:range rdf:resource="http://purl.org/olia/system.owl#UnitOfAnnotation"/>
        <rdfs:comment>A Relation is a directed edge between a source and a target concept.</rdfs:comment>
        <rdfs:label xml:lang="en">has source</rdfs:label>
    </owl:ObjectProperty>
    


    <!-- http://purl.org/olia/system.owl#hasTarget -->

    <owl:ObjectProperty rdf:about="http://purl.org/olia/system.owl#hasTarget">
        <rdfs:domain rdf:resource="http://purl.org/olia/system.owl#Relation"/>
        <rdfs:range rdf:resource="http://purl.org/olia/system.owl#UnitOfAnnotation"/>
        <rdfs:comment>A Relation is a directed edge between a source and a target concept.</rdfs:comment>
        <rdfs:label xml:lang="en">has target</rdfs:label>
    </owl:ObjectProperty>
    


    <!-- 
    ///////////////////////////////////////////////////////////////////////////////////////
    //
    // Data properties
    //
    ///////////////////////////////////////////////////////////////////////////////////////
     -->

    


    <!-- http://purl.org/olia/system.owl#hasTag -->

    <owl:DatatypeProperty rdf:about="http://purl.org/olia/system.owl#hasTag">
        <rdfs:domain rdf:resource="http://purl.org/olia/system.owl#LinguisticAnnotation"/>
        <rdfs:comment>Assigns a Linguistic Annotation a String representation, e.g., a particular Part of Speech tag, the respective abbreviation of the grammatical cases used in an annotation scheme, etc.
implicit semantics: hasTag is to be used if the tag is equal to the string value, otherwise use hasTagContaining, hasTagStartingWith, hasTagEndingWith</rdfs:comment>
        <rdfs:label xml:lang="en">has tag</rdfs:label>
    </owl:DatatypeProperty>
    


    <!-- http://purl.org/olia/system.owl#hasTagContaining -->

    <owl:DatatypeProperty rdf:about="http://purl.org/olia/system.owl#hasTagContaining">
        <rdfs:subPropertyOf rdf:resource="http://purl.org/olia/system.owl#hasTag"/>
        <rdfs:comment>As opposed to hasTag proper, the string representation defines a substring of a concrete annotation.
The respective linguistic annotation then applies to every element whose annotation (tag) contains this substring.</rdfs:comment>
        <rdfs:label xml:lang="en">has tag containing</rdfs:label>
    </owl:DatatypeProperty>
    


    <!-- http://purl.org/olia/system.owl#hasTagEndingWith -->

    <owl:DatatypeProperty rdf:about="http://purl.org/olia/system.owl#hasTagEndingWith">
        <rdfs:subPropertyOf rdf:resource="http://purl.org/olia/system.owl#hasTag"/>
        <rdfs:comment>As opposed to hasTag proper, the string representation defines the final subsequence of a concrete annotation.
The respective linguistic annotation then applies to every element whose annotation (tag) ends with this substring.</rdfs:comment>
        <rdfs:label xml:lang="en">has tag ending with</rdfs:label>
    </owl:DatatypeProperty>
    


    <!-- http://purl.org/olia/system.owl#hasTagMatching -->

    <owl:DatatypeProperty rdf:about="http://purl.org/olia/system.owl#hasTagMatching">
        <rdfs:subPropertyOf rdf:resource="http://purl.org/olia/system.owl#hasTag"/>
        <rdfs:comment>hasTagMatching is a subproperty of hasTag, so that results can be retrieved if the regular expression match is requested, but an exact value with reserved characters is defined
	</rdfs:comment>
        <rdfs:comment>hasTagMatching allows to provide regular expressions as those used in XSLT and XPath, see http://www.w3.org/TR/xquery-operators/#func-matches</rdfs:comment>
        <rdfs:label xml:lang="en">has tag matching</rdfs:label>
    </owl:DatatypeProperty>
    


    <!-- http://purl.org/olia/system.owl#hasTagStartingWith -->

    <owl:DatatypeProperty rdf:about="http://purl.org/olia/system.owl#hasTagStartingWith">
        <rdfs:subPropertyOf rdf:resource="http://purl.org/olia/system.owl#hasTag"/>
        <rdfs:comment>As opposed to hasTag proper, the string representation specifies only the beginning of a concrete annotation.
The respective linguistic annotation then applies to every element whose annotation (tag) startsWith this substring.</rdfs:comment>
        <rdfs:label xml:lang="en">has tag starting with</rdfs:label>
    </owl:DatatypeProperty>
    


    <!-- http://purl.org/olia/system.owl#hasTier -->

    <owl:DatatypeProperty rdf:about="http://purl.org/olia/system.owl#hasTier">
        <rdfs:domain rdf:resource="http://purl.org/olia/system.owl#LinguisticAnnotation"/>
        <rdfs:comment>Assigns a linguistic annotation a string representation of the annotation layer (&quot;tier&quot;, &quot;level&quot;) where it is to be found, e.g., &quot;pos&quot; for Part of Speech annotation, &quot;gloss&quot; for linguistic glosses, etc.</rdfs:comment>
        <rdfs:label xml:lang="en">has tier</rdfs:label>
    </owl:DatatypeProperty>
    


    <!-- 
    ///////////////////////////////////////////////////////////////////////////////////////
    //
    // Classes
    //
    ///////////////////////////////////////////////////////////////////////////////////////
     -->

    


    <!-- http://purl.org/olia/system.owl#AnnotationProcess -->

    <owl:Class rdf:about="http://purl.org/olia/system.owl#AnnotationProcess">
        <rdfs:label xml:lang="en">annotation process</rdfs:label>
        <owl:versionInfo>DCR annotation and editing operations ignored, e.g., add first vowel  http://www.isocat.org/datcat/DC-2199		 
		</owl:versionInfo>
        <owl:versionInfo>categories for annotation and editing operations added to account for the &quot;Processes&quot; profile in the DCR</owl:versionInfo>
    </owl:Class>
    


    <!-- http://purl.org/olia/system.owl#Feature -->

    <owl:Class rdf:about="http://purl.org/olia/system.owl#Feature">
        <rdfs:subClassOf rdf:resource="http://purl.org/olia/system.owl#LinguisticAnnotation"/>
        <rdfs:comment>UnitsOfAnnotation and Relations can be described in a more detailed way by the features that are attached to them, e.g., case, number, or aspect. Features are, however, not subject to further annotations (by means of hasFeature), they are thus disjoint from Relations and UnitsOfAnnotation.</rdfs:comment>
        <rdfs:label xml:lang="en">feature</rdfs:label>
    </owl:Class>
    


    <!-- http://purl.org/olia/system.owl#LinguisticAnnotation -->

    <owl:Class rdf:about="http://purl.org/olia/system.owl#LinguisticAnnotation">
        <rdfs:comment>label: Text attached to an element</rdfs:comment>
        <rdfs:comment>Linguistic annotations pertain to either structural entities (words, tokens, constituents, sentences =&gt; UnitOfAnnotation), relations between these (dependency, dominance, coreference, etc. =&gt; Relation), or grammatical features attached to these (case, gender, number, agreement, tense, mood, aspect, ... =&gt; Feature).</rdfs:comment>
        <rdfs:isDefinedBy>http://www.isocat.org/datcat/DC-1857</rdfs:isDefinedBy>
        <rdfs:label xml:lang="en">linguistic annotation</rdfs:label>
    </owl:Class>
    


    <!-- http://purl.org/olia/system.owl#Relation -->

    <owl:Class rdf:about="http://purl.org/olia/system.owl#Relation">
        <owl:equivalentClass>
            <owl:Class>
                <owl:unionOf rdf:parseType="Collection">
                    <owl:Restriction>
                        <owl:onProperty rdf:resource="http://purl.org/olia/system.owl#hasSource"/>
                        <owl:minCardinality rdf:datatype="http://www.w3.org/2001/XMLSchema#nonNegativeInteger">1</owl:minCardinality>
                    </owl:Restriction>
                    <owl:Restriction>
                        <owl:onProperty rdf:resource="http://purl.org/olia/system.owl#hasTarget"/>
                        <owl:minCardinality rdf:datatype="http://www.w3.org/2001/XMLSchema#nonNegativeInteger">1</owl:minCardinality>
                    </owl:Restriction>
                </owl:unionOf>
            </owl:Class>
        </owl:equivalentClass>
        <rdfs:subClassOf rdf:resource="http://purl.org/olia/system.owl#LinguisticAnnotation"/>
        <rdfs:subClassOf>
            <owl:Restriction>
                <owl:onProperty rdf:resource="http://purl.org/olia/system.owl#hasSource"/>
                <owl:cardinality rdf:datatype="http://www.w3.org/2001/XMLSchema#nonNegativeInteger">1</owl:cardinality>
            </owl:Restriction>
        </rdfs:subClassOf>
        <rdfs:subClassOf>
            <owl:Restriction>
                <owl:onProperty rdf:resource="http://purl.org/olia/system.owl#hasTarget"/>
                <owl:cardinality rdf:datatype="http://www.w3.org/2001/XMLSchema#nonNegativeInteger">1</owl:cardinality>
            </owl:Restriction>
        </rdfs:subClassOf>
        <rdfs:comment>Between instances of two Categories, a Relation can be established that links these together, e.g., a dominance relation (constituent X is grammatical subject of sentence Y), a dependency relation (token X is a modifier of token Y), a discourse relation (discourse unit X is in contrast to discourse unit Y), an anaphoric relation (referring expression X is coreferent with referring expressing Y), an alignment relation (word X expresses the same meaning as word Y).
Note that Relation and UnitOfAnnotation are not disjoint, because in some approaches, establishing a Relation between two concepts entails that a structural entity is formed, consisting of Relation and the Categories connected by the Relation, e.g., in Rhetorical Structure Theory (Mann and Thompson 1987).</rdfs:comment>
        <rdfs:label xml:lang="en">relation</rdfs:label>
    </owl:Class>
    


    <!-- http://purl.org/olia/system.owl#UnitOfAnnotation -->

    <owl:Class rdf:about="http://purl.org/olia/system.owl#UnitOfAnnotation">
        <rdfs:subClassOf rdf:resource="http://purl.org/olia/system.owl#LinguisticAnnotation"/>
        <rdfs:comment>A UnitOfAnnotation is a structural entity that can be annotated, e.g., a word, token, constituent, or another types of markable.
Word classes, etc., are then modelled as indirect children of UnitOfAnnotation. The division between Features and classes of UnitsOfAnnotation follows conventional standards.
    </rdfs:comment>
        <rdfs:label xml:lang="en">unit of annotation</rdfs:label>
    </owl:Class>
</rdf:RDF>



<!-- Generated by the OWL API (version 4.5.25.2023-02-15T19:15:49Z) https://github.com/owlcs/owlapi -->

