<?xml version="1.0"?>


<!DOCTYPE rdf:RDF [
    <!ENTITY owl "http://www.w3.org/2002/07/owl#" >
    <!ENTITY xsd "http://www.w3.org/2001/XMLSchema#" >
    <!ENTITY rdfs "http://www.w3.org/2000/01/rdf-schema#" >
    <!ENTITY rdf "http://www.w3.org/1999/02/22-rdf-syntax-ns#" >
    <!ENTITY stts "file:/C:/Users/Christian/Desktop/onto/owl/stts.owl#" >
    <!ENTITY system "file:/C:/Users/Christian/Desktop/onto/owl/system.owl#" >
]>


<rdf:RDF xmlns="file:/C:/Users/Christian/Desktop/onto/owl/tueba.owl#"
     xml:base="file:/C:/Users/Christian/Desktop/onto/owl/tueba.owl"
     xmlns:rdfs="http://www.w3.org/2000/01/rdf-schema#"
     xmlns:system="file:/C:/Users/Christian/Desktop/onto/owl/system.owl#"
     xmlns:stts="file:/C:/Users/Christian/Desktop/onto/owl/stts.owl#"
     xmlns:owl="http://www.w3.org/2002/07/owl#"
     xmlns:xsd="http://www.w3.org/2001/XMLSchema#"
     xmlns:rdf="http://www.w3.org/1999/02/22-rdf-syntax-ns#">
    <owl:Ontology rdf:about="file:/C:/Users/Christian/Desktop/onto/owl/tueba.owl">
        <rdfs:comment>Annotation Model of morposyntactic, morphological and syntactic annotations of the T&#252;Ba-D/Z corpus (v5) following Telljohann et al. (2009), unless marked otherwise

Heike Telljohann, Erhard W. Hinrichs, Sandra K&#168;ubler, Heike Zinsmeister, Kathrin Beck (2009),
Stylebook for the T&#168;ubingen Treebank of Written German (T&#168;uBa-D/Z), Tech. rep. Universit&#228;t T&#252;bingen, Seminar f&#252;r Sprachwissenschaft, version of November 2009 (T&#252;Ba-D/Z v5)</rdfs:comment>
        <owl:versionInfo>2007/11/07 implemented first version based upon Telljohann, H. et al. (2006), &quot;Stylebook for the T&#252;bingen Treebank of Written German (T&#252;Ba-D/Z)&quot;, University of T&#252;bingen, version of July 2006. (incomplete, no topological fields)
2008/05/23 update
2010/11/30 re-built for T&#252;Ba-D/Z v5 (Telljohann et al. 2009)
(Only up to p. 26, definitions provided only for the topological field model)

Christian Chiarcos, chiarcos@uni-potsdam.de</owl:versionInfo>
        <owl:imports rdf:resource="file:/C:/Users/Christian/Desktop/onto/owl/stts.owl"/>
    </owl:Ontology>
    


    <!-- 
    ///////////////////////////////////////////////////////////////////////////////////////
    //
    // Annotation properties
    //
    ///////////////////////////////////////////////////////////////////////////////////////
     -->

    <owl:AnnotationProperty rdf:about="&owl;versionInfo"/>
    <owl:AnnotationProperty rdf:about="&rdfs;comment"/>
    


    <!-- 
    ///////////////////////////////////////////////////////////////////////////////////////
    //
    // Object Properties
    //
    ///////////////////////////////////////////////////////////////////////////////////////
     -->

    


    <!-- file:/C:/Users/Christian/Desktop/onto/owl/tueba.owl#hasCase -->

    <owl:ObjectProperty rdf:about="file:/C:/Users/Christian/Desktop/onto/owl/tueba.owl#hasCase">
        <rdfs:range rdf:resource="file:/C:/Users/Christian/Desktop/onto/owl/tueba.owl#Case"/>
        <rdfs:subPropertyOf rdf:resource="file:/C:/Users/Christian/Desktop/onto/owl/tueba.owl#hasMorphologicalFeature"/>
        <rdfs:domain>
            <owl:Class>
                <owl:unionOf rdf:parseType="Collection">
                    <rdf:Description rdf:about="&stts;Article"/>
                    <rdf:Description rdf:about="&stts;AttributiveAdjective"/>
                    <rdf:Description rdf:about="&stts;DemonstrativePronoun"/>
                    <rdf:Description rdf:about="&stts;IndefinitePronoun"/>
                    <rdf:Description rdf:about="&stts;InterrogativePronoun"/>
                    <rdf:Description rdf:about="&stts;Noun"/>
                    <rdf:Description rdf:about="&stts;PersonalPronoun"/>
                    <rdf:Description rdf:about="&stts;PossessivePronoun"/>
                    <rdf:Description rdf:about="&stts;Postposition"/>
                    <rdf:Description rdf:about="&stts;Preposition"/>
                    <rdf:Description rdf:about="&stts;ReflexivePronoun"/>
                    <rdf:Description rdf:about="&stts;RelativePronoun"/>
                </owl:unionOf>
            </owl:Class>
        </rdfs:domain>
    </owl:ObjectProperty>
    


    <!-- file:/C:/Users/Christian/Desktop/onto/owl/tueba.owl#hasGender -->

    <owl:ObjectProperty rdf:about="file:/C:/Users/Christian/Desktop/onto/owl/tueba.owl#hasGender">
        <rdfs:range rdf:resource="file:/C:/Users/Christian/Desktop/onto/owl/tueba.owl#Gender"/>
        <rdfs:subPropertyOf rdf:resource="file:/C:/Users/Christian/Desktop/onto/owl/tueba.owl#hasMorphologicalFeature"/>
    </owl:ObjectProperty>
    


    <!-- file:/C:/Users/Christian/Desktop/onto/owl/tueba.owl#hasMood -->

    <owl:ObjectProperty rdf:about="file:/C:/Users/Christian/Desktop/onto/owl/tueba.owl#hasMood">
        <rdfs:range rdf:resource="file:/C:/Users/Christian/Desktop/onto/owl/tueba.owl#Mood"/>
        <rdfs:subPropertyOf rdf:resource="file:/C:/Users/Christian/Desktop/onto/owl/tueba.owl#hasMorphologicalFeature"/>
        <rdfs:domain>
            <owl:Class>
                <owl:unionOf rdf:parseType="Collection">
                    <rdf:Description rdf:about="&stts;FiniteAuxiliaryVerb"/>
                    <rdf:Description rdf:about="&stts;FiniteModalVerb"/>
                    <rdf:Description rdf:about="&stts;FiniteVerb"/>
                </owl:unionOf>
            </owl:Class>
        </rdfs:domain>
    </owl:ObjectProperty>
    


    <!-- file:/C:/Users/Christian/Desktop/onto/owl/tueba.owl#hasMorphologicalFeature -->

    <owl:ObjectProperty rdf:about="file:/C:/Users/Christian/Desktop/onto/owl/tueba.owl#hasMorphologicalFeature">
        <owl:versionInfo>Telljohann et al. (2009, p. 22f)</owl:versionInfo>
        <rdfs:domain rdf:resource="&stts;Tag"/>
        <rdfs:range rdf:resource="file:/C:/Users/Christian/Desktop/onto/owl/tueba.owl#MorphologicalFeature"/>
        <rdfs:subPropertyOf rdf:resource="&owl;topObjectProperty"/>
    </owl:ObjectProperty>
    


    <!-- file:/C:/Users/Christian/Desktop/onto/owl/tueba.owl#hasNumber -->

    <owl:ObjectProperty rdf:about="file:/C:/Users/Christian/Desktop/onto/owl/tueba.owl#hasNumber">
        <rdfs:range rdf:resource="file:/C:/Users/Christian/Desktop/onto/owl/tueba.owl#Number"/>
        <rdfs:subPropertyOf rdf:resource="file:/C:/Users/Christian/Desktop/onto/owl/tueba.owl#hasMorphologicalFeature"/>
        <rdfs:domain>
            <owl:Class>
                <owl:unionOf rdf:parseType="Collection">
                    <rdf:Description rdf:about="&stts;Article"/>
                    <rdf:Description rdf:about="&stts;AttributiveAdjective"/>
                    <rdf:Description rdf:about="&stts;AuxiliaryImperative"/>
                    <rdf:Description rdf:about="&stts;DemonstrativePronoun"/>
                    <rdf:Description rdf:about="&stts;FiniteAuxiliaryVerb"/>
                    <rdf:Description rdf:about="&stts;FiniteModalVerb"/>
                    <rdf:Description rdf:about="&stts;FiniteVerb"/>
                    <rdf:Description rdf:about="&stts;Imperative"/>
                    <rdf:Description rdf:about="&stts;IndefinitePronoun"/>
                    <rdf:Description rdf:about="&stts;InterrogativePronoun"/>
                    <rdf:Description rdf:about="&stts;Noun"/>
                    <rdf:Description rdf:about="&stts;PersonalPronoun"/>
                    <rdf:Description rdf:about="&stts;PossessivePronoun"/>
                    <rdf:Description rdf:about="&stts;ReflexivePronoun"/>
                    <rdf:Description rdf:about="&stts;RelativePronoun"/>
                </owl:unionOf>
            </owl:Class>
        </rdfs:domain>
    </owl:ObjectProperty>
    


    <!-- file:/C:/Users/Christian/Desktop/onto/owl/tueba.owl#hasPerson -->

    <owl:ObjectProperty rdf:about="file:/C:/Users/Christian/Desktop/onto/owl/tueba.owl#hasPerson">
        <rdfs:range rdf:resource="file:/C:/Users/Christian/Desktop/onto/owl/tueba.owl#Person"/>
        <rdfs:subPropertyOf rdf:resource="file:/C:/Users/Christian/Desktop/onto/owl/tueba.owl#hasMorphologicalFeature"/>
        <rdfs:domain>
            <owl:Class>
                <owl:unionOf rdf:parseType="Collection">
                    <rdf:Description rdf:about="&stts;FiniteAuxiliaryVerb"/>
                    <rdf:Description rdf:about="&stts;FiniteModalVerb"/>
                    <rdf:Description rdf:about="&stts;FiniteVerb"/>
                    <rdf:Description rdf:about="&stts;PersonalPronoun"/>
                    <rdf:Description rdf:about="&stts;ReflexivePronoun"/>
                </owl:unionOf>
            </owl:Class>
        </rdfs:domain>
    </owl:ObjectProperty>
    


    <!-- file:/C:/Users/Christian/Desktop/onto/owl/tueba.owl#hasTense -->

    <owl:ObjectProperty rdf:about="file:/C:/Users/Christian/Desktop/onto/owl/tueba.owl#hasTense">
        <rdfs:range rdf:resource="file:/C:/Users/Christian/Desktop/onto/owl/tueba.owl#Tense"/>
        <rdfs:subPropertyOf rdf:resource="file:/C:/Users/Christian/Desktop/onto/owl/tueba.owl#hasMorphologicalFeature"/>
        <rdfs:domain>
            <owl:Class>
                <owl:unionOf rdf:parseType="Collection">
                    <rdf:Description rdf:about="&stts;FiniteAuxiliaryVerb"/>
                    <rdf:Description rdf:about="&stts;FiniteModalVerb"/>
                    <rdf:Description rdf:about="&stts;FiniteVerb"/>
                </owl:unionOf>
            </owl:Class>
        </rdfs:domain>
    </owl:ObjectProperty>
    


    <!-- http://www.w3.org/2002/07/owl#topObjectProperty -->

    <owl:ObjectProperty rdf:about="&owl;topObjectProperty"/>
    


    <!-- 
    ///////////////////////////////////////////////////////////////////////////////////////
    //
    // Data properties
    //
    ///////////////////////////////////////////////////////////////////////////////////////
     -->

    


    <!-- file:/C:/Users/Christian/Desktop/onto/owl/system.owl#hasTag -->

    <owl:DatatypeProperty rdf:about="&system;hasTag"/>
    


    <!-- file:/C:/Users/Christian/Desktop/onto/owl/tueba.owl#hasTagContaining -->

    <owl:DatatypeProperty rdf:about="file:/C:/Users/Christian/Desktop/onto/owl/tueba.owl#hasTagContaining">
        <rdfs:subPropertyOf rdf:resource="&system;hasTag"/>
    </owl:DatatypeProperty>
    


    <!-- file:/C:/Users/Christian/Desktop/onto/owl/tueba.owl#hasTagEndingWith -->

    <owl:DatatypeProperty rdf:about="file:/C:/Users/Christian/Desktop/onto/owl/tueba.owl#hasTagEndingWith">
        <rdfs:subPropertyOf rdf:resource="&system;hasTag"/>
    </owl:DatatypeProperty>
    


    <!-- file:/C:/Users/Christian/Desktop/onto/owl/tueba.owl#hasTagStartingWith -->

    <owl:DatatypeProperty rdf:about="file:/C:/Users/Christian/Desktop/onto/owl/tueba.owl#hasTagStartingWith">
        <rdfs:subPropertyOf rdf:resource="&system;hasTag"/>
    </owl:DatatypeProperty>
    


    <!-- 
    ///////////////////////////////////////////////////////////////////////////////////////
    //
    // Classes
    //
    ///////////////////////////////////////////////////////////////////////////////////////
     -->

    


    <!-- file:/C:/Users/Christian/Desktop/onto/owl/stts.owl#Article -->

    <owl:Class rdf:about="&stts;Article"/>
    


    <!-- file:/C:/Users/Christian/Desktop/onto/owl/stts.owl#AttributiveAdjective -->

    <owl:Class rdf:about="&stts;AttributiveAdjective"/>
    


    <!-- file:/C:/Users/Christian/Desktop/onto/owl/stts.owl#AuxiliaryImperative -->

    <owl:Class rdf:about="&stts;AuxiliaryImperative"/>
    


    <!-- file:/C:/Users/Christian/Desktop/onto/owl/stts.owl#DemonstrativePronoun -->

    <owl:Class rdf:about="&stts;DemonstrativePronoun"/>
    


    <!-- file:/C:/Users/Christian/Desktop/onto/owl/stts.owl#FiniteAuxiliaryVerb -->

    <owl:Class rdf:about="&stts;FiniteAuxiliaryVerb"/>
    


    <!-- file:/C:/Users/Christian/Desktop/onto/owl/stts.owl#FiniteModalVerb -->

    <owl:Class rdf:about="&stts;FiniteModalVerb"/>
    


    <!-- file:/C:/Users/Christian/Desktop/onto/owl/stts.owl#FiniteVerb -->

    <owl:Class rdf:about="&stts;FiniteVerb"/>
    


    <!-- file:/C:/Users/Christian/Desktop/onto/owl/stts.owl#Imperative -->

    <owl:Class rdf:about="&stts;Imperative"/>
    


    <!-- file:/C:/Users/Christian/Desktop/onto/owl/stts.owl#IndefinitePronoun -->

    <owl:Class rdf:about="&stts;IndefinitePronoun"/>
    


    <!-- file:/C:/Users/Christian/Desktop/onto/owl/stts.owl#InterrogativePronoun -->

    <owl:Class rdf:about="&stts;InterrogativePronoun"/>
    


    <!-- file:/C:/Users/Christian/Desktop/onto/owl/stts.owl#Noun -->

    <owl:Class rdf:about="&stts;Noun"/>
    


    <!-- file:/C:/Users/Christian/Desktop/onto/owl/stts.owl#PersonalPronoun -->

    <owl:Class rdf:about="&stts;PersonalPronoun"/>
    


    <!-- file:/C:/Users/Christian/Desktop/onto/owl/stts.owl#PossessivePronoun -->

    <owl:Class rdf:about="&stts;PossessivePronoun"/>
    


    <!-- file:/C:/Users/Christian/Desktop/onto/owl/stts.owl#Postposition -->

    <owl:Class rdf:about="&stts;Postposition"/>
    


    <!-- file:/C:/Users/Christian/Desktop/onto/owl/stts.owl#Preposition -->

    <owl:Class rdf:about="&stts;Preposition"/>
    


    <!-- file:/C:/Users/Christian/Desktop/onto/owl/stts.owl#ReflexivePronoun -->

    <owl:Class rdf:about="&stts;ReflexivePronoun"/>
    


    <!-- file:/C:/Users/Christian/Desktop/onto/owl/stts.owl#RelativePronoun -->

    <owl:Class rdf:about="&stts;RelativePronoun"/>
    


    <!-- file:/C:/Users/Christian/Desktop/onto/owl/stts.owl#Tag -->

    <owl:Class rdf:about="&stts;Tag">
        <owl:versionInfo>Telljohann et al. (2009, p. 20-21)</owl:versionInfo>
    </owl:Class>
    


    <!-- file:/C:/Users/Christian/Desktop/onto/owl/system.owl#LinguisticAnnotation -->

    <owl:Class rdf:about="&system;LinguisticAnnotation"/>
    


    <!-- file:/C:/Users/Christian/Desktop/onto/owl/tueba.owl#Case -->

    <owl:Class rdf:about="file:/C:/Users/Christian/Desktop/onto/owl/tueba.owl#Case">
        <rdfs:subClassOf rdf:resource="file:/C:/Users/Christian/Desktop/onto/owl/tueba.owl#MorphologicalFeature"/>
    </owl:Class>
    


    <!-- file:/C:/Users/Christian/Desktop/onto/owl/tueba.owl#Complement -->

    <owl:Class rdf:about="file:/C:/Users/Christian/Desktop/onto/owl/tueba.owl#Complement">
        <rdfs:subClassOf rdf:resource="file:/C:/Users/Christian/Desktop/onto/owl/tueba.owl#SyntacticEdgeLabel"/>
    </owl:Class>
    


    <!-- file:/C:/Users/Christian/Desktop/onto/owl/tueba.owl#Gender -->

    <owl:Class rdf:about="file:/C:/Users/Christian/Desktop/onto/owl/tueba.owl#Gender">
        <rdfs:subClassOf rdf:resource="file:/C:/Users/Christian/Desktop/onto/owl/tueba.owl#MorphologicalFeature"/>
    </owl:Class>
    


    <!-- file:/C:/Users/Christian/Desktop/onto/owl/tueba.owl#HeadOrConjunct -->

    <owl:Class rdf:about="file:/C:/Users/Christian/Desktop/onto/owl/tueba.owl#HeadOrConjunct">
        <rdfs:subClassOf rdf:resource="file:/C:/Users/Christian/Desktop/onto/owl/tueba.owl#SyntacticEdgeLabel"/>
    </owl:Class>
    


    <!-- file:/C:/Users/Christian/Desktop/onto/owl/tueba.owl#Modifier -->

    <owl:Class rdf:about="file:/C:/Users/Christian/Desktop/onto/owl/tueba.owl#Modifier">
        <rdfs:subClassOf rdf:resource="file:/C:/Users/Christian/Desktop/onto/owl/tueba.owl#SyntacticEdgeLabel"/>
    </owl:Class>
    


    <!-- file:/C:/Users/Christian/Desktop/onto/owl/tueba.owl#Mood -->

    <owl:Class rdf:about="file:/C:/Users/Christian/Desktop/onto/owl/tueba.owl#Mood">
        <rdfs:subClassOf rdf:resource="file:/C:/Users/Christian/Desktop/onto/owl/tueba.owl#MorphologicalFeature"/>
    </owl:Class>
    


    <!-- file:/C:/Users/Christian/Desktop/onto/owl/tueba.owl#MorphologicalFeature -->

    <owl:Class rdf:about="file:/C:/Users/Christian/Desktop/onto/owl/tueba.owl#MorphologicalFeature">
        <rdfs:subClassOf rdf:resource="&system;LinguisticAnnotation"/>
        <owl:versionInfo>Telljohann et al. (2009, p.22 ff)

Note that hasTagContaining() is used whenever a feature is unambiguously recognizable. The only exceptions to this rule are
(1) the features singular (s) and present (s),
(2) the features nominative (n) and neuter (n)

These are disambiguated by means of possible surrounding features</owl:versionInfo>
    </owl:Class>
    


    <!-- file:/C:/Users/Christian/Desktop/onto/owl/tueba.owl#Number -->

    <owl:Class rdf:about="file:/C:/Users/Christian/Desktop/onto/owl/tueba.owl#Number">
        <rdfs:subClassOf rdf:resource="file:/C:/Users/Christian/Desktop/onto/owl/tueba.owl#MorphologicalFeature"/>
    </owl:Class>
    


    <!-- file:/C:/Users/Christian/Desktop/onto/owl/tueba.owl#Person -->

    <owl:Class rdf:about="file:/C:/Users/Christian/Desktop/onto/owl/tueba.owl#Person">
        <rdfs:subClassOf rdf:resource="file:/C:/Users/Christian/Desktop/onto/owl/tueba.owl#MorphologicalFeature"/>
    </owl:Class>
    


    <!-- file:/C:/Users/Christian/Desktop/onto/owl/tueba.owl#Phrase -->

    <owl:Class rdf:about="file:/C:/Users/Christian/Desktop/onto/owl/tueba.owl#Phrase">
        <rdfs:subClassOf rdf:resource="file:/C:/Users/Christian/Desktop/onto/owl/tueba.owl#SyntacticNodeLabel"/>
    </owl:Class>
    


    <!-- file:/C:/Users/Christian/Desktop/onto/owl/tueba.owl#Root -->

    <owl:Class rdf:about="file:/C:/Users/Christian/Desktop/onto/owl/tueba.owl#Root">
        <rdfs:subClassOf rdf:resource="file:/C:/Users/Christian/Desktop/onto/owl/tueba.owl#SyntacticNodeLabel"/>
    </owl:Class>
    


    <!-- file:/C:/Users/Christian/Desktop/onto/owl/tueba.owl#SecondaryEdge -->

    <owl:Class rdf:about="file:/C:/Users/Christian/Desktop/onto/owl/tueba.owl#SecondaryEdge">
        <rdfs:subClassOf rdf:resource="file:/C:/Users/Christian/Desktop/onto/owl/tueba.owl#SyntacticEdgeLabel"/>
    </owl:Class>
    


    <!-- file:/C:/Users/Christian/Desktop/onto/owl/tueba.owl#SplitCoordination -->

    <owl:Class rdf:about="file:/C:/Users/Christian/Desktop/onto/owl/tueba.owl#SplitCoordination">
        <rdfs:subClassOf rdf:resource="file:/C:/Users/Christian/Desktop/onto/owl/tueba.owl#SyntacticEdgeLabel"/>
    </owl:Class>
    


    <!-- file:/C:/Users/Christian/Desktop/onto/owl/tueba.owl#StructuralExpletive -->

    <owl:Class rdf:about="file:/C:/Users/Christian/Desktop/onto/owl/tueba.owl#StructuralExpletive">
        <rdfs:subClassOf rdf:resource="file:/C:/Users/Christian/Desktop/onto/owl/tueba.owl#SyntacticEdgeLabel"/>
    </owl:Class>
    


    <!-- file:/C:/Users/Christian/Desktop/onto/owl/tueba.owl#SyntacticEdgeLabel -->

    <owl:Class rdf:about="file:/C:/Users/Christian/Desktop/onto/owl/tueba.owl#SyntacticEdgeLabel">
        <rdfs:subClassOf rdf:resource="&system;LinguisticAnnotation"/>
        <owl:versionInfo>Edge labels indicate the grammatical function of lexical entries, phrases, topological
fields, and clauses. Since case information is given and a distinction of different modifiers
is made by these labels, the syntactic tree structures also contain semantic roles.
(Telljohann et al. 2009, p. 19)

The subclasses of edges are taken from Telljohann (2009, p. 25) unless marked otherwise.</owl:versionInfo>
    </owl:Class>
    


    <!-- file:/C:/Users/Christian/Desktop/onto/owl/tueba.owl#SyntacticNodeLabel -->

    <owl:Class rdf:about="file:/C:/Users/Christian/Desktop/onto/owl/tueba.owl#SyntacticNodeLabel">
        <rdfs:subClassOf rdf:resource="&system;LinguisticAnnotation"/>
        <owl:versionInfo>Node labels indicate the syntactic category of a phrase or sentence, but they are also
used to label topological fields and sequences of topological fields within coordinations or
to indicate specific grammatical properties of constituents.
(Telljohann et al. 2009, p.19)

Subclasses are adopted from Telljohann et al. (2009, p. 24) unless marked otherwise.

</owl:versionInfo>
    </owl:Class>
    


    <!-- file:/C:/Users/Christian/Desktop/onto/owl/tueba.owl#Tense -->

    <owl:Class rdf:about="file:/C:/Users/Christian/Desktop/onto/owl/tueba.owl#Tense">
        <rdfs:subClassOf rdf:resource="file:/C:/Users/Christian/Desktop/onto/owl/tueba.owl#MorphologicalFeature"/>
    </owl:Class>
    


    <!-- file:/C:/Users/Christian/Desktop/onto/owl/tueba.owl#TopologicalField -->

    <owl:Class rdf:about="file:/C:/Users/Christian/Desktop/onto/owl/tueba.owl#TopologicalField">
        <rdfs:subClassOf rdf:resource="file:/C:/Users/Christian/Desktop/onto/owl/tueba.owl#SyntacticNodeLabel"/>
        <rdfs:comment>In a German clause, the finite verb can appear in three different positions: verb-second,
verb-initial, and verb-final. Only in verb-final clauses the verb complex consisting of the
finite verb and non-finite verbal elements forms a unit. The discontinuous positioning
of the verbal elements in verb-first and verb-second clauses is the traditional reason
for structuring German clauses into fields. The positions of the verbal elements form
the Satzklammer (sentence bracket) which divides the sentence into a Vorfeld (initial
field), a Mittelfeld (middle field), and a Nachfeld (final field). The Vorfeld and the
Mittelfeld are divided by the linke Satzklammer (left sentence bracket), which is the finite
verb, the rechte Satzklammer (right sentence bracket) is the verb complex between the
Mittelfeld and the Nachfeld. 
(Telljohann et al. 2009, p.13)</rdfs:comment>
    </owl:Class>
    


    <!-- 
    ///////////////////////////////////////////////////////////////////////////////////////
    //
    // Individuals
    //
    ///////////////////////////////////////////////////////////////////////////////////////
     -->

    


    <!-- file:/C:/Users/Christian/Desktop/onto/owl/tueba.owl#ADJX -->

    <owl:NamedIndividual rdf:about="file:/C:/Users/Christian/Desktop/onto/owl/tueba.owl#ADJX">
        <rdf:type rdf:resource="file:/C:/Users/Christian/Desktop/onto/owl/tueba.owl#Phrase"/>
        <rdfs:comment>adjectival phrase</rdfs:comment>
        <system:hasTag>ADJX</system:hasTag>
    </owl:NamedIndividual>
    


    <!-- file:/C:/Users/Christian/Desktop/onto/owl/tueba.owl#ADVX -->

    <owl:NamedIndividual rdf:about="file:/C:/Users/Christian/Desktop/onto/owl/tueba.owl#ADVX">
        <rdf:type rdf:resource="file:/C:/Users/Christian/Desktop/onto/owl/tueba.owl#Phrase"/>
        <system:hasTag>ADVX</system:hasTag>
        <rdfs:comment>adverbial phrase</rdfs:comment>
    </owl:NamedIndividual>
    


    <!-- file:/C:/Users/Christian/Desktop/onto/owl/tueba.owl#APP -->

    <owl:NamedIndividual rdf:about="file:/C:/Users/Christian/Desktop/onto/owl/tueba.owl#APP">
        <rdf:type rdf:resource="file:/C:/Users/Christian/Desktop/onto/owl/tueba.owl#Complement"/>
        <system:hasTag>APP</system:hasTag>
        <rdfs:comment>apposition</rdfs:comment>
    </owl:NamedIndividual>
    


    <!-- file:/C:/Users/Christian/Desktop/onto/owl/tueba.owl#C -->

    <owl:NamedIndividual rdf:about="file:/C:/Users/Christian/Desktop/onto/owl/tueba.owl#C">
        <rdf:type rdf:resource="file:/C:/Users/Christian/Desktop/onto/owl/tueba.owl#TopologicalField"/>
        <system:hasTag>C</system:hasTag>
        <rdfs:comment>The C-Feld only occurs in verb-final clauses (exception: the conjunction als in
subordinated sentences of comparison als w&#168;are es nie geschehen.). It is obligatorily
occupied in finite verb-final clauses if there is no conjunction in the Linke Klammer. In
non-finite verb-final clauses the C-position may be empty. This field can be occupied by
conjunctions of sentential objects (e.g. da&#223;, ob) or sentence initial conjunctions like um,
obwohl, wenn and also by complex interrogative or relative phrases, e.g. ..., &#8217;um wieviel
Geld&#8217; geht es dabei? / ..., &#8217;an der&#8217; Max Daniel Professor f&#252;r Klavier ist.
(Telljohann et al. 2009)
</rdfs:comment>
    </owl:NamedIndividual>
    


    <!-- file:/C:/Users/Christian/Desktop/onto/owl/tueba.owl#DM -->

    <owl:NamedIndividual rdf:about="file:/C:/Users/Christian/Desktop/onto/owl/tueba.owl#DM">
        <rdf:type rdf:resource="file:/C:/Users/Christian/Desktop/onto/owl/tueba.owl#Root"/>
        <system:hasTag>DM</system:hasTag>
        <rdfs:comment>discourse marker</rdfs:comment>
    </owl:NamedIndividual>
    


    <!-- file:/C:/Users/Christian/Desktop/onto/owl/tueba.owl#DP -->

    <owl:NamedIndividual rdf:about="file:/C:/Users/Christian/Desktop/onto/owl/tueba.owl#DP">
        <rdf:type rdf:resource="file:/C:/Users/Christian/Desktop/onto/owl/tueba.owl#Phrase"/>
        <rdfs:comment>determiner phrase (e.g., &quot;gar keine&quot;)</rdfs:comment>
        <system:hasTag>DP</system:hasTag>
    </owl:NamedIndividual>
    


    <!-- file:/C:/Users/Christian/Desktop/onto/owl/tueba.owl#EN -->

    <owl:NamedIndividual rdf:about="file:/C:/Users/Christian/Desktop/onto/owl/tueba.owl#EN">
        <rdf:type rdf:resource="file:/C:/Users/Christian/Desktop/onto/owl/tueba.owl#SecondaryEdge"/>
        <rdfs:comment>phrase internal relation between two parts of a proper noun (Telljohann et al. 2009, p. 26)</rdfs:comment>
    </owl:NamedIndividual>
    


    <!-- file:/C:/Users/Christian/Desktop/onto/owl/tueba.owl#EN-ADD -->

    <owl:NamedIndividual rdf:about="file:/C:/Users/Christian/Desktop/onto/owl/tueba.owl#EN-ADD">
        <rdf:type rdf:resource="file:/C:/Users/Christian/Desktop/onto/owl/tueba.owl#Phrase"/>
        <rdfs:comment>proper noun or named entity (additional phrase node label, Telljohann et al 2009, p.26)</rdfs:comment>
        <system:hasTag>EN-ADD</system:hasTag>
    </owl:NamedIndividual>
    


    <!-- file:/C:/Users/Christian/Desktop/onto/owl/tueba.owl#ES -->

    <owl:NamedIndividual rdf:about="file:/C:/Users/Christian/Desktop/onto/owl/tueba.owl#ES">
        <rdf:type rdf:resource="file:/C:/Users/Christian/Desktop/onto/owl/tueba.owl#StructuralExpletive"/>
        <rdfs:comment>Vorfeld-es</rdfs:comment>
        <system:hasTag>ES</system:hasTag>
    </owl:NamedIndividual>
    


    <!-- file:/C:/Users/Christian/Desktop/onto/owl/tueba.owl#FKONJ -->

    <owl:NamedIndividual rdf:about="file:/C:/Users/Christian/Desktop/onto/owl/tueba.owl#FKONJ">
        <rdf:type rdf:resource="file:/C:/Users/Christian/Desktop/onto/owl/tueba.owl#TopologicalField"/>
        <rdfs:comment>conjunct consisting of more than one field</rdfs:comment>
        <system:hasTag>FKONJ</system:hasTag>
    </owl:NamedIndividual>
    


    <!-- file:/C:/Users/Christian/Desktop/onto/owl/tueba.owl#FKOORD -->

    <owl:NamedIndividual rdf:about="file:/C:/Users/Christian/Desktop/onto/owl/tueba.owl#FKOORD">
        <rdf:type rdf:resource="file:/C:/Users/Christian/Desktop/onto/owl/tueba.owl#TopologicalField"/>
        <system:hasTag>FKOORD</system:hasTag>
        <rdfs:comment>coordination consisting of conjuncts of fields</rdfs:comment>
    </owl:NamedIndividual>
    


    <!-- file:/C:/Users/Christian/Desktop/onto/owl/tueba.owl#FOPP -->

    <owl:NamedIndividual rdf:about="file:/C:/Users/Christian/Desktop/onto/owl/tueba.owl#FOPP">
        <rdf:type rdf:resource="file:/C:/Users/Christian/Desktop/onto/owl/tueba.owl#Complement"/>
        <system:hasTag>FOPP</system:hasTag>
        <rdfs:comment>facultative (i.e. optional) prepositional object, passivized subject (von-phrase)</rdfs:comment>
    </owl:NamedIndividual>
    


    <!-- file:/C:/Users/Christian/Desktop/onto/owl/tueba.owl#FOPP-MOD -->

    <owl:NamedIndividual rdf:about="file:/C:/Users/Christian/Desktop/onto/owl/tueba.owl#FOPP-MOD">
        <rdf:type rdf:resource="file:/C:/Users/Christian/Desktop/onto/owl/tueba.owl#Modifier"/>
        <rdfs:comment>modifiers modifying complements or modifiers, e.g. V-MOD = modifier of the verb</rdfs:comment>
        <system:hasTag>FOPP-MOD</system:hasTag>
    </owl:NamedIndividual>
    


    <!-- file:/C:/Users/Christian/Desktop/onto/owl/tueba.owl#FOPPK -->

    <owl:NamedIndividual rdf:about="file:/C:/Users/Christian/Desktop/onto/owl/tueba.owl#FOPPK">
        <rdf:type rdf:resource="file:/C:/Users/Christian/Desktop/onto/owl/tueba.owl#SplitCoordination"/>
        <rdfs:comment>second conjunct (K) in split coordinations, e.g. ONK = second conjunct of a nominative object</rdfs:comment>
        <system:hasTag>FOPPK</system:hasTag>
    </owl:NamedIndividual>
    


    <!-- file:/C:/Users/Christian/Desktop/onto/owl/tueba.owl#FX -->

    <owl:NamedIndividual rdf:about="file:/C:/Users/Christian/Desktop/onto/owl/tueba.owl#FX">
        <rdf:type rdf:resource="file:/C:/Users/Christian/Desktop/onto/owl/tueba.owl#Phrase"/>
        <system:hasTag>FX</system:hasTag>
        <rdfs:comment>foreign language phrase</rdfs:comment>
    </owl:NamedIndividual>
    


    <!-- file:/C:/Users/Christian/Desktop/onto/owl/tueba.owl#HD -->

    <owl:NamedIndividual rdf:about="file:/C:/Users/Christian/Desktop/onto/owl/tueba.owl#HD">
        <rdf:type rdf:resource="file:/C:/Users/Christian/Desktop/onto/owl/tueba.owl#HeadOrConjunct"/>
        <rdfs:comment>head</rdfs:comment>
        <system:hasTag>HD</system:hasTag>
    </owl:NamedIndividual>
    


    <!-- file:/C:/Users/Christian/Desktop/onto/owl/tueba.owl#KONJ -->

    <owl:NamedIndividual rdf:about="file:/C:/Users/Christian/Desktop/onto/owl/tueba.owl#KONJ">
        <rdf:type rdf:resource="file:/C:/Users/Christian/Desktop/onto/owl/tueba.owl#HeadOrConjunct"/>
        <hasTagContaining>KONJ</hasTagContaining>
        <rdfs:comment>conjunct</rdfs:comment>
    </owl:NamedIndividual>
    


    <!-- file:/C:/Users/Christian/Desktop/onto/owl/tueba.owl#KOORD -->

    <owl:NamedIndividual rdf:about="file:/C:/Users/Christian/Desktop/onto/owl/tueba.owl#KOORD">
        <rdf:type rdf:resource="file:/C:/Users/Christian/Desktop/onto/owl/tueba.owl#TopologicalField"/>
        <rdfs:comment>The KOORD-field is the field for coordinating particles. In contrast to
the PARORD-field, it can optionally occur as the left-most element of all clause types
(Telljohann et al. 2009, p. 15)</rdfs:comment>
        <rdfs:comment>field for coordinating particles</rdfs:comment>
        <system:hasTag>KOORD</system:hasTag>
    </owl:NamedIndividual>
    


    <!-- file:/C:/Users/Christian/Desktop/onto/owl/tueba.owl#LK -->

    <owl:NamedIndividual rdf:about="file:/C:/Users/Christian/Desktop/onto/owl/tueba.owl#LK">
        <rdf:type rdf:resource="file:/C:/Users/Christian/Desktop/onto/owl/tueba.owl#TopologicalField"/>
        <rdfs:comment>The Linke Klammer is the position of the finite verb in verb-second and
verb-first clauses or a conjunction in verb-final clauses. It consists of exactly one element.
(Telljohann et al. 2009)</rdfs:comment>
        <system:hasTag>LK</system:hasTag>
        <rdfs:comment>left sentence bracket (Linke (Satz-)Klammer)</rdfs:comment>
    </owl:NamedIndividual>
    


    <!-- file:/C:/Users/Christian/Desktop/onto/owl/tueba.owl#LV -->

    <owl:NamedIndividual rdf:about="file:/C:/Users/Christian/Desktop/onto/owl/tueba.owl#LV">
        <rdf:type rdf:resource="file:/C:/Users/Christian/Desktop/onto/owl/tueba.owl#TopologicalField"/>
        <system:hasTag>LV</system:hasTag>
        <rdfs:comment>resumptive construction (Linksversetzung)</rdfs:comment>
        <rdfs:comment>The Linksversetzungsfeld is a field for the left-dislocated phrase of resump-
tive constructions. A Linksversetzung is a pendent constituent. It can be regarded as
a syntactic anticipation of a part of a sentence.
(Telljohann et al. 2009)</rdfs:comment>
    </owl:NamedIndividual>
    


    <!-- file:/C:/Users/Christian/Desktop/onto/owl/tueba.owl#MF -->

    <owl:NamedIndividual rdf:about="file:/C:/Users/Christian/Desktop/onto/owl/tueba.owl#MF">
        <rdf:type rdf:resource="file:/C:/Users/Christian/Desktop/onto/owl/tueba.owl#TopologicalField"/>
        <rdfs:comment>Apart from those units which are optionally located in other fields, any
non-verbal constituent may occur in the Mittelfeld. It consists of a sequence of any
number of constituents. The linear order of the constituents depends on the specific
word order principles for German and their interaction.
(Telljohann et al. 2009)</rdfs:comment>
        <rdfs:comment>middle field (Mittelfeld)</rdfs:comment>
        <system:hasTag>MF</system:hasTag>
    </owl:NamedIndividual>
    


    <!-- file:/C:/Users/Christian/Desktop/onto/owl/tueba.owl#MFE -->

    <owl:NamedIndividual rdf:about="file:/C:/Users/Christian/Desktop/onto/owl/tueba.owl#MFE">
        <rdf:type rdf:resource="file:/C:/Users/Christian/Desktop/onto/owl/tueba.owl#TopologicalField"/>
        <system:hasTag>MFE</system:hasTag>
        <rdfs:comment>middle field between VCE and VC</rdfs:comment>
    </owl:NamedIndividual>
    


    <!-- file:/C:/Users/Christian/Desktop/onto/owl/tueba.owl#MOD -->

    <owl:NamedIndividual rdf:about="file:/C:/Users/Christian/Desktop/onto/owl/tueba.owl#MOD">
        <rdf:type rdf:resource="file:/C:/Users/Christian/Desktop/onto/owl/tueba.owl#Modifier"/>
        <rdfs:comment>amiguous modifier</rdfs:comment>
        <system:hasTag>MOD</system:hasTag>
    </owl:NamedIndividual>
    


    <!-- file:/C:/Users/Christian/Desktop/onto/owl/tueba.owl#MOD-MOD -->

    <owl:NamedIndividual rdf:about="file:/C:/Users/Christian/Desktop/onto/owl/tueba.owl#MOD-MOD">
        <rdf:type rdf:resource="file:/C:/Users/Christian/Desktop/onto/owl/tueba.owl#Modifier"/>
        <system:hasTag>MOD-MOD</system:hasTag>
        <rdfs:comment>modifiers modifying complements or modifiers, e.g. V-MOD = modifier of the verb</rdfs:comment>
    </owl:NamedIndividual>
    


    <!-- file:/C:/Users/Christian/Desktop/onto/owl/tueba.owl#MODK -->

    <owl:NamedIndividual rdf:about="file:/C:/Users/Christian/Desktop/onto/owl/tueba.owl#MODK">
        <rdf:type rdf:resource="file:/C:/Users/Christian/Desktop/onto/owl/tueba.owl#SplitCoordination"/>
        <system:hasTag>MODK</system:hasTag>
        <rdfs:comment>second conjunct (K) in split coordinations, e.g. ONK = second conjunct of a nominative object</rdfs:comment>
    </owl:NamedIndividual>
    


    <!-- file:/C:/Users/Christian/Desktop/onto/owl/tueba.owl#NF -->

    <owl:NamedIndividual rdf:about="file:/C:/Users/Christian/Desktop/onto/owl/tueba.owl#NF">
        <rdf:type rdf:resource="file:/C:/Users/Christian/Desktop/onto/owl/tueba.owl#TopologicalField"/>
        <system:hasTag>NF</system:hasTag>
        <rdfs:comment>final field (Nachfeld)</rdfs:comment>
        <rdfs:comment>For some clause types (e.g. so da&#223;-S&#168;atze), the Nachfeld is the obligatory po-
sition. Embedded complement clauses, relative clauses, and single constituents can
optionally occur in the Nachfeld. In contrast to the Vorfeld it may be occupied by any
number of constituents.
(Telljohann et al. 2009)</rdfs:comment>
    </owl:NamedIndividual>
    


    <!-- file:/C:/Users/Christian/Desktop/onto/owl/tueba.owl#NX -->

    <owl:NamedIndividual rdf:about="file:/C:/Users/Christian/Desktop/onto/owl/tueba.owl#NX">
        <rdf:type rdf:resource="file:/C:/Users/Christian/Desktop/onto/owl/tueba.owl#Phrase"/>
        <rdfs:comment>noun phrase</rdfs:comment>
        <system:hasTag>NX</system:hasTag>
    </owl:NamedIndividual>
    


    <!-- file:/C:/Users/Christian/Desktop/onto/owl/tueba.owl#OA -->

    <owl:NamedIndividual rdf:about="file:/C:/Users/Christian/Desktop/onto/owl/tueba.owl#OA">
        <rdf:type rdf:resource="file:/C:/Users/Christian/Desktop/onto/owl/tueba.owl#Complement"/>
        <rdfs:comment>accusative object</rdfs:comment>
        <system:hasTag>OA</system:hasTag>
    </owl:NamedIndividual>
    


    <!-- file:/C:/Users/Christian/Desktop/onto/owl/tueba.owl#OA-MOD -->

    <owl:NamedIndividual rdf:about="file:/C:/Users/Christian/Desktop/onto/owl/tueba.owl#OA-MOD">
        <rdf:type rdf:resource="file:/C:/Users/Christian/Desktop/onto/owl/tueba.owl#Modifier"/>
        <system:hasTag>OA-MOD</system:hasTag>
        <rdfs:comment>modifiers modifying complements or modifiers, e.g. V-MOD = modifier of the verb</rdfs:comment>
    </owl:NamedIndividual>
    


    <!-- file:/C:/Users/Christian/Desktop/onto/owl/tueba.owl#OA-MODK -->

    <owl:NamedIndividual rdf:about="file:/C:/Users/Christian/Desktop/onto/owl/tueba.owl#OA-MODK">
        <rdf:type rdf:resource="file:/C:/Users/Christian/Desktop/onto/owl/tueba.owl#SplitCoordination"/>
        <system:hasTag>OA-MODK</system:hasTag>
        <rdfs:comment>second conjunct (K) in split coordinations, e.g. ONK = second conjunct of a nominative object</rdfs:comment>
    </owl:NamedIndividual>
    


    <!-- file:/C:/Users/Christian/Desktop/onto/owl/tueba.owl#OADJP -->

    <owl:NamedIndividual rdf:about="file:/C:/Users/Christian/Desktop/onto/owl/tueba.owl#OADJP">
        <rdf:type rdf:resource="file:/C:/Users/Christian/Desktop/onto/owl/tueba.owl#Complement"/>
        <system:hasTag>OADJP</system:hasTag>
        <rdfs:comment>adjectival object</rdfs:comment>
    </owl:NamedIndividual>
    


    <!-- file:/C:/Users/Christian/Desktop/onto/owl/tueba.owl#OADJP-MOD -->

    <owl:NamedIndividual rdf:about="file:/C:/Users/Christian/Desktop/onto/owl/tueba.owl#OADJP-MOD">
        <rdf:type rdf:resource="file:/C:/Users/Christian/Desktop/onto/owl/tueba.owl#Modifier"/>
        <system:hasTag>OADJP-MOD</system:hasTag>
        <rdfs:comment>modifiers modifying complements or modifiers, e.g. V-MOD = modifier of the verb</rdfs:comment>
    </owl:NamedIndividual>
    


    <!-- file:/C:/Users/Christian/Desktop/onto/owl/tueba.owl#OADVP -->

    <owl:NamedIndividual rdf:about="file:/C:/Users/Christian/Desktop/onto/owl/tueba.owl#OADVP">
        <rdf:type rdf:resource="file:/C:/Users/Christian/Desktop/onto/owl/tueba.owl#Complement"/>
        <rdfs:comment>adverbial object</rdfs:comment>
        <system:hasTag>OADVP</system:hasTag>
    </owl:NamedIndividual>
    


    <!-- file:/C:/Users/Christian/Desktop/onto/owl/tueba.owl#OADVP-MOD -->

    <owl:NamedIndividual rdf:about="file:/C:/Users/Christian/Desktop/onto/owl/tueba.owl#OADVP-MOD">
        <rdf:type rdf:resource="file:/C:/Users/Christian/Desktop/onto/owl/tueba.owl#Modifier"/>
        <rdfs:comment>modifiers modifying complements or modifiers, e.g. V-MOD = modifier of the verb</rdfs:comment>
        <system:hasTag>OADVP-MOD</system:hasTag>
    </owl:NamedIndividual>
    


    <!-- file:/C:/Users/Christian/Desktop/onto/owl/tueba.owl#OADVPK -->

    <owl:NamedIndividual rdf:about="file:/C:/Users/Christian/Desktop/onto/owl/tueba.owl#OADVPK">
        <rdf:type rdf:resource="file:/C:/Users/Christian/Desktop/onto/owl/tueba.owl#SplitCoordination"/>
        <rdfs:comment>second conjunct (K) in split coordinations, e.g. ONK = second conjunct of a nominative object</rdfs:comment>
        <system:hasTag>OADVPK</system:hasTag>
    </owl:NamedIndividual>
    


    <!-- file:/C:/Users/Christian/Desktop/onto/owl/tueba.owl#OAK -->

    <owl:NamedIndividual rdf:about="file:/C:/Users/Christian/Desktop/onto/owl/tueba.owl#OAK">
        <rdf:type rdf:resource="file:/C:/Users/Christian/Desktop/onto/owl/tueba.owl#SplitCoordination"/>
        <rdfs:comment>second conjunct (K) in split coordinations, e.g. ONK = second conjunct of a nominative object</rdfs:comment>
        <system:hasTag>OAK</system:hasTag>
    </owl:NamedIndividual>
    


    <!-- file:/C:/Users/Christian/Desktop/onto/owl/tueba.owl#OD -->

    <owl:NamedIndividual rdf:about="file:/C:/Users/Christian/Desktop/onto/owl/tueba.owl#OD">
        <rdf:type rdf:resource="file:/C:/Users/Christian/Desktop/onto/owl/tueba.owl#Complement"/>
        <system:hasTag>OD</system:hasTag>
        <rdfs:comment>dative object</rdfs:comment>
    </owl:NamedIndividual>
    


    <!-- file:/C:/Users/Christian/Desktop/onto/owl/tueba.owl#OD-MOD -->

    <owl:NamedIndividual rdf:about="file:/C:/Users/Christian/Desktop/onto/owl/tueba.owl#OD-MOD">
        <rdf:type rdf:resource="file:/C:/Users/Christian/Desktop/onto/owl/tueba.owl#Modifier"/>
        <rdfs:comment>modifiers modifying complements or modifiers, e.g. V-MOD = modifier of the verb</rdfs:comment>
        <system:hasTag>OD-MOD</system:hasTag>
    </owl:NamedIndividual>
    


    <!-- file:/C:/Users/Christian/Desktop/onto/owl/tueba.owl#ODK -->

    <owl:NamedIndividual rdf:about="file:/C:/Users/Christian/Desktop/onto/owl/tueba.owl#ODK">
        <rdf:type rdf:resource="file:/C:/Users/Christian/Desktop/onto/owl/tueba.owl#SplitCoordination"/>
        <system:hasTag>ODK</system:hasTag>
        <rdfs:comment>second conjunct (K) in split coordinations, e.g. ONK = second conjunct of a nominative object</rdfs:comment>
    </owl:NamedIndividual>
    


    <!-- file:/C:/Users/Christian/Desktop/onto/owl/tueba.owl#OG -->

    <owl:NamedIndividual rdf:about="file:/C:/Users/Christian/Desktop/onto/owl/tueba.owl#OG">
        <rdf:type rdf:resource="file:/C:/Users/Christian/Desktop/onto/owl/tueba.owl#Complement"/>
        <rdfs:comment>genitive object</rdfs:comment>
        <system:hasTag>OG</system:hasTag>
    </owl:NamedIndividual>
    


    <!-- file:/C:/Users/Christian/Desktop/onto/owl/tueba.owl#OG-MOD -->

    <owl:NamedIndividual rdf:about="file:/C:/Users/Christian/Desktop/onto/owl/tueba.owl#OG-MOD">
        <rdf:type rdf:resource="file:/C:/Users/Christian/Desktop/onto/owl/tueba.owl#Modifier"/>
        <system:hasTag>OG-MOD</system:hasTag>
        <rdfs:comment>modifiers modifying complements or modifiers, e.g. V-MOD = modifier of the verb</rdfs:comment>
    </owl:NamedIndividual>
    


    <!-- file:/C:/Users/Christian/Desktop/onto/owl/tueba.owl#ON -->

    <owl:NamedIndividual rdf:about="file:/C:/Users/Christian/Desktop/onto/owl/tueba.owl#ON">
        <rdf:type rdf:resource="file:/C:/Users/Christian/Desktop/onto/owl/tueba.owl#Complement"/>
        <rdfs:comment>nominative object (i.e. subject; also clausal subjects)</rdfs:comment>
        <system:hasTag>ON</system:hasTag>
    </owl:NamedIndividual>
    


    <!-- file:/C:/Users/Christian/Desktop/onto/owl/tueba.owl#ON-MOD -->

    <owl:NamedIndividual rdf:about="file:/C:/Users/Christian/Desktop/onto/owl/tueba.owl#ON-MOD">
        <rdf:type rdf:resource="file:/C:/Users/Christian/Desktop/onto/owl/tueba.owl#Modifier"/>
        <rdfs:comment>modifiers modifying complements or modifiers, e.g. V-MOD = modifier of the verb</rdfs:comment>
        <system:hasTag>ON-MOD</system:hasTag>
    </owl:NamedIndividual>
    


    <!-- file:/C:/Users/Christian/Desktop/onto/owl/tueba.owl#ONK -->

    <owl:NamedIndividual rdf:about="file:/C:/Users/Christian/Desktop/onto/owl/tueba.owl#ONK">
        <rdf:type rdf:resource="file:/C:/Users/Christian/Desktop/onto/owl/tueba.owl#SplitCoordination"/>
        <rdfs:comment>second conjunct (K) in split coordinations, e.g. ONK = second conjunct of a nominative object</rdfs:comment>
        <system:hasTag>ONK</system:hasTag>
    </owl:NamedIndividual>
    


    <!-- file:/C:/Users/Christian/Desktop/onto/owl/tueba.owl#OPP -->

    <owl:NamedIndividual rdf:about="file:/C:/Users/Christian/Desktop/onto/owl/tueba.owl#OPP">
        <rdf:type rdf:resource="file:/C:/Users/Christian/Desktop/onto/owl/tueba.owl#Complement"/>
        <rdfs:comment>prepositional object</rdfs:comment>
        <system:hasTag>OPP</system:hasTag>
    </owl:NamedIndividual>
    


    <!-- file:/C:/Users/Christian/Desktop/onto/owl/tueba.owl#OPP-MOD -->

    <owl:NamedIndividual rdf:about="file:/C:/Users/Christian/Desktop/onto/owl/tueba.owl#OPP-MOD">
        <rdf:type rdf:resource="file:/C:/Users/Christian/Desktop/onto/owl/tueba.owl#Modifier"/>
        <system:hasTag>OPP-MOD</system:hasTag>
        <rdfs:comment>modifiers modifying complements or modifiers, e.g. V-MOD = modifier of the verb</rdfs:comment>
    </owl:NamedIndividual>
    


    <!-- file:/C:/Users/Christian/Desktop/onto/owl/tueba.owl#OPPK -->

    <owl:NamedIndividual rdf:about="file:/C:/Users/Christian/Desktop/onto/owl/tueba.owl#OPPK">
        <rdf:type rdf:resource="file:/C:/Users/Christian/Desktop/onto/owl/tueba.owl#SplitCoordination"/>
        <rdfs:comment>second conjunct (K) in split coordinations, e.g. ONK = second conjunct of a nominative object</rdfs:comment>
        <system:hasTag>OPPK</system:hasTag>
    </owl:NamedIndividual>
    


    <!-- file:/C:/Users/Christian/Desktop/onto/owl/tueba.owl#OS -->

    <owl:NamedIndividual rdf:about="file:/C:/Users/Christian/Desktop/onto/owl/tueba.owl#OS">
        <rdf:type rdf:resource="file:/C:/Users/Christian/Desktop/onto/owl/tueba.owl#Complement"/>
        <system:hasTag>OS</system:hasTag>
        <rdfs:comment>sentential object</rdfs:comment>
    </owl:NamedIndividual>
    


    <!-- file:/C:/Users/Christian/Desktop/onto/owl/tueba.owl#OS-MOD -->

    <owl:NamedIndividual rdf:about="file:/C:/Users/Christian/Desktop/onto/owl/tueba.owl#OS-MOD">
        <rdf:type rdf:resource="file:/C:/Users/Christian/Desktop/onto/owl/tueba.owl#Modifier"/>
        <system:hasTag>OS-MOD</system:hasTag>
        <rdfs:comment>modifiers modifying complements or modifiers, e.g. V-MOD = modifier of the verb</rdfs:comment>
    </owl:NamedIndividual>
    


    <!-- file:/C:/Users/Christian/Desktop/onto/owl/tueba.owl#OSK -->

    <owl:NamedIndividual rdf:about="file:/C:/Users/Christian/Desktop/onto/owl/tueba.owl#OSK">
        <rdf:type rdf:resource="file:/C:/Users/Christian/Desktop/onto/owl/tueba.owl#SplitCoordination"/>
        <rdfs:comment>second conjunct (K) in split coordinations, e.g. ONK = second conjunct of a nominative object</rdfs:comment>
        <system:hasTag>OSK</system:hasTag>
    </owl:NamedIndividual>
    


    <!-- file:/C:/Users/Christian/Desktop/onto/owl/tueba.owl#OV -->

    <owl:NamedIndividual rdf:about="file:/C:/Users/Christian/Desktop/onto/owl/tueba.owl#OV">
        <rdf:type rdf:resource="file:/C:/Users/Christian/Desktop/onto/owl/tueba.owl#Complement"/>
        <rdfs:comment>verbal object</rdfs:comment>
        <system:hasTag>OV</system:hasTag>
    </owl:NamedIndividual>
    


    <!-- file:/C:/Users/Christian/Desktop/onto/owl/tueba.owl#P-SIMPX -->

    <owl:NamedIndividual rdf:about="file:/C:/Users/Christian/Desktop/onto/owl/tueba.owl#P-SIMPX">
        <rdf:type rdf:resource="file:/C:/Users/Christian/Desktop/onto/owl/tueba.owl#Root"/>
        <system:hasTag>P-SIMPX</system:hasTag>
        <rdfs:comment>paratactic construction of simplex clauses</rdfs:comment>
    </owl:NamedIndividual>
    


    <!-- file:/C:/Users/Christian/Desktop/onto/owl/tueba.owl#PARORD -->

    <owl:NamedIndividual rdf:about="file:/C:/Users/Christian/Desktop/onto/owl/tueba.owl#PARORD">
        <rdf:type rdf:resource="file:/C:/Users/Christian/Desktop/onto/owl/tueba.owl#TopologicalField"/>
        <rdfs:comment>field for non-coordinating particles</rdfs:comment>
        <system:hasTag>PARORD</system:hasTag>
        <rdfs:comment>The PARORD-field is the field for non-coordinating particles which
optionally occur as the left-most element of a verb-second clause
(Telljohann et al. 2009)</rdfs:comment>
    </owl:NamedIndividual>
    


    <!-- file:/C:/Users/Christian/Desktop/onto/owl/tueba.owl#PRED -->

    <owl:NamedIndividual rdf:about="file:/C:/Users/Christian/Desktop/onto/owl/tueba.owl#PRED">
        <rdf:type rdf:resource="file:/C:/Users/Christian/Desktop/onto/owl/tueba.owl#Complement"/>
        <system:hasTag>PRED</system:hasTag>
        <rdfs:comment>predicate</rdfs:comment>
    </owl:NamedIndividual>
    


    <!-- file:/C:/Users/Christian/Desktop/onto/owl/tueba.owl#PRED-MOD -->

    <owl:NamedIndividual rdf:about="file:/C:/Users/Christian/Desktop/onto/owl/tueba.owl#PRED-MOD">
        <rdf:type rdf:resource="file:/C:/Users/Christian/Desktop/onto/owl/tueba.owl#Modifier"/>
        <rdfs:comment>modifiers modifying complements or modifiers, e.g. V-MOD = modifier of the verb</rdfs:comment>
        <system:hasTag>PRED-MOD</system:hasTag>
    </owl:NamedIndividual>
    


    <!-- file:/C:/Users/Christian/Desktop/onto/owl/tueba.owl#PREDK -->

    <owl:NamedIndividual rdf:about="file:/C:/Users/Christian/Desktop/onto/owl/tueba.owl#PREDK">
        <rdf:type rdf:resource="file:/C:/Users/Christian/Desktop/onto/owl/tueba.owl#SplitCoordination"/>
        <rdfs:comment>second conjunct (K) in split coordinations, e.g. ONK = second conjunct of a nominative object</rdfs:comment>
        <system:hasTag>PREDK</system:hasTag>
    </owl:NamedIndividual>
    


    <!-- file:/C:/Users/Christian/Desktop/onto/owl/tueba.owl#PX -->

    <owl:NamedIndividual rdf:about="file:/C:/Users/Christian/Desktop/onto/owl/tueba.owl#PX">
        <rdf:type rdf:resource="file:/C:/Users/Christian/Desktop/onto/owl/tueba.owl#Phrase"/>
        <rdfs:comment>prepositional phrase</rdfs:comment>
        <system:hasTag>PX</system:hasTag>
    </owl:NamedIndividual>
    


    <!-- file:/C:/Users/Christian/Desktop/onto/owl/tueba.owl#R-SIMPX -->

    <owl:NamedIndividual rdf:about="file:/C:/Users/Christian/Desktop/onto/owl/tueba.owl#R-SIMPX">
        <rdf:type rdf:resource="file:/C:/Users/Christian/Desktop/onto/owl/tueba.owl#Root"/>
        <system:hasTag>R-SIMPX</system:hasTag>
        <rdfs:comment>relative clause</rdfs:comment>
    </owl:NamedIndividual>
    


    <!-- file:/C:/Users/Christian/Desktop/onto/owl/tueba.owl#REFCONTR -->

    <owl:NamedIndividual rdf:about="file:/C:/Users/Christian/Desktop/onto/owl/tueba.owl#REFCONTR">
        <rdf:type rdf:resource="file:/C:/Users/Christian/Desktop/onto/owl/tueba.owl#SecondaryEdge"/>
        <rdfs:comment>dependency relation between control verb and its complement across clause boundaries.</rdfs:comment>
        <system:hasTag>REFCONTR</system:hasTag>
    </owl:NamedIndividual>
    


    <!-- file:/C:/Users/Christian/Desktop/onto/owl/tueba.owl#REFINT -->

    <owl:NamedIndividual rdf:about="file:/C:/Users/Christian/Desktop/onto/owl/tueba.owl#REFINT">
        <rdf:type rdf:resource="file:/C:/Users/Christian/Desktop/onto/owl/tueba.owl#SecondaryEdge"/>
        <system:hasTag>REFINT</system:hasTag>
        <rdfs:comment>dependency relation between a phrase-internal part and its modifier</rdfs:comment>
    </owl:NamedIndividual>
    


    <!-- file:/C:/Users/Christian/Desktop/onto/owl/tueba.owl#REFMOD -->

    <owl:NamedIndividual rdf:about="file:/C:/Users/Christian/Desktop/onto/owl/tueba.owl#REFMOD">
        <rdf:type rdf:resource="file:/C:/Users/Christian/Desktop/onto/owl/tueba.owl#SecondaryEdge"/>
        <system:hasTag>REFMOD</system:hasTag>
        <rdfs:comment>dependency relation between two ambiguous modifiers</rdfs:comment>
    </owl:NamedIndividual>
    


    <!-- file:/C:/Users/Christian/Desktop/onto/owl/tueba.owl#REFVC -->

    <owl:NamedIndividual rdf:about="file:/C:/Users/Christian/Desktop/onto/owl/tueba.owl#REFVC">
        <rdf:type rdf:resource="file:/C:/Users/Christian/Desktop/onto/owl/tueba.owl#SecondaryEdge"/>
        <rdfs:comment>dependency relation between two verbal objects in VC</rdfs:comment>
        <system:hasTag>REFVC</system:hasTag>
    </owl:NamedIndividual>
    


    <!-- file:/C:/Users/Christian/Desktop/onto/owl/tueba.owl#SIMPX -->

    <owl:NamedIndividual rdf:about="file:/C:/Users/Christian/Desktop/onto/owl/tueba.owl#SIMPX">
        <rdf:type rdf:resource="file:/C:/Users/Christian/Desktop/onto/owl/tueba.owl#Root"/>
        <rdfs:comment>simplex clause</rdfs:comment>
        <system:hasTag>SIMPX</system:hasTag>
    </owl:NamedIndividual>
    


    <!-- file:/C:/Users/Christian/Desktop/onto/owl/tueba.owl#V-MOD -->

    <owl:NamedIndividual rdf:about="file:/C:/Users/Christian/Desktop/onto/owl/tueba.owl#V-MOD">
        <rdf:type rdf:resource="file:/C:/Users/Christian/Desktop/onto/owl/tueba.owl#Modifier"/>
        <rdfs:comment>modifiers modifying complements or modifiers, e.g. V-MOD = modifier of the verb</rdfs:comment>
        <system:hasTag>V-MOD</system:hasTag>
    </owl:NamedIndividual>
    


    <!-- file:/C:/Users/Christian/Desktop/onto/owl/tueba.owl#V-MODK -->

    <owl:NamedIndividual rdf:about="file:/C:/Users/Christian/Desktop/onto/owl/tueba.owl#V-MODK">
        <rdf:type rdf:resource="file:/C:/Users/Christian/Desktop/onto/owl/tueba.owl#SplitCoordination"/>
        <system:hasTag>V-MODK</system:hasTag>
        <rdfs:comment>second conjunct (K) in split coordinations, e.g. ONK = second conjunct of a nominative object</rdfs:comment>
    </owl:NamedIndividual>
    


    <!-- file:/C:/Users/Christian/Desktop/onto/owl/tueba.owl#VC -->

    <owl:NamedIndividual rdf:about="file:/C:/Users/Christian/Desktop/onto/owl/tueba.owl#VC">
        <rdf:type rdf:resource="file:/C:/Users/Christian/Desktop/onto/owl/tueba.owl#TopologicalField"/>
        <system:hasTag>VC</system:hasTag>
        <rdfs:comment>The Verbkomplex is a sequence of verb forms. In verb-second and verb-first
clauses it consists of one or more non-finite elements or - depending on the verb - of
a separable prefix. In verb-final clauses it also contains the finite verb. The rule for
the linear order in general is: right determines left. If there is a finite verb in the verb
complex, it is usually the right-most element.
(Telljohann et al. 2009)</rdfs:comment>
        <rdfs:comment>verb complex (Verbkomplex)</rdfs:comment>
    </owl:NamedIndividual>
    


    <!-- file:/C:/Users/Christian/Desktop/onto/owl/tueba.owl#VCE -->

    <owl:NamedIndividual rdf:about="file:/C:/Users/Christian/Desktop/onto/owl/tueba.owl#VCE">
        <rdf:type rdf:resource="file:/C:/Users/Christian/Desktop/onto/owl/tueba.owl#TopologicalField"/>
        <rdfs:comment>verb complex with the split finite verb of Ersatzinfinitiv constructions</rdfs:comment>
        <system:hasTag>VCE</system:hasTag>
    </owl:NamedIndividual>
    


    <!-- file:/C:/Users/Christian/Desktop/onto/owl/tueba.owl#VF -->

    <owl:NamedIndividual rdf:about="file:/C:/Users/Christian/Desktop/onto/owl/tueba.owl#VF">
        <rdf:type rdf:resource="file:/C:/Users/Christian/Desktop/onto/owl/tueba.owl#TopologicalField"/>
        <system:hasTag>VF</system:hasTag>
        <rdfs:comment>The Vorfeld consists of only one constituent. Usually it is the subject. But
because of the high degree of non-configurationality in German, the subject can also
occur in theMittelfeld, thus allowing almost every other constituent to occupy the Vorfeld.
(Telljohann et al. 2009, p.15)</rdfs:comment>
        <rdfs:comment>initial field (Vorfeld)</rdfs:comment>
    </owl:NamedIndividual>
    


    <!-- file:/C:/Users/Christian/Desktop/onto/owl/tueba.owl#VPT -->

    <owl:NamedIndividual rdf:about="file:/C:/Users/Christian/Desktop/onto/owl/tueba.owl#VPT">
        <rdf:type rdf:resource="file:/C:/Users/Christian/Desktop/onto/owl/tueba.owl#Complement"/>
        <rdfs:comment>separable verb prefix</rdfs:comment>
        <system:hasTag>VPT</system:hasTag>
    </owl:NamedIndividual>
    


    <!-- file:/C:/Users/Christian/Desktop/onto/owl/tueba.owl#VXFIN -->

    <owl:NamedIndividual rdf:about="file:/C:/Users/Christian/Desktop/onto/owl/tueba.owl#VXFIN">
        <rdf:type rdf:resource="file:/C:/Users/Christian/Desktop/onto/owl/tueba.owl#Phrase"/>
        <system:hasTag>VXFIN</system:hasTag>
        <rdfs:comment>finite verb phrase</rdfs:comment>
    </owl:NamedIndividual>
    


    <!-- file:/C:/Users/Christian/Desktop/onto/owl/tueba.owl#VXINF -->

    <owl:NamedIndividual rdf:about="file:/C:/Users/Christian/Desktop/onto/owl/tueba.owl#VXINF">
        <rdf:type rdf:resource="file:/C:/Users/Christian/Desktop/onto/owl/tueba.owl#Phrase"/>
        <system:hasTag>VXINF</system:hasTag>
        <rdfs:comment>non-finite verb phrase</rdfs:comment>
    </owl:NamedIndividual>
    


    <!-- file:/C:/Users/Christian/Desktop/onto/owl/tueba.owl#accusative -->

    <owl:NamedIndividual rdf:about="file:/C:/Users/Christian/Desktop/onto/owl/tueba.owl#accusative">
        <rdf:type rdf:resource="file:/C:/Users/Christian/Desktop/onto/owl/tueba.owl#Case"/>
        <hasTagContaining>a</hasTagContaining>
    </owl:NamedIndividual>
    


    <!-- file:/C:/Users/Christian/Desktop/onto/owl/tueba.owl#dative -->

    <owl:NamedIndividual rdf:about="file:/C:/Users/Christian/Desktop/onto/owl/tueba.owl#dative">
        <rdf:type rdf:resource="file:/C:/Users/Christian/Desktop/onto/owl/tueba.owl#Case"/>
        <hasTagContaining>d</hasTagContaining>
    </owl:NamedIndividual>
    


    <!-- file:/C:/Users/Christian/Desktop/onto/owl/tueba.owl#feminine -->

    <owl:NamedIndividual rdf:about="file:/C:/Users/Christian/Desktop/onto/owl/tueba.owl#feminine">
        <rdf:type rdf:resource="file:/C:/Users/Christian/Desktop/onto/owl/tueba.owl#Gender"/>
        <hasTagContaining>f</hasTagContaining>
    </owl:NamedIndividual>
    


    <!-- file:/C:/Users/Christian/Desktop/onto/owl/tueba.owl#first -->

    <owl:NamedIndividual rdf:about="file:/C:/Users/Christian/Desktop/onto/owl/tueba.owl#first">
        <rdf:type rdf:resource="file:/C:/Users/Christian/Desktop/onto/owl/tueba.owl#Person"/>
        <hasTagContaining>1</hasTagContaining>
    </owl:NamedIndividual>
    


    <!-- file:/C:/Users/Christian/Desktop/onto/owl/tueba.owl#genitive -->

    <owl:NamedIndividual rdf:about="file:/C:/Users/Christian/Desktop/onto/owl/tueba.owl#genitive">
        <rdf:type rdf:resource="file:/C:/Users/Christian/Desktop/onto/owl/tueba.owl#Case"/>
        <hasTagContaining>g</hasTagContaining>
    </owl:NamedIndividual>
    


    <!-- file:/C:/Users/Christian/Desktop/onto/owl/tueba.owl#indicative -->

    <owl:NamedIndividual rdf:about="file:/C:/Users/Christian/Desktop/onto/owl/tueba.owl#indicative">
        <rdf:type rdf:resource="file:/C:/Users/Christian/Desktop/onto/owl/tueba.owl#Mood"/>
        <hasTagContaining>i</hasTagContaining>
    </owl:NamedIndividual>
    


    <!-- file:/C:/Users/Christian/Desktop/onto/owl/tueba.owl#masculine -->

    <owl:NamedIndividual rdf:about="file:/C:/Users/Christian/Desktop/onto/owl/tueba.owl#masculine">
        <rdf:type rdf:resource="file:/C:/Users/Christian/Desktop/onto/owl/tueba.owl#Gender"/>
        <hasTagContaining>m</hasTagContaining>
    </owl:NamedIndividual>
    


    <!-- file:/C:/Users/Christian/Desktop/onto/owl/tueba.owl#neuter -->

    <owl:NamedIndividual rdf:about="file:/C:/Users/Christian/Desktop/onto/owl/tueba.owl#neuter">
        <rdf:type rdf:resource="file:/C:/Users/Christian/Desktop/onto/owl/tueba.owl#Gender"/>
        <hasTagContaining>sn</hasTagContaining>
        <hasTagContaining>*n</hasTagContaining>
        <hasTagContaining>pn</hasTagContaining>
        <rdfs:comment>gender is always preceded by number, hence disambiguation by filtering for all possible values of number</rdfs:comment>
    </owl:NamedIndividual>
    


    <!-- file:/C:/Users/Christian/Desktop/onto/owl/tueba.owl#nominative -->

    <owl:NamedIndividual rdf:about="file:/C:/Users/Christian/Desktop/onto/owl/tueba.owl#nominative">
        <rdf:type rdf:resource="file:/C:/Users/Christian/Desktop/onto/owl/tueba.owl#Case"/>
        <rdfs:comment>case is always the first feature (Telljohann et al. 2009, p. 22), disambiguation by position</rdfs:comment>
        <hasTagStartingWith>n</hasTagStartingWith>
    </owl:NamedIndividual>
    


    <!-- file:/C:/Users/Christian/Desktop/onto/owl/tueba.owl#non-head -->

    <owl:NamedIndividual rdf:about="file:/C:/Users/Christian/Desktop/onto/owl/tueba.owl#non-head">
        <rdf:type rdf:resource="file:/C:/Users/Christian/Desktop/onto/owl/tueba.owl#HeadOrConjunct"/>
        <hasTagContaining>-</hasTagContaining>
        <rdfs:comment>non-head</rdfs:comment>
    </owl:NamedIndividual>
    


    <!-- file:/C:/Users/Christian/Desktop/onto/owl/tueba.owl#past -->

    <owl:NamedIndividual rdf:about="file:/C:/Users/Christian/Desktop/onto/owl/tueba.owl#past">
        <rdf:type rdf:resource="file:/C:/Users/Christian/Desktop/onto/owl/tueba.owl#Tense"/>
        <hasTagContaining>t</hasTagContaining>
    </owl:NamedIndividual>
    


    <!-- file:/C:/Users/Christian/Desktop/onto/owl/tueba.owl#plural -->

    <owl:NamedIndividual rdf:about="file:/C:/Users/Christian/Desktop/onto/owl/tueba.owl#plural">
        <rdf:type rdf:resource="file:/C:/Users/Christian/Desktop/onto/owl/tueba.owl#Number"/>
        <hasTagContaining>p</hasTagContaining>
    </owl:NamedIndividual>
    


    <!-- file:/C:/Users/Christian/Desktop/onto/owl/tueba.owl#present -->

    <owl:NamedIndividual rdf:about="file:/C:/Users/Christian/Desktop/onto/owl/tueba.owl#present">
        <rdf:type rdf:resource="file:/C:/Users/Christian/Desktop/onto/owl/tueba.owl#Tense"/>
        <hasTagEndingWith>is</hasTagEndingWith>
        <rdfs:comment>tag ambiguous with singular, tense, however, always following mood, disambiguated by combination with all possible mood values</rdfs:comment>
        <hasTagEndingWith>ks</hasTagEndingWith>
    </owl:NamedIndividual>
    


    <!-- file:/C:/Users/Christian/Desktop/onto/owl/tueba.owl#second -->

    <owl:NamedIndividual rdf:about="file:/C:/Users/Christian/Desktop/onto/owl/tueba.owl#second">
        <rdf:type rdf:resource="file:/C:/Users/Christian/Desktop/onto/owl/tueba.owl#Person"/>
        <hasTagContaining>2</hasTagContaining>
    </owl:NamedIndividual>
    


    <!-- file:/C:/Users/Christian/Desktop/onto/owl/tueba.owl#singular -->

    <owl:NamedIndividual rdf:about="file:/C:/Users/Christian/Desktop/onto/owl/tueba.owl#singular">
        <rdf:type rdf:resource="file:/C:/Users/Christian/Desktop/onto/owl/tueba.owl#Number"/>
        <hasTagContaining>2s</hasTagContaining>
        <hasTagContaining>ds</hasTagContaining>
        <hasTagContaining>1s</hasTagContaining>
        <hasTagContaining>*s</hasTagContaining>
        <hasTagContaining>3s</hasTagContaining>
        <hasTagContaining>gs</hasTagContaining>
        <hasTagContaining>ns</hasTagContaining>
        <hasTagContaining>as</hasTagContaining>
        <system:hasTag>s</system:hasTag>
        <rdfs:comment>tag ambiguous with present (s), ambiguity distributionally resolved:
1) number may stand alone
2) number follows case
3) number follows person</rdfs:comment>
    </owl:NamedIndividual>
    


    <!-- file:/C:/Users/Christian/Desktop/onto/owl/tueba.owl#subjunctive -->

    <owl:NamedIndividual rdf:about="file:/C:/Users/Christian/Desktop/onto/owl/tueba.owl#subjunctive">
        <rdf:type rdf:resource="file:/C:/Users/Christian/Desktop/onto/owl/tueba.owl#Mood"/>
        <rdfs:comment>German &quot;Konjunktiv&quot;</rdfs:comment>
        <hasTagContaining>k</hasTagContaining>
    </owl:NamedIndividual>
    


    <!-- file:/C:/Users/Christian/Desktop/onto/owl/tueba.owl#third -->

    <owl:NamedIndividual rdf:about="file:/C:/Users/Christian/Desktop/onto/owl/tueba.owl#third">
        <rdf:type rdf:resource="file:/C:/Users/Christian/Desktop/onto/owl/tueba.owl#Person"/>
        <hasTagContaining>3</hasTagContaining>
    </owl:NamedIndividual>
    


    <!-- 
    ///////////////////////////////////////////////////////////////////////////////////////
    //
    // Annotations
    //
    ///////////////////////////////////////////////////////////////////////////////////////
     -->

    <rdf:Description rdf:about="&stts;VVPP">
        <rdfs:comment>past participle, main, e.g., &quot;gegangen&quot;, &quot;angekommen&quot;</rdfs:comment>
    </rdf:Description>
    <rdf:Description rdf:about="&stts;PPER">
        <rdfs:comment>irreflexive personal pronoun, e.g., &quot;ich&quot;, &quot;er&quot;, &quot;ihm&quot;, &quot;mich&quot;, &quot;dir&quot;</rdfs:comment>
    </rdf:Description>
    <rdf:Description rdf:about="&stts;VMFIN">
        <rdfs:comment>finite verb, modal, e.g., &quot;d&#252;rfen&quot;</rdfs:comment>
    </rdf:Description>
    <rdf:Description rdf:about="&stts;PTKNEG">
        <rdfs:comment>negation particle &quot;nicht&quot;</rdfs:comment>
    </rdf:Description>
    <rdf:Description rdf:about="&stts;KON">
        <rdfs:comment>coordinative conjunction, e.g., &quot;und&quot;, &quot;oder&quot;, &quot;aber&quot;</rdfs:comment>
    </rdf:Description>
    <rdf:Description rdf:about="&stts;ADJA">
        <rdfs:comment>attributive adjective, e.g. &quot;[das] gro&#223;e [Haus]&quot;</rdfs:comment>
    </rdf:Description>
    <rdf:Description rdf:about="&stts;ART">
        <rdfs:comment>definite or indefinite article, e.g.,  &quot;der&quot;, &quot;die&quot;, &quot;das&quot;, &quot;ein&quot;, &quot;eine&quot;</rdfs:comment>
    </rdf:Description>
    <rdf:Description rdf:about="&stts;VVIMP">
        <rdfs:comment>imperative, main verb, e.g., &quot;komm [!]&quot;</rdfs:comment>
    </rdf:Description>
    <rdf:Description rdf:about="&stts;VMINF">
        <rdfs:comment>infinitive, modal, e.g., &quot;wollen&quot;</rdfs:comment>
    </rdf:Description>
    <rdf:Description rdf:about="&stts;PPOSAT">
        <rdfs:comment>attributive possessive pronoun, e.g., &quot;mein [Buch]&quot;, &quot;deine [Mutter]&quot;</rdfs:comment>
    </rdf:Description>
    <rdf:Description rdf:about="&stts;VVINF">
        <rdfs:comment>infinitive, main, e.g., &quot;gehen&quot;, &quot;ankommen&quot;</rdfs:comment>
    </rdf:Description>
    <rdf:Description rdf:about="&stts;PRELAT">
        <rdfs:comment>attributive relative pronoun, e.g., &quot;[der Mann ,] dessen [Hund]&quot;</rdfs:comment>
    </rdf:Description>
    <rdf:Description rdf:about="&stts;VAIMP">
        <rdfs:comment>imperative, aux, e.g., &quot;sei [ruhig !]&quot;</rdfs:comment>
    </rdf:Description>
    <rdf:Description rdf:about="&stts;ADV">
        <rdfs:comment>adverb, e.g., &quot;schon&quot;, &quot;bald&quot;, &quot;doch&quot;</rdfs:comment>
    </rdf:Description>
    <rdf:Description rdf:about="&stts;ADJD">
        <rdfs:comment>adverbial or predicative adjective, e.g. &quot;[er f&#168;ahrt] schnell&quot;, &quot;[er ist] schnell&quot;</rdfs:comment>
    </rdf:Description>
    <rdf:Description rdf:about="&stts;PIS">
        <rdfs:comment>substituting indefinite pronoun, e.g., &quot;keiner&quot;, &quot;viele&quot;, &quot;man&quot;, &quot;niemand&quot;
</rdfs:comment>
    </rdf:Description>
    <rdf:Description rdf:about="&stts;CARD">
        <rdfs:comment>cardinal number, e.g.,  &quot;zwei [M&#228;nner]&quot;, &quot;[im Jahre] 1994&quot;</rdfs:comment>
    </rdf:Description>
    <rdf:Description rdf:about="&stts;NN">
        <rdfs:comment>noun, e.g.,  &quot;Tisch&quot;, &quot;Herr&quot;, &quot;[das] Reisen&quot;</rdfs:comment>
    </rdf:Description>
    <rdf:Description rdf:about="&stts;KOKOM">
        <rdfs:comment>particle of comparison, no clause, e.g., &quot;als&quot;, &quot;wie&quot;</rdfs:comment>
    </rdf:Description>
    <rdf:Description rdf:about="&stts;VVIZU">
        <rdfs:comment>infinitive + zu, main, e.g., &quot;anzukommen, loszulassen&quot;</rdfs:comment>
    </rdf:Description>
    <rdf:Description rdf:about="&stts;PIDAT">
        <rdfs:comment>attributive indefinite pronoun with determiner, e g., &quot;[ein] wenig [Wasser]&quot;, &quot;[die] beiden [Br&#252;der]&quot;</rdfs:comment>
    </rdf:Description>
    <rdf:Description rdf:about="&stts;FM">
        <rdfs:comment>foreign language material, e.g.,  &quot;[Er hat das mit &#8220;A big fish &#8221; &#252;bersetzt]&quot;</rdfs:comment>
    </rdf:Description>
    <rdf:Description rdf:about="&stts;KOUS">
        <rdfs:comment>subordinating conjunction with clause, e.g., &quot;weil&quot;, &quot;da&#223;&quot;, &quot;damit&quot;, &quot;wenn&quot;, &quot;ob&quot; (Telljohann et al. 2009)
</rdfs:comment>
    </rdf:Description>
    <rdf:Description rdf:about="&stts;APPR">
        <rdfs:comment>preposition; left circumposition, e.g., &quot;in [der Stadt]&quot;, &quot;ohne [mich]&quot;</rdfs:comment>
    </rdf:Description>
    <rdf:Description rdf:about="&stts;TRUNC">
        <rdfs:comment>truncated word - first part, e.g., &quot;An&#8211; [und Abreise]&quot;</rdfs:comment>
    </rdf:Description>
    <rdf:Description rdf:about="&stts;APPO">
        <rdfs:comment>postposition, e.g., &quot;[ihm] zufolge&quot;, &quot;[der Sache] wegen&quot;</rdfs:comment>
    </rdf:Description>
    <rdf:Description rdf:about="&stts;VAINF">
        <rdfs:comment>infinitive, aux, e.g., &quot;werden&quot;, &quot;sein&quot;</rdfs:comment>
    </rdf:Description>
    <rdf:Description rdf:about="&stts;PWAT">
        <rdfs:comment>attributive interrogative pronoun, e.g., &quot;welche [Farbe]&quot;, &quot;wessen [Hut]&quot;
</rdfs:comment>
    </rdf:Description>
    <rdf:Description rdf:about="&stts;PTKANT">
        <rdfs:comment>answer particle, e.g. &quot;ja&quot;, &quot;nein&quot;, &quot;danke&quot;, &quot;bitte&quot;</rdfs:comment>
    </rdf:Description>
    <rdf:Description rdf:about="&stts;PTKA">
        <rdfs:comment>particle with adjective or adverb, e.g., &quot;am [sch&#246;nsten]&quot;, &quot;zu [schnell]&quot;
</rdfs:comment>
    </rdf:Description>
    <rdf:Description rdf:about="&stts;NNE">
        <rdfs:comment>not used in T&#252;Ba-D/Z (cf. Telljohann et al. 2009, p. 20f.)</rdfs:comment>
    </rdf:Description>
    <rdf:Description rdf:about="&stts;APPRART">
        <rdfs:comment>preposition + article, e.g., &quot;im [Haus]&quot;, &quot;zur [Sache]&quot;</rdfs:comment>
    </rdf:Description>
    <rdf:Description rdf:about="&stts;NE">
        <rdfs:comment>proper noun, e.g., &quot;Hans&quot;, &quot;Hamburg&quot;, &quot;HSV&quot;</rdfs:comment>
    </rdf:Description>
    <rdf:Description rdf:about="&stts;PWAV">
        <rdfs:comment>adverbial interrogative or relative pronoun, e.g., &quot;warum&quot;, &quot;wo&quot;, &quot;wann&quot;, &quot;wor&#252;ber&quot;, &quot;wobei&quot;
</rdfs:comment>
    </rdf:Description>
    <rdf:Description rdf:about="&stts;PPOSS">
        <rdfs:comment>substituting possessive pronoun, e.g., &quot;meins&quot;, &quot;deiner&quot;</rdfs:comment>
    </rdf:Description>
    <rdf:Description rdf:about="&stts;PROP">
        <rdfs:comment>pronominal adverb, e.g., &quot;daf&#252;r&quot;, &quot;dabei&quot;, &quot;deswegen&quot;, &quot;trotzdem&quot;</rdfs:comment>
    </rdf:Description>
    <rdf:Description rdf:about="&stts;PRF">
        <rdfs:comment>reflexive personal pronoun &quot;sich&quot;, &quot;einander&quot;, &quot;dich&quot;, &quot;mir&quot;</rdfs:comment>
    </rdf:Description>
    <rdf:Description rdf:about="&stts;VMPP">
        <rdfs:comment>past participle, modal, e.g., &quot;[er hat] gekonnt&quot;</rdfs:comment>
    </rdf:Description>
    <rdf:Description rdf:about="&stts;PDS">
        <rdfs:comment>substituting demonstrative pronoun, e.g., &quot;dieser&quot;, &quot;jener&quot;
</rdfs:comment>
    </rdf:Description>
    <rdf:Description rdf:about="&stts;XY">
        <rdfs:comment>non-word containing special characters, e.g., &quot;D2XW3&quot;, letters
</rdfs:comment>
    </rdf:Description>
    <rdf:Description rdf:about="&stts;VAFIN">
        <rdfs:comment>finite verb, aux, e.g., &quot;[du] bist&quot;, &quot;[wir] werden&quot;</rdfs:comment>
    </rdf:Description>
    <rdf:Description rdf:about="&stts;PWS">
        <rdfs:comment>substituting interrogative pronoun, e.g., &quot;wer&quot;, &quot;was&quot;
</rdfs:comment>
    </rdf:Description>
    <rdf:Description rdf:about="&stts;APZR">
        <rdfs:comment>right circumposition, e.g., &quot;[von jetzt] an&quot;</rdfs:comment>
    </rdf:Description>
    <rdf:Description rdf:about="&stts;VVFIN">
        <rdfs:comment>finite main verb, e.g., &quot;[du] gehst&quot;, &quot;[wir] kommen [an]&quot;</rdfs:comment>
    </rdf:Description>
    <rdf:Description rdf:about="&stts;PTKVZ">
        <rdfs:comment>separated verb particle, e.g., &quot;[er kommt] an&quot;, &quot;[er f&#228;hrt] rad&quot;</rdfs:comment>
    </rdf:Description>
    <rdf:Description rdf:about="&stts;PDAT">
        <rdfs:comment>attributive demonstrative pronoun, e.g., &quot;jener [Mensch]&quot;
</rdfs:comment>
    </rdf:Description>
    <rdf:Description rdf:about="&stts;VAPP">
        <rdfs:comment>past participle, aux, e.g., &quot;gewesen&quot;</rdfs:comment>
    </rdf:Description>
    <rdf:Description rdf:about="&stts;ITJ">
        <rdfs:comment>interjection, e.g., &quot;mhm&quot;, &quot;ach&quot;, &quot;tja&quot;</rdfs:comment>
    </rdf:Description>
    <rdf:Description rdf:about="&stts;PTKZU">
        <rdfs:comment>zu + infinitive, e.g.,  &quot;zu [gehen]&quot;</rdfs:comment>
    </rdf:Description>
    <rdf:Description rdf:about="&stts;KOUI">
        <rdfs:comment>subordinating conjunction with zu + infinitive, e.g.,  &quot;um [zu leben]&quot;, &quot;anstatt [zu fragen]&quot; (Telljohann et al. 2009)
</rdfs:comment>
    </rdf:Description>
    <rdf:Description rdf:about="&stts;PIAT">
        <rdfs:comment>attributive indefinite pronoun without determiner, e.g., &quot;kein [Mensch]&quot;, &quot;irgendein [Glas]&quot;
</rdfs:comment>
    </rdf:Description>
    <rdf:Description rdf:about="&stts;PRELS">
        <rdfs:comment>substituting relative pronoun, e.g., &quot;[der Hund,] der&quot;</rdfs:comment>
    </rdf:Description>
</rdf:RDF>



<!-- Generated by the OWL API (version 3.0.0.1451) http://owlapi.sourceforge.net -->

