<?xml version="1.0" encoding="UTF-8"?>
<rdf:RDF xmlns:xsd="http://www.w3.org/2001/XMLSchema#"
         xmlns="http://www.isocat.org/ns/dcr.owl#"
         xmlns:dcr="http://www.isocat.org/ns/dcr.rdf#"
         xmlns:rdfs="http://www.w3.org/2000/01/rdf-schema#"
         xmlns:owl="http://www.w3.org/2002/07/owl#"
         xmlns:dcif="http://www.isocat.org/ns/dcif"
         xmlns:rdf="http://www.w3.org/1999/02/22-rdf-syntax-ns#"
         xml:base="http://www.isocat.org/ns/dcr.owl">
   <owl:Ontology>
      <rdfs:comment>OWL representation of ISOcat DCIF exported Data Categories</rdfs:comment>
   </owl:Ontology>
   <owl:Class rdf:ID="ppron3">
      <dcr:datcat rdf:resource="http://www.isocat.org/datcat/DC-2762"/>
      <owl:versionInfo>http://www.isocat.org/datcat/DC-2762</owl:versionInfo>
      <rdfs:comment>
            3rd person pronoun [ppron3] contains exactly one flexeme, on `he', with lexically determined person (3rd), inflecting for number, case and gender; some forms additionally inflect for accentability and post-prepositionality (e.g., niego vs. go, `him.acc'). Grammatical categories of [ppron3]: number (http://www.isocat.org/datcat/DC-2709), case (http://www.isocat.org/datcat/DC-2720), gender (http://www.isocat.org/datcat/DC-2728), person (http://www.isocat.org/datcat/DC-2775), accentability (http://www.isocat.org/datcat/DC-2737) (optional), post-prepositionality (http://www.isocat.org/datcat/DC-2740) (optional).
                (http://www.isocat.org/datcat/DC-2762)
            </rdfs:comment>
      <rdfs:label>3rd person pronoun</rdfs:label>
   </owl:Class>
   <owl:Class rdf:ID="brev">
      <dcr:datcat rdf:resource="http://www.isocat.org/datcat/DC-2774"/>
      <owl:versionInfo>http://www.isocat.org/datcat/DC-2774</owl:versionInfo>
      <rdfs:comment>
            Abbreviation [brev] class has a technical category associated with it, “fullstoppedness”, which may take one of two values: pun (the abbreviation segment should be followed by a full stop) and npun (the segment does not have to be followed by a full stop). Grammatical categories of abbreviation [brev]: fullstoppedness (http://www.isocat.org/datcat/DC-2789).
                (http://www.isocat.org/datcat/DC-2774)
            </rdfs:comment>
      <rdfs:label>abbreviation</rdfs:label>
   </owl:Class>
   <owl:Class rdf:ID="accentability">
      <dcr:datcat rdf:resource="http://www.isocat.org/datcat/DC-2737"/>
      <owl:versionInfo>http://www.isocat.org/datcat/DC-2737</owl:versionInfo>
      <rdfs:comment>
            Accentability [accentability] is a grammatical category appropriate for some forms of personal pronouns which takes one of two values depending on whether the pronominal form is accented (strong) or not (weak).
                (http://www.isocat.org/datcat/DC-2737)
            </rdfs:comment>
      <rdfs:label>accentability</rdfs:label>
   </owl:Class>
   <owl:Class rdf:ID="akc">
      <dcr:datcat rdf:resource="http://www.isocat.org/datcat/DC-2738"/>
      <owl:versionInfo>http://www.isocat.org/datcat/DC-2738</owl:versionInfo>
      <rdfs:comment>
            accented (strong) [akc] form of the pronoun
                (http://www.isocat.org/datcat/DC-2738)
            </rdfs:comment>
      <rdfs:label>accented (strong)</rdfs:label>
      <rdfs:subClassOf>
         <owl:Class rdf:about="#accentability"/>
      </rdfs:subClassOf>
      <owl:versionInfo>subClassOf accentability (dcif:conceptualDomain)</owl:versionInfo>
   </owl:Class>
   <owl:Class rdf:ID="accommodability">
      <dcr:datcat rdf:resource="http://www.isocat.org/datcat/DC-2734"/>
      <owl:versionInfo>http://www.isocat.org/datcat/DC-2734</owl:versionInfo>
      <rdfs:comment>
            The category of accommodability [accommodability] is appropriate to all numeral forms. The value of this category for a given numeral form is 'agreeing' if and only if that numeral form agrees in case with the accompanying noun.
                (http://www.isocat.org/datcat/DC-2734)
            </rdfs:comment>
      <rdfs:label>accommodability</rdfs:label>
   </owl:Class>
   <owl:Class rdf:ID="acc">
      <dcr:datcat rdf:resource="http://www.isocat.org/datcat/DC-2724"/>
      <owl:versionInfo>http://www.isocat.org/datcat/DC-2724</owl:versionInfo>
      <rdfs:comment>
            Accusative [acc] is a value of the grammatical category of case paradigmatically appropriate for structural objects.
                (http://www.isocat.org/datcat/DC-2724)
            </rdfs:comment>
      <rdfs:label>accusative case</rdfs:label>
      <rdfs:subClassOf>
         <owl:Class rdf:about="#case"/>
      </rdfs:subClassOf>
      <owl:versionInfo>subClassOf case (dcif:conceptualDomain)</owl:versionInfo>
   </owl:Class>
   <owl:Class rdf:ID="pact">
      <dcr:datcat rdf:resource="http://www.isocat.org/datcat/DC-2766"/>
      <owl:versionInfo>http://www.isocat.org/datcat/DC-2766</owl:versionInfo>
      <rdfs:comment>
            Active adjectival participle [pact] contains active adjectival participles, inflecting for number, case, gender and negation, with lexical aspect (always imperfective), e.g., pijący `drinking'. Grammatical categories of active adjectival participle [pact]: number (http://www.isocat.org/datcat/DC-2709), case (http://www.isocat.org/datcat/DC-2720), gender (http://www.isocat.org/datcat/DC-2728), aspect (http://www.isocat.org/datcat/DC-2783), negation (http://www.isocat.org/datcat/DC-2786).
                (http://www.isocat.org/datcat/DC-2766)
            </rdfs:comment>
      <rdfs:label>active adjectival participle</rdfs:label>
   </owl:Class>
   <owl:Class rdf:ID="adja">
      <dcr:datcat rdf:resource="http://www.isocat.org/datcat/DC-2705"/>
      <owl:versionInfo>http://www.isocat.org/datcat/DC-2705</owl:versionInfo>
      <rdfs:comment>
            ad-adjectival adjective [adja] contains non-inflecting de-adjectival lexemes such as polsko 'Polish' and niemiecko 'German'
                (http://www.isocat.org/datcat/DC-2705)
            </rdfs:comment>
      <rdfs:label>ad-adjectival adjective</rdfs:label>
   </owl:Class>
   <owl:Class rdf:ID="adj">
      <dcr:datcat rdf:resource="http://www.isocat.org/datcat/DC-2765"/>
      <owl:versionInfo>http://www.isocat.org/datcat/DC-2765</owl:versionInfo>
      <rdfs:comment>
            Adjective [adj] contains flexemes inflecting for number, case and gender, as well as - in some cases - for degree, e.g., miły `nice', techniczny `technical', taki `such', który `which', piąty `fifth', wielokrotny `manifold' and jeden `one'. Grammatical categories of adjective [adj]: number (http://www.isocat.org/datcat/DC-2709), case (http://www.isocat.org/datcat/DC-2720), gender (http://www.isocat.org/datcat/DC-2728), degree (http://www.isocat.org/datcat/DC-2779).
                (http://www.isocat.org/datcat/DC-2765)
            </rdfs:comment>
      <rdfs:label>adjective</rdfs:label>
   </owl:Class>
   <owl:Class rdf:ID="adv">
      <dcr:datcat rdf:resource="http://www.isocat.org/datcat/DC-2751"/>
      <owl:versionInfo>http://www.isocat.org/datcat/DC-2751</owl:versionInfo>
      <rdfs:comment>
            Adverb [adv] contains those flexemes which only inflect for degree (gradable adverbs, e.g., bardzo `very', miło `nicely'), as well as non-inflecting deadjectival flexemes such as non-gradable de-adjectival adverbs, e.g., technicznie which belong to neither of these classes: ad-adjectival adjective (http://www.isocat.org/datcat/DC-2705) and post-prepositional adjective (http://www.isocat.org/datcat/DC-2706). Grammatical categories of adverb [adv]: degree (http://www.isocat.org/datcat/DC-2779) (optional).
                (http://www.isocat.org/datcat/DC-2751)
            </rdfs:comment>
      <rdfs:label>adverb</rdfs:label>
   </owl:Class>
   <owl:Class rdf:ID="aff">
      <dcr:datcat rdf:resource="http://www.isocat.org/datcat/DC-2787"/>
      <owl:versionInfo>http://www.isocat.org/datcat/DC-2787</owl:versionInfo>
      <rdfs:comment>
            Affirmative [aff] is a value of the grammatical category of negation appropriate for the non-negated variant of the verbal form which can be negated by ortographically joining the negative prefix nie-.
                (http://www.isocat.org/datcat/DC-2787)
            </rdfs:comment>
      <rdfs:label>affirmative</rdfs:label>
      <rdfs:subClassOf>
         <owl:Class rdf:about="#negation"/>
      </rdfs:subClassOf>
      <owl:versionInfo>subClassOf negation (dcif:conceptualDomain)</owl:versionInfo>
   </owl:Class>
   <owl:Class rdf:ID="aglt">
      <dcr:datcat rdf:resource="http://www.isocat.org/datcat/DC-2773"/>
      <owl:versionInfo>http://www.isocat.org/datcat/DC-2773</owl:versionInfo>
      <rdfs:comment>
            Agglutinate BYĆ [aglt] contains one flexeme, consisting of the agglutinative forms of być: -m, -em, -śmy, etc. Grammatical categories of agglutinate BYĆ [aglt]: number (http://www.isocat.org/datcat/DC-2709), person (http://www.isocat.org/datcat/DC-2775), aspect (http://www.isocat.org/datcat/DC-2783), vocalicity (http://www.isocat.org/datcat/DC-2748).
                (http://www.isocat.org/datcat/DC-2773)
            </rdfs:comment>
      <rdfs:label>agglutinate BYĆ</rdfs:label>
   </owl:Class>
   <owl:Class rdf:ID="agglutination">
      <dcr:datcat rdf:resource="http://www.isocat.org/datcat/DC-2745"/>
      <owl:versionInfo>http://www.isocat.org/datcat/DC-2745</owl:versionInfo>
      <rdfs:comment>
            The form which combines with the agglutinate (e.g., with -em), for example the form niosł-, will be marked as agglutinative [agl], while the form occurring on its own, e.g., the form niósł, will be marked as non-agglutinative [nagl].
                (http://www.isocat.org/datcat/DC-2745)
            </rdfs:comment>
      <rdfs:label>agglutination</rdfs:label>
   </owl:Class>
   <owl:Class rdf:ID="agl">
      <dcr:datcat rdf:resource="http://www.isocat.org/datcat/DC-2747"/>
      <owl:versionInfo>http://www.isocat.org/datcat/DC-2747</owl:versionInfo>
      <rdfs:comment>
            Agglutinative [agl] form does not occur on its own, it combines with the agglutinate.
                (http://www.isocat.org/datcat/DC-2747)
            </rdfs:comment>
      <rdfs:label>agglutinative</rdfs:label>
      <rdfs:subClassOf>
         <owl:Class rdf:about="#agglutination"/>
      </rdfs:subClassOf>
      <owl:versionInfo>subClassOf agglutination (dcif:conceptualDomain)</owl:versionInfo>
   </owl:Class>
   <owl:Class rdf:ID="congr">
      <dcr:datcat rdf:resource="http://www.isocat.org/datcat/DC-2735"/>
      <owl:versionInfo>http://www.isocat.org/datcat/DC-2735</owl:versionInfo>
      <rdfs:comment>
            Agreeing [congr] is a value of the grammatical category of accommodability appropriate for a numeral form if and only if it agrees in case with the accompanying noun.
                (http://www.isocat.org/datcat/DC-2735)
            </rdfs:comment>
      <rdfs:label>agreeing accommodability</rdfs:label>
      <rdfs:subClassOf>
         <owl:Class rdf:about="#accommodability"/>
      </rdfs:subClassOf>
      <owl:versionInfo>subClassOf accommodability (dcif:conceptualDomain)</owl:versionInfo>
   </owl:Class>
   <owl:Class rdf:ID="xxx">
      <dcr:datcat rdf:resource="http://www.isocat.org/datcat/DC-2715"/>
      <owl:versionInfo>http://www.isocat.org/datcat/DC-2715</owl:versionInfo>
      <rdfs:comment>
            Alien elements class [xxx] is used mostly for annotating longer foreign expressions or whole passages in a foreign language (segments which do not enter into relations with other (non-alien) segments in the sentence)
                (http://www.isocat.org/datcat/DC-2715)
            </rdfs:comment>
      <rdfs:label>alien elements</rdfs:label>
   </owl:Class>
   <owl:Class rdf:ID="m2">
      <dcr:datcat rdf:resource="http://www.isocat.org/datcat/DC-2730"/>
      <owl:versionInfo>http://www.isocat.org/datcat/DC-2730</owl:versionInfo>
      <rdfs:comment>
            Animate masculine [m2] is a value of the grammatical category of gender appropriate for forms which can be modified with the following forms of the flexeme TEN: te (nominative plural), tego (accusative singular).
                (http://www.isocat.org/datcat/DC-2730)
            </rdfs:comment>
      <rdfs:label>animate masculine gender</rdfs:label>
      <rdfs:subClassOf>
         <owl:Class rdf:about="#gender"/>
      </rdfs:subClassOf>
      <owl:versionInfo>subClassOf gender (dcif:conceptualDomain)</owl:versionInfo>
   </owl:Class>
   <owl:Class rdf:ID="pant">
      <dcr:datcat rdf:resource="http://www.isocat.org/datcat/DC-2754"/>
      <owl:versionInfo>http://www.isocat.org/datcat/DC-2754</owl:versionInfo>
      <rdfs:comment>
            Anterior adverbial participle [pant] consists of single-element flexemes containing perfective adverbial participles, e.g., wypiwszy `having drunk up'. Grammatical categories of anterior adverbial participle [pant]: aspect (http://www.isocat.org/datcat/DC-2783).
                (http://www.isocat.org/datcat/DC-2754)
            </rdfs:comment>
      <rdfs:label>anterior adverbial participle</rdfs:label>
   </owl:Class>
   <owl:Class rdf:ID="aspect">
      <dcr:datcat rdf:resource="http://www.isocat.org/datcat/DC-2783"/>
      <owl:versionInfo>http://www.isocat.org/datcat/DC-2783</owl:versionInfo>
      <rdfs:comment>
            Aspect [aspect] is a lexical category: forms do not inflect for aspect, but rather have the value of aspect, constant for all forms of a given verb, determined lexically.
                (http://www.isocat.org/datcat/DC-2783)
            </rdfs:comment>
      <rdfs:label>aspect</rdfs:label>
   </owl:Class>
   <owl:Class rdf:ID="burk">
      <dcr:datcat rdf:resource="http://www.isocat.org/datcat/DC-2716"/>
      <owl:versionInfo>http://www.isocat.org/datcat/DC-2716</owl:versionInfo>
      <rdfs:comment>
            Bound word [burk], occurring only in a particular construction, indeterminate as to its morphosyntactic category
                (http://www.isocat.org/datcat/DC-2716)
            </rdfs:comment>
      <rdfs:label>bound word</rdfs:label>
   </owl:Class>
   <owl:Class rdf:ID="case">
      <dcr:datcat rdf:resource="http://www.isocat.org/datcat/DC-2720"/>
      <owl:versionInfo>http://www.isocat.org/datcat/DC-2720</owl:versionInfo>
      <rdfs:comment>
            Case [case] is a grammatical category appropriate for inflecting grammatical classes displaying nominal or adjectival features, as well as for prepositions where case is understood as a governed case.
                (http://www.isocat.org/datcat/DC-2720)
            </rdfs:comment>
      <rdfs:label>case</rdfs:label>
   </owl:Class>
   <owl:Class rdf:ID="numcol">
      <dcr:datcat rdf:resource="http://www.isocat.org/datcat/DC-2764"/>
      <owl:versionInfo>http://www.isocat.org/datcat/DC-2764</owl:versionInfo>
      <rdfs:comment>
            Collective numeral [numcol] contains flexemes which inflect for case and - defectively - for accommodability, with lexically determined number (always plural) and gender (always neuter), i.e., flexemes such as pięcioro `five'. Grammatical categories of collective numeral [numcol]: number (http://www.isocat.org/datcat/DC-2709), case (http://www.isocat.org/datcat/DC-2720), gender (http://www.isocat.org/datcat/DC-2728), accommodability (http://www.isocat.org/datcat/DC-2734).
                (http://www.isocat.org/datcat/DC-2764)
            </rdfs:comment>
      <rdfs:label>collective numeral</rdfs:label>
   </owl:Class>
   <owl:Class rdf:ID="com">
      <dcr:datcat rdf:resource="http://www.isocat.org/datcat/DC-2781"/>
      <owl:versionInfo>http://www.isocat.org/datcat/DC-2781</owl:versionInfo>
      <rdfs:comment>
            Comparative [com] is a value of the grammatical category of degree appropriate for adjectives and adverbs expressing a higher than basic level of intensity of the named feature.
                (http://www.isocat.org/datcat/DC-2781)
            </rdfs:comment>
      <rdfs:label>comparative degree</rdfs:label>
      <rdfs:subClassOf>
         <owl:Class rdf:about="#degree"/>
      </rdfs:subClassOf>
      <owl:versionInfo>subClassOf degree (dcif:conceptualDomain)</owl:versionInfo>
   </owl:Class>
   <owl:Class rdf:ID="comp">
      <dcr:datcat rdf:resource="http://www.isocat.org/datcat/DC-2712"/>
      <owl:versionInfo>http://www.isocat.org/datcat/DC-2712</owl:versionInfo>
      <rdfs:comment>
            Subordinate conjunction
                (http://www.isocat.org/datcat/DC-2712)
            </rdfs:comment>
      <rdfs:label>complementiser</rdfs:label>
   </owl:Class>
   <owl:Class rdf:ID="pcon">
      <dcr:datcat rdf:resource="http://www.isocat.org/datcat/DC-2755"/>
      <owl:versionInfo>http://www.isocat.org/datcat/DC-2755</owl:versionInfo>
      <rdfs:comment>
            Contemporary adverbial participle [pcon] consists of single-element flexemes containing imperfective adverbial participles, e.g., pijąc `drinking'. Grammatical categories of contemporary adverbial participle [pcon]: aspect (http://www.isocat.org/datcat/DC-2783).
                (http://www.isocat.org/datcat/DC-2755)
            </rdfs:comment>
      <rdfs:label>contemporary adverbial participle</rdfs:label>
   </owl:Class>
   <owl:Class rdf:ID="conj">
      <dcr:datcat rdf:resource="http://www.isocat.org/datcat/DC-2711"/>
      <owl:versionInfo>http://www.isocat.org/datcat/DC-2711</owl:versionInfo>
      <rdfs:comment>
            Coordinate conjunction
                (http://www.isocat.org/datcat/DC-2711)
            </rdfs:comment>
      <rdfs:label>coordinate conjunction</rdfs:label>
   </owl:Class>
   <owl:Class rdf:ID="dat">
      <dcr:datcat rdf:resource="http://www.isocat.org/datcat/DC-2723"/>
      <owl:versionInfo>http://www.isocat.org/datcat/DC-2723</owl:versionInfo>
      <rdfs:comment>
            Dative [dat] is a value of the grammatical category of case paradigmatically appropriate for oblique objects and experiencers.
                (http://www.isocat.org/datcat/DC-2723)
            </rdfs:comment>
      <rdfs:label>dative case</rdfs:label>
      <rdfs:subClassOf>
         <owl:Class rdf:about="#case"/>
      </rdfs:subClassOf>
      <owl:versionInfo>subClassOf case (dcif:conceptualDomain)</owl:versionInfo>
   </owl:Class>
   <owl:Class rdf:ID="degree">
      <dcr:datcat rdf:resource="http://www.isocat.org/datcat/DC-2779"/>
      <owl:versionInfo>http://www.isocat.org/datcat/DC-2779</owl:versionInfo>
      <rdfs:comment>
            Degree [degree] is a grammatical category appropriate for grammatical classes of adjectives and adverbs expressing the gradation in the level of intensity of the named feature.
                (http://www.isocat.org/datcat/DC-2779)
            </rdfs:comment>
      <rdfs:label>degree</rdfs:label>
   </owl:Class>
   <owl:Class rdf:ID="depr">
      <dcr:datcat rdf:resource="http://www.isocat.org/datcat/DC-2759"/>
      <owl:versionInfo>http://www.isocat.org/datcat/DC-2759</owl:versionInfo>
      <rdfs:comment>
            Depreciative form [depr] contains depreciative flexemes, i.e., flexemes with fixed number (plural) and gender (animate masculine), defectively inflecting for case (only nominative and vocative), e.g., profesory `professors', studenty `students'. Grammatical categories of depreciative form [depr]: number (http://www.isocat.org/datcat/DC-2709), case (http://www.isocat.org/datcat/DC-2720), gender (http://www.isocat.org/datcat/DC-2728).
                (http://www.isocat.org/datcat/DC-2759)
            </rdfs:comment>
      <rdfs:label>depreciative form</rdfs:label>
   </owl:Class>
   <owl:Class rdf:ID="">
      <dcr:datcat rdf:resource="http://www.isocat.org/datcat/DC-2732"/>
      <owl:versionInfo>http://www.isocat.org/datcat/DC-2732</owl:versionInfo>
      <rdfs:comment>
            Feminine [f] is a value of the grammatical category of gender appropriate for forms which can be modified with the following distinctive form of the flexeme TEN: ta (nominative singular).
                (http://www.isocat.org/datcat/DC-2732)
            </rdfs:comment>
      <rdfs:label>feminine gender</rdfs:label>
      <rdfs:subClassOf>
         <owl:Class rdf:about="#gender"/>
      </rdfs:subClassOf>
      <owl:versionInfo>subClassOf gender (dcif:conceptualDomain)</owl:versionInfo>
   </owl:Class>
   <owl:Class rdf:ID="pri">
      <dcr:datcat rdf:resource="http://www.isocat.org/datcat/DC-2776"/>
      <owl:versionInfo>http://www.isocat.org/datcat/DC-2776</owl:versionInfo>
      <rdfs:comment>
            First [pri] is a value of the grammatical category of person appropriate for participants identified as the speaker.
                (http://www.isocat.org/datcat/DC-2776)
            </rdfs:comment>
      <rdfs:label>first person</rdfs:label>
      <rdfs:subClassOf>
         <owl:Class rdf:about="#person"/>
      </rdfs:subClassOf>
      <owl:versionInfo>subClassOf person (dcif:conceptualDomain)</owl:versionInfo>
   </owl:Class>
   <owl:Class rdf:ID="pun">
      <dcr:datcat rdf:resource="http://www.isocat.org/datcat/DC-2790"/>
      <owl:versionInfo>http://www.isocat.org/datcat/DC-2790</owl:versionInfo>
      <rdfs:comment>
            Full stop [pun] is a value of the grammatical category of fullstoppedness appropriate for an abbreviation segment which should be followed by a full stop.
                (http://www.isocat.org/datcat/DC-2790)
            </rdfs:comment>
      <rdfs:label>full stop</rdfs:label>
      <rdfs:subClassOf>
         <owl:Class rdf:about="#fullstoppedness"/>
      </rdfs:subClassOf>
      <owl:versionInfo>subClassOf fullstoppedness (dcif:conceptualDomain)</owl:versionInfo>
   </owl:Class>
   <owl:Class rdf:ID="fullstoppedness">
      <dcr:datcat rdf:resource="http://www.isocat.org/datcat/DC-2789"/>
      <owl:versionInfo>http://www.isocat.org/datcat/DC-2789</owl:versionInfo>
      <rdfs:comment>
            Fullstoppedness [fullstoppedness], a technical category associated with the abbreviation class [brev], may take one of two values: pun (the abbreviation segment should be followed by a full stop) and npun (the segment does not have to be followed by a full stop).
                (http://www.isocat.org/datcat/DC-2789)
            </rdfs:comment>
      <rdfs:label>fullstoppedness</rdfs:label>
   </owl:Class>
   <owl:Class rdf:ID="bedzie">
      <dcr:datcat rdf:resource="http://www.isocat.org/datcat/DC-2770"/>
      <owl:versionInfo>http://www.isocat.org/datcat/DC-2770</owl:versionInfo>
      <rdfs:comment>
            Future form of BYĆ [bedzie] contains just one flexeme, consisting of the future forms of the imperfective verb być `to be': będę, będziesz, etc. Grammatical categories of future form of BYĆ [bedzie]: number (http://www.isocat.org/datcat/DC-2709), person (http://www.isocat.org/datcat/DC-2775), aspect (http://www.isocat.org/datcat/DC-2783).
                (http://www.isocat.org/datcat/DC-2770)
            </rdfs:comment>
      <rdfs:label>future form of BYĆ</rdfs:label>
   </owl:Class>
   <owl:Class rdf:ID="gender">
      <dcr:datcat rdf:resource="http://www.isocat.org/datcat/DC-2728"/>
      <owl:versionInfo>http://www.isocat.org/datcat/DC-2728</owl:versionInfo>
      <rdfs:comment>
            The grammatical category of gender [gender] is understood as in Mańczak 1956, i.e., unlike in the `preliminary school grammar', the gender of a noun does not depend on that noun's number.
                (http://www.isocat.org/datcat/DC-2728)
            </rdfs:comment>
      <rdfs:label>gender</rdfs:label>
   </owl:Class>
   <owl:Class rdf:ID="gen">
      <dcr:datcat rdf:resource="http://www.isocat.org/datcat/DC-2722"/>
      <owl:versionInfo>http://www.isocat.org/datcat/DC-2722</owl:versionInfo>
      <rdfs:comment>
            Genitive [gen] is a value of the grammatical category of case paradigmatically appropriate for possessors, partitives, non-inherent case arguments of gerunds and structural objects under sentential negation.
                (http://www.isocat.org/datcat/DC-2722)
            </rdfs:comment>
      <rdfs:label>genitive case</rdfs:label>
      <rdfs:subClassOf>
         <owl:Class rdf:about="#case"/>
      </rdfs:subClassOf>
      <owl:versionInfo>subClassOf case (dcif:conceptualDomain)</owl:versionInfo>
   </owl:Class>
   <owl:Class rdf:ID="ger">
      <dcr:datcat rdf:resource="http://www.isocat.org/datcat/DC-2760"/>
      <owl:versionInfo>http://www.isocat.org/datcat/DC-2760</owl:versionInfo>
      <rdfs:comment>
            Gerund [ger] contains flexemes which inflect for number, case and negation, and have the lexical categories of gender (always neuter) and aspect, e.g., picie `drinking' and wypicie `drinking up'. Grammatical categories of gerund [ger]: number (http://www.isocat.org/datcat/DC-2709), case (http://www.isocat.org/datcat/DC-2720), gender (http://www.isocat.org/datcat/DC-2728), aspect (http://www.isocat.org/datcat/DC-2783), negation (http://www.isocat.org/datcat/DC-2786).
                (http://www.isocat.org/datcat/DC-2760)
            </rdfs:comment>
      <rdfs:label>gerund</rdfs:label>
   </owl:Class>
   <owl:Class rdf:ID="rec">
      <dcr:datcat rdf:resource="http://www.isocat.org/datcat/DC-2736"/>
      <owl:versionInfo>http://www.isocat.org/datcat/DC-2736</owl:versionInfo>
      <rdfs:comment>
            Governing [rec] is a value of the grammatical category of accommodability appropriate for a numeral form if and only if it does not agree in case with the accompanying noun.
                (http://www.isocat.org/datcat/DC-2736)
            </rdfs:comment>
      <rdfs:label>governing accommodability</rdfs:label>
      <rdfs:subClassOf>
         <owl:Class rdf:about="#accommodability"/>
      </rdfs:subClassOf>
      <owl:versionInfo>subClassOf accommodability (dcif:conceptualDomain)</owl:versionInfo>
   </owl:Class>
   <owl:Class rdf:ID="m1">
      <dcr:datcat rdf:resource="http://www.isocat.org/datcat/DC-2729"/>
      <owl:versionInfo>http://www.isocat.org/datcat/DC-2729</owl:versionInfo>
      <rdfs:comment>
            Human masculine (virile) [m1] is a value of the grammatical category of gender appropriate for forms which can be modified with the following distinctive form of the flexeme TEN: ci (nominative plural).
                (http://www.isocat.org/datcat/DC-2729)
            </rdfs:comment>
      <rdfs:label>human masculine (virile) gender</rdfs:label>
      <rdfs:subClassOf>
         <owl:Class rdf:about="#gender"/>
      </rdfs:subClassOf>
      <owl:versionInfo>subClassOf gender (dcif:conceptualDomain)</owl:versionInfo>
   </owl:Class>
   <owl:Class rdf:ID="impt">
      <dcr:datcat rdf:resource="http://www.isocat.org/datcat/DC-2772"/>
      <owl:versionInfo>http://www.isocat.org/datcat/DC-2772</owl:versionInfo>
      <rdfs:comment>
            Imperative [impt] contains flexemes with a lexically determined value of aspect, inflecting for number and gender, but only defectively so (only the 1.sg, 2.sg and 2.pl forms), e.g., the flexeme containing the forms pij `you.sg drink!', pijcie `you.pl drink', pijmy `let us drink!'. Grammatical categories of imperative [impt]: number (http://www.isocat.org/datcat/DC-2709), person (http://www.isocat.org/datcat/DC-2775), aspect (http://www.isocat.org/datcat/DC-2783).
                (http://www.isocat.org/datcat/DC-2772)
            </rdfs:comment>
      <rdfs:label>imperative</rdfs:label>
   </owl:Class>
   <owl:Class rdf:ID="imperf">
      <dcr:datcat rdf:resource="http://www.isocat.org/datcat/DC-2784"/>
      <owl:versionInfo>http://www.isocat.org/datcat/DC-2784</owl:versionInfo>
      <rdfs:comment>
            Imperfective [imperf] is a value of the lexical grammatical category of aspect appropriate for verbal forms referring to actions which are not completed (ongoing, habitual or repeating) in the future, present or past.
                (http://www.isocat.org/datcat/DC-2784)
            </rdfs:comment>
      <rdfs:label>imperfective aspect</rdfs:label>
      <rdfs:subClassOf>
         <owl:Class rdf:about="#aspect"/>
      </rdfs:subClassOf>
      <owl:versionInfo>subClassOf aspect (dcif:conceptualDomain)</owl:versionInfo>
   </owl:Class>
   <owl:Class rdf:ID="imps">
      <dcr:datcat rdf:resource="http://www.isocat.org/datcat/DC-2752"/>
      <owl:versionInfo>http://www.isocat.org/datcat/DC-2752</owl:versionInfo>
      <rdfs:comment>
            Impersonal [imps] consists of single-element flexemes containing non-inflecting aspectual forms ending in -no or -to, e.g., pito `was drunk'. Grammatical categories of impersonal [imps]: aspect (http://www.isocat.org/datcat/DC-2783).
                (http://www.isocat.org/datcat/DC-2752)
            </rdfs:comment>
      <rdfs:label>impersonal</rdfs:label>
   </owl:Class>
   <owl:Class rdf:ID="m3">
      <dcr:datcat rdf:resource="http://www.isocat.org/datcat/DC-2731"/>
      <owl:versionInfo>http://www.isocat.org/datcat/DC-2731</owl:versionInfo>
      <rdfs:comment>
            Inanimate masculine [m3] is a value of the grammatical category of gender appropriate for forms which can be modified with the following distinctive form of the flexeme TEN: ten (accusative singular).
                (http://www.isocat.org/datcat/DC-2731)
            </rdfs:comment>
      <rdfs:label>inanimate masculine gender</rdfs:label>
      <rdfs:subClassOf>
         <owl:Class rdf:about="#gender"/>
      </rdfs:subClassOf>
      <owl:versionInfo>subClassOf gender (dcif:conceptualDomain)</owl:versionInfo>
   </owl:Class>
   <owl:Class rdf:ID="inf">
      <dcr:datcat rdf:resource="http://www.isocat.org/datcat/DC-2753"/>
      <owl:versionInfo>http://www.isocat.org/datcat/DC-2753</owl:versionInfo>
      <rdfs:comment>
            Infinitive [inf] consists of single-element flexemes which contain infinitive forms, e.g., pić 'to drink'. Grammatical categories of infinitive [inf]: aspect (http://www.isocat.org/datcat/DC-2783).
                (http://www.isocat.org/datcat/DC-2753)
            </rdfs:comment>
      <rdfs:label>infinitive</rdfs:label>
   </owl:Class>
   <owl:Class rdf:ID="inst">
      <dcr:datcat rdf:resource="http://www.isocat.org/datcat/DC-2725"/>
      <owl:versionInfo>http://www.isocat.org/datcat/DC-2725</owl:versionInfo>
      <rdfs:comment>
            Instrumental [inst] is a value of the grammatical category of case paradigmatically appropriate for instruments, oblique objects and predicates.
                (http://www.isocat.org/datcat/DC-2725)
            </rdfs:comment>
      <rdfs:label>instrumental case</rdfs:label>
      <rdfs:subClassOf>
         <owl:Class rdf:about="#case"/>
      </rdfs:subClassOf>
      <owl:versionInfo>subClassOf case (dcif:conceptualDomain)</owl:versionInfo>
   </owl:Class>
   <owl:Class rdf:ID="interj">
      <dcr:datcat rdf:resource="http://www.isocat.org/datcat/DC-2717"/>
      <owl:versionInfo>http://www.isocat.org/datcat/DC-2717</owl:versionInfo>
      <rdfs:comment>
            A segment (i.e., a word-level token receiving a morphosyntactic interpretation) is marked as an interjection [interj], if one of the following holds: – it may only be used as an interjection, e.g., segments such as ach, och, oj, – if the same form has other interpretations, they are not related to the interjection use of that form, e.g., a (which may also be a conjunction or an abbreviation), – it is onomatopoeic, e.g., mu or kukuryku. Examples of segments which may be used interjectively but are not marked as interjections are tak ‘yes’ and kurwa ‘whore’.
                (http://www.isocat.org/datcat/DC-2717)
            </rdfs:comment>
      <rdfs:label>interjection</rdfs:label>
   </owl:Class>
   <owl:Class rdf:ID="praet">
      <dcr:datcat rdf:resource="http://www.isocat.org/datcat/DC-2769"/>
      <owl:versionInfo>http://www.isocat.org/datcat/DC-2769</owl:versionInfo>
      <rdfs:comment>
            L-participle [praet] contains flexemes inflecting for number and gender, with a lexically determined value of aspect, e.g., the flexeme containing the forms niósł, niosł-, niosła, nieśli, niosły `carry'. Grammatical categories of l-participle [praet]: number (http://www.isocat.org/datcat/DC-2709), gender (http://www.isocat.org/datcat/DC-2728), aspect (http://www.isocat.org/datcat/DC-2783), agglutination (http://www.isocat.org/datcat/DC-2745) (optional).
                (http://www.isocat.org/datcat/DC-2769)
            </rdfs:comment>
      <rdfs:label>l-participle</rdfs:label>
   </owl:Class>
   <owl:Class rdf:ID="loc">
      <dcr:datcat rdf:resource="http://www.isocat.org/datcat/DC-2726"/>
      <owl:versionInfo>http://www.isocat.org/datcat/DC-2726</owl:versionInfo>
      <rdfs:comment>
            Locative [loc] is a value of the grammatical category of case appropriate for forms governed exclusively by prepositions.
                (http://www.isocat.org/datcat/DC-2726)
            </rdfs:comment>
      <rdfs:label>locative case</rdfs:label>
      <rdfs:subClassOf>
         <owl:Class rdf:about="#case"/>
      </rdfs:subClassOf>
      <owl:versionInfo>subClassOf case (dcif:conceptualDomain)</owl:versionInfo>
   </owl:Class>
   <owl:Class rdf:ID="num">
      <dcr:datcat rdf:resource="http://www.isocat.org/datcat/DC-2763"/>
      <owl:versionInfo>http://www.isocat.org/datcat/DC-2763</owl:versionInfo>
      <rdfs:comment>
            Main numeral [num] contains flexemes inflecting for case, gender and - defectively - for accommodability, with lexically determined number (normally plural), i.e., flexemes such as pięć `five' and wiele `many', also including defective numeral flexemes such as trochę `some' and dużo `much, many', whose case values are limited to nominative, accusative and genitive. Grammatical categories of main numeral [num]: number (http://www.isocat.org/datcat/DC-2709), case (http://www.isocat.org/datcat/DC-2720), gender (http://www.isocat.org/datcat/DC-2728), accommodability (http://www.isocat.org/datcat/DC-2734).
                (http://www.isocat.org/datcat/DC-2763)
            </rdfs:comment>
      <rdfs:label>main numeral</rdfs:label>
   </owl:Class>
   <owl:Class rdf:ID="negation">
      <dcr:datcat rdf:resource="http://www.isocat.org/datcat/DC-2786"/>
      <owl:versionInfo>http://www.isocat.org/datcat/DC-2786</owl:versionInfo>
      <rdfs:comment>
            Negation [negation] is appropriate for those verbal forms for which the negative prefix nie- is orthographically joined to the verbal form, i.e., this category is useful for distinguishing forms such as pisanie `writing' and niepisanie `non-writing', napisany `written' and nienapisany `unwritten', but not for distinguishing pisać `to write' and nie pisać `not to write'.
                (http://www.isocat.org/datcat/DC-2786)
            </rdfs:comment>
      <rdfs:label>negation</rdfs:label>
   </owl:Class>
   <owl:Class rdf:ID="neg">
      <dcr:datcat rdf:resource="http://www.isocat.org/datcat/DC-2788"/>
      <owl:versionInfo>http://www.isocat.org/datcat/DC-2788</owl:versionInfo>
      <rdfs:comment>
            Negative [neg] is a value of the grammatical category of negation appropriate for a verbal form with the ortographically joined negative prefix nie-.
                (http://www.isocat.org/datcat/DC-2788)
            </rdfs:comment>
      <rdfs:label>negative</rdfs:label>
      <rdfs:subClassOf>
         <owl:Class rdf:about="#negation"/>
      </rdfs:subClassOf>
      <owl:versionInfo>subClassOf negation (dcif:conceptualDomain)</owl:versionInfo>
   </owl:Class>
   <owl:Class rdf:ID="">
      <dcr:datcat rdf:resource="http://www.isocat.org/datcat/DC-2733"/>
      <owl:versionInfo>http://www.isocat.org/datcat/DC-2733</owl:versionInfo>
      <rdfs:comment>
            Neuter [n] is a value of the grammatical category of gender appropriate for forms which can be modified with the following distinctive form of the flexeme TEN: to (nominative singular).
                (http://www.isocat.org/datcat/DC-2733)
            </rdfs:comment>
      <rdfs:label>neuter gender</rdfs:label>
      <rdfs:subClassOf>
         <owl:Class rdf:about="#gender"/>
      </rdfs:subClassOf>
      <owl:versionInfo>subClassOf gender (dcif:conceptualDomain)</owl:versionInfo>
   </owl:Class>
   <owl:Class rdf:ID="npun">
      <dcr:datcat rdf:resource="http://www.isocat.org/datcat/DC-2791"/>
      <owl:versionInfo>http://www.isocat.org/datcat/DC-2791</owl:versionInfo>
      <rdfs:comment>
            No full stop [npun] is a value of the grammatical category of fullstoppedness appropriate for an abbreviation segment which does not have to be followed by a full stop.
                (http://www.isocat.org/datcat/DC-2791)
            </rdfs:comment>
      <rdfs:label>no full stop</rdfs:label>
      <rdfs:subClassOf>
         <owl:Class rdf:about="#fullstoppedness"/>
      </rdfs:subClassOf>
      <owl:versionInfo>subClassOf fullstoppedness (dcif:conceptualDomain)</owl:versionInfo>
   </owl:Class>
   <owl:Class rdf:ID="nom">
      <dcr:datcat rdf:resource="http://www.isocat.org/datcat/DC-2721"/>
      <owl:versionInfo>http://www.isocat.org/datcat/DC-2721</owl:versionInfo>
      <rdfs:comment>
            Nominative [nom] is a value of the grammatical category of case paradigmatically appropriate for subjects.
                (http://www.isocat.org/datcat/DC-2721)
            </rdfs:comment>
      <rdfs:label>nominative case</rdfs:label>
      <rdfs:subClassOf>
         <owl:Class rdf:about="#case"/>
      </rdfs:subClassOf>
      <owl:versionInfo>subClassOf case (dcif:conceptualDomain)</owl:versionInfo>
   </owl:Class>
   <owl:Class rdf:ID="ppron12">
      <dcr:datcat rdf:resource="http://www.isocat.org/datcat/DC-2761"/>
      <owl:versionInfo>http://www.isocat.org/datcat/DC-2761</owl:versionInfo>
      <rdfs:comment>
            Non-3rd person pronoun [ppron12] contains exactly four flexemes, which inflect for case and gender, but have lexically determined number and person: ja `I', my `we', ty `you.sg', wy `you.pl'; some forms of the flexemes ja and ty additionally inflect for accentability (e.g., ci vs. tobie, `you.sg.dat'). Grammatical categories of non-3rd person pronoun [ppron12]: number (http://www.isocat.org/datcat/DC-2709), case (http://www.isocat.org/datcat/DC-2720), gender (http://www.isocat.org/datcat/DC-2728), person (http://www.isocat.org/datcat/DC-2775), accentability (http://www.isocat.org/datcat/DC-2737) (optional).
                (http://www.isocat.org/datcat/DC-2761)
            </rdfs:comment>
      <rdfs:label>non-3rd person pronoun</rdfs:label>
   </owl:Class>
   <owl:Class rdf:ID="nakc">
      <dcr:datcat rdf:resource="http://www.isocat.org/datcat/DC-2739"/>
      <owl:versionInfo>http://www.isocat.org/datcat/DC-2739</owl:versionInfo>
      <rdfs:comment>
            non-accented (weak) [nakc] form of the pronoun
                (http://www.isocat.org/datcat/DC-2739)
            </rdfs:comment>
      <rdfs:label>non-accented (weak)</rdfs:label>
      <rdfs:subClassOf>
         <owl:Class rdf:about="#accentability"/>
      </rdfs:subClassOf>
      <owl:versionInfo>subClassOf accentability (dcif:conceptualDomain)</owl:versionInfo>
   </owl:Class>
   <owl:Class rdf:ID="nagl">
      <dcr:datcat rdf:resource="http://www.isocat.org/datcat/DC-2746"/>
      <owl:versionInfo>http://www.isocat.org/datcat/DC-2746</owl:versionInfo>
      <rdfs:comment>
            Non-agglutinative [nagl] form occurs on its own.
                (http://www.isocat.org/datcat/DC-2746)
            </rdfs:comment>
      <rdfs:label>non-agglutinative</rdfs:label>
      <rdfs:subClassOf>
         <owl:Class rdf:about="#agglutination"/>
      </rdfs:subClassOf>
      <owl:versionInfo>subClassOf agglutination (dcif:conceptualDomain)</owl:versionInfo>
   </owl:Class>
   <owl:Class rdf:ID="fin">
      <dcr:datcat rdf:resource="http://www.isocat.org/datcat/DC-2771"/>
      <owl:versionInfo>http://www.isocat.org/datcat/DC-2771</owl:versionInfo>
      <rdfs:comment>
            Non-past form [fin] contains flexemes which inflect for number and person, and have the lexical category of aspect: future forms (with perfective aspect), e.g., wypiję `I will drink up', and present forms (with imperfective aspect), e.g., piję `I am drinking'. Grammatical categories of non-past form [fin]: number (http://www.isocat.org/datcat/DC-2709), person (http://www.isocat.org/datcat/DC-2775), aspect (http://www.isocat.org/datcat/DC-2783).
                (http://www.isocat.org/datcat/DC-2771)
            </rdfs:comment>
      <rdfs:label>non-past form</rdfs:label>
   </owl:Class>
   <owl:Class rdf:ID="npraep">
      <dcr:datcat rdf:resource="http://www.isocat.org/datcat/DC-2742"/>
      <owl:versionInfo>http://www.isocat.org/datcat/DC-2742</owl:versionInfo>
      <rdfs:comment>
            non-post-prepositional [npraep] form of the pronoun
                (http://www.isocat.org/datcat/DC-2742)
            </rdfs:comment>
      <rdfs:label>non-post-prepositional</rdfs:label>
      <rdfs:subClassOf>
         <owl:Class rdf:about="#postprepositionality"/>
      </rdfs:subClassOf>
      <owl:versionInfo>subClassOf postprepositionality (dcif:conceptualDomain)</owl:versionInfo>
   </owl:Class>
   <owl:Class rdf:ID="nwok">
      <dcr:datcat rdf:resource="http://www.isocat.org/datcat/DC-2750"/>
      <owl:versionInfo>http://www.isocat.org/datcat/DC-2750</owl:versionInfo>
      <rdfs:comment>
            Non-vocalic [nwok] agglutinates attach to forms ending in a vowel.
                (http://www.isocat.org/datcat/DC-2750)
            </rdfs:comment>
      <rdfs:label>non-vocalic</rdfs:label>
      <rdfs:subClassOf>
         <owl:Class rdf:about="#vocalicity"/>
      </rdfs:subClassOf>
      <owl:versionInfo>subClassOf vocalicity (dcif:conceptualDomain)</owl:versionInfo>
   </owl:Class>
   <owl:Class rdf:ID="subst">
      <dcr:datcat rdf:resource="http://www.isocat.org/datcat/DC-2704"/>
      <owl:versionInfo>http://www.isocat.org/datcat/DC-2704</owl:versionInfo>
      <rdfs:comment>
            Noun [subst] contains lexemes infecting for number and case, with a lexically determined grammatical gender, which do not have the category of person, e.g., woda `water', profesor `professor', pięciokrotność 'fivefoldness'; this class also contains defective plurale tantum and singulare tantum lexemes, but not depreciative lexemes. Grammatical categories of noun [subst]: number (http://www.isocat.org/datcat/DC-2709), case (http://www.isocat.org/datcat/DC-2720), gender (http://www.isocat.org/datcat/DC-2728).
                (http://www.isocat.org/datcat/DC-2704)
            </rdfs:comment>
      <rdfs:label>noun</rdfs:label>
   </owl:Class>
   <owl:Class rdf:ID="number">
      <dcr:datcat rdf:resource="http://www.isocat.org/datcat/DC-2709"/>
      <owl:versionInfo>http://www.isocat.org/datcat/DC-2709</owl:versionInfo>
      <rdfs:comment>
            Number [number] is a grammatical category appropriate for all inflecting grammatical classes as a classifying or inflectional category expressing morphologically the perceived difference in quantity.
                (http://www.isocat.org/datcat/DC-2709)
            </rdfs:comment>
      <rdfs:label>number</rdfs:label>
   </owl:Class>
   <owl:Class rdf:ID="qub">
      <dcr:datcat rdf:resource="http://www.isocat.org/datcat/DC-2756"/>
      <owl:versionInfo>http://www.isocat.org/datcat/DC-2756</owl:versionInfo>
      <rdfs:comment>
            Particle-adverb [qub] contains contain various particles, the reflexive marker się, ad-numeral operators such as około ‘around’ and blisko ‘almost’, and intensifiers such as jedynie ‘only’ and nawet ‘even’. Grammatical categories of particle-adverb [qub]: vocalicity (http://www.isocat.org/datcat/DC-2748) (optional).
                (http://www.isocat.org/datcat/DC-2756)
            </rdfs:comment>
      <rdfs:label>particle-adverb</rdfs:label>
   </owl:Class>
   <owl:Class rdf:ID="ppas">
      <dcr:datcat rdf:resource="http://www.isocat.org/datcat/DC-2767"/>
      <owl:versionInfo>http://www.isocat.org/datcat/DC-2767</owl:versionInfo>
      <rdfs:comment>
            Passive adjectival participle [ppas] contains passive adjectival participles, inflecting for number, case, gender and negation, with lexical aspect, e.g., pity `drunk', wypity `drunk up'. Grammatical categories of passive adjectival participle [ppas]: number (http://www.isocat.org/datcat/DC-2709), case (http://www.isocat.org/datcat/DC-2720), gender (http://www.isocat.org/datcat/DC-2728), aspect (http://www.isocat.org/datcat/DC-2783), negation (http://www.isocat.org/datcat/DC-2786).
                (http://www.isocat.org/datcat/DC-2767)
            </rdfs:comment>
      <rdfs:label>passive adjectival participle</rdfs:label>
   </owl:Class>
   <owl:Class rdf:ID="perf">
      <dcr:datcat rdf:resource="http://www.isocat.org/datcat/DC-2785"/>
      <owl:versionInfo>http://www.isocat.org/datcat/DC-2785</owl:versionInfo>
      <rdfs:comment>
            Perfective [perf] is a value of the lexical grammatical category of aspect appropriate for verbal forms referring to actions completed in the future or past.
                (http://www.isocat.org/datcat/DC-2785)
            </rdfs:comment>
      <rdfs:label>perfective aspect</rdfs:label>
      <rdfs:subClassOf>
         <owl:Class rdf:about="#aspect"/>
      </rdfs:subClassOf>
      <owl:versionInfo>subClassOf aspect (dcif:conceptualDomain)</owl:versionInfo>
   </owl:Class>
   <owl:Class rdf:ID="person">
      <dcr:datcat rdf:resource="http://www.isocat.org/datcat/DC-2775"/>
      <owl:versionInfo>http://www.isocat.org/datcat/DC-2775</owl:versionInfo>
      <rdfs:comment>
            Person [person] is a grammatical category appropriate for finite verbal forms as an inflectional category and for pronouns as a classifying category identifying the participants of the utterance with reference to their roles in the speech act.
                (http://www.isocat.org/datcat/DC-2775)
            </rdfs:comment>
      <rdfs:label>person</rdfs:label>
   </owl:Class>
   <owl:Class rdf:ID="pl">
      <dcr:datcat rdf:resource="http://www.isocat.org/datcat/DC-2708"/>
      <owl:versionInfo>http://www.isocat.org/datcat/DC-2708</owl:versionInfo>
      <rdfs:comment>
            Plural [pl] is a value of the grammatical category of number typically appropriate for lexemes whose reference is aggregate or is perceived as such.
                (http://www.isocat.org/datcat/DC-2708)
            </rdfs:comment>
      <rdfs:label>plural number</rdfs:label>
      <rdfs:subClassOf>
         <owl:Class rdf:about="#number"/>
      </rdfs:subClassOf>
      <owl:versionInfo>subClassOf number (dcif:conceptualDomain)</owl:versionInfo>
   </owl:Class>
   <owl:Class rdf:ID="pos">
      <dcr:datcat rdf:resource="http://www.isocat.org/datcat/DC-2780"/>
      <owl:versionInfo>http://www.isocat.org/datcat/DC-2780</owl:versionInfo>
      <rdfs:comment>
            Positive [pos] is a value of the grammatical category of degree appropriate for adjectives and adverbs expressing the basic level of intensity of the named feature.
                (http://www.isocat.org/datcat/DC-2780)
            </rdfs:comment>
      <rdfs:label>positive degree</rdfs:label>
      <rdfs:subClassOf>
         <owl:Class rdf:about="#degree"/>
      </rdfs:subClassOf>
      <owl:versionInfo>subClassOf degree (dcif:conceptualDomain)</owl:versionInfo>
   </owl:Class>
   <owl:Class rdf:ID="praep">
      <dcr:datcat rdf:resource="http://www.isocat.org/datcat/DC-2741"/>
      <owl:versionInfo>http://www.isocat.org/datcat/DC-2741</owl:versionInfo>
      <rdfs:comment>
            post-prepositional [praep] form of the pronoun
                (http://www.isocat.org/datcat/DC-2741)
            </rdfs:comment>
      <rdfs:label>post-prepositional</rdfs:label>
      <rdfs:subClassOf>
         <owl:Class rdf:about="#postprepositionality"/>
      </rdfs:subClassOf>
      <owl:versionInfo>subClassOf postprepositionality (dcif:conceptualDomain)</owl:versionInfo>
   </owl:Class>
   <owl:Class rdf:ID="adjp">
      <dcr:datcat rdf:resource="http://www.isocat.org/datcat/DC-2706"/>
      <owl:versionInfo>http://www.isocat.org/datcat/DC-2706</owl:versionInfo>
      <rdfs:comment>
            post-prepositional adjective [adjp] contains non-inflecting de-adjectival flexemes such as polsku 'Polish' and niemiecku 'German'
                (http://www.isocat.org/datcat/DC-2706)
            </rdfs:comment>
      <rdfs:label>post-prepositional adjective</rdfs:label>
   </owl:Class>
   <owl:Class rdf:ID="postprepositionality">
      <dcr:datcat rdf:resource="http://www.isocat.org/datcat/DC-2740"/>
      <owl:versionInfo>http://www.isocat.org/datcat/DC-2740</owl:versionInfo>
      <rdfs:comment>
            Post-prepositionality [post-prepositionality] is a grammatical category appropriate for some forms of the 3rd-person personal pronoun which takes one of two values depending on whether the pronominal form can follow or attach to a preposition (post-prepositional) or not (non-post-prepositional).
                (http://www.isocat.org/datcat/DC-2740)
            </rdfs:comment>
      <rdfs:label>post-prepositionality</rdfs:label>
   </owl:Class>
   <owl:Class rdf:ID="pred">
      <dcr:datcat rdf:resource="http://www.isocat.org/datcat/DC-2714"/>
      <owl:versionInfo>http://www.isocat.org/datcat/DC-2714</owl:versionInfo>
      <rdfs:comment>
            predicative [pred] contains non-inflecting lexemes such as brak `to lack, to miss', trzeba (deontic modality), warto `to be worth it', etc., which analytically inflect for tense and mood (e.g., było warto, warto, warto by, będzie warto)
                (http://www.isocat.org/datcat/DC-2714)
            </rdfs:comment>
      <rdfs:label>predicative</rdfs:label>
   </owl:Class>
   <owl:Class rdf:ID="adjc">
      <dcr:datcat rdf:resource="http://www.isocat.org/datcat/DC-2710"/>
      <owl:versionInfo>http://www.isocat.org/datcat/DC-2710</owl:versionInfo>
      <rdfs:comment>
            non-inflecting adjectival class [adjc] of one-form lexemes consisting of forms which may only be used in predicative contexts (adjc)4, e.g., zdrów ‘healthy’ (cf. On wydaje się zdrów ‘He seems healthy’, but not *zdrów człowiek ‘healthy man’) or ciekaw ‘curious’ (e.g., Jestem ciekaw ‘I am curious’, but not *ciekaw człowiek ‘curious man’).
                (http://www.isocat.org/datcat/DC-2710)
            </rdfs:comment>
      <rdfs:label>predicative adjective</rdfs:label>
   </owl:Class>
   <owl:Class rdf:ID="prep">
      <dcr:datcat rdf:resource="http://www.isocat.org/datcat/DC-2757"/>
      <owl:versionInfo>http://www.isocat.org/datcat/DC-2757</owl:versionInfo>
      <rdfs:comment>
            Preposition [prep] contains non-inflecting prepositional flexemes, which have the lexical category of case, indicating the subcategorisation properties of the preposition, and which do not occur with non-postprepositional forms of pronouns. Grammatical categories of preposition [prep]: case (http://www.isocat.org/datcat/DC-2720), vocalicity (http://www.isocat.org/datcat/DC-2748) (optional).
                (http://www.isocat.org/datcat/DC-2757)
            </rdfs:comment>
      <rdfs:label>preposition</rdfs:label>
   </owl:Class>
   <owl:Class rdf:ID="siebie">
      <dcr:datcat rdf:resource="http://www.isocat.org/datcat/DC-2758"/>
      <owl:versionInfo>http://www.isocat.org/datcat/DC-2758</owl:versionInfo>
      <rdfs:comment>
            Pronoun siebie [siebie] contains exactly one flexeme, siebie, apparently the only Polish flexeme which inflects only for case (defectively, without nominative and vocative forms). Grammatical categories of pronoun siebie [siebie]: case (http://www.isocat.org/datcat/DC-2720).
                (http://www.isocat.org/datcat/DC-2758)
            </rdfs:comment>
      <rdfs:label>pronoun siebie</rdfs:label>
   </owl:Class>
   <owl:Class rdf:ID="interp">
      <dcr:datcat rdf:resource="http://www.isocat.org/datcat/DC-2713"/>
      <owl:versionInfo>http://www.isocat.org/datcat/DC-2713</owl:versionInfo>
      <rdfs:comment>
            punctuation [interp] contains non-infecting punctuation 'lexemes', e.g., :, ., !, etc.
                (http://www.isocat.org/datcat/DC-2713)
            </rdfs:comment>
      <rdfs:label>punctuation</rdfs:label>
   </owl:Class>
   <owl:Class rdf:ID="sec">
      <dcr:datcat rdf:resource="http://www.isocat.org/datcat/DC-2777"/>
      <owl:versionInfo>http://www.isocat.org/datcat/DC-2777</owl:versionInfo>
      <rdfs:comment>
            Second [sec] is a value of the grammatical category of person appropriate for participants taking part in the speech act but different from the speaker.
                (http://www.isocat.org/datcat/DC-2777)
            </rdfs:comment>
      <rdfs:label>second person</rdfs:label>
      <rdfs:subClassOf>
         <owl:Class rdf:about="#person"/>
      </rdfs:subClassOf>
      <owl:versionInfo>subClassOf person (dcif:conceptualDomain)</owl:versionInfo>
   </owl:Class>
   <owl:Class rdf:ID="sg">
      <dcr:datcat rdf:resource="http://www.isocat.org/datcat/DC-2707"/>
      <owl:versionInfo>http://www.isocat.org/datcat/DC-2707</owl:versionInfo>
      <rdfs:comment>
            Singular [sg] is a value of the grammatical category of number typically appropriate for lexemes whose reference is non-aggregate or is perceived as such.
                (http://www.isocat.org/datcat/DC-2707)
            </rdfs:comment>
      <rdfs:label>singular number</rdfs:label>
      <rdfs:subClassOf>
         <owl:Class rdf:about="#number"/>
      </rdfs:subClassOf>
      <owl:versionInfo>subClassOf number (dcif:conceptualDomain)</owl:versionInfo>
   </owl:Class>
   <owl:Class rdf:ID="sup">
      <dcr:datcat rdf:resource="http://www.isocat.org/datcat/DC-2782"/>
      <owl:versionInfo>http://www.isocat.org/datcat/DC-2782</owl:versionInfo>
      <rdfs:comment>
            Superlative [sup] is a value of the grammatical category of degree appropriate for adjectives and adverbs expressing the highest level of intensity of the named feature.
                (http://www.isocat.org/datcat/DC-2782)
            </rdfs:comment>
      <rdfs:label>superlative degree</rdfs:label>
      <rdfs:subClassOf>
         <owl:Class rdf:about="#degree"/>
      </rdfs:subClassOf>
      <owl:versionInfo>subClassOf degree (dcif:conceptualDomain)</owl:versionInfo>
   </owl:Class>
   <owl:Class rdf:ID="ter">
      <dcr:datcat rdf:resource="http://www.isocat.org/datcat/DC-2778"/>
      <owl:versionInfo>http://www.isocat.org/datcat/DC-2778</owl:versionInfo>
      <rdfs:comment>
            Third [ter] is a value of the grammatical category of person appropriate for participants not taking part in the speech act.
                (http://www.isocat.org/datcat/DC-2778)
            </rdfs:comment>
      <rdfs:label>third person</rdfs:label>
      <rdfs:subClassOf>
         <owl:Class rdf:about="#person"/>
      </rdfs:subClassOf>
      <owl:versionInfo>subClassOf person (dcif:conceptualDomain)</owl:versionInfo>
   </owl:Class>
   <owl:Class rdf:ID="ign">
      <dcr:datcat rdf:resource="http://www.isocat.org/datcat/DC-2719"/>
      <owl:versionInfo>http://www.isocat.org/datcat/DC-2719</owl:versionInfo>
      <rdfs:comment>
            unknown form [ign] contains forms which have not been recognised in the process of morphological analysis
                (http://www.isocat.org/datcat/DC-2719)
            </rdfs:comment>
      <rdfs:label>unknown form</rdfs:label>
   </owl:Class>
   <owl:Class rdf:ID="wok">
      <dcr:datcat rdf:resource="http://www.isocat.org/datcat/DC-2749"/>
      <owl:versionInfo>http://www.isocat.org/datcat/DC-2749</owl:versionInfo>
      <rdfs:comment>
            Vocalic [wok] agglutinates attach to forms ending in a consonant.
                (http://www.isocat.org/datcat/DC-2749)
            </rdfs:comment>
      <rdfs:label>vocalic</rdfs:label>
      <rdfs:subClassOf>
         <owl:Class rdf:about="#vocalicity"/>
      </rdfs:subClassOf>
      <owl:versionInfo>subClassOf vocalicity (dcif:conceptualDomain)</owl:versionInfo>
   </owl:Class>
   <owl:Class rdf:ID="vocalicity">
      <dcr:datcat rdf:resource="http://www.isocat.org/datcat/DC-2748"/>
      <owl:versionInfo>http://www.isocat.org/datcat/DC-2748</owl:versionInfo>
      <rdfs:comment>
            Vocalicity distinguishes those agglutinates (e.g., -em) [wok] which attach to forms ending in a consonant, from those (e.g., -m) [nwok] which attach to forms ending in a vowel.
                (http://www.isocat.org/datcat/DC-2748)
            </rdfs:comment>
      <rdfs:label>vocalicity</rdfs:label>
   </owl:Class>
   <owl:Class rdf:ID="voc">
      <dcr:datcat rdf:resource="http://www.isocat.org/datcat/DC-2727"/>
      <owl:versionInfo>http://www.isocat.org/datcat/DC-2727</owl:versionInfo>
      <rdfs:comment>
            Vocative [voc] is a value of the grammatical category of case paradigmatically appropriate for forms not conditioned syntactically but rather used in the function of address.
                (http://www.isocat.org/datcat/DC-2727)
            </rdfs:comment>
      <rdfs:label>vocative case</rdfs:label>
      <rdfs:subClassOf>
         <owl:Class rdf:about="#case"/>
      </rdfs:subClassOf>
      <owl:versionInfo>subClassOf case (dcif:conceptualDomain)</owl:versionInfo>
   </owl:Class>
   <owl:Class rdf:ID="winien">
      <dcr:datcat rdf:resource="http://www.isocat.org/datcat/DC-2768"/>
      <owl:versionInfo>http://www.isocat.org/datcat/DC-2768</owl:versionInfo>
      <rdfs:comment>
            Winien [winien] contains the flexemes winien `should', powinien `should' and rad `eager, pleased', inflecting for number and gender, with only analytical past tense and conditional forms. Grammatical categories of winien [winien]: number (http://www.isocat.org/datcat/DC-2709), gender (http://www.isocat.org/datcat/DC-2728), aspect.
                (http://www.isocat.org/datcat/DC-2768)
            </rdfs:comment>
      <rdfs:label>winien</rdfs:label>
   </owl:Class>
</rdf:RDF>