<?xml version="1.0" encoding="UTF-8"?>
<rdf:RDF xmlns:xsd="http://www.w3.org/2001/XMLSchema#"
         xmlns="http://www.isocat.org/ns/dcr.owl#"
         xmlns:dcr="http://www.isocat.org/ns/dcr.rdf#"
         xmlns:rdfs="http://www.w3.org/2000/01/rdf-schema#"
         xmlns:owl="http://www.w3.org/2002/07/owl#"
         xmlns:dcif="http://www.isocat.org/ns/dcif"
         xmlns:rdf="http://www.w3.org/1999/02/22-rdf-syntax-ns#"
         xml:base="http://www.isocat.org/ns/dcr.owl">
   <owl:Ontology>
      <rdfs:comment>OWL representation of ISOcat DCIF exported Data Categories</rdfs:comment>
   </owl:Ontology>
   <owl:Class rdf:ID="attributiveAdjective">
      <dcr:datcat rdf:resource="http://www.isocat.org/datcat/DC-1243"/>
      <owl:versionInfo>http://www.isocat.org/datcat/DC-1243</owl:versionInfo>
      <rdfs:comment>
                            An Attributive Adjective comes before a Noun and not after a Copula Verb, like BE, SEEM, etc.
                                (www.usingEnglish.com/glossary/attributive-adjective.html; http://www.isocat.org/datcat/DC-1243)
                            </rdfs:comment>
      <rdfs:comment>
                            (of an adjective or adjectival phrase) modifying a noun and constituting part of the same noun phrase, in English normally preceding the noun, as black in Fido is a black dog (as opposed to Fido is black)
                                (www.wordreference.com/English/definition.asp?en=attributive+adjective; http://www.isocat.org/datcat/DC-1243)
                            </rdfs:comment>
      <rdfs:label>Attributive adjective</rdfs:label>
   </owl:Class>
   <owl:Class rdf:ID="futurePerfect">
      <dcr:datcat rdf:resource="http://www.isocat.org/datcat/DC-1292"/>
      <owl:versionInfo>http://www.isocat.org/datcat/DC-1292</owl:versionInfo>
      <rdfs:comment>
                            A verb tense that refers to an action or state of being completed in the future. into English requires the use of the auxiliary verbs will/shall have.
                                (www.southwestern.edu/~carlg/Latin_Web/glossary.html; http://www.isocat.org/datcat/DC-1292)
                            </rdfs:comment>
      <rdfs:comment>
                            Denoting a tense of verbs describing an action that will have been performed by a certain time. In English this is formed with will have or shall have plus the past participle.
                                (www.wordreference.com/English/definition.asp?en=future+perfect; http://www.isocat.org/datcat/DC-1292)
                            </rdfs:comment>
      <rdfs:label>Future perfect</rdfs:label>
   </owl:Class>
   <owl:Class rdf:ID="gerundive">
      <dcr:datcat rdf:resource="http://www.isocat.org/datcat/DC-1294"/>
      <owl:versionInfo>http://www.isocat.org/datcat/DC-1294</owl:versionInfo>
      <rdfs:comment>
                            an adjective formed from a verb, expressing the desirability of the activity denoted by the verb
                                (www.wordreference.com/English/definition.asp?en=gerundive); http://www.isocat.org/datcat/DC-1294)
                            </rdfs:comment>
      <rdfs:comment>
                            a noun formed from a verb, denoting an action or state. In English, the gerund, like the present participle, is formed in -ing
                                (www.wordreference.com/English/definition.asp?en=gerund; http://www.isocat.org/datcat/DC-1294)
                            </rdfs:comment>
      <rdfs:label>Gerundive</rdfs:label>
   </owl:Class>
   <owl:Class rdf:ID="impersonal">
      <dcr:datcat rdf:resource="http://www.isocat.org/datcat/DC-1306"/>
      <owl:versionInfo>http://www.isocat.org/datcat/DC-1306</owl:versionInfo>
      <rdfs:comment>
                            An impersonal verb is a verb that - occurs only in third person singular forms - has no specified agent , and - has a dummy subject or no subject.
                                (www.sil.org/linguistics/GlossaryOfLinguisticTerms/WhatIsAnImpersonalVerb.htm; http://www.isocat.org/datcat/DC-1306)
                            </rdfs:comment>
      <rdfs:comment>
                            (of a verb) having no logical subject. Usually in English the pronoun it is used in such cases as a grammatical subject, as for example in It is raining. (of a pronoun) not denoting a person
                                (www.wordreference.com/English/definition.asp?en=impersonal; http://www.isocat.org/datcat/DC-1306)
                            </rdfs:comment>
      <rdfs:label>Impersonal</rdfs:label>
   </owl:Class>
   <owl:Class rdf:ID="order">
      <dcr:datcat rdf:resource="http://www.isocat.org/datcat/DC-1337"/>
      <owl:versionInfo>http://www.isocat.org/datcat/DC-1337</owl:versionInfo>
      <rdfs:comment>
                            A state in which all components or elements are arranged logically, comprehensibly, or naturally
                                (www.wordreference.com/English/definition.asp?en=order; http://www.isocat.org/datcat/DC-1337)
                            </rdfs:comment>
      <rdfs:label>Order</rdfs:label>
   </owl:Class>
   <owl:Class rdf:ID="pastPerfect">
      <dcr:datcat rdf:resource="http://www.isocat.org/datcat/DC-1348"/>
      <owl:versionInfo>http://www.isocat.org/datcat/DC-1348</owl:versionInfo>
      <rdfs:comment>
                            Past perfect tense is an absolute-relative tense that refers to a time in the past relative to a reference point, which itself is in the past relative to the moment of utterance
                                (www.sil.org/linguistics/GlossaryOfLinguisticTerms/WhatIsPastPerfectTense.htm; http://www.isocat.org/datcat/DC-1348)
                            </rdfs:comment>
      <rdfs:comment>
                            denoting a tense of verbs used in relating past events where the action had already occurred at the time of the action of a main verb that is itself in a past tense. In English this is a compound tense formed with had plus the past participle
                                (www.wordreference.com/English/definition.asp?en=past+perfect; http://www.isocat.org/datcat/DC-1348)
                            </rdfs:comment>
      <rdfs:label>Past perfect</rdfs:label>
   </owl:Class>
   <owl:Class rdf:ID="perfect">
      <dcr:datcat rdf:resource="http://www.isocat.org/datcat/DC-1351"/>
      <owl:versionInfo>http://www.isocat.org/datcat/DC-1351</owl:versionInfo>
      <rdfs:comment>
                            A verb tense that refers to completed action in the past. It corresponds to three English tenses.
                                (www.southwestern.edu/~carlg/Latin_Web/glossary.html; http://www.isocat.org/datcat/DC-1351)
                            </rdfs:comment>
      <rdfs:label>Perfect</rdfs:label>
   </owl:Class>
   <owl:Class rdf:ID="pluperfect">
      <dcr:datcat rdf:resource="http://www.isocat.org/datcat/DC-1353"/>
      <owl:versionInfo>http://www.isocat.org/datcat/DC-1353</owl:versionInfo>
      <rdfs:comment>
                            A verb tense that refers to action or state of being completed before some other event in the past. Its translation into English requires the use of the auxiliariy verb had.
                                (www.southwestern.edu/~carlg/Latin_Web/glossary.html; http://www.isocat.org/datcat/DC-1353)
                            </rdfs:comment>
      <rdfs:label>Pluperfect</rdfs:label>
   </owl:Class>
   <owl:Class rdf:ID="pronominal">
      <dcr:datcat rdf:resource="http://www.isocat.org/datcat/DC-1369"/>
      <owl:versionInfo>http://www.isocat.org/datcat/DC-1369</owl:versionInfo>
      <rdfs:comment>
                            A pronominal is a phrase that functions as a pronoun
                                (www.sil.org/linguistics/GlossaryOfLinguisticTerms/WhatIsAPronominal.htm; http://www.isocat.org/datcat/DC-1369)
                            </rdfs:comment>
      <rdfs:label>Pronominal</rdfs:label>
   </owl:Class>
   <owl:Class rdf:ID="qualifier">
      <dcr:datcat rdf:resource="http://www.isocat.org/datcat/DC-1373"/>
      <owl:versionInfo>http://www.isocat.org/datcat/DC-1373</owl:versionInfo>
      <rdfs:comment>
                            Also called MODIFIER : A word or phrase that qualifies the sense of another word; for example, the noun alarm is a modifier of clock in "alarm clock" and the phrase every day is an adverbial modifier of walks in "he walks every day"
                                (www.wordreference.com/English/definition.asp?en=modifier; http://www.isocat.org/datcat/DC-1373)
                            </rdfs:comment>
      <rdfs:label>Qualifier</rdfs:label>
   </owl:Class>
   <owl:Class rdf:ID="substantiveAdjective">
      <dcr:datcat rdf:resource="http://www.isocat.org/datcat/DC-1394"/>
      <owl:versionInfo>http://www.isocat.org/datcat/DC-1394</owl:versionInfo>
      <rdfs:comment>
                            An adjective that modifies an implied, but not expressed, noun. When translating such an adjective into English, you must supply the missing noun.
                                (www.southwestern.edu/~carlg/Latin_Web/glossary.html; http://www.isocat.org/datcat/DC-1394)
                            </rdfs:comment>
      <rdfs:label>Substantive adjective</rdfs:label>
   </owl:Class>
   <owl:Class rdf:ID="supine">
      <dcr:datcat rdf:resource="http://www.isocat.org/datcat/DC-1397"/>
      <owl:versionInfo>http://www.isocat.org/datcat/DC-1397</owl:versionInfo>
      <rdfs:comment>
                            The supine form of the verb in Swedish is used with the auxiliary verb ha (`to have') to form the perfective. The supine form is easy to spot a verb form that always ends with a t.
                                (www-linguistics.stanford.edu/linguistics/semgroup/archive/1999/sf_sells.html; http://www.isocat.org/datcat/DC-1397)
                            </rdfs:comment>
      <rdfs:label>Supine</rdfs:label>
   </owl:Class>
   <owl:Class rdf:ID="transgressive">
      <dcr:datcat rdf:resource="http://www.isocat.org/datcat/DC-1404"/>
      <owl:versionInfo>http://www.isocat.org/datcat/DC-1404</owl:versionInfo>
      <rdfs:comment>
                            present (action in the same time as of the predicate): The dog going through the house barks. past (action premature to the one of predicate): He has started to read the book after he had sat down.
                                (ark.wz.cz/cidarke/mverb.html; http://www.isocat.org/datcat/DC-1404)
                            </rdfs:comment>
      <rdfs:label>Transgressive</rdfs:label>
   </owl:Class>
   <owl:Class rdf:ID="abbreviation">
      <dcr:datcat rdf:resource="http://www.isocat.org/datcat/DC-1418"/>
      <owl:versionInfo>http://www.isocat.org/datcat/DC-1418</owl:versionInfo>
      <rdfs:comment>
                            Designation formed by omitting words or letters from a longer form and refering to the same concept.
                                (http://www.isocat.org/datcat/DC-1418)
                            </rdfs:comment>
      <rdfs:label>abbreviation</rdfs:label>
   </owl:Class>
   <owl:Class rdf:ID="abessiveCase">
      <dcr:datcat rdf:resource="http://www.isocat.org/datcat/DC-1223"/>
      <owl:versionInfo>http://www.isocat.org/datcat/DC-1223</owl:versionInfo>
      <rdfs:comment>
                            Case that expresses the lack or absence of the referent of the noun it marks.
                                (Pei and Gaynor 1954 &amp; Gove 1966; http://www.isocat.org/datcat/DC-1223)
                            </rdfs:comment>
      <rdfs:label>abessive case</rdfs:label>
      <rdfs:subClassOf>
         <owl:Class rdf:about="#case"/>
      </rdfs:subClassOf>
      <owl:versionInfo>subClassOf case (dcif:conceptualDomain)</owl:versionInfo>
   </owl:Class>
   <owl:Class rdf:ID="ablativeCase">
      <dcr:datcat rdf:resource="http://www.isocat.org/datcat/DC-1224"/>
      <owl:versionInfo>http://www.isocat.org/datcat/DC-1224</owl:versionInfo>
      <rdfs:comment>
                            Case used to typically indicate locative or instrumental function.
                                (Crystal 2003; http://www.isocat.org/datcat/DC-1224)
                            </rdfs:comment>
      <rdfs:label>ablative case</rdfs:label>
      <rdfs:subClassOf>
         <owl:Class rdf:about="#case"/>
      </rdfs:subClassOf>
      <owl:versionInfo>subClassOf case (dcif:conceptualDomain)</owl:versionInfo>
   </owl:Class>
   <owl:Class rdf:ID="absolutiveCase">
      <dcr:datcat rdf:resource="http://www.isocat.org/datcat/DC-1225"/>
      <owl:versionInfo>http://www.isocat.org/datcat/DC-1225</owl:versionInfo>
      <rdfs:comment>
                            Case for nouns in ergative-absolute languages that would generally be the subjects of intransitive verbs or the objects of transitive verbs in the translational equivalents of nominative-accusative languages such as English.
                                (dfki; http://www.isocat.org/datcat/DC-1225)
                            </rdfs:comment>
      <rdfs:label>absolutive case</rdfs:label>
      <rdfs:subClassOf>
         <owl:Class rdf:about="#case"/>
      </rdfs:subClassOf>
      <owl:versionInfo>subClassOf case (dcif:conceptualDomain)</owl:versionInfo>
   </owl:Class>
   <owl:Class rdf:ID="accusativeCase">
      <dcr:datcat rdf:resource="http://www.isocat.org/datcat/DC-1226"/>
      <owl:versionInfo>http://www.isocat.org/datcat/DC-1226</owl:versionInfo>
      <rdfs:comment>
                            Case used to indicate direct object.
                                (Crystal 2003; http://www.isocat.org/datcat/DC-1226)
                            </rdfs:comment>
      <rdfs:label>accusative case</rdfs:label>
      <rdfs:subClassOf>
         <owl:Class rdf:about="#case"/>
      </rdfs:subClassOf>
      <owl:versionInfo>subClassOf case (dcif:conceptualDomain)</owl:versionInfo>
   </owl:Class>
   <owl:Class rdf:ID="activeVoice">
      <dcr:datcat rdf:resource="http://www.isocat.org/datcat/DC-1227"/>
      <owl:versionInfo>http://www.isocat.org/datcat/DC-1227</owl:versionInfo>
      <rdfs:comment>
                            Value that expresses the situation where the grammatical subject is also the semantic actor of the verb.
                                (http://www.isocat.org/datcat/DC-1227)
                            </rdfs:comment>
      <rdfs:label>active voice</rdfs:label>
      <rdfs:subClassOf>
         <owl:Class rdf:about="#voice"/>
      </rdfs:subClassOf>
      <owl:versionInfo>subClassOf voice (dcif:conceptualDomain)</owl:versionInfo>
   </owl:Class>
   <owl:Class rdf:ID="add">
      <dcr:datcat rdf:resource="http://www.isocat.org/datcat/DC-2093"/>
      <owl:versionInfo>http://www.isocat.org/datcat/DC-2093</owl:versionInfo>
      <rdfs:comment>
                            Add a string at position X.
                                (http://www.isocat.org/datcat/DC-2093)
                            </rdfs:comment>
      <rdfs:label>add</rdfs:label>
   </owl:Class>
   <owl:Class rdf:ID="addAffix">
      <dcr:datcat rdf:resource="http://www.isocat.org/datcat/DC-2201"/>
      <owl:versionInfo>http://www.isocat.org/datcat/DC-2201</owl:versionInfo>
      <rdfs:comment>
                            Operation that adds the specified affix
                                (http://www.isocat.org/datcat/DC-2201)
                            </rdfs:comment>
      <rdfs:label>add affix</rdfs:label>
   </owl:Class>
   <owl:Class rdf:ID="addAfter">
      <dcr:datcat rdf:resource="http://www.isocat.org/datcat/DC-1831"/>
      <owl:versionInfo>http://www.isocat.org/datcat/DC-1831</owl:versionInfo>
      <rdfs:comment>
                            Operation that adds a string to the right
                                (http://www.isocat.org/datcat/DC-1831)
                            </rdfs:comment>
      <rdfs:label>add after</rdfs:label>
   </owl:Class>
   <owl:Class rdf:ID="addBefore">
      <dcr:datcat rdf:resource="http://www.isocat.org/datcat/DC-1829"/>
      <owl:versionInfo>http://www.isocat.org/datcat/DC-1829</owl:versionInfo>
      <rdfs:comment>
                            Operation that adds a string to the left
                                (http://www.isocat.org/datcat/DC-1829)
                            </rdfs:comment>
      <rdfs:label>add before</rdfs:label>
   </owl:Class>
   <owl:Class rdf:ID="addComponentLemma">
      <dcr:datcat rdf:resource="http://www.isocat.org/datcat/DC-2202"/>
      <owl:versionInfo>http://www.isocat.org/datcat/DC-2202</owl:versionInfo>
      <rdfs:comment>
                            Operation that adds the lemma of a specific component
                                (http://www.isocat.org/datcat/DC-2202)
                            </rdfs:comment>
      <rdfs:label>add component lemma</rdfs:label>
   </owl:Class>
   <owl:Class rdf:ID="addComponentStem">
      <dcr:datcat rdf:resource="http://www.isocat.org/datcat/DC-2204"/>
      <owl:versionInfo>http://www.isocat.org/datcat/DC-2204</owl:versionInfo>
      <rdfs:comment>
                            Operation that adds the stem of the specified component
                                (http://www.isocat.org/datcat/DC-2204)
                            </rdfs:comment>
      <rdfs:label>add component stem</rdfs:label>
   </owl:Class>
   <owl:Class rdf:ID="addFirstConsonant">
      <dcr:datcat rdf:resource="http://www.isocat.org/datcat/DC-2198"/>
      <owl:versionInfo>http://www.isocat.org/datcat/DC-2198</owl:versionInfo>
      <rdfs:comment>
                            Operation that adds the first consonant of the operand
                                (http://www.isocat.org/datcat/DC-2198)
                            </rdfs:comment>
      <rdfs:label>add first consonant</rdfs:label>
   </owl:Class>
   <owl:Class rdf:ID="addFirstVowel">
      <dcr:datcat rdf:resource="http://www.isocat.org/datcat/DC-2199"/>
      <owl:versionInfo>http://www.isocat.org/datcat/DC-2199</owl:versionInfo>
      <rdfs:comment>
                            Operation that adds the first vowel of the operand
                                (http://www.isocat.org/datcat/DC-2199)
                            </rdfs:comment>
      <rdfs:label>add first vowel</rdfs:label>
   </owl:Class>
   <owl:Class rdf:ID="addLemma">
      <dcr:datcat rdf:resource="http://www.isocat.org/datcat/DC-2200"/>
      <owl:versionInfo>http://www.isocat.org/datcat/DC-2200</owl:versionInfo>
      <rdfs:comment>
                            Operation that adds the given lemma
                                (http://www.isocat.org/datcat/DC-2200)
                            </rdfs:comment>
      <rdfs:label>add lemma</rdfs:label>
   </owl:Class>
   <owl:Class rdf:ID="addLowerCaseComponentLemma">
      <dcr:datcat rdf:resource="http://www.isocat.org/datcat/DC-2203"/>
      <owl:versionInfo>http://www.isocat.org/datcat/DC-2203</owl:versionInfo>
      <rdfs:comment>
                            Operation that adds the lemma of the component in lower case initiale
                                (http://www.isocat.org/datcat/DC-2203)
                            </rdfs:comment>
      <rdfs:label>add lower case component lemma</rdfs:label>
   </owl:Class>
   <owl:Class rdf:ID="adessiveCase">
      <dcr:datcat rdf:resource="http://www.isocat.org/datcat/DC-1228"/>
      <owl:versionInfo>http://www.isocat.org/datcat/DC-1228</owl:versionInfo>
      <rdfs:comment>
                            Case which expresses the meaning of presence 'at' or 'near' a place.
                                (Crystal 2003; http://www.isocat.org/datcat/DC-1228)
                            </rdfs:comment>
      <rdfs:label>adessive case</rdfs:label>
      <rdfs:subClassOf>
         <owl:Class rdf:about="#case"/>
      </rdfs:subClassOf>
      <owl:versionInfo>subClassOf case (dcif:conceptualDomain)</owl:versionInfo>
   </owl:Class>
   <owl:Class rdf:ID="aditiveCase">
      <dcr:datcat rdf:resource="http://www.isocat.org/datcat/DC-1229"/>
      <owl:versionInfo>http://www.isocat.org/datcat/DC-1229</owl:versionInfo>
      <rdfs:comment>
                            Case expressing "to" in Basque studies.
                                (SIL; http://www.isocat.org/datcat/DC-1229)
                            </rdfs:comment>
      <rdfs:label>aditive case</rdfs:label>
      <rdfs:subClassOf>
         <owl:Class rdf:about="#case"/>
      </rdfs:subClassOf>
      <owl:versionInfo>subClassOf case (dcif:conceptualDomain)</owl:versionInfo>
   </owl:Class>
   <owl:Class rdf:ID="adjective">
      <dcr:datcat rdf:resource="http://www.isocat.org/datcat/DC-1230"/>
      <owl:versionInfo>http://www.isocat.org/datcat/DC-1230</owl:versionInfo>
      <rdfs:comment>
                            Part of speech related to attributes of noun.
                                (http://www.isocat.org/datcat/DC-1230)
                            </rdfs:comment>
      <rdfs:label>adjective</rdfs:label>
      <rdfs:subClassOf>
         <owl:Class rdf:about="#partOfSpeech"/>
      </rdfs:subClassOf>
      <owl:versionInfo>subClassOf partOfSpeech (dcif:conceptualDomain)</owl:versionInfo>
      <rdfs:subClassOf>
         <owl:Class rdf:about="#syntacticType"/>
      </rdfs:subClassOf>
      <owl:versionInfo>subClassOf syntacticType (dcif:conceptualDomain)</owl:versionInfo>
   </owl:Class>
   <owl:Class rdf:ID="adposition">
      <dcr:datcat rdf:resource="http://www.isocat.org/datcat/DC-1231"/>
      <owl:versionInfo>http://www.isocat.org/datcat/DC-1231</owl:versionInfo>
      <rdfs:comment>
                            Part of speech that occurs before/inside/after a complement composed of a noun phrase, noun, pronoun or clause that functions as a noun phrase and form a single structure with the complement to express its grammatical and semantic relation to another unit.
                                (http://www.isocat.org/datcat/DC-1231)
                            </rdfs:comment>
      <rdfs:label>adposition</rdfs:label>
      <rdfs:subClassOf>
         <owl:Class rdf:about="#partOfSpeech"/>
      </rdfs:subClassOf>
      <owl:versionInfo>subClassOf partOfSpeech (dcif:conceptualDomain)</owl:versionInfo>
   </owl:Class>
   <owl:Class rdf:ID="adverb">
      <dcr:datcat rdf:resource="http://www.isocat.org/datcat/DC-1232"/>
      <owl:versionInfo>http://www.isocat.org/datcat/DC-1232</owl:versionInfo>
      <rdfs:comment>
                            Part of speech to refer to an heterogeneous group of words whose most frequent function is to specify the mode of action of the verb.
                                (Crystal 2003; http://www.isocat.org/datcat/DC-1232)
                            </rdfs:comment>
      <rdfs:label>adverb</rdfs:label>
      <rdfs:subClassOf>
         <owl:Class rdf:about="#partOfSpeech"/>
      </rdfs:subClassOf>
      <owl:versionInfo>subClassOf partOfSpeech (dcif:conceptualDomain)</owl:versionInfo>
      <rdfs:subClassOf>
         <owl:Class rdf:about="#syntacticType"/>
      </rdfs:subClassOf>
      <owl:versionInfo>subClassOf syntacticType (dcif:conceptualDomain)</owl:versionInfo>
   </owl:Class>
   <owl:Class rdf:ID="affix">
      <dcr:datcat rdf:resource="http://www.isocat.org/datcat/DC-1234"/>
      <owl:versionInfo>http://www.isocat.org/datcat/DC-1234</owl:versionInfo>
      <rdfs:comment>
                            Letter or group of letters which are added to a word to make a new word.
                                (Sue Ellen Wright; http://www.isocat.org/datcat/DC-1234)
                            </rdfs:comment>
      <rdfs:label>affix</rdfs:label>
   </owl:Class>
   <owl:Class rdf:ID="affixRank">
      <dcr:datcat rdf:resource="http://www.isocat.org/datcat/DC-2184"/>
      <owl:versionInfo>http://www.isocat.org/datcat/DC-2184</owl:versionInfo>
      <rdfs:comment>
                            Rank of an affix
                                (http://www.isocat.org/datcat/DC-2184)
                            </rdfs:comment>
      <rdfs:label>affix rank</rdfs:label>
   </owl:Class>
   <owl:Class rdf:ID="affixedPersonalPronoun">
      <dcr:datcat rdf:resource="http://www.isocat.org/datcat/DC-2221"/>
      <owl:versionInfo>http://www.isocat.org/datcat/DC-2221</owl:versionInfo>
      <rdfs:comment>
                            Personnal pronoun that is affixed.
                                (MIRACL &amp; LSCA; http://www.isocat.org/datcat/DC-2221)
                            </rdfs:comment>
      <rdfs:label>affixed personal pronoun</rdfs:label>
      <rdfs:subClassOf>
         <owl:Class rdf:about="#pronoun"/>
      </rdfs:subClassOf>
      <owl:versionInfo>subClassOf pronoun (dcif:isA)</owl:versionInfo>
   </owl:Class>
   <owl:Class rdf:ID="allativeCase">
      <dcr:datcat rdf:resource="http://www.isocat.org/datcat/DC-1236"/>
      <owl:versionInfo>http://www.isocat.org/datcat/DC-1236</owl:versionInfo>
      <rdfs:comment>
                            Case which expresses the meaning of motion 'to' or 'towards' the referent it marks.
                                (Crystal 2003; http://www.isocat.org/datcat/DC-1236)
                            </rdfs:comment>
      <rdfs:label>allative case</rdfs:label>
      <rdfs:subClassOf>
         <owl:Class rdf:about="#case"/>
      </rdfs:subClassOf>
      <owl:versionInfo>subClassOf case (dcif:conceptualDomain)</owl:versionInfo>
   </owl:Class>
   <owl:Class rdf:ID="allomorph">
      <dcr:datcat rdf:resource="http://www.isocat.org/datcat/DC-1237"/>
      <owl:versionInfo>http://www.isocat.org/datcat/DC-1237</owl:versionInfo>
      <rdfs:comment>
                            One of two or more complementary morphs which manifest a morpheme in its different phonological or morphological environments.
                                (www.sil.org/linguistics/GlossaryOfLinguisticTerms/WhatIsAnAllomorph.htm; http://www.isocat.org/datcat/DC-1237)
                            </rdfs:comment>
      <rdfs:label>allomorph</rdfs:label>
   </owl:Class>
   <owl:Class rdf:ID="allusivePronoun">
      <dcr:datcat rdf:resource="http://www.isocat.org/datcat/DC-2223"/>
      <owl:versionInfo>http://www.isocat.org/datcat/DC-2223</owl:versionInfo>
      <rdfs:comment>
                            pronoun that have reference to something characterized by allusions.
                                (MIRACL &amp; LSCA; http://www.isocat.org/datcat/DC-2223)
                            </rdfs:comment>
      <rdfs:label>allusive pronoun</rdfs:label>
      <rdfs:subClassOf>
         <owl:Class rdf:about="#pronoun"/>
      </rdfs:subClassOf>
      <owl:versionInfo>subClassOf pronoun (dcif:isA)</owl:versionInfo>
   </owl:Class>
   <owl:Class rdf:ID="animacy">
      <dcr:datcat rdf:resource="http://www.isocat.org/datcat/DC-1902"/>
      <owl:versionInfo>http://www.isocat.org/datcat/DC-1902</owl:versionInfo>
      <rdfs:comment>
                            The characteristic of a word indicating that in a given discourse community, its referent is considered to be alive or to possess a quality of volition or consciousness.
                                (ISO12620; http://www.isocat.org/datcat/DC-1902)
                            </rdfs:comment>
      <rdfs:label>animacy</rdfs:label>
   </owl:Class>
   <owl:Class rdf:ID="animate">
      <dcr:datcat rdf:resource="http://www.isocat.org/datcat/DC-1911"/>
      <owl:versionInfo>http://www.isocat.org/datcat/DC-1911</owl:versionInfo>
      <rdfs:comment>
                            Perceived as alive.
                                (ISO12620; http://www.isocat.org/datcat/DC-1911)
                            </rdfs:comment>
      <rdfs:label>animate</rdfs:label>
      <rdfs:subClassOf>
         <owl:Class rdf:about="#animacy"/>
      </rdfs:subClassOf>
      <owl:versionInfo>subClassOf animacy (dcif:conceptualDomain)</owl:versionInfo>
   </owl:Class>
   <owl:Class rdf:ID="any">
      <dcr:datcat rdf:resource="http://www.isocat.org/datcat/DC-2193"/>
      <owl:versionInfo>http://www.isocat.org/datcat/DC-2193</owl:versionInfo>
      <rdfs:comment>
                            Markup meaning that all values are allowed
                                (http://www.isocat.org/datcat/DC-2193)
                            </rdfs:comment>
      <rdfs:label>any</rdfs:label>
   </owl:Class>
   <owl:Class rdf:ID="aorist">
      <dcr:datcat rdf:resource="http://www.isocat.org/datcat/DC-1240"/>
      <owl:versionInfo>http://www.isocat.org/datcat/DC-1240</owl:versionInfo>
      <rdfs:comment>
                            Simple past tense that is predominantly used for narration. Both the perfective and the imperfective forms can be used in the aorist without any restrictions.
                                (www.helsinki.fi/~bontchev/grammar/index.html; http://www.isocat.org/datcat/DC-1240)
                            </rdfs:comment>
      <rdfs:label>aorist</rdfs:label>
   </owl:Class>
   <owl:Class rdf:ID="apocope">
      <dcr:datcat rdf:resource="http://www.isocat.org/datcat/DC-2254"/>
      <owl:versionInfo>http://www.isocat.org/datcat/DC-2254</owl:versionInfo>
      <rdfs:comment>
                            property concerning the deletion of the final element in a word
                                (http://www.isocat.org/datcat/DC-2254)
                            </rdfs:comment>
      <rdfs:label>apocopate</rdfs:label>
      <rdfs:label>apocope</rdfs:label>
   </owl:Class>
   <owl:Class rdf:ID="approximate">
      <dcr:datcat rdf:resource="http://www.isocat.org/datcat/DC-2206"/>
      <owl:versionInfo>http://www.isocat.org/datcat/DC-2206</owl:versionInfo>
      <rdfs:comment>
                            Property used to qualify something similar but not exactly the same
                                (http://www.isocat.org/datcat/DC-2206)
                            </rdfs:comment>
      <rdfs:label>approximate</rdfs:label>
   </owl:Class>
   <owl:Class rdf:ID="aspect">
      <dcr:datcat rdf:resource="http://www.isocat.org/datcat/DC-1242"/>
      <owl:versionInfo>http://www.isocat.org/datcat/DC-1242</owl:versionInfo>
      <rdfs:comment>
                            Category associated to verbs and referring to the way the grammar marks the duration or type of temporal activity.
                                (Crystal; http://www.isocat.org/datcat/DC-1242)
                            </rdfs:comment>
      <rdfs:label>aspect</rdfs:label>
   </owl:Class>
   <owl:Class rdf:ID="auxiliary">
      <dcr:datcat rdf:resource="http://www.isocat.org/datcat/DC-1244"/>
      <owl:versionInfo>http://www.isocat.org/datcat/DC-1244</owl:versionInfo>
      <rdfs:comment>
                            Part of speech referring to the set of verbs, subordinate to the main lexical verb which help to make distinction in mood, aspect, voice etc.
                                (Crystal 2003; http://www.isocat.org/datcat/DC-1244)
                            </rdfs:comment>
      <rdfs:label>auxiliary</rdfs:label>
      <rdfs:subClassOf>
         <owl:Class rdf:about="#verb"/>
      </rdfs:subClassOf>
      <owl:versionInfo>subClassOf verb (dcif:isA)</owl:versionInfo>
   </owl:Class>
   <owl:Class rdf:ID="be">
      <dcr:datcat rdf:resource="http://www.isocat.org/datcat/DC-1246"/>
      <owl:versionInfo>http://www.isocat.org/datcat/DC-1246</owl:versionInfo>
      <rdfs:comment>
                            Verb used to link the subject of a sentence and its noun or adjective complement or complementing phrase in certain languages. This verb could be used also to form the passive voice.
                                (www.wordreference.com/English/definition.asp?en=be -&gt; 4); http://www.isocat.org/datcat/DC-1246)
                            </rdfs:comment>
      <rdfs:label>be</rdfs:label>
      <rdfs:subClassOf>
         <owl:Class rdf:about="#partOfSpeech"/>
      </rdfs:subClassOf>
      <owl:versionInfo>subClassOf partOfSpeech (dcif:conceptualDomain)</owl:versionInfo>
   </owl:Class>
   <owl:Class rdf:ID="benchLevelRegister">
      <dcr:datcat rdf:resource="http://www.isocat.org/datcat/DC-1989"/>
      <owl:versionInfo>http://www.isocat.org/datcat/DC-1989</owl:versionInfo>
      <rdfs:comment>
                            Register of terms used in applications-oriented as opposed to theoretical or academic levels of language.
                                (ISO12620; http://www.isocat.org/datcat/DC-1989)
                            </rdfs:comment>
      <rdfs:label>bench-level register</rdfs:label>
      <rdfs:label>shop term</rdfs:label>
      <rdfs:subClassOf>
         <owl:Class rdf:about="#register"/>
      </rdfs:subClassOf>
      <owl:versionInfo>subClassOf register (dcif:conceptualDomain)</owl:versionInfo>
   </owl:Class>
   <owl:Class rdf:ID="benefactiveCase">
      <dcr:datcat rdf:resource="http://www.isocat.org/datcat/DC-1247"/>
      <owl:versionInfo>http://www.isocat.org/datcat/DC-1247</owl:versionInfo>
      <rdfs:comment>
                            Case that expresses that the referent of the noun it marks receives the benefit of the situation expressed by the clause.
                                (SIL; http://www.isocat.org/datcat/DC-1247)
                            </rdfs:comment>
      <rdfs:label>benefactive case</rdfs:label>
      <rdfs:subClassOf>
         <owl:Class rdf:about="#case"/>
      </rdfs:subClassOf>
      <owl:versionInfo>subClassOf case (dcif:conceptualDomain)</owl:versionInfo>
   </owl:Class>
   <owl:Class rdf:ID="bound">
      <dcr:datcat rdf:resource="http://www.isocat.org/datcat/DC-1933"/>
      <owl:versionInfo>http://www.isocat.org/datcat/DC-1933</owl:versionInfo>
      <rdfs:comment>
                            Linked to a particular element.
                                (http://www.isocat.org/datcat/DC-1933)
                            </rdfs:comment>
      <rdfs:label>bound</rdfs:label>
      <rdfs:subClassOf>
         <owl:Class rdf:about="#cliticness"/>
      </rdfs:subClassOf>
      <owl:versionInfo>subClassOf cliticness (dcif:conceptualDomain)</owl:versionInfo>
   </owl:Class>
   <owl:Class rdf:ID="brokenPlural">
      <dcr:datcat rdf:resource="http://www.isocat.org/datcat/DC-2218"/>
      <owl:versionInfo>http://www.isocat.org/datcat/DC-2218</owl:versionInfo>
      <rdfs:comment>
                            Internal plural that do not have any inflection.
                                (http://www.isocat.org/datcat/DC-2218)
                            </rdfs:comment>
      <rdfs:label>broken plural</rdfs:label>
      <rdfs:subClassOf>
         <owl:Class rdf:about="#plural"/>
      </rdfs:subClassOf>
      <owl:versionInfo>subClassOf plural (dcif:isA)</owl:versionInfo>
   </owl:Class>
   <owl:Class rdf:ID="bullet">
      <dcr:datcat rdf:resource="http://www.isocat.org/datcat/DC-1438"/>
      <owl:versionInfo>http://www.isocat.org/datcat/DC-1438</owl:versionInfo>
      <rdfs:comment>
                            Sign used to mark an item in a list.
                                (http://www.isocat.org/datcat/DC-1438)
                            </rdfs:comment>
      <rdfs:label>bullet</rdfs:label>
      <rdfs:subClassOf>
         <owl:Class rdf:about="#partOfSpeech"/>
      </rdfs:subClassOf>
      <owl:versionInfo>subClassOf partOfSpeech (dcif:conceptualDomain)</owl:versionInfo>
   </owl:Class>
   <owl:Class rdf:ID="case">
      <dcr:datcat rdf:resource="http://www.isocat.org/datcat/DC-1840"/>
      <owl:versionInfo>http://www.isocat.org/datcat/DC-1840</owl:versionInfo>
      <rdfs:comment>
                            In a given sentence, the way in which the form of a word changes in order to express a relationship with one or several words of the sentence. The morphological modification may apply to nouns, pronouns noun phrase constituents, such as adjectives or numerals.
                                (http://www.isocat.org/datcat/DC-1840)
                            </rdfs:comment>
      <rdfs:label>case</rdfs:label>
   </owl:Class>
   <owl:Class rdf:ID="causativeCase">
      <dcr:datcat rdf:resource="http://www.isocat.org/datcat/DC-1253"/>
      <owl:versionInfo>http://www.isocat.org/datcat/DC-1253</owl:versionInfo>
      <rdfs:comment>
                            Case which expresses that the referent of the noun it marks is the cause of the situation expressed by the clause.
                                (SIL; http://www.isocat.org/datcat/DC-1253)
                            </rdfs:comment>
      <rdfs:label>causative case</rdfs:label>
      <rdfs:subClassOf>
         <owl:Class rdf:about="#case"/>
      </rdfs:subClassOf>
      <owl:versionInfo>subClassOf case (dcif:conceptualDomain)</owl:versionInfo>
   </owl:Class>
   <owl:Class rdf:ID="cessative">
      <dcr:datcat rdf:resource="http://www.isocat.org/datcat/DC-2001"/>
      <owl:versionInfo>http://www.isocat.org/datcat/DC-2001</owl:versionInfo>
      <rdfs:comment>
                            Aspect that expresses the cessation of an event or state.
                                (SIL; http://www.isocat.org/datcat/DC-2001)
                            </rdfs:comment>
      <rdfs:label>accomplished</rdfs:label>
      <rdfs:label>cessative</rdfs:label>
      <rdfs:subClassOf>
         <owl:Class rdf:about="#aspect"/>
      </rdfs:subClassOf>
      <owl:versionInfo>subClassOf aspect (dcif:conceptualDomain)</owl:versionInfo>
   </owl:Class>
   <owl:Class rdf:ID="characterCoding">
      <dcr:datcat rdf:resource="http://www.isocat.org/datcat/DC-2089"/>
      <owl:versionInfo>http://www.isocat.org/datcat/DC-2089</owl:versionInfo>
      <rdfs:comment>
                            Designation of the standard used to code the characters.
                                (http://www.isocat.org/datcat/DC-2089)
                            </rdfs:comment>
      <rdfs:label>character coding</rdfs:label>
   </owl:Class>
   <owl:Class rdf:ID="circumposition">
      <dcr:datcat rdf:resource="http://www.isocat.org/datcat/DC-1906"/>
      <owl:versionInfo>http://www.isocat.org/datcat/DC-1906</owl:versionInfo>
      <rdfs:comment>
                            Adposition which consists of two parts which are positioned ahead and after the adpositional foci.
                                (Academic grammar of new Persian 2005; http://www.isocat.org/datcat/DC-1906)
                            </rdfs:comment>
      <rdfs:label>circumposition</rdfs:label>
      <rdfs:subClassOf>
         <owl:Class rdf:about="#adposition"/>
      </rdfs:subClassOf>
      <owl:versionInfo>subClassOf adposition (dcif:isA)</owl:versionInfo>
   </owl:Class>
   <owl:Class rdf:ID="classifier">
      <dcr:datcat rdf:resource="http://www.isocat.org/datcat/DC-2345"/>
      <owl:versionInfo>http://www.isocat.org/datcat/DC-2345</owl:versionInfo>
      <rdfs:comment>
                            part of speech related to a noun to express the sub-classes to which a noun belongs.
                                (http://www.isocat.org/datcat/DC-2345)
                            </rdfs:comment>
      <rdfs:label>classifier</rdfs:label>
   </owl:Class>
   <owl:Class rdf:ID="cliticness">
      <dcr:datcat rdf:resource="http://www.isocat.org/datcat/DC-1903"/>
      <owl:versionInfo>http://www.isocat.org/datcat/DC-1903</owl:versionInfo>
      <rdfs:comment>
                            Categorization of the different types of clitics
                                (MultText-East; http://www.isocat.org/datcat/DC-1903)
                            </rdfs:comment>
      <rdfs:label>cliticness</rdfs:label>
   </owl:Class>
   <owl:Class rdf:ID="closeBracket">
      <dcr:datcat rdf:resource="http://www.isocat.org/datcat/DC-2083"/>
      <owl:versionInfo>http://www.isocat.org/datcat/DC-2083</owl:versionInfo>
      <rdfs:comment>
                            Punctuation that is graphically represented by ]
                                (http://www.isocat.org/datcat/DC-2083)
                            </rdfs:comment>
      <rdfs:label>close bracket</rdfs:label>
   </owl:Class>
   <owl:Class rdf:ID="closeCurlyBracket">
      <dcr:datcat rdf:resource="http://www.isocat.org/datcat/DC-2085"/>
      <owl:versionInfo>http://www.isocat.org/datcat/DC-2085</owl:versionInfo>
      <rdfs:comment>
                            Punctuation that is graphically represented by }
                                (http://www.isocat.org/datcat/DC-2085)
                            </rdfs:comment>
      <rdfs:label>close curly bracket</rdfs:label>
   </owl:Class>
   <owl:Class rdf:ID="closeParenthesis">
      <dcr:datcat rdf:resource="http://www.isocat.org/datcat/DC-1440"/>
      <owl:versionInfo>http://www.isocat.org/datcat/DC-1440</owl:versionInfo>
      <rdfs:comment>
                            End of a parenthesis pair.
                                (http://www.isocat.org/datcat/DC-1440)
                            </rdfs:comment>
      <rdfs:label>close parenthesis</rdfs:label>
      <rdfs:subClassOf>
         <owl:Class rdf:about="#partOfSpeech"/>
      </rdfs:subClassOf>
      <owl:versionInfo>subClassOf partOfSpeech (dcif:conceptualDomain)</owl:versionInfo>
   </owl:Class>
   <owl:Class rdf:ID="closePunctuation">
      <dcr:datcat rdf:resource="http://www.isocat.org/datcat/DC-2079"/>
      <owl:versionInfo>http://www.isocat.org/datcat/DC-2079</owl:versionInfo>
      <rdfs:comment>
                            End of a paired punctuation.
                                (http://www.isocat.org/datcat/DC-2079)
                            </rdfs:comment>
      <rdfs:label>close punctuation</rdfs:label>
      <rdfs:subClassOf>
         <owl:Class rdf:about="#punctuation"/>
      </rdfs:subClassOf>
      <owl:versionInfo>subClassOf punctuation (dcif:isA)</owl:versionInfo>
   </owl:Class>
   <owl:Class rdf:ID="coding">
      <dcr:datcat rdf:resource="http://www.isocat.org/datcat/DC-2242"/>
      <owl:versionInfo>http://www.isocat.org/datcat/DC-2242</owl:versionInfo>
      <rdfs:comment>
                            system of marking so that data can be understood
                                (http://www.isocat.org/datcat/DC-2242)
                            </rdfs:comment>
      <rdfs:label>coding</rdfs:label>
   </owl:Class>
   <owl:Class rdf:ID="collective">
      <dcr:datcat rdf:resource="http://www.isocat.org/datcat/DC-1254"/>
      <owl:versionInfo>http://www.isocat.org/datcat/DC-1254</owl:versionInfo>
      <rdfs:comment>
                            A collective number is a number referring to 'a set of things'. Languages that have this feature can use it to get a phrase like 'flock of sheeps' by using 'sheep' in collective number.
                                (en2.wikipedia.org/wiki/Collective_number; http://www.isocat.org/datcat/DC-1254)
                            </rdfs:comment>
      <rdfs:label>collective</rdfs:label>
      <rdfs:subClassOf>
         <owl:Class rdf:about="#grammaticalNumber"/>
      </rdfs:subClassOf>
      <owl:versionInfo>subClassOf grammaticalNumber (dcif:conceptualDomain)</owl:versionInfo>
   </owl:Class>
   <owl:Class rdf:ID="colon">
      <dcr:datcat rdf:resource="http://www.isocat.org/datcat/DC-1439"/>
      <owl:versionInfo>http://www.isocat.org/datcat/DC-1439</owl:versionInfo>
      <rdfs:comment>
                            Sign with two vertical points that is used in writing and printing to introduce an explanation, example or quotation.
                                (Gil Francopoulo; http://www.isocat.org/datcat/DC-1439)
                            </rdfs:comment>
      <rdfs:label>colon</rdfs:label>
      <rdfs:subClassOf>
         <owl:Class rdf:about="#partOfSpeech"/>
      </rdfs:subClassOf>
      <owl:versionInfo>subClassOf partOfSpeech (dcif:conceptualDomain)</owl:versionInfo>
   </owl:Class>
   <owl:Class rdf:ID="comitativeCase">
      <dcr:datcat rdf:resource="http://www.isocat.org/datcat/DC-1255"/>
      <owl:versionInfo>http://www.isocat.org/datcat/DC-1255</owl:versionInfo>
      <rdfs:comment>
                            Case which expresses a meaning similar to 'along with' or 'accompagnied by'.
                                (Crystal 2003; http://www.isocat.org/datcat/DC-1255)
                            </rdfs:comment>
      <rdfs:label>comitative case</rdfs:label>
      <rdfs:subClassOf>
         <owl:Class rdf:about="#case"/>
      </rdfs:subClassOf>
      <owl:versionInfo>subClassOf case (dcif:conceptualDomain)</owl:versionInfo>
   </owl:Class>
   <owl:Class rdf:ID="comma">
      <dcr:datcat rdf:resource="http://www.isocat.org/datcat/DC-1448"/>
      <owl:versionInfo>http://www.isocat.org/datcat/DC-1448</owl:versionInfo>
      <rdfs:comment>
                            Mark (,) used in writing to show a short pause or to separate items in a list.
                                (Longman DCE 2005; http://www.isocat.org/datcat/DC-1448)
                            </rdfs:comment>
      <rdfs:label>comma</rdfs:label>
      <rdfs:subClassOf>
         <owl:Class rdf:about="#partOfSpeech"/>
      </rdfs:subClassOf>
      <owl:versionInfo>subClassOf partOfSpeech (dcif:conceptualDomain)</owl:versionInfo>
   </owl:Class>
   <owl:Class rdf:ID="comment">
      <dcr:datcat rdf:resource="http://www.isocat.org/datcat/DC-1846"/>
      <owl:versionInfo>http://www.isocat.org/datcat/DC-1846</owl:versionInfo>
      <rdfs:comment>
                            Textual content about an element
                                (http://www.isocat.org/datcat/DC-1846)
                            </rdfs:comment>
      <rdfs:label>comment</rdfs:label>
   </owl:Class>
   <owl:Class rdf:ID="commonGender">
      <dcr:datcat rdf:resource="http://www.isocat.org/datcat/DC-1558"/>
      <owl:versionInfo>http://www.isocat.org/datcat/DC-1558</owl:versionInfo>
      <rdfs:comment>
                            Indistinguished gender for epicenes.
                                (Gil Francopoulo; http://www.isocat.org/datcat/DC-1558)
                            </rdfs:comment>
      <rdfs:label>common gender</rdfs:label>
      <rdfs:subClassOf>
         <owl:Class rdf:about="#grammaticalGender"/>
      </rdfs:subClassOf>
      <owl:versionInfo>subClassOf grammaticalGender (dcif:conceptualDomain)</owl:versionInfo>
   </owl:Class>
   <owl:Class rdf:ID="commonNoun">
      <dcr:datcat rdf:resource="http://www.isocat.org/datcat/DC-1256"/>
      <owl:versionInfo>http://www.isocat.org/datcat/DC-1256</owl:versionInfo>
      <rdfs:comment>
                            Noun that signifies a non-specific member of a group.
                                (www.sil.org/linguistics/GlossaryOfLinguisticTerms/WhatIsACommonNoun.htm; http://www.isocat.org/datcat/DC-1256)
                            </rdfs:comment>
      <rdfs:label>common noun</rdfs:label>
      <rdfs:subClassOf>
         <owl:Class rdf:about="#noun"/>
      </rdfs:subClassOf>
      <owl:versionInfo>subClassOf noun (dcif:isA)</owl:versionInfo>
   </owl:Class>
   <owl:Class rdf:ID="commonlyUsed">
      <dcr:datcat rdf:resource="http://www.isocat.org/datcat/DC-1984"/>
      <owl:versionInfo>http://www.isocat.org/datcat/DC-1984</owl:versionInfo>
      <rdfs:comment>
                            Said of a term that appears frequently.
                                (ISO12620; http://www.isocat.org/datcat/DC-1984)
                            </rdfs:comment>
      <rdfs:label>commonly used</rdfs:label>
      <rdfs:subClassOf>
         <owl:Class rdf:about="#frequency"/>
      </rdfs:subClassOf>
      <owl:versionInfo>subClassOf frequency (dcif:conceptualDomain)</owl:versionInfo>
   </owl:Class>
   <owl:Class rdf:ID="comparative">
      <dcr:datcat rdf:resource="http://www.isocat.org/datcat/DC-1421"/>
      <owl:versionInfo>http://www.isocat.org/datcat/DC-1421</owl:versionInfo>
      <rdfs:comment>
                            Comparative is the comparison where only two entites are involved.
                                (http://www.isocat.org/datcat/DC-1421)
                            </rdfs:comment>
      <rdfs:label>comparative</rdfs:label>
      <rdfs:subClassOf>
         <owl:Class rdf:about="#degree"/>
      </rdfs:subClassOf>
      <owl:versionInfo>subClassOf degree (dcif:conceptualDomain)</owl:versionInfo>
   </owl:Class>
   <owl:Class rdf:ID="comparativeParticle">
      <dcr:datcat rdf:resource="http://www.isocat.org/datcat/DC-1922"/>
      <owl:versionInfo>http://www.isocat.org/datcat/DC-1922</owl:versionInfo>
      <rdfs:comment>
                            Particle used to compare.
                                (http://www.isocat.org/datcat/DC-1922)
                            </rdfs:comment>
      <rdfs:label>comparative particle</rdfs:label>
      <rdfs:subClassOf>
         <owl:Class rdf:about="#particle"/>
      </rdfs:subClassOf>
      <owl:versionInfo>subClassOf particle (dcif:isA)</owl:versionInfo>
   </owl:Class>
   <owl:Class rdf:ID="componentRank">
      <dcr:datcat rdf:resource="http://www.isocat.org/datcat/DC-2185"/>
      <owl:versionInfo>http://www.isocat.org/datcat/DC-2185</owl:versionInfo>
      <rdfs:comment>
                            Rank of a component
                                (http://www.isocat.org/datcat/DC-2185)
                            </rdfs:comment>
      <rdfs:label>component rank</rdfs:label>
   </owl:Class>
   <owl:Class rdf:ID="compoundPreposition">
      <dcr:datcat rdf:resource="http://www.isocat.org/datcat/DC-1934"/>
      <owl:versionInfo>http://www.isocat.org/datcat/DC-1934</owl:versionInfo>
      <rdfs:comment>
                            Preposition that is a aggregation of words
                                (http://www.isocat.org/datcat/DC-1934)
                            </rdfs:comment>
      <rdfs:label>compound preposition</rdfs:label>
      <rdfs:subClassOf>
         <owl:Class rdf:about="#preposition"/>
      </rdfs:subClassOf>
      <owl:versionInfo>subClassOf preposition (dcif:isA)</owl:versionInfo>
   </owl:Class>
   <owl:Class rdf:ID="conditional">
      <dcr:datcat rdf:resource="http://www.isocat.org/datcat/DC-1258"/>
      <owl:versionInfo>http://www.isocat.org/datcat/DC-1258</owl:versionInfo>
      <rdfs:comment>
                            A conditional relation is a logical relation in which the illocutionary act employing one of a pair of propositions is expressed or implied to be true or in force if the other proposition is true.
                                (www.sil.org/linguistics/GlossaryOfLinguisticTerms/WhatIsAConditionalRelation.htm; http://www.isocat.org/datcat/DC-1258)
                            </rdfs:comment>
      <rdfs:label>conditional</rdfs:label>
      <rdfs:subClassOf>
         <owl:Class rdf:about="#verbFormMood"/>
      </rdfs:subClassOf>
      <owl:versionInfo>subClassOf verbFormMood (dcif:conceptualDomain)</owl:versionInfo>
   </owl:Class>
   <owl:Class rdf:ID="conditionalParticle">
      <dcr:datcat rdf:resource="http://www.isocat.org/datcat/DC-2230"/>
      <owl:versionInfo>http://www.isocat.org/datcat/DC-2230</owl:versionInfo>
      <rdfs:comment>
                            conditional particule
                                (MIRACL &amp; LSCA; http://www.isocat.org/datcat/DC-2230)
                            </rdfs:comment>
      <rdfs:label>conditional particule</rdfs:label>
      <rdfs:subClassOf>
         <owl:Class rdf:about="#particle"/>
      </rdfs:subClassOf>
      <owl:versionInfo>subClassOf particle (dcif:isA)</owl:versionInfo>
   </owl:Class>
   <owl:Class rdf:ID="conditionalPronoun">
      <dcr:datcat rdf:resource="http://www.isocat.org/datcat/DC-2222"/>
      <owl:versionInfo>http://www.isocat.org/datcat/DC-2222</owl:versionInfo>
      <rdfs:comment>
                            conditional pronoun
                                (MIRACL &amp; LSCA; http://www.isocat.org/datcat/DC-2222)
                            </rdfs:comment>
      <rdfs:label>conditional pronoun</rdfs:label>
      <rdfs:subClassOf>
         <owl:Class rdf:about="#pronoun"/>
      </rdfs:subClassOf>
      <owl:versionInfo>subClassOf pronoun (dcif:isA)</owl:versionInfo>
   </owl:Class>
   <owl:Class rdf:ID="conjugated">
      <dcr:datcat rdf:resource="http://www.isocat.org/datcat/DC-2207"/>
      <owl:versionInfo>http://www.isocat.org/datcat/DC-2207</owl:versionInfo>
      <rdfs:comment>
                            Property of a verbal form when inflected
                                (http://www.isocat.org/datcat/DC-2207)
                            </rdfs:comment>
      <rdfs:label>conjugated</rdfs:label>
   </owl:Class>
   <owl:Class rdf:ID="conjunction">
      <dcr:datcat rdf:resource="http://www.isocat.org/datcat/DC-1260"/>
      <owl:versionInfo>http://www.isocat.org/datcat/DC-1260</owl:versionInfo>
      <rdfs:comment>
                            Word that syntactically links words or constituents, and expresses a semantic relationship between them.
                                (www.sil.org/linguistics/GlossaryOfLinguisticTerms/WhatIsAConjunction.htm; http://www.isocat.org/datcat/DC-1260)
                            </rdfs:comment>
      <rdfs:label>conjunction</rdfs:label>
      <rdfs:subClassOf>
         <owl:Class rdf:about="#partOfSpeech"/>
      </rdfs:subClassOf>
      <owl:versionInfo>subClassOf partOfSpeech (dcif:conceptualDomain)</owl:versionInfo>
   </owl:Class>
   <owl:Class rdf:ID="contextualVariation">
      <dcr:datcat rdf:resource="http://www.isocat.org/datcat/DC-1977"/>
      <owl:versionInfo>http://www.isocat.org/datcat/DC-1977</owl:versionInfo>
      <rdfs:comment>
                            Variation on a particular usage or immediate proximity of words.
                                (Gil Francopoulo; http://www.isocat.org/datcat/DC-1977)
                            </rdfs:comment>
      <rdfs:label>contextual variation</rdfs:label>
   </owl:Class>
   <owl:Class rdf:ID="coordinatingConjunction">
      <dcr:datcat rdf:resource="http://www.isocat.org/datcat/DC-1262"/>
      <owl:versionInfo>http://www.isocat.org/datcat/DC-1262</owl:versionInfo>
      <rdfs:comment>
                            Conjunction that links constituents.
                                (www.sil.org/linguistics/GlossaryOfLinguisticTerms/WhatIsACoordinatingConjunction.htm; http://www.isocat.org/datcat/DC-1262)
                            </rdfs:comment>
      <rdfs:label>coordinating conjunction</rdfs:label>
      <rdfs:subClassOf>
         <owl:Class rdf:about="#conjunction"/>
      </rdfs:subClassOf>
      <owl:versionInfo>subClassOf conjunction (dcif:isA)</owl:versionInfo>
   </owl:Class>
   <owl:Class rdf:ID="coordinationParticle">
      <dcr:datcat rdf:resource="http://www.isocat.org/datcat/DC-2227"/>
      <owl:versionInfo>http://www.isocat.org/datcat/DC-2227</owl:versionInfo>
      <rdfs:comment>
                            particle for coordination
                                (MIRACL &amp; LSCA; http://www.isocat.org/datcat/DC-2227)
                            </rdfs:comment>
      <rdfs:label>coordination particle</rdfs:label>
      <rdfs:subClassOf>
         <owl:Class rdf:about="#particle"/>
      </rdfs:subClassOf>
      <owl:versionInfo>subClassOf particle (dcif:isA)</owl:versionInfo>
   </owl:Class>
   <owl:Class rdf:ID="copula">
      <dcr:datcat rdf:resource="http://www.isocat.org/datcat/DC-1263"/>
      <owl:versionInfo>http://www.isocat.org/datcat/DC-1263</owl:versionInfo>
      <rdfs:comment>
                            Special word that combines the subject of a sentence and its description.
                                (www.sf.airnet.ne.jp/~ts/japanese/copula.html; http://www.isocat.org/datcat/DC-1263)
                            </rdfs:comment>
      <rdfs:label>copula</rdfs:label>
      <rdfs:subClassOf>
         <owl:Class rdf:about="#verb"/>
      </rdfs:subClassOf>
      <owl:versionInfo>subClassOf verb (dcif:isA)</owl:versionInfo>
   </owl:Class>
   <owl:Class rdf:ID="copy">
      <dcr:datcat rdf:resource="http://www.isocat.org/datcat/DC-1835"/>
      <owl:versionInfo>http://www.isocat.org/datcat/DC-1835</owl:versionInfo>
      <rdfs:comment>
                            Operation that duplicates N characters from position X at position Y
                                (http://www.isocat.org/datcat/DC-1835)
                            </rdfs:comment>
      <rdfs:label>copy</rdfs:label>
   </owl:Class>
   <owl:Class rdf:ID="countableNoun">
      <dcr:datcat rdf:resource="http://www.isocat.org/datcat/DC-2276"/>
      <owl:versionInfo>http://www.isocat.org/datcat/DC-2276</owl:versionInfo>
      <rdfs:comment>
                            noun referring to one or several concepts that may be counted
                                (http://www.isocat.org/datcat/DC-2276)
                            </rdfs:comment>
      <rdfs:label>countable noun</rdfs:label>
      <rdfs:subClassOf>
         <owl:Class rdf:about="#noun"/>
      </rdfs:subClassOf>
      <owl:versionInfo>subClassOf noun (dcif:isA)</owl:versionInfo>
   </owl:Class>
   <owl:Class rdf:ID="countryCoding">
      <dcr:datcat rdf:resource="http://www.isocat.org/datcat/DC-2092"/>
      <owl:versionInfo>http://www.isocat.org/datcat/DC-2092</owl:versionInfo>
      <rdfs:comment>
                            Designation of the standard used to code the country.
                                (http://www.isocat.org/datcat/DC-2092)
                            </rdfs:comment>
      <rdfs:label>country coding</rdfs:label>
   </owl:Class>
   <owl:Class rdf:ID="creationDate">
      <dcr:datcat rdf:resource="http://www.isocat.org/datcat/DC-2251"/>
      <owl:versionInfo>http://www.isocat.org/datcat/DC-2251</owl:versionInfo>
      <rdfs:comment>
                            date of creation
                                (http://www.isocat.org/datcat/DC-2251)
                            </rdfs:comment>
      <rdfs:label>creation date</rdfs:label>
   </owl:Class>
   <owl:Class rdf:ID="dateCoding">
      <dcr:datcat rdf:resource="http://www.isocat.org/datcat/DC-2090"/>
      <owl:versionInfo>http://www.isocat.org/datcat/DC-2090</owl:versionInfo>
      <rdfs:comment>
                            Designation of the standard used to code the dates.
                                (http://www.isocat.org/datcat/DC-2090)
                            </rdfs:comment>
      <rdfs:label>date coding</rdfs:label>
   </owl:Class>
   <owl:Class rdf:ID="dating">
      <dcr:datcat rdf:resource="http://www.isocat.org/datcat/DC-1959"/>
      <owl:versionInfo>http://www.isocat.org/datcat/DC-1959</owl:versionInfo>
      <rdfs:comment>
                            Indication specifying whether the usage is old or modern.
                                (http://www.isocat.org/datcat/DC-1959)
                            </rdfs:comment>
      <rdfs:label>dating</rdfs:label>
   </owl:Class>
   <owl:Class rdf:ID="dativeCase">
      <dcr:datcat rdf:resource="http://www.isocat.org/datcat/DC-1265"/>
      <owl:versionInfo>http://www.isocat.org/datcat/DC-1265</owl:versionInfo>
      <rdfs:comment>
                            Case that expresses an indirect object relationship or a range of meaning similar to that covered by 'to' or 'for' in English; but there is a great deal of variation between languages in the way this case is used.
                                (Crystal 2003; http://www.isocat.org/datcat/DC-1265)
                            </rdfs:comment>
      <rdfs:label>dative case</rdfs:label>
      <rdfs:subClassOf>
         <owl:Class rdf:about="#case"/>
      </rdfs:subClassOf>
      <owl:versionInfo>subClassOf case (dcif:conceptualDomain)</owl:versionInfo>
   </owl:Class>
   <owl:Class rdf:ID="definite">
      <dcr:datcat rdf:resource="http://www.isocat.org/datcat/DC-2004"/>
      <owl:versionInfo>http://www.isocat.org/datcat/DC-2004</owl:versionInfo>
      <rdfs:comment>
                            Value referring to the capacity of identification of an entity.
                                (http://www.isocat.org/datcat/DC-2004)
                            </rdfs:comment>
      <rdfs:label>definite</rdfs:label>
      <rdfs:subClassOf>
         <owl:Class rdf:about="#definiteness"/>
      </rdfs:subClassOf>
      <owl:versionInfo>subClassOf definiteness (dcif:conceptualDomain)</owl:versionInfo>
   </owl:Class>
   <owl:Class rdf:ID="definiteArticle">
      <dcr:datcat rdf:resource="http://www.isocat.org/datcat/DC-1430"/>
      <owl:versionInfo>http://www.isocat.org/datcat/DC-1430</owl:versionInfo>
      <rdfs:comment>
                            Article that allows the reference to a specific, identifiable entity (or class of entities).
                                (Crytal 2003; http://www.isocat.org/datcat/DC-1430)
                            </rdfs:comment>
      <rdfs:label>definite article</rdfs:label>
      <rdfs:subClassOf>
         <owl:Class rdf:about="#partOfSpeech"/>
      </rdfs:subClassOf>
      <owl:versionInfo>subClassOf partOfSpeech (dcif:conceptualDomain)</owl:versionInfo>
   </owl:Class>
   <owl:Class rdf:ID="definiteness">
      <dcr:datcat rdf:resource="http://www.isocat.org/datcat/DC-1926"/>
      <owl:versionInfo>http://www.isocat.org/datcat/DC-1926</owl:versionInfo>
      <rdfs:comment>
                            Property about the possiblity to identify an entity.
                                (http://www.isocat.org/datcat/DC-1926)
                            </rdfs:comment>
      <rdfs:label>definiteness</rdfs:label>
   </owl:Class>
   <owl:Class rdf:ID="definition">
      <dcr:datcat rdf:resource="http://www.isocat.org/datcat/DC-1972"/>
      <owl:versionInfo>http://www.isocat.org/datcat/DC-1972</owl:versionInfo>
      <rdfs:comment>
                            Representation of a concept by a descriptive statement which serves to differentiate it from related concepts.
                                (http://www.isocat.org/datcat/DC-1972)
                            </rdfs:comment>
      <rdfs:label>definition</rdfs:label>
   </owl:Class>
   <owl:Class rdf:ID="degree">
      <dcr:datcat rdf:resource="http://www.isocat.org/datcat/DC-1419"/>
      <owl:versionInfo>http://www.isocat.org/datcat/DC-1419</owl:versionInfo>
      <rdfs:comment>
                            Property concerning comparison.
                                (http://www.isocat.org/datcat/DC-1419)
                            </rdfs:comment>
      <rdfs:label>degree</rdfs:label>
   </owl:Class>
   <owl:Class rdf:ID="delativeCase">
      <dcr:datcat rdf:resource="http://www.isocat.org/datcat/DC-1268"/>
      <owl:versionInfo>http://www.isocat.org/datcat/DC-1268</owl:versionInfo>
      <rdfs:comment>
                            Case which expresses motion downward from the referent of the noun it marks.
                                (SIL; http://www.isocat.org/datcat/DC-1268)
                            </rdfs:comment>
      <rdfs:label>delative case</rdfs:label>
      <rdfs:subClassOf>
         <owl:Class rdf:about="#case"/>
      </rdfs:subClassOf>
      <owl:versionInfo>subClassOf case (dcif:conceptualDomain)</owl:versionInfo>
   </owl:Class>
   <owl:Class rdf:ID="demonstrativeDeterminer">
      <dcr:datcat rdf:resource="http://www.isocat.org/datcat/DC-1269"/>
      <owl:versionInfo>http://www.isocat.org/datcat/DC-1269</owl:versionInfo>
      <rdfs:comment>
                            Determiner used to point to an entity in the situation or elsewhere in a sentence.
                                (Crystal 2003; http://www.isocat.org/datcat/DC-1269)
                            </rdfs:comment>
      <rdfs:label>demonstrative determiner</rdfs:label>
      <rdfs:subClassOf>
         <owl:Class rdf:about="#determiner"/>
      </rdfs:subClassOf>
      <owl:versionInfo>subClassOf determiner (dcif:isA)</owl:versionInfo>
   </owl:Class>
   <owl:Class rdf:ID="demonstrativePronoun">
      <dcr:datcat rdf:resource="http://www.isocat.org/datcat/DC-1270"/>
      <owl:versionInfo>http://www.isocat.org/datcat/DC-1270</owl:versionInfo>
      <rdfs:comment>
                            Pronoun used to point to an entity in the situation or elsewhere in a sentence.
                                (Crystal 2003; http://www.isocat.org/datcat/DC-1270)
                            </rdfs:comment>
      <rdfs:label>demonstrative pronoun</rdfs:label>
      <rdfs:subClassOf>
         <owl:Class rdf:about="#pronoun"/>
      </rdfs:subClassOf>
      <owl:versionInfo>subClassOf pronoun (dcif:isA)</owl:versionInfo>
   </owl:Class>
   <owl:Class rdf:ID="derivation">
      <dcr:datcat rdf:resource="http://www.isocat.org/datcat/DC-1271"/>
      <owl:versionInfo>http://www.isocat.org/datcat/DC-1271</owl:versionInfo>
      <rdfs:comment>
                            Change in the form of a linguistic unit, usually modification in the base/root or affixation to create a new word.
                                (Sue Ellen Wright + Gil Francopoulo; http://www.isocat.org/datcat/DC-1271)
                            </rdfs:comment>
      <rdfs:label>derivation</rdfs:label>
   </owl:Class>
   <owl:Class rdf:ID="determiner">
      <dcr:datcat rdf:resource="http://www.isocat.org/datcat/DC-1272"/>
      <owl:versionInfo>http://www.isocat.org/datcat/DC-1272</owl:versionInfo>
      <rdfs:comment>
                            Word or affix that belongs to a class of noun modifiers that expresses the reference, including quantity, of a noun.
                                (www.sil.org/linguistics/GlossaryOfLinguisticTerms/WhatIsADeterminer.htm; http://www.isocat.org/datcat/DC-1272)
                            </rdfs:comment>
      <rdfs:label>determiner</rdfs:label>
      <rdfs:subClassOf>
         <owl:Class rdf:about="#partOfSpeech"/>
      </rdfs:subClassOf>
      <owl:versionInfo>subClassOf partOfSpeech (dcif:conceptualDomain)</owl:versionInfo>
   </owl:Class>
   <owl:Class rdf:ID="dialectRegister">
      <dcr:datcat rdf:resource="http://www.isocat.org/datcat/DC-1990"/>
      <owl:versionInfo>http://www.isocat.org/datcat/DC-1990</owl:versionInfo>
      <rdfs:comment>
                            Register that is specific to a dialect.
                                (http://www.isocat.org/datcat/DC-1990)
                            </rdfs:comment>
      <rdfs:label>dialect register</rdfs:label>
      <rdfs:subClassOf>
         <owl:Class rdf:about="#register"/>
      </rdfs:subClassOf>
      <owl:versionInfo>subClassOf register (dcif:conceptualDomain)</owl:versionInfo>
   </owl:Class>
   <owl:Class rdf:ID="diminutiveNoun">
      <dcr:datcat rdf:resource="http://www.isocat.org/datcat/DC-2225"/>
      <owl:versionInfo>http://www.isocat.org/datcat/DC-2225</owl:versionInfo>
      <rdfs:comment>
                            diminutive noun
                                (MIRACL LSCA; http://www.isocat.org/datcat/DC-2225)
                            </rdfs:comment>
      <rdfs:label>diminutive noun</rdfs:label>
      <rdfs:subClassOf>
         <owl:Class rdf:about="#noun"/>
      </rdfs:subClassOf>
      <owl:versionInfo>subClassOf noun (dcif:isA)</owl:versionInfo>
   </owl:Class>
   <owl:Class rdf:ID="direction">
      <dcr:datcat rdf:resource="http://www.isocat.org/datcat/DC-2238"/>
      <owl:versionInfo>http://www.isocat.org/datcat/DC-2238</owl:versionInfo>
      <rdfs:comment>
                            general way in which something changes or develops
                                (Gil Francopoulo; http://www.isocat.org/datcat/DC-2238)
                            </rdfs:comment>
      <rdfs:label>direction</rdfs:label>
   </owl:Class>
   <owl:Class rdf:ID="distinctiveParticle">
      <dcr:datcat rdf:resource="http://www.isocat.org/datcat/DC-2228"/>
      <owl:versionInfo>http://www.isocat.org/datcat/DC-2228</owl:versionInfo>
      <rdfs:comment>
                            distinctive particle
                                (MIRACL &amp; LSCA; http://www.isocat.org/datcat/DC-2228)
                            </rdfs:comment>
      <rdfs:label>distinctive particle</rdfs:label>
      <rdfs:subClassOf>
         <owl:Class rdf:about="#particle"/>
      </rdfs:subClassOf>
      <owl:versionInfo>subClassOf particle (dcif:isA)</owl:versionInfo>
   </owl:Class>
   <owl:Class rdf:ID="domain">
      <dcr:datcat rdf:resource="http://www.isocat.org/datcat/DC-2212"/>
      <owl:versionInfo>http://www.isocat.org/datcat/DC-2212</owl:versionInfo>
      <rdfs:comment>
                            area of activity, interest, or knowledge
                                (http://www.isocat.org/datcat/DC-2212)
                            </rdfs:comment>
      <rdfs:label>domain</rdfs:label>
   </owl:Class>
   <owl:Class rdf:ID="dual">
      <dcr:datcat rdf:resource="http://www.isocat.org/datcat/DC-1879"/>
      <owl:versionInfo>http://www.isocat.org/datcat/DC-1879</owl:versionInfo>
      <rdfs:comment>
                            Form used in some languages to designate two persons or things.
                                (ISO12620; http://www.isocat.org/datcat/DC-1879)
                            </rdfs:comment>
      <rdfs:label>dual</rdfs:label>
      <rdfs:subClassOf>
         <owl:Class rdf:about="#grammaticalNumber"/>
      </rdfs:subClassOf>
      <owl:versionInfo>subClassOf grammaticalNumber (dcif:conceptualDomain)</owl:versionInfo>
   </owl:Class>
   <owl:Class rdf:ID="elativeCase">
      <dcr:datcat rdf:resource="http://www.isocat.org/datcat/DC-1276"/>
      <owl:versionInfo>http://www.isocat.org/datcat/DC-1276</owl:versionInfo>
      <rdfs:comment>
                            Case which expresses the meaning of motion 'away from' from the referent of the noun it marks.
                                (Crystal 2003; http://www.isocat.org/datcat/DC-1276)
                            </rdfs:comment>
      <rdfs:label>elative case</rdfs:label>
      <rdfs:subClassOf>
         <owl:Class rdf:about="#case"/>
      </rdfs:subClassOf>
      <owl:versionInfo>subClassOf case (dcif:conceptualDomain)</owl:versionInfo>
   </owl:Class>
   <owl:Class rdf:ID="elision">
      <dcr:datcat rdf:resource="http://www.isocat.org/datcat/DC-1277"/>
      <owl:versionInfo>http://www.isocat.org/datcat/DC-1277</owl:versionInfo>
      <rdfs:comment>
                            The omission of a syllable or vowel at the beginning or end of a word, esp. when a word ending with a vowel is next to one beginning with a vowel.
                                (www.wordreference.com/English/definition.asp?en=elision; http://www.isocat.org/datcat/DC-1277)
                            </rdfs:comment>
      <rdfs:label>elision</rdfs:label>
   </owl:Class>
   <owl:Class rdf:ID="emphaticPronoun">
      <dcr:datcat rdf:resource="http://www.isocat.org/datcat/DC-1941"/>
      <owl:versionInfo>http://www.isocat.org/datcat/DC-1941</owl:versionInfo>
      <rdfs:comment>
                            Pronoun marked to show its importance.
                                (http://www.isocat.org/datcat/DC-1941)
                            </rdfs:comment>
      <rdfs:label>emphatic pronoun</rdfs:label>
      <rdfs:subClassOf>
         <owl:Class rdf:about="#pronoun"/>
      </rdfs:subClassOf>
      <owl:versionInfo>subClassOf pronoun (dcif:isA)</owl:versionInfo>
   </owl:Class>
   <owl:Class rdf:ID="equativeCase">
      <dcr:datcat rdf:resource="http://www.isocat.org/datcat/DC-1279"/>
      <owl:versionInfo>http://www.isocat.org/datcat/DC-1279</owl:versionInfo>
      <rdfs:comment>
                            Case that expresses likeness or identity to the referent of the noun it marks. It can have meaning, such as: 'as', 'like', or 'in the capacity of'.
                                (SIL; http://www.isocat.org/datcat/DC-1279)
                            </rdfs:comment>
      <rdfs:label>equative case</rdfs:label>
      <rdfs:subClassOf>
         <owl:Class rdf:about="#case"/>
      </rdfs:subClassOf>
      <owl:versionInfo>subClassOf case (dcif:conceptualDomain)</owl:versionInfo>
   </owl:Class>
   <owl:Class rdf:ID="ergativeCase">
      <dcr:datcat rdf:resource="http://www.isocat.org/datcat/DC-1280"/>
      <owl:versionInfo>http://www.isocat.org/datcat/DC-1280</owl:versionInfo>
      <rdfs:comment>
                            Case assigned to the subject of a transitive verb as opposed to absolutive case.
                                (www.wikipedia.org/wiki/Ergative_case; http://www.isocat.org/datcat/DC-1280)
                            </rdfs:comment>
      <rdfs:label>ergative case</rdfs:label>
      <rdfs:subClassOf>
         <owl:Class rdf:about="#case"/>
      </rdfs:subClassOf>
      <owl:versionInfo>subClassOf case (dcif:conceptualDomain)</owl:versionInfo>
   </owl:Class>
   <owl:Class rdf:ID="essiveCase">
      <dcr:datcat rdf:resource="http://www.isocat.org/datcat/DC-1281"/>
      <owl:versionInfo>http://www.isocat.org/datcat/DC-1281</owl:versionInfo>
      <rdfs:comment>
                            Case which expresses a state of being.
                                (Crystal 2003; http://www.isocat.org/datcat/DC-1281)
                            </rdfs:comment>
      <rdfs:label>essive case</rdfs:label>
      <rdfs:subClassOf>
         <owl:Class rdf:about="#case"/>
      </rdfs:subClassOf>
      <owl:versionInfo>subClassOf case (dcif:conceptualDomain)</owl:versionInfo>
   </owl:Class>
   <owl:Class rdf:ID="etymologicalRoot">
      <dcr:datcat rdf:resource="http://www.isocat.org/datcat/DC-1987"/>
      <owl:versionInfo>http://www.isocat.org/datcat/DC-1987</owl:versionInfo>
      <rdfs:comment>
                            Morpheme that has a particular status with regards to the word's etymology.
                                (http://www.isocat.org/datcat/DC-1987)
                            </rdfs:comment>
      <rdfs:label>etymological root</rdfs:label>
   </owl:Class>
   <owl:Class rdf:ID="exact">
      <dcr:datcat rdf:resource="http://www.isocat.org/datcat/DC-2205"/>
      <owl:versionInfo>http://www.isocat.org/datcat/DC-2205</owl:versionInfo>
      <rdfs:comment>
                            Completely correct in every detail
                                (http://www.isocat.org/datcat/DC-2205)
                            </rdfs:comment>
      <rdfs:label>exact</rdfs:label>
   </owl:Class>
   <owl:Class rdf:ID="example">
      <dcr:datcat rdf:resource="http://www.isocat.org/datcat/DC-1958"/>
      <owl:versionInfo>http://www.isocat.org/datcat/DC-1958</owl:versionInfo>
      <rdfs:comment>
                            Descriptive material that provides a sample of an object or entity defined in the entry.
                                (ISO12620; http://www.isocat.org/datcat/DC-1958)
                            </rdfs:comment>
      <rdfs:label>example</rdfs:label>
   </owl:Class>
   <owl:Class rdf:ID="exclamativeDeterminer">
      <dcr:datcat rdf:resource="http://www.isocat.org/datcat/DC-1284"/>
      <owl:versionInfo>http://www.isocat.org/datcat/DC-1284</owl:versionInfo>
      <rdfs:comment>
                            Determiner expressing an emotional utterance and marked with a strong intonation.
                                (Crystal 2003; http://www.isocat.org/datcat/DC-1284)
                            </rdfs:comment>
      <rdfs:label>exclamative determiner</rdfs:label>
      <rdfs:subClassOf>
         <owl:Class rdf:about="#determiner"/>
      </rdfs:subClassOf>
      <owl:versionInfo>subClassOf determiner (dcif:isA)</owl:versionInfo>
   </owl:Class>
   <owl:Class rdf:ID="exclamativePoint">
      <dcr:datcat rdf:resource="http://www.isocat.org/datcat/DC-1441"/>
      <owl:versionInfo>http://www.isocat.org/datcat/DC-1441</owl:versionInfo>
      <rdfs:comment>
                            Special sign (!) usually used in writing to mark exclamation.
                                (http://www.isocat.org/datcat/DC-1441)
                            </rdfs:comment>
      <rdfs:label>exclamative point</rdfs:label>
      <rdfs:subClassOf>
         <owl:Class rdf:about="#partOfSpeech"/>
      </rdfs:subClassOf>
      <owl:versionInfo>subClassOf partOfSpeech (dcif:conceptualDomain)</owl:versionInfo>
   </owl:Class>
   <owl:Class rdf:ID="exclamativePronoun">
      <dcr:datcat rdf:resource="http://www.isocat.org/datcat/DC-1285"/>
      <owl:versionInfo>http://www.isocat.org/datcat/DC-1285</owl:versionInfo>
      <rdfs:comment>
                            Pronoun marked with an emotional utterance and/or a strong intonation.
                                (Crystal 2003; http://www.isocat.org/datcat/DC-1285)
                            </rdfs:comment>
      <rdfs:label>exclamative pronoun</rdfs:label>
      <rdfs:subClassOf>
         <owl:Class rdf:about="#pronoun"/>
      </rdfs:subClassOf>
      <owl:versionInfo>subClassOf pronoun (dcif:isA)</owl:versionInfo>
   </owl:Class>
   <owl:Class rdf:ID="expansionVariation">
      <dcr:datcat rdf:resource="http://www.isocat.org/datcat/DC-1850"/>
      <owl:versionInfo>http://www.isocat.org/datcat/DC-1850</owl:versionInfo>
      <rdfs:comment>
                            Description of the kind of variation between full and abbreviated forms.
                                (http://www.isocat.org/datcat/DC-1850)
                            </rdfs:comment>
      <rdfs:label>expansion variation</rdfs:label>
   </owl:Class>
   <owl:Class rdf:ID="expletive">
      <dcr:datcat rdf:resource="http://www.isocat.org/datcat/DC-1283"/>
      <owl:versionInfo>http://www.isocat.org/datcat/DC-1283</owl:versionInfo>
      <rdfs:comment>
                            Word which serves no grammatical function, but which fills up a sentence or gives emphasis.
                                (www.southwestern.edu/~carlg/Latin_Web/glossary.html; http://www.isocat.org/datcat/DC-1283)
                            </rdfs:comment>
      <rdfs:label>expletive</rdfs:label>
   </owl:Class>
   <owl:Class rdf:ID="externalReference">
      <dcr:datcat rdf:resource="http://www.isocat.org/datcat/DC-1975"/>
      <owl:versionInfo>http://www.isocat.org/datcat/DC-1975</owl:versionInfo>
      <rdfs:comment>
                            Reference to a particular node of an external descriptive system.
                                (LMF; http://www.isocat.org/datcat/DC-1975)
                            </rdfs:comment>
      <rdfs:label>external reference</rdfs:label>
      <rdfs:label>hook</rdfs:label>
   </owl:Class>
   <owl:Class rdf:ID="externalSystem">
      <dcr:datcat rdf:resource="http://www.isocat.org/datcat/DC-1974"/>
      <owl:versionInfo>http://www.isocat.org/datcat/DC-1974</owl:versionInfo>
      <rdfs:comment>
                            Reference to an external descriptive system.
                                (LMF; http://www.isocat.org/datcat/DC-1974)
                            </rdfs:comment>
      <rdfs:label>external system</rdfs:label>
   </owl:Class>
   <owl:Class rdf:ID="facetiousRegister">
      <dcr:datcat rdf:resource="http://www.isocat.org/datcat/DC-1991"/>
      <owl:versionInfo>http://www.isocat.org/datcat/DC-1991</owl:versionInfo>
      <rdfs:comment>
                            Register related to an expression that is intended to be clever and funny but that is really silly and annoying.
                                (Longma DCE; http://www.isocat.org/datcat/DC-1991)
                            </rdfs:comment>
      <rdfs:label>facecious register</rdfs:label>
      <rdfs:subClassOf>
         <owl:Class rdf:about="#register"/>
      </rdfs:subClassOf>
      <owl:versionInfo>subClassOf register (dcif:conceptualDomain)</owl:versionInfo>
   </owl:Class>
   <owl:Class rdf:ID="feminine">
      <dcr:datcat rdf:resource="http://www.isocat.org/datcat/DC-1880"/>
      <owl:versionInfo>http://www.isocat.org/datcat/DC-1880</owl:versionInfo>
      <rdfs:comment>
                            Of, relating to, or constituting the gender that ordinarily includes most words or grammatical forms referring to females.
                                (ISO12620; http://www.isocat.org/datcat/DC-1880)
                            </rdfs:comment>
      <rdfs:label>feminine</rdfs:label>
      <rdfs:subClassOf>
         <owl:Class rdf:about="#grammaticalGender"/>
      </rdfs:subClassOf>
      <owl:versionInfo>subClassOf grammaticalGender (dcif:conceptualDomain)</owl:versionInfo>
      <rdfs:subClassOf>
         <owl:Class rdf:about="#ownerGender"/>
      </rdfs:subClassOf>
      <owl:versionInfo>subClassOf ownerGender (dcif:conceptualDomain)</owl:versionInfo>
   </owl:Class>
   <owl:Class rdf:ID="finite">
      <dcr:datcat rdf:resource="http://www.isocat.org/datcat/DC-1287"/>
      <owl:versionInfo>http://www.isocat.org/datcat/DC-1287</owl:versionInfo>
      <rdfs:comment>
                            Property applied to a verb form that can occur on its own in an independent sentence.
                                (Crystal 2003; http://www.isocat.org/datcat/DC-1287)
                            </rdfs:comment>
      <rdfs:label>finite</rdfs:label>
      <rdfs:subClassOf>
         <owl:Class rdf:about="#finiteness"/>
      </rdfs:subClassOf>
      <owl:versionInfo>subClassOf finiteness (dcif:conceptualDomain)</owl:versionInfo>
   </owl:Class>
   <owl:Class rdf:ID="finiteness">
      <dcr:datcat rdf:resource="http://www.isocat.org/datcat/DC-1893"/>
      <owl:versionInfo>http://www.isocat.org/datcat/DC-1893</owl:versionInfo>
      <rdfs:comment>
                            Property referring to finite and non-finite status of a verbal form.
                                (http://www.isocat.org/datcat/DC-1893)
                            </rdfs:comment>
      <rdfs:label>finitness</rdfs:label>
   </owl:Class>
   <owl:Class rdf:ID="firstPerson">
      <dcr:datcat rdf:resource="http://www.isocat.org/datcat/DC-1288"/>
      <owl:versionInfo>http://www.isocat.org/datcat/DC-1288</owl:versionInfo>
      <rdfs:comment>
                            First person deixis is deictic reference that refers to the speaker, or both the speaker and referents grouped with the speaker
                                (www.sil.org/linguistics/GlossaryOfLinguisticTerms/WhatIsFirstPersonDeixis.htm; http://www.isocat.org/datcat/DC-1288)
                            </rdfs:comment>
      <rdfs:label>first person</rdfs:label>
      <rdfs:subClassOf>
         <owl:Class rdf:about="#ownerPerson"/>
      </rdfs:subClassOf>
      <owl:versionInfo>subClassOf ownerPerson (dcif:conceptualDomain)</owl:versionInfo>
      <rdfs:subClassOf>
         <owl:Class rdf:about="#person"/>
      </rdfs:subClassOf>
      <owl:versionInfo>subClassOf person (dcif:conceptualDomain)</owl:versionInfo>
   </owl:Class>
   <owl:Class rdf:ID="foreignText">
      <dcr:datcat rdf:resource="http://www.isocat.org/datcat/DC-1423"/>
      <owl:versionInfo>http://www.isocat.org/datcat/DC-1423</owl:versionInfo>
      <rdfs:comment>
                            Markup used to identify a word, phrase, or extended text as belonging to some language other than that of the surrounding text.
                                (ISO12620; http://www.isocat.org/datcat/DC-1423)
                            </rdfs:comment>
      <rdfs:label>foreign text</rdfs:label>
   </owl:Class>
   <owl:Class rdf:ID="formalRegister">
      <dcr:datcat rdf:resource="http://www.isocat.org/datcat/DC-1992"/>
      <owl:versionInfo>http://www.isocat.org/datcat/DC-1992</owl:versionInfo>
      <rdfs:comment>
                            Formal register.
                                (12620; http://www.isocat.org/datcat/DC-1992)
                            </rdfs:comment>
      <rdfs:label>formal register</rdfs:label>
      <rdfs:subClassOf>
         <owl:Class rdf:about="#register"/>
      </rdfs:subClassOf>
      <owl:versionInfo>subClassOf register (dcif:conceptualDomain)</owl:versionInfo>
   </owl:Class>
   <owl:Class rdf:ID="formula">
      <dcr:datcat rdf:resource="http://www.isocat.org/datcat/DC-1888"/>
      <owl:versionInfo>http://www.isocat.org/datcat/DC-1888</owl:versionInfo>
      <rdfs:comment>
                            Figures, symbols or the like used to express a concept briefly, such as a mathematical or chemical formula.
                                (ISO12620; http://www.isocat.org/datcat/DC-1888)
                            </rdfs:comment>
      <rdfs:label>formula</rdfs:label>
   </owl:Class>
   <owl:Class rdf:ID="frequency">
      <dcr:datcat rdf:resource="http://www.isocat.org/datcat/DC-1965"/>
      <owl:versionInfo>http://www.isocat.org/datcat/DC-1965</owl:versionInfo>
      <rdfs:comment>
                            The relative commonness with which a term occurs.
                                (ISO12620; http://www.isocat.org/datcat/DC-1965)
                            </rdfs:comment>
      <rdfs:label>frequency</rdfs:label>
   </owl:Class>
   <owl:Class rdf:ID="fullArticle">
      <dcr:datcat rdf:resource="http://www.isocat.org/datcat/DC-1928"/>
      <owl:versionInfo>http://www.isocat.org/datcat/DC-1928</owl:versionInfo>
      <rdfs:comment>
                            For definiteness, when a specific form is the syntactic subject of the clause.
                                (DFKI; http://www.isocat.org/datcat/DC-1928)
                            </rdfs:comment>
      <rdfs:label>full article</rdfs:label>
      <rdfs:subClassOf>
         <owl:Class rdf:about="#definiteness"/>
      </rdfs:subClassOf>
      <owl:versionInfo>subClassOf definiteness (dcif:conceptualDomain)</owl:versionInfo>
   </owl:Class>
   <owl:Class rdf:ID="fusedPreposition">
      <dcr:datcat rdf:resource="http://www.isocat.org/datcat/DC-1901"/>
      <owl:versionInfo>http://www.isocat.org/datcat/DC-1901</owl:versionInfo>
      <rdfs:comment>
                            Preposition that is the result of a morphological merge from at least two words.
                                (http://www.isocat.org/datcat/DC-1901)
                            </rdfs:comment>
      <rdfs:label>fused preposition</rdfs:label>
      <rdfs:subClassOf>
         <owl:Class rdf:about="#preposition"/>
      </rdfs:subClassOf>
      <owl:versionInfo>subClassOf preposition (dcif:isA)</owl:versionInfo>
   </owl:Class>
   <owl:Class rdf:ID="future">
      <dcr:datcat rdf:resource="http://www.isocat.org/datcat/DC-1291"/>
      <owl:versionInfo>http://www.isocat.org/datcat/DC-1291</owl:versionInfo>
      <rdfs:comment>
                            Verb tense that indicates action or state of being in the future.
                                (www.southwestern.edu/~carlg/Latin_Web/glossary.html; http://www.isocat.org/datcat/DC-1291)
                            </rdfs:comment>
      <rdfs:label>future</rdfs:label>
      <rdfs:subClassOf>
         <owl:Class rdf:about="#grammaticalTense"/>
      </rdfs:subClassOf>
      <owl:versionInfo>subClassOf grammaticalTense (dcif:conceptualDomain)</owl:versionInfo>
   </owl:Class>
   <owl:Class rdf:ID="futureParticle">
      <dcr:datcat rdf:resource="http://www.isocat.org/datcat/DC-1919"/>
      <owl:versionInfo>http://www.isocat.org/datcat/DC-1919</owl:versionInfo>
      <rdfs:comment>
                            Particle used in order to express future.
                                (http://www.isocat.org/datcat/DC-1919)
                            </rdfs:comment>
      <rdfs:label>future particle</rdfs:label>
      <rdfs:subClassOf>
         <owl:Class rdf:about="#particle"/>
      </rdfs:subClassOf>
      <owl:versionInfo>subClassOf particle (dcif:isA)</owl:versionInfo>
   </owl:Class>
   <owl:Class rdf:ID="generalAdverb">
      <dcr:datcat rdf:resource="http://www.isocat.org/datcat/DC-1435"/>
      <owl:versionInfo>http://www.isocat.org/datcat/DC-1435</owl:versionInfo>
      <rdfs:comment>
                            Adverb belonging to the general class of adverbs
                                (http://www.isocat.org/datcat/DC-1435)
                            </rdfs:comment>
      <rdfs:label>general adverb</rdfs:label>
      <rdfs:subClassOf>
         <owl:Class rdf:about="#adverb"/>
      </rdfs:subClassOf>
      <owl:versionInfo>subClassOf adverb (dcif:isA)</owl:versionInfo>
   </owl:Class>
   <owl:Class rdf:ID="genitiveCase">
      <dcr:datcat rdf:resource="http://www.isocat.org/datcat/DC-1293"/>
      <owl:versionInfo>http://www.isocat.org/datcat/DC-1293</owl:versionInfo>
      <rdfs:comment>
                            Case which expresses a possessive relationship (e.g. the boy's book) or some other similarly close connection (e.g. a summer's day).
                                (Crystal 2003; http://www.isocat.org/datcat/DC-1293)
                            </rdfs:comment>
      <rdfs:label>genitive case</rdfs:label>
      <rdfs:label>possessive case</rdfs:label>
      <rdfs:subClassOf>
         <owl:Class rdf:about="#case"/>
      </rdfs:subClassOf>
      <owl:versionInfo>subClassOf case (dcif:conceptualDomain)</owl:versionInfo>
   </owl:Class>
   <owl:Class rdf:ID="geographicalVariant">
      <dcr:datcat rdf:resource="http://www.isocat.org/datcat/DC-1851"/>
      <owl:versionInfo>http://www.isocat.org/datcat/DC-1851</owl:versionInfo>
      <rdfs:comment>
                            Description of a specific form used in a certain region as opposed to another form used in another region
                                (http://www.isocat.org/datcat/DC-1851)
                            </rdfs:comment>
      <rdfs:label>geographical variant</rdfs:label>
   </owl:Class>
   <owl:Class rdf:ID="gerundive">
      <dcr:datcat rdf:resource="http://www.isocat.org/datcat/DC-2243"/>
      <owl:versionInfo>http://www.isocat.org/datcat/DC-2243</owl:versionInfo>
      <rdfs:comment>
                            property for a non-finite form of a verb other than the infinitive.
                                (http://www.isocat.org/datcat/DC-2243)
                            </rdfs:comment>
      <rdfs:label>gerund</rdfs:label>
      <rdfs:label>gerundive</rdfs:label>
      <rdfs:subClassOf>
         <owl:Class rdf:about="#verbFormMood"/>
      </rdfs:subClassOf>
      <owl:versionInfo>subClassOf verbFormMood (dcif:conceptualDomain)</owl:versionInfo>
   </owl:Class>
   <owl:Class rdf:ID="grammaticalGender">
      <dcr:datcat rdf:resource="http://www.isocat.org/datcat/DC-1297"/>
      <owl:versionInfo>http://www.isocat.org/datcat/DC-1297</owl:versionInfo>
      <rdfs:comment>
                            Category based on (depending on languages) the natural distinction between sex and formal criteria.
                                (http://www.isocat.org/datcat/DC-1297)
                            </rdfs:comment>
      <rdfs:comment>
                            the common value is used for the word combines feminine and masculine
                                (http://www.isocat.org/datcat/DC-1297)
                            </rdfs:comment>
      <rdfs:label>grammatical gender</rdfs:label>
   </owl:Class>
   <owl:Class rdf:ID="grammaticalNumber">
      <dcr:datcat rdf:resource="http://www.isocat.org/datcat/DC-1298"/>
      <owl:versionInfo>http://www.isocat.org/datcat/DC-1298</owl:versionInfo>
      <rdfs:comment>
                            Grammatical category for the variation in form of nouns, pronouns, and any words agreeing with them, depending on how many persons or things are referred to.
                                (www.wordreference.com/English/definition.asp?en=number 12; http://www.isocat.org/datcat/DC-1298)
                            </rdfs:comment>
      <rdfs:label>grammatical number</rdfs:label>
   </owl:Class>
   <owl:Class rdf:ID="graphicalOperator">
      <dcr:datcat rdf:resource="http://www.isocat.org/datcat/DC-1860"/>
      <owl:versionInfo>http://www.isocat.org/datcat/DC-1860</owl:versionInfo>
      <rdfs:comment>
                            Description of the modification of a written form
                                (Gil Francopoulo; http://www.isocat.org/datcat/DC-1860)
                            </rdfs:comment>
      <rdfs:label>graphical operator</rdfs:label>
   </owl:Class>
   <owl:Class rdf:ID="graphicalSeparator">
      <dcr:datcat rdf:resource="http://www.isocat.org/datcat/DC-1863"/>
      <owl:versionInfo>http://www.isocat.org/datcat/DC-1863</owl:versionInfo>
      <rdfs:comment>
                            Character string that appears between two written forms
                                (Gil Francopoulo; http://www.isocat.org/datcat/DC-1863)
                            </rdfs:comment>
      <rdfs:label>graphical separator</rdfs:label>
   </owl:Class>
   <owl:Class rdf:ID="have">
      <dcr:datcat rdf:resource="http://www.isocat.org/datcat/DC-1299"/>
      <owl:versionInfo>http://www.isocat.org/datcat/DC-1299</owl:versionInfo>
      <rdfs:comment>
                            The verb have as an auxiliary.
                                (www.sil.org/linguistics/GlossaryOfLinguisticTerms/WhatIsAnAuxiliaryVerb.htm; http://www.isocat.org/datcat/DC-1299)
                            </rdfs:comment>
      <rdfs:label>have</rdfs:label>
      <rdfs:subClassOf>
         <owl:Class rdf:about="#partOfSpeech"/>
      </rdfs:subClassOf>
      <owl:versionInfo>subClassOf partOfSpeech (dcif:conceptualDomain)</owl:versionInfo>
   </owl:Class>
   <owl:Class rdf:ID="homograph">
      <dcr:datcat rdf:resource="http://www.isocat.org/datcat/DC-1300"/>
      <owl:versionInfo>http://www.isocat.org/datcat/DC-1300</owl:versionInfo>
      <rdfs:comment>
                            Word that is written like another, but that has a different pronunciation, meaning, and/or origin.
                                (adapted from ISO12620; http://www.isocat.org/datcat/DC-1300)
                            </rdfs:comment>
      <rdfs:label>homograph</rdfs:label>
   </owl:Class>
   <owl:Class rdf:ID="homonym">
      <dcr:datcat rdf:resource="http://www.isocat.org/datcat/DC-1301"/>
      <owl:versionInfo>http://www.isocat.org/datcat/DC-1301</owl:versionInfo>
      <rdfs:comment>
                            Word that sounds the same and is written the same as another word but is different in meaning.
                                (http://www.isocat.org/datcat/DC-1301)
                            </rdfs:comment>
      <rdfs:label>homonym</rdfs:label>
   </owl:Class>
   <owl:Class rdf:ID="homophone">
      <dcr:datcat rdf:resource="http://www.isocat.org/datcat/DC-1302"/>
      <owl:versionInfo>http://www.isocat.org/datcat/DC-1302</owl:versionInfo>
      <rdfs:comment>
                            Word that sounds like another word, but is different in writiing or meaning.
                                (http://www.isocat.org/datcat/DC-1302)
                            </rdfs:comment>
      <rdfs:label>homophone</rdfs:label>
   </owl:Class>
   <owl:Class rdf:ID="honorific">
      <dcr:datcat rdf:resource="http://www.isocat.org/datcat/DC-2347"/>
      <owl:versionInfo>http://www.isocat.org/datcat/DC-2347</owl:versionInfo>
      <rdfs:comment>
                            special form of language used when talking about those in positions of social situation
                                (http://www.isocat.org/datcat/DC-2347)
                            </rdfs:comment>
      <rdfs:label>honorific</rdfs:label>
   </owl:Class>
   <owl:Class rdf:ID="hyphen">
      <dcr:datcat rdf:resource="http://www.isocat.org/datcat/DC-2077"/>
      <owl:versionInfo>http://www.isocat.org/datcat/DC-2077</owl:versionInfo>
      <rdfs:comment>
                            Punctuation that is graphically presented as "-".
                                (http://www.isocat.org/datcat/DC-2077)
                            </rdfs:comment>
      <rdfs:label>hyphen</rdfs:label>
   </owl:Class>
   <owl:Class rdf:ID="id">
      <dcr:datcat rdf:resource="http://www.isocat.org/datcat/DC-1845"/>
      <owl:versionInfo>http://www.isocat.org/datcat/DC-1845</owl:versionInfo>
      <rdfs:comment>
                            Identification of an element
                                (http://www.isocat.org/datcat/DC-1845)
                            </rdfs:comment>
      <rdfs:label>identifier</rdfs:label>
      <rdfs:label>id</rdfs:label>
   </owl:Class>
   <owl:Class rdf:ID="illativeCase">
      <dcr:datcat rdf:resource="http://www.isocat.org/datcat/DC-1303"/>
      <owl:versionInfo>http://www.isocat.org/datcat/DC-1303</owl:versionInfo>
      <rdfs:comment>
                            Case which expresses the meaning of 'motion into' or 'direction towards' the referent of the noun it marks.
                                (Crystal 2003; http://www.isocat.org/datcat/DC-1303)
                            </rdfs:comment>
      <rdfs:label>illative case</rdfs:label>
      <rdfs:subClassOf>
         <owl:Class rdf:about="#case"/>
      </rdfs:subClassOf>
      <owl:versionInfo>subClassOf case (dcif:conceptualDomain)</owl:versionInfo>
   </owl:Class>
   <owl:Class rdf:ID="image">
      <dcr:datcat rdf:resource="http://www.isocat.org/datcat/DC-2249"/>
      <owl:versionInfo>http://www.isocat.org/datcat/DC-2249</owl:versionInfo>
      <rdfs:comment>
                            graphical representation
                                (http://www.isocat.org/datcat/DC-2249)
                            </rdfs:comment>
      <rdfs:label>image</rdfs:label>
   </owl:Class>
   <owl:Class rdf:ID="imperative">
      <dcr:datcat rdf:resource="http://www.isocat.org/datcat/DC-1844"/>
      <owl:versionInfo>http://www.isocat.org/datcat/DC-1844</owl:versionInfo>
      <rdfs:comment>
                            Mood used to express an order.
                                (http://www.isocat.org/datcat/DC-1844)
                            </rdfs:comment>
      <rdfs:label>imperative</rdfs:label>
      <rdfs:subClassOf>
         <owl:Class rdf:about="#verbFormMood"/>
      </rdfs:subClassOf>
      <owl:versionInfo>subClassOf verbFormMood (dcif:conceptualDomain)</owl:versionInfo>
   </owl:Class>
   <owl:Class rdf:ID="imperfect">
      <dcr:datcat rdf:resource="http://www.isocat.org/datcat/DC-1304"/>
      <owl:versionInfo>http://www.isocat.org/datcat/DC-1304</owl:versionInfo>
      <rdfs:comment>
                            Verb tense that refers to action in the past that is incomplete or ongoing.
                                (www.southwestern.edu/~carlg/Latin_Web/glossary.html; http://www.isocat.org/datcat/DC-1304)
                            </rdfs:comment>
      <rdfs:label>imperfect</rdfs:label>
      <rdfs:subClassOf>
         <owl:Class rdf:about="#grammaticalTense"/>
      </rdfs:subClassOf>
      <owl:versionInfo>subClassOf grammaticalTense (dcif:conceptualDomain)</owl:versionInfo>
   </owl:Class>
   <owl:Class rdf:ID="imperfective">
      <dcr:datcat rdf:resource="http://www.isocat.org/datcat/DC-1305"/>
      <owl:versionInfo>http://www.isocat.org/datcat/DC-1305</owl:versionInfo>
      <rdfs:comment>
                            Imperfective aspect is an aspect that expresses an event or state, with respect to its internal structure, instead of expressing it as a simple whole.
                                (www.sil.org/linguistics/GlossaryOfLinguisticTerms/WhatIsImperfectiveAspect.htm; http://www.isocat.org/datcat/DC-1305)
                            </rdfs:comment>
      <rdfs:label>imperfective</rdfs:label>
      <rdfs:subClassOf>
         <owl:Class rdf:about="#aspect"/>
      </rdfs:subClassOf>
      <owl:versionInfo>subClassOf aspect (dcif:conceptualDomain)</owl:versionInfo>
   </owl:Class>
   <owl:Class rdf:ID="impersonalPronoun">
      <dcr:datcat rdf:resource="http://www.isocat.org/datcat/DC-1426"/>
      <owl:versionInfo>http://www.isocat.org/datcat/DC-1426</owl:versionInfo>
      <rdfs:comment>
                            Pronoun lacking person referent.
                                (Gil Francopoulo; http://www.isocat.org/datcat/DC-1426)
                            </rdfs:comment>
      <rdfs:label>impersonal pronoun</rdfs:label>
      <rdfs:subClassOf>
         <owl:Class rdf:about="#pronoun"/>
      </rdfs:subClassOf>
      <owl:versionInfo>subClassOf pronoun (dcif:isA)</owl:versionInfo>
   </owl:Class>
   <owl:Class rdf:ID="impossible">
      <dcr:datcat rdf:resource="http://www.isocat.org/datcat/DC-1866"/>
      <owl:versionInfo>http://www.isocat.org/datcat/DC-1866</owl:versionInfo>
      <rdfs:comment>
                            to denote something that cannot be considered as being correct in a given language
                                (Gil Francopoulo; http://www.isocat.org/datcat/DC-1866)
                            </rdfs:comment>
      <rdfs:label>impossible</rdfs:label>
   </owl:Class>
   <owl:Class rdf:ID="inHouseRegister">
      <dcr:datcat rdf:resource="http://www.isocat.org/datcat/DC-1993"/>
      <owl:versionInfo>http://www.isocat.org/datcat/DC-1993</owl:versionInfo>
      <rdfs:comment>
                            Register of terms that are company-specific and not readily recognized outside this environment.
                                (ISO12620; http://www.isocat.org/datcat/DC-1993)
                            </rdfs:comment>
      <rdfs:label>in house register</rdfs:label>
      <rdfs:subClassOf>
         <owl:Class rdf:about="#register"/>
      </rdfs:subClassOf>
      <owl:versionInfo>subClassOf register (dcif:conceptualDomain)</owl:versionInfo>
   </owl:Class>
   <owl:Class rdf:ID="inanimate">
      <dcr:datcat rdf:resource="http://www.isocat.org/datcat/DC-1952"/>
      <owl:versionInfo>http://www.isocat.org/datcat/DC-1952</owl:versionInfo>
      <rdfs:comment>
                            Perceived as not living.
                                (ISO12620; http://www.isocat.org/datcat/DC-1952)
                            </rdfs:comment>
      <rdfs:label>inanimate</rdfs:label>
      <rdfs:subClassOf>
         <owl:Class rdf:about="#animacy"/>
      </rdfs:subClassOf>
      <owl:versionInfo>subClassOf animacy (dcif:conceptualDomain)</owl:versionInfo>
   </owl:Class>
   <owl:Class rdf:ID="indefiniteArticle">
      <dcr:datcat rdf:resource="http://www.isocat.org/datcat/DC-1308"/>
      <owl:versionInfo>http://www.isocat.org/datcat/DC-1308</owl:versionInfo>
      <rdfs:comment>
                            Article not capable of expressing identification.
                                (Gil Francopoulo; http://www.isocat.org/datcat/DC-1308)
                            </rdfs:comment>
      <rdfs:label>indefinite article</rdfs:label>
      <rdfs:subClassOf>
         <owl:Class rdf:about="#partOfSpeech"/>
      </rdfs:subClassOf>
      <owl:versionInfo>subClassOf partOfSpeech (dcif:conceptualDomain)</owl:versionInfo>
   </owl:Class>
   <owl:Class rdf:ID="indefiniteDeterminer">
      <dcr:datcat rdf:resource="http://www.isocat.org/datcat/DC-1307"/>
      <owl:versionInfo>http://www.isocat.org/datcat/DC-1307</owl:versionInfo>
      <rdfs:comment>
                            Determiner not capable of identification.
                                (Gil Francopoulo; http://www.isocat.org/datcat/DC-1307)
                            </rdfs:comment>
      <rdfs:label>indefinite determiner</rdfs:label>
      <rdfs:subClassOf>
         <owl:Class rdf:about="#determiner"/>
      </rdfs:subClassOf>
      <owl:versionInfo>subClassOf determiner (dcif:isA)</owl:versionInfo>
   </owl:Class>
   <owl:Class rdf:ID="indefinitePronoun">
      <dcr:datcat rdf:resource="http://www.isocat.org/datcat/DC-1309"/>
      <owl:versionInfo>http://www.isocat.org/datcat/DC-1309</owl:versionInfo>
      <rdfs:comment>
                            Pronoun that does not allow reference.
                                (Gil Francopoulo; http://www.isocat.org/datcat/DC-1309)
                            </rdfs:comment>
      <rdfs:label>indefinite pronoun</rdfs:label>
      <rdfs:subClassOf>
         <owl:Class rdf:about="#pronoun"/>
      </rdfs:subClassOf>
      <owl:versionInfo>subClassOf pronoun (dcif:isA)</owl:versionInfo>
   </owl:Class>
   <owl:Class rdf:ID="indicative">
      <dcr:datcat rdf:resource="http://www.isocat.org/datcat/DC-1885"/>
      <owl:versionInfo>http://www.isocat.org/datcat/DC-1885</owl:versionInfo>
      <rdfs:comment>
                            Mood value used in the expression of statements and questions.
                                (Crystal 2003; http://www.isocat.org/datcat/DC-1885)
                            </rdfs:comment>
      <rdfs:label>indicative</rdfs:label>
      <rdfs:subClassOf>
         <owl:Class rdf:about="#verbFormMood"/>
      </rdfs:subClassOf>
      <owl:versionInfo>subClassOf verbFormMood (dcif:conceptualDomain)</owl:versionInfo>
   </owl:Class>
   <owl:Class rdf:ID="indifferent">
      <dcr:datcat rdf:resource="http://www.isocat.org/datcat/DC-1944"/>
      <owl:versionInfo>http://www.isocat.org/datcat/DC-1944</owl:versionInfo>
      <rdfs:comment>
                            Markup to express that there is not any pertinence.
                                (http://www.isocat.org/datcat/DC-1944)
                            </rdfs:comment>
      <rdfs:label>indifferent</rdfs:label>
      <rdfs:subClassOf>
         <owl:Class rdf:about="#modificationType"/>
      </rdfs:subClassOf>
      <owl:versionInfo>subClassOf modificationType (dcif:conceptualDomain)</owl:versionInfo>
   </owl:Class>
   <owl:Class rdf:ID="inessiveCase">
      <dcr:datcat rdf:resource="http://www.isocat.org/datcat/DC-1311"/>
      <owl:versionInfo>http://www.isocat.org/datcat/DC-1311</owl:versionInfo>
      <rdfs:comment>
                            Case which expresses the meaning of location or position within a place.
                                (Crystal 2003; http://www.isocat.org/datcat/DC-1311)
                            </rdfs:comment>
      <rdfs:label>inessive case</rdfs:label>
      <rdfs:subClassOf>
         <owl:Class rdf:about="#case"/>
      </rdfs:subClassOf>
      <owl:versionInfo>subClassOf case (dcif:conceptualDomain)</owl:versionInfo>
   </owl:Class>
   <owl:Class rdf:ID="infinitive">
      <dcr:datcat rdf:resource="http://www.isocat.org/datcat/DC-1312"/>
      <owl:versionInfo>http://www.isocat.org/datcat/DC-1312</owl:versionInfo>
      <rdfs:comment>
                            Mood cited as unmarked or base form.
                                (Crystal 2003; http://www.isocat.org/datcat/DC-1312)
                            </rdfs:comment>
      <rdfs:label>infinitive</rdfs:label>
      <rdfs:subClassOf>
         <owl:Class rdf:about="#verbFormMood"/>
      </rdfs:subClassOf>
      <owl:versionInfo>subClassOf verbFormMood (dcif:conceptualDomain)</owl:versionInfo>
   </owl:Class>
   <owl:Class rdf:ID="infinitiveParticle">
      <dcr:datcat rdf:resource="http://www.isocat.org/datcat/DC-1896"/>
      <owl:versionInfo>http://www.isocat.org/datcat/DC-1896</owl:versionInfo>
      <rdfs:comment>
                            Particle used to express infinitive.
                                (http://www.isocat.org/datcat/DC-1896)
                            </rdfs:comment>
      <rdfs:label>infinitive particle</rdfs:label>
      <rdfs:subClassOf>
         <owl:Class rdf:about="#particle"/>
      </rdfs:subClassOf>
      <owl:versionInfo>subClassOf particle (dcif:isA)</owl:versionInfo>
   </owl:Class>
   <owl:Class rdf:ID="infix">
      <dcr:datcat rdf:resource="http://www.isocat.org/datcat/DC-1313"/>
      <owl:versionInfo>http://www.isocat.org/datcat/DC-1313</owl:versionInfo>
      <rdfs:comment>
                            Affix inserted in the middle of a word to change its meaning or part of speech value.
                                (Sue Ellen Wright; http://www.isocat.org/datcat/DC-1313)
                            </rdfs:comment>
      <rdfs:label>infix</rdfs:label>
   </owl:Class>
   <owl:Class rdf:ID="infrequentlyUsed">
      <dcr:datcat rdf:resource="http://www.isocat.org/datcat/DC-1985"/>
      <owl:versionInfo>http://www.isocat.org/datcat/DC-1985</owl:versionInfo>
      <rdfs:comment>
                            Said of a term that does not appear frequently.
                                (ISO12620; http://www.isocat.org/datcat/DC-1985)
                            </rdfs:comment>
      <rdfs:label>infrequently used</rdfs:label>
      <rdfs:subClassOf>
         <owl:Class rdf:about="#frequency"/>
      </rdfs:subClassOf>
      <owl:versionInfo>subClassOf frequency (dcif:conceptualDomain)</owl:versionInfo>
   </owl:Class>
   <owl:Class rdf:ID="instrumentalCase">
      <dcr:datcat rdf:resource="http://www.isocat.org/datcat/DC-1316"/>
      <owl:versionInfo>http://www.isocat.org/datcat/DC-1316</owl:versionInfo>
      <rdfs:comment>
                            Case indicating that the referent of the noun it marks is the means of the accomplishment of the action expressed by the clause.
                                (SIL; http://www.isocat.org/datcat/DC-1316)
                            </rdfs:comment>
      <rdfs:label>instrumental case</rdfs:label>
      <rdfs:subClassOf>
         <owl:Class rdf:about="#case"/>
      </rdfs:subClassOf>
      <owl:versionInfo>subClassOf case (dcif:conceptualDomain)</owl:versionInfo>
   </owl:Class>
   <owl:Class rdf:ID="intensity">
      <dcr:datcat rdf:resource="http://www.isocat.org/datcat/DC-2197"/>
      <owl:versionInfo>http://www.isocat.org/datcat/DC-2197</owl:versionInfo>
      <rdfs:comment>
                            Quality of being felt very strongly or having a strong effect
                                (http://www.isocat.org/datcat/DC-2197)
                            </rdfs:comment>
      <rdfs:label>intensity</rdfs:label>
   </owl:Class>
   <owl:Class rdf:ID="interjection">
      <dcr:datcat rdf:resource="http://www.isocat.org/datcat/DC-1318"/>
      <owl:versionInfo>http://www.isocat.org/datcat/DC-1318</owl:versionInfo>
      <rdfs:comment>
                            Word or sound that expresses an emotion.
                                (www.southwestern.edu/~carlg/Latin_Web/glossary.html; http://www.isocat.org/datcat/DC-1318)
                            </rdfs:comment>
      <rdfs:label>interjection</rdfs:label>
      <rdfs:subClassOf>
         <owl:Class rdf:about="#partOfSpeech"/>
      </rdfs:subClassOf>
      <owl:versionInfo>subClassOf partOfSpeech (dcif:conceptualDomain)</owl:versionInfo>
   </owl:Class>
   <owl:Class rdf:ID="interrogativeDeterminer">
      <dcr:datcat rdf:resource="http://www.isocat.org/datcat/DC-1320"/>
      <owl:versionInfo>http://www.isocat.org/datcat/DC-1320</owl:versionInfo>
      <rdfs:comment>
                            Determiner used to express a question.
                                (http://www.isocat.org/datcat/DC-1320)
                            </rdfs:comment>
      <rdfs:label>interrogative determiner</rdfs:label>
      <rdfs:subClassOf>
         <owl:Class rdf:about="#determiner"/>
      </rdfs:subClassOf>
      <owl:versionInfo>subClassOf determiner (dcif:isA)</owl:versionInfo>
   </owl:Class>
   <owl:Class rdf:ID="interrogativeParticle">
      <dcr:datcat rdf:resource="http://www.isocat.org/datcat/DC-1921"/>
      <owl:versionInfo>http://www.isocat.org/datcat/DC-1921</owl:versionInfo>
      <rdfs:comment>
                            Particle used to express a question.
                                (http://www.isocat.org/datcat/DC-1921)
                            </rdfs:comment>
      <rdfs:label>interrogative particle</rdfs:label>
      <rdfs:subClassOf>
         <owl:Class rdf:about="#particle"/>
      </rdfs:subClassOf>
      <owl:versionInfo>subClassOf particle (dcif:isA)</owl:versionInfo>
   </owl:Class>
   <owl:Class rdf:ID="interrogativePronoun">
      <dcr:datcat rdf:resource="http://www.isocat.org/datcat/DC-1321"/>
      <owl:versionInfo>http://www.isocat.org/datcat/DC-1321</owl:versionInfo>
      <rdfs:comment>
                            Pronoun used to express a question.
                                (http://www.isocat.org/datcat/DC-1321)
                            </rdfs:comment>
      <rdfs:label>interrogative pronoun</rdfs:label>
      <rdfs:subClassOf>
         <owl:Class rdf:about="#pronoun"/>
      </rdfs:subClassOf>
      <owl:versionInfo>subClassOf pronoun (dcif:isA)</owl:versionInfo>
   </owl:Class>
   <owl:Class rdf:ID="interrogativePunctuation">
      <dcr:datcat rdf:resource="http://www.isocat.org/datcat/DC-2087"/>
      <owl:versionInfo>http://www.isocat.org/datcat/DC-2087</owl:versionInfo>
      <rdfs:comment>
                            Punctuation used when the sentence is interrogative.
                                (http://www.isocat.org/datcat/DC-2087)
                            </rdfs:comment>
      <rdfs:label>interrogative punctuation</rdfs:label>
   </owl:Class>
   <owl:Class rdf:ID="invertedComma">
      <dcr:datcat rdf:resource="http://www.isocat.org/datcat/DC-1443"/>
      <owl:versionInfo>http://www.isocat.org/datcat/DC-1443</owl:versionInfo>
      <rdfs:comment>
                            Inverted comma.
                                (http://www.isocat.org/datcat/DC-1443)
                            </rdfs:comment>
      <rdfs:label>inverted comma</rdfs:label>
      <rdfs:subClassOf>
         <owl:Class rdf:about="#partOfSpeech"/>
      </rdfs:subClassOf>
      <owl:versionInfo>subClassOf partOfSpeech (dcif:conceptualDomain)</owl:versionInfo>
   </owl:Class>
   <owl:Class rdf:ID="invertedQuestionMark">
      <dcr:datcat rdf:resource="http://www.isocat.org/datcat/DC-2088"/>
      <owl:versionInfo>http://www.isocat.org/datcat/DC-2088</owl:versionInfo>
      <rdfs:comment>
                            Punctuation used in certain languages at the beginning of an interrogative sentence.
                                (http://www.isocat.org/datcat/DC-2088)
                            </rdfs:comment>
      <rdfs:label>inverted question mark</rdfs:label>
      <rdfs:label>inverted interrogative point</rdfs:label>
   </owl:Class>
   <owl:Class rdf:ID="ironicRegister">
      <dcr:datcat rdf:resource="http://www.isocat.org/datcat/DC-1994"/>
      <owl:versionInfo>http://www.isocat.org/datcat/DC-1994</owl:versionInfo>
      <rdfs:comment>
                            Register for irony.
                                (12620; http://www.isocat.org/datcat/DC-1994)
                            </rdfs:comment>
      <rdfs:label>ironic register</rdfs:label>
      <rdfs:subClassOf>
         <owl:Class rdf:about="#register"/>
      </rdfs:subClassOf>
      <owl:versionInfo>subClassOf register (dcif:conceptualDomain)</owl:versionInfo>
   </owl:Class>
   <owl:Class rdf:ID="label">
      <dcr:datcat rdf:resource="http://www.isocat.org/datcat/DC-1857"/>
      <owl:versionInfo>http://www.isocat.org/datcat/DC-1857</owl:versionInfo>
      <rdfs:comment>
                            Text attached to an element
                                (Gil Francopoulo; http://www.isocat.org/datcat/DC-1857)
                            </rdfs:comment>
      <rdfs:label>label</rdfs:label>
   </owl:Class>
   <owl:Class rdf:ID="language">
      <dcr:datcat rdf:resource="http://www.isocat.org/datcat/DC-1969"/>
      <owl:versionInfo>http://www.isocat.org/datcat/DC-1969</owl:versionInfo>
      <rdfs:comment>
                            System of communication by written or spoken words which is used by the people of a particular country or area.
                                (Longman dictionay of contemporary English 2005; http://www.isocat.org/datcat/DC-1969)
                            </rdfs:comment>
      <rdfs:label>language</rdfs:label>
   </owl:Class>
   <owl:Class rdf:ID="languageCoding">
      <dcr:datcat rdf:resource="http://www.isocat.org/datcat/DC-2008"/>
      <owl:versionInfo>http://www.isocat.org/datcat/DC-2008</owl:versionInfo>
      <rdfs:comment>
                            Designation of the standard used to code the name of the languages.
                                (http://www.isocat.org/datcat/DC-2008)
                            </rdfs:comment>
      <rdfs:label>language code</rdfs:label>
   </owl:Class>
   <owl:Class rdf:ID="lativeCase">
      <dcr:datcat rdf:resource="http://www.isocat.org/datcat/DC-1323"/>
      <owl:versionInfo>http://www.isocat.org/datcat/DC-1323</owl:versionInfo>
      <rdfs:comment>
                            Case which expresses motion to a location.
                                (http://en.wikipedia.org/wiki/Lative_case; http://www.isocat.org/datcat/DC-1323)
                            </rdfs:comment>
      <rdfs:label>lative case</rdfs:label>
      <rdfs:subClassOf>
         <owl:Class rdf:about="#case"/>
      </rdfs:subClassOf>
      <owl:versionInfo>subClassOf case (dcif:conceptualDomain)</owl:versionInfo>
   </owl:Class>
   <owl:Class rdf:ID="leftEnvironment">
      <dcr:datcat rdf:resource="http://www.isocat.org/datcat/DC-2194"/>
      <owl:versionInfo>http://www.isocat.org/datcat/DC-2194</owl:versionInfo>
      <rdfs:comment>
                            Left side from a specific point
                                (http://www.isocat.org/datcat/DC-2194)
                            </rdfs:comment>
      <rdfs:label>left environment</rdfs:label>
   </owl:Class>
   <owl:Class rdf:ID="lemma">
      <dcr:datcat rdf:resource="http://www.isocat.org/datcat/DC-1324"/>
      <owl:versionInfo>http://www.isocat.org/datcat/DC-1324</owl:versionInfo>
      <rdfs:comment>
                            Base form a word or term that is used as the formal entry in a dictionary.
                                (ISO12620A-020803 Sue Ellen Wright + Francopoulo; http://www.isocat.org/datcat/DC-1324)
                            </rdfs:comment>
      <rdfs:label>lemma</rdfs:label>
   </owl:Class>
   <owl:Class rdf:ID="letter">
      <dcr:datcat rdf:resource="http://www.isocat.org/datcat/DC-1889"/>
      <owl:versionInfo>http://www.isocat.org/datcat/DC-1889</owl:versionInfo>
      <rdfs:comment>
                            Letter.
                                (http://www.isocat.org/datcat/DC-1889)
                            </rdfs:comment>
      <rdfs:label>letter</rdfs:label>
   </owl:Class>
   <owl:Class rdf:ID="lexeme">
      <dcr:datcat rdf:resource="http://www.isocat.org/datcat/DC-1325"/>
      <owl:versionInfo>http://www.isocat.org/datcat/DC-1325</owl:versionInfo>
      <rdfs:comment>
                            Minimal unit of language which : has a semantic interpretation and embodies a distinct cultural concept.
                                (www.sil.org/linguistics/GlossaryOfLinguisticTerms/WhatIsALexeme.htm; http://www.isocat.org/datcat/DC-1325)
                            </rdfs:comment>
      <rdfs:label>lexeme</rdfs:label>
   </owl:Class>
   <owl:Class rdf:ID="lexicalType">
      <dcr:datcat rdf:resource="http://www.isocat.org/datcat/DC-2175"/>
      <owl:versionInfo>http://www.isocat.org/datcat/DC-2175</owl:versionInfo>
      <rdfs:comment>
                            Type of an entry in a lexicon
                                (http://www.isocat.org/datcat/DC-2175)
                            </rdfs:comment>
      <rdfs:label>lexical type</rdfs:label>
   </owl:Class>
   <owl:Class rdf:ID="location">
      <dcr:datcat rdf:resource="http://www.isocat.org/datcat/DC-2237"/>
      <owl:versionInfo>http://www.isocat.org/datcat/DC-2237</owl:versionInfo>
      <rdfs:comment>
                            position of something
                                (http://www.isocat.org/datcat/DC-2237)
                            </rdfs:comment>
      <rdfs:label>location</rdfs:label>
   </owl:Class>
   <owl:Class rdf:ID="locativeCase">
      <dcr:datcat rdf:resource="http://www.isocat.org/datcat/DC-1326"/>
      <owl:versionInfo>http://www.isocat.org/datcat/DC-1326</owl:versionInfo>
      <rdfs:comment>
                            Case that indicates a final location of action or a time of the action.
                                (www.wikipedia.org/wiki/Locative_case; http://www.isocat.org/datcat/DC-1326)
                            </rdfs:comment>
      <rdfs:label>locative case</rdfs:label>
      <rdfs:subClassOf>
         <owl:Class rdf:about="#case"/>
      </rdfs:subClassOf>
      <owl:versionInfo>subClassOf case (dcif:conceptualDomain)</owl:versionInfo>
   </owl:Class>
   <owl:Class rdf:ID="logicalAnd">
      <dcr:datcat rdf:resource="http://www.isocat.org/datcat/DC-2190"/>
      <owl:versionInfo>http://www.isocat.org/datcat/DC-2190</owl:versionInfo>
      <rdfs:comment>
                            Logical operation that results in a value of true if all of its operands are true, otherwise a value of false
                                (http://www.isocat.org/datcat/DC-2190)
                            </rdfs:comment>
      <rdfs:label>logical and</rdfs:label>
   </owl:Class>
   <owl:Class rdf:ID="logicalNot">
      <dcr:datcat rdf:resource="http://www.isocat.org/datcat/DC-2192"/>
      <owl:versionInfo>http://www.isocat.org/datcat/DC-2192</owl:versionInfo>
      <rdfs:comment>
                            Logical unary operation that returns true when its operand is false, otherwise returns true
                                (http://www.isocat.org/datcat/DC-2192)
                            </rdfs:comment>
      <rdfs:label>logical not</rdfs:label>
   </owl:Class>
   <owl:Class rdf:ID="logicalOperator">
      <dcr:datcat rdf:resource="http://www.isocat.org/datcat/DC-2208"/>
      <owl:versionInfo>http://www.isocat.org/datcat/DC-2208</owl:versionInfo>
      <rdfs:comment>
                            Type of action that gives a value of true or false
                                (http://www.isocat.org/datcat/DC-2208)
                            </rdfs:comment>
      <rdfs:label>logical operator</rdfs:label>
   </owl:Class>
   <owl:Class rdf:ID="logicalValue">
      <dcr:datcat rdf:resource="http://www.isocat.org/datcat/DC-2209"/>
      <owl:versionInfo>http://www.isocat.org/datcat/DC-2209</owl:versionInfo>
      <rdfs:comment>
                            Value used in a logical operation
                                (http://www.isocat.org/datcat/DC-2209)
                            </rdfs:comment>
      <rdfs:label>logical value</rdfs:label>
   </owl:Class>
   <owl:Class rdf:ID="macron">
      <dcr:datcat rdf:resource="http://www.isocat.org/datcat/DC-1327"/>
      <owl:versionInfo>http://www.isocat.org/datcat/DC-1327</owl:versionInfo>
      <rdfs:comment>
                            Mark placed over a long vowel to mark quantity.
                                (www.southwestern.edu/~carlg/Latin_Web/glossary.html; http://www.isocat.org/datcat/DC-1327)
                            </rdfs:comment>
      <rdfs:label>macron</rdfs:label>
   </owl:Class>
   <owl:Class rdf:ID="mainPunctuation">
      <dcr:datcat rdf:resource="http://www.isocat.org/datcat/DC-2075"/>
      <owl:versionInfo>http://www.isocat.org/datcat/DC-2075</owl:versionInfo>
      <rdfs:comment>
                            Punctuation that is more important than a secondary punctuation with regards to sentence splitting in a text.
                                (http://www.isocat.org/datcat/DC-2075)
                            </rdfs:comment>
      <rdfs:label>main punctuation</rdfs:label>
      <rdfs:subClassOf>
         <owl:Class rdf:about="#punctuation"/>
      </rdfs:subClassOf>
      <owl:versionInfo>subClassOf punctuation (dcif:isA)</owl:versionInfo>
   </owl:Class>
   <owl:Class rdf:ID="mainVerb">
      <dcr:datcat rdf:resource="http://www.isocat.org/datcat/DC-1400"/>
      <owl:versionInfo>http://www.isocat.org/datcat/DC-1400</owl:versionInfo>
      <rdfs:comment>
                            Main verb in contrast to a modal or an auxiliary.
                                (http://www.isocat.org/datcat/DC-1400)
                            </rdfs:comment>
      <rdfs:label>main verb</rdfs:label>
      <rdfs:subClassOf>
         <owl:Class rdf:about="#verb"/>
      </rdfs:subClassOf>
      <owl:versionInfo>subClassOf verb (dcif:isA)</owl:versionInfo>
   </owl:Class>
   <owl:Class rdf:ID="masculine">
      <dcr:datcat rdf:resource="http://www.isocat.org/datcat/DC-1883"/>
      <owl:versionInfo>http://www.isocat.org/datcat/DC-1883</owl:versionInfo>
      <rdfs:comment>
                            Of, relating to, or constituting the gender that ordinarily includes most words or grammatical forms referring to males.
                                (ISO12620; http://www.isocat.org/datcat/DC-1883)
                            </rdfs:comment>
      <rdfs:label>masculine</rdfs:label>
      <rdfs:subClassOf>
         <owl:Class rdf:about="#grammaticalGender"/>
      </rdfs:subClassOf>
      <owl:versionInfo>subClassOf grammaticalGender (dcif:conceptualDomain)</owl:versionInfo>
      <rdfs:subClassOf>
         <owl:Class rdf:about="#ownerGender"/>
      </rdfs:subClassOf>
      <owl:versionInfo>subClassOf ownerGender (dcif:conceptualDomain)</owl:versionInfo>
   </owl:Class>
   <owl:Class rdf:ID="masdar">
      <dcr:datcat rdf:resource="http://www.isocat.org/datcat/DC-2224"/>
      <owl:versionInfo>http://www.isocat.org/datcat/DC-2224</owl:versionInfo>
      <rdfs:comment>
                            property that expresses a verbal idea under an abstract form.
                                (MIRACL &amp; LSCA; http://www.isocat.org/datcat/DC-2224)
                            </rdfs:comment>
      <rdfs:label>masdar</rdfs:label>
   </owl:Class>
   <owl:Class rdf:ID="middleVoice">
      <dcr:datcat rdf:resource="http://www.isocat.org/datcat/DC-1983"/>
      <owl:versionInfo>http://www.isocat.org/datcat/DC-1983</owl:versionInfo>
      <rdfs:comment>
                            Value for middle voice that expresses that the subject is both the agent and object, or that the subject is separate from the agent or that the receiver is the agent him/herself.
                                (Dictionnaire de linguistique Larousse 2002; http://www.isocat.org/datcat/DC-1983)
                            </rdfs:comment>
      <rdfs:label>middle voice</rdfs:label>
      <rdfs:subClassOf>
         <owl:Class rdf:about="#voice"/>
      </rdfs:subClassOf>
      <owl:versionInfo>subClassOf voice (dcif:conceptualDomain)</owl:versionInfo>
   </owl:Class>
   <owl:Class rdf:ID="modal">
      <dcr:datcat rdf:resource="http://www.isocat.org/datcat/DC-1329"/>
      <owl:versionInfo>http://www.isocat.org/datcat/DC-1329</owl:versionInfo>
      <rdfs:comment>
                            Verb form that is usually used with another verb to express ideas such as possibilities, permission, or intention.
                                (Gil Francopoulo; http://www.isocat.org/datcat/DC-1329)
                            </rdfs:comment>
      <rdfs:label>modal</rdfs:label>
      <rdfs:subClassOf>
         <owl:Class rdf:about="#verb"/>
      </rdfs:subClassOf>
      <owl:versionInfo>subClassOf verb (dcif:isA)</owl:versionInfo>
   </owl:Class>
   <owl:Class rdf:ID="modalParticle">
      <dcr:datcat rdf:resource="http://www.isocat.org/datcat/DC-1920"/>
      <owl:versionInfo>http://www.isocat.org/datcat/DC-1920</owl:versionInfo>
      <rdfs:comment>
                            Particle which functions as a modal.
                                (http://www.isocat.org/datcat/DC-1920)
                            </rdfs:comment>
      <rdfs:label>modal particle</rdfs:label>
      <rdfs:subClassOf>
         <owl:Class rdf:about="#particle"/>
      </rdfs:subClassOf>
      <owl:versionInfo>subClassOf particle (dcif:isA)</owl:versionInfo>
   </owl:Class>
   <owl:Class rdf:ID="modern">
      <dcr:datcat rdf:resource="http://www.isocat.org/datcat/DC-1962"/>
      <owl:versionInfo>http://www.isocat.org/datcat/DC-1962</owl:versionInfo>
      <rdfs:comment>
                            Currently in use.
                                (http://www.isocat.org/datcat/DC-1962)
                            </rdfs:comment>
      <rdfs:label>modern</rdfs:label>
      <rdfs:subClassOf>
         <owl:Class rdf:about="#dating"/>
      </rdfs:subClassOf>
      <owl:versionInfo>subClassOf dating (dcif:conceptualDomain)</owl:versionInfo>
   </owl:Class>
   <owl:Class rdf:ID="modificationType">
      <dcr:datcat rdf:resource="http://www.isocat.org/datcat/DC-1931"/>
      <owl:versionInfo>http://www.isocat.org/datcat/DC-1931</owl:versionInfo>
      <rdfs:comment>
                            Refers to the prenominal or postnominal positions of determiners which distinguish different forms.
                                (http://www.isocat.org/datcat/DC-1931)
                            </rdfs:comment>
      <rdfs:label>modification type</rdfs:label>
   </owl:Class>
   <owl:Class rdf:ID="morpheme">
      <dcr:datcat rdf:resource="http://www.isocat.org/datcat/DC-1330"/>
      <owl:versionInfo>http://www.isocat.org/datcat/DC-1330</owl:versionInfo>
      <rdfs:comment>
                            A morpheme is the smallest meaningful unit in the grammar of a language.
                                (www.sil.org/linguistics/GlossaryOfLinguisticTerms/WhatIsAMorpheme.htm; http://www.isocat.org/datcat/DC-1330)
                            </rdfs:comment>
      <rdfs:label>morpheme</rdfs:label>
   </owl:Class>
   <owl:Class rdf:ID="morphologicalFeature">
      <dcr:datcat rdf:resource="http://www.isocat.org/datcat/DC-1425"/>
      <owl:versionInfo>http://www.isocat.org/datcat/DC-1425</owl:versionInfo>
      <rdfs:comment>
                            Property attached to a given inflected form that usually permits to distinguish this form from the generic lemmatised form of the word.
                                (http://www.isocat.org/datcat/DC-1425)
                            </rdfs:comment>
      <rdfs:label>morphological feature</rdfs:label>
   </owl:Class>
   <owl:Class rdf:ID="namedEntity">
      <dcr:datcat rdf:resource="http://www.isocat.org/datcat/DC-2275"/>
      <owl:versionInfo>http://www.isocat.org/datcat/DC-2275</owl:versionInfo>
      <rdfs:comment>
                            segment of text for which one or many rigid designators stands for the referent
                                (Gil Francopoulo; http://www.isocat.org/datcat/DC-2275)
                            </rdfs:comment>
      <rdfs:label>named entity</rdfs:label>
   </owl:Class>
   <owl:Class rdf:ID="native">
      <dcr:datcat rdf:resource="http://www.isocat.org/datcat/DC-1871"/>
      <owl:versionInfo>http://www.isocat.org/datcat/DC-1871</owl:versionInfo>
      <rdfs:comment>
                            Value that expresses the absence of transformation
                                (Gil Francopoulo; http://www.isocat.org/datcat/DC-1871)
                            </rdfs:comment>
      <rdfs:label>native</rdfs:label>
   </owl:Class>
   <owl:Class rdf:ID="negative">
      <dcr:datcat rdf:resource="http://www.isocat.org/datcat/DC-1839"/>
      <owl:versionInfo>http://www.isocat.org/datcat/DC-1839</owl:versionInfo>
      <rdfs:comment>
                            denotes the negation or the absence
                                (http://www.isocat.org/datcat/DC-1839)
                            </rdfs:comment>
      <rdfs:label>negative</rdfs:label>
   </owl:Class>
   <owl:Class rdf:ID="negativeParticle">
      <dcr:datcat rdf:resource="http://www.isocat.org/datcat/DC-1894"/>
      <owl:versionInfo>http://www.isocat.org/datcat/DC-1894</owl:versionInfo>
      <rdfs:comment>
                            Particle used to express negation.
                                (Gil Francopoulo; http://www.isocat.org/datcat/DC-1894)
                            </rdfs:comment>
      <rdfs:label>negative particle</rdfs:label>
      <rdfs:subClassOf>
         <owl:Class rdf:about="#particle"/>
      </rdfs:subClassOf>
      <owl:versionInfo>subClassOf particle (dcif:isA)</owl:versionInfo>
   </owl:Class>
   <owl:Class rdf:ID="negativePronoun">
      <dcr:datcat rdf:resource="http://www.isocat.org/datcat/DC-1925"/>
      <owl:versionInfo>http://www.isocat.org/datcat/DC-1925</owl:versionInfo>
      <rdfs:comment>
                            Pronoun used in a context of a negation or for expressing a negation.
                                (http://www.isocat.org/datcat/DC-1925)
                            </rdfs:comment>
      <rdfs:label>negative pronoun</rdfs:label>
      <rdfs:subClassOf>
         <owl:Class rdf:about="#pronoun"/>
      </rdfs:subClassOf>
      <owl:versionInfo>subClassOf pronoun (dcif:isA)</owl:versionInfo>
   </owl:Class>
   <owl:Class rdf:ID="neuter">
      <dcr:datcat rdf:resource="http://www.isocat.org/datcat/DC-1884"/>
      <owl:versionInfo>http://www.isocat.org/datcat/DC-1884</owl:versionInfo>
      <rdfs:comment>
                            Of, relating to, or constituting the gender that ordinarily includes most words or grammatical forms referring to objects that are not characterized as male or female.
                                (ISO12620; http://www.isocat.org/datcat/DC-1884)
                            </rdfs:comment>
      <rdfs:label>neuter</rdfs:label>
      <rdfs:subClassOf>
         <owl:Class rdf:about="#grammaticalGender"/>
      </rdfs:subClassOf>
      <owl:versionInfo>subClassOf grammaticalGender (dcif:conceptualDomain)</owl:versionInfo>
      <rdfs:subClassOf>
         <owl:Class rdf:about="#ownerGender"/>
      </rdfs:subClassOf>
      <owl:versionInfo>subClassOf ownerGender (dcif:conceptualDomain)</owl:versionInfo>
   </owl:Class>
   <owl:Class rdf:ID="neutralRegister">
      <dcr:datcat rdf:resource="http://www.isocat.org/datcat/DC-1999"/>
      <owl:versionInfo>http://www.isocat.org/datcat/DC-1999</owl:versionInfo>
      <rdfs:comment>
                            The register appropriate to general texts or discourse.
                                (ISO12620; http://www.isocat.org/datcat/DC-1999)
                            </rdfs:comment>
      <rdfs:label>neutral register</rdfs:label>
      <rdfs:label>standard register</rdfs:label>
      <rdfs:subClassOf>
         <owl:Class rdf:about="#register"/>
      </rdfs:subClassOf>
      <owl:versionInfo>subClassOf register (dcif:conceptualDomain)</owl:versionInfo>
   </owl:Class>
   <owl:Class rdf:ID="no">
      <dcr:datcat rdf:resource="http://www.isocat.org/datcat/DC-1905"/>
      <owl:versionInfo>http://www.isocat.org/datcat/DC-1905</owl:versionInfo>
      <rdfs:comment>
                            Value for negation.
                                (http://www.isocat.org/datcat/DC-1905)
                            </rdfs:comment>
      <rdfs:label>no</rdfs:label>
      <rdfs:subClassOf>
         <owl:Class rdf:about="#cliticness"/>
      </rdfs:subClassOf>
      <owl:versionInfo>subClassOf cliticness (dcif:conceptualDomain)</owl:versionInfo>
      <rdfs:subClassOf>
         <owl:Class rdf:about="#negative"/>
      </rdfs:subClassOf>
      <owl:versionInfo>subClassOf negative (dcif:conceptualDomain)</owl:versionInfo>
      <rdfs:subClassOf>
         <owl:Class rdf:about="#zuInclusion"/>
      </rdfs:subClassOf>
      <owl:versionInfo>subClassOf zuInclusion (dcif:conceptualDomain)</owl:versionInfo>
   </owl:Class>
   <owl:Class rdf:ID="nominativeCase">
      <dcr:datcat rdf:resource="http://www.isocat.org/datcat/DC-1331"/>
      <owl:versionInfo>http://www.isocat.org/datcat/DC-1331</owl:versionInfo>
      <rdfs:comment>
                            Case used to indicate the subject of a verb.
                                (www.southwestern.edu/~carlg/Latin_Web/glossary.html; http://www.isocat.org/datcat/DC-1331)
                            </rdfs:comment>
      <rdfs:label>nominative case</rdfs:label>
      <rdfs:subClassOf>
         <owl:Class rdf:about="#case"/>
      </rdfs:subClassOf>
      <owl:versionInfo>subClassOf case (dcif:conceptualDomain)</owl:versionInfo>
   </owl:Class>
   <owl:Class rdf:ID="nonSpacedPinyin">
      <dcr:datcat rdf:resource="http://www.isocat.org/datcat/DC-1853"/>
      <owl:versionInfo>http://www.isocat.org/datcat/DC-1853</owl:versionInfo>
      <rdfs:comment>
                            Pinyin without any space characters
                                (Gil Francopoulo; http://www.isocat.org/datcat/DC-1853)
                            </rdfs:comment>
      <rdfs:label>non spaced pinyin</rdfs:label>
   </owl:Class>
   <owl:Class rdf:ID="nonFinite">
      <dcr:datcat rdf:resource="http://www.isocat.org/datcat/DC-1332"/>
      <owl:versionInfo>http://www.isocat.org/datcat/DC-1332</owl:versionInfo>
      <rdfs:comment>
                            Property related for verb forms occurring on their own only in dependent clauses and lacking tense and mood contrasts.
                                (adapted from Crystal 2003; http://www.isocat.org/datcat/DC-1332)
                            </rdfs:comment>
      <rdfs:label>non-finite</rdfs:label>
      <rdfs:subClassOf>
         <owl:Class rdf:about="#finiteness"/>
      </rdfs:subClassOf>
      <owl:versionInfo>subClassOf finiteness (dcif:conceptualDomain)</owl:versionInfo>
   </owl:Class>
   <owl:Class rdf:ID="noun">
      <dcr:datcat rdf:resource="http://www.isocat.org/datcat/DC-1333"/>
      <owl:versionInfo>http://www.isocat.org/datcat/DC-1333</owl:versionInfo>
      <rdfs:comment>
                            Part of speech used to express the name of a person, place, action or thing.
                                (http://www.isocat.org/datcat/DC-1333)
                            </rdfs:comment>
      <rdfs:label>noun</rdfs:label>
      <rdfs:subClassOf>
         <owl:Class rdf:about="#partOfSpeech"/>
      </rdfs:subClassOf>
      <owl:versionInfo>subClassOf partOfSpeech (dcif:conceptualDomain)</owl:versionInfo>
      <rdfs:subClassOf>
         <owl:Class rdf:about="#syntacticType"/>
      </rdfs:subClassOf>
      <owl:versionInfo>subClassOf syntacticType (dcif:conceptualDomain)</owl:versionInfo>
   </owl:Class>
   <owl:Class rdf:ID="numeral">
      <dcr:datcat rdf:resource="http://www.isocat.org/datcat/DC-1334"/>
      <owl:versionInfo>http://www.isocat.org/datcat/DC-1334</owl:versionInfo>
      <rdfs:comment>
                            Part of speech that expresses a number or the relation to a number.
                                (http://www.isocat.org/datcat/DC-1334)
                            </rdfs:comment>
      <rdfs:label>numeral</rdfs:label>
   </owl:Class>
   <owl:Class rdf:ID="numeralMForm">
      <dcr:datcat rdf:resource="http://www.isocat.org/datcat/DC-1939"/>
      <owl:versionInfo>http://www.isocat.org/datcat/DC-1939</owl:versionInfo>
      <rdfs:comment>
                            Numeral MForm.
                                (http://www.isocat.org/datcat/DC-1939)
                            </rdfs:comment>
      <rdfs:label>numeral MForm</rdfs:label>
   </owl:Class>
   <owl:Class rdf:ID="numeralApprox">
      <dcr:datcat rdf:resource="http://www.isocat.org/datcat/DC-1940"/>
      <owl:versionInfo>http://www.isocat.org/datcat/DC-1940</owl:versionInfo>
      <rdfs:comment>
                            Numeric approximation.
                                (http://www.isocat.org/datcat/DC-1940)
                            </rdfs:comment>
      <rdfs:label>numeral approximation</rdfs:label>
   </owl:Class>
   <owl:Class rdf:ID="numeralBoth">
      <dcr:datcat rdf:resource="http://www.isocat.org/datcat/DC-1938"/>
      <owl:versionInfo>http://www.isocat.org/datcat/DC-1938</owl:versionInfo>
      <rdfs:comment>
                            Numeric value for two.
                                (http://www.isocat.org/datcat/DC-1938)
                            </rdfs:comment>
      <rdfs:label>numeral both</rdfs:label>
   </owl:Class>
   <owl:Class rdf:ID="numeralDigit">
      <dcr:datcat rdf:resource="http://www.isocat.org/datcat/DC-1935"/>
      <owl:versionInfo>http://www.isocat.org/datcat/DC-1935</owl:versionInfo>
      <rdfs:comment>
                            Numeral expressed by an arabic digit.
                                (http://www.isocat.org/datcat/DC-1935)
                            </rdfs:comment>
      <rdfs:label>numeral digit</rdfs:label>
   </owl:Class>
   <owl:Class rdf:ID="numeralLetter">
      <dcr:datcat rdf:resource="http://www.isocat.org/datcat/DC-1937"/>
      <owl:versionInfo>http://www.isocat.org/datcat/DC-1937</owl:versionInfo>
      <rdfs:comment>
                            Numeral expressed with letters.
                                (http://www.isocat.org/datcat/DC-1937)
                            </rdfs:comment>
      <rdfs:label>numeral letter</rdfs:label>
   </owl:Class>
   <owl:Class rdf:ID="numeralRoman">
      <dcr:datcat rdf:resource="http://www.isocat.org/datcat/DC-1936"/>
      <owl:versionInfo>http://www.isocat.org/datcat/DC-1936</owl:versionInfo>
      <rdfs:comment>
                            Numeral expressed with roman digits.
                                (http://www.isocat.org/datcat/DC-1936)
                            </rdfs:comment>
      <rdfs:label>numeral roman</rdfs:label>
   </owl:Class>
   <owl:Class rdf:ID="numValue">
      <dcr:datcat rdf:resource="http://www.isocat.org/datcat/DC-2211"/>
      <owl:versionInfo>http://www.isocat.org/datcat/DC-2211</owl:versionInfo>
      <rdfs:comment>
                            Numerical value to be interpreted in context.
                                (http://www.isocat.org/datcat/DC-2211)
                            </rdfs:comment>
      <rdfs:label>numerical value</rdfs:label>
   </owl:Class>
   <owl:Class rdf:ID="objectPerson">
      <dcr:datcat rdf:resource="http://www.isocat.org/datcat/DC-2279"/>
      <owl:versionInfo>http://www.isocat.org/datcat/DC-2279</owl:versionInfo>
      <rdfs:comment>
                            person for the object of the verb
                                (http://www.isocat.org/datcat/DC-2279)
                            </rdfs:comment>
      <rdfs:label>object person</rdfs:label>
   </owl:Class>
   <owl:Class rdf:ID="obliqueCase">
      <dcr:datcat rdf:resource="http://www.isocat.org/datcat/DC-1336"/>
      <owl:versionInfo>http://www.isocat.org/datcat/DC-1336</owl:versionInfo>
      <rdfs:comment>
                            Case that is used when a noun is the object of a verb or a proposition, except for nominative and vocative case.
                                (www.hyperdictionary.com/dictionary/oblique+case +; http://www.isocat.org/datcat/DC-1336)
                            </rdfs:comment>
      <rdfs:label>oblique case</rdfs:label>
      <rdfs:subClassOf>
         <owl:Class rdf:about="#case"/>
      </rdfs:subClassOf>
      <owl:versionInfo>subClassOf case (dcif:conceptualDomain)</owl:versionInfo>
   </owl:Class>
   <owl:Class rdf:ID="old">
      <dcr:datcat rdf:resource="http://www.isocat.org/datcat/DC-1961"/>
      <owl:versionInfo>http://www.isocat.org/datcat/DC-1961</owl:versionInfo>
      <rdfs:comment>
                            Used in the past.
                                (http://www.isocat.org/datcat/DC-1961)
                            </rdfs:comment>
      <rdfs:label>old</rdfs:label>
      <rdfs:subClassOf>
         <owl:Class rdf:about="#dating"/>
      </rdfs:subClassOf>
      <owl:versionInfo>subClassOf dating (dcif:conceptualDomain)</owl:versionInfo>
   </owl:Class>
   <owl:Class rdf:ID="openBracket">
      <dcr:datcat rdf:resource="http://www.isocat.org/datcat/DC-2082"/>
      <owl:versionInfo>http://www.isocat.org/datcat/DC-2082</owl:versionInfo>
      <rdfs:comment>
                            Punctuation that is represented graphically as [
                                (http://www.isocat.org/datcat/DC-2082)
                            </rdfs:comment>
      <rdfs:label>open bracket</rdfs:label>
   </owl:Class>
   <owl:Class rdf:ID="openCurlyBracket">
      <dcr:datcat rdf:resource="http://www.isocat.org/datcat/DC-2084"/>
      <owl:versionInfo>http://www.isocat.org/datcat/DC-2084</owl:versionInfo>
      <rdfs:comment>
                            Punctuation that is graphically represented as {
                                (http://www.isocat.org/datcat/DC-2084)
                            </rdfs:comment>
      <rdfs:label>open curly bracket</rdfs:label>
   </owl:Class>
   <owl:Class rdf:ID="openParenthesis">
      <dcr:datcat rdf:resource="http://www.isocat.org/datcat/DC-1442"/>
      <owl:versionInfo>http://www.isocat.org/datcat/DC-1442</owl:versionInfo>
      <rdfs:comment>
                            Beginning of a pair of parenthesis.
                                (http://www.isocat.org/datcat/DC-1442)
                            </rdfs:comment>
      <rdfs:label>open parenthesis</rdfs:label>
      <rdfs:subClassOf>
         <owl:Class rdf:about="#partOfSpeech"/>
      </rdfs:subClassOf>
      <owl:versionInfo>subClassOf partOfSpeech (dcif:conceptualDomain)</owl:versionInfo>
   </owl:Class>
   <owl:Class rdf:ID="openPunctuation">
      <dcr:datcat rdf:resource="http://www.isocat.org/datcat/DC-2078"/>
      <owl:versionInfo>http://www.isocat.org/datcat/DC-2078</owl:versionInfo>
      <rdfs:comment>
                            Beginning of a paired punctuation.
                                (http://www.isocat.org/datcat/DC-2078)
                            </rdfs:comment>
      <rdfs:label>open punctuation</rdfs:label>
      <rdfs:subClassOf>
         <owl:Class rdf:about="#punctuation"/>
      </rdfs:subClassOf>
      <owl:versionInfo>subClassOf punctuation (dcif:isA)</owl:versionInfo>
   </owl:Class>
   <owl:Class rdf:ID="operation">
      <dcr:datcat rdf:resource="http://www.isocat.org/datcat/DC-2179"/>
      <owl:versionInfo>http://www.isocat.org/datcat/DC-2179</owl:versionInfo>
      <rdfs:comment>
                            Way something such as a principle or law works or has an effect
                                (http://www.isocat.org/datcat/DC-2179)
                            </rdfs:comment>
      <rdfs:label>operation</rdfs:label>
   </owl:Class>
   <owl:Class rdf:ID="operator">
      <dcr:datcat rdf:resource="http://www.isocat.org/datcat/DC-2235"/>
      <owl:versionInfo>http://www.isocat.org/datcat/DC-2235</owl:versionInfo>
      <rdfs:comment>
                            action name that can be applied to any number of operands
                                (http://www.isocat.org/datcat/DC-2235)
                            </rdfs:comment>
      <rdfs:label>operator</rdfs:label>
   </owl:Class>
   <owl:Class rdf:ID="order">
      <dcr:datcat rdf:resource="http://www.isocat.org/datcat/DC-2356"/>
      <owl:versionInfo>http://www.isocat.org/datcat/DC-2356</owl:versionInfo>
      <rdfs:comment>
                            way things are arranged in relation to each other
                                (http://www.isocat.org/datcat/DC-2356)
                            </rdfs:comment>
      <rdfs:label>order</rdfs:label>
   </owl:Class>
   <owl:Class rdf:ID="ordinalAdjective">
      <dcr:datcat rdf:resource="http://www.isocat.org/datcat/DC-1338"/>
      <owl:versionInfo>http://www.isocat.org/datcat/DC-1338</owl:versionInfo>
      <rdfs:comment>
                            Adjective expressing a numeric ranking.
                                (http://www.isocat.org/datcat/DC-1338)
                            </rdfs:comment>
      <rdfs:label>ordinal adjective</rdfs:label>
      <rdfs:subClassOf>
         <owl:Class rdf:about="#adjective"/>
      </rdfs:subClassOf>
      <owl:versionInfo>subClassOf adjective (dcif:isA)</owl:versionInfo>
   </owl:Class>
   <owl:Class rdf:ID="orthographyName">
      <dcr:datcat rdf:resource="http://www.isocat.org/datcat/DC-2176"/>
      <owl:versionInfo>http://www.isocat.org/datcat/DC-2176</owl:versionInfo>
      <rdfs:comment>
                            Precision concerning the orthography
                                (http://www.isocat.org/datcat/DC-2176)
                            </rdfs:comment>
      <rdfs:label>orthography name</rdfs:label>
   </owl:Class>
   <owl:Class rdf:ID="otherAnimacy">
      <dcr:datcat rdf:resource="http://www.isocat.org/datcat/DC-1953"/>
      <owl:versionInfo>http://www.isocat.org/datcat/DC-1953</owl:versionInfo>
      <rdfs:comment>
                            Perceived as related to animacy, but without specific reference to the previous items.
                                (ISO12620; http://www.isocat.org/datcat/DC-1953)
                            </rdfs:comment>
      <rdfs:label>other animacy</rdfs:label>
      <rdfs:subClassOf>
         <owl:Class rdf:about="#animacy"/>
      </rdfs:subClassOf>
      <owl:versionInfo>subClassOf animacy (dcif:conceptualDomain)</owl:versionInfo>
   </owl:Class>
   <owl:Class rdf:ID="ownedNumber">
      <dcr:datcat rdf:resource="http://www.isocat.org/datcat/DC-1930"/>
      <owl:versionInfo>http://www.isocat.org/datcat/DC-1930</owl:versionInfo>
      <rdfs:comment>
                            Indication concerning the number of the possessed thing.
                                (http://www.isocat.org/datcat/DC-1930)
                            </rdfs:comment>
      <rdfs:label>owned number</rdfs:label>
   </owl:Class>
   <owl:Class rdf:ID="ownerGender">
      <dcr:datcat rdf:resource="http://www.isocat.org/datcat/DC-1416"/>
      <owl:versionInfo>http://www.isocat.org/datcat/DC-1416</owl:versionInfo>
      <rdfs:comment>
                            Indication concerning the gender of the person that ownes something.
                                (http://www.isocat.org/datcat/DC-1416)
                            </rdfs:comment>
      <rdfs:label>owner gender</rdfs:label>
   </owl:Class>
   <owl:Class rdf:ID="ownerNumber">
      <dcr:datcat rdf:resource="http://www.isocat.org/datcat/DC-1417"/>
      <owl:versionInfo>http://www.isocat.org/datcat/DC-1417</owl:versionInfo>
      <rdfs:comment>
                            Indication concerning the number of the person that ownes something.
                                (http://www.isocat.org/datcat/DC-1417)
                            </rdfs:comment>
      <rdfs:label>owner number</rdfs:label>
   </owl:Class>
   <owl:Class rdf:ID="ownerPerson">
      <dcr:datcat rdf:resource="http://www.isocat.org/datcat/DC-1929"/>
      <owl:versionInfo>http://www.isocat.org/datcat/DC-1929</owl:versionInfo>
      <rdfs:comment>
                            Indication concerning the person that ownes something.
                                (http://www.isocat.org/datcat/DC-1929)
                            </rdfs:comment>
      <rdfs:label>owner person</rdfs:label>
   </owl:Class>
   <owl:Class rdf:ID="partOfSpeech">
      <dcr:datcat rdf:resource="http://www.isocat.org/datcat/DC-1345"/>
      <owl:versionInfo>http://www.isocat.org/datcat/DC-1345</owl:versionInfo>
      <rdfs:comment>
                            Term used to describe how a particular word is used in a sentence.
                                (www.southwestern.edu/~carlg/Latin_Web/glossary.html; http://www.isocat.org/datcat/DC-1345)
                            </rdfs:comment>
      <rdfs:label>part of speech</rdfs:label>
   </owl:Class>
   <owl:Class rdf:ID="participle">
      <dcr:datcat rdf:resource="http://www.isocat.org/datcat/DC-1341"/>
      <owl:versionInfo>http://www.isocat.org/datcat/DC-1341</owl:versionInfo>
      <rdfs:comment>
                            Term referring to a word derived from a verb and used as an adjective.
                                (Crystal 2003; http://www.isocat.org/datcat/DC-1341)
                            </rdfs:comment>
      <rdfs:label>participle</rdfs:label>
      <rdfs:subClassOf>
         <owl:Class rdf:about="#verbFormMood"/>
      </rdfs:subClassOf>
      <owl:versionInfo>subClassOf verbFormMood (dcif:conceptualDomain)</owl:versionInfo>
   </owl:Class>
   <owl:Class rdf:ID="participleAdjective">
      <dcr:datcat rdf:resource="http://www.isocat.org/datcat/DC-1598"/>
      <owl:versionInfo>http://www.isocat.org/datcat/DC-1598</owl:versionInfo>
      <rdfs:comment>
                            Adjective based on a verb.
                                (http://www.isocat.org/datcat/DC-1598)
                            </rdfs:comment>
      <rdfs:label>participle adjective</rdfs:label>
      <rdfs:subClassOf>
         <owl:Class rdf:about="#adjective"/>
      </rdfs:subClassOf>
      <owl:versionInfo>subClassOf adjective (dcif:isA)</owl:versionInfo>
   </owl:Class>
   <owl:Class rdf:ID="particle">
      <dcr:datcat rdf:resource="http://www.isocat.org/datcat/DC-1342"/>
      <owl:versionInfo>http://www.isocat.org/datcat/DC-1342</owl:versionInfo>
      <rdfs:comment>
                            Word that does not belong to one of the main classes of words, is invariable in form, and typically has grammatical or pragmatic meaning.
                                (www.sil.org/linguistics/GlossaryOfLinguisticTerms/WhatIsAParticle.htm; http://www.isocat.org/datcat/DC-1342)
                            </rdfs:comment>
      <rdfs:label>particle</rdfs:label>
      <rdfs:subClassOf>
         <owl:Class rdf:about="#partOfSpeech"/>
      </rdfs:subClassOf>
      <owl:versionInfo>subClassOf partOfSpeech (dcif:conceptualDomain)</owl:versionInfo>
   </owl:Class>
   <owl:Class rdf:ID="affirmativeParticle">
      <dcr:datcat rdf:resource="http://www.isocat.org/datcat/DC-1918"/>
      <owl:versionInfo>http://www.isocat.org/datcat/DC-1918</owl:versionInfo>
      <rdfs:comment>
                            Particle used to express affirmation.
                                (http://www.isocat.org/datcat/DC-1918)
                            </rdfs:comment>
      <rdfs:label>particule affirmative</rdfs:label>
      <rdfs:subClassOf>
         <owl:Class rdf:about="#particle"/>
      </rdfs:subClassOf>
      <owl:versionInfo>subClassOf particle (dcif:isA)</owl:versionInfo>
   </owl:Class>
   <owl:Class rdf:ID="partitiveArticle">
      <dcr:datcat rdf:resource="http://www.isocat.org/datcat/DC-1898"/>
      <owl:versionInfo>http://www.isocat.org/datcat/DC-1898</owl:versionInfo>
      <rdfs:comment>
                            Article expressing a part or quantity.
                                (Gil Francopoulo; http://www.isocat.org/datcat/DC-1898)
                            </rdfs:comment>
      <rdfs:label>partitive article</rdfs:label>
      <rdfs:subClassOf>
         <owl:Class rdf:about="#partOfSpeech"/>
      </rdfs:subClassOf>
      <owl:versionInfo>subClassOf partOfSpeech (dcif:conceptualDomain)</owl:versionInfo>
   </owl:Class>
   <owl:Class rdf:ID="partitiveCase">
      <dcr:datcat rdf:resource="http://www.isocat.org/datcat/DC-2003"/>
      <owl:versionInfo>http://www.isocat.org/datcat/DC-2003</owl:versionInfo>
      <rdfs:comment>
                            Case that expresses the partial nature of the referent of the noun it marks, as opposed to expressing the whole unit or class of which the referent is a part.
                                (DFKI; http://www.isocat.org/datcat/DC-2003)
                            </rdfs:comment>
      <rdfs:label>partitive case</rdfs:label>
      <rdfs:subClassOf>
         <owl:Class rdf:about="#case"/>
      </rdfs:subClassOf>
      <owl:versionInfo>subClassOf case (dcif:conceptualDomain)</owl:versionInfo>
   </owl:Class>
   <owl:Class rdf:ID="passiveVoice">
      <dcr:datcat rdf:resource="http://www.isocat.org/datcat/DC-1346"/>
      <owl:versionInfo>http://www.isocat.org/datcat/DC-1346</owl:versionInfo>
      <rdfs:comment>
                            Term referring to a situation where the grammatical subject is typically the recipient or goal of the action denoted by the verb.
                                (Crystal 2003; http://www.isocat.org/datcat/DC-1346)
                            </rdfs:comment>
      <rdfs:label>passive voice</rdfs:label>
      <rdfs:subClassOf>
         <owl:Class rdf:about="#voice"/>
      </rdfs:subClassOf>
      <owl:versionInfo>subClassOf voice (dcif:conceptualDomain)</owl:versionInfo>
   </owl:Class>
   <owl:Class rdf:ID="past">
      <dcr:datcat rdf:resource="http://www.isocat.org/datcat/DC-1347"/>
      <owl:versionInfo>http://www.isocat.org/datcat/DC-1347</owl:versionInfo>
      <rdfs:comment>
                            Past tense is an absolute tense that refers to a time before the moment of utterance.
                                (www.sil.org/linguistics/GlossaryOfLinguisticTerms/WhatIsPastTense.htm; http://www.isocat.org/datcat/DC-1347)
                            </rdfs:comment>
      <rdfs:label>past</rdfs:label>
      <rdfs:subClassOf>
         <owl:Class rdf:about="#grammaticalTense"/>
      </rdfs:subClassOf>
      <owl:versionInfo>subClassOf grammaticalTense (dcif:conceptualDomain)</owl:versionInfo>
   </owl:Class>
   <owl:Class rdf:ID="pastParticipleAdjective">
      <dcr:datcat rdf:resource="http://www.isocat.org/datcat/DC-1596"/>
      <owl:versionInfo>http://www.isocat.org/datcat/DC-1596</owl:versionInfo>
      <rdfs:comment>
                            Adjective based on a past participle.
                                (http://www.isocat.org/datcat/DC-1596)
                            </rdfs:comment>
      <rdfs:label>past participle adjective</rdfs:label>
      <rdfs:subClassOf>
         <owl:Class rdf:about="#participleAdjective"/>
      </rdfs:subClassOf>
      <owl:versionInfo>subClassOf participleAdjective (dcif:isA)</owl:versionInfo>
   </owl:Class>
   <owl:Class rdf:ID="patternType">
      <dcr:datcat rdf:resource="http://www.isocat.org/datcat/DC-2178"/>
      <owl:versionInfo>http://www.isocat.org/datcat/DC-2178</owl:versionInfo>
      <rdfs:comment>
                            Sub-type of a pattern class
                                (http://www.isocat.org/datcat/DC-2178)
                            </rdfs:comment>
      <rdfs:label>pattern type</rdfs:label>
   </owl:Class>
   <owl:Class rdf:ID="paucal">
      <dcr:datcat rdf:resource="http://www.isocat.org/datcat/DC-1350"/>
      <owl:versionInfo>http://www.isocat.org/datcat/DC-1350</owl:versionInfo>
      <rdfs:comment>
                            Number that specifies 'a few' things.
                                (en2.wikipedia.org/wiki/Paucal_number; http://www.isocat.org/datcat/DC-1350)
                            </rdfs:comment>
      <rdfs:label>paucal</rdfs:label>
      <rdfs:subClassOf>
         <owl:Class rdf:about="#grammaticalNumber"/>
      </rdfs:subClassOf>
      <owl:versionInfo>subClassOf grammaticalNumber (dcif:conceptualDomain)</owl:versionInfo>
   </owl:Class>
   <owl:Class rdf:ID="perfective">
      <dcr:datcat rdf:resource="http://www.isocat.org/datcat/DC-1352"/>
      <owl:versionInfo>http://www.isocat.org/datcat/DC-1352</owl:versionInfo>
      <rdfs:comment>
                            Perfective aspect is an aspect that expresses a temporal view of an event or state as a simple whole, apart from the consideration of the internal structure of the time in which it occurs.
                                (www.sil.org/linguistics/GlossaryOfLinguisticTerms/WhatIsPerfectiveAspect.htm; http://www.isocat.org/datcat/DC-1352)
                            </rdfs:comment>
      <rdfs:label>perfective</rdfs:label>
      <rdfs:subClassOf>
         <owl:Class rdf:about="#aspect"/>
      </rdfs:subClassOf>
      <owl:versionInfo>subClassOf aspect (dcif:conceptualDomain)</owl:versionInfo>
   </owl:Class>
   <owl:Class rdf:ID="person">
      <dcr:datcat rdf:resource="http://www.isocat.org/datcat/DC-1328"/>
      <owl:versionInfo>http://www.isocat.org/datcat/DC-1328</owl:versionInfo>
      <rdfs:comment>
                            Indication of grammatical person (1st, 2nd, 3rd, etc.) associated with a given inflected form.
                                (ISO12620; http://www.isocat.org/datcat/DC-1328)
                            </rdfs:comment>
      <rdfs:label>person</rdfs:label>
   </owl:Class>
   <owl:Class rdf:ID="personal">
      <dcr:datcat rdf:resource="http://www.isocat.org/datcat/DC-1946"/>
      <owl:versionInfo>http://www.isocat.org/datcat/DC-1946</owl:versionInfo>
      <rdfs:comment>
                            Property that refers to the person.
                                (http://www.isocat.org/datcat/DC-1946)
                            </rdfs:comment>
      <rdfs:label>personal</rdfs:label>
      <rdfs:subClassOf>
         <owl:Class rdf:about="#referentType"/>
      </rdfs:subClassOf>
      <owl:versionInfo>subClassOf referentType (dcif:conceptualDomain)</owl:versionInfo>
   </owl:Class>
   <owl:Class rdf:ID="personalPronoun">
      <dcr:datcat rdf:resource="http://www.isocat.org/datcat/DC-1463"/>
      <owl:versionInfo>http://www.isocat.org/datcat/DC-1463</owl:versionInfo>
      <rdfs:comment>
                            Pronoun referring a person.
                                (http://www.isocat.org/datcat/DC-1463)
                            </rdfs:comment>
      <rdfs:label>personal pronoun</rdfs:label>
      <rdfs:subClassOf>
         <owl:Class rdf:about="#pronoun"/>
      </rdfs:subClassOf>
      <owl:versionInfo>subClassOf pronoun (dcif:isA)</owl:versionInfo>
   </owl:Class>
   <owl:Class rdf:ID="phoneticForm">
      <dcr:datcat rdf:resource="http://www.isocat.org/datcat/DC-1837"/>
      <owl:versionInfo>http://www.isocat.org/datcat/DC-1837</owl:versionInfo>
      <rdfs:comment>
                            Representation of the spoken string of a form
                                (http://www.isocat.org/datcat/DC-1837)
                            </rdfs:comment>
      <rdfs:label>phonetic form</rdfs:label>
   </owl:Class>
   <owl:Class rdf:ID="phoneticOperator">
      <dcr:datcat rdf:resource="http://www.isocat.org/datcat/DC-1861"/>
      <owl:versionInfo>http://www.isocat.org/datcat/DC-1861</owl:versionInfo>
      <rdfs:comment>
                            Description of the modification of a spoken form
                                (Gil Francopoulo; http://www.isocat.org/datcat/DC-1861)
                            </rdfs:comment>
      <rdfs:label>phonetic operator</rdfs:label>
   </owl:Class>
   <owl:Class rdf:ID="pinyin">
      <dcr:datcat rdf:resource="http://www.isocat.org/datcat/DC-1852"/>
      <owl:versionInfo>http://www.isocat.org/datcat/DC-1852</owl:versionInfo>
      <rdfs:comment>
                            Transcription of Chinese ideograms
                                (http://www.isocat.org/datcat/DC-1852)
                            </rdfs:comment>
      <rdfs:label>pinyin</rdfs:label>
   </owl:Class>
   <owl:Class rdf:ID="plural">
      <dcr:datcat rdf:resource="http://www.isocat.org/datcat/DC-1354"/>
      <owl:versionInfo>http://www.isocat.org/datcat/DC-1354</owl:versionInfo>
      <rdfs:comment>
                            Value that expresses more than one element.
                                (http://www.isocat.org/datcat/DC-1354)
                            </rdfs:comment>
      <rdfs:label>plural</rdfs:label>
      <rdfs:subClassOf>
         <owl:Class rdf:about="#grammaticalNumber"/>
      </rdfs:subClassOf>
      <owl:versionInfo>subClassOf grammaticalNumber (dcif:conceptualDomain)</owl:versionInfo>
      <rdfs:subClassOf>
         <owl:Class rdf:about="#ownerNumber"/>
      </rdfs:subClassOf>
      <owl:versionInfo>subClassOf ownerNumber (dcif:conceptualDomain)</owl:versionInfo>
   </owl:Class>
   <owl:Class rdf:ID="pluralType">
      <dcr:datcat rdf:resource="http://www.isocat.org/datcat/DC-2232"/>
      <owl:versionInfo>http://www.isocat.org/datcat/DC-2232</owl:versionInfo>
      <rdfs:comment>
                            type of plural
                                (http://www.isocat.org/datcat/DC-2232)
                            </rdfs:comment>
      <rdfs:label>plural type</rdfs:label>
   </owl:Class>
   <owl:Class rdf:ID="point">
      <dcr:datcat rdf:resource="http://www.isocat.org/datcat/DC-1445"/>
      <owl:versionInfo>http://www.isocat.org/datcat/DC-1445</owl:versionInfo>
      <rdfs:comment>
                            Sign (.) used to expresses the end of a sentence or an abbreviation.
                                (http://www.isocat.org/datcat/DC-1445)
                            </rdfs:comment>
      <rdfs:label>dot</rdfs:label>
      <rdfs:label>point</rdfs:label>
      <rdfs:subClassOf>
         <owl:Class rdf:about="#partOfSpeech"/>
      </rdfs:subClassOf>
      <owl:versionInfo>subClassOf partOfSpeech (dcif:conceptualDomain)</owl:versionInfo>
   </owl:Class>
   <owl:Class rdf:ID="position">
      <dcr:datcat rdf:resource="http://www.isocat.org/datcat/DC-2183"/>
      <owl:versionInfo>http://www.isocat.org/datcat/DC-2183</owl:versionInfo>
      <rdfs:comment>
                            Place where something is needed or supposed to be
                                (http://www.isocat.org/datcat/DC-2183)
                            </rdfs:comment>
      <rdfs:label>position</rdfs:label>
   </owl:Class>
   <owl:Class rdf:ID="positive">
      <dcr:datcat rdf:resource="http://www.isocat.org/datcat/DC-1420"/>
      <owl:versionInfo>http://www.isocat.org/datcat/DC-1420</owl:versionInfo>
      <rdfs:comment>
                            Value used in a comparison relationship when no comparison is involved.
                                (http://www.isocat.org/datcat/DC-1420)
                            </rdfs:comment>
      <rdfs:label>positive</rdfs:label>
      <rdfs:subClassOf>
         <owl:Class rdf:about="#degree"/>
      </rdfs:subClassOf>
      <owl:versionInfo>subClassOf degree (dcif:conceptualDomain)</owl:versionInfo>
   </owl:Class>
   <owl:Class rdf:ID="possessive">
      <dcr:datcat rdf:resource="http://www.isocat.org/datcat/DC-1355"/>
      <owl:versionInfo>http://www.isocat.org/datcat/DC-1355</owl:versionInfo>
      <rdfs:comment>
                            Relative to the possession or association.
                                (www.wordreference.com/English/definition.asp?en=possessive; http://www.isocat.org/datcat/DC-1355)
                            </rdfs:comment>
      <rdfs:label>possessive</rdfs:label>
      <rdfs:subClassOf>
         <owl:Class rdf:about="#referentType"/>
      </rdfs:subClassOf>
      <owl:versionInfo>subClassOf referentType (dcif:conceptualDomain)</owl:versionInfo>
   </owl:Class>
   <owl:Class rdf:ID="possessiveDeterminer">
      <dcr:datcat rdf:resource="http://www.isocat.org/datcat/DC-1357"/>
      <owl:versionInfo>http://www.isocat.org/datcat/DC-1357</owl:versionInfo>
      <rdfs:comment>
                            Determiner that expresses ownership.
                                (http://www.isocat.org/datcat/DC-1357)
                            </rdfs:comment>
      <rdfs:label>possessive determiner</rdfs:label>
      <rdfs:subClassOf>
         <owl:Class rdf:about="#determiner"/>
      </rdfs:subClassOf>
      <owl:versionInfo>subClassOf determiner (dcif:isA)</owl:versionInfo>
   </owl:Class>
   <owl:Class rdf:ID="possessiveParticle">
      <dcr:datcat rdf:resource="http://www.isocat.org/datcat/DC-1895"/>
      <owl:versionInfo>http://www.isocat.org/datcat/DC-1895</owl:versionInfo>
      <rdfs:comment>
                            Particle expressing ownship.
                                (http://www.isocat.org/datcat/DC-1895)
                            </rdfs:comment>
      <rdfs:label>possessive particle</rdfs:label>
      <rdfs:subClassOf>
         <owl:Class rdf:about="#particle"/>
      </rdfs:subClassOf>
      <owl:versionInfo>subClassOf particle (dcif:isA)</owl:versionInfo>
   </owl:Class>
   <owl:Class rdf:ID="possessivePronoun">
      <dcr:datcat rdf:resource="http://www.isocat.org/datcat/DC-1359"/>
      <owl:versionInfo>http://www.isocat.org/datcat/DC-1359</owl:versionInfo>
      <rdfs:comment>
                            Pronoun that expresses ownership and relationships like ownership, such as kinship, and other forms of association.
                                (www.sil.org/linguistics/GlossaryOfLinguisticTerms/WhatIsAPossessivePronoun.htm; http://www.isocat.org/datcat/DC-1359)
                            </rdfs:comment>
      <rdfs:label>possessive pronoun</rdfs:label>
      <rdfs:subClassOf>
         <owl:Class rdf:about="#pronoun"/>
      </rdfs:subClassOf>
      <owl:versionInfo>subClassOf pronoun (dcif:isA)</owl:versionInfo>
   </owl:Class>
   <owl:Class rdf:ID="possible">
      <dcr:datcat rdf:resource="http://www.isocat.org/datcat/DC-1865"/>
      <owl:versionInfo>http://www.isocat.org/datcat/DC-1865</owl:versionInfo>
      <rdfs:comment>
                            Value that denotes a linguistic situation considered as being correct in the given language
                                (http://www.isocat.org/datcat/DC-1865)
                            </rdfs:comment>
      <rdfs:label>possible</rdfs:label>
   </owl:Class>
   <owl:Class rdf:ID="postModifier">
      <dcr:datcat rdf:resource="http://www.isocat.org/datcat/DC-1945"/>
      <owl:versionInfo>http://www.isocat.org/datcat/DC-1945</owl:versionInfo>
      <rdfs:comment>
                            Situation where the modifier is after the modified.
                                (http://www.isocat.org/datcat/DC-1945)
                            </rdfs:comment>
      <rdfs:label>post modifier</rdfs:label>
      <rdfs:subClassOf>
         <owl:Class rdf:about="#modificationType"/>
      </rdfs:subClassOf>
      <owl:versionInfo>subClassOf modificationType (dcif:conceptualDomain)</owl:versionInfo>
   </owl:Class>
   <owl:Class rdf:ID="postposition">
      <dcr:datcat rdf:resource="http://www.isocat.org/datcat/DC-1360"/>
      <owl:versionInfo>http://www.isocat.org/datcat/DC-1360</owl:versionInfo>
      <rdfs:comment>
                            Adposition that appears at the end of the noun phrase.
                                (Gil Francopoulo; http://www.isocat.org/datcat/DC-1360)
                            </rdfs:comment>
      <rdfs:label>postposition</rdfs:label>
      <rdfs:subClassOf>
         <owl:Class rdf:about="#adposition"/>
      </rdfs:subClassOf>
      <owl:versionInfo>subClassOf adposition (dcif:isA)</owl:versionInfo>
   </owl:Class>
   <owl:Class rdf:ID="prefix">
      <dcr:datcat rdf:resource="http://www.isocat.org/datcat/DC-1365"/>
      <owl:versionInfo>http://www.isocat.org/datcat/DC-1365</owl:versionInfo>
      <rdfs:comment>
                            Affix added before a word to change its meaning or part of speech.
                                (Sue Ellen Wright + Gil Francopoulo; http://www.isocat.org/datcat/DC-1365)
                            </rdfs:comment>
      <rdfs:label>prefix</rdfs:label>
   </owl:Class>
   <owl:Class rdf:ID="preModifier">
      <dcr:datcat rdf:resource="http://www.isocat.org/datcat/DC-1943"/>
      <owl:versionInfo>http://www.isocat.org/datcat/DC-1943</owl:versionInfo>
      <rdfs:comment>
                            Situation where the modifier is before the modified.
                                (http://www.isocat.org/datcat/DC-1943)
                            </rdfs:comment>
      <rdfs:label>premodifier</rdfs:label>
      <rdfs:subClassOf>
         <owl:Class rdf:about="#modificationType"/>
      </rdfs:subClassOf>
      <owl:versionInfo>subClassOf modificationType (dcif:conceptualDomain)</owl:versionInfo>
   </owl:Class>
   <owl:Class rdf:ID="preposition">
      <dcr:datcat rdf:resource="http://www.isocat.org/datcat/DC-1366"/>
      <owl:versionInfo>http://www.isocat.org/datcat/DC-1366</owl:versionInfo>
      <rdfs:comment>
                            Adposition placed at the beginning of a noun phrase.
                                (http://www.isocat.org/datcat/DC-1366)
                            </rdfs:comment>
      <rdfs:label>preposition</rdfs:label>
      <rdfs:subClassOf>
         <owl:Class rdf:about="#adposition"/>
      </rdfs:subClassOf>
      <owl:versionInfo>subClassOf adposition (dcif:isA)</owl:versionInfo>
   </owl:Class>
   <owl:Class rdf:ID="present">
      <dcr:datcat rdf:resource="http://www.isocat.org/datcat/DC-1367"/>
      <owl:versionInfo>http://www.isocat.org/datcat/DC-1367</owl:versionInfo>
      <rdfs:comment>
                            Verb tense that indicates action or state of being in the present.
                                (www.southwestern.edu/~carlg/Latin_Web/glossary.html; http://www.isocat.org/datcat/DC-1367)
                            </rdfs:comment>
      <rdfs:label>present</rdfs:label>
      <rdfs:subClassOf>
         <owl:Class rdf:about="#grammaticalTense"/>
      </rdfs:subClassOf>
      <owl:versionInfo>subClassOf grammaticalTense (dcif:conceptualDomain)</owl:versionInfo>
   </owl:Class>
   <owl:Class rdf:ID="presentParticipleAdjective">
      <dcr:datcat rdf:resource="http://www.isocat.org/datcat/DC-1597"/>
      <owl:versionInfo>http://www.isocat.org/datcat/DC-1597</owl:versionInfo>
      <rdfs:comment>
                            Adjective based on a present participle.
                                (http://www.isocat.org/datcat/DC-1597)
                            </rdfs:comment>
      <rdfs:label>present participle adjective</rdfs:label>
      <rdfs:subClassOf>
         <owl:Class rdf:about="#participleAdjective"/>
      </rdfs:subClassOf>
      <owl:versionInfo>subClassOf participleAdjective (dcif:isA)</owl:versionInfo>
   </owl:Class>
   <owl:Class rdf:ID="preverbalParticleLmf">
      <dcr:datcat rdf:resource="http://www.isocat.org/datcat/DC-1455"/>
      <owl:versionInfo>http://www.isocat.org/datcat/DC-1455</owl:versionInfo>
   </owl:Class>
   <owl:Class rdf:ID="prolativeCase">
      <dcr:datcat rdf:resource="http://www.isocat.org/datcat/DC-1368"/>
      <owl:versionInfo>http://www.isocat.org/datcat/DC-1368</owl:versionInfo>
      <rdfs:comment>
                            Case for a noun or a pronoun that expresses motion within a place or a period of time needed for an event.
                                (http://www.isocat.org/datcat/DC-1368)
                            </rdfs:comment>
      <rdfs:label>prolative case</rdfs:label>
      <rdfs:subClassOf>
         <owl:Class rdf:about="#case"/>
      </rdfs:subClassOf>
      <owl:versionInfo>subClassOf case (dcif:conceptualDomain)</owl:versionInfo>
   </owl:Class>
   <owl:Class rdf:ID="pronoun">
      <dcr:datcat rdf:resource="http://www.isocat.org/datcat/DC-1370"/>
      <owl:versionInfo>http://www.isocat.org/datcat/DC-1370</owl:versionInfo>
      <rdfs:comment>
                            Word used in place of a noun or a noun phrase.
                                (http://www.isocat.org/datcat/DC-1370)
                            </rdfs:comment>
      <rdfs:label>pronoun</rdfs:label>
      <rdfs:subClassOf>
         <owl:Class rdf:about="#partOfSpeech"/>
      </rdfs:subClassOf>
      <owl:versionInfo>subClassOf partOfSpeech (dcif:conceptualDomain)</owl:versionInfo>
   </owl:Class>
   <owl:Class rdf:ID="properNoun">
      <dcr:datcat rdf:resource="http://www.isocat.org/datcat/DC-1371"/>
      <owl:versionInfo>http://www.isocat.org/datcat/DC-1371</owl:versionInfo>
      <rdfs:comment>
                            Noun that is the name of a specific individual, place, or object.
                                (www.sil.org/linguistics/GlossaryOfLinguisticTerms/WhatIsAProperNoun.htm; http://www.isocat.org/datcat/DC-1371)
                            </rdfs:comment>
      <rdfs:label>proper noun</rdfs:label>
      <rdfs:subClassOf>
         <owl:Class rdf:about="#noun"/>
      </rdfs:subClassOf>
      <owl:versionInfo>subClassOf noun (dcif:isA)</owl:versionInfo>
   </owl:Class>
   <owl:Class rdf:ID="punctuation">
      <dcr:datcat rdf:resource="http://www.isocat.org/datcat/DC-1372"/>
      <owl:versionInfo>http://www.isocat.org/datcat/DC-1372</owl:versionInfo>
      <rdfs:comment>
                            Graphical mark used either at word level to indicate an abbreviation or at a text level to separate phrases or sentences.
                                (http://www.isocat.org/datcat/DC-1372)
                            </rdfs:comment>
      <rdfs:label>punctuation</rdfs:label>
      <rdfs:subClassOf>
         <owl:Class rdf:about="#partOfSpeech"/>
      </rdfs:subClassOf>
      <owl:versionInfo>subClassOf partOfSpeech (dcif:conceptualDomain)</owl:versionInfo>
   </owl:Class>
   <owl:Class rdf:ID="quadrial">
      <dcr:datcat rdf:resource="http://www.isocat.org/datcat/DC-2000"/>
      <owl:versionInfo>http://www.isocat.org/datcat/DC-2000</owl:versionInfo>
      <rdfs:comment>
                            Property related to four elements.
                                (http://www.isocat.org/datcat/DC-2000)
                            </rdfs:comment>
      <rdfs:label>quadrial</rdfs:label>
      <rdfs:subClassOf>
         <owl:Class rdf:about="#grammaticalNumber"/>
      </rdfs:subClassOf>
      <owl:versionInfo>subClassOf grammaticalNumber (dcif:conceptualDomain)</owl:versionInfo>
   </owl:Class>
   <owl:Class rdf:ID="qualifierAdjective">
      <dcr:datcat rdf:resource="http://www.isocat.org/datcat/DC-1477"/>
      <owl:versionInfo>http://www.isocat.org/datcat/DC-1477</owl:versionInfo>
      <rdfs:comment>
                            Adjective used to qualify.
                                (http://www.isocat.org/datcat/DC-1477)
                            </rdfs:comment>
      <rdfs:label>qualifier adjective</rdfs:label>
      <rdfs:subClassOf>
         <owl:Class rdf:about="#adjective"/>
      </rdfs:subClassOf>
      <owl:versionInfo>subClassOf adjective (dcif:isA)</owl:versionInfo>
   </owl:Class>
   <owl:Class rdf:ID="questionMark">
      <dcr:datcat rdf:resource="http://www.isocat.org/datcat/DC-1444"/>
      <owl:versionInfo>http://www.isocat.org/datcat/DC-1444</owl:versionInfo>
      <rdfs:comment>
                            Sign used to express a question.
                                (http://www.isocat.org/datcat/DC-1444)
                            </rdfs:comment>
      <rdfs:label>interrogative point</rdfs:label>
      <rdfs:label>question mark</rdfs:label>
      <rdfs:subClassOf>
         <owl:Class rdf:about="#partOfSpeech"/>
      </rdfs:subClassOf>
      <owl:versionInfo>subClassOf partOfSpeech (dcif:conceptualDomain)</owl:versionInfo>
   </owl:Class>
   <owl:Class rdf:ID="quotative">
      <dcr:datcat rdf:resource="http://www.isocat.org/datcat/DC-1375"/>
      <owl:versionInfo>http://www.isocat.org/datcat/DC-1375</owl:versionInfo>
      <rdfs:comment>
                            The Quotative modality is used when the speakers evidence is based on second hand information.
                                (www.graywizard.net/Conlinguistics/amman_iar/ai_auxiliary_verb.htm#quotative/hearsay; http://www.isocat.org/datcat/DC-1375)
                            </rdfs:comment>
      <rdfs:label>quotative</rdfs:label>
   </owl:Class>
   <owl:Class rdf:ID="quote">
      <dcr:datcat rdf:resource="http://www.isocat.org/datcat/DC-2081"/>
      <owl:versionInfo>http://www.isocat.org/datcat/DC-2081</owl:versionInfo>
      <rdfs:comment>
                            Punctuation usually used to surround a quotation.
                                (http://www.isocat.org/datcat/DC-2081)
                            </rdfs:comment>
      <rdfs:label>quote</rdfs:label>
   </owl:Class>
   <owl:Class rdf:ID="rank">
      <dcr:datcat rdf:resource="http://www.isocat.org/datcat/DC-1862"/>
      <owl:versionInfo>http://www.isocat.org/datcat/DC-1862</owl:versionInfo>
      <rdfs:comment>
                            Reference to one specific element in an ordered list of elements
                                (Gil Francopoulo; http://www.isocat.org/datcat/DC-1862)
                            </rdfs:comment>
      <rdfs:label>rank</rdfs:label>
   </owl:Class>
   <owl:Class rdf:ID="rarelyUsed">
      <dcr:datcat rdf:resource="http://www.isocat.org/datcat/DC-1986"/>
      <owl:versionInfo>http://www.isocat.org/datcat/DC-1986</owl:versionInfo>
      <rdfs:comment>
                            Said of a term that is almost never used.
                                (ISO12620; http://www.isocat.org/datcat/DC-1986)
                            </rdfs:comment>
      <rdfs:label>rarely used</rdfs:label>
      <rdfs:subClassOf>
         <owl:Class rdf:about="#frequency"/>
      </rdfs:subClassOf>
      <owl:versionInfo>subClassOf frequency (dcif:conceptualDomain)</owl:versionInfo>
   </owl:Class>
   <owl:Class rdf:ID="reciprocalPronoun">
      <dcr:datcat rdf:resource="http://www.isocat.org/datcat/DC-1924"/>
      <owl:versionInfo>http://www.isocat.org/datcat/DC-1924</owl:versionInfo>
      <rdfs:comment>
                            Pronoun expressing mutual relationship.
                                (Gil Francopoulo; http://www.isocat.org/datcat/DC-1924)
                            </rdfs:comment>
      <rdfs:label>reciprocal pronoun</rdfs:label>
      <rdfs:subClassOf>
         <owl:Class rdf:about="#pronoun"/>
      </rdfs:subClassOf>
      <owl:versionInfo>subClassOf pronoun (dcif:isA)</owl:versionInfo>
   </owl:Class>
   <owl:Class rdf:ID="reduplication">
      <dcr:datcat rdf:resource="http://www.isocat.org/datcat/DC-2346"/>
      <owl:versionInfo>http://www.isocat.org/datcat/DC-2346</owl:versionInfo>
      <rdfs:comment>
                            process to modify the sense of a word by some operations to repeat the sound of a word.
                                (http://www.isocat.org/datcat/DC-2346)
                            </rdfs:comment>
      <rdfs:label>reduplication</rdfs:label>
   </owl:Class>
   <owl:Class rdf:ID="reduplicationType">
      <dcr:datcat rdf:resource="http://www.isocat.org/datcat/DC-2240"/>
      <owl:versionInfo>http://www.isocat.org/datcat/DC-2240</owl:versionInfo>
      <rdfs:comment>
                            type of reduplication
                                (http://www.isocat.org/datcat/DC-2240)
                            </rdfs:comment>
      <rdfs:label>reduplication type</rdfs:label>
   </owl:Class>
   <owl:Class rdf:ID="ref">
      <dcr:datcat rdf:resource="http://www.isocat.org/datcat/DC-2352"/>
      <owl:versionInfo>http://www.isocat.org/datcat/DC-2352</owl:versionInfo>
      <rdfs:comment>
                            reference to another description
                                (http://www.isocat.org/datcat/DC-2352)
                            </rdfs:comment>
      <rdfs:label>ref</rdfs:label>
   </owl:Class>
   <owl:Class rdf:ID="referentType">
      <dcr:datcat rdf:resource="http://www.isocat.org/datcat/DC-1376"/>
      <owl:versionInfo>http://www.isocat.org/datcat/DC-1376</owl:versionInfo>
      <rdfs:comment>
                            Type of concrete object or concept (the referent) that an expression represents (the reference).
                                (DFKI; http://www.isocat.org/datcat/DC-1376)
                            </rdfs:comment>
      <rdfs:label>referent type</rdfs:label>
   </owl:Class>
   <owl:Class rdf:ID="reflexiveDeterminer">
      <dcr:datcat rdf:resource="http://www.isocat.org/datcat/DC-1377"/>
      <owl:versionInfo>http://www.isocat.org/datcat/DC-1377</owl:versionInfo>
      <rdfs:comment>
                            Determiner that refers to the same entity.
                                (http://www.isocat.org/datcat/DC-1377)
                            </rdfs:comment>
      <rdfs:label>reflexive adjective</rdfs:label>
      <rdfs:subClassOf>
         <owl:Class rdf:about="#determiner"/>
      </rdfs:subClassOf>
      <owl:versionInfo>subClassOf determiner (dcif:isA)</owl:versionInfo>
   </owl:Class>
   <owl:Class rdf:ID="reflexivePronoun">
      <dcr:datcat rdf:resource="http://www.isocat.org/datcat/DC-1378"/>
      <owl:versionInfo>http://www.isocat.org/datcat/DC-1378</owl:versionInfo>
      <rdfs:comment>
                            Pronoun that refers to the subject of the sentence.
                                (www.southwestern.edu/~carlg/Latin_Web/glossary.html; http://www.isocat.org/datcat/DC-1378)
                            </rdfs:comment>
      <rdfs:label>reflexive pronoun</rdfs:label>
      <rdfs:subClassOf>
         <owl:Class rdf:about="#pronoun"/>
      </rdfs:subClassOf>
      <owl:versionInfo>subClassOf pronoun (dcif:isA)</owl:versionInfo>
   </owl:Class>
   <owl:Class rdf:ID="register">
      <dcr:datcat rdf:resource="http://www.isocat.org/datcat/DC-1988"/>
      <owl:versionInfo>http://www.isocat.org/datcat/DC-1988</owl:versionInfo>
      <rdfs:comment>
                            Classification indicating the relative level of language individually assigned to a lexeme or term or to a text type.
                                (ISO12620; http://www.isocat.org/datcat/DC-1988)
                            </rdfs:comment>
      <rdfs:label>register</rdfs:label>
   </owl:Class>
   <owl:Class rdf:ID="relationNoun">
      <dcr:datcat rdf:resource="http://www.isocat.org/datcat/DC-2226"/>
      <owl:versionInfo>http://www.isocat.org/datcat/DC-2226</owl:versionInfo>
      <rdfs:comment>
                            relation noun
                                (MIRACL &amp; LSCA; http://www.isocat.org/datcat/DC-2226)
                            </rdfs:comment>
      <rdfs:label>relation noun</rdfs:label>
      <rdfs:subClassOf>
         <owl:Class rdf:about="#partOfSpeech"/>
      </rdfs:subClassOf>
      <owl:versionInfo>subClassOf partOfSpeech (dcif:conceptualDomain)</owl:versionInfo>
   </owl:Class>
   <owl:Class rdf:ID="relativeDeterminer">
      <dcr:datcat rdf:resource="http://www.isocat.org/datcat/DC-1379"/>
      <owl:versionInfo>http://www.isocat.org/datcat/DC-1379</owl:versionInfo>
      <rdfs:comment>
                            Determiner related to a referent.
                                (http://www.isocat.org/datcat/DC-1379)
                            </rdfs:comment>
      <rdfs:label>relative determiner</rdfs:label>
      <rdfs:subClassOf>
         <owl:Class rdf:about="#determiner"/>
      </rdfs:subClassOf>
      <owl:versionInfo>subClassOf determiner (dcif:isA)</owl:versionInfo>
   </owl:Class>
   <owl:Class rdf:ID="relativeParticle">
      <dcr:datcat rdf:resource="http://www.isocat.org/datcat/DC-2229"/>
      <owl:versionInfo>http://www.isocat.org/datcat/DC-2229</owl:versionInfo>
      <rdfs:comment>
                            relative particle
                                (MIRACL &amp; LSCA; http://www.isocat.org/datcat/DC-2229)
                            </rdfs:comment>
      <rdfs:label>relative particle</rdfs:label>
      <rdfs:subClassOf>
         <owl:Class rdf:about="#particle"/>
      </rdfs:subClassOf>
      <owl:versionInfo>subClassOf particle (dcif:isA)</owl:versionInfo>
   </owl:Class>
   <owl:Class rdf:ID="relativePronoun">
      <dcr:datcat rdf:resource="http://www.isocat.org/datcat/DC-1380"/>
      <owl:versionInfo>http://www.isocat.org/datcat/DC-1380</owl:versionInfo>
      <rdfs:comment>
                            Pronoun which introduces a relative clause and refers to something that has been said before.
                                (www.southwestern.edu/~carlg/Latin_Web/glossary.html + Canoonet; http://www.isocat.org/datcat/DC-1380)
                            </rdfs:comment>
      <rdfs:label>relative pronoun</rdfs:label>
      <rdfs:subClassOf>
         <owl:Class rdf:about="#pronoun"/>
      </rdfs:subClassOf>
      <owl:versionInfo>subClassOf pronoun (dcif:isA)</owl:versionInfo>
   </owl:Class>
   <owl:Class rdf:ID="remove">
      <dcr:datcat rdf:resource="http://www.isocat.org/datcat/DC-2094"/>
      <owl:versionInfo>http://www.isocat.org/datcat/DC-2094</owl:versionInfo>
      <rdfs:comment>
                            Operation that remover N characters at position X.
                                (http://www.isocat.org/datcat/DC-2094)
                            </rdfs:comment>
      <rdfs:label>remove</rdfs:label>
   </owl:Class>
   <owl:Class rdf:ID="removeAfter">
      <dcr:datcat rdf:resource="http://www.isocat.org/datcat/DC-1830"/>
      <owl:versionInfo>http://www.isocat.org/datcat/DC-1830</owl:versionInfo>
      <rdfs:comment>
                            remove N characters from the right
                                (http://www.isocat.org/datcat/DC-1830)
                            </rdfs:comment>
      <rdfs:label>remove after</rdfs:label>
   </owl:Class>
   <owl:Class rdf:ID="removeBefore">
      <dcr:datcat rdf:resource="http://www.isocat.org/datcat/DC-1834"/>
      <owl:versionInfo>http://www.isocat.org/datcat/DC-1834</owl:versionInfo>
      <rdfs:comment>
                            Operation that removes N characters from the left
                                (http://www.isocat.org/datcat/DC-1834)
                            </rdfs:comment>
      <rdfs:label>remove before</rdfs:label>
   </owl:Class>
   <owl:Class rdf:ID="required">
      <dcr:datcat rdf:resource="http://www.isocat.org/datcat/DC-2239"/>
      <owl:versionInfo>http://www.isocat.org/datcat/DC-2239</owl:versionInfo>
      <rdfs:comment>
                            property concerning something that is mandatory
                                (http://www.isocat.org/datcat/DC-2239)
                            </rdfs:comment>
      <rdfs:label>required</rdfs:label>
   </owl:Class>
   <owl:Class rdf:ID="residual">
      <dcr:datcat rdf:resource="http://www.isocat.org/datcat/DC-1382"/>
      <owl:versionInfo>http://www.isocat.org/datcat/DC-1382</owl:versionInfo>
      <rdfs:comment>
                            The residual value is assigned to classes of textword which lie outside the traditionally accepted range of grammatical classes, although they occur quite commonly in many texts.
                                (www.ilc.cnr.it/EAGLES96/annotate/node16.html#cmobli; http://www.isocat.org/datcat/DC-1382)
                            </rdfs:comment>
      <rdfs:label>residual</rdfs:label>
   </owl:Class>
   <owl:Class rdf:ID="restriction">
      <dcr:datcat rdf:resource="http://www.isocat.org/datcat/DC-1956"/>
      <owl:versionInfo>http://www.isocat.org/datcat/DC-1956</owl:versionInfo>
      <rdfs:comment>
                            General purpose additional specification for a given type of limitation.
                                (Gil Francopoulo; http://www.isocat.org/datcat/DC-1956)
                            </rdfs:comment>
      <rdfs:label>restriction</rdfs:label>
   </owl:Class>
   <owl:Class rdf:ID="rightEnvironment">
      <dcr:datcat rdf:resource="http://www.isocat.org/datcat/DC-2195"/>
      <owl:versionInfo>http://www.isocat.org/datcat/DC-2195</owl:versionInfo>
      <rdfs:comment>
                            Right side from a particular point
                                (http://www.isocat.org/datcat/DC-2195)
                            </rdfs:comment>
      <rdfs:label>right environment</rdfs:label>
   </owl:Class>
   <owl:Class rdf:ID="romanization">
      <dcr:datcat rdf:resource="http://www.isocat.org/datcat/DC-1873"/>
      <owl:versionInfo>http://www.isocat.org/datcat/DC-1873</owl:versionInfo>
      <rdfs:comment>
                            Transcription or transliteration from non-Latin script into Latin script.
                                (Gil Francopoulo; http://www.isocat.org/datcat/DC-1873)
                            </rdfs:comment>
      <rdfs:label>romanization</rdfs:label>
   </owl:Class>
   <owl:Class rdf:ID="root">
      <dcr:datcat rdf:resource="http://www.isocat.org/datcat/DC-2231"/>
      <owl:versionInfo>http://www.isocat.org/datcat/DC-2231</owl:versionInfo>
      <rdfs:comment>
                            base of a word
                                (MIRACL &amp; LSCA; http://www.isocat.org/datcat/DC-2231)
                            </rdfs:comment>
      <rdfs:label>root</rdfs:label>
   </owl:Class>
   <owl:Class rdf:ID="rule">
      <dcr:datcat rdf:resource="http://www.isocat.org/datcat/DC-2180"/>
      <owl:versionInfo>http://www.isocat.org/datcat/DC-2180</owl:versionInfo>
      <rdfs:comment>
                            instruction that states how things are done or allowed
                                (Gil Francopoulo; http://www.isocat.org/datcat/DC-2180)
                            </rdfs:comment>
      <rdfs:label>rule</rdfs:label>
   </owl:Class>
   <owl:Class rdf:ID="scheme">
      <dcr:datcat rdf:resource="http://www.isocat.org/datcat/DC-2174"/>
      <owl:versionInfo>http://www.isocat.org/datcat/DC-2174</owl:versionInfo>
      <rdfs:comment>
                            Pattern for word creation
                                (http://www.isocat.org/datcat/DC-2174)
                            </rdfs:comment>
      <rdfs:label>scheme</rdfs:label>
   </owl:Class>
   <owl:Class rdf:ID="scope">
      <dcr:datcat rdf:resource="http://www.isocat.org/datcat/DC-2196"/>
      <owl:versionInfo>http://www.isocat.org/datcat/DC-2196</owl:versionInfo>
      <rdfs:comment>
                            Set of situations where a given property is valid
                                (http://www.isocat.org/datcat/DC-2196)
                            </rdfs:comment>
      <rdfs:label>scope</rdfs:label>
   </owl:Class>
   <owl:Class rdf:ID="script">
      <dcr:datcat rdf:resource="http://www.isocat.org/datcat/DC-1855"/>
      <owl:versionInfo>http://www.isocat.org/datcat/DC-1855</owl:versionInfo>
      <rdfs:comment>
                            Set of graphic characters used for the written form of one or more languages.
                                (ISO-IEC 10646-1, 4.14; http://www.isocat.org/datcat/DC-1855)
                            </rdfs:comment>
      <rdfs:label>script</rdfs:label>
   </owl:Class>
   <owl:Class rdf:ID="scriptCoding">
      <dcr:datcat rdf:resource="http://www.isocat.org/datcat/DC-2091"/>
      <owl:versionInfo>http://www.isocat.org/datcat/DC-2091</owl:versionInfo>
      <rdfs:comment>
                            Designation of the standard used to code the script.
                                (http://www.isocat.org/datcat/DC-2091)
                            </rdfs:comment>
      <rdfs:label>script coding</rdfs:label>
   </owl:Class>
   <owl:Class rdf:ID="secondPerson">
      <dcr:datcat rdf:resource="http://www.isocat.org/datcat/DC-1384"/>
      <owl:versionInfo>http://www.isocat.org/datcat/DC-1384</owl:versionInfo>
      <rdfs:comment>
                            Second person deixis is deictic reference to a person or persons identified as addressee.
                                (www.sil.org/linguistics/GlossaryOfLinguisticTerms/WhatIsSecondPersonDeixis.htm; http://www.isocat.org/datcat/DC-1384)
                            </rdfs:comment>
      <rdfs:label>second person</rdfs:label>
      <rdfs:subClassOf>
         <owl:Class rdf:about="#ownerPerson"/>
      </rdfs:subClassOf>
      <owl:versionInfo>subClassOf ownerPerson (dcif:conceptualDomain)</owl:versionInfo>
      <rdfs:subClassOf>
         <owl:Class rdf:about="#person"/>
      </rdfs:subClassOf>
      <owl:versionInfo>subClassOf person (dcif:conceptualDomain)</owl:versionInfo>
   </owl:Class>
   <owl:Class rdf:ID="secondaryPunctuation">
      <dcr:datcat rdf:resource="http://www.isocat.org/datcat/DC-2076"/>
      <owl:versionInfo>http://www.isocat.org/datcat/DC-2076</owl:versionInfo>
      <rdfs:comment>
                            Punctuation that is not very important with regards to sentence splitting in a text.
                                (http://www.isocat.org/datcat/DC-2076)
                            </rdfs:comment>
      <rdfs:label>secondary punctuation</rdfs:label>
      <rdfs:subClassOf>
         <owl:Class rdf:about="#punctuation"/>
      </rdfs:subClassOf>
      <owl:versionInfo>subClassOf punctuation (dcif:isA)</owl:versionInfo>
   </owl:Class>
   <owl:Class rdf:ID="semiColon">
      <dcr:datcat rdf:resource="http://www.isocat.org/datcat/DC-1446"/>
      <owl:versionInfo>http://www.isocat.org/datcat/DC-1446</owl:versionInfo>
      <rdfs:comment>
                            Sign (;) usually used to separate phrases.
                                (http://www.isocat.org/datcat/DC-1446)
                            </rdfs:comment>
      <rdfs:label>semi-colon</rdfs:label>
      <rdfs:subClassOf>
         <owl:Class rdf:about="#partOfSpeech"/>
      </rdfs:subClassOf>
      <owl:versionInfo>subClassOf partOfSpeech (dcif:conceptualDomain)</owl:versionInfo>
   </owl:Class>
   <owl:Class rdf:ID="shortArticle">
      <dcr:datcat rdf:resource="http://www.isocat.org/datcat/DC-1927"/>
      <owl:versionInfo>http://www.isocat.org/datcat/DC-1927</owl:versionInfo>
      <rdfs:comment>
                            For definiteness, when a specific form is not the syntactic subject of the clause.
                                (http://www.isocat.org/datcat/DC-1927)
                            </rdfs:comment>
      <rdfs:label>short article</rdfs:label>
      <rdfs:subClassOf>
         <owl:Class rdf:about="#definiteness"/>
      </rdfs:subClassOf>
      <owl:versionInfo>subClassOf definiteness (dcif:conceptualDomain)</owl:versionInfo>
   </owl:Class>
   <owl:Class rdf:ID="simplePreposition">
      <dcr:datcat rdf:resource="http://www.isocat.org/datcat/DC-1900"/>
      <owl:versionInfo>http://www.isocat.org/datcat/DC-1900</owl:versionInfo>
      <rdfs:comment>
                            Preposition that is a pure simple word in contrast with the notion of fused preposition.
                                (http://www.isocat.org/datcat/DC-1900)
                            </rdfs:comment>
      <rdfs:label>simple preposition</rdfs:label>
      <rdfs:subClassOf>
         <owl:Class rdf:about="#preposition"/>
      </rdfs:subClassOf>
      <owl:versionInfo>subClassOf preposition (dcif:isA)</owl:versionInfo>
   </owl:Class>
   <owl:Class rdf:ID="singular">
      <dcr:datcat rdf:resource="http://www.isocat.org/datcat/DC-1387"/>
      <owl:versionInfo>http://www.isocat.org/datcat/DC-1387</owl:versionInfo>
      <rdfs:comment>
                            Value that expresses one element.
                                (http://www.isocat.org/datcat/DC-1387)
                            </rdfs:comment>
      <rdfs:label>singular</rdfs:label>
      <rdfs:subClassOf>
         <owl:Class rdf:about="#grammaticalNumber"/>
      </rdfs:subClassOf>
      <owl:versionInfo>subClassOf grammaticalNumber (dcif:conceptualDomain)</owl:versionInfo>
      <rdfs:subClassOf>
         <owl:Class rdf:about="#ownerNumber"/>
      </rdfs:subClassOf>
      <owl:versionInfo>subClassOf ownerNumber (dcif:conceptualDomain)</owl:versionInfo>
   </owl:Class>
   <owl:Class rdf:ID="slangRegister">
      <dcr:datcat rdf:resource="http://www.isocat.org/datcat/DC-1995"/>
      <owl:versionInfo>http://www.isocat.org/datcat/DC-1995</owl:versionInfo>
      <rdfs:comment>
                            An extremely informal register of a word, term, or text that is used in spoken and everyday language and less commonly in documents.
                                (ISO12620; http://www.isocat.org/datcat/DC-1995)
                            </rdfs:comment>
      <rdfs:label>slang register</rdfs:label>
      <rdfs:subClassOf>
         <owl:Class rdf:about="#register"/>
      </rdfs:subClassOf>
      <owl:versionInfo>subClassOf register (dcif:conceptualDomain)</owl:versionInfo>
   </owl:Class>
   <owl:Class rdf:ID="slash">
      <dcr:datcat rdf:resource="http://www.isocat.org/datcat/DC-1437"/>
      <owl:versionInfo>http://www.isocat.org/datcat/DC-1437</owl:versionInfo>
      <rdfs:comment>
                            The punctuation sign /
                                (http://www.isocat.org/datcat/DC-1437)
                            </rdfs:comment>
      <rdfs:label>slash</rdfs:label>
      <rdfs:subClassOf>
         <owl:Class rdf:about="#partOfSpeech"/>
      </rdfs:subClassOf>
      <owl:versionInfo>subClassOf partOfSpeech (dcif:conceptualDomain)</owl:versionInfo>
   </owl:Class>
   <owl:Class rdf:ID="sociativeCase">
      <dcr:datcat rdf:resource="http://www.isocat.org/datcat/DC-1388"/>
      <owl:versionInfo>http://www.isocat.org/datcat/DC-1388</owl:versionInfo>
      <rdfs:comment>
                            Case related to the person in whose company the action is carried out, or to any belongings of people which take part in the action.
                                (http://en.wikipedia.org/wiki/Sociative_case; http://www.isocat.org/datcat/DC-1388)
                            </rdfs:comment>
      <rdfs:label>sociative case</rdfs:label>
      <rdfs:subClassOf>
         <owl:Class rdf:about="#case"/>
      </rdfs:subClassOf>
      <owl:versionInfo>subClassOf case (dcif:conceptualDomain)</owl:versionInfo>
   </owl:Class>
   <owl:Class rdf:ID="sound">
      <dcr:datcat rdf:resource="http://www.isocat.org/datcat/DC-2250"/>
      <owl:versionInfo>http://www.isocat.org/datcat/DC-2250</owl:versionInfo>
      <rdfs:comment>
                            pronunciation that is on a record
                                (http://www.isocat.org/datcat/DC-2250)
                            </rdfs:comment>
      <rdfs:label>sound</rdfs:label>
   </owl:Class>
   <owl:Class rdf:ID="source">
      <dcr:datcat rdf:resource="http://www.isocat.org/datcat/DC-1968"/>
      <owl:versionInfo>http://www.isocat.org/datcat/DC-1968</owl:versionInfo>
      <rdfs:comment>
                            A complete citation of the bibliographic information pertaining to a document or other resource.
                                (ISO12620; http://www.isocat.org/datcat/DC-1968)
                            </rdfs:comment>
      <rdfs:label>source</rdfs:label>
   </owl:Class>
   <owl:Class rdf:ID="space">
      <dcr:datcat rdf:resource="http://www.isocat.org/datcat/DC-2189"/>
      <owl:versionInfo>http://www.isocat.org/datcat/DC-2189</owl:versionInfo>
      <rdfs:comment>
                            Empty area between words, lines or columns
                                (http://www.isocat.org/datcat/DC-2189)
                            </rdfs:comment>
      <rdfs:label>space</rdfs:label>
   </owl:Class>
   <owl:Class rdf:ID="spacedPinyinAndTone">
      <dcr:datcat rdf:resource="http://www.isocat.org/datcat/DC-1854"/>
      <owl:versionInfo>http://www.isocat.org/datcat/DC-1854</owl:versionInfo>
      <rdfs:comment>
                            Pinyin with space and tone
                                (Gil Francopoulo; http://www.isocat.org/datcat/DC-1854)
                            </rdfs:comment>
      <rdfs:label>spaced pinyin and tone</rdfs:label>
   </owl:Class>
   <owl:Class rdf:ID="stem">
      <dcr:datcat rdf:resource="http://www.isocat.org/datcat/DC-1389"/>
      <owl:versionInfo>http://www.isocat.org/datcat/DC-1389</owl:versionInfo>
      <rdfs:comment>
                            Root of a word, together with any derivational affixes, to which inflectional affixes are added.
                                (www.sil.org/linguistics/GlossaryOfLinguisticTerms/WhatIsAStem.htm; http://www.isocat.org/datcat/DC-1389)
                            </rdfs:comment>
      <rdfs:label>stem</rdfs:label>
      <rdfs:label>base</rdfs:label>
      <rdfs:label>root</rdfs:label>
   </owl:Class>
   <owl:Class rdf:ID="stemRank">
      <dcr:datcat rdf:resource="http://www.isocat.org/datcat/DC-2186"/>
      <owl:versionInfo>http://www.isocat.org/datcat/DC-2186</owl:versionInfo>
      <rdfs:comment>
                            Rank of a stem
                                (http://www.isocat.org/datcat/DC-2186)
                            </rdfs:comment>
      <rdfs:label>stem rank</rdfs:label>
   </owl:Class>
   <owl:Class rdf:ID="stringValue">
      <dcr:datcat rdf:resource="http://www.isocat.org/datcat/DC-2182"/>
      <owl:versionInfo>http://www.isocat.org/datcat/DC-2182</owl:versionInfo>
      <rdfs:comment>
                            Character string to be interpreted in context
                                (http://www.isocat.org/datcat/DC-2182)
                            </rdfs:comment>
      <rdfs:label>string value</rdfs:label>
   </owl:Class>
   <owl:Class rdf:ID="strongPersonalPronoun">
      <dcr:datcat rdf:resource="http://www.isocat.org/datcat/DC-1390"/>
      <owl:versionInfo>http://www.isocat.org/datcat/DC-1390</owl:versionInfo>
      <rdfs:comment>
                            Personal pronoun that can occupy the position after a preposition and/or reinforce a weak personal pronoun.
                                (Eagles; http://www.isocat.org/datcat/DC-1390)
                            </rdfs:comment>
      <rdfs:label>strong personal pronoun</rdfs:label>
      <rdfs:subClassOf>
         <owl:Class rdf:about="#personalPronoun"/>
      </rdfs:subClassOf>
      <owl:versionInfo>subClassOf personalPronoun (dcif:isA)</owl:versionInfo>
   </owl:Class>
   <owl:Class rdf:ID="subjectPerson">
      <dcr:datcat rdf:resource="http://www.isocat.org/datcat/DC-2278"/>
      <owl:versionInfo>http://www.isocat.org/datcat/DC-2278</owl:versionInfo>
      <rdfs:comment>
                            person for the subject of the verb
                                (http://www.isocat.org/datcat/DC-2278)
                            </rdfs:comment>
      <rdfs:label>subject person</rdfs:label>
   </owl:Class>
   <owl:Class rdf:ID="subjunctive">
      <dcr:datcat rdf:resource="http://www.isocat.org/datcat/DC-1843"/>
      <owl:versionInfo>http://www.isocat.org/datcat/DC-1843</owl:versionInfo>
      <rdfs:comment>
                            Mood often used to express uncertainty, whishes or desires.
                                (http://www.isocat.org/datcat/DC-1843)
                            </rdfs:comment>
      <rdfs:label>subjunctive</rdfs:label>
      <rdfs:subClassOf>
         <owl:Class rdf:about="#verbFormMood"/>
      </rdfs:subClassOf>
      <owl:versionInfo>subClassOf verbFormMood (dcif:conceptualDomain)</owl:versionInfo>
   </owl:Class>
   <owl:Class rdf:ID="sublativeCase">
      <dcr:datcat rdf:resource="http://www.isocat.org/datcat/DC-1392"/>
      <owl:versionInfo>http://www.isocat.org/datcat/DC-1392</owl:versionInfo>
      <rdfs:comment>
                            Case for a move of something to the surface of another object.
                                (www.hungarotips.com/hungarian/i/fonev1.html; http://www.isocat.org/datcat/DC-1392)
                            </rdfs:comment>
      <rdfs:label>sublative case</rdfs:label>
      <rdfs:subClassOf>
         <owl:Class rdf:about="#case"/>
      </rdfs:subClassOf>
      <owl:versionInfo>subClassOf case (dcif:conceptualDomain)</owl:versionInfo>
   </owl:Class>
   <owl:Class rdf:ID="subordinatingConjunction">
      <dcr:datcat rdf:resource="http://www.isocat.org/datcat/DC-1393"/>
      <owl:versionInfo>http://www.isocat.org/datcat/DC-1393</owl:versionInfo>
      <rdfs:comment>
                            Conjunction that links constructions by making one of them a constituent of another. The subordinating conjunction typically marks the incorporated constituent.
                                (www.sil.org/linguistics/GlossaryOfLinguisticTerms/WhatIsASubordinatingConjunctio.htm; http://www.isocat.org/datcat/DC-1393)
                            </rdfs:comment>
      <rdfs:label>subordinating conjunction</rdfs:label>
      <rdfs:subClassOf>
         <owl:Class rdf:about="#conjunction"/>
      </rdfs:subClassOf>
      <owl:versionInfo>subClassOf conjunction (dcif:isA)</owl:versionInfo>
   </owl:Class>
   <owl:Class rdf:ID="substitute">
      <dcr:datcat rdf:resource="http://www.isocat.org/datcat/DC-1832"/>
      <owl:versionInfo>http://www.isocat.org/datcat/DC-1832</owl:versionInfo>
      <rdfs:comment>
                            Operation that replaces N characters at position X by a string
                                (http://www.isocat.org/datcat/DC-1832)
                            </rdfs:comment>
      <rdfs:label>substitute</rdfs:label>
   </owl:Class>
   <owl:Class rdf:ID="suffix">
      <dcr:datcat rdf:resource="http://www.isocat.org/datcat/DC-1395"/>
      <owl:versionInfo>http://www.isocat.org/datcat/DC-1395</owl:versionInfo>
      <rdfs:comment>
                            Affix added at the end of the word to change its meaning or part of speech.
                                (Sue Ellen Wright + Gil Francopoulo; http://www.isocat.org/datcat/DC-1395)
                            </rdfs:comment>
      <rdfs:label>suffix</rdfs:label>
   </owl:Class>
   <owl:Class rdf:ID="superessiveCase">
      <dcr:datcat rdf:resource="http://www.isocat.org/datcat/DC-1396"/>
      <owl:versionInfo>http://www.isocat.org/datcat/DC-1396</owl:versionInfo>
      <rdfs:comment>
                            Case indicating location on top of something or on the surface of something.
                                (http://en.wikipedia.org/wiki/Superessive_case; http://www.isocat.org/datcat/DC-1396)
                            </rdfs:comment>
      <rdfs:label>superessive case</rdfs:label>
      <rdfs:subClassOf>
         <owl:Class rdf:about="#case"/>
      </rdfs:subClassOf>
      <owl:versionInfo>subClassOf case (dcif:conceptualDomain)</owl:versionInfo>
   </owl:Class>
   <owl:Class rdf:ID="superlative">
      <dcr:datcat rdf:resource="http://www.isocat.org/datcat/DC-1422"/>
      <owl:versionInfo>http://www.isocat.org/datcat/DC-1422</owl:versionInfo>
      <rdfs:comment>
                            Value used in a comparison between more than two entities.
                                (http://www.isocat.org/datcat/DC-1422)
                            </rdfs:comment>
      <rdfs:label>superlative</rdfs:label>
      <rdfs:subClassOf>
         <owl:Class rdf:about="#degree"/>
      </rdfs:subClassOf>
      <owl:versionInfo>subClassOf degree (dcif:conceptualDomain)</owl:versionInfo>
   </owl:Class>
   <owl:Class rdf:ID="superlativeParticle">
      <dcr:datcat rdf:resource="http://www.isocat.org/datcat/DC-1923"/>
      <owl:versionInfo>http://www.isocat.org/datcat/DC-1923</owl:versionInfo>
      <rdfs:comment>
                            Particle expressing superlative degree. Superlative is the comparison between more than two entities and contrasts with comparative where only two entities are involved and positive where no comparison is implied.
                                (Crystal 2003; http://www.isocat.org/datcat/DC-1923)
                            </rdfs:comment>
      <rdfs:label>superlative particle</rdfs:label>
      <rdfs:subClassOf>
         <owl:Class rdf:about="#particle"/>
      </rdfs:subClassOf>
      <owl:versionInfo>subClassOf particle (dcif:isA)</owl:versionInfo>
   </owl:Class>
   <owl:Class rdf:ID="suspensionPoints">
      <dcr:datcat rdf:resource="http://www.isocat.org/datcat/DC-1447"/>
      <owl:versionInfo>http://www.isocat.org/datcat/DC-1447</owl:versionInfo>
      <rdfs:comment>
                            Sequence of three dots having the same meaning as "et cetera" (full form) or "etc" (abbreviated form).
                                (http://www.isocat.org/datcat/DC-1447)
                            </rdfs:comment>
      <rdfs:label>suspension points</rdfs:label>
      <rdfs:subClassOf>
         <owl:Class rdf:about="#partOfSpeech"/>
      </rdfs:subClassOf>
      <owl:versionInfo>subClassOf partOfSpeech (dcif:conceptualDomain)</owl:versionInfo>
   </owl:Class>
   <owl:Class rdf:ID="symbol">
      <dcr:datcat rdf:resource="http://www.isocat.org/datcat/DC-1398"/>
      <owl:versionInfo>http://www.isocat.org/datcat/DC-1398</owl:versionInfo>
      <rdfs:comment>
                            A non-splittable sequence of letters, numbers or signs that represents a particular meaning.
                                (Gil Francopoulo; http://www.isocat.org/datcat/DC-1398)
                            </rdfs:comment>
      <rdfs:label>symbol</rdfs:label>
   </owl:Class>
   <owl:Class rdf:ID="syntacticType">
      <dcr:datcat rdf:resource="http://www.isocat.org/datcat/DC-1948"/>
      <owl:versionInfo>http://www.isocat.org/datcat/DC-1948</owl:versionInfo>
      <rdfs:comment>
                            Type of part of speech.
                                (Multext-East; http://www.isocat.org/datcat/DC-1948)
                            </rdfs:comment>
      <rdfs:label>syntactic type</rdfs:label>
   </owl:Class>
   <owl:Class rdf:ID="tabooRegister">
      <dcr:datcat rdf:resource="http://www.isocat.org/datcat/DC-1996"/>
      <owl:versionInfo>http://www.isocat.org/datcat/DC-1996</owl:versionInfo>
      <rdfs:comment>
                            Register that expresses a situation that people avoid because it is extremely offensive or embarrassing.
                                (ISO12620; http://www.isocat.org/datcat/DC-1996)
                            </rdfs:comment>
      <rdfs:label>taboo register</rdfs:label>
      <rdfs:subClassOf>
         <owl:Class rdf:about="#register"/>
      </rdfs:subClassOf>
      <owl:versionInfo>subClassOf register (dcif:conceptualDomain)</owl:versionInfo>
   </owl:Class>
   <owl:Class rdf:ID="technicalRegister">
      <dcr:datcat rdf:resource="http://www.isocat.org/datcat/DC-1997"/>
      <owl:versionInfo>http://www.isocat.org/datcat/DC-1997</owl:versionInfo>
      <rdfs:comment>
                            The register appropriate to scientific texts or special languages.
                                (ISO12620; http://www.isocat.org/datcat/DC-1997)
                            </rdfs:comment>
      <rdfs:label>technical register</rdfs:label>
      <rdfs:subClassOf>
         <owl:Class rdf:about="#register"/>
      </rdfs:subClassOf>
      <owl:versionInfo>subClassOf register (dcif:conceptualDomain)</owl:versionInfo>
   </owl:Class>
   <owl:Class rdf:ID="grammaticalTense">
      <dcr:datcat rdf:resource="http://www.isocat.org/datcat/DC-1286"/>
      <owl:versionInfo>http://www.isocat.org/datcat/DC-1286</owl:versionInfo>
      <rdfs:comment>
                            Property referring to the way the grammar marks the time at which the action denoted by the verb took place.
                                (Crystal 2003; http://www.isocat.org/datcat/DC-1286)
                            </rdfs:comment>
      <rdfs:label>tense</rdfs:label>
   </owl:Class>
   <owl:Class rdf:ID="terminativeCase">
      <dcr:datcat rdf:resource="http://www.isocat.org/datcat/DC-1401"/>
      <owl:versionInfo>http://www.isocat.org/datcat/DC-1401</owl:versionInfo>
      <rdfs:comment>
                            Case that indicates to what or where something ends.
                                (http://en.wikipedia.org/wiki/Terminative_case; http://www.isocat.org/datcat/DC-1401)
                            </rdfs:comment>
      <rdfs:label>terminative case</rdfs:label>
      <rdfs:subClassOf>
         <owl:Class rdf:about="#case"/>
      </rdfs:subClassOf>
      <owl:versionInfo>subClassOf case (dcif:conceptualDomain)</owl:versionInfo>
   </owl:Class>
   <owl:Class rdf:ID="text">
      <dcr:datcat rdf:resource="http://www.isocat.org/datcat/DC-1847"/>
      <owl:versionInfo>http://www.isocat.org/datcat/DC-1847</owl:versionInfo>
      <rdfs:comment>
                            Series of sentences expressed in a natural language.
                                (Gil Francopoulo; http://www.isocat.org/datcat/DC-1847)
                            </rdfs:comment>
      <rdfs:label>text</rdfs:label>
   </owl:Class>
   <owl:Class rdf:ID="thirdPerson">
      <dcr:datcat rdf:resource="http://www.isocat.org/datcat/DC-1402"/>
      <owl:versionInfo>http://www.isocat.org/datcat/DC-1402</owl:versionInfo>
      <rdfs:comment>
                            Third person deixis is deictic reference to a referent(s) not identified as the speaker or addressee.
                                (www.sil.org/linguistics/GlossaryOfLinguisticTerms/WhatIsThirdPersonDeixis.htm; http://www.isocat.org/datcat/DC-1402)
                            </rdfs:comment>
      <rdfs:label>third person</rdfs:label>
      <rdfs:subClassOf>
         <owl:Class rdf:about="#ownerPerson"/>
      </rdfs:subClassOf>
      <owl:versionInfo>subClassOf ownerPerson (dcif:conceptualDomain)</owl:versionInfo>
      <rdfs:subClassOf>
         <owl:Class rdf:about="#person"/>
      </rdfs:subClassOf>
      <owl:versionInfo>subClassOf person (dcif:conceptualDomain)</owl:versionInfo>
   </owl:Class>
   <owl:Class rdf:ID="token">
      <dcr:datcat rdf:resource="http://www.isocat.org/datcat/DC-1403"/>
      <owl:versionInfo>http://www.isocat.org/datcat/DC-1403</owl:versionInfo>
      <rdfs:comment>
                            Character string surrounded by separators.
                                (Gil Francopoulo; http://www.isocat.org/datcat/DC-1403)
                            </rdfs:comment>
      <rdfs:label>token</rdfs:label>
   </owl:Class>
   <owl:Class rdf:ID="transcription">
      <dcr:datcat rdf:resource="http://www.isocat.org/datcat/DC-1849"/>
      <owl:versionInfo>http://www.isocat.org/datcat/DC-1849</owl:versionInfo>
      <rdfs:comment>
                            Form resulting from a coherent method of writing down speech sounds
                                (http://www.isocat.org/datcat/DC-1849)
                            </rdfs:comment>
      <rdfs:label>transcription</rdfs:label>
   </owl:Class>
   <owl:Class rdf:ID="transformType">
      <dcr:datcat rdf:resource="http://www.isocat.org/datcat/DC-2181"/>
      <owl:versionInfo>http://www.isocat.org/datcat/DC-2181</owl:versionInfo>
      <rdfs:comment>
                            Type of transformation
                                (http://www.isocat.org/datcat/DC-2181)
                            </rdfs:comment>
      <rdfs:label>transform type</rdfs:label>
   </owl:Class>
   <owl:Class rdf:ID="translativeCase">
      <dcr:datcat rdf:resource="http://www.isocat.org/datcat/DC-1406"/>
      <owl:versionInfo>http://www.isocat.org/datcat/DC-1406</owl:versionInfo>
      <rdfs:comment>
                            Case indicating that the referent of the noun, or the quality of the adjective, that it marks is the result of a process of change.
                                (SIL; http://www.isocat.org/datcat/DC-1406)
                            </rdfs:comment>
      <rdfs:label>translative case</rdfs:label>
      <rdfs:subClassOf>
         <owl:Class rdf:about="#case"/>
      </rdfs:subClassOf>
      <owl:versionInfo>subClassOf case (dcif:conceptualDomain)</owl:versionInfo>
   </owl:Class>
   <owl:Class rdf:ID="transliteration">
      <dcr:datcat rdf:resource="http://www.isocat.org/datcat/DC-1848"/>
      <owl:versionInfo>http://www.isocat.org/datcat/DC-1848</owl:versionInfo>
      <rdfs:comment>
                            Form resulting from the conversion of one writing system into another
                                (http://www.isocat.org/datcat/DC-1848)
                            </rdfs:comment>
      <rdfs:label>transliteration</rdfs:label>
   </owl:Class>
   <owl:Class rdf:ID="trial">
      <dcr:datcat rdf:resource="http://www.isocat.org/datcat/DC-1407"/>
      <owl:versionInfo>http://www.isocat.org/datcat/DC-1407</owl:versionInfo>
      <rdfs:comment>
                            Grammatical number referring to 'three things', as opposed to 'singular' and 'plural'.
                                (en2.wikipedia.org/wiki/Trial_number; http://www.isocat.org/datcat/DC-1407)
                            </rdfs:comment>
      <rdfs:label>trial</rdfs:label>
      <rdfs:subClassOf>
         <owl:Class rdf:about="#grammaticalNumber"/>
      </rdfs:subClassOf>
      <owl:versionInfo>subClassOf grammaticalNumber (dcif:conceptualDomain)</owl:versionInfo>
   </owl:Class>
   <owl:Class rdf:ID="type">
      <dcr:datcat rdf:resource="http://www.isocat.org/datcat/DC-1971"/>
      <owl:versionInfo>http://www.isocat.org/datcat/DC-1971</owl:versionInfo>
      <rdfs:comment>
                            One member of a group of people or things that have similar features or qualities.
                                (Longma dictionary contemporay English 2005; http://www.isocat.org/datcat/DC-1971)
                            </rdfs:comment>
      <rdfs:label>type</rdfs:label>
   </owl:Class>
   <owl:Class rdf:ID="unaccomplished">
      <dcr:datcat rdf:resource="http://www.isocat.org/datcat/DC-2217"/>
      <owl:versionInfo>http://www.isocat.org/datcat/DC-2217</owl:versionInfo>
      <rdfs:comment>
                            aspect that expresses an event or state that is not finished.
                                (http://www.isocat.org/datcat/DC-2217)
                            </rdfs:comment>
      <rdfs:label>unaccomplished</rdfs:label>
      <rdfs:subClassOf>
         <owl:Class rdf:about="#aspect"/>
      </rdfs:subClassOf>
      <owl:versionInfo>subClassOf aspect (dcif:conceptualDomain)</owl:versionInfo>
   </owl:Class>
   <owl:Class rdf:ID="unclassifiedParticle">
      <dcr:datcat rdf:resource="http://www.isocat.org/datcat/DC-1897"/>
      <owl:versionInfo>http://www.isocat.org/datcat/DC-1897</owl:versionInfo>
      <rdfs:comment>
                            Particle that is not covered by other sorts of particle definitions.
                                (http://www.isocat.org/datcat/DC-1897)
                            </rdfs:comment>
      <rdfs:label>unclassified particle</rdfs:label>
      <rdfs:subClassOf>
         <owl:Class rdf:about="#particle"/>
      </rdfs:subClassOf>
      <owl:versionInfo>subClassOf particle (dcif:isA)</owl:versionInfo>
   </owl:Class>
   <owl:Class rdf:ID="unclassifiedPunctuation">
      <dcr:datcat rdf:resource="http://www.isocat.org/datcat/DC-2080"/>
      <owl:versionInfo>http://www.isocat.org/datcat/DC-2080</owl:versionInfo>
      <rdfs:comment>
                            Punctuation that cannot fit in the other sorts of punctuations.
                                (http://www.isocat.org/datcat/DC-2080)
                            </rdfs:comment>
      <rdfs:label>unclassified punctuation</rdfs:label>
      <rdfs:subClassOf>
         <owl:Class rdf:about="#punctuation"/>
      </rdfs:subClassOf>
      <owl:versionInfo>subClassOf punctuation (dcif:isA)</owl:versionInfo>
   </owl:Class>
   <owl:Class rdf:ID="unclassifiedResidual">
      <dcr:datcat rdf:resource="http://www.isocat.org/datcat/DC-1891"/>
      <owl:versionInfo>http://www.isocat.org/datcat/DC-1891</owl:versionInfo>
      <rdfs:comment>
                            Part of speech not covered by all other definitions.
                                (http://www.isocat.org/datcat/DC-1891)
                            </rdfs:comment>
      <rdfs:label>unclassified residual</rdfs:label>
   </owl:Class>
   <owl:Class rdf:ID="unspecified">
      <dcr:datcat rdf:resource="http://www.isocat.org/datcat/DC-1908"/>
      <owl:versionInfo>http://www.isocat.org/datcat/DC-1908</owl:versionInfo>
      <rdfs:comment>
                            Value that expresses the absence of specification.
                                (http://www.isocat.org/datcat/DC-1908)
                            </rdfs:comment>
      <rdfs:label>unspecified</rdfs:label>
   </owl:Class>
   <owl:Class rdf:ID="utterance">
      <dcr:datcat rdf:resource="http://www.isocat.org/datcat/DC-1409"/>
      <owl:versionInfo>http://www.isocat.org/datcat/DC-1409</owl:versionInfo>
      <rdfs:comment>
                            Complete unit of talk, bounded by the speaker's silence.
                                (www.sil.org/linguistics/GlossaryOfLinguisticTerms/WhatIsAnUtterance.htm; http://www.isocat.org/datcat/DC-1409)
                            </rdfs:comment>
      <rdfs:label>utterance</rdfs:label>
   </owl:Class>
   <owl:Class rdf:ID="value">
      <dcr:datcat rdf:resource="http://www.isocat.org/datcat/DC-1978"/>
      <owl:versionInfo>http://www.isocat.org/datcat/DC-1978</owl:versionInfo>
      <rdfs:comment>
                            Generic name for a value.
                                (http://www.isocat.org/datcat/DC-1978)
                            </rdfs:comment>
      <rdfs:label>value</rdfs:label>
   </owl:Class>
   <owl:Class rdf:ID="variation">
      <dcr:datcat rdf:resource="http://www.isocat.org/datcat/DC-2177"/>
      <owl:versionInfo>http://www.isocat.org/datcat/DC-2177</owl:versionInfo>
      <rdfs:comment>
                            Difference between similar objects
                                (http://www.isocat.org/datcat/DC-2177)
                            </rdfs:comment>
      <rdfs:label>variation</rdfs:label>
   </owl:Class>
   <owl:Class rdf:ID="verb">
      <dcr:datcat rdf:resource="http://www.isocat.org/datcat/DC-1424"/>
      <owl:versionInfo>http://www.isocat.org/datcat/DC-1424</owl:versionInfo>
      <rdfs:comment>
                            Element which, singly or in combination with other verbs is used as the minimal predicate of a sentence, co-occurring with a subject. If the predicate contains other elements (e.g. object, complement), then it is the verb which more than any other is the unit which influences the choice and extent of these elements.
                                (Crystal 2003; http://www.isocat.org/datcat/DC-1424)
                            </rdfs:comment>
      <rdfs:label>verb</rdfs:label>
      <rdfs:subClassOf>
         <owl:Class rdf:about="#partOfSpeech"/>
      </rdfs:subClassOf>
      <owl:versionInfo>subClassOf partOfSpeech (dcif:conceptualDomain)</owl:versionInfo>
   </owl:Class>
   <owl:Class rdf:ID="verbFormMood">
      <dcr:datcat rdf:resource="http://www.isocat.org/datcat/DC-1427"/>
      <owl:versionInfo>http://www.isocat.org/datcat/DC-1427</owl:versionInfo>
      <rdfs:comment>
                            One of a set of distinctive forms that are used to signal modality. Modality is a facet of illocutionary point or general intent of a speaker, or a speaker's degree of commitment to the expressed proposition's believability, obligatoriness, desirability or reality.
                                (ISO12620; http://www.isocat.org/datcat/DC-1427)
                            </rdfs:comment>
      <rdfs:label>verb form mood</rdfs:label>
   </owl:Class>
   <owl:Class rdf:ID="view">
      <dcr:datcat rdf:resource="http://www.isocat.org/datcat/DC-1970"/>
      <owl:versionInfo>http://www.isocat.org/datcat/DC-1970</owl:versionInfo>
      <rdfs:comment>
                            Way of thinking about or understanding something.
                                (Longman dictionary of contemporary English 2005; http://www.isocat.org/datcat/DC-1970)
                            </rdfs:comment>
      <rdfs:label>view</rdfs:label>
   </owl:Class>
   <owl:Class rdf:ID="vocativeCase">
      <dcr:datcat rdf:resource="http://www.isocat.org/datcat/DC-1412"/>
      <owl:versionInfo>http://www.isocat.org/datcat/DC-1412</owl:versionInfo>
      <rdfs:comment>
                            Case used to indicate direct address.
                                (www.southwestern.edu/~carlg/Latin_Web/glossary.html; http://www.isocat.org/datcat/DC-1412)
                            </rdfs:comment>
      <rdfs:label>vocative case</rdfs:label>
      <rdfs:subClassOf>
         <owl:Class rdf:about="#case"/>
      </rdfs:subClassOf>
      <owl:versionInfo>subClassOf case (dcif:conceptualDomain)</owl:versionInfo>
   </owl:Class>
   <owl:Class rdf:ID="voice">
      <dcr:datcat rdf:resource="http://www.isocat.org/datcat/DC-1413"/>
      <owl:versionInfo>http://www.isocat.org/datcat/DC-1413</owl:versionInfo>
      <rdfs:comment>
                            Way sentences may alter the relationship between the subject and object of a verb, without changing the meaning of the sentence.
                                (Crystal 2003; http://www.isocat.org/datcat/DC-1413)
                            </rdfs:comment>
      <rdfs:label>voice</rdfs:label>
   </owl:Class>
   <owl:Class rdf:ID="voiceNoun">
      <dcr:datcat rdf:resource="http://www.isocat.org/datcat/DC-2253"/>
      <owl:versionInfo>http://www.isocat.org/datcat/DC-2253</owl:versionInfo>
      <rdfs:comment>
                            noun of a voice
                                (http://www.isocat.org/datcat/DC-2253)
                            </rdfs:comment>
      <rdfs:label>voice noun</rdfs:label>
      <rdfs:subClassOf>
         <owl:Class rdf:about="#partOfSpeech"/>
      </rdfs:subClassOf>
      <owl:versionInfo>subClassOf partOfSpeech (dcif:conceptualDomain)</owl:versionInfo>
   </owl:Class>
   <owl:Class rdf:ID="vulgarRegister">
      <dcr:datcat rdf:resource="http://www.isocat.org/datcat/DC-1998"/>
      <owl:versionInfo>http://www.isocat.org/datcat/DC-1998</owl:versionInfo>
      <rdfs:comment>
                            Register of a term or text type that can be characterized as profane or socially unacceptable.
                                (ISO12620; http://www.isocat.org/datcat/DC-1998)
                            </rdfs:comment>
      <rdfs:label>vulgar register</rdfs:label>
      <rdfs:subClassOf>
         <owl:Class rdf:about="#register"/>
      </rdfs:subClassOf>
      <owl:versionInfo>subClassOf register (dcif:conceptualDomain)</owl:versionInfo>
   </owl:Class>
   <owl:Class rdf:ID="weakPersonalPronoun">
      <dcr:datcat rdf:resource="http://www.isocat.org/datcat/DC-1414"/>
      <owl:versionInfo>http://www.isocat.org/datcat/DC-1414</owl:versionInfo>
      <rdfs:comment>
                            Personal pronoun that cannot occupy the position after a preposition and/or reinforce a strong personal pronoun.
                                (http://www.isocat.org/datcat/DC-1414)
                            </rdfs:comment>
      <rdfs:label>weak personal pronoun</rdfs:label>
      <rdfs:subClassOf>
         <owl:Class rdf:about="#personalPronoun"/>
      </rdfs:subClassOf>
      <owl:versionInfo>subClassOf personalPronoun (dcif:isA)</owl:versionInfo>
   </owl:Class>
   <owl:Class rdf:ID="word">
      <dcr:datcat rdf:resource="http://www.isocat.org/datcat/DC-1415"/>
      <owl:versionInfo>http://www.isocat.org/datcat/DC-1415</owl:versionInfo>
      <rdfs:comment>
                            Linguistic unit composed of at least a part of speech and a lemma.
                                (Gil Francopoulo; http://www.isocat.org/datcat/DC-1415)
                            </rdfs:comment>
      <rdfs:label>word</rdfs:label>
   </owl:Class>
   <owl:Class rdf:ID="writtenForm">
      <dcr:datcat rdf:resource="http://www.isocat.org/datcat/DC-1836"/>
      <owl:versionInfo>http://www.isocat.org/datcat/DC-1836</owl:versionInfo>
      <rdfs:comment>
                            Representation of the written string of a form
                                (http://www.isocat.org/datcat/DC-1836)
                            </rdfs:comment>
      <rdfs:label>written form</rdfs:label>
   </owl:Class>
   <owl:Class rdf:ID="yes">
      <dcr:datcat rdf:resource="http://www.isocat.org/datcat/DC-1904"/>
      <owl:versionInfo>http://www.isocat.org/datcat/DC-1904</owl:versionInfo>
      <rdfs:comment>
                            Positive value
                                (http://www.isocat.org/datcat/DC-1904)
                            </rdfs:comment>
      <rdfs:label>yes</rdfs:label>
      <rdfs:subClassOf>
         <owl:Class rdf:about="#cliticness"/>
      </rdfs:subClassOf>
      <owl:versionInfo>subClassOf cliticness (dcif:conceptualDomain)</owl:versionInfo>
      <rdfs:subClassOf>
         <owl:Class rdf:about="#negative"/>
      </rdfs:subClassOf>
      <owl:versionInfo>subClassOf negative (dcif:conceptualDomain)</owl:versionInfo>
      <rdfs:subClassOf>
         <owl:Class rdf:about="#zuInclusion"/>
      </rdfs:subClassOf>
      <owl:versionInfo>subClassOf zuInclusion (dcif:conceptualDomain)</owl:versionInfo>
   </owl:Class>
   <owl:Class rdf:ID="zuInclusion">
      <dcr:datcat rdf:resource="http://www.isocat.org/datcat/DC-1954"/>
      <owl:versionInfo>http://www.isocat.org/datcat/DC-1954</owl:versionInfo>
      <rdfs:comment>
                            Inclusion of zu.
                                (DFKI; http://www.isocat.org/datcat/DC-1954)
                            </rdfs:comment>
      <rdfs:label>zu inclusion</rdfs:label>
   </owl:Class>
</rdf:RDF>