<?xml version="1.0" encoding="UTF-8"?>
<rdf:RDF xmlns:rdfs="http://www.w3.org/2000/01/rdf-schema#"
         xmlns:dcr="http://www.isocat.org/ns/dcr.rdf#"
         xmlns:rdf="http://www.w3.org/1999/02/22-rdf-syntax-ns#">
   <owl:Ontology xmlns:owl="http://www.w3.org/2002/07/owl#">
      <rdfs:comment>OWL representation of ISOcat RDF exported Data Categories</rdfs:comment>
   </owl:Ontology>
   <owl:Class xmlns:owl="http://www.w3.org/2002/07/owl#" rdf:about="#adjective">
      <rdfs:comment>subClassOf partOfSpeech inferred from rdfs:comment.</rdfs:comment>
      <rdfs:subClassOf>
         <owl:Class rdf:about="#partOfSpeech"/>
      </rdfs:subClassOf>
   </owl:Class>
   <owl:Class xmlns:owl="http://www.w3.org/2002/07/owl#" rdf:about="#adposition">
      <rdfs:comment>subClassOf partOfSpeech inferred from rdfs:comment.</rdfs:comment>
      <rdfs:subClassOf>
         <owl:Class rdf:about="#partOfSpeech"/>
      </rdfs:subClassOf>
   </owl:Class>
   <owl:Class xmlns:owl="http://www.w3.org/2002/07/owl#" rdf:about="#adverb">
      <rdfs:comment>subClassOf partOfSpeech inferred from rdfs:comment.</rdfs:comment>
      <rdfs:subClassOf>
         <owl:Class rdf:about="#partOfSpeech"/>
      </rdfs:subClassOf>
   </owl:Class>
   <owl:Class xmlns:owl="http://www.w3.org/2002/07/owl#" rdf:about="#auxiliary">
      <rdfs:comment>subClassOf partOfSpeech inferred from rdfs:comment.</rdfs:comment>
      <rdfs:subClassOf>
         <owl:Class rdf:about="#partOfSpeech"/>
      </rdfs:subClassOf>
   </owl:Class>
   <owl:Class xmlns:owl="http://www.w3.org/2002/07/owl#" rdf:about="#classifier">
      <rdfs:comment>subClassOf partOfSpeech inferred from rdfs:comment.</rdfs:comment>
      <rdfs:subClassOf>
         <owl:Class rdf:about="#partOfSpeech"/>
      </rdfs:subClassOf>
   </owl:Class>
   <owl:Class xmlns:owl="http://www.w3.org/2002/07/owl#" rdf:about="#noun">
      <rdfs:comment>subClassOf partOfSpeech inferred from rdfs:comment.</rdfs:comment>
      <rdfs:subClassOf>
         <owl:Class rdf:about="#partOfSpeech"/>
      </rdfs:subClassOf>
   </owl:Class>
   <owl:Class xmlns:owl="http://www.w3.org/2002/07/owl#" rdf:about="#numeral">
      <rdfs:comment>subClassOf partOfSpeech inferred from rdfs:comment.</rdfs:comment>
      <rdfs:subClassOf>
         <owl:Class rdf:about="#partOfSpeech"/>
      </rdfs:subClassOf>
   </owl:Class>
   <owl:Class xmlns:owl="http://www.w3.org/2002/07/owl#" rdf:about="#strongPersonalPronoun">
      <rdfs:comment>subClassOf personalPronoun inferred from rdfs:comment.</rdfs:comment>
      <rdfs:subClassOf>
         <owl:Class rdf:about="#personalPronoun"/>
      </rdfs:subClassOf>
   </owl:Class>
   <owl:Class xmlns:owl="http://www.w3.org/2002/07/owl#" rdf:about="#trial">
      <rdfs:comment>subClassOf grammaticalNumber inferred from rdfs:comment.</rdfs:comment>
      <rdfs:subClassOf>
         <owl:Class rdf:about="#grammaticalNumber"/>
      </rdfs:subClassOf>
   </owl:Class>
   <owl:Class xmlns:owl="http://www.w3.org/2002/07/owl#" rdf:about="#unclassifiedResidual">
      <rdfs:comment>subClassOf partOfSpeech inferred from rdfs:comment.</rdfs:comment>
      <rdfs:subClassOf>
         <owl:Class rdf:about="#partOfSpeech"/>
      </rdfs:subClassOf>
   </owl:Class>
   <owl:Class xmlns:owl="http://www.w3.org/2002/07/owl#" rdf:about="#weakPersonalPronoun">
      <rdfs:comment>subClassOf personalPronoun inferred from rdfs:comment.</rdfs:comment>
      <rdfs:subClassOf>
         <owl:Class rdf:about="#personalPronoun"/>
      </rdfs:subClassOf>
   </owl:Class>
   <owl:Class xmlns:owl="http://www.w3.org/2002/07/owl#" rdf:about="#attributiveAdjective">
      <rdfs:comment>subClassOf adjective inferred from naming conventions.</rdfs:comment>
      <rdfs:subClassOf>
         <owl:Class rdf:about="#adjective"/>
      </rdfs:subClassOf>
   </owl:Class>
   <owl:Class xmlns:owl="http://www.w3.org/2002/07/owl#" rdf:ID="object"/>
   <owl:Class xmlns:owl="http://www.w3.org/2002/07/owl#" rdf:about="#directObject">
      <rdfs:comment>subClassOf object inferred from naming conventions.</rdfs:comment>
      <rdfs:subClassOf>
         <owl:Class rdf:about="#object"/>
      </rdfs:subClassOf>
   </owl:Class>
   <owl:Class xmlns:owl="http://www.w3.org/2002/07/owl#" rdf:about="#futurePerfect">
      <rdfs:comment>subClassOf perfect inferred from naming conventions.</rdfs:comment>
      <rdfs:subClassOf>
         <owl:Class rdf:about="#perfect"/>
      </rdfs:subClassOf>
   </owl:Class>
   <owl:Class xmlns:owl="http://www.w3.org/2002/07/owl#" rdf:about="#indirectObject">
      <rdfs:comment>subClassOf object inferred from naming conventions.</rdfs:comment>
      <rdfs:subClassOf>
         <owl:Class rdf:about="#object"/>
      </rdfs:subClassOf>
   </owl:Class>
   <owl:Class xmlns:owl="http://www.w3.org/2002/07/owl#" rdf:about="#pastPerfect">
      <rdfs:comment>subClassOf perfect inferred from naming conventions.</rdfs:comment>
      <rdfs:subClassOf>
         <owl:Class rdf:about="#perfect"/>
      </rdfs:subClassOf>
   </owl:Class>
   <owl:Class xmlns:owl="http://www.w3.org/2002/07/owl#" rdf:about="#substantiveAdjective">
      <rdfs:comment>subClassOf adjective inferred from naming conventions.</rdfs:comment>
      <rdfs:subClassOf>
         <owl:Class rdf:about="#adjective"/>
      </rdfs:subClassOf>
   </owl:Class>
   <owl:Class xmlns:owl="http://www.w3.org/2002/07/owl#" rdf:about="#abessiveCase">
      <rdfs:comment>subClassOf case inferred from naming conventions.</rdfs:comment>
      <rdfs:subClassOf>
         <owl:Class rdf:about="#case"/>
      </rdfs:subClassOf>
   </owl:Class>
   <owl:Class xmlns:owl="http://www.w3.org/2002/07/owl#" rdf:about="#ablativeCase">
      <rdfs:comment>subClassOf case inferred from naming conventions.</rdfs:comment>
      <rdfs:subClassOf>
         <owl:Class rdf:about="#case"/>
      </rdfs:subClassOf>
   </owl:Class>
   <owl:Class xmlns:owl="http://www.w3.org/2002/07/owl#" rdf:about="#absolutiveCase">
      <rdfs:comment>subClassOf case inferred from naming conventions.</rdfs:comment>
      <rdfs:subClassOf>
         <owl:Class rdf:about="#case"/>
      </rdfs:subClassOf>
   </owl:Class>
   <owl:Class xmlns:owl="http://www.w3.org/2002/07/owl#" rdf:about="#accusativeCase">
      <rdfs:comment>subClassOf case inferred from naming conventions.</rdfs:comment>
      <rdfs:subClassOf>
         <owl:Class rdf:about="#case"/>
      </rdfs:subClassOf>
   </owl:Class>
   <owl:Class xmlns:owl="http://www.w3.org/2002/07/owl#" rdf:about="#activeVoice">
      <rdfs:comment>subClassOf voice inferred from naming conventions.</rdfs:comment>
      <rdfs:subClassOf>
         <owl:Class rdf:about="#voice"/>
      </rdfs:subClassOf>
   </owl:Class>
   <owl:Class xmlns:owl="http://www.w3.org/2002/07/owl#" rdf:about="#addAffix">
      <rdfs:comment>subClassOf affix inferred from naming conventions.</rdfs:comment>
      <rdfs:subClassOf>
         <owl:Class rdf:about="#affix"/>
      </rdfs:subClassOf>
   </owl:Class>
   <owl:Class xmlns:owl="http://www.w3.org/2002/07/owl#" rdf:ID="after"/>
   <owl:Class xmlns:owl="http://www.w3.org/2002/07/owl#" rdf:about="#addAfter">
      <rdfs:comment>subClassOf after inferred from naming conventions.</rdfs:comment>
      <rdfs:subClassOf>
         <owl:Class rdf:about="#after"/>
      </rdfs:subClassOf>
   </owl:Class>
   <owl:Class xmlns:owl="http://www.w3.org/2002/07/owl#" rdf:ID="before"/>
   <owl:Class xmlns:owl="http://www.w3.org/2002/07/owl#" rdf:about="#addBefore">
      <rdfs:comment>subClassOf before inferred from naming conventions.</rdfs:comment>
      <rdfs:subClassOf>
         <owl:Class rdf:about="#before"/>
      </rdfs:subClassOf>
   </owl:Class>
   <owl:Class xmlns:owl="http://www.w3.org/2002/07/owl#" rdf:about="#addComponentLemma">
      <rdfs:comment>subClassOf lemma inferred from naming conventions.</rdfs:comment>
      <rdfs:subClassOf>
         <owl:Class rdf:about="#lemma"/>
      </rdfs:subClassOf>
   </owl:Class>
   <owl:Class xmlns:owl="http://www.w3.org/2002/07/owl#" rdf:ID="componentLemma"/>
   <owl:Class xmlns:owl="http://www.w3.org/2002/07/owl#" rdf:about="#addComponentLemma">
      <rdfs:comment>subClassOf componentLemma inferred from naming conventions.</rdfs:comment>
      <rdfs:subClassOf>
         <owl:Class rdf:about="#componentLemma"/>
      </rdfs:subClassOf>
   </owl:Class>
   <owl:Class xmlns:owl="http://www.w3.org/2002/07/owl#" rdf:about="#addComponentStem">
      <rdfs:comment>subClassOf stem inferred from naming conventions.</rdfs:comment>
      <rdfs:subClassOf>
         <owl:Class rdf:about="#stem"/>
      </rdfs:subClassOf>
   </owl:Class>
   <owl:Class xmlns:owl="http://www.w3.org/2002/07/owl#" rdf:about="#addLemma">
      <rdfs:comment>subClassOf lemma inferred from naming conventions.</rdfs:comment>
      <rdfs:subClassOf>
         <owl:Class rdf:about="#lemma"/>
      </rdfs:subClassOf>
   </owl:Class>
   <owl:Class xmlns:owl="http://www.w3.org/2002/07/owl#"
              rdf:about="#addLowerCaseComponentLemma">
      <rdfs:comment>subClassOf lemma inferred from naming conventions.</rdfs:comment>
      <rdfs:subClassOf>
         <owl:Class rdf:about="#lemma"/>
      </rdfs:subClassOf>
   </owl:Class>
   <owl:Class xmlns:owl="http://www.w3.org/2002/07/owl#"
              rdf:about="#addLowerCaseComponentLemma">
      <rdfs:comment>subClassOf componentLemma inferred from naming conventions.</rdfs:comment>
      <rdfs:subClassOf>
         <owl:Class rdf:about="#componentLemma"/>
      </rdfs:subClassOf>
   </owl:Class>
   <owl:Class xmlns:owl="http://www.w3.org/2002/07/owl#" rdf:about="#adessiveCase">
      <rdfs:comment>subClassOf case inferred from naming conventions.</rdfs:comment>
      <rdfs:subClassOf>
         <owl:Class rdf:about="#case"/>
      </rdfs:subClassOf>
   </owl:Class>
   <owl:Class xmlns:owl="http://www.w3.org/2002/07/owl#" rdf:about="#aditiveCase">
      <rdfs:comment>subClassOf case inferred from naming conventions.</rdfs:comment>
      <rdfs:subClassOf>
         <owl:Class rdf:about="#case"/>
      </rdfs:subClassOf>
   </owl:Class>
   <owl:Class xmlns:owl="http://www.w3.org/2002/07/owl#" rdf:about="#affixRank">
      <rdfs:comment>subClassOf rank inferred from naming conventions.</rdfs:comment>
      <rdfs:subClassOf>
         <owl:Class rdf:about="#rank"/>
      </rdfs:subClassOf>
   </owl:Class>
   <owl:Class xmlns:owl="http://www.w3.org/2002/07/owl#" rdf:about="#affixedPersonalPronoun">
      <rdfs:comment>subClassOf pronoun inferred from naming conventions.</rdfs:comment>
      <rdfs:subClassOf>
         <owl:Class rdf:about="#pronoun"/>
      </rdfs:subClassOf>
   </owl:Class>
   <owl:Class xmlns:owl="http://www.w3.org/2002/07/owl#" rdf:about="#affixedPersonalPronoun">
      <rdfs:comment>subClassOf personalPronoun inferred from naming conventions.</rdfs:comment>
      <rdfs:subClassOf>
         <owl:Class rdf:about="#personalPronoun"/>
      </rdfs:subClassOf>
   </owl:Class>
   <owl:Class xmlns:owl="http://www.w3.org/2002/07/owl#" rdf:about="#allativeCase">
      <rdfs:comment>subClassOf case inferred from naming conventions.</rdfs:comment>
      <rdfs:subClassOf>
         <owl:Class rdf:about="#case"/>
      </rdfs:subClassOf>
   </owl:Class>
   <owl:Class xmlns:owl="http://www.w3.org/2002/07/owl#" rdf:about="#allusivePronoun">
      <rdfs:comment>subClassOf pronoun inferred from naming conventions.</rdfs:comment>
      <rdfs:subClassOf>
         <owl:Class rdf:about="#pronoun"/>
      </rdfs:subClassOf>
   </owl:Class>
   <owl:Class xmlns:owl="http://www.w3.org/2002/07/owl#" rdf:about="#benchLevelRegister">
      <rdfs:comment>subClassOf register inferred from naming conventions.</rdfs:comment>
      <rdfs:subClassOf>
         <owl:Class rdf:about="#register"/>
      </rdfs:subClassOf>
   </owl:Class>
   <owl:Class xmlns:owl="http://www.w3.org/2002/07/owl#" rdf:about="#benefactiveCase">
      <rdfs:comment>subClassOf case inferred from naming conventions.</rdfs:comment>
      <rdfs:subClassOf>
         <owl:Class rdf:about="#case"/>
      </rdfs:subClassOf>
   </owl:Class>
   <owl:Class xmlns:owl="http://www.w3.org/2002/07/owl#" rdf:about="#brokenPlural">
      <rdfs:comment>subClassOf plural inferred from naming conventions.</rdfs:comment>
      <rdfs:subClassOf>
         <owl:Class rdf:about="#plural"/>
      </rdfs:subClassOf>
   </owl:Class>
   <owl:Class xmlns:owl="http://www.w3.org/2002/07/owl#" rdf:about="#causativeCase">
      <rdfs:comment>subClassOf case inferred from naming conventions.</rdfs:comment>
      <rdfs:subClassOf>
         <owl:Class rdf:about="#case"/>
      </rdfs:subClassOf>
   </owl:Class>
   <owl:Class xmlns:owl="http://www.w3.org/2002/07/owl#" rdf:about="#characterCoding">
      <rdfs:comment>subClassOf coding inferred from naming conventions.</rdfs:comment>
      <rdfs:subClassOf>
         <owl:Class rdf:about="#coding"/>
      </rdfs:subClassOf>
   </owl:Class>
   <owl:Class xmlns:owl="http://www.w3.org/2002/07/owl#" rdf:ID="bracket"/>
   <owl:Class xmlns:owl="http://www.w3.org/2002/07/owl#" rdf:about="#closeBracket">
      <rdfs:comment>subClassOf bracket inferred from naming conventions.</rdfs:comment>
      <rdfs:subClassOf>
         <owl:Class rdf:about="#bracket"/>
      </rdfs:subClassOf>
   </owl:Class>
   <owl:Class xmlns:owl="http://www.w3.org/2002/07/owl#" rdf:about="#closeCurlyBracket">
      <rdfs:comment>subClassOf bracket inferred from naming conventions.</rdfs:comment>
      <rdfs:subClassOf>
         <owl:Class rdf:about="#bracket"/>
      </rdfs:subClassOf>
   </owl:Class>
   <owl:Class xmlns:owl="http://www.w3.org/2002/07/owl#" rdf:ID="curlyBracket"/>
   <owl:Class xmlns:owl="http://www.w3.org/2002/07/owl#" rdf:about="#closeCurlyBracket">
      <rdfs:comment>subClassOf curlyBracket inferred from naming conventions.</rdfs:comment>
      <rdfs:subClassOf>
         <owl:Class rdf:about="#curlyBracket"/>
      </rdfs:subClassOf>
   </owl:Class>
   <owl:Class xmlns:owl="http://www.w3.org/2002/07/owl#" rdf:ID="parenthesis"/>
   <owl:Class xmlns:owl="http://www.w3.org/2002/07/owl#" rdf:about="#closeParenthesis">
      <rdfs:comment>subClassOf parenthesis inferred from naming conventions.</rdfs:comment>
      <rdfs:subClassOf>
         <owl:Class rdf:about="#parenthesis"/>
      </rdfs:subClassOf>
   </owl:Class>
   <owl:Class xmlns:owl="http://www.w3.org/2002/07/owl#" rdf:about="#closePunctuation">
      <rdfs:comment>subClassOf punctuation inferred from naming conventions.</rdfs:comment>
      <rdfs:subClassOf>
         <owl:Class rdf:about="#punctuation"/>
      </rdfs:subClassOf>
   </owl:Class>
   <owl:Class xmlns:owl="http://www.w3.org/2002/07/owl#" rdf:about="#comitativeCase">
      <rdfs:comment>subClassOf case inferred from naming conventions.</rdfs:comment>
      <rdfs:subClassOf>
         <owl:Class rdf:about="#case"/>
      </rdfs:subClassOf>
   </owl:Class>
   <owl:Class xmlns:owl="http://www.w3.org/2002/07/owl#" rdf:ID="gender"/>
   <owl:Class xmlns:owl="http://www.w3.org/2002/07/owl#" rdf:about="#commonGender">
      <rdfs:comment>subClassOf gender inferred from naming conventions.</rdfs:comment>
      <rdfs:subClassOf>
         <owl:Class rdf:about="#gender"/>
      </rdfs:subClassOf>
   </owl:Class>
   <owl:Class xmlns:owl="http://www.w3.org/2002/07/owl#" rdf:about="#commonNoun">
      <rdfs:comment>subClassOf noun inferred from naming conventions.</rdfs:comment>
      <rdfs:subClassOf>
         <owl:Class rdf:about="#noun"/>
      </rdfs:subClassOf>
   </owl:Class>
   <owl:Class xmlns:owl="http://www.w3.org/2002/07/owl#" rdf:ID="used"/>
   <owl:Class xmlns:owl="http://www.w3.org/2002/07/owl#" rdf:about="#commonlyUsed">
      <rdfs:comment>subClassOf used inferred from naming conventions.</rdfs:comment>
      <rdfs:subClassOf>
         <owl:Class rdf:about="#used"/>
      </rdfs:subClassOf>
   </owl:Class>
   <owl:Class xmlns:owl="http://www.w3.org/2002/07/owl#" rdf:about="#comparativeParticle">
      <rdfs:comment>subClassOf particle inferred from naming conventions.</rdfs:comment>
      <rdfs:subClassOf>
         <owl:Class rdf:about="#particle"/>
      </rdfs:subClassOf>
   </owl:Class>
   <owl:Class xmlns:owl="http://www.w3.org/2002/07/owl#" rdf:about="#componentRank">
      <rdfs:comment>subClassOf rank inferred from naming conventions.</rdfs:comment>
      <rdfs:subClassOf>
         <owl:Class rdf:about="#rank"/>
      </rdfs:subClassOf>
   </owl:Class>
   <owl:Class xmlns:owl="http://www.w3.org/2002/07/owl#" rdf:about="#compoundPreposition">
      <rdfs:comment>subClassOf preposition inferred from naming conventions.</rdfs:comment>
      <rdfs:subClassOf>
         <owl:Class rdf:about="#preposition"/>
      </rdfs:subClassOf>
   </owl:Class>
   <owl:Class xmlns:owl="http://www.w3.org/2002/07/owl#" rdf:about="#conditionalParticle">
      <rdfs:comment>subClassOf particle inferred from naming conventions.</rdfs:comment>
      <rdfs:subClassOf>
         <owl:Class rdf:about="#particle"/>
      </rdfs:subClassOf>
   </owl:Class>
   <owl:Class xmlns:owl="http://www.w3.org/2002/07/owl#" rdf:about="#conditionalPronoun">
      <rdfs:comment>subClassOf pronoun inferred from naming conventions.</rdfs:comment>
      <rdfs:subClassOf>
         <owl:Class rdf:about="#pronoun"/>
      </rdfs:subClassOf>
   </owl:Class>
   <owl:Class xmlns:owl="http://www.w3.org/2002/07/owl#" rdf:about="#contextualVariation">
      <rdfs:comment>subClassOf variation inferred from naming conventions.</rdfs:comment>
      <rdfs:subClassOf>
         <owl:Class rdf:about="#variation"/>
      </rdfs:subClassOf>
   </owl:Class>
   <owl:Class xmlns:owl="http://www.w3.org/2002/07/owl#" rdf:about="#coordinatingConjunction">
      <rdfs:comment>subClassOf conjunction inferred from naming conventions.</rdfs:comment>
      <rdfs:subClassOf>
         <owl:Class rdf:about="#conjunction"/>
      </rdfs:subClassOf>
   </owl:Class>
   <owl:Class xmlns:owl="http://www.w3.org/2002/07/owl#" rdf:about="#coordinationParticle">
      <rdfs:comment>subClassOf particle inferred from naming conventions.</rdfs:comment>
      <rdfs:subClassOf>
         <owl:Class rdf:about="#particle"/>
      </rdfs:subClassOf>
   </owl:Class>
   <owl:Class xmlns:owl="http://www.w3.org/2002/07/owl#" rdf:about="#countableNoun">
      <rdfs:comment>subClassOf noun inferred from naming conventions.</rdfs:comment>
      <rdfs:subClassOf>
         <owl:Class rdf:about="#noun"/>
      </rdfs:subClassOf>
   </owl:Class>
   <owl:Class xmlns:owl="http://www.w3.org/2002/07/owl#" rdf:about="#countryCoding">
      <rdfs:comment>subClassOf coding inferred from naming conventions.</rdfs:comment>
      <rdfs:subClassOf>
         <owl:Class rdf:about="#coding"/>
      </rdfs:subClassOf>
   </owl:Class>
   <owl:Class xmlns:owl="http://www.w3.org/2002/07/owl#" rdf:about="#dateCoding">
      <rdfs:comment>subClassOf coding inferred from naming conventions.</rdfs:comment>
      <rdfs:subClassOf>
         <owl:Class rdf:about="#coding"/>
      </rdfs:subClassOf>
   </owl:Class>
   <owl:Class xmlns:owl="http://www.w3.org/2002/07/owl#" rdf:about="#dativeCase">
      <rdfs:comment>subClassOf case inferred from naming conventions.</rdfs:comment>
      <rdfs:subClassOf>
         <owl:Class rdf:about="#case"/>
      </rdfs:subClassOf>
   </owl:Class>
   <owl:Class xmlns:owl="http://www.w3.org/2002/07/owl#" rdf:ID="article"/>
   <owl:Class xmlns:owl="http://www.w3.org/2002/07/owl#" rdf:about="#definiteArticle">
      <rdfs:comment>subClassOf article inferred from naming conventions.</rdfs:comment>
      <rdfs:subClassOf>
         <owl:Class rdf:about="#article"/>
      </rdfs:subClassOf>
   </owl:Class>
   <owl:Class xmlns:owl="http://www.w3.org/2002/07/owl#" rdf:about="#delativeCase">
      <rdfs:comment>subClassOf case inferred from naming conventions.</rdfs:comment>
      <rdfs:subClassOf>
         <owl:Class rdf:about="#case"/>
      </rdfs:subClassOf>
   </owl:Class>
   <owl:Class xmlns:owl="http://www.w3.org/2002/07/owl#" rdf:about="#demonstrativeDeterminer">
      <rdfs:comment>subClassOf determiner inferred from naming conventions.</rdfs:comment>
      <rdfs:subClassOf>
         <owl:Class rdf:about="#determiner"/>
      </rdfs:subClassOf>
   </owl:Class>
   <owl:Class xmlns:owl="http://www.w3.org/2002/07/owl#" rdf:about="#demonstrativePronoun">
      <rdfs:comment>subClassOf pronoun inferred from naming conventions.</rdfs:comment>
      <rdfs:subClassOf>
         <owl:Class rdf:about="#pronoun"/>
      </rdfs:subClassOf>
   </owl:Class>
   <owl:Class xmlns:owl="http://www.w3.org/2002/07/owl#" rdf:about="#dialectRegister">
      <rdfs:comment>subClassOf register inferred from naming conventions.</rdfs:comment>
      <rdfs:subClassOf>
         <owl:Class rdf:about="#register"/>
      </rdfs:subClassOf>
   </owl:Class>
   <owl:Class xmlns:owl="http://www.w3.org/2002/07/owl#" rdf:about="#diminutiveNoun">
      <rdfs:comment>subClassOf noun inferred from naming conventions.</rdfs:comment>
      <rdfs:subClassOf>
         <owl:Class rdf:about="#noun"/>
      </rdfs:subClassOf>
   </owl:Class>
   <owl:Class xmlns:owl="http://www.w3.org/2002/07/owl#" rdf:about="#distinctiveParticle">
      <rdfs:comment>subClassOf particle inferred from naming conventions.</rdfs:comment>
      <rdfs:subClassOf>
         <owl:Class rdf:about="#particle"/>
      </rdfs:subClassOf>
   </owl:Class>
   <owl:Class xmlns:owl="http://www.w3.org/2002/07/owl#" rdf:about="#elativeCase">
      <rdfs:comment>subClassOf case inferred from naming conventions.</rdfs:comment>
      <rdfs:subClassOf>
         <owl:Class rdf:about="#case"/>
      </rdfs:subClassOf>
   </owl:Class>
   <owl:Class xmlns:owl="http://www.w3.org/2002/07/owl#" rdf:about="#emphaticPronoun">
      <rdfs:comment>subClassOf pronoun inferred from naming conventions.</rdfs:comment>
      <rdfs:subClassOf>
         <owl:Class rdf:about="#pronoun"/>
      </rdfs:subClassOf>
   </owl:Class>
   <owl:Class xmlns:owl="http://www.w3.org/2002/07/owl#" rdf:about="#equativeCase">
      <rdfs:comment>subClassOf case inferred from naming conventions.</rdfs:comment>
      <rdfs:subClassOf>
         <owl:Class rdf:about="#case"/>
      </rdfs:subClassOf>
   </owl:Class>
   <owl:Class xmlns:owl="http://www.w3.org/2002/07/owl#" rdf:about="#ergativeCase">
      <rdfs:comment>subClassOf case inferred from naming conventions.</rdfs:comment>
      <rdfs:subClassOf>
         <owl:Class rdf:about="#case"/>
      </rdfs:subClassOf>
   </owl:Class>
   <owl:Class xmlns:owl="http://www.w3.org/2002/07/owl#" rdf:about="#essiveCase">
      <rdfs:comment>subClassOf case inferred from naming conventions.</rdfs:comment>
      <rdfs:subClassOf>
         <owl:Class rdf:about="#case"/>
      </rdfs:subClassOf>
   </owl:Class>
   <owl:Class xmlns:owl="http://www.w3.org/2002/07/owl#" rdf:about="#etymologicalRoot">
      <rdfs:comment>subClassOf root inferred from naming conventions.</rdfs:comment>
      <rdfs:subClassOf>
         <owl:Class rdf:about="#root"/>
      </rdfs:subClassOf>
   </owl:Class>
   <owl:Class xmlns:owl="http://www.w3.org/2002/07/owl#" rdf:about="#exclamativeDeterminer">
      <rdfs:comment>subClassOf determiner inferred from naming conventions.</rdfs:comment>
      <rdfs:subClassOf>
         <owl:Class rdf:about="#determiner"/>
      </rdfs:subClassOf>
   </owl:Class>
   <owl:Class xmlns:owl="http://www.w3.org/2002/07/owl#" rdf:about="#exclamativePoint">
      <rdfs:comment>subClassOf point inferred from naming conventions.</rdfs:comment>
      <rdfs:subClassOf>
         <owl:Class rdf:about="#point"/>
      </rdfs:subClassOf>
   </owl:Class>
   <owl:Class xmlns:owl="http://www.w3.org/2002/07/owl#" rdf:about="#exclamativePronoun">
      <rdfs:comment>subClassOf pronoun inferred from naming conventions.</rdfs:comment>
      <rdfs:subClassOf>
         <owl:Class rdf:about="#pronoun"/>
      </rdfs:subClassOf>
   </owl:Class>
   <owl:Class xmlns:owl="http://www.w3.org/2002/07/owl#" rdf:about="#expansionVariation">
      <rdfs:comment>subClassOf variation inferred from naming conventions.</rdfs:comment>
      <rdfs:subClassOf>
         <owl:Class rdf:about="#variation"/>
      </rdfs:subClassOf>
   </owl:Class>
   <owl:Class xmlns:owl="http://www.w3.org/2002/07/owl#" rdf:about="#facetiousRegister">
      <rdfs:comment>subClassOf register inferred from naming conventions.</rdfs:comment>
      <rdfs:subClassOf>
         <owl:Class rdf:about="#register"/>
      </rdfs:subClassOf>
   </owl:Class>
   <owl:Class xmlns:owl="http://www.w3.org/2002/07/owl#" rdf:about="#firstPerson">
      <rdfs:comment>subClassOf person inferred from naming conventions.</rdfs:comment>
      <rdfs:subClassOf>
         <owl:Class rdf:about="#person"/>
      </rdfs:subClassOf>
   </owl:Class>
   <owl:Class xmlns:owl="http://www.w3.org/2002/07/owl#" rdf:about="#foreignText">
      <rdfs:comment>subClassOf text inferred from naming conventions.</rdfs:comment>
      <rdfs:subClassOf>
         <owl:Class rdf:about="#text"/>
      </rdfs:subClassOf>
   </owl:Class>
   <owl:Class xmlns:owl="http://www.w3.org/2002/07/owl#" rdf:about="#formalRegister">
      <rdfs:comment>subClassOf register inferred from naming conventions.</rdfs:comment>
      <rdfs:subClassOf>
         <owl:Class rdf:about="#register"/>
      </rdfs:subClassOf>
   </owl:Class>
   <owl:Class xmlns:owl="http://www.w3.org/2002/07/owl#" rdf:about="#fullArticle">
      <rdfs:comment>subClassOf article inferred from naming conventions.</rdfs:comment>
      <rdfs:subClassOf>
         <owl:Class rdf:about="#article"/>
      </rdfs:subClassOf>
   </owl:Class>
   <owl:Class xmlns:owl="http://www.w3.org/2002/07/owl#" rdf:about="#fusedPreposition">
      <rdfs:comment>subClassOf preposition inferred from naming conventions.</rdfs:comment>
      <rdfs:subClassOf>
         <owl:Class rdf:about="#preposition"/>
      </rdfs:subClassOf>
   </owl:Class>
   <owl:Class xmlns:owl="http://www.w3.org/2002/07/owl#" rdf:about="#futureParticle">
      <rdfs:comment>subClassOf particle inferred from naming conventions.</rdfs:comment>
      <rdfs:subClassOf>
         <owl:Class rdf:about="#particle"/>
      </rdfs:subClassOf>
   </owl:Class>
   <owl:Class xmlns:owl="http://www.w3.org/2002/07/owl#" rdf:about="#generalAdverb">
      <rdfs:comment>subClassOf adverb inferred from naming conventions.</rdfs:comment>
      <rdfs:subClassOf>
         <owl:Class rdf:about="#adverb"/>
      </rdfs:subClassOf>
   </owl:Class>
   <owl:Class xmlns:owl="http://www.w3.org/2002/07/owl#" rdf:about="#genitiveCase">
      <rdfs:comment>subClassOf case inferred from naming conventions.</rdfs:comment>
      <rdfs:subClassOf>
         <owl:Class rdf:about="#case"/>
      </rdfs:subClassOf>
   </owl:Class>
   <owl:Class xmlns:owl="http://www.w3.org/2002/07/owl#" rdf:about="#grammaticalGender">
      <rdfs:comment>subClassOf gender inferred from naming conventions.</rdfs:comment>
      <rdfs:subClassOf>
         <owl:Class rdf:about="#gender"/>
      </rdfs:subClassOf>
   </owl:Class>
   <owl:Class xmlns:owl="http://www.w3.org/2002/07/owl#" rdf:ID="number"/>
   <owl:Class xmlns:owl="http://www.w3.org/2002/07/owl#" rdf:about="#grammaticalNumber">
      <rdfs:comment>subClassOf number inferred from naming conventions.</rdfs:comment>
      <rdfs:subClassOf>
         <owl:Class rdf:about="#number"/>
      </rdfs:subClassOf>
   </owl:Class>
   <owl:Class xmlns:owl="http://www.w3.org/2002/07/owl#" rdf:about="#graphicalOperator">
      <rdfs:comment>subClassOf operator inferred from naming conventions.</rdfs:comment>
      <rdfs:subClassOf>
         <owl:Class rdf:about="#operator"/>
      </rdfs:subClassOf>
   </owl:Class>
   <owl:Class xmlns:owl="http://www.w3.org/2002/07/owl#" rdf:about="#illativeCase">
      <rdfs:comment>subClassOf case inferred from naming conventions.</rdfs:comment>
      <rdfs:subClassOf>
         <owl:Class rdf:about="#case"/>
      </rdfs:subClassOf>
   </owl:Class>
   <owl:Class xmlns:owl="http://www.w3.org/2002/07/owl#" rdf:about="#impersonalPronoun">
      <rdfs:comment>subClassOf pronoun inferred from naming conventions.</rdfs:comment>
      <rdfs:subClassOf>
         <owl:Class rdf:about="#pronoun"/>
      </rdfs:subClassOf>
   </owl:Class>
   <owl:Class xmlns:owl="http://www.w3.org/2002/07/owl#" rdf:about="#inHouseRegister">
      <rdfs:comment>subClassOf register inferred from naming conventions.</rdfs:comment>
      <rdfs:subClassOf>
         <owl:Class rdf:about="#register"/>
      </rdfs:subClassOf>
   </owl:Class>
   <owl:Class xmlns:owl="http://www.w3.org/2002/07/owl#" rdf:about="#indefiniteArticle">
      <rdfs:comment>subClassOf article inferred from naming conventions.</rdfs:comment>
      <rdfs:subClassOf>
         <owl:Class rdf:about="#article"/>
      </rdfs:subClassOf>
   </owl:Class>
   <owl:Class xmlns:owl="http://www.w3.org/2002/07/owl#" rdf:about="#indefiniteDeterminer">
      <rdfs:comment>subClassOf determiner inferred from naming conventions.</rdfs:comment>
      <rdfs:subClassOf>
         <owl:Class rdf:about="#determiner"/>
      </rdfs:subClassOf>
   </owl:Class>
   <owl:Class xmlns:owl="http://www.w3.org/2002/07/owl#" rdf:about="#indefinitePronoun">
      <rdfs:comment>subClassOf pronoun inferred from naming conventions.</rdfs:comment>
      <rdfs:subClassOf>
         <owl:Class rdf:about="#pronoun"/>
      </rdfs:subClassOf>
   </owl:Class>
   <owl:Class xmlns:owl="http://www.w3.org/2002/07/owl#" rdf:about="#inessiveCase">
      <rdfs:comment>subClassOf case inferred from naming conventions.</rdfs:comment>
      <rdfs:subClassOf>
         <owl:Class rdf:about="#case"/>
      </rdfs:subClassOf>
   </owl:Class>
   <owl:Class xmlns:owl="http://www.w3.org/2002/07/owl#" rdf:about="#infinitiveParticle">
      <rdfs:comment>subClassOf particle inferred from naming conventions.</rdfs:comment>
      <rdfs:subClassOf>
         <owl:Class rdf:about="#particle"/>
      </rdfs:subClassOf>
   </owl:Class>
   <owl:Class xmlns:owl="http://www.w3.org/2002/07/owl#" rdf:about="#infrequentlyUsed">
      <rdfs:comment>subClassOf used inferred from naming conventions.</rdfs:comment>
      <rdfs:subClassOf>
         <owl:Class rdf:about="#used"/>
      </rdfs:subClassOf>
   </owl:Class>
   <owl:Class xmlns:owl="http://www.w3.org/2002/07/owl#" rdf:about="#instrumentalCase">
      <rdfs:comment>subClassOf case inferred from naming conventions.</rdfs:comment>
      <rdfs:subClassOf>
         <owl:Class rdf:about="#case"/>
      </rdfs:subClassOf>
   </owl:Class>
   <owl:Class xmlns:owl="http://www.w3.org/2002/07/owl#" rdf:about="#interrogativeDeterminer">
      <rdfs:comment>subClassOf determiner inferred from naming conventions.</rdfs:comment>
      <rdfs:subClassOf>
         <owl:Class rdf:about="#determiner"/>
      </rdfs:subClassOf>
   </owl:Class>
   <owl:Class xmlns:owl="http://www.w3.org/2002/07/owl#" rdf:about="#interrogativeParticle">
      <rdfs:comment>subClassOf particle inferred from naming conventions.</rdfs:comment>
      <rdfs:subClassOf>
         <owl:Class rdf:about="#particle"/>
      </rdfs:subClassOf>
   </owl:Class>
   <owl:Class xmlns:owl="http://www.w3.org/2002/07/owl#" rdf:about="#interrogativePronoun">
      <rdfs:comment>subClassOf pronoun inferred from naming conventions.</rdfs:comment>
      <rdfs:subClassOf>
         <owl:Class rdf:about="#pronoun"/>
      </rdfs:subClassOf>
   </owl:Class>
   <owl:Class xmlns:owl="http://www.w3.org/2002/07/owl#" rdf:about="#interrogativePunctuation">
      <rdfs:comment>subClassOf punctuation inferred from naming conventions.</rdfs:comment>
      <rdfs:subClassOf>
         <owl:Class rdf:about="#punctuation"/>
      </rdfs:subClassOf>
   </owl:Class>
   <owl:Class xmlns:owl="http://www.w3.org/2002/07/owl#" rdf:about="#invertedComma">
      <rdfs:comment>subClassOf comma inferred from naming conventions.</rdfs:comment>
      <rdfs:subClassOf>
         <owl:Class rdf:about="#comma"/>
      </rdfs:subClassOf>
   </owl:Class>
   <owl:Class xmlns:owl="http://www.w3.org/2002/07/owl#" rdf:ID="mark"/>
   <owl:Class xmlns:owl="http://www.w3.org/2002/07/owl#" rdf:about="#invertedQuestionMark">
      <rdfs:comment>subClassOf mark inferred from naming conventions.</rdfs:comment>
      <rdfs:subClassOf>
         <owl:Class rdf:about="#mark"/>
      </rdfs:subClassOf>
   </owl:Class>
   <owl:Class xmlns:owl="http://www.w3.org/2002/07/owl#" rdf:about="#invertedQuestionMark">
      <rdfs:comment>subClassOf questionMark inferred from naming conventions.</rdfs:comment>
      <rdfs:subClassOf>
         <owl:Class rdf:about="#questionMark"/>
      </rdfs:subClassOf>
   </owl:Class>
   <owl:Class xmlns:owl="http://www.w3.org/2002/07/owl#" rdf:about="#ironicRegister">
      <rdfs:comment>subClassOf register inferred from naming conventions.</rdfs:comment>
      <rdfs:subClassOf>
         <owl:Class rdf:about="#register"/>
      </rdfs:subClassOf>
   </owl:Class>
   <owl:Class xmlns:owl="http://www.w3.org/2002/07/owl#" rdf:about="#languageCoding">
      <rdfs:comment>subClassOf coding inferred from naming conventions.</rdfs:comment>
      <rdfs:subClassOf>
         <owl:Class rdf:about="#coding"/>
      </rdfs:subClassOf>
   </owl:Class>
   <owl:Class xmlns:owl="http://www.w3.org/2002/07/owl#" rdf:about="#lativeCase">
      <rdfs:comment>subClassOf case inferred from naming conventions.</rdfs:comment>
      <rdfs:subClassOf>
         <owl:Class rdf:about="#case"/>
      </rdfs:subClassOf>
   </owl:Class>
   <owl:Class xmlns:owl="http://www.w3.org/2002/07/owl#" rdf:ID="environment"/>
   <owl:Class xmlns:owl="http://www.w3.org/2002/07/owl#" rdf:about="#leftEnvironment">
      <rdfs:comment>subClassOf environment inferred from naming conventions.</rdfs:comment>
      <rdfs:subClassOf>
         <owl:Class rdf:about="#environment"/>
      </rdfs:subClassOf>
   </owl:Class>
   <owl:Class xmlns:owl="http://www.w3.org/2002/07/owl#" rdf:about="#lexicalType">
      <rdfs:comment>subClassOf type inferred from naming conventions.</rdfs:comment>
      <rdfs:subClassOf>
         <owl:Class rdf:about="#type"/>
      </rdfs:subClassOf>
   </owl:Class>
   <owl:Class xmlns:owl="http://www.w3.org/2002/07/owl#" rdf:about="#locativeCase">
      <rdfs:comment>subClassOf case inferred from naming conventions.</rdfs:comment>
      <rdfs:subClassOf>
         <owl:Class rdf:about="#case"/>
      </rdfs:subClassOf>
   </owl:Class>
   <owl:Class xmlns:owl="http://www.w3.org/2002/07/owl#" rdf:about="#logicalOperator">
      <rdfs:comment>subClassOf operator inferred from naming conventions.</rdfs:comment>
      <rdfs:subClassOf>
         <owl:Class rdf:about="#operator"/>
      </rdfs:subClassOf>
   </owl:Class>
   <owl:Class xmlns:owl="http://www.w3.org/2002/07/owl#" rdf:about="#logicalValue">
      <rdfs:comment>subClassOf value inferred from naming conventions.</rdfs:comment>
      <rdfs:subClassOf>
         <owl:Class rdf:about="#value"/>
      </rdfs:subClassOf>
   </owl:Class>
   <owl:Class xmlns:owl="http://www.w3.org/2002/07/owl#" rdf:about="#mainPunctuation">
      <rdfs:comment>subClassOf punctuation inferred from naming conventions.</rdfs:comment>
      <rdfs:subClassOf>
         <owl:Class rdf:about="#punctuation"/>
      </rdfs:subClassOf>
   </owl:Class>
   <owl:Class xmlns:owl="http://www.w3.org/2002/07/owl#" rdf:about="#mainVerb">
      <rdfs:comment>subClassOf verb inferred from naming conventions.</rdfs:comment>
      <rdfs:subClassOf>
         <owl:Class rdf:about="#verb"/>
      </rdfs:subClassOf>
   </owl:Class>
   <owl:Class xmlns:owl="http://www.w3.org/2002/07/owl#" rdf:about="#middleVoice">
      <rdfs:comment>subClassOf voice inferred from naming conventions.</rdfs:comment>
      <rdfs:subClassOf>
         <owl:Class rdf:about="#voice"/>
      </rdfs:subClassOf>
   </owl:Class>
   <owl:Class xmlns:owl="http://www.w3.org/2002/07/owl#" rdf:about="#modalParticle">
      <rdfs:comment>subClassOf particle inferred from naming conventions.</rdfs:comment>
      <rdfs:subClassOf>
         <owl:Class rdf:about="#particle"/>
      </rdfs:subClassOf>
   </owl:Class>
   <owl:Class xmlns:owl="http://www.w3.org/2002/07/owl#" rdf:about="#modificationType">
      <rdfs:comment>subClassOf type inferred from naming conventions.</rdfs:comment>
      <rdfs:subClassOf>
         <owl:Class rdf:about="#type"/>
      </rdfs:subClassOf>
   </owl:Class>
   <owl:Class xmlns:owl="http://www.w3.org/2002/07/owl#" rdf:about="#negativeParticle">
      <rdfs:comment>subClassOf particle inferred from naming conventions.</rdfs:comment>
      <rdfs:subClassOf>
         <owl:Class rdf:about="#particle"/>
      </rdfs:subClassOf>
   </owl:Class>
   <owl:Class xmlns:owl="http://www.w3.org/2002/07/owl#" rdf:about="#negativePronoun">
      <rdfs:comment>subClassOf pronoun inferred from naming conventions.</rdfs:comment>
      <rdfs:subClassOf>
         <owl:Class rdf:about="#pronoun"/>
      </rdfs:subClassOf>
   </owl:Class>
   <owl:Class xmlns:owl="http://www.w3.org/2002/07/owl#" rdf:about="#neutralRegister">
      <rdfs:comment>subClassOf register inferred from naming conventions.</rdfs:comment>
      <rdfs:subClassOf>
         <owl:Class rdf:about="#register"/>
      </rdfs:subClassOf>
   </owl:Class>
   <owl:Class xmlns:owl="http://www.w3.org/2002/07/owl#" rdf:about="#nominativeCase">
      <rdfs:comment>subClassOf case inferred from naming conventions.</rdfs:comment>
      <rdfs:subClassOf>
         <owl:Class rdf:about="#case"/>
      </rdfs:subClassOf>
   </owl:Class>
   <owl:Class xmlns:owl="http://www.w3.org/2002/07/owl#" rdf:about="#nonSpacedPinyin">
      <rdfs:comment>subClassOf pinyin inferred from naming conventions.</rdfs:comment>
      <rdfs:subClassOf>
         <owl:Class rdf:about="#pinyin"/>
      </rdfs:subClassOf>
   </owl:Class>
   <owl:Class xmlns:owl="http://www.w3.org/2002/07/owl#" rdf:about="#nonFinite">
      <rdfs:comment>subClassOf finite inferred from naming conventions.</rdfs:comment>
      <rdfs:subClassOf>
         <owl:Class rdf:about="#finite"/>
      </rdfs:subClassOf>
   </owl:Class>
   <owl:Class xmlns:owl="http://www.w3.org/2002/07/owl#" rdf:ID="form"/>
   <owl:Class xmlns:owl="http://www.w3.org/2002/07/owl#" rdf:about="#numeralMForm">
      <rdfs:comment>subClassOf form inferred from naming conventions.</rdfs:comment>
      <rdfs:subClassOf>
         <owl:Class rdf:about="#form"/>
      </rdfs:subClassOf>
   </owl:Class>
   <owl:Class xmlns:owl="http://www.w3.org/2002/07/owl#" rdf:about="#numeralLetter">
      <rdfs:comment>subClassOf letter inferred from naming conventions.</rdfs:comment>
      <rdfs:subClassOf>
         <owl:Class rdf:about="#letter"/>
      </rdfs:subClassOf>
   </owl:Class>
   <owl:Class xmlns:owl="http://www.w3.org/2002/07/owl#" rdf:about="#numValue">
      <rdfs:comment>subClassOf value inferred from naming conventions.</rdfs:comment>
      <rdfs:subClassOf>
         <owl:Class rdf:about="#value"/>
      </rdfs:subClassOf>
   </owl:Class>
   <owl:Class xmlns:owl="http://www.w3.org/2002/07/owl#" rdf:about="#objectPerson">
      <rdfs:comment>subClassOf person inferred from naming conventions.</rdfs:comment>
      <rdfs:subClassOf>
         <owl:Class rdf:about="#person"/>
      </rdfs:subClassOf>
   </owl:Class>
   <owl:Class xmlns:owl="http://www.w3.org/2002/07/owl#" rdf:about="#obliqueCase">
      <rdfs:comment>subClassOf case inferred from naming conventions.</rdfs:comment>
      <rdfs:subClassOf>
         <owl:Class rdf:about="#case"/>
      </rdfs:subClassOf>
   </owl:Class>
   <owl:Class xmlns:owl="http://www.w3.org/2002/07/owl#" rdf:about="#openBracket">
      <rdfs:comment>subClassOf bracket inferred from naming conventions.</rdfs:comment>
      <rdfs:subClassOf>
         <owl:Class rdf:about="#bracket"/>
      </rdfs:subClassOf>
   </owl:Class>
   <owl:Class xmlns:owl="http://www.w3.org/2002/07/owl#" rdf:about="#openCurlyBracket">
      <rdfs:comment>subClassOf bracket inferred from naming conventions.</rdfs:comment>
      <rdfs:subClassOf>
         <owl:Class rdf:about="#bracket"/>
      </rdfs:subClassOf>
   </owl:Class>
   <owl:Class xmlns:owl="http://www.w3.org/2002/07/owl#" rdf:about="#openCurlyBracket">
      <rdfs:comment>subClassOf curlyBracket inferred from naming conventions.</rdfs:comment>
      <rdfs:subClassOf>
         <owl:Class rdf:about="#curlyBracket"/>
      </rdfs:subClassOf>
   </owl:Class>
   <owl:Class xmlns:owl="http://www.w3.org/2002/07/owl#" rdf:about="#openParenthesis">
      <rdfs:comment>subClassOf parenthesis inferred from naming conventions.</rdfs:comment>
      <rdfs:subClassOf>
         <owl:Class rdf:about="#parenthesis"/>
      </rdfs:subClassOf>
   </owl:Class>
   <owl:Class xmlns:owl="http://www.w3.org/2002/07/owl#" rdf:about="#openPunctuation">
      <rdfs:comment>subClassOf punctuation inferred from naming conventions.</rdfs:comment>
      <rdfs:subClassOf>
         <owl:Class rdf:about="#punctuation"/>
      </rdfs:subClassOf>
   </owl:Class>
   <owl:Class xmlns:owl="http://www.w3.org/2002/07/owl#" rdf:about="#ordinalAdjective">
      <rdfs:comment>subClassOf adjective inferred from naming conventions.</rdfs:comment>
      <rdfs:subClassOf>
         <owl:Class rdf:about="#adjective"/>
      </rdfs:subClassOf>
   </owl:Class>
   <owl:Class xmlns:owl="http://www.w3.org/2002/07/owl#" rdf:about="#otherAnimacy">
      <rdfs:comment>subClassOf animacy inferred from naming conventions.</rdfs:comment>
      <rdfs:subClassOf>
         <owl:Class rdf:about="#animacy"/>
      </rdfs:subClassOf>
   </owl:Class>
   <owl:Class xmlns:owl="http://www.w3.org/2002/07/owl#" rdf:about="#ownedNumber">
      <rdfs:comment>subClassOf number inferred from naming conventions.</rdfs:comment>
      <rdfs:subClassOf>
         <owl:Class rdf:about="#number"/>
      </rdfs:subClassOf>
   </owl:Class>
   <owl:Class xmlns:owl="http://www.w3.org/2002/07/owl#" rdf:about="#ownerGender">
      <rdfs:comment>subClassOf gender inferred from naming conventions.</rdfs:comment>
      <rdfs:subClassOf>
         <owl:Class rdf:about="#gender"/>
      </rdfs:subClassOf>
   </owl:Class>
   <owl:Class xmlns:owl="http://www.w3.org/2002/07/owl#" rdf:about="#ownerNumber">
      <rdfs:comment>subClassOf number inferred from naming conventions.</rdfs:comment>
      <rdfs:subClassOf>
         <owl:Class rdf:about="#number"/>
      </rdfs:subClassOf>
   </owl:Class>
   <owl:Class xmlns:owl="http://www.w3.org/2002/07/owl#" rdf:about="#ownerPerson">
      <rdfs:comment>subClassOf person inferred from naming conventions.</rdfs:comment>
      <rdfs:subClassOf>
         <owl:Class rdf:about="#person"/>
      </rdfs:subClassOf>
   </owl:Class>
   <owl:Class xmlns:owl="http://www.w3.org/2002/07/owl#" rdf:about="#participleAdjective">
      <rdfs:comment>subClassOf adjective inferred from naming conventions.</rdfs:comment>
      <rdfs:subClassOf>
         <owl:Class rdf:about="#adjective"/>
      </rdfs:subClassOf>
   </owl:Class>
   <owl:Class xmlns:owl="http://www.w3.org/2002/07/owl#" rdf:about="#affirmativeParticle">
      <rdfs:comment>subClassOf particle inferred from naming conventions.</rdfs:comment>
      <rdfs:subClassOf>
         <owl:Class rdf:about="#particle"/>
      </rdfs:subClassOf>
   </owl:Class>
   <owl:Class xmlns:owl="http://www.w3.org/2002/07/owl#" rdf:about="#partitiveArticle">
      <rdfs:comment>subClassOf article inferred from naming conventions.</rdfs:comment>
      <rdfs:subClassOf>
         <owl:Class rdf:about="#article"/>
      </rdfs:subClassOf>
   </owl:Class>
   <owl:Class xmlns:owl="http://www.w3.org/2002/07/owl#" rdf:about="#partitiveCase">
      <rdfs:comment>subClassOf case inferred from naming conventions.</rdfs:comment>
      <rdfs:subClassOf>
         <owl:Class rdf:about="#case"/>
      </rdfs:subClassOf>
   </owl:Class>
   <owl:Class xmlns:owl="http://www.w3.org/2002/07/owl#" rdf:about="#passiveVoice">
      <rdfs:comment>subClassOf voice inferred from naming conventions.</rdfs:comment>
      <rdfs:subClassOf>
         <owl:Class rdf:about="#voice"/>
      </rdfs:subClassOf>
   </owl:Class>
   <owl:Class xmlns:owl="http://www.w3.org/2002/07/owl#" rdf:about="#pastParticipleAdjective">
      <rdfs:comment>subClassOf adjective inferred from naming conventions.</rdfs:comment>
      <rdfs:subClassOf>
         <owl:Class rdf:about="#adjective"/>
      </rdfs:subClassOf>
   </owl:Class>
   <owl:Class xmlns:owl="http://www.w3.org/2002/07/owl#" rdf:about="#pastParticipleAdjective">
      <rdfs:comment>subClassOf participleAdjective inferred from naming conventions.</rdfs:comment>
      <rdfs:subClassOf>
         <owl:Class rdf:about="#participleAdjective"/>
      </rdfs:subClassOf>
   </owl:Class>
   <owl:Class xmlns:owl="http://www.w3.org/2002/07/owl#" rdf:about="#patternType">
      <rdfs:comment>subClassOf type inferred from naming conventions.</rdfs:comment>
      <rdfs:subClassOf>
         <owl:Class rdf:about="#type"/>
      </rdfs:subClassOf>
   </owl:Class>
   <owl:Class xmlns:owl="http://www.w3.org/2002/07/owl#" rdf:about="#personalPronoun">
      <rdfs:comment>subClassOf pronoun inferred from naming conventions.</rdfs:comment>
      <rdfs:subClassOf>
         <owl:Class rdf:about="#pronoun"/>
      </rdfs:subClassOf>
   </owl:Class>
   <owl:Class xmlns:owl="http://www.w3.org/2002/07/owl#" rdf:about="#phoneticForm">
      <rdfs:comment>subClassOf form inferred from naming conventions.</rdfs:comment>
      <rdfs:subClassOf>
         <owl:Class rdf:about="#form"/>
      </rdfs:subClassOf>
   </owl:Class>
   <owl:Class xmlns:owl="http://www.w3.org/2002/07/owl#" rdf:about="#phoneticOperator">
      <rdfs:comment>subClassOf operator inferred from naming conventions.</rdfs:comment>
      <rdfs:subClassOf>
         <owl:Class rdf:about="#operator"/>
      </rdfs:subClassOf>
   </owl:Class>
   <owl:Class xmlns:owl="http://www.w3.org/2002/07/owl#" rdf:about="#pluralType">
      <rdfs:comment>subClassOf type inferred from naming conventions.</rdfs:comment>
      <rdfs:subClassOf>
         <owl:Class rdf:about="#type"/>
      </rdfs:subClassOf>
   </owl:Class>
   <owl:Class xmlns:owl="http://www.w3.org/2002/07/owl#" rdf:about="#possessiveDeterminer">
      <rdfs:comment>subClassOf determiner inferred from naming conventions.</rdfs:comment>
      <rdfs:subClassOf>
         <owl:Class rdf:about="#determiner"/>
      </rdfs:subClassOf>
   </owl:Class>
   <owl:Class xmlns:owl="http://www.w3.org/2002/07/owl#" rdf:about="#possessiveParticle">
      <rdfs:comment>subClassOf particle inferred from naming conventions.</rdfs:comment>
      <rdfs:subClassOf>
         <owl:Class rdf:about="#particle"/>
      </rdfs:subClassOf>
   </owl:Class>
   <owl:Class xmlns:owl="http://www.w3.org/2002/07/owl#" rdf:about="#possessivePronoun">
      <rdfs:comment>subClassOf pronoun inferred from naming conventions.</rdfs:comment>
      <rdfs:subClassOf>
         <owl:Class rdf:about="#pronoun"/>
      </rdfs:subClassOf>
   </owl:Class>
   <owl:Class xmlns:owl="http://www.w3.org/2002/07/owl#" rdf:ID="modifier"/>
   <owl:Class xmlns:owl="http://www.w3.org/2002/07/owl#" rdf:about="#postModifier">
      <rdfs:comment>subClassOf modifier inferred from naming conventions.</rdfs:comment>
      <rdfs:subClassOf>
         <owl:Class rdf:about="#modifier"/>
      </rdfs:subClassOf>
   </owl:Class>
   <owl:Class xmlns:owl="http://www.w3.org/2002/07/owl#" rdf:about="#preModifier">
      <rdfs:comment>subClassOf modifier inferred from naming conventions.</rdfs:comment>
      <rdfs:subClassOf>
         <owl:Class rdf:about="#modifier"/>
      </rdfs:subClassOf>
   </owl:Class>
   <owl:Class xmlns:owl="http://www.w3.org/2002/07/owl#"
              rdf:about="#presentParticipleAdjective">
      <rdfs:comment>subClassOf adjective inferred from naming conventions.</rdfs:comment>
      <rdfs:subClassOf>
         <owl:Class rdf:about="#adjective"/>
      </rdfs:subClassOf>
   </owl:Class>
   <owl:Class xmlns:owl="http://www.w3.org/2002/07/owl#"
              rdf:about="#presentParticipleAdjective">
      <rdfs:comment>subClassOf participleAdjective inferred from naming conventions.</rdfs:comment>
      <rdfs:subClassOf>
         <owl:Class rdf:about="#participleAdjective"/>
      </rdfs:subClassOf>
   </owl:Class>
   <owl:Class xmlns:owl="http://www.w3.org/2002/07/owl#" rdf:about="#prolativeCase">
      <rdfs:comment>subClassOf case inferred from naming conventions.</rdfs:comment>
      <rdfs:subClassOf>
         <owl:Class rdf:about="#case"/>
      </rdfs:subClassOf>
   </owl:Class>
   <owl:Class xmlns:owl="http://www.w3.org/2002/07/owl#" rdf:about="#properNoun">
      <rdfs:comment>subClassOf noun inferred from naming conventions.</rdfs:comment>
      <rdfs:subClassOf>
         <owl:Class rdf:about="#noun"/>
      </rdfs:subClassOf>
   </owl:Class>
   <owl:Class xmlns:owl="http://www.w3.org/2002/07/owl#" rdf:about="#qualifierAdjective">
      <rdfs:comment>subClassOf adjective inferred from naming conventions.</rdfs:comment>
      <rdfs:subClassOf>
         <owl:Class rdf:about="#adjective"/>
      </rdfs:subClassOf>
   </owl:Class>
   <owl:Class xmlns:owl="http://www.w3.org/2002/07/owl#" rdf:about="#questionMark">
      <rdfs:comment>subClassOf mark inferred from naming conventions.</rdfs:comment>
      <rdfs:subClassOf>
         <owl:Class rdf:about="#mark"/>
      </rdfs:subClassOf>
   </owl:Class>
   <owl:Class xmlns:owl="http://www.w3.org/2002/07/owl#" rdf:about="#rarelyUsed">
      <rdfs:comment>subClassOf used inferred from naming conventions.</rdfs:comment>
      <rdfs:subClassOf>
         <owl:Class rdf:about="#used"/>
      </rdfs:subClassOf>
   </owl:Class>
   <owl:Class xmlns:owl="http://www.w3.org/2002/07/owl#" rdf:about="#reciprocalPronoun">
      <rdfs:comment>subClassOf pronoun inferred from naming conventions.</rdfs:comment>
      <rdfs:subClassOf>
         <owl:Class rdf:about="#pronoun"/>
      </rdfs:subClassOf>
   </owl:Class>
   <owl:Class xmlns:owl="http://www.w3.org/2002/07/owl#" rdf:about="#reduplicationType">
      <rdfs:comment>subClassOf type inferred from naming conventions.</rdfs:comment>
      <rdfs:subClassOf>
         <owl:Class rdf:about="#type"/>
      </rdfs:subClassOf>
   </owl:Class>
   <owl:Class xmlns:owl="http://www.w3.org/2002/07/owl#" rdf:about="#referentType">
      <rdfs:comment>subClassOf type inferred from naming conventions.</rdfs:comment>
      <rdfs:subClassOf>
         <owl:Class rdf:about="#type"/>
      </rdfs:subClassOf>
   </owl:Class>
   <owl:Class xmlns:owl="http://www.w3.org/2002/07/owl#" rdf:about="#reflexiveDeterminer">
      <rdfs:comment>subClassOf determiner inferred from naming conventions.</rdfs:comment>
      <rdfs:subClassOf>
         <owl:Class rdf:about="#determiner"/>
      </rdfs:subClassOf>
   </owl:Class>
   <owl:Class xmlns:owl="http://www.w3.org/2002/07/owl#" rdf:about="#reflexivePronoun">
      <rdfs:comment>subClassOf pronoun inferred from naming conventions.</rdfs:comment>
      <rdfs:subClassOf>
         <owl:Class rdf:about="#pronoun"/>
      </rdfs:subClassOf>
   </owl:Class>
   <owl:Class xmlns:owl="http://www.w3.org/2002/07/owl#" rdf:about="#relationNoun">
      <rdfs:comment>subClassOf noun inferred from naming conventions.</rdfs:comment>
      <rdfs:subClassOf>
         <owl:Class rdf:about="#noun"/>
      </rdfs:subClassOf>
   </owl:Class>
   <owl:Class xmlns:owl="http://www.w3.org/2002/07/owl#" rdf:about="#relativeDeterminer">
      <rdfs:comment>subClassOf determiner inferred from naming conventions.</rdfs:comment>
      <rdfs:subClassOf>
         <owl:Class rdf:about="#determiner"/>
      </rdfs:subClassOf>
   </owl:Class>
   <owl:Class xmlns:owl="http://www.w3.org/2002/07/owl#" rdf:about="#relativeParticle">
      <rdfs:comment>subClassOf particle inferred from naming conventions.</rdfs:comment>
      <rdfs:subClassOf>
         <owl:Class rdf:about="#particle"/>
      </rdfs:subClassOf>
   </owl:Class>
   <owl:Class xmlns:owl="http://www.w3.org/2002/07/owl#" rdf:about="#relativePronoun">
      <rdfs:comment>subClassOf pronoun inferred from naming conventions.</rdfs:comment>
      <rdfs:subClassOf>
         <owl:Class rdf:about="#pronoun"/>
      </rdfs:subClassOf>
   </owl:Class>
   <owl:Class xmlns:owl="http://www.w3.org/2002/07/owl#" rdf:about="#removeAfter">
      <rdfs:comment>subClassOf after inferred from naming conventions.</rdfs:comment>
      <rdfs:subClassOf>
         <owl:Class rdf:about="#after"/>
      </rdfs:subClassOf>
   </owl:Class>
   <owl:Class xmlns:owl="http://www.w3.org/2002/07/owl#" rdf:about="#removeBefore">
      <rdfs:comment>subClassOf before inferred from naming conventions.</rdfs:comment>
      <rdfs:subClassOf>
         <owl:Class rdf:about="#before"/>
      </rdfs:subClassOf>
   </owl:Class>
   <owl:Class xmlns:owl="http://www.w3.org/2002/07/owl#" rdf:about="#rightEnvironment">
      <rdfs:comment>subClassOf environment inferred from naming conventions.</rdfs:comment>
      <rdfs:subClassOf>
         <owl:Class rdf:about="#environment"/>
      </rdfs:subClassOf>
   </owl:Class>
   <owl:Class xmlns:owl="http://www.w3.org/2002/07/owl#" rdf:about="#scriptCoding">
      <rdfs:comment>subClassOf coding inferred from naming conventions.</rdfs:comment>
      <rdfs:subClassOf>
         <owl:Class rdf:about="#coding"/>
      </rdfs:subClassOf>
   </owl:Class>
   <owl:Class xmlns:owl="http://www.w3.org/2002/07/owl#" rdf:about="#secondPerson">
      <rdfs:comment>subClassOf person inferred from naming conventions.</rdfs:comment>
      <rdfs:subClassOf>
         <owl:Class rdf:about="#person"/>
      </rdfs:subClassOf>
   </owl:Class>
   <owl:Class xmlns:owl="http://www.w3.org/2002/07/owl#" rdf:about="#secondaryPunctuation">
      <rdfs:comment>subClassOf punctuation inferred from naming conventions.</rdfs:comment>
      <rdfs:subClassOf>
         <owl:Class rdf:about="#punctuation"/>
      </rdfs:subClassOf>
   </owl:Class>
   <owl:Class xmlns:owl="http://www.w3.org/2002/07/owl#" rdf:about="#semiColon">
      <rdfs:comment>subClassOf colon inferred from naming conventions.</rdfs:comment>
      <rdfs:subClassOf>
         <owl:Class rdf:about="#colon"/>
      </rdfs:subClassOf>
   </owl:Class>
   <owl:Class xmlns:owl="http://www.w3.org/2002/07/owl#" rdf:about="#shortArticle">
      <rdfs:comment>subClassOf article inferred from naming conventions.</rdfs:comment>
      <rdfs:subClassOf>
         <owl:Class rdf:about="#article"/>
      </rdfs:subClassOf>
   </owl:Class>
   <owl:Class xmlns:owl="http://www.w3.org/2002/07/owl#" rdf:about="#simplePreposition">
      <rdfs:comment>subClassOf preposition inferred from naming conventions.</rdfs:comment>
      <rdfs:subClassOf>
         <owl:Class rdf:about="#preposition"/>
      </rdfs:subClassOf>
   </owl:Class>
   <owl:Class xmlns:owl="http://www.w3.org/2002/07/owl#" rdf:about="#slangRegister">
      <rdfs:comment>subClassOf register inferred from naming conventions.</rdfs:comment>
      <rdfs:subClassOf>
         <owl:Class rdf:about="#register"/>
      </rdfs:subClassOf>
   </owl:Class>
   <owl:Class xmlns:owl="http://www.w3.org/2002/07/owl#" rdf:about="#sociativeCase">
      <rdfs:comment>subClassOf case inferred from naming conventions.</rdfs:comment>
      <rdfs:subClassOf>
         <owl:Class rdf:about="#case"/>
      </rdfs:subClassOf>
   </owl:Class>
   <owl:Class xmlns:owl="http://www.w3.org/2002/07/owl#" rdf:about="#stemRank">
      <rdfs:comment>subClassOf rank inferred from naming conventions.</rdfs:comment>
      <rdfs:subClassOf>
         <owl:Class rdf:about="#rank"/>
      </rdfs:subClassOf>
   </owl:Class>
   <owl:Class xmlns:owl="http://www.w3.org/2002/07/owl#" rdf:about="#stringValue">
      <rdfs:comment>subClassOf value inferred from naming conventions.</rdfs:comment>
      <rdfs:subClassOf>
         <owl:Class rdf:about="#value"/>
      </rdfs:subClassOf>
   </owl:Class>
   <owl:Class xmlns:owl="http://www.w3.org/2002/07/owl#" rdf:about="#strongPersonalPronoun">
      <rdfs:comment>subClassOf pronoun inferred from naming conventions.</rdfs:comment>
      <rdfs:subClassOf>
         <owl:Class rdf:about="#pronoun"/>
      </rdfs:subClassOf>
   </owl:Class>
   <owl:Class xmlns:owl="http://www.w3.org/2002/07/owl#" rdf:about="#strongPersonalPronoun">
      <rdfs:comment>subClassOf personalPronoun inferred from naming conventions.</rdfs:comment>
      <rdfs:subClassOf>
         <owl:Class rdf:about="#personalPronoun"/>
      </rdfs:subClassOf>
   </owl:Class>
   <owl:Class xmlns:owl="http://www.w3.org/2002/07/owl#" rdf:about="#subjectPerson">
      <rdfs:comment>subClassOf person inferred from naming conventions.</rdfs:comment>
      <rdfs:subClassOf>
         <owl:Class rdf:about="#person"/>
      </rdfs:subClassOf>
   </owl:Class>
   <owl:Class xmlns:owl="http://www.w3.org/2002/07/owl#" rdf:about="#sublativeCase">
      <rdfs:comment>subClassOf case inferred from naming conventions.</rdfs:comment>
      <rdfs:subClassOf>
         <owl:Class rdf:about="#case"/>
      </rdfs:subClassOf>
   </owl:Class>
   <owl:Class xmlns:owl="http://www.w3.org/2002/07/owl#" rdf:about="#subordinatingConjunction">
      <rdfs:comment>subClassOf conjunction inferred from naming conventions.</rdfs:comment>
      <rdfs:subClassOf>
         <owl:Class rdf:about="#conjunction"/>
      </rdfs:subClassOf>
   </owl:Class>
   <owl:Class xmlns:owl="http://www.w3.org/2002/07/owl#" rdf:about="#superessiveCase">
      <rdfs:comment>subClassOf case inferred from naming conventions.</rdfs:comment>
      <rdfs:subClassOf>
         <owl:Class rdf:about="#case"/>
      </rdfs:subClassOf>
   </owl:Class>
   <owl:Class xmlns:owl="http://www.w3.org/2002/07/owl#" rdf:about="#superlativeParticle">
      <rdfs:comment>subClassOf particle inferred from naming conventions.</rdfs:comment>
      <rdfs:subClassOf>
         <owl:Class rdf:about="#particle"/>
      </rdfs:subClassOf>
   </owl:Class>
   <owl:Class xmlns:owl="http://www.w3.org/2002/07/owl#" rdf:about="#syntacticType">
      <rdfs:comment>subClassOf type inferred from naming conventions.</rdfs:comment>
      <rdfs:subClassOf>
         <owl:Class rdf:about="#type"/>
      </rdfs:subClassOf>
   </owl:Class>
   <owl:Class xmlns:owl="http://www.w3.org/2002/07/owl#" rdf:about="#tabooRegister">
      <rdfs:comment>subClassOf register inferred from naming conventions.</rdfs:comment>
      <rdfs:subClassOf>
         <owl:Class rdf:about="#register"/>
      </rdfs:subClassOf>
   </owl:Class>
   <owl:Class xmlns:owl="http://www.w3.org/2002/07/owl#" rdf:about="#technicalRegister">
      <rdfs:comment>subClassOf register inferred from naming conventions.</rdfs:comment>
      <rdfs:subClassOf>
         <owl:Class rdf:about="#register"/>
      </rdfs:subClassOf>
   </owl:Class>
   <owl:Class xmlns:owl="http://www.w3.org/2002/07/owl#" rdf:about="#terminativeCase">
      <rdfs:comment>subClassOf case inferred from naming conventions.</rdfs:comment>
      <rdfs:subClassOf>
         <owl:Class rdf:about="#case"/>
      </rdfs:subClassOf>
   </owl:Class>
   <owl:Class xmlns:owl="http://www.w3.org/2002/07/owl#" rdf:about="#thirdPerson">
      <rdfs:comment>subClassOf person inferred from naming conventions.</rdfs:comment>
      <rdfs:subClassOf>
         <owl:Class rdf:about="#person"/>
      </rdfs:subClassOf>
   </owl:Class>
   <owl:Class xmlns:owl="http://www.w3.org/2002/07/owl#" rdf:about="#transformType">
      <rdfs:comment>subClassOf type inferred from naming conventions.</rdfs:comment>
      <rdfs:subClassOf>
         <owl:Class rdf:about="#type"/>
      </rdfs:subClassOf>
   </owl:Class>
   <owl:Class xmlns:owl="http://www.w3.org/2002/07/owl#" rdf:about="#translativeCase">
      <rdfs:comment>subClassOf case inferred from naming conventions.</rdfs:comment>
      <rdfs:subClassOf>
         <owl:Class rdf:about="#case"/>
      </rdfs:subClassOf>
   </owl:Class>
   <owl:Class xmlns:owl="http://www.w3.org/2002/07/owl#" rdf:about="#unclassifiedParticle">
      <rdfs:comment>subClassOf particle inferred from naming conventions.</rdfs:comment>
      <rdfs:subClassOf>
         <owl:Class rdf:about="#particle"/>
      </rdfs:subClassOf>
   </owl:Class>
   <owl:Class xmlns:owl="http://www.w3.org/2002/07/owl#" rdf:about="#unclassifiedPunctuation">
      <rdfs:comment>subClassOf punctuation inferred from naming conventions.</rdfs:comment>
      <rdfs:subClassOf>
         <owl:Class rdf:about="#punctuation"/>
      </rdfs:subClassOf>
   </owl:Class>
   <owl:Class xmlns:owl="http://www.w3.org/2002/07/owl#" rdf:about="#unclassifiedResidual">
      <rdfs:comment>subClassOf residual inferred from naming conventions.</rdfs:comment>
      <rdfs:subClassOf>
         <owl:Class rdf:about="#residual"/>
      </rdfs:subClassOf>
   </owl:Class>
   <owl:Class xmlns:owl="http://www.w3.org/2002/07/owl#" rdf:about="#vocativeCase">
      <rdfs:comment>subClassOf case inferred from naming conventions.</rdfs:comment>
      <rdfs:subClassOf>
         <owl:Class rdf:about="#case"/>
      </rdfs:subClassOf>
   </owl:Class>
   <owl:Class xmlns:owl="http://www.w3.org/2002/07/owl#" rdf:about="#voiceNoun">
      <rdfs:comment>subClassOf noun inferred from naming conventions.</rdfs:comment>
      <rdfs:subClassOf>
         <owl:Class rdf:about="#noun"/>
      </rdfs:subClassOf>
   </owl:Class>
   <owl:Class xmlns:owl="http://www.w3.org/2002/07/owl#" rdf:about="#vulgarRegister">
      <rdfs:comment>subClassOf register inferred from naming conventions.</rdfs:comment>
      <rdfs:subClassOf>
         <owl:Class rdf:about="#register"/>
      </rdfs:subClassOf>
   </owl:Class>
   <owl:Class xmlns:owl="http://www.w3.org/2002/07/owl#" rdf:about="#weakPersonalPronoun">
      <rdfs:comment>subClassOf pronoun inferred from naming conventions.</rdfs:comment>
      <rdfs:subClassOf>
         <owl:Class rdf:about="#pronoun"/>
      </rdfs:subClassOf>
   </owl:Class>
   <owl:Class xmlns:owl="http://www.w3.org/2002/07/owl#" rdf:about="#weakPersonalPronoun">
      <rdfs:comment>subClassOf personalPronoun inferred from naming conventions.</rdfs:comment>
      <rdfs:subClassOf>
         <owl:Class rdf:about="#personalPronoun"/>
      </rdfs:subClassOf>
   </owl:Class>
   <owl:Class xmlns:owl="http://www.w3.org/2002/07/owl#" rdf:about="#writtenForm">
      <rdfs:comment>subClassOf form inferred from naming conventions.</rdfs:comment>
      <rdfs:subClassOf>
         <owl:Class rdf:about="#form"/>
      </rdfs:subClassOf>
   </owl:Class>
   <owl:Class xmlns:owl="http://www.w3.org/2002/07/owl#" rdf:ID="attributiveAdjective">
      <dcr:datcat rdf:resource="http://www.isocat.org/datcat/DC-1243"/>
      <rdfs:label xml:lang="en">Attributive adjective</rdfs:label>
      <rdfs:comment xml:lang="en"> An Attributive Adjective comes before a Noun and not after a Copula
   Verb, like BE, SEEM, etc. (of an adjective or adjectival phrase) modifying a noun and
   constituting part of the same noun phrase, in English normally preceding the noun, as black in
   Fido is a black dog (as opposed to Fido is black) </rdfs:comment>
   </owl:Class>
   <owl:Class xmlns:owl="http://www.w3.org/2002/07/owl#" rdf:ID="complement">
      <dcr:datcat rdf:resource="http://www.isocat.org/datcat/DC-1257"/>
      <rdfs:label xml:lang="en">Complement</rdfs:label>
      <rdfs:comment xml:lang="en"> - A noun phrase that follows a copula or similar verb, as for example
   an idiot in the sentence He is an idiot. - A clause that serves as the subject or direct object
   of a verb or the direct object of a preposition, as for example that he would be early in the
   sentence I hoped that he would be early. </rdfs:comment>
   </owl:Class>
   <owl:Class xmlns:owl="http://www.w3.org/2002/07/owl#" rdf:ID="syntacticConstituent">
      <dcr:datcat rdf:resource="http://www.isocat.org/datcat/DC-1261"/>
      <rdfs:label xml:lang="en">Constituent</rdfs:label>
      <rdfs:comment xml:lang="en"> A constituent is one of two or more grammatical units that enter
   syntactically or morphologically into a construction at any level. </rdfs:comment>
   </owl:Class>
   <owl:Class xmlns:owl="http://www.w3.org/2002/07/owl#" rdf:ID="directObject">
      <dcr:datcat rdf:resource="http://www.isocat.org/datcat/DC-1274"/>
      <rdfs:label xml:lang="en">Direct object</rdfs:label>
      <rdfs:comment xml:lang="en"> A direct object is a grammatical relation that exhibits a combination
   of certain independent syntactic properties, such as the following: - The usual grammatical
   characteristics of the patient of typically transitive verbs - A particular case marking - A
   particular clause position - The conditioning of an agreement affix on the verb - The capability
   of becoming the clause subject in passivization - The capability of reflexivization A noun,
   pronoun, or noun phrase whose referent receives the direct action of a verb. </rdfs:comment>
   </owl:Class>
   <owl:Class xmlns:owl="http://www.w3.org/2002/07/owl#" rdf:ID="ditransitive">
      <dcr:datcat rdf:resource="http://www.isocat.org/datcat/DC-1275"/>
      <rdfs:label xml:lang="en">Ditransitive</rdfs:label>
      <rdfs:comment xml:lang="en"> Ditransitivity (or Bitransitivity) is a term which describes a verb
   or clause which takes two objects. </rdfs:comment>
   </owl:Class>
   <owl:Class xmlns:owl="http://www.w3.org/2002/07/owl#" rdf:ID="futurePerfect">
      <dcr:datcat rdf:resource="http://www.isocat.org/datcat/DC-1292"/>
      <rdfs:label xml:lang="en">Future perfect</rdfs:label>
      <rdfs:comment xml:lang="en"> A verb tense that refers to an action or state of being completed in
   the future. into English requires the use of the auxiliary verbs will/shall have. Denoting a
   tense of verbs describing an action that will have been performed by a certain time. In English
   this is formed with will have or shall have plus the past participle. </rdfs:comment>
   </owl:Class>
   <owl:Class xmlns:owl="http://www.w3.org/2002/07/owl#" rdf:ID="gerundive">
      <dcr:datcat rdf:resource="http://www.isocat.org/datcat/DC-1294"/>
      <rdfs:label xml:lang="en">Gerundive</rdfs:label>
      <rdfs:comment xml:lang="en"> an adjective formed from a verb, expressing the desirability of the
   activity denoted by the verb a noun formed from a verb, denoting an action or state. In English,
   the gerund, like the present participle, is formed in -ing </rdfs:comment>
   </owl:Class>
   <owl:Class xmlns:owl="http://www.w3.org/2002/07/owl#" rdf:ID="grammaticalFunction">
      <dcr:datcat rdf:resource="http://www.isocat.org/datcat/DC-1296"/>
      <rdfs:label xml:lang="en">Grammatical function</rdfs:label>
   </owl:Class>
   <owl:Class xmlns:owl="http://www.w3.org/2002/07/owl#" rdf:ID="impersonal">
      <dcr:datcat rdf:resource="http://www.isocat.org/datcat/DC-1306"/>
      <rdfs:label xml:lang="en">Impersonal</rdfs:label>
      <rdfs:comment xml:lang="en"> An impersonal verb is a verb that - occurs only in third person
   singular forms - has no specified agent , and - has a dummy subject or no subject. (of a verb)
   having no logical subject. Usually in English the pronoun it is used in such cases as a
   grammatical subject, as for example in It is raining. (of a pronoun) not denoting a person
  </rdfs:comment>
   </owl:Class>
   <owl:Class xmlns:owl="http://www.w3.org/2002/07/owl#" rdf:ID="indirectObject">
      <dcr:datcat rdf:resource="http://www.isocat.org/datcat/DC-1310"/>
      <rdfs:label xml:lang="en">Indirect object</rdfs:label>
      <rdfs:comment xml:lang="en"> An indirect object is a grammatical relation that is one means of
   expressing the semantic role of goal and other similar roles. It is proposed for languages in
   which the role is distinct from the direct object and the oblique object on the basis of multiple
   independent syntactic or morphological criteria, such as the following: - Having a particular
   case marking, commonly dative - Governing an agreement affix on the verb, such as person or
   number - Being distinct from oblique relations in that it may be relativized A noun, pronoun, or
   noun phrase indicating the recipient or beneficiary of the action of a verb and its direct object
  </rdfs:comment>
   </owl:Class>
   <owl:Class xmlns:owl="http://www.w3.org/2002/07/owl#" rdf:ID="interrogative">
      <dcr:datcat rdf:resource="http://www.isocat.org/datcat/DC-1319"/>
      <rdfs:label xml:lang="en">Interrogative</rdfs:label>
      <rdfs:comment xml:lang="en"> An interrogative mood is an epistemic mood that signals that the
   speaker wishes to elicit information concerning the content of his or her utterance from the
   addressee. Denoting or belonging to a class of words, such as which and whom, that are
   determiners, adjectives, or pronouns and serve to question which individual referent or referents
   are intended </rdfs:comment>
   </owl:Class>
   <owl:Class xmlns:owl="http://www.w3.org/2002/07/owl#" rdf:ID="intransitive">
      <dcr:datcat rdf:resource="http://www.isocat.org/datcat/DC-1322"/>
      <rdfs:label xml:lang="en">Intransitive</rdfs:label>
      <rdfs:comment xml:lang="en"> Refers to a verb that does not take a direct object; that is, to a
   verb that does not express an action which directly affects another person or thing.
  </rdfs:comment>
   </owl:Class>
   <owl:Class xmlns:owl="http://www.w3.org/2002/07/owl#" rdf:ID="order">
      <dcr:datcat rdf:resource="http://www.isocat.org/datcat/DC-1337"/>
      <rdfs:label xml:lang="en">Order</rdfs:label>
      <rdfs:comment xml:lang="en">A state in which all components or elements are arranged logically,
   comprehensibly, or naturally </rdfs:comment>
   </owl:Class>
   <owl:Class xmlns:owl="http://www.w3.org/2002/07/owl#" rdf:ID="pastPerfect">
      <dcr:datcat rdf:resource="http://www.isocat.org/datcat/DC-1348"/>
      <rdfs:label xml:lang="en">Past perfect</rdfs:label>
      <rdfs:comment xml:lang="en">Past perfect tense is an absolute-relative tense that refers to a time
   in the past relative to a reference point, which itself is in the past relative to the moment of
   utterance denoting a tense of verbs used in relating past events where the action had already
   occurred at the time of the action of a main verb that is itself in a past tense. In English this
   is a compound tense formed with had plus the past participle </rdfs:comment>
   </owl:Class>
   <owl:Class xmlns:owl="http://www.w3.org/2002/07/owl#" rdf:ID="perfect">
      <dcr:datcat rdf:resource="http://www.isocat.org/datcat/DC-1351"/>
      <rdfs:label xml:lang="en">Perfect</rdfs:label>
      <rdfs:comment xml:lang="en"> A verb tense that refers to completed action in the past. It
   corresponds to three English tenses. </rdfs:comment>
   </owl:Class>
   <owl:Class xmlns:owl="http://www.w3.org/2002/07/owl#" rdf:ID="pluperfect">
      <dcr:datcat rdf:resource="http://www.isocat.org/datcat/DC-1353"/>
      <rdfs:label xml:lang="en">Pluperfect</rdfs:label>
      <rdfs:comment xml:lang="en">A verb tense that refers to action or state of being completed before
   some other event in the past. Its translation into English requires the use of the auxiliariy
   verb had. </rdfs:comment>
   </owl:Class>
   <owl:Class xmlns:owl="http://www.w3.org/2002/07/owl#" rdf:ID="pronominal">
      <dcr:datcat rdf:resource="http://www.isocat.org/datcat/DC-1369"/>
      <rdfs:label xml:lang="en">Pronominal</rdfs:label>
      <rdfs:comment xml:lang="en"> A pronominal is a phrase that functions as a pronoun </rdfs:comment>
   </owl:Class>
   <owl:Class xmlns:owl="http://www.w3.org/2002/07/owl#" rdf:ID="qualifier">
      <dcr:datcat rdf:resource="http://www.isocat.org/datcat/DC-1373"/>
      <rdfs:label xml:lang="en">Qualifier</rdfs:label>
      <rdfs:comment xml:lang="en"> Also called MODIFIER : A word or phrase that qualifies the sense of
   another word; for example, the noun alarm is a modifier of clock in "alarm clock" and the phrase
   every day is an adverbial modifier of walks in "he walks every day" </rdfs:comment>
   </owl:Class>
   <owl:Class xmlns:owl="http://www.w3.org/2002/07/owl#" rdf:ID="subject">
      <dcr:datcat rdf:resource="http://www.isocat.org/datcat/DC-1391"/>
      <rdfs:label xml:lang="en">Subject</rdfs:label>
      <rdfs:comment xml:lang="en"> The noun or pronoun that, with all of its modifiers, immediately
   precedes the verb. He Is defined entierely in terms of position. A word, phrase, or formal
   expression about which something is predicated or stated in a sentence; for example, the cat in
   the sentence The cat catches mice. </rdfs:comment>
   </owl:Class>
   <owl:Class xmlns:owl="http://www.w3.org/2002/07/owl#" rdf:ID="substantiveAdjective">
      <dcr:datcat rdf:resource="http://www.isocat.org/datcat/DC-1394"/>
      <rdfs:label xml:lang="en">Substantive adjective</rdfs:label>
      <rdfs:comment xml:lang="en">An adjective that modifies an implied, but not expressed, noun. When
   translating such an adjective into English, you must supply the missing noun. </rdfs:comment>
   </owl:Class>
   <owl:Class xmlns:owl="http://www.w3.org/2002/07/owl#" rdf:ID="supine">
      <dcr:datcat rdf:resource="http://www.isocat.org/datcat/DC-1397"/>
      <rdfs:label xml:lang="en">Supine</rdfs:label>
      <rdfs:comment xml:lang="en"> The supine form of the verb in Swedish is used with the auxiliary
   verb ha (`to have') to form the perfective. The supine form is easy to spot a verb form that
   always ends with a t. </rdfs:comment>
   </owl:Class>
   <owl:Class xmlns:owl="http://www.w3.org/2002/07/owl#" rdf:ID="syntax">
      <dcr:datcat rdf:resource="http://www.isocat.org/datcat/DC-1399"/>
      <rdfs:label xml:lang="en">Syntax</rdfs:label>
      <rdfs:comment xml:lang="en"> The relationship of words to each other in a sentence </rdfs:comment>
   </owl:Class>
   <owl:Class xmlns:owl="http://www.w3.org/2002/07/owl#" rdf:ID="transgressive">
      <dcr:datcat rdf:resource="http://www.isocat.org/datcat/DC-1404"/>
      <rdfs:label xml:lang="en">Transgressive</rdfs:label>
      <rdfs:comment xml:lang="en">present (action in the same time as of the predicate): The dog going
   through the house barks. past (action premature to the one of predicate): He has started to read
   the book after he had sat down. </rdfs:comment>
   </owl:Class>
   <owl:Class xmlns:owl="http://www.w3.org/2002/07/owl#" rdf:ID="transitive">
      <dcr:datcat rdf:resource="http://www.isocat.org/datcat/DC-1405"/>
      <rdfs:label xml:lang="en">Transitive</rdfs:label>
      <rdfs:comment xml:lang="en"> A verb which takes a direct object; that is, a verb that expresses an
   action which directly affects another person or thing. </rdfs:comment>
   </owl:Class>
   <owl:Class xmlns:owl="http://www.w3.org/2002/07/owl#" rdf:ID="valency">
      <dcr:datcat rdf:resource="http://www.isocat.org/datcat/DC-1410"/>
      <rdfs:label xml:lang="en">Valency</rdfs:label>
   </owl:Class>
   <owl:Class xmlns:owl="http://www.w3.org/2002/07/owl#" rdf:ID="verbFrame">
      <dcr:datcat rdf:resource="http://www.isocat.org/datcat/DC-1411"/>
      <rdfs:label xml:lang="en">Verb frame</rdfs:label>
      <rdfs:comment xml:lang="en"> A word used to express an action or state of being. Finite verbs have
   five variables: person, number, tense, mood, and voice. </rdfs:comment>
   </owl:Class>
   <owl:Class xmlns:owl="http://www.w3.org/2002/07/owl#" rdf:ID="abbreviation">
      <dcr:datcat rdf:resource="http://www.isocat.org/datcat/DC-1418"/>
      <rdfs:label xml:lang="en">abbreviation</rdfs:label>
      <rdfs:comment xml:lang="en">Designation formed by omitting words or letters from a longer form and
   refering to the same concept.</rdfs:comment>
   </owl:Class>
   <owl:Class xmlns:owl="http://www.w3.org/2002/07/owl#" rdf:ID="abessiveCase">
      <dcr:datcat rdf:resource="http://www.isocat.org/datcat/DC-1223"/>
      <rdfs:label xml:lang="en">abessive case</rdfs:label>
      <rdfs:comment xml:lang="en">Case that expresses the lack or absence of the referent of the noun it
   marks.</rdfs:comment>
   </owl:Class>
   <owl:Class xmlns:owl="http://www.w3.org/2002/07/owl#" rdf:ID="ablativeCase">
      <dcr:datcat rdf:resource="http://www.isocat.org/datcat/DC-1224"/>
      <rdfs:label xml:lang="en">ablative case</rdfs:label>
      <rdfs:comment xml:lang="en">Case used to typically indicate locative or instrumental function.
  </rdfs:comment>
   </owl:Class>
   <owl:Class xmlns:owl="http://www.w3.org/2002/07/owl#" rdf:ID="absolutiveCase">
      <dcr:datcat rdf:resource="http://www.isocat.org/datcat/DC-1225"/>
      <rdfs:label xml:lang="en">absolutive case</rdfs:label>
      <rdfs:comment xml:lang="en">Case for nouns in ergative-absolute languages that would generally be
   the subjects of intransitive verbs or the objects of transitive verbs in the translational
   equivalents of nominative-accusative languages such as English.</rdfs:comment>
   </owl:Class>
   <owl:Class xmlns:owl="http://www.w3.org/2002/07/owl#" rdf:ID="accusativeCase">
      <dcr:datcat rdf:resource="http://www.isocat.org/datcat/DC-1226"/>
      <rdfs:label xml:lang="en">accusative case</rdfs:label>
      <rdfs:comment xml:lang="en">Case used to indicate direct object. </rdfs:comment>
   </owl:Class>
   <owl:Class xmlns:owl="http://www.w3.org/2002/07/owl#" rdf:ID="activeVoice">
      <dcr:datcat rdf:resource="http://www.isocat.org/datcat/DC-1227"/>
      <rdfs:label xml:lang="en">active voice</rdfs:label>
      <rdfs:comment xml:lang="en">Value that expresses the situation where the grammatical subject is
   also the semantic actor of the verb.</rdfs:comment>
   </owl:Class>
   <owl:Class xmlns:owl="http://www.w3.org/2002/07/owl#" rdf:ID="add">
      <dcr:datcat rdf:resource="http://www.isocat.org/datcat/DC-2093"/>
      <rdfs:label xml:lang="en">add</rdfs:label>
      <rdfs:comment xml:lang="en">Add a string at position X.</rdfs:comment>
   </owl:Class>
   <owl:Class xmlns:owl="http://www.w3.org/2002/07/owl#" rdf:ID="addAffix">
      <dcr:datcat rdf:resource="http://www.isocat.org/datcat/DC-2201"/>
      <rdfs:label xml:lang="en">add affix</rdfs:label>
      <rdfs:comment xml:lang="en">Operation that adds the specified affix</rdfs:comment>
   </owl:Class>
   <owl:Class xmlns:owl="http://www.w3.org/2002/07/owl#" rdf:ID="addAfter">
      <dcr:datcat rdf:resource="http://www.isocat.org/datcat/DC-1831"/>
      <rdfs:label xml:lang="en">add after</rdfs:label>
      <rdfs:comment xml:lang="en">Operation that adds a string to the right</rdfs:comment>
   </owl:Class>
   <owl:Class xmlns:owl="http://www.w3.org/2002/07/owl#" rdf:ID="addBefore">
      <dcr:datcat rdf:resource="http://www.isocat.org/datcat/DC-1829"/>
      <rdfs:label xml:lang="en">add before</rdfs:label>
      <rdfs:comment xml:lang="en">Operation that adds a string to the left</rdfs:comment>
   </owl:Class>
   <owl:Class xmlns:owl="http://www.w3.org/2002/07/owl#" rdf:ID="addComponentLemma">
      <dcr:datcat rdf:resource="http://www.isocat.org/datcat/DC-2202"/>
      <rdfs:label xml:lang="en">add component lemma</rdfs:label>
      <rdfs:comment xml:lang="en">Operation that adds the lemma of a specific component</rdfs:comment>
   </owl:Class>
   <owl:Class xmlns:owl="http://www.w3.org/2002/07/owl#" rdf:ID="addComponentStem">
      <dcr:datcat rdf:resource="http://www.isocat.org/datcat/DC-2204"/>
      <rdfs:label xml:lang="en">add component stem</rdfs:label>
      <rdfs:comment xml:lang="en">Operation that adds the stem of the specified component</rdfs:comment>
   </owl:Class>
   <owl:Class xmlns:owl="http://www.w3.org/2002/07/owl#" rdf:ID="addFirstConsonant">
      <dcr:datcat rdf:resource="http://www.isocat.org/datcat/DC-2198"/>
      <rdfs:label xml:lang="en">add first consonant</rdfs:label>
      <rdfs:comment xml:lang="en">Operation that adds the first consonant of the operand</rdfs:comment>
   </owl:Class>
   <owl:Class xmlns:owl="http://www.w3.org/2002/07/owl#" rdf:ID="addFirstVowel">
      <dcr:datcat rdf:resource="http://www.isocat.org/datcat/DC-2199"/>
      <rdfs:label xml:lang="en">add first vowel</rdfs:label>
      <rdfs:comment xml:lang="en">Operation that adds the first vowel of the operand</rdfs:comment>
   </owl:Class>
   <owl:Class xmlns:owl="http://www.w3.org/2002/07/owl#" rdf:ID="addLemma">
      <dcr:datcat rdf:resource="http://www.isocat.org/datcat/DC-2200"/>
      <rdfs:label xml:lang="en">add lemma</rdfs:label>
      <rdfs:comment xml:lang="en">Operation that adds the given lemma</rdfs:comment>
   </owl:Class>
   <owl:Class xmlns:owl="http://www.w3.org/2002/07/owl#" rdf:ID="addLowerCaseComponentLemma">
      <dcr:datcat rdf:resource="http://www.isocat.org/datcat/DC-2203"/>
      <rdfs:label xml:lang="en">add lower case component lemma</rdfs:label>
      <rdfs:comment xml:lang="en">Operation that adds the lemma of the component in lower case
   initiale</rdfs:comment>
   </owl:Class>
   <owl:Class xmlns:owl="http://www.w3.org/2002/07/owl#" rdf:ID="adessiveCase">
      <dcr:datcat rdf:resource="http://www.isocat.org/datcat/DC-1228"/>
      <rdfs:label xml:lang="en">adessive case</rdfs:label>
      <rdfs:comment xml:lang="en">Case which expresses the meaning of presence 'at' or 'near' a
   place.</rdfs:comment>
   </owl:Class>
   <owl:Class xmlns:owl="http://www.w3.org/2002/07/owl#" rdf:ID="aditiveCase">
      <dcr:datcat rdf:resource="http://www.isocat.org/datcat/DC-1229"/>
      <rdfs:label xml:lang="en">aditive case</rdfs:label>
      <rdfs:comment xml:lang="en">Case expressing "to" in Basque studies.</rdfs:comment>
   </owl:Class>
   <owl:Class xmlns:owl="http://www.w3.org/2002/07/owl#" rdf:ID="adjective">
      <dcr:datcat rdf:resource="http://www.isocat.org/datcat/DC-1230"/>
      <rdfs:label xml:lang="en">adjective</rdfs:label>
      <rdfs:comment xml:lang="en">Part of speech related to attributes of noun.</rdfs:comment>
   </owl:Class>
   <owl:Class xmlns:owl="http://www.w3.org/2002/07/owl#" rdf:ID="adposition">
      <dcr:datcat rdf:resource="http://www.isocat.org/datcat/DC-1231"/>
      <rdfs:label xml:lang="en">adposition</rdfs:label>
      <rdfs:comment xml:lang="en">Part of speech that occurs before/inside/after a complement composed
   of a noun phrase, noun, pronoun or clause that functions as a noun phrase and form a single
   structure with the complement to express its grammatical and semantic relation to another
   unit.</rdfs:comment>
   </owl:Class>
   <owl:Class xmlns:owl="http://www.w3.org/2002/07/owl#" rdf:ID="adverb">
      <dcr:datcat rdf:resource="http://www.isocat.org/datcat/DC-1232"/>
      <rdfs:label xml:lang="en">adverb</rdfs:label>
      <rdfs:comment xml:lang="en">Part of speech to refer to an heterogeneous group of words whose most
   frequent function is to specify the mode of action of the verb.</rdfs:comment>
   </owl:Class>
   <owl:Class xmlns:owl="http://www.w3.org/2002/07/owl#" rdf:ID="affix">
      <dcr:datcat rdf:resource="http://www.isocat.org/datcat/DC-1234"/>
      <rdfs:label xml:lang="en">affix</rdfs:label>
      <rdfs:comment xml:lang="en">Letter or group of letters which are added to a word to make a new
   word. </rdfs:comment>
   </owl:Class>
   <owl:Class xmlns:owl="http://www.w3.org/2002/07/owl#" rdf:ID="affixRank">
      <dcr:datcat rdf:resource="http://www.isocat.org/datcat/DC-2184"/>
      <rdfs:label xml:lang="en">affix rank</rdfs:label>
      <rdfs:comment xml:lang="en">Rank of an affix</rdfs:comment>
   </owl:Class>
   <owl:Class xmlns:owl="http://www.w3.org/2002/07/owl#" rdf:ID="affixedPersonalPronoun">
      <dcr:datcat rdf:resource="http://www.isocat.org/datcat/DC-2221"/>
      <rdfs:label xml:lang="en">affixed personal pronoun</rdfs:label>
      <rdfs:comment xml:lang="en">Personnal pronoun that is affixed.</rdfs:comment>
   </owl:Class>
   <owl:Class xmlns:owl="http://www.w3.org/2002/07/owl#" rdf:ID="allativeCase">
      <dcr:datcat rdf:resource="http://www.isocat.org/datcat/DC-1236"/>
      <rdfs:label xml:lang="en">allative case</rdfs:label>
      <rdfs:comment xml:lang="en">Case which expresses the meaning of motion 'to' or 'towards' the
   referent it marks.</rdfs:comment>
   </owl:Class>
   <owl:Class xmlns:owl="http://www.w3.org/2002/07/owl#" rdf:ID="allomorph">
      <dcr:datcat rdf:resource="http://www.isocat.org/datcat/DC-1237"/>
      <rdfs:label xml:lang="en">allomorph</rdfs:label>
      <rdfs:comment xml:lang="en">One of two or more complementary morphs which manifest a morpheme in
   its different phonological or morphological environments. </rdfs:comment>
   </owl:Class>
   <owl:Class xmlns:owl="http://www.w3.org/2002/07/owl#" rdf:ID="allusivePronoun">
      <dcr:datcat rdf:resource="http://www.isocat.org/datcat/DC-2223"/>
      <rdfs:label xml:lang="en">allusive pronoun</rdfs:label>
      <rdfs:comment xml:lang="en">allusive pronoun.</rdfs:comment>
   </owl:Class>
   <owl:Class xmlns:owl="http://www.w3.org/2002/07/owl#" rdf:ID="animacy">
      <dcr:datcat rdf:resource="http://www.isocat.org/datcat/DC-1902"/>
      <rdfs:label xml:lang="en">animacy</rdfs:label>
      <rdfs:comment xml:lang="en">The characteristic of a word indicating that in a given discourse
   community, its referent is considered to be alive or to possess a quality of volition or
   consciousness.</rdfs:comment>
   </owl:Class>
   <owl:Class xmlns:owl="http://www.w3.org/2002/07/owl#" rdf:ID="animate">
      <dcr:datcat rdf:resource="http://www.isocat.org/datcat/DC-1911"/>
      <rdfs:label xml:lang="en">animate</rdfs:label>
      <rdfs:comment xml:lang="en">Perceived as alive.</rdfs:comment>
   </owl:Class>
   <owl:Class xmlns:owl="http://www.w3.org/2002/07/owl#" rdf:ID="any">
      <dcr:datcat rdf:resource="http://www.isocat.org/datcat/DC-2193"/>
      <rdfs:label xml:lang="en">any</rdfs:label>
      <rdfs:comment xml:lang="en">Markup meaning that all values are allowed</rdfs:comment>
   </owl:Class>
   <owl:Class xmlns:owl="http://www.w3.org/2002/07/owl#" rdf:ID="aorist">
      <dcr:datcat rdf:resource="http://www.isocat.org/datcat/DC-1240"/>
      <rdfs:label xml:lang="en">aorist</rdfs:label>
      <rdfs:comment xml:lang="en">Simple past tense that is predominantly used for narration. Both the
   perfective and the imperfective forms can be used in the aorist without any restrictions.
  </rdfs:comment>
   </owl:Class>
   <owl:Class xmlns:owl="http://www.w3.org/2002/07/owl#" rdf:ID="apocope">
      <dcr:datcat rdf:resource="http://www.isocat.org/datcat/DC-2254"/>
      <rdfs:label xml:lang="en">apocope</rdfs:label>
      <rdfs:comment xml:lang="en">property concerning the deletion of the final element in a
   word</rdfs:comment>
   </owl:Class>
   <owl:Class xmlns:owl="http://www.w3.org/2002/07/owl#" rdf:ID="approximate">
      <dcr:datcat rdf:resource="http://www.isocat.org/datcat/DC-2206"/>
      <rdfs:label xml:lang="en">approximate</rdfs:label>
      <rdfs:comment xml:lang="en">Property used to qualify something similar but not exactly the
   same</rdfs:comment>
   </owl:Class>
   <owl:Class xmlns:owl="http://www.w3.org/2002/07/owl#" rdf:ID="aspect">
      <dcr:datcat rdf:resource="http://www.isocat.org/datcat/DC-1242"/>
      <rdfs:label xml:lang="en">aspect</rdfs:label>
      <rdfs:comment xml:lang="en">Category associated to verbs and referring to the way the grammar
   marks the duration or type of temporal activity.</rdfs:comment>
   </owl:Class>
   <owl:Class xmlns:owl="http://www.w3.org/2002/07/owl#" rdf:ID="auxiliary">
      <dcr:datcat rdf:resource="http://www.isocat.org/datcat/DC-1244"/>
      <rdfs:label xml:lang="en">auxiliary</rdfs:label>
      <rdfs:comment xml:lang="en">Part of speech referring to the set of verbs, subordinate to the main
   lexical verb which help to make distinction in mood, aspect, voice etc.</rdfs:comment>
   </owl:Class>
   <owl:Class xmlns:owl="http://www.w3.org/2002/07/owl#" rdf:ID="be">
      <dcr:datcat rdf:resource="http://www.isocat.org/datcat/DC-1246"/>
      <rdfs:label xml:lang="en">be</rdfs:label>
      <rdfs:comment xml:lang="en">Verb used to link the subject of a sentence and its noun or adjective
   complement or complementing phrase. </rdfs:comment>
   </owl:Class>
   <owl:Class xmlns:owl="http://www.w3.org/2002/07/owl#" rdf:ID="benchLevelRegister">
      <dcr:datcat rdf:resource="http://www.isocat.org/datcat/DC-1989"/>
      <rdfs:label xml:lang="en">bench-level register</rdfs:label>
      <rdfs:comment xml:lang="en">Register of terms used in applications-oriented as opposed to
   theoretical or academic levels of language.</rdfs:comment>
   </owl:Class>
   <owl:Class xmlns:owl="http://www.w3.org/2002/07/owl#" rdf:ID="benefactiveCase">
      <dcr:datcat rdf:resource="http://www.isocat.org/datcat/DC-1247"/>
      <rdfs:label xml:lang="en">benefactive case</rdfs:label>
      <rdfs:comment xml:lang="en">Case that expresses that the referent of the noun it marks receives
   the benefit of the situation expressed by the clause. </rdfs:comment>
   </owl:Class>
   <owl:Class xmlns:owl="http://www.w3.org/2002/07/owl#" rdf:ID="bound">
      <dcr:datcat rdf:resource="http://www.isocat.org/datcat/DC-1933"/>
      <rdfs:label xml:lang="en">bound</rdfs:label>
      <rdfs:comment xml:lang="en">Linked to a particular element.</rdfs:comment>
   </owl:Class>
   <owl:Class xmlns:owl="http://www.w3.org/2002/07/owl#" rdf:ID="brokenPlural">
      <dcr:datcat rdf:resource="http://www.isocat.org/datcat/DC-2218"/>
      <rdfs:label xml:lang="en">broken plural</rdfs:label>
      <rdfs:comment xml:lang="en">Internal plural that do not have any inflection.</rdfs:comment>
   </owl:Class>
   <owl:Class xmlns:owl="http://www.w3.org/2002/07/owl#" rdf:ID="bullet">
      <dcr:datcat rdf:resource="http://www.isocat.org/datcat/DC-1438"/>
      <rdfs:label xml:lang="en">bullet</rdfs:label>
      <rdfs:comment xml:lang="en">Sign used to mark an item in a list.</rdfs:comment>
   </owl:Class>
   <owl:Class xmlns:owl="http://www.w3.org/2002/07/owl#" rdf:ID="case">
      <dcr:datcat rdf:resource="http://www.isocat.org/datcat/DC-1840"/>
      <rdfs:label xml:lang="en">case</rdfs:label>
      <rdfs:comment xml:lang="en">In a given sentence, the way in which the form of a word changes in
   order to express a relationship with one or several words of the sentence. The morphological
   modification may apply to nouns, pronouns noun phrase constituents, such as adjectives or
   numerals.</rdfs:comment>
   </owl:Class>
   <owl:Class xmlns:owl="http://www.w3.org/2002/07/owl#" rdf:ID="causativeCase">
      <dcr:datcat rdf:resource="http://www.isocat.org/datcat/DC-1253"/>
      <rdfs:label xml:lang="en">causative case</rdfs:label>
      <rdfs:comment xml:lang="en">Case which expresses that the referent of the noun it marks is the
   cause of the situation expressed by the clause. </rdfs:comment>
   </owl:Class>
   <owl:Class xmlns:owl="http://www.w3.org/2002/07/owl#" rdf:ID="cessative">
      <dcr:datcat rdf:resource="http://www.isocat.org/datcat/DC-2001"/>
      <rdfs:label xml:lang="en">cessative</rdfs:label>
      <rdfs:comment xml:lang="en">Aspect that expresses the cessation of an event or
   state.</rdfs:comment>
   </owl:Class>
   <owl:Class xmlns:owl="http://www.w3.org/2002/07/owl#" rdf:ID="characterCoding">
      <dcr:datcat rdf:resource="http://www.isocat.org/datcat/DC-2089"/>
      <rdfs:label xml:lang="en">character coding</rdfs:label>
      <rdfs:comment xml:lang="en">Designation of the standard used to code the
   characters.</rdfs:comment>
   </owl:Class>
   <owl:Class xmlns:owl="http://www.w3.org/2002/07/owl#" rdf:ID="circumposition">
      <dcr:datcat rdf:resource="http://www.isocat.org/datcat/DC-1906"/>
      <rdfs:label xml:lang="en">circumposition</rdfs:label>
      <rdfs:comment xml:lang="en">Adposition which consists of two parts which are positioned ahead and
   after the adpositional foci.</rdfs:comment>
   </owl:Class>
   <owl:Class xmlns:owl="http://www.w3.org/2002/07/owl#" rdf:ID="classifier">
      <dcr:datcat rdf:resource="http://www.isocat.org/datcat/DC-2345"/>
      <rdfs:label xml:lang="en">classifier</rdfs:label>
      <rdfs:comment xml:lang="en">part of speech related to a noun to express the sub-classes to which a
   noun belongs.</rdfs:comment>
   </owl:Class>
   <owl:Class xmlns:owl="http://www.w3.org/2002/07/owl#" rdf:ID="cliticness">
      <dcr:datcat rdf:resource="http://www.isocat.org/datcat/DC-1903"/>
      <rdfs:label xml:lang="en">cliticness</rdfs:label>
      <rdfs:comment xml:lang="en">Categorization of the different types of clitics</rdfs:comment>
   </owl:Class>
   <owl:Class xmlns:owl="http://www.w3.org/2002/07/owl#" rdf:ID="closeBracket">
      <dcr:datcat rdf:resource="http://www.isocat.org/datcat/DC-2083"/>
      <rdfs:label xml:lang="en">close bracket</rdfs:label>
      <rdfs:comment xml:lang="en">Punctuation that is graphically represented by ]</rdfs:comment>
   </owl:Class>
   <owl:Class xmlns:owl="http://www.w3.org/2002/07/owl#" rdf:ID="closeCurlyBracket">
      <dcr:datcat rdf:resource="http://www.isocat.org/datcat/DC-2085"/>
      <rdfs:label xml:lang="en">close curly bracket</rdfs:label>
      <rdfs:comment xml:lang="en">Punctuation that is graphically represented by }</rdfs:comment>
   </owl:Class>
   <owl:Class xmlns:owl="http://www.w3.org/2002/07/owl#" rdf:ID="closeParenthesis">
      <dcr:datcat rdf:resource="http://www.isocat.org/datcat/DC-1440"/>
      <rdfs:label xml:lang="en">close parenthesis</rdfs:label>
      <rdfs:comment xml:lang="en">End of a parenthesis pair.</rdfs:comment>
   </owl:Class>
   <owl:Class xmlns:owl="http://www.w3.org/2002/07/owl#" rdf:ID="closePunctuation">
      <dcr:datcat rdf:resource="http://www.isocat.org/datcat/DC-2079"/>
      <rdfs:label xml:lang="en">close punctuation</rdfs:label>
      <rdfs:comment xml:lang="en">End of a paired punctuation.</rdfs:comment>
   </owl:Class>
   <owl:Class xmlns:owl="http://www.w3.org/2002/07/owl#" rdf:ID="coding">
      <dcr:datcat rdf:resource="http://www.isocat.org/datcat/DC-2242"/>
      <rdfs:label xml:lang="en">coding</rdfs:label>
      <rdfs:comment xml:lang="en">system of marking so that data can be understood</rdfs:comment>
   </owl:Class>
   <owl:Class xmlns:owl="http://www.w3.org/2002/07/owl#" rdf:ID="collective">
      <dcr:datcat rdf:resource="http://www.isocat.org/datcat/DC-1254"/>
      <rdfs:label xml:lang="en">collective</rdfs:label>
      <rdfs:comment xml:lang="en">A collective number is a number referring to 'a set of things'.
   Languages that have this feature can use it to get a phrase like 'flock of sheeps' by using
   'sheep' in collective number. </rdfs:comment>
   </owl:Class>
   <owl:Class xmlns:owl="http://www.w3.org/2002/07/owl#" rdf:ID="colon">
      <dcr:datcat rdf:resource="http://www.isocat.org/datcat/DC-1439"/>
      <rdfs:label xml:lang="en">colon</rdfs:label>
      <rdfs:comment xml:lang="en">Sign with two vertical points that is used in writing and printing to
   introduce an explanation, example or quotation.</rdfs:comment>
   </owl:Class>
   <owl:Class xmlns:owl="http://www.w3.org/2002/07/owl#" rdf:ID="comitativeCase">
      <dcr:datcat rdf:resource="http://www.isocat.org/datcat/DC-1255"/>
      <rdfs:label xml:lang="en">comitative case</rdfs:label>
      <rdfs:comment xml:lang="en">Case which expresses a meaning similar to 'along with' or
   'accompagnied by'.</rdfs:comment>
   </owl:Class>
   <owl:Class xmlns:owl="http://www.w3.org/2002/07/owl#" rdf:ID="comma">
      <dcr:datcat rdf:resource="http://www.isocat.org/datcat/DC-1448"/>
      <rdfs:label xml:lang="en">comma</rdfs:label>
      <rdfs:comment xml:lang="en">Mark (,) used in writing to show a short pause or to separate items in
   a list.</rdfs:comment>
   </owl:Class>
   <owl:Class xmlns:owl="http://www.w3.org/2002/07/owl#" rdf:ID="comment">
      <dcr:datcat rdf:resource="http://www.isocat.org/datcat/DC-1846"/>
      <rdfs:label xml:lang="en">comment</rdfs:label>
      <rdfs:comment xml:lang="en">Textual content about an element</rdfs:comment>
   </owl:Class>
   <owl:Class xmlns:owl="http://www.w3.org/2002/07/owl#" rdf:ID="commonGender">
      <dcr:datcat rdf:resource="http://www.isocat.org/datcat/DC-1558"/>
      <rdfs:label xml:lang="en">common gender</rdfs:label>
      <rdfs:comment xml:lang="en">Indistinguished gender for epicenes.</rdfs:comment>
   </owl:Class>
   <owl:Class xmlns:owl="http://www.w3.org/2002/07/owl#" rdf:ID="commonNoun">
      <dcr:datcat rdf:resource="http://www.isocat.org/datcat/DC-1256"/>
      <rdfs:label xml:lang="en">common noun</rdfs:label>
      <rdfs:comment xml:lang="en">Noun that signifies a non-specific member of a group. </rdfs:comment>
   </owl:Class>
   <owl:Class xmlns:owl="http://www.w3.org/2002/07/owl#" rdf:ID="commonlyUsed">
      <dcr:datcat rdf:resource="http://www.isocat.org/datcat/DC-1984"/>
      <rdfs:label xml:lang="en">commonly used</rdfs:label>
      <rdfs:comment xml:lang="en">Said of a term that appears frequently.</rdfs:comment>
   </owl:Class>
   <owl:Class xmlns:owl="http://www.w3.org/2002/07/owl#" rdf:ID="comparative">
      <dcr:datcat rdf:resource="http://www.isocat.org/datcat/DC-1421"/>
      <rdfs:label xml:lang="en">comparative</rdfs:label>
      <rdfs:comment xml:lang="en">Comparative is the comparison where only two entites are
   involved.</rdfs:comment>
   </owl:Class>
   <owl:Class xmlns:owl="http://www.w3.org/2002/07/owl#" rdf:ID="comparativeParticle">
      <dcr:datcat rdf:resource="http://www.isocat.org/datcat/DC-1922"/>
      <rdfs:label xml:lang="en">comparative particle</rdfs:label>
      <rdfs:comment xml:lang="en">Particle used to compare.</rdfs:comment>
   </owl:Class>
   <owl:Class xmlns:owl="http://www.w3.org/2002/07/owl#" rdf:ID="componentRank">
      <dcr:datcat rdf:resource="http://www.isocat.org/datcat/DC-2185"/>
      <rdfs:label xml:lang="en">component rank</rdfs:label>
      <rdfs:comment xml:lang="en">Rank of a component</rdfs:comment>
   </owl:Class>
   <owl:Class xmlns:owl="http://www.w3.org/2002/07/owl#" rdf:ID="compoundPreposition">
      <dcr:datcat rdf:resource="http://www.isocat.org/datcat/DC-1934"/>
      <rdfs:label xml:lang="en">compound preposition</rdfs:label>
      <rdfs:comment xml:lang="en">Preposition that is a aggregation of words</rdfs:comment>
   </owl:Class>
   <owl:Class xmlns:owl="http://www.w3.org/2002/07/owl#" rdf:ID="conditional">
      <dcr:datcat rdf:resource="http://www.isocat.org/datcat/DC-1258"/>
      <rdfs:label xml:lang="en">conditional</rdfs:label>
      <rdfs:comment xml:lang="en">A conditional relation is a logical relation in which the
   illocutionary act employing one of a pair of propositions is expressed or implied to be true or
   in force if the other proposition is true. </rdfs:comment>
   </owl:Class>
   <owl:Class xmlns:owl="http://www.w3.org/2002/07/owl#" rdf:ID="conditionalParticle">
      <dcr:datcat rdf:resource="http://www.isocat.org/datcat/DC-2230"/>
      <rdfs:label xml:lang="en">conditional particule</rdfs:label>
      <rdfs:comment xml:lang="en">conditional particule</rdfs:comment>
   </owl:Class>
   <owl:Class xmlns:owl="http://www.w3.org/2002/07/owl#" rdf:ID="conditionalPronoun">
      <dcr:datcat rdf:resource="http://www.isocat.org/datcat/DC-2222"/>
      <rdfs:label xml:lang="en">conditional pronoun</rdfs:label>
      <rdfs:comment xml:lang="en">conditional pronoun</rdfs:comment>
   </owl:Class>
   <owl:Class xmlns:owl="http://www.w3.org/2002/07/owl#" rdf:ID="conjugated">
      <dcr:datcat rdf:resource="http://www.isocat.org/datcat/DC-2207"/>
      <rdfs:label xml:lang="en">conjugated</rdfs:label>
      <rdfs:comment xml:lang="en">Property of a verbal form when inflected</rdfs:comment>
   </owl:Class>
   <owl:Class xmlns:owl="http://www.w3.org/2002/07/owl#" rdf:ID="conjunction">
      <dcr:datcat rdf:resource="http://www.isocat.org/datcat/DC-1260"/>
      <rdfs:label xml:lang="en">conjunction</rdfs:label>
      <rdfs:comment xml:lang="en">Word that syntactically links words or constituents, and expresses a
   semantic relationship between them. </rdfs:comment>
   </owl:Class>
   <owl:Class xmlns:owl="http://www.w3.org/2002/07/owl#" rdf:ID="contextualVariation">
      <dcr:datcat rdf:resource="http://www.isocat.org/datcat/DC-1977"/>
      <rdfs:label xml:lang="en">contextual variation</rdfs:label>
      <rdfs:comment xml:lang="en">Variation on a particular usage or immediate proximity of
   words.</rdfs:comment>
   </owl:Class>
   <owl:Class xmlns:owl="http://www.w3.org/2002/07/owl#" rdf:ID="coordinatingConjunction">
      <dcr:datcat rdf:resource="http://www.isocat.org/datcat/DC-1262"/>
      <rdfs:label xml:lang="en">coordinating conjunction</rdfs:label>
      <rdfs:comment xml:lang="en">Conjunction that links constituents. </rdfs:comment>
   </owl:Class>
   <owl:Class xmlns:owl="http://www.w3.org/2002/07/owl#" rdf:ID="coordinationParticle">
      <dcr:datcat rdf:resource="http://www.isocat.org/datcat/DC-2227"/>
      <rdfs:label xml:lang="en">coordination particle</rdfs:label>
      <rdfs:comment xml:lang="en">particle for coordination</rdfs:comment>
   </owl:Class>
   <owl:Class xmlns:owl="http://www.w3.org/2002/07/owl#" rdf:ID="copula">
      <dcr:datcat rdf:resource="http://www.isocat.org/datcat/DC-1263"/>
      <rdfs:label xml:lang="en">copula</rdfs:label>
      <rdfs:comment xml:lang="en">Special word that combines the subject of a sentence and its
   description. </rdfs:comment>
   </owl:Class>
   <owl:Class xmlns:owl="http://www.w3.org/2002/07/owl#" rdf:ID="copy">
      <dcr:datcat rdf:resource="http://www.isocat.org/datcat/DC-1835"/>
      <rdfs:label xml:lang="en">copy</rdfs:label>
      <rdfs:comment xml:lang="en">Operation that duplicates N characters from position X at position
   Y</rdfs:comment>
   </owl:Class>
   <owl:Class xmlns:owl="http://www.w3.org/2002/07/owl#" rdf:ID="countableNoun">
      <dcr:datcat rdf:resource="http://www.isocat.org/datcat/DC-2276"/>
      <rdfs:label xml:lang="en">countable noun</rdfs:label>
      <rdfs:comment xml:lang="en">noun referring to one or several concepts that may be
   counted</rdfs:comment>
   </owl:Class>
   <owl:Class xmlns:owl="http://www.w3.org/2002/07/owl#" rdf:ID="countryCoding">
      <dcr:datcat rdf:resource="http://www.isocat.org/datcat/DC-2092"/>
      <rdfs:label xml:lang="en">country coding</rdfs:label>
      <rdfs:comment xml:lang="en">Designation of the standard used to code the country.</rdfs:comment>
   </owl:Class>
   <owl:Class xmlns:owl="http://www.w3.org/2002/07/owl#" rdf:ID="creationDate">
      <dcr:datcat rdf:resource="http://www.isocat.org/datcat/DC-2251"/>
      <rdfs:label xml:lang="en">creation date</rdfs:label>
      <rdfs:comment xml:lang="en">date of creation</rdfs:comment>
   </owl:Class>
   <owl:Class xmlns:owl="http://www.w3.org/2002/07/owl#" rdf:ID="dateCoding">
      <dcr:datcat rdf:resource="http://www.isocat.org/datcat/DC-2090"/>
      <rdfs:label xml:lang="en">date coding</rdfs:label>
      <rdfs:comment xml:lang="en">Designation of the standard used to code the dates.</rdfs:comment>
   </owl:Class>
   <owl:Class xmlns:owl="http://www.w3.org/2002/07/owl#" rdf:ID="dating">
      <dcr:datcat rdf:resource="http://www.isocat.org/datcat/DC-1959"/>
      <rdfs:label xml:lang="en">dating</rdfs:label>
      <rdfs:comment xml:lang="en">Indication specifying whether the usage is old or
   modern.</rdfs:comment>
   </owl:Class>
   <owl:Class xmlns:owl="http://www.w3.org/2002/07/owl#" rdf:ID="dativeCase">
      <dcr:datcat rdf:resource="http://www.isocat.org/datcat/DC-1265"/>
      <rdfs:label xml:lang="en">dative case</rdfs:label>
      <rdfs:comment xml:lang="en">Case that expresses an indirect object relationship or a range of
   meaning similar to that covered by 'to' or 'for' in English; but there is a great deal of
   variation between languages in the way this case is used. </rdfs:comment>
   </owl:Class>
   <owl:Class xmlns:owl="http://www.w3.org/2002/07/owl#" rdf:ID="definite">
      <dcr:datcat rdf:resource="http://www.isocat.org/datcat/DC-2004"/>
      <rdfs:label xml:lang="en">definite</rdfs:label>
      <rdfs:comment xml:lang="en">Value referring to the capacity of identification of an
   entity.</rdfs:comment>
   </owl:Class>
   <owl:Class xmlns:owl="http://www.w3.org/2002/07/owl#" rdf:ID="definiteArticle">
      <dcr:datcat rdf:resource="http://www.isocat.org/datcat/DC-1430"/>
      <rdfs:label xml:lang="en">definite article</rdfs:label>
      <rdfs:comment xml:lang="en">Article that allows the reference to a specific, identifiable entity
   (or class of entities).</rdfs:comment>
   </owl:Class>
   <owl:Class xmlns:owl="http://www.w3.org/2002/07/owl#" rdf:ID="definiteness">
      <dcr:datcat rdf:resource="http://www.isocat.org/datcat/DC-1926"/>
      <rdfs:label xml:lang="en">definiteness</rdfs:label>
      <rdfs:comment xml:lang="en">Property about the possiblity to identify an entity.</rdfs:comment>
   </owl:Class>
   <owl:Class xmlns:owl="http://www.w3.org/2002/07/owl#" rdf:ID="definition">
      <dcr:datcat rdf:resource="http://www.isocat.org/datcat/DC-1972"/>
      <rdfs:label xml:lang="en">definition</rdfs:label>
      <rdfs:comment xml:lang="en">Representation of a concept by a descriptive statement which serves to
   differentiate it from related concepts.</rdfs:comment>
   </owl:Class>
   <owl:Class xmlns:owl="http://www.w3.org/2002/07/owl#" rdf:ID="degree">
      <dcr:datcat rdf:resource="http://www.isocat.org/datcat/DC-1419"/>
      <rdfs:label xml:lang="en">degree</rdfs:label>
      <rdfs:comment xml:lang="en">Property concerning comparison.</rdfs:comment>
   </owl:Class>
   <owl:Class xmlns:owl="http://www.w3.org/2002/07/owl#" rdf:ID="delativeCase">
      <dcr:datcat rdf:resource="http://www.isocat.org/datcat/DC-1268"/>
      <rdfs:label xml:lang="en">delative case</rdfs:label>
      <rdfs:comment xml:lang="en">Case which expresses motion downward from the referent of the noun it
   marks. </rdfs:comment>
   </owl:Class>
   <owl:Class xmlns:owl="http://www.w3.org/2002/07/owl#" rdf:ID="demonstrativeDeterminer">
      <dcr:datcat rdf:resource="http://www.isocat.org/datcat/DC-1269"/>
      <rdfs:label xml:lang="en">demonstrative determiner</rdfs:label>
      <rdfs:comment xml:lang="en">Determiner used to point to an entity in the situation or elsewhere in
   a sentence.</rdfs:comment>
   </owl:Class>
   <owl:Class xmlns:owl="http://www.w3.org/2002/07/owl#" rdf:ID="demonstrativePronoun">
      <dcr:datcat rdf:resource="http://www.isocat.org/datcat/DC-1270"/>
      <rdfs:label xml:lang="en">demonstrative pronoun</rdfs:label>
      <rdfs:comment xml:lang="en">Pronoun used to point to an entity in the situation or elsewhere in a
   sentence.</rdfs:comment>
   </owl:Class>
   <owl:Class xmlns:owl="http://www.w3.org/2002/07/owl#" rdf:ID="derivation">
      <dcr:datcat rdf:resource="http://www.isocat.org/datcat/DC-1271"/>
      <rdfs:label xml:lang="en">derivation</rdfs:label>
      <rdfs:comment xml:lang="en">Change in the form of a linguistic unit, usually modification in the
   base/root or affixation to create a new word.</rdfs:comment>
   </owl:Class>
   <owl:Class xmlns:owl="http://www.w3.org/2002/07/owl#" rdf:ID="determiner">
      <dcr:datcat rdf:resource="http://www.isocat.org/datcat/DC-1272"/>
      <rdfs:label xml:lang="en">determiner</rdfs:label>
      <rdfs:comment xml:lang="en">Word or affix that belongs to a class of noun modifiers that expresses
   the reference, including quantity, of a noun. </rdfs:comment>
   </owl:Class>
   <owl:Class xmlns:owl="http://www.w3.org/2002/07/owl#" rdf:ID="dialectRegister">
      <dcr:datcat rdf:resource="http://www.isocat.org/datcat/DC-1990"/>
      <rdfs:label xml:lang="en">dialect register</rdfs:label>
      <rdfs:comment xml:lang="en">Register that is specific to a dialect.</rdfs:comment>
   </owl:Class>
   <owl:Class xmlns:owl="http://www.w3.org/2002/07/owl#" rdf:ID="diminutiveNoun">
      <dcr:datcat rdf:resource="http://www.isocat.org/datcat/DC-2225"/>
      <rdfs:label xml:lang="en">diminutive noun</rdfs:label>
      <rdfs:comment xml:lang="en">diminutive noun</rdfs:comment>
   </owl:Class>
   <owl:Class xmlns:owl="http://www.w3.org/2002/07/owl#" rdf:ID="direction">
      <dcr:datcat rdf:resource="http://www.isocat.org/datcat/DC-2238"/>
      <rdfs:label xml:lang="en">direction</rdfs:label>
      <rdfs:comment xml:lang="en">general way in which something changes or develops</rdfs:comment>
   </owl:Class>
   <owl:Class xmlns:owl="http://www.w3.org/2002/07/owl#" rdf:ID="distinctiveParticle">
      <dcr:datcat rdf:resource="http://www.isocat.org/datcat/DC-2228"/>
      <rdfs:label xml:lang="en">distinctive particle</rdfs:label>
      <rdfs:comment xml:lang="en">distinctive particle</rdfs:comment>
   </owl:Class>
   <owl:Class xmlns:owl="http://www.w3.org/2002/07/owl#" rdf:ID="domain">
      <dcr:datcat rdf:resource="http://www.isocat.org/datcat/DC-2212"/>
      <rdfs:label xml:lang="en">domain</rdfs:label>
      <rdfs:comment xml:lang="en">area of activity, interest, or knowledge</rdfs:comment>
   </owl:Class>
   <owl:Class xmlns:owl="http://www.w3.org/2002/07/owl#" rdf:ID="dual">
      <dcr:datcat rdf:resource="http://www.isocat.org/datcat/DC-1879"/>
      <rdfs:label xml:lang="en">dual</rdfs:label>
      <rdfs:comment xml:lang="en">Form used in some languages to designate two persons or
   things.</rdfs:comment>
   </owl:Class>
   <owl:Class xmlns:owl="http://www.w3.org/2002/07/owl#" rdf:ID="elativeCase">
      <dcr:datcat rdf:resource="http://www.isocat.org/datcat/DC-1276"/>
      <rdfs:label xml:lang="en">elative case</rdfs:label>
      <rdfs:comment xml:lang="en">Case which expresses the meaning of motion 'away from' from the
   referent of the noun it marks.</rdfs:comment>
   </owl:Class>
   <owl:Class xmlns:owl="http://www.w3.org/2002/07/owl#" rdf:ID="elision">
      <dcr:datcat rdf:resource="http://www.isocat.org/datcat/DC-1277"/>
      <rdfs:label xml:lang="en">elision</rdfs:label>
      <rdfs:comment xml:lang="en">The omission of a syllable or vowel at the beginning or end of a word,
   esp. when a word ending with a vowel is next to one beginning with a vowel. </rdfs:comment>
   </owl:Class>
   <owl:Class xmlns:owl="http://www.w3.org/2002/07/owl#" rdf:ID="emphaticPronoun">
      <dcr:datcat rdf:resource="http://www.isocat.org/datcat/DC-1941"/>
      <rdfs:label xml:lang="en">emphatic pronoun</rdfs:label>
      <rdfs:comment xml:lang="en">Pronoun marked to show its importance.</rdfs:comment>
   </owl:Class>
   <owl:Class xmlns:owl="http://www.w3.org/2002/07/owl#" rdf:ID="equativeCase">
      <dcr:datcat rdf:resource="http://www.isocat.org/datcat/DC-1279"/>
      <rdfs:label xml:lang="en">equative case</rdfs:label>
      <rdfs:comment xml:lang="en">Case that expresses likeness or identity to the referent of the noun
   it marks. It can have meaning, such as: 'as', 'like', or 'in the capacity of'. </rdfs:comment>
   </owl:Class>
   <owl:Class xmlns:owl="http://www.w3.org/2002/07/owl#" rdf:ID="ergativeCase">
      <dcr:datcat rdf:resource="http://www.isocat.org/datcat/DC-1280"/>
      <rdfs:label xml:lang="en">ergative case</rdfs:label>
      <rdfs:comment xml:lang="en">Case assigned to the subject of a transitive verb as opposed to
   absolutive case. </rdfs:comment>
   </owl:Class>
   <owl:Class xmlns:owl="http://www.w3.org/2002/07/owl#" rdf:ID="essiveCase">
      <dcr:datcat rdf:resource="http://www.isocat.org/datcat/DC-1281"/>
      <rdfs:label xml:lang="en">essive case</rdfs:label>
      <rdfs:comment xml:lang="en">Case which expresses a state of being.</rdfs:comment>
   </owl:Class>
   <owl:Class xmlns:owl="http://www.w3.org/2002/07/owl#" rdf:ID="etymologicalRoot">
      <dcr:datcat rdf:resource="http://www.isocat.org/datcat/DC-1987"/>
      <rdfs:label xml:lang="en">etymological root</rdfs:label>
      <rdfs:comment xml:lang="en">Morpheme that has a particular status with regards to the word's
   etymology.</rdfs:comment>
   </owl:Class>
   <owl:Class xmlns:owl="http://www.w3.org/2002/07/owl#" rdf:ID="exact">
      <dcr:datcat rdf:resource="http://www.isocat.org/datcat/DC-2205"/>
      <rdfs:label xml:lang="en">exact</rdfs:label>
      <rdfs:comment xml:lang="en">Completely correct in every detail</rdfs:comment>
   </owl:Class>
   <owl:Class xmlns:owl="http://www.w3.org/2002/07/owl#" rdf:ID="example">
      <dcr:datcat rdf:resource="http://www.isocat.org/datcat/DC-1958"/>
      <rdfs:label xml:lang="en">example</rdfs:label>
      <rdfs:comment xml:lang="en">Descriptive material that provides a sample of an object or entity
   defined in the entry.</rdfs:comment>
   </owl:Class>
   <owl:Class xmlns:owl="http://www.w3.org/2002/07/owl#" rdf:ID="exclamativeDeterminer">
      <dcr:datcat rdf:resource="http://www.isocat.org/datcat/DC-1284"/>
      <rdfs:label xml:lang="en">exclamative determiner</rdfs:label>
      <rdfs:comment xml:lang="en">Determiner expressing an emotional utterance and marked with a strong
   intonation.</rdfs:comment>
   </owl:Class>
   <owl:Class xmlns:owl="http://www.w3.org/2002/07/owl#" rdf:ID="exclamativePoint">
      <dcr:datcat rdf:resource="http://www.isocat.org/datcat/DC-1441"/>
      <rdfs:label xml:lang="en">exclamative point</rdfs:label>
      <rdfs:comment xml:lang="en">Special sign (!) usually used in writing to mark
   exclamation.</rdfs:comment>
   </owl:Class>
   <owl:Class xmlns:owl="http://www.w3.org/2002/07/owl#" rdf:ID="exclamativePronoun">
      <dcr:datcat rdf:resource="http://www.isocat.org/datcat/DC-1285"/>
      <rdfs:label xml:lang="en">exclamative pronoun</rdfs:label>
      <rdfs:comment xml:lang="en">Pronoun marked with an emotional utterance and/or a strong
   intonation.</rdfs:comment>
   </owl:Class>
   <owl:Class xmlns:owl="http://www.w3.org/2002/07/owl#" rdf:ID="expansionVariation">
      <dcr:datcat rdf:resource="http://www.isocat.org/datcat/DC-1850"/>
      <rdfs:label xml:lang="en">expansion variation</rdfs:label>
      <rdfs:comment xml:lang="en">Description of the kind of variation between full and abbreviated
   forms.</rdfs:comment>
   </owl:Class>
   <owl:Class xmlns:owl="http://www.w3.org/2002/07/owl#" rdf:ID="expletive">
      <dcr:datcat rdf:resource="http://www.isocat.org/datcat/DC-1283"/>
      <rdfs:label xml:lang="en">expletive</rdfs:label>
      <rdfs:comment xml:lang="en">Word which serves no grammatical function, but which fills up a
   sentence or gives emphasis. </rdfs:comment>
   </owl:Class>
   <owl:Class xmlns:owl="http://www.w3.org/2002/07/owl#" rdf:ID="externalReference">
      <dcr:datcat rdf:resource="http://www.isocat.org/datcat/DC-1975"/>
      <rdfs:label xml:lang="en">external reference</rdfs:label>
      <rdfs:comment xml:lang="en">Reference to a particular node of an external descriptive
   system.</rdfs:comment>
   </owl:Class>
   <owl:Class xmlns:owl="http://www.w3.org/2002/07/owl#" rdf:ID="externalSystem">
      <dcr:datcat rdf:resource="http://www.isocat.org/datcat/DC-1974"/>
      <rdfs:label xml:lang="en">external system</rdfs:label>
      <rdfs:comment xml:lang="en">Reference to an external descriptive system.</rdfs:comment>
   </owl:Class>
   <owl:Class xmlns:owl="http://www.w3.org/2002/07/owl#" rdf:ID="facetiousRegister">
      <dcr:datcat rdf:resource="http://www.isocat.org/datcat/DC-1991"/>
      <rdfs:label xml:lang="en">facecious register</rdfs:label>
      <rdfs:comment xml:lang="en">Register related to an expression that is intended to be clever and
   funny but that is really silly and annoying.</rdfs:comment>
   </owl:Class>
   <owl:Class xmlns:owl="http://www.w3.org/2002/07/owl#" rdf:ID="feminine">
      <dcr:datcat rdf:resource="http://www.isocat.org/datcat/DC-1880"/>
      <rdfs:label xml:lang="en">feminine</rdfs:label>
      <rdfs:comment xml:lang="en">Of, relating to, or constituting the gender that ordinarily includes
   most words or grammatical forms referring to females.</rdfs:comment>
   </owl:Class>
   <owl:Class xmlns:owl="http://www.w3.org/2002/07/owl#" rdf:ID="finite">
      <dcr:datcat rdf:resource="http://www.isocat.org/datcat/DC-1287"/>
      <rdfs:label xml:lang="en">finite</rdfs:label>
      <rdfs:comment xml:lang="en">Property applied to a verb form that can occur on its own in an
   independent sentence. </rdfs:comment>
   </owl:Class>
   <owl:Class xmlns:owl="http://www.w3.org/2002/07/owl#" rdf:ID="finiteness">
      <dcr:datcat rdf:resource="http://www.isocat.org/datcat/DC-1893"/>
      <rdfs:label xml:lang="en">finitness</rdfs:label>
      <rdfs:comment xml:lang="en">Property referring to finite and non-finite status of a verbal
   form.</rdfs:comment>
   </owl:Class>
   <owl:Class xmlns:owl="http://www.w3.org/2002/07/owl#" rdf:ID="firstPerson">
      <dcr:datcat rdf:resource="http://www.isocat.org/datcat/DC-1288"/>
      <rdfs:label xml:lang="en">first person</rdfs:label>
      <rdfs:comment xml:lang="en">First person deixis is deictic reference that refers to the speaker,
   or both the speaker and referents grouped with the speaker </rdfs:comment>
   </owl:Class>
   <owl:Class xmlns:owl="http://www.w3.org/2002/07/owl#" rdf:ID="foreignText">
      <dcr:datcat rdf:resource="http://www.isocat.org/datcat/DC-1423"/>
      <rdfs:label xml:lang="en">foreign text</rdfs:label>
      <rdfs:comment xml:lang="en">Markup used to identify a word, phrase, or extended text as belonging
   to some language other than that of the surrounding text.</rdfs:comment>
   </owl:Class>
   <owl:Class xmlns:owl="http://www.w3.org/2002/07/owl#" rdf:ID="formalRegister">
      <dcr:datcat rdf:resource="http://www.isocat.org/datcat/DC-1992"/>
      <rdfs:label xml:lang="en">formal register</rdfs:label>
      <rdfs:comment xml:lang="en">Formal register.</rdfs:comment>
   </owl:Class>
   <owl:Class xmlns:owl="http://www.w3.org/2002/07/owl#" rdf:ID="formula">
      <dcr:datcat rdf:resource="http://www.isocat.org/datcat/DC-1888"/>
      <rdfs:label xml:lang="en">formula</rdfs:label>
      <rdfs:comment xml:lang="en">Figures, symbols or the like used to express a concept briefly, such
   as a mathematical or chemical formula.</rdfs:comment>
   </owl:Class>
   <owl:Class xmlns:owl="http://www.w3.org/2002/07/owl#" rdf:ID="frequency">
      <dcr:datcat rdf:resource="http://www.isocat.org/datcat/DC-1965"/>
      <rdfs:label xml:lang="en">frequency</rdfs:label>
      <rdfs:comment xml:lang="en">The relative commonness with which a term occurs.</rdfs:comment>
   </owl:Class>
   <owl:Class xmlns:owl="http://www.w3.org/2002/07/owl#" rdf:ID="fullArticle">
      <dcr:datcat rdf:resource="http://www.isocat.org/datcat/DC-1928"/>
      <rdfs:label xml:lang="en">full article</rdfs:label>
      <rdfs:comment xml:lang="en">For definiteness, when a specific form is the syntactic subject of the
   clause.</rdfs:comment>
   </owl:Class>
   <owl:Class xmlns:owl="http://www.w3.org/2002/07/owl#" rdf:ID="fusedPreposition">
      <dcr:datcat rdf:resource="http://www.isocat.org/datcat/DC-1901"/>
      <rdfs:label xml:lang="en">fused preposition</rdfs:label>
      <rdfs:comment xml:lang="en">Preposition that is the result of a morphological merge from at least
   two words.</rdfs:comment>
   </owl:Class>
   <owl:Class xmlns:owl="http://www.w3.org/2002/07/owl#" rdf:ID="future">
      <dcr:datcat rdf:resource="http://www.isocat.org/datcat/DC-1291"/>
      <rdfs:label xml:lang="en">future</rdfs:label>
      <rdfs:comment xml:lang="en">Verb tense that indicates action or state of being in the future.
  </rdfs:comment>
   </owl:Class>
   <owl:Class xmlns:owl="http://www.w3.org/2002/07/owl#" rdf:ID="futureParticle">
      <dcr:datcat rdf:resource="http://www.isocat.org/datcat/DC-1919"/>
      <rdfs:label xml:lang="en">future particle</rdfs:label>
      <rdfs:comment xml:lang="en">Particle used in order to express future.</rdfs:comment>
   </owl:Class>
   <owl:Class xmlns:owl="http://www.w3.org/2002/07/owl#" rdf:ID="generalAdverb">
      <dcr:datcat rdf:resource="http://www.isocat.org/datcat/DC-1435"/>
      <rdfs:label xml:lang="en">general adverb</rdfs:label>
      <rdfs:comment xml:lang="en">Adverb belonging to the general class of adverbs</rdfs:comment>
   </owl:Class>
   <owl:Class xmlns:owl="http://www.w3.org/2002/07/owl#" rdf:ID="genitiveCase">
      <dcr:datcat rdf:resource="http://www.isocat.org/datcat/DC-1293"/>
      <rdfs:label xml:lang="en">genitive case</rdfs:label>
      <rdfs:comment xml:lang="en">Case which expresses a possessive relationship (e.g. the boy's book)
   or some other similarly close connection (e.g. a summer's day).</rdfs:comment>
   </owl:Class>
   <owl:Class xmlns:owl="http://www.w3.org/2002/07/owl#" rdf:ID="geographicalVariant">
      <dcr:datcat rdf:resource="http://www.isocat.org/datcat/DC-1851"/>
      <rdfs:label xml:lang="en">geographical variant</rdfs:label>
      <rdfs:comment xml:lang="en">Description of a specific form used in a certain region as opposed to
   another form used in another region</rdfs:comment>
   </owl:Class>
   <owl:Class xmlns:owl="http://www.w3.org/2002/07/owl#" rdf:ID="gerundive">
      <dcr:datcat rdf:resource="http://www.isocat.org/datcat/DC-2243"/>
      <rdfs:label xml:lang="en">gerundive</rdfs:label>
      <rdfs:comment xml:lang="en">property for a non-finite form of a verb other than the
   infinitive.</rdfs:comment>
   </owl:Class>
   <owl:Class xmlns:owl="http://www.w3.org/2002/07/owl#" rdf:ID="grammaticalGender">
      <dcr:datcat rdf:resource="http://www.isocat.org/datcat/DC-1297"/>
      <rdfs:label xml:lang="en">grammatical gender</rdfs:label>
      <rdfs:comment xml:lang="en">Category based on (depending on languages) the natural distinction
   between sex and formal criteria. the common value is used for the word combines feminine and
   masculine</rdfs:comment>
   </owl:Class>
   <owl:Class xmlns:owl="http://www.w3.org/2002/07/owl#" rdf:ID="grammaticalNumber">
      <dcr:datcat rdf:resource="http://www.isocat.org/datcat/DC-1298"/>
      <rdfs:label xml:lang="en">grammatical number</rdfs:label>
      <rdfs:comment xml:lang="en">Grammatical category for the variation in form of nouns, pronouns, and
   any words agreeing with them, depending on how many persons or things are referred
   to.</rdfs:comment>
   </owl:Class>
   <owl:Class xmlns:owl="http://www.w3.org/2002/07/owl#" rdf:ID="graphicalOperator">
      <dcr:datcat rdf:resource="http://www.isocat.org/datcat/DC-1860"/>
      <rdfs:label xml:lang="en">graphical operator</rdfs:label>
      <rdfs:comment xml:lang="en">Description of the modification of a written form</rdfs:comment>
   </owl:Class>
   <owl:Class xmlns:owl="http://www.w3.org/2002/07/owl#" rdf:ID="graphicalSeparator">
      <dcr:datcat rdf:resource="http://www.isocat.org/datcat/DC-1863"/>
      <rdfs:label xml:lang="en">graphical separator</rdfs:label>
      <rdfs:comment xml:lang="en">Character string that appears between two written forms</rdfs:comment>
   </owl:Class>
   <owl:Class xmlns:owl="http://www.w3.org/2002/07/owl#" rdf:ID="have">
      <dcr:datcat rdf:resource="http://www.isocat.org/datcat/DC-1299"/>
      <rdfs:label xml:lang="en">have</rdfs:label>
      <rdfs:comment xml:lang="en">The verb have.</rdfs:comment>
   </owl:Class>
   <owl:Class xmlns:owl="http://www.w3.org/2002/07/owl#" rdf:ID="homograph">
      <dcr:datcat rdf:resource="http://www.isocat.org/datcat/DC-1300"/>
      <rdfs:label xml:lang="en">homograph</rdfs:label>
      <rdfs:comment xml:lang="en">Word that is written like another, but that has a different
   pronunciation, meaning, and/or origin. </rdfs:comment>
   </owl:Class>
   <owl:Class xmlns:owl="http://www.w3.org/2002/07/owl#" rdf:ID="homonym">
      <dcr:datcat rdf:resource="http://www.isocat.org/datcat/DC-1301"/>
      <rdfs:label xml:lang="en">homonym</rdfs:label>
      <rdfs:comment xml:lang="en">Word that sounds the same and is written the same as another word but
   is different in meaning.</rdfs:comment>
   </owl:Class>
   <owl:Class xmlns:owl="http://www.w3.org/2002/07/owl#" rdf:ID="homophone">
      <dcr:datcat rdf:resource="http://www.isocat.org/datcat/DC-1302"/>
      <rdfs:label xml:lang="en">homophone</rdfs:label>
      <rdfs:comment xml:lang="en">Word that sounds like another word, but is different in writiing or
   meaning.</rdfs:comment>
   </owl:Class>
   <owl:Class xmlns:owl="http://www.w3.org/2002/07/owl#" rdf:ID="honorific">
      <dcr:datcat rdf:resource="http://www.isocat.org/datcat/DC-2347"/>
      <rdfs:label xml:lang="en">honorific</rdfs:label>
      <rdfs:comment xml:lang="en">special form of language used when talking about those in positions of
   social situation</rdfs:comment>
   </owl:Class>
   <owl:Class xmlns:owl="http://www.w3.org/2002/07/owl#" rdf:ID="hyphen">
      <dcr:datcat rdf:resource="http://www.isocat.org/datcat/DC-2077"/>
      <rdfs:label xml:lang="en">hyphen</rdfs:label>
      <rdfs:comment xml:lang="en">Punctuation that is graphically presented as "-".</rdfs:comment>
   </owl:Class>
   <owl:Class xmlns:owl="http://www.w3.org/2002/07/owl#" rdf:ID="id">
      <dcr:datcat rdf:resource="http://www.isocat.org/datcat/DC-1845"/>
      <rdfs:label xml:lang="en">id</rdfs:label>
      <rdfs:comment xml:lang="en">Identification of an element</rdfs:comment>
   </owl:Class>
   <owl:Class xmlns:owl="http://www.w3.org/2002/07/owl#" rdf:ID="illativeCase">
      <dcr:datcat rdf:resource="http://www.isocat.org/datcat/DC-1303"/>
      <rdfs:label xml:lang="en">illative case</rdfs:label>
      <rdfs:comment xml:lang="en">Case which expresses the meaning of 'motion into' or 'direction
   towards' the referent of the noun it marks.</rdfs:comment>
   </owl:Class>
   <owl:Class xmlns:owl="http://www.w3.org/2002/07/owl#" rdf:ID="image">
      <dcr:datcat rdf:resource="http://www.isocat.org/datcat/DC-2249"/>
      <rdfs:label xml:lang="en">image</rdfs:label>
      <rdfs:comment xml:lang="en">graphical representation</rdfs:comment>
   </owl:Class>
   <owl:Class xmlns:owl="http://www.w3.org/2002/07/owl#" rdf:ID="imperative">
      <dcr:datcat rdf:resource="http://www.isocat.org/datcat/DC-1844"/>
      <rdfs:label xml:lang="en">imperative</rdfs:label>
      <rdfs:comment xml:lang="en">Mood used to express an order.</rdfs:comment>
   </owl:Class>
   <owl:Class xmlns:owl="http://www.w3.org/2002/07/owl#" rdf:ID="imperfect">
      <dcr:datcat rdf:resource="http://www.isocat.org/datcat/DC-1304"/>
      <rdfs:label xml:lang="en">imperfect</rdfs:label>
      <rdfs:comment xml:lang="en">Verb tense that refers to action in the past that is incomplete or
   ongoing. </rdfs:comment>
   </owl:Class>
   <owl:Class xmlns:owl="http://www.w3.org/2002/07/owl#" rdf:ID="imperfective">
      <dcr:datcat rdf:resource="http://www.isocat.org/datcat/DC-1305"/>
      <rdfs:label xml:lang="en">imperfective</rdfs:label>
      <rdfs:comment xml:lang="en">Imperfective aspect is an aspect that expresses an event or state,
   with respect to its internal structure, instead of expressing it as a simple whole.
  </rdfs:comment>
   </owl:Class>
   <owl:Class xmlns:owl="http://www.w3.org/2002/07/owl#" rdf:ID="impersonalPronoun">
      <dcr:datcat rdf:resource="http://www.isocat.org/datcat/DC-1426"/>
      <rdfs:label xml:lang="en">impersonal pronoun</rdfs:label>
      <rdfs:comment xml:lang="en">Pronoun lacking person referent.</rdfs:comment>
   </owl:Class>
   <owl:Class xmlns:owl="http://www.w3.org/2002/07/owl#" rdf:ID="impossible">
      <dcr:datcat rdf:resource="http://www.isocat.org/datcat/DC-1866"/>
      <rdfs:label xml:lang="en">impossible</rdfs:label>
      <rdfs:comment xml:lang="en">to denote something that cannot be considered as being correct in a
   given language</rdfs:comment>
   </owl:Class>
   <owl:Class xmlns:owl="http://www.w3.org/2002/07/owl#" rdf:ID="inHouseRegister">
      <dcr:datcat rdf:resource="http://www.isocat.org/datcat/DC-1993"/>
      <rdfs:label xml:lang="en">in house register</rdfs:label>
      <rdfs:comment xml:lang="en">Register of terms that are company-specific and not readily recognized
   outside this environment.</rdfs:comment>
   </owl:Class>
   <owl:Class xmlns:owl="http://www.w3.org/2002/07/owl#" rdf:ID="inanimate">
      <dcr:datcat rdf:resource="http://www.isocat.org/datcat/DC-1952"/>
      <rdfs:label xml:lang="en">inanimate</rdfs:label>
      <rdfs:comment xml:lang="en">Perceived as not living.</rdfs:comment>
   </owl:Class>
   <owl:Class xmlns:owl="http://www.w3.org/2002/07/owl#" rdf:ID="indefiniteArticle">
      <dcr:datcat rdf:resource="http://www.isocat.org/datcat/DC-1308"/>
      <rdfs:label xml:lang="en">indefinite article</rdfs:label>
      <rdfs:comment xml:lang="en">Article not capable of expressing identification.</rdfs:comment>
   </owl:Class>
   <owl:Class xmlns:owl="http://www.w3.org/2002/07/owl#" rdf:ID="indefiniteDeterminer">
      <dcr:datcat rdf:resource="http://www.isocat.org/datcat/DC-1307"/>
      <rdfs:label xml:lang="en">indefinite determiner</rdfs:label>
      <rdfs:comment xml:lang="en">Determiner not capable of identification.</rdfs:comment>
   </owl:Class>
   <owl:Class xmlns:owl="http://www.w3.org/2002/07/owl#" rdf:ID="indefinitePronoun">
      <dcr:datcat rdf:resource="http://www.isocat.org/datcat/DC-1309"/>
      <rdfs:label xml:lang="en">indefinite pronoun</rdfs:label>
      <rdfs:comment xml:lang="en">Pronoun that does not allow reference.</rdfs:comment>
   </owl:Class>
   <owl:Class xmlns:owl="http://www.w3.org/2002/07/owl#" rdf:ID="indicative">
      <dcr:datcat rdf:resource="http://www.isocat.org/datcat/DC-1885"/>
      <rdfs:label xml:lang="en">indicative</rdfs:label>
      <rdfs:comment xml:lang="en">Mood value used in the expression of statements and
   questions.</rdfs:comment>
   </owl:Class>
   <owl:Class xmlns:owl="http://www.w3.org/2002/07/owl#" rdf:ID="indifferent">
      <dcr:datcat rdf:resource="http://www.isocat.org/datcat/DC-1944"/>
      <rdfs:label xml:lang="en">indifferent</rdfs:label>
      <rdfs:comment xml:lang="en">Markup to express that there is not any pertinence.</rdfs:comment>
   </owl:Class>
   <owl:Class xmlns:owl="http://www.w3.org/2002/07/owl#" rdf:ID="inessiveCase">
      <dcr:datcat rdf:resource="http://www.isocat.org/datcat/DC-1311"/>
      <rdfs:label xml:lang="en">inessive case</rdfs:label>
      <rdfs:comment xml:lang="en">Case which expresses the meaning of location or position within a
   place.</rdfs:comment>
   </owl:Class>
   <owl:Class xmlns:owl="http://www.w3.org/2002/07/owl#" rdf:ID="infinitive">
      <dcr:datcat rdf:resource="http://www.isocat.org/datcat/DC-1312"/>
      <rdfs:label xml:lang="en">infinitive</rdfs:label>
      <rdfs:comment xml:lang="en">Mood cited as unmarked or base form.</rdfs:comment>
   </owl:Class>
   <owl:Class xmlns:owl="http://www.w3.org/2002/07/owl#" rdf:ID="infinitiveParticle">
      <dcr:datcat rdf:resource="http://www.isocat.org/datcat/DC-1896"/>
      <rdfs:label xml:lang="en">infinitive particle</rdfs:label>
      <rdfs:comment xml:lang="en">Particle used to express infinitive.</rdfs:comment>
   </owl:Class>
   <owl:Class xmlns:owl="http://www.w3.org/2002/07/owl#" rdf:ID="infix">
      <dcr:datcat rdf:resource="http://www.isocat.org/datcat/DC-1313"/>
      <rdfs:label xml:lang="en">infix</rdfs:label>
      <rdfs:comment xml:lang="en">Affix inserted in the middle of a word to change its meaning or part
   of speech value. </rdfs:comment>
   </owl:Class>
   <owl:Class xmlns:owl="http://www.w3.org/2002/07/owl#" rdf:ID="infrequentlyUsed">
      <dcr:datcat rdf:resource="http://www.isocat.org/datcat/DC-1985"/>
      <rdfs:label xml:lang="en">infrequently used</rdfs:label>
      <rdfs:comment xml:lang="en">Said of a term that does not appear frequently.</rdfs:comment>
   </owl:Class>
   <owl:Class xmlns:owl="http://www.w3.org/2002/07/owl#" rdf:ID="instrumentalCase">
      <dcr:datcat rdf:resource="http://www.isocat.org/datcat/DC-1316"/>
      <rdfs:label xml:lang="en">instrumental case</rdfs:label>
      <rdfs:comment xml:lang="en">Case indicating that the referent of the noun it marks is the means of
   the accomplishment of the action expressed by the clause. </rdfs:comment>
   </owl:Class>
   <owl:Class xmlns:owl="http://www.w3.org/2002/07/owl#" rdf:ID="intensity">
      <dcr:datcat rdf:resource="http://www.isocat.org/datcat/DC-2197"/>
      <rdfs:label xml:lang="en">intensity</rdfs:label>
      <rdfs:comment xml:lang="en">Quality of being felt very strongly or having a strong
   effect</rdfs:comment>
   </owl:Class>
   <owl:Class xmlns:owl="http://www.w3.org/2002/07/owl#" rdf:ID="interjection">
      <dcr:datcat rdf:resource="http://www.isocat.org/datcat/DC-1318"/>
      <rdfs:label xml:lang="en">interjection</rdfs:label>
      <rdfs:comment xml:lang="en">Word or sound that expresses an emotion. </rdfs:comment>
   </owl:Class>
   <owl:Class xmlns:owl="http://www.w3.org/2002/07/owl#" rdf:ID="interrogativeDeterminer">
      <dcr:datcat rdf:resource="http://www.isocat.org/datcat/DC-1320"/>
      <rdfs:label xml:lang="en">interrogative determiner</rdfs:label>
      <rdfs:comment xml:lang="en">Determiner used to express a question.</rdfs:comment>
   </owl:Class>
   <owl:Class xmlns:owl="http://www.w3.org/2002/07/owl#" rdf:ID="interrogativeParticle">
      <dcr:datcat rdf:resource="http://www.isocat.org/datcat/DC-1921"/>
      <rdfs:label xml:lang="en">interrogative particle</rdfs:label>
      <rdfs:comment xml:lang="en">Particle used to express a question.</rdfs:comment>
   </owl:Class>
   <owl:Class xmlns:owl="http://www.w3.org/2002/07/owl#" rdf:ID="interrogativePronoun">
      <dcr:datcat rdf:resource="http://www.isocat.org/datcat/DC-1321"/>
      <rdfs:label xml:lang="en">interrogative pronoun</rdfs:label>
      <rdfs:comment xml:lang="en">Pronoun used to express a question.</rdfs:comment>
   </owl:Class>
   <owl:Class xmlns:owl="http://www.w3.org/2002/07/owl#" rdf:ID="interrogativePunctuation">
      <dcr:datcat rdf:resource="http://www.isocat.org/datcat/DC-2087"/>
      <rdfs:label xml:lang="en">interrogative punctuation</rdfs:label>
      <rdfs:comment xml:lang="en">Punctuation used when the sentence is interrogative.</rdfs:comment>
   </owl:Class>
   <owl:Class xmlns:owl="http://www.w3.org/2002/07/owl#" rdf:ID="invertedComma">
      <dcr:datcat rdf:resource="http://www.isocat.org/datcat/DC-1443"/>
      <rdfs:label xml:lang="en">inverted comma</rdfs:label>
      <rdfs:comment xml:lang="en">Inverted comma.</rdfs:comment>
   </owl:Class>
   <owl:Class xmlns:owl="http://www.w3.org/2002/07/owl#" rdf:ID="invertedQuestionMark">
      <dcr:datcat rdf:resource="http://www.isocat.org/datcat/DC-2088"/>
      <rdfs:label xml:lang="en">inverted question mark</rdfs:label>
      <rdfs:comment xml:lang="en">Punctuation used in certain languages at the beginning of an
   interrogative sentence.</rdfs:comment>
   </owl:Class>
   <owl:Class xmlns:owl="http://www.w3.org/2002/07/owl#" rdf:ID="ironicRegister">
      <dcr:datcat rdf:resource="http://www.isocat.org/datcat/DC-1994"/>
      <rdfs:label xml:lang="en">ironic register</rdfs:label>
      <rdfs:comment xml:lang="en">Register for irony.</rdfs:comment>
   </owl:Class>
   <owl:Class xmlns:owl="http://www.w3.org/2002/07/owl#" rdf:ID="label">
      <dcr:datcat rdf:resource="http://www.isocat.org/datcat/DC-1857"/>
      <rdfs:label xml:lang="en">label</rdfs:label>
      <rdfs:comment xml:lang="en">Text attached to an element</rdfs:comment>
   </owl:Class>
   <owl:Class xmlns:owl="http://www.w3.org/2002/07/owl#" rdf:ID="language">
      <dcr:datcat rdf:resource="http://www.isocat.org/datcat/DC-1969"/>
      <rdfs:label xml:lang="en">language</rdfs:label>
      <rdfs:comment xml:lang="en">System of communication by written or spoken words which is used by
   the people of a particular country or area.</rdfs:comment>
   </owl:Class>
   <owl:Class xmlns:owl="http://www.w3.org/2002/07/owl#" rdf:ID="languageCoding">
      <dcr:datcat rdf:resource="http://www.isocat.org/datcat/DC-2008"/>
      <rdfs:label xml:lang="en">language code</rdfs:label>
      <rdfs:comment xml:lang="en">Designation of the standard used to code the name of the
   languages.</rdfs:comment>
   </owl:Class>
   <owl:Class xmlns:owl="http://www.w3.org/2002/07/owl#" rdf:ID="lativeCase">
      <dcr:datcat rdf:resource="http://www.isocat.org/datcat/DC-1323"/>
      <rdfs:label xml:lang="en">lative case</rdfs:label>
      <rdfs:comment xml:lang="en">Case which expresses motion to a location. </rdfs:comment>
   </owl:Class>
   <owl:Class xmlns:owl="http://www.w3.org/2002/07/owl#" rdf:ID="leftEnvironment">
      <dcr:datcat rdf:resource="http://www.isocat.org/datcat/DC-2194"/>
      <rdfs:label xml:lang="en">left environment</rdfs:label>
      <rdfs:comment xml:lang="en">Left side from a specific point</rdfs:comment>
   </owl:Class>
   <owl:Class xmlns:owl="http://www.w3.org/2002/07/owl#" rdf:ID="lemma">
      <dcr:datcat rdf:resource="http://www.isocat.org/datcat/DC-1324"/>
      <rdfs:label xml:lang="en">lemma</rdfs:label>
      <rdfs:comment xml:lang="en">Base form a word or term that is used as the formal entry in a
   dictionary. </rdfs:comment>
   </owl:Class>
   <owl:Class xmlns:owl="http://www.w3.org/2002/07/owl#" rdf:ID="letter">
      <dcr:datcat rdf:resource="http://www.isocat.org/datcat/DC-1889"/>
      <rdfs:label xml:lang="en">letter</rdfs:label>
      <rdfs:comment xml:lang="en">Letter.</rdfs:comment>
   </owl:Class>
   <owl:Class xmlns:owl="http://www.w3.org/2002/07/owl#" rdf:ID="lexeme">
      <dcr:datcat rdf:resource="http://www.isocat.org/datcat/DC-1325"/>
      <rdfs:label xml:lang="en">lexeme</rdfs:label>
      <rdfs:comment xml:lang="en">Minimal unit of language which : has a semantic interpretation and
   embodies a distinct cultural concept. </rdfs:comment>
   </owl:Class>
   <owl:Class xmlns:owl="http://www.w3.org/2002/07/owl#" rdf:ID="lexicalType">
      <dcr:datcat rdf:resource="http://www.isocat.org/datcat/DC-2175"/>
      <rdfs:label xml:lang="en">lexical type</rdfs:label>
      <rdfs:comment xml:lang="en">Type of an entry in a lexicon</rdfs:comment>
   </owl:Class>
   <owl:Class xmlns:owl="http://www.w3.org/2002/07/owl#" rdf:ID="location">
      <dcr:datcat rdf:resource="http://www.isocat.org/datcat/DC-2237"/>
      <rdfs:label xml:lang="en">location</rdfs:label>
      <rdfs:comment xml:lang="en">position of something</rdfs:comment>
   </owl:Class>
   <owl:Class xmlns:owl="http://www.w3.org/2002/07/owl#" rdf:ID="locativeCase">
      <dcr:datcat rdf:resource="http://www.isocat.org/datcat/DC-1326"/>
      <rdfs:label xml:lang="en">locative case</rdfs:label>
      <rdfs:comment xml:lang="en">Case that indicates a final location of action or a time of the
   action. </rdfs:comment>
   </owl:Class>
   <owl:Class xmlns:owl="http://www.w3.org/2002/07/owl#" rdf:ID="logicalAnd">
      <dcr:datcat rdf:resource="http://www.isocat.org/datcat/DC-2190"/>
      <rdfs:label xml:lang="en">logical and</rdfs:label>
      <rdfs:comment xml:lang="en">Logical operation that results in a value of true if all of its
   operands are true, otherwise a value of false</rdfs:comment>
   </owl:Class>
   <owl:Class xmlns:owl="http://www.w3.org/2002/07/owl#" rdf:ID="logicalNot">
      <dcr:datcat rdf:resource="http://www.isocat.org/datcat/DC-2192"/>
      <rdfs:label xml:lang="en">logical not</rdfs:label>
      <rdfs:comment xml:lang="en">Logical unary operation that returns true when its operand is false,
   otherwise returns true</rdfs:comment>
   </owl:Class>
   <owl:Class xmlns:owl="http://www.w3.org/2002/07/owl#" rdf:ID="logicalOperator">
      <dcr:datcat rdf:resource="http://www.isocat.org/datcat/DC-2208"/>
      <rdfs:label xml:lang="en">logical operator</rdfs:label>
      <rdfs:comment xml:lang="en">Type of action that gives a value of true or false</rdfs:comment>
   </owl:Class>
   <owl:Class xmlns:owl="http://www.w3.org/2002/07/owl#" rdf:ID="logicalValue">
      <dcr:datcat rdf:resource="http://www.isocat.org/datcat/DC-2209"/>
      <rdfs:label xml:lang="en">logical value</rdfs:label>
      <rdfs:comment xml:lang="en">Value used in a logical operation</rdfs:comment>
   </owl:Class>
   <owl:Class xmlns:owl="http://www.w3.org/2002/07/owl#" rdf:ID="macron">
      <dcr:datcat rdf:resource="http://www.isocat.org/datcat/DC-1327"/>
      <rdfs:label xml:lang="en">macron</rdfs:label>
      <rdfs:comment xml:lang="en">Mark placed over a long vowel to mark quantity. </rdfs:comment>
   </owl:Class>
   <owl:Class xmlns:owl="http://www.w3.org/2002/07/owl#" rdf:ID="mainPunctuation">
      <dcr:datcat rdf:resource="http://www.isocat.org/datcat/DC-2075"/>
      <rdfs:label xml:lang="en">main punctuation</rdfs:label>
      <rdfs:comment xml:lang="en">Punctuation that is more important than a secondary punctuation with
   regards to sentence splitting in a text.</rdfs:comment>
   </owl:Class>
   <owl:Class xmlns:owl="http://www.w3.org/2002/07/owl#" rdf:ID="mainVerb">
      <dcr:datcat rdf:resource="http://www.isocat.org/datcat/DC-1400"/>
      <rdfs:label xml:lang="en">main verb</rdfs:label>
      <rdfs:comment xml:lang="en">Main verb in contrast to a modal or an auxiliary.</rdfs:comment>
   </owl:Class>
   <owl:Class xmlns:owl="http://www.w3.org/2002/07/owl#" rdf:ID="masculine">
      <dcr:datcat rdf:resource="http://www.isocat.org/datcat/DC-1883"/>
      <rdfs:label xml:lang="en">masculine</rdfs:label>
      <rdfs:comment xml:lang="en">Of, relating to, or constituting the gender that ordinarily includes
   most words or grammatical forms referring to males.</rdfs:comment>
   </owl:Class>
   <owl:Class xmlns:owl="http://www.w3.org/2002/07/owl#" rdf:ID="masdar">
      <dcr:datcat rdf:resource="http://www.isocat.org/datcat/DC-2224"/>
      <rdfs:label xml:lang="en">masdar</rdfs:label>
      <rdfs:comment xml:lang="en">property that expresses a verbal idea under an abstract
   form.</rdfs:comment>
   </owl:Class>
   <owl:Class xmlns:owl="http://www.w3.org/2002/07/owl#" rdf:ID="middleVoice">
      <dcr:datcat rdf:resource="http://www.isocat.org/datcat/DC-1983"/>
      <rdfs:label xml:lang="en">middle voice</rdfs:label>
      <rdfs:comment xml:lang="en">Value for middle voice that expresses that the subject is both the
   agent and object, or that the subject is separate from the agent or that the receiver is the
   agent him/herself.</rdfs:comment>
   </owl:Class>
   <owl:Class xmlns:owl="http://www.w3.org/2002/07/owl#" rdf:ID="modal">
      <dcr:datcat rdf:resource="http://www.isocat.org/datcat/DC-1329"/>
      <rdfs:label xml:lang="en">modal</rdfs:label>
      <rdfs:comment xml:lang="en">Verb form that is usually used with another verb to express ideas such
   as possibilities, permission, or intention.</rdfs:comment>
   </owl:Class>
   <owl:Class xmlns:owl="http://www.w3.org/2002/07/owl#" rdf:ID="modalParticle">
      <dcr:datcat rdf:resource="http://www.isocat.org/datcat/DC-1920"/>
      <rdfs:label xml:lang="en">modal particle</rdfs:label>
      <rdfs:comment xml:lang="en">Particle which functions as a modal.</rdfs:comment>
   </owl:Class>
   <owl:Class xmlns:owl="http://www.w3.org/2002/07/owl#" rdf:ID="modern">
      <dcr:datcat rdf:resource="http://www.isocat.org/datcat/DC-1962"/>
      <rdfs:label xml:lang="en">modern</rdfs:label>
      <rdfs:comment xml:lang="en">Currently in use.</rdfs:comment>
   </owl:Class>
   <owl:Class xmlns:owl="http://www.w3.org/2002/07/owl#" rdf:ID="modificationType">
      <dcr:datcat rdf:resource="http://www.isocat.org/datcat/DC-1931"/>
      <rdfs:label xml:lang="en">modification type</rdfs:label>
      <rdfs:comment xml:lang="en">Refers to the prenominal or postnominal positions of determiners which
   distinguish different forms.</rdfs:comment>
   </owl:Class>
   <owl:Class xmlns:owl="http://www.w3.org/2002/07/owl#" rdf:ID="morpheme">
      <dcr:datcat rdf:resource="http://www.isocat.org/datcat/DC-1330"/>
      <rdfs:label xml:lang="en">morpheme</rdfs:label>
      <rdfs:comment xml:lang="en">A morpheme is the smallest meaningful unit in the grammar of a
   language. </rdfs:comment>
   </owl:Class>
   <owl:Class xmlns:owl="http://www.w3.org/2002/07/owl#" rdf:ID="morphologicalFeature">
      <dcr:datcat rdf:resource="http://www.isocat.org/datcat/DC-1425"/>
      <rdfs:label xml:lang="en">morphological feature</rdfs:label>
      <rdfs:comment xml:lang="en">Property attached to a given inflected form that usually permits to
   distinguish this form from the generic lemmatised form of the word.</rdfs:comment>
   </owl:Class>
   <owl:Class xmlns:owl="http://www.w3.org/2002/07/owl#" rdf:ID="namedEntity">
      <dcr:datcat rdf:resource="http://www.isocat.org/datcat/DC-2275"/>
      <rdfs:label xml:lang="en">named entity</rdfs:label>
      <rdfs:comment xml:lang="en">segment of text for which one or many rigid designators stands for the
   referent</rdfs:comment>
   </owl:Class>
   <owl:Class xmlns:owl="http://www.w3.org/2002/07/owl#" rdf:ID="native">
      <dcr:datcat rdf:resource="http://www.isocat.org/datcat/DC-1871"/>
      <rdfs:label xml:lang="en">native</rdfs:label>
      <rdfs:comment xml:lang="en">Value that expresses the absence of transformation</rdfs:comment>
   </owl:Class>
   <owl:Class xmlns:owl="http://www.w3.org/2002/07/owl#" rdf:ID="negative">
      <dcr:datcat rdf:resource="http://www.isocat.org/datcat/DC-1839"/>
      <rdfs:label xml:lang="en">negative</rdfs:label>
      <rdfs:comment xml:lang="en">denotes the negation or the absence</rdfs:comment>
   </owl:Class>
   <owl:Class xmlns:owl="http://www.w3.org/2002/07/owl#" rdf:ID="negativeParticle">
      <dcr:datcat rdf:resource="http://www.isocat.org/datcat/DC-1894"/>
      <rdfs:label xml:lang="en">negative particle</rdfs:label>
      <rdfs:comment xml:lang="en">Particle used to express negation.</rdfs:comment>
   </owl:Class>
   <owl:Class xmlns:owl="http://www.w3.org/2002/07/owl#" rdf:ID="negativePronoun">
      <dcr:datcat rdf:resource="http://www.isocat.org/datcat/DC-1925"/>
      <rdfs:label xml:lang="en">negative pronoun</rdfs:label>
      <rdfs:comment xml:lang="en">Pronoun used in a context of a negation or for expressing a
   negation.</rdfs:comment>
   </owl:Class>
   <owl:Class xmlns:owl="http://www.w3.org/2002/07/owl#" rdf:ID="neuter">
      <dcr:datcat rdf:resource="http://www.isocat.org/datcat/DC-1884"/>
      <rdfs:label xml:lang="en">neuter</rdfs:label>
      <rdfs:comment xml:lang="en">Of, relating to, or constituting the gender that ordinarily includes
   most words or grammatical forms referring to objects that are not characterized as male or
   female.</rdfs:comment>
   </owl:Class>
   <owl:Class xmlns:owl="http://www.w3.org/2002/07/owl#" rdf:ID="neutralRegister">
      <dcr:datcat rdf:resource="http://www.isocat.org/datcat/DC-1999"/>
      <rdfs:label xml:lang="en">neutral register</rdfs:label>
      <rdfs:comment xml:lang="en">The register appropriate to general texts or discourse.</rdfs:comment>
   </owl:Class>
   <owl:Class xmlns:owl="http://www.w3.org/2002/07/owl#" rdf:ID="no">
      <dcr:datcat rdf:resource="http://www.isocat.org/datcat/DC-1905"/>
      <rdfs:label xml:lang="en">no</rdfs:label>
      <rdfs:comment xml:lang="en">Value for negation.</rdfs:comment>
   </owl:Class>
   <owl:Class xmlns:owl="http://www.w3.org/2002/07/owl#" rdf:ID="nominativeCase">
      <dcr:datcat rdf:resource="http://www.isocat.org/datcat/DC-1331"/>
      <rdfs:label xml:lang="en">nominative case</rdfs:label>
      <rdfs:comment xml:lang="en">Case used to indicate the subject of a verb. </rdfs:comment>
   </owl:Class>
   <owl:Class xmlns:owl="http://www.w3.org/2002/07/owl#" rdf:ID="nonSpacedPinyin">
      <dcr:datcat rdf:resource="http://www.isocat.org/datcat/DC-1853"/>
      <rdfs:label xml:lang="en">non spaced pinyin</rdfs:label>
      <rdfs:comment xml:lang="en">Pinyin without any space characters</rdfs:comment>
   </owl:Class>
   <owl:Class xmlns:owl="http://www.w3.org/2002/07/owl#" rdf:ID="nonFinite">
      <dcr:datcat rdf:resource="http://www.isocat.org/datcat/DC-1332"/>
      <rdfs:label xml:lang="en">non-finite</rdfs:label>
      <rdfs:comment xml:lang="en">Property related for verb forms occurring on their own only in
   dependent clauses and lacking tense and mood contrasts. </rdfs:comment>
   </owl:Class>
   <owl:Class xmlns:owl="http://www.w3.org/2002/07/owl#" rdf:ID="noun">
      <dcr:datcat rdf:resource="http://www.isocat.org/datcat/DC-1333"/>
      <rdfs:label xml:lang="en">noun</rdfs:label>
      <rdfs:comment xml:lang="en">Part of speech used to express the name of a person, place, action or
   thing. </rdfs:comment>
   </owl:Class>
   <owl:Class xmlns:owl="http://www.w3.org/2002/07/owl#" rdf:ID="numeral">
      <dcr:datcat rdf:resource="http://www.isocat.org/datcat/DC-1334"/>
      <rdfs:label xml:lang="en">numeral</rdfs:label>
      <rdfs:comment xml:lang="en">Part of speech that expresses a number or the relation to a
   number.</rdfs:comment>
   </owl:Class>
   <owl:Class xmlns:owl="http://www.w3.org/2002/07/owl#" rdf:ID="numeralMForm">
      <dcr:datcat rdf:resource="http://www.isocat.org/datcat/DC-1939"/>
      <rdfs:label xml:lang="en">numeral MForm</rdfs:label>
      <rdfs:comment xml:lang="en">Numeral MForm.</rdfs:comment>
   </owl:Class>
   <owl:Class xmlns:owl="http://www.w3.org/2002/07/owl#" rdf:ID="numeralApprox">
      <dcr:datcat rdf:resource="http://www.isocat.org/datcat/DC-1940"/>
      <rdfs:label xml:lang="en">numeral approximation</rdfs:label>
      <rdfs:comment xml:lang="en">Numeric approximation.</rdfs:comment>
   </owl:Class>
   <owl:Class xmlns:owl="http://www.w3.org/2002/07/owl#" rdf:ID="numeralBoth">
      <dcr:datcat rdf:resource="http://www.isocat.org/datcat/DC-1938"/>
      <rdfs:label xml:lang="en">numeral both</rdfs:label>
      <rdfs:comment xml:lang="en">Numeric value for two.</rdfs:comment>
   </owl:Class>
   <owl:Class xmlns:owl="http://www.w3.org/2002/07/owl#" rdf:ID="numeralDigit">
      <dcr:datcat rdf:resource="http://www.isocat.org/datcat/DC-1935"/>
      <rdfs:label xml:lang="en">numeral digit</rdfs:label>
      <rdfs:comment xml:lang="en">Numeral expressed by an arabic digit.</rdfs:comment>
   </owl:Class>
   <owl:Class xmlns:owl="http://www.w3.org/2002/07/owl#" rdf:ID="numeralLetter">
      <dcr:datcat rdf:resource="http://www.isocat.org/datcat/DC-1937"/>
      <rdfs:label xml:lang="en">numeral letter</rdfs:label>
      <rdfs:comment xml:lang="en">Numeral expressed with letters.</rdfs:comment>
   </owl:Class>
   <owl:Class xmlns:owl="http://www.w3.org/2002/07/owl#" rdf:ID="numeralRoman">
      <dcr:datcat rdf:resource="http://www.isocat.org/datcat/DC-1936"/>
      <rdfs:label xml:lang="en">numeral roman</rdfs:label>
      <rdfs:comment xml:lang="en">Numeral expressed with roman digits.</rdfs:comment>
   </owl:Class>
   <owl:Class xmlns:owl="http://www.w3.org/2002/07/owl#" rdf:ID="numValue">
      <dcr:datcat rdf:resource="http://www.isocat.org/datcat/DC-2211"/>
      <rdfs:label xml:lang="en">numerical value</rdfs:label>
      <rdfs:comment xml:lang="en">Numerical value to be interpreted in context.</rdfs:comment>
   </owl:Class>
   <owl:Class xmlns:owl="http://www.w3.org/2002/07/owl#" rdf:ID="objectPerson">
      <dcr:datcat rdf:resource="http://www.isocat.org/datcat/DC-2279"/>
      <rdfs:label xml:lang="en">object person</rdfs:label>
      <rdfs:comment xml:lang="en">person for the object of the verb</rdfs:comment>
   </owl:Class>
   <owl:Class xmlns:owl="http://www.w3.org/2002/07/owl#" rdf:ID="obliqueCase">
      <dcr:datcat rdf:resource="http://www.isocat.org/datcat/DC-1336"/>
      <rdfs:label xml:lang="en">oblique case</rdfs:label>
      <rdfs:comment xml:lang="en">Case that is used when a noun is the object of a verb or a
   proposition, except for nominative and vocative case. </rdfs:comment>
   </owl:Class>
   <owl:Class xmlns:owl="http://www.w3.org/2002/07/owl#" rdf:ID="old">
      <dcr:datcat rdf:resource="http://www.isocat.org/datcat/DC-1961"/>
      <rdfs:label xml:lang="en">old</rdfs:label>
      <rdfs:comment xml:lang="en">Used in the past.</rdfs:comment>
   </owl:Class>
   <owl:Class xmlns:owl="http://www.w3.org/2002/07/owl#" rdf:ID="openBracket">
      <dcr:datcat rdf:resource="http://www.isocat.org/datcat/DC-2082"/>
      <rdfs:label xml:lang="en">open bracket</rdfs:label>
      <rdfs:comment xml:lang="en">Punctuation that is represented graphically as [</rdfs:comment>
   </owl:Class>
   <owl:Class xmlns:owl="http://www.w3.org/2002/07/owl#" rdf:ID="openCurlyBracket">
      <dcr:datcat rdf:resource="http://www.isocat.org/datcat/DC-2084"/>
      <rdfs:label xml:lang="en">open curly bracket</rdfs:label>
      <rdfs:comment xml:lang="en">Punctuation that is graphically represented as {</rdfs:comment>
   </owl:Class>
   <owl:Class xmlns:owl="http://www.w3.org/2002/07/owl#" rdf:ID="openParenthesis">
      <dcr:datcat rdf:resource="http://www.isocat.org/datcat/DC-1442"/>
      <rdfs:label xml:lang="en">open parenthesis</rdfs:label>
      <rdfs:comment xml:lang="en">Beginning of a pair of parenthesis.</rdfs:comment>
   </owl:Class>
   <owl:Class xmlns:owl="http://www.w3.org/2002/07/owl#" rdf:ID="openPunctuation">
      <dcr:datcat rdf:resource="http://www.isocat.org/datcat/DC-2078"/>
      <rdfs:label xml:lang="en">open punctuation</rdfs:label>
      <rdfs:comment xml:lang="en">Beginning of a paired punctuation.</rdfs:comment>
   </owl:Class>
   <owl:Class xmlns:owl="http://www.w3.org/2002/07/owl#" rdf:ID="operation">
      <dcr:datcat rdf:resource="http://www.isocat.org/datcat/DC-2179"/>
      <rdfs:label xml:lang="en">operation</rdfs:label>
      <rdfs:comment xml:lang="en">Way something such as a principle or law works or has an
   effect</rdfs:comment>
   </owl:Class>
   <owl:Class xmlns:owl="http://www.w3.org/2002/07/owl#" rdf:ID="operator">
      <dcr:datcat rdf:resource="http://www.isocat.org/datcat/DC-2235"/>
      <rdfs:label xml:lang="en">operator</rdfs:label>
      <rdfs:comment xml:lang="en">action name that can be applied to any number of
   operands</rdfs:comment>
   </owl:Class>
   <owl:Class xmlns:owl="http://www.w3.org/2002/07/owl#" rdf:ID="order">
      <dcr:datcat rdf:resource="http://www.isocat.org/datcat/DC-2356"/>
      <rdfs:label xml:lang="en">order</rdfs:label>
      <rdfs:comment xml:lang="en">way things are arranged in relation to each other</rdfs:comment>
   </owl:Class>
   <owl:Class xmlns:owl="http://www.w3.org/2002/07/owl#" rdf:ID="ordinalAdjective">
      <dcr:datcat rdf:resource="http://www.isocat.org/datcat/DC-1338"/>
      <rdfs:label xml:lang="en">ordinal adjective</rdfs:label>
      <rdfs:comment xml:lang="en">Adjective expressing a numeric ranking.</rdfs:comment>
   </owl:Class>
   <owl:Class xmlns:owl="http://www.w3.org/2002/07/owl#" rdf:ID="orthographyName">
      <dcr:datcat rdf:resource="http://www.isocat.org/datcat/DC-2176"/>
      <rdfs:label xml:lang="en">orthography name</rdfs:label>
      <rdfs:comment xml:lang="en">Precision concerning the orthography</rdfs:comment>
   </owl:Class>
   <owl:Class xmlns:owl="http://www.w3.org/2002/07/owl#" rdf:ID="otherAnimacy">
      <dcr:datcat rdf:resource="http://www.isocat.org/datcat/DC-1953"/>
      <rdfs:label xml:lang="en">other animacy</rdfs:label>
      <rdfs:comment xml:lang="en">Perceived as related to animacy, but without specific reference to the
   previous items.</rdfs:comment>
   </owl:Class>
   <owl:Class xmlns:owl="http://www.w3.org/2002/07/owl#" rdf:ID="ownedNumber">
      <dcr:datcat rdf:resource="http://www.isocat.org/datcat/DC-1930"/>
      <rdfs:label xml:lang="en">owned number</rdfs:label>
      <rdfs:comment xml:lang="en">Indication concerning the number of the possessed
   thing.</rdfs:comment>
   </owl:Class>
   <owl:Class xmlns:owl="http://www.w3.org/2002/07/owl#" rdf:ID="ownerGender">
      <dcr:datcat rdf:resource="http://www.isocat.org/datcat/DC-1416"/>
      <rdfs:label xml:lang="en">owner gender</rdfs:label>
      <rdfs:comment xml:lang="en">Indication concerning the gender of the person that ownes
   something.</rdfs:comment>
   </owl:Class>
   <owl:Class xmlns:owl="http://www.w3.org/2002/07/owl#" rdf:ID="ownerNumber">
      <dcr:datcat rdf:resource="http://www.isocat.org/datcat/DC-1417"/>
      <rdfs:label xml:lang="en">owner number</rdfs:label>
      <rdfs:comment xml:lang="en">Indication concerning the number of the person that ownes
   something.</rdfs:comment>
   </owl:Class>
   <owl:Class xmlns:owl="http://www.w3.org/2002/07/owl#" rdf:ID="ownerPerson">
      <dcr:datcat rdf:resource="http://www.isocat.org/datcat/DC-1929"/>
      <rdfs:label xml:lang="en">owner person</rdfs:label>
      <rdfs:comment xml:lang="en">Indication concerning the person that ownes something.</rdfs:comment>
   </owl:Class>
   <owl:Class xmlns:owl="http://www.w3.org/2002/07/owl#" rdf:ID="partOfSpeech">
      <dcr:datcat rdf:resource="http://www.isocat.org/datcat/DC-1345"/>
      <rdfs:label xml:lang="en">part of speech</rdfs:label>
      <rdfs:comment xml:lang="en">Term used to describe how a particular word is used in a
   sentence.</rdfs:comment>
   </owl:Class>
   <owl:Class xmlns:owl="http://www.w3.org/2002/07/owl#" rdf:ID="participle">
      <dcr:datcat rdf:resource="http://www.isocat.org/datcat/DC-1341"/>
      <rdfs:label xml:lang="en">participle</rdfs:label>
      <rdfs:comment xml:lang="en">Term referring to a word derived from a verb and used as an
   adjective.</rdfs:comment>
   </owl:Class>
   <owl:Class xmlns:owl="http://www.w3.org/2002/07/owl#" rdf:ID="participleAdjective">
      <dcr:datcat rdf:resource="http://www.isocat.org/datcat/DC-1598"/>
      <rdfs:label xml:lang="en">participle adjective</rdfs:label>
      <rdfs:comment xml:lang="en">Adjective based on a verb.</rdfs:comment>
   </owl:Class>
   <owl:Class xmlns:owl="http://www.w3.org/2002/07/owl#" rdf:ID="particle">
      <dcr:datcat rdf:resource="http://www.isocat.org/datcat/DC-1342"/>
      <rdfs:label xml:lang="en">particle</rdfs:label>
      <rdfs:comment xml:lang="en">Word that does not belong to one of the main classes of words, is
   invariable in form, and typically has grammatical or pragmatic meaning. </rdfs:comment>
   </owl:Class>
   <owl:Class xmlns:owl="http://www.w3.org/2002/07/owl#" rdf:ID="affirmativeParticle">
      <dcr:datcat rdf:resource="http://www.isocat.org/datcat/DC-1918"/>
      <rdfs:label xml:lang="en">particule affirmative</rdfs:label>
      <rdfs:comment xml:lang="en">Particle used to express affirmation.</rdfs:comment>
   </owl:Class>
   <owl:Class xmlns:owl="http://www.w3.org/2002/07/owl#" rdf:ID="partitiveArticle">
      <dcr:datcat rdf:resource="http://www.isocat.org/datcat/DC-1898"/>
      <rdfs:label xml:lang="en">partitive article</rdfs:label>
      <rdfs:comment xml:lang="en">Article expressing a part or quantity.</rdfs:comment>
   </owl:Class>
   <owl:Class xmlns:owl="http://www.w3.org/2002/07/owl#" rdf:ID="partitiveCase">
      <dcr:datcat rdf:resource="http://www.isocat.org/datcat/DC-2003"/>
      <rdfs:label xml:lang="en">partitive case</rdfs:label>
      <rdfs:comment xml:lang="en">Case that expresses the partial nature of the referent of the noun it
   marks, as opposed to expressing the whole unit or class of which the referent is a
   part.</rdfs:comment>
   </owl:Class>
   <owl:Class xmlns:owl="http://www.w3.org/2002/07/owl#" rdf:ID="passiveVoice">
      <dcr:datcat rdf:resource="http://www.isocat.org/datcat/DC-1346"/>
      <rdfs:label xml:lang="en">passive voice</rdfs:label>
      <rdfs:comment xml:lang="en">Term referring to a situation where the grammatical subject is
   typically the recipient or goal of the action denoted by the verb.</rdfs:comment>
   </owl:Class>
   <owl:Class xmlns:owl="http://www.w3.org/2002/07/owl#" rdf:ID="past">
      <dcr:datcat rdf:resource="http://www.isocat.org/datcat/DC-1347"/>
      <rdfs:label xml:lang="en">past</rdfs:label>
      <rdfs:comment xml:lang="en">Past tense is an absolute tense that refers to a time before the
   moment of utterance. </rdfs:comment>
   </owl:Class>
   <owl:Class xmlns:owl="http://www.w3.org/2002/07/owl#" rdf:ID="pastParticipleAdjective">
      <dcr:datcat rdf:resource="http://www.isocat.org/datcat/DC-1596"/>
      <rdfs:label xml:lang="en">past participle adjective</rdfs:label>
      <rdfs:comment xml:lang="en">Adjective based on a past participle.</rdfs:comment>
   </owl:Class>
   <owl:Class xmlns:owl="http://www.w3.org/2002/07/owl#" rdf:ID="patternType">
      <dcr:datcat rdf:resource="http://www.isocat.org/datcat/DC-2178"/>
      <rdfs:label xml:lang="en">pattern type</rdfs:label>
      <rdfs:comment xml:lang="en">Sub-type of a pattern class</rdfs:comment>
   </owl:Class>
   <owl:Class xmlns:owl="http://www.w3.org/2002/07/owl#" rdf:ID="paucal">
      <dcr:datcat rdf:resource="http://www.isocat.org/datcat/DC-1350"/>
      <rdfs:label xml:lang="en">paucal</rdfs:label>
      <rdfs:comment xml:lang="en">Number that specifies 'a few' things.</rdfs:comment>
   </owl:Class>
   <owl:Class xmlns:owl="http://www.w3.org/2002/07/owl#" rdf:ID="perfective">
      <dcr:datcat rdf:resource="http://www.isocat.org/datcat/DC-1352"/>
      <rdfs:label xml:lang="en">perfective</rdfs:label>
      <rdfs:comment xml:lang="en">Perfective aspect is an aspect that expresses a temporal view of an
   event or state as a simple whole, apart from the consideration of the internal structure of the
   time in which it occurs. </rdfs:comment>
   </owl:Class>
   <owl:Class xmlns:owl="http://www.w3.org/2002/07/owl#" rdf:ID="person">
      <dcr:datcat rdf:resource="http://www.isocat.org/datcat/DC-1328"/>
      <rdfs:label xml:lang="en">person</rdfs:label>
      <rdfs:comment xml:lang="en">Indication of grammatical person (1st, 2nd, 3rd, etc.) associated with
   a given inflected form.</rdfs:comment>
   </owl:Class>
   <owl:Class xmlns:owl="http://www.w3.org/2002/07/owl#" rdf:ID="personal">
      <dcr:datcat rdf:resource="http://www.isocat.org/datcat/DC-1946"/>
      <rdfs:label xml:lang="en">personal</rdfs:label>
      <rdfs:comment xml:lang="en">Property that refers to the person.</rdfs:comment>
   </owl:Class>
   <owl:Class xmlns:owl="http://www.w3.org/2002/07/owl#" rdf:ID="personalPronoun">
      <dcr:datcat rdf:resource="http://www.isocat.org/datcat/DC-1463"/>
      <rdfs:label xml:lang="en">personal pronoun</rdfs:label>
      <rdfs:comment xml:lang="en">Pronoun referring a person.</rdfs:comment>
   </owl:Class>
   <owl:Class xmlns:owl="http://www.w3.org/2002/07/owl#" rdf:ID="phoneticForm">
      <dcr:datcat rdf:resource="http://www.isocat.org/datcat/DC-1837"/>
      <rdfs:label xml:lang="en">phonetic form</rdfs:label>
      <rdfs:comment xml:lang="en">Representation of the spoken string of a form</rdfs:comment>
   </owl:Class>
   <owl:Class xmlns:owl="http://www.w3.org/2002/07/owl#" rdf:ID="phoneticOperator">
      <dcr:datcat rdf:resource="http://www.isocat.org/datcat/DC-1861"/>
      <rdfs:label xml:lang="en">phonetic operator</rdfs:label>
      <rdfs:comment xml:lang="en">Description of the modification of a spoken form</rdfs:comment>
   </owl:Class>
   <owl:Class xmlns:owl="http://www.w3.org/2002/07/owl#" rdf:ID="pinyin">
      <dcr:datcat rdf:resource="http://www.isocat.org/datcat/DC-1852"/>
      <rdfs:label xml:lang="en">pinyin</rdfs:label>
      <rdfs:comment xml:lang="en">Transcription of Chinese ideograms</rdfs:comment>
   </owl:Class>
   <owl:Class xmlns:owl="http://www.w3.org/2002/07/owl#" rdf:ID="plural">
      <dcr:datcat rdf:resource="http://www.isocat.org/datcat/DC-1354"/>
      <rdfs:label xml:lang="en">plural</rdfs:label>
      <rdfs:comment xml:lang="en">Value that expresses more than one element.</rdfs:comment>
   </owl:Class>
   <owl:Class xmlns:owl="http://www.w3.org/2002/07/owl#" rdf:ID="pluralType">
      <dcr:datcat rdf:resource="http://www.isocat.org/datcat/DC-2232"/>
      <rdfs:label xml:lang="en">plural type</rdfs:label>
      <rdfs:comment xml:lang="en">type of plural</rdfs:comment>
   </owl:Class>
   <owl:Class xmlns:owl="http://www.w3.org/2002/07/owl#" rdf:ID="point">
      <dcr:datcat rdf:resource="http://www.isocat.org/datcat/DC-1445"/>
      <rdfs:label xml:lang="en">point</rdfs:label>
      <rdfs:comment xml:lang="en">Sign (.) used to expresses the end of a sentence or an
   abbreviation.</rdfs:comment>
   </owl:Class>
   <owl:Class xmlns:owl="http://www.w3.org/2002/07/owl#" rdf:ID="position">
      <dcr:datcat rdf:resource="http://www.isocat.org/datcat/DC-2183"/>
      <rdfs:label xml:lang="en">position</rdfs:label>
      <rdfs:comment xml:lang="en">Place where something is needed or supposed to be</rdfs:comment>
   </owl:Class>
   <owl:Class xmlns:owl="http://www.w3.org/2002/07/owl#" rdf:ID="positive">
      <dcr:datcat rdf:resource="http://www.isocat.org/datcat/DC-1420"/>
      <rdfs:label xml:lang="en">positive</rdfs:label>
      <rdfs:comment xml:lang="en">Value used in a comparison relationship when no comparison is
   involved.</rdfs:comment>
   </owl:Class>
   <owl:Class xmlns:owl="http://www.w3.org/2002/07/owl#" rdf:ID="possessive">
      <dcr:datcat rdf:resource="http://www.isocat.org/datcat/DC-1355"/>
      <rdfs:label xml:lang="en">possessive</rdfs:label>
      <rdfs:comment xml:lang="en">Relative to the possession or association. </rdfs:comment>
   </owl:Class>
   <owl:Class xmlns:owl="http://www.w3.org/2002/07/owl#" rdf:ID="possessiveDeterminer">
      <dcr:datcat rdf:resource="http://www.isocat.org/datcat/DC-1357"/>
      <rdfs:label xml:lang="en">possessive determiner</rdfs:label>
      <rdfs:comment xml:lang="en">Determiner that expresses ownership.</rdfs:comment>
   </owl:Class>
   <owl:Class xmlns:owl="http://www.w3.org/2002/07/owl#" rdf:ID="possessiveParticle">
      <dcr:datcat rdf:resource="http://www.isocat.org/datcat/DC-1895"/>
      <rdfs:label xml:lang="en">possessive particle</rdfs:label>
      <rdfs:comment xml:lang="en">Particle expressing ownship.</rdfs:comment>
   </owl:Class>
   <owl:Class xmlns:owl="http://www.w3.org/2002/07/owl#" rdf:ID="possessivePronoun">
      <dcr:datcat rdf:resource="http://www.isocat.org/datcat/DC-1359"/>
      <rdfs:label xml:lang="en">possessive pronoun</rdfs:label>
      <rdfs:comment xml:lang="en">Pronoun that expresses ownership and relationships like ownership,
   such as kinship, and other forms of association. </rdfs:comment>
   </owl:Class>
   <owl:Class xmlns:owl="http://www.w3.org/2002/07/owl#" rdf:ID="possible">
      <dcr:datcat rdf:resource="http://www.isocat.org/datcat/DC-1865"/>
      <rdfs:label xml:lang="en">possible</rdfs:label>
      <rdfs:comment xml:lang="en">Value that denotes a linguistic situation considered as being correct
   in the given language</rdfs:comment>
   </owl:Class>
   <owl:Class xmlns:owl="http://www.w3.org/2002/07/owl#" rdf:ID="postModifier">
      <dcr:datcat rdf:resource="http://www.isocat.org/datcat/DC-1945"/>
      <rdfs:label xml:lang="en">post modifier</rdfs:label>
      <rdfs:comment xml:lang="en">Situation where the modifier is after the modified.</rdfs:comment>
   </owl:Class>
   <owl:Class xmlns:owl="http://www.w3.org/2002/07/owl#" rdf:ID="postposition">
      <dcr:datcat rdf:resource="http://www.isocat.org/datcat/DC-1360"/>
      <rdfs:label xml:lang="en">postposition</rdfs:label>
      <rdfs:comment xml:lang="en">Adposition that appears at the end of the noun phrase.</rdfs:comment>
   </owl:Class>
   <owl:Class xmlns:owl="http://www.w3.org/2002/07/owl#" rdf:ID="prefix">
      <dcr:datcat rdf:resource="http://www.isocat.org/datcat/DC-1365"/>
      <rdfs:label xml:lang="en">prefix</rdfs:label>
      <rdfs:comment xml:lang="en">Affix added before a word to change its meaning or part of
   speech.</rdfs:comment>
   </owl:Class>
   <owl:Class xmlns:owl="http://www.w3.org/2002/07/owl#" rdf:ID="preModifier">
      <dcr:datcat rdf:resource="http://www.isocat.org/datcat/DC-1943"/>
      <rdfs:label xml:lang="en">premodifier</rdfs:label>
      <rdfs:comment xml:lang="en">Situation where the modifier is before the modified.</rdfs:comment>
   </owl:Class>
   <owl:Class xmlns:owl="http://www.w3.org/2002/07/owl#" rdf:ID="preposition">
      <dcr:datcat rdf:resource="http://www.isocat.org/datcat/DC-1366"/>
      <rdfs:label xml:lang="en">preposition</rdfs:label>
      <rdfs:comment xml:lang="en">Adposition placed at the beginning of a noun phrase.</rdfs:comment>
   </owl:Class>
   <owl:Class xmlns:owl="http://www.w3.org/2002/07/owl#" rdf:ID="present">
      <dcr:datcat rdf:resource="http://www.isocat.org/datcat/DC-1367"/>
      <rdfs:label xml:lang="en">present</rdfs:label>
      <rdfs:comment xml:lang="en">Verb tense that indicates action or state of being in the present.
  </rdfs:comment>
   </owl:Class>
   <owl:Class xmlns:owl="http://www.w3.org/2002/07/owl#" rdf:ID="presentParticipleAdjective">
      <dcr:datcat rdf:resource="http://www.isocat.org/datcat/DC-1597"/>
      <rdfs:label xml:lang="en">present participle adjective</rdfs:label>
      <rdfs:comment xml:lang="en">Adjective based on a present participle.</rdfs:comment>
   </owl:Class>
   <owl:Class xmlns:owl="http://www.w3.org/2002/07/owl#" rdf:ID="preverbalParticleLmf">
      <dcr:datcat rdf:resource="http://www.isocat.org/datcat/DC-1455"/>
      <rdfs:label xml:lang="en">preverbalParticleLmf</rdfs:label>
   </owl:Class>
   <owl:Class xmlns:owl="http://www.w3.org/2002/07/owl#" rdf:ID="prolativeCase">
      <dcr:datcat rdf:resource="http://www.isocat.org/datcat/DC-1368"/>
      <rdfs:label xml:lang="en">prolative case</rdfs:label>
      <rdfs:comment xml:lang="en">Case for a noun or a pronoun that expresses motion within a place or a
   period of time needed for an event.</rdfs:comment>
   </owl:Class>
   <owl:Class xmlns:owl="http://www.w3.org/2002/07/owl#" rdf:ID="pronoun">
      <dcr:datcat rdf:resource="http://www.isocat.org/datcat/DC-1370"/>
      <rdfs:label xml:lang="en">pronoun</rdfs:label>
      <rdfs:comment xml:lang="en">Word used in place of a noun or a noun phrase.</rdfs:comment>
   </owl:Class>
   <owl:Class xmlns:owl="http://www.w3.org/2002/07/owl#" rdf:ID="properNoun">
      <dcr:datcat rdf:resource="http://www.isocat.org/datcat/DC-1371"/>
      <rdfs:label xml:lang="en">proper noun</rdfs:label>
      <rdfs:comment xml:lang="en">Noun that is the name of a specific individual, place, or object.
  </rdfs:comment>
   </owl:Class>
   <owl:Class xmlns:owl="http://www.w3.org/2002/07/owl#" rdf:ID="punctuation">
      <dcr:datcat rdf:resource="http://www.isocat.org/datcat/DC-1372"/>
      <rdfs:label xml:lang="en">punctuation</rdfs:label>
      <rdfs:comment xml:lang="en">Graphical mark used either at word level to indicate an abbreviation
   or at a text level to separate phrases or sentences.</rdfs:comment>
   </owl:Class>
   <owl:Class xmlns:owl="http://www.w3.org/2002/07/owl#" rdf:ID="quadrial">
      <dcr:datcat rdf:resource="http://www.isocat.org/datcat/DC-2000"/>
      <rdfs:label xml:lang="en">quadrial</rdfs:label>
      <rdfs:comment xml:lang="en">Property related to four elements.</rdfs:comment>
   </owl:Class>
   <owl:Class xmlns:owl="http://www.w3.org/2002/07/owl#" rdf:ID="qualifierAdjective">
      <dcr:datcat rdf:resource="http://www.isocat.org/datcat/DC-1477"/>
      <rdfs:label xml:lang="en">qualifier adjective</rdfs:label>
      <rdfs:comment xml:lang="en">Adjective used to qualify.</rdfs:comment>
   </owl:Class>
   <owl:Class xmlns:owl="http://www.w3.org/2002/07/owl#" rdf:ID="questionMark">
      <dcr:datcat rdf:resource="http://www.isocat.org/datcat/DC-1444"/>
      <rdfs:label xml:lang="en">question mark</rdfs:label>
      <rdfs:comment xml:lang="en">Sign used to express a question.</rdfs:comment>
   </owl:Class>
   <owl:Class xmlns:owl="http://www.w3.org/2002/07/owl#" rdf:ID="quotative">
      <dcr:datcat rdf:resource="http://www.isocat.org/datcat/DC-1375"/>
      <rdfs:label xml:lang="en">quotative</rdfs:label>
      <rdfs:comment xml:lang="en">The Quotative modality is used when the speakers evidence is based on
   second hand information. </rdfs:comment>
   </owl:Class>
   <owl:Class xmlns:owl="http://www.w3.org/2002/07/owl#" rdf:ID="quote">
      <dcr:datcat rdf:resource="http://www.isocat.org/datcat/DC-2081"/>
      <rdfs:label xml:lang="en">quote</rdfs:label>
      <rdfs:comment xml:lang="en">Punctuation usually used to surround a quotation.</rdfs:comment>
   </owl:Class>
   <owl:Class xmlns:owl="http://www.w3.org/2002/07/owl#" rdf:ID="rank">
      <dcr:datcat rdf:resource="http://www.isocat.org/datcat/DC-1862"/>
      <rdfs:label xml:lang="en">rank</rdfs:label>
      <rdfs:comment xml:lang="en">Reference to one specific element in an ordered list of
   elements</rdfs:comment>
   </owl:Class>
   <owl:Class xmlns:owl="http://www.w3.org/2002/07/owl#" rdf:ID="rarelyUsed">
      <dcr:datcat rdf:resource="http://www.isocat.org/datcat/DC-1986"/>
      <rdfs:label xml:lang="en">rarely used</rdfs:label>
      <rdfs:comment xml:lang="en">Said of a term that is almost never used.</rdfs:comment>
   </owl:Class>
   <owl:Class xmlns:owl="http://www.w3.org/2002/07/owl#" rdf:ID="reciprocalPronoun">
      <dcr:datcat rdf:resource="http://www.isocat.org/datcat/DC-1924"/>
      <rdfs:label xml:lang="en">reciprocal pronoun</rdfs:label>
      <rdfs:comment xml:lang="en">Pronoun expressing mutual relationship.</rdfs:comment>
   </owl:Class>
   <owl:Class xmlns:owl="http://www.w3.org/2002/07/owl#" rdf:ID="reduplication">
      <dcr:datcat rdf:resource="http://www.isocat.org/datcat/DC-2346"/>
      <rdfs:label xml:lang="en">reduplication</rdfs:label>
      <rdfs:comment xml:lang="en">process to modify the sense of a word by some operations to repeat the
   sound of a word.</rdfs:comment>
   </owl:Class>
   <owl:Class xmlns:owl="http://www.w3.org/2002/07/owl#" rdf:ID="reduplicationType">
      <dcr:datcat rdf:resource="http://www.isocat.org/datcat/DC-2240"/>
      <rdfs:label xml:lang="en">reduplication type</rdfs:label>
      <rdfs:comment xml:lang="en">type of reduplication</rdfs:comment>
   </owl:Class>
   <owl:Class xmlns:owl="http://www.w3.org/2002/07/owl#" rdf:ID="ref">
      <dcr:datcat rdf:resource="http://www.isocat.org/datcat/DC-2352"/>
      <rdfs:label xml:lang="en">ref</rdfs:label>
      <rdfs:comment xml:lang="en">reference to another description</rdfs:comment>
   </owl:Class>
   <owl:Class xmlns:owl="http://www.w3.org/2002/07/owl#" rdf:ID="referentType">
      <dcr:datcat rdf:resource="http://www.isocat.org/datcat/DC-1376"/>
      <rdfs:label xml:lang="en">referent type</rdfs:label>
      <rdfs:comment xml:lang="en">Type of concrete object or concept (the referent) that an expression
   represents (the reference). </rdfs:comment>
   </owl:Class>
   <owl:Class xmlns:owl="http://www.w3.org/2002/07/owl#" rdf:ID="reflexiveDeterminer">
      <dcr:datcat rdf:resource="http://www.isocat.org/datcat/DC-1377"/>
      <rdfs:label xml:lang="en">reflexive adjective</rdfs:label>
      <rdfs:comment xml:lang="en">Determiner that refers to the same entity. </rdfs:comment>
   </owl:Class>
   <owl:Class xmlns:owl="http://www.w3.org/2002/07/owl#" rdf:ID="reflexivePronoun">
      <dcr:datcat rdf:resource="http://www.isocat.org/datcat/DC-1378"/>
      <rdfs:label xml:lang="en">reflexive pronoun</rdfs:label>
      <rdfs:comment xml:lang="en">Pronoun that refers to the subject of the sentence. </rdfs:comment>
   </owl:Class>
   <owl:Class xmlns:owl="http://www.w3.org/2002/07/owl#" rdf:ID="register">
      <dcr:datcat rdf:resource="http://www.isocat.org/datcat/DC-1988"/>
      <rdfs:label xml:lang="en">register</rdfs:label>
      <rdfs:comment xml:lang="en">Classification indicating the relative level of language individually
   assigned to a lexeme or term or to a text type.</rdfs:comment>
   </owl:Class>
   <owl:Class xmlns:owl="http://www.w3.org/2002/07/owl#" rdf:ID="relationNoun">
      <dcr:datcat rdf:resource="http://www.isocat.org/datcat/DC-2226"/>
      <rdfs:label xml:lang="en">relation noun</rdfs:label>
      <rdfs:comment xml:lang="en">relation noun</rdfs:comment>
   </owl:Class>
   <owl:Class xmlns:owl="http://www.w3.org/2002/07/owl#" rdf:ID="relativeDeterminer">
      <dcr:datcat rdf:resource="http://www.isocat.org/datcat/DC-1379"/>
      <rdfs:label xml:lang="en">relative determiner</rdfs:label>
      <rdfs:comment xml:lang="en">Determiner related to a referent.</rdfs:comment>
   </owl:Class>
   <owl:Class xmlns:owl="http://www.w3.org/2002/07/owl#" rdf:ID="relativeParticle">
      <dcr:datcat rdf:resource="http://www.isocat.org/datcat/DC-2229"/>
      <rdfs:label xml:lang="en">relative particle</rdfs:label>
      <rdfs:comment xml:lang="en">relative particle</rdfs:comment>
   </owl:Class>
   <owl:Class xmlns:owl="http://www.w3.org/2002/07/owl#" rdf:ID="relativePronoun">
      <dcr:datcat rdf:resource="http://www.isocat.org/datcat/DC-1380"/>
      <rdfs:label xml:lang="en">relative pronoun</rdfs:label>
      <rdfs:comment xml:lang="en">Pronoun which introduces a relative clause and refers to something
   that has been said before. </rdfs:comment>
   </owl:Class>
   <owl:Class xmlns:owl="http://www.w3.org/2002/07/owl#" rdf:ID="remove">
      <dcr:datcat rdf:resource="http://www.isocat.org/datcat/DC-2094"/>
      <rdfs:label xml:lang="en">remove</rdfs:label>
      <rdfs:comment xml:lang="en">Operation that remover N characters at position X.</rdfs:comment>
   </owl:Class>
   <owl:Class xmlns:owl="http://www.w3.org/2002/07/owl#" rdf:ID="removeAfter">
      <dcr:datcat rdf:resource="http://www.isocat.org/datcat/DC-1830"/>
      <rdfs:label xml:lang="en">remove after</rdfs:label>
      <rdfs:comment xml:lang="en">remove N characters from the right</rdfs:comment>
   </owl:Class>
   <owl:Class xmlns:owl="http://www.w3.org/2002/07/owl#" rdf:ID="removeBefore">
      <dcr:datcat rdf:resource="http://www.isocat.org/datcat/DC-1834"/>
      <rdfs:label xml:lang="en">remove before</rdfs:label>
      <rdfs:comment xml:lang="en">Operation that removes N characters from the left</rdfs:comment>
   </owl:Class>
   <owl:Class xmlns:owl="http://www.w3.org/2002/07/owl#" rdf:ID="required">
      <dcr:datcat rdf:resource="http://www.isocat.org/datcat/DC-2239"/>
      <rdfs:label xml:lang="en">required</rdfs:label>
      <rdfs:comment xml:lang="en">property concerning something that is mandatory</rdfs:comment>
   </owl:Class>
   <owl:Class xmlns:owl="http://www.w3.org/2002/07/owl#" rdf:ID="residual">
      <dcr:datcat rdf:resource="http://www.isocat.org/datcat/DC-1382"/>
      <rdfs:label xml:lang="en">residual</rdfs:label>
      <rdfs:comment xml:lang="en">The residual value is assigned to classes of textword which lie
   outside the traditionally accepted range of grammatical classes, although they occur quite
   commonly in many texts.</rdfs:comment>
   </owl:Class>
   <owl:Class xmlns:owl="http://www.w3.org/2002/07/owl#" rdf:ID="restriction">
      <dcr:datcat rdf:resource="http://www.isocat.org/datcat/DC-1956"/>
      <rdfs:label xml:lang="en">restriction</rdfs:label>
      <rdfs:comment xml:lang="en">General purpose additional specification for a given type of
   limitation.</rdfs:comment>
   </owl:Class>
   <owl:Class xmlns:owl="http://www.w3.org/2002/07/owl#" rdf:ID="rightEnvironment">
      <dcr:datcat rdf:resource="http://www.isocat.org/datcat/DC-2195"/>
      <rdfs:label xml:lang="en">right environment</rdfs:label>
      <rdfs:comment xml:lang="en">Right side from a particular point</rdfs:comment>
   </owl:Class>
   <owl:Class xmlns:owl="http://www.w3.org/2002/07/owl#" rdf:ID="romanization">
      <dcr:datcat rdf:resource="http://www.isocat.org/datcat/DC-1873"/>
      <rdfs:label xml:lang="en">romanization</rdfs:label>
      <rdfs:comment xml:lang="en">Transcription or transliteration from non-Latin script into Latin
   script.</rdfs:comment>
   </owl:Class>
   <owl:Class xmlns:owl="http://www.w3.org/2002/07/owl#" rdf:ID="root">
      <dcr:datcat rdf:resource="http://www.isocat.org/datcat/DC-2231"/>
      <rdfs:label xml:lang="en">root</rdfs:label>
      <rdfs:comment xml:lang="en">base of a word</rdfs:comment>
   </owl:Class>
   <owl:Class xmlns:owl="http://www.w3.org/2002/07/owl#" rdf:ID="rule">
      <dcr:datcat rdf:resource="http://www.isocat.org/datcat/DC-2180"/>
      <rdfs:label xml:lang="en">rule</rdfs:label>
      <rdfs:comment xml:lang="en">instruction that states how things are done or allowed</rdfs:comment>
   </owl:Class>
   <owl:Class xmlns:owl="http://www.w3.org/2002/07/owl#" rdf:ID="scheme">
      <dcr:datcat rdf:resource="http://www.isocat.org/datcat/DC-2174"/>
      <rdfs:label xml:lang="en">scheme</rdfs:label>
      <rdfs:comment xml:lang="en">Pattern for word creation</rdfs:comment>
   </owl:Class>
   <owl:Class xmlns:owl="http://www.w3.org/2002/07/owl#" rdf:ID="scope">
      <dcr:datcat rdf:resource="http://www.isocat.org/datcat/DC-2196"/>
      <rdfs:label xml:lang="en">scope</rdfs:label>
      <rdfs:comment xml:lang="en">Set of situations where a given property is valid</rdfs:comment>
   </owl:Class>
   <owl:Class xmlns:owl="http://www.w3.org/2002/07/owl#" rdf:ID="script">
      <dcr:datcat rdf:resource="http://www.isocat.org/datcat/DC-1855"/>
      <rdfs:label xml:lang="en">script</rdfs:label>
      <rdfs:comment xml:lang="en">Set of graphic characters used for the written form of one or more
   languages.</rdfs:comment>
   </owl:Class>
   <owl:Class xmlns:owl="http://www.w3.org/2002/07/owl#" rdf:ID="scriptCoding">
      <dcr:datcat rdf:resource="http://www.isocat.org/datcat/DC-2091"/>
      <rdfs:label xml:lang="en">script coding</rdfs:label>
      <rdfs:comment xml:lang="en">Designation of the standard used to code the script.</rdfs:comment>
   </owl:Class>
   <owl:Class xmlns:owl="http://www.w3.org/2002/07/owl#" rdf:ID="secondPerson">
      <dcr:datcat rdf:resource="http://www.isocat.org/datcat/DC-1384"/>
      <rdfs:label xml:lang="en">second person</rdfs:label>
      <rdfs:comment xml:lang="en">Second person deixis is deictic reference to a person or persons
   identified as addressee. </rdfs:comment>
   </owl:Class>
   <owl:Class xmlns:owl="http://www.w3.org/2002/07/owl#" rdf:ID="secondaryPunctuation">
      <dcr:datcat rdf:resource="http://www.isocat.org/datcat/DC-2076"/>
      <rdfs:label xml:lang="en">secondary punctuation</rdfs:label>
      <rdfs:comment xml:lang="en">Punctuation that is not very important with regards to sentence
   splitting in a text.</rdfs:comment>
   </owl:Class>
   <owl:Class xmlns:owl="http://www.w3.org/2002/07/owl#" rdf:ID="semiColon">
      <dcr:datcat rdf:resource="http://www.isocat.org/datcat/DC-1446"/>
      <rdfs:label xml:lang="en">semi-colon</rdfs:label>
      <rdfs:comment xml:lang="en">Sign (;) usually used to separate phrases.</rdfs:comment>
   </owl:Class>
   <owl:Class xmlns:owl="http://www.w3.org/2002/07/owl#" rdf:ID="sentence">
      <dcr:datcat rdf:resource="http://www.isocat.org/datcat/DC-1386"/>
      <rdfs:label xml:lang="en">sentence</rdfs:label>
      <rdfs:comment xml:lang="en"> A sentence is a grammatical unit that is composed of one or more
   clauses. A sequence of words capable of standing alone to make an assertion, ask a question, or
   give a command, usually consisting of a subject and a predicate containing a finite verb.
  </rdfs:comment>
   </owl:Class>
   <owl:Class xmlns:owl="http://www.w3.org/2002/07/owl#" rdf:ID="shortArticle">
      <dcr:datcat rdf:resource="http://www.isocat.org/datcat/DC-1927"/>
      <rdfs:label xml:lang="en">short article</rdfs:label>
      <rdfs:comment xml:lang="en">For definiteness, when a specific form is not the syntactic subject of
   the clause.</rdfs:comment>
   </owl:Class>
   <owl:Class xmlns:owl="http://www.w3.org/2002/07/owl#" rdf:ID="simplePreposition">
      <dcr:datcat rdf:resource="http://www.isocat.org/datcat/DC-1900"/>
      <rdfs:label xml:lang="en">simple preposition</rdfs:label>
      <rdfs:comment xml:lang="en">Preposition that is a pure simple word in contrast with the notion of
   fused preposition.</rdfs:comment>
   </owl:Class>
   <owl:Class xmlns:owl="http://www.w3.org/2002/07/owl#" rdf:ID="singular">
      <dcr:datcat rdf:resource="http://www.isocat.org/datcat/DC-1387"/>
      <rdfs:label xml:lang="en">singular</rdfs:label>
      <rdfs:comment xml:lang="en">Value that expresses one element.</rdfs:comment>
   </owl:Class>
   <owl:Class xmlns:owl="http://www.w3.org/2002/07/owl#" rdf:ID="slangRegister">
      <dcr:datcat rdf:resource="http://www.isocat.org/datcat/DC-1995"/>
      <rdfs:label xml:lang="en">slang register</rdfs:label>
      <rdfs:comment xml:lang="en">An extremely informal register of a word, term, or text that is used
   in spoken and everyday language and less commonly in documents.</rdfs:comment>
   </owl:Class>
   <owl:Class xmlns:owl="http://www.w3.org/2002/07/owl#" rdf:ID="slash">
      <dcr:datcat rdf:resource="http://www.isocat.org/datcat/DC-1437"/>
      <rdfs:label xml:lang="en">slash</rdfs:label>
      <rdfs:comment xml:lang="en">The punctuation sign /</rdfs:comment>
   </owl:Class>
   <owl:Class xmlns:owl="http://www.w3.org/2002/07/owl#" rdf:ID="sociativeCase">
      <dcr:datcat rdf:resource="http://www.isocat.org/datcat/DC-1388"/>
      <rdfs:label xml:lang="en">sociative case</rdfs:label>
      <rdfs:comment xml:lang="en">Case related to the person in whose company the action is carried out,
   or to any belongings of people which take part in the action.</rdfs:comment>
   </owl:Class>
   <owl:Class xmlns:owl="http://www.w3.org/2002/07/owl#" rdf:ID="sound">
      <dcr:datcat rdf:resource="http://www.isocat.org/datcat/DC-2250"/>
      <rdfs:label xml:lang="en">sound</rdfs:label>
      <rdfs:comment xml:lang="en">pronunciation that is on a record</rdfs:comment>
   </owl:Class>
   <owl:Class xmlns:owl="http://www.w3.org/2002/07/owl#" rdf:ID="source">
      <dcr:datcat rdf:resource="http://www.isocat.org/datcat/DC-1968"/>
      <rdfs:label xml:lang="en">source</rdfs:label>
      <rdfs:comment xml:lang="en">A complete citation of the bibliographic information pertaining to a
   document or other resource.</rdfs:comment>
   </owl:Class>
   <owl:Class xmlns:owl="http://www.w3.org/2002/07/owl#" rdf:ID="space">
      <dcr:datcat rdf:resource="http://www.isocat.org/datcat/DC-2189"/>
      <rdfs:label xml:lang="en">space</rdfs:label>
      <rdfs:comment xml:lang="en">Empty area between words, lines or columns</rdfs:comment>
   </owl:Class>
   <owl:Class xmlns:owl="http://www.w3.org/2002/07/owl#" rdf:ID="spacedPinyinAndTone">
      <dcr:datcat rdf:resource="http://www.isocat.org/datcat/DC-1854"/>
      <rdfs:label xml:lang="en">spaced pinyin and tone</rdfs:label>
      <rdfs:comment xml:lang="en">Pinyin with space and tone</rdfs:comment>
   </owl:Class>
   <owl:Class xmlns:owl="http://www.w3.org/2002/07/owl#" rdf:ID="stem">
      <dcr:datcat rdf:resource="http://www.isocat.org/datcat/DC-1389"/>
      <rdfs:label xml:lang="en">stem</rdfs:label>
      <rdfs:comment xml:lang="en">Root of a word, together with any derivational affixes, to which
   inflectional affixes are added. </rdfs:comment>
   </owl:Class>
   <owl:Class xmlns:owl="http://www.w3.org/2002/07/owl#" rdf:ID="stemRank">
      <dcr:datcat rdf:resource="http://www.isocat.org/datcat/DC-2186"/>
      <rdfs:label xml:lang="en">stem rank</rdfs:label>
      <rdfs:comment xml:lang="en">Rank of a stem</rdfs:comment>
   </owl:Class>
   <owl:Class xmlns:owl="http://www.w3.org/2002/07/owl#" rdf:ID="stringValue">
      <dcr:datcat rdf:resource="http://www.isocat.org/datcat/DC-2182"/>
      <rdfs:label xml:lang="en">string value</rdfs:label>
      <rdfs:comment xml:lang="en">Character string to be interpreted in context</rdfs:comment>
   </owl:Class>
   <owl:Class xmlns:owl="http://www.w3.org/2002/07/owl#" rdf:ID="strongPersonalPronoun">
      <dcr:datcat rdf:resource="http://www.isocat.org/datcat/DC-1390"/>
      <rdfs:label xml:lang="en">strong personal pronoun</rdfs:label>
      <rdfs:comment xml:lang="en">Personal pronoun that can occupy the position after a preposition
   and/or reinforce a weak personal pronoun.</rdfs:comment>
   </owl:Class>
   <owl:Class xmlns:owl="http://www.w3.org/2002/07/owl#" rdf:ID="subjectPerson">
      <dcr:datcat rdf:resource="http://www.isocat.org/datcat/DC-2278"/>
      <rdfs:label xml:lang="en">subject person</rdfs:label>
      <rdfs:comment xml:lang="en">person for the subject of the verb</rdfs:comment>
   </owl:Class>
   <owl:Class xmlns:owl="http://www.w3.org/2002/07/owl#" rdf:ID="subjunctive">
      <dcr:datcat rdf:resource="http://www.isocat.org/datcat/DC-1843"/>
      <rdfs:label xml:lang="en">subjunctive</rdfs:label>
      <rdfs:comment xml:lang="en">Mood often used to express uncertainty, whishes or
   desires.</rdfs:comment>
   </owl:Class>
   <owl:Class xmlns:owl="http://www.w3.org/2002/07/owl#" rdf:ID="sublativeCase">
      <dcr:datcat rdf:resource="http://www.isocat.org/datcat/DC-1392"/>
      <rdfs:label xml:lang="en">sublative case</rdfs:label>
      <rdfs:comment xml:lang="en">Case for a move of something to the surface of another object.
  </rdfs:comment>
   </owl:Class>
   <owl:Class xmlns:owl="http://www.w3.org/2002/07/owl#" rdf:ID="subordinatingConjunction">
      <dcr:datcat rdf:resource="http://www.isocat.org/datcat/DC-1393"/>
      <rdfs:label xml:lang="en">subordinating conjunction</rdfs:label>
      <rdfs:comment xml:lang="en">Conjunction that links constructions by making one of them a
   constituent of another. The subordinating conjunction typically marks the incorporated
   constituent.</rdfs:comment>
   </owl:Class>
   <owl:Class xmlns:owl="http://www.w3.org/2002/07/owl#" rdf:ID="substitute">
      <dcr:datcat rdf:resource="http://www.isocat.org/datcat/DC-1832"/>
      <rdfs:label xml:lang="en">substitute</rdfs:label>
      <rdfs:comment xml:lang="en">Operation that replaces N characters at position X by a
   string</rdfs:comment>
   </owl:Class>
   <owl:Class xmlns:owl="http://www.w3.org/2002/07/owl#" rdf:ID="suffix">
      <dcr:datcat rdf:resource="http://www.isocat.org/datcat/DC-1395"/>
      <rdfs:label xml:lang="en">suffix</rdfs:label>
      <rdfs:comment xml:lang="en">Affix added at the end of the word to change its meaning or part of
   speech. </rdfs:comment>
   </owl:Class>
   <owl:Class xmlns:owl="http://www.w3.org/2002/07/owl#" rdf:ID="superessiveCase">
      <dcr:datcat rdf:resource="http://www.isocat.org/datcat/DC-1396"/>
      <rdfs:label xml:lang="en">superessive case</rdfs:label>
      <rdfs:comment xml:lang="en">Case indicating location on top of something or on the surface of
   something.</rdfs:comment>
   </owl:Class>
   <owl:Class xmlns:owl="http://www.w3.org/2002/07/owl#" rdf:ID="superlative">
      <dcr:datcat rdf:resource="http://www.isocat.org/datcat/DC-1422"/>
      <rdfs:label xml:lang="en">superlative</rdfs:label>
      <rdfs:comment xml:lang="en">Value used in a comparison between more than two
   entities.</rdfs:comment>
   </owl:Class>
   <owl:Class xmlns:owl="http://www.w3.org/2002/07/owl#" rdf:ID="superlativeParticle">
      <dcr:datcat rdf:resource="http://www.isocat.org/datcat/DC-1923"/>
      <rdfs:label xml:lang="en">superlative particle</rdfs:label>
      <rdfs:comment xml:lang="en">Particle expressing superlative degree. Superlative is the comparison
   between more than two entities and contrasts with comparative where only two entities are
   involved and positive where no comparison is implied.</rdfs:comment>
   </owl:Class>
   <owl:Class xmlns:owl="http://www.w3.org/2002/07/owl#" rdf:ID="suspensionPoints">
      <dcr:datcat rdf:resource="http://www.isocat.org/datcat/DC-1447"/>
      <rdfs:label xml:lang="en">suspension points</rdfs:label>
      <rdfs:comment xml:lang="en">Sequence of three dots having the same meaning as "et cetera" (full
   form) or "etc" (abbreviated form).</rdfs:comment>
   </owl:Class>
   <owl:Class xmlns:owl="http://www.w3.org/2002/07/owl#" rdf:ID="symbol">
      <dcr:datcat rdf:resource="http://www.isocat.org/datcat/DC-1398"/>
      <rdfs:label xml:lang="en">symbol</rdfs:label>
      <rdfs:comment xml:lang="en">A non-splittable sequence of letters, numbers or signs that represents
   a particular meaning.</rdfs:comment>
   </owl:Class>
   <owl:Class xmlns:owl="http://www.w3.org/2002/07/owl#" rdf:ID="syntacticType">
      <dcr:datcat rdf:resource="http://www.isocat.org/datcat/DC-1948"/>
      <rdfs:label xml:lang="en">syntactic type</rdfs:label>
      <rdfs:comment xml:lang="en">Type of part of speech.</rdfs:comment>
   </owl:Class>
   <owl:Class xmlns:owl="http://www.w3.org/2002/07/owl#" rdf:ID="tabooRegister">
      <dcr:datcat rdf:resource="http://www.isocat.org/datcat/DC-1996"/>
      <rdfs:label xml:lang="en">taboo register</rdfs:label>
      <rdfs:comment xml:lang="en">Register that expresses a situation that people avoid because it is
   extremely offensive or embarrassing.</rdfs:comment>
   </owl:Class>
   <owl:Class xmlns:owl="http://www.w3.org/2002/07/owl#" rdf:ID="technicalRegister">
      <dcr:datcat rdf:resource="http://www.isocat.org/datcat/DC-1997"/>
      <rdfs:label xml:lang="en">technical register</rdfs:label>
      <rdfs:comment xml:lang="en">The register appropriate to scientific texts or special
   languages.</rdfs:comment>
   </owl:Class>
   <owl:Class xmlns:owl="http://www.w3.org/2002/07/owl#" rdf:ID="grammaticalTense">
      <dcr:datcat rdf:resource="http://www.isocat.org/datcat/DC-1286"/>
      <rdfs:label xml:lang="en">tense</rdfs:label>
      <rdfs:comment xml:lang="en">Property referring to the way the grammar marks the time at which the
   action denoted by the verb took place.</rdfs:comment>
   </owl:Class>
   <owl:Class xmlns:owl="http://www.w3.org/2002/07/owl#" rdf:ID="terminativeCase">
      <dcr:datcat rdf:resource="http://www.isocat.org/datcat/DC-1401"/>
      <rdfs:label xml:lang="en">terminative case</rdfs:label>
      <rdfs:comment xml:lang="en">Case that indicates to what or where something ends. </rdfs:comment>
   </owl:Class>
   <owl:Class xmlns:owl="http://www.w3.org/2002/07/owl#" rdf:ID="text">
      <dcr:datcat rdf:resource="http://www.isocat.org/datcat/DC-1847"/>
      <rdfs:label xml:lang="en">text</rdfs:label>
      <rdfs:comment xml:lang="en">Series of sentences expressed in a natural language.</rdfs:comment>
   </owl:Class>
   <owl:Class xmlns:owl="http://www.w3.org/2002/07/owl#" rdf:ID="thirdPerson">
      <dcr:datcat rdf:resource="http://www.isocat.org/datcat/DC-1402"/>
      <rdfs:label xml:lang="en">third person</rdfs:label>
      <rdfs:comment xml:lang="en">Third person deixis is deictic reference to a referent(s) not
   identified as the speaker or addressee. </rdfs:comment>
   </owl:Class>
   <owl:Class xmlns:owl="http://www.w3.org/2002/07/owl#" rdf:ID="token">
      <dcr:datcat rdf:resource="http://www.isocat.org/datcat/DC-1403"/>
      <rdfs:label xml:lang="en">token</rdfs:label>
      <rdfs:comment xml:lang="en">Character string surrounded by separators.</rdfs:comment>
   </owl:Class>
   <owl:Class xmlns:owl="http://www.w3.org/2002/07/owl#" rdf:ID="transcription">
      <dcr:datcat rdf:resource="http://www.isocat.org/datcat/DC-1849"/>
      <rdfs:label xml:lang="en">transcription</rdfs:label>
      <rdfs:comment xml:lang="en">Form resulting from a coherent method of writing down speech
   sounds</rdfs:comment>
   </owl:Class>
   <owl:Class xmlns:owl="http://www.w3.org/2002/07/owl#" rdf:ID="transformType">
      <dcr:datcat rdf:resource="http://www.isocat.org/datcat/DC-2181"/>
      <rdfs:label xml:lang="en">transform type</rdfs:label>
      <rdfs:comment xml:lang="en">Type of transformation</rdfs:comment>
   </owl:Class>
   <owl:Class xmlns:owl="http://www.w3.org/2002/07/owl#" rdf:ID="translativeCase">
      <dcr:datcat rdf:resource="http://www.isocat.org/datcat/DC-1406"/>
      <rdfs:label xml:lang="en">translative case</rdfs:label>
      <rdfs:comment xml:lang="en">Case indicating that the referent of the noun, or the quality of the
   adjective, that it marks is the result of a process of change. </rdfs:comment>
   </owl:Class>
   <owl:Class xmlns:owl="http://www.w3.org/2002/07/owl#" rdf:ID="transliteration">
      <dcr:datcat rdf:resource="http://www.isocat.org/datcat/DC-1848"/>
      <rdfs:label xml:lang="en">transliteration</rdfs:label>
      <rdfs:comment xml:lang="en">Form resulting from the conversion of one writing system into
   another</rdfs:comment>
   </owl:Class>
   <owl:Class xmlns:owl="http://www.w3.org/2002/07/owl#" rdf:ID="trial">
      <dcr:datcat rdf:resource="http://www.isocat.org/datcat/DC-1407"/>
      <rdfs:label xml:lang="en">trial</rdfs:label>
      <rdfs:comment xml:lang="en">Grammatical number referring to 'three things', as opposed to
   'singular' and 'plural'. </rdfs:comment>
   </owl:Class>
   <owl:Class xmlns:owl="http://www.w3.org/2002/07/owl#" rdf:ID="type">
      <dcr:datcat rdf:resource="http://www.isocat.org/datcat/DC-1971"/>
      <rdfs:label xml:lang="en">type</rdfs:label>
      <rdfs:comment xml:lang="en">One member of a group of people or things that have similar features
   or qualities.</rdfs:comment>
   </owl:Class>
   <owl:Class xmlns:owl="http://www.w3.org/2002/07/owl#" rdf:ID="unaccomplished">
      <dcr:datcat rdf:resource="http://www.isocat.org/datcat/DC-2217"/>
      <rdfs:label xml:lang="en">unaccomplished</rdfs:label>
      <rdfs:comment xml:lang="en">aspect that expresses an event or state that is not
   finished.</rdfs:comment>
   </owl:Class>
   <owl:Class xmlns:owl="http://www.w3.org/2002/07/owl#" rdf:ID="unclassifiedParticle">
      <dcr:datcat rdf:resource="http://www.isocat.org/datcat/DC-1897"/>
      <rdfs:label xml:lang="en">unclassified particle</rdfs:label>
      <rdfs:comment xml:lang="en">Particle that is not covered by other sorts of particle
   definitions.</rdfs:comment>
   </owl:Class>
   <owl:Class xmlns:owl="http://www.w3.org/2002/07/owl#" rdf:ID="unclassifiedPunctuation">
      <dcr:datcat rdf:resource="http://www.isocat.org/datcat/DC-2080"/>
      <rdfs:label xml:lang="en">unclassified punctuation</rdfs:label>
      <rdfs:comment xml:lang="en">Punctuation that cannot fit in the other sorts of
   punctuations.</rdfs:comment>
   </owl:Class>
   <owl:Class xmlns:owl="http://www.w3.org/2002/07/owl#" rdf:ID="unclassifiedResidual">
      <dcr:datcat rdf:resource="http://www.isocat.org/datcat/DC-1891"/>
      <rdfs:label xml:lang="en">unclassified residual</rdfs:label>
      <rdfs:comment xml:lang="en">Part of speech not covered by all other definitions.</rdfs:comment>
   </owl:Class>
   <owl:Class xmlns:owl="http://www.w3.org/2002/07/owl#" rdf:ID="unspecified">
      <dcr:datcat rdf:resource="http://www.isocat.org/datcat/DC-1908"/>
      <rdfs:label xml:lang="en">unspecified</rdfs:label>
      <rdfs:comment xml:lang="en">Value that expresses the absence of specification.</rdfs:comment>
   </owl:Class>
   <owl:Class xmlns:owl="http://www.w3.org/2002/07/owl#" rdf:ID="utterance">
      <dcr:datcat rdf:resource="http://www.isocat.org/datcat/DC-1409"/>
      <rdfs:label xml:lang="en">utterance</rdfs:label>
      <rdfs:comment xml:lang="en">Complete unit of talk, bounded by the speaker's silence.
  </rdfs:comment>
   </owl:Class>
   <owl:Class xmlns:owl="http://www.w3.org/2002/07/owl#" rdf:ID="value">
      <dcr:datcat rdf:resource="http://www.isocat.org/datcat/DC-1978"/>
      <rdfs:label xml:lang="en">value</rdfs:label>
      <rdfs:comment xml:lang="en">Generic name for a value.</rdfs:comment>
   </owl:Class>
   <owl:Class xmlns:owl="http://www.w3.org/2002/07/owl#" rdf:ID="variation">
      <dcr:datcat rdf:resource="http://www.isocat.org/datcat/DC-2177"/>
      <rdfs:label xml:lang="en">variation</rdfs:label>
      <rdfs:comment xml:lang="en">Difference between similar objects</rdfs:comment>
   </owl:Class>
   <owl:Class xmlns:owl="http://www.w3.org/2002/07/owl#" rdf:ID="verb">
      <dcr:datcat rdf:resource="http://www.isocat.org/datcat/DC-1424"/>
      <rdfs:label xml:lang="en">verb</rdfs:label>
      <rdfs:comment xml:lang="en">Element which, singly or in combination with other verbs is used as
   the minimal predicate of a sentence, co-occurring with a subject. If the predicate contains other
   elements (e.g. object, complement), then it is the verb which more than any other is the unit
   which influences the choice and extent of these elements.</rdfs:comment>
   </owl:Class>
   <owl:Class xmlns:owl="http://www.w3.org/2002/07/owl#" rdf:ID="verbFormMood">
      <dcr:datcat rdf:resource="http://www.isocat.org/datcat/DC-1427"/>
      <rdfs:label xml:lang="en">verb form mood</rdfs:label>
      <rdfs:comment xml:lang="en">One of a set of distinctive forms that are used to signal modality.
   Modality is a facet of illocutionary point or general intent of a speaker, or a speaker's degree
   of commitment to the expressed proposition's believability, obligatoriness, desirability or
   reality.</rdfs:comment>
   </owl:Class>
   <owl:Class xmlns:owl="http://www.w3.org/2002/07/owl#" rdf:ID="view">
      <dcr:datcat rdf:resource="http://www.isocat.org/datcat/DC-1970"/>
      <rdfs:label xml:lang="en">view</rdfs:label>
      <rdfs:comment xml:lang="en">Way of thinking about or understanding something.</rdfs:comment>
   </owl:Class>
   <owl:Class xmlns:owl="http://www.w3.org/2002/07/owl#" rdf:ID="vocativeCase">
      <dcr:datcat rdf:resource="http://www.isocat.org/datcat/DC-1412"/>
      <rdfs:label xml:lang="en">vocative case</rdfs:label>
      <rdfs:comment xml:lang="en">Case used to indicate direct address.</rdfs:comment>
   </owl:Class>
   <owl:Class xmlns:owl="http://www.w3.org/2002/07/owl#" rdf:ID="voice">
      <dcr:datcat rdf:resource="http://www.isocat.org/datcat/DC-1413"/>
      <rdfs:label xml:lang="en">voice</rdfs:label>
      <rdfs:comment xml:lang="en">Way sentences may alter the relationship between the subject and
   object of a verb, without changing the meaning of the sentence.</rdfs:comment>
   </owl:Class>
   <owl:Class xmlns:owl="http://www.w3.org/2002/07/owl#" rdf:ID="voiceNoun">
      <dcr:datcat rdf:resource="http://www.isocat.org/datcat/DC-2253"/>
      <rdfs:label xml:lang="en">voice noun</rdfs:label>
      <rdfs:comment xml:lang="en">noun of a voice</rdfs:comment>
   </owl:Class>
   <owl:Class xmlns:owl="http://www.w3.org/2002/07/owl#" rdf:ID="vulgarRegister">
      <dcr:datcat rdf:resource="http://www.isocat.org/datcat/DC-1998"/>
      <rdfs:label xml:lang="en">vulgar register</rdfs:label>
      <rdfs:comment xml:lang="en">Register of a term or text type that can be characterized as profane
   or socially unacceptable.</rdfs:comment>
   </owl:Class>
   <owl:Class xmlns:owl="http://www.w3.org/2002/07/owl#" rdf:ID="weakPersonalPronoun">
      <dcr:datcat rdf:resource="http://www.isocat.org/datcat/DC-1414"/>
      <rdfs:label xml:lang="en">weak personal pronoun</rdfs:label>
      <rdfs:comment xml:lang="en">Personal pronoun that cannot occupy the position after a preposition
   and/or reinforce a strong personal pronoun.</rdfs:comment>
   </owl:Class>
   <owl:Class xmlns:owl="http://www.w3.org/2002/07/owl#" rdf:ID="word">
      <dcr:datcat rdf:resource="http://www.isocat.org/datcat/DC-1415"/>
      <rdfs:label xml:lang="en">word</rdfs:label>
      <rdfs:comment xml:lang="en">Linguistic unit composed of at least a part of speech and a
   lemma.</rdfs:comment>
   </owl:Class>
   <owl:Class xmlns:owl="http://www.w3.org/2002/07/owl#" rdf:ID="writtenForm">
      <dcr:datcat rdf:resource="http://www.isocat.org/datcat/DC-1836"/>
      <rdfs:label xml:lang="en">written form</rdfs:label>
      <rdfs:comment xml:lang="en">Representation of the written string of a form</rdfs:comment>
   </owl:Class>
   <owl:Class xmlns:owl="http://www.w3.org/2002/07/owl#" rdf:ID="yes">
      <dcr:datcat rdf:resource="http://www.isocat.org/datcat/DC-1904"/>
      <rdfs:label xml:lang="en">yes</rdfs:label>
      <rdfs:comment xml:lang="en">Positive value</rdfs:comment>
   </owl:Class>
   <owl:Class xmlns:owl="http://www.w3.org/2002/07/owl#" rdf:ID="zuInclusion">
      <dcr:datcat rdf:resource="http://www.isocat.org/datcat/DC-1954"/>
      <rdfs:label xml:lang="en">zu inclusion</rdfs:label>
      <rdfs:comment xml:lang="en">Inclusion of zu.</rdfs:comment>
   </owl:Class>
</rdf:RDF>