<?xml version="1.0"?>


<!DOCTYPE rdf:RDF [
    <!ENTITY system2 "system:" >
    <!ENTITY olia "http://purl.org/olia/" >
    <!ENTITY owl "http://www.w3.org/2002/07/owl#" >
    <!ENTITY system "http://purl.org/olia/system.owl#" >
    <!ENTITY dc "http://purl.org/dc/elements/1.1/" >
    <!ENTITY bambara "http://purl.org/olia/bambara.owl#" >
    <!ENTITY xsd "http://www.w3.org/2001/XMLSchema#" >
    <!ENTITY bambara2 "http://purl.org/olia/bambara.owl#1" >
    <!ENTITY bambara3 "http://purl.org/olia/bambara.owl#2" >
    <!ENTITY bambara4 "http://purl.org/olia/bambara.owl#3" >
    <!ENTITY owl2xml "http://www.w3.org/2006/12/owl2-xml#" >
    <!ENTITY rdfs "http://www.w3.org/2000/01/rdf-schema#" >
    <!ENTITY rdf "http://www.w3.org/1999/02/22-rdf-syntax-ns#" >
]>


<rdf:RDF xmlns="http://purl.org/olia/bambara.owl#"
     xml:base="http://purl.org/olia/bambara.owl"
     xmlns:owl2xml="http://www.w3.org/2006/12/owl2-xml#"
     xmlns:xsd="http://www.w3.org/2001/XMLSchema#"
     xmlns:system2="system:"
     xmlns:rdfs="http://www.w3.org/2000/01/rdf-schema#"
     xmlns:bambara4="http://purl.org/olia/bambara.owl#3"
     xmlns:bambara="http://purl.org/olia/bambara.owl#"
     xmlns:owl="http://www.w3.org/2002/07/owl#"
     xmlns:olia="http://purl.org/olia/"
     xmlns:bambara3="http://purl.org/olia/bambara.owl#2"
     xmlns:dc="http://purl.org/dc/elements/1.1/"
     xmlns:system="http://purl.org/olia/system.owl#"
     xmlns:bambara2="http://purl.org/olia/bambara.owl#1"
     xmlns:rdf="http://www.w3.org/1999/02/22-rdf-syntax-ns#">
    <owl:Ontology rdf:about="">
        <rdfs:seeAlso rdf:datatype="&xsd;anyURI"
            >http://cormand.huma-num.fr/gloses.html</rdfs:seeAlso>
        <owl:versionInfo xml:lang="en"
            >2016-04-03 created (CC)
2016-07-04 updated with input from Valentin Vydrine

Christian Chiarcos (CC)</owl:versionInfo>
        <dc:creator xml:lang="en"
            >Christian Chiarcos, Goethe Universit&#228;t Frankfurt am Main, Germany, christian.chiarcos@web.de</dc:creator>
        <rdfs:comment xml:lang="en"
            >OLiA Annotation Model for the Bambara Reference Corpus / Corpus Bambara de Reference

Bambara / Bamanankan (bam) is a West African language of the Mande group, primarily spoken in Mali.
The Bambara Reference Corpus is accessible from  http://cormand.huma-num.fr.

Note that there are several tags expressing uncertainty, or indistinguishability of two parts of speech, resp. a high likelihood of conversion, written with &quot;/&quot;. In these cases, they are treated as conjunction here, because either interpretation would be feasible.

Also note that derivation is currently not supported in OLiA. Selectional restrictions for morphosyntactic features are thus not formalized.

Unless marked otherwise, this ontology and all quotes herein follows http://cormand.huma-num.fr/gloses.html and explicit feedback by BRC developers (Valentin Vydrine, Damien Nouvel). Comments are made by ontology editor(s).

Christian Chiarcos (christian.chiarcos@web.de), 2016-04-03</rdfs:comment>
        <owl:imports rdf:resource="http://purl.org/olia/system.owl"/>
    </owl:Ontology>
    


    <!-- 
    ///////////////////////////////////////////////////////////////////////////////////////
    //
    // Annotation properties
    //
    ///////////////////////////////////////////////////////////////////////////////////////
     -->

    <owl:AnnotationProperty rdf:about="&dc;creator"/>
    <owl:AnnotationProperty rdf:about="system:hasTag"/>
    


    <!-- 
    ///////////////////////////////////////////////////////////////////////////////////////
    //
    // Object Properties
    //
    ///////////////////////////////////////////////////////////////////////////////////////
     -->

    


    <!-- http://purl.org/olia/bambara.owl#derivation -->

    <owl:ObjectProperty rdf:about="#derivation">
        <rdfs:range rdf:resource="#Derivation"/>
        <rdfs:domain rdf:resource="#Glose"/>
        <rdfs:subPropertyOf rdf:resource="http://purl.org/olia/system.owl#hasFeature"/>
    </owl:ObjectProperty>
    


    <!-- http://purl.org/olia/bambara.owl#flexion -->

    <owl:ObjectProperty rdf:about="#flexion">
        <rdfs:range rdf:resource="#Flexion"/>
        <rdfs:domain rdf:resource="#Glose"/>
        <rdfs:subPropertyOf rdf:resource="http://purl.org/olia/system.owl#hasFeature"/>
    </owl:ObjectProperty>
    


    <!-- http://purl.org/olia/system.owl#hasFeature -->

    <owl:ObjectProperty rdf:about="http://purl.org/olia/system.owl#hasFeature"/>
    


    <!-- 
    ///////////////////////////////////////////////////////////////////////////////////////
    //
    // Data properties
    //
    ///////////////////////////////////////////////////////////////////////////////////////
     -->

    


    <!-- http://purl.org/olia/system.owl#hasTag -->

    <owl:DatatypeProperty rdf:about="http://purl.org/olia/system.owl#hasTag"/>
    


    <!-- http://purl.org/olia/system.owl#hasTagContaining -->

    <owl:DatatypeProperty rdf:about="http://purl.org/olia/system.owl#hasTagContaining"/>
    


    <!-- http://purl.org/olia/system.owl#hasTagEndingWith -->

    <owl:DatatypeProperty rdf:about="http://purl.org/olia/system.owl#hasTagEndingWith"/>
    


    <!-- http://purl.org/olia/system.owl#hasTagMatching -->

    <owl:DatatypeProperty rdf:about="http://purl.org/olia/system.owl#hasTagMatching"/>
    


    <!-- 
    ///////////////////////////////////////////////////////////////////////////////////////
    //
    // Classes
    //
    ///////////////////////////////////////////////////////////////////////////////////////
     -->

    


    <!-- http://purl.org/olia/bambara.owl#Adjectif -->

    <owl:Class rdf:about="#Adjectif">
        <rdfs:subClassOf rdf:resource="#POS"/>
    </owl:Class>
    


    <!-- http://purl.org/olia/bambara.owl#Adverbe -->

    <owl:Class rdf:about="#Adverbe">
        <rdfs:subClassOf rdf:resource="#POS"/>
        <rdfs:comment xml:lang="en"
            >Note that Auxiliaire is not to be confused with auxiliary (verb). This category refers to closed-class expressions with primarily grammatical function. (V. Vydrine)</rdfs:comment>
    </owl:Class>
    


    <!-- http://purl.org/olia/bambara.owl#AutreAbreviation -->

    <owl:Class rdf:about="#AutreAbreviation">
        <rdfs:subClassOf rdf:resource="#Glose"/>
        <owl:versionInfo xml:lang="en"
            >The individuals assembled here have also been tentatively assigned to other parts of speech (as interpreted by the ontology editor)</owl:versionInfo>
        <rdfs:comment xml:lang="fr"
            >Autres abr&#233;viations utilis&#233;es dans les gloses</rdfs:comment>
    </owl:Class>
    


    <!-- http://purl.org/olia/bambara.owl#Auxiliaire -->

    <owl:Class rdf:about="#Auxiliaire">
        <rdfs:subClassOf rdf:resource="#POS"/>
        <owl:versionInfo xml:lang="en"
            >Created for the glosage des auxiliaires, contains
conj 
cop 
dtm 
pers 
pm
pron 
prt</owl:versionInfo>
    </owl:Class>
    


    <!-- http://purl.org/olia/bambara.owl#Conjonction -->

    <owl:Class rdf:about="#Conjonction">
        <rdfs:subClassOf rdf:resource="#Auxiliaire"/>
    </owl:Class>
    


    <!-- http://purl.org/olia/bambara.owl#Copule -->

    <owl:Class rdf:about="#Copule">
        <rdfs:subClassOf rdf:resource="#Auxiliaire"/>
        <rdfs:comment xml:lang="en"
            >Note that the Bambara copula is not a verbal element. Even though it syntactically resembles a verb, it is morphologically different and non-verbal in origin. (V. Vydrine)</rdfs:comment>
    </owl:Class>
    


    <!-- http://purl.org/olia/bambara.owl#Derivation -->

    <owl:Class rdf:about="#Derivation">
        <rdfs:subClassOf rdf:resource="http://purl.org/olia/system.owl#Feature"/>
        <rdfs:subClassOf>
            <owl:Restriction>
                <owl:onProperty rdf:resource="#derivation"/>
                <owl:hasSelf rdf:datatype="&xsd;boolean">true</owl:hasSelf>
            </owl:Restriction>
        </rdfs:subClassOf>
    </owl:Class>
    


    <!-- http://purl.org/olia/bambara.owl#Determinatif -->

    <owl:Class rdf:about="#Determinatif">
        <rdfs:subClassOf rdf:resource="#PronomDeterminatif"/>
    </owl:Class>
    


    <!-- http://purl.org/olia/bambara.owl#Flexion -->

    <owl:Class rdf:about="#Flexion">
        <rdfs:subClassOf rdf:resource="http://purl.org/olia/system.owl#Feature"/>
        <rdfs:subClassOf>
            <owl:Restriction>
                <owl:onProperty rdf:resource="#flexion"/>
                <owl:hasSelf rdf:datatype="&xsd;boolean">true</owl:hasSelf>
            </owl:Restriction>
        </rdfs:subClassOf>
    </owl:Class>
    


    <!-- http://purl.org/olia/bambara.owl#Glose -->

    <owl:Class rdf:about="#Glose">
        <rdfs:subClassOf rdf:resource="http://purl.org/olia/system.owl#UnitOfAnnotation"/>
    </owl:Class>
    


    <!-- http://purl.org/olia/bambara.owl#Interjection -->

    <owl:Class rdf:about="#Interjection">
        <rdfs:subClassOf rdf:resource="#POS"/>
    </owl:Class>
    


    <!-- http://purl.org/olia/bambara.owl#MarquePredicative -->

    <owl:Class rdf:about="#MarquePredicative">
        <rdfs:subClassOf rdf:resource="#Auxiliaire"/>
        <rdfs:comment xml:lang="en"
            >Predicative markers represent the syntactic center of the sentence. They resemble, but are different from both verbs and copulas and they must not be confused with particles which serve a peripheral function in sentences, only. (V. Vydrine)</rdfs:comment>
    </owl:Class>
    


    <!-- http://purl.org/olia/bambara.owl#MotEtranger -->

    <owl:Class rdf:about="#MotEtranger">
        <rdfs:subClassOf rdf:resource="#AutreAbreviation"/>
        <owl:versionInfo xml:lang="en"
            >created as a cover term for ETRG...</owl:versionInfo>
    </owl:Class>
    


    <!-- http://purl.org/olia/bambara.owl#Nom -->

    <owl:Class rdf:about="#Nom">
        <rdfs:subClassOf rdf:resource="#POS"/>
    </owl:Class>
    


    <!-- http://purl.org/olia/bambara.owl#NomPropre -->

    <owl:Class rdf:about="#NomPropre">
        <rdfs:subClassOf rdf:resource="#AutreAbreviation"/>
        <rdfs:subClassOf rdf:resource="#Nom"/>
        <owl:versionInfo xml:lang="en"
            >created as a cover term for NOM.F, NOM.M, etc.</owl:versionInfo>
    </owl:Class>
    


    <!-- http://purl.org/olia/bambara.owl#Num&#233;ratif -->

    <owl:Class rdf:about="#Num&#233;ratif">
        <rdfs:subClassOf rdf:resource="#POS"/>
        <rdfs:comment xml:lang="en"
            >Num&#233;ratif refers to cardinal numbers, ordinal numbers are adjectives, non-numeric quantifiers are determiners. (V. Vydrine)</rdfs:comment>
    </owl:Class>
    


    <!-- http://purl.org/olia/bambara.owl#Onomatopee -->

    <owl:Class rdf:about="#Onomatopee">
        <rdfs:subClassOf rdf:resource="#POS"/>
        <rdfs:comment xml:lang="en"
            >Onomatop&#233;e refers to the onomatopoetic mimicking of natural sounds, e.g., as made by an animal, when these are not lexicalized as another constituent, e.g., a noun. In this sense, Onomatop&#233;e is related to interjection. (V. Vydrine)</rdfs:comment>
    </owl:Class>
    


    <!-- http://purl.org/olia/bambara.owl#POS -->

    <owl:Class rdf:about="#POS">
        <rdfs:subClassOf rdf:resource="#Glose"/>
        <rdfs:comment rdf:datatype="&xsd;anyURI"
            >Marques des parties de discours dans le Corpus bambara de r&#233;f&#233;rence</rdfs:comment>
        <rdfs:comment rdf:datatype="&rdf;XMLLiteral"
            >Note that not all POS categories found in the corpus are listed here, only those found under http://cormand.huma-num.fr/marques.html.
&quot;Unknown&quot; pos tags are listed below:
c, adv/n (= n/adv?), n.prop, conj/prep (= prep/conj?), mrph, _ (= unclear?), prn/dtm, n/v, v/n. 
Additional rare tags not covered by the documentation include 
conv.n, n.prop/dtm/prn/n/ptcp/adj (2x), n/intj (2x), vt (2x)</rdfs:comment>
        <rdfs:seeAlso rdf:datatype="&xsd;anyURI"
            >http://cormand.huma-num.fr/marques.html</rdfs:seeAlso>
    </owl:Class>
    


    <!-- http://purl.org/olia/bambara.owl#Participe -->

    <owl:Class rdf:about="#Participe">
        <rdfs:subClassOf rdf:resource="#POS"/>
        <rdfs:comment xml:lang="en"
            >As in Europen languages, Bambara participles are multi-functional, they have morphological characteristics of verbs, but often syntactic characteristics of Adjectives. (V. Vydrine)</rdfs:comment>
    </owl:Class>
    


    <!-- http://purl.org/olia/bambara.owl#Particule -->

    <owl:Class rdf:about="#Particule">
        <rdfs:subClassOf rdf:resource="#Auxiliaire"/>
        <rdfs:comment xml:lang="en"
            >Bambara particles convey modal/episthemic senses. In the BRC tagset, particle only refers to elements at the syntactic periphery of sentences. In this regard, they differ fundamentally from perdicative markers (V. Vydrine)</rdfs:comment>
        <owl:versionInfo xml:lang="en"
            >TODO: Valentin mentioned a possible relation with determiners. To be confirmed.</owl:versionInfo>
    </owl:Class>
    


    <!-- http://purl.org/olia/bambara.owl#Ponctuation -->

    <owl:Class rdf:about="#Ponctuation">
        <rdfs:subClassOf rdf:resource="#AutreAbreviation"/>
        <rdfs:comment xml:lang="en"
            >added for punctuation signs (CC), not part of the original glosses, but treated differently</rdfs:comment>
    </owl:Class>
    


    <!-- http://purl.org/olia/bambara.owl#Postposition -->

    <owl:Class rdf:about="#Postposition">
        <rdfs:subClassOf rdf:resource="#POS"/>
    </owl:Class>
    


    <!-- http://purl.org/olia/bambara.owl#PronomDeterminatif -->

    <owl:Class rdf:about="#PronomDeterminatif">
        <rdfs:subClassOf rdf:resource="#Auxiliaire"/>
        <owl:versionInfo xml:lang="en"
            >created for tags (glosses) classified as &quot;dtm, pron&quot;, as no holistic term is available, we also followed EAGLES to include PronounPersonnel</owl:versionInfo>
    </owl:Class>
    


    <!-- http://purl.org/olia/bambara.owl#PronomNonPersonnel -->

    <owl:Class rdf:about="#PronomNonPersonnel">
        <rdfs:subClassOf rdf:resource="#PronomDeterminatif"/>
    </owl:Class>
    


    <!-- http://purl.org/olia/bambara.owl#PronomPersonnel -->

    <owl:Class rdf:about="#PronomPersonnel">
        <rdfs:subClassOf rdf:resource="#PronomDeterminatif"/>
    </owl:Class>
    


    <!-- http://purl.org/olia/bambara.owl#Pr&#233;position -->

    <owl:Class rdf:about="#Pr&#233;position">
        <rdfs:subClassOf rdf:resource="#POS"/>
    </owl:Class>
    


    <!-- http://purl.org/olia/bambara.owl#Verbe -->

    <owl:Class rdf:about="#Verbe">
        <rdfs:subClassOf rdf:resource="#POS"/>
    </owl:Class>
    


    <!-- http://purl.org/olia/bambara.owl#VerbeDynamique -->

    <owl:Class rdf:about="#VerbeDynamique">
        <rdfs:subClassOf rdf:resource="#Verbe"/>
    </owl:Class>
    


    <!-- http://purl.org/olia/bambara.owl#VerbeQualitatif -->

    <owl:Class rdf:about="#VerbeQualitatif">
        <rdfs:subClassOf rdf:resource="#Verbe"/>
    </owl:Class>
    


    <!-- http://purl.org/olia/bambara.owl#derive.adj -->

    <owl:Class rdf:about="#derive.adj">
        <rdfs:subClassOf rdf:resource="#Derivation"/>
    </owl:Class>
    


    <!-- http://purl.org/olia/bambara.owl#derive.n -->

    <owl:Class rdf:about="#derive.n">
        <rdfs:subClassOf rdf:resource="#Derivation"/>
    </owl:Class>
    


    <!-- http://purl.org/olia/bambara.owl#derive.ptcp -->

    <owl:Class rdf:about="#derive.ptcp">
        <rdfs:subClassOf rdf:resource="#Derivation"/>
    </owl:Class>
    


    <!-- http://purl.org/olia/bambara.owl#derive.v -->

    <owl:Class rdf:about="#derive.v">
        <rdfs:subClassOf rdf:resource="#Derivation"/>
    </owl:Class>
    


    <!-- http://purl.org/olia/bambara.owl#initial.adj -->

    <owl:Class rdf:about="#initial.adj">
        <rdfs:subClassOf rdf:resource="#Derivation"/>
    </owl:Class>
    


    <!-- http://purl.org/olia/bambara.owl#initial.n -->

    <owl:Class rdf:about="#initial.n">
        <rdfs:subClassOf rdf:resource="#Derivation"/>
    </owl:Class>
    


    <!-- http://purl.org/olia/bambara.owl#initial.num -->

    <owl:Class rdf:about="#initial.num">
        <rdfs:subClassOf rdf:resource="#Derivation"/>
    </owl:Class>
    


    <!-- http://purl.org/olia/bambara.owl#initial.pp -->

    <owl:Class rdf:about="#initial.pp">
        <rdfs:subClassOf rdf:resource="#Derivation"/>
    </owl:Class>
    


    <!-- http://purl.org/olia/bambara.owl#initial.ptcp -->

    <owl:Class rdf:about="#initial.ptcp">
        <rdfs:subClassOf rdf:resource="#Derivation"/>
    </owl:Class>
    


    <!-- http://purl.org/olia/bambara.owl#initial.v -->

    <owl:Class rdf:about="#initial.v">
        <rdfs:subClassOf rdf:resource="#Derivation"/>
    </owl:Class>
    


    <!-- http://purl.org/olia/bambara.owl#initial.vp -->

    <owl:Class rdf:about="#initial.vp">
        <rdfs:subClassOf rdf:resource="#Derivation"/>
    </owl:Class>
    


    <!-- http://purl.org/olia/bambara.owl#initial.vq -->

    <owl:Class rdf:about="#initial.vq">
        <rdfs:subClassOf rdf:resource="#Derivation"/>
    </owl:Class>
    


    <!-- http://purl.org/olia/system.owl#Feature -->

    <owl:Class rdf:about="http://purl.org/olia/system.owl#Feature">
        <owl:versionInfo xml:lang="en"
            >both Feature subclasses have reflexitivy axioms. This is to facilitate relational querying, cf. Chiarcos (2016, Linked Data in Linguistics)</owl:versionInfo>
    </owl:Class>
    


    <!-- http://purl.org/olia/system.owl#UnitOfAnnotation -->

    <owl:Class rdf:about="http://purl.org/olia/system.owl#UnitOfAnnotation"/>
    


    <!-- http://www.w3.org/2002/07/owl#Thing -->

    <owl:Class rdf:about="&owl;Thing"/>
    


    <!-- 
    ///////////////////////////////////////////////////////////////////////////////////////
    //
    // Individuals
    //
    ///////////////////////////////////////////////////////////////////////////////////////
     -->

    


    <!-- http://purl.org/olia/bambara.owl#1PL -->

    <PronomPersonnel rdf:about="#1PL">
        <rdf:type rdf:resource="&owl;Thing"/>
        <system:hasTag>1PL</system:hasTag>
        <rdfs:comment xml:lang="fr"
            >&#225;n;
            pronom personnel non-emphatique 1&#232;re pers. pl.</rdfs:comment>
    </PronomPersonnel>
    


    <!-- http://purl.org/olia/bambara.owl#1PL.EMPH -->

    <PronomPersonnel rdf:about="#1PL.EMPH">
        <rdf:type rdf:resource="&owl;Thing"/>
        <system:hasTag>1PL.EMPH</system:hasTag>
        <rdfs:comment xml:lang="fr"
            >&#225;nw;
            pronom personnel emphatique 1&#232;re pers. pl.</rdfs:comment>
    </PronomPersonnel>
    


    <!-- http://purl.org/olia/bambara.owl#2PL -->

    <owl:Thing rdf:about="#2PL">
        <rdf:type rdf:resource="#PronomPersonnel"/>
        <system:hasTag>2PL</system:hasTag>
        <rdfs:comment xml:lang="fr"
            >&#225;;
            pronom personnel non-emphatique 2&#232;me pers. pl.</rdfs:comment>
    </owl:Thing>
    


    <!-- http://purl.org/olia/bambara.owl#2PL.EMPH -->

    <owl:Thing rdf:about="#2PL.EMPH">
        <rdf:type rdf:resource="#PronomPersonnel"/>
        <system:hasTag>2PL.EMPH</system:hasTag>
        <rdfs:comment xml:lang="fr"
            >&#225;w;
            pronom personnel emphatique 2&#232;me pers. pl.</rdfs:comment>
    </owl:Thing>
    


    <!-- http://purl.org/olia/bambara.owl#2SG.EMPH -->

    <owl:Thing rdf:about="#2SG.EMPH">
        <rdf:type rdf:resource="#PronomPersonnel"/>
        <system:hasTag>2SG.EMPH</system:hasTag>
        <rdfs:comment xml:lang="fr"
            >&#233;;
            pronom personnel emphatique 2&#232;me pers. sg.</rdfs:comment>
    </owl:Thing>
    


    <!-- http://purl.org/olia/bambara.owl#3SG -->

    <PronomPersonnel rdf:about="#3SG">
        <rdf:type rdf:resource="&owl;Thing"/>
        <system:hasTag>3SG</system:hasTag>
        <rdfs:comment xml:lang="fr"
            >&#224; pronom personnel non-emphatique 3&#232;me pers. sg.</rdfs:comment>
        <rdfs:comment xml:lang="fr"
            >&#237;;
            pronom personnel non-emphatique 2&#232;me pers. sg.</rdfs:comment>
    </PronomPersonnel>
    


    <!-- http://purl.org/olia/bambara.owl#ABSTR -->

    <Derivation rdf:about="#ABSTR">
        <rdf:type rdf:resource="#derive.n"/>
        <rdf:type rdf:resource="#initial.adj"/>
        <rdf:type rdf:resource="#initial.n"/>
        <rdf:type rdf:resource="&owl;Thing"/>
        <system:hasTagContaining>ABSTR</system:hasTagContaining>
        <rdfs:comment xml:lang="fr"
            >-ya;
            n, adj, (v);
            n, (v);
            nom de statut ou d&#8217;&#233;tat (d&#233;riv&#233; des noms de personnes ou de certains animaux), du nom de qualit&#233; (d&#233;riv&#233; des adjectifs) ; rarement, des verbes &#224; valeurs inchoatives</rdfs:comment>
    </Derivation>
    


    <!-- http://purl.org/olia/bambara.owl#ADJ -->

    <Derivation rdf:about="#ADJ">
        <rdf:type rdf:resource="#derive.adj"/>
        <rdf:type rdf:resource="#initial.vq"/>
        <rdf:type rdf:resource="&owl;Thing"/>
        <system:hasTagContaining>ADJ</system:hasTagContaining>
        <rdfs:comment xml:lang="fr"
            >-man;
            vq;
            adj;
            adjectiviseur des verbes qualitatifs</rdfs:comment>
    </Derivation>
    


    <!-- http://purl.org/olia/bambara.owl#AG.EX -->

    <initial.v rdf:about="#AG.EX">
        <rdf:type rdf:resource="#Derivation"/>
        <rdf:type rdf:resource="#derive.n"/>
        <rdf:type rdf:resource="#initial.adj"/>
        <rdf:type rdf:resource="#initial.n"/>
        <rdf:type rdf:resource="&owl;Thing"/>
        <rdfs:comment xml:lang="fr"
            >-nci; 
            n, adj, v;
            n;
            nom d&#8217;agent excessif</rdfs:comment>
        <system:hasTagContaining>AG.EX</system:hasTagContaining>
    </initial.v>
    


    <!-- http://purl.org/olia/bambara.owl#AG.OCC -->

    <owl:Thing rdf:about="#AG.OCC">
        <rdf:type rdf:resource="#Derivation"/>
        <rdf:type rdf:resource="#derive.n"/>
        <rdf:type rdf:resource="#initial.v"/>
        <system:hasTagContaining>AG.OCC</system:hasTagContaining>
        <rdfs:comment xml:lang="fr"
            >-baa / -baga;
            v;
            n, (adj);
            nom d&#8217;agent occasionnel</rdfs:comment>
    </owl:Thing>
    


    <!-- http://purl.org/olia/bambara.owl#AG.PRM -->

    <initial.v rdf:about="#AG.PRM">
        <rdf:type rdf:resource="#Derivation"/>
        <rdf:type rdf:resource="#derive.n"/>
        <rdf:type rdf:resource="&owl;Thing"/>
        <system:hasTagContaining>AG.PRM</system:hasTagContaining>
        <rdfs:comment xml:lang="fr"
            >-la / -na; 
            v;
            n;
            nom d&#8217;agent</rdfs:comment>
    </initial.v>
    


    <!-- http://purl.org/olia/bambara.owl#ART -->

    <Flexion rdf:about="#ART">
        <rdf:type rdf:resource="&owl;Thing"/>
        <rdfs:comment xml:lang="fr"
            >-;
            n, adj;
            article sp&#233;cifique;
            ton bas flottant suivant le mot</rdfs:comment>
        <system:hasTagEndingWith>ART</system:hasTagEndingWith>
    </Flexion>
    


    <!-- http://purl.org/olia/bambara.owl#AUGM -->

    <owl:Thing rdf:about="#AUGM">
        <rdf:type rdf:resource="#Derivation"/>
        <rdf:type rdf:resource="#initial.adj"/>
        <rdf:type rdf:resource="#initial.n"/>
        <rdf:type rdf:resource="#initial.ptcp"/>
        <system:hasTagContaining>AUGM</system:hasTagContaining>
        <rdfs:comment xml:lang="fr"
            >-ba; 
            n, adj, ptcp;
            ne change pas;
            augmentatif</rdfs:comment>
    </owl:Thing>
    


    <!-- http://purl.org/olia/bambara.owl#BE -->

    <owl:Thing rdf:about="#BE">
        <rdf:type rdf:resource="#Copule"/>
        <system:hasTag>BE</system:hasTag>
        <rdfs:comment xml:lang="fr"
            >b&#603;&#769;;
            copule d&#8217;un &#233;nonc&#233; non-verbal locatif affirmatif</rdfs:comment>
    </owl:Thing>
    


    <!-- http://purl.org/olia/bambara.owl#CAUS -->

    <initial.v rdf:about="#CAUS">
        <rdf:type rdf:resource="#Derivation"/>
        <rdf:type rdf:resource="#derive.v"/>
        <rdf:type rdf:resource="&owl;Thing"/>
        <system:hasTagContaining>CAUS</system:hasTagContaining>
        <rdfs:comment xml:lang="fr"
            >l&#225;-/n&#225;-;
            v;
            v;
            pr&#233;fixe causatif</rdfs:comment>
    </initial.v>
    


    <!-- http://purl.org/olia/bambara.owl#CERT -->

    <MarquePredicative rdf:about="#CERT">
        <rdf:type rdf:resource="&owl;Thing"/>
        <system:hasTag>CERT</system:hasTag>
        <rdfs:comment xml:lang="fr"
            >n&#224; ~ n&#225;;
            marque du futur certain</rdfs:comment>
    </MarquePredicative>
    


    <!-- http://purl.org/olia/bambara.owl#COM -->

    <initial.n rdf:about="#COM">
        <rdf:type rdf:resource="#Derivation"/>
        <rdf:type rdf:resource="#derive.adj"/>
        <rdf:type rdf:resource="&owl;Thing"/>
        <rdfs:comment xml:lang="fr"
            >-ma;
            n;
            adj, (n);
            adjectif d&#233;nominal &#224; valeur comitative/ornative</rdfs:comment>
        <system:hasTagContaining>COM</system:hasTagContaining>
    </initial.n>
    


    <!-- http://purl.org/olia/bambara.owl#COND.AFF -->

    <MarquePredicative rdf:about="#COND.AFF">
        <rdf:type rdf:resource="&owl;Thing"/>
        <system:hasTag>COND.AFF</system:hasTag>
        <rdfs:comment xml:lang="fr"
            >m&#225;na ~ m&#225;a;
            marque du conditionnel affirmatif;
            m&#225;a est une forme des dialectes du nord</rdfs:comment>
    </MarquePredicative>
    


    <!-- http://purl.org/olia/bambara.owl#COND.NEG -->

    <owl:Thing rdf:about="#COND.NEG">
        <rdf:type rdf:resource="#MarquePredicative"/>
        <system:hasTag>COND.NEG</system:hasTag>
        <rdfs:comment xml:lang="fr"
            >b&#236;len ~ b&#236;le ~ b&#232;len;
            marque n&#233;gative du conditionnel;
            archa&#239;que, rare</rdfs:comment>
    </owl:Thing>
    


    <!-- http://purl.org/olia/bambara.owl#CONV.PROG -->

    <Derivation rdf:about="#CONV.PROG">
        <rdf:type rdf:resource="#derive.ptcp"/>
        <rdf:type rdf:resource="#initial.v"/>
        <rdf:type rdf:resource="&owl;Thing"/>
        <rdfs:comment xml:lang="fr"
            >-t&#596;;
            v;
            ptcp;
            converbe progressif et prospectif (la valeur progressive avec les verbes at&#233;liques, la valeur prospective avec les verbes t&#233;liques)</rdfs:comment>
        <system:hasTagContaining>CONV.PROG</system:hasTagContaining>
    </Derivation>
    


    <!-- http://purl.org/olia/bambara.owl#COP.NEG -->

    <Copule rdf:about="#COP.NEG">
        <rdf:type rdf:resource="&owl;Thing"/>
        <system:hasTag>COP.NEG</system:hasTag>
        <rdfs:comment xml:lang="fr"
            >t&#603;&#769;;
            copule d&#8217;un &#233;nonc&#233; non-verbal locatif ou pr&#233;sentatif affirmatif</rdfs:comment>
    </Copule>
    


    <!-- http://purl.org/olia/bambara.owl#DEF -->

    <owl:Thing rdf:about="#DEF">
        <rdf:type rdf:resource="#Determinatif"/>
        <system:hasTag>DEF</system:hasTag>
        <rdfs:comment xml:lang="fr"
            >&#236;n;
            le &#171; nouvel article d&#233;fini &#187;</rdfs:comment>
    </owl:Thing>
    


    <!-- http://purl.org/olia/bambara.owl#DEM -->

    <owl:Thing rdf:about="#DEM">
        <rdf:type rdf:resource="#PronomDeterminatif"/>
        <rdf:type>
            <owl:Class>
                <owl:unionOf rdf:parseType="Collection">
                    <rdf:Description rdf:about="#Determinatif"/>
                    <rdf:Description rdf:about="#PronomNonPersonnel"/>
                </owl:unionOf>
            </owl:Class>
        </rdf:type>
        <system:hasTag>DEM</system:hasTag>
        <rdfs:comment xml:lang="fr"
            >n&#236;n;
            dtm, pron;
            remplace le groupe nominal, le suit ou le pr&#233;c&#232;de;
            pronom d&#233;monstratif</rdfs:comment>
    </owl:Thing>
    


    <!-- http://purl.org/olia/bambara.owl#DEQU -->

    <initial.vp rdf:about="#DEQU">
        <rdf:type rdf:resource="#Derivation"/>
        <rdf:type rdf:resource="#derive.n"/>
        <rdf:type rdf:resource="#derive.v"/>
        <rdf:type rdf:resource="&owl;Thing"/>
        <system:hasTagContaining>DEQU</system:hasTagContaining>
        <rdfs:comment xml:lang="fr"
            >-ya;
            vq;
            n, v;
            verbes dynamiques et noms de qualit&#233;s d&#233;riv&#233;s des verbes qualitatifs</rdfs:comment>
    </initial.vp>
    


    <!-- http://purl.org/olia/bambara.owl#DES -->

    <owl:Thing rdf:about="#DES">
        <rdf:type rdf:resource="#MarquePredicative"/>
        <system:hasTag>DES</system:hasTag>
        <rdfs:comment xml:lang="fr"
            >m&#224; ~ m&#224;a;
            suit le groupe nominal du sujet repr&#233;sent&#233; par le mot Ala ; le verbe a le suffixe &#8211;ra / -la / -na PFV.INTR;
            marque pr&#233;dicative dans l&#8217;&#233;nonc&#233; exprimant une b&#233;n&#233;diction</rdfs:comment>
    </owl:Thing>
    


    <!-- http://purl.org/olia/bambara.owl#DIM -->

    <initial.n rdf:about="#DIM">
        <rdf:type rdf:resource="#Derivation"/>
        <rdf:type rdf:resource="#initial.adj"/>
        <rdf:type rdf:resource="#initial.ptcp"/>
        <rdf:type rdf:resource="&owl;Thing"/>
        <rdfs:comment xml:lang="fr"
            >-nin;
            n, adj, ptcp;
            ne change pas;
            diminutif</rdfs:comment>
        <system:hasTagContaining>DIM</system:hasTagContaining>
    </initial.n>
    


    <!-- http://purl.org/olia/bambara.owl#DIR -->

    <derive.v rdf:about="#DIR">
        <rdf:type rdf:resource="#Derivation"/>
        <rdf:type rdf:resource="#initial.v"/>
        <rdf:type rdf:resource="&owl;Thing"/>
        <system:hasTagContaining>DIR</system:hasTagContaining>
        <rdfs:comment xml:lang="fr"
            >-ma;
            v;
            v;
            suffixe non-productif qui se combine surtout avec les verbes d&#8217;action orient&#233;e, souvent sans modifier le sens originel</rdfs:comment>
    </derive.v>
    


    <!-- http://purl.org/olia/bambara.owl#DISTR -->

    <Conjonction rdf:about="#DISTR">
        <rdf:type rdf:resource="&owl;Thing"/>
        <system:hasTag>DISTR</system:hasTag>
        <rdfs:comment xml:lang="fr"
            >&#243;`;
            marque du distributif</rdfs:comment>
    </Conjonction>
    


    <!-- http://purl.org/olia/bambara.owl#EN -->

    <initial.v rdf:about="#EN">
        <rdf:type rdf:resource="#Derivation"/>
        <rdf:type rdf:resource="#derive.v"/>
        <rdf:type rdf:resource="&owl;Thing"/>
        <system:hasTagContaining>EN</system:hasTagContaining>
        <rdfs:comment xml:lang="fr"
            >s&#596;&#768;-;
            v;
            v;
            suffixe non-productif, se combine avec quelques verbes de mouvement; se d&#233;rive du mot s&#596;&#768;n &#8216;coeur&#8217; (cf. la postposition courante dans le marka-dafin, s&#596;&#769;n)</rdfs:comment>
    </initial.v>
    


    <!-- http://purl.org/olia/bambara.owl#EQU -->

    <Copule rdf:about="#EQU">
        <rdf:type rdf:resource="&owl;Thing"/>
        <system:hasTag>EQU</system:hasTag>
        <rdfs:comment xml:lang="fr"
            >y&#233;;
            copule d&#8217;un &#233;nonc&#233; &#233;quatif non-verbal affirmatif</rdfs:comment>
    </Copule>
    


    <!-- http://purl.org/olia/bambara.owl#ETRG -->

    <owl:Thing rdf:about="#ETRG">
        <rdf:type rdf:resource="#MotEtranger"/>
        <rdfs:comment
            >un mot &#233;tranger non-adapt&#233;</rdfs:comment>
        <system:hasTag>ETRG</system:hasTag>
    </owl:Thing>
    


    <!-- http://purl.org/olia/bambara.owl#ETRG.ARB -->

    <owl:Thing rdf:about="#ETRG.ARB">
        <rdf:type rdf:resource="#MotEtranger"/>
        <rdfs:comment>un mot arabe</rdfs:comment>
        <system:hasTag>ETRG.ARB</system:hasTag>
    </owl:Thing>
    


    <!-- http://purl.org/olia/bambara.owl#ETRG.FRA -->

    <MotEtranger rdf:about="#ETRG.FRA">
        <rdf:type rdf:resource="&owl;Thing"/>
        <system:hasTag>ETRG.FRA</system:hasTag>
        <rdfs:comment>un mot fran&#231;ais</rdfs:comment>
    </MotEtranger>
    


    <!-- http://purl.org/olia/bambara.owl#ETRG.FUL -->

    <MotEtranger rdf:about="#ETRG.FUL">
        <rdf:type rdf:resource="&owl;Thing"/>
        <rdfs:comment>un mot peul</rdfs:comment>
        <system:hasTag>ETRG.FUL</system:hasTag>
    </MotEtranger>
    


    <!-- http://purl.org/olia/bambara.owl#FOC -->

    <Particule rdf:about="#FOC">
        <rdf:type rdf:resource="&owl;Thing"/>
        <system:hasTag>FOC</system:hasTag>
        <rdfs:comment xml:lang="fr"
            >d&#232;;
            marque du focus contrastif</rdfs:comment>
    </Particule>
    


    <!-- http://purl.org/olia/bambara.owl#FUT.AFF -->

    <MarquePredicative rdf:about="#FUT.AFF">
        <rdf:type rdf:resource="&owl;Thing"/>
        <system:hasTag>FUT.AFF</system:hasTag>
        <rdfs:comment xml:lang="fr"
            >b&#603;&#769;n&#224; ~ b&#237;n&#224; ~ b&#233;n&#224;;
            marque affirmative du futur</rdfs:comment>
    </MarquePredicative>
    


    <!-- http://purl.org/olia/bambara.owl#FUT.NEG -->

    <MarquePredicative rdf:about="#FUT.NEG">
        <rdf:type rdf:resource="&owl;Thing"/>
        <system:hasTag>FUT.NEG</system:hasTag>
        <rdfs:comment xml:lang="fr"
            >t&#603;&#769;n&#224; ~ t&#233;n&#224; ~ t&#237;n&#224;,
            marque du futur n&#233;gatif</rdfs:comment>
    </MarquePredicative>
    


    <!-- http://purl.org/olia/bambara.owl#GENT -->

    <initial.n rdf:about="#GENT">
        <rdf:type rdf:resource="#Derivation"/>
        <rdf:type rdf:resource="#derive.n"/>
        <rdf:type rdf:resource="&owl;Thing"/>
        <system:hasTagContaining>GENT</system:hasTagContaining>
        <rdfs:comment xml:lang="fr"
            >-ka;
            n;
            n;
            suffixe du nom d&#8217;habitant ou originaire d&#8217;une localit&#233;</rdfs:comment>
    </initial.n>
    


    <!-- http://purl.org/olia/bambara.owl#IMP -->

    <owl:Thing rdf:about="#IMP">
        <rdf:type rdf:resource="#MarquePredicative"/>
        <system:hasTag>IMP</system:hasTag>
        <rdfs:comment xml:lang="fr"
            >y&#233;;
            suit le groupe nominal du sujet au 2&#232;me pl;
            marque de l&#8217;imp&#233;ratif 2&#232;me pl</rdfs:comment>
    </owl:Thing>
    


    <!-- http://purl.org/olia/bambara.owl#IN -->

    <derive.adj rdf:about="#IN">
        <rdf:type rdf:resource="#Derivation"/>
        <rdf:type rdf:resource="&owl;Thing"/>
        <system:hasTagContaining>IN</system:hasTagContaining>
        <rdfs:comment xml:lang="fr"
            >-r&#596;- / -n&#596;-;
            (dans);
            adj;
            connecteur des composantes des adjectifs compos&#233;s; -r&#596;- suivant une voyelle orale, -n&#596;- suivant une voyelle orale</rdfs:comment>
    </derive.adj>
    


    <!-- http://purl.org/olia/bambara.owl#IN2 -->

    <initial.v rdf:about="#IN2">
        <rdf:type rdf:resource="#Derivation"/>
        <rdf:type rdf:resource="#derive.v"/>
        <rdf:type rdf:resource="&owl;Thing"/>
        <system:hasTagContaining>IN</system:hasTagContaining>
        <owl:versionInfo
            >TODO: disambiguate with the other gloss value IN (for homographic morphemes), these two will get conflated</owl:versionInfo>
        <rdfs:comment xml:lang="fr"
            >r&#225;-/r&#596;&#769;-;
            v;
            v;
            pr&#233;fixe &#224; valeur obscure (&#233;tymologiquement, valeur inessive)</rdfs:comment>
    </initial.v>
    


    <!-- http://purl.org/olia/bambara.owl#INF -->

    <owl:Thing rdf:about="#INF">
        <rdf:type rdf:resource="#MarquePredicative"/>
        <system:hasTag>INF</system:hasTag>
        <rdfs:comment xml:lang="fr"
            >k&#224;; 
            pr&#233;c&#232;de le groupe nominal du compl&#233;ment d&#8217;objet direct, ou, en son absence, le verbe;
            marque d&#8217;infinitif</rdfs:comment>
    </owl:Thing>
    


    <!-- http://purl.org/olia/bambara.owl#INFR.AFF -->

    <MarquePredicative rdf:about="#INFR.AFF">
        <rdf:type rdf:resource="&owl;Thing"/>
        <system:hasTag>INFR.AFF</system:hasTag>
        <rdfs:comment xml:lang="fr"
            >b&#603;&#769;ka ~ b&#603;&#769;ga ~ b&#225;ga ~ b&#250;ga;
            marque affirmative du parfait inf&#233;rentif;
            peu utilis&#233; en bambara standard</rdfs:comment>
    </MarquePredicative>
    


    <!-- http://purl.org/olia/bambara.owl#INFR.NEG -->

    <MarquePredicative rdf:about="#INFR.NEG">
        <rdf:type rdf:resource="&owl;Thing"/>
        <system:hasTag>INFR.NEG</system:hasTag>
        <rdfs:comment xml:lang="fr"
            >t&#603;&#769;ka ~ t&#603;&#769;ga;
            marque n&#233;gative du parfait inf&#233;rentif;
            peu utilis&#233; en bambara standard</rdfs:comment>
    </MarquePredicative>
    


    <!-- http://purl.org/olia/bambara.owl#INSTR -->

    <initial.v rdf:about="#INSTR">
        <rdf:type rdf:resource="#Derivation"/>
        <rdf:type rdf:resource="#derive.n"/>
        <rdf:type rdf:resource="&owl;Thing"/>
        <system:hasTagContaining>INSTR</system:hasTagContaining>
        <rdfs:comment xml:lang="fr"
            >-lan/-nan/-ran; 
            v;
            n;
            nom d&#8217;instrument</rdfs:comment>
    </initial.v>
    


    <!-- http://purl.org/olia/bambara.owl#IPFV.AFF -->

    <owl:Thing rdf:about="#IPFV.AFF">
        <rdf:type rdf:resource="#MarquePredicative"/>
        <system:hasTag>IPFV.AFF</system:hasTag>
        <rdfs:comment xml:lang="fr"
            >b&#603;&#769; ~ b&#237; ~ b&#233;;
            marque affirmative de l&#8217;imperfectif</rdfs:comment>
    </owl:Thing>
    


    <!-- http://purl.org/olia/bambara.owl#IPFV.NEG -->

    <MarquePredicative rdf:about="#IPFV.NEG">
        <rdf:type rdf:resource="&owl;Thing"/>
        <system:hasTag>IPFV.NEG</system:hasTag>
        <rdfs:comment xml:lang="fr"
            >t&#603;&#769; ~ t&#237; ~ t&#233;;
            marque de l&#8217;imperfectif n&#233;gatif</rdfs:comment>
    </MarquePredicative>
    


    <!-- http://purl.org/olia/bambara.owl#LOC -->

    <Derivation rdf:about="#LOC">
        <rdf:type rdf:resource="#derive.n"/>
        <rdf:type rdf:resource="#initial.n"/>
        <rdf:type rdf:resource="&owl;Thing"/>
        <rdfs:comment xml:lang="fr"
            >-la / -na;
            n;
            n;
            nom de place</rdfs:comment>
        <system:hasTagContaining>LOC</system:hasTagContaining>
    </Derivation>
    


    <!-- http://purl.org/olia/bambara.owl#MNT1 -->

    <initial.v rdf:about="#MNT1">
        <rdf:type rdf:resource="#Derivation"/>
        <rdf:type rdf:resource="#derive.n"/>
        <rdf:type rdf:resource="#initial.n"/>
        <rdf:type rdf:resource="#initial.pp"/>
        <rdf:type rdf:resource="&owl;Thing"/>
        <system:hasTagContaining>MNT1</system:hasTagContaining>
        <rdfs:comment xml:lang="fr"
            >-la / -na;
            v, n, pp;
            n;
            nom d&#8217;activit&#233; mentale ou de son r&#233;sultat</rdfs:comment>
    </initial.v>
    


    <!-- http://purl.org/olia/bambara.owl#MNT2 -->

    <Derivation rdf:about="#MNT2">
        <rdf:type rdf:resource="#derive.n"/>
        <rdf:type rdf:resource="#initial.n"/>
        <rdf:type rdf:resource="#initial.pp"/>
        <rdf:type rdf:resource="#initial.v"/>
        <rdf:type rdf:resource="&owl;Thing"/>
        <system:hasTagContaining>MNT2</system:hasTagContaining>
        <rdfs:comment xml:lang="fr"
            >-lata / -nata;
            v, n, pp;
            n;
            nom d&#8217;activit&#233; mentale ou de son r&#233;sultat</rdfs:comment>
    </Derivation>
    


    <!-- http://purl.org/olia/bambara.owl#NMLZ -->

    <owl:Thing rdf:about="#NMLZ">
        <rdf:type rdf:resource="#Derivation"/>
        <rdf:type rdf:resource="#derive.n"/>
        <rdf:type rdf:resource="#initial.v"/>
        <rdfs:comment xml:lang="fr"
            >-li/-ni;
            v;
            n;
            nom verbal (nom d&#8217;action)</rdfs:comment>
        <system:hasTagContaining>NMLZ</system:hasTagContaining>
    </owl:Thing>
    


    <!-- http://purl.org/olia/bambara.owl#NOM.CL -->

    <NomPropre rdf:about="#NOM.CL">
        <rdf:type rdf:resource="&owl;Thing"/>
        <rdfs:comment
            >nom clanique (j&#224;mu)</rdfs:comment>
        <system:hasTag>NOM.CL</system:hasTag>
    </NomPropre>
    


    <!-- http://purl.org/olia/bambara.owl#NOM.F -->

    <owl:Thing rdf:about="#NOM.F">
        <rdf:type rdf:resource="#NomPropre"/>
        <system:hasTag>NOM.F</system:hasTag>
        <rdfs:comment>pr&#233;nom f&#233;minin</rdfs:comment>
    </owl:Thing>
    


    <!-- http://purl.org/olia/bambara.owl#NOM.M -->

    <owl:Thing rdf:about="#NOM.M">
        <rdf:type rdf:resource="#NomPropre"/>
        <system:hasTag>NOM.M</system:hasTag>
        <rdfs:comment>pr&#233;nom masculin</rdfs:comment>
    </owl:Thing>
    


    <!-- http://purl.org/olia/bambara.owl#NOM.MF -->

    <NomPropre rdf:about="#NOM.MF">
        <rdf:type rdf:resource="&owl;Thing"/>
        <rdfs:comment
            >pr&#233;nom ne distinguant pas entre les sexes</rdfs:comment>
        <system:hasTag>NOM.MF</system:hasTag>
    </NomPropre>
    


    <!-- http://purl.org/olia/bambara.owl#OPT -->

    <MarquePredicative rdf:about="#OPT">
        <rdf:type rdf:resource="&owl;Thing"/>
        <system:hasTag>OPT</system:hasTag>
        <rdfs:comment xml:lang="fr"
            >k&#225;;
            marque d&#8217;optatif</rdfs:comment>
    </MarquePredicative>
    


    <!-- http://purl.org/olia/bambara.owl#ORD -->

    <initial.num rdf:about="#ORD">
        <rdf:type rdf:resource="#Derivation"/>
        <rdf:type rdf:resource="#derive.adj"/>
        <rdf:type rdf:resource="&owl;Thing"/>
        <system:hasTagContaining>ORD</system:hasTagContaining>
        <rdfs:comment xml:lang="fr"
            >-nan;
            num;
            adj;
            suffixe des num&#233;raux ordinaux</rdfs:comment>
    </initial.num>
    


    <!-- http://purl.org/olia/bambara.owl#PFV.EMPH -->

    <owl:Thing rdf:about="#PFV.EMPH">
        <rdf:type rdf:resource="#MarquePredicative"/>
        <system:hasTag>PFV.EMPH</system:hasTag>
        <rdfs:comment xml:lang="fr"
            >y&#233; k&#224;;
            EQU INF (une marque disjoint; autrement,PFV.EMPH);
            marque du pass&#233; r&#233;cent;
            rarement utilis&#233;</rdfs:comment>
    </owl:Thing>
    


    <!-- http://purl.org/olia/bambara.owl#PFV.INTR -->

    <owl:Thing rdf:about="#PFV.INTR">
        <rdf:type rdf:resource="#Flexion"/>
        <rdfs:comment xml:lang="fr"
            >-ra/-la/-na;
            v (v.i);
            marque du perfectif intransitif;
            - na apr&#232;s une syllable comportant un &#233;lement nasal ;
            - la apr&#232;s une syllabe orale &#224; consonnes r ou l ;
            - ra dans tous les autres cas</rdfs:comment>
        <system:hasTagEndingWith>PFV.INTR</system:hasTagEndingWith>
        <rdfs:comment xml:lang="en"
            >Perfective intransitive marker (V. Vydrine)</rdfs:comment>
    </owl:Thing>
    


    <!-- http://purl.org/olia/bambara.owl#PFV.NEG -->

    <owl:Thing rdf:about="#PFV.NEG">
        <rdf:type rdf:resource="#MarquePredicative"/>
        <system:hasTag>PFV.NEG</system:hasTag>
        <rdfs:comment xml:lang="fr"
            >m&#225;;
            marque n&#233;gative du perfectif</rdfs:comment>
    </owl:Thing>
    


    <!-- http://purl.org/olia/bambara.owl#PFV.TR -->

    <owl:Thing rdf:about="#PFV.TR">
        <rdf:type rdf:resource="#Particule"/>
        <system:hasTag>PFV.TR</system:hasTag>
        <rdfs:comment xml:lang="fr"
            >y&#233;;
            marque du perfectif affirmatif transitif</rdfs:comment>
    </owl:Thing>
    


    <!-- http://purl.org/olia/bambara.owl#PL -->

    <owl:Thing rdf:about="#PL">
        <rdf:type rdf:resource="#Flexion"/>
        <rdfs:comment xml:lang="fr"
            >-w;
            n, adj, dtm, prn;
            marque du pluriel</rdfs:comment>
        <system:hasTagEndingWith>PL</system:hasTagEndingWith>
    </owl:Thing>
    


    <!-- http://purl.org/olia/bambara.owl#PL2 -->

    <Flexion rdf:about="#PL2">
        <rdf:type rdf:resource="&owl;Thing"/>
        <system:hasTagEndingWith>PL2</system:hasTagEndingWith>
        <rdfs:comment xml:lang="en"
            >There is no semantic difference between PL and PL2, the latter is used with specific lexemes. (V. Vydrine)</rdfs:comment>
        <rdfs:comment xml:lang="fr"
            >-l&#250;/-n&#250;;
            prn, n, dtm;
            marque non-productive du pluriel (se combine avec les pronoms n&#236;n, &#242;, m&#237;n, et avec le nom m&#224;a &#8216;homme&#8217;);
            -n&#250; apr&#232;s une voyelle nasale, -l&#250; ailleurs</rdfs:comment>
    </Flexion>
    


    <!-- http://purl.org/olia/bambara.owl#POSS -->

    <owl:Thing rdf:about="#POSS">
        <rdf:type rdf:resource="#Conjonction"/>
        <system:hasTag>POSS</system:hasTag>
        <rdfs:comment xml:lang="fr"
            >k&#225;; 
            marque possessive</rdfs:comment>
    </owl:Thing>
    


    <!-- http://purl.org/olia/bambara.owl#PRES -->

    <owl:Thing rdf:about="#PRES">
        <rdf:type rdf:resource="#Copule"/>
        <system:hasTag>PRES</system:hasTag>
        <rdfs:comment xml:lang="fr"
            >d&#242;n;
            copule de l&#8217;&#233;nonc&#233; non-verbal pr&#233;sentatif affirmatif</rdfs:comment>
    </owl:Thing>
    


    <!-- http://purl.org/olia/bambara.owl#PREV -->

    <owl:Thing rdf:about="#PREV">
        <rdf:type rdf:resource="#AutreAbreviation"/>
        <owl:versionInfo
            >TODO: clarify whether this can be annotated as (part of) Verb</owl:versionInfo>
        <rdfs:comment
            >l&#8217;&#233;l&#233;ment initial d&#8217;un verbe compos&#233; n&#8217;ayant pas d&#8217;&#233;tymologie &#233;vidente (et pouvant parfois se d&#233;tacher de la base verbale)</rdfs:comment>
        <system:hasTag>PREV</system:hasTag>
    </owl:Thing>
    


    <!-- http://purl.org/olia/bambara.owl#PRICE -->

    <Derivation rdf:about="#PRICE">
        <rdf:type rdf:resource="#derive.n"/>
        <rdf:type rdf:resource="#initial.num"/>
        <rdf:type rdf:resource="&owl;Thing"/>
        <rdfs:comment xml:lang="fr"
            >-la / -na;
            num;
            n;
            nom de prix (&#171; quantit&#233; de marchandise pour la valeur de X &#187;)</rdfs:comment>
        <system:hasTagContaining>PRICE</system:hasTagContaining>
    </Derivation>
    


    <!-- http://purl.org/olia/bambara.owl#PRIV -->

    <initial.n rdf:about="#PRIV">
        <rdf:type rdf:resource="#Derivation"/>
        <rdf:type rdf:resource="#derive.adj"/>
        <rdf:type rdf:resource="&owl;Thing"/>
        <system:hasTagContaining>PRIV</system:hasTagContaining>
        <rdfs:comment xml:lang="fr"
            >-ntan;
            n;
            adj, (n);
            adjectif d&#233;nominal privatif</rdfs:comment>
    </initial.n>
    


    <!-- http://purl.org/olia/bambara.owl#PROG -->

    <Flexion rdf:about="#PROG">
        <rdf:type rdf:resource="&owl;Thing"/>
        <system:hasTagEndingWith>PROG</system:hasTagEndingWith>
        <rdfs:comment xml:lang="fr"
            >-la/-na;
            v, ptcp;
suffixe verbal du progressif (va de paire avec le pm b&#603;&#769; (affirmatif), t&#603;&#769; (n&#233;gatif);
-na apr&#232;s une voyelle nasale ; -la apr&#232;s une voyelle orale ; se combine avec les verbes et avec le participe progressif-prospectif en &#8211;t&#596;</rdfs:comment>
    </Flexion>
    


    <!-- http://purl.org/olia/bambara.owl#PROG.AFF -->

    <owl:Thing rdf:about="#PROG.AFF">
        <rdf:type rdf:resource="#MarquePredicative"/>
        <system:hasTag>PROG.AFF</system:hasTag>
        <rdfs:comment xml:lang="fr"
            >b&#603;&#769; k&#224;;
            BE INF (une marque disjoint; autrement, PROG.AFF);
            marque affirmative du progressif</rdfs:comment>
    </owl:Thing>
    


    <!-- http://purl.org/olia/bambara.owl#PROG.NEG -->

    <owl:Thing rdf:about="#PROG.NEG">
        <rdf:type rdf:resource="#MarquePredicative"/>
        <system:hasTag>PROG.NEG</system:hasTag>
        <rdfs:comment xml:lang="fr"
            >t&#603;&#769; k&#224;;
            COP.NEG INF (une marque disjoint; autrement, PROG.NEG);
            marque du progressif n&#233;gatif</rdfs:comment>
    </owl:Thing>
    


    <!-- http://purl.org/olia/bambara.owl#PROH -->

    <owl:Thing rdf:about="#PROH">
        <rdf:type rdf:resource="#MarquePredicative"/>
        <system:hasTag>PROH</system:hasTag>
        <rdfs:comment xml:lang="fr"
            >k&#224;n&#225; ~ k&#225;n&#224;;
            marque du prohibitif</rdfs:comment>
    </owl:Thing>
    


    <!-- http://purl.org/olia/bambara.owl#PST -->

    <Particule rdf:about="#PST">
        <rdf:type rdf:resource="&owl;Thing"/>
        <system:hasTag>PST</system:hasTag>
        <rdfs:comment xml:lang="fr"
            >t&#249;n;
            le plus souvent, pr&#233;c&#232;de la marque pr&#233;dicative ou la copule;
            marque du pass&#233; discontinu</rdfs:comment>
    </Particule>
    


    <!-- http://purl.org/olia/bambara.owl#PTCP.POT -->

    <Derivation rdf:about="#PTCP.POT">
        <rdf:type rdf:resource="#derive.ptcp"/>
        <rdf:type rdf:resource="#initial.v"/>
        <rdf:type rdf:resource="&owl;Thing"/>
        <rdfs:comment xml:lang="fr"
            >-ta;
            v;
            ptcp;
            participe potentiel</rdfs:comment>
        <system:hasTagContaining>PTCP.POT</system:hasTagContaining>
    </Derivation>
    


    <!-- http://purl.org/olia/bambara.owl#PTCP.PRIV -->

    <Derivation rdf:about="#PTCP.PRIV">
        <rdf:type rdf:resource="#derive.ptcp"/>
        <rdf:type rdf:resource="#initial.v"/>
        <rdf:type rdf:resource="&owl;Thing"/>
        <system:hasTagContaining>PCTCP.PRIV</system:hasTagContaining>
        <rdfs:comment xml:lang="fr"
            >-bali;
            v;
            ptcp;
            participe privatif</rdfs:comment>
    </Derivation>
    


    <!-- http://purl.org/olia/bambara.owl#PTCP.RES -->

    <Derivation rdf:about="#PTCP.RES">
        <rdf:type rdf:resource="#derive.ptcp"/>
        <rdf:type rdf:resource="#initial.v"/>
        <rdf:type rdf:resource="&owl;Thing"/>
        <rdfs:comment xml:lang="fr"
            >-len/-nen;
            v;
            ptcp;
            participe &#224; valeur r&#233;sultative</rdfs:comment>
        <system:hasTagContaining>PTCP.RES</system:hasTagContaining>
    </Derivation>
    


    <!-- http://purl.org/olia/bambara.owl#Q -->

    <owl:Thing rdf:about="#Q">
        <rdf:type rdf:resource="#Particule"/>
        <system:hasTag>Q</system:hasTag>
        <rdfs:comment xml:lang="fr"
            >w&#224;;
            en fin d&#8217;&#233;nonc&#233;;
            particule de question g&#233;n&#233;rale</rdfs:comment>
    </owl:Thing>
    


    <!-- http://purl.org/olia/bambara.owl#QUAL.AFF -->

    <owl:Thing rdf:about="#QUAL.AFF">
        <rdf:type rdf:resource="#MarquePredicative"/>
        <system:hasTag>QUAL.AFF</system:hasTag>
        <rdfs:comment xml:lang="fr"
            >k&#225;;
            marque affirmative de l&#8217;&#233;nonc&#233; qualitatif</rdfs:comment>
    </owl:Thing>
    


    <!-- http://purl.org/olia/bambara.owl#QUAL.NEG -->

    <MarquePredicative rdf:about="#QUAL.NEG">
        <rdf:type rdf:resource="&owl;Thing"/>
        <system:hasTag>QUAL.NEG</system:hasTag>
        <rdfs:comment xml:lang="fr"
            >m&#225;n;
            marque n&#233;gative de l&#8217;&#233;nonc&#233; qualitati</rdfs:comment>
    </MarquePredicative>
    


    <!-- http://purl.org/olia/bambara.owl#RECP -->

    <owl:Thing rdf:about="#RECP">
        <rdf:type rdf:resource="#Derivation"/>
        <rdf:type rdf:resource="#PronomNonPersonnel"/>
        <rdf:type rdf:resource="#derive.n"/>
        <rdf:type rdf:resource="#initial.n"/>
        <rdf:type rdf:resource="#initial.v"/>
        <system:hasTag>RECP</system:hasTag>
        <system:hasTagContaining>RECP</system:hasTagContaining>
        <rdfs:comment xml:lang="fr"
            >&#626;&#596;g&#596;n/&#626;wan/ &#626;waan;
            v, n;
            n;
            suffixo&#239;de &#224; valeur de &#171; nom de partenaire &#187;</rdfs:comment>
        <rdfs:comment xml:lang="fr"
            >&#626;&#596;&#769;g&#596;n;
            pronom r&#233;ciproque</rdfs:comment>
    </owl:Thing>
    


    <!-- http://purl.org/olia/bambara.owl#RECP.PRN -->

    <derive.n rdf:about="#RECP.PRN">
        <rdf:type rdf:resource="#Derivation"/>
        <rdf:type rdf:resource="#initial.n"/>
        <rdf:type rdf:resource="&owl;Thing"/>
        <rdfs:comment xml:lang="fr"
            >-ma;
            n;
            n;
            suffixe nominal r&#233;ciproque</rdfs:comment>
        <system:hasTagContaining>RECP.PRN</system:hasTagContaining>
    </derive.n>
    


    <!-- http://purl.org/olia/bambara.owl#REFL -->

    <PronomNonPersonnel rdf:about="#REFL">
        <rdf:type rdf:resource="&owl;Thing"/>
        <system:hasTag>REFL</system:hasTag>
        <rdfs:comment xml:lang="fr"
            >&#237;;
            pronom r&#233;fl&#233;chi</rdfs:comment>
    </PronomNonPersonnel>
    


    <!-- http://purl.org/olia/bambara.owl#REL -->

    <owl:Thing rdf:about="#REL">
        <rdf:type rdf:resource="#PronomDeterminatif"/>
        <rdf:type>
            <owl:Class>
                <owl:unionOf rdf:parseType="Collection">
                    <rdf:Description rdf:about="#Determinatif"/>
                    <rdf:Description rdf:about="#PronomNonPersonnel"/>
                </owl:unionOf>
            </owl:Class>
        </rdf:type>
        <system:hasTag>REL</system:hasTag>
        <rdfs:comment xml:lang="fr"
            >m&#237;n;
            dtm, pron;
            suit le groupe nominal relativis&#233; dans la clause subordonn&#233; &#224; gauche ; remplace le groupe nominal dans la clause subordonn&#233;e &#224; droite;
            marque de relativisation</rdfs:comment>
    </owl:Thing>
    


    <!-- http://purl.org/olia/bambara.owl#SEQ -->

    <MarquePredicative rdf:about="#SEQ">
        <rdf:type rdf:resource="&owl;Thing"/>
        <system:hasTag>SEQ</system:hasTag>
        <rdfs:comment xml:lang="fr"
            >d&#236;y&#233;;
            marque s&#233;quentative;
            dialecte de Sikasso</rdfs:comment>
    </MarquePredicative>
    


    <!-- http://purl.org/olia/bambara.owl#ST -->

    <owl:Thing rdf:about="#ST">
        <rdf:type rdf:resource="#Derivation"/>
        <rdf:type rdf:resource="#derive.adj"/>
        <rdf:type rdf:resource="#derive.n"/>
        <rdf:type rdf:resource="#initial.n"/>
        <system:hasTagMatching>.*[^a-zA-Z]ST.*</system:hasTagMatching>
        <rdfs:comment xml:lang="fr"
            >-t&#596;;
            n;
            n, adj;
            nom du sujet d&#8217;&#233;tat (le plus souvent, infavorable)</rdfs:comment>
    </owl:Thing>
    


    <!-- http://purl.org/olia/bambara.owl#STAT -->

    <Derivation rdf:about="#STAT">
        <rdf:type rdf:resource="#derive.adj"/>
        <rdf:type rdf:resource="#initial.n"/>
        <rdf:type rdf:resource="&owl;Thing"/>
        <system:hasTagContaining>STAT</system:hasTagContaining>
        <rdfs:comment xml:lang="fr"
            >-lama / -nama;
            n;
            adj;
            adjectif d&#233;nominal &#224; valeur &#171; en guise de &#187;, &#171; en qualit&#233; de &#187;, &#171; fait de &#187;, &#171; en tant que...</rdfs:comment>
    </Derivation>
    


    <!-- http://purl.org/olia/bambara.owl#SUPER -->

    <owl:Thing rdf:about="#SUPER">
        <rdf:type rdf:resource="#Derivation"/>
        <rdf:type rdf:resource="#derive.adj"/>
        <system:hasTagContaining>SUPER</system:hasTagContaining>
        <rdfs:comment xml:lang="fr"
            >-ma- / -man-;
            (dans);
            adj;
            connecteur des composantes des adjectifs compos&#233;s; les variantes avec les voyelles nasale et orale sont distribu&#233;es lexicalement</rdfs:comment>
    </owl:Thing>
    


    <!-- http://purl.org/olia/bambara.owl#SUPER2 -->

    <derive.v rdf:about="#SUPER2">
        <rdf:type rdf:resource="#Derivation"/>
        <rdf:type rdf:resource="#initial.v"/>
        <rdf:type rdf:resource="&owl;Thing"/>
        <owl:versionInfo
            >TODO: disambiguate with the other gloss value SUPER (for homographic morphemes), these two will get conflated</owl:versionInfo>
        <system:hasTagContaining>SUPER</system:hasTagContaining>
        <rdfs:comment xml:lang="fr"
            >m&#224;- ~ m&#224;n-;
            v;
            v;
            pr&#233;fixe &#224; valeur obscure (&#233;tymologiquement, valeur suppressive)</rdfs:comment>
    </derive.v>
    


    <!-- http://purl.org/olia/bambara.owl#TOP -->

    <owl:Thing rdf:about="#TOP">
        <rdf:type rdf:resource="#Particule"/>
        <system:hasTag>TOP</system:hasTag>
        <rdfs:comment xml:lang="fr"
            >k&#596;&#768;ni;
            marque de topicalisation contrastive</rdfs:comment>
    </owl:Thing>
    


    <!-- http://purl.org/olia/bambara.owl#TOP.CNTR -->

    <Particule rdf:about="#TOP.CNTR">
        <rdf:type rdf:resource="&owl;Thing"/>
        <system:hasTag>TOP.CNTR</system:hasTag>
        <rdfs:comment xml:lang="fr"
            >d&#249;n;
            marque dela topicalisation contrastive du sujet</rdfs:comment>
    </Particule>
    


    <!-- http://purl.org/olia/bambara.owl#TOP2 -->

    <AutreAbreviation rdf:about="#TOP2">
        <rdf:type rdf:resource="&owl;Thing"/>
        <rdfs:comment>toponyme</rdfs:comment>
        <system:hasTag>TOP</system:hasTag>
        <owl:versionInfo
            >TODO: disambiguate TOP=topic and TOP=toponymic</owl:versionInfo>
    </AutreAbreviation>
    


    <!-- http://purl.org/olia/bambara.owl#adj -->

    <owl:Thing rdf:about="#adj">
        <rdf:type rdf:resource="#Adjectif"/>
        <rdfs:comment>adjectif</rdfs:comment>
        <system:hasTag>adj</system:hasTag>
    </owl:Thing>
    


    <!-- http://purl.org/olia/bambara.owl#adj_n -->

    <Adjectif rdf:about="#adj_n">
        <rdf:type rdf:resource="#Nom"/>
        <rdf:type rdf:resource="&owl;Thing"/>
        <system:hasTag>adj/n</system:hasTag>
    </Adjectif>
    


    <!-- http://purl.org/olia/bambara.owl#adv -->

    <Adverbe rdf:about="#adv">
        <rdf:type rdf:resource="&owl;Thing"/>
        <system:hasTag>adv</system:hasTag>
        <rdfs:comment xml:lang="en"
            >adverb (in postverbal position) [V. Vydrine]</rdfs:comment>
    </Adverbe>
    


    <!-- http://purl.org/olia/bambara.owl#adv.p -->

    <Adverbe rdf:about="#adv.p">
        <rdf:type rdf:resource="&owl;Thing"/>
        <system:hasTag>adv.p</system:hasTag>
        <rdfs:comment
            >adverbe pr&#233;verbal</rdfs:comment>
    </Adverbe>
    


    <!-- http://purl.org/olia/bambara.owl#c -->

    <owl:Thing rdf:about="#c">
        <rdf:type rdf:resource="#Ponctuation"/>
        <system:hasTag>c</system:hasTag>
    </owl:Thing>
    


    <!-- http://purl.org/olia/bambara.owl#ce -->

    <owl:Thing rdf:about="#ce">
        <rdf:type rdf:resource="#PronomNonPersonnel"/>
        <system:hasTag>ce</system:hasTag>
        <rdfs:comment xml:lang="fr"
            >&#242;;
            pronom anaphorique et d&#233;monstratif</rdfs:comment>
    </owl:Thing>
    


    <!-- http://purl.org/olia/bambara.owl#ce.PL -->

    <owl:Thing rdf:about="#ce.PL">
        <rdf:type rdf:resource="#PronomNonPersonnel"/>
        <system:hasTag>ce.PL</system:hasTag>
        <rdfs:comment xml:lang="fr"
            >&#242;.l&#250;;
            pronom anaphorique pluriel ; pronom emphatique 3&#232;me pl</rdfs:comment>
    </owl:Thing>
    


    <!-- http://purl.org/olia/bambara.owl#conj -->

    <owl:Thing rdf:about="#conj">
        <rdf:type rdf:resource="#Conjonction"/>
        <system:hasTag>conj</system:hasTag>
        <rdfs:comment>conjonction</rdfs:comment>
    </owl:Thing>
    


    <!-- http://purl.org/olia/bambara.owl#cop -->

    <owl:Thing rdf:about="#cop">
        <rdf:type rdf:resource="#Copule"/>
        <system:hasTag>cop</system:hasTag>
        <rdfs:comment>copule</rdfs:comment>
    </owl:Thing>
    


    <!-- http://purl.org/olia/bambara.owl#intj -->

    <owl:Thing rdf:about="#intj">
        <rdf:type rdf:resource="#Interjection"/>
        <system:hasTag>intj</system:hasTag>
        <rdfs:comment>interjection</rdfs:comment>
    </owl:Thing>
    


    <!-- http://purl.org/olia/bambara.owl#n -->

    <owl:Thing rdf:about="#n">
        <rdf:type rdf:resource="#Nom"/>
        <rdfs:comment>nom</rdfs:comment>
        <system:hasTag>n</system:hasTag>
    </owl:Thing>
    


    <!-- http://purl.org/olia/bambara.owl#n_adv -->

    <Adverbe rdf:about="#n_adv">
        <rdf:type rdf:resource="#Nom"/>
        <rdf:type rdf:resource="&owl;Thing"/>
        <system:hasTag>n/adv</system:hasTag>
        <system:hasTag>adv/n</system:hasTag>
        <owl:versionInfo xml:lang="en"
            >added adv/n as also found in sample file (CC)</owl:versionInfo>
    </Adverbe>
    


    <!-- http://purl.org/olia/bambara.owl#num -->

    <owl:Thing rdf:about="#num">
        <rdf:type rdf:resource="#Num&#233;ratif"/>
        <system:hasTag>num</system:hasTag>
        <rdfs:comment>num&#233;ratif</rdfs:comment>
    </owl:Thing>
    


    <!-- http://purl.org/olia/bambara.owl#onomat -->

    <Onomatopee rdf:about="#onomat">
        <rdf:type rdf:resource="&owl;Thing"/>
        <rdfs:comment>onomatop&#233;e</rdfs:comment>
        <system:hasTag>onomat</system:hasTag>
    </Onomatopee>
    


    <!-- http://purl.org/olia/bambara.owl#pers -->

    <PronomPersonnel rdf:about="#pers">
        <rdf:type rdf:resource="&owl;Thing"/>
        <system:hasTag>pers</system:hasTag>
        <rdfs:comment
            >pronom personnel</rdfs:comment>
    </PronomPersonnel>
    


    <!-- http://purl.org/olia/bambara.owl#pm -->

    <owl:Thing rdf:about="#pm">
        <rdf:type rdf:resource="#MarquePredicative"/>
        <system:hasTag>pm</system:hasTag>
        <rdfs:comment
            >marque pr&#233;dicative</rdfs:comment>
    </owl:Thing>
    


    <!-- http://purl.org/olia/bambara.owl#prep -->

    <owl:Thing rdf:about="#prep">
        <rdf:type rdf:resource="#Pr&#233;position"/>
        <system:hasTag>prep</system:hasTag>
        <rdfs:comment>pr&#233;position</rdfs:comment>
    </owl:Thing>
    


    <!-- http://purl.org/olia/bambara.owl#prep_conj -->

    <Conjonction rdf:about="#prep_conj">
        <rdf:type rdf:resource="#Pr&#233;position"/>
        <rdf:type rdf:resource="&owl;Thing"/>
        <owl:versionInfo xml:lang="en"
            >CC: guidelines provide prep/conj only, I added conj/prep as found in sample file</owl:versionInfo>
        <system:hasTag>conj/prep</system:hasTag>
        <system:hasTag>prep/conj</system:hasTag>
        <rdfs:comment xml:lang="en"
            >all Bambara prepositions can also be used as conjunctions (not necessarily the other way around) [V. Vydrine]</rdfs:comment>
    </Conjonction>
    


    <!-- http://purl.org/olia/bambara.owl#prn -->

    <owl:Thing rdf:about="#prn">
        <rdf:type rdf:resource="#PronomNonPersonnel"/>
        <system:hasTag>prn</system:hasTag>
        <rdfs:comment
            >pronom (non-personnel)</rdfs:comment>
    </owl:Thing>
    


    <!-- http://purl.org/olia/bambara.owl#prn_dtm -->

    <owl:Thing rdf:about="#prn_dtm">
        <rdf:type rdf:resource="#PronomDeterminatif"/>
        <system:hasTag>prn/dtm</system:hasTag>
        <rdfs:comment
            >a tag used in the sample file, but not found in the documentation (CC)</rdfs:comment>
    </owl:Thing>
    


    <!-- http://purl.org/olia/bambara.owl#prt -->

    <owl:Thing rdf:about="#prt">
        <rdf:type rdf:resource="#Particule"/>
        <rdfs:comment>particule</rdfs:comment>
        <system:hasTag>prt</system:hasTag>
    </owl:Thing>
    


    <!-- http://purl.org/olia/bambara.owl#ptcp -->

    <owl:Thing rdf:about="#ptcp">
        <rdf:type rdf:resource="#Participe"/>
        <rdfs:comment>participe</rdfs:comment>
        <system:hasTag>ptcp</system:hasTag>
    </owl:Thing>
    


    <!-- http://purl.org/olia/bambara.owl#v -->

    <owl:Thing rdf:about="#v">
        <rdf:type rdf:resource="#VerbeDynamique"/>
        <system:hasTag>v</system:hasTag>
        <rdfs:comment>verbe</rdfs:comment>
    </owl:Thing>
    


    <!-- http://purl.org/olia/bambara.owl#vq -->

    <VerbeQualitatif rdf:about="#vq">
        <rdf:type rdf:resource="&owl;Thing"/>
        <rdfs:comment
            >verbe qualitativ</rdfs:comment>
        <system:hasTag>vq</system:hasTag>
    </VerbeQualitatif>
    


    <!-- http://purl.org/olia/bambara.owl#vq_adj -->

    <Adjectif rdf:about="#vq_adj">
        <rdf:type rdf:resource="#VerbeQualitatif"/>
        <rdf:type rdf:resource="&owl;Thing"/>
        <system:hasTag>vq/adj</system:hasTag>
    </Adjectif>
    


    <!-- http://purl.org/olia/dtm -->

    <owl:Thing rdf:about="http://purl.org/olia/dtm">
        <rdf:type rdf:resource="#Determinatif"/>
        <system:hasTag>dtm</system:hasTag>
        <rdfs:comment>d&#233;terminatif</rdfs:comment>
    </owl:Thing>
    


    <!-- http://purl.org/olia/pp -->

    <Postposition rdf:about="http://purl.org/olia/pp">
        <rdf:type rdf:resource="&owl;Thing"/>
        <rdfs:comment>postposition</rdfs:comment>
        <system:hasTag>pp</system:hasTag>
    </Postposition>
</rdf:RDF>



<!-- Generated by the OWL API (version 2.2.1.1138) http://owlapi.sourceforge.net -->

