<?xml version="1.0"?>


<!DOCTYPE rdf:RDF [
    <!ENTITY owl "http://www.w3.org/2002/07/owl#" >
    <!ENTITY dc "http://purl.org/dc/elements/1.1/" >
    <!ENTITY xsd "http://www.w3.org/2001/XMLSchema#" >
    <!ENTITY rdfs "http://www.w3.org/2000/01/rdf-schema#" >
    <!ENTITY rdf "http://www.w3.org/1999/02/22-rdf-syntax-ns#" >
]>


<rdf:RDF xmlns="http://purl.org/olia/dzongkha.owl#"
     xml:base="http://purl.org/olia/dzongkha.owl"
     xmlns:dc="http://purl.org/dc/elements/1.1/"
     xmlns:rdfs="http://www.w3.org/2000/01/rdf-schema#"
     xmlns:owl="http://www.w3.org/2002/07/owl#"
     xmlns:xsd="http://www.w3.org/2001/XMLSchema#"
     xmlns:rdf="http://www.w3.org/1999/02/22-rdf-syntax-ns#">
    <owl:Ontology rdf:about="http://purl.org/olia/dzongkha.owl">
        <rdfs:comment>2010-09-23 created&lt;br/&gt;
2010-10-12 NominalNoun and QuantifierNoun updated according to Jurmey&#39;s email&lt;br/&gt;
2021-11-25 update URI schema

Christian Chiarcos, christian.chiarcos@gmail.com
</rdfs:comment>
        <dc:description>Dzongkha is the national language of Bhutan. It is categorized as a Sino-Tibetan Language and said to have derived from the classical Tibetan or choka: Dzongkha consonants, vowels, phonemes, phonetics and writing system are all identical.
The tagset applied here contains 66 tags, which is based on the Penn Treebank.

The POS tagged data is already in use in projects concerning Dzongkha Text to Speech (TTS) processing, further tests on word segmentation, and in corpus-linguistic research. Future work entails its utilization for higher-level NLP tasks such as parsing, building parallel corpora, research on semantics, machine translation, and many more. (Chungku et al. 2010)

Unless marked otherwise, all comments are quoted from Chungku et al. (2010).

Chungku Chungku, Jurmey Rabgay and Gertrud Faa&#223; (2010), Building NLP resources for Dzongkha: A Tagset and A Tagged Corpus, In: Proceedings of the 8th Workshop on Asian Language Resources, pages 103&#8211;110, Beijing, China, 21-22 August 2010.

</dc:description>
    </owl:Ontology>



    <!--
    ///////////////////////////////////////////////////////////////////////////////////////
    //
    // Annotation properties
    //
    ///////////////////////////////////////////////////////////////////////////////////////
     -->

    <owl:AnnotationProperty rdf:about="&dc;description"/>
    <owl:AnnotationProperty rdf:about="&rdfs;comment"/>



    <!--
    ///////////////////////////////////////////////////////////////////////////////////////
    //
    // Data properties
    //
    ///////////////////////////////////////////////////////////////////////////////////////
     -->




    <!-- http://purl.org/olia/dzongkha.owl#hasTag -->

    <owl:DatatypeProperty rdf:about="http://purl.org/olia/dzongkha.owl#hasTag">
        <rdfs:domain rdf:resource="http://purl.org/olia/dzongkha.owl#Tag"/>
        <rdfs:subPropertyOf rdf:resource="&owl;topDataProperty"/>
    </owl:DatatypeProperty>



    <!-- http://www.w3.org/2002/07/owl#topDataProperty -->

    <owl:DatatypeProperty rdf:about="&owl;topDataProperty"/>



    <!--
    ///////////////////////////////////////////////////////////////////////////////////////
    //
    // Classes
    //
    ///////////////////////////////////////////////////////////////////////////////////////
     -->




    <!-- http://purl.org/olia/dzongkha.owl#AblativeCaseMarker -->

    <owl:Class rdf:about="http://purl.org/olia/dzongkha.owl#AblativeCaseMarker">
        <rdfs:subClassOf rdf:resource="http://purl.org/olia/dzongkha.owl#CaseMarker"/>
        <rdfs:comment>Concerning case, we added two subclasses of
case: CDt and CA. These differentiate between
dative (CDt) and ablative (CA): The CDt
(Dative case) labels e.g.&#3921;&#3964;&#3923;&#3851;&#3939;&#3942;&#3851;/doen le/(for it)
and &#3921;&#3964;&#3923;&#3851;&#3939;&#3851;/doen lu/(for this). The Ablative case
(CA) is used when the argument of the
preposition describes a source. For example, in
the phrase &#3940;&#3954;&#3908;&#3851;&#3939;&#3942;&#3851;&#3938;&#3908;&#3851;&#3905;&#3954;&#3851;/shing le kang thri/(from
wood chair), &#3939;&#3942;&#3851;/le/from/ will be labeled CA
since the chair described is made from (the
source) wood (Muaz, et al. 2009).
(Chungku et al. 2010)

A case, whose basic role, or one of its basic roles, is to indicate the source or origin of a person and an object.

&#3851;&#3928; &#3851; &#3939;&#3942;&#3851; &#3938;&#3851; &#3853;
Jamtsho L&#234;[CAt] Nob&#251;
ocean from jewel
&#39;A jewel from the ocean&#39;
(http://panl10n.net/english/Outputs%20Phase%202/CCs/Bhutan/Papers/2007/0701/PartOfSpeech.pdf)</rdfs:comment>
    </owl:Class>



    <!-- http://purl.org/olia/dzongkha.owl#Adjective -->

    <owl:Class rdf:about="http://purl.org/olia/dzongkha.owl#Adjective">
        <rdfs:subClassOf rdf:resource="http://purl.org/olia/dzongkha.owl#OpenClassCategory"/>
    </owl:Class>



    <!-- http://purl.org/olia/dzongkha.owl#Adposition -->

    <owl:Class rdf:about="http://purl.org/olia/dzongkha.owl#Adposition">
        <rdfs:subClassOf rdf:resource="http://purl.org/olia/dzongkha.owl#ClosedClassCategory"/>
    </owl:Class>



    <!-- http://purl.org/olia/dzongkha.owl#Adverb -->

    <owl:Class rdf:about="http://purl.org/olia/dzongkha.owl#Adverb">
        <rdfs:subClassOf rdf:resource="http://purl.org/olia/dzongkha.owl#OpenClassCategory"/>
    </owl:Class>



    <!-- http://purl.org/olia/dzongkha.owl#AffirmativeMarker -->

    <owl:Class rdf:about="http://purl.org/olia/dzongkha.owl#AffirmativeMarker">
        <rdfs:subClassOf rdf:resource="http://purl.org/olia/dzongkha.owl#Marker"/>
    </owl:Class>



    <!-- http://purl.org/olia/dzongkha.owl#AgentiveVerb -->

    <owl:Class rdf:about="http://purl.org/olia/dzongkha.owl#AgentiveVerb">
        <rdfs:subClassOf rdf:resource="http://purl.org/olia/dzongkha.owl#Verb"/>
        <rdfs:comment>An agentive verb marks the semantic role of agent or the doer of an action.

Example:
&#3851; &#3851; &#3942;&#3851; &#3851; &#3851; &#3926;&#3942;&#3921;&#3851; &#3906;&#3853;
Dorji-gi jele s&#228;nu
&#39;Dorji killed the cat&#39;
(http://panl10n.net/english/Outputs%20Phase%202/CCs/Bhutan/Papers/2007/0701/PartOfSpeech.pdf)</rdfs:comment>
    </owl:Class>



    <!-- http://purl.org/olia/dzongkha.owl#AspirationalVerb -->

    <owl:Class rdf:about="http://purl.org/olia/dzongkha.owl#AspirationalVerb">
        <rdfs:subClassOf rdf:resource="http://purl.org/olia/dzongkha.owl#Verb"/>
        <rdfs:comment>It is a verb, which indicates a strong desire to achieve something, without the doer.

&#3921;&#3906;&#3851;&#3924; &#3851; &#3908;&#3851; &#3851; &#3851;&#3926;&#3938;&#3851; &#3906;&#3853;
dag-pai zhing-lu kewa sh&#212;
&#39;May i be born in pure land&#39;
(http://panl10n.net/english/Outputs%20Phase%202/CCs/Bhutan/Papers/2007/0701/PartOfSpeech.pdf)</rdfs:comment>
    </owl:Class>



    <!-- http://purl.org/olia/dzongkha.owl#AuxiliaryVerb -->

    <owl:Class rdf:about="http://purl.org/olia/dzongkha.owl#AuxiliaryVerb">
        <rdfs:subClassOf rdf:resource="http://purl.org/olia/dzongkha.owl#Verb"/>
    </owl:Class>



    <!-- http://purl.org/olia/dzongkha.owl#BehaviouralAdverb -->

    <owl:Class rdf:about="http://purl.org/olia/dzongkha.owl#BehaviouralAdverb">
        <rdfs:subClassOf rdf:resource="http://purl.org/olia/dzongkha.owl#Adverb"/>
        <rdfs:comment>It is an adverb, that expresses the manner or behavior of any kind, whether good or bad, slow or fast etc.

&#3851;&#3923;&#3928;&#3851;&#3924;&#3851; &#3851; &#3908;&#3851;&#3923;&#3908;&#3851; &#3851;&#3936; &#3908;&#3942;&#3851; &#3851; &#3851;&#3936;&#3926;&#3921;&#3851; &#3942;&#3853;
Sonampa-tshu Zhing-na Tsagyeng-te L&#226;b&#228;d&#228;
&#39;Farmers are putting their efforts in the field&#39;
(http://panl10n.net/english/Outputs%20Phase%202/CCs/Bhutan/Papers/2007/0701/PartOfSpeech.pdf)</rdfs:comment>
    </owl:Class>



    <!-- http://purl.org/olia/dzongkha.owl#CardinalNumber -->

    <owl:Class rdf:about="http://purl.org/olia/dzongkha.owl#CardinalNumber">
        <rdfs:subClassOf rdf:resource="http://purl.org/olia/dzongkha.owl#Number"/>
    </owl:Class>



    <!-- http://purl.org/olia/dzongkha.owl#CaseMarker -->

    <owl:Class rdf:about="http://purl.org/olia/dzongkha.owl#CaseMarker">
        <rdfs:subClassOf rdf:resource="http://purl.org/olia/dzongkha.owl#ClosedClassCategory"/>
    </owl:Class>



    <!-- http://purl.org/olia/dzongkha.owl#CharacteristicAdjective -->

    <owl:Class rdf:about="http://purl.org/olia/dzongkha.owl#CharacteristicAdjective">
        <rdfs:subClassOf rdf:resource="http://purl.org/olia/dzongkha.owl#Adjective"/>
        <rdfs:comment>It is an adjective, which expresses the character and feature of subject or an object, while modifying a noun.

&#3908;&#3851;&#3936; &#3851; &#3908; &#3851; &#3936; &#3906;&#3853;
Shing-di rim du
&#39;The tree is tall&#39;
(http://panl10n.net/english/Outputs%20Phase%202/CCs/Bhutan/Papers/2007/0701/PartOfSpeech.pdf)</rdfs:comment>
    </owl:Class>



    <!-- http://purl.org/olia/dzongkha.owl#ClosedClassCategory -->

    <owl:Class rdf:about="http://purl.org/olia/dzongkha.owl#ClosedClassCategory">
        <rdfs:subClassOf rdf:resource="http://purl.org/olia/dzongkha.owl#Tag"/>
        <rdfs:comment>In Dzongkha it is mainly the function words that
are ambiguous in terms of their POS. A typical
example is le (from) belonging to the
category PP (post position) and le (so)
which is of the category CC (conjunction).</rdfs:comment>
    </owl:Class>



    <!-- http://purl.org/olia/dzongkha.owl#CombinedTag -->

    <owl:Class rdf:about="http://purl.org/olia/dzongkha.owl#CombinedTag">
        <rdfs:subClassOf rdf:resource="http://purl.org/olia/dzongkha.owl#Tag"/>
    </owl:Class>



    <!-- http://purl.org/olia/dzongkha.owl#CommonNoun -->

    <owl:Class rdf:about="http://purl.org/olia/dzongkha.owl#CommonNoun">
        <rdfs:subClassOf rdf:resource="http://purl.org/olia/dzongkha.owl#Noun"/>
    </owl:Class>



    <!-- http://purl.org/olia/dzongkha.owl#ComparativeAdjective -->

    <owl:Class rdf:about="http://purl.org/olia/dzongkha.owl#ComparativeAdjective">
        <rdfs:subClassOf rdf:resource="http://purl.org/olia/dzongkha.owl#Adjective"/>
    </owl:Class>



    <!-- http://purl.org/olia/dzongkha.owl#ComparativeAdverb -->

    <owl:Class rdf:about="http://purl.org/olia/dzongkha.owl#ComparativeAdverb">
        <rdfs:subClassOf rdf:resource="http://purl.org/olia/dzongkha.owl#Adverb"/>
    </owl:Class>



    <!-- http://purl.org/olia/dzongkha.owl#Conjunction -->

    <owl:Class rdf:about="http://purl.org/olia/dzongkha.owl#Conjunction">
        <rdfs:subClassOf rdf:resource="http://purl.org/olia/dzongkha.owl#ClosedClassCategory"/>
    </owl:Class>



    <!-- http://purl.org/olia/dzongkha.owl#CoordinateConjunction -->

    <owl:Class rdf:about="http://purl.org/olia/dzongkha.owl#CoordinateConjunction">
        <rdfs:subClassOf rdf:resource="http://purl.org/olia/dzongkha.owl#Conjunction"/>
    </owl:Class>



    <!-- http://purl.org/olia/dzongkha.owl#DativeCaseMarker -->

    <owl:Class rdf:about="http://purl.org/olia/dzongkha.owl#DativeCaseMarker">
        <rdfs:subClassOf rdf:resource="http://purl.org/olia/dzongkha.owl#CaseMarker"/>
        <rdfs:comment>Concerning case, we added two subclasses of
case: CDt and CA. These differentiate between
dative (CDt) and ablative (CA): The CDt
(Dative case) labels e.g.&#3921;&#3964;&#3923;&#3851;&#3939;&#3942;&#3851;/doen le/(for it)
and &#3921;&#3964;&#3923;&#3851;&#3939;&#3851;/doen lu/(for this). The Ablative case
(CA) is used when the argument of the
preposition describes a source. For example, in
the phrase &#3940;&#3954;&#3908;&#3851;&#3939;&#3942;&#3851;&#3938;&#3908;&#3851;&#3905;&#3954;&#3851;/shing le kang thri/(from
wood chair), &#3939;&#3942;&#3851;/le/from/ will be labeled CA
since the chair described is made from (the
source) wood (Muaz, et al. 2009).
(Chungku et al. 2010)

A case, whose basic role, or one of its basic roles, is to distinguish the recipient of something given, transferred etc.

&#3908;&#3851; &#3942;&#3851; &#3904; &#3851; &#3851; &#3851; &#3926;&#3851; &#3923;&#3851; &#3853;
Nga-gi[AuxV] Karma-lu[CD] Kideb bjeyi[past tense]
i karma to book gave
&#39;I gave the book to Karma&#39;
(http://panl10n.net/english/Outputs%20Phase%202/CCs/Bhutan/Papers/2007/0701/PartOfSpeech.pdf)</rdfs:comment>
    </owl:Class>



    <!-- http://purl.org/olia/dzongkha.owl#DefiniteDeterminer -->

    <owl:Class rdf:about="http://purl.org/olia/dzongkha.owl#DefiniteDeterminer">
        <rdfs:subClassOf rdf:resource="http://purl.org/olia/dzongkha.owl#Determiner"/>
        <rdfs:comment>An article, which is used after the subject or an object, that refers to a particular thing.

&#3851; &#3851;&#3936; &#3851; &#3851; &#3906;&#3942;&#3851; &#3928;&#3851; &#3921;&#3853;&#3936;
D&#244;ji-d&#39;i &#39;mi lezhim y&#246;
Dorji-[DA] person good be
&#39;Dorji is a good boy&#39;
(http://panl10n.net/english/Outputs%20Phase%202/CCs/Bhutan/Papers/2007/0701/PartOfSpeech.pdf)</rdfs:comment>
    </owl:Class>



    <!-- http://purl.org/olia/dzongkha.owl#Determiner -->

    <owl:Class rdf:about="http://purl.org/olia/dzongkha.owl#Determiner">
        <rdfs:subClassOf rdf:resource="http://purl.org/olia/dzongkha.owl#ClosedClassCategory"/>
        <rdfs:comment>Any of a class of grammatical units characterized by ones that are seen as limiting the potential referent of a noun phrase.
(http://panl10n.net/english/Outputs%20Phase%202/CCs/Bhutan/Papers/2007/0701/PartOfSpeech.pdf)</rdfs:comment>
    </owl:Class>



    <!-- http://purl.org/olia/dzongkha.owl#DifferentialPronoun -->

    <owl:Class rdf:about="http://purl.org/olia/dzongkha.owl#DifferentialPronoun">
        <rdfs:subClassOf rdf:resource="http://purl.org/olia/dzongkha.owl#Pronoun"/>
        <rdfs:comment>A pronoun, which classifies or differentiates(pronoun) by a single basis, like everybody; each; individual etc.

&#3936; &#3906;&#3851;&#3924; &#3851; &#3851; &#3938;&#3851; &#3906;&#3851;&#3938;&#3851; &#3923;&#3851; &#3908;&#3851; &#3908;&#3851;&#3905;&#3851; &#3942;&#3851;&#3921; &#3853;
Drupai Miser Gara Enrung Dzongkha Sheg&#212;
&#39;Every Bhutanese must know Dzongkha&#39;
(http://panl10n.net/english/Outputs%20Phase%202/CCs/Bhutan/Papers/2007/0701/PartOfSpeech.pdf)</rdfs:comment>
    </owl:Class>



    <!-- http://purl.org/olia/dzongkha.owl#GenitiveCaseMarker -->

    <owl:Class rdf:about="http://purl.org/olia/dzongkha.owl#GenitiveCaseMarker">
        <rdfs:subClassOf rdf:resource="http://purl.org/olia/dzongkha.owl#CaseMarker"/>
        <rdfs:comment>A case, whose basic role, or one of its basic roles, is to make link with the preceding noun(a person or an object).

&#3905;&#3926;&#3851; &#3851; &#3853;
khab-ki[CG] ts&#228;
needle of tip
&#39;A tip of needle&#39;
(http://panl10n.net/english/Outputs%20Phase%202/CCs/Bhutan/Papers/2007/0701/PartOfSpeech.pdf)
</rdfs:comment>
    </owl:Class>



    <!-- http://purl.org/olia/dzongkha.owl#HonorificCommonNoun -->

    <owl:Class rdf:about="http://purl.org/olia/dzongkha.owl#HonorificCommonNoun">
        <rdfs:subClassOf rdf:resource="http://purl.org/olia/dzongkha.owl#Noun"/>
        <rdfs:comment>Dzongkha uses honorific forms: &#3923;&#3851;&#3926;&#3935;&#3936;&#3851;/nam za/
(cloths) is the honorific form of the noun &#3906;&#3964;&#3851;
&#3939;&#3851;/gola/(cloths), &#3906;&#3942;&#3908;&#3942;&#3851;/sung/(tell) the honorific
form of the verb &#3942;&#3926;&#3851;/lab/(tell). We opted to mark
them by adding the tag NNH (honorific
common noun) and VBH (honorific verb) to
enable future research on this specific usage of
Dzongkha language. A number of tags were
added to the set, of which we describe four in
more detail: two of the additional tags are subclasses
of verbs: VBH (honorific verb form),
and VBN which describes past participle forms,
like, e.g. &#3926;&#3908;&#3928;&#3851;/jun/(created), the past particle
form of &#3926;&#3908;&#3851;/jung/(create).
(Chungku et al. 2010)

A noun, which indicates respect for the person being addressed, e.g., Miwang Gel-poi Yab &#8220;A king&#39;s father&#8221; [Though father=Apa, but colloquially we say YAB in Dzongkha]
(http://panl10n.net/english/Outputs%20Phase%202/CCs/Bhutan/Papers/2007/0701/PartOfSpeech.pdf)</rdfs:comment>
    </owl:Class>



    <!-- http://purl.org/olia/dzongkha.owl#HonorificVerb -->

    <owl:Class rdf:about="http://purl.org/olia/dzongkha.owl#HonorificVerb">
        <rdfs:subClassOf rdf:resource="http://purl.org/olia/dzongkha.owl#Verb"/>
        <rdfs:comment>Dzongkha uses honorific forms: &#3923;&#3851;&#3926;&#3935;&#3936;&#3851;/nam za/
(cloths) is the honorific form of the noun &#3906;&#3964;&#3851;
&#3939;&#3851;/gola/(cloths), &#3906;&#3942;&#3908;&#3942;&#3851;/sung/(tell) the honorific
form of the verb &#3942;&#3926;&#3851;/lab/(tell). We opted to mark
them by adding the tag NNH (honorific
common noun) and VBH (honorific verb) to
enable future research on this specific usage of
Dzongkha language. A number of tags were
added to the set, of which we describe four in
more detail: two of the additional tags are subclasses
of verbs: VBH (honorific verb form),
and VBN which describes past participle forms,
like, e.g. &#3926;&#3908;&#3928;&#3851;/jun/(created), the past particle
form of &#3926;&#3908;&#3851;/jung/(create).</rdfs:comment>
    </owl:Class>



    <!-- http://purl.org/olia/dzongkha.owl#ImperativeVerb -->

    <owl:Class rdf:about="http://purl.org/olia/dzongkha.owl#ImperativeVerb">
        <rdfs:subClassOf rdf:resource="http://purl.org/olia/dzongkha.owl#Verb"/>
        <rdfs:comment>Imperative verb is a mood, that expresses a command to someone or somebody.
Example:
&#3851; &#3851; &#3942;&#3851; &#3906;&#3853;
yigu drish
&#39;write a letter&#39;
(http://panl10n.net/english/Outputs%20Phase%202/CCs/Bhutan/Papers/2007/0701/PartOfSpeech.pdf)</rdfs:comment>
    </owl:Class>



    <!-- http://purl.org/olia/dzongkha.owl#IndefiniteDeterminer -->

    <owl:Class rdf:about="http://purl.org/olia/dzongkha.owl#IndefiniteDeterminer">
        <rdfs:subClassOf rdf:resource="http://purl.org/olia/dzongkha.owl#Determiner"/>
        <rdfs:comment>An article, which is used after the subject or an object, that doesn&#39;t refer to a particular thing, but simply refer to an individual or individuals of the noun in a broad sense.

&#3851;&#3939;&#3851; &#3851; &#3906; &#3942;&#3851; &#3926;&#3851;&#3928;&#3942;&#3853; &#3906;&#3851;
&#39;Mi lalu ce[IA]-gi &#39;labm&#228;
people some-[IA](AuxV) say be
&#39;Some people say...&#39;
(http://panl10n.net/english/Outputs%20Phase%202/CCs/Bhutan/Papers/2007/0701/PartOfSpeech.pdf)</rdfs:comment>
    </owl:Class>



    <!-- http://purl.org/olia/dzongkha.owl#Interjection -->

    <owl:Class rdf:about="http://purl.org/olia/dzongkha.owl#Interjection">
        <rdfs:subClassOf rdf:resource="http://purl.org/olia/dzongkha.owl#OpenClassCategory"/>
    </owl:Class>



    <!-- http://purl.org/olia/dzongkha.owl#InterrogativeMarker -->

    <owl:Class rdf:about="http://purl.org/olia/dzongkha.owl#InterrogativeMarker">
        <rdfs:subClassOf rdf:resource="http://purl.org/olia/dzongkha.owl#Marker"/>
        <rdfs:comment>Example:

&#3921;&#3851; &#3906;&#3851; &#3851; &#3936; &#3851; &#3851; &#3853;
Ch&#246; gat&#39;&#228; joni mo
you where going-[IrD]
&#39;Where are you going?&#39;

&#3921;&#3851; &#3851;&#3936;&#3926;&#3921;&#3933;&#3851; &#3923;&#3851;&#3923;&#3853;
Ch&#246; l&#226; b&#228;yi &#39;in&#226;
you work do be-[IdI]
&#39;Are you working?&#39;
(http://panl10n.net/english/Outputs%20Phase%202/CCs/Bhutan/Papers/2007/0701/PartOfSpeech.pdf)

</rdfs:comment>
    </owl:Class>



    <!-- http://purl.org/olia/dzongkha.owl#LocativePronoun -->

    <owl:Class rdf:about="http://purl.org/olia/dzongkha.owl#LocativePronoun">
        <rdfs:subClassOf rdf:resource="http://purl.org/olia/dzongkha.owl#Pronoun"/>
        <rdfs:comment>A Locative pronoun is a pronoun, which locates the object of a noun or place of anything.

&#3851; &#3923;&#3851; &#3906;&#3942;&#3851; &#3908;&#3851; &#3851; &#3906;&#3853;
N&#226;[LP] Ph&#220;ntsho&#39;ling-lu Sh&#212;
&#39;Come here at Phuntsholing&#39;
(http://panl10n.net/english/Outputs%20Phase%202/CCs/Bhutan/Papers/2007/0701/PartOfSpeech.pdf)</rdfs:comment>
    </owl:Class>



    <!-- http://purl.org/olia/dzongkha.owl#Marker -->

    <owl:Class rdf:about="http://purl.org/olia/dzongkha.owl#Marker">
        <rdfs:subClassOf rdf:resource="http://purl.org/olia/dzongkha.owl#ClosedClassCategory"/>
    </owl:Class>



    <!-- http://purl.org/olia/dzongkha.owl#ModalVerb -->

    <owl:Class rdf:about="http://purl.org/olia/dzongkha.owl#ModalVerb">
        <rdfs:subClassOf rdf:resource="http://purl.org/olia/dzongkha.owl#Verb"/>
    </owl:Class>



    <!-- http://purl.org/olia/dzongkha.owl#Negator -->

    <owl:Class rdf:about="http://purl.org/olia/dzongkha.owl#Negator">
        <rdfs:subClassOf rdf:resource="http://purl.org/olia/dzongkha.owl#ClosedClassCategory"/>
    </owl:Class>



    <!-- http://purl.org/olia/dzongkha.owl#NominalNumber -->

    <owl:Class rdf:about="http://purl.org/olia/dzongkha.owl#NominalNumber">
        <rdfs:subClassOf rdf:resource="http://purl.org/olia/dzongkha.owl#Number"/>
        <rdfs:comment>Nominal numbers are used to identify or refer the things. It does not show the quantity or rank.

Example:
&#3908;&#3962;&#3851;&#3906;&#3954;&#3851; &#3936;&#3906;&#3939;&#3851;&#3936;&#3925;&#3954;&#3923;&#3851; &#3944;&#3908;&#3851;&#3906;&#3908;&#3942;&#3851; &#3936;&#3921;&#3954;&#3851; &#3873;&#3879;&#3878;&#3876;&#3881;&#3872;&#3875;&#3879; &#3944;&#3954;&#3923;&#3853;
NGIGI DRUELTHRIN ANGDRANG &#39;DI 17649037 INN
my mobile number is 17649037 be
&#8220; My mobile number is 17649037.&#8221;
(Jurmey Rabgay, email Sep 20, 2010)</rdfs:comment>
    </owl:Class>



    <!-- http://purl.org/olia/dzongkha.owl#NonAgentiveVerb -->

    <owl:Class rdf:about="http://purl.org/olia/dzongkha.owl#NonAgentiveVerb">
        <rdfs:subClassOf rdf:resource="http://purl.org/olia/dzongkha.owl#Verb"/>
        <rdfs:comment>A non-agentive verb is a type of verb, which indicates an action without the doer.

Example:
&#3908;&#3851;&#3928;&#3851; &#3936; &#3938;&#3851; &#3942;&#3853;
&#39;lungma phur-d&#228;
&#39;A wind is blowing&#39;
(http://panl10n.net/english/Outputs%20Phase%202/CCs/Bhutan/Papers/2007/0701/PartOfSpeech.pdf)</rdfs:comment>
    </owl:Class>



    <!-- http://purl.org/olia/dzongkha.owl#Noun -->

    <owl:Class rdf:about="http://purl.org/olia/dzongkha.owl#Noun">
        <rdfs:subClassOf rdf:resource="http://purl.org/olia/dzongkha.owl#OpenClassCategory"/>
    </owl:Class>



    <!-- http://purl.org/olia/dzongkha.owl#Number -->

    <owl:Class rdf:about="http://purl.org/olia/dzongkha.owl#Number">
        <rdfs:subClassOf rdf:resource="http://purl.org/olia/dzongkha.owl#ClosedClassCategory"/>
    </owl:Class>



    <!-- http://purl.org/olia/dzongkha.owl#OpenClassCategory -->

    <owl:Class rdf:about="http://purl.org/olia/dzongkha.owl#OpenClassCategory">
        <rdfs:subClassOf rdf:resource="http://purl.org/olia/dzongkha.owl#Tag"/>
    </owl:Class>



    <!-- http://purl.org/olia/dzongkha.owl#OrdinalNumber -->

    <owl:Class rdf:about="http://purl.org/olia/dzongkha.owl#OrdinalNumber">
        <rdfs:subClassOf rdf:resource="http://purl.org/olia/dzongkha.owl#Number"/>
    </owl:Class>



    <!-- http://purl.org/olia/dzongkha.owl#ParticularPersonNoun -->

    <owl:Class rdf:about="http://purl.org/olia/dzongkha.owl#ParticularPersonNoun">
        <rdfs:subClassOf rdf:resource="http://purl.org/olia/dzongkha.owl#Noun"/>
        <rdfs:comment>A name, which particularly focusses to a particular thing, e.g., &#8220;Jigme Singye Wangchuk&#8221; (the Fourth King of Bhutan)
(http://panl10n.net/english/Outputs%20Phase%202/CCs/Bhutan/Papers/2007/0701/PartOfSpeech.pdf)</rdfs:comment>
    </owl:Class>



    <!-- http://purl.org/olia/dzongkha.owl#PastParticiple -->

    <owl:Class rdf:about="http://purl.org/olia/dzongkha.owl#PastParticiple">
        <rdfs:subClassOf rdf:resource="http://purl.org/olia/dzongkha.owl#Verb"/>
        <rdfs:comment>The past participle expresses an event which precedes the event, denoted by the main verb.

&#3908;&#3851; &#3921;&#3926;&#3908;&#3851;&#3936; &#3942;&#3851; &#3851; &#3908;&#3851; &#3851; &#3921;&#3904;&#3936;&#3851;&#3908;&#3939;&#3851; &#3926;&#3851; &#3853;
Nga &#39;Wangd&#252;-lu Song-di Kany&#228; Thopce
i wangd&#39;i-to-[prep] go-[pp] problem get-[pt]
&#39;Having gone to &#39;Wangdi, I ran into a problem&#39;
(http://panl10n.net/english/Outputs%20Phase%202/CCs/Bhutan/Papers/2007/0701/PartOfSpeech.pdf)</rdfs:comment>
    </owl:Class>



    <!-- http://purl.org/olia/dzongkha.owl#PeriodicAdjective -->

    <owl:Class rdf:about="http://purl.org/olia/dzongkha.owl#PeriodicAdjective">
        <rdfs:subClassOf rdf:resource="http://purl.org/olia/dzongkha.owl#Adjective"/>
        <rdfs:comment>It is an adjective, which expresses the time or period of the circumstances, while modifying a noun.

&#3923;&#3851; &#3908;&#3851; &#3908;&#3851; &#3851; &#3939;&#3851; &#3851; &#3936; &#3851; &#3853;
Nahing Nga chigyel-lu joyi
&#39;I went abroad last year&#39;
(http://panl10n.net/english/Outputs%20Phase%202/CCs/Bhutan/Papers/2007/0701/PartOfSpeech.pdf)</rdfs:comment>
    </owl:Class>



    <!-- http://purl.org/olia/dzongkha.owl#PersonalPronoun -->

    <owl:Class rdf:about="http://purl.org/olia/dzongkha.owl#PersonalPronoun">
        <rdfs:subClassOf rdf:resource="http://purl.org/olia/dzongkha.owl#Pronoun"/>
    </owl:Class>



    <!-- http://purl.org/olia/dzongkha.owl#PluralNoun -->

    <owl:Class rdf:about="http://purl.org/olia/dzongkha.owl#PluralNoun">
        <rdfs:subClassOf rdf:resource="http://purl.org/olia/dzongkha.owl#Noun"/>
    </owl:Class>



    <!-- http://purl.org/olia/dzongkha.owl#PossessiveDeterminer -->

    <owl:Class rdf:about="http://purl.org/olia/dzongkha.owl#PossessiveDeterminer">
        <rdfs:subClassOf rdf:resource="http://purl.org/olia/dzongkha.owl#Determiner"/>
        <rdfs:comment>An article, that modifies a noun by attributing possession to some one or something.

&#3851; &#3851; &#3851; &#3926;&#3853;
Ng&#228;-gi kid&#39;eb
my[PsA] book
&#39;My book&#39;
(http://panl10n.net/english/Outputs%20Phase%202/CCs/Bhutan/Papers/2007/0701/PartOfSpeech.pdf)</rdfs:comment>
    </owl:Class>



    <!-- http://purl.org/olia/dzongkha.owl#Postposition -->

    <owl:Class rdf:about="http://purl.org/olia/dzongkha.owl#Postposition">
        <rdfs:subClassOf rdf:resource="http://purl.org/olia/dzongkha.owl#Adposition"/>
        <rdfs:comment>As an example for such dissimilarity [between the Penn Treebank tagset and the Dzongkha tagset -- CC], Dzongkha postpositions are mentioned here, cf. (1); the respective tag (PP) only exist for Dzongkha whereas in English the whole set of ad position tags (preposition and postpositions) exist.
(1) j&#39;ili shing-gi w&#244;lu -d&#251;
Cat tree[posp] under[PP] be
&#39;&#39;A cat is under the tree&#39;&#39;
(Chungku et al. 2010)

An element related to a noun phrase in the same way as a preposition, except that it comes after instead of before. Dzongkha is a postpositional language.

&#3851; &#3851; &#3908;&#3851; &#3851; &#3906;&#3851; &#3851;&#3936; &#3906;&#3853;
j&#39;ili shing-gi w&#244;lu-d&#251;
cat tree-[posp] under-[PP] be
&#39;A cat is under the tree&#39;
(http://panl10n.net/english/Outputs%20Phase%202/CCs/Bhutan/Papers/2007/0701/PartOfSpeech.pdf)</rdfs:comment>
    </owl:Class>



    <!-- http://purl.org/olia/dzongkha.owl#Pronoun -->

    <owl:Class rdf:about="http://purl.org/olia/dzongkha.owl#Pronoun">
        <rdfs:subClassOf rdf:resource="http://purl.org/olia/dzongkha.owl#ClosedClassCategory"/>
    </owl:Class>



    <!-- http://purl.org/olia/dzongkha.owl#Punctuation -->

    <owl:Class rdf:about="http://purl.org/olia/dzongkha.owl#Punctuation">
        <rdfs:subClassOf rdf:resource="http://purl.org/olia/dzongkha.owl#ClosedClassCategory"/>
    </owl:Class>



    <!-- http://purl.org/olia/dzongkha.owl#QuantifierNoun -->

    <owl:Class rdf:about="http://purl.org/olia/dzongkha.owl#QuantifierNoun">
        <rdfs:subClassOf rdf:resource="http://purl.org/olia/dzongkha.owl#Noun"/>
        <rdfs:comment>A noun which quantifies one or more things, regardless of subject and an object.

&#3908;&#3851;&#3906;&#3954;&#3942;&#3851; &#3926;&#3928;&#3964;&#3851; &#3939;&#3851; &#3921;&#3908;&#3851; &#3925;&#3921;&#3851;&#3909;&#3954;&#3853;
NGAGI BUM &#39;NGA &#39;DA CHECI
I girl five with met
&#8220;I met with five girls.&#8221;
(Jurmey Rabgay, email Sep 20, 2010)</rdfs:comment>
    </owl:Class>



    <!-- http://purl.org/olia/dzongkha.owl#ReflexivePronoun -->

    <owl:Class rdf:about="http://purl.org/olia/dzongkha.owl#ReflexivePronoun">
        <rdfs:subClassOf rdf:resource="http://purl.org/olia/dzongkha.owl#Pronoun"/>
        <rdfs:comment>A Reflexive pronoun is something one is doing to or for oneself and it applies to the above subjective pronoun, common pronoun etc.

&#3921;&#3851;&#3938;&#3851;&#3938;&#3908;&#3851; &#3851; &#3942;&#3851;&#3924;&#3942;&#3853;
Ch&#246;-rarang Mish&#234;-p&#228;
&#39;Yourself don&#39;t know&#39;
(http://panl10n.net/english/Outputs%20Phase%202/CCs/Bhutan/Papers/2007/0701/PartOfSpeech.pdf)</rdfs:comment>
    </owl:Class>



    <!-- http://purl.org/olia/dzongkha.owl#SubordinateConjunction -->

    <owl:Class rdf:about="http://purl.org/olia/dzongkha.owl#SubordinateConjunction">
        <rdfs:subClassOf rdf:resource="http://purl.org/olia/dzongkha.owl#Conjunction"/>
    </owl:Class>



    <!-- http://purl.org/olia/dzongkha.owl#SuperlativeAdjective -->

    <owl:Class rdf:about="http://purl.org/olia/dzongkha.owl#SuperlativeAdjective">
        <rdfs:subClassOf rdf:resource="http://purl.org/olia/dzongkha.owl#Adjective"/>
    </owl:Class>



    <!-- http://purl.org/olia/dzongkha.owl#SuperlativeAdverb -->

    <owl:Class rdf:about="http://purl.org/olia/dzongkha.owl#SuperlativeAdverb">
        <rdfs:subClassOf rdf:resource="http://purl.org/olia/dzongkha.owl#Adverb"/>
    </owl:Class>



    <!-- http://purl.org/olia/dzongkha.owl#Tag -->

    <owl:Class rdf:about="http://purl.org/olia/dzongkha.owl#Tag">
        <rdfs:subClassOf>
            <owl:Restriction>
                <owl:onProperty rdf:resource="http://purl.org/olia/dzongkha.owl#hasTag"/>
                <owl:minCardinality rdf:datatype="&xsd;nonNegativeInteger">1</owl:minCardinality>
            </owl:Restriction>
        </rdfs:subClassOf>
        <rdfs:comment>Examining the similar features exhibited by
both the languages (Dzongkha and English),
tags that were applicable to Dzongkha were
taken directly from the Penn Treebank. In cases
where these languages showed dissimilarities in
their nature, new tags for Dzongkha were
assigned</rdfs:comment>
    </owl:Class>



    <!-- http://purl.org/olia/dzongkha.owl#TenseMarker -->

    <owl:Class rdf:about="http://purl.org/olia/dzongkha.owl#TenseMarker">
        <rdfs:subClassOf rdf:resource="http://purl.org/olia/dzongkha.owl#Marker"/>
        <rdfs:comment>Dzongkha has also a tense marker, which is not complicated like in other languages. It has got only six tense markers and can be used in a very simple and effective way. They are: (&#39;Ni&#39;+&#39;Wong&#39;) for future, (&#39;D&#39;o&#39;+&#39;D&#39;&#228;&#39;) for present and (&#39;Ci&#39;+&#39;Yi&#39;) for past tense.

&#3908;&#3851; &#3923;&#3908;&#3942;&#3851;&#3924;&#3851; &#3936; &#3851; &#3853;
Nga naba jo-ni[past tense]
I tomorrow go-will-[past]
&#39;I am going tomorrow&#39;
(http://panl10n.net/english/Outputs%20Phase%202/CCs/Bhutan/Papers/2007/0701/PartOfSpeech.pdf)</rdfs:comment>
    </owl:Class>



    <!-- http://purl.org/olia/dzongkha.owl#Verb -->

    <owl:Class rdf:about="http://purl.org/olia/dzongkha.owl#Verb">
        <rdfs:subClassOf rdf:resource="http://purl.org/olia/dzongkha.owl#ClosedClassCategory"/>
    </owl:Class>



    <!-- http://purl.org/olia/dzongkha.owl#VocativeCaseMarker -->

    <owl:Class rdf:about="http://purl.org/olia/dzongkha.owl#VocativeCaseMarker">
        <rdfs:subClassOf rdf:resource="http://purl.org/olia/dzongkha.owl#CaseMarker"/>
        <rdfs:comment>A case, whose basic role, or one of its basic roles, is to address or invoke a person or thing.

&#3921;&#3926; ! &#3851; &#3906;&#3853;
&#39;W&#228; N&#226;sh&#212;
heyi-[CV], here come
&#39;Hey, come here!&#39;
(http://panl10n.net/english/Outputs%20Phase%202/CCs/Bhutan/Papers/2007/0701/PartOfSpeech.pdf)

</rdfs:comment>
    </owl:Class>



    <!--
    ///////////////////////////////////////////////////////////////////////////////////////
    //
    // Individuals
    //
    ///////////////////////////////////////////////////////////////////////////////////////
     -->




    <!-- http://purl.org/olia/dzongkha.owl#AM -->

    <owl:NamedIndividual rdf:about="http://purl.org/olia/dzongkha.owl#AM">
        <rdf:type rdf:resource="http://purl.org/olia/dzongkha.owl#AffirmativeMarker"/>
        <rdfs:comment>Marker, Affirmative</rdfs:comment>
        <hasTag>AM</hasTag>
    </owl:NamedIndividual>



    <!-- http://purl.org/olia/dzongkha.owl#AMSC -->

    <owl:NamedIndividual rdf:about="http://purl.org/olia/dzongkha.owl#AMSC">
        <rdf:type rdf:resource="http://purl.org/olia/dzongkha.owl#AffirmativeMarker"/>
        <rdf:type rdf:resource="http://purl.org/olia/dzongkha.owl#CombinedTag"/>
        <rdf:type rdf:resource="http://purl.org/olia/dzongkha.owl#SubordinateConjunction"/>
        <hasTag>AMSC</hasTag>
        <rdfs:comment>Affirmative + Subordinate Conjunction</rdfs:comment>
    </owl:NamedIndividual>



    <!-- http://purl.org/olia/dzongkha.owl#CA -->

    <owl:NamedIndividual rdf:about="http://purl.org/olia/dzongkha.owl#CA">
        <rdf:type rdf:resource="http://purl.org/olia/dzongkha.owl#AblativeCaseMarker"/>
        <rdfs:comment>Case marker, Ablative case</rdfs:comment>
        <rdfs:comment>Concerning case, we added two subclasses of
case: CDt and CA. These differentiate between
dative (CDt) and ablative (CA): The CDt
(Dative case) labels e.g.&#3921;&#3964;&#3923;&#3851;&#3939;&#3942;&#3851;/doen le/(for it)
and &#3921;&#3964;&#3923;&#3851;&#3939;&#3851;/doen lu/(for this). The Ablative case
(CA) is used when the argument of the
preposition describes a source. For example, in
the phrase &#3940;&#3954;&#3908;&#3851;&#3939;&#3942;&#3851;&#3938;&#3908;&#3851;&#3905;&#3954;&#3851;/shing le kang thri/(from
wood chair), &#3939;&#3942;&#3851;/le/from/ will be labeled CA
since the chair described is made from (the
source) wood (Muaz, et al. 2009).</rdfs:comment>
        <hasTag>CA</hasTag>
    </owl:NamedIndividual>



    <!-- http://purl.org/olia/dzongkha.owl#CC -->

    <owl:NamedIndividual rdf:about="http://purl.org/olia/dzongkha.owl#CC">
        <rdf:type rdf:resource="http://purl.org/olia/dzongkha.owl#CoordinateConjunction"/>
        <rdfs:comment>Conjunction, Coordinate</rdfs:comment>
        <hasTag>CC</hasTag>
    </owl:NamedIndividual>



    <!-- http://purl.org/olia/dzongkha.owl#CD -->

    <owl:NamedIndividual rdf:about="http://purl.org/olia/dzongkha.owl#CD">
        <rdf:type rdf:resource="http://purl.org/olia/dzongkha.owl#CardinalNumber"/>
        <hasTag>CD</hasTag>
        <rdfs:comment>Number, Cardinal</rdfs:comment>
    </owl:NamedIndividual>



    <!-- http://purl.org/olia/dzongkha.owl#CDt -->

    <owl:NamedIndividual rdf:about="http://purl.org/olia/dzongkha.owl#CDt">
        <rdf:type rdf:resource="http://purl.org/olia/dzongkha.owl#DativeCaseMarker"/>
        <rdfs:comment>Case marker, Dative case</rdfs:comment>
        <rdfs:comment>Concerning case, we added two subclasses of
case: CDt and CA. These differentiate between
dative (CDt) and ablative (CA): The CDt
(Dative case) labels e.g.&#3921;&#3964;&#3923;&#3851;&#3939;&#3942;&#3851;/doen le/(for it)
and &#3921;&#3964;&#3923;&#3851;&#3939;&#3851;/doen lu/(for this). The Ablative case
(CA) is used when the argument of the
preposition describes a source. For example, in
the phrase &#3940;&#3954;&#3908;&#3851;&#3939;&#3942;&#3851;&#3938;&#3908;&#3851;&#3905;&#3954;&#3851;/shing le kang thri/(from
wood chair), &#3939;&#3942;&#3851;/le/from/ will be labeled CA
since the chair described is made from (the
source) wood (Muaz, et al. 2009).</rdfs:comment>
        <hasTag>CDt</hasTag>
    </owl:NamedIndividual>



    <!-- http://purl.org/olia/dzongkha.owl#CG -->

    <owl:NamedIndividual rdf:about="http://purl.org/olia/dzongkha.owl#CG">
        <rdf:type rdf:resource="http://purl.org/olia/dzongkha.owl#GenitiveCaseMarker"/>
        <hasTag>CG</hasTag>
        <rdfs:comment>Case marker, Genitive case</rdfs:comment>
    </owl:NamedIndividual>



    <!-- http://purl.org/olia/dzongkha.owl#CV -->

    <owl:NamedIndividual rdf:about="http://purl.org/olia/dzongkha.owl#CV">
        <rdf:type rdf:resource="http://purl.org/olia/dzongkha.owl#VocativeCaseMarker"/>
        <hasTag>CV</hasTag>
        <rdfs:comment>Case marker, Vocative case</rdfs:comment>
    </owl:NamedIndividual>



    <!-- http://purl.org/olia/dzongkha.owl#DT -->

    <owl:NamedIndividual rdf:about="http://purl.org/olia/dzongkha.owl#DT">
        <rdf:type rdf:resource="http://purl.org/olia/dzongkha.owl#DefiniteDeterminer"/>
        <rdfs:comment>Determiner, Definite</rdfs:comment>
        <hasTag>DT</hasTag>
    </owl:NamedIndividual>



    <!-- http://purl.org/olia/dzongkha.owl#DTCG -->

    <owl:NamedIndividual rdf:about="http://purl.org/olia/dzongkha.owl#DTCG">
        <rdf:type rdf:resource="http://purl.org/olia/dzongkha.owl#CombinedTag"/>
        <rdf:type rdf:resource="http://purl.org/olia/dzongkha.owl#DefiniteDeterminer"/>
        <rdf:type rdf:resource="http://purl.org/olia/dzongkha.owl#GenitiveCaseMarker"/>
        <hasTag>DTCG</hasTag>
        <rdfs:comment>DefiniteDeterminer + Genitive case</rdfs:comment>
    </owl:NamedIndividual>



    <!-- http://purl.org/olia/dzongkha.owl#DTDOLLAR -->

    <owl:NamedIndividual rdf:about="http://purl.org/olia/dzongkha.owl#DTDOLLAR">
        <rdf:type rdf:resource="http://purl.org/olia/dzongkha.owl#PossessiveDeterminer"/>
        <rdfs:comment>Determiner, Possessive</rdfs:comment>
        <hasTag>DT$</hasTag>
    </owl:NamedIndividual>



    <!-- http://purl.org/olia/dzongkha.owl#DTI -->

    <owl:NamedIndividual rdf:about="http://purl.org/olia/dzongkha.owl#DTI">
        <rdf:type rdf:resource="http://purl.org/olia/dzongkha.owl#IndefiniteDeterminer"/>
        <hasTag>DTI</hasTag>
        <rdfs:comment>Determiner, Indefinite</rdfs:comment>
    </owl:NamedIndividual>



    <!-- http://purl.org/olia/dzongkha.owl#IrM -->

    <owl:NamedIndividual rdf:about="http://purl.org/olia/dzongkha.owl#IrM">
        <rdf:type rdf:resource="http://purl.org/olia/dzongkha.owl#InterrogativeMarker"/>
        <hasTag>IrM</hasTag>
        <rdfs:comment>Marker, Interrogative</rdfs:comment>
    </owl:NamedIndividual>



    <!-- http://purl.org/olia/dzongkha.owl#JJ -->

    <owl:NamedIndividual rdf:about="http://purl.org/olia/dzongkha.owl#JJ">
        <rdf:type rdf:resource="http://purl.org/olia/dzongkha.owl#Adjective"/>
        <rdfs:comment>Adjective, Adjective</rdfs:comment>
        <hasTag>JJ</hasTag>
    </owl:NamedIndividual>



    <!-- http://purl.org/olia/dzongkha.owl#JJCG -->

    <owl:NamedIndividual rdf:about="http://purl.org/olia/dzongkha.owl#JJCG">
        <rdf:type rdf:resource="http://purl.org/olia/dzongkha.owl#Adjective"/>
        <rdf:type rdf:resource="http://purl.org/olia/dzongkha.owl#CombinedTag"/>
        <rdf:type rdf:resource="http://purl.org/olia/dzongkha.owl#GenitiveCaseMarker"/>
        <rdfs:comment>Adjective+CG</rdfs:comment>
        <hasTag>JJCG</hasTag>
    </owl:NamedIndividual>



    <!-- http://purl.org/olia/dzongkha.owl#JJCt -->

    <owl:NamedIndividual rdf:about="http://purl.org/olia/dzongkha.owl#JJCt">
        <rdf:type rdf:resource="http://purl.org/olia/dzongkha.owl#CharacteristicAdjective"/>
        <rdfs:comment>Adjective, Characteristic</rdfs:comment>
        <hasTag>JJCt</hasTag>
    </owl:NamedIndividual>



    <!-- http://purl.org/olia/dzongkha.owl#JJCtCG -->

    <owl:NamedIndividual rdf:about="http://purl.org/olia/dzongkha.owl#JJCtCG">
        <rdf:type rdf:resource="http://purl.org/olia/dzongkha.owl#CharacteristicAdjective"/>
        <rdf:type rdf:resource="http://purl.org/olia/dzongkha.owl#CombinedTag"/>
        <rdf:type rdf:resource="http://purl.org/olia/dzongkha.owl#GenitiveCaseMarker"/>
        <hasTag>JJCtCG</hasTag>
        <rdfs:comment>Adjective, Characteristic + Genitive case</rdfs:comment>
    </owl:NamedIndividual>



    <!-- http://purl.org/olia/dzongkha.owl#JJP -->

    <owl:NamedIndividual rdf:about="http://purl.org/olia/dzongkha.owl#JJP">
        <rdf:type rdf:resource="http://purl.org/olia/dzongkha.owl#PeriodicAdjective"/>
        <hasTag>JJP</hasTag>
        <rdfs:comment>Adjective, Periodic</rdfs:comment>
    </owl:NamedIndividual>



    <!-- http://purl.org/olia/dzongkha.owl#JJPCG -->

    <owl:NamedIndividual rdf:about="http://purl.org/olia/dzongkha.owl#JJPCG">
        <rdf:type rdf:resource="http://purl.org/olia/dzongkha.owl#CombinedTag"/>
        <rdf:type rdf:resource="http://purl.org/olia/dzongkha.owl#GenitiveCaseMarker"/>
        <rdf:type rdf:resource="http://purl.org/olia/dzongkha.owl#PeriodicAdjective"/>
        <hasTag>JJPCG</hasTag>
        <rdfs:comment>Adjective, Periodic + Genitive case</rdfs:comment>
    </owl:NamedIndividual>



    <!-- http://purl.org/olia/dzongkha.owl#JJR -->

    <owl:NamedIndividual rdf:about="http://purl.org/olia/dzongkha.owl#JJR">
        <rdf:type rdf:resource="http://purl.org/olia/dzongkha.owl#ComparativeAdjective"/>
        <rdfs:comment>Adjective, Comparative</rdfs:comment>
        <hasTag>JJR</hasTag>
    </owl:NamedIndividual>



    <!-- http://purl.org/olia/dzongkha.owl#JJS -->

    <owl:NamedIndividual rdf:about="http://purl.org/olia/dzongkha.owl#JJS">
        <rdf:type rdf:resource="http://purl.org/olia/dzongkha.owl#SuperlativeAdjective"/>
        <hasTag>JJS</hasTag>
        <rdfs:comment>Adjective, Superlative</rdfs:comment>
    </owl:NamedIndividual>



    <!-- http://purl.org/olia/dzongkha.owl#ND -->

    <owl:NamedIndividual rdf:about="http://purl.org/olia/dzongkha.owl#ND">
        <rdf:type rdf:resource="http://purl.org/olia/dzongkha.owl#NominalNumber"/>
        <rdfs:comment>Number, Nominal</rdfs:comment>
        <hasTag>ND</hasTag>
    </owl:NamedIndividual>



    <!-- http://purl.org/olia/dzongkha.owl#NEG -->

    <owl:NamedIndividual rdf:about="http://purl.org/olia/dzongkha.owl#NEG">
        <rdf:type rdf:resource="http://purl.org/olia/dzongkha.owl#Negator"/>
        <hasTag>NEG</hasTag>
        <rdfs:comment>Negator</rdfs:comment>
    </owl:NamedIndividual>



    <!-- http://purl.org/olia/dzongkha.owl#NEGCG -->

    <owl:NamedIndividual rdf:about="http://purl.org/olia/dzongkha.owl#NEGCG">
        <rdf:type rdf:resource="http://purl.org/olia/dzongkha.owl#CombinedTag"/>
        <rdf:type rdf:resource="http://purl.org/olia/dzongkha.owl#GenitiveCaseMarker"/>
        <rdf:type rdf:resource="http://purl.org/olia/dzongkha.owl#Negator"/>
        <rdfs:comment>Negator + Genitive case</rdfs:comment>
        <hasTag>NEGCG</hasTag>
    </owl:NamedIndividual>



    <!-- http://purl.org/olia/dzongkha.owl#NEGSC -->

    <owl:NamedIndividual rdf:about="http://purl.org/olia/dzongkha.owl#NEGSC">
        <rdf:type rdf:resource="http://purl.org/olia/dzongkha.owl#CombinedTag"/>
        <rdf:type rdf:resource="http://purl.org/olia/dzongkha.owl#Negator"/>
        <rdf:type rdf:resource="http://purl.org/olia/dzongkha.owl#SubordinateConjunction"/>
        <rdfs:comment>Negator + Subordinate Conjunction</rdfs:comment>
        <hasTag>NEGSC</hasTag>
    </owl:NamedIndividual>



    <!-- http://purl.org/olia/dzongkha.owl#NN -->

    <owl:NamedIndividual rdf:about="http://purl.org/olia/dzongkha.owl#NN">
        <rdf:type rdf:resource="http://purl.org/olia/dzongkha.owl#CommonNoun"/>
        <hasTag>NN</hasTag>
        <rdfs:comment>Noun, Common Noun</rdfs:comment>
    </owl:NamedIndividual>



    <!-- http://purl.org/olia/dzongkha.owl#NNCG -->

    <owl:NamedIndividual rdf:about="http://purl.org/olia/dzongkha.owl#NNCG">
        <rdf:type rdf:resource="http://purl.org/olia/dzongkha.owl#CombinedTag"/>
        <rdf:type rdf:resource="http://purl.org/olia/dzongkha.owl#CommonNoun"/>
        <rdf:type rdf:resource="http://purl.org/olia/dzongkha.owl#GenitiveCaseMarker"/>
        <rdfs:comment>Noun, Common + Genitive case</rdfs:comment>
        <hasTag>NNCG</hasTag>
    </owl:NamedIndividual>



    <!-- http://purl.org/olia/dzongkha.owl#NNH -->

    <owl:NamedIndividual rdf:about="http://purl.org/olia/dzongkha.owl#NNH">
        <rdf:type rdf:resource="http://purl.org/olia/dzongkha.owl#HonorificCommonNoun"/>
        <rdfs:comment>Noun, honorific form</rdfs:comment>
        <hasTag>NNH</hasTag>
    </owl:NamedIndividual>



    <!-- http://purl.org/olia/dzongkha.owl#NNP -->

    <owl:NamedIndividual rdf:about="http://purl.org/olia/dzongkha.owl#NNP">
        <rdf:type rdf:resource="http://purl.org/olia/dzongkha.owl#ParticularPersonNoun"/>
        <rdfs:comment>Noun, Particular/Person</rdfs:comment>
        <hasTag>NNP</hasTag>
    </owl:NamedIndividual>



    <!-- http://purl.org/olia/dzongkha.owl#NNPCG -->

    <owl:NamedIndividual rdf:about="http://purl.org/olia/dzongkha.owl#NNPCG">
        <rdf:type rdf:resource="http://purl.org/olia/dzongkha.owl#CombinedTag"/>
        <rdf:type rdf:resource="http://purl.org/olia/dzongkha.owl#GenitiveCaseMarker"/>
        <rdf:type rdf:resource="http://purl.org/olia/dzongkha.owl#ParticularPersonNoun"/>
        <hasTag>NNPCG</hasTag>
        <rdfs:comment>Noun, Particular + Genitive case</rdfs:comment>
    </owl:NamedIndividual>



    <!-- http://purl.org/olia/dzongkha.owl#NNQ -->

    <owl:NamedIndividual rdf:about="http://purl.org/olia/dzongkha.owl#NNQ">
        <rdf:type rdf:resource="http://purl.org/olia/dzongkha.owl#QuantifierNoun"/>
        <hasTag>NNQ</hasTag>
        <rdfs:comment>Noun, Quantifier</rdfs:comment>
    </owl:NamedIndividual>



    <!-- http://purl.org/olia/dzongkha.owl#NNQCG -->

    <owl:NamedIndividual rdf:about="http://purl.org/olia/dzongkha.owl#NNQCG">
        <rdf:type rdf:resource="http://purl.org/olia/dzongkha.owl#CombinedTag"/>
        <rdf:type rdf:resource="http://purl.org/olia/dzongkha.owl#GenitiveCaseMarker"/>
        <rdf:type rdf:resource="http://purl.org/olia/dzongkha.owl#QuantifierNoun"/>
        <rdfs:comment>Noun, Quantifier + Genitive case</rdfs:comment>
        <hasTag>NNQCG</hasTag>
    </owl:NamedIndividual>



    <!-- http://purl.org/olia/dzongkha.owl#NNS -->

    <owl:NamedIndividual rdf:about="http://purl.org/olia/dzongkha.owl#NNS">
        <rdf:type rdf:resource="http://purl.org/olia/dzongkha.owl#PluralNoun"/>
        <rdfs:comment>Noun, Plural</rdfs:comment>
        <hasTag>NNS</hasTag>
    </owl:NamedIndividual>



    <!-- http://purl.org/olia/dzongkha.owl#NNSC -->

    <owl:NamedIndividual rdf:about="http://purl.org/olia/dzongkha.owl#NNSC">
        <rdf:type rdf:resource="http://purl.org/olia/dzongkha.owl#CombinedTag"/>
        <rdf:type rdf:resource="http://purl.org/olia/dzongkha.owl#CommonNoun"/>
        <rdf:type rdf:resource="http://purl.org/olia/dzongkha.owl#SubordinateConjunction"/>
        <hasTag>NNSC</hasTag>
        <rdfs:comment>Common Noun + Subordinate Conjunction</rdfs:comment>
    </owl:NamedIndividual>



    <!-- http://purl.org/olia/dzongkha.owl#NNSCG -->

    <owl:NamedIndividual rdf:about="http://purl.org/olia/dzongkha.owl#NNSCG">
        <rdf:type rdf:resource="http://purl.org/olia/dzongkha.owl#CombinedTag"/>
        <rdf:type rdf:resource="http://purl.org/olia/dzongkha.owl#GenitiveCaseMarker"/>
        <rdf:type rdf:resource="http://purl.org/olia/dzongkha.owl#PluralNoun"/>
        <hasTag>NNSCG</hasTag>
        <rdfs:comment>Noun, Plural + Genitive case</rdfs:comment>
    </owl:NamedIndividual>



    <!-- http://purl.org/olia/dzongkha.owl#OD -->

    <owl:NamedIndividual rdf:about="http://purl.org/olia/dzongkha.owl#OD">
        <rdf:type rdf:resource="http://purl.org/olia/dzongkha.owl#OrdinalNumber"/>
        <rdfs:comment>Number, Ordinal</rdfs:comment>
        <hasTag>OD</hasTag>
    </owl:NamedIndividual>



    <!-- http://purl.org/olia/dzongkha.owl#PP -->

    <owl:NamedIndividual rdf:about="http://purl.org/olia/dzongkha.owl#PP">
        <rdf:type rdf:resource="http://purl.org/olia/dzongkha.owl#Postposition"/>
        <hasTag>PP</hasTag>
        <rdfs:comment>As an example for such dissimilarity [between the Penn Treebank tagset and the Dzongkha tagset -- CC], Dzongkha postpositions are mentioned here, cf. (1); the respective tag (PP) only exist for Dzongkha whereas in English the whole set of ad position tags (preposition and postpositions) exist.
(1) j&#39;ili shing-gi w&#244;lu -d&#251;
Cat tree[posp] under[PP] be
&#39;&#39;A cat is under the tree&#39;&#39;</rdfs:comment>
        <rdfs:comment>Adposition, Postposition</rdfs:comment>
    </owl:NamedIndividual>



    <!-- http://purl.org/olia/dzongkha.owl#PRD -->

    <owl:NamedIndividual rdf:about="http://purl.org/olia/dzongkha.owl#PRD">
        <rdf:type rdf:resource="http://purl.org/olia/dzongkha.owl#DifferentialPronoun"/>
        <hasTag>PRD</hasTag>
        <rdfs:comment>Pronouns, Differential</rdfs:comment>
    </owl:NamedIndividual>



    <!-- http://purl.org/olia/dzongkha.owl#PRL -->

    <owl:NamedIndividual rdf:about="http://purl.org/olia/dzongkha.owl#PRL">
        <rdf:type rdf:resource="http://purl.org/olia/dzongkha.owl#LocativePronoun"/>
        <rdfs:comment>Pronouns, Locative</rdfs:comment>
        <hasTag>PRL</hasTag>
    </owl:NamedIndividual>



    <!-- http://purl.org/olia/dzongkha.owl#PRLCG -->

    <owl:NamedIndividual rdf:about="http://purl.org/olia/dzongkha.owl#PRLCG">
        <rdf:type rdf:resource="http://purl.org/olia/dzongkha.owl#CombinedTag"/>
        <rdf:type rdf:resource="http://purl.org/olia/dzongkha.owl#GenitiveCaseMarker"/>
        <rdf:type rdf:resource="http://purl.org/olia/dzongkha.owl#LocativePronoun"/>
        <hasTag>PRLCG</hasTag>
        <rdfs:comment>Locative Pronoun + Genitive case</rdfs:comment>
    </owl:NamedIndividual>



    <!-- http://purl.org/olia/dzongkha.owl#PRP -->

    <owl:NamedIndividual rdf:about="http://purl.org/olia/dzongkha.owl#PRP">
        <rdf:type rdf:resource="http://purl.org/olia/dzongkha.owl#PersonalPronoun"/>
        <hasTag>PRP</hasTag>
        <rdfs:comment>Pronouns, Personal</rdfs:comment>
    </owl:NamedIndividual>



    <!-- http://purl.org/olia/dzongkha.owl#PRRF -->

    <owl:NamedIndividual rdf:about="http://purl.org/olia/dzongkha.owl#PRRF">
        <rdf:type rdf:resource="http://purl.org/olia/dzongkha.owl#ReflexivePronoun"/>
        <rdfs:comment>Pronouns, Reflexive</rdfs:comment>
        <hasTag>PRRF</hasTag>
    </owl:NamedIndividual>



    <!-- http://purl.org/olia/dzongkha.owl#PUN -->

    <owl:NamedIndividual rdf:about="http://purl.org/olia/dzongkha.owl#PUN">
        <rdf:type rdf:resource="http://purl.org/olia/dzongkha.owl#Punctuation"/>
        <rdfs:comment>Punctuation</rdfs:comment>
        <hasTag>PUN</hasTag>
    </owl:NamedIndividual>



    <!-- http://purl.org/olia/dzongkha.owl#RB -->

    <owl:NamedIndividual rdf:about="http://purl.org/olia/dzongkha.owl#RB">
        <rdf:type rdf:resource="http://purl.org/olia/dzongkha.owl#Adverb"/>
        <rdfs:comment>Adverb, Adverb</rdfs:comment>
        <hasTag>RB</hasTag>
    </owl:NamedIndividual>



    <!-- http://purl.org/olia/dzongkha.owl#RBB -->

    <owl:NamedIndividual rdf:about="http://purl.org/olia/dzongkha.owl#RBB">
        <rdf:type rdf:resource="http://purl.org/olia/dzongkha.owl#BehaviouralAdverb"/>
        <rdfs:comment>Adverb, Behavioural</rdfs:comment>
        <hasTag>RBB</hasTag>
    </owl:NamedIndividual>



    <!-- http://purl.org/olia/dzongkha.owl#RBR -->

    <owl:NamedIndividual rdf:about="http://purl.org/olia/dzongkha.owl#RBR">
        <rdf:type rdf:resource="http://purl.org/olia/dzongkha.owl#ComparativeAdverb"/>
        <rdfs:comment>Adverb, Comparative</rdfs:comment>
        <hasTag>RBR</hasTag>
    </owl:NamedIndividual>



    <!-- http://purl.org/olia/dzongkha.owl#RBS -->

    <owl:NamedIndividual rdf:about="http://purl.org/olia/dzongkha.owl#RBS">
        <rdf:type rdf:resource="http://purl.org/olia/dzongkha.owl#SuperlativeAdverb"/>
        <hasTag>RBS</hasTag>
        <rdfs:comment>Adverb, Superlative</rdfs:comment>
    </owl:NamedIndividual>



    <!-- http://purl.org/olia/dzongkha.owl#SC -->

    <owl:NamedIndividual rdf:about="http://purl.org/olia/dzongkha.owl#SC">
        <rdf:type rdf:resource="http://purl.org/olia/dzongkha.owl#SubordinateConjunction"/>
        <hasTag>SC</hasTag>
        <rdfs:comment>Conjunction, Subordinate</rdfs:comment>
    </owl:NamedIndividual>



    <!-- http://purl.org/olia/dzongkha.owl#TM -->

    <owl:NamedIndividual rdf:about="http://purl.org/olia/dzongkha.owl#TM">
        <rdf:type rdf:resource="http://purl.org/olia/dzongkha.owl#TenseMarker"/>
        <hasTag>TM</hasTag>
        <rdfs:comment>Marker, Tense</rdfs:comment>
    </owl:NamedIndividual>



    <!-- http://purl.org/olia/dzongkha.owl#UH -->

    <owl:NamedIndividual rdf:about="http://purl.org/olia/dzongkha.owl#UH">
        <rdf:type rdf:resource="http://purl.org/olia/dzongkha.owl#Interjection"/>
        <hasTag>UH</hasTag>
        <rdfs:comment>Interjection</rdfs:comment>
    </owl:NamedIndividual>



    <!-- http://purl.org/olia/dzongkha.owl#VB -->

    <owl:NamedIndividual rdf:about="http://purl.org/olia/dzongkha.owl#VB">
        <rdf:type rdf:resource="http://purl.org/olia/dzongkha.owl#Verb"/>
        <hasTag>VB</hasTag>
        <rdfs:comment>Verb, Verb</rdfs:comment>
    </owl:NamedIndividual>



    <!-- http://purl.org/olia/dzongkha.owl#VBAUX -->

    <owl:NamedIndividual rdf:about="http://purl.org/olia/dzongkha.owl#VBAUX">
        <rdf:type rdf:resource="http://purl.org/olia/dzongkha.owl#AuxiliaryVerb"/>
        <rdfs:comment>Verb, Auxiliary</rdfs:comment>
        <hasTag>VBAUX</hasTag>
    </owl:NamedIndividual>



    <!-- http://purl.org/olia/dzongkha.owl#VBAs -->

    <owl:NamedIndividual rdf:about="http://purl.org/olia/dzongkha.owl#VBAs">
        <rdf:type rdf:resource="http://purl.org/olia/dzongkha.owl#AspirationalVerb"/>
        <hasTag>VBAs</hasTag>
        <rdfs:comment>Verb, Aspirational</rdfs:comment>
    </owl:NamedIndividual>



    <!-- http://purl.org/olia/dzongkha.owl#VBAt -->

    <owl:NamedIndividual rdf:about="http://purl.org/olia/dzongkha.owl#VBAt">
        <rdf:type rdf:resource="http://purl.org/olia/dzongkha.owl#AgentiveVerb"/>
        <hasTag>VBAt</hasTag>
        <rdfs:comment>Verb, Agentive</rdfs:comment>
    </owl:NamedIndividual>



    <!-- http://purl.org/olia/dzongkha.owl#VBAtCG -->

    <owl:NamedIndividual rdf:about="http://purl.org/olia/dzongkha.owl#VBAtCG">
        <rdf:type rdf:resource="http://purl.org/olia/dzongkha.owl#AgentiveVerb"/>
        <rdf:type rdf:resource="http://purl.org/olia/dzongkha.owl#CombinedTag"/>
        <rdf:type rdf:resource="http://purl.org/olia/dzongkha.owl#GenitiveCaseMarker"/>
        <rdfs:comment>Veb, Agentive + Genitive case</rdfs:comment>
        <hasTag>VBAtCG</hasTag>
    </owl:NamedIndividual>



    <!-- http://purl.org/olia/dzongkha.owl#VBAtSC -->

    <owl:NamedIndividual rdf:about="http://purl.org/olia/dzongkha.owl#VBAtSC">
        <rdf:type rdf:resource="http://purl.org/olia/dzongkha.owl#AgentiveVerb"/>
        <rdf:type rdf:resource="http://purl.org/olia/dzongkha.owl#CombinedTag"/>
        <rdf:type rdf:resource="http://purl.org/olia/dzongkha.owl#SubordinateConjunction"/>
        <hasTag>VBAtSC</hasTag>
        <rdfs:comment>Verb, Agentive + Subordinate Conjunction</rdfs:comment>
    </owl:NamedIndividual>



    <!-- http://purl.org/olia/dzongkha.owl#VBCG -->

    <owl:NamedIndividual rdf:about="http://purl.org/olia/dzongkha.owl#VBCG">
        <rdf:type rdf:resource="http://purl.org/olia/dzongkha.owl#CombinedTag"/>
        <rdf:type rdf:resource="http://purl.org/olia/dzongkha.owl#GenitiveCaseMarker"/>
        <rdf:type rdf:resource="http://purl.org/olia/dzongkha.owl#Verb"/>
        <rdfs:comment>Verb, Verb + Genitive case</rdfs:comment>
        <hasTag>VBCG</hasTag>
    </owl:NamedIndividual>



    <!-- http://purl.org/olia/dzongkha.owl#VBH -->

    <owl:NamedIndividual rdf:about="http://purl.org/olia/dzongkha.owl#VBH">
        <rdf:type rdf:resource="http://purl.org/olia/dzongkha.owl#HonorificVerb"/>
        <hasTag>VBH</hasTag>
        <rdfs:comment>Verb, Honorific

Dzongkha uses honorific forms: &#3923;&#3851;&#3926;&#3935;&#3936;&#3851;/nam za/
(cloths) is the honorific form of the noun &#3906;&#3964;&#3851;
&#3939;&#3851;/gola/(cloths), &#3906;&#3942;&#3908;&#3942;&#3851;/sung/(tell) the honorific
form of the verb &#3942;&#3926;&#3851;/lab/(tell). We opted to mark
them by adding the tag NNH (honorific
common noun) and VBH (honorific verb) to
enable future research on this specific usage of
Dzongkha language. A number of tags were
added to the set, of which we describe four in
more detail: two of the additional tags are subclasses
of verbs: VBH (honorific verb form),
and VBN which describes past participle forms,
like, e.g. &#3926;&#3908;&#3928;&#3851;/jun/(created), the past particle
form of &#3926;&#3908;&#3851;/jung/(create).</rdfs:comment>
    </owl:NamedIndividual>



    <!-- http://purl.org/olia/dzongkha.owl#VBHCG -->

    <owl:NamedIndividual rdf:about="http://purl.org/olia/dzongkha.owl#VBHCG">
        <rdf:type rdf:resource="http://purl.org/olia/dzongkha.owl#CombinedTag"/>
        <rdf:type rdf:resource="http://purl.org/olia/dzongkha.owl#GenitiveCaseMarker"/>
        <rdf:type rdf:resource="http://purl.org/olia/dzongkha.owl#HonorificVerb"/>
        <hasTag>VBHCG</hasTag>
        <rdfs:comment>Verb, Honorific + Genitive case</rdfs:comment>
    </owl:NamedIndividual>



    <!-- http://purl.org/olia/dzongkha.owl#VBI -->

    <owl:NamedIndividual rdf:about="http://purl.org/olia/dzongkha.owl#VBI">
        <rdf:type rdf:resource="http://purl.org/olia/dzongkha.owl#ImperativeVerb"/>
        <hasTag>VBI</hasTag>
        <rdfs:comment>Verb, Imperative</rdfs:comment>
    </owl:NamedIndividual>



    <!-- http://purl.org/olia/dzongkha.owl#VBMD -->

    <owl:NamedIndividual rdf:about="http://purl.org/olia/dzongkha.owl#VBMD">
        <rdf:type rdf:resource="http://purl.org/olia/dzongkha.owl#ModalVerb"/>
        <rdfs:comment>Verb, Modal</rdfs:comment>
        <hasTag>VBMD</hasTag>
    </owl:NamedIndividual>



    <!-- http://purl.org/olia/dzongkha.owl#VBMDCG -->

    <owl:NamedIndividual rdf:about="http://purl.org/olia/dzongkha.owl#VBMDCG">
        <rdf:type rdf:resource="http://purl.org/olia/dzongkha.owl#CombinedTag"/>
        <rdf:type rdf:resource="http://purl.org/olia/dzongkha.owl#GenitiveCaseMarker"/>
        <rdf:type rdf:resource="http://purl.org/olia/dzongkha.owl#ModalVerb"/>
        <rdfs:comment>Verb, Modal + Genitive case</rdfs:comment>
        <hasTag>VBMDCG</hasTag>
    </owl:NamedIndividual>



    <!-- http://purl.org/olia/dzongkha.owl#VBMDSC -->

    <owl:NamedIndividual rdf:about="http://purl.org/olia/dzongkha.owl#VBMDSC">
        <rdf:type rdf:resource="http://purl.org/olia/dzongkha.owl#CombinedTag"/>
        <rdf:type rdf:resource="http://purl.org/olia/dzongkha.owl#ModalVerb"/>
        <rdf:type rdf:resource="http://purl.org/olia/dzongkha.owl#SubordinateConjunction"/>
        <rdfs:comment>Verb, Modal + Subordinate Conjunction</rdfs:comment>
        <hasTag>VBMDC</hasTag>
        <hasTag>VBMDSC</hasTag>
        <rdfs:comment>form of the tag in the document is given as VBMDC, in analogy with other fused forms, however, VBMDSC should be appropriate</rdfs:comment>
    </owl:NamedIndividual>



    <!-- http://purl.org/olia/dzongkha.owl#VBN -->

    <owl:NamedIndividual rdf:about="http://purl.org/olia/dzongkha.owl#VBN">
        <rdf:type rdf:resource="http://purl.org/olia/dzongkha.owl#PastParticiple"/>
        <rdfs:comment>Verb, Past Participle</rdfs:comment>
        <hasTag>VBN</hasTag>
    </owl:NamedIndividual>



    <!-- http://purl.org/olia/dzongkha.owl#VBNa -->

    <owl:NamedIndividual rdf:about="http://purl.org/olia/dzongkha.owl#VBNa">
        <rdf:type rdf:resource="http://purl.org/olia/dzongkha.owl#NonAgentiveVerb"/>
        <hasTag>VBNa</hasTag>
        <rdfs:comment>Verb, Non-Agentive</rdfs:comment>
    </owl:NamedIndividual>



    <!-- http://purl.org/olia/dzongkha.owl#VBSC -->

    <owl:NamedIndividual rdf:about="http://purl.org/olia/dzongkha.owl#VBSC">
        <rdf:type rdf:resource="http://purl.org/olia/dzongkha.owl#CombinedTag"/>
        <rdf:type rdf:resource="http://purl.org/olia/dzongkha.owl#SubordinateConjunction"/>
        <rdf:type rdf:resource="http://purl.org/olia/dzongkha.owl#Verb"/>
        <rdfs:comment>Verb, Verb + Subordinate Conjunction</rdfs:comment>
        <hasTag>VBSC</hasTag>
    </owl:NamedIndividual>
</rdf:RDF>



<!-- Generated by the OWL API (version 3.0.0.1451) http://owlapi.sourceforge.net -->
