<?xml version="1.0"?>
<rdf:RDF xmlns="http://purl.org/olia/arabic_khoja.owl#"
     xml:base="http://purl.org/olia/arabic_khoja.owl"
     xmlns:ms="http://w3id.org/meta-share/meta-share/"
     xmlns:dct="http://purl.org/dc/terms/"
     xmlns:owl="http://www.w3.org/2002/07/owl#"
     xmlns:rdf="http://www.w3.org/1999/02/22-rdf-syntax-ns#"
     xmlns:xml="http://www.w3.org/XML/1998/namespace"
     xmlns:xsd="http://www.w3.org/2001/XMLSchema#"
     xmlns:rdfs="http://www.w3.org/2000/01/rdf-schema#"
     xmlns:system="http://purl.org/olia/system.owl#"
     xmlns:arabic_khoja="http://purl.org/olia/arabic_khoja.owl#">
    <owl:Ontology rdf:about="http://purl.org/olia/arabic_khoja.owl">
        <owl:imports rdf:resource="http://purl.org/olia/system.owl"/>
        <dct:license rdf:resource="https://creativecommons.org/licenses/by/3.0/"/>
        <ms:language rdf:resource="http://lexvo.org/id/iso639-3/ara"/>
        <rdfs:comment>OLiA Annotation Model for morphosyntactic annotation of Arabic, following Khoja et al. (2001)

Arabic grammar has been studied for centuries, and the principles of describing the language already exist. Since so much knowledge is readily available, it is logical to derive our tagset from this wealth of information. The alternative to this is to base the Arabic tagset on an Indo-European one, but by doing this we may lose a lot of the information that an Arabic tagset would give us. Also, by moulding Arabic to fit an Indo-European language, we might distort the way Arabic is perceived by its native speakers. (Khoja et al, 2001)

The prototype tagger reported in (Khoja 2003) was based on a lexicon of under 10,000 word-types, extracted from a corpus of about 50,000 word-tokens. The initial 50,000-word training corpus was extracted from the Saudi Al-Jazirah newspaper (date 03/03/1999); initial tagging experiments were done on other newspaper texts, and a social science paper. (Atwell 2007)

Unless specified otherwise, all comments are quotes from Khoja et al. (2001).

References:

Khoja, S, Garside, R, and Knowles, G (2001) A tagset for the morphosyntactic tagging of Arabic. Paper given at the Corpus Linguistics 2001 conference, Lancaster, http://zeus.cs.pacificu.edu/shereen/CL2001.pdf

Eric Atwell (2007), Development of tag sets for part-of-speech tagging, Corpus Linguistics Conference 2007, Birmingham, http://www.comp.leeds.ac.uk/eric/atwell07clih.pdf</rdfs:comment>
        <owl:versionInfo>
2011/08/17-18 created
2020/02/25 explanation of common relative pronoun added

Christian Chiarcos, chiarcos@informatik.uni-frankfurt.de</owl:versionInfo>
    </owl:Ontology>
    


    <!-- 
    ///////////////////////////////////////////////////////////////////////////////////////
    //
    // Annotation properties
    //
    ///////////////////////////////////////////////////////////////////////////////////////
     -->

    


    <!-- http://purl.org/olia/system.owl#hasTagMatching -->

    <owl:AnnotationProperty rdf:about="http://purl.org/olia/system.owl#hasTagMatching"/>
    


    <!-- http://w3id.org/meta-share/meta-share/language -->

    <owl:AnnotationProperty rdf:about="http://w3id.org/meta-share/meta-share/language"/>
    


    <!-- 
    ///////////////////////////////////////////////////////////////////////////////////////
    //
    // Object Properties
    //
    ///////////////////////////////////////////////////////////////////////////////////////
     -->

    


    <!-- http://purl.org/olia/arabic_khoja.owl#hasCase -->

    <owl:ObjectProperty rdf:about="http://purl.org/olia/arabic_khoja.owl#hasCase">
        <rdfs:subPropertyOf rdf:resource="http://purl.org/olia/system.owl#hasFeature"/>
        <rdfs:domain rdf:resource="http://purl.org/olia/arabic_khoja.owl#Noun"/>
        <rdfs:range rdf:resource="http://purl.org/olia/arabic_khoja.owl#Case"/>
    </owl:ObjectProperty>
    


    <!-- http://purl.org/olia/arabic_khoja.owl#hasDefiniteness -->

    <owl:ObjectProperty rdf:about="http://purl.org/olia/arabic_khoja.owl#hasDefiniteness">
        <rdfs:subPropertyOf rdf:resource="http://purl.org/olia/system.owl#hasFeature"/>
        <rdfs:domain rdf:resource="http://purl.org/olia/arabic_khoja.owl#Noun"/>
        <rdfs:range rdf:resource="http://purl.org/olia/arabic_khoja.owl#Definiteness"/>
    </owl:ObjectProperty>
    


    <!-- http://purl.org/olia/arabic_khoja.owl#hasGender -->

    <owl:ObjectProperty rdf:about="http://purl.org/olia/arabic_khoja.owl#hasGender">
        <rdfs:subPropertyOf rdf:resource="http://purl.org/olia/system.owl#hasFeature"/>
        <rdfs:domain>
            <owl:Class>
                <owl:unionOf rdf:parseType="Collection">
                    <rdf:Description rdf:about="http://purl.org/olia/arabic_khoja.owl#Noun"/>
                    <rdf:Description rdf:about="http://purl.org/olia/arabic_khoja.owl#Verb"/>
                </owl:unionOf>
            </owl:Class>
        </rdfs:domain>
        <rdfs:range rdf:resource="http://purl.org/olia/arabic_khoja.owl#Gender"/>
    </owl:ObjectProperty>
    


    <!-- http://purl.org/olia/arabic_khoja.owl#hasMood -->

    <owl:ObjectProperty rdf:about="http://purl.org/olia/arabic_khoja.owl#hasMood">
        <rdfs:subPropertyOf rdf:resource="http://purl.org/olia/system.owl#hasFeature"/>
        <rdfs:domain rdf:resource="http://purl.org/olia/arabic_khoja.owl#Verb"/>
        <rdfs:range rdf:resource="http://purl.org/olia/arabic_khoja.owl#Mood"/>
    </owl:ObjectProperty>
    


    <!-- http://purl.org/olia/arabic_khoja.owl#hasNumber -->

    <owl:ObjectProperty rdf:about="http://purl.org/olia/arabic_khoja.owl#hasNumber">
        <rdfs:subPropertyOf rdf:resource="http://purl.org/olia/system.owl#hasFeature"/>
        <rdfs:domain>
            <owl:Class>
                <owl:unionOf rdf:parseType="Collection">
                    <rdf:Description rdf:about="http://purl.org/olia/arabic_khoja.owl#Noun"/>
                    <rdf:Description rdf:about="http://purl.org/olia/arabic_khoja.owl#Verb"/>
                </owl:unionOf>
            </owl:Class>
        </rdfs:domain>
        <rdfs:range rdf:resource="http://purl.org/olia/arabic_khoja.owl#Number"/>
    </owl:ObjectProperty>
    


    <!-- http://purl.org/olia/arabic_khoja.owl#hasPerson -->

    <owl:ObjectProperty rdf:about="http://purl.org/olia/arabic_khoja.owl#hasPerson">
        <rdfs:subPropertyOf rdf:resource="http://purl.org/olia/system.owl#hasFeature"/>
        <rdfs:domain>
            <owl:Class>
                <owl:unionOf rdf:parseType="Collection">
                    <rdf:Description rdf:about="http://purl.org/olia/arabic_khoja.owl#Noun"/>
                    <rdf:Description rdf:about="http://purl.org/olia/arabic_khoja.owl#Verb"/>
                </owl:unionOf>
            </owl:Class>
        </rdfs:domain>
        <rdfs:range rdf:resource="http://purl.org/olia/arabic_khoja.owl#Person"/>
    </owl:ObjectProperty>
    


    <!-- 
    ///////////////////////////////////////////////////////////////////////////////////////
    //
    // Classes
    //
    ///////////////////////////////////////////////////////////////////////////////////////
     -->

    


    <!-- http://purl.org/olia/arabic_khoja.owl#Abbreviation -->

    <owl:Class rdf:about="http://purl.org/olia/arabic_khoja.owl#Abbreviation">
        <rdfs:subClassOf rdf:resource="http://purl.org/olia/arabic_khoja.owl#Residual"/>
        <rdfs:comment>RA
Residual, abbreviation
ساو
was
</rdfs:comment>
    </owl:Class>
    


    <!-- http://purl.org/olia/arabic_khoja.owl#AccusativeCase -->

    <owl:Class rdf:about="http://purl.org/olia/arabic_khoja.owl#AccusativeCase">
        <rdfs:subClassOf rdf:resource="http://purl.org/olia/arabic_khoja.owl#Case"/>
    </owl:Class>
    


    <!-- http://purl.org/olia/arabic_khoja.owl#Adjective -->

    <owl:Class rdf:about="http://purl.org/olia/arabic_khoja.owl#Adjective">
        <rdfs:subClassOf rdf:resource="http://purl.org/olia/arabic_khoja.owl#Noun"/>
        <rdfs:comment>Adjectives are nouns that describe the aspects of an object. Adjectives inherit the properties of nouns, so they take “nunation” when in the indefinite and can take the definite article when definite. For example, alwld sghyr “The small boy” contains the adjective sghyr “small”. This adjective can take the definite article as in ‘darasa alwaladu alsaghyr’ “the small boy studied”, and it can also have “nunation” as in ‘hasanu saghyrun’ “Hassan is small”.</rdfs:comment>
        <rdfs:comment>NACSgMNI
Singular, masculine, nominative,
indefinite adjective
ﺪﻴﻌﺳ
ٌ
sa’ydun
happy
NACSgMAI
Singular, masculine, accusative, indefinite
adjective
اﺪ ﻌﺳ
َ ﻴ
sa’ydan
happy
NACSgMGI
Singular, masculine, genitive, indefinite
adjective
ﺪﻴﻌﺳ
ٍ
sa’ydin
happy
NACSgMND
Singular, masculine, nominative, definite
adjective
ﺪﻴﻌﺴﻟا
ُ
alsa’ydu
the happy
NACSgMAD
Singular, masculine, accusative, definite
adjective
ﺪَﻴﻌﺴﻟا
alsa’yda
the happy
NACSgMGD
Singular, masculine, genitive, definite
adjective
ﺪﻴﻌﺴﻟا
ِ
alsa’ydi
the happy
NACSgFNI
Singular, feminine, nominative, indefinite
adjective
ةﺪﻴﻌﺳ
ٌ
sa’ydatun
happy
Page 10
NACSgFAI
Singular, feminine, accusative, indefinite
adjective
ﺎﺗﺪﻴﻌﺳ
ً
sa’ydatan
happy
NACSgFGI
Singular, feminine, genitive, indefinite
adjective
ةﺪﻴﻌﺳ
ٍ
sa’ydatin
happy
NACSgFND
Singular, feminine, nominative, definite
adjective
ةﺪﻴﻌﺴﻟا
ُ
alsa’ydatu
the happy
NACSgFAD
Singular, feminine, accusative, definite
adjective
ةﺪﻴﻌﺴﻟا
َ
alsa’ydata
the happy
NACSgFGD
Singular, feminine, genitive, definite
adjective
ةﺪﻴﻌﺴﻟا
ِ
alsa’ydati
the happy
NACDuMNI
Dual, masculine, nominative, indefinite
adjective
ناﺪﻴﻌﺳ
sa’ydan
two happy
NACDuMAI
Dual, masculine, accusative, indefinite
adjective
ﻦﻱﺪﻴﻌﺳ
sa’ydain
two happy
NACDuMGI
Dual, masculine, genitive, indefinite
adjective
ﻦﻱﺪﻴﻌﺳ
sa’ydain
two happy
NACDuMND
Dual, masculine, nominative, definite
adjective
ناﺪﻴﻌﺴﻟا
alkitaban
the two happy
NACDuMAD
Dual, masculine, accusative, definite
adjective
ﻦﻱﺪﻴﻌﺴﻟا
alsa’ydain
the two happy
NACDuMGD
Dual, masculine, genitive, definite
adjective
ﻦﻱﺪﻴﻌﺴﻟا
alsa’ydain
the two happy
NACDuFNI
Dual, feminine, nominative, indefinite
adjective
نﺎﺗﺪﻴﻌﺳ
sa’ydatan
two happy
NACDuFAI
Dual, feminine, accusative, indefinite
adjective
ﻦﻴﺗﺪﻴﻌﺳ
sa’ydatain
two happy
NACDuFGI
Dual, feminine, genitive, indefinite
adjective
ﻦﻴﺗﺪﻴﻌﺳ
sa’ydatain
two happy
NACDuFND
Dual, feminine, nominative, definite
adjective
نﺎﺗﺪﻴﻌﺴﻟا
alsa’ydatan
the two happy
NACDuFAD
Dual, feminine, accusative, definite
adjective
ﻦﻴﺗﺪﻴﻌﺴﻟا
alsa’ydatain
the two happy
NACDuFGD Dual, feminine, genitive, definite adjective
ﻦﻴﺗﺪﻴﻌﺴﻟا
alsa’ydatain
the two happy
NACPlMNI
Plural, masculine, nominative, indefinite
adjective
نوﺪﻴﻌﺳ
sa’ydoon
happy
NACPlMAI
Plural, masculine, accusative, indefinite
adjective
ﻦﻱﺪﻴﻌﺳ
sa’ydeen
happy
NACPlMGI
Plural, masculine, genitive, indefinite
adjective
ﻦﻱﺪﻴﻌﺳ
sa’ydeen
happy
NACPlMND
Plural, masculine, nominative, definite
adjective
وﺪﻴﻌﺴﻟا
ن
alsa’ydoon
the happy
NACPlMAD
Plural, masculine, accusative, definite
adjective
ﺪﻴﻌﺴﻟا
ﻦﻱ
alsa’ydeen
the happy
NACPlMGD
Plural, masculine, genitive, definite
adjective
ﺪﻴﻌﺴﻟا
ﻦﻱ
alsa’ydeen
the happy
NACPlFNI
Plural, feminine, nominative, indefinite
adjective
تاﺪﻴﻌﺳ
ٌ
sa’ydaatun
happy
NACPlFAI
Plural, feminine, accusative, indefinite
adjective
ﺎﺗاﺪﻴﻌﺳ
ً
sa’ydaatan
happy
NACPlFGI
Plural, feminine, genitive, indefinite,
adjective
تاﺪﻴﻌﺳ
ٍ
sa’ydaatin
happy
NACPlFND
Plural, feminine, nominative, definite
adjective
تاﺪﻴﻌﺴﻟا
ُ
alsa’ydaatu
the happy
NACPlFAD
Plural, feminine, accusative, definite
adjective
تاﺪﻴﻌﺴﻟا
َ
alsa’ydaata
the happy
NACPlFGD
Plural, feminine, genitive, definite
adjective
تاﺪﻴﻌﺴﻟا
ِ
alsa’ydaati
</rdfs:comment>
    </owl:Class>
    


    <!-- http://purl.org/olia/arabic_khoja.owl#Adverbial -->

    <owl:Class rdf:about="http://purl.org/olia/arabic_khoja.owl#Adverbial">
        <rdfs:subClassOf rdf:resource="http://purl.org/olia/arabic_khoja.owl#Particle"/>
        <rdfs:comment>PA
Adverbial particles
إاذ– ﻢﺛ – فﻮﺳ –ﻦﻟ
idhaa – thumma –
swf – ln
</rdfs:comment>
    </owl:Class>
    


    <!-- http://purl.org/olia/arabic_khoja.owl#Answer -->

    <owl:Class rdf:about="http://purl.org/olia/arabic_khoja.owl#Answer">
        <rdfs:subClassOf rdf:resource="http://purl.org/olia/arabic_khoja.owl#Particle"/>
        <rdfs:comment>PW
Answers
ﻞﺟأ–ﻻ
la – ajl
</rdfs:comment>
    </owl:Class>
    


    <!-- http://purl.org/olia/arabic_khoja.owl#CardinalNumeral -->

    <owl:Class rdf:about="http://purl.org/olia/arabic_khoja.owl#CardinalNumeral">
        <rdfs:subClassOf rdf:resource="http://purl.org/olia/arabic_khoja.owl#Numeral"/>
        <rdfs:comment>NNuCaSgM Singular, masculine, cardinal number
ﻊﺑرأ
arba’
Four
NNuCaSgF Singular, feminine, cardinal number
ﺔﻌﺑرأ
arba’a
</rdfs:comment>
    </owl:Class>
    


    <!-- http://purl.org/olia/arabic_khoja.owl#Case -->

    <owl:Class rdf:about="http://purl.org/olia/arabic_khoja.owl#Case">
        <rdfs:subClassOf rdf:resource="http://purl.org/olia/arabic_khoja.owl#Feature"/>
    </owl:Class>
    


    <!-- http://purl.org/olia/arabic_khoja.owl#CommonNoun -->

    <owl:Class rdf:about="http://purl.org/olia/arabic_khoja.owl#CommonNoun">
        <rdfs:subClassOf rdf:resource="http://purl.org/olia/arabic_khoja.owl#Noun"/>
        <rdfs:comment>NCSgMNI
Singular, masculine, nominative,
indefinite common noun
بﺎﺘآ
ٌ
kitabun
book
NCSgMAI
Singular, masculine, accusative, indefinite
common noun
ﺎﺑﺎﺘآ
َ
kitaban
book
NCSgMGI
Singular, masculine, genitive, indefinite
common noun
بﺎﺘآ
ٍ
kitabin
book
NCSgMND
Singular, masculine, nominative, definite
common noun
بﺎﺘﻜﻟا
ُ
alkitabu
the book
NCSgMAD
Singular, masculine, accusative, definite
common noun
بَ ﺎﺘﻜﻟا
alkitaba
the book
NCSgMGD
Singular, masculine, genitive, definite
common noun
بﺎﺘﻜﻟا
ِ
alkitabi
the book
NCSgFNI
Singular, feminine, nominative, indefinite
common noun
ﺔﺳرﺪﻣ
ٌ
madrasatun
school
NCSgFAI
Singular, feminine, accusative, indefinite
common noun
ﺎﺘﺳرﺪﻣ
ً
madrasatan
school
NCSgFGI
Singular, feminine, genitive, indefinite
common noun
ﺔﺳرﺪﻣ
ٍ
madrasatin
school
NCSgFND
Singular, feminine, nominative, definite
common noun
ﺔﺳرﺪﻤﻟا
ُ
almadrasatu
NCSgFAD
Singular, feminine, accusative, definite
common noun
ﺔﺳرﺪﻤﻟا
َ
almadrasata
the school
NCSgFGD
Singular, feminine, genitive, definite
common noun
ﺔﺳرﺪﻤﻟا
ِ
aladrasati
the school
NCDuMNI
Dual, masculine, nominative, indefinite
common noun
نﺎﺑﺎﺘآ
kitaban
two books
NCDuMAI
Dual, masculine, accusative, indefinite
common noun
ﻦﻴﺑﺎﺘآ
kitabain
two books
NCDuMGI
Dual, masculine, genitive, indefinite
common noun
ﻦﻴﺑﺎﺘآ
kitabain
two books
NCDuMND
Dual, masculine, nominative, definite
common noun
نﺎﺑﺎﺘﻜﻟا
alkitaban
the two books
NCDuMAD
Dual, masculine, accusative, definite
common noun
ﻦﻴﺑﺎﺘﻜﻟا
alkitabain
the two books
NCDuMGD
Dual, masculine, genitive, definite
common noun
ﻦﻴﺑﺎﺘﻜﻟا
alkitabain
the two books
NCDuFNI
Dual, feminine, nominative, indefinite
common noun
نﺎﺘﺳرﺪﻣ
madrasatan
two books
NCDuFAI
Dual, feminine, accusative, indefinite
common noun
ﻦﻴﺘﺳرﺪﻣ
madrasatain
two schools
NCDuFGI
Dual, feminine, genitive, indefinite
common noun
ﻦﻴﺘﺳرﺪﻣ
madrasatain
two schools
NCDuFND
Dual, feminine, nominative, definite
common noun
نﺎﺘﺳرﺪﻤﻟا
almadrasatan
the two
schools
NCDuFAD
Dual, feminine, accusative, definite
common noun
ﻦﻴﺘﺳرﺪﻤﻟا
almadrasatain
the two
schools
NCDuFGD
Dual, feminine, genitive, definite common
noun
ﻦﻴﺘﺳرﺪﻤﻟا
almadrasatain
the two
schools
NCPlMNI
Plural, masculine, nominative, indefinite
common noun
ﺐﺘآ
ٌ-
نﻮﻤﻠﺴﻣ
muslimoon –
kutubun
Muslims –
books
NCPlMAI
Plural, masculine, accusative, indefinite
common noun
ﺎﺒﺘآ
َ-
ﻦﻴﻤﻠﺴﻣ
muslimeen –
kutuban
Muslims –
books
NCPlMGI
Plural, masculine, genitive, indefinite
common noun
ﺐﺘآ
ٍ-
ﻦﻴﻤﻠﺴﻣ
muslimeen –
kutubin
Muslims –
books
NCPlMND
Plural, masculine, nominative, definite
common noun
ﺐﺘﻜﻟا
ُ-
نﻮﻤﻠﺴﻤﻟا
almuslimoon –
alkutubu
the Muslims –
the books
NCPlMAD
Plural, masculine, accusative, definite
common noun
ﺐﺘﻜﻟا
َ-
ﻦﻴﻤﻠﺴﻤﻟا
aluslimeen –
alkutuba
the Muslims –
the books
NCPlMGD
Plural, masculine, genitive, definite
common noun
ﺐﺘﻜﻟا
ِ-
ﻦﻴﻤﻠﺴﻤﻟا
almuslimeen –
alkutubi
the Muslims –
the books
NCPlFNI
Plural, feminine, nominative, indefinite
common noun
سراﺪﻣ
ٌ
تﺎﻤﻠﺴﻣ
ٌ–
madarisun –
muslimaatun
schools –
Muslims
NCPlFAI
Plural, feminine, accusative, indefinite
common noun
ﺎﺳراﺪﻣ
ً
ﺎﺗﺎﻤﻠﺴﻣ
ً–
madarisan –
muslimaatan
schools –
Muslims
NCPlFGI
Plural, feminine, genitive, indefinite,
common noun
سراﺪﻣ
ٍ
تﺎﻤﻠﺴﻣ
ٍ–
madarisin –
muslimaatin
schools –
Muslims
NCPlFND
Plural, feminine, nominative, definite
common noun
سراﺪﻤﻟا
ُ
تﺎﻤﻠﺴﻤﻟا
ُ–
almadarisu –
almuslimaatu
the schools –
the Muslims
NCPlFAD
Plural, feminine, accusative, definite
common noun
سراﺪﻤﻟا
َ
تﺎﻤﻠﺴﻤﻟا
َ–
almadarisa –
almuslimaata
the schools –
the Muslims
NCPlFGD
Plural, feminine, genitive, definite
common noun
سراﺪﻤﻟا
ِ
تﺎﻤﻠﺴﻤﻟا
ِ–
almadarisi –
almuslimaati</rdfs:comment>
        <rdfs:comment>The noun category can be subcategorised to include many of the subclasses described by Arabic grammarians that lend meaning to the word, for example, nouns of instrument and nouns of place and time.</rdfs:comment>
    </owl:Class>
    


    <!-- http://purl.org/olia/arabic_khoja.owl#CommonRelativePronoun -->

    <owl:Class rdf:about="http://purl.org/olia/arabic_khoja.owl#CommonRelativePronoun">
        <rdfs:subClassOf rdf:resource="http://purl.org/olia/arabic_khoja.owl#RelativePronoun"/>
        <rdfs:comment>
		Relative pronouns in Arabic are two types: special and common. The special relative pronouns are the those that have singular, dual, plural. These are six: الَّذِي ، اللَّذَان ، الَّذِيْن ، الَّتِي ، اللَّتَان ، اللَّاتِي, as listed in the table above. اللَّذان and اللَّتَان become اللَّذَيْن and اللَّتَيْن in the accusative and genitive cases. The common relative pronouns that has the same form for the singular, dual, and plural. These are مَنْ and مَا. The first (مَنْ) is used for human, while مَا is used for non-human. ...
		
		مَنْ is used for human masculine and feminine singular, dual, and plural nouns. The kind of nouns it refers to is known from the relative clause that follows, as in these examples:
		أَحْتَرِم مَنْ يَقُول الحَق.                     ‘I respect him who says the truth.’
		أَحْتَرِم مَنْ يَقُولُون الحَق.                  ‘I respect them who say the truth.’
		أَحْتَرِم مَنْ تَقُول الحَق.                     ‘I respect her who says the truth.’
		أَحْتَرِم مَنْ قَالَتَا الحَق.                      ‘I respect the two ladies who said the truth.’

		...

		مَا is used for non-human masculine and feminine singular, dual and plural nouns. Like مَنْ, the noun it refers to is know from the context, as in these examples:
		قَرَأتُ مَا كَتَبْتَ مِنْ مَقَالات.                ‘I read what you wrote (of the articles).’
		هَل سَمِعْتُ مَا قَالُوا (مِنْ خَبَر)؟          ‘did you hear what they said? (of the news)’
		
		(https://blogs.transparent.com/arabic/relative-clauses-in-arabic/)
		</rdfs:comment>
    </owl:Class>
    


    <!-- http://purl.org/olia/arabic_khoja.owl#Conjunction -->

    <owl:Class rdf:about="http://purl.org/olia/arabic_khoja.owl#Conjunction">
        <rdfs:subClassOf rdf:resource="http://purl.org/olia/arabic_khoja.owl#Particle"/>
        <rdfs:comment>PC
Conjunctions
ف– ﻰﺘﺡ –و
f – hta – w
</rdfs:comment>
    </owl:Class>
    


    <!-- http://purl.org/olia/arabic_khoja.owl#DayOfTheWeek -->

    <owl:Class rdf:about="http://purl.org/olia/arabic_khoja.owl#DayOfTheWeek">
        <rdfs:subClassOf rdf:resource="http://purl.org/olia/arabic_khoja.owl#Residual"/>
        <rdfs:comment>RD
Residual, day of the week
ﻦﻴﻨﺛﻻا
alithnyn
</rdfs:comment>
    </owl:Class>
    


    <!-- http://purl.org/olia/arabic_khoja.owl#Definite -->

    <owl:Class rdf:about="http://purl.org/olia/arabic_khoja.owl#Definite">
        <rdfs:subClassOf rdf:resource="http://purl.org/olia/arabic_khoja.owl#Definiteness"/>
        <rdfs:comment>In Arabic nouns are marked for definiteness by the prefix that is the definite article.</rdfs:comment>
    </owl:Class>
    


    <!-- http://purl.org/olia/arabic_khoja.owl#Definiteness -->

    <owl:Class rdf:about="http://purl.org/olia/arabic_khoja.owl#Definiteness">
        <rdfs:subClassOf rdf:resource="http://purl.org/olia/arabic_khoja.owl#Feature"/>
        <rdfs:comment>The article is not described in Arabic as a category at all, and definiteness is just a linguistic feature that is realised by the definite article.

The way that definiteness is handled in Arabic is quite different to the way it is handled in EAGLES, and this difference is apparent when comparing the tagsets. In Arabic nouns are marked for definiteness by the prefix that is the definite article, unlike in English where the article itself can be definite or indefinite. In Arabic there is no indefinite article, and instead “nunation” is used.

Nunation is the doubling of the vowels at the end of nouns and all subclasses of nouns when they are indefinite. This doubling has the effect of adding a final “n” to the pronunciation, so that, kitabu becomes kitabun “book”.</rdfs:comment>
    </owl:Class>
    


    <!-- http://purl.org/olia/arabic_khoja.owl#DemonstrativePronoun -->

    <owl:Class rdf:about="http://purl.org/olia/arabic_khoja.owl#DemonstrativePronoun">
        <rdfs:subClassOf rdf:resource="http://purl.org/olia/arabic_khoja.owl#Pronoun"/>
        <rdfs:comment>NPrDSgM
Singular, masculine, demonstrative
pronoun
اﺬه– اذ – كاذ –ﻚﻟذ
hadhaa – dhaa –
dhaaka – dhaalika
This – that
NPrDSgF Singular, feminine, demonstrative pronoun
ﻩﺬه– يﺬه – ﻩذ – يذ – ﻚﻠﺗ –
كﺎﺗ–ﻚﻴﺗ
haadhihi – haadhee
– dhih – dhy – tilka
– taaka – teeka
This – that
NprDDuM Dual, masculine, demonstrative pronoun
ناﺬه– ناذ – ﻚﻥاذ – ﻦﻱﺬه –
ﻦﻱذ–ﻚﻨﻱذ
haadhani – dhaani
– dhaanika –
hadhaini –dhaini
This – that
NprDDuF Dual, feminine, demonstrative pronoun
نﺎﺘه– نﺎﺗ – ﻚﻥﺎﺗ – ﻦﻴﺘه – ﻦﻴﺗ
–ﻚﻨﻴﺗ
haatani – taani-
taanika – haataini
This – that
NPrDPl
Plural, neutral, demonstrative pronoun
ءﻻﺆه– ﻰﻟوأ – ءﻻوأ – ﻚﺉﻻوأ
– ﻚﻟﻻوأ –كﻻوأ
haaolaai – olaa-
olaaika- olaalika –
olaaka
</rdfs:comment>
    </owl:Class>
    


    <!-- http://purl.org/olia/arabic_khoja.owl#DualNumber -->

    <owl:Class rdf:about="http://purl.org/olia/arabic_khoja.owl#DualNumber">
        <rdfs:subClassOf rdf:resource="http://purl.org/olia/arabic_khoja.owl#Number"/>
    </owl:Class>
    


    <!-- http://purl.org/olia/arabic_khoja.owl#Exception -->

    <owl:Class rdf:about="http://purl.org/olia/arabic_khoja.owl#Exception">
        <rdfs:subClassOf rdf:resource="http://purl.org/olia/arabic_khoja.owl#Particle"/>
        <rdfs:comment>Arabic grammatical tradition already recognizes a subclass of Particle translated as Exceptions by Khoja, to cover some idiosyncratic words which do not fit other patterns: “ ... These include the Arabic words that are equivalent to the word except and the prefixes non-, un-, and im-.”
(Atwell 2007)</rdfs:comment>
        <rdfs:comment>PE
Exceptions
ﺮﻴﻏ–ىﻮﺳ
ghyr – swa
</rdfs:comment>
    </owl:Class>
    


    <!-- http://purl.org/olia/arabic_khoja.owl#Explanation -->

    <owl:Class rdf:about="http://purl.org/olia/arabic_khoja.owl#Explanation">
        <rdfs:subClassOf rdf:resource="http://purl.org/olia/arabic_khoja.owl#Particle"/>
        <rdfs:comment>PX
Explanations
يأ
ay
</rdfs:comment>
    </owl:Class>
    


    <!-- http://purl.org/olia/arabic_khoja.owl#Feature -->

    <owl:Class rdf:about="http://purl.org/olia/arabic_khoja.owl#Feature">
        <rdfs:subClassOf rdf:resource="http://purl.org/olia/system.owl#Feature"/>
        <rdfs:subClassOf>
            <owl:Restriction>
                <owl:onProperty rdf:resource="http://purl.org/olia/system.owl#hasTier"/>
                <owl:hasValue>POS</owl:hasValue>
            </owl:Restriction>
        </rdfs:subClassOf>
        <rdfs:comment>The current Arabic tagset can be extended to include many other features such as transitivity and voice for verbs, and derivation for nouns.

Arabic has two voices, the active and the passive.
Nouns in Arabic can be derived from other nouns or they can be derived from verbs.</rdfs:comment>
    </owl:Class>
    


    <!-- http://purl.org/olia/arabic_khoja.owl#FeminineGender -->

    <owl:Class rdf:about="http://purl.org/olia/arabic_khoja.owl#FeminineGender">
        <rdfs:subClassOf rdf:resource="http://purl.org/olia/arabic_khoja.owl#Gender"/>
    </owl:Class>
    


    <!-- http://purl.org/olia/arabic_khoja.owl#FirstPerson -->

    <owl:Class rdf:about="http://purl.org/olia/arabic_khoja.owl#FirstPerson">
        <rdfs:subClassOf rdf:resource="http://purl.org/olia/arabic_khoja.owl#Person"/>
    </owl:Class>
    


    <!-- http://purl.org/olia/arabic_khoja.owl#Foreign -->

    <owl:Class rdf:about="http://purl.org/olia/arabic_khoja.owl#Foreign">
        <rdfs:subClassOf rdf:resource="http://purl.org/olia/arabic_khoja.owl#Residual"/>
        <rdfs:comment>RF
Residual, foreign
رﻮﺟور
rwjwr
</rdfs:comment>
    </owl:Class>
    


    <!-- http://purl.org/olia/arabic_khoja.owl#Gender -->

    <owl:Class rdf:about="http://purl.org/olia/arabic_khoja.owl#Gender">
        <rdfs:subClassOf rdf:resource="http://purl.org/olia/arabic_khoja.owl#Feature"/>
    </owl:Class>
    


    <!-- http://purl.org/olia/arabic_khoja.owl#GenitiveCase -->

    <owl:Class rdf:about="http://purl.org/olia/arabic_khoja.owl#GenitiveCase">
        <rdfs:subClassOf rdf:resource="http://purl.org/olia/arabic_khoja.owl#Case"/>
    </owl:Class>
    


    <!-- http://purl.org/olia/arabic_khoja.owl#ImperativeVerb -->

    <owl:Class rdf:about="http://purl.org/olia/arabic_khoja.owl#ImperativeVerb">
        <rdfs:subClassOf rdf:resource="http://purl.org/olia/arabic_khoja.owl#Verb"/>
        <rdfs:comment>VIvSg2M
Second person, singular, masculine,
imperative verb
ﺮﺴآأ
ْ
aksir
Break!
VIvSg2F
Second person, singular, feminine,
imperative verb
يﺮﺴآأ
aksiry
Break!
VIvDu2
Second person, dual, neuter, imperative
verb
اﺮﺴآأ
aksiraa
Break!
VIvPl2M
Second person, plural, masculine,
imperative verb
اوﺮﺴآأ
aksroo
Break!
VIvPl2F
Second person, plural, feminine,
imperative verb
نﺮﺴآأ
aksirna
</rdfs:comment>
    </owl:Class>
    


    <!-- http://purl.org/olia/arabic_khoja.owl#ImperfectVerb -->

    <owl:Class rdf:about="http://purl.org/olia/arabic_khoja.owl#ImperfectVerb">
        <rdfs:subClassOf rdf:resource="http://purl.org/olia/arabic_khoja.owl#Verb"/>
        <rdfs:comment>The imperfect does not in itself express any idea of time, it merely indicates a begun, incomplete, or enduring existence either in present, past or future time. While the imperative verbs order or ask for something to be done in the future.</rdfs:comment>
        <rdfs:comment>VISg1I
First person, singular, neuter, indicative,
imperfect verb
ﺮﺴآأ
ُ
aksiru
I break
VISg1S
First person, singular, neuter, subjunctive,
imperfect verb
ﺮﺴآأ
َ
aksira
I break
VISg1J
First person, singular, neuter, jussive,
imperfect verb
ﺮﺴآأ
ْ
aksir
I break
VISg2MI
Second person, singular, masculine,
indicative, imperfect verb
ﺮﺴﻜﺗ
ُ
taksiru
You break
VISg2MS
Second person, singular, masculine,
subjunctive, imperfect verb
ﺮﺴﻜﺗ
َ
taksira
You break
VISg2MJ
Second person, singular, masculine,
jussive, imperfect verb
ﺮﺴﻜﺗ
ْ
taksir
You break
VISg2FI
Second person, singular, feminine,
indicative, imperfect verb
ﻦﻱﺮﺴﻜﺗ
taksiryna
You break
VISg2FS
Second person, singular, feminine,
subjunctive, imperfect verb
يﺮﺴﻜﺗ
taksiry
You break
VISg2FJ
Second person, singular, feminine, jussive,
imperfect verb
يﺮﺴﻜﺗ
taksiry
You break
VISg3MI
Third person, singular, masculine,
indicative, imperfect verb
ﺮﺴﻜﻱ
ُ
yaksiru
He breaks
VISg3MS
Third person, singular, masculine,
subjunctive, imperfect verb
ﺮﺴﻜﻱ
َ
yaksira
He breaks
VISg3MJ
Third person, singular, masculine, jussive,
imperfect verb
ﺮﺴﻜﻱ
ْ
yaksir
He breaks
VISg3FI
Third person, singular, feminine,
indicative, imperfect verb
ﺮﺴﻜﺗ
ُ
taksiru
She breaks
VISg3FS
Third person, singular, feminine,
subjunctive, imperfect verb
ﺮﺴﻜﺗ
َ
taksira
She breaks
VISg3FJ
Third person, singular, feminine, jussive,
imperfect verb
ﺮﺴﻜﺗ
ْ
taksir
She breaks
VIDu2I
Second person, dual, neuter, indicative,
imperfect verb
ناﺮﺴﻜﺗ
taksiraani
You break
VIDu2S
Second person, dual, neuter, subjunctive,
imperfect verb
اﺮﺴﻜﺗ
taksiraa
You break
VIDu2J
Second person, dual, neuter, jussive,
imperfect verb
اﺮﺴﻜﺗ
taksiraa
You break
VIDu3MI
Third person, dual, masculine, indicative,
imperfect verb
ناﺮﺴﻜﻱ
yaksiraani
They break
VIDu3MS
Third person, dual, masculine,
subjunctive, imperfect verb
اﺮﺴﻜﻱ
yaksiraa
They break
VIDu3MJ
Third person, dual, masculine, jussive,
imperfect verb
اﺮﺴﻜﻱ
yaksiraa
They break
VIDu3FI
Third person, dual, feminine, indicative,
imperfect verb
ناﺮﺴﻜﻱ
yaksiraan
They break
VIDu3FS
Third person, dual, feminine, subjunctive,
imperfect verb
اﺮﺴﻜﻱ
yaksiraa
They break
VIDu3FJ
Third person, dual, feminine, jussive,
imperfect verb
اﺮﺴﻜﻱ
yaksiraa
They break
VIPl1I
First person, plural, neuter, indicative,
imperfect verb
ﺮﺴﻜﻥ
ُ
naksiru
We break
VIPl1S
First person, plural, neuter, subjunctive,
imperfect verb
ﺮﺴﻜﻥ
َ
naksira
We break
VIPl1J
First person, plural, neuter, jussive,
imperfect verb
ﺮﺴﻜﻥ
ْ
naksir
We break
VIPl2MI
Second person, plural, masculine,
indicative, imperfect verb
نوﺮﺴﻜﺗ
taksiroon
You break
Page 12
VIPl2MS
Second person, plural, masculine,
subjunctive, imperfect verb
اوﺮﺴﻜﺗ
taksiroo
You break
VIPl2MJ
Second person, plural, masculine, jussive,
imperfect verb
اوﺮﺴﻜﺗ
taksiroo
You break
VIPl2FI
Second person, plural, feminine,
indicative, imperfect verb
نﺮﺴﻜﺗ
taksirna
You break
VIPl2FS
Second person, plural, feminine,
subjunctive, imperfect verb
نﺮﺴﻜﺗ
taksirna
You break
VIPl2FJ
Second person, plural, feminine, jussive,
imperfect verb
نﺮﺴﻜﺗ
taksirna
You break
VIPl3MI
Third person, plural, masculine, indicative,
imperfect verb
نوﺮﺴﻜﻱ
yaksiroon
They break
VIPl3MS
Third person, plural, masculine,
subjunctive, imperfect verb
اوﺮﺴﻜﻱ
yaksiroo
They break
VIPl3MJ
Third person, plural, masculine, jussive,
imperfect verb
اوﺮﺴﻜﻱ
yaksiroo
They break
VIPl3FI
Third person, plural, feminine, indicative,
imperfect verb
نﺮﺴﻜﻱ
yaksirna
They break
VIPl3FS
Third person, plural, feminine,
subjunctive, imperfect verb
نﺮﺴﻜﻱ
yaksirna
They break
VIPl3FJ
Third person, plural, feminine, jussive,
imperfect verb
نﺮﺴﻜﻱ
yaksirna
</rdfs:comment>
    </owl:Class>
    


    <!-- http://purl.org/olia/arabic_khoja.owl#Indefinite -->

    <owl:Class rdf:about="http://purl.org/olia/arabic_khoja.owl#Indefinite">
        <rdfs:subClassOf rdf:resource="http://purl.org/olia/arabic_khoja.owl#Definiteness"/>
        <rdfs:comment>In Arabic there is no indefinite article, and instead “nunation” is used. Nunation is the doubling of the vowels at the end of nouns and all subclasses of nouns when they are indefinite. This doubling has the effect of adding a final “n” to the pronunciation, so that, kitabu becomes kitabun “book”.</rdfs:comment>
    </owl:Class>
    


    <!-- http://purl.org/olia/arabic_khoja.owl#IndicativeMood -->

    <owl:Class rdf:about="http://purl.org/olia/arabic_khoja.owl#IndicativeMood">
        <rdfs:subClassOf rdf:resource="http://purl.org/olia/arabic_khoja.owl#Mood"/>
    </owl:Class>
    


    <!-- http://purl.org/olia/arabic_khoja.owl#Interjection -->

    <owl:Class rdf:about="http://purl.org/olia/arabic_khoja.owl#Interjection">
        <rdfs:subClassOf rdf:resource="http://purl.org/olia/arabic_khoja.owl#Particle"/>
        <rdfs:comment>PI
Interjections
ﺎﻱ–ﺎﻬﺘﻱأ
ya – aytha
</rdfs:comment>
    </owl:Class>
    


    <!-- http://purl.org/olia/arabic_khoja.owl#JussiveMood -->

    <owl:Class rdf:about="http://purl.org/olia/arabic_khoja.owl#JussiveMood">
        <rdfs:subClassOf rdf:resource="http://purl.org/olia/arabic_khoja.owl#Mood"/>
        <rdfs:comment>The jussive is needed to express a command in the first and third person. This mood is realised in Arabic by rejecting the final vowel and is sometimes called the apocopated imperfect.

The purpose of the jussive is to express a command in the first or third person as in ‘heena yahduru yalbas thiyaban nazyfatan’ which means “when he attends, let him (he must) wear clean clothes”, where the jussive is the word ‘yalbas’ “wear”. Also, there is no negative imperative in Arabic, so the negative particle followed by the jussive is used in its place, such as ‘la taktub’ “do not write”, where the jussive is the word ‘taktub’ “write”.</rdfs:comment>
    </owl:Class>
    


    <!-- http://purl.org/olia/arabic_khoja.owl#MasculineGender -->

    <owl:Class rdf:about="http://purl.org/olia/arabic_khoja.owl#MasculineGender">
        <rdfs:subClassOf rdf:resource="http://purl.org/olia/arabic_khoja.owl#Gender"/>
    </owl:Class>
    


    <!-- http://purl.org/olia/arabic_khoja.owl#Mathematical -->

    <owl:Class rdf:about="http://purl.org/olia/arabic_khoja.owl#Mathematical">
        <rdfs:subClassOf rdf:resource="http://purl.org/olia/arabic_khoja.owl#Residual"/>
        <rdfs:comment>RM
Residual, mathematical
÷
/
</rdfs:comment>
    </owl:Class>
    


    <!-- http://purl.org/olia/arabic_khoja.owl#MonthOfTheYear -->

    <owl:Class rdf:about="http://purl.org/olia/arabic_khoja.owl#MonthOfTheYear">
        <rdfs:subClassOf rdf:resource="http://purl.org/olia/arabic_khoja.owl#Residual"/>
        <rdfs:comment>Rmy
Residual, month of the year
مﺮﺤﻣ
mhrm
</rdfs:comment>
    </owl:Class>
    


    <!-- http://purl.org/olia/arabic_khoja.owl#Mood -->

    <owl:Class rdf:about="http://purl.org/olia/arabic_khoja.owl#Mood">
        <rdfs:subClassOf rdf:resource="http://purl.org/olia/arabic_khoja.owl#Feature"/>
    </owl:Class>
    


    <!-- http://purl.org/olia/arabic_khoja.owl#Negative -->

    <owl:Class rdf:about="http://purl.org/olia/arabic_khoja.owl#Negative">
        <rdfs:subClassOf rdf:resource="http://purl.org/olia/arabic_khoja.owl#Particle"/>
        <rdfs:comment>PN
Negatives
ﻢﻟ-
ﻻ
la – lm
</rdfs:comment>
    </owl:Class>
    


    <!-- http://purl.org/olia/arabic_khoja.owl#NeuterGender -->

    <owl:Class rdf:about="http://purl.org/olia/arabic_khoja.owl#NeuterGender">
        <rdfs:subClassOf rdf:resource="http://purl.org/olia/arabic_khoja.owl#Gender"/>
    </owl:Class>
    


    <!-- http://purl.org/olia/arabic_khoja.owl#NominativeCase -->

    <owl:Class rdf:about="http://purl.org/olia/arabic_khoja.owl#NominativeCase">
        <rdfs:subClassOf rdf:resource="http://purl.org/olia/arabic_khoja.owl#Case"/>
    </owl:Class>
    


    <!-- http://purl.org/olia/arabic_khoja.owl#Noun -->

    <owl:Class rdf:about="http://purl.org/olia/arabic_khoja.owl#Noun">
        <rdfs:subClassOf rdf:resource="http://purl.org/olia/arabic_khoja.owl#Word"/>
        <rdfs:comment>All subclasses of the noun inherit the tnwyn “nunation” when in the indefinite which is one of the main properties of the noun: Nunation is the doubling of the vowels at the end of nouns and all subclasses of nouns when they are indefinite. This doubling has the effect of adding a final “n” to the pronunciation, so that, kitabu becomes kitabun “book”.

Examples of these subcategories include:
• Singular, masculine, accusative, common noun such as ktab “book” in the sentence ‘akhadha alwaladu kitaban’ “the boy took a book”.
• Singular, masculine, genitive, common noun such as ktab “book” in the sentence ‘darastu min kitabin’ “I studied from a book”.
• Singular, feminine, nominative, common noun such as ktab “book” in the sentence ‘hadhihi madrasatun’ “this is a school”.

The linguistic attributes of nouns that have been used in this tagset are:
(i) Gender: M [masculine] F [feminine] N [neuter]
(ii) Number: Sg [singular] Pl [plural] Du [dual]
(iii) Person: 1 [first] 2 [second] 3 [third] 
(iv) Case: N [nominative] A [accusative] G [genitive] 
(v) Definiteness: D [definite] I [indefinite] </rdfs:comment>
    </owl:Class>
    


    <!-- http://purl.org/olia/arabic_khoja.owl#Number -->

    <owl:Class rdf:about="http://purl.org/olia/arabic_khoja.owl#Number">
        <rdfs:subClassOf rdf:resource="http://purl.org/olia/arabic_khoja.owl#Feature"/>
        <rdfs:comment>Arabic marks words not just for singular and plural but also for dual.</rdfs:comment>
    </owl:Class>
    


    <!-- http://purl.org/olia/arabic_khoja.owl#Numeral -->

    <owl:Class rdf:about="http://purl.org/olia/arabic_khoja.owl#Numeral">
        <rdfs:subClassOf rdf:resource="http://purl.org/olia/arabic_khoja.owl#Noun"/>
        <rdfs:comment>Examples of numerals include:
• Singular, masculine, nominative, indefinite cardinal number such as ‘arba’atun’ “four”.
• Singular, masculine, nominative, indefinite ordinal number such as ‘rabi’un’ “fourth”.
• Singular, masculine, numerical adjective such as ‘ruba’iyun’ “of four”.</rdfs:comment>
    </owl:Class>
    


    <!-- http://purl.org/olia/arabic_khoja.owl#NumericalAdjective -->

    <owl:Class rdf:about="http://purl.org/olia/arabic_khoja.owl#NumericalAdjective">
        <rdfs:subClassOf rdf:resource="http://purl.org/olia/arabic_khoja.owl#Numeral"/>
        <rdfs:comment>Numerical adjectives describe the number of sides to a shape, for example thmany “octagonal”. They also indicate a pair or couple when describing two people as in thna`y. 

NNuNaSgM Singular, masculine, numerical adjective
ﻲﻋﺎﺑر
rubaa’y
Of four
NNuNaSgF Singular, feminine, numerical adjective
ﺔﻴﻋﺎﺑر
rubaa’iya</rdfs:comment>
    </owl:Class>
    


    <!-- http://purl.org/olia/arabic_khoja.owl#OrdinalNumeral -->

    <owl:Class rdf:about="http://purl.org/olia/arabic_khoja.owl#OrdinalNumeral">
        <rdfs:subClassOf rdf:resource="http://purl.org/olia/arabic_khoja.owl#Numeral"/>
        <rdfs:comment>NNuOrSgM Singular, masculine, ordinal number
ﻊﺑار
raabi’
Fourth
NNuOrSgF Singular, feminine, ordinal number
ﺔﻌﺑار
raabia
</rdfs:comment>
    </owl:Class>
    


    <!-- http://purl.org/olia/arabic_khoja.owl#OtherResidual -->

    <owl:Class rdf:about="http://purl.org/olia/arabic_khoja.owl#OtherResidual">
        <rdfs:subClassOf rdf:resource="http://purl.org/olia/arabic_khoja.owl#Residual"/>
        <rdfs:comment>RO
Residual, other
لﺁ
Aal</rdfs:comment>
    </owl:Class>
    


    <!-- http://purl.org/olia/arabic_khoja.owl#Particle -->

    <owl:Class rdf:about="http://purl.org/olia/arabic_khoja.owl#Particle">
        <rdfs:subClassOf rdf:resource="http://purl.org/olia/arabic_khoja.owl#Word"/>
        <rdfs:comment>Examples of particles include:
• Prepositions fy “in”
• Adverbial particles swf “shall”
• Conjunctions w “and”
• Interjections ya “you”
• Exceptions swa “Except”
• Negatives lm “Not”
• Answers ajl “yes”
• Explanations ay “that is”
• Subordinates lw “if”</rdfs:comment>
        <rdfs:comment>Particles are sometimes affixes; for example the definite article ‘al’ is well-known as a prefix in Arabic loan-words in other languages, e.g. algebra, Algarve. These are handled by a compound tag, reminiscent of the Brown tagging scheme: “... For morphologically complex words a combination of tags is used. For example, the word walktab ‘and the book’ is given the tag PC+NCSgMND, where PC indicates a particle that is a conjunction, and NCSgMND indicates a singular, masculine, nominative, definite noun.” (Atwell 2007)</rdfs:comment>
    </owl:Class>
    


    <!-- http://purl.org/olia/arabic_khoja.owl#PerfectVerb -->

    <owl:Class rdf:about="http://purl.org/olia/arabic_khoja.owl#PerfectVerb">
        <rdfs:subClassOf rdf:resource="http://purl.org/olia/arabic_khoja.owl#Verb"/>
        <rdfs:comment>The definition of perfect verbs not only includes (i) the equivalent of English past tense verbs (i.e. to describe acts completed in some past time) but also (ii) describes acts which at the moment of speaking have already been completed and remain in a state of completion, (iii) describes a past act that often took place or still takes place (i.e. commentators are agreed (have agreed and still agree)), (iv) describes an act which is just completed at the moment by the very act of speaking it (I sell thee this), and (v) describes acts which is certain to occur that it can be described as having already taken place (mostly used in promises, treaties and so on).</rdfs:comment>
        <rdfs:comment>VPSg1
First person, singular, neuter, perfect verb
تﺮﺴآ
ُ
kasartu
I broke
VPSg2M
Second person, singular, masculine,
perfect verb
تﺮﺴآ
َ
kasarta
You broke
VPSg2F
Second person, singular, feminine, perfect
verb
تﺮﺴآ
ِ
kasarti
You broke
VPSg3M
Third person, singular, masculine, perfect
verb
آ
ﺮﺴ
kasara
He broke
VPSg3F
Third person, singular, feminine, perfect
verb
تﺮﺴآ
ْ
kasarat
She broke
VPDu2
Second person, dual, neuter, perfect verb
ﺎﻤﺗﺮﺴآ
kasartumaa
You (two)
broke
Page 11
VPDu3M Third person, dual, masculine, perfect verb
اﺮﺴآ
kasaraa
They (two)
broke
VPDu3F Third person, dual, feminine, perfect verb
ﺎﺗﺮﺴآ
kasarataa
They (two)
broke
VPPl1
First person, plural, neuter, perfect verb
ﺎﻥﺮﺴآ
kasarnaa
We broke
VPPl2M
Second person, plural, masculine, perfect
verb
ﻢﺗﺮﺴآ
kasartum
You broke
VPPl2F
Second person, plural, feminine, perfect
verb
ﻦﺗﺮﺴآ
kasartunna
You broke
VPPl3M
Third person, plural, masculine, perfect
verb
اوﺮﺴآ
kasaroo
They broke
VPPl3F
Third person, plural, feminine, perfect
verb
نﺮﺴآ
kasarna
</rdfs:comment>
    </owl:Class>
    


    <!-- http://purl.org/olia/arabic_khoja.owl#Person -->

    <owl:Class rdf:about="http://purl.org/olia/arabic_khoja.owl#Person">
        <rdfs:subClassOf rdf:resource="http://purl.org/olia/arabic_khoja.owl#Feature"/>
    </owl:Class>
    


    <!-- http://purl.org/olia/arabic_khoja.owl#PersonalPronoun -->

    <owl:Class rdf:about="http://purl.org/olia/arabic_khoja.owl#PersonalPronoun">
        <rdfs:subClassOf rdf:resource="http://purl.org/olia/arabic_khoja.owl#Pronoun"/>
        <rdfs:comment>NPrPSg1
First person, singular, neuter, personal
pronoun
ﺎﻥأ–
ﻲﺑﺎﺘآ
-
ﻲﻨﺑﺮﺿ
ana- kitaabee –
darabanee
Me – my book
– he hit me
NPrPSg2M
Second person, singular, masculine,
personal pronoun
ﺖﻥأ
َ
ﻚﺑﺎﺘآ
َ–
anta – kitaabuka
You – your
book
NPrPSg2F
Second person, singular, feminine,
personal pronoun
ﺖﻥأ
ِ
ﻚﺑﺎﺘآ
ِ–
anti – kitaabuki
You – your
book
NPrPSg3M
Third person, singular, masculine,
personal pronoun
ﻮه
-
ﻪﺑﺎﺘآ
kitaabahu – huwa
His book –
him
NPrPSg3F Third person, singular, feminine, personal
ﻲه
-
ﺎﻬﺑﺎﺘآ
kitaabuhaa – hiya Her book –
Page 9
pronoun
her
NPrPDu2
Second person, dual, neuter, personal
pronoun
ﺎﻤﺘﻥأ–ﺎﻤﻜﺑﺎﺘآ
antumaa –
kitaabakumaa
You two –
your book
NPrPDu3
Third person, dual, neuter, personal
pronoun
ﺎﻤه–ﺎﻤﻬﺑﺎﺘآ
humaa –
kitaabahumaa
Those two –
their book
NPrPPl1
First person, plural, neuter, personal
pronoun
ﻦﺤﻥ–ﺎﻨﺑﺎﺘآ
nahnu – kitaabunaa Us – our book
NPrPPl2M
Second person, plural, masculine, personal
pronoun
ﻢﺘﻥأ–ﻢﻜﺑﺎﺘآ
antum –
kitaabakum
You – your
book
NPrPPl2F
Second person, plural, feminine, personal
pronoun
ﻦﺘﻥأ–ﻦﻜﺑﺎﺘآ
antunna –
kitaabakunna
You – your
book
NPrPPl3M
Third person, plural, masculine, personal
pronoun
ﻢه–ﻢﻬﺑﺎﺘآ
hum – kitaabahum
Them – their
book
NPrPPl3F
Third person, plural, feminine, personal
pronoun
ﻦه
-
ﻦﻬﺑﺎﺘآ
kitaabahunna –
hunna</rdfs:comment>
    </owl:Class>
    


    <!-- http://purl.org/olia/arabic_khoja.owl#PluralNumber -->

    <owl:Class rdf:about="http://purl.org/olia/arabic_khoja.owl#PluralNumber">
        <rdfs:subClassOf rdf:resource="http://purl.org/olia/arabic_khoja.owl#Number"/>
        <rdfs:comment>Since Arabic contains three different kinds of plurals, these could also be included in the tagset. The three types of plurals are: the masculine sound plural, the feminine sound plural, and the broken plural. The first two are recognised in Arabic morphologically by suffixes, while the last, is derived by the following of fixed patterns.</rdfs:comment>
    </owl:Class>
    


    <!-- http://purl.org/olia/arabic_khoja.owl#Preposition -->

    <owl:Class rdf:about="http://purl.org/olia/arabic_khoja.owl#Preposition">
        <rdfs:subClassOf rdf:resource="http://purl.org/olia/arabic_khoja.owl#Particle"/>
        <rdfs:comment>PPr
Prepositions
ك– ل – ﻦﻣ – ﻊﻣ –ﻲﻓ
ka – li – min –
ma’a – fy
</rdfs:comment>
    </owl:Class>
    


    <!-- http://purl.org/olia/arabic_khoja.owl#Pronoun -->

    <owl:Class rdf:about="http://purl.org/olia/arabic_khoja.owl#Pronoun">
        <rdfs:subClassOf rdf:resource="http://purl.org/olia/arabic_khoja.owl#Noun"/>
        <rdfs:comment>The personal pronouns can be detached words such as hwa “he”, or attached to a word in the form of a clitic. The attached pronouns can be attached to nouns to indicate possession, to verbs as direct object, or attached to prepositions such as fyh “in it”.
Some examples of pronouns include:
• Third person, singular, masculine, personal pronoun such as hwa “him”.
• Singular, feminine, demonstrative pronoun such as hdhh “this”.</rdfs:comment>
    </owl:Class>
    


    <!-- http://purl.org/olia/arabic_khoja.owl#ProperNoun -->

    <owl:Class rdf:about="http://purl.org/olia/arabic_khoja.owl#ProperNoun">
        <rdfs:subClassOf rdf:resource="http://purl.org/olia/arabic_khoja.owl#Noun"/>
        <rdfs:comment>NP
Proper noun
ﻩﺪﺟ–ﻦﻱﺮﻴﺵ
Jiddah – Shyryn</rdfs:comment>
    </owl:Class>
    


    <!-- http://purl.org/olia/arabic_khoja.owl#Punctuation -->

    <owl:Class rdf:about="http://purl.org/olia/arabic_khoja.owl#Punctuation">
        <rdfs:subClassOf rdf:resource="http://purl.org/olia/arabic_khoja.owl#Word"/>
        <rdfs:comment>The punctuation category contains all punctuation symbols, both Arabic and foreign.

PU
Punctuation
؟
?
</rdfs:comment>
    </owl:Class>
    


    <!-- http://purl.org/olia/arabic_khoja.owl#RelativePronoun -->

    <owl:Class rdf:about="http://purl.org/olia/arabic_khoja.owl#RelativePronoun">
        <rdfs:subClassOf rdf:resource="http://purl.org/olia/arabic_khoja.owl#Pronoun"/>
        <rdfs:comment>Examples of relative pronouns include:
• Dual, feminine, specific, relative pronoun such as alltan “who”.
• Plural, masculine, specific, relative pronoun such as alldhyn “who”.
• Common, relative pronoun such as ‘men’ “who”.</rdfs:comment>
        <rdfs:comment>NPrRSSgM
Singular, masculine, specific, relative
pronoun
يﺬﻟا
allathi
Who
NPrRSSgF
Singular, feminines, specific, relative
pronoun
ﻲﺘﻟا
allati
Who
NPrRSDuM Dual, masculine, specific, relative pronoun
ناﺬﻠﻟا–ﻦﻱﺬﻠﻟا
alladhaani –
alladhaini
Who
NPrRSDuF Dual, feminine, specific, relative pronoun
ﻠﻟا
نﺎﺘ –ﻦﻴﺘﻠﻟا
allataani –
allataini
Who
NPrRSPlM
Plural, masculine, specific, relative
pronoun
ﻦﻱﺬﻠﻟا
-
ﻲﺉﻼﻟا
allaiy – alladheena
Who
NPrRSPlf Plural, feminine, specific, relative pronoun
ﻲﺗﻼﻟا
-
ﻲﺉﻼﻟا
allaaiy - allatee
Who
NPrRC
Common, relative pronoun
ﻦﻣ– ﺎﻣ –ﺎﻤﻬﻣ
men – maa –
mahmaa</rdfs:comment>
    </owl:Class>
    


    <!-- http://purl.org/olia/arabic_khoja.owl#Residual -->

    <owl:Class rdf:about="http://purl.org/olia/arabic_khoja.owl#Residual">
        <rdfs:subClassOf rdf:resource="http://purl.org/olia/arabic_khoja.owl#Word"/>
        <rdfs:comment>The residual category contains foreign words, mathematical formulae and numbers.</rdfs:comment>
    </owl:Class>
    


    <!-- http://purl.org/olia/arabic_khoja.owl#ResidualNumber -->

    <owl:Class rdf:about="http://purl.org/olia/arabic_khoja.owl#ResidualNumber">
        <rdfs:subClassOf rdf:resource="http://purl.org/olia/arabic_khoja.owl#Residual"/>
        <rdfs:comment>RN
Residual, number
3
3
</rdfs:comment>
    </owl:Class>
    


    <!-- http://purl.org/olia/arabic_khoja.owl#SecondPerson -->

    <owl:Class rdf:about="http://purl.org/olia/arabic_khoja.owl#SecondPerson">
        <rdfs:subClassOf rdf:resource="http://purl.org/olia/arabic_khoja.owl#Person"/>
    </owl:Class>
    


    <!-- http://purl.org/olia/arabic_khoja.owl#SingularNumber -->

    <owl:Class rdf:about="http://purl.org/olia/arabic_khoja.owl#SingularNumber">
        <rdfs:subClassOf rdf:resource="http://purl.org/olia/arabic_khoja.owl#Number"/>
    </owl:Class>
    


    <!-- http://purl.org/olia/arabic_khoja.owl#SpecificRelativePronoun -->

    <owl:Class rdf:about="http://purl.org/olia/arabic_khoja.owl#SpecificRelativePronoun">
        <rdfs:subClassOf rdf:resource="http://purl.org/olia/arabic_khoja.owl#RelativePronoun"/>
    </owl:Class>
    


    <!-- http://purl.org/olia/arabic_khoja.owl#SubjunctiveMood -->

    <owl:Class rdf:about="http://purl.org/olia/arabic_khoja.owl#SubjunctiveMood">
        <rdfs:subClassOf rdf:resource="http://purl.org/olia/arabic_khoja.owl#Mood"/>
    </owl:Class>
    


    <!-- http://purl.org/olia/arabic_khoja.owl#Subordinate -->

    <owl:Class rdf:about="http://purl.org/olia/arabic_khoja.owl#Subordinate">
        <rdfs:subClassOf rdf:resource="http://purl.org/olia/arabic_khoja.owl#Particle"/>
        <rdfs:comment>PS
Subordinates
ﺎﻣ–ﻮﻟ
ma – lw
</rdfs:comment>
    </owl:Class>
    


    <!-- http://purl.org/olia/arabic_khoja.owl#ThirdPerson -->

    <owl:Class rdf:about="http://purl.org/olia/arabic_khoja.owl#ThirdPerson">
        <rdfs:subClassOf rdf:resource="http://purl.org/olia/arabic_khoja.owl#Person"/>
    </owl:Class>
    


    <!-- http://purl.org/olia/arabic_khoja.owl#Verb -->

    <owl:Class rdf:about="http://purl.org/olia/arabic_khoja.owl#Verb">
        <rdfs:subClassOf rdf:resource="http://purl.org/olia/arabic_khoja.owl#Word"/>
        <rdfs:comment>Verbs are defined in ancient Arabic grammar as being perfect, imperfect or imperative. This classification is an important part of Arabic, and trying to mould Arabic verbs to fit the traditional past, present and future tenses of Indo-European languages would be very unnatural.

Examples of verbs include:
• First person, singular, neuter, perfect verb ‘kasartu’ “I broke”.
• First person, singular, neuter, indicative, imperfect verb ‘aksiru’ “I break”
• Second person, singular, masculine, imperative verb ‘aksir’ “Break!

The verbal attributes that have been used in our tagset are:
(i) Gender: M [masculine] F [feminine] N [neuter] 
(ii) Number: Sg [singular] Pl [plural] Du [dual]
(iii) Person: 1 [first] 2 [second] 3 [third] 
(iv) Mood: I [indicative] S [subjunctive] J [jussive]
The two most notable verbal attributes that are fundamental to Arabic but do not normally appear in Indo-European tagsets are the dual number, and the jussive mood.</rdfs:comment>
    </owl:Class>
    


    <!-- http://purl.org/olia/arabic_khoja.owl#Word -->

    <owl:Class rdf:about="http://purl.org/olia/arabic_khoja.owl#Word">
        <rdfs:subClassOf rdf:resource="http://purl.org/olia/system.owl#UnitOfAnnotation"/>
        <rdfs:subClassOf>
            <owl:Restriction>
                <owl:onProperty rdf:resource="http://purl.org/olia/system.owl#hasTier"/>
                <owl:hasValue>POS</owl:hasValue>
            </owl:Restriction>
        </rdfs:subClassOf>
        <owl:versionInfo>Word taxonomy follows Khoja et al. (2001), Appendix C.</owl:versionInfo>
    </owl:Class>
    


    <!-- 
    ///////////////////////////////////////////////////////////////////////////////////////
    //
    // Individuals
    //
    ///////////////////////////////////////////////////////////////////////////////////////
     -->

    


    <!-- http://purl.org/olia/arabic_khoja.owl#Du -->

    <owl:NamedIndividual rdf:about="http://purl.org/olia/arabic_khoja.owl#Du">
        <rdf:type rdf:resource="http://purl.org/olia/arabic_khoja.owl#DualNumber"/>
        <hasCase rdf:resource="http://purl.org/olia/arabic_khoja.owl#Du"/>
        <system:hasTagContaining>Du</system:hasTagContaining>
    </owl:NamedIndividual>
    


    <!-- http://purl.org/olia/arabic_khoja.owl#N -->

    <owl:NamedIndividual rdf:about="http://purl.org/olia/arabic_khoja.owl#N">
        <rdf:type rdf:resource="http://purl.org/olia/arabic_khoja.owl#Noun"/>
        <system:hasTagStartingWith>N</system:hasTagStartingWith>
    </owl:NamedIndividual>
    


    <!-- http://purl.org/olia/arabic_khoja.owl#N......D -->

    <owl:NamedIndividual rdf:about="http://purl.org/olia/arabic_khoja.owl#N......D">
        <rdf:type rdf:resource="http://purl.org/olia/arabic_khoja.owl#Definite"/>
        <hasCase rdf:resource="http://purl.org/olia/arabic_khoja.owl#N......D"/>
        <system:hasTagMatching>^N[CPA].....D$</system:hasTagMatching>
    </owl:NamedIndividual>
    


    <!-- http://purl.org/olia/arabic_khoja.owl#N......I -->

    <owl:NamedIndividual rdf:about="http://purl.org/olia/arabic_khoja.owl#N......I">
        <rdf:type rdf:resource="http://purl.org/olia/arabic_khoja.owl#Indefinite"/>
        <hasCase rdf:resource="http://purl.org/olia/arabic_khoja.owl#N......I"/>
        <system:hasTagMatching>^N[CPA].....I$</system:hasTagMatching>
    </owl:NamedIndividual>
    


    <!-- http://purl.org/olia/arabic_khoja.owl#N.....A. -->

    <owl:NamedIndividual rdf:about="http://purl.org/olia/arabic_khoja.owl#N.....A.">
        <rdf:type rdf:resource="http://purl.org/olia/arabic_khoja.owl#AccusativeCase"/>
        <hasCase rdf:resource="http://purl.org/olia/arabic_khoja.owl#N.....A."/>
        <system:hasTagMatching>^N[CPA]....A.$</system:hasTagMatching>
    </owl:NamedIndividual>
    


    <!-- http://purl.org/olia/arabic_khoja.owl#N.....G. -->

    <owl:NamedIndividual rdf:about="http://purl.org/olia/arabic_khoja.owl#N.....G.">
        <rdf:type rdf:resource="http://purl.org/olia/arabic_khoja.owl#GenitiveCase"/>
        <hasCase rdf:resource="http://purl.org/olia/arabic_khoja.owl#N.....G."/>
        <system:hasTagMatching>^N[CPA]....G.$</system:hasTagMatching>
    </owl:NamedIndividual>
    


    <!-- http://purl.org/olia/arabic_khoja.owl#N.....N. -->

    <owl:NamedIndividual rdf:about="http://purl.org/olia/arabic_khoja.owl#N.....N.">
        <rdf:type rdf:resource="http://purl.org/olia/arabic_khoja.owl#NominativeCase"/>
        <hasCase rdf:resource="http://purl.org/olia/arabic_khoja.owl#N.....N."/>
        <system:hasTagMatching>^N[CPA]....N.$</system:hasTagMatching>
    </owl:NamedIndividual>
    


    <!-- http://purl.org/olia/arabic_khoja.owl#N....F.. -->

    <owl:NamedIndividual rdf:about="http://purl.org/olia/arabic_khoja.owl#N....F..">
        <rdf:type rdf:resource="http://purl.org/olia/arabic_khoja.owl#FeminineGender"/>
        <hasCase rdf:resource="http://purl.org/olia/arabic_khoja.owl#N....F.."/>
        <system:hasTagMatching>^N[CPA]...F..$</system:hasTagMatching>
    </owl:NamedIndividual>
    


    <!-- http://purl.org/olia/arabic_khoja.owl#N....M.. -->

    <owl:NamedIndividual rdf:about="http://purl.org/olia/arabic_khoja.owl#N....M..">
        <rdf:type rdf:resource="http://purl.org/olia/arabic_khoja.owl#MasculineGender"/>
        <hasCase rdf:resource="http://purl.org/olia/arabic_khoja.owl#N....M.."/>
        <system:hasTagMatching>^N[CPA]...M..$</system:hasTagMatching>
    </owl:NamedIndividual>
    


    <!-- http://purl.org/olia/arabic_khoja.owl#N....N.. -->

    <owl:NamedIndividual rdf:about="http://purl.org/olia/arabic_khoja.owl#N....N..">
        <rdf:type rdf:resource="http://purl.org/olia/arabic_khoja.owl#NeuterGender"/>
        <hasCase rdf:resource="http://purl.org/olia/arabic_khoja.owl#N....N.."/>
        <system:hasTagMatching>^N[CPA]...N..$</system:hasTagMatching>
    </owl:NamedIndividual>
    


    <!-- http://purl.org/olia/arabic_khoja.owl#NAC -->

    <owl:NamedIndividual rdf:about="http://purl.org/olia/arabic_khoja.owl#NAC">
        <rdf:type rdf:resource="http://purl.org/olia/arabic_khoja.owl#Adjective"/>
        <system:hasTagStartingWith>NAC</system:hasTagStartingWith>
    </owl:NamedIndividual>
    


    <!-- http://purl.org/olia/arabic_khoja.owl#NAC..F -->

    <owl:NamedIndividual rdf:about="http://purl.org/olia/arabic_khoja.owl#NAC..F">
        <rdf:type rdf:resource="http://purl.org/olia/arabic_khoja.owl#FeminineGender"/>
        <hasCase rdf:resource="http://purl.org/olia/arabic_khoja.owl#NAC..F"/>
        <system:hasTagStartingWith>^NAC..F.*</system:hasTagStartingWith>
    </owl:NamedIndividual>
    


    <!-- http://purl.org/olia/arabic_khoja.owl#NAC..M -->

    <owl:NamedIndividual rdf:about="http://purl.org/olia/arabic_khoja.owl#NAC..M">
        <rdf:type rdf:resource="http://purl.org/olia/arabic_khoja.owl#MasculineGender"/>
        <hasCase rdf:resource="http://purl.org/olia/arabic_khoja.owl#NAC..M"/>
        <system:hasTagStartingWith>^NAC..M.*</system:hasTagStartingWith>
    </owl:NamedIndividual>
    


    <!-- http://purl.org/olia/arabic_khoja.owl#NAC..N -->

    <owl:NamedIndividual rdf:about="http://purl.org/olia/arabic_khoja.owl#NAC..N">
        <rdf:type rdf:resource="http://purl.org/olia/arabic_khoja.owl#NeuterGender"/>
        <hasCase rdf:resource="http://purl.org/olia/arabic_khoja.owl#NAC..N"/>
        <system:hasTagStartingWith>^NAC..N.*</system:hasTagStartingWith>
    </owl:NamedIndividual>
    


    <!-- http://purl.org/olia/arabic_khoja.owl#NAC.A. -->

    <owl:NamedIndividual rdf:about="http://purl.org/olia/arabic_khoja.owl#NAC.A.">
        <rdf:type rdf:resource="http://purl.org/olia/arabic_khoja.owl#AccusativeCase"/>
        <hasCase rdf:resource="http://purl.org/olia/arabic_khoja.owl#NAC.A."/>
        <system:hasTagMatching>^NAC.*A[DI]$</system:hasTagMatching>
    </owl:NamedIndividual>
    


    <!-- http://purl.org/olia/arabic_khoja.owl#NAC.G. -->

    <owl:NamedIndividual rdf:about="http://purl.org/olia/arabic_khoja.owl#NAC.G.">
        <rdf:type rdf:resource="http://purl.org/olia/arabic_khoja.owl#GenitiveCase"/>
        <hasCase rdf:resource="http://purl.org/olia/arabic_khoja.owl#NAC.G."/>
        <system:hasTagMatching>^NAC.*G[DI]$</system:hasTagMatching>
    </owl:NamedIndividual>
    


    <!-- http://purl.org/olia/arabic_khoja.owl#NAC.N. -->

    <owl:NamedIndividual rdf:about="http://purl.org/olia/arabic_khoja.owl#NAC.N.">
        <rdf:type rdf:resource="http://purl.org/olia/arabic_khoja.owl#NominativeCase"/>
        <hasCase rdf:resource="http://purl.org/olia/arabic_khoja.owl#NAC.N."/>
        <system:hasTagMatching>^NAC.*N[DI]$</system:hasTagMatching>
    </owl:NamedIndividual>
    


    <!-- http://purl.org/olia/arabic_khoja.owl#NC -->

    <owl:NamedIndividual rdf:about="http://purl.org/olia/arabic_khoja.owl#NC">
        <rdf:type rdf:resource="http://purl.org/olia/arabic_khoja.owl#CommonNoun"/>
        <system:hasTagStartingWith>NC</system:hasTagStartingWith>
    </owl:NamedIndividual>
    


    <!-- http://purl.org/olia/arabic_khoja.owl#NNu -->

    <owl:NamedIndividual rdf:about="http://purl.org/olia/arabic_khoja.owl#NNu">
        <rdf:type rdf:resource="http://purl.org/olia/arabic_khoja.owl#Numeral"/>
        <system:hasTagStartingWith>NNu</system:hasTagStartingWith>
    </owl:NamedIndividual>
    


    <!-- http://purl.org/olia/arabic_khoja.owl#NNu.F -->

    <owl:NamedIndividual rdf:about="http://purl.org/olia/arabic_khoja.owl#NNu.F">
        <rdf:type rdf:resource="http://purl.org/olia/arabic_khoja.owl#FeminineGender"/>
        <hasCase rdf:resource="http://purl.org/olia/arabic_khoja.owl#NNu.F"/>
        <system:hasTagMatching>^NNu.*F$</system:hasTagMatching>
    </owl:NamedIndividual>
    


    <!-- http://purl.org/olia/arabic_khoja.owl#NNu.M -->

    <owl:NamedIndividual rdf:about="http://purl.org/olia/arabic_khoja.owl#NNu.M">
        <rdf:type rdf:resource="http://purl.org/olia/arabic_khoja.owl#MasculineGender"/>
        <hasCase rdf:resource="http://purl.org/olia/arabic_khoja.owl#NNu.M"/>
        <system:hasTagMatching>^NNu.*M$</system:hasTagMatching>
    </owl:NamedIndividual>
    


    <!-- http://purl.org/olia/arabic_khoja.owl#NNu.N -->

    <owl:NamedIndividual rdf:about="http://purl.org/olia/arabic_khoja.owl#NNu.N">
        <rdf:type rdf:resource="http://purl.org/olia/arabic_khoja.owl#NeuterGender"/>
        <hasCase rdf:resource="http://purl.org/olia/arabic_khoja.owl#NNu.N"/>
        <system:hasTagMatching>^NNu.*N$</system:hasTagMatching>
    </owl:NamedIndividual>
    


    <!-- http://purl.org/olia/arabic_khoja.owl#NNuCa -->

    <owl:NamedIndividual rdf:about="http://purl.org/olia/arabic_khoja.owl#NNuCa">
        <rdf:type rdf:resource="http://purl.org/olia/arabic_khoja.owl#CardinalNumeral"/>
        <system:hasTagStartingWith>NNuCa</system:hasTagStartingWith>
    </owl:NamedIndividual>
    


    <!-- http://purl.org/olia/arabic_khoja.owl#NNuNa -->

    <owl:NamedIndividual rdf:about="http://purl.org/olia/arabic_khoja.owl#NNuNa">
        <rdf:type rdf:resource="http://purl.org/olia/arabic_khoja.owl#NumericalAdjective"/>
        <system:hasTagStartingWith>NNuNa</system:hasTagStartingWith>
    </owl:NamedIndividual>
    


    <!-- http://purl.org/olia/arabic_khoja.owl#NNuOr -->

    <owl:NamedIndividual rdf:about="http://purl.org/olia/arabic_khoja.owl#NNuOr">
        <rdf:type rdf:resource="http://purl.org/olia/arabic_khoja.owl#OrdinalNumeral"/>
        <system:hasTagStartingWith>NNuOr</system:hasTagStartingWith>
    </owl:NamedIndividual>
    


    <!-- http://purl.org/olia/arabic_khoja.owl#NP -->

    <owl:NamedIndividual rdf:about="http://purl.org/olia/arabic_khoja.owl#NP">
        <rdf:type rdf:resource="http://purl.org/olia/arabic_khoja.owl#ProperNoun"/>
        <system:hasTag>NP</system:hasTag>
    </owl:NamedIndividual>
    


    <!-- http://purl.org/olia/arabic_khoja.owl#NPr -->

    <owl:NamedIndividual rdf:about="http://purl.org/olia/arabic_khoja.owl#NPr">
        <rdf:type rdf:resource="http://purl.org/olia/arabic_khoja.owl#Pronoun"/>
        <system:hasTagStartingWith>NPr</system:hasTagStartingWith>
    </owl:NamedIndividual>
    


    <!-- http://purl.org/olia/arabic_khoja.owl#NPr.F -->

    <owl:NamedIndividual rdf:about="http://purl.org/olia/arabic_khoja.owl#NPr.F">
        <rdf:type rdf:resource="http://purl.org/olia/arabic_khoja.owl#FeminineGender"/>
        <hasCase rdf:resource="http://purl.org/olia/arabic_khoja.owl#NPr.F"/>
        <system:hasTagMatching>^NPr.*F$</system:hasTagMatching>
    </owl:NamedIndividual>
    


    <!-- http://purl.org/olia/arabic_khoja.owl#NPr.M -->

    <owl:NamedIndividual rdf:about="http://purl.org/olia/arabic_khoja.owl#NPr.M">
        <rdf:type rdf:resource="http://purl.org/olia/arabic_khoja.owl#MasculineGender"/>
        <hasCase rdf:resource="http://purl.org/olia/arabic_khoja.owl#NPr.M"/>
        <system:hasTagMatching>^NPr.*M$</system:hasTagMatching>
    </owl:NamedIndividual>
    


    <!-- http://purl.org/olia/arabic_khoja.owl#NPr.N -->

    <owl:NamedIndividual rdf:about="http://purl.org/olia/arabic_khoja.owl#NPr.N">
        <rdf:type rdf:resource="http://purl.org/olia/arabic_khoja.owl#NeuterGender"/>
        <hasCase rdf:resource="http://purl.org/olia/arabic_khoja.owl#NPr.N"/>
        <system:hasTagMatching>^NPr.*N$</system:hasTagMatching>
    </owl:NamedIndividual>
    


    <!-- http://purl.org/olia/arabic_khoja.owl#NPrD -->

    <owl:NamedIndividual rdf:about="http://purl.org/olia/arabic_khoja.owl#NPrD">
        <rdf:type rdf:resource="http://purl.org/olia/arabic_khoja.owl#DemonstrativePronoun"/>
        <system:hasTagStartingWith>NPrD</system:hasTagStartingWith>
    </owl:NamedIndividual>
    


    <!-- http://purl.org/olia/arabic_khoja.owl#NPrP -->

    <owl:NamedIndividual rdf:about="http://purl.org/olia/arabic_khoja.owl#NPrP">
        <rdf:type rdf:resource="http://purl.org/olia/arabic_khoja.owl#PersonalPronoun"/>
        <system:hasTagStartingWith>NPrP</system:hasTagStartingWith>
    </owl:NamedIndividual>
    


    <!-- http://purl.org/olia/arabic_khoja.owl#NPrR -->

    <owl:NamedIndividual rdf:about="http://purl.org/olia/arabic_khoja.owl#NPrR">
        <rdf:type rdf:resource="http://purl.org/olia/arabic_khoja.owl#RelativePronoun"/>
        <system:hasTagStartingWith>NPrR</system:hasTagStartingWith>
    </owl:NamedIndividual>
    


    <!-- http://purl.org/olia/arabic_khoja.owl#NPrRC -->

    <owl:NamedIndividual rdf:about="http://purl.org/olia/arabic_khoja.owl#NPrRC">
        <rdf:type rdf:resource="http://purl.org/olia/arabic_khoja.owl#CommonRelativePronoun"/>
        <system:hasTag>NPrRC</system:hasTag>
    </owl:NamedIndividual>
    


    <!-- http://purl.org/olia/arabic_khoja.owl#NPrRS -->

    <owl:NamedIndividual rdf:about="http://purl.org/olia/arabic_khoja.owl#NPrRS">
        <rdf:type rdf:resource="http://purl.org/olia/arabic_khoja.owl#SpecificRelativePronoun"/>
        <system:hasTagStartingWith>NPrRS</system:hasTagStartingWith>
    </owl:NamedIndividual>
    


    <!-- http://purl.org/olia/arabic_khoja.owl#P -->

    <owl:NamedIndividual rdf:about="http://purl.org/olia/arabic_khoja.owl#P">
        <rdf:type rdf:resource="http://purl.org/olia/arabic_khoja.owl#Particle"/>
        <system:hasTagStartingWith>P</system:hasTagStartingWith>
    </owl:NamedIndividual>
    


    <!-- http://purl.org/olia/arabic_khoja.owl#PA -->

    <owl:NamedIndividual rdf:about="http://purl.org/olia/arabic_khoja.owl#PA">
        <rdf:type rdf:resource="http://purl.org/olia/arabic_khoja.owl#Adverbial"/>
        <system:hasTag>PA</system:hasTag>
    </owl:NamedIndividual>
    


    <!-- http://purl.org/olia/arabic_khoja.owl#PC -->

    <owl:NamedIndividual rdf:about="http://purl.org/olia/arabic_khoja.owl#PC">
        <rdf:type rdf:resource="http://purl.org/olia/arabic_khoja.owl#Conjunction"/>
        <system:hasTag>PC</system:hasTag>
    </owl:NamedIndividual>
    


    <!-- http://purl.org/olia/arabic_khoja.owl#PE -->

    <owl:NamedIndividual rdf:about="http://purl.org/olia/arabic_khoja.owl#PE">
        <rdf:type rdf:resource="http://purl.org/olia/arabic_khoja.owl#Exception"/>
        <system:hasTag>PE</system:hasTag>
    </owl:NamedIndividual>
    


    <!-- http://purl.org/olia/arabic_khoja.owl#PI -->

    <owl:NamedIndividual rdf:about="http://purl.org/olia/arabic_khoja.owl#PI">
        <rdf:type rdf:resource="http://purl.org/olia/arabic_khoja.owl#Interjection"/>
        <system:hasTag>PI</system:hasTag>
    </owl:NamedIndividual>
    


    <!-- http://purl.org/olia/arabic_khoja.owl#PN -->

    <owl:NamedIndividual rdf:about="http://purl.org/olia/arabic_khoja.owl#PN">
        <rdf:type rdf:resource="http://purl.org/olia/arabic_khoja.owl#Negative"/>
        <system:hasTag>PN</system:hasTag>
    </owl:NamedIndividual>
    


    <!-- http://purl.org/olia/arabic_khoja.owl#PPr -->

    <owl:NamedIndividual rdf:about="http://purl.org/olia/arabic_khoja.owl#PPr">
        <rdf:type rdf:resource="http://purl.org/olia/arabic_khoja.owl#Preposition"/>
        <system:hasTag>PPr</system:hasTag>
    </owl:NamedIndividual>
    


    <!-- http://purl.org/olia/arabic_khoja.owl#PS -->

    <owl:NamedIndividual rdf:about="http://purl.org/olia/arabic_khoja.owl#PS">
        <rdf:type rdf:resource="http://purl.org/olia/arabic_khoja.owl#Subordinate"/>
        <system:hasTag>PS</system:hasTag>
    </owl:NamedIndividual>
    


    <!-- http://purl.org/olia/arabic_khoja.owl#PU -->

    <owl:NamedIndividual rdf:about="http://purl.org/olia/arabic_khoja.owl#PU">
        <rdf:type rdf:resource="http://purl.org/olia/arabic_khoja.owl#Punctuation"/>
        <system:hasTag>PU</system:hasTag>
    </owl:NamedIndividual>
    


    <!-- http://purl.org/olia/arabic_khoja.owl#PW -->

    <owl:NamedIndividual rdf:about="http://purl.org/olia/arabic_khoja.owl#PW">
        <rdf:type rdf:resource="http://purl.org/olia/arabic_khoja.owl#Answer"/>
        <system:hasTag>PW</system:hasTag>
    </owl:NamedIndividual>
    


    <!-- http://purl.org/olia/arabic_khoja.owl#PX -->

    <owl:NamedIndividual rdf:about="http://purl.org/olia/arabic_khoja.owl#PX">
        <rdf:type rdf:resource="http://purl.org/olia/arabic_khoja.owl#Explanation"/>
        <system:hasTag>PX</system:hasTag>
    </owl:NamedIndividual>
    


    <!-- http://purl.org/olia/arabic_khoja.owl#Pl -->

    <owl:NamedIndividual rdf:about="http://purl.org/olia/arabic_khoja.owl#Pl">
        <rdf:type rdf:resource="http://purl.org/olia/arabic_khoja.owl#PluralNumber"/>
        <hasCase rdf:resource="http://purl.org/olia/arabic_khoja.owl#Pl"/>
        <system:hasTagContaining>Pl</system:hasTagContaining>
    </owl:NamedIndividual>
    


    <!-- http://purl.org/olia/arabic_khoja.owl#R -->

    <owl:NamedIndividual rdf:about="http://purl.org/olia/arabic_khoja.owl#R">
        <rdf:type rdf:resource="http://purl.org/olia/arabic_khoja.owl#Residual"/>
        <system:hasTagStartingWith>R</system:hasTagStartingWith>
    </owl:NamedIndividual>
    


    <!-- http://purl.org/olia/arabic_khoja.owl#RA -->

    <owl:NamedIndividual rdf:about="http://purl.org/olia/arabic_khoja.owl#RA">
        <rdf:type rdf:resource="http://purl.org/olia/arabic_khoja.owl#Abbreviation"/>
        <system:hasTag>RA</system:hasTag>
    </owl:NamedIndividual>
    


    <!-- http://purl.org/olia/arabic_khoja.owl#RD -->

    <owl:NamedIndividual rdf:about="http://purl.org/olia/arabic_khoja.owl#RD">
        <rdf:type rdf:resource="http://purl.org/olia/arabic_khoja.owl#DayOfTheWeek"/>
        <system:hasTag>RD</system:hasTag>
    </owl:NamedIndividual>
    


    <!-- http://purl.org/olia/arabic_khoja.owl#RF -->

    <owl:NamedIndividual rdf:about="http://purl.org/olia/arabic_khoja.owl#RF">
        <rdf:type rdf:resource="http://purl.org/olia/arabic_khoja.owl#Foreign"/>
        <system:hasTag>RF</system:hasTag>
    </owl:NamedIndividual>
    


    <!-- http://purl.org/olia/arabic_khoja.owl#RM -->

    <owl:NamedIndividual rdf:about="http://purl.org/olia/arabic_khoja.owl#RM">
        <rdf:type rdf:resource="http://purl.org/olia/arabic_khoja.owl#Mathematical"/>
        <system:hasTag>RM</system:hasTag>
    </owl:NamedIndividual>
    


    <!-- http://purl.org/olia/arabic_khoja.owl#RN -->

    <owl:NamedIndividual rdf:about="http://purl.org/olia/arabic_khoja.owl#RN">
        <rdf:type rdf:resource="http://purl.org/olia/arabic_khoja.owl#ResidualNumber"/>
        <system:hasTag>RN</system:hasTag>
    </owl:NamedIndividual>
    


    <!-- http://purl.org/olia/arabic_khoja.owl#RO -->

    <owl:NamedIndividual rdf:about="http://purl.org/olia/arabic_khoja.owl#RO">
        <rdf:type rdf:resource="http://purl.org/olia/arabic_khoja.owl#OtherResidual"/>
        <system:hasTag>RO</system:hasTag>
    </owl:NamedIndividual>
    


    <!-- http://purl.org/olia/arabic_khoja.owl#Rmy -->

    <owl:NamedIndividual rdf:about="http://purl.org/olia/arabic_khoja.owl#Rmy">
        <rdf:type rdf:resource="http://purl.org/olia/arabic_khoja.owl#MonthOfTheYear"/>
        <system:hasTag>Rmy</system:hasTag>
    </owl:NamedIndividual>
    


    <!-- http://purl.org/olia/arabic_khoja.owl#Sg -->

    <owl:NamedIndividual rdf:about="http://purl.org/olia/arabic_khoja.owl#Sg">
        <rdf:type rdf:resource="http://purl.org/olia/arabic_khoja.owl#SingularNumber"/>
        <hasCase rdf:resource="http://purl.org/olia/arabic_khoja.owl#Sg"/>
        <system:hasTagContaining>Sg</system:hasTagContaining>
    </owl:NamedIndividual>
    


    <!-- http://purl.org/olia/arabic_khoja.owl#V -->

    <owl:NamedIndividual rdf:about="http://purl.org/olia/arabic_khoja.owl#V">
        <rdf:type rdf:resource="http://purl.org/olia/arabic_khoja.owl#Verb"/>
        <system:hasTagStartingWith>V</system:hasTagStartingWith>
    </owl:NamedIndividual>
    


    <!-- http://purl.org/olia/arabic_khoja.owl#V.F -->

    <owl:NamedIndividual rdf:about="http://purl.org/olia/arabic_khoja.owl#V.F">
        <rdf:type rdf:resource="http://purl.org/olia/arabic_khoja.owl#FeminineGender"/>
        <hasCase rdf:resource="http://purl.org/olia/arabic_khoja.owl#V.F"/>
        <system:hasTagMatching>^V.*[123]F.*</system:hasTagMatching>
    </owl:NamedIndividual>
    


    <!-- http://purl.org/olia/arabic_khoja.owl#V.I -->

    <owl:NamedIndividual rdf:about="http://purl.org/olia/arabic_khoja.owl#V.I">
        <rdf:type rdf:resource="http://purl.org/olia/arabic_khoja.owl#IndicativeMood"/>
        <hasCase rdf:resource="http://purl.org/olia/arabic_khoja.owl#V.I"/>
        <system:hasTagMatching>^V.*I$</system:hasTagMatching>
    </owl:NamedIndividual>
    


    <!-- http://purl.org/olia/arabic_khoja.owl#V.J -->

    <owl:NamedIndividual rdf:about="http://purl.org/olia/arabic_khoja.owl#V.J">
        <rdf:type rdf:resource="http://purl.org/olia/arabic_khoja.owl#JussiveMood"/>
        <hasCase rdf:resource="http://purl.org/olia/arabic_khoja.owl#V.J"/>
        <system:hasTagMatching>^V.*J$</system:hasTagMatching>
    </owl:NamedIndividual>
    


    <!-- http://purl.org/olia/arabic_khoja.owl#V.M -->

    <owl:NamedIndividual rdf:about="http://purl.org/olia/arabic_khoja.owl#V.M">
        <rdf:type rdf:resource="http://purl.org/olia/arabic_khoja.owl#MasculineGender"/>
        <hasCase rdf:resource="http://purl.org/olia/arabic_khoja.owl#V.M"/>
        <system:hasTagMatching>^V.*[123]M.*</system:hasTagMatching>
    </owl:NamedIndividual>
    


    <!-- http://purl.org/olia/arabic_khoja.owl#V.N -->

    <owl:NamedIndividual rdf:about="http://purl.org/olia/arabic_khoja.owl#V.N">
        <rdf:type rdf:resource="http://purl.org/olia/arabic_khoja.owl#NeuterGender"/>
        <hasCase rdf:resource="http://purl.org/olia/arabic_khoja.owl#V.N"/>
        <system:hasTagMatching>^V.*[123]N.*</system:hasTagMatching>
    </owl:NamedIndividual>
    


    <!-- http://purl.org/olia/arabic_khoja.owl#V.S -->

    <owl:NamedIndividual rdf:about="http://purl.org/olia/arabic_khoja.owl#V.S">
        <rdf:type rdf:resource="http://purl.org/olia/arabic_khoja.owl#SubjunctiveMood"/>
        <hasCase rdf:resource="http://purl.org/olia/arabic_khoja.owl#V.S"/>
        <system:hasTagMatching>^V.*S$</system:hasTagMatching>
    </owl:NamedIndividual>
    


    <!-- http://purl.org/olia/arabic_khoja.owl#VI -->

    <owl:NamedIndividual rdf:about="http://purl.org/olia/arabic_khoja.owl#VI">
        <rdf:type rdf:resource="http://purl.org/olia/arabic_khoja.owl#ImperfectVerb"/>
        <system:hasTagMatching>^VI[^v].*</system:hasTagMatching>
    </owl:NamedIndividual>
    


    <!-- http://purl.org/olia/arabic_khoja.owl#VIv -->

    <owl:NamedIndividual rdf:about="http://purl.org/olia/arabic_khoja.owl#VIv">
        <rdf:type rdf:resource="http://purl.org/olia/arabic_khoja.owl#ImperativeVerb"/>
        <system:hasTagStartingWith>VIv</system:hasTagStartingWith>
    </owl:NamedIndividual>
    


    <!-- http://purl.org/olia/arabic_khoja.owl#VP -->

    <owl:NamedIndividual rdf:about="http://purl.org/olia/arabic_khoja.owl#VP">
        <rdf:type rdf:resource="http://purl.org/olia/arabic_khoja.owl#PerfectVerb"/>
        <system:hasTagStartingWith>VP</system:hasTagStartingWith>
    </owl:NamedIndividual>
    


    <!-- http://purl.org/olia/arabic_khoja.owl#1 -->

    <owl:NamedIndividual rdf:about="http://purl.org/olia/arabic_khoja.owl#1">
        <rdf:type rdf:resource="http://purl.org/olia/arabic_khoja.owl#FirstPerson"/>
        <hasCase rdf:resource="http://purl.org/olia/arabic_khoja.owl#1"/>
        <system:hasTagContaining>1</system:hasTagContaining>
    </owl:NamedIndividual>
    


    <!-- http://purl.org/olia/arabic_khoja.owl#2 -->

    <owl:NamedIndividual rdf:about="http://purl.org/olia/arabic_khoja.owl#2">
        <rdf:type rdf:resource="http://purl.org/olia/arabic_khoja.owl#SecondPerson"/>
        <hasCase rdf:resource="http://purl.org/olia/arabic_khoja.owl#2"/>
        <system:hasTagContaining>2</system:hasTagContaining>
    </owl:NamedIndividual>
    


    <!-- http://purl.org/olia/arabic_khoja.owl#3 -->

    <owl:NamedIndividual rdf:about="http://purl.org/olia/arabic_khoja.owl#3">
        <rdf:type rdf:resource="http://purl.org/olia/arabic_khoja.owl#ThirdPerson"/>
        <hasCase rdf:resource="http://purl.org/olia/arabic_khoja.owl#3"/>
        <system:hasTagContaining>3</system:hasTagContaining>
    </owl:NamedIndividual>
</rdf:RDF>



<!-- Generated by the OWL API (version 4.5.25.2023-02-15T19:15:49Z) https://github.com/owlcs/owlapi -->

