<?xml version="1.0"?>
<rdf:RDF xmlns="http://purl.org/olia/bambara.owl#"
     xml:base="http://purl.org/olia/bambara.owl"
     xmlns:dc="http://purl.org/dc/elements/1.1/"
     xmlns:owl="http://www.w3.org/2002/07/owl#"
     xmlns:rdf="http://www.w3.org/1999/02/22-rdf-syntax-ns#"
     xmlns:xml="http://www.w3.org/XML/1998/namespace"
     xmlns:xsd="http://www.w3.org/2001/XMLSchema#"
     xmlns:olia="http://purl.org/olia/"
     xmlns:rdfs="http://www.w3.org/2000/01/rdf-schema#"
     xmlns:terms="http://purl.org/dc/terms/"
     xmlns:system="http://purl.org/olia/system.owl#"
     xmlns:bambara="http://purl.org/olia/bambara.owl#"
     xmlns:owl2xml="http://www.w3.org/2006/12/owl2-xml#"
     xmlns:system2="system:"
     xmlns:bambara2="http://purl.org/olia/bambara.owl#1"
     xmlns:bambara3="http://purl.org/olia/bambara.owl#2"
     xmlns:bambara4="http://purl.org/olia/bambara.owl#3">
    <owl:Ontology rdf:about="http://purl.org/olia/bambara.owl">
        <owl:imports rdf:resource="http://purl.org/olia/system.owl"/>
        <dc:creator xml:lang="en">Christian Chiarcos, Goethe Universität Frankfurt am Main, Germany, christian.chiarcos@web.de</dc:creator>
        <rdfs:comment xml:lang="en">OLiA Annotation Model for the Bambara Reference Corpus / Corpus Bambara de Reference

Bambara / Bamanankan (bam) is a West African language of the Mande group, primarily spoken in Mali.
The Bambara Reference Corpus is accessible from  http://cormand.huma-num.fr.

Note that there are several tags expressing uncertainty, or indistinguishability of two parts of speech, resp. a high likelihood of conversion, written with &quot;/&quot;. In these cases, they are treated as conjunction here, because either interpretation would be feasible.

Also note that derivation is currently not supported in OLiA. Selectional restrictions for morphosyntactic features are thus not formalized.

Unless marked otherwise, this ontology and all quotes herein follows http://cormand.huma-num.fr/gloses.html and explicit feedback by BRC developers (Valentin Vydrine, Damien Nouvel). Comments are made by ontology editor(s).

Christian Chiarcos (christian.chiarcos@web.de), 2016-04-03</rdfs:comment>
        <rdfs:seeAlso rdf:datatype="http://www.w3.org/2001/XMLSchema#anyURI">http://cormand.huma-num.fr/gloses.html</rdfs:seeAlso>
        <owl:versionInfo xml:lang="en">2016-04-03 created (CC)
2016-07-04 updated with input from Valentin Vydrine

Christian Chiarcos (CC)</owl:versionInfo>
    </owl:Ontology>
    


    <!-- 
    ///////////////////////////////////////////////////////////////////////////////////////
    //
    // Annotation properties
    //
    ///////////////////////////////////////////////////////////////////////////////////////
     -->

    


    <!-- http://purl.org/dc/elements/1.1/creator -->

    <owl:AnnotationProperty rdf:about="http://purl.org/dc/elements/1.1/creator"/>
    


    <!-- system:hasTag -->

    <owl:AnnotationProperty rdf:about="system:hasTag"/>
    


    <!-- 
    ///////////////////////////////////////////////////////////////////////////////////////
    //
    // Object Properties
    //
    ///////////////////////////////////////////////////////////////////////////////////////
     -->

    


    <!-- http://purl.org/olia/bambara.owl#derivation -->

    <owl:ObjectProperty rdf:about="http://purl.org/olia/bambara.owl#derivation">
        <rdfs:subPropertyOf rdf:resource="http://purl.org/olia/system.owl#hasFeature"/>
        <rdfs:domain rdf:resource="http://purl.org/olia/bambara.owl#Glose"/>
        <rdfs:range rdf:resource="http://purl.org/olia/bambara.owl#Derivation"/>
    </owl:ObjectProperty>
    


    <!-- http://purl.org/olia/bambara.owl#flexion -->

    <owl:ObjectProperty rdf:about="http://purl.org/olia/bambara.owl#flexion">
        <rdfs:subPropertyOf rdf:resource="http://purl.org/olia/system.owl#hasFeature"/>
        <rdfs:domain rdf:resource="http://purl.org/olia/bambara.owl#Glose"/>
        <rdfs:range rdf:resource="http://purl.org/olia/bambara.owl#Flexion"/>
    </owl:ObjectProperty>
    


    <!-- http://purl.org/olia/system.owl#hasFeature -->

    <owl:ObjectProperty rdf:about="http://purl.org/olia/system.owl#hasFeature"/>
    


    <!-- 
    ///////////////////////////////////////////////////////////////////////////////////////
    //
    // Data properties
    //
    ///////////////////////////////////////////////////////////////////////////////////////
     -->

    


    <!-- http://purl.org/olia/system.owl#hasTag -->

    <owl:DatatypeProperty rdf:about="http://purl.org/olia/system.owl#hasTag"/>
    


    <!-- http://purl.org/olia/system.owl#hasTagContaining -->

    <owl:DatatypeProperty rdf:about="http://purl.org/olia/system.owl#hasTagContaining"/>
    


    <!-- http://purl.org/olia/system.owl#hasTagEndingWith -->

    <owl:DatatypeProperty rdf:about="http://purl.org/olia/system.owl#hasTagEndingWith"/>
    


    <!-- http://purl.org/olia/system.owl#hasTagMatching -->

    <owl:DatatypeProperty rdf:about="http://purl.org/olia/system.owl#hasTagMatching"/>
    


    <!-- 
    ///////////////////////////////////////////////////////////////////////////////////////
    //
    // Classes
    //
    ///////////////////////////////////////////////////////////////////////////////////////
     -->

    


    <!-- http://purl.org/olia/bambara.owl#Adjectif -->

    <owl:Class rdf:about="http://purl.org/olia/bambara.owl#Adjectif">
        <rdfs:subClassOf rdf:resource="http://purl.org/olia/bambara.owl#POS"/>
    </owl:Class>
    


    <!-- http://purl.org/olia/bambara.owl#Adverbe -->

    <owl:Class rdf:about="http://purl.org/olia/bambara.owl#Adverbe">
        <rdfs:subClassOf rdf:resource="http://purl.org/olia/bambara.owl#POS"/>
        <rdfs:comment xml:lang="en">Note that Auxiliaire is not to be confused with auxiliary (verb). This category refers to closed-class expressions with primarily grammatical function. (V. Vydrine)</rdfs:comment>
    </owl:Class>
    


    <!-- http://purl.org/olia/bambara.owl#AutreAbreviation -->

    <owl:Class rdf:about="http://purl.org/olia/bambara.owl#AutreAbreviation">
        <rdfs:subClassOf rdf:resource="http://purl.org/olia/bambara.owl#Glose"/>
        <rdfs:comment xml:lang="fr">Autres abréviations utilisées dans les gloses</rdfs:comment>
        <owl:versionInfo xml:lang="en">The individuals assembled here have also been tentatively assigned to other parts of speech (as interpreted by the ontology editor)</owl:versionInfo>
    </owl:Class>
    


    <!-- http://purl.org/olia/bambara.owl#Auxiliaire -->

    <owl:Class rdf:about="http://purl.org/olia/bambara.owl#Auxiliaire">
        <rdfs:subClassOf rdf:resource="http://purl.org/olia/bambara.owl#POS"/>
        <owl:versionInfo xml:lang="en">Created for the glosage des auxiliaires, contains
conj 
cop 
dtm 
pers 
pm
pron 
prt</owl:versionInfo>
    </owl:Class>
    


    <!-- http://purl.org/olia/bambara.owl#Conjonction -->

    <owl:Class rdf:about="http://purl.org/olia/bambara.owl#Conjonction">
        <rdfs:subClassOf rdf:resource="http://purl.org/olia/bambara.owl#Auxiliaire"/>
    </owl:Class>
    


    <!-- http://purl.org/olia/bambara.owl#Copule -->

    <owl:Class rdf:about="http://purl.org/olia/bambara.owl#Copule">
        <rdfs:subClassOf rdf:resource="http://purl.org/olia/bambara.owl#Auxiliaire"/>
        <rdfs:comment xml:lang="en">Note that the Bambara copula is not a verbal element. Even though it syntactically resembles a verb, it is morphologically different and non-verbal in origin. (V. Vydrine)</rdfs:comment>
    </owl:Class>
    


    <!-- http://purl.org/olia/bambara.owl#Derivation -->

    <owl:Class rdf:about="http://purl.org/olia/bambara.owl#Derivation">
        <rdfs:subClassOf rdf:resource="http://purl.org/olia/system.owl#Feature"/>
        <rdfs:subClassOf>
            <owl:Restriction>
                <owl:onProperty rdf:resource="http://purl.org/olia/bambara.owl#derivation"/>
                <owl:hasSelf rdf:datatype="http://www.w3.org/2001/XMLSchema#boolean">true</owl:hasSelf>
            </owl:Restriction>
        </rdfs:subClassOf>
    </owl:Class>
    


    <!-- http://purl.org/olia/bambara.owl#Determinatif -->

    <owl:Class rdf:about="http://purl.org/olia/bambara.owl#Determinatif">
        <rdfs:subClassOf rdf:resource="http://purl.org/olia/bambara.owl#PronomDeterminatif"/>
    </owl:Class>
    


    <!-- http://purl.org/olia/bambara.owl#Flexion -->

    <owl:Class rdf:about="http://purl.org/olia/bambara.owl#Flexion">
        <rdfs:subClassOf rdf:resource="http://purl.org/olia/system.owl#Feature"/>
        <rdfs:subClassOf>
            <owl:Restriction>
                <owl:onProperty rdf:resource="http://purl.org/olia/bambara.owl#flexion"/>
                <owl:hasSelf rdf:datatype="http://www.w3.org/2001/XMLSchema#boolean">true</owl:hasSelf>
            </owl:Restriction>
        </rdfs:subClassOf>
    </owl:Class>
    


    <!-- http://purl.org/olia/bambara.owl#Glose -->

    <owl:Class rdf:about="http://purl.org/olia/bambara.owl#Glose">
        <rdfs:subClassOf rdf:resource="http://purl.org/olia/system.owl#UnitOfAnnotation"/>
        <rdfs:subClassOf>
            <owl:Restriction>
                <owl:onProperty rdf:resource="http://purl.org/olia/system.owl#hasTier"/>
                <owl:hasValue>POS</owl:hasValue>
            </owl:Restriction>
        </rdfs:subClassOf>
    </owl:Class>
    


    <!-- http://purl.org/olia/bambara.owl#Interjection -->

    <owl:Class rdf:about="http://purl.org/olia/bambara.owl#Interjection">
        <rdfs:subClassOf rdf:resource="http://purl.org/olia/bambara.owl#POS"/>
    </owl:Class>
    


    <!-- http://purl.org/olia/bambara.owl#MarquePredicative -->

    <owl:Class rdf:about="http://purl.org/olia/bambara.owl#MarquePredicative">
        <rdfs:subClassOf rdf:resource="http://purl.org/olia/bambara.owl#Auxiliaire"/>
        <rdfs:comment xml:lang="en">Predicative markers represent the syntactic center of the sentence. They resemble, but are different from both verbs and copulas and they must not be confused with particles which serve a peripheral function in sentences, only. (V. Vydrine)</rdfs:comment>
    </owl:Class>
    


    <!-- http://purl.org/olia/bambara.owl#MotEtranger -->

    <owl:Class rdf:about="http://purl.org/olia/bambara.owl#MotEtranger">
        <rdfs:subClassOf rdf:resource="http://purl.org/olia/bambara.owl#AutreAbreviation"/>
        <owl:versionInfo xml:lang="en">created as a cover term for ETRG...</owl:versionInfo>
    </owl:Class>
    


    <!-- http://purl.org/olia/bambara.owl#Nom -->

    <owl:Class rdf:about="http://purl.org/olia/bambara.owl#Nom">
        <rdfs:subClassOf rdf:resource="http://purl.org/olia/bambara.owl#POS"/>
    </owl:Class>
    


    <!-- http://purl.org/olia/bambara.owl#NomPropre -->

    <owl:Class rdf:about="http://purl.org/olia/bambara.owl#NomPropre">
        <rdfs:subClassOf rdf:resource="http://purl.org/olia/bambara.owl#AutreAbreviation"/>
        <rdfs:subClassOf rdf:resource="http://purl.org/olia/bambara.owl#Nom"/>
        <owl:versionInfo xml:lang="en">created as a cover term for NOM.F, NOM.M, etc.</owl:versionInfo>
    </owl:Class>
    


    <!-- http://purl.org/olia/bambara.owl#Numératif -->

    <owl:Class rdf:about="http://purl.org/olia/bambara.owl#Numératif">
        <rdfs:subClassOf rdf:resource="http://purl.org/olia/bambara.owl#POS"/>
        <rdfs:comment xml:lang="en">Numératif refers to cardinal numbers, ordinal numbers are adjectives, non-numeric quantifiers are determiners. (V. Vydrine)</rdfs:comment>
    </owl:Class>
    


    <!-- http://purl.org/olia/bambara.owl#Onomatopee -->

    <owl:Class rdf:about="http://purl.org/olia/bambara.owl#Onomatopee">
        <rdfs:subClassOf rdf:resource="http://purl.org/olia/bambara.owl#POS"/>
        <rdfs:comment xml:lang="en">Onomatopée refers to the onomatopoetic mimicking of natural sounds, e.g., as made by an animal, when these are not lexicalized as another constituent, e.g., a noun. In this sense, Onomatopée is related to interjection. (V. Vydrine)</rdfs:comment>
    </owl:Class>
    


    <!-- http://purl.org/olia/bambara.owl#POS -->

    <owl:Class rdf:about="http://purl.org/olia/bambara.owl#POS">
        <rdfs:subClassOf rdf:resource="http://purl.org/olia/bambara.owl#Glose"/>
        <rdfs:comment>Note that not all POS categories found in the corpus are listed here, only those found under http://cormand.huma-num.fr/marques.html.
&apos;Unknown&apos; pos tags are: c, adv/n (= n/adv?), n.prop, conj/prep (= prep/conj?), mrph, _ (= unclear?), prn/dtm, n/v, v/n.  Additional rare tags not covered by the documentation include  conv.n, n.prop/dtm/prn/n/ptcp/adj (2x), n/intj (2x), vt (2x)</rdfs:comment>
        <rdfs:comment rdf:datatype="http://www.w3.org/2001/XMLSchema#anyURI">Marques des parties de discours dans le Corpus bambara de référence</rdfs:comment>
        <rdfs:seeAlso rdf:datatype="http://www.w3.org/2001/XMLSchema#anyURI">http://cormand.huma-num.fr/marques.html</rdfs:seeAlso>
    </owl:Class>
    


    <!-- http://purl.org/olia/bambara.owl#Participe -->

    <owl:Class rdf:about="http://purl.org/olia/bambara.owl#Participe">
        <rdfs:subClassOf rdf:resource="http://purl.org/olia/bambara.owl#POS"/>
        <rdfs:comment xml:lang="en">As in Europen languages, Bambara participles are multi-functional, they have morphological characteristics of verbs, but often syntactic characteristics of Adjectives. (V. Vydrine)</rdfs:comment>
    </owl:Class>
    


    <!-- http://purl.org/olia/bambara.owl#Particule -->

    <owl:Class rdf:about="http://purl.org/olia/bambara.owl#Particule">
        <rdfs:subClassOf rdf:resource="http://purl.org/olia/bambara.owl#Auxiliaire"/>
        <rdfs:comment xml:lang="en">Bambara particles convey modal/episthemic senses. In the BRC tagset, particle only refers to elements at the syntactic periphery of sentences. In this regard, they differ fundamentally from perdicative markers (V. Vydrine)</rdfs:comment>
        <owl:versionInfo xml:lang="en">TODO: Valentin mentioned a possible relation with determiners. To be confirmed.</owl:versionInfo>
    </owl:Class>
    


    <!-- http://purl.org/olia/bambara.owl#Ponctuation -->

    <owl:Class rdf:about="http://purl.org/olia/bambara.owl#Ponctuation">
        <rdfs:subClassOf rdf:resource="http://purl.org/olia/bambara.owl#AutreAbreviation"/>
        <rdfs:comment xml:lang="en">added for punctuation signs (CC), not part of the original glosses, but treated differently</rdfs:comment>
    </owl:Class>
    


    <!-- http://purl.org/olia/bambara.owl#Postposition -->

    <owl:Class rdf:about="http://purl.org/olia/bambara.owl#Postposition">
        <rdfs:subClassOf rdf:resource="http://purl.org/olia/bambara.owl#POS"/>
    </owl:Class>
    


    <!-- http://purl.org/olia/bambara.owl#PronomDeterminatif -->

    <owl:Class rdf:about="http://purl.org/olia/bambara.owl#PronomDeterminatif">
        <rdfs:subClassOf rdf:resource="http://purl.org/olia/bambara.owl#Auxiliaire"/>
        <owl:versionInfo xml:lang="en">created for tags (glosses) classified as &quot;dtm, pron&quot;, as no holistic term is available, we also followed EAGLES to include PronounPersonnel</owl:versionInfo>
    </owl:Class>
    


    <!-- http://purl.org/olia/bambara.owl#PronomNonPersonnel -->

    <owl:Class rdf:about="http://purl.org/olia/bambara.owl#PronomNonPersonnel">
        <rdfs:subClassOf rdf:resource="http://purl.org/olia/bambara.owl#PronomDeterminatif"/>
    </owl:Class>
    


    <!-- http://purl.org/olia/bambara.owl#PronomPersonnel -->

    <owl:Class rdf:about="http://purl.org/olia/bambara.owl#PronomPersonnel">
        <rdfs:subClassOf rdf:resource="http://purl.org/olia/bambara.owl#PronomDeterminatif"/>
    </owl:Class>
    


    <!-- http://purl.org/olia/bambara.owl#Préposition -->

    <owl:Class rdf:about="http://purl.org/olia/bambara.owl#Préposition">
        <rdfs:subClassOf rdf:resource="http://purl.org/olia/bambara.owl#POS"/>
    </owl:Class>
    


    <!-- http://purl.org/olia/bambara.owl#Verbe -->

    <owl:Class rdf:about="http://purl.org/olia/bambara.owl#Verbe">
        <rdfs:subClassOf rdf:resource="http://purl.org/olia/bambara.owl#POS"/>
    </owl:Class>
    


    <!-- http://purl.org/olia/bambara.owl#VerbeDynamique -->

    <owl:Class rdf:about="http://purl.org/olia/bambara.owl#VerbeDynamique">
        <rdfs:subClassOf rdf:resource="http://purl.org/olia/bambara.owl#Verbe"/>
    </owl:Class>
    


    <!-- http://purl.org/olia/bambara.owl#VerbeQualitatif -->

    <owl:Class rdf:about="http://purl.org/olia/bambara.owl#VerbeQualitatif">
        <rdfs:subClassOf rdf:resource="http://purl.org/olia/bambara.owl#Verbe"/>
    </owl:Class>
    


    <!-- http://purl.org/olia/bambara.owl#derive.adj -->

    <owl:Class rdf:about="http://purl.org/olia/bambara.owl#derive.adj">
        <rdfs:subClassOf rdf:resource="http://purl.org/olia/bambara.owl#Derivation"/>
    </owl:Class>
    


    <!-- http://purl.org/olia/bambara.owl#derive.n -->

    <owl:Class rdf:about="http://purl.org/olia/bambara.owl#derive.n">
        <rdfs:subClassOf rdf:resource="http://purl.org/olia/bambara.owl#Derivation"/>
    </owl:Class>
    


    <!-- http://purl.org/olia/bambara.owl#derive.ptcp -->

    <owl:Class rdf:about="http://purl.org/olia/bambara.owl#derive.ptcp">
        <rdfs:subClassOf rdf:resource="http://purl.org/olia/bambara.owl#Derivation"/>
    </owl:Class>
    


    <!-- http://purl.org/olia/bambara.owl#derive.v -->

    <owl:Class rdf:about="http://purl.org/olia/bambara.owl#derive.v">
        <rdfs:subClassOf rdf:resource="http://purl.org/olia/bambara.owl#Derivation"/>
    </owl:Class>
    


    <!-- http://purl.org/olia/bambara.owl#initial.adj -->

    <owl:Class rdf:about="http://purl.org/olia/bambara.owl#initial.adj">
        <rdfs:subClassOf rdf:resource="http://purl.org/olia/bambara.owl#Derivation"/>
    </owl:Class>
    


    <!-- http://purl.org/olia/bambara.owl#initial.n -->

    <owl:Class rdf:about="http://purl.org/olia/bambara.owl#initial.n">
        <rdfs:subClassOf rdf:resource="http://purl.org/olia/bambara.owl#Derivation"/>
    </owl:Class>
    


    <!-- http://purl.org/olia/bambara.owl#initial.num -->

    <owl:Class rdf:about="http://purl.org/olia/bambara.owl#initial.num">
        <rdfs:subClassOf rdf:resource="http://purl.org/olia/bambara.owl#Derivation"/>
    </owl:Class>
    


    <!-- http://purl.org/olia/bambara.owl#initial.pp -->

    <owl:Class rdf:about="http://purl.org/olia/bambara.owl#initial.pp">
        <rdfs:subClassOf rdf:resource="http://purl.org/olia/bambara.owl#Derivation"/>
    </owl:Class>
    


    <!-- http://purl.org/olia/bambara.owl#initial.ptcp -->

    <owl:Class rdf:about="http://purl.org/olia/bambara.owl#initial.ptcp">
        <rdfs:subClassOf rdf:resource="http://purl.org/olia/bambara.owl#Derivation"/>
    </owl:Class>
    


    <!-- http://purl.org/olia/bambara.owl#initial.v -->

    <owl:Class rdf:about="http://purl.org/olia/bambara.owl#initial.v">
        <rdfs:subClassOf rdf:resource="http://purl.org/olia/bambara.owl#Derivation"/>
    </owl:Class>
    


    <!-- http://purl.org/olia/bambara.owl#initial.vp -->

    <owl:Class rdf:about="http://purl.org/olia/bambara.owl#initial.vp">
        <rdfs:subClassOf rdf:resource="http://purl.org/olia/bambara.owl#Derivation"/>
    </owl:Class>
    


    <!-- http://purl.org/olia/bambara.owl#initial.vq -->

    <owl:Class rdf:about="http://purl.org/olia/bambara.owl#initial.vq">
        <rdfs:subClassOf rdf:resource="http://purl.org/olia/bambara.owl#Derivation"/>
    </owl:Class>
    


    <!-- http://purl.org/olia/system.owl#Feature -->

    <owl:Class rdf:about="http://purl.org/olia/system.owl#Feature">
        <owl:versionInfo xml:lang="en">both Feature subclasses have reflexitivy axioms. This is to facilitate relational querying, cf. Chiarcos (2016, Linked Data in Linguistics)</owl:versionInfo>
    </owl:Class>
    


    <!-- http://purl.org/olia/system.owl#UnitOfAnnotation -->

    <owl:Class rdf:about="http://purl.org/olia/system.owl#UnitOfAnnotation"/>
    


    <!-- http://www.w3.org/2002/07/owl#Thing -->

    <owl:Class rdf:about="http://www.w3.org/2002/07/owl#Thing"/>
    


    <!-- 
    ///////////////////////////////////////////////////////////////////////////////////////
    //
    // Individuals
    //
    ///////////////////////////////////////////////////////////////////////////////////////
     -->

    


    <!-- http://purl.org/olia/dtm -->

    <owl:Thing rdf:about="http://purl.org/olia/dtm">
        <rdf:type rdf:resource="http://www.w3.org/2002/07/owl#NamedIndividual"/>
        <rdf:type rdf:resource="http://purl.org/olia/bambara.owl#Determinatif"/>
        <system:hasTag>dtm</system:hasTag>
        <rdfs:comment>déterminatif</rdfs:comment>
    </owl:Thing>
    


    <!-- http://purl.org/olia/pp -->

    <owl:Thing rdf:about="http://purl.org/olia/pp">
        <rdf:type rdf:resource="http://www.w3.org/2002/07/owl#NamedIndividual"/>
        <rdf:type rdf:resource="http://purl.org/olia/bambara.owl#Postposition"/>
        <system:hasTag>pp</system:hasTag>
        <rdfs:comment>postposition</rdfs:comment>
    </owl:Thing>
    


    <!-- http://purl.org/olia/bambara.owl#ABSTR -->

    <owl:Thing rdf:about="http://purl.org/olia/bambara.owl#ABSTR">
        <rdf:type rdf:resource="http://www.w3.org/2002/07/owl#NamedIndividual"/>
        <rdf:type rdf:resource="http://purl.org/olia/bambara.owl#Derivation"/>
        <rdf:type rdf:resource="http://purl.org/olia/bambara.owl#derive.n"/>
        <rdf:type rdf:resource="http://purl.org/olia/bambara.owl#initial.adj"/>
        <rdf:type rdf:resource="http://purl.org/olia/bambara.owl#initial.n"/>
        <system:hasTagContaining>ABSTR</system:hasTagContaining>
        <rdfs:comment xml:lang="fr">-ya;
            n, adj, (v);
            n, (v);
            nom de statut ou d’état (dérivé des noms de personnes ou de certains animaux), du nom de qualité (dérivé des adjectifs) ; rarement, des verbes à valeurs inchoatives</rdfs:comment>
    </owl:Thing>
    


    <!-- http://purl.org/olia/bambara.owl#ADJ -->

    <owl:Thing rdf:about="http://purl.org/olia/bambara.owl#ADJ">
        <rdf:type rdf:resource="http://www.w3.org/2002/07/owl#NamedIndividual"/>
        <rdf:type rdf:resource="http://purl.org/olia/bambara.owl#Derivation"/>
        <rdf:type rdf:resource="http://purl.org/olia/bambara.owl#derive.adj"/>
        <rdf:type rdf:resource="http://purl.org/olia/bambara.owl#initial.vq"/>
        <system:hasTagContaining>ADJ</system:hasTagContaining>
        <rdfs:comment xml:lang="fr">-man;
            vq;
            adj;
            adjectiviseur des verbes qualitatifs</rdfs:comment>
    </owl:Thing>
    


    <!-- http://purl.org/olia/bambara.owl#AG.EX -->

    <owl:Thing rdf:about="http://purl.org/olia/bambara.owl#AG.EX">
        <rdf:type rdf:resource="http://www.w3.org/2002/07/owl#NamedIndividual"/>
        <rdf:type rdf:resource="http://purl.org/olia/bambara.owl#Derivation"/>
        <rdf:type rdf:resource="http://purl.org/olia/bambara.owl#derive.n"/>
        <rdf:type rdf:resource="http://purl.org/olia/bambara.owl#initial.adj"/>
        <rdf:type rdf:resource="http://purl.org/olia/bambara.owl#initial.n"/>
        <rdf:type rdf:resource="http://purl.org/olia/bambara.owl#initial.v"/>
        <system:hasTagContaining>AG.EX</system:hasTagContaining>
        <rdfs:comment xml:lang="fr">-nci; 
            n, adj, v;
            n;
            nom d’agent excessif</rdfs:comment>
    </owl:Thing>
    


    <!-- http://purl.org/olia/bambara.owl#AG.OCC -->

    <owl:Thing rdf:about="http://purl.org/olia/bambara.owl#AG.OCC">
        <rdf:type rdf:resource="http://www.w3.org/2002/07/owl#NamedIndividual"/>
        <rdf:type rdf:resource="http://purl.org/olia/bambara.owl#Derivation"/>
        <rdf:type rdf:resource="http://purl.org/olia/bambara.owl#derive.n"/>
        <rdf:type rdf:resource="http://purl.org/olia/bambara.owl#initial.v"/>
        <system:hasTagContaining>AG.OCC</system:hasTagContaining>
        <rdfs:comment xml:lang="fr">-baa / -baga;
            v;
            n, (adj);
            nom d’agent occasionnel</rdfs:comment>
    </owl:Thing>
    


    <!-- http://purl.org/olia/bambara.owl#AG.PRM -->

    <owl:Thing rdf:about="http://purl.org/olia/bambara.owl#AG.PRM">
        <rdf:type rdf:resource="http://www.w3.org/2002/07/owl#NamedIndividual"/>
        <rdf:type rdf:resource="http://purl.org/olia/bambara.owl#Derivation"/>
        <rdf:type rdf:resource="http://purl.org/olia/bambara.owl#derive.n"/>
        <rdf:type rdf:resource="http://purl.org/olia/bambara.owl#initial.v"/>
        <system:hasTagContaining>AG.PRM</system:hasTagContaining>
        <rdfs:comment xml:lang="fr">-la / -na; 
            v;
            n;
            nom d’agent</rdfs:comment>
    </owl:Thing>
    


    <!-- http://purl.org/olia/bambara.owl#ART -->

    <owl:Thing rdf:about="http://purl.org/olia/bambara.owl#ART">
        <rdf:type rdf:resource="http://www.w3.org/2002/07/owl#NamedIndividual"/>
        <rdf:type rdf:resource="http://purl.org/olia/bambara.owl#Flexion"/>
        <system:hasTagEndingWith>ART</system:hasTagEndingWith>
        <rdfs:comment xml:lang="fr">-;
            n, adj;
            article spécifique;
            ton bas flottant suivant le mot</rdfs:comment>
    </owl:Thing>
    


    <!-- http://purl.org/olia/bambara.owl#AUGM -->

    <owl:Thing rdf:about="http://purl.org/olia/bambara.owl#AUGM">
        <rdf:type rdf:resource="http://www.w3.org/2002/07/owl#NamedIndividual"/>
        <rdf:type rdf:resource="http://purl.org/olia/bambara.owl#Derivation"/>
        <rdf:type rdf:resource="http://purl.org/olia/bambara.owl#initial.adj"/>
        <rdf:type rdf:resource="http://purl.org/olia/bambara.owl#initial.n"/>
        <rdf:type rdf:resource="http://purl.org/olia/bambara.owl#initial.ptcp"/>
        <system:hasTagContaining>AUGM</system:hasTagContaining>
        <rdfs:comment xml:lang="fr">-ba; 
            n, adj, ptcp;
            ne change pas;
            augmentatif</rdfs:comment>
    </owl:Thing>
    


    <!-- http://purl.org/olia/bambara.owl#BE -->

    <owl:Thing rdf:about="http://purl.org/olia/bambara.owl#BE">
        <rdf:type rdf:resource="http://www.w3.org/2002/07/owl#NamedIndividual"/>
        <rdf:type rdf:resource="http://purl.org/olia/bambara.owl#Copule"/>
        <system:hasTag>BE</system:hasTag>
        <rdfs:comment xml:lang="fr">bɛ́;
            copule d’un énoncé non-verbal locatif affirmatif</rdfs:comment>
    </owl:Thing>
    


    <!-- http://purl.org/olia/bambara.owl#CAUS -->

    <owl:Thing rdf:about="http://purl.org/olia/bambara.owl#CAUS">
        <rdf:type rdf:resource="http://www.w3.org/2002/07/owl#NamedIndividual"/>
        <rdf:type rdf:resource="http://purl.org/olia/bambara.owl#Derivation"/>
        <rdf:type rdf:resource="http://purl.org/olia/bambara.owl#derive.v"/>
        <rdf:type rdf:resource="http://purl.org/olia/bambara.owl#initial.v"/>
        <system:hasTagContaining>CAUS</system:hasTagContaining>
        <rdfs:comment xml:lang="fr">lá-/ná-;
            v;
            v;
            préfixe causatif</rdfs:comment>
    </owl:Thing>
    


    <!-- http://purl.org/olia/bambara.owl#CERT -->

    <owl:Thing rdf:about="http://purl.org/olia/bambara.owl#CERT">
        <rdf:type rdf:resource="http://www.w3.org/2002/07/owl#NamedIndividual"/>
        <rdf:type rdf:resource="http://purl.org/olia/bambara.owl#MarquePredicative"/>
        <system:hasTag>CERT</system:hasTag>
        <rdfs:comment xml:lang="fr">nà ~ ná;
            marque du futur certain</rdfs:comment>
    </owl:Thing>
    


    <!-- http://purl.org/olia/bambara.owl#COM -->

    <owl:Thing rdf:about="http://purl.org/olia/bambara.owl#COM">
        <rdf:type rdf:resource="http://www.w3.org/2002/07/owl#NamedIndividual"/>
        <rdf:type rdf:resource="http://purl.org/olia/bambara.owl#Derivation"/>
        <rdf:type rdf:resource="http://purl.org/olia/bambara.owl#derive.adj"/>
        <rdf:type rdf:resource="http://purl.org/olia/bambara.owl#initial.n"/>
        <system:hasTagContaining>COM</system:hasTagContaining>
        <rdfs:comment xml:lang="fr">-ma;
            n;
            adj, (n);
            adjectif dénominal à valeur comitative/ornative</rdfs:comment>
    </owl:Thing>
    


    <!-- http://purl.org/olia/bambara.owl#COND.AFF -->

    <owl:Thing rdf:about="http://purl.org/olia/bambara.owl#COND.AFF">
        <rdf:type rdf:resource="http://www.w3.org/2002/07/owl#NamedIndividual"/>
        <rdf:type rdf:resource="http://purl.org/olia/bambara.owl#MarquePredicative"/>
        <system:hasTag>COND.AFF</system:hasTag>
        <rdfs:comment xml:lang="fr">mána ~ máa;
            marque du conditionnel affirmatif;
            máa est une forme des dialectes du nord</rdfs:comment>
    </owl:Thing>
    


    <!-- http://purl.org/olia/bambara.owl#COND.NEG -->

    <owl:Thing rdf:about="http://purl.org/olia/bambara.owl#COND.NEG">
        <rdf:type rdf:resource="http://www.w3.org/2002/07/owl#NamedIndividual"/>
        <rdf:type rdf:resource="http://purl.org/olia/bambara.owl#MarquePredicative"/>
        <system:hasTag>COND.NEG</system:hasTag>
        <rdfs:comment xml:lang="fr">bìlen ~ bìle ~ bèlen;
            marque négative du conditionnel;
            archaïque, rare</rdfs:comment>
    </owl:Thing>
    


    <!-- http://purl.org/olia/bambara.owl#CONV.PROG -->

    <owl:Thing rdf:about="http://purl.org/olia/bambara.owl#CONV.PROG">
        <rdf:type rdf:resource="http://www.w3.org/2002/07/owl#NamedIndividual"/>
        <rdf:type rdf:resource="http://purl.org/olia/bambara.owl#Derivation"/>
        <rdf:type rdf:resource="http://purl.org/olia/bambara.owl#derive.ptcp"/>
        <rdf:type rdf:resource="http://purl.org/olia/bambara.owl#initial.v"/>
        <system:hasTagContaining>CONV.PROG</system:hasTagContaining>
        <rdfs:comment xml:lang="fr">-tɔ;
            v;
            ptcp;
            converbe progressif et prospectif (la valeur progressive avec les verbes atéliques, la valeur prospective avec les verbes téliques)</rdfs:comment>
    </owl:Thing>
    


    <!-- http://purl.org/olia/bambara.owl#COP.NEG -->

    <owl:Thing rdf:about="http://purl.org/olia/bambara.owl#COP.NEG">
        <rdf:type rdf:resource="http://www.w3.org/2002/07/owl#NamedIndividual"/>
        <rdf:type rdf:resource="http://purl.org/olia/bambara.owl#Copule"/>
        <system:hasTag>COP.NEG</system:hasTag>
        <rdfs:comment xml:lang="fr">tɛ́;
            copule d’un énoncé non-verbal locatif ou présentatif affirmatif</rdfs:comment>
    </owl:Thing>
    


    <!-- http://purl.org/olia/bambara.owl#DEF -->

    <owl:Thing rdf:about="http://purl.org/olia/bambara.owl#DEF">
        <rdf:type rdf:resource="http://www.w3.org/2002/07/owl#NamedIndividual"/>
        <rdf:type rdf:resource="http://purl.org/olia/bambara.owl#Determinatif"/>
        <system:hasTag>DEF</system:hasTag>
        <rdfs:comment xml:lang="fr">ìn;
            le « nouvel article défini »</rdfs:comment>
    </owl:Thing>
    


    <!-- http://purl.org/olia/bambara.owl#DEM -->

    <owl:Thing rdf:about="http://purl.org/olia/bambara.owl#DEM">
        <rdf:type rdf:resource="http://www.w3.org/2002/07/owl#NamedIndividual"/>
        <rdf:type rdf:resource="http://purl.org/olia/bambara.owl#PronomDeterminatif"/>
        <rdf:type>
            <owl:Class>
                <owl:unionOf rdf:parseType="Collection">
                    <rdf:Description rdf:about="http://purl.org/olia/bambara.owl#Determinatif"/>
                    <rdf:Description rdf:about="http://purl.org/olia/bambara.owl#PronomNonPersonnel"/>
                </owl:unionOf>
            </owl:Class>
        </rdf:type>
        <system:hasTag>DEM</system:hasTag>
        <rdfs:comment xml:lang="fr">nìn;
            dtm, pron;
            remplace le groupe nominal, le suit ou le précède;
            pronom démonstratif</rdfs:comment>
    </owl:Thing>
    


    <!-- http://purl.org/olia/bambara.owl#DEQU -->

    <owl:Thing rdf:about="http://purl.org/olia/bambara.owl#DEQU">
        <rdf:type rdf:resource="http://www.w3.org/2002/07/owl#NamedIndividual"/>
        <rdf:type rdf:resource="http://purl.org/olia/bambara.owl#Derivation"/>
        <rdf:type rdf:resource="http://purl.org/olia/bambara.owl#derive.n"/>
        <rdf:type rdf:resource="http://purl.org/olia/bambara.owl#derive.v"/>
        <rdf:type rdf:resource="http://purl.org/olia/bambara.owl#initial.vp"/>
        <system:hasTagContaining>DEQU</system:hasTagContaining>
        <rdfs:comment xml:lang="fr">-ya;
            vq;
            n, v;
            verbes dynamiques et noms de qualités dérivés des verbes qualitatifs</rdfs:comment>
    </owl:Thing>
    


    <!-- http://purl.org/olia/bambara.owl#DES -->

    <owl:Thing rdf:about="http://purl.org/olia/bambara.owl#DES">
        <rdf:type rdf:resource="http://www.w3.org/2002/07/owl#NamedIndividual"/>
        <rdf:type rdf:resource="http://purl.org/olia/bambara.owl#MarquePredicative"/>
        <system:hasTag>DES</system:hasTag>
        <rdfs:comment xml:lang="fr">mà ~ màa;
            suit le groupe nominal du sujet représenté par le mot Ala ; le verbe a le suffixe –ra / -la / -na PFV.INTR;
            marque prédicative dans l’énoncé exprimant une bénédiction</rdfs:comment>
    </owl:Thing>
    


    <!-- http://purl.org/olia/bambara.owl#DIM -->

    <owl:Thing rdf:about="http://purl.org/olia/bambara.owl#DIM">
        <rdf:type rdf:resource="http://www.w3.org/2002/07/owl#NamedIndividual"/>
        <rdf:type rdf:resource="http://purl.org/olia/bambara.owl#Derivation"/>
        <rdf:type rdf:resource="http://purl.org/olia/bambara.owl#initial.adj"/>
        <rdf:type rdf:resource="http://purl.org/olia/bambara.owl#initial.n"/>
        <rdf:type rdf:resource="http://purl.org/olia/bambara.owl#initial.ptcp"/>
        <system:hasTagContaining>DIM</system:hasTagContaining>
        <rdfs:comment xml:lang="fr">-nin;
            n, adj, ptcp;
            ne change pas;
            diminutif</rdfs:comment>
    </owl:Thing>
    


    <!-- http://purl.org/olia/bambara.owl#DIR -->

    <owl:Thing rdf:about="http://purl.org/olia/bambara.owl#DIR">
        <rdf:type rdf:resource="http://www.w3.org/2002/07/owl#NamedIndividual"/>
        <rdf:type rdf:resource="http://purl.org/olia/bambara.owl#Derivation"/>
        <rdf:type rdf:resource="http://purl.org/olia/bambara.owl#derive.v"/>
        <rdf:type rdf:resource="http://purl.org/olia/bambara.owl#initial.v"/>
        <system:hasTagContaining>DIR</system:hasTagContaining>
        <rdfs:comment xml:lang="fr">-ma;
            v;
            v;
            suffixe non-productif qui se combine surtout avec les verbes d’action orientée, souvent sans modifier le sens originel</rdfs:comment>
    </owl:Thing>
    


    <!-- http://purl.org/olia/bambara.owl#DISTR -->

    <owl:Thing rdf:about="http://purl.org/olia/bambara.owl#DISTR">
        <rdf:type rdf:resource="http://www.w3.org/2002/07/owl#NamedIndividual"/>
        <rdf:type rdf:resource="http://purl.org/olia/bambara.owl#Conjonction"/>
        <system:hasTag>DISTR</system:hasTag>
        <rdfs:comment xml:lang="fr">ó`;
            marque du distributif</rdfs:comment>
    </owl:Thing>
    


    <!-- http://purl.org/olia/bambara.owl#EN -->

    <owl:Thing rdf:about="http://purl.org/olia/bambara.owl#EN">
        <rdf:type rdf:resource="http://www.w3.org/2002/07/owl#NamedIndividual"/>
        <rdf:type rdf:resource="http://purl.org/olia/bambara.owl#Derivation"/>
        <rdf:type rdf:resource="http://purl.org/olia/bambara.owl#derive.v"/>
        <rdf:type rdf:resource="http://purl.org/olia/bambara.owl#initial.v"/>
        <system:hasTagContaining>EN</system:hasTagContaining>
        <rdfs:comment xml:lang="fr">sɔ̀-;
            v;
            v;
            suffixe non-productif, se combine avec quelques verbes de mouvement; se dérive du mot sɔ̀n ‘coeur’ (cf. la postposition courante dans le marka-dafin, sɔ́n)</rdfs:comment>
    </owl:Thing>
    


    <!-- http://purl.org/olia/bambara.owl#EQU -->

    <owl:Thing rdf:about="http://purl.org/olia/bambara.owl#EQU">
        <rdf:type rdf:resource="http://www.w3.org/2002/07/owl#NamedIndividual"/>
        <rdf:type rdf:resource="http://purl.org/olia/bambara.owl#Copule"/>
        <system:hasTag>EQU</system:hasTag>
        <rdfs:comment xml:lang="fr">yé;
            copule d’un énoncé équatif non-verbal affirmatif</rdfs:comment>
    </owl:Thing>
    


    <!-- http://purl.org/olia/bambara.owl#ETRG -->

    <owl:Thing rdf:about="http://purl.org/olia/bambara.owl#ETRG">
        <rdf:type rdf:resource="http://www.w3.org/2002/07/owl#NamedIndividual"/>
        <rdf:type rdf:resource="http://purl.org/olia/bambara.owl#MotEtranger"/>
        <system:hasTag>ETRG</system:hasTag>
        <rdfs:comment>un mot étranger non-adapté</rdfs:comment>
    </owl:Thing>
    


    <!-- http://purl.org/olia/bambara.owl#ETRG.ARB -->

    <owl:Thing rdf:about="http://purl.org/olia/bambara.owl#ETRG.ARB">
        <rdf:type rdf:resource="http://www.w3.org/2002/07/owl#NamedIndividual"/>
        <rdf:type rdf:resource="http://purl.org/olia/bambara.owl#MotEtranger"/>
        <system:hasTag>ETRG.ARB</system:hasTag>
        <rdfs:comment>un mot arabe</rdfs:comment>
    </owl:Thing>
    


    <!-- http://purl.org/olia/bambara.owl#ETRG.FRA -->

    <owl:Thing rdf:about="http://purl.org/olia/bambara.owl#ETRG.FRA">
        <rdf:type rdf:resource="http://www.w3.org/2002/07/owl#NamedIndividual"/>
        <rdf:type rdf:resource="http://purl.org/olia/bambara.owl#MotEtranger"/>
        <system:hasTag>ETRG.FRA</system:hasTag>
        <rdfs:comment>un mot français</rdfs:comment>
    </owl:Thing>
    


    <!-- http://purl.org/olia/bambara.owl#ETRG.FUL -->

    <owl:Thing rdf:about="http://purl.org/olia/bambara.owl#ETRG.FUL">
        <rdf:type rdf:resource="http://www.w3.org/2002/07/owl#NamedIndividual"/>
        <rdf:type rdf:resource="http://purl.org/olia/bambara.owl#MotEtranger"/>
        <system:hasTag>ETRG.FUL</system:hasTag>
        <rdfs:comment>un mot peul</rdfs:comment>
    </owl:Thing>
    


    <!-- http://purl.org/olia/bambara.owl#FOC -->

    <owl:Thing rdf:about="http://purl.org/olia/bambara.owl#FOC">
        <rdf:type rdf:resource="http://www.w3.org/2002/07/owl#NamedIndividual"/>
        <rdf:type rdf:resource="http://purl.org/olia/bambara.owl#Particule"/>
        <system:hasTag>FOC</system:hasTag>
        <rdfs:comment xml:lang="fr">dè;
            marque du focus contrastif</rdfs:comment>
    </owl:Thing>
    


    <!-- http://purl.org/olia/bambara.owl#FUT.AFF -->

    <owl:Thing rdf:about="http://purl.org/olia/bambara.owl#FUT.AFF">
        <rdf:type rdf:resource="http://www.w3.org/2002/07/owl#NamedIndividual"/>
        <rdf:type rdf:resource="http://purl.org/olia/bambara.owl#MarquePredicative"/>
        <system:hasTag>FUT.AFF</system:hasTag>
        <rdfs:comment xml:lang="fr">bɛ́nà ~ bínà ~ bénà;
            marque affirmative du futur</rdfs:comment>
    </owl:Thing>
    


    <!-- http://purl.org/olia/bambara.owl#FUT.NEG -->

    <owl:Thing rdf:about="http://purl.org/olia/bambara.owl#FUT.NEG">
        <rdf:type rdf:resource="http://www.w3.org/2002/07/owl#NamedIndividual"/>
        <rdf:type rdf:resource="http://purl.org/olia/bambara.owl#MarquePredicative"/>
        <system:hasTag>FUT.NEG</system:hasTag>
        <rdfs:comment xml:lang="fr">tɛ́nà ~ ténà ~ tínà,
            marque du futur négatif</rdfs:comment>
    </owl:Thing>
    


    <!-- http://purl.org/olia/bambara.owl#GENT -->

    <owl:Thing rdf:about="http://purl.org/olia/bambara.owl#GENT">
        <rdf:type rdf:resource="http://www.w3.org/2002/07/owl#NamedIndividual"/>
        <rdf:type rdf:resource="http://purl.org/olia/bambara.owl#Derivation"/>
        <rdf:type rdf:resource="http://purl.org/olia/bambara.owl#derive.n"/>
        <rdf:type rdf:resource="http://purl.org/olia/bambara.owl#initial.n"/>
        <system:hasTagContaining>GENT</system:hasTagContaining>
        <rdfs:comment xml:lang="fr">-ka;
            n;
            n;
            suffixe du nom d’habitant ou originaire d’une localité</rdfs:comment>
    </owl:Thing>
    


    <!-- http://purl.org/olia/bambara.owl#IMP -->

    <owl:Thing rdf:about="http://purl.org/olia/bambara.owl#IMP">
        <rdf:type rdf:resource="http://www.w3.org/2002/07/owl#NamedIndividual"/>
        <rdf:type rdf:resource="http://purl.org/olia/bambara.owl#MarquePredicative"/>
        <system:hasTag>IMP</system:hasTag>
        <rdfs:comment xml:lang="fr">yé;
            suit le groupe nominal du sujet au 2ème pl;
            marque de l’impératif 2ème pl</rdfs:comment>
    </owl:Thing>
    


    <!-- http://purl.org/olia/bambara.owl#IN -->

    <owl:Thing rdf:about="http://purl.org/olia/bambara.owl#IN">
        <rdf:type rdf:resource="http://www.w3.org/2002/07/owl#NamedIndividual"/>
        <rdf:type rdf:resource="http://purl.org/olia/bambara.owl#Derivation"/>
        <rdf:type rdf:resource="http://purl.org/olia/bambara.owl#derive.adj"/>
        <system:hasTagContaining>IN</system:hasTagContaining>
        <rdfs:comment xml:lang="fr">-rɔ- / -nɔ-;
            (dans);
            adj;
            connecteur des composantes des adjectifs composés; -rɔ- suivant une voyelle orale, -nɔ- suivant une voyelle orale</rdfs:comment>
    </owl:Thing>
    


    <!-- http://purl.org/olia/bambara.owl#IN2 -->

    <owl:Thing rdf:about="http://purl.org/olia/bambara.owl#IN2">
        <rdf:type rdf:resource="http://www.w3.org/2002/07/owl#NamedIndividual"/>
        <rdf:type rdf:resource="http://purl.org/olia/bambara.owl#Derivation"/>
        <rdf:type rdf:resource="http://purl.org/olia/bambara.owl#derive.v"/>
        <rdf:type rdf:resource="http://purl.org/olia/bambara.owl#initial.v"/>
        <system:hasTagContaining>IN</system:hasTagContaining>
        <rdfs:comment xml:lang="fr">rá-/rɔ́-;
            v;
            v;
            préfixe à valeur obscure (étymologiquement, valeur inessive)</rdfs:comment>
        <owl:versionInfo>TODO: disambiguate with the other gloss value IN (for homographic morphemes), these two will get conflated</owl:versionInfo>
    </owl:Thing>
    


    <!-- http://purl.org/olia/bambara.owl#INF -->

    <owl:Thing rdf:about="http://purl.org/olia/bambara.owl#INF">
        <rdf:type rdf:resource="http://www.w3.org/2002/07/owl#NamedIndividual"/>
        <rdf:type rdf:resource="http://purl.org/olia/bambara.owl#MarquePredicative"/>
        <system:hasTag>INF</system:hasTag>
        <rdfs:comment xml:lang="fr">kà; 
            précède le groupe nominal du complément d’objet direct, ou, en son absence, le verbe;
            marque d’infinitif</rdfs:comment>
    </owl:Thing>
    


    <!-- http://purl.org/olia/bambara.owl#INFR.AFF -->

    <owl:Thing rdf:about="http://purl.org/olia/bambara.owl#INFR.AFF">
        <rdf:type rdf:resource="http://www.w3.org/2002/07/owl#NamedIndividual"/>
        <rdf:type rdf:resource="http://purl.org/olia/bambara.owl#MarquePredicative"/>
        <system:hasTag>INFR.AFF</system:hasTag>
        <rdfs:comment xml:lang="fr">bɛ́ka ~ bɛ́ga ~ bága ~ búga;
            marque affirmative du parfait inférentif;
            peu utilisé en bambara standard</rdfs:comment>
    </owl:Thing>
    


    <!-- http://purl.org/olia/bambara.owl#INFR.NEG -->

    <owl:Thing rdf:about="http://purl.org/olia/bambara.owl#INFR.NEG">
        <rdf:type rdf:resource="http://www.w3.org/2002/07/owl#NamedIndividual"/>
        <rdf:type rdf:resource="http://purl.org/olia/bambara.owl#MarquePredicative"/>
        <system:hasTag>INFR.NEG</system:hasTag>
        <rdfs:comment xml:lang="fr">tɛ́ka ~ tɛ́ga;
            marque négative du parfait inférentif;
            peu utilisé en bambara standard</rdfs:comment>
    </owl:Thing>
    


    <!-- http://purl.org/olia/bambara.owl#INSTR -->

    <owl:Thing rdf:about="http://purl.org/olia/bambara.owl#INSTR">
        <rdf:type rdf:resource="http://www.w3.org/2002/07/owl#NamedIndividual"/>
        <rdf:type rdf:resource="http://purl.org/olia/bambara.owl#Derivation"/>
        <rdf:type rdf:resource="http://purl.org/olia/bambara.owl#derive.n"/>
        <rdf:type rdf:resource="http://purl.org/olia/bambara.owl#initial.v"/>
        <system:hasTagContaining>INSTR</system:hasTagContaining>
        <rdfs:comment xml:lang="fr">-lan/-nan/-ran; 
            v;
            n;
            nom d’instrument</rdfs:comment>
    </owl:Thing>
    


    <!-- http://purl.org/olia/bambara.owl#IPFV.AFF -->

    <owl:Thing rdf:about="http://purl.org/olia/bambara.owl#IPFV.AFF">
        <rdf:type rdf:resource="http://www.w3.org/2002/07/owl#NamedIndividual"/>
        <rdf:type rdf:resource="http://purl.org/olia/bambara.owl#MarquePredicative"/>
        <system:hasTag>IPFV.AFF</system:hasTag>
        <rdfs:comment xml:lang="fr">bɛ́ ~ bí ~ bé;
            marque affirmative de l’imperfectif</rdfs:comment>
    </owl:Thing>
    


    <!-- http://purl.org/olia/bambara.owl#IPFV.NEG -->

    <owl:Thing rdf:about="http://purl.org/olia/bambara.owl#IPFV.NEG">
        <rdf:type rdf:resource="http://www.w3.org/2002/07/owl#NamedIndividual"/>
        <rdf:type rdf:resource="http://purl.org/olia/bambara.owl#MarquePredicative"/>
        <system:hasTag>IPFV.NEG</system:hasTag>
        <rdfs:comment xml:lang="fr">tɛ́ ~ tí ~ té;
            marque de l’imperfectif négatif</rdfs:comment>
    </owl:Thing>
    


    <!-- http://purl.org/olia/bambara.owl#LOC -->

    <owl:Thing rdf:about="http://purl.org/olia/bambara.owl#LOC">
        <rdf:type rdf:resource="http://www.w3.org/2002/07/owl#NamedIndividual"/>
        <rdf:type rdf:resource="http://purl.org/olia/bambara.owl#Derivation"/>
        <rdf:type rdf:resource="http://purl.org/olia/bambara.owl#derive.n"/>
        <rdf:type rdf:resource="http://purl.org/olia/bambara.owl#initial.n"/>
        <system:hasTagContaining>LOC</system:hasTagContaining>
        <rdfs:comment xml:lang="fr">-la / -na;
            n;
            n;
            nom de place</rdfs:comment>
    </owl:Thing>
    


    <!-- http://purl.org/olia/bambara.owl#MNT1 -->

    <owl:Thing rdf:about="http://purl.org/olia/bambara.owl#MNT1">
        <rdf:type rdf:resource="http://www.w3.org/2002/07/owl#NamedIndividual"/>
        <rdf:type rdf:resource="http://purl.org/olia/bambara.owl#Derivation"/>
        <rdf:type rdf:resource="http://purl.org/olia/bambara.owl#derive.n"/>
        <rdf:type rdf:resource="http://purl.org/olia/bambara.owl#initial.n"/>
        <rdf:type rdf:resource="http://purl.org/olia/bambara.owl#initial.pp"/>
        <rdf:type rdf:resource="http://purl.org/olia/bambara.owl#initial.v"/>
        <system:hasTagContaining>MNT1</system:hasTagContaining>
        <rdfs:comment xml:lang="fr">-la / -na;
            v, n, pp;
            n;
            nom d’activité mentale ou de son résultat</rdfs:comment>
    </owl:Thing>
    


    <!-- http://purl.org/olia/bambara.owl#MNT2 -->

    <owl:Thing rdf:about="http://purl.org/olia/bambara.owl#MNT2">
        <rdf:type rdf:resource="http://www.w3.org/2002/07/owl#NamedIndividual"/>
        <rdf:type rdf:resource="http://purl.org/olia/bambara.owl#Derivation"/>
        <rdf:type rdf:resource="http://purl.org/olia/bambara.owl#derive.n"/>
        <rdf:type rdf:resource="http://purl.org/olia/bambara.owl#initial.n"/>
        <rdf:type rdf:resource="http://purl.org/olia/bambara.owl#initial.pp"/>
        <rdf:type rdf:resource="http://purl.org/olia/bambara.owl#initial.v"/>
        <system:hasTagContaining>MNT2</system:hasTagContaining>
        <rdfs:comment xml:lang="fr">-lata / -nata;
            v, n, pp;
            n;
            nom d’activité mentale ou de son résultat</rdfs:comment>
    </owl:Thing>
    


    <!-- http://purl.org/olia/bambara.owl#NMLZ -->

    <owl:Thing rdf:about="http://purl.org/olia/bambara.owl#NMLZ">
        <rdf:type rdf:resource="http://www.w3.org/2002/07/owl#NamedIndividual"/>
        <rdf:type rdf:resource="http://purl.org/olia/bambara.owl#Derivation"/>
        <rdf:type rdf:resource="http://purl.org/olia/bambara.owl#derive.n"/>
        <rdf:type rdf:resource="http://purl.org/olia/bambara.owl#initial.v"/>
        <system:hasTagContaining>NMLZ</system:hasTagContaining>
        <rdfs:comment xml:lang="fr">-li/-ni;
            v;
            n;
            nom verbal (nom d’action)</rdfs:comment>
    </owl:Thing>
    


    <!-- http://purl.org/olia/bambara.owl#NOM.CL -->

    <owl:Thing rdf:about="http://purl.org/olia/bambara.owl#NOM.CL">
        <rdf:type rdf:resource="http://www.w3.org/2002/07/owl#NamedIndividual"/>
        <rdf:type rdf:resource="http://purl.org/olia/bambara.owl#NomPropre"/>
        <system:hasTag>NOM.CL</system:hasTag>
        <rdfs:comment>nom clanique (jàmu)</rdfs:comment>
    </owl:Thing>
    


    <!-- http://purl.org/olia/bambara.owl#NOM.F -->

    <owl:Thing rdf:about="http://purl.org/olia/bambara.owl#NOM.F">
        <rdf:type rdf:resource="http://www.w3.org/2002/07/owl#NamedIndividual"/>
        <rdf:type rdf:resource="http://purl.org/olia/bambara.owl#NomPropre"/>
        <system:hasTag>NOM.F</system:hasTag>
        <rdfs:comment>prénom féminin</rdfs:comment>
    </owl:Thing>
    


    <!-- http://purl.org/olia/bambara.owl#NOM.M -->

    <owl:Thing rdf:about="http://purl.org/olia/bambara.owl#NOM.M">
        <rdf:type rdf:resource="http://www.w3.org/2002/07/owl#NamedIndividual"/>
        <rdf:type rdf:resource="http://purl.org/olia/bambara.owl#NomPropre"/>
        <system:hasTag>NOM.M</system:hasTag>
        <rdfs:comment>prénom masculin</rdfs:comment>
    </owl:Thing>
    


    <!-- http://purl.org/olia/bambara.owl#NOM.MF -->

    <owl:Thing rdf:about="http://purl.org/olia/bambara.owl#NOM.MF">
        <rdf:type rdf:resource="http://www.w3.org/2002/07/owl#NamedIndividual"/>
        <rdf:type rdf:resource="http://purl.org/olia/bambara.owl#NomPropre"/>
        <system:hasTag>NOM.MF</system:hasTag>
        <rdfs:comment>prénom ne distinguant pas entre les sexes</rdfs:comment>
    </owl:Thing>
    


    <!-- http://purl.org/olia/bambara.owl#OPT -->

    <owl:Thing rdf:about="http://purl.org/olia/bambara.owl#OPT">
        <rdf:type rdf:resource="http://www.w3.org/2002/07/owl#NamedIndividual"/>
        <rdf:type rdf:resource="http://purl.org/olia/bambara.owl#MarquePredicative"/>
        <system:hasTag>OPT</system:hasTag>
        <rdfs:comment xml:lang="fr">ká;
            marque d’optatif</rdfs:comment>
    </owl:Thing>
    


    <!-- http://purl.org/olia/bambara.owl#ORD -->

    <owl:Thing rdf:about="http://purl.org/olia/bambara.owl#ORD">
        <rdf:type rdf:resource="http://www.w3.org/2002/07/owl#NamedIndividual"/>
        <rdf:type rdf:resource="http://purl.org/olia/bambara.owl#Derivation"/>
        <rdf:type rdf:resource="http://purl.org/olia/bambara.owl#derive.adj"/>
        <rdf:type rdf:resource="http://purl.org/olia/bambara.owl#initial.num"/>
        <system:hasTagContaining>ORD</system:hasTagContaining>
        <rdfs:comment xml:lang="fr">-nan;
            num;
            adj;
            suffixe des numéraux ordinaux</rdfs:comment>
    </owl:Thing>
    


    <!-- http://purl.org/olia/bambara.owl#PFV.EMPH -->

    <owl:Thing rdf:about="http://purl.org/olia/bambara.owl#PFV.EMPH">
        <rdf:type rdf:resource="http://www.w3.org/2002/07/owl#NamedIndividual"/>
        <rdf:type rdf:resource="http://purl.org/olia/bambara.owl#MarquePredicative"/>
        <system:hasTag>PFV.EMPH</system:hasTag>
        <rdfs:comment xml:lang="fr">yé kà;
            EQU INF (une marque disjoint; autrement,PFV.EMPH);
            marque du passé récent;
            rarement utilisé</rdfs:comment>
    </owl:Thing>
    


    <!-- http://purl.org/olia/bambara.owl#PFV.INTR -->

    <owl:Thing rdf:about="http://purl.org/olia/bambara.owl#PFV.INTR">
        <rdf:type rdf:resource="http://www.w3.org/2002/07/owl#NamedIndividual"/>
        <rdf:type rdf:resource="http://purl.org/olia/bambara.owl#Flexion"/>
        <system:hasTagEndingWith>PFV.INTR</system:hasTagEndingWith>
        <rdfs:comment xml:lang="fr">-ra/-la/-na;
            v (v.i);
            marque du perfectif intransitif;
            - na après une syllable comportant un élement nasal ;
            - la après une syllabe orale à consonnes r ou l ;
            - ra dans tous les autres cas</rdfs:comment>
        <rdfs:comment xml:lang="en">Perfective intransitive marker (V. Vydrine)</rdfs:comment>
    </owl:Thing>
    


    <!-- http://purl.org/olia/bambara.owl#PFV.NEG -->

    <owl:Thing rdf:about="http://purl.org/olia/bambara.owl#PFV.NEG">
        <rdf:type rdf:resource="http://www.w3.org/2002/07/owl#NamedIndividual"/>
        <rdf:type rdf:resource="http://purl.org/olia/bambara.owl#MarquePredicative"/>
        <system:hasTag>PFV.NEG</system:hasTag>
        <rdfs:comment xml:lang="fr">má;
            marque négative du perfectif</rdfs:comment>
    </owl:Thing>
    


    <!-- http://purl.org/olia/bambara.owl#PFV.TR -->

    <owl:Thing rdf:about="http://purl.org/olia/bambara.owl#PFV.TR">
        <rdf:type rdf:resource="http://www.w3.org/2002/07/owl#NamedIndividual"/>
        <rdf:type rdf:resource="http://purl.org/olia/bambara.owl#Particule"/>
        <system:hasTag>PFV.TR</system:hasTag>
        <rdfs:comment xml:lang="fr">yé;
            marque du perfectif affirmatif transitif</rdfs:comment>
    </owl:Thing>
    


    <!-- http://purl.org/olia/bambara.owl#PL -->

    <owl:Thing rdf:about="http://purl.org/olia/bambara.owl#PL">
        <rdf:type rdf:resource="http://www.w3.org/2002/07/owl#NamedIndividual"/>
        <rdf:type rdf:resource="http://purl.org/olia/bambara.owl#Flexion"/>
        <system:hasTagEndingWith>PL</system:hasTagEndingWith>
        <rdfs:comment xml:lang="fr">-w;
            n, adj, dtm, prn;
            marque du pluriel</rdfs:comment>
    </owl:Thing>
    


    <!-- http://purl.org/olia/bambara.owl#PL2 -->

    <owl:Thing rdf:about="http://purl.org/olia/bambara.owl#PL2">
        <rdf:type rdf:resource="http://www.w3.org/2002/07/owl#NamedIndividual"/>
        <rdf:type rdf:resource="http://purl.org/olia/bambara.owl#Flexion"/>
        <system:hasTagEndingWith>PL2</system:hasTagEndingWith>
        <rdfs:comment xml:lang="fr">-lú/-nú;
            prn, n, dtm;
            marque non-productive du pluriel (se combine avec les pronoms nìn, ò, mín, et avec le nom màa ‘homme’);
            -nú après une voyelle nasale, -lú ailleurs</rdfs:comment>
        <rdfs:comment xml:lang="en">There is no semantic difference between PL and PL2, the latter is used with specific lexemes. (V. Vydrine)</rdfs:comment>
    </owl:Thing>
    


    <!-- http://purl.org/olia/bambara.owl#POSS -->

    <owl:Thing rdf:about="http://purl.org/olia/bambara.owl#POSS">
        <rdf:type rdf:resource="http://www.w3.org/2002/07/owl#NamedIndividual"/>
        <rdf:type rdf:resource="http://purl.org/olia/bambara.owl#Conjonction"/>
        <system:hasTag>POSS</system:hasTag>
        <rdfs:comment xml:lang="fr">ká; 
            marque possessive</rdfs:comment>
    </owl:Thing>
    


    <!-- http://purl.org/olia/bambara.owl#PRES -->

    <owl:Thing rdf:about="http://purl.org/olia/bambara.owl#PRES">
        <rdf:type rdf:resource="http://www.w3.org/2002/07/owl#NamedIndividual"/>
        <rdf:type rdf:resource="http://purl.org/olia/bambara.owl#Copule"/>
        <system:hasTag>PRES</system:hasTag>
        <rdfs:comment xml:lang="fr">dòn;
            copule de l’énoncé non-verbal présentatif affirmatif</rdfs:comment>
    </owl:Thing>
    


    <!-- http://purl.org/olia/bambara.owl#PREV -->

    <owl:Thing rdf:about="http://purl.org/olia/bambara.owl#PREV">
        <rdf:type rdf:resource="http://www.w3.org/2002/07/owl#NamedIndividual"/>
        <rdf:type rdf:resource="http://purl.org/olia/bambara.owl#AutreAbreviation"/>
        <system:hasTag>PREV</system:hasTag>
        <rdfs:comment>l’élément initial d’un verbe composé n’ayant pas d’étymologie évidente (et pouvant parfois se détacher de la base verbale)</rdfs:comment>
        <owl:versionInfo>TODO: clarify whether this can be annotated as (part of) Verb</owl:versionInfo>
    </owl:Thing>
    


    <!-- http://purl.org/olia/bambara.owl#PRICE -->

    <owl:Thing rdf:about="http://purl.org/olia/bambara.owl#PRICE">
        <rdf:type rdf:resource="http://www.w3.org/2002/07/owl#NamedIndividual"/>
        <rdf:type rdf:resource="http://purl.org/olia/bambara.owl#Derivation"/>
        <rdf:type rdf:resource="http://purl.org/olia/bambara.owl#derive.n"/>
        <rdf:type rdf:resource="http://purl.org/olia/bambara.owl#initial.num"/>
        <system:hasTagContaining>PRICE</system:hasTagContaining>
        <rdfs:comment xml:lang="fr">-la / -na;
            num;
            n;
            nom de prix (« quantité de marchandise pour la valeur de X »)</rdfs:comment>
    </owl:Thing>
    


    <!-- http://purl.org/olia/bambara.owl#PRIV -->

    <owl:Thing rdf:about="http://purl.org/olia/bambara.owl#PRIV">
        <rdf:type rdf:resource="http://www.w3.org/2002/07/owl#NamedIndividual"/>
        <rdf:type rdf:resource="http://purl.org/olia/bambara.owl#Derivation"/>
        <rdf:type rdf:resource="http://purl.org/olia/bambara.owl#derive.adj"/>
        <rdf:type rdf:resource="http://purl.org/olia/bambara.owl#initial.n"/>
        <system:hasTagContaining>PRIV</system:hasTagContaining>
        <rdfs:comment xml:lang="fr">-ntan;
            n;
            adj, (n);
            adjectif dénominal privatif</rdfs:comment>
    </owl:Thing>
    


    <!-- http://purl.org/olia/bambara.owl#PROG -->

    <owl:Thing rdf:about="http://purl.org/olia/bambara.owl#PROG">
        <rdf:type rdf:resource="http://www.w3.org/2002/07/owl#NamedIndividual"/>
        <rdf:type rdf:resource="http://purl.org/olia/bambara.owl#Flexion"/>
        <system:hasTagEndingWith>PROG</system:hasTagEndingWith>
        <rdfs:comment xml:lang="fr">-la/-na;
            v, ptcp;
suffixe verbal du progressif (va de paire avec le pm bɛ́ (affirmatif), tɛ́ (négatif);
-na après une voyelle nasale ; -la après une voyelle orale ; se combine avec les verbes et avec le participe progressif-prospectif en –tɔ</rdfs:comment>
    </owl:Thing>
    


    <!-- http://purl.org/olia/bambara.owl#PROG.AFF -->

    <owl:Thing rdf:about="http://purl.org/olia/bambara.owl#PROG.AFF">
        <rdf:type rdf:resource="http://www.w3.org/2002/07/owl#NamedIndividual"/>
        <rdf:type rdf:resource="http://purl.org/olia/bambara.owl#MarquePredicative"/>
        <system:hasTag>PROG.AFF</system:hasTag>
        <rdfs:comment xml:lang="fr">bɛ́ kà;
            BE INF (une marque disjoint; autrement, PROG.AFF);
            marque affirmative du progressif</rdfs:comment>
    </owl:Thing>
    


    <!-- http://purl.org/olia/bambara.owl#PROG.NEG -->

    <owl:Thing rdf:about="http://purl.org/olia/bambara.owl#PROG.NEG">
        <rdf:type rdf:resource="http://www.w3.org/2002/07/owl#NamedIndividual"/>
        <rdf:type rdf:resource="http://purl.org/olia/bambara.owl#MarquePredicative"/>
        <system:hasTag>PROG.NEG</system:hasTag>
        <rdfs:comment xml:lang="fr">tɛ́ kà;
            COP.NEG INF (une marque disjoint; autrement, PROG.NEG);
            marque du progressif négatif</rdfs:comment>
    </owl:Thing>
    


    <!-- http://purl.org/olia/bambara.owl#PROH -->

    <owl:Thing rdf:about="http://purl.org/olia/bambara.owl#PROH">
        <rdf:type rdf:resource="http://www.w3.org/2002/07/owl#NamedIndividual"/>
        <rdf:type rdf:resource="http://purl.org/olia/bambara.owl#MarquePredicative"/>
        <system:hasTag>PROH</system:hasTag>
        <rdfs:comment xml:lang="fr">kàná ~ kánà;
            marque du prohibitif</rdfs:comment>
    </owl:Thing>
    


    <!-- http://purl.org/olia/bambara.owl#PST -->

    <owl:Thing rdf:about="http://purl.org/olia/bambara.owl#PST">
        <rdf:type rdf:resource="http://www.w3.org/2002/07/owl#NamedIndividual"/>
        <rdf:type rdf:resource="http://purl.org/olia/bambara.owl#Particule"/>
        <system:hasTag>PST</system:hasTag>
        <rdfs:comment xml:lang="fr">tùn;
            le plus souvent, précède la marque prédicative ou la copule;
            marque du passé discontinu</rdfs:comment>
    </owl:Thing>
    


    <!-- http://purl.org/olia/bambara.owl#PTCP.POT -->

    <owl:Thing rdf:about="http://purl.org/olia/bambara.owl#PTCP.POT">
        <rdf:type rdf:resource="http://www.w3.org/2002/07/owl#NamedIndividual"/>
        <rdf:type rdf:resource="http://purl.org/olia/bambara.owl#Derivation"/>
        <rdf:type rdf:resource="http://purl.org/olia/bambara.owl#derive.ptcp"/>
        <rdf:type rdf:resource="http://purl.org/olia/bambara.owl#initial.v"/>
        <system:hasTagContaining>PTCP.POT</system:hasTagContaining>
        <rdfs:comment xml:lang="fr">-ta;
            v;
            ptcp;
            participe potentiel</rdfs:comment>
    </owl:Thing>
    


    <!-- http://purl.org/olia/bambara.owl#PTCP.PRIV -->

    <owl:Thing rdf:about="http://purl.org/olia/bambara.owl#PTCP.PRIV">
        <rdf:type rdf:resource="http://www.w3.org/2002/07/owl#NamedIndividual"/>
        <rdf:type rdf:resource="http://purl.org/olia/bambara.owl#Derivation"/>
        <rdf:type rdf:resource="http://purl.org/olia/bambara.owl#derive.ptcp"/>
        <rdf:type rdf:resource="http://purl.org/olia/bambara.owl#initial.v"/>
        <system:hasTagContaining>PCTCP.PRIV</system:hasTagContaining>
        <rdfs:comment xml:lang="fr">-bali;
            v;
            ptcp;
            participe privatif</rdfs:comment>
    </owl:Thing>
    


    <!-- http://purl.org/olia/bambara.owl#PTCP.RES -->

    <owl:Thing rdf:about="http://purl.org/olia/bambara.owl#PTCP.RES">
        <rdf:type rdf:resource="http://www.w3.org/2002/07/owl#NamedIndividual"/>
        <rdf:type rdf:resource="http://purl.org/olia/bambara.owl#Derivation"/>
        <rdf:type rdf:resource="http://purl.org/olia/bambara.owl#derive.ptcp"/>
        <rdf:type rdf:resource="http://purl.org/olia/bambara.owl#initial.v"/>
        <system:hasTagContaining>PTCP.RES</system:hasTagContaining>
        <rdfs:comment xml:lang="fr">-len/-nen;
            v;
            ptcp;
            participe à valeur résultative</rdfs:comment>
    </owl:Thing>
    


    <!-- http://purl.org/olia/bambara.owl#Q -->

    <owl:Thing rdf:about="http://purl.org/olia/bambara.owl#Q">
        <rdf:type rdf:resource="http://www.w3.org/2002/07/owl#NamedIndividual"/>
        <rdf:type rdf:resource="http://purl.org/olia/bambara.owl#Particule"/>
        <system:hasTag>Q</system:hasTag>
        <rdfs:comment xml:lang="fr">wà;
            en fin d’énoncé;
            particule de question générale</rdfs:comment>
    </owl:Thing>
    


    <!-- http://purl.org/olia/bambara.owl#QUAL.AFF -->

    <owl:Thing rdf:about="http://purl.org/olia/bambara.owl#QUAL.AFF">
        <rdf:type rdf:resource="http://www.w3.org/2002/07/owl#NamedIndividual"/>
        <rdf:type rdf:resource="http://purl.org/olia/bambara.owl#MarquePredicative"/>
        <system:hasTag>QUAL.AFF</system:hasTag>
        <rdfs:comment xml:lang="fr">ká;
            marque affirmative de l’énoncé qualitatif</rdfs:comment>
    </owl:Thing>
    


    <!-- http://purl.org/olia/bambara.owl#QUAL.NEG -->

    <owl:Thing rdf:about="http://purl.org/olia/bambara.owl#QUAL.NEG">
        <rdf:type rdf:resource="http://www.w3.org/2002/07/owl#NamedIndividual"/>
        <rdf:type rdf:resource="http://purl.org/olia/bambara.owl#MarquePredicative"/>
        <system:hasTag>QUAL.NEG</system:hasTag>
        <rdfs:comment xml:lang="fr">mán;
            marque négative de l’énoncé qualitati</rdfs:comment>
    </owl:Thing>
    


    <!-- http://purl.org/olia/bambara.owl#RECP -->

    <owl:Thing rdf:about="http://purl.org/olia/bambara.owl#RECP">
        <rdf:type rdf:resource="http://www.w3.org/2002/07/owl#NamedIndividual"/>
        <rdf:type rdf:resource="http://purl.org/olia/bambara.owl#Derivation"/>
        <rdf:type rdf:resource="http://purl.org/olia/bambara.owl#PronomNonPersonnel"/>
        <rdf:type rdf:resource="http://purl.org/olia/bambara.owl#derive.n"/>
        <rdf:type rdf:resource="http://purl.org/olia/bambara.owl#initial.n"/>
        <rdf:type rdf:resource="http://purl.org/olia/bambara.owl#initial.v"/>
        <system:hasTag>RECP</system:hasTag>
        <system:hasTagContaining>RECP</system:hasTagContaining>
        <rdfs:comment xml:lang="fr">ɲɔgɔn/ɲwan/ ɲwaan;
            v, n;
            n;
            suffixoïde à valeur de « nom de partenaire »</rdfs:comment>
        <rdfs:comment xml:lang="fr">ɲɔ́gɔn;
            pronom réciproque</rdfs:comment>
    </owl:Thing>
    


    <!-- http://purl.org/olia/bambara.owl#RECP.PRN -->

    <owl:Thing rdf:about="http://purl.org/olia/bambara.owl#RECP.PRN">
        <rdf:type rdf:resource="http://www.w3.org/2002/07/owl#NamedIndividual"/>
        <rdf:type rdf:resource="http://purl.org/olia/bambara.owl#Derivation"/>
        <rdf:type rdf:resource="http://purl.org/olia/bambara.owl#derive.n"/>
        <rdf:type rdf:resource="http://purl.org/olia/bambara.owl#initial.n"/>
        <system:hasTagContaining>RECP.PRN</system:hasTagContaining>
        <rdfs:comment xml:lang="fr">-ma;
            n;
            n;
            suffixe nominal réciproque</rdfs:comment>
    </owl:Thing>
    


    <!-- http://purl.org/olia/bambara.owl#REFL -->

    <owl:Thing rdf:about="http://purl.org/olia/bambara.owl#REFL">
        <rdf:type rdf:resource="http://www.w3.org/2002/07/owl#NamedIndividual"/>
        <rdf:type rdf:resource="http://purl.org/olia/bambara.owl#PronomNonPersonnel"/>
        <system:hasTag>REFL</system:hasTag>
        <rdfs:comment xml:lang="fr">í;
            pronom réfléchi</rdfs:comment>
    </owl:Thing>
    


    <!-- http://purl.org/olia/bambara.owl#REL -->

    <owl:Thing rdf:about="http://purl.org/olia/bambara.owl#REL">
        <rdf:type rdf:resource="http://www.w3.org/2002/07/owl#NamedIndividual"/>
        <rdf:type rdf:resource="http://purl.org/olia/bambara.owl#PronomDeterminatif"/>
        <rdf:type>
            <owl:Class>
                <owl:unionOf rdf:parseType="Collection">
                    <rdf:Description rdf:about="http://purl.org/olia/bambara.owl#Determinatif"/>
                    <rdf:Description rdf:about="http://purl.org/olia/bambara.owl#PronomNonPersonnel"/>
                </owl:unionOf>
            </owl:Class>
        </rdf:type>
        <system:hasTag>REL</system:hasTag>
        <rdfs:comment xml:lang="fr">mín;
            dtm, pron;
            suit le groupe nominal relativisé dans la clause subordonné à gauche ; remplace le groupe nominal dans la clause subordonnée à droite;
            marque de relativisation</rdfs:comment>
    </owl:Thing>
    


    <!-- http://purl.org/olia/bambara.owl#SEQ -->

    <owl:Thing rdf:about="http://purl.org/olia/bambara.owl#SEQ">
        <rdf:type rdf:resource="http://www.w3.org/2002/07/owl#NamedIndividual"/>
        <rdf:type rdf:resource="http://purl.org/olia/bambara.owl#MarquePredicative"/>
        <system:hasTag>SEQ</system:hasTag>
        <rdfs:comment xml:lang="fr">dìyé;
            marque séquentative;
            dialecte de Sikasso</rdfs:comment>
    </owl:Thing>
    


    <!-- http://purl.org/olia/bambara.owl#ST -->

    <owl:Thing rdf:about="http://purl.org/olia/bambara.owl#ST">
        <rdf:type rdf:resource="http://www.w3.org/2002/07/owl#NamedIndividual"/>
        <rdf:type rdf:resource="http://purl.org/olia/bambara.owl#Derivation"/>
        <rdf:type rdf:resource="http://purl.org/olia/bambara.owl#derive.adj"/>
        <rdf:type rdf:resource="http://purl.org/olia/bambara.owl#derive.n"/>
        <rdf:type rdf:resource="http://purl.org/olia/bambara.owl#initial.n"/>
        <system:hasTagMatching>.*[^a-zA-Z]ST.*</system:hasTagMatching>
        <rdfs:comment xml:lang="fr">-tɔ;
            n;
            n, adj;
            nom du sujet d’état (le plus souvent, infavorable)</rdfs:comment>
    </owl:Thing>
    


    <!-- http://purl.org/olia/bambara.owl#STAT -->

    <owl:Thing rdf:about="http://purl.org/olia/bambara.owl#STAT">
        <rdf:type rdf:resource="http://www.w3.org/2002/07/owl#NamedIndividual"/>
        <rdf:type rdf:resource="http://purl.org/olia/bambara.owl#Derivation"/>
        <rdf:type rdf:resource="http://purl.org/olia/bambara.owl#derive.adj"/>
        <rdf:type rdf:resource="http://purl.org/olia/bambara.owl#initial.n"/>
        <system:hasTagContaining>STAT</system:hasTagContaining>
        <rdfs:comment xml:lang="fr">-lama / -nama;
            n;
            adj;
            adjectif dénominal à valeur « en guise de », « en qualité de », « fait de », « en tant que...</rdfs:comment>
    </owl:Thing>
    


    <!-- http://purl.org/olia/bambara.owl#SUPER -->

    <owl:Thing rdf:about="http://purl.org/olia/bambara.owl#SUPER">
        <rdf:type rdf:resource="http://www.w3.org/2002/07/owl#NamedIndividual"/>
        <rdf:type rdf:resource="http://purl.org/olia/bambara.owl#Derivation"/>
        <rdf:type rdf:resource="http://purl.org/olia/bambara.owl#derive.adj"/>
        <system:hasTagContaining>SUPER</system:hasTagContaining>
        <rdfs:comment xml:lang="fr">-ma- / -man-;
            (dans);
            adj;
            connecteur des composantes des adjectifs composés; les variantes avec les voyelles nasale et orale sont distribuées lexicalement</rdfs:comment>
    </owl:Thing>
    


    <!-- http://purl.org/olia/bambara.owl#SUPER2 -->

    <owl:Thing rdf:about="http://purl.org/olia/bambara.owl#SUPER2">
        <rdf:type rdf:resource="http://www.w3.org/2002/07/owl#NamedIndividual"/>
        <rdf:type rdf:resource="http://purl.org/olia/bambara.owl#Derivation"/>
        <rdf:type rdf:resource="http://purl.org/olia/bambara.owl#derive.v"/>
        <rdf:type rdf:resource="http://purl.org/olia/bambara.owl#initial.v"/>
        <system:hasTagContaining>SUPER</system:hasTagContaining>
        <rdfs:comment xml:lang="fr">mà- ~ màn-;
            v;
            v;
            préfixe à valeur obscure (étymologiquement, valeur suppressive)</rdfs:comment>
        <owl:versionInfo>TODO: disambiguate with the other gloss value SUPER (for homographic morphemes), these two will get conflated</owl:versionInfo>
    </owl:Thing>
    


    <!-- http://purl.org/olia/bambara.owl#TOP -->

    <owl:Thing rdf:about="http://purl.org/olia/bambara.owl#TOP">
        <rdf:type rdf:resource="http://www.w3.org/2002/07/owl#NamedIndividual"/>
        <rdf:type rdf:resource="http://purl.org/olia/bambara.owl#Particule"/>
        <system:hasTag>TOP</system:hasTag>
        <rdfs:comment xml:lang="fr">kɔ̀ni;
            marque de topicalisation contrastive</rdfs:comment>
    </owl:Thing>
    


    <!-- http://purl.org/olia/bambara.owl#TOP.CNTR -->

    <owl:Thing rdf:about="http://purl.org/olia/bambara.owl#TOP.CNTR">
        <rdf:type rdf:resource="http://www.w3.org/2002/07/owl#NamedIndividual"/>
        <rdf:type rdf:resource="http://purl.org/olia/bambara.owl#Particule"/>
        <system:hasTag>TOP.CNTR</system:hasTag>
        <rdfs:comment xml:lang="fr">dùn;
            marque dela topicalisation contrastive du sujet</rdfs:comment>
    </owl:Thing>
    


    <!-- http://purl.org/olia/bambara.owl#TOP2 -->

    <owl:Thing rdf:about="http://purl.org/olia/bambara.owl#TOP2">
        <rdf:type rdf:resource="http://www.w3.org/2002/07/owl#NamedIndividual"/>
        <rdf:type rdf:resource="http://purl.org/olia/bambara.owl#AutreAbreviation"/>
        <system:hasTag>TOP</system:hasTag>
        <rdfs:comment>toponyme</rdfs:comment>
        <owl:versionInfo>TODO: disambiguate TOP=topic and TOP=toponymic</owl:versionInfo>
    </owl:Thing>
    


    <!-- http://purl.org/olia/bambara.owl#adj -->

    <owl:Thing rdf:about="http://purl.org/olia/bambara.owl#adj">
        <rdf:type rdf:resource="http://www.w3.org/2002/07/owl#NamedIndividual"/>
        <rdf:type rdf:resource="http://purl.org/olia/bambara.owl#Adjectif"/>
        <system:hasTag>adj</system:hasTag>
        <rdfs:comment>adjectif</rdfs:comment>
    </owl:Thing>
    


    <!-- http://purl.org/olia/bambara.owl#adj_n -->

    <owl:Thing rdf:about="http://purl.org/olia/bambara.owl#adj_n">
        <rdf:type rdf:resource="http://www.w3.org/2002/07/owl#NamedIndividual"/>
        <rdf:type rdf:resource="http://purl.org/olia/bambara.owl#Adjectif"/>
        <rdf:type rdf:resource="http://purl.org/olia/bambara.owl#Nom"/>
        <system:hasTag>adj/n</system:hasTag>
    </owl:Thing>
    


    <!-- http://purl.org/olia/bambara.owl#adv -->

    <owl:Thing rdf:about="http://purl.org/olia/bambara.owl#adv">
        <rdf:type rdf:resource="http://www.w3.org/2002/07/owl#NamedIndividual"/>
        <rdf:type rdf:resource="http://purl.org/olia/bambara.owl#Adverbe"/>
        <system:hasTag>adv</system:hasTag>
        <rdfs:comment xml:lang="en">adverb (in postverbal position) [V. Vydrine]</rdfs:comment>
    </owl:Thing>
    


    <!-- http://purl.org/olia/bambara.owl#adv.p -->

    <owl:Thing rdf:about="http://purl.org/olia/bambara.owl#adv.p">
        <rdf:type rdf:resource="http://www.w3.org/2002/07/owl#NamedIndividual"/>
        <rdf:type rdf:resource="http://purl.org/olia/bambara.owl#Adverbe"/>
        <system:hasTag>adv.p</system:hasTag>
        <rdfs:comment>adverbe préverbal</rdfs:comment>
    </owl:Thing>
    


    <!-- http://purl.org/olia/bambara.owl#c -->

    <owl:Thing rdf:about="http://purl.org/olia/bambara.owl#c">
        <rdf:type rdf:resource="http://www.w3.org/2002/07/owl#NamedIndividual"/>
        <rdf:type rdf:resource="http://purl.org/olia/bambara.owl#Ponctuation"/>
        <system:hasTag>c</system:hasTag>
    </owl:Thing>
    


    <!-- http://purl.org/olia/bambara.owl#ce -->

    <owl:Thing rdf:about="http://purl.org/olia/bambara.owl#ce">
        <rdf:type rdf:resource="http://www.w3.org/2002/07/owl#NamedIndividual"/>
        <rdf:type rdf:resource="http://purl.org/olia/bambara.owl#PronomNonPersonnel"/>
        <system:hasTag>ce</system:hasTag>
        <rdfs:comment xml:lang="fr">ò;
            pronom anaphorique et démonstratif</rdfs:comment>
    </owl:Thing>
    


    <!-- http://purl.org/olia/bambara.owl#ce.PL -->

    <owl:Thing rdf:about="http://purl.org/olia/bambara.owl#ce.PL">
        <rdf:type rdf:resource="http://www.w3.org/2002/07/owl#NamedIndividual"/>
        <rdf:type rdf:resource="http://purl.org/olia/bambara.owl#PronomNonPersonnel"/>
        <system:hasTag>ce.PL</system:hasTag>
        <rdfs:comment xml:lang="fr">ò.lú;
            pronom anaphorique pluriel ; pronom emphatique 3ème pl</rdfs:comment>
    </owl:Thing>
    


    <!-- http://purl.org/olia/bambara.owl#conj -->

    <owl:Thing rdf:about="http://purl.org/olia/bambara.owl#conj">
        <rdf:type rdf:resource="http://www.w3.org/2002/07/owl#NamedIndividual"/>
        <rdf:type rdf:resource="http://purl.org/olia/bambara.owl#Conjonction"/>
        <system:hasTag>conj</system:hasTag>
        <rdfs:comment>conjonction</rdfs:comment>
    </owl:Thing>
    


    <!-- http://purl.org/olia/bambara.owl#cop -->

    <owl:Thing rdf:about="http://purl.org/olia/bambara.owl#cop">
        <rdf:type rdf:resource="http://www.w3.org/2002/07/owl#NamedIndividual"/>
        <rdf:type rdf:resource="http://purl.org/olia/bambara.owl#Copule"/>
        <system:hasTag>cop</system:hasTag>
        <rdfs:comment>copule</rdfs:comment>
    </owl:Thing>
    


    <!-- http://purl.org/olia/bambara.owl#intj -->

    <owl:Thing rdf:about="http://purl.org/olia/bambara.owl#intj">
        <rdf:type rdf:resource="http://www.w3.org/2002/07/owl#NamedIndividual"/>
        <rdf:type rdf:resource="http://purl.org/olia/bambara.owl#Interjection"/>
        <system:hasTag>intj</system:hasTag>
        <rdfs:comment>interjection</rdfs:comment>
    </owl:Thing>
    


    <!-- http://purl.org/olia/bambara.owl#n -->

    <owl:Thing rdf:about="http://purl.org/olia/bambara.owl#n">
        <rdf:type rdf:resource="http://www.w3.org/2002/07/owl#NamedIndividual"/>
        <rdf:type rdf:resource="http://purl.org/olia/bambara.owl#Nom"/>
        <system:hasTag>n</system:hasTag>
        <rdfs:comment>nom</rdfs:comment>
    </owl:Thing>
    


    <!-- http://purl.org/olia/bambara.owl#n_adv -->

    <owl:Thing rdf:about="http://purl.org/olia/bambara.owl#n_adv">
        <rdf:type rdf:resource="http://www.w3.org/2002/07/owl#NamedIndividual"/>
        <rdf:type rdf:resource="http://purl.org/olia/bambara.owl#Adverbe"/>
        <rdf:type rdf:resource="http://purl.org/olia/bambara.owl#Nom"/>
        <system:hasTag>adv/n</system:hasTag>
        <system:hasTag>n/adv</system:hasTag>
        <owl:versionInfo xml:lang="en">added adv/n as also found in sample file (CC)</owl:versionInfo>
    </owl:Thing>
    


    <!-- http://purl.org/olia/bambara.owl#num -->

    <owl:Thing rdf:about="http://purl.org/olia/bambara.owl#num">
        <rdf:type rdf:resource="http://www.w3.org/2002/07/owl#NamedIndividual"/>
        <rdf:type rdf:resource="http://purl.org/olia/bambara.owl#Numératif"/>
        <system:hasTag>num</system:hasTag>
        <rdfs:comment>numératif</rdfs:comment>
    </owl:Thing>
    


    <!-- http://purl.org/olia/bambara.owl#onomat -->

    <owl:Thing rdf:about="http://purl.org/olia/bambara.owl#onomat">
        <rdf:type rdf:resource="http://www.w3.org/2002/07/owl#NamedIndividual"/>
        <rdf:type rdf:resource="http://purl.org/olia/bambara.owl#Onomatopee"/>
        <system:hasTag>onomat</system:hasTag>
        <rdfs:comment>onomatopée</rdfs:comment>
    </owl:Thing>
    


    <!-- http://purl.org/olia/bambara.owl#pers -->

    <owl:Thing rdf:about="http://purl.org/olia/bambara.owl#pers">
        <rdf:type rdf:resource="http://www.w3.org/2002/07/owl#NamedIndividual"/>
        <rdf:type rdf:resource="http://purl.org/olia/bambara.owl#PronomPersonnel"/>
        <system:hasTag>pers</system:hasTag>
        <rdfs:comment>pronom personnel</rdfs:comment>
    </owl:Thing>
    


    <!-- http://purl.org/olia/bambara.owl#pm -->

    <owl:Thing rdf:about="http://purl.org/olia/bambara.owl#pm">
        <rdf:type rdf:resource="http://www.w3.org/2002/07/owl#NamedIndividual"/>
        <rdf:type rdf:resource="http://purl.org/olia/bambara.owl#MarquePredicative"/>
        <system:hasTag>pm</system:hasTag>
        <rdfs:comment>marque prédicative</rdfs:comment>
    </owl:Thing>
    


    <!-- http://purl.org/olia/bambara.owl#prep -->

    <owl:Thing rdf:about="http://purl.org/olia/bambara.owl#prep">
        <rdf:type rdf:resource="http://www.w3.org/2002/07/owl#NamedIndividual"/>
        <rdf:type rdf:resource="http://purl.org/olia/bambara.owl#Préposition"/>
        <system:hasTag>prep</system:hasTag>
        <rdfs:comment>préposition</rdfs:comment>
    </owl:Thing>
    


    <!-- http://purl.org/olia/bambara.owl#prep_conj -->

    <owl:Thing rdf:about="http://purl.org/olia/bambara.owl#prep_conj">
        <rdf:type rdf:resource="http://www.w3.org/2002/07/owl#NamedIndividual"/>
        <rdf:type rdf:resource="http://purl.org/olia/bambara.owl#Conjonction"/>
        <rdf:type rdf:resource="http://purl.org/olia/bambara.owl#Préposition"/>
        <system:hasTag>conj/prep</system:hasTag>
        <system:hasTag>prep/conj</system:hasTag>
        <rdfs:comment xml:lang="en">all Bambara prepositions can also be used as conjunctions (not necessarily the other way around) [V. Vydrine]</rdfs:comment>
        <owl:versionInfo xml:lang="en">CC: guidelines provide prep/conj only, I added conj/prep as found in sample file</owl:versionInfo>
    </owl:Thing>
    


    <!-- http://purl.org/olia/bambara.owl#prn -->

    <owl:Thing rdf:about="http://purl.org/olia/bambara.owl#prn">
        <rdf:type rdf:resource="http://www.w3.org/2002/07/owl#NamedIndividual"/>
        <rdf:type rdf:resource="http://purl.org/olia/bambara.owl#PronomNonPersonnel"/>
        <system:hasTag>prn</system:hasTag>
        <rdfs:comment>pronom (non-personnel)</rdfs:comment>
    </owl:Thing>
    


    <!-- http://purl.org/olia/bambara.owl#prn_dtm -->

    <owl:Thing rdf:about="http://purl.org/olia/bambara.owl#prn_dtm">
        <rdf:type rdf:resource="http://www.w3.org/2002/07/owl#NamedIndividual"/>
        <rdf:type rdf:resource="http://purl.org/olia/bambara.owl#PronomDeterminatif"/>
        <system:hasTag>prn/dtm</system:hasTag>
        <rdfs:comment>a tag used in the sample file, but not found in the documentation (CC)</rdfs:comment>
    </owl:Thing>
    


    <!-- http://purl.org/olia/bambara.owl#prt -->

    <owl:Thing rdf:about="http://purl.org/olia/bambara.owl#prt">
        <rdf:type rdf:resource="http://www.w3.org/2002/07/owl#NamedIndividual"/>
        <rdf:type rdf:resource="http://purl.org/olia/bambara.owl#Particule"/>
        <system:hasTag>prt</system:hasTag>
        <rdfs:comment>particule</rdfs:comment>
    </owl:Thing>
    


    <!-- http://purl.org/olia/bambara.owl#ptcp -->

    <owl:Thing rdf:about="http://purl.org/olia/bambara.owl#ptcp">
        <rdf:type rdf:resource="http://www.w3.org/2002/07/owl#NamedIndividual"/>
        <rdf:type rdf:resource="http://purl.org/olia/bambara.owl#Participe"/>
        <system:hasTag>ptcp</system:hasTag>
        <rdfs:comment>participe</rdfs:comment>
    </owl:Thing>
    


    <!-- http://purl.org/olia/bambara.owl#v -->

    <owl:Thing rdf:about="http://purl.org/olia/bambara.owl#v">
        <rdf:type rdf:resource="http://www.w3.org/2002/07/owl#NamedIndividual"/>
        <rdf:type rdf:resource="http://purl.org/olia/bambara.owl#VerbeDynamique"/>
        <system:hasTag>v</system:hasTag>
        <rdfs:comment>verbe</rdfs:comment>
    </owl:Thing>
    


    <!-- http://purl.org/olia/bambara.owl#vq -->

    <owl:Thing rdf:about="http://purl.org/olia/bambara.owl#vq">
        <rdf:type rdf:resource="http://www.w3.org/2002/07/owl#NamedIndividual"/>
        <rdf:type rdf:resource="http://purl.org/olia/bambara.owl#VerbeQualitatif"/>
        <system:hasTag>vq</system:hasTag>
        <rdfs:comment>verbe qualitativ</rdfs:comment>
    </owl:Thing>
    


    <!-- http://purl.org/olia/bambara.owl#vq_adj -->

    <owl:Thing rdf:about="http://purl.org/olia/bambara.owl#vq_adj">
        <rdf:type rdf:resource="http://www.w3.org/2002/07/owl#NamedIndividual"/>
        <rdf:type rdf:resource="http://purl.org/olia/bambara.owl#Adjectif"/>
        <rdf:type rdf:resource="http://purl.org/olia/bambara.owl#VerbeQualitatif"/>
        <system:hasTag>vq/adj</system:hasTag>
    </owl:Thing>
    


    <!-- http://purl.org/olia/bambara.owl#1PL -->

    <owl:Thing rdf:about="http://purl.org/olia/bambara.owl#1PL">
        <rdf:type rdf:resource="http://www.w3.org/2002/07/owl#NamedIndividual"/>
        <rdf:type rdf:resource="http://purl.org/olia/bambara.owl#PronomPersonnel"/>
        <system:hasTag>1PL</system:hasTag>
        <rdfs:comment xml:lang="fr">án;
            pronom personnel non-emphatique 1ère pers. pl.</rdfs:comment>
    </owl:Thing>
    


    <!-- http://purl.org/olia/bambara.owl#1PL.EMPH -->

    <owl:Thing rdf:about="http://purl.org/olia/bambara.owl#1PL.EMPH">
        <rdf:type rdf:resource="http://www.w3.org/2002/07/owl#NamedIndividual"/>
        <rdf:type rdf:resource="http://purl.org/olia/bambara.owl#PronomPersonnel"/>
        <system:hasTag>1PL.EMPH</system:hasTag>
        <rdfs:comment xml:lang="fr">ánw;
            pronom personnel emphatique 1ère pers. pl.</rdfs:comment>
    </owl:Thing>
    


    <!-- http://purl.org/olia/bambara.owl#2PL -->

    <owl:Thing rdf:about="http://purl.org/olia/bambara.owl#2PL">
        <rdf:type rdf:resource="http://www.w3.org/2002/07/owl#NamedIndividual"/>
        <rdf:type rdf:resource="http://purl.org/olia/bambara.owl#PronomPersonnel"/>
        <system:hasTag>2PL</system:hasTag>
        <rdfs:comment xml:lang="fr">á;
            pronom personnel non-emphatique 2ème pers. pl.</rdfs:comment>
    </owl:Thing>
    


    <!-- http://purl.org/olia/bambara.owl#2PL.EMPH -->

    <owl:Thing rdf:about="http://purl.org/olia/bambara.owl#2PL.EMPH">
        <rdf:type rdf:resource="http://www.w3.org/2002/07/owl#NamedIndividual"/>
        <rdf:type rdf:resource="http://purl.org/olia/bambara.owl#PronomPersonnel"/>
        <system:hasTag>2PL.EMPH</system:hasTag>
        <rdfs:comment xml:lang="fr">áw;
            pronom personnel emphatique 2ème pers. pl.</rdfs:comment>
    </owl:Thing>
    


    <!-- http://purl.org/olia/bambara.owl#2SG.EMPH -->

    <owl:Thing rdf:about="http://purl.org/olia/bambara.owl#2SG.EMPH">
        <rdf:type rdf:resource="http://www.w3.org/2002/07/owl#NamedIndividual"/>
        <rdf:type rdf:resource="http://purl.org/olia/bambara.owl#PronomPersonnel"/>
        <system:hasTag>2SG.EMPH</system:hasTag>
        <rdfs:comment xml:lang="fr">é;
            pronom personnel emphatique 2ème pers. sg.</rdfs:comment>
    </owl:Thing>
    


    <!-- http://purl.org/olia/bambara.owl#3SG -->

    <owl:Thing rdf:about="http://purl.org/olia/bambara.owl#3SG">
        <rdf:type rdf:resource="http://www.w3.org/2002/07/owl#NamedIndividual"/>
        <rdf:type rdf:resource="http://purl.org/olia/bambara.owl#PronomPersonnel"/>
        <system:hasTag>3SG</system:hasTag>
        <rdfs:comment xml:lang="fr">à pronom personnel non-emphatique 3ème pers. sg.</rdfs:comment>
        <rdfs:comment xml:lang="fr">í;
            pronom personnel non-emphatique 2ème pers. sg.</rdfs:comment>
    </owl:Thing>
</rdf:RDF>



<!-- Generated by the OWL API (version 4.5.25.2023-02-15T19:15:49Z) https://github.com/owlcs/owlapi -->

