<?xml version="1.0"?>
<rdf:RDF xmlns="http://purl.org/olia/genia.owl#"
     xml:base="http://purl.org/olia/genia.owl"
     xmlns:ms="http://w3id.org/meta-share/meta-share/"
     xmlns:dct="http://purl.org/dc/terms/"
     xmlns:owl="http://www.w3.org/2002/07/owl#"
     xmlns:rdf="http://www.w3.org/1999/02/22-rdf-syntax-ns#"
     xmlns:xml="http://www.w3.org/XML/1998/namespace"
     xmlns:xsd="http://www.w3.org/2001/XMLSchema#"
     xmlns:rdfs="http://www.w3.org/2000/01/rdf-schema#"
     xmlns:olia_system="http://purl.org/olia/system.owl#">
    <owl:Ontology rdf:about="http://purl.org/olia/genia.owl">
        <dct:license rdf:resource="https://creativecommons.org/licenses/by/3.0/"/>
        <ms:language rdf:resource="http://lexvo.org/id/iso639-3/eng"/>
        <rdfs:comment>
		Annotation scheme of the GENIA corpus (Kim et al. 2003).&lt;br/&gt;
		Kim, J.D. and Ohta, T. and Tateisi, Y. and Tsujii, J. (2003), 
		GENIA corpus-a semantically annotated corpus for bio-textmining,
		Bioinformatics 19(1):180-182
	</rdfs:comment>
        <owl:versionInfo> 2008-03-12 created 2010-04-06 updated Christian Chiarcos </owl:versionInfo>
        <owl:versionInfo>Derived from the Penn Annotation Model and the translation table given below
      &lt;br&gt; &lt;p align=&quot;justify&quot; class=&quot;caption&quot; style=&quot;text-indent: 42.0pt;
      margin-left: 42.0pt&quot;&gt; Part-of-speech labels of GENIA and PTB &lt;/p&gt;
      &lt;table cellpadding=&quot;0&quot; cellspacing=&quot;0&quot; class=&quot;msonormaltable&quot; border=&quot;0&quot;
      style=&quot;margin-left: -.5pt&quot;&gt; &lt;tr style=&quot;height: 1.15pt&quot;&gt; &lt;td
      valign=&quot;top&quot; width=&quot;83&quot; style=&quot;padding-left: 5.4pt; padding-top: 0cm; width: 62.1pt; border:
      solid black 1.0pt; border-right: none; height: 1.15pt; padding-right: 5.4pt; padding-bottom:
      0cm&quot;&gt; &lt;p class=&quot;msonormal&quot;&gt; PTB label &lt;/p&gt;
      &lt;/td&gt; &lt;td valign=&quot;top&quot; width=&quot;104&quot; style=&quot;padding-left: 5.4pt;
      padding-top: 0cm; width: 78.3pt; border: solid black 1.0pt; border-right: none; height:
      1.15pt; padding-right: 5.4pt; padding-bottom: 0cm&quot;&gt; &lt;p class=&quot;msonormal&quot;&gt;
      GENIA label &lt;/p&gt; &lt;/td&gt; &lt;td valign=&quot;top&quot; width=&quot;374&quot;
      style=&quot;padding-left: 5.4pt; padding-top: 0cm; width: 280.25pt; border: solid black 1.0pt;
      height: 1.15pt; padding-right: 5.4pt; padding-bottom: 0cm&quot;&gt; &lt;p
      class=&quot;msonormal&quot;&gt; Part-of-speech &lt;/p&gt; &lt;/td&gt;
      &lt;/tr&gt; &lt;tr style=&quot;height: 1.15pt&quot;&gt; &lt;td valign=&quot;top&quot;
      colspan=&quot;2&quot; width=&quot;187&quot; style=&quot;padding-bottom: 0cm; width: 140.4pt; border-left: solid black
      1.0pt; border-right: none; border-top: none; height: 1.15pt; padding-top: 0cm; padding-right:
      5.4pt; border-bottom: solid black 1.0pt; padding-left: 5.4pt&quot;&gt; &lt;p align=&quot;center&quot;
      class=&quot;msonormal&quot;&gt; CC &lt;/p&gt; &lt;/td&gt; &lt;td valign=&quot;top&quot;
      width=&quot;374&quot; style=&quot;padding-left: 5.4pt; padding-top: 0cm; width: 280.25pt; border-top: none;
      border: solid black 1.0pt; height: 1.15pt; padding-right: 5.4pt; padding-bottom: 0cm&quot;&gt;
      &lt;p class=&quot;msonormal&quot;&gt; Coordinating conjunction &lt;/p&gt;
      &lt;/td&gt; &lt;/tr&gt; &lt;tr style=&quot;height: 1.15pt&quot;&gt; &lt;td
      valign=&quot;top&quot; colspan=&quot;2&quot; width=&quot;187&quot; style=&quot;padding-bottom: 0cm; width: 140.4pt; border-left:
      solid black 1.0pt; border-right: none; border-top: none; height: 1.15pt; padding-top: 0cm;
      padding-right: 5.4pt; border-bottom: solid black 1.0pt; padding-left: 5.4pt&quot;&gt; &lt;p
      align=&quot;center&quot; class=&quot;msonormal&quot;&gt; CD &lt;/p&gt; &lt;/td&gt; &lt;td
      valign=&quot;top&quot; width=&quot;374&quot; style=&quot;padding-left: 5.4pt; padding-top: 0cm; width: 280.25pt;
      border-top: none; border: solid black 1.0pt; height: 1.15pt; padding-right: 5.4pt;
      padding-bottom: 0cm&quot;&gt; &lt;p class=&quot;msonormal&quot;&gt; Cardinal number
      &lt;/p&gt; &lt;/td&gt; &lt;/tr&gt; &lt;tr style=&quot;height:
      1.15pt&quot;&gt; &lt;td valign=&quot;top&quot; width=&quot;83&quot; style=&quot;padding-bottom: 0cm; width: 62.1pt;
      border-left: solid black 1.0pt; border-right: none; border-top: none; height: 1.15pt;
      padding-top: 0cm; padding-right: 5.4pt; border-bottom: solid black 1.0pt; padding-left:
      5.4pt&quot;&gt; &lt;p align=&quot;center&quot; class=&quot;msonormal&quot;&gt; : &lt;/p&gt;
      &lt;/td&gt; &lt;td valign=&quot;top&quot; width=&quot;104&quot; style=&quot;padding-bottom: 0cm; width:
      78.3pt; border-left: solid black 1.0pt; border-right: none; border-top: none; height: 1.15pt;
      padding-top: 0cm; padding-right: 5.4pt; border-bottom: solid black 1.0pt; padding-left:
      5.4pt&quot;&gt; &lt;p align=&quot;center&quot; class=&quot;msonormal&quot;&gt; COLON &lt;/p&gt;
      &lt;/td&gt; &lt;td valign=&quot;top&quot; width=&quot;374&quot; style=&quot;padding-left: 5.4pt;
      padding-top: 0cm; width: 280.25pt; border-top: none; border: solid black 1.0pt; height:
      1.15pt; padding-right: 5.4pt; padding-bottom: 0cm&quot;&gt; &lt;p class=&quot;msonormal&quot;&gt;
      Colon &lt;/p&gt; &lt;/td&gt; &lt;/tr&gt; &lt;tr style=&quot;height:
      1.15pt&quot;&gt; &lt;td valign=&quot;top&quot; width=&quot;83&quot; style=&quot;padding-bottom: 0cm; width: 62.1pt;
      border-left: solid black 1.0pt; border-right: none; border-top: none; height: 1.15pt;
      padding-top: 0cm; padding-right: 5.4pt; border-bottom: solid black 1.0pt; padding-left:
      5.4pt&quot;&gt; &lt;p align=&quot;center&quot; class=&quot;msonormal&quot;&gt; , &lt;/p&gt;
      &lt;/td&gt; &lt;td valign=&quot;top&quot; width=&quot;104&quot; style=&quot;padding-bottom: 0cm; width:
      78.3pt; border-left: solid black 1.0pt; border-right: none; border-top: none; height: 1.15pt;
      padding-top: 0cm; padding-right: 5.4pt; border-bottom: solid black 1.0pt; padding-left:
      5.4pt&quot;&gt; &lt;p align=&quot;center&quot; class=&quot;msonormal&quot;&gt; COMMA &lt;/p&gt;
      &lt;/td&gt; &lt;td valign=&quot;top&quot; width=&quot;374&quot; style=&quot;padding-left: 5.4pt;
      padding-top: 0cm; width: 280.25pt; border-top: none; border: solid black 1.0pt; height:
      1.15pt; padding-right: 5.4pt; padding-bottom: 0cm&quot;&gt; &lt;p class=&quot;msonormal&quot;&gt;
      Comma &lt;/p&gt; &lt;/td&gt; &lt;/tr&gt; &lt;tr style=&quot;height:
      1.15pt&quot;&gt; &lt;td valign=&quot;top&quot; colspan=&quot;2&quot; width=&quot;187&quot; style=&quot;padding-bottom: 0cm;
      width: 140.4pt; border-left: solid black 1.0pt; border-right: none; border-top: none; height:
      1.15pt; padding-top: 0cm; padding-right: 5.4pt; border-bottom: solid black 1.0pt;
      padding-left: 5.4pt&quot;&gt; &lt;p align=&quot;center&quot; class=&quot;msonormal&quot;&gt; DT
      &lt;/p&gt; &lt;/td&gt; &lt;td valign=&quot;top&quot; width=&quot;374&quot;
      style=&quot;padding-left: 5.4pt; padding-top: 0cm; width: 280.25pt; border-top: none; border: solid
      black 1.0pt; height: 1.15pt; padding-right: 5.4pt; padding-bottom: 0cm&quot;&gt; &lt;p
      class=&quot;msonormal&quot;&gt; Determiner &lt;/p&gt; &lt;/td&gt;
      &lt;/tr&gt; &lt;tr style=&quot;height: 1.15pt&quot;&gt; &lt;td valign=&quot;top&quot;
      colspan=&quot;2&quot; width=&quot;187&quot; style=&quot;padding-bottom: 0cm; width: 140.4pt; border-left: solid black
      1.0pt; border-right: none; border-top: none; height: 1.15pt; padding-top: 0cm; padding-right:
      5.4pt; border-bottom: solid black 1.0pt; padding-left: 5.4pt&quot;&gt; &lt;p align=&quot;center&quot;
      class=&quot;msonormal&quot;&gt; EX &lt;/p&gt; &lt;/td&gt; &lt;td valign=&quot;top&quot;
      width=&quot;374&quot; style=&quot;padding-left: 5.4pt; padding-top: 0cm; width: 280.25pt; border-top: none;
      border: solid black 1.0pt; height: 1.15pt; padding-right: 5.4pt; padding-bottom: 0cm&quot;&gt;
      &lt;p class=&quot;msonormal&quot;&gt; Existential (there) &lt;/p&gt; &lt;/td&gt;
      &lt;/tr&gt; &lt;tr style=&quot;height: 1.15pt&quot;&gt; &lt;td valign=&quot;top&quot;
      colspan=&quot;2&quot; width=&quot;187&quot; style=&quot;padding-bottom: 0cm; width: 140.4pt; border-left: solid black
      1.0pt; border-right: none; border-top: none; height: 1.15pt; padding-top: 0cm; padding-right:
      5.4pt; border-bottom: solid black 1.0pt; padding-left: 5.4pt&quot;&gt; &lt;p align=&quot;center&quot;
      class=&quot;msonormal&quot;&gt; FW &lt;/p&gt; &lt;/td&gt; &lt;td valign=&quot;top&quot;
      width=&quot;374&quot; style=&quot;padding-left: 5.4pt; padding-top: 0cm; width: 280.25pt; border-top: none;
      border: solid black 1.0pt; height: 1.15pt; padding-right: 5.4pt; padding-bottom: 0cm&quot;&gt;
      &lt;p class=&quot;msonormal&quot;&gt; Foreign words &lt;/p&gt; &lt;/td&gt;
      &lt;/tr&gt; &lt;tr style=&quot;height: 1.15pt&quot;&gt; &lt;td valign=&quot;top&quot;
      colspan=&quot;2&quot; width=&quot;187&quot; style=&quot;padding-bottom: 0cm; width: 140.4pt; border-left: solid black
      1.0pt; border-right: none; border-top: none; height: 1.15pt; padding-top: 0cm; padding-right:
      5.4pt; border-bottom: solid black 1.0pt; padding-left: 5.4pt&quot;&gt; &lt;p align=&quot;center&quot;
      class=&quot;msonormal&quot;&gt; IN &lt;/p&gt; &lt;/td&gt; &lt;td valign=&quot;top&quot;
      width=&quot;374&quot; style=&quot;padding-left: 5.4pt; padding-top: 0cm; width: 280.25pt; border-top: none;
      border: solid black 1.0pt; height: 1.15pt; padding-right: 5.4pt; padding-bottom: 0cm&quot;&gt;
      &lt;p class=&quot;msonormal&quot;&gt; Preposition or subordinating conjunction
      &lt;/p&gt; &lt;/td&gt; &lt;/tr&gt; &lt;tr style=&quot;height:
      1.15pt&quot;&gt; &lt;td valign=&quot;top&quot; colspan=&quot;2&quot; width=&quot;187&quot; style=&quot;padding-bottom: 0cm;
      width: 140.4pt; border-left: solid black 1.0pt; border-right: none; border-top: none; height:
      1.15pt; padding-top: 0cm; padding-right: 5.4pt; border-bottom: solid black 1.0pt;
      padding-left: 5.4pt&quot;&gt; &lt;p align=&quot;center&quot; class=&quot;msonormal&quot;&gt; JJ
      &lt;/p&gt; &lt;/td&gt; &lt;td valign=&quot;top&quot; width=&quot;374&quot;
      style=&quot;padding-left: 5.4pt; padding-top: 0cm; width: 280.25pt; border-top: none; border: solid
      black 1.0pt; height: 1.15pt; padding-right: 5.4pt; padding-bottom: 0cm&quot;&gt; &lt;p
      class=&quot;msonormal&quot;&gt; Adjective &lt;/p&gt; &lt;/td&gt; &lt;/tr&gt;
      &lt;tr style=&quot;height: 1.15pt&quot;&gt; &lt;td valign=&quot;top&quot; colspan=&quot;2&quot; width=&quot;187&quot;
      style=&quot;padding-bottom: 0cm; width: 140.4pt; border-left: solid black 1.0pt; border-right:
      none; border-top: none; height: 1.15pt; padding-top: 0cm; padding-right: 5.4pt; border-bottom:
      solid black 1.0pt; padding-left: 5.4pt&quot;&gt; &lt;p align=&quot;center&quot;
      class=&quot;msonormal&quot;&gt; JJR &lt;/p&gt; &lt;/td&gt; &lt;td valign=&quot;top&quot;
      width=&quot;374&quot; style=&quot;padding-left: 5.4pt; padding-top: 0cm; width: 280.25pt; border-top: none;
      border: solid black 1.0pt; height: 1.15pt; padding-right: 5.4pt; padding-bottom: 0cm&quot;&gt;
      &lt;p class=&quot;msonormal&quot;&gt; Adjective, comparative &lt;/p&gt;
      &lt;/td&gt; &lt;/tr&gt; &lt;tr style=&quot;height: 1.15pt&quot;&gt; &lt;td
      valign=&quot;top&quot; colspan=&quot;2&quot; width=&quot;187&quot; style=&quot;padding-bottom: 0cm; width: 140.4pt; border-left:
      solid black 1.0pt; border-right: none; border-top: none; height: 1.15pt; padding-top: 0cm;
      padding-right: 5.4pt; border-bottom: solid black 1.0pt; padding-left: 5.4pt&quot;&gt; &lt;p
      align=&quot;center&quot; class=&quot;msonormal&quot;&gt; JJS &lt;/p&gt; &lt;/td&gt; &lt;td
      valign=&quot;top&quot; width=&quot;374&quot; style=&quot;padding-left: 5.4pt; padding-top: 0cm; width: 280.25pt;
      border-top: none; border: solid black 1.0pt; height: 1.15pt; padding-right: 5.4pt;
      padding-bottom: 0cm&quot;&gt; &lt;p class=&quot;msonormal&quot;&gt; Adjective, superlative
      &lt;/p&gt; &lt;/td&gt; &lt;/tr&gt; &lt;tr style=&quot;height:
      1.15pt&quot;&gt; &lt;td valign=&quot;top&quot; width=&quot;83&quot; style=&quot;padding-bottom: 0cm; width: 62.1pt;
      border-left: solid black 1.0pt; border-right: none; border-top: none; height: 1.15pt;
      padding-top: 0cm; padding-right: 5.4pt; border-bottom: solid black 1.0pt; padding-left:
      5.4pt&quot;&gt; &lt;p align=&quot;center&quot; class=&quot;msonormal&quot;&gt; &amp;#143;&amp;#179;
      &lt;/p&gt; &lt;/td&gt; &lt;td valign=&quot;top&quot; width=&quot;104&quot;
      style=&quot;padding-bottom: 0cm; width: 78.3pt; border-left: solid black 1.0pt; border-right: none;
      border-top: none; height: 1.15pt; padding-top: 0cm; padding-right: 5.4pt; border-bottom: solid
      black 1.0pt; padding-left: 5.4pt&quot;&gt; &lt;p align=&quot;center&quot; class=&quot;msonormal&quot;&gt;
      LQT &lt;/p&gt; &lt;/td&gt; &lt;td valign=&quot;top&quot; width=&quot;374&quot;
      style=&quot;padding-left: 5.4pt; padding-top: 0cm; width: 280.25pt; border-top: none; border: solid
      black 1.0pt; height: 1.15pt; padding-right: 5.4pt; padding-bottom: 0cm&quot;&gt; &lt;p
      class=&quot;msonormal&quot;&gt; Left quotation mark &lt;/p&gt; &lt;/td&gt;
      &lt;/tr&gt; &lt;tr style=&quot;height: 1.15pt&quot;&gt; &lt;td valign=&quot;top&quot;
      width=&quot;83&quot; style=&quot;padding-bottom: 0cm; width: 62.1pt; border-left: solid black 1.0pt;
      border-right: none; border-top: none; height: 1.15pt; padding-top: 0cm; padding-right: 5.4pt;
      border-bottom: solid black 1.0pt; padding-left: 5.4pt&quot;&gt; &lt;p align=&quot;center&quot;
      class=&quot;msonormal&quot;&gt; ( &lt;/p&gt; &lt;/td&gt; &lt;td valign=&quot;top&quot;
      width=&quot;104&quot; style=&quot;padding-bottom: 0cm; width: 78.3pt; border-left: solid black 1.0pt;
      border-right: none; border-top: none; height: 1.15pt; padding-top: 0cm; padding-right: 5.4pt;
      border-bottom: solid black 1.0pt; padding-left: 5.4pt&quot;&gt; &lt;p align=&quot;center&quot;
      class=&quot;msonormal&quot;&gt; LRB &lt;/p&gt; &lt;/td&gt; &lt;td valign=&quot;top&quot;
      width=&quot;374&quot; style=&quot;padding-left: 5.4pt; padding-top: 0cm; width: 280.25pt; border-top: none;
      border: solid black 1.0pt; height: 1.15pt; padding-right: 5.4pt; padding-bottom: 0cm&quot;&gt;
      &lt;p class=&quot;msonormal&quot;&gt; Left round bracket &lt;/p&gt; &lt;/td&gt;
      &lt;/tr&gt; &lt;tr style=&quot;height: 1.15pt&quot;&gt; &lt;td valign=&quot;top&quot;
      colspan=&quot;2&quot; width=&quot;187&quot; style=&quot;padding-bottom: 0cm; width: 140.4pt; border-left: solid black
      1.0pt; border-right: none; border-top: none; height: 1.15pt; padding-top: 0cm; padding-right:
      5.4pt; border-bottom: solid black 1.0pt; padding-left: 5.4pt&quot;&gt; &lt;p align=&quot;center&quot;
      class=&quot;msonormal&quot;&gt; LS &lt;/p&gt; &lt;/td&gt; &lt;td valign=&quot;top&quot;
      width=&quot;374&quot; style=&quot;padding-left: 5.4pt; padding-top: 0cm; width: 280.25pt; border-top: none;
      border: solid black 1.0pt; height: 1.15pt; padding-right: 5.4pt; padding-bottom: 0cm&quot;&gt;
      &lt;p class=&quot;msonormal&quot;&gt; List item marker &lt;/p&gt; &lt;/td&gt;
      &lt;/tr&gt; &lt;tr style=&quot;height: 1.15pt&quot;&gt; &lt;td valign=&quot;top&quot;
      colspan=&quot;2&quot; width=&quot;187&quot; style=&quot;padding-bottom: 0cm; width: 140.4pt; border-left: solid black
      1.0pt; border-right: none; border-top: none; height: 1.15pt; padding-top: 0cm; padding-right:
      5.4pt; border-bottom: solid black 1.0pt; padding-left: 5.4pt&quot;&gt; &lt;p align=&quot;center&quot;
      class=&quot;msonormal&quot;&gt; MD &lt;/p&gt; &lt;/td&gt; &lt;td valign=&quot;top&quot;
      width=&quot;374&quot; style=&quot;padding-left: 5.4pt; padding-top: 0cm; width: 280.25pt; border-top: none;
      border: solid black 1.0pt; height: 1.15pt; padding-right: 5.4pt; padding-bottom: 0cm&quot;&gt;
      &lt;p class=&quot;msonormal&quot;&gt; Modal verb &lt;/p&gt; &lt;/td&gt;
      &lt;/tr&gt; &lt;tr style=&quot;height: 1.15pt&quot;&gt; &lt;td valign=&quot;top&quot;
      colspan=&quot;2&quot; width=&quot;187&quot; style=&quot;padding-bottom: 0cm; width: 140.4pt; border-left: solid black
      1.0pt; border-right: none; border-top: none; height: 1.15pt; padding-top: 0cm; padding-right:
      5.4pt; border-bottom: solid black 1.0pt; padding-left: 5.4pt&quot;&gt; &lt;p align=&quot;center&quot;
      class=&quot;msonormal&quot;&gt; NN &lt;/p&gt; &lt;/td&gt; &lt;td valign=&quot;top&quot;
      width=&quot;374&quot; style=&quot;padding-left: 5.4pt; padding-top: 0cm; width: 280.25pt; border-top: none;
      border: solid black 1.0pt; height: 1.15pt; padding-right: 5.4pt; padding-bottom: 0cm&quot;&gt;
      &lt;p class=&quot;msonormal&quot;&gt; Common noun, singular &lt;/p&gt;
      &lt;/td&gt; &lt;/tr&gt; &lt;tr style=&quot;height: 1.15pt&quot;&gt; &lt;td
      valign=&quot;top&quot; colspan=&quot;2&quot; width=&quot;187&quot; style=&quot;padding-bottom: 0cm; width: 140.4pt; border-left:
      solid black 1.0pt; border-right: none; border-top: none; height: 1.15pt; padding-top: 0cm;
      padding-right: 5.4pt; border-bottom: solid black 1.0pt; padding-left: 5.4pt&quot;&gt; &lt;p
      align=&quot;center&quot; class=&quot;msonormal&quot;&gt; NNP &lt;/p&gt; &lt;/td&gt; &lt;td
      valign=&quot;top&quot; width=&quot;374&quot; style=&quot;padding-left: 5.4pt; padding-top: 0cm; width: 280.25pt;
      border-top: none; border: solid black 1.0pt; height: 1.15pt; padding-right: 5.4pt;
      padding-bottom: 0cm&quot;&gt; &lt;p class=&quot;msonormal&quot;&gt; Proper noun, singular
      &lt;/p&gt; &lt;/td&gt; &lt;/tr&gt; &lt;tr style=&quot;height:
      1.15pt&quot;&gt; &lt;td valign=&quot;top&quot; colspan=&quot;2&quot; width=&quot;187&quot; style=&quot;padding-bottom: 0cm;
      width: 140.4pt; border-left: solid black 1.0pt; border-right: none; border-top: none; height:
      1.15pt; padding-top: 0cm; padding-right: 5.4pt; border-bottom: solid black 1.0pt;
      padding-left: 5.4pt&quot;&gt; &lt;p align=&quot;center&quot; class=&quot;msonormal&quot;&gt; NNPS
      &lt;/p&gt; &lt;/td&gt; &lt;td valign=&quot;top&quot; width=&quot;374&quot;
      style=&quot;padding-left: 5.4pt; padding-top: 0cm; width: 280.25pt; border-top: none; border: solid
      black 1.0pt; height: 1.15pt; padding-right: 5.4pt; padding-bottom: 0cm&quot;&gt; &lt;p
      class=&quot;msonormal&quot;&gt; Proper noun, plural &lt;/p&gt; &lt;/td&gt;
      &lt;/tr&gt; &lt;tr style=&quot;height: 1.15pt&quot;&gt; &lt;td valign=&quot;top&quot;
      colspan=&quot;2&quot; width=&quot;187&quot; style=&quot;padding-bottom: 0cm; width: 140.4pt; border-left: solid black
      1.0pt; border-right: none; border-top: none; height: 1.15pt; padding-top: 0cm; padding-right:
      5.4pt; border-bottom: solid black 1.0pt; padding-left: 5.4pt&quot;&gt; &lt;p align=&quot;center&quot;
      class=&quot;msonormal&quot;&gt; NNS &lt;/p&gt; &lt;/td&gt; &lt;td valign=&quot;top&quot;
      width=&quot;374&quot; style=&quot;padding-left: 5.4pt; padding-top: 0cm; width: 280.25pt; border-top: none;
      border: solid black 1.0pt; height: 1.15pt; padding-right: 5.4pt; padding-bottom: 0cm&quot;&gt;
      &lt;p class=&quot;msonormal&quot;&gt; Common noun, plural &lt;/p&gt; &lt;/td&gt;
      &lt;/tr&gt; &lt;tr style=&quot;height: 1.15pt&quot;&gt; &lt;td valign=&quot;top&quot;
      colspan=&quot;2&quot; width=&quot;187&quot; style=&quot;padding-bottom: 0cm; width: 140.4pt; border-left: solid black
      1.0pt; border-right: none; border-top: none; height: 1.15pt; padding-top: 0cm; padding-right:
      5.4pt; border-bottom: solid black 1.0pt; padding-left: 5.4pt&quot;&gt; &lt;p align=&quot;center&quot;
      class=&quot;msonormal&quot;&gt; PDT &lt;/p&gt; &lt;/td&gt; &lt;td valign=&quot;top&quot;
      width=&quot;374&quot; style=&quot;padding-left: 5.4pt; padding-top: 0cm; width: 280.25pt; border-top: none;
      border: solid black 1.0pt; height: 1.15pt; padding-right: 5.4pt; padding-bottom: 0cm&quot;&gt;
      &lt;p class=&quot;msonormal&quot;&gt; Pre-determiner &lt;/p&gt; &lt;/td&gt;
      &lt;/tr&gt; &lt;tr style=&quot;height: 1.15pt&quot;&gt; &lt;td valign=&quot;top&quot;
      width=&quot;83&quot; style=&quot;padding-bottom: 0cm; width: 62.1pt; border-left: solid black 1.0pt;
      border-right: none; border-top: none; height: 1.15pt; padding-top: 0cm; padding-right: 5.4pt;
      border-bottom: solid black 1.0pt; padding-left: 5.4pt&quot;&gt; &lt;p align=&quot;center&quot;
      class=&quot;msonormal&quot;&gt; . &lt;/p&gt; &lt;/td&gt; &lt;td valign=&quot;top&quot;
      width=&quot;104&quot; style=&quot;padding-bottom: 0cm; width: 78.3pt; border-left: solid black 1.0pt;
      border-right: none; border-top: none; height: 1.15pt; padding-top: 0cm; padding-right: 5.4pt;
      border-bottom: solid black 1.0pt; padding-left: 5.4pt&quot;&gt; &lt;p align=&quot;center&quot;
      class=&quot;msonormal&quot;&gt; PERIOD &lt;/p&gt; &lt;/td&gt; &lt;td
      valign=&quot;top&quot; width=&quot;374&quot; style=&quot;padding-left: 5.4pt; padding-top: 0cm; width: 280.25pt;
      border-top: none; border: solid black 1.0pt; height: 1.15pt; padding-right: 5.4pt;
      padding-bottom: 0cm&quot;&gt; &lt;p class=&quot;msonormal&quot;&gt; Period &lt;/p&gt;
      &lt;/td&gt; &lt;/tr&gt; &lt;tr style=&quot;height: 1.15pt&quot;&gt; &lt;td
      valign=&quot;top&quot; colspan=&quot;2&quot; width=&quot;187&quot; style=&quot;padding-bottom: 0cm; width: 140.4pt; border-left:
      solid black 1.0pt; border-right: none; border-top: none; height: 1.15pt; padding-top: 0cm;
      padding-right: 5.4pt; border-bottom: solid black 1.0pt; padding-left: 5.4pt&quot;&gt; &lt;p
      align=&quot;center&quot; class=&quot;msonormal&quot;&gt; POS &lt;/p&gt; &lt;/td&gt; &lt;td
      valign=&quot;top&quot; width=&quot;374&quot; style=&quot;padding-left: 5.4pt; padding-top: 0cm; width: 280.25pt;
      border-top: none; border: solid black 1.0pt; height: 1.15pt; padding-right: 5.4pt;
      padding-bottom: 0cm&quot;&gt; &lt;p class=&quot;msonormal&quot;&gt; Possessive marker
      (&amp;#143;&amp;#178;s and &amp;#143;&amp;#178;) &lt;/p&gt;
      &lt;/td&gt; &lt;/tr&gt; &lt;tr style=&quot;height: 1.15pt&quot;&gt; &lt;td
      valign=&quot;top&quot; colspan=&quot;2&quot; width=&quot;187&quot; style=&quot;padding-bottom: 0cm; width: 140.4pt; border-left:
      solid black 1.0pt; border-right: none; border-top: none; height: 1.15pt; padding-top: 0cm;
      padding-right: 5.4pt; border-bottom: solid black 1.0pt; padding-left: 5.4pt&quot;&gt; &lt;p
      align=&quot;center&quot; class=&quot;msonormal&quot;&gt; PRP &lt;/p&gt; &lt;/td&gt; &lt;td
      valign=&quot;top&quot; width=&quot;374&quot; style=&quot;padding-left: 5.4pt; padding-top: 0cm; width: 280.25pt;
      border-top: none; border: solid black 1.0pt; height: 1.15pt; padding-right: 5.4pt;
      padding-bottom: 0cm&quot;&gt; &lt;p class=&quot;msonormal&quot;&gt; Personal pronoun
      &lt;/p&gt; &lt;/td&gt; &lt;/tr&gt; &lt;tr style=&quot;height:
      1.15pt&quot;&gt; &lt;td valign=&quot;top&quot; width=&quot;83&quot; style=&quot;padding-bottom: 0cm; width: 62.1pt;
      border-left: solid black 1.0pt; border-right: none; border-top: none; height: 1.15pt;
      padding-top: 0cm; padding-right: 5.4pt; border-bottom: solid black 1.0pt; padding-left:
      5.4pt&quot;&gt; &lt;p align=&quot;center&quot; class=&quot;msonormal&quot;&gt; PRPP$ &lt;/p&gt;
      &lt;/td&gt; &lt;td valign=&quot;top&quot; width=&quot;104&quot; style=&quot;padding-bottom: 0cm; width:
      78.3pt; border-left: solid black 1.0pt; border-right: none; border-top: none; height: 1.15pt;
      padding-top: 0cm; padding-right: 5.4pt; border-bottom: solid black 1.0pt; padding-left:
      5.4pt&quot;&gt; &lt;p align=&quot;center&quot; class=&quot;msonormal&quot;&gt; PRPP &lt;/p&gt;
      &lt;/td&gt; &lt;td valign=&quot;top&quot; width=&quot;374&quot; style=&quot;padding-left: 5.4pt;
      padding-top: 0cm; width: 280.25pt; border-top: none; border: solid black 1.0pt; height:
      1.15pt; padding-right: 5.4pt; padding-bottom: 0cm&quot;&gt; &lt;p class=&quot;msonormal&quot;&gt;
      Personal pronoun, possessive &lt;/p&gt; &lt;/td&gt; &lt;/tr&gt;
      &lt;tr style=&quot;height: 1.15pt&quot;&gt; &lt;td valign=&quot;top&quot; colspan=&quot;2&quot; width=&quot;187&quot;
      style=&quot;padding-bottom: 0cm; width: 140.4pt; border-left: solid black 1.0pt; border-right:
      none; border-top: none; height: 1.15pt; padding-top: 0cm; padding-right: 5.4pt; border-bottom:
      solid black 1.0pt; padding-left: 5.4pt&quot;&gt; &lt;p align=&quot;center&quot;
      class=&quot;msonormal&quot;&gt; RB &lt;/p&gt; &lt;/td&gt; &lt;td valign=&quot;top&quot;
      width=&quot;374&quot; style=&quot;padding-left: 5.4pt; padding-top: 0cm; width: 280.25pt; border-top: none;
      border: solid black 1.0pt; height: 1.15pt; padding-right: 5.4pt; padding-bottom: 0cm&quot;&gt;
      &lt;p class=&quot;msonormal&quot;&gt; Adverb &lt;/p&gt; &lt;/td&gt;
      &lt;/tr&gt; &lt;tr style=&quot;height: 1.15pt&quot;&gt; &lt;td valign=&quot;top&quot;
      colspan=&quot;2&quot; width=&quot;187&quot; style=&quot;padding-bottom: 0cm; width: 140.4pt; border-left: solid black
      1.0pt; border-right: none; border-top: none; height: 1.15pt; padding-top: 0cm; padding-right:
      5.4pt; border-bottom: solid black 1.0pt; padding-left: 5.4pt&quot;&gt; &lt;p align=&quot;center&quot;
      class=&quot;msonormal&quot;&gt; RBR &lt;/p&gt; &lt;/td&gt; &lt;td valign=&quot;top&quot;
      width=&quot;374&quot; style=&quot;padding-left: 5.4pt; padding-top: 0cm; width: 280.25pt; border-top: none;
      border: solid black 1.0pt; height: 1.15pt; padding-right: 5.4pt; padding-bottom: 0cm&quot;&gt;
      &lt;p class=&quot;msonormal&quot;&gt; Adverb, comparative &lt;/p&gt; &lt;/td&gt;
      &lt;/tr&gt; &lt;tr style=&quot;height: 1.15pt&quot;&gt; &lt;td valign=&quot;top&quot;
      colspan=&quot;2&quot; width=&quot;187&quot; style=&quot;padding-bottom: 0cm; width: 140.4pt; border-left: solid black
      1.0pt; border-right: none; border-top: none; height: 1.15pt; padding-top: 0cm; padding-right:
      5.4pt; border-bottom: solid black 1.0pt; padding-left: 5.4pt&quot;&gt; &lt;p align=&quot;center&quot;
      class=&quot;msonormal&quot;&gt; RBS &lt;/p&gt; &lt;/td&gt; &lt;td valign=&quot;top&quot;
      width=&quot;374&quot; style=&quot;padding-left: 5.4pt; padding-top: 0cm; width: 280.25pt; border-top: none;
      border: solid black 1.0pt; height: 1.15pt; padding-right: 5.4pt; padding-bottom: 0cm&quot;&gt;
      &lt;p class=&quot;msonormal&quot;&gt; Adverb, superlative &lt;/p&gt; &lt;/td&gt;
      &lt;/tr&gt; &lt;tr style=&quot;height: 1.15pt&quot;&gt; &lt;td valign=&quot;top&quot;
      colspan=&quot;2&quot; width=&quot;187&quot; style=&quot;padding-bottom: 0cm; width: 140.4pt; border-left: solid black
      1.0pt; border-right: none; border-top: none; height: 1.15pt; padding-top: 0cm; padding-right:
      5.4pt; border-bottom: solid black 1.0pt; padding-left: 5.4pt&quot;&gt; &lt;p align=&quot;center&quot;
      class=&quot;msonormal&quot;&gt; RP &lt;/p&gt; &lt;/td&gt; &lt;td valign=&quot;top&quot;
      width=&quot;374&quot; style=&quot;padding-left: 5.4pt; padding-top: 0cm; width: 280.25pt; border-top: none;
      border: solid black 1.0pt; height: 1.15pt; padding-right: 5.4pt; padding-bottom: 0cm&quot;&gt;
      &lt;p class=&quot;msonormal&quot;&gt; Particle &lt;/p&gt; &lt;/td&gt;
      &lt;/tr&gt; &lt;tr style=&quot;height: 1.15pt&quot;&gt; &lt;td valign=&quot;top&quot;
      width=&quot;83&quot; style=&quot;padding-bottom: 0cm; width: 62.1pt; border-left: solid black 1.0pt;
      border-right: none; border-top: none; height: 1.15pt; padding-top: 0cm; padding-right: 5.4pt;
      border-bottom: solid black 1.0pt; padding-left: 5.4pt&quot;&gt; &lt;p align=&quot;center&quot;
      class=&quot;msonormal&quot;&gt; &amp;#143;&amp;#180; &lt;/p&gt; &lt;/td&gt;
      &lt;td valign=&quot;top&quot; width=&quot;104&quot; style=&quot;padding-bottom: 0cm; width: 78.3pt; border-left:
      solid black 1.0pt; border-right: none; border-top: none; height: 1.15pt; padding-top: 0cm;
      padding-right: 5.4pt; border-bottom: solid black 1.0pt; padding-left: 5.4pt&quot;&gt; &lt;p
      align=&quot;center&quot; class=&quot;msonormal&quot;&gt; RQT &lt;/p&gt; &lt;/td&gt; &lt;td
      valign=&quot;top&quot; width=&quot;374&quot; style=&quot;padding-left: 5.4pt; padding-top: 0cm; width: 280.25pt;
      border-top: none; border: solid black 1.0pt; height: 1.15pt; padding-right: 5.4pt;
      padding-bottom: 0cm&quot;&gt; &lt;p class=&quot;msonormal&quot;&gt; Right quotation mark
      &lt;/p&gt; &lt;/td&gt; &lt;/tr&gt; &lt;tr style=&quot;height:
      1.15pt&quot;&gt; &lt;td valign=&quot;top&quot; width=&quot;83&quot; style=&quot;padding-bottom: 0cm; width: 62.1pt;
      border-left: solid black 1.0pt; border-right: none; border-top: none; height: 1.15pt;
      padding-top: 0cm; padding-right: 5.4pt; border-bottom: solid black 1.0pt; padding-left:
      5.4pt&quot;&gt; &lt;p align=&quot;center&quot; class=&quot;msonormal&quot;&gt; ) &lt;/p&gt;
      &lt;/td&gt; &lt;td valign=&quot;top&quot; width=&quot;104&quot; style=&quot;padding-bottom: 0cm; width:
      78.3pt; border-left: solid black 1.0pt; border-right: none; border-top: none; height: 1.15pt;
      padding-top: 0cm; padding-right: 5.4pt; border-bottom: solid black 1.0pt; padding-left:
      5.4pt&quot;&gt; &lt;p align=&quot;center&quot; class=&quot;msonormal&quot;&gt; RRB &lt;/p&gt;
      &lt;/td&gt; &lt;td valign=&quot;top&quot; width=&quot;374&quot; style=&quot;padding-left: 5.4pt;
      padding-top: 0cm; width: 280.25pt; border-top: none; border: solid black 1.0pt; height:
      1.15pt; padding-right: 5.4pt; padding-bottom: 0cm&quot;&gt; &lt;p class=&quot;msonormal&quot;&gt;
      Right round bracket &lt;/p&gt; &lt;/td&gt; &lt;/tr&gt; &lt;tr
      style=&quot;height: 1.15pt&quot;&gt; &lt;td valign=&quot;top&quot; colspan=&quot;2&quot; width=&quot;187&quot;
      style=&quot;padding-bottom: 0cm; width: 140.4pt; border-left: solid black 1.0pt; border-right:
      none; border-top: none; height: 1.15pt; padding-top: 0cm; padding-right: 5.4pt; border-bottom:
      solid black 1.0pt; padding-left: 5.4pt&quot;&gt; &lt;p align=&quot;center&quot;
      class=&quot;msonormal&quot;&gt; SYM &lt;/p&gt; &lt;/td&gt; &lt;td valign=&quot;top&quot;
      width=&quot;374&quot; style=&quot;padding-left: 5.4pt; padding-top: 0cm; width: 280.25pt; border-top: none;
      border: solid black 1.0pt; height: 1.15pt; padding-right: 5.4pt; padding-bottom: 0cm&quot;&gt;
      &lt;p class=&quot;msonormal&quot;&gt; Symbol &lt;/p&gt; &lt;/td&gt;
      &lt;/tr&gt; &lt;tr style=&quot;height: 1.15pt&quot;&gt; &lt;td valign=&quot;top&quot;
      colspan=&quot;2&quot; width=&quot;187&quot; style=&quot;padding-bottom: 0cm; width: 140.4pt; border-left: solid black
      1.0pt; border-right: none; border-top: none; height: 1.15pt; padding-top: 0cm; padding-right:
      5.4pt; border-bottom: solid black 1.0pt; padding-left: 5.4pt&quot;&gt; &lt;p align=&quot;center&quot;
      class=&quot;msonormal&quot;&gt; TO &lt;/p&gt; &lt;/td&gt; &lt;td valign=&quot;top&quot;
      width=&quot;374&quot; style=&quot;padding-left: 5.4pt; padding-top: 0cm; width: 280.25pt; border-top: none;
      border: solid black 1.0pt; height: 1.15pt; padding-right: 5.4pt; padding-bottom: 0cm&quot;&gt;
      &lt;p class=&quot;msonormal&quot;&gt; To &lt;/p&gt; &lt;/td&gt;
      &lt;/tr&gt; &lt;tr style=&quot;height: 1.15pt&quot;&gt; &lt;td valign=&quot;top&quot;
      colspan=&quot;2&quot; width=&quot;187&quot; style=&quot;padding-bottom: 0cm; width: 140.4pt; border-left: solid black
      1.0pt; border-right: none; border-top: none; height: 1.15pt; padding-top: 0cm; padding-right:
      5.4pt; border-bottom: solid black 1.0pt; padding-left: 5.4pt&quot;&gt; &lt;p align=&quot;center&quot;
      class=&quot;msonormal&quot;&gt; VB &lt;/p&gt; &lt;/td&gt; &lt;td valign=&quot;top&quot;
      width=&quot;374&quot; style=&quot;padding-left: 5.4pt; padding-top: 0cm; width: 280.25pt; border-top: none;
      border: solid black 1.0pt; height: 1.15pt; padding-right: 5.4pt; padding-bottom: 0cm&quot;&gt;
      &lt;p class=&quot;msonormal&quot;&gt; Verb, base form &lt;/p&gt; &lt;/td&gt;
      &lt;/tr&gt; &lt;tr style=&quot;height: 1.15pt&quot;&gt; &lt;td valign=&quot;top&quot;
      colspan=&quot;2&quot; width=&quot;187&quot; style=&quot;padding-bottom: 0cm; width: 140.4pt; border-left: solid black
      1.0pt; border-right: none; border-top: none; height: 1.15pt; padding-top: 0cm; padding-right:
      5.4pt; border-bottom: solid black 1.0pt; padding-left: 5.4pt&quot;&gt; &lt;p align=&quot;center&quot;
      class=&quot;msonormal&quot;&gt; VBD &lt;/p&gt; &lt;/td&gt; &lt;td valign=&quot;top&quot;
      width=&quot;374&quot; style=&quot;padding-left: 5.4pt; padding-top: 0cm; width: 280.25pt; border-top: none;
      border: solid black 1.0pt; height: 1.15pt; padding-right: 5.4pt; padding-bottom: 0cm&quot;&gt;
      &lt;p class=&quot;msonormal&quot;&gt; Verb, past tense &lt;/p&gt; &lt;/td&gt;
      &lt;/tr&gt; &lt;tr style=&quot;height: 1.15pt&quot;&gt; &lt;td valign=&quot;top&quot;
      colspan=&quot;2&quot; width=&quot;187&quot; style=&quot;padding-bottom: 0cm; width: 140.4pt; border-left: solid black
      1.0pt; border-right: none; border-top: none; height: 1.15pt; padding-top: 0cm; padding-right:
      5.4pt; border-bottom: solid black 1.0pt; padding-left: 5.4pt&quot;&gt; &lt;p align=&quot;center&quot;
      class=&quot;msonormal&quot;&gt; VBG &lt;/p&gt; &lt;/td&gt; &lt;td valign=&quot;top&quot;
      width=&quot;374&quot; style=&quot;padding-left: 5.4pt; padding-top: 0cm; width: 280.25pt; border-top: none;
      border: solid black 1.0pt; height: 1.15pt; padding-right: 5.4pt; padding-bottom: 0cm&quot;&gt;
      &lt;p class=&quot;msonormal&quot;&gt; Verb, present participle or gerund &lt;/p&gt;
      &lt;/td&gt; &lt;/tr&gt; &lt;tr style=&quot;height: 1.15pt&quot;&gt; &lt;td
      valign=&quot;top&quot; colspan=&quot;2&quot; width=&quot;187&quot; style=&quot;padding-bottom: 0cm; width: 140.4pt; border-left:
      solid black 1.0pt; border-right: none; border-top: none; height: 1.15pt; padding-top: 0cm;
      padding-right: 5.4pt; border-bottom: solid black 1.0pt; padding-left: 5.4pt&quot;&gt; &lt;p
      align=&quot;center&quot; class=&quot;msonormal&quot;&gt; VBN &lt;/p&gt; &lt;/td&gt; &lt;td
      valign=&quot;top&quot; width=&quot;374&quot; style=&quot;padding-left: 5.4pt; padding-top: 0cm; width: 280.25pt;
      border-top: none; border: solid black 1.0pt; height: 1.15pt; padding-right: 5.4pt;
      padding-bottom: 0cm&quot;&gt; &lt;p class=&quot;msonormal&quot;&gt; Verb, past participle
      &lt;/p&gt; &lt;/td&gt; &lt;/tr&gt; &lt;tr style=&quot;height:
      1.15pt&quot;&gt; &lt;td valign=&quot;top&quot; colspan=&quot;2&quot; width=&quot;187&quot; style=&quot;padding-bottom: 0cm;
      width: 140.4pt; border-left: solid black 1.0pt; border-right: none; border-top: none; height:
      1.15pt; padding-top: 0cm; padding-right: 5.4pt; border-bottom: solid black 1.0pt;
      padding-left: 5.4pt&quot;&gt; &lt;p align=&quot;center&quot; class=&quot;msonormal&quot;&gt; VBP
      &lt;/p&gt; &lt;/td&gt; &lt;td valign=&quot;top&quot; width=&quot;374&quot;
      style=&quot;padding-left: 5.4pt; padding-top: 0cm; width: 280.25pt; border-top: none; border: solid
      black 1.0pt; height: 1.15pt; padding-right: 5.4pt; padding-bottom: 0cm&quot;&gt; &lt;p
      class=&quot;msonormal&quot;&gt; Verb, present tense, other than third person singular
      &lt;/p&gt; &lt;/td&gt; &lt;/tr&gt; &lt;tr style=&quot;height:
      1.15pt&quot;&gt; &lt;td valign=&quot;top&quot; colspan=&quot;2&quot; width=&quot;187&quot; style=&quot;padding-bottom: 0cm;
      width: 140.4pt; border-left: solid black 1.0pt; border-right: none; border-top: none; height:
      1.15pt; padding-top: 0cm; padding-right: 5.4pt; border-bottom: solid black 1.0pt;
      padding-left: 5.4pt&quot;&gt; &lt;p align=&quot;center&quot; class=&quot;msonormal&quot;&gt; VBZ
      &lt;/p&gt; &lt;/td&gt; &lt;td valign=&quot;top&quot; width=&quot;374&quot;
      style=&quot;padding-left: 5.4pt; padding-top: 0cm; width: 280.25pt; border-top: none; border: solid
      black 1.0pt; height: 1.15pt; padding-right: 5.4pt; padding-bottom: 0cm&quot;&gt; &lt;p
      class=&quot;msonormal&quot;&gt; Verb, present tense, third person singular &lt;/p&gt;
      &lt;/td&gt; &lt;/tr&gt; &lt;tr style=&quot;height: 1.15pt&quot;&gt; &lt;td
      valign=&quot;top&quot; colspan=&quot;2&quot; width=&quot;187&quot; style=&quot;padding-bottom: 0cm; width: 140.4pt; border-left:
      solid black 1.0pt; border-right: none; border-top: none; height: 1.15pt; padding-top: 0cm;
      padding-right: 5.4pt; border-bottom: solid black 1.0pt; padding-left: 5.4pt&quot;&gt; &lt;p
      align=&quot;center&quot; class=&quot;msonormal&quot;&gt; WDT &lt;/p&gt; &lt;/td&gt; &lt;td
      valign=&quot;top&quot; width=&quot;374&quot; style=&quot;padding-left: 5.4pt; padding-top: 0cm; width: 280.25pt;
      border-top: none; border: solid black 1.0pt; height: 1.15pt; padding-right: 5.4pt;
      padding-bottom: 0cm&quot;&gt; &lt;p class=&quot;msonormal&quot;&gt; Wh-determiner
      &lt;/p&gt; &lt;/td&gt; &lt;/tr&gt; &lt;tr style=&quot;height:
      1.15pt&quot;&gt; &lt;td valign=&quot;top&quot; colspan=&quot;2&quot; width=&quot;187&quot; style=&quot;padding-bottom: 0cm;
      width: 140.4pt; border-left: solid black 1.0pt; border-right: none; border-top: none; height:
      1.15pt; padding-top: 0cm; padding-right: 5.4pt; border-bottom: solid black 1.0pt;
      padding-left: 5.4pt&quot;&gt; &lt;p align=&quot;center&quot; class=&quot;msonormal&quot;&gt; WP
      &lt;/p&gt; &lt;/td&gt; &lt;td valign=&quot;top&quot; width=&quot;374&quot;
      style=&quot;padding-left: 5.4pt; padding-top: 0cm; width: 280.25pt; border-top: none; border: solid
      black 1.0pt; height: 1.15pt; padding-right: 5.4pt; padding-bottom: 0cm&quot;&gt; &lt;p
      class=&quot;msonormal&quot;&gt; Wh-pronoun &lt;/p&gt; &lt;/td&gt;
      &lt;/tr&gt; &lt;tr style=&quot;height: 1.15pt&quot;&gt; &lt;td valign=&quot;top&quot;
      width=&quot;83&quot; style=&quot;padding-bottom: 0cm; width: 62.1pt; border-left: solid black 1.0pt;
      border-right: none; border-top: none; height: 1.15pt; padding-top: 0cm; padding-right: 5.4pt;
      border-bottom: solid black 1.0pt; padding-left: 5.4pt&quot;&gt; &lt;p align=&quot;center&quot;
      class=&quot;msonormal&quot;&gt; WP$ &lt;/p&gt; &lt;/td&gt; &lt;td valign=&quot;top&quot;
      width=&quot;104&quot; style=&quot;padding-bottom: 0cm; width: 78.3pt; border-left: solid black 1.0pt;
      border-right: none; border-top: none; height: 1.15pt; padding-top: 0cm; padding-right: 5.4pt;
      border-bottom: solid black 1.0pt; padding-left: 5.4pt&quot;&gt; &lt;p align=&quot;center&quot;
      class=&quot;msonormal&quot;&gt; WPP &lt;/p&gt; &lt;/td&gt; &lt;td valign=&quot;top&quot;
      width=&quot;374&quot; style=&quot;padding-left: 5.4pt; padding-top: 0cm; width: 280.25pt; border-top: none;
      border: solid black 1.0pt; height: 1.15pt; padding-right: 5.4pt; padding-bottom: 0cm&quot;&gt;
      &lt;p class=&quot;msonormal&quot;&gt; Wh-pronoun, possessive &lt;/p&gt;
      &lt;/td&gt; &lt;/tr&gt; &lt;tr style=&quot;height: 1.15pt&quot;&gt; &lt;td
      valign=&quot;top&quot; colspan=&quot;2&quot; width=&quot;187&quot; style=&quot;padding-bottom: 0cm; width: 140.4pt; border-left:
      solid black 1.0pt; border-right: none; border-top: none; height: 1.15pt; padding-top: 0cm;
      padding-right: 5.4pt; border-bottom: solid black 1.0pt; padding-left: 5.4pt&quot;&gt; &lt;p
      align=&quot;center&quot; class=&quot;msonormal&quot;&gt; WRB &lt;/p&gt; &lt;/td&gt; &lt;td
      valign=&quot;top&quot; width=&quot;374&quot; style=&quot;padding-left: 5.4pt; padding-top: 0cm; width: 280.25pt;
      border-top: none; border: solid black 1.0pt; height: 1.15pt; padding-right: 5.4pt;
      padding-bottom: 0cm&quot;&gt; &lt;p class=&quot;msonormal&quot;&gt; WH-adverb &lt;/p&gt;
      &lt;/td&gt; &lt;/tr&gt; &lt;/table&gt; &lt;p
      class=&quot;msonormal&quot;&gt; &lt;o p=&quot;#DEFAULT&quot;&gt; &amp;#160;&lt;/o&gt;
      &lt;/p&gt;</owl:versionInfo>
    </owl:Ontology>
    


    <!-- 
    ///////////////////////////////////////////////////////////////////////////////////////
    //
    // Annotation properties
    //
    ///////////////////////////////////////////////////////////////////////////////////////
     -->

    


    <!-- http://purl.org/dc/terms/license -->

    <owl:AnnotationProperty rdf:about="http://purl.org/dc/terms/license"/>
    


    <!-- http://w3id.org/meta-share/meta-share/language -->

    <owl:AnnotationProperty rdf:about="http://w3id.org/meta-share/meta-share/language"/>
    


    <!-- 
    ///////////////////////////////////////////////////////////////////////////////////////
    //
    // Data properties
    //
    ///////////////////////////////////////////////////////////////////////////////////////
     -->

    


    <!-- http://purl.org/olia/system.owl#hasTag -->

    <owl:DatatypeProperty rdf:about="http://purl.org/olia/system.owl#hasTag">
        <rdfs:domain rdf:resource="http://purl.org/olia/genia.owl#Tag"/>
    </owl:DatatypeProperty>
    


    <!-- http://purl.org/olia/system.owl#hasTier -->

    <owl:DatatypeProperty rdf:about="http://purl.org/olia/system.owl#hasTier"/>
    


    <!-- 
    ///////////////////////////////////////////////////////////////////////////////////////
    //
    // Classes
    //
    ///////////////////////////////////////////////////////////////////////////////////////
     -->

    


    <!-- http://purl.org/olia/genia.owl#Adjective -->

    <owl:Class rdf:about="http://purl.org/olia/genia.owl#Adjective">
        <rdfs:subClassOf rdf:resource="http://purl.org/olia/genia.owl#Tag"/>
        <rdfs:comment>These are adjectives,
      ordinal numerals, and ordinal numbers. Hyphenated compounds that are used as modifiers are
      tagged as adjectives, e.g. &quot;happy-go-lucky&quot;, &quot;one-of-a-kind&quot;, &quot;run-of-the-mill&quot;. Ordinal
      numbers are tagged as adjectives, as are compounds of the form &quot;n-th&quot; or &quot;X-est&quot;, like
      &quot;fourth-largest&quot;.</rdfs:comment>
    </owl:Class>
    


    <!-- http://purl.org/olia/genia.owl#Adverb -->

    <owl:Class rdf:about="http://purl.org/olia/genia.owl#Adverb">
        <rdfs:subClassOf rdf:resource="http://purl.org/olia/genia.owl#Tag"/>
        <rdfs:comment>This category includes most
      words that end in -ly as well as degree words like &quot;quite&quot;, &quot;too&quot; and &quot;very&quot;, posthead
      modifiers like &quot;enough&quot; and &quot;indeed&quot; (as in &quot;good enough&quot;, &quot;very well indeed&quot;), and negative
      markers like &quot;not&quot;, &quot;n&apos; t&quot; and &quot;never&quot;.</rdfs:comment>
    </owl:Class>
    


    <!-- http://purl.org/olia/genia.owl#BaseForm -->

    <owl:Class rdf:about="http://purl.org/olia/genia.owl#BaseForm">
        <rdfs:subClassOf rdf:resource="http://purl.org/olia/genia.owl#Verb"/>
        <rdfs:comment>This tag subsumes
      imperatives, infinitives and subjunctives. EXAMPLES: Imperative: Do/VB it. Infinitive: You
      should do/VB it. We want them to do/VB it. We made them do/VB it. Subjunctive: We suggested
      that he do/VB it.</rdfs:comment>
    </owl:Class>
    


    <!-- http://purl.org/olia/genia.owl#BePastTense -->

    <owl:Class rdf:about="http://purl.org/olia/genia.owl#BePastTense">
        <rdfs:subClassOf rdf:resource="http://purl.org/olia/genia.owl#Verb"/>
        <rdfs:comment>This category includes the
      conditional form of the verb to be. EXAMPLES: If I were/VBD rich... If I were/VBD to win the
      lottery...</rdfs:comment>
    </owl:Class>
    


    <!-- http://purl.org/olia/genia.owl#BePresentTense -->

    <owl:Class rdf:about="http://purl.org/olia/genia.owl#BePresentTense">
        <rdfs:subClassOf rdf:resource="http://purl.org/olia/genia.owl#Verb"/>
        <rdfs:comment>These are verbforms in
      present tense. This class includes 3rd person singular or other than 3rd person singular
      verbforms.</rdfs:comment>
    </owl:Class>
    


    <!-- http://purl.org/olia/genia.owl#CardinalNumber -->

    <owl:Class rdf:about="http://purl.org/olia/genia.owl#CardinalNumber">
        <rdfs:subClassOf rdf:resource="http://purl.org/olia/genia.owl#Tag"/>
        <rdfs:comment>These are cardinal
      numbers.</rdfs:comment>
    </owl:Class>
    


    <!-- http://purl.org/olia/genia.owl#CommonNoun -->

    <owl:Class rdf:about="http://purl.org/olia/genia.owl#CommonNoun">
        <rdfs:subClassOf rdf:resource="http://purl.org/olia/genia.owl#Noun"/>
        <rdfs:comment>These are common nouns in
      singular or plural, or mass nouns.</rdfs:comment>
    </owl:Class>
    


    <!-- http://purl.org/olia/genia.owl#ComparativeAdjective -->

    <owl:Class rdf:about="http://purl.org/olia/genia.owl#ComparativeAdjective">
        <rdfs:subClassOf rdf:resource="http://purl.org/olia/genia.owl#Adjective"/>
        <rdfs:comment>These are adjectives mostly
      with the comparative ending -er and a comparative meaning. &quot;More&quot; or &quot;less&quot; should be tagged
      as a comparative adjective when it is used without a head noun and it corresponds to the
      object of a verb or preposition.</rdfs:comment>
    </owl:Class>
    


    <!-- http://purl.org/olia/genia.owl#ComparativeAdverb -->

    <owl:Class rdf:about="http://purl.org/olia/genia.owl#ComparativeAdverb">
        <rdfs:subClassOf rdf:resource="http://purl.org/olia/genia.owl#Adverb"/>
        <rdfs:comment>These are comparative
      adverbs.</rdfs:comment>
    </owl:Class>
    


    <!-- http://purl.org/olia/genia.owl#Conjunction -->

    <owl:Class rdf:about="http://purl.org/olia/genia.owl#Conjunction">
        <rdfs:subClassOf rdf:resource="http://purl.org/olia/genia.owl#Tag"/>
        <rdfs:comment>This is a class, we
      inserted to structure the tagset.</rdfs:comment>
    </owl:Class>
    


    <!-- http://purl.org/olia/genia.owl#CoordinatingConjunction -->

    <owl:Class rdf:about="http://purl.org/olia/genia.owl#CoordinatingConjunction">
        <rdfs:subClassOf rdf:resource="http://purl.org/olia/genia.owl#Conjunction"/>
        <rdfs:comment>This category includes
      &quot;and&quot;, &quot;but&quot;, &quot;nor&quot;, &quot;or&quot;, &quot;yet&quot; (as in &quot;Yet it&apos;s cheap&quot;, &quot;cheap yet good&quot;), as well as the
      mathematical operators &quot;plus&quot;, &quot;minus&quot;, &quot;less&quot;, &quot;times&quot; (in the sense of &quot;multiplied by&quot;) and
      &quot;over&quot; (in the sense of &quot;divided by&quot;), when they are spelled out. For in the sense of
      &quot;because&quot; is a coordinating conjunction.</rdfs:comment>
    </owl:Class>
    


    <!-- http://purl.org/olia/genia.owl#Determiner -->

    <owl:Class rdf:about="http://purl.org/olia/genia.owl#Determiner">
        <rdfs:subClassOf rdf:resource="http://purl.org/olia/genia.owl#Tag"/>
        <rdfs:comment>This category includes the
      articles &quot;a(n)&quot;, &quot;every&quot;, &quot;no&quot; and &quot;the&quot;, the indefinite determiners &quot;another&quot;, &quot;any&quot; and
      &quot;some&quot;, &quot;each&quot;, &quot;either&quot; (as in &quot;either way&quot;), &quot;neither&quot; (as in &quot;neither decision&quot;), &quot;that&quot;,
      &quot;these&quot;, &quot;this&quot; and &quot;those&quot;, and instances of &quot;all&quot; and &quot;both&quot; when they do not precede a
      determiner or possessive pronoun (as in &quot;all roads&quot; or &quot;both times&quot;).</rdfs:comment>
    </owl:Class>
    


    <!-- http://purl.org/olia/genia.owl#ExistentialThere -->

    <owl:Class rdf:about="http://purl.org/olia/genia.owl#ExistentialThere">
        <rdfs:subClassOf rdf:resource="http://purl.org/olia/genia.owl#Tag"/>
        <rdfs:comment>Existential &quot;there&quot; is the
      unstressed &quot;there&quot; that triggers inversion of the inflected verb and the logical subject of a
      sentence, e.g. &quot;There/EX was a party in progress.&quot;, &quot;There/EX ensued a melee.&quot;.</rdfs:comment>
    </owl:Class>
    


    <!-- http://purl.org/olia/genia.owl#ForeignWord -->

    <owl:Class rdf:about="http://purl.org/olia/genia.owl#ForeignWord">
        <rdfs:subClassOf rdf:resource="http://purl.org/olia/genia.owl#Tag"/>
        <rdfs:comment>These are foreign
      words.</rdfs:comment>
    </owl:Class>
    


    <!-- http://purl.org/olia/genia.owl#GerundOrPresentParticiple -->

    <owl:Class rdf:about="http://purl.org/olia/genia.owl#GerundOrPresentParticiple">
        <rdfs:subClassOf rdf:resource="http://purl.org/olia/genia.owl#Verb"/>
        <rdfs:comment>This is a verb in present
      participle or in gerund.</rdfs:comment>
    </owl:Class>
    


    <!-- http://purl.org/olia/genia.owl#Interjection -->

    <owl:Class rdf:about="http://purl.org/olia/genia.owl#Interjection">
        <rdfs:subClassOf rdf:resource="http://purl.org/olia/genia.owl#Tag"/>
        <rdfs:comment>This PTB part of speech was
      excluded from GENIA.</rdfs:comment>
    </owl:Class>
    


    <!-- http://purl.org/olia/genia.owl#ListItemMarker -->

    <owl:Class rdf:about="http://purl.org/olia/genia.owl#ListItemMarker">
        <rdfs:subClassOf rdf:resource="http://purl.org/olia/genia.owl#Tag"/>
        <rdfs:comment>This category includes
      letters and numerals when they are used to identify items in a list.</rdfs:comment>
    </owl:Class>
    


    <!-- http://purl.org/olia/genia.owl#ModalVerb -->

    <owl:Class rdf:about="http://purl.org/olia/genia.owl#ModalVerb">
        <rdfs:subClassOf rdf:resource="http://purl.org/olia/genia.owl#Verb"/>
        <rdfs:comment>This category includes all
      verbs that don&apos;t take an -s ending in the third person singular present: &quot;can&quot;, &quot;could&quot;,
      (&quot;dare&quot;), &quot;may&quot;, &quot;might&quot;, &quot;must&quot;, &quot;ought&quot;, &quot;shall&quot;, &quot;should&quot;, &quot;will&quot;, &quot;would&quot;.</rdfs:comment>
    </owl:Class>
    


    <!-- http://purl.org/olia/genia.owl#Noun -->

    <owl:Class rdf:about="http://purl.org/olia/genia.owl#Noun">
        <rdfs:subClassOf rdf:resource="http://purl.org/olia/genia.owl#Tag"/>
        <rdfs:comment>This is a class, we
      inserted to structure the tagset.</rdfs:comment>
    </owl:Class>
    


    <!-- http://purl.org/olia/genia.owl#Particle -->

    <owl:Class rdf:about="http://purl.org/olia/genia.owl#Particle">
        <rdfs:subClassOf rdf:resource="http://purl.org/olia/genia.owl#Tag"/>
        <rdfs:comment>This category includes a
      number of mostly monosyllabic words that also double as directional adverbs and
      prepositions.</rdfs:comment>
    </owl:Class>
    


    <!-- http://purl.org/olia/genia.owl#PastParticiple -->

    <owl:Class rdf:about="http://purl.org/olia/genia.owl#PastParticiple">
        <rdfs:subClassOf rdf:resource="http://purl.org/olia/genia.owl#Verb"/>
        <rdfs:comment>This is a verb in past
      participle.</rdfs:comment>
    </owl:Class>
    


    <!-- http://purl.org/olia/genia.owl#PersonalPronoun -->

    <owl:Class rdf:about="http://purl.org/olia/genia.owl#PersonalPronoun">
        <rdfs:subClassOf rdf:resource="http://purl.org/olia/genia.owl#Pronoun"/>
        <rdfs:comment>This category includes the
      personal pronouns proper, without regard for case distinctions (&quot;I&quot;, &quot;me&quot;, &quot;you&quot;, &quot;he&quot;, &quot;him&quot;,
      etc.), the reflexive pronouns ending in -self or -selves, and the nominal possessive pronouns
      &quot;mine&quot;, &quot;yours&quot;, &quot;his&quot;, &quot;hers&quot;, &quot;ours&quot; and &quot;theirs&quot;.</rdfs:comment>
    </owl:Class>
    


    <!-- http://purl.org/olia/genia.owl#PossessiveMarker -->

    <owl:Class rdf:about="http://purl.org/olia/genia.owl#PossessiveMarker">
        <rdfs:subClassOf rdf:resource="http://purl.org/olia/genia.owl#Tag"/>
        <rdfs:comment>The possessive ending on
      nouns ending in &apos;s or is split off by the tagging algorithm and tagged as if it were a
      separate word. e.g. &quot;John/ NP &apos;s/POS idea&quot;, &quot;the parents/NNS&apos;/POS distress&quot;.</rdfs:comment>
    </owl:Class>
    


    <!-- http://purl.org/olia/genia.owl#PossessivePronoun -->

    <owl:Class rdf:about="http://purl.org/olia/genia.owl#PossessivePronoun">
        <rdfs:subClassOf rdf:resource="http://purl.org/olia/genia.owl#Pronoun"/>
        <rdfs:comment>This category includes the
      adjectival possessive forms &quot;my&quot;, &quot;your&quot;, &quot;his&quot;, &quot;her&quot;, &quot;its&quot;, &quot;one&apos;s&quot;, &quot;our&quot; and
      &quot;their&quot;.</rdfs:comment>
    </owl:Class>
    


    <!-- http://purl.org/olia/genia.owl#PossessiveWhPronoun -->

    <owl:Class rdf:about="http://purl.org/olia/genia.owl#PossessiveWhPronoun">
        <rdfs:subClassOf rdf:resource="http://purl.org/olia/genia.owl#Pronoun"/>
        <rdfs:comment>This category includes the
      wh-word &quot;whose&quot;.</rdfs:comment>
    </owl:Class>
    


    <!-- http://purl.org/olia/genia.owl#Predeterminer -->

    <owl:Class rdf:about="http://purl.org/olia/genia.owl#Predeterminer">
        <rdfs:subClassOf rdf:resource="http://purl.org/olia/genia.owl#Determiner"/>
        <rdfs:comment>This category includes the
      following determinerlike elements when they precede an article or possessive pronoun.
      EXAMPLES: all/PDT his marbles nary/PDT a soul both/PDT the girls quite/PDT a mess half/PDT his
      time rather/PDT a nuisance many/PDT a moon such/PDT a good time</rdfs:comment>
    </owl:Class>
    


    <!-- http://purl.org/olia/genia.owl#PrepositionOrSubordinatingConjunction -->

    <owl:Class rdf:about="http://purl.org/olia/genia.owl#PrepositionOrSubordinatingConjunction">
        <rdfs:subClassOf rdf:resource="http://purl.org/olia/genia.owl#Conjunction"/>
        <rdfs:comment>We make no explicit
      distinction between prepositions and subordinating conjunctions. (The distinction is not lost,
      however - a preposition is an IN that precedes a noun phrase or a prepositional phrase, and a
      subordinate conjunction is an IN that precedes a clause). The preposition &quot;to&quot; has its own
      special tag TO.</rdfs:comment>
    </owl:Class>
    


    <!-- http://purl.org/olia/genia.owl#Pronoun -->

    <owl:Class rdf:about="http://purl.org/olia/genia.owl#Pronoun">
        <rdfs:subClassOf rdf:resource="http://purl.org/olia/genia.owl#Tag"/>
        <rdfs:comment>This is a class, we
      inserted to structure the tagset.</rdfs:comment>
    </owl:Class>
    


    <!-- http://purl.org/olia/genia.owl#ProperNoun -->

    <owl:Class rdf:about="http://purl.org/olia/genia.owl#ProperNoun">
        <rdfs:subClassOf rdf:resource="http://purl.org/olia/genia.owl#Noun"/>
        <rdfs:comment>These are singular or
      plural proper nouns.</rdfs:comment>
    </owl:Class>
    


    <!-- http://purl.org/olia/genia.owl#Punctuation -->

    <owl:Class rdf:about="http://purl.org/olia/genia.owl#Punctuation">
        <rdfs:subClassOf rdf:resource="http://purl.org/olia/genia.owl#Tag"/>
        <rdfs:comment>Punctuation, in PTB tagged
      with :,&quot;()</rdfs:comment>
    </owl:Class>
    


    <!-- http://purl.org/olia/genia.owl#SuperlativeAdjective -->

    <owl:Class rdf:about="http://purl.org/olia/genia.owl#SuperlativeAdjective">
        <rdfs:subClassOf rdf:resource="http://purl.org/olia/genia.owl#Adjective"/>
        <rdfs:comment>These are adjectives with
      the superlative ending -est (as well as &quot;worst&quot;). &quot;Most&quot; and &quot;least&quot; can also be tagged as
      superlative adjective when they occur by themselves.</rdfs:comment>
    </owl:Class>
    


    <!-- http://purl.org/olia/genia.owl#SuperlativeAdverb -->

    <owl:Class rdf:about="http://purl.org/olia/genia.owl#SuperlativeAdverb">
        <rdfs:subClassOf rdf:resource="http://purl.org/olia/genia.owl#Adverb"/>
        <rdfs:comment>These are superlative
      adverbs.</rdfs:comment>
    </owl:Class>
    


    <!-- http://purl.org/olia/genia.owl#Symbol -->

    <owl:Class rdf:about="http://purl.org/olia/genia.owl#Symbol">
        <rdfs:subClassOf rdf:resource="http://purl.org/olia/genia.owl#Tag"/>
        <rdfs:comment>This tag should be used for
      mathematical, scientific and technical symbols or expressions that aren&apos;t words of English. It
      should not used for any and all technical expressions. For instance, the names of chemicals,
      units of measurements (including abbreviations thereof) and the like should be tagged as
      nouns.</rdfs:comment>
    </owl:Class>
    


    <!-- http://purl.org/olia/genia.owl#Tag -->

    <owl:Class rdf:about="http://purl.org/olia/genia.owl#Tag">
        <rdfs:subClassOf rdf:resource="http://purl.org/olia/system.owl#UnitOfAnnotation"/>
        <rdfs:subClassOf>
            <owl:Restriction>
                <owl:onProperty rdf:resource="http://purl.org/olia/system.owl#hasTier"/>
                <owl:hasValue>POS</owl:hasValue>
            </owl:Restriction>
        </rdfs:subClassOf>
    </owl:Class>
    


    <!-- http://purl.org/olia/genia.owl#To -->

    <owl:Class rdf:about="http://purl.org/olia/genia.owl#To">
        <rdfs:subClassOf rdf:resource="http://purl.org/olia/genia.owl#Tag"/>
        <rdfs:comment>&quot;To&quot; is tagged TO,
      regardless of whether it is a preposition or an infinitival marker.</rdfs:comment>
    </owl:Class>
    


    <!-- http://purl.org/olia/genia.owl#Verb -->

    <owl:Class rdf:about="http://purl.org/olia/genia.owl#Verb">
        <rdfs:subClassOf rdf:resource="http://purl.org/olia/genia.owl#Tag"/>
    </owl:Class>
    


    <!-- http://purl.org/olia/genia.owl#WhAdverb -->

    <owl:Class rdf:about="http://purl.org/olia/genia.owl#WhAdverb">
        <rdfs:subClassOf rdf:resource="http://purl.org/olia/genia.owl#Adverb"/>
        <rdfs:comment>This category includes
      &quot;how&quot;, &quot;where&quot;, &quot;why&quot;, etc. When in a temporal sense is tagged as wh-adverb. In the sense of
      &quot;if&quot;, on the other hand, it is a subordinating conjunction. EXAMPLES: &quot;When/WRB he finally
      arrived, I was on my way out.&quot;</rdfs:comment>
    </owl:Class>
    


    <!-- http://purl.org/olia/genia.owl#WhDeterminer -->

    <owl:Class rdf:about="http://purl.org/olia/genia.owl#WhDeterminer">
        <rdfs:subClassOf rdf:resource="http://purl.org/olia/genia.owl#Determiner"/>
        <rdfs:comment>This category includes
      &quot;which&quot;, as well as that when it is used as a relative pronoun.</rdfs:comment>
    </owl:Class>
    


    <!-- http://purl.org/olia/genia.owl#WhPronoun -->

    <owl:Class rdf:about="http://purl.org/olia/genia.owl#WhPronoun">
        <rdfs:subClassOf rdf:resource="http://purl.org/olia/genia.owl#Pronoun"/>
        <rdfs:comment>This category includes
      &quot;what&quot;, &quot;who&quot; and &quot;whom&quot;.</rdfs:comment>
    </owl:Class>
    


    <!-- http://purl.org/olia/system.owl#UnitOfAnnotation -->

    <owl:Class rdf:about="http://purl.org/olia/system.owl#UnitOfAnnotation"/>
    


    <!-- 
    ///////////////////////////////////////////////////////////////////////////////////////
    //
    // Individuals
    //
    ///////////////////////////////////////////////////////////////////////////////////////
     -->

    


    <!-- http://purl.org/olia/genia.owl#CC -->

    <owl:NamedIndividual rdf:about="http://purl.org/olia/genia.owl#CC">
        <rdf:type rdf:resource="http://purl.org/olia/genia.owl#CoordinatingConjunction"/>
        <olia_system:hasTag>CC</olia_system:hasTag>
    </owl:NamedIndividual>
    


    <!-- http://purl.org/olia/genia.owl#CD -->

    <owl:NamedIndividual rdf:about="http://purl.org/olia/genia.owl#CD">
        <rdf:type rdf:resource="http://purl.org/olia/genia.owl#CardinalNumber"/>
        <olia_system:hasTag>CD</olia_system:hasTag>
        <rdfs:comment>cardinal
      number</rdfs:comment>
    </owl:NamedIndividual>
    


    <!-- http://purl.org/olia/genia.owl#COLON -->

    <owl:NamedIndividual rdf:about="http://purl.org/olia/genia.owl#COLON">
        <rdf:type rdf:resource="http://purl.org/olia/genia.owl#Punctuation"/>
        <olia_system:hasTag>COLON</olia_system:hasTag>
        <rdfs:comment>colon, _:_</rdfs:comment>
    </owl:NamedIndividual>
    


    <!-- http://purl.org/olia/genia.owl#COMMA -->

    <owl:NamedIndividual rdf:about="http://purl.org/olia/genia.owl#COMMA">
        <rdf:type rdf:resource="http://purl.org/olia/genia.owl#Punctuation"/>
        <olia_system:hasTag>COMMA</olia_system:hasTag>
        <rdfs:comment>comma, _,_</rdfs:comment>
    </owl:NamedIndividual>
    


    <!-- http://purl.org/olia/genia.owl#DT -->

    <owl:NamedIndividual rdf:about="http://purl.org/olia/genia.owl#DT">
        <rdf:type rdf:resource="http://purl.org/olia/genia.owl#Determiner"/>
        <olia_system:hasTag>DT</olia_system:hasTag>
        <rdfs:comment>determiner, also
      article</rdfs:comment>
    </owl:NamedIndividual>
    


    <!-- http://purl.org/olia/genia.owl#EX -->

    <owl:NamedIndividual rdf:about="http://purl.org/olia/genia.owl#EX">
        <rdf:type rdf:resource="http://purl.org/olia/genia.owl#ExistentialThere"/>
        <olia_system:hasTag>EX</olia_system:hasTag>
    </owl:NamedIndividual>
    


    <!-- http://purl.org/olia/genia.owl#FW -->

    <owl:NamedIndividual rdf:about="http://purl.org/olia/genia.owl#FW">
        <rdf:type rdf:resource="http://purl.org/olia/genia.owl#ForeignWord"/>
        <olia_system:hasTag>FW</olia_system:hasTag>
    </owl:NamedIndividual>
    


    <!-- http://purl.org/olia/genia.owl#IN -->

    <owl:NamedIndividual rdf:about="http://purl.org/olia/genia.owl#IN">
        <rdf:type rdf:resource="http://purl.org/olia/genia.owl#PrepositionOrSubordinatingConjunction"/>
        <olia_system:hasTag>IN</olia_system:hasTag>
    </owl:NamedIndividual>
    


    <!-- http://purl.org/olia/genia.owl#JJ -->

    <owl:NamedIndividual rdf:about="http://purl.org/olia/genia.owl#JJ">
        <rdf:type rdf:resource="http://purl.org/olia/genia.owl#Adjective"/>
        <olia_system:hasTag>JJ</olia_system:hasTag>
        <rdfs:comment>adjective, ordinal numeral,
      ordinal number</rdfs:comment>
    </owl:NamedIndividual>
    


    <!-- http://purl.org/olia/genia.owl#JJR -->

    <owl:NamedIndividual rdf:about="http://purl.org/olia/genia.owl#JJR">
        <rdf:type rdf:resource="http://purl.org/olia/genia.owl#ComparativeAdjective"/>
        <olia_system:hasTag>JJR</olia_system:hasTag>
        <rdfs:comment>comparative
      adjective</rdfs:comment>
    </owl:NamedIndividual>
    


    <!-- http://purl.org/olia/genia.owl#JJS -->

    <owl:NamedIndividual rdf:about="http://purl.org/olia/genia.owl#JJS">
        <rdf:type rdf:resource="http://purl.org/olia/genia.owl#SuperlativeAdjective"/>
        <olia_system:hasTag>JJS</olia_system:hasTag>
        <rdfs:comment>superlative
      adjective</rdfs:comment>
    </owl:NamedIndividual>
    


    <!-- http://purl.org/olia/genia.owl#LQT -->

    <owl:NamedIndividual rdf:about="http://purl.org/olia/genia.owl#LQT">
        <rdf:type rdf:resource="http://purl.org/olia/genia.owl#Punctuation"/>
        <olia_system:hasTag>LQT</olia_system:hasTag>
        <rdfs:comment>left quotation mark,
      _&quot;_</rdfs:comment>
    </owl:NamedIndividual>
    


    <!-- http://purl.org/olia/genia.owl#LRB -->

    <owl:NamedIndividual rdf:about="http://purl.org/olia/genia.owl#LRB">
        <rdf:type rdf:resource="http://purl.org/olia/genia.owl#Punctuation"/>
        <olia_system:hasTag>LRB</olia_system:hasTag>
        <rdfs:comment>left round bracket,
      _(_</rdfs:comment>
    </owl:NamedIndividual>
    


    <!-- http://purl.org/olia/genia.owl#LS -->

    <owl:NamedIndividual rdf:about="http://purl.org/olia/genia.owl#LS">
        <rdf:type rdf:resource="http://purl.org/olia/genia.owl#ListItemMarker"/>
        <olia_system:hasTag>LS</olia_system:hasTag>
    </owl:NamedIndividual>
    


    <!-- http://purl.org/olia/genia.owl#MD -->

    <owl:NamedIndividual rdf:about="http://purl.org/olia/genia.owl#MD">
        <rdf:type rdf:resource="http://purl.org/olia/genia.owl#ModalVerb"/>
        <olia_system:hasTag>MD</olia_system:hasTag>
    </owl:NamedIndividual>
    


    <!-- http://purl.org/olia/genia.owl#NN -->

    <owl:NamedIndividual rdf:about="http://purl.org/olia/genia.owl#NN">
        <rdf:type rdf:resource="http://purl.org/olia/genia.owl#CommonNoun"/>
        <olia_system:hasTag>NN</olia_system:hasTag>
        <rdfs:comment>Noun singular or
      mass</rdfs:comment>
    </owl:NamedIndividual>
    


    <!-- http://purl.org/olia/genia.owl#NNP -->

    <owl:NamedIndividual rdf:about="http://purl.org/olia/genia.owl#NNP">
        <rdf:type rdf:resource="http://purl.org/olia/genia.owl#ProperNoun"/>
        <olia_system:hasTag>NNP</olia_system:hasTag>
        <rdfs:comment>Proper noun
      singular</rdfs:comment>
    </owl:NamedIndividual>
    


    <!-- http://purl.org/olia/genia.owl#NNPS -->

    <owl:NamedIndividual rdf:about="http://purl.org/olia/genia.owl#NNPS">
        <rdf:type rdf:resource="http://purl.org/olia/genia.owl#ProperNoun"/>
        <olia_system:hasTag>NNPS</olia_system:hasTag>
        <rdfs:comment>Proper noun
      plural</rdfs:comment>
    </owl:NamedIndividual>
    


    <!-- http://purl.org/olia/genia.owl#NNS -->

    <owl:NamedIndividual rdf:about="http://purl.org/olia/genia.owl#NNS">
        <rdf:type rdf:resource="http://purl.org/olia/genia.owl#CommonNoun"/>
        <olia_system:hasTag>NNS</olia_system:hasTag>
        <rdfs:comment>Noun plural</rdfs:comment>
    </owl:NamedIndividual>
    


    <!-- http://purl.org/olia/genia.owl#PDT -->

    <owl:NamedIndividual rdf:about="http://purl.org/olia/genia.owl#PDT">
        <rdf:type rdf:resource="http://purl.org/olia/genia.owl#Predeterminer"/>
        <olia_system:hasTag>PDT</olia_system:hasTag>
    </owl:NamedIndividual>
    


    <!-- http://purl.org/olia/genia.owl#PERIOD -->

    <owl:NamedIndividual rdf:about="http://purl.org/olia/genia.owl#PERIOD">
        <rdf:type rdf:resource="http://purl.org/olia/genia.owl#Punctuation"/>
        <olia_system:hasTag>PERIOD</olia_system:hasTag>
        <rdfs:comment>period, _._</rdfs:comment>
    </owl:NamedIndividual>
    


    <!-- http://purl.org/olia/genia.owl#POS -->

    <owl:NamedIndividual rdf:about="http://purl.org/olia/genia.owl#POS">
        <rdf:type rdf:resource="http://purl.org/olia/genia.owl#PossessiveMarker"/>
        <olia_system:hasTag>POS</olia_system:hasTag>
        <rdfs:comment>possessive &apos;s and
      &apos;</rdfs:comment>
    </owl:NamedIndividual>
    


    <!-- http://purl.org/olia/genia.owl#PRP -->

    <owl:NamedIndividual rdf:about="http://purl.org/olia/genia.owl#PRP">
        <rdf:type rdf:resource="http://purl.org/olia/genia.owl#PersonalPronoun"/>
        <olia_system:hasTag>PRP</olia_system:hasTag>
        <rdfs:comment>personal
      pronoun</rdfs:comment>
    </owl:NamedIndividual>
    


    <!-- http://purl.org/olia/genia.owl#PRPpossessive -->

    <owl:NamedIndividual rdf:about="http://purl.org/olia/genia.owl#PRPpossessive">
        <rdf:type rdf:resource="http://purl.org/olia/genia.owl#PossessivePronoun"/>
        <olia_system:hasTag>PRP$</olia_system:hasTag>
        <rdfs:comment>personal pronoun,
      possessive</rdfs:comment>
    </owl:NamedIndividual>
    


    <!-- http://purl.org/olia/genia.owl#RB -->

    <owl:NamedIndividual rdf:about="http://purl.org/olia/genia.owl#RB">
        <rdf:type rdf:resource="http://purl.org/olia/genia.owl#Adverb"/>
        <olia_system:hasTag>RB</olia_system:hasTag>
        <rdfs:comment>adverb (in PTB also
      negation)</rdfs:comment>
    </owl:NamedIndividual>
    


    <!-- http://purl.org/olia/genia.owl#RBR -->

    <owl:NamedIndividual rdf:about="http://purl.org/olia/genia.owl#RBR">
        <rdf:type rdf:resource="http://purl.org/olia/genia.owl#ComparativeAdverb"/>
        <olia_system:hasTag>RBR</olia_system:hasTag>
        <rdfs:comment>adverb,
      comparative</rdfs:comment>
    </owl:NamedIndividual>
    


    <!-- http://purl.org/olia/genia.owl#RBS -->

    <owl:NamedIndividual rdf:about="http://purl.org/olia/genia.owl#RBS">
        <rdf:type rdf:resource="http://purl.org/olia/genia.owl#SuperlativeAdverb"/>
        <olia_system:hasTag>RBS</olia_system:hasTag>
        <rdfs:comment>adverb,
      superlative</rdfs:comment>
    </owl:NamedIndividual>
    


    <!-- http://purl.org/olia/genia.owl#RP -->

    <owl:NamedIndividual rdf:about="http://purl.org/olia/genia.owl#RP">
        <rdf:type rdf:resource="http://purl.org/olia/genia.owl#Particle"/>
        <olia_system:hasTag>RP</olia_system:hasTag>
        <rdfs:comment>particle</rdfs:comment>
    </owl:NamedIndividual>
    


    <!-- http://purl.org/olia/genia.owl#RQT -->

    <owl:NamedIndividual rdf:about="http://purl.org/olia/genia.owl#RQT">
        <rdf:type rdf:resource="http://purl.org/olia/genia.owl#Punctuation"/>
        <olia_system:hasTag>RQT</olia_system:hasTag>
        <rdfs:comment>right quotation mark,
      _&quot;_</rdfs:comment>
    </owl:NamedIndividual>
    


    <!-- http://purl.org/olia/genia.owl#RRB -->

    <owl:NamedIndividual rdf:about="http://purl.org/olia/genia.owl#RRB">
        <rdf:type rdf:resource="http://purl.org/olia/genia.owl#Punctuation"/>
        <olia_system:hasTag>RRB</olia_system:hasTag>
        <rdfs:comment>right round bracket,
      _)_</rdfs:comment>
    </owl:NamedIndividual>
    


    <!-- http://purl.org/olia/genia.owl#SYM -->

    <owl:NamedIndividual rdf:about="http://purl.org/olia/genia.owl#SYM">
        <rdf:type rdf:resource="http://purl.org/olia/genia.owl#Symbol"/>
        <olia_system:hasTag>SYM</olia_system:hasTag>
    </owl:NamedIndividual>
    


    <!-- http://purl.org/olia/genia.owl#TO -->

    <owl:NamedIndividual rdf:about="http://purl.org/olia/genia.owl#TO">
        <rdf:type rdf:resource="http://purl.org/olia/genia.owl#To"/>
        <olia_system:hasTag>TO</olia_system:hasTag>
        <rdfs:comment>to</rdfs:comment>
    </owl:NamedIndividual>
    


    <!-- http://purl.org/olia/genia.owl#VB -->

    <owl:NamedIndividual rdf:about="http://purl.org/olia/genia.owl#VB">
        <rdf:type rdf:resource="http://purl.org/olia/genia.owl#BaseForm"/>
        <olia_system:hasTag>VB</olia_system:hasTag>
    </owl:NamedIndividual>
    


    <!-- http://purl.org/olia/genia.owl#VBD -->

    <owl:NamedIndividual rdf:about="http://purl.org/olia/genia.owl#VBD">
        <rdf:type rdf:resource="http://purl.org/olia/genia.owl#BePastTense"/>
        <olia_system:hasTag>VBD</olia_system:hasTag>
    </owl:NamedIndividual>
    


    <!-- http://purl.org/olia/genia.owl#VBG -->

    <owl:NamedIndividual rdf:about="http://purl.org/olia/genia.owl#VBG">
        <rdf:type rdf:resource="http://purl.org/olia/genia.owl#GerundOrPresentParticiple"/>
        <olia_system:hasTag>VBG</olia_system:hasTag>
    </owl:NamedIndividual>
    


    <!-- http://purl.org/olia/genia.owl#VBN -->

    <owl:NamedIndividual rdf:about="http://purl.org/olia/genia.owl#VBN">
        <rdf:type rdf:resource="http://purl.org/olia/genia.owl#PastParticiple"/>
        <olia_system:hasTag>VBN</olia_system:hasTag>
    </owl:NamedIndividual>
    


    <!-- http://purl.org/olia/genia.owl#VBP -->

    <owl:NamedIndividual rdf:about="http://purl.org/olia/genia.owl#VBP">
        <rdf:type rdf:resource="http://purl.org/olia/genia.owl#BePresentTense"/>
        <olia_system:hasTag>VBP</olia_system:hasTag>
        <rdfs:comment>Verb non 3-rd person
      singular present</rdfs:comment>
    </owl:NamedIndividual>
    


    <!-- http://purl.org/olia/genia.owl#VBZ -->

    <owl:NamedIndividual rdf:about="http://purl.org/olia/genia.owl#VBZ">
        <rdf:type rdf:resource="http://purl.org/olia/genia.owl#BePresentTense"/>
        <olia_system:hasTag>VBZ</olia_system:hasTag>
        <rdfs:comment>Verb 3-rd person singular
      present</rdfs:comment>
    </owl:NamedIndividual>
    


    <!-- http://purl.org/olia/genia.owl#WDT -->

    <owl:NamedIndividual rdf:about="http://purl.org/olia/genia.owl#WDT">
        <rdf:type rdf:resource="http://purl.org/olia/genia.owl#WhDeterminer"/>
        <olia_system:hasTag>WDT</olia_system:hasTag>
    </owl:NamedIndividual>
    


    <!-- http://purl.org/olia/genia.owl#WP -->

    <owl:NamedIndividual rdf:about="http://purl.org/olia/genia.owl#WP">
        <rdf:type rdf:resource="http://purl.org/olia/genia.owl#WhPronoun"/>
        <olia_system:hasTag>WP</olia_system:hasTag>
    </owl:NamedIndividual>
    


    <!-- http://purl.org/olia/genia.owl#WPpossessive -->

    <owl:NamedIndividual rdf:about="http://purl.org/olia/genia.owl#WPpossessive">
        <rdf:type rdf:resource="http://purl.org/olia/genia.owl#PossessiveWhPronoun"/>
        <olia_system:hasTag>WP$</olia_system:hasTag>
    </owl:NamedIndividual>
    


    <!-- http://purl.org/olia/genia.owl#WRB -->

    <owl:NamedIndividual rdf:about="http://purl.org/olia/genia.owl#WRB">
        <rdf:type rdf:resource="http://purl.org/olia/genia.owl#WhAdverb"/>
        <olia_system:hasTag>WRB</olia_system:hasTag>
        <rdfs:comment>WH-adverb</rdfs:comment>
    </owl:NamedIndividual>
</rdf:RDF>



<!-- Generated by the OWL API (version 4.5.25.2023-02-15T19:15:49Z) https://github.com/owlcs/owlapi -->

