<?xml version="1.0"?>
<rdf:RDF xmlns="http://purl.org/olia/mte/multext-east.owl#"
     xml:base="http://purl.org/olia/mte/multext-east.owl"
     xmlns:ms="http://w3id.org/meta-share/meta-share/"
     xmlns:dct="http://purl.org/dc/terms/"
     xmlns:owl="http://www.w3.org/2002/07/owl#"
     xmlns:rdf="http://www.w3.org/1999/02/22-rdf-syntax-ns#"
     xmlns:xml="http://www.w3.org/XML/1998/namespace"
     xmlns:xsd="http://www.w3.org/2001/XMLSchema#"
     xmlns:rdfs="http://www.w3.org/2000/01/rdf-schema#">
    <owl:Ontology rdf:about="http://purl.org/olia/mte/multext-east.owl">
        <dct:license rdf:resource="https://creativecommons.org/licenses/by/3.0/"/>
        <ms:language rdf:resource="http://lexvo.org/id/iso639-3/bul"/>
        <ms:language rdf:resource="http://lexvo.org/id/iso639-3/ces"/>
        <ms:language rdf:resource="http://lexvo.org/id/iso639-3/eng"/>
        <ms:language rdf:resource="http://lexvo.org/id/iso639-3/est"/>
        <ms:language rdf:resource="http://lexvo.org/id/iso639-3/fas"/>
        <ms:language rdf:resource="http://lexvo.org/id/iso639-3/hun"/>
        <ms:language rdf:resource="http://lexvo.org/id/iso639-3/mkd"/>
        <ms:language rdf:resource="http://lexvo.org/id/iso639-3/pol"/>
        <ms:language rdf:resource="http://lexvo.org/id/iso639-3/ron"/>
        <ms:language rdf:resource="http://lexvo.org/id/iso639-3/rus"/>
        <ms:language rdf:resource="http://lexvo.org/id/iso639-3/slk"/>
        <ms:language rdf:resource="http://lexvo.org/id/iso639-3/slv"/>
        <ms:language rdf:resource="http://lexvo.org/id/iso639-3/srp"/>
        <ms:language rdf:resource="http://lexvo.org/id/iso639-3/ukr"/>
        <rdfs:comment>OWL/DL Ontology for MULTEXT-East morphosyntactic specifications -- OLiA annotation model for the morphosyntactic specifications of MULTEXT-East v. 4. (Erjavec 2010)&lt;br/&gt;

http://nl.ijs.si/ME/owl/&lt;br/&gt;
Christian Chiarcos, 2010-2011&lt;br/&gt;&lt;br/&gt;

Licence:&lt;br/&gt;
The ontologies are distributed under the Creative Commons Attribution 3.0 Unported (CC BY 3.0) licence. You are free to to copy, distribute and transmit the work, to adapt the work and to make commercial use of the work under the condition that you make a reference to:&lt;br/&gt;

Christian Chiarcos and Tomaz Erjavec (2011), OWL/DL formalization of the MULTEXT-East morphosyntactic specifications. In: Proceedings of the 5th Linguistic Annotation Workshop (LAW-V), held in conjunction with the ACL-HLT 2011, June 2011, Portland, Oregon, USA, p. 11--20. &lt;br/&gt;

Please note that these ontologies are still under development, and that more detailed and precise definitions will be added incrementally.&lt;br/&gt;&lt;br/&gt;

Sources: &lt;br/&gt;
Unless marked otherwise, all comments refer to Erjavec (2010).
Additionally, Qasemizadeh &amp; Rahimi (2006), Dimitrova et al. (2009) and Derzhanski &amp; Kotsyba (2009) were consulted for clarification. Email communication with Tomaž Erjavec, Serge Sharoff, Dan Tufis, Ivan A. Derzhanski, Natalia Kosyba, Csaba Oravecz and Hamidreza Kobdani represents the third source of information consulted for this ontology.&lt;br/&gt;

References:&lt;br/&gt;

Ivan Derzhanski, Natalia Kotsyba (2009), Towards a Consistent Morphological Tagset for Slavic Languages: Extending MULTEXT-East for Polish, Ukrainian and Belarusian, In: Proc. MONDILEX Third Open Workshop
Bratislava, Slovakia, 15–16 April, 2009, p. 9-26&lt;br/&gt;

Ludmila Dimitrova, Radovan Garabík, Daniela Majchráková (2009), Comparing Bulgarian and Slovak Multext-East morphology tagset, In: Proceedings of MONDILEX Second Open Workshop, Kyiv, Ukraine, 2–4 February, 2009, p. 38-46&lt;br/&gt;

Tomaž Erjavec (ed., 2010),  MULTEXT-East Morphosyntactic Specifications Version 4. 2010-05-12, http://nl.ijs.si/ME/V4/msd/html/index.html&lt;br/&gt;

Behrang Qasemizadeh and Saeed Rahimi (2006), Persian in MULTEXT-East Framework, in T. Salakoski et al. (eds.): FinTAL 2006, LNAI 4139, pp. 541 – 551, 2006.</rdfs:comment>
        <owl:versionInfo>
2010/05/30 created &lt;br/&gt;
2010/06/10-2010/06/25 discussion on the mocky mailing list and corresponding updates&lt;br/&gt;
2010/07/22 removed deprecated classes and properties&lt;br/&gt;
2010/07/29 added examples (using enrich-mte-owl-with-examples.sh)&lt;br/&gt;
2010/10/13-2010/10/18 consolidation of definitions&lt;br/&gt;
2010/10/18 Wh_Type merged with InterrogativeOrRelativeAdverb, InterrogativeOrRelativePronoun, InterrogativeOrRelativeDeterminer&lt;br/&gt;
2011/06/01 initial release&lt;br/&gt;
2011/07/15  mte urls replaced by purls, ISO 693-3 language codes added to language-specific specifications, licence statement (see XML),
	    inconsistencies between mtecore and language-specific owls resolved, hasWHType reestablished&lt;br/&gt;
2011/08/03 revised definition of DistributiveCase, MultiplicativeCase, SpecifierAdverb
2011/08/04 revised treatment of OrdinalAdjective (conflates &quot;relational adjective&quot; for Slovene, Ukrainian and Czech and &quot;ordinal numeral&quot; for Macedonian):
    OrdinalAdjective sub AmbiguousAdjective and (RelationalAdjective or (Adjective and OrdinalNumeral)) 
&lt;br/&gt;

Christian Chiarcos, chiarcos@uni-potsdam.de</owl:versionInfo>
    </owl:Ontology>
    


    <!-- 
    ///////////////////////////////////////////////////////////////////////////////////////
    //
    // Annotation properties
    //
    ///////////////////////////////////////////////////////////////////////////////////////
     -->

    


    <!-- http://purl.org/dc/terms/license -->

    <owl:AnnotationProperty rdf:about="http://purl.org/dc/terms/license"/>
    


    <!-- http://w3id.org/meta-share/meta-share/language -->

    <owl:AnnotationProperty rdf:about="http://w3id.org/meta-share/meta-share/language"/>
    


    <!-- http://www.w3.org/2000/01/rdf-schema#comment -->

    <owl:AnnotationProperty rdf:about="http://www.w3.org/2000/01/rdf-schema#comment"/>
    


    <!-- http://www.w3.org/2002/07/owl#deprecated -->

    <owl:AnnotationProperty rdf:about="http://www.w3.org/2002/07/owl#deprecated"/>
    


    <!-- http://www.w3.org/2002/07/owl#versionInfo -->

    <owl:AnnotationProperty rdf:about="http://www.w3.org/2002/07/owl#versionInfo"/>
    


    <!-- 
    ///////////////////////////////////////////////////////////////////////////////////////
    //
    // Object Properties
    //
    ///////////////////////////////////////////////////////////////////////////////////////
     -->

    


    <!-- http://purl.org/olia/mte/multext-east.owl#hasAdjectiveFormation -->

    <owl:ObjectProperty rdf:about="http://purl.org/olia/mte/multext-east.owl#hasAdjectiveFormation">
        <rdfs:subPropertyOf rdf:resource="http://purl.org/olia/mte/multext-east.owl#hasFormation"/>
        <rdfs:domain rdf:resource="http://purl.org/olia/mte/multext-east.owl#Adjective"/>
        <rdfs:range rdf:resource="http://purl.org/olia/mte/multext-east.owl#AdjectiveFormation"/>
    </owl:ObjectProperty>
    


    <!-- http://purl.org/olia/mte/multext-east.owl#hasAdpositionFormation -->

    <owl:ObjectProperty rdf:about="http://purl.org/olia/mte/multext-east.owl#hasAdpositionFormation">
        <rdfs:subPropertyOf rdf:resource="http://purl.org/olia/mte/multext-east.owl#hasFormation"/>
        <rdfs:domain rdf:resource="http://purl.org/olia/mte/multext-east.owl#Adposition"/>
        <rdfs:range rdf:resource="http://purl.org/olia/mte/multext-east.owl#AdpositionFormation"/>
    </owl:ObjectProperty>
    


    <!-- http://purl.org/olia/mte/multext-east.owl#hasAnimacy -->

    <owl:ObjectProperty rdf:about="http://purl.org/olia/mte/multext-east.owl#hasAnimacy">
        <rdfs:subPropertyOf rdf:resource="http://purl.org/olia/mte/multext-east.owl#hasFeature"/>
        <rdfs:domain>
            <owl:Class>
                <owl:unionOf rdf:parseType="Collection">
                    <rdf:Description rdf:about="http://purl.org/olia/mte/multext-east.owl#Adjective"/>
                    <rdf:Description rdf:about="http://purl.org/olia/mte/multext-east.owl#Article"/>
                    <rdf:Description rdf:about="http://purl.org/olia/mte/multext-east.owl#Noun"/>
                    <rdf:Description rdf:about="http://purl.org/olia/mte/multext-east.owl#Numeral"/>
                    <rdf:Description rdf:about="http://purl.org/olia/mte/multext-east.owl#Pronoun"/>
                    <rdf:Description rdf:about="http://purl.org/olia/mte/multext-east.owl#Verb"/>
                </owl:unionOf>
            </owl:Class>
        </rdfs:domain>
        <rdfs:range rdf:resource="http://purl.org/olia/mte/multext-east.owl#Animacy"/>
    </owl:ObjectProperty>
    


    <!-- http://purl.org/olia/mte/multext-east.owl#hasAspect -->

    <owl:ObjectProperty rdf:about="http://purl.org/olia/mte/multext-east.owl#hasAspect">
        <rdfs:subPropertyOf rdf:resource="http://purl.org/olia/mte/multext-east.owl#hasFeature"/>
        <rdfs:domain>
            <owl:Class>
                <owl:unionOf rdf:parseType="Collection">
                    <rdf:Description rdf:about="http://purl.org/olia/mte/multext-east.owl#Adjective"/>
                    <rdf:Description rdf:about="http://purl.org/olia/mte/multext-east.owl#Noun"/>
                    <rdf:Description rdf:about="http://purl.org/olia/mte/multext-east.owl#Verb"/>
                </owl:unionOf>
            </owl:Class>
        </rdfs:domain>
        <rdfs:range rdf:resource="http://purl.org/olia/mte/multext-east.owl#Aspect"/>
        <rdfs:comment>also applicable to Polish nouns, and Polish and Ukrainian adjectives</rdfs:comment>
    </owl:ObjectProperty>
    


    <!-- http://purl.org/olia/mte/multext-east.owl#hasCase -->

    <owl:ObjectProperty rdf:about="http://purl.org/olia/mte/multext-east.owl#hasCase">
        <rdfs:subPropertyOf rdf:resource="http://purl.org/olia/mte/multext-east.owl#hasFeature"/>
        <rdfs:domain>
            <owl:Class>
                <owl:unionOf rdf:parseType="Collection">
                    <rdf:Description rdf:about="http://purl.org/olia/mte/multext-east.owl#Abbreviation"/>
                    <rdf:Description rdf:about="http://purl.org/olia/mte/multext-east.owl#Adjective"/>
                    <rdf:Description rdf:about="http://purl.org/olia/mte/multext-east.owl#Adposition"/>
                    <rdf:Description rdf:about="http://purl.org/olia/mte/multext-east.owl#Adverb"/>
                    <rdf:Description rdf:about="http://purl.org/olia/mte/multext-east.owl#Article"/>
                    <rdf:Description rdf:about="http://purl.org/olia/mte/multext-east.owl#Determiner"/>
                    <rdf:Description rdf:about="http://purl.org/olia/mte/multext-east.owl#Noun"/>
                    <rdf:Description rdf:about="http://purl.org/olia/mte/multext-east.owl#Numeral"/>
                    <rdf:Description rdf:about="http://purl.org/olia/mte/multext-east.owl#Pronoun"/>
                    <rdf:Description rdf:about="http://purl.org/olia/mte/multext-east.owl#Verb"/>
                </owl:unionOf>
            </owl:Class>
        </rdfs:domain>
        <rdfs:range rdf:resource="http://purl.org/olia/mte/multext-east.owl#Case"/>
    </owl:ObjectProperty>
    


    <!-- http://purl.org/olia/mte/multext-east.owl#hasClitic -->

    <owl:ObjectProperty rdf:about="http://purl.org/olia/mte/multext-east.owl#hasClitic">
        <rdfs:subPropertyOf rdf:resource="http://purl.org/olia/mte/multext-east.owl#hasFeature"/>
        <rdfs:domain>
            <owl:Class>
                <owl:unionOf rdf:parseType="Collection">
                    <rdf:Description rdf:about="http://purl.org/olia/mte/multext-east.owl#Adjective"/>
                    <rdf:Description rdf:about="http://purl.org/olia/mte/multext-east.owl#Adposition"/>
                    <rdf:Description rdf:about="http://purl.org/olia/mte/multext-east.owl#Adverb"/>
                    <rdf:Description rdf:about="http://purl.org/olia/mte/multext-east.owl#Article"/>
                    <rdf:Description rdf:about="http://purl.org/olia/mte/multext-east.owl#Conjunction"/>
                    <rdf:Description rdf:about="http://purl.org/olia/mte/multext-east.owl#Determiner"/>
                    <rdf:Description rdf:about="http://purl.org/olia/mte/multext-east.owl#Noun"/>
                    <rdf:Description rdf:about="http://purl.org/olia/mte/multext-east.owl#Numeral"/>
                    <rdf:Description rdf:about="http://purl.org/olia/mte/multext-east.owl#Particle"/>
                    <rdf:Description rdf:about="http://purl.org/olia/mte/multext-east.owl#Pronoun"/>
                    <rdf:Description rdf:about="http://purl.org/olia/mte/multext-east.owl#Verb"/>
                </owl:unionOf>
            </owl:Class>
        </rdfs:domain>
        <rdfs:range rdf:resource="http://purl.org/olia/mte/multext-east.owl#Cliticness"/>
    </owl:ObjectProperty>
    


    <!-- http://purl.org/olia/mte/multext-east.owl#hasConjunctionFormation -->

    <owl:ObjectProperty rdf:about="http://purl.org/olia/mte/multext-east.owl#hasConjunctionFormation">
        <rdfs:subPropertyOf rdf:resource="http://purl.org/olia/mte/multext-east.owl#hasFormation"/>
        <rdfs:domain rdf:resource="http://purl.org/olia/mte/multext-east.owl#Conjunction"/>
        <rdfs:range rdf:resource="http://purl.org/olia/mte/multext-east.owl#ConjunctionFormation"/>
    </owl:ObjectProperty>
    


    <!-- http://purl.org/olia/mte/multext-east.owl#hasCourtesy -->

    <owl:ObjectProperty rdf:about="http://purl.org/olia/mte/multext-east.owl#hasCourtesy">
        <rdfs:subPropertyOf rdf:resource="http://purl.org/olia/mte/multext-east.owl#hasFeature"/>
        <rdfs:domain>
            <owl:Class>
                <owl:unionOf rdf:parseType="Collection">
                    <rdf:Description rdf:about="http://purl.org/olia/mte/multext-east.owl#Pronoun"/>
                    <rdf:Description rdf:about="http://purl.org/olia/mte/multext-east.owl#Verb"/>
                </owl:unionOf>
            </owl:Class>
        </rdfs:domain>
        <rdfs:range rdf:resource="http://purl.org/olia/mte/multext-east.owl#Courtesy"/>
    </owl:ObjectProperty>
    


    <!-- http://purl.org/olia/mte/multext-east.owl#hasDefiniteness -->

    <owl:ObjectProperty rdf:about="http://purl.org/olia/mte/multext-east.owl#hasDefiniteness">
        <rdfs:subPropertyOf rdf:resource="http://purl.org/olia/mte/multext-east.owl#hasFeature"/>
        <rdfs:domain>
            <owl:Class>
                <owl:unionOf rdf:parseType="Collection">
                    <rdf:Description rdf:about="http://purl.org/olia/mte/multext-east.owl#Abbreviation"/>
                    <rdf:Description rdf:about="http://purl.org/olia/mte/multext-east.owl#Adjective"/>
                    <rdf:Description rdf:about="http://purl.org/olia/mte/multext-east.owl#Noun"/>
                    <rdf:Description rdf:about="http://purl.org/olia/mte/multext-east.owl#Numeral"/>
                    <rdf:Description rdf:about="http://purl.org/olia/mte/multext-east.owl#Pronoun"/>
                    <rdf:Description rdf:about="http://purl.org/olia/mte/multext-east.owl#Verb"/>
                </owl:unionOf>
            </owl:Class>
        </rdfs:domain>
        <rdfs:range rdf:resource="http://purl.org/olia/mte/multext-east.owl#Definiteness"/>
    </owl:ObjectProperty>
    


    <!-- http://purl.org/olia/mte/multext-east.owl#hasDegree -->

    <owl:ObjectProperty rdf:about="http://purl.org/olia/mte/multext-east.owl#hasDegree">
        <rdfs:subPropertyOf rdf:resource="http://purl.org/olia/mte/multext-east.owl#hasFeature"/>
        <rdfs:domain>
            <owl:Class>
                <owl:unionOf rdf:parseType="Collection">
                    <rdf:Description rdf:about="http://purl.org/olia/mte/multext-east.owl#Adjective"/>
                    <rdf:Description rdf:about="http://purl.org/olia/mte/multext-east.owl#Adverb"/>
                </owl:unionOf>
            </owl:Class>
        </rdfs:domain>
        <rdfs:range rdf:resource="http://purl.org/olia/mte/multext-east.owl#Degree"/>
    </owl:ObjectProperty>
    


    <!-- http://purl.org/olia/mte/multext-east.owl#hasFeature -->

    <owl:ObjectProperty rdf:about="http://purl.org/olia/mte/multext-east.owl#hasFeature">
        <rdfs:domain rdf:resource="http://purl.org/olia/mte/multext-east.owl#MorphosyntacticCategory"/>
        <rdfs:range rdf:resource="http://purl.org/olia/mte/multext-east.owl#MorphosyntacticFeature"/>
    </owl:ObjectProperty>
    


    <!-- http://purl.org/olia/mte/multext-east.owl#hasFormation -->

    <owl:ObjectProperty rdf:about="http://purl.org/olia/mte/multext-east.owl#hasFormation">
        <rdfs:subPropertyOf rdf:resource="http://purl.org/olia/mte/multext-east.owl#hasFeature"/>
        <rdfs:range rdf:resource="http://purl.org/olia/mte/multext-east.owl#Formation"/>
        <rdfs:comment>Formation:
   refers to the graphical components: simple, i.e. consisting of one word; compound, i.e. consisting of more than one word.</rdfs:comment>
    </owl:ObjectProperty>
    


    <!-- http://purl.org/olia/mte/multext-east.owl#hasGender -->

    <owl:ObjectProperty rdf:about="http://purl.org/olia/mte/multext-east.owl#hasGender">
        <rdfs:subPropertyOf rdf:resource="http://purl.org/olia/mte/multext-east.owl#hasFeature"/>
        <rdfs:domain>
            <owl:Class>
                <owl:unionOf rdf:parseType="Collection">
                    <rdf:Description rdf:about="http://purl.org/olia/mte/multext-east.owl#Abbreviation"/>
                    <rdf:Description rdf:about="http://purl.org/olia/mte/multext-east.owl#Adjective"/>
                    <rdf:Description rdf:about="http://purl.org/olia/mte/multext-east.owl#Article"/>
                    <rdf:Description rdf:about="http://purl.org/olia/mte/multext-east.owl#Determiner"/>
                    <rdf:Description rdf:about="http://purl.org/olia/mte/multext-east.owl#Noun"/>
                    <rdf:Description rdf:about="http://purl.org/olia/mte/multext-east.owl#Numeral"/>
                    <rdf:Description rdf:about="http://purl.org/olia/mte/multext-east.owl#Pronoun"/>
                    <rdf:Description rdf:about="http://purl.org/olia/mte/multext-east.owl#Verb"/>
                </owl:unionOf>
            </owl:Class>
        </rdfs:domain>
        <rdfs:range rdf:resource="http://purl.org/olia/mte/multext-east.owl#Gender"/>
    </owl:ObjectProperty>
    


    <!-- http://purl.org/olia/mte/multext-east.owl#hasHumanness -->

    <owl:ObjectProperty rdf:about="http://purl.org/olia/mte/multext-east.owl#hasHumanness">
        <rdfs:subPropertyOf rdf:resource="http://purl.org/olia/mte/multext-east.owl#hasFeature"/>
        <rdfs:domain>
            <owl:Class>
                <owl:unionOf rdf:parseType="Collection">
                    <rdf:Description rdf:about="http://purl.org/olia/mte/multext-east.owl#Adjective"/>
                    <rdf:Description rdf:about="http://purl.org/olia/mte/multext-east.owl#Noun"/>
                    <rdf:Description rdf:about="http://purl.org/olia/mte/multext-east.owl#Numeral"/>
                    <rdf:Description rdf:about="http://purl.org/olia/mte/multext-east.owl#Pronoun"/>
                    <rdf:Description rdf:about="http://purl.org/olia/mte/multext-east.owl#Verb"/>
                </owl:unionOf>
            </owl:Class>
        </rdfs:domain>
        <rdfs:range rdf:resource="http://purl.org/olia/mte/multext-east.owl#Humanness"/>
    </owl:ObjectProperty>
    


    <!-- http://purl.org/olia/mte/multext-east.owl#hasInterjectionFormation -->

    <owl:ObjectProperty rdf:about="http://purl.org/olia/mte/multext-east.owl#hasInterjectionFormation">
        <rdfs:subPropertyOf rdf:resource="http://purl.org/olia/mte/multext-east.owl#hasFormation"/>
        <rdfs:domain rdf:resource="http://purl.org/olia/mte/multext-east.owl#Interjection"/>
        <rdfs:range rdf:resource="http://purl.org/olia/mte/multext-east.owl#InterjectionFormation"/>
    </owl:ObjectProperty>
    


    <!-- http://purl.org/olia/mte/multext-east.owl#hasModificationType -->

    <owl:ObjectProperty rdf:about="http://purl.org/olia/mte/multext-east.owl#hasModificationType">
        <rdfs:subPropertyOf rdf:resource="http://purl.org/olia/mte/multext-east.owl#hasFeature"/>
        <rdfs:domain rdf:resource="http://purl.org/olia/mte/multext-east.owl#Determiner"/>
        <rdfs:range rdf:resource="http://purl.org/olia/mte/multext-east.owl#ModificationType"/>
    </owl:ObjectProperty>
    


    <!-- http://purl.org/olia/mte/multext-east.owl#hasNegation -->

    <owl:ObjectProperty rdf:about="http://purl.org/olia/mte/multext-east.owl#hasNegation">
        <rdfs:subPropertyOf rdf:resource="http://purl.org/olia/mte/multext-east.owl#hasFeature"/>
        <rdfs:domain>
            <owl:Class>
                <owl:unionOf rdf:parseType="Collection">
                    <rdf:Description rdf:about="http://purl.org/olia/mte/multext-east.owl#Adjective"/>
                    <rdf:Description rdf:about="http://purl.org/olia/mte/multext-east.owl#Noun"/>
                    <rdf:Description rdf:about="http://purl.org/olia/mte/multext-east.owl#Verb"/>
                </owl:unionOf>
            </owl:Class>
        </rdfs:domain>
        <rdfs:range rdf:resource="http://purl.org/olia/mte/multext-east.owl#Negation"/>
    </owl:ObjectProperty>
    


    <!-- http://purl.org/olia/mte/multext-east.owl#hasNumber -->

    <owl:ObjectProperty rdf:about="http://purl.org/olia/mte/multext-east.owl#hasNumber">
        <rdfs:subPropertyOf rdf:resource="http://purl.org/olia/mte/multext-east.owl#hasFeature"/>
        <rdfs:domain>
            <owl:Class>
                <owl:unionOf rdf:parseType="Collection">
                    <rdf:Description rdf:about="http://purl.org/olia/mte/multext-east.owl#Abbreviation"/>
                    <rdf:Description rdf:about="http://purl.org/olia/mte/multext-east.owl#Adjective"/>
                    <rdf:Description rdf:about="http://purl.org/olia/mte/multext-east.owl#Adverb"/>
                    <rdf:Description rdf:about="http://purl.org/olia/mte/multext-east.owl#Article"/>
                    <rdf:Description rdf:about="http://purl.org/olia/mte/multext-east.owl#Conjunction"/>
                    <rdf:Description rdf:about="http://purl.org/olia/mte/multext-east.owl#Determiner"/>
                    <rdf:Description rdf:about="http://purl.org/olia/mte/multext-east.owl#Noun"/>
                    <rdf:Description rdf:about="http://purl.org/olia/mte/multext-east.owl#Numeral"/>
                    <rdf:Description rdf:about="http://purl.org/olia/mte/multext-east.owl#Pronoun"/>
                    <rdf:Description rdf:about="http://purl.org/olia/mte/multext-east.owl#Verb"/>
                </owl:unionOf>
            </owl:Class>
        </rdfs:domain>
        <rdfs:range rdf:resource="http://purl.org/olia/mte/multext-east.owl#Number"/>
    </owl:ObjectProperty>
    


    <!-- http://purl.org/olia/mte/multext-east.owl#hasNumeralForm -->

    <owl:ObjectProperty rdf:about="http://purl.org/olia/mte/multext-east.owl#hasNumeralForm">
        <rdfs:subPropertyOf rdf:resource="http://purl.org/olia/mte/multext-east.owl#hasFeature"/>
        <rdfs:domain rdf:resource="http://purl.org/olia/mte/multext-east.owl#Numeral"/>
        <rdfs:range rdf:resource="http://purl.org/olia/mte/multext-east.owl#NumeralForm"/>
    </owl:ObjectProperty>
    


    <!-- http://purl.org/olia/mte/multext-east.owl#hasOwnedNumber -->

    <owl:ObjectProperty rdf:about="http://purl.org/olia/mte/multext-east.owl#hasOwnedNumber">
        <rdfs:subPropertyOf rdf:resource="http://purl.org/olia/mte/multext-east.owl#hasFeature"/>
        <rdfs:domain>
            <owl:Class>
                <owl:unionOf rdf:parseType="Collection">
                    <rdf:Description rdf:about="http://purl.org/olia/mte/multext-east.owl#Adjective"/>
                    <rdf:Description rdf:about="http://purl.org/olia/mte/multext-east.owl#Noun"/>
                    <rdf:Description rdf:about="http://purl.org/olia/mte/multext-east.owl#Numeral"/>
                    <rdf:Description rdf:about="http://purl.org/olia/mte/multext-east.owl#Pronoun"/>
                </owl:unionOf>
            </owl:Class>
        </rdfs:domain>
        <rdfs:range rdf:resource="http://purl.org/olia/mte/multext-east.owl#Number"/>
        <rdfs:comment>feature &quot;Owned_Number&quot; (Pronoun and PronominalAdjectives; Hungarian Noun, Numeral)
Owned_Number:
    in the Hungarian system, different word-forms are distinguished for nominals on the basis of so called &apos;anaphoric possessive&apos; number, i.e. the number of the thing(s) possessed by the nominal in question.</rdfs:comment>
    </owl:ObjectProperty>
    


    <!-- http://purl.org/olia/mte/multext-east.owl#hasOwnerGender -->

    <owl:ObjectProperty rdf:about="http://purl.org/olia/mte/multext-east.owl#hasOwnerGender">
        <rdfs:subPropertyOf rdf:resource="http://purl.org/olia/mte/multext-east.owl#hasFeature"/>
        <rdfs:domain>
            <owl:Class>
                <owl:unionOf rdf:parseType="Collection">
                    <rdf:Description rdf:about="http://purl.org/olia/mte/multext-east.owl#Determiner"/>
                    <rdf:Description rdf:about="http://purl.org/olia/mte/multext-east.owl#Pronoun"/>
                </owl:unionOf>
            </owl:Class>
        </rdfs:domain>
        <rdfs:range rdf:resource="http://purl.org/olia/mte/multext-east.owl#Gender"/>
        <rdfs:comment>Pronoun/Owner_Gender
Owner_Gender:
    used to encode the Gender of the possessor in Pronouns and (in Romanian) Determiners.</rdfs:comment>
    </owl:ObjectProperty>
    


    <!-- http://purl.org/olia/mte/multext-east.owl#hasOwnerNumber -->

    <owl:ObjectProperty rdf:about="http://purl.org/olia/mte/multext-east.owl#hasOwnerNumber">
        <rdfs:subPropertyOf rdf:resource="http://purl.org/olia/mte/multext-east.owl#hasFeature"/>
        <rdfs:domain>
            <owl:Class>
                <owl:unionOf rdf:parseType="Collection">
                    <rdf:Description rdf:about="http://purl.org/olia/mte/multext-east.owl#Adjective"/>
                    <rdf:Description rdf:about="http://purl.org/olia/mte/multext-east.owl#Determiner"/>
                    <rdf:Description rdf:about="http://purl.org/olia/mte/multext-east.owl#Noun"/>
                    <rdf:Description rdf:about="http://purl.org/olia/mte/multext-east.owl#Numeral"/>
                    <rdf:Description rdf:about="http://purl.org/olia/mte/multext-east.owl#Pronoun"/>
                </owl:unionOf>
            </owl:Class>
        </rdfs:domain>
        <rdfs:range rdf:resource="http://purl.org/olia/mte/multext-east.owl#Number"/>
        <rdfs:comment>feature &quot;Owner_Number&quot; (Pronoun, for Hungarian also Noun and Adjective)
Owner_Number:
    used to specify the possessor number in Pronouns, as well as (in Romanian) in Determiners, and (in Hungarian) in Adjectives and Nouns.</rdfs:comment>
    </owl:ObjectProperty>
    


    <!-- http://purl.org/olia/mte/multext-east.owl#hasOwnerPerson -->

    <owl:ObjectProperty rdf:about="http://purl.org/olia/mte/multext-east.owl#hasOwnerPerson">
        <rdfs:subPropertyOf rdf:resource="http://purl.org/olia/mte/multext-east.owl#hasFeature"/>
        <rdfs:domain>
            <owl:Class>
                <owl:unionOf rdf:parseType="Collection">
                    <rdf:Description rdf:about="http://purl.org/olia/mte/multext-east.owl#Adjective"/>
                    <rdf:Description rdf:about="http://purl.org/olia/mte/multext-east.owl#Noun"/>
                    <rdf:Description rdf:about="http://purl.org/olia/mte/multext-east.owl#Numeral"/>
                    <rdf:Description rdf:about="http://purl.org/olia/mte/multext-east.owl#Pronoun"/>
                </owl:unionOf>
            </owl:Class>
        </rdfs:domain>
        <rdfs:range rdf:resource="http://purl.org/olia/mte/multext-east.owl#Person"/>
        <rdfs:comment>feature &quot;Owner_Person&quot; (Pronoun (and pronominal Adjectives),  Noun: Hungarian)
Owner_Person:
    used to specify the possessor person in in Hungarian in Adjectives and Nouns.</rdfs:comment>
    </owl:ObjectProperty>
    


    <!-- http://purl.org/olia/mte/multext-east.owl#hasParticleFormation -->

    <owl:ObjectProperty rdf:about="http://purl.org/olia/mte/multext-east.owl#hasParticleFormation">
        <rdfs:subPropertyOf rdf:resource="http://purl.org/olia/mte/multext-east.owl#hasFormation"/>
        <rdfs:domain rdf:resource="http://purl.org/olia/mte/multext-east.owl#Particle"/>
        <rdfs:range rdf:resource="http://purl.org/olia/mte/multext-east.owl#ParticleFormation"/>
    </owl:ObjectProperty>
    


    <!-- http://purl.org/olia/mte/multext-east.owl#hasPerson -->

    <owl:ObjectProperty rdf:about="http://purl.org/olia/mte/multext-east.owl#hasPerson">
        <rdfs:subPropertyOf rdf:resource="http://purl.org/olia/mte/multext-east.owl#hasFeature"/>
        <rdfs:domain>
            <owl:Class>
                <owl:unionOf rdf:parseType="Collection">
                    <rdf:Description rdf:about="http://purl.org/olia/mte/multext-east.owl#Adverb"/>
                    <rdf:Description rdf:about="http://purl.org/olia/mte/multext-east.owl#Conjunction"/>
                    <rdf:Description rdf:about="http://purl.org/olia/mte/multext-east.owl#Determiner"/>
                    <rdf:Description rdf:about="http://purl.org/olia/mte/multext-east.owl#Pronoun"/>
                    <rdf:Description rdf:about="http://purl.org/olia/mte/multext-east.owl#Verb"/>
                </owl:unionOf>
            </owl:Class>
        </rdfs:domain>
        <rdfs:range rdf:resource="http://purl.org/olia/mte/multext-east.owl#Person"/>
    </owl:ObjectProperty>
    


    <!-- http://purl.org/olia/mte/multext-east.owl#hasPronounForm -->

    <owl:ObjectProperty rdf:about="http://purl.org/olia/mte/multext-east.owl#hasPronounForm">
        <rdfs:subPropertyOf rdf:resource="http://purl.org/olia/mte/multext-east.owl#hasFeature"/>
        <rdfs:domain rdf:resource="http://purl.org/olia/mte/multext-east.owl#Pronoun"/>
        <rdfs:range rdf:resource="http://purl.org/olia/mte/multext-east.owl#PronounForm"/>
        <rdfs:comment>Pronoun/Pronoun_Form</rdfs:comment>
    </owl:ObjectProperty>
    


    <!-- http://purl.org/olia/mte/multext-east.owl#hasQuantifier -->

    <owl:ObjectProperty rdf:about="http://purl.org/olia/mte/multext-east.owl#hasQuantifier">
        <rdfs:subPropertyOf rdf:resource="http://purl.org/olia/mte/multext-east.owl#hasFeature"/>
        <rdfs:domain rdf:resource="http://purl.org/olia/mte/multext-east.owl#Numeral"/>
        <rdfs:range rdf:resource="http://purl.org/olia/mte/multext-east.owl#Quantifier"/>
    </owl:ObjectProperty>
    


    <!-- http://purl.org/olia/mte/multext-east.owl#hasSubCase -->

    <owl:ObjectProperty rdf:about="http://purl.org/olia/mte/multext-east.owl#hasSubCase">
        <rdfs:subPropertyOf rdf:resource="http://purl.org/olia/mte/multext-east.owl#hasCase"/>
        <rdfs:domain rdf:resource="http://purl.org/olia/mte/multext-east.owl#Noun"/>
        <rdfs:range rdf:resource="http://purl.org/olia/mte/multext-east.owl#Case"/>
        <rdfs:comment>
			A SubCase refers to non-standard cases, i.e., a grammatical differentiation that occurs in few inflection paradigms that is
			regularly expressed by a single case.
			Some Russian genitive nouns take the non-standard ending &quot;-у,-ю&quot; in genitive to express partitive meaning (&quot;чашка горячего чаю&quot;) or in prepositive (locative) to express locative meaning (&quot;на шкафу&quot;).
			(MTE 4; Serge Sharoff)
		</rdfs:comment>
        <owl:versionInfo>
			Introduced to account for the case2 attribute of Russian Nouns.
			MTE feature &quot;Case2&quot; with values &quot;partitive&quot; and &quot;locative&quot; for Russian nouns.
		</owl:versionInfo>
    </owl:ObjectProperty>
    


    <!-- http://purl.org/olia/mte/multext-east.owl#hasSyntacticType -->

    <owl:ObjectProperty rdf:about="http://purl.org/olia/mte/multext-east.owl#hasSyntacticType">
        <rdfs:subPropertyOf rdf:resource="http://purl.org/olia/mte/multext-east.owl#hasFeature"/>
        <rdfs:domain>
            <owl:Class>
                <owl:unionOf rdf:parseType="Collection">
                    <rdf:Description rdf:about="http://purl.org/olia/mte/multext-east.owl#Abbreviation"/>
                    <rdf:Description rdf:about="http://purl.org/olia/mte/multext-east.owl#Pronoun"/>
                </owl:unionOf>
            </owl:Class>
        </rdfs:domain>
        <rdfs:range rdf:resource="http://purl.org/olia/mte/multext-east.owl#SyntacticType"/>
        <rdfs:comment>Pronoun/Syntactic_Type and Abbreviation/Syntactic_Type</rdfs:comment>
    </owl:ObjectProperty>
    


    <!-- http://purl.org/olia/mte/multext-east.owl#hasTense -->

    <owl:ObjectProperty rdf:about="http://purl.org/olia/mte/multext-east.owl#hasTense">
        <rdfs:subPropertyOf rdf:resource="http://purl.org/olia/mte/multext-east.owl#hasFeature"/>
        <rdfs:domain>
            <owl:Class>
                <owl:unionOf rdf:parseType="Collection">
                    <rdf:Description rdf:about="http://purl.org/olia/mte/multext-east.owl#Adjective"/>
                    <rdf:Description rdf:about="http://purl.org/olia/mte/multext-east.owl#Verb"/>
                </owl:unionOf>
            </owl:Class>
        </rdfs:domain>
        <rdfs:range rdf:resource="http://purl.org/olia/mte/multext-east.owl#Tense"/>
        <rdfs:comment>also applied to Ukrainian Adjective</rdfs:comment>
    </owl:ObjectProperty>
    


    <!-- http://purl.org/olia/mte/multext-east.owl#hasTransitivity -->

    <owl:ObjectProperty rdf:about="http://purl.org/olia/mte/multext-east.owl#hasTransitivity">
        <rdfs:subPropertyOf rdf:resource="http://purl.org/olia/mte/multext-east.owl#hasFeature"/>
        <rdfs:domain rdf:resource="http://purl.org/olia/mte/multext-east.owl#Verb"/>
        <rdfs:range rdf:resource="http://purl.org/olia/mte/multext-east.owl#Transitivity"/>
    </owl:ObjectProperty>
    


    <!-- http://purl.org/olia/mte/multext-east.owl#hasVerbForm -->

    <owl:ObjectProperty rdf:about="http://purl.org/olia/mte/multext-east.owl#hasVerbForm">
        <rdfs:subPropertyOf rdf:resource="http://purl.org/olia/mte/multext-east.owl#hasFeature"/>
        <rdfs:domain rdf:resource="http://purl.org/olia/mte/multext-east.owl#Verb"/>
        <rdfs:range rdf:resource="http://purl.org/olia/mte/multext-east.owl#VerbForm"/>
    </owl:ObjectProperty>
    


    <!-- http://purl.org/olia/mte/multext-east.owl#hasVoice -->

    <owl:ObjectProperty rdf:about="http://purl.org/olia/mte/multext-east.owl#hasVoice">
        <rdfs:subPropertyOf rdf:resource="http://purl.org/olia/mte/multext-east.owl#hasFeature"/>
        <rdfs:domain>
            <owl:Class>
                <owl:unionOf rdf:parseType="Collection">
                    <rdf:Description rdf:about="http://purl.org/olia/mte/multext-east.owl#Adjective"/>
                    <rdf:Description rdf:about="http://purl.org/olia/mte/multext-east.owl#Verb"/>
                </owl:unionOf>
            </owl:Class>
        </rdfs:domain>
        <rdfs:range rdf:resource="http://purl.org/olia/mte/multext-east.owl#Voice"/>
        <rdfs:comment>applied to Polish and Hungarian adjective</rdfs:comment>
    </owl:ObjectProperty>
    


    <!-- http://purl.org/olia/mte/multext-east.owl#hasWHType -->

    <owl:ObjectProperty rdf:about="http://purl.org/olia/mte/multext-east.owl#hasWHType">
        <rdfs:subPropertyOf rdf:resource="http://purl.org/olia/mte/multext-east.owl#hasFeature"/>
        <rdfs:domain>
            <owl:Class>
                <owl:unionOf rdf:parseType="Collection">
                    <rdf:Description rdf:about="http://purl.org/olia/mte/multext-east.owl#Adverb"/>
                    <rdf:Description rdf:about="http://purl.org/olia/mte/multext-east.owl#Determiner"/>
                    <rdf:Description rdf:about="http://purl.org/olia/mte/multext-east.owl#Pronoun"/>
                </owl:unionOf>
            </owl:Class>
        </rdfs:domain>
        <rdfs:range rdf:resource="http://purl.org/olia/mte/multext-east.owl#WHType"/>
    </owl:ObjectProperty>
    


    <!-- 
    ///////////////////////////////////////////////////////////////////////////////////////
    //
    // Data properties
    //
    ///////////////////////////////////////////////////////////////////////////////////////
     -->

    


    <!-- http://purl.org/olia/system.owl#hasTier -->

    <owl:DatatypeProperty rdf:about="http://purl.org/olia/system.owl#hasTier"/>
    


    <!-- 
    ///////////////////////////////////////////////////////////////////////////////////////
    //
    // Classes
    //
    ///////////////////////////////////////////////////////////////////////////////////////
     -->

    


    <!-- http://purl.org/olia/mte/multext-east.owl#Abbreviation -->

    <owl:Class rdf:about="http://purl.org/olia/mte/multext-east.owl#Abbreviation">
        <rdfs:subClassOf rdf:resource="http://purl.org/olia/mte/multext-east.owl#MorphosyntacticCategory"/>
        <rdfs:subClassOf>
            <owl:Class>
                <owl:intersectionOf rdf:parseType="Collection">
                    <owl:Restriction>
                        <owl:onProperty rdf:resource="http://purl.org/olia/mte/multext-east.owl#hasCase"/>
                        <owl:maxCardinality rdf:datatype="http://www.w3.org/2001/XMLSchema#nonNegativeInteger">1</owl:maxCardinality>
                    </owl:Restriction>
                    <owl:Restriction>
                        <owl:onProperty rdf:resource="http://purl.org/olia/mte/multext-east.owl#hasDefiniteness"/>
                        <owl:maxCardinality rdf:datatype="http://www.w3.org/2001/XMLSchema#nonNegativeInteger">1</owl:maxCardinality>
                    </owl:Restriction>
                    <owl:Restriction>
                        <owl:onProperty rdf:resource="http://purl.org/olia/mte/multext-east.owl#hasGender"/>
                        <owl:maxCardinality rdf:datatype="http://www.w3.org/2001/XMLSchema#nonNegativeInteger">1</owl:maxCardinality>
                    </owl:Restriction>
                    <owl:Restriction>
                        <owl:onProperty rdf:resource="http://purl.org/olia/mte/multext-east.owl#hasNumber"/>
                        <owl:maxCardinality rdf:datatype="http://www.w3.org/2001/XMLSchema#nonNegativeInteger">1</owl:maxCardinality>
                    </owl:Restriction>
                    <owl:Restriction>
                        <owl:onProperty rdf:resource="http://purl.org/olia/mte/multext-east.owl#hasSyntacticType"/>
                        <owl:maxCardinality rdf:datatype="http://www.w3.org/2001/XMLSchema#nonNegativeInteger">1</owl:maxCardinality>
                    </owl:Restriction>
                </owl:intersectionOf>
            </owl:Class>
        </rdfs:subClassOf>
        <rdfs:comment>e.g., Dr. (en)</rdfs:comment>
        <rdfs:comment>e.g., R/r, s/s (sl-rozaj)</rdfs:comment>
        <rdfs:comment>e.g., d-ei/dumneaei, d-le/domnule, d-lor/doamnelor, d-lor/domnilor, d-lor/dumnealor, d-lui/domnului, d-lui/dumnealui, d-na/doamna, d-nei/doamnei (ro)</rdfs:comment>
        <rdfs:comment>e.g., j.i./j.i., k.p.k./k.p.k., m.in./m.in. (pl)</rdfs:comment>
        <rdfs:comment>e.g., kg-ga/kg, kt-ks/kt, NLKP-d/NLKP, NSV-sse/NSV, NSVd/NSV, TPId/TPI, TRÜ-sse/TRÜ, USA-ga/USA, USA-sse/USA (et)</rdfs:comment>
        <rdfs:comment>e.g., АЕС АЗС АНДР АПК АСЕАН АТ АТП АТР АТС БРСР ВДНГ ВІЛ ВЛКСМ ВМС ВМСУ ВПК ВПС ВР ВУАН ВУЦВК (uk)</rdfs:comment>
        <rdfs:comment>e.g., ок (mk)</rdfs:comment>
        <rdfs:comment>e.g., و ج (fa)</rdfs:comment>
    </owl:Class>
    


    <!-- http://purl.org/olia/mte/multext-east.owl#AbessiveCase -->

    <owl:Class rdf:about="http://purl.org/olia/mte/multext-east.owl#AbessiveCase">
        <rdfs:subClassOf rdf:resource="http://purl.org/olia/mte/multext-east.owl#Case"/>
        <rdfs:comment>e.g., kelleta/kes, milleta/mis, minutagi/mina, muuta/muu, nendetagi/see, nendetagi/tema, olemata/olema, pidamata/pidama, pikemata/pikem (et)</rdfs:comment>
        <rdfs:comment>Case=&quot;abessive&quot; (Estonian)</rdfs:comment>
    </owl:Class>
    


    <!-- http://purl.org/olia/mte/multext-east.owl#AblativeCase -->

    <owl:Class rdf:about="http://purl.org/olia/mte/multext-east.owl#AblativeCase">
        <rdfs:subClassOf rdf:resource="http://purl.org/olia/mte/multext-east.owl#Case"/>
        <rdfs:comment>e.g., -, 1900-tól/1900, 2050-től/2050, akiktől/aki, amelytől/amely, amitől/ami, attól/az, azoktól/az, betegségünktől/betegség (hu)</rdfs:comment>
        <rdfs:comment>e.g., endalt/ise, endilt/ise, eneselt/ise, Kallastelt/Kallas, kellelt/kes, kõigilt/kõik, meilt/mina, millelt/mis, minult/mina (et)</rdfs:comment>
        <rdfs:comment>Case=&quot;ablative&quot; (Estonian, Hungarian)</rdfs:comment>
    </owl:Class>
    


    <!-- http://purl.org/olia/mte/multext-east.owl#AccusativeCase -->

    <owl:Class rdf:about="http://purl.org/olia/mte/multext-east.owl#AccusativeCase">
        <rdfs:subClassOf rdf:resource="http://purl.org/olia/mte/multext-east.owl#Case"/>
        <rdfs:comment>e.g., &apos;Em/them, &apos;Er/her, her, thee/you, them, us, whom (en)</rdfs:comment>
        <rdfs:comment>e.g., , drug/=, druga/drug, druge/drug, drugega/drug, drugi/drug, drugo/drug, dva/=, dve/dva (sl)</rdfs:comment>
        <rdfs:comment>e.g., -, akiét/aki, Aladárét/Aladár, azét/az, benneteket/ti, bennünket/ti, borúlátónkat/borúlátó, egyikét/egyik, egymást/egymás (hu)</rdfs:comment>
        <rdfs:comment>e.g., -i/el, -l/el, -le/el, -ne/noi, -o/el, -te/tu, i-/el, l-/el, l/el (ro)</rdfs:comment>
        <rdfs:comment>e.g., 0, a незважаючи/=, Аахен/= Абай/= Абакан/= Абакан/= Абіджан/= Абовян/= Авентин/= Адамстаун/= Аден/= Аджаристан/= Адлер/= Адоніс/= Адріанополь/= Азенкур/= Азербайджан/= Азов/= Акерман/= Акмолінськ/= Акрополь/= Актюбінськ/=, Абакумів/= Абрамів/= Авакумів/= Августин/= Августинів/= Августів/= Авенірів/= Аверкіїв/= Авер&apos;янів/= Авіятин/= Авксентіїв/= Аврамів/= Авреліїн/= Аврорин/= Автономів/= авторів/= авторчин/= Агапіїв/= Агапіїн/= Агапітів/=, Або/= Абруццо/= Абу-Дабі/= Адріатичне море/= Азовське море/= Айдахо/= Ай-Петрі/= Аконкагуа/= Актау/= Алеппо/= Аліканте/= Алмати/= Альбі/= Андаманське море/= Анжу/= Ані/= Антананаріву/= Антигуа/= Апіа/= Апостолове/=, Абіссінію/Абіссінія Абуджу/Абуджа Абхазію/Абхазія Авдіївку/Авдіївка Австралію/Австралія Австрію/Австрія Австро-Угорщину/Австро-Угорщина Аддис-Абебу/Аддис-Абеба Аджарію/Аджарія Адигею/Адигея Адріатику/Адріатика Азію/Азія Айову/Айова Аквітанію/Аквітанія Аккру/Аккра Ак-Мечеть/= Акмолу/Акмола акрилову кислоту/акрилова кислота Алабаму/Алабама Албанію/Албанія, Азорські острови/= Аландські острови/= Алеутські острови/= Андаманські острови/= Антильські острови/= Багамські острови/= Балеарські острови/= Бельбеки/Бельбек Бермудські острови/= Буги/Буг Великодні/Великдень Великі Сорочинці/= Віргінські острови/= Гавайські острови/= Гебридські острови/= Драконові гори/= ЖЕКи/ЖЕК Зеленого Мису острови/= Змієві вали/= Зондські острови/=, Альпи/= Анди/= Апенніни/= Аппалачі/= Арденни/= Афіни/= Багами/= Балкани/= Байдарські ворота/= Барановичі/= Бендери/= Березняки/= Бермуди/= Бескиди/= Біличі/= Близнюки/= Богородчани/= Боровичі/= Бортничі/= Бровари/=, Америки/Америка Андалуські гори/= Атлаські гори/= Бистриці/Бистриця Держдуми/Держдума Жовті Води/= Збройні Сили України/Збройні сили України Індії/Індія Інтернет-газети/Інтернет-газета Караваєві дачі/= Магелланові хмари/= Македонії/Македонія Мате Залка/= Пасхи/Пасха Пилипівки/Пилипівка Ради/Рада Родезії/Родезія Інтернет-технології/Інтернет-технологія (uk)</rdfs:comment>
        <rdfs:comment>e.g., XXIV/xxiv, ВАС/вы, Вас/вы, ДВА/два, Женечку/женечка, Женьку/женька, НАС/мы, Нас/мы, Насекомых/насекомое (ru)</rdfs:comment>
        <rdfs:comment>e.g., blishgnaha/blïžnji, Bohouv/böguw, Bohove/böguw, božjega/böžji, cach/kak, Christusa/krïštuš, coga/du, Coj/koj, colina/kolënu (sl-rozaj)</rdfs:comment>
        <rdfs:comment>e.g., bliższe/bliski, będące/być, cały/cały, chorego/chory, ciebie/ty, cię/ty, co/co, cokolwiek/cokolwiek, coś/coś (pl)</rdfs:comment>
        <rdfs:comment>e.g., brillská/brillský, desátá/desátý, devatenácté/devatenáctý, druhej/druhý, druhou/druhý, druhá/druhý, druhé/druhý, druhého/druhý, druhý (cs)</rdfs:comment>
        <rdfs:comment>e.g., druhé/druhý, druhého/druhý, druhú/druhý, druhý, druhých/druhý, dva, dve/dva, dvoch/dva, henten (sk)</rdfs:comment>
        <rdfs:comment>e.g., dva, dve/dva, dvoja/dvoje, dvoje, gipsani/gipsan, Goldštajnov, govornikov, gvozdene/gvozden, ih/ona (sr)</rdfs:comment>
        <rdfs:comment>e.g., Вас/Вие, Ве/Вие, вас/вие, ве/вие, ги/тие, го/тоа, го/тој, кого/кој, ме/јас (mk)</rdfs:comment>
        <rdfs:comment>e.g., вас/вие, ви/вие, всекиго/всеки, ги/те, го/то, го/той, кого/кой, когото/който, ме/аз (bg)</rdfs:comment>
        <rdfs:comment>e.g., تان/تو, ترا/تو, ش/آن, شان/آنها, م/من, مرا/من م/من, يش/او ش/او اش/او, ِت/تو ت/تو ات/تو (fa)</rdfs:comment>
    </owl:Class>
    


    <!-- http://purl.org/olia/mte/multext-east.owl#ActiveVoice -->

    <owl:Class rdf:about="http://purl.org/olia/mte/multext-east.owl#ActiveVoice">
        <rdfs:subClassOf rdf:resource="http://purl.org/olia/mte/multext-east.owl#Voice"/>
        <rdfs:comment>e.g., 0, аглютинуюча/аглютинуючий анестезуюча/анестезуючий апроксимуюча/апроксимуючий асимілююча/асимілюючий атакуюча/атакуючий мінімізуюча/мінімізуючий мобілізуюча/мобілізуючий нейтралізуюча/нейтралізуючий профілююча/профілюючий рандомізуюча/рандомізуючий сенсибілізуюча/сенсибілізуючий синтезуюча/синтезуючий стабілізуюча/стабілізуючий стимулююча/стимулюючий типізуюча/типізуючий тонізуюча/тонізуючий центруюча/центруючий, аглютинуючая/аглютинуючий анестезуючая/анестезуючий апроксимуючая/апроксимуючий асимілюючая/асимілюючий атакуючая/атакуючий мінімізуючая/мінімізуючий мобілізуючая/мобілізуючий нейтралізуючая/нейтралізуючий профілюючая/профілюючий рандомізуючая/рандомізуючий сенсибілізуючая/сенсибілізуючий синтезуючая/синтезуючий стабілізуючая/стабілізуючий стимулюючая/стимулюючий типізуючая/типізуючий тонізуючая/тонізуючий центруючая/центруючий, аглютинуюче/аглютинуючий анестезуюче/анестезуючий апроксимуюче/апроксимуючий асимілююче/асимілюючий атакуюче/атакуючий мінімізуюче/мінімізуючий мобілізуюче/мобілізуючий нейтралізуюче/нейтралізуючий профілююче/профілюючий рандомізуюче/рандомізуючий сенсибілізуюче/сенсибілізуючий синтезуюче/синтезуючий стабілізуюче/стабілізуючий стимулююче/стимулюючий типізуюче/типізуючий тонізуюче/тонізуючий центруюче/центруючий, аглютинуючеє/аглютинуючий анестезуючеє/анестезуючий апроксимуючеє/апроксимуючий асимілюючеє/асимілюючий атакуючеє/атакуючий мінімізуючеє/мінімізуючий мобілізуючеє/мобілізуючий нейтралізуючеє/нейтралізуючий профілюючеє/профілюючий рандомізуючеє/рандомізуючий сенсибілізуючеє/сенсибілізуючий синтезуючеє/синтезуючий стабілізуючеє/стабілізуючий стимулюючеє/стимулюючий типізуючеє/типізуючий тонізуючеє/тонізуючий центруючеє/центруючий, аглютинуючеє/аглютинуючий анестезуючеє/анестезуючий апроксимуючеє/апроксимуючий атакуючеє/атакуючий мінімізуючеє/мінімізуючий мобілізуючеє/мобілізуючий нейтралізуючеє/нейтралізуючий рандомізуючеє/рандомізуючий сенсибілізуючеє/сенсибілізуючий синтезуючеє/синтезуючий стабілізуючеє/стабілізуючий типізуючеє/типізуючий тонізуючеє/тонізуючий центруючеє/центруючий, аглютинуючий/= анестезуючий/= апроксимуючий/= асимілюючий/= атакуючий/= мінімізуючий/= мобілізуючий/= нейтралізуючий/= профілюючий/= рандомізуючий/= сенсибілізуючий/= синтезуючий/= стабілізуючий/= стимулюючий/= типізуючий/= тонізуючий/= центруючий/=, аглютинуючим/аглютинуючий анестезуючим/анестезуючий апроксимуючим/апроксимуючий асимілюючим/асимілюючий атакуючим/атакуючий мінімізуючим/мінімізуючий мобілізуючим/мобілізуючий нейтралізуючим/нейтралізуючий профілюючим/профілюючий рандомізуючим/рандомізуючий сенсибілізуючим/сенсибілізуючий синтезуючим/синтезуючий стабілізуючим/стабілізуючий стимулюючим/стимулюючий типізуючим/типізуючий тонізуючим/тонізуючий центруючим/центруючий, аглютинуючими/аглютинуючий анестезуючими/анестезуючий апроксимуючими/апроксимуючий асимілюючими/асимілюючий атакуючими/атакуючий мінімізуючими/мінімізуючий мобілізуючими/мобілізуючий нейтралізуючими/нейтралізуючий профілюючими/профілюючий рандомізуючими/рандомізуючий сенсибілізуючими/сенсибілізуючий синтезуючими/синтезуючий стабілізуючими/стабілізуючий стимулюючими/стимулюючий типізуючими/типізуючий тонізуючими/тонізуючий центруючими/центруючий (uk)</rdfs:comment>
        <rdfs:comment>e.g., abdykujący/abdykować, adoptujących/adoptować, akredytujące/akredytować, akredytujących/akredytować, akredytującą/akredytować, awansującym/awansować, bieżącego/bieżeć, bieżącym/bieżeć, będące/być (pl)</rdfs:comment>
        <rdfs:comment>e.g., bejt/být, bude/být, budeme/být, budete/být, budeš/být, budou/být, budu/být, buď/být, byl/být (cs)</rdfs:comment>
        <rdfs:comment>e.g., benedila/binidet, bil/bet, Bila/bet, bile/bet, bili/bet, bilo/bet, bilu/bet, biu/bet, blíshghnili/blïžnjit (sl-rozaj)</rdfs:comment>
        <rdfs:comment>e.g., bi&apos;/biti, bi/biti, bih/biti, bila/biti, bile/biti, bilo/biti, bio/biti, bismo/biti, biste/biti (sr)</rdfs:comment>
        <rdfs:comment>e.g., ole/olema, oled/olema, oledki/olema, olegi/olema, oleks/olema, oleksime/olema, oleksin/olema, oleksite/olema, olekski/olema (et)</rdfs:comment>
        <rdfs:comment>e.g., БУДЕМ/быть, БУДЕТ/быть, БУДЕТЕ/быть, БУДЕШЬ/быть, БУДУ/быть, БУДУТ/быть, Бежим/бежать, Будет/быть, Будете/быть (ru)</rdfs:comment>
        <rdfs:comment>e.g., бидел/сум, бидела/сум, биделе/сум, бидело/сум, бил/сум, била/сум, биле/сум, било/сум, имал/има (mk)</rdfs:comment>
        <rdfs:comment>e.g., бил/бъда, бил/съм, била/бъда, била/съм, били/бъда, били/съм, било/бъда, било/съм, бъдещ/бъда (bg)</rdfs:comment>
        <rdfs:comment>Voice=&quot;active&quot;&lt;br/&gt;

Macedonian has two types of (adjectival) participles: active and passive. Active corresponds to Macedonian L-form and passive to verbal adjective, neuter gender, singular. For example, nosel is encoded as VForm=Participle, Voice=Active, nosen as VForm=participle, Voice=Passive. (MTE v4)</rdfs:comment>
    </owl:Class>
    


    <!-- http://purl.org/olia/mte/multext-east.owl#AdessiveCase -->

    <owl:Class rdf:about="http://purl.org/olia/mte/multext-east.owl#AdessiveCase">
        <rdfs:subClassOf rdf:resource="http://purl.org/olia/mte/multext-east.owl#Case"/>
        <rdfs:comment>e.g., Baltimaadel/Baltimaad, Kallastel/Kallas, tal/tema, teil/sina, teistel/teine, temal/tema, temalgi/tema, varasematel/varasem, varasematelgi/varasem (et)</rdfs:comment>
        <rdfs:comment>e.g., határátkelőinél/határátkelő, művészeteknél/művész, nálatok/ti, szentjénél/szent, teázásaiknál/teázás, tudósításoknál/tudósítás (hu)</rdfs:comment>
        <rdfs:comment>Case=&quot;adessive&quot; (Estonian, Hungarian)</rdfs:comment>
    </owl:Class>
    


    <!-- http://purl.org/olia/mte/multext-east.owl#AditiveCase -->

    <owl:Class rdf:about="http://purl.org/olia/mte/multext-east.owl#AditiveCase">
        <rdfs:subClassOf rdf:resource="http://purl.org/olia/mte/multext-east.owl#Case"/>
        <rdfs:comment>e.g., esimesse/esimene, kumba/kumb, teineteise, teise/teine, teisegi/teine, üksteise, žurnaali/žurnaal, žurnaalorderisüsteemi/žurnaalorderisüsteem (et)</rdfs:comment>
        <rdfs:comment>Case=&quot;aditive&quot; (Estonian)</rdfs:comment>
    </owl:Class>
    


    <!-- http://purl.org/olia/mte/multext-east.owl#Adjectival -->

    <owl:Class rdf:about="http://purl.org/olia/mte/multext-east.owl#Adjectival">
        <rdfs:subClassOf rdf:resource="http://purl.org/olia/mte/multext-east.owl#SyntacticType"/>
        <rdfs:comment>e.g., cach/kak, chirj/kiri, etej/iti, gni/nji, gnih/njeh, isa/isi, ise/isi, ishtes/ištës, isi/isi (sl-rozaj)</rdfs:comment>
        <rdfs:comment>e.g., ci/ten, czyichkolwiek/czyjkolwiek, czyichś/czyjś, czyimikolwiek/czyjkolwiek, czyimiś/czyjś, czyimkolwiek/czyjkolwiek, czyimś/czyjś, czyjakolwiek/czyjkolwiek, czyjaś/czyjś (pl)</rdfs:comment>
        <rdfs:comment>e.g., ich, jeho, jej, koľkonásobnej/koľkonásobný, koľkonásobného/koľkonásobný, koľkonásobnému/koľkonásobný, koľkorakej/koľkoraký, koľkorakého/koľkoraký, koľkorakému/koľkoraký (sk)</rdfs:comment>
        <rdfs:comment>e.g., jaká/jaký, jaké/jaký, jakého/jaký, jakém/jaký, jakému/jaký, jakých/jaký, jakým/jaký, jakými/jaký, jeho (cs)</rdfs:comment>
        <rdfs:comment>e.g., абичий/= бозна-чий/= будь-чий/= дечий/= хтозна-чий/= чий-будь/= чий-небудь/= чийсь/=, абичийого/абичий аби до чийого/абичий бозна-чийого/бозна-чий будь-чийого/будь-чий дечийого/дечий хтозна-чийого/хтозна-чий чийого-будь/чий-будь чийого-небудь/чий-небудь чийогось/чийсь, абичийого/абичий бозна-чийого/бозна-чий будь-чийого/будь-чий дечийого/дечий хтозна-чийого/хтозна-чий чийого-будь/чий-будь чийого-небудь/чий-небудь чийогось/чийсь, абичийому/абичий абичиєму/абичий абичиїм/абичий аби на чийому/абичий аби на чиєму/абичий аби на чиїм/абичий бозна на чийому/бозна-чий бозна на чиєму/бозна-чий бозна на чиїм/бозна-чий будь-чийому/будь-чий будь-чиєму/будь-чий будь-чиїм/будь-чий будь на чийому/будь-чий будь на чиєму/будь-чий будь на чиїм/будь-чий дечийому/дечий дечиєму/дечий дечиїм/дечий де на чийому/дечий де на чиєму/дечий, абичийому/абичий абичиєму/абичий бозна-чийому/бозна-чий бозна-чиєму/бозна-чий будь-чийому/будь-чий будь-чиєму/будь-чий дечийому/дечий дечиєму/дечий хтозна-чийому/хтозна-чий хтозна-чиєму/хтозна-чий чийому-будь/чий-будь чиєму-будь/чий-будь чийому-небудь/чий-небудь чиєму-небудь/чий-небудь чийомусь/чийсь чиємусь/чийсь, абичийому/абичий абичиєму/абичий бозна-чийому/бозна-чий будь-чийому/будь-чий будь-чиєму/будь-чий дечийому/дечий хтозна-чийому/хтозна-чий чийому-будь/чий-будь чийому-небудь/чий-небудь чийомусь/чийсь, абичию/абичий бозна-чию/бозна-чий будь-чию/будь-чий дечию/дечий хтозна-чию/хтозна-чий чию-будь/чий-будь чию-небудь/чий-небудь чиюсь/чийсь, абичия/абичий бозна-чия/бозна-чий будь-чия/будь-чий дечия/дечий хтозна-чия/хтозна-чий чия-будь/чий-будь чия-небудь/чий-небудь чиясь/чийсь, абичиє/абичий бозна-чиє/бозна-чий будь-чиє/будь-чий дечиє/дечий хтозна-чиє/хтозна-чий чиє-будь/чий-будь чиє-небудь/чий-небудь чиєсь/чийсь (uk)</rdfs:comment>
        <rdfs:comment>Pronoun/Syntactic_Type=&quot;adjectival&quot; (Slavic), Abbreviation/Syntactic_Type=&quot;adjectival&quot;&lt;br/&gt;

Pronouns can be distinguished between having a (syntactically) nominal and (syntactically) adjectival function. All pronominal types except the demonstrative and possessive one can be nominal, and all except for the personal one can be adjectival. (MTE v4)</rdfs:comment>
    </owl:Class>
    


    <!-- http://purl.org/olia/mte/multext-east.owl#AdjectivalAdverb -->

    <owl:Class rdf:about="http://purl.org/olia/mte/multext-east.owl#AdjectivalAdverb">
        <rdfs:subClassOf rdf:resource="http://purl.org/olia/mte/multext-east.owl#Adverb"/>
        <rdfs:comment>Adverb/Type=&quot;adjectival&quot; (Serbian, Macedonian, Bulgarian)&lt;br/&gt;

Bulgarian AdjectivalAdverbs have the same form as adjectives in Gender = neuter, Person = 3, Number = singular. (MTE v4)</rdfs:comment>
    </owl:Class>
    


    <!-- http://purl.org/olia/mte/multext-east.owl#Adjective -->

    <owl:Class rdf:about="http://purl.org/olia/mte/multext-east.owl#Adjective">
        <rdfs:subClassOf rdf:resource="http://purl.org/olia/mte/multext-east.owl#MorphosyntacticCategory"/>
        <rdfs:subClassOf>
            <owl:Class>
                <owl:intersectionOf rdf:parseType="Collection">
                    <owl:Restriction>
                        <owl:onProperty rdf:resource="http://purl.org/olia/mte/multext-east.owl#hasAdjectiveFormation"/>
                        <owl:maxCardinality rdf:datatype="http://www.w3.org/2001/XMLSchema#nonNegativeInteger">1</owl:maxCardinality>
                    </owl:Restriction>
                    <owl:Restriction>
                        <owl:onProperty rdf:resource="http://purl.org/olia/mte/multext-east.owl#hasAnimacy"/>
                        <owl:maxCardinality rdf:datatype="http://www.w3.org/2001/XMLSchema#nonNegativeInteger">1</owl:maxCardinality>
                    </owl:Restriction>
                    <owl:Restriction>
                        <owl:onProperty rdf:resource="http://purl.org/olia/mte/multext-east.owl#hasCase"/>
                        <owl:maxCardinality rdf:datatype="http://www.w3.org/2001/XMLSchema#nonNegativeInteger">1</owl:maxCardinality>
                    </owl:Restriction>
                    <owl:Restriction>
                        <owl:onProperty rdf:resource="http://purl.org/olia/mte/multext-east.owl#hasClitic"/>
                        <owl:maxCardinality rdf:datatype="http://www.w3.org/2001/XMLSchema#nonNegativeInteger">1</owl:maxCardinality>
                    </owl:Restriction>
                    <owl:Restriction>
                        <owl:onProperty rdf:resource="http://purl.org/olia/mte/multext-east.owl#hasDefiniteness"/>
                        <owl:maxCardinality rdf:datatype="http://www.w3.org/2001/XMLSchema#nonNegativeInteger">1</owl:maxCardinality>
                    </owl:Restriction>
                    <owl:Restriction>
                        <owl:onProperty rdf:resource="http://purl.org/olia/mte/multext-east.owl#hasDegree"/>
                        <owl:maxCardinality rdf:datatype="http://www.w3.org/2001/XMLSchema#nonNegativeInteger">1</owl:maxCardinality>
                    </owl:Restriction>
                    <owl:Restriction>
                        <owl:onProperty rdf:resource="http://purl.org/olia/mte/multext-east.owl#hasGender"/>
                        <owl:maxCardinality rdf:datatype="http://www.w3.org/2001/XMLSchema#nonNegativeInteger">1</owl:maxCardinality>
                    </owl:Restriction>
                    <owl:Restriction>
                        <owl:onProperty rdf:resource="http://purl.org/olia/mte/multext-east.owl#hasNumber"/>
                        <owl:maxCardinality rdf:datatype="http://www.w3.org/2001/XMLSchema#nonNegativeInteger">1</owl:maxCardinality>
                    </owl:Restriction>
                </owl:intersectionOf>
            </owl:Class>
        </rdfs:subClassOf>
        <rdfs:subClassOf>
            <owl:Class>
                <owl:intersectionOf rdf:parseType="Collection">
                    <owl:Restriction>
                        <owl:onProperty rdf:resource="http://purl.org/olia/mte/multext-east.owl#hasAspect"/>
                        <owl:maxCardinality rdf:datatype="http://www.w3.org/2001/XMLSchema#nonNegativeInteger">1</owl:maxCardinality>
                    </owl:Restriction>
                    <owl:Restriction>
                        <owl:onProperty rdf:resource="http://purl.org/olia/mte/multext-east.owl#hasHumanness"/>
                        <owl:maxCardinality rdf:datatype="http://www.w3.org/2001/XMLSchema#nonNegativeInteger">1</owl:maxCardinality>
                    </owl:Restriction>
                    <owl:Restriction>
                        <owl:onProperty rdf:resource="http://purl.org/olia/mte/multext-east.owl#hasNegation"/>
                        <owl:maxCardinality rdf:datatype="http://www.w3.org/2001/XMLSchema#nonNegativeInteger">1</owl:maxCardinality>
                    </owl:Restriction>
                    <owl:Restriction>
                        <owl:onProperty rdf:resource="http://purl.org/olia/mte/multext-east.owl#hasOwnedNumber"/>
                        <owl:maxCardinality rdf:datatype="http://www.w3.org/2001/XMLSchema#nonNegativeInteger">1</owl:maxCardinality>
                    </owl:Restriction>
                    <owl:Restriction>
                        <owl:onProperty rdf:resource="http://purl.org/olia/mte/multext-east.owl#hasOwnerNumber"/>
                        <owl:maxCardinality rdf:datatype="http://www.w3.org/2001/XMLSchema#nonNegativeInteger">1</owl:maxCardinality>
                    </owl:Restriction>
                    <owl:Restriction>
                        <owl:onProperty rdf:resource="http://purl.org/olia/mte/multext-east.owl#hasOwnerPerson"/>
                        <owl:maxCardinality rdf:datatype="http://www.w3.org/2001/XMLSchema#nonNegativeInteger">1</owl:maxCardinality>
                    </owl:Restriction>
                    <owl:Restriction>
                        <owl:onProperty rdf:resource="http://purl.org/olia/mte/multext-east.owl#hasTense"/>
                        <owl:maxCardinality rdf:datatype="http://www.w3.org/2001/XMLSchema#nonNegativeInteger">1</owl:maxCardinality>
                    </owl:Restriction>
                    <owl:Restriction>
                        <owl:onProperty rdf:resource="http://purl.org/olia/mte/multext-east.owl#hasVoice"/>
                        <owl:maxCardinality rdf:datatype="http://www.w3.org/2001/XMLSchema#nonNegativeInteger">1</owl:maxCardinality>
                    </owl:Restriction>
                </owl:intersectionOf>
            </owl:Class>
        </rdfs:subClassOf>
        <rdfs:comment>e.g., -, bensőnkben/benső, borúlátónkat/borúlátó, buktatóin/buktató, csigaformákba/csigaformá, derekukkal/derék, derekukra/derék, dolgozóiból/dolgozó, dolgozójukba/dolgozó (hu)</rdfs:comment>
        <rdfs:comment>e.g., -ntrebătoare/întrebător, -ntregi/întreg, -ntreprinzătoare/întreprinzător, -nvăluitoare/învăluitor, -nzestrata/înzestrat, -nzestrate/înzestrat, -nzestratei/înzestrat, -nzestratele/înzestrat, -nzestratelor/înzestrat (ro)</rdfs:comment>
        <rdfs:comment>e.g., 0, Абакумів/= Абрамів/= Авакумів/= Августин/= Августинів/= Августів/= Авенірів/= Аверкіїв/= Авер&apos;янів/= Авіятин/= Авксентіїв/= Аврамів/= Авреліїн/= Аврорин/= Автономів/= авторів/= авторчин/= Агапіїв/= Агапіїн/= Агапітів/=, абеткована/абеткований авізована/авізований акомпанована/акомпанований актована/актований аналізована/аналізований анкетована/анкетований анодована/анодований артикульована/артикульований балотована/балотований балувана/балуваний бальзамована/бальзамований банітована/банітований багнітована/багнітований байцьована/байцьований балакана/балаканий бачена/бачений белетризована/белетризований бережена/бережений бетонована/бетонований бинтована/бинтований, абеткованая/абеткований авізованая/авізований акомпанованая/акомпанований актованая/актований аналізованая/аналізований анкетованая/анкетований анодованая/анодований артикульованая/артикульований балотованая/балотований балуваная/балуваний бальзамованая/бальзамований банітованая/банітований багнітованая/багнітований байцьованая/байцьований балаканая/балаканий баченая/бачений белетризованая/белетризований береженая/бережений бетонованая/бетонований бинтованая/бинтований, абетковане/абеткований авізоване/авізований акомпановане/акомпанований актоване/актований аналізоване/аналізований анкетоване/анкетований анодоване/анодований артикульоване/артикульований балотоване/балотований балуване/балуваний бальзамоване/бальзамований банітоване/банітований багнітоване/багнітований байцьоване/байцьований балакане/балаканий бачене/бачений белетризоване/белетризований бережене/бережений бетоноване/бетонований бинтоване/бинтований, абеткованеє/абеткований авізованеє/авізований акомпанованеє/акомпанований актованеє/актований аналізованеє/аналізований анкетованеє/анкетований анодованеє/анодований артикульованеє/артикульований балотованеє/балотований балуванеє/балуваний бальзамованеє/бальзамований банітованеє/банітований багнітованеє/багнітований байцьованеє/байцьований балаканеє/балаканий баченеє/бачений белетризованеє/белетризований береженеє/бережений бетонованеє/бетонований бинтованеє/бинтований, абеткований/= авізований/= акомпанований/= актований/= аналізований/= анкетований/= анодований/= артикульований/= балотований/= балуваний/= бальзамований/= банітований/= багнітований/= байцьований/= балаканий/= бачений/= белетризований/= бережений/= бетонований/= бинтований/=, абеткованим/абеткований авізованим/авізований акомпанованим/акомпанований актованим/актований аналізованим/аналізований анкетованим/анкетований анодованим/анодований артикульованим/артикульований балотованим/балотований балуваним/балуваний бальзамованим/бальзамований банітованим/банітований багнітованим/багнітований байцьованим/байцьований балаканим/балаканий баченим/бачений белетризованим/белетризований береженим/бережений бетонованим/бетонований бинтованим/бинтований, абеткованими/абеткований авізованими/авізований акомпанованими/акомпанований актованими/актований аналізованими/аналізований анкетованими/анкетований анодованими/анодований артикульованими/артикульований балотованими/балотований балуваними/балуваний бальзамованими/бальзамований банітованими/банітований багнітованими/багнітований байцьованими/байцьований балаканими/балаканий баченими/бачений белетризованими/белетризований береженими/бережений бетонованими/бетонований бинтованими/бинтований (uk)</rdfs:comment>
        <rdfs:comment>e.g., Weberovi/Weberův, Wertherovi/Wertherův, Winstonovi/Winstonův (cs)</rdfs:comment>
        <rdfs:comment>e.g., abdykujący/abdykować, adoptujących/adoptować, akceptowanymi/akceptować, akredytujące/akredytować, akredytujących/akredytować, akredytującą/akredytować, amerykański/amerykański, amerykańskiej/amerykański, amerykańskim/amerykański (pl)</rdfs:comment>
        <rdfs:comment>e.g., aktuaalseimatesse/aktuaalseim, kiireimale/kiireim, kõrgeimale/kõrgeim, parematelt/parem, parimail/parim, parimale/parim, parimalt/parim, parimana/parim, parimateks/parim (et)</rdfs:comment>
        <rdfs:comment>e.g., belim/beo, bezbrojnih/bezbrojni, crnobrko/crnobrki, devetogodišnji, druge/drugi, evroazijske/evroazijska, evroazijskih/evroazijski, evroazijskog/evroazijski, Faroskih/Faroska (sr)</rdfs:comment>
        <rdfs:comment>e.g., blishgnaha/blïžnji, Bohavei/böguw, Bohouv/böguw, Bohovaha/böguw, Bohove/böguw, Bohovih/böguw, Bohovij/böguw, Bohovin/böguw, Bohuvin/böguw (sl-rozaj)</rdfs:comment>
        <rdfs:comment>e.g., blishgnaha/blïžnji, božjega/böžji, kunvirtínaga/kunvirten, sladkega/sladak, tulstaga/tulst, túlstaga/tulst (sl-rozaj)</rdfs:comment>
        <rdfs:comment>e.g., brillská/brillský, nejubožejšími/ubohý, nejvyspělejších/vyspělý, nejvyšších/vysoký, nejvznešenějšímu/vznešený, nejvážnějšímu/vážný, nejvýznamnějších/významný, nejvýznamnějšími/významný, nejvýznamnějšímu/významný (cs)</rdfs:comment>
        <rdfs:comment>e.g., chorego/chory, debiutującego/debiutować, debiutujący/debiutować, interweniującego/interweniować, interweniujący/interweniować, interweniujących/interweniować, kierowani/kierować, lepszego/dobry, lepszych/dobry (pl)</rdfs:comment>
        <rdfs:comment>e.g., devetogodišnji, mlađa/mlad, najbigotnije/bigotan, nepokorne/nepokoran, nerođene/nerođen, neustrašivi/neustrašiv, O&apos;Brajenov, premanjeg/premali, premanjega/premali (sr)</rdfs:comment>
        <rdfs:comment>e.g., dušikovima/dušikov, Marsovi/Marsov, največja/velik, največji/velik, navedenih/naveden, slabša/slab, večjih/velik (sl)</rdfs:comment>
        <rdfs:comment>e.g., najžoviálnejšej/žoviálny, najžoviálnejšia/žoviálny, najžoviálnejšie/žoviálny, najžoviálnejšieho/žoviálny, najžoviálnejšiemu/žoviálny, najžoviálnejšiu/žoviálny, najžoviálnejšom/žoviálny, najžoviálnejšou/žoviálny, najžoviálnejší/žoviálny (sk)</rdfs:comment>
        <rdfs:comment>e.g., Чертова/чертовый, Швейцарских/швейцарский, Язвительно/язвительный, га, микро, участковым/участковый, фен, форсированным/форсированный, частным/частный (ru)</rdfs:comment>
        <rdfs:comment>e.g., најшпионска/шпионски, најшпионскава/шпионски, најшпионскана/шпионски, најшпионската/шпионски, најшпионски/шпионски, најшпионскиве/шпионски, најшпионскине/шпионски, најшпионскиов/шпионски, најшпионскион/шпионски (mk)</rdfs:comment>
        <rdfs:comment>e.g., щастливият/щастлив, югославският/югославски, юношеският/юношески (bg)</rdfs:comment>
        <rdfs:comment>e.g., بلندتري/بلند انساني‌تري/انساني‌ آرام‌تري/آرام, تازه تار بسيج, رنگيِ/رنگي بي‌امانِ/بي‌امان بوکسورمانندِ/بوکسورمانند, زنگداري/زنگدار تهوع‌آوري/تهوع‌آور برهنه‌اي/برهنه, سرگرمِ/سرگرم روانهٔ/روانه حاويِ/حاوي, قوي‌ترِ/قوي بيشترِ/بيش اعظمِ/اعظم, متعصّب‌ترين/متعصّب قديمي‌ترين/قديمي ترسناک‌ترين/ترسناک, مطمئن‌تر/مطمئن عاقلانه‌تر/عاقلانه بدبوتر/بدبو, موذي عاري سبيلو (fa)</rdfs:comment>
        <rdfs:comment>For some MTE languages, Adjective also includes adjectival participles (Ukrainian), adverbs in certain positions (Macedonian mnogu, malku, nekolku are also considered adjectives in cases they are used before nouns, because they can have definiteness in their inflectional paradigm), and pronominal forms (Resian &apos;swöj&apos; / own is considered an adjective, not a pronoun).</rdfs:comment>
    </owl:Class>
    


    <!-- http://purl.org/olia/mte/multext-east.owl#AdjectiveFormation -->

    <owl:Class rdf:about="http://purl.org/olia/mte/multext-east.owl#AdjectiveFormation">
        <owl:equivalentClass rdf:resource="http://purl.org/olia/mte/multext-east.owl#ReductionFeature"/>
        <rdfs:subClassOf rdf:resource="http://purl.org/olia/mte/multext-east.owl#Formation"/>
        <rdfs:comment>Adjective with feature &quot;Formation&quot;&lt;br/&gt;

The Formation attribute distinguishes a nominal (short) form from a so-called compound (long) form of an Adjective in Czech. The nominal form can be used in the predicative function only. It is specified for nominative and accusative Case only. (MTE v4)

This corresponds to the use of Definiteness (i.e., ReductionFeature) for Polish.</rdfs:comment>
    </owl:Class>
    


    <!-- http://purl.org/olia/mte/multext-east.owl#Adposition -->

    <owl:Class rdf:about="http://purl.org/olia/mte/multext-east.owl#Adposition">
        <rdfs:subClassOf rdf:resource="http://purl.org/olia/mte/multext-east.owl#MorphosyntacticCategory"/>
        <rdfs:subClassOf>
            <owl:Class>
                <owl:intersectionOf rdf:parseType="Collection">
                    <owl:Restriction>
                        <owl:onProperty rdf:resource="http://purl.org/olia/mte/multext-east.owl#hasAdpositionFormation"/>
                        <owl:maxCardinality rdf:datatype="http://www.w3.org/2001/XMLSchema#nonNegativeInteger">1</owl:maxCardinality>
                    </owl:Restriction>
                    <owl:Restriction>
                        <owl:onProperty rdf:resource="http://purl.org/olia/mte/multext-east.owl#hasCase"/>
                        <owl:maxCardinality rdf:datatype="http://www.w3.org/2001/XMLSchema#nonNegativeInteger">1</owl:maxCardinality>
                    </owl:Restriction>
                    <owl:Restriction>
                        <owl:onProperty rdf:resource="http://purl.org/olia/mte/multext-east.owl#hasClitic"/>
                        <owl:maxCardinality rdf:datatype="http://www.w3.org/2001/XMLSchema#nonNegativeInteger">1</owl:maxCardinality>
                    </owl:Restriction>
                </owl:intersectionOf>
            </owl:Class>
        </rdfs:subClassOf>
        <rdfs:comment>e.g., -mpotriva/împotriva, -naintea/înaintea, asupră/asupra (ro)</rdfs:comment>
        <rdfs:comment>e.g., a незважаючи/=, без біля близько в вві взамін вздовж від вколо внаслідок для до з задля замість заради зверх зверху звиш здовж, в за крізь меж межи на над невважаючи незважаючи о об перед під по повз поза поміж понад понадо поперед, в на о по попри при у ув уві, всупереч завдяки противно уздогін усупереч, з за із меж межи над наді надо перед передо під підо поза помежи поміж понад понадо поперед попід пред, за те за тим з-від з-за з-між з-навпроти з-над з-перед з-під з-поверхні з-поза з-позад з-позаду з-поміж з-понад з-поперед з-попід з-посеред з-проміж з-серед, згідно з, на противагу (uk)</rdfs:comment>
        <rdfs:comment>e.g., dardu/dardu, h/h, na/na, od/od, ot/od, par/par, per/par, po/po, prid/prid (sl-rozaj)</rdfs:comment>
        <rdfs:comment>e.g., dla/dla, do/do, dzięki/dzięki, ku/ku, między/między, na/na, nad/nad, o/o, od/od (pl)</rdfs:comment>
        <rdfs:comment>e.g., از‌لايِ/ازلا ازلحاظِ/ازلحاظ ازجانبِ/ازجانب, و/را رو/را را, پشتِ‌سر طي طرفِ/طرف (fa)</rdfs:comment>
    </owl:Class>
    


    <!-- http://purl.org/olia/mte/multext-east.owl#AdpositionFormation -->

    <owl:Class rdf:about="http://purl.org/olia/mte/multext-east.owl#AdpositionFormation">
        <rdfs:subClassOf rdf:resource="http://purl.org/olia/mte/multext-east.owl#Formation"/>
        <rdfs:comment>Adposition/Formation

Czech: A preposition can be contracted with a pronoun; such a preposition has Formation=c(ompound). (MTE v4)</rdfs:comment>
    </owl:Class>
    


    <!-- http://purl.org/olia/mte/multext-east.owl#Adverb -->

    <owl:Class rdf:about="http://purl.org/olia/mte/multext-east.owl#Adverb">
        <rdfs:subClassOf rdf:resource="http://purl.org/olia/mte/multext-east.owl#MorphosyntacticCategory"/>
        <rdfs:subClassOf>
            <owl:Class>
                <owl:intersectionOf rdf:parseType="Collection">
                    <owl:Restriction>
                        <owl:onProperty rdf:resource="http://purl.org/olia/mte/multext-east.owl#hasCase"/>
                        <owl:maxCardinality rdf:datatype="http://www.w3.org/2001/XMLSchema#nonNegativeInteger">1</owl:maxCardinality>
                    </owl:Restriction>
                    <owl:Restriction>
                        <owl:onProperty rdf:resource="http://purl.org/olia/mte/multext-east.owl#hasClitic"/>
                        <owl:maxCardinality rdf:datatype="http://www.w3.org/2001/XMLSchema#nonNegativeInteger">1</owl:maxCardinality>
                    </owl:Restriction>
                    <owl:Restriction>
                        <owl:onProperty rdf:resource="http://purl.org/olia/mte/multext-east.owl#hasDegree"/>
                        <owl:maxCardinality rdf:datatype="http://www.w3.org/2001/XMLSchema#nonNegativeInteger">1</owl:maxCardinality>
                    </owl:Restriction>
                    <owl:Restriction>
                        <owl:onProperty rdf:resource="http://purl.org/olia/mte/multext-east.owl#hasNumber"/>
                        <owl:maxCardinality rdf:datatype="http://www.w3.org/2001/XMLSchema#nonNegativeInteger">1</owl:maxCardinality>
                    </owl:Restriction>
                    <owl:Restriction>
                        <owl:onProperty rdf:resource="http://purl.org/olia/mte/multext-east.owl#hasPerson"/>
                        <owl:maxCardinality rdf:datatype="http://www.w3.org/2001/XMLSchema#nonNegativeInteger">1</owl:maxCardinality>
                    </owl:Restriction>
                    <owl:Restriction>
                        <owl:onProperty rdf:resource="http://purl.org/olia/mte/multext-east.owl#hasWHType"/>
                        <owl:maxCardinality rdf:datatype="http://www.w3.org/2001/XMLSchema#nonNegativeInteger">1</owl:maxCardinality>
                    </owl:Restriction>
                </owl:intersectionOf>
            </owl:Class>
        </rdfs:subClassOf>
        <rdfs:comment>e.g., better (en)</rdfs:comment>
        <rdfs:comment>e.g., itu/ito (sl-rozaj)</rdfs:comment>
        <rdfs:comment>e.g., prostu/prosty (pl)</rdfs:comment>
        <rdfs:comment>e.g., to&apos;/tot (ro)</rdfs:comment>
        <rdfs:comment>e.g., zárásaként/zárás, záróakkordjaként/záróakkord, zászlóként/zászló (hu)</rdfs:comment>
        <rdfs:comment>Adverb and Adjective overlap, and in MTE v4, different language-specific resolution strategies are applied:
Polish post-prepositional adjectives like (po) polsku are treated as adverbs, Macedonian pre-nominal adverbs like mnogu, malku, nekolku are considered adjectives (like adjectives, they can have definiteness in their inflectional paradigm).

Also, definitions for Adverb and Particle may overlap, see Adverb/Type=&quot;particle&quot; as used for Hungarian and Romanian MTE v4. In Slovak MTE v4, however, Particles form a separate part of speech category as is customary in Slovak grammars.

As for the overlap between Adverb and Conjunction, Adverb/Type=&quot;portmanteau&quot; was introduced for Romanian to cover some few words which can be both adverbs and conjunctions (with adverbial reading more frequent). Romanian Conjunction/Type=&quot;portmanteau&quot; applies only to the word &quot;şi&quot; which can be both a coordonating conjunction and an adverb. The distinctionamong these interpretations is rather tricky for the average native speaker and was a constant source of noise in automatic tagging. Therefore, for the sake of automatic processing we defined this &quot;portmanteau&quot; type value. (MTE v4)</rdfs:comment>
    </owl:Class>
    


    <!-- http://purl.org/olia/mte/multext-east.owl#Adverbial -->

    <owl:Class rdf:about="http://purl.org/olia/mte/multext-east.owl#Adverbial">
        <rdfs:subClassOf rdf:resource="http://purl.org/olia/mte/multext-east.owl#SyntacticType"/>
        <rdfs:comment>e.g., dlatego/dlatego, tam/tam, tu/tu (pl)</rdfs:comment>
        <rdfs:comment>Pronoun/Syntactic_Type=&quot;adverbial&quot; (Polish, Serbian, Russian, Ukrainian), Abbreviation/Syntactic_Type=&quot;adverbial&quot;</rdfs:comment>
    </owl:Class>
    


    <!-- http://purl.org/olia/mte/multext-east.owl#AffirmativeParticle -->

    <owl:Class rdf:about="http://purl.org/olia/mte/multext-east.owl#AffirmativeParticle">
        <rdfs:subClassOf rdf:resource="http://purl.org/olia/mte/multext-east.owl#Particle"/>
        <rdfs:comment>Particle/Type=&quot;affirmative&quot;</rdfs:comment>
    </owl:Class>
    


    <!-- http://purl.org/olia/mte/multext-east.owl#AgglutinantClitic -->

    <owl:Class rdf:about="http://purl.org/olia/mte/multext-east.owl#AgglutinantClitic">
        <rdfs:subClassOf rdf:resource="http://purl.org/olia/mte/multext-east.owl#CliticElement"/>
        <rdfs:comment>e.g., em/być, eś/być, ideowo/ideowy, m/być, niej/ona, polsko/polski, społeczno/społeczny, ń/on, ś/być (pl)</rdfs:comment>
        <rdfs:comment>Clitic=&quot;agglutinant&quot; (Verb, Pronoun: Polish)&lt;br/&gt;

Polish: The agglutination phenomenon in Polish is similar to Czech clitic_s for pronouns, but has a wider scope and can be found in more parts of speech. It is encoded as a more general &quot;Clitic(y/n/a/d)&quot; attribute and is specified, e.g., for the indicative VForm with Tense=pa(s)t, corresponding to &quot;praet&quot; flexeme in the IPIC to differentiate between forms like gniótł (clitic=&quot;n&quot;) and gniotł- (clitic=&quot;d&quot;), where the latter not only demands a clitic but also has different form. The value &quot;(a)gglutinant&quot; indicates the clitic itself, e.g., -em in gniotłem. Values &quot;y&quot; and &quot;n&quot; are left to enable showing that a graphical word, i.e., delimited by white spaces, is a combination of a (d)emanding (or free) segment and an (a)gglutinant in case the word segmentation should be revised in the future.
Prepositionality is encoded as Clitic with values &quot;y(es)&quot; for nią, niego etc., &quot;n(o)&quot; for ją, go etc., &quot;a(gglutinant)&quot; for -ń. Cf. the Clitic value &quot;bound&quot; for Slovene pronouns like zate which refers to the whole cluster, formally a combination of a preposition and a pronoun. This coding can be used for similar phenomena in Polish, e.g dlań (for him), given the word segmentation is revised towards a more trraditional one.</rdfs:comment>
    </owl:Class>
    


    <!-- http://purl.org/olia/mte/multext-east.owl#AllativeCase -->

    <owl:Class rdf:about="http://purl.org/olia/mte/multext-east.owl#AllativeCase">
        <rdfs:subClassOf rdf:resource="http://purl.org/olia/mte/multext-east.owl#Case"/>
        <rdfs:comment>e.g., -, ahhoz/az, akikhez/aki, amelyekhez/amely, betegségedhez/betegség, cilindereikhez/cilinder, csődhöz/cső, egymáshoz/egymás, ehhez/ez (hu)</rdfs:comment>
        <rdfs:comment>e.g., endile/ise, esimestele/esimene, iseendile/iseenese, Kallastele/Kallas, kellele/kes, kiireimale/kiireim, kõrgeimale/kõrgeim, meile/mina, meilegi/mina (et)</rdfs:comment>
        <rdfs:comment>Case=&quot;allative&quot; (Estonian, Hungarian)</rdfs:comment>
    </owl:Class>
    


    <!-- http://purl.org/olia/mte/multext-east.owl#AmbiguousAdjective -->

    <owl:Class rdf:about="http://purl.org/olia/mte/multext-east.owl#AmbiguousAdjective">
        <rdfs:subClassOf rdf:resource="http://purl.org/olia/mte/multext-east.owl#Adjective"/>
        <rdfs:comment>Adjective subcategories that refer to different phenomena in different languages</rdfs:comment>
    </owl:Class>
    


    <!-- http://purl.org/olia/mte/multext-east.owl#AmbiguousCliticness -->

    <owl:Class rdf:about="http://purl.org/olia/mte/multext-east.owl#AmbiguousCliticness">
        <rdfs:subClassOf rdf:resource="http://purl.org/olia/mte/multext-east.owl#Cliticness"/>
        <owl:versionInfo>MTE feature values that fall in more than one of the devised classes. I suggest to distangle such ambiguities in forthcoming versions of Multext/East. (Ch. Chiarcos)</owl:versionInfo>
    </owl:Class>
    


    <!-- http://purl.org/olia/mte/multext-east.owl#AmbiguousDefinitenessFeature -->

    <owl:Class rdf:about="http://purl.org/olia/mte/multext-east.owl#AmbiguousDefinitenessFeature">
        <rdfs:subClassOf rdf:resource="http://purl.org/olia/mte/multext-east.owl#Definiteness"/>
    </owl:Class>
    


    <!-- http://purl.org/olia/mte/multext-east.owl#Animacy -->

    <owl:Class rdf:about="http://purl.org/olia/mte/multext-east.owl#Animacy">
        <rdfs:subClassOf rdf:resource="http://purl.org/olia/mte/multext-east.owl#MorphosyntacticFeature"/>
    </owl:Class>
    


    <!-- http://purl.org/olia/mte/multext-east.owl#Animate -->

    <owl:Class rdf:about="http://purl.org/olia/mte/multext-east.owl#Animate">
        <rdfs:subClassOf rdf:resource="http://purl.org/olia/mte/multext-east.owl#Animacy"/>
        <rdfs:comment>e.g., 0, Абакуми/Абакум Абакумовичі/Абакумович Аббаси/Аббас Абдули/Абдула Абелі/Абель Абовяни/Абовян Абрами/Абрам Абрамовичі/Абрамович Абрамовичі/Абрамович Абрамчуки/Абрамчук Авакуми/Авакум Авакумовичі/Авакумович Августи/Август Августини/Августин Августиновичі/Августинович Августиновичі/Августинович Августовичі/Августович Авелі/Авель Авенаріуси/Авенаріус Авеніри/Авенір, Антропов/= Абай/= Абакум/= Абакумович/= Абалкін/= Абашидзе/= Аббас/= Абдула/= Абдуллоджанов/= Абель/= Абовян/= Абрам/= Абрамович/= Абрамович/= Абрамчук/= Абуладзе/= Авакум/= Авакумович/= Август/= Августимов/=, Антропова/Антропов Абакумівна/= Абалкіна/Абалкін Абашидзе/= Абдуллоджанова/Абдуллоджанов Абрамівна/= Абуладзе/= Авакумівна/= Августа/= Августимова/Августимов Августинівна/= Авдієвська/Авдієвський Авенірівна/= Аверіна/Аверін Аверкіївна/= Авер&apos;янівна/= Авіята/= Авксентіївна/= Авогадро/= Аврамівна/=, Антропова/Антропов Абакумівно/Абакумівна Абалкіна/Абалкін Абашидзе/= Абдуллоджанова/Абдуллоджанов Абрамівно/Абрамівна Абуладзе/= Авакумівно/Авакумівна Августо/Августа Августимова/Августимов Августинівно/Августинівна Авдієвська/Авдієвський Авенірівно/Авенірівна Аверіна/Аверін Аверкіївно/Аверкіївна Авер&apos;янівно/Авер&apos;янівна Авіято/Авіята Авксентіївно/Авксентіївна Авогадро/= Аврамівно/Аврамівна, Антропова/Антропов Абая/Абай Абакума/Абакум Абакумовича/Абакумович Абалкіна/Абалкін Абашидзе/= Аббаса/Аббас Абдули/Абдула Абдуллоджанова/Абдуллоджанов Абеля/Абель Абовяна/Абовян Абрама/Абрам Абрамовича/Абрамович Абрамовича/Абрамович Абрамчука/Абрамчук Абуладзе/= Авакума/Авакум Авакумовича/Авакумович Августа/Август Августимова/Августимов, Антропова/Антропов Абая/Абай Абакума/Абакум Абакумовича/Абакумович Абалкіна/Абалкін Абашидзе/= Аббаса/Аббас Абдулу/Абдула Абдуллоджанова/Абдуллоджанов Абеля/Абель Абовяна/Абовян Абрама/Абрам Абрамовича/Абрамович Абрамовича/Абрамович Абрамчука/Абрамчук Абуладзе/= Авакума/Авакум Авакумовича/Авакумович Августа/Август Августимова/Августимов, Антропове/Антропов Антропов/= Абаю/Абай Абакуме/Абакум Абакумовичу/Абакумович Абалкіне/Абалкін Абалкін/= Абашидзе/= Аббасе/Аббас Абдуло/Абдула Абдуллоджанове/Абдуллоджанов Абдуллоджанов/= Абелю/Абель Абель/= Абовяне/Абовян Абовян/= Абраме/Абрам Абрамовичу/Абрамович Абрамовичу/Абрамович Абрамович/=, Антропови/Антропов Абакуми/Абакум Абакумовичі/Абакумович Абалкіни/Абалкін Абашидзе/= Аббаси/Аббас Абдули/Абдула Абдуллоджанови/Абдуллоджанов Абелі/Абель Абовяни/Абовян Абрами/Абрам Абрамовичі/Абрамович Абрамовичі/Абрамович Абрамчуки/Абрамчук Абуладзе/= Авакуми/Авакум Авакумовичі/Авакумович Августи/Август Августимови/Августимов Августини/Августин (uk)</rdfs:comment>
        <rdfs:comment>e.g., druhom/druhý, druhého/druhý, druhému/druhý, druhí/druhý, druhý, druhých/druhý, druhým/druhý, druhými/druhý, dvaja/dva (sk)</rdfs:comment>
        <rdfs:comment>Animate=&quot;yes&quot; (Slavic Noun, Pronoun; Czech verb)&lt;br/&gt;

Slovak (like most other Slavic languages) distinguishes masculine animate (Animate=&quot;yes&quot;) and masculine inanimate (Animate=&quot;no&quot;) gender. Masculine inanimate nouns always have the same form in the nominative and accusative case, whereas masculine animate nouns have predominantly the same form in the genitive and accusative case. Masculine animate nouns and masculine inanimate nouns differ in accusative singular, nominative (vocative) and accusative plural only (Slovak MTE v4). In Resian, Animacy can also be marked on neuter singular accusative Nouns. The feminine declension masculine noun has only one Ncmsa, that is marked as animate: oćo / father is Ncmsa--y. (Resian MTE v4).

</rdfs:comment>
    </owl:Class>
    


    <!-- http://purl.org/olia/mte/multext-east.owl#AoristTense -->

    <owl:Class rdf:about="http://purl.org/olia/mte/multext-east.owl#AoristTense">
        <rdfs:subClassOf rdf:resource="http://purl.org/olia/mte/multext-east.owl#Tense"/>
        <rdfs:comment>e.g., bi&apos;/biti, bi/biti, bih/biti, bismo/biti, biste/biti, biše/biti, će/hteti (sr)</rdfs:comment>
        <rdfs:comment>e.g., bè/bet, bé/bet, bě/bet, idu/tet, nalese/nalëst, povi/puvet (sl-rozaj)</rdfs:comment>
        <rdfs:comment>e.g., бе/съм, би/бъда, бил/бъда, бил/съм, била/бъда, била/съм, били/бъда, били/съм, било/бъда (bg)</rdfs:comment>
        <rdfs:comment>e.g., могоа/може, могов/може, моговме/може, моговте/може, може, недоспаа/недоспие, недоспав/недоспие, недоспавме/недоспие, недоспавте/недоспие (mk)</rdfs:comment>
        <rdfs:comment>In Bulgarian, there is a language specific Tense=&quot;aorist&quot; value for the Tense attribute. Past perfect tense “aorist” expresses a past action (event) carried out or completed in a given moment or during a given period and finished before the state of speaking. (Dimitrova et al. 2009)&lt;br/&gt;

In Resian, the aorist is encountered sporadically in historical texts only. (MTE v4)
</rdfs:comment>
    </owl:Class>
    


    <!-- http://purl.org/olia/mte/multext-east.owl#ApproximateNumeral -->

    <owl:Class rdf:about="http://purl.org/olia/mte/multext-east.owl#ApproximateNumeral">
        <rdfs:subClassOf rdf:resource="http://purl.org/olia/mte/multext-east.owl#MorphologicalFormOfNumeral"/>
        <rdfs:comment>Bulgarian has Numeral/Form=approx(a), used for approximate numerals (десетина /about a ten/, стотина /about a hundred/) (Dimitrova et al. 2009)
</rdfs:comment>
        <owl:versionInfo>Form=&quot;approx&quot; (Bulgarian MTE)</owl:versionInfo>
    </owl:Class>
    


    <!-- http://purl.org/olia/mte/multext-east.owl#Article -->

    <owl:Class rdf:about="http://purl.org/olia/mte/multext-east.owl#Article">
        <rdfs:subClassOf rdf:resource="http://purl.org/olia/mte/multext-east.owl#MorphosyntacticCategory"/>
        <rdfs:subClassOf>
            <owl:Class>
                <owl:intersectionOf rdf:parseType="Collection">
                    <owl:Restriction>
                        <owl:onProperty rdf:resource="http://purl.org/olia/mte/multext-east.owl#hasAnimacy"/>
                        <owl:maxCardinality rdf:datatype="http://www.w3.org/2001/XMLSchema#nonNegativeInteger">1</owl:maxCardinality>
                    </owl:Restriction>
                    <owl:Restriction>
                        <owl:onProperty rdf:resource="http://purl.org/olia/mte/multext-east.owl#hasCase"/>
                        <owl:maxCardinality rdf:datatype="http://www.w3.org/2001/XMLSchema#nonNegativeInteger">1</owl:maxCardinality>
                    </owl:Restriction>
                    <owl:Restriction>
                        <owl:onProperty rdf:resource="http://purl.org/olia/mte/multext-east.owl#hasClitic"/>
                        <owl:maxCardinality rdf:datatype="http://www.w3.org/2001/XMLSchema#nonNegativeInteger">1</owl:maxCardinality>
                    </owl:Restriction>
                    <owl:Restriction>
                        <owl:onProperty rdf:resource="http://purl.org/olia/mte/multext-east.owl#hasGender"/>
                        <owl:maxCardinality rdf:datatype="http://www.w3.org/2001/XMLSchema#nonNegativeInteger">1</owl:maxCardinality>
                    </owl:Restriction>
                    <owl:Restriction>
                        <owl:onProperty rdf:resource="http://purl.org/olia/mte/multext-east.owl#hasNumber"/>
                        <owl:maxCardinality rdf:datatype="http://www.w3.org/2001/XMLSchema#nonNegativeInteger">1</owl:maxCardinality>
                    </owl:Restriction>
                </owl:intersectionOf>
            </owl:Class>
        </rdfs:subClassOf>
        <rdfs:comment>e.g., -a, -al/al, -i, -ilor, -ist, -iste, -istei, -istele, -istelor (ro)</rdfs:comment>
        <rdfs:comment>e.g., -a, -i, -ilor, -ist, -iste, -istei, -istele, -istelor, -istul (ro)</rdfs:comment>
        <rdfs:comment>e.g., a, az, egy (hu)</rdfs:comment>
        <rdfs:comment>e.g., dan/dan, den/dan, dnaha/dan, dneha/dan, dni/dan, dnin/dan, itoga/te, na/dan, naga/dan (sl-rozaj)</rdfs:comment>
        <rdfs:comment>e.g., dnaha/dan, nagha/dan, noga/dan, toga/te (sl-rozaj)</rdfs:comment>
        <rdfs:comment>e.g., يکي/يک يک يه/يک (fa)</rdfs:comment>
        <rdfs:comment>Article and Determiner are independent top-level concepts that may, however, overlap for some languages:
For Romanian, the distribition of articles is fixed, while for determiners is not. Also, the determiners are Person marked while the articles are not (Dan Tufis, email 2010/06/09). Determiner/Type=&quot;article&quot; as used for Persian thus means that the token is in the intersection between Article and Determiner.

In Persian, there are different types of determiners namely demonstrative, indefinite, interrogative, exclamative, and article. As defined here, there is just one article in Farsi; i.e, &apos;‫( &apos;ﻳﮏ‬yek). It is homonym with ‘‫ ’ﻳﮏ‬which is a number. (Qasemizadeh and Rahimi 2006) The Persian article marks specificity rather than definiteness.
(Ivan A. Derzhanski, email 2010/06/18)

MTE distinguishes four subclasses of Article, fully instantiated for Romanian only. Unlike in most of the European languages, the article in Romanian has four types. Beside the types definite and indefinite which have the generally known semantic value, Romanian uses two additional types of articles, which are semantically subordinated to the definite article but which have special forms and meanings: (1) the possessive article (also called genitival article) is an element in the structure of the possessive pronoun, of the ordinal numeral (e.g. al meu (mine) and al treilea (the third)), and of the indefinite genitive forms of the nouns (e.g. capitol al cărţii (chapter of the book)). (2) the demonstrative article links a definite noun to its determinants, links a numeral or an adjective to a noun, and it is a constituent part of the relative superlative (e.g. fata cea mare (the elder girl), cel lenes, (the lazy), respectively prietenul cel mai bun (the best friend)). (MTE v4)</rdfs:comment>
    </owl:Class>
    


    <!-- http://purl.org/olia/mte/multext-east.owl#Aspect -->

    <owl:Class rdf:about="http://purl.org/olia/mte/multext-east.owl#Aspect">
        <rdfs:subClassOf rdf:resource="http://purl.org/olia/mte/multext-east.owl#MorphosyntacticFeature"/>
    </owl:Class>
    


    <!-- http://purl.org/olia/mte/multext-east.owl#AspectParticle -->

    <owl:Class rdf:about="http://purl.org/olia/mte/multext-east.owl#AspectParticle">
        <rdfs:subClassOf rdf:resource="http://purl.org/olia/mte/multext-east.owl#VerbalParticle"/>
        <rdfs:comment>Particle/Type=&quot;aspect&quot; (Romanian)

A verbal particle with Particle/Type=&quot;aspect&quot; modifies the verbs and carries information on the verb form, i.e., on its aspect  (Dan Tufis, email 2010/06/09)</rdfs:comment>
    </owl:Class>
    


    <!-- http://purl.org/olia/mte/multext-east.owl#AttributivePronoun -->

    <owl:Class rdf:about="http://purl.org/olia/mte/multext-east.owl#AttributivePronoun">
        <owl:equivalentClass>
            <owl:Class>
                <owl:intersectionOf rdf:parseType="Collection">
                    <rdf:Description rdf:about="http://purl.org/olia/mte/multext-east.owl#Adjectival"/>
                    <rdf:Description rdf:about="http://purl.org/olia/mte/multext-east.owl#Pronoun"/>
                </owl:intersectionOf>
            </owl:Class>
        </owl:equivalentClass>
        <rdfs:subClassOf rdf:resource="http://purl.org/olia/mte/multext-east.owl#Adjectival"/>
        <rdfs:subClassOf rdf:resource="http://purl.org/olia/mte/multext-east.owl#Pronoun"/>
        <rdfs:comment>Pronoun/Referent_Type=&quot;attributive&quot; (Bulgarian) and  Pronoun/Syntactic_Type=&quot;adjectival&quot; (other Slavic languages) are  essentially the same thing (though in the Bulgarian tagset the value also contrasts with &quot;possessive&quot;)
(Ivan A Derzhanski, email 2010/06/09)</rdfs:comment>
        <rdfs:comment>e.g., всякаква/всякакъв, всякакви/всякакъв, всякакво/всякакъв, всякакъв, каква/какъв, каквато/какъвто, какви/какъв, каквито/какъвто, какво/какъв (bg)</rdfs:comment>
    </owl:Class>
    


    <!-- http://purl.org/olia/mte/multext-east.owl#AuxiliaryVerb -->

    <owl:Class rdf:about="http://purl.org/olia/mte/multext-east.owl#AuxiliaryVerb">
        <rdfs:subClassOf rdf:resource="http://purl.org/olia/mte/multext-east.owl#Verb"/>
        <rdfs:comment>e.g., biste/biti, bićete/biti, htedni/hteti, htednimo/hteti, htele/hteti, htelo/hteti, hteo/hteti, hteti, htio/htjeti (sr)</rdfs:comment>
        <rdfs:comment>e.g., bit/bet, biti/bet, bodete/bet, bodite/bet, bota/bet, giò/tët, sta/bet, ste/bet, tiemo/tët (sl-rozaj)</rdfs:comment>
        <rdfs:comment>e.g., bodita/biti, bodite/biti, bosta/biti, boste/biti, niste/biti, sta/biti, ste/biti, tlelevš/= (sl)</rdfs:comment>
        <rdfs:comment>e.g., dostal/dostat, dostala/dostat, dostali/dostat, dostaly/dostat, dostane/dostat, dostanou/dostat, dostanu/dostat, dostat, máte/mít (cs)</rdfs:comment>
        <rdfs:comment>e.g., majte/mať, máte/mať (sk)</rdfs:comment>
        <rdfs:comment>e.g., oleksite/olema, olemast/olema, olemata/olema, olete/olema, olevat/olema, olevatki/olema, olite/olema, polevat/olema (et)</rdfs:comment>
        <rdfs:comment>e.g., oughter/have, wasn&apos;t/be+not, weren&apos;t/be+not (en)</rdfs:comment>
        <rdfs:comment>Type=&quot;auxiliary&quot;&lt;br/&gt;

In Persian, future tense is made by the help of Auxiliary verbs. In order to make progressive form in Farsi, verbs are inflected with the prefix &apos;‫( &apos;ﻣﯽ‬mī). Perfective forms of verbs are usually made using auxiliary verbs &apos;… ‫( &apos;ام، اﺳﺖ‬am, ast, …). Passive form of the verbs in Farsi are made by the help of Auxiliary verbs. Passive form of the verb is made of Past Participle + Auxiliary verb &apos;‫( &apos;ﺷﺪن‬šodan).
(Qasemizadeh and Rahimi 2006)&lt;br/&gt;

Note that the extension of AuxiliaryVerb may be defined differently. For many languages, AuxiliaryVerb does generally not include forms of &quot;to be&quot; (e.g., Czech být, Slovak byť, Macedonian bi), or modal verbs (e.g., Czech, Slovak, Macedonian). In other languages, however, verbs are classified according to their function rather than their form, e.g., Resian byt / to be can be main, copula or auxiliary.  (MTE v4)</rdfs:comment>
    </owl:Class>
    


    <!-- http://purl.org/olia/mte/multext-east.owl#BaseVerb -->

    <owl:Class rdf:about="http://purl.org/olia/mte/multext-east.owl#BaseVerb">
        <rdfs:subClassOf rdf:resource="http://purl.org/olia/mte/multext-east.owl#Verb"/>
        <rdfs:comment>Type=&quot;base&quot; (English)</rdfs:comment>
    </owl:Class>
    


    <!-- http://purl.org/olia/mte/multext-east.owl#Biaspectual -->

    <owl:Class rdf:about="http://purl.org/olia/mte/multext-east.owl#Biaspectual">
        <rdfs:subClassOf rdf:resource="http://purl.org/olia/mte/multext-east.owl#Aspect"/>
        <rdfs:comment>e.g., , pojde/iti, pojdita/iti (sl)</rdfs:comment>
        <rdfs:comment>e.g., 0, аблактована/аблактований абонована/абонований абордована/абордований абортована/абортований абсолютизована/абсолютизований абстрагована/абстрагований абшитована/абшитований авансована/авансований автоматизована/автоматизований авторизована/авторизований агрегатована/агрегатований адаптована/адаптований адоптована/адоптований адресована/адресований адсорбована/адсорбований азотизована/азотизований азотована/азотований акліматизована/акліматизований акомодована/акомодований акредитована/акредитований, аблактованая/аблактований абонованая/абонований абордованая/абордований абортованая/абортований абсолютизованая/абсолютизований абстрагованая/абстрагований абшитованая/абшитований авансованая/авансований автоматизованая/автоматизований авторизованая/авторизований агрегатованая/агрегатований адаптованая/адаптований адоптованая/адоптований адресованая/адресований адсорбованая/адсорбований азотизованая/азотизований азотованая/азотований акліматизованая/акліматизований акомодованая/акомодований акредитованая/акредитований, аблактоване/аблактований абоноване/абонований абордоване/абордований абортоване/абортований абсолютизоване/абсолютизований абстраговане/абстрагований абшитоване/абшитований авансоване/авансований автоматизоване/автоматизований авторизоване/авторизований агрегатоване/агрегатований адаптоване/адаптований адоптоване/адоптований адресоване/адресований адсорбоване/адсорбований азотизоване/азотизований азотоване/азотований акліматизоване/акліматизований акомодоване/акомодований акредитоване/акредитований, аблактованеє/аблактований абонованеє/абонований абордованеє/абордований абортованеє/абортований абсолютизованеє/абсолютизований абстрагованеє/абстрагований абшитованеє/абшитований авансованеє/авансований автоматизованеє/автоматизований авторизованеє/авторизований агрегатованеє/агрегатований адаптованеє/адаптований адоптованеє/адоптований адресованеє/адресований адсорбованеє/адсорбований азотизованеє/азотизований азотованеє/азотований акліматизованеє/акліматизований акомодованеє/акомодований акредитованеє/акредитований, аблактований/= абонований/= абордований/= абортований/= абсолютизований/= абстрагований/= абшитований/= авансований/= автоматизований/= авторизований/= агрегатований/= адаптований/= адоптований/= адресований/= адсорбований/= азотизований/= азотований/= акліматизований/= акомодований/= акредитований/=, аблактованим/аблактований абонованим/абонований абордованим/абордований абортованим/абортований абсолютизованим/абсолютизований абстрагованим/абстрагований абшитованим/абшитований авансованим/авансований автоматизованим/автоматизований авторизованим/авторизований агрегатованим/агрегатований адаптованим/адаптований адоптованим/адоптований адресованим/адресований адсорбованим/адсорбований азотизованим/азотизований азотованим/азотований акліматизованим/акліматизований акомодованим/акомодований акредитованим/акредитований, аблактованими/аблактований абонованими/абонований абордованими/абордований абортованими/абортований абсолютизованими/абсолютизований абстрагованими/абстрагований абшитованими/абшитований авансованими/авансований автоматизованими/автоматизований авторизованими/авторизований агрегатованими/агрегатований адаптованими/адаптований адоптованими/адоптований адресованими/адресований адсорбованими/адсорбований азотизованими/азотизований азотованими/азотований акліматизованими/акліматизований акомодованими/акомодований акредитованими/акредитований, аблактованих/аблактований абонованих/абонований абордованих/абордований абортованих/абортований абсолютизованих/абсолютизований абстрагованих/абстрагований абшитованих/абшитований авансованих/авансований автоматизованих/автоматизований авторизованих/авторизований агрегатованих/агрегатований адаптованих/адаптований адоптованих/адоптований адресованих/адресований адсорбованих/адсорбований азотизованих/азотизований азотованих/азотований акліматизованих/акліматизований акомодованих/акомодований акредитованих/акредитований (uk)</rdfs:comment>
        <rdfs:comment>e.g., nepostačia/nestačiť, nepostačí/nestačiť, nepostačím/nestačiť, nepostačíme/nestačiť, nepostačíte/nestačiť, nepostačíš/nestačiť, nezvestovali/nezvestovať, nezvestuj/nezvestovať, nezvestuje/nezvestovať (sk)</rdfs:comment>
        <rdfs:comment>Aspect=&quot;biaspectual&quot; (Verb: Slovene, Russian, Ukranian; Adjective: Ukrainian), identified with Aspect=&quot;ambivalent&quot; (Verb: Slovak)

Every Russian verb form is either perfective or imperfective. This applies to the majority of Russian verbs, but there is a small number of biaspectual verbs. A biaspectual verb can either take a perfective or an imperfective value, depending on the context. Examples of biaspectual verbs are: использовать &apos;utilize&apos;, казнить &apos;execute&apos;, жениться &apos;get married&apos;. (Feldman &amp; Arshavskaya 2007)

In the Slovak MTE v4, Aspect=&quot;ambivalent&quot;, presents a special class of verbs that have the same form in
perfective and imperfective/progressive aspect (the difference is only semantic/syntactic, not morphological).
(Dimitrova et al. 2009)

Anna Feldman &amp; Katya Arshavskaya (2007), English and Russian event annotation: A pilot study. Studies in Variation, Contacts and Change in English 1, http://www.helsinki.fi/varieng/journal/volumes/01/feldman_arshavskaya/</rdfs:comment>
    </owl:Class>
    


    <!-- http://purl.org/olia/mte/multext-east.owl#BothNumeral -->

    <owl:Class rdf:about="http://purl.org/olia/mte/multext-east.owl#BothNumeral">
        <rdfs:subClassOf rdf:resource="http://purl.org/olia/mte/multext-east.owl#OrthographicalRepresentationOfNumeral"/>
        <rdfs:comment>Form=&quot;both&quot; (Romanian)

A combination of digit (or roman) and letter representation, cf. English &quot;2nd&quot;.</rdfs:comment>
        <owl:versionInfo>no examples in the msd index. As it contrasts with &quot;roman&quot;, &quot;digit&quot; and &quot;letter&quot;, I can only assume that &quot;both&quot; means a combination of digit (or roman) and letter representation. Classified here as such.</owl:versionInfo>
    </owl:Class>
    


    <!-- http://purl.org/olia/mte/multext-east.owl#BoundClitic -->

    <owl:Class rdf:about="http://purl.org/olia/mte/multext-east.owl#BoundClitic">
        <rdfs:subClassOf rdf:resource="http://purl.org/olia/mte/multext-east.owl#AmbiguousCliticness"/>
        <rdfs:subClassOf>
            <owl:Class>
                <owl:unionOf rdf:parseType="Collection">
                    <rdf:Description rdf:about="http://purl.org/olia/mte/multext-east.owl#CliticElement"/>
                    <rdf:Description rdf:about="http://purl.org/olia/mte/multext-east.owl#ElementWithClitic"/>
                </owl:unionOf>
            </owl:Class>
        </rdfs:subClassOf>
        <rdfs:comment>e.g., gne/un, gnega/un, me/jä, nas/mï, te/tï (sl-rozaj)</rdfs:comment>
        <rdfs:comment>e.g., zanju/zame (sl)</rdfs:comment>
        <rdfs:comment>Clitic=&quot;bound&quot; (Slovene and Resian pronoun)&lt;br/&gt;

Clitic=&quot;bound&quot; appears in Slovene and indicates in fact the whole cluster, e.g. &quot;zame, pome&quot;, a combination of a preposition and a pronoun. So, ontologically, &quot;bound&quot; is rather ElementWith Clitic for Slovene.
(Natalia Kotsyba, email 2010/06/21)&lt;br/&gt;

In Resian, however, &quot;bound&quot; seems to be a CliticElement. At least, the Resian MSD index lists for nas/mï both Clitic=bound (Pp1-pa--b-n) and Clitic=no (Pp1-pa--n-n).  This is really a problem, because the only proper generalization over both uses would be to specify it as being ambiguous between CliticElement (for Resian) and ElementWithClitic (for Slovene). </rdfs:comment>
    </owl:Class>
    


    <!-- http://purl.org/olia/mte/multext-east.owl#CardinalNumeral -->

    <owl:Class rdf:about="http://purl.org/olia/mte/multext-east.owl#CardinalNumeral">
        <rdfs:subClassOf rdf:resource="http://purl.org/olia/mte/multext-east.owl#Numeral"/>
        <rdfs:comment>e.g., 1900-tól/1900, 2050-től/2050, egyenként/egy, egynegyedét/egynegyed, egytizedének/egytized, egytizedére/egytized, elsőként/első, ezerért/ezer, hetekben/hét (hu)</rdfs:comment>
        <rdfs:comment>e.g., 32/trïstinudwa, shtiri/štirji, starkrat duísti anu dévatnist/štirkratdwistinudëvatnist, treh/trïji, tri/trïji, trij/trïji, trì/trïji, šesterdov/šastardu (sl-rozaj)</rdfs:comment>
        <rdfs:comment>e.g., czterech/cztery, czterem/cztery, czterema/cztery, cztery/cztery, dwudziestu/dwadzieścia, dwustu/dwieście, dziewięćset/dziewięćset, jedenastu/jedenaście, piętnastu/piętnaście (pl)</rdfs:comment>
        <rdfs:comment>e.g., kümneteks/kümme, miljonitesse/miljon, tuhandetega/tuhat, tuhandeteni/tuhat, viiekümnest/viiskümmend, viiest/viis, viieteistkümnest/viisteist, viitega/viis (et)</rdfs:comment>
        <rdfs:comment>e.g., sta/sto, stem/sto, stě/sto, tolik, tolika/tolik, třech/tři, třem/tři, třemi/tři, tři (cs)</rdfs:comment>
        <rdfs:comment>e.g., suta/sută, sute/sută, sutei/sută, sută (ro)</rdfs:comment>
        <rdfs:comment>e.g., tisícinou/tisícina, traja/tri, tretinou/tretina, tri, tridsatinou/tridsatina, troch/tri, trom/tri, štyri, štyria/štyri (sk)</rdfs:comment>
        <rdfs:comment>e.g., treh/trije, trem/trije, tremi/trije, štiri/štirje, štirih/štirje, štirim/štirje (sl)</rdfs:comment>
        <rdfs:comment>e.g., tri, trima/tri, Četiri/četiri, četiri (sr)</rdfs:comment>
        <rdfs:comment>Cardinal numerals signify a numerical (quantitative) property of objects, e.g., Sloval jeden
dom, dve ženy, tri knihy; Bulgarian един дом, две жени, три книги /one home, two women, three books/.
(Dimitrova et al. 2009)&lt;br/&gt;

Traditional Romanian grammars usually distinguish seven numeral types, where five of them have specific forms and the other two are obtained by composition. The first group is made up by the following numeral types: cardinal (trei-three), ordinal (al treilea-the third), fractional (treime-one third), multiple (întreit-trine), collective (amândoi-both). The second group contains the numeral types which are composed by means of other parts of speech: distributive (câte trei-...each three...), adverbial (de trei ori-thrice) and again the collective numeral which also has compound forms (toţi trei-all three). Nonetheless, as the numerals of the second group have a weak syntactic cohesion, namely each composition element may be regarded as an element of the sentence, with its own grammatical function, these last numeral types are irrelevant for the morphosyntactic annotation.
(Romanian MTE v4)</rdfs:comment>
    </owl:Class>
    


    <!-- http://purl.org/olia/mte/multext-east.owl#Case -->

    <owl:Class rdf:about="http://purl.org/olia/mte/multext-east.owl#Case">
        <rdfs:subClassOf rdf:resource="http://purl.org/olia/mte/multext-east.owl#MorphosyntacticFeature"/>
        <rdfs:comment>feature of Noun (http://nl.ijs.si/ME/V4/msd/html/msd.N.html) and Verb (Russian and Estonian, http://nl.ijs.si/ME/V4/msd/html/msd.V.html)</rdfs:comment>
    </owl:Class>
    


    <!-- http://purl.org/olia/mte/multext-east.owl#CausalAdverb -->

    <owl:Class rdf:about="http://purl.org/olia/mte/multext-east.owl#CausalAdverb">
        <rdfs:subClassOf rdf:resource="http://purl.org/olia/mte/multext-east.owl#Adverb"/>
        <rdfs:comment>Adverb/Type=&quot;causal&quot; is used in the Hungarian MTE v4, but no examples are provided.</rdfs:comment>
    </owl:Class>
    


    <!-- http://purl.org/olia/mte/multext-east.owl#CausalisCase -->

    <owl:Class rdf:about="http://purl.org/olia/mte/multext-east.owl#CausalisCase">
        <rdfs:subClassOf rdf:resource="http://purl.org/olia/mte/multext-east.owl#Case"/>
        <rdfs:comment>e.g., amelyekért/amely, ezerért/ezer, javáért/jav, jövőjéért/jövő, kimért/ki, lelkiismeretedért/lelkiismeret, magáért/maga, milliárdért/milliárd, mindnyájukért/mindnyáj (hu)</rdfs:comment>
        <rdfs:comment>Case=&quot;causalis&quot; (Hungarian)</rdfs:comment>
    </owl:Class>
    


    <!-- http://purl.org/olia/mte/multext-east.owl#Clitic -->

    <owl:Class rdf:about="http://purl.org/olia/mte/multext-east.owl#Clitic">
        <rdfs:subClassOf rdf:resource="http://purl.org/olia/mte/multext-east.owl#AmbiguousCliticness"/>
        <rdfs:subClassOf>
            <owl:Class>
                <owl:unionOf rdf:parseType="Collection">
                    <rdf:Description rdf:about="http://purl.org/olia/mte/multext-east.owl#CliticElement"/>
                    <rdf:Description rdf:about="http://purl.org/olia/mte/multext-east.owl#ElementWithClitic"/>
                </owl:unionOf>
            </owl:Class>
        </rdfs:subClassOf>
        <rdfs:comment>Clitic=&quot;yes&quot; (Noun/Adjective: Romanian; Verb: Romanian, Polish, Serbian, Persian)&lt;br/&gt;

Slovak Pronoun: Type=reflexive ecompasses all reflexive pronouns (sa, sebe, si, svoj, seba) as well as &quot;sa&quot; in its role as the obligatory particle of reflexive verbs. Personal and possessive reflexives are further distinguished via the Referent_Type attribute. &quot;sa&quot; in all its roles will be marked as the reflexive personal clitic pronoun. 
The Clitic attribute distinguishes clitical vs. nonclitical pronominal forms, e.g. &quot;ti&quot; vs. &quot;tebe&quot;.&lt;br/&gt;

Polish Pronoun: Prepositionality is encoded as Clitic with values &quot;y(es)&quot; for nią, niego etc., &quot;n(o)&quot; for ją, go etc., &quot;a(gglutinant)&quot; for -ń. Cf. the Clitic value &quot;bound&quot; for Slovene pronouns like zate which refers to the whole cluster, formally a combination of a preposition and a pronoun. This coding can be used for similar phenomena in Polish, e.g dlań (for him), given the word segmentation is revised towards a more trraditional one.&lt;br/&gt;

Hungarian Adverb: The modifier -e question word (the only Hungarian clitic) is attached to the preceding word with a hyphen.&lt;br/&gt;

Romanian Verb, Noun, Adjective: The cliticization phenomenon in Romanian is not restricted to verb-pronoun relationship, but may also be observed with the (main) verb and the auxiliary, the noun or adjective with pronoun, with noun or adjective with copula, pronoun with auxiliary, preposition with (indefinite) article, numeral or (indefinite) pronoun, negative adverb with verb, auxiliary or pronoun, and some others (mainly created through the contracted forms of the verb &quot;a fi&quot;-to be). We restrict ourselves to considering only the graphically marked clicitizations. In such cases, the two, three or (sometimes) four constituents of a cliticized word-form are always separated by a hyphen. Omitting the hyphen in such cases is an unacceptable error in written Romanian.&lt;br/&gt;

Romanian Article: Note that the definite article has only enclitic forms, except for one proclitical form (lui + proper noun: lui Ion). The inflected forms of the foreign-origin words (mainly nouns) not fully assimilated, are usually written with a hyphen between the base-form and the inflectional ending. In our encoding, we classified these endings (which are supposed to be split by the segmenter) as clitic articles (clitic attribute is always &quot;y&quot;) which can be either definite (type=f, &quot;-istul&quot;) or indefinite (type=i, &quot;ist&quot;) and are characterised by gender (gender=m, &quot;ist&quot;; gender=f, &quot;istă&quot;), number (number=s, &quot;ist&quot;; number=p, &quot;işti&quot;) and case (case=r, &quot;istul&quot;; case=o, &quot;istului&quot;).</rdfs:comment>
        <owl:versionInfo>Seems to be CliticElement in Slovak and Polish, but ElementWithClitic in Hungarian and Romanian.</owl:versionInfo>
    </owl:Class>
    


    <!-- http://purl.org/olia/mte/multext-east.owl#CliticDefiniteDeterminer -->

    <owl:Class rdf:about="http://purl.org/olia/mte/multext-east.owl#CliticDefiniteDeterminer">
        <rdfs:subClassOf rdf:resource="http://purl.org/olia/mte/multext-east.owl#CliticDeterminerType"/>
    </owl:Class>
    


    <!-- http://purl.org/olia/mte/multext-east.owl#CliticDeterminerType -->

    <owl:Class rdf:about="http://purl.org/olia/mte/multext-east.owl#CliticDeterminerType">
        <rdfs:subClassOf rdf:resource="http://purl.org/olia/mte/multext-east.owl#Definiteness"/>
        <owl:versionInfo>Bulgarian, Macedonian and Romanian employ a postfixed article (http://en.wikipedia.org/wiki/Macedonian_grammar)&lt;br/&gt;

Etymologically speaking, CliticDeterminerType and ReductionFeature are the same: the ending of the full form was originally a cliticised demonstrative pronoun (just like the article in Bg or Ro), and the semantic distinction was [+/- definite], but it has shifted to [attributive:predicative] or some such on some occasions.
However, keeping them together wouldn&apos;t be correct: Bulgarian has preserved (to a limited extent) the old long form, and has a fourfold opposition of, say, _nov : novi : novija : novijat_, the first two members of which have counterparts in several Slavic languages (although the functions differ), while the second two are 
restricted to the Balkan sprachbund.  I&apos;d call them [-article short], [-article full], [+article short] and [+article full] respectively. (Ivan A. Derzhanski, emails 2010/06/18)

</owl:versionInfo>
    </owl:Class>
    


    <!-- http://purl.org/olia/mte/multext-east.owl#CliticDistalDeterminer -->

    <owl:Class rdf:about="http://purl.org/olia/mte/multext-east.owl#CliticDistalDeterminer">
        <rdfs:subClassOf rdf:resource="http://purl.org/olia/mte/multext-east.owl#CliticDefiniteDeterminer"/>
        <rdfs:comment>Definiteness=&quot;distal&quot; (Noun/Adjective/Pronoun: Macedonian)

For Macedonian, the definiteness attributes can take the values: non definite (no), generally definite (yes), definite at short visible distance (proximal), and definite at longer visible distance (distal). (MTE v4)</rdfs:comment>
    </owl:Class>
    


    <!-- http://purl.org/olia/mte/multext-east.owl#CliticElement -->

    <owl:Class rdf:about="http://purl.org/olia/mte/multext-east.owl#CliticElement">
        <rdfs:subClassOf rdf:resource="http://purl.org/olia/mte/multext-east.owl#Cliticness"/>
        <owl:versionInfo>Introduced to annotations that mark an element as *being* a clitic, and to distinguish them from elements that merely *cointain* clitic elements (i.e., that are composed of nonclitics and clitics).</owl:versionInfo>
    </owl:Class>
    


    <!-- http://purl.org/olia/mte/multext-east.owl#CliticIndefiniteDeterminer -->

    <owl:Class rdf:about="http://purl.org/olia/mte/multext-east.owl#CliticIndefiniteDeterminer">
        <rdfs:subClassOf rdf:resource="http://purl.org/olia/mte/multext-east.owl#CliticDeterminerType"/>
    </owl:Class>
    


    <!-- http://purl.org/olia/mte/multext-east.owl#CliticProximalDeterminer -->

    <owl:Class rdf:about="http://purl.org/olia/mte/multext-east.owl#CliticProximalDeterminer">
        <rdfs:subClassOf rdf:resource="http://purl.org/olia/mte/multext-east.owl#CliticDefiniteDeterminer"/>
        <rdfs:comment>Definiteness=&quot;proximal&quot; (Noun/Adjective/Pronoun Macedonian)

For Macedonian, the definiteness attributes can take the values: non definite (no), generally definite (yes), definite at short visible distance (proximal), and definite at longer visible distance (distal). (MTE v4)</rdfs:comment>
    </owl:Class>
    


    <!-- http://purl.org/olia/mte/multext-east.owl#CliticSpecificDeterminer -->

    <owl:Class rdf:about="http://purl.org/olia/mte/multext-east.owl#CliticSpecificDeterminer">
        <rdfs:subClassOf rdf:resource="http://purl.org/olia/mte/multext-east.owl#CliticDeterminerType"/>
        <rdfs:comment>Persian does have an article, but it marks specificity rather than definiteness. The Persian article is similar to the Balkan one (a clitic of pronominal origin that&apos;s written together with the word), except that it isn&apos;t exactly definite (you can even see it described as an indefinite article).
(Ivan A. Derzhanski, emails 2010/06/18)</rdfs:comment>
    </owl:Class>
    


    <!-- http://purl.org/olia/mte/multext-east.owl#Cliticness -->

    <owl:Class rdf:about="http://purl.org/olia/mte/multext-east.owl#Cliticness">
        <rdfs:subClassOf rdf:resource="http://purl.org/olia/mte/multext-east.owl#MorphosyntacticFeature"/>
        <rdfs:comment>feature &quot;Clitic&quot;&lt;br/&gt;

This is a highly feature used in different ways in different MTE tagsets. Therefore, no definition is attempted, but rather, different functions are represented in subconcepts. A proper ontological model would have to clarify the situation further.

The attribute Clitic means either &quot;hasClitic&quot; (if applied to Noun) or &quot;isClitic&quot; (if applied to Article): This is similar to Case, which on Adpositions means &quot;requiresCase&quot; rathen than hasCase. Definitely something to think about; is it better to be formally correct or have small set of attributes? (Tomaz Erjavec, email 2010/06/09)&lt;br/&gt;

[Romanian] Clitic feature denotes:
1) a character ellision: i-am dat = îi am dat (î is deleted) - I gave him
2) insertion: ducându-mă = ducând+U+mă (U is inserted +for phonological
reasons) - carrying myself
3) or both: mâncându-l = mâncând+U+_e_l (U is inserted and e is deleted)
- eating it
4) &quot;fast speaking&quot; that is pronuntiation of two words as if a single
word: maică-mea - my mother
it is interesting to note that in &quot;normal speaking&quot; this would be &quot;maica
mea&quot; where the word &quot;maica&quot; is in definite form
while in the previous form was in indefinite form (notice the final
&amp;abreve;)
It is always signaled by a hyphen between the content word and the
functional word that are cliticized.
(Dan Tufis, email 2010/06/09)&lt;br/&gt;

Polish Pronoun: Prepositionality is encoded as Clitic with values &quot;y(es)&quot; for nią, niego etc., &quot;n(o)&quot; for ją, go etc., &quot;a(gglutinant)&quot; for -ń. Cf. the Clitic value &quot;bound&quot; for Slovene pronouns like zate which refers to the whole cluster, formally a combination of a preposition and a pronoun. This coding can be used for similar phenomena in Polish, e.g dlań (for him), given the word segmentation is revised towards a more trraditional one.
(MTE, v4.0)&lt;br/&gt;

Czech Pronoun: The Clitic attribute distinguishes clitical vs. nonclitical pronominal forms, e.g. &quot;ti&quot; vs. &quot;tobě&quot;.
(MTE, v4.0)</rdfs:comment>
        <owl:versionInfo>Cliticness (attribute Clitic) conflates three different aspects:&lt;br/&gt;

(a) whether an element *is* a clitic, 
(b) whether an element *contains* a clitic, and
(c) whether an element *should contain* a clitic, that is, however, represented as a separate token.&lt;br/&gt;

The subclassification makes this explicit:
(a) CliticElement, NoncliticElement (Clitic=&quot;bound&quot;, Clitic=&quot;agglutinant&quot;)
(b) ElementWithClitic, ElementWithoutClitic (Clitic_s=&quot;yes&quot;, Clitic_s=&quot;no&quot;)
(c) ElementDemanticClitic (Clitic=&quot;demanding&quot;)&lt;br/&gt;

Further, a subconcept Collocation is introduced to account for Polish &quot;Burkinostka&quot;s (Clitic=&quot;burkinostka&quot;) with a language-independent term. Expressions that occur only in a fixed context are superficially similar to white-space separated Clitics, but no Clitics, of course.&lt;br/&gt;

Clitic=&quot;yes&quot; and Clitic=&quot;no&quot; are ambiguous (ElementWithClitic or CliticElement; ElementWithoutClitic or NoncliticElement) and represented as NonClitic and Clitic as sunconcepts of AmbiguousCliticness.</owl:versionInfo>
    </owl:Class>
    


    <!-- http://purl.org/olia/mte/multext-east.owl#Collective -->

    <owl:Class rdf:about="http://purl.org/olia/mte/multext-east.owl#Collective">
        <rdfs:subClassOf rdf:resource="http://purl.org/olia/mte/multext-east.owl#MorphologicalDerivation"/>
        <rdfs:comment>
			Collective plurals are usually considered as derivation rather than an inflection, but modelled as a number feature in the 
			MTE schema of Resian (Slovene dialect in Italy).
</rdfs:comment>
        <owl:versionInfo>... after great fights we got rid of collective for most langauges, but not Resian, alas.
(Tomaz Erjavec, email 2010/06/09)&lt;br/&gt;

Collective plural has been removed for the sake of compatibility with other Slavic languages. It is considered as derivation, thus collective plurals are separate entries in the dictionary. (Macedonian MTE)
</owl:versionInfo>
    </owl:Class>
    


    <!-- http://purl.org/olia/mte/multext-east.owl#CollectiveNumber -->

    <owl:Class rdf:about="http://purl.org/olia/mte/multext-east.owl#CollectiveNumber">
        <rdfs:subClassOf rdf:resource="http://purl.org/olia/mte/multext-east.owl#Number"/>
        <rdfs:comment>Collective plurals, though usually considered as derivation rather than an inflection, are modelled as a number feature in the MTE schema of Resian (Slovene dialect in Italy).
</rdfs:comment>
        <owl:versionInfo>... after great fights we got rid of collective for most langauges, but not Resian, alas.
(Tomaz Erjavec, email 2010/06/09)&lt;br/&gt;

Collective plural has been removed for the sake of compatibility with other Slavic languages. It is considered as derivation, thus collective plurals are separate entries in the dictionary. (Macedonian MTE)
</owl:versionInfo>
    </owl:Class>
    


    <!-- http://purl.org/olia/mte/multext-east.owl#CollectiveNumeral -->

    <owl:Class rdf:about="http://purl.org/olia/mte/multext-east.owl#CollectiveNumeral">
        <rdfs:subClassOf rdf:resource="http://purl.org/olia/mte/multext-east.owl#Numeral"/>
        <rdfs:comment>e.g., ambelor/ambii, ambilor/ambii, amânduror/amândoi, amândurora/amândoi, câteşipatru, tuspatru (ro)</rdfs:comment>
        <rdfs:comment>e.g., czworga/czworo, czworgiem/czworo, czworgu/czworo, czworo/czworo, dwoje/dwoje, dwojga/dwoje, dwojgiem/dwoje, dwojgu/dwoje, jedenaścioro/jedenaścioro (pl)</rdfs:comment>
        <rdfs:comment>e.g., dvadesetora/dvadesetoro, dvoja/dvoje, dvoje, dvoji/dvoje, dvojih/dvoje, dvojim/dvoje, oboje, tridesetora/tridesetoro, troja/troje (sr)</rdfs:comment>
        <rdfs:comment>e.g., обата, обајцата, обете, шеесетминава/шеесетмина, шеесетминана/шеесетмина, шеесетмината/шеесетмина, шеснаесетминава/шеснаесетмина, шеснаесетминана/шеснаесетмина, шеснаесетмината/шеснаесетмина (mk)</rdfs:comment>
        <rdfs:comment>Numeral/Type=&quot;collect&quot; (Romanian)&lt;br/&gt;

In traditional Romanian grammars, expressions like amândoi-both, toţi trei-all three are referred to as collective numerals. (MTE v4)</rdfs:comment>
    </owl:Class>
    


    <!-- http://purl.org/olia/mte/multext-east.owl#Collocation -->

    <owl:Class rdf:about="http://purl.org/olia/mte/multext-east.owl#Collocation">
        <rdfs:subClassOf rdf:resource="http://purl.org/olia/mte/multext-east.owl#Cliticness"/>
        <owl:versionInfo>&quot;Burkinostka&quot; is certainly not a clitic, but grouped together with cliticization phenomena in analogy with clitics that are represented as separate tokens. A more general term would be &quot;collocation&quot;, or, more precisely, &quot;element that occurs only as a component of a particular collocation&quot;.</owl:versionInfo>
    </owl:Class>
    


    <!-- http://purl.org/olia/mte/multext-east.owl#ComitativeCase -->

    <owl:Class rdf:about="http://purl.org/olia/mte/multext-east.owl#ComitativeCase">
        <rdfs:subClassOf rdf:resource="http://purl.org/olia/mte/multext-east.owl#Case"/>
        <rdfs:comment>e.g., iseenestega/iseenese, kelledega/kes, kellega/kes, kg-ga/kg, kõigiga/kõik, meiega/mina, millega/mis, minuga/mina, neljandaga/neljas (et)</rdfs:comment>
        <rdfs:comment>Case=&quot;komitative&quot; (Estonian)</rdfs:comment>
        <owl:versionInfo>&quot;komitative&quot; was just a typo in the original Estonian MTE, &quot;comitative&quot; is right.</owl:versionInfo>
    </owl:Class>
    


    <!-- http://purl.org/olia/mte/multext-east.owl#CommonGender -->

    <owl:Class rdf:about="http://purl.org/olia/mte/multext-east.owl#CommonGender">
        <rdfs:subClassOf rdf:resource="http://purl.org/olia/mte/multext-east.owl#Gender"/>
        <rdfs:comment>The Gender value &quot;common&quot; is assigned to nouns that can combine with adjectives in either feminine or masculine,e.g., Ukrainian сирота  or either neutral or masculine gender, e.g. Ukrainian Самоа. In Russian, Gender=common is used for words such as судья, коллега, чукча, саша, убийца, etc. (MTE v4)</rdfs:comment>
    </owl:Class>
    


    <!-- http://purl.org/olia/mte/multext-east.owl#CommonNoun -->

    <owl:Class rdf:about="http://purl.org/olia/mte/multext-east.owl#CommonNoun">
        <rdfs:subClassOf rdf:resource="http://purl.org/olia/mte/multext-east.owl#Noun"/>
        <rdfs:comment>e.g., -mpărate/împărat, -ngrijitoare/îngrijitoare, -nsoţitoare/însoţitoare, -nvingători/învingător, -nvingătorii/învingător, -nvingătorilor/învingător, -nvingătorului/învingător, -nvăţătoare/învăţătoare, -nvăţători/învăţător (ro)</rdfs:comment>
        <rdfs:comment>e.g., Comandatmiteh/komandament, costi/kust, dialëte/dijalët, dobrute/dubruta, fiesto/fjëšta, istriki/štrïk, kitinami/këtina, lit/lëtu, lita/lëtu (sl-rozaj)</rdfs:comment>
        <rdfs:comment>e.g., barátoddal/barát, betegségedhez/betegség, betegségünktől/betegség, botrányoddal/botrány, cselekedeteidről/cselekedet, cselekedeteiteken/cselekedet, csontjaiig/csont, embereinktől/ember, estéi/est (hu)</rdfs:comment>
        <rdfs:comment>e.g., country, kontra, kontras/kontra, turné, ztotožněním/ztotožnění, ztělesněním/ztělesnění, zvyklostem/zvyklost, žurnalisté/žurnalista (cs)</rdfs:comment>
        <rdfs:comment>e.g., derišteta/derište, drveta/drvo, javnosti/javnost, kategorije/kategorija, Ketrin, ministarstva/ministarstvo, opštenje, osobenosti/osobenost, poteza/potez (sr)</rdfs:comment>
        <rdfs:comment>e.g., trükivigadeni/trükiviga, tulemusteni/tulemus, vasksiltidelt/vasksilt, veistelt/veis, vesiväravateni/vesivärav, vormimütsidelt/vormimüts, vormiüksustest/vormiüksus, vorstidest/vorst, võrranditest/võrrand (et)</rdfs:comment>
        <rdfs:comment>e.g., viscounts/viscount, welterweights/welterweight (en)</rdfs:comment>
        <rdfs:comment>e.g., žurnalistiek/žurnalistka, žurnalistikami/žurnalistika, žurnalistike/žurnalistika, žurnalistikou/žurnalistika, žurnalistiku/žurnalistika, žurnalistiky/žurnalistika, žurnalistikách/žurnalistika, žurnalistikám/žurnalistika, žurnalistkami/žurnalistka (sk)</rdfs:comment>
        <rdfs:comment>Noun/Type=Common</rdfs:comment>
    </owl:Class>
    


    <!-- http://purl.org/olia/mte/multext-east.owl#ComparativeDegree -->

    <owl:Class rdf:about="http://purl.org/olia/mte/multext-east.owl#ComparativeDegree">
        <rdfs:subClassOf rdf:resource="http://purl.org/olia/mte/multext-east.owl#Degree"/>
        <rdfs:comment>e.g., -, esendőségbe/esendő, fiatalabbaknak/fiatal, fontosabbaké/fontos, illendőségből/illendő, jobbkor/jó, kedvezőbbeknek/kedvező, kevesebbe/kevés, kisebbeken/kis (hu)</rdfs:comment>
        <rdfs:comment>e.g., bardziej/bardzo, bliższe/bliski, bliższej/bliski, bliższych/bliski, bogatszych/bogaty, dalsza/daleki, dalsze/daleki, dalszego/daleki, dalszej/daleki (pl)</rdfs:comment>
        <rdfs:comment>e.g., better, less, more, worse (en)</rdfs:comment>
        <rdfs:comment>e.g., bo/bö, bujše/bujši, lípce/lip, mlaisi/mlad, staraisi/stär, vagh/već, vec/već, vinzha/vinči, vénci/vilek (sl-rozaj)</rdfs:comment>
        <rdfs:comment>e.g., din_ce_în_ce_mai, succesiv, superioara/superior, superioare/superior, superioarei/superior, superioarele/superior, superioarelor/superior, superioară/superior, superior (ro)</rdfs:comment>
        <rdfs:comment>e.g., mlađa/mlad, najmanji/mali, najmanju/mali, severnijeg/severni, severnijemu/severni, severnijim/severni, suštinskijeg/suštinski, suštinskijega/suštinski, suštinskijem/suštinski (sr)</rdfs:comment>
        <rdfs:comment>e.g., parematelt/parem, pikemata/pikem, rohkematessegi/rohkem, spetsiaalsematesse/spetsiaalsem, suurematesse/suurem, tooremata/toorem, tootmisvõimsamana/tootmisvõimsam, tublimateks/tublim, tõelisemateks/tõelisem (et)</rdfs:comment>
        <rdfs:comment>e.g., působivějšími/působivý, rytířštějšími/rytířský, těžšími/těžký, vyššímu/vysoký, zajímavějšímu/zajímavý, závažnějšímu/závažný (cs)</rdfs:comment>
        <rdfs:comment>e.g., slabša/slab, večjih/velik (sl)</rdfs:comment>
        <rdfs:comment>e.g., žoviálnejšej/žoviálny, žoviálnejšia/žoviálny, žoviálnejšie/žoviálny, žoviálnejšieho/žoviálny, žoviálnejšiemu/žoviálny, žoviálnejšiu/žoviálny, žoviálnejšom/žoviálny, žoviálnejšou/žoviálny, žoviálnejších/žoviálny (sk)</rdfs:comment>
        <rdfs:comment>e.g., азартніша/азартніший активніша/активніший актуальніша/актуальніший амбіціозніша/амбіціозніший ароматніша/ароматніший багатозначніша/багатозначніший бадьоріша/бадьоріший бажаніша/бажаніший балакливіша/балакливіший балакучіша/балакучіший бережливіша/бережливіший бідніша/бідніший біліша/біліший більша/більший благонадійніша/благонадійніший благородніша/благородніший блискучіша/блискучіший блідіша/блідіший блякліша/блякліший болісніша/болісніший, азартнішая/азартніший активнішая/активніший актуальнішая/актуальніший амбіціознішая/амбіціозніший ароматнішая/ароматніший багатозначнішая/багатозначніший бадьорішая/бадьоріший бажанішая/бажаніший балакливішая/балакливіший балакучішая/балакучіший бережливішая/бережливіший біднішая/бідніший білішая/біліший більшая/більший благонадійнішая/благонадійніший благороднішая/благородніший блискучішая/блискучіший блідішая/блідіший бляклішая/блякліший боліснішая/болісніший, азартніше/азартніший активніше/активніший актуальніше/актуальніший амбіціозніше/амбіціозніший ароматніше/ароматніший багатозначніше/багатозначніший бадьоріше/бадьоріший бажаніше/бажаніший балакливіше/балакливіший балакучіше/балакучіший бережливіше/бережливіший бідніше/бідніший біліше/біліший більше/більший благонадійніше/благонадійніший благородніше/благородніший блискучіше/блискучіший блідіше/блідіший блякліше/блякліший болісніше/болісніший, азартнішеє/азартніший активнішеє/активніший актуальнішеє/актуальніший амбіціознішеє/амбіціозніший ароматнішеє/ароматніший багатозначнішеє/багатозначніший бадьорішеє/бадьоріший бажанішеє/бажаніший балакливішеє/балакливіший балакучішеє/балакучіший бережливішеє/бережливіший біднішеє/бідніший білішеє/біліший більшеє/більший благонадійнішеє/благонадійніший благороднішеє/благородніший блискучішеє/блискучіший блідішеє/блідіший бляклішеє/блякліший боліснішеє/болісніший, азартніший/= активніший/= актуальніший/= амбіціозніший/= ароматніший/= багатозначніший/= бадьоріший/= бажаніший/= балакливіший/= балакучіший/= бережливіший/= бідніший/= біліший/= більший/= благонадійніший/= благородніший/= блискучіший/= блідіший/= блякліший/= болісніший/=, азартнішим/азартніший активнішим/активніший актуальнішим/актуальніший амбіціознішим/амбіціозніший ароматнішим/ароматніший багатозначнішим/багатозначніший бадьорішим/бадьоріший бажанішим/бажаніший балакливішим/балакливіший балакучішим/балакучіший бережливішим/бережливіший біднішим/бідніший білішим/біліший більшим/більший благонадійнішим/благонадійніший благороднішим/благородніший блискучішим/блискучіший блідішим/блідіший бляклішим/блякліший боліснішим/болісніший, азартнішими/азартніший активнішими/активніший актуальнішими/актуальніший амбіціознішими/амбіціозніший ароматнішими/ароматніший багатозначнішими/багатозначніший бадьорішими/бадьоріший бажанішими/бажаніший балакливішими/балакливіший балакучішими/балакучіший бережливішими/бережливіший біднішими/бідніший білішими/біліший більшими/більший благонадійнішими/благонадійніший благороднішими/благородніший блискучішими/блискучіший блідішими/блідіший бляклішими/блякліший боліснішими/болісніший, азартніших/азартніший активніших/активніший актуальніших/актуальніший амбіціозніших/амбіціозніший ароматніших/ароматніший багатозначніших/багатозначніший бадьоріших/бадьоріший бажаніших/бажаніший балакливіших/балакливіший балакучіших/балакучіший бережливіших/бережливіший бідніших/бідніший біліших/біліший більших/більший благонадійніших/благонадійніший благородніших/благородніший блискучіших/блискучіший блідіших/блідіший блякліших/блякліший болісніших/болісніший, азартнішого/азартніший активнішого/активніший актуальнішого/актуальніший амбіціознішого/амбіціозніший ароматнішого/ароматніший багатозначнішого/багатозначніший бадьорішого/бадьоріший бажанішого/бажаніший балакливішого/балакливіший балакучішого/балакучіший бережливішого/бережливіший біднішого/бідніший білішого/біліший більшого/більший благонадійнішого/благонадійніший благороднішого/благородніший блискучішого/блискучіший блідішого/блідіший бляклішого/блякліший боліснішого/болісніший (uk)</rdfs:comment>
        <rdfs:comment>e.g., пошпионска/шпионски, пошпионскава/шпионски, пошпионскана/шпионски, пошпионската/шпионски, пошпионски/шпионски, пошпионскиве/шпионски, пошпионскине/шпионски, пошпионскиов/шпионски, пошпионскион/шпионски (mk)</rdfs:comment>
        <rdfs:comment>e.g., явственнее/явственный, явственней/явственный, ядовитее/ядовитый (ru)</rdfs:comment>
        <rdfs:comment>e.g., بالاتر/بالا استوارتر/استوار آرام‌تر/آرام, بلندتري/بلند انساني‌تري/انساني‌ آرام‌تري/آرام, قوي‌ترِ/قوي بيشترِ/بيش اعظمِ/اعظم, مطمئن‌تر/مطمئن عاقلانه‌تر/عاقلانه بدبوتر/بدبو, کمتر/کم نزديک‌تر/نزديک سست‌تر/سست (fa)</rdfs:comment>
    </owl:Class>
    


    <!-- http://purl.org/olia/mte/multext-east.owl#ComparativeParticle -->

    <owl:Class rdf:about="http://purl.org/olia/mte/multext-east.owl#ComparativeParticle">
        <rdfs:subClassOf rdf:resource="http://purl.org/olia/mte/multext-east.owl#Particle"/>
        <rdfs:comment>In the Bulgarian MTE v4 specs, Particle/Type=&quot;comparative&quot; is used for particles used to create comparatives or superlatives (по, най). In other Slavic languages, e.g., Slovak, comparatives are formed through a morphology suffix, naj- is written together with superlatives (although this could be considered just a difference in orthography), so that ComparativeParticle is applied to Bulgarian only. (Dimitrova et al. 2009)</rdfs:comment>
    </owl:Class>
    


    <!-- http://purl.org/olia/mte/multext-east.owl#CompoundAdjective -->

    <owl:Class rdf:about="http://purl.org/olia/mte/multext-east.owl#CompoundAdjective">
        <owl:equivalentClass>
            <owl:Class>
                <owl:intersectionOf rdf:parseType="Collection">
                    <rdf:Description rdf:about="http://purl.org/olia/mte/multext-east.owl#FullArticle"/>
                    <rdf:Description rdf:about="http://purl.org/olia/mte/multext-east.owl#ReductionFeature"/>
                </owl:intersectionOf>
            </owl:Class>
        </owl:equivalentClass>
        <rdfs:subClassOf rdf:resource="http://purl.org/olia/mte/multext-east.owl#AdjectiveFormation"/>
        <rdfs:comment>e.g., nejubožejšími/ubohý, nejvyspělejších/vyspělý, nejvyšších/vysoký, nejvznešenějšímu/vznešený, nejvážnějšímu/vážný, nejvýznamnějších/významný, nejvýznamnějšími/významný, nejvýznamnějšímu/významný, největšími/velký (cs)</rdfs:comment>
        <rdfs:comment>Formation=&quot;compound&quot; (Czech)</rdfs:comment>
    </owl:Class>
    


    <!-- http://purl.org/olia/mte/multext-east.owl#CompoundAdposition -->

    <owl:Class rdf:about="http://purl.org/olia/mte/multext-east.owl#CompoundAdposition">
        <rdfs:subClassOf rdf:resource="http://purl.org/olia/mte/multext-east.owl#AdpositionFormation"/>
        <rdfs:comment>e.g., a незважаючи/=, за те за тим з-від з-за з-між з-навпроти з-над з-перед з-під з-поверхні з-поза з-позад з-позаду з-поміж з-понад з-поперед з-попід з-посеред з-проміж з-серед, згідно з, на противагу (uk)</rdfs:comment>
        <rdfs:comment>e.g., sauvojo/zawojo, ses med/zizmid, ta h/tah, ta mej/tami, ta pod/tapod, ta-mi/tamid, ta/tah, tana/tana, taper/tapar (sl-rozaj)</rdfs:comment>
        <rdfs:comment>e.g., از‌لايِ/ازلا ازلحاظِ/ازلحاظ ازجانبِ/ازجانب (fa)</rdfs:comment>
        <rdfs:comment>Adposition/Formation=&quot;compound&quot;&lt;br/&gt;

In several languages, there is a distinct class of compound prepositions. Each of them forms a formal and semantic unit, although graphically they stay unfused, e.g. Romanian de la, pe la, de pe, etc., or Resian ta-na / in (MTE v4)</rdfs:comment>
    </owl:Class>
    


    <!-- http://purl.org/olia/mte/multext-east.owl#CompoundConjunction -->

    <owl:Class rdf:about="http://purl.org/olia/mte/multext-east.owl#CompoundConjunction">
        <rdfs:subClassOf rdf:resource="http://purl.org/olia/mte/multext-east.owl#ConjunctionFormation"/>
        <rdfs:comment>e.g., aşa_că, va_să_zică (ro)</rdfs:comment>
        <rdfs:comment>e.g., mabej/mabej, prit nikoj/pridniköj, sa ito kir/zajtökir, sauvocha/zawojoka (sl-rozaj)</rdfs:comment>
        <rdfs:comment>e.g., а_пък (bg)</rdfs:comment>
        <rdfs:comment>e.g., аби-но аби-то все-таки для того щоб за винятком замість того щоб не вважаючи на те що не зважаючи на те що отож-то тим-то тільки-но тому що усе-таки якби-то, при цьому та й (uk)</rdfs:comment>
        <rdfs:comment>e.g., برخلافِ/برخلاف برايِ‌همين آن‌چنانکه, به‌اين‌دليل‌که ازبس‌که ازآنجاکه (fa)</rdfs:comment>
        <rdfs:comment>Conjunction/Formation=&quot;compound&quot;&lt;br/&gt;

In Romanian, CompoundConjunction refers to conjunctions formed periphrastically, with some word/phrase combined by a conjunction: din moment ce, fără să, fat,ă de cum etc. Also compare Resian za wojo ki / because.  MTE v4)</rdfs:comment>
    </owl:Class>
    


    <!-- http://purl.org/olia/mte/multext-east.owl#CompoundInterjection -->

    <owl:Class rdf:about="http://purl.org/olia/mte/multext-east.owl#CompoundInterjection">
        <rdfs:subClassOf rdf:resource="http://purl.org/olia/mte/multext-east.owl#InterjectionFormation"/>
        <rdfs:comment>Interjection/Formation=&quot;compound&quot;</rdfs:comment>
    </owl:Class>
    


    <!-- http://purl.org/olia/mte/multext-east.owl#CompoundParticle -->

    <owl:Class rdf:about="http://purl.org/olia/mte/multext-east.owl#CompoundParticle">
        <rdfs:subClassOf rdf:resource="http://purl.org/olia/mte/multext-east.owl#ParticleFormation"/>
        <rdfs:comment>e.g., а_бе, ей-сега, ей-тъй (bg)</rdfs:comment>
        <rdfs:comment>Particle/Formation=&quot;compound&quot;</rdfs:comment>
    </owl:Class>
    


    <!-- http://purl.org/olia/mte/multext-east.owl#Conditional -->

    <owl:Class rdf:about="http://purl.org/olia/mte/multext-east.owl#Conditional">
        <rdfs:subClassOf rdf:resource="http://purl.org/olia/mte/multext-east.owl#VerbForm"/>
        <rdfs:comment>In Bulgarian and Slovak, the conditional is expressed roughly in the same way, by using a separate word би, by, and the L-participle form (called just participle in Bulgarian). Slovak by is for the MTE purpose highly arbitrarily classified as a verb in conditional (Vform=conditional(c), the only such verb). No other grammar categories (person, gender, tense) are marked, purely for pragmatic reasons – to avoid the need of disambiguation. On the other hand, the Bulgarian би is classified as a full verb, Vform=active(a)
(Dimitrova et al. 2009)</rdfs:comment>
        <rdfs:comment>e.g., bi&apos;/biti, bi/biti, bih/biti, bismo/biti, biste/biti, biše/biti (sr)</rdfs:comment>
        <rdfs:comment>e.g., bude/byť, budem/byť, budeme/byť, budete/byť, budeš/byť, budú/byť, by, nepostačia/nestačiť, nepostačí/nestačiť (sk)</rdfs:comment>
        <rdfs:comment>e.g., by, bych/by, bychom/by, bys/by, byste/by (cs)</rdfs:comment>
        <rdfs:comment>e.g., byliby/być, byłaby/być, byłby/być, byłbyś/być, byłoby/być, byłyby/być, byłybyście/być, byłybyśmy/być, chciałaby/chcieć (pl)</rdfs:comment>
        <rdfs:comment>e.g., lennétek/lesz, továbbtaníttatnátok/továbbtaníttat, tudnálak/tud, tudnátok/tud, venné/vesz, veszélyeztetné/veszélyeztet, visszakapná/visszakap (hu)</rdfs:comment>
        <rdfs:comment>e.g., oleks/olema, oleksime/olema, oleksin/olema, oleksite/olema, olekski/olema, olnuks/olema, olnukski/olema, peetaks/pidama, polnuks/olema (et)</rdfs:comment>
        <rdfs:comment>e.g., were/be, weren&apos;t/be+not (en)</rdfs:comment>
    </owl:Class>
    


    <!-- http://purl.org/olia/mte/multext-east.owl#Conjunction -->

    <owl:Class rdf:about="http://purl.org/olia/mte/multext-east.owl#Conjunction">
        <rdfs:subClassOf rdf:resource="http://purl.org/olia/mte/multext-east.owl#MorphosyntacticCategory"/>
        <rdfs:subClassOf>
            <owl:Class>
                <owl:intersectionOf rdf:parseType="Collection">
                    <owl:Restriction>
                        <owl:onProperty rdf:resource="http://purl.org/olia/mte/multext-east.owl#hasClitic"/>
                        <owl:maxCardinality rdf:datatype="http://www.w3.org/2001/XMLSchema#nonNegativeInteger">1</owl:maxCardinality>
                    </owl:Restriction>
                    <owl:Restriction>
                        <owl:onProperty rdf:resource="http://purl.org/olia/mte/multext-east.owl#hasConjunctionFormation"/>
                        <owl:maxCardinality rdf:datatype="http://www.w3.org/2001/XMLSchema#nonNegativeInteger">1</owl:maxCardinality>
                    </owl:Restriction>
                    <owl:Restriction>
                        <owl:onProperty rdf:resource="http://purl.org/olia/mte/multext-east.owl#hasNumber"/>
                        <owl:maxCardinality rdf:datatype="http://www.w3.org/2001/XMLSchema#nonNegativeInteger">1</owl:maxCardinality>
                    </owl:Restriction>
                    <owl:Restriction>
                        <owl:onProperty rdf:resource="http://purl.org/olia/mte/multext-east.owl#hasPerson"/>
                        <owl:maxCardinality rdf:datatype="http://www.w3.org/2001/XMLSchema#nonNegativeInteger">1</owl:maxCardinality>
                    </owl:Restriction>
                </owl:intersectionOf>
            </owl:Class>
        </rdfs:subClassOf>
        <rdfs:comment>As for the overlap between Adverb and Conjunction, Adverb/Type=&quot;portmanteau&quot; was introduced for Romanian to cover some few words which can be both adverbs and conjunctions (with adverbial reading more frequent). Romanian Conjunction/Type=&quot;portmanteau&quot; applies only to the word &quot;şi&quot; which can be both a coordonating conjunction and an adverb. The distinctionamong these interpretations is rather tricky for the average native speaker and was a constant source of noise in automatic tagging. Therefore, for the sake of automatic processing we defined this &quot;portmanteau&quot; type value. (MTE v4)</rdfs:comment>
        <rdfs:comment>e.g., - (hu)</rdfs:comment>
        <rdfs:comment>e.g., a/a, i/i, że/że (pl)</rdfs:comment>
        <rdfs:comment>e.g., aby, abych/aby, abychom/aby, abys/aby, abyste/aby, kdyby, kdybych/kdyby, kdybychom/kdyby, kdybys/kdyby (cs)</rdfs:comment>
        <rdfs:comment>e.g., ano/anu, anu/anu, k/ka, kir/kir, k’/ka, mabej/mabej, prit nikoj/pridniköj, sa ito kir/zajtökir, sauvocha/zawojoka (sl-rozaj)</rdfs:comment>
        <rdfs:comment>e.g., as, either, neither (en)</rdfs:comment>
        <rdfs:comment>e.g., aşa_că, va_să_zică (ro)</rdfs:comment>
        <rdfs:comment>e.g., а або абощо але ані зате зачим і іно й йно но однак одначе притім притому причім причому проте та, аби адже аж аніж ба бо буцім буцімто все втім гейби доки допіру допоки же заки заким замісто зас коб, аби-но аби-то все-таки для того щоб за винятком замість того щоб не вважаючи на те що не зважаючи на те що отож-то тим-то тільки-но тому що усе-таки якби-то, при цьому та й (uk)</rdfs:comment>
        <rdfs:comment>e.g., а_пък (bg)</rdfs:comment>
        <rdfs:comment>e.g., برخلافِ/برخلاف برايِ‌همين آن‌چنانکه, به‌اين‌دليل‌که ازبس‌که ازآنجاکه, حتي اگه/اگر اگر, طيِّ/طيّ ضمناً بلکه (fa)</rdfs:comment>
    </owl:Class>
    


    <!-- http://purl.org/olia/mte/multext-east.owl#ConjunctionFormation -->

    <owl:Class rdf:about="http://purl.org/olia/mte/multext-east.owl#ConjunctionFormation">
        <rdfs:subClassOf rdf:resource="http://purl.org/olia/mte/multext-east.owl#Formation"/>
        <rdfs:comment>Conjunction/Formation refers to the graphical components: simple, i.e. consisting of one word; compound, i.e. consisting of more than one word. (MTE v4)</rdfs:comment>
    </owl:Class>
    


    <!-- http://purl.org/olia/mte/multext-east.owl#CoordinatingConjunction -->

    <owl:Class rdf:about="http://purl.org/olia/mte/multext-east.owl#CoordinatingConjunction">
        <rdfs:subClassOf rdf:resource="http://purl.org/olia/mte/multext-east.owl#Conjunction"/>
        <rdfs:comment>e.g., - (hu)</rdfs:comment>
        <rdfs:comment>e.g., ano/anu, anu/anu, prit nikoj/pridniköj, tácui/takoj (sl-rozaj)</rdfs:comment>
        <rdfs:comment>e.g., as, either, neither (en)</rdfs:comment>
        <rdfs:comment>e.g., aşa_că, va_să_zică (ro)</rdfs:comment>
        <rdfs:comment>e.g., а або абощо але ані зате зачим і іно й йно но однак одначе притім притому причім причому проте та, при цьому та й (uk)</rdfs:comment>
        <rdfs:comment>e.g., а_пък (bg)</rdfs:comment>
        <rdfs:comment>e.g., برخلافِ/برخلاف برايِ‌همين آن‌چنانکه, طيِّ/طيّ ضمناً بلکه (fa)</rdfs:comment>
        <rdfs:comment>Conjunction/Type=&quot;coordinating&quot;</rdfs:comment>
        <owl:versionInfo>CoordinatingConjunction conflates two different classifications of conjunctions:
(a) according to position and distribution
(b) according to the elements conjoined.

These are resolved here by CoordinatingConjunction_PositionalType and CoordinatingConjunction_ConjunctType.</owl:versionInfo>
    </owl:Class>
    


    <!-- http://purl.org/olia/mte/multext-east.owl#CoordinatingConjunction_ConjunctType -->

    <owl:Class rdf:about="http://purl.org/olia/mte/multext-east.owl#CoordinatingConjunction_ConjunctType">
        <rdfs:subClassOf rdf:resource="http://purl.org/olia/mte/multext-east.owl#CoordinatingConjunction"/>
        <rdfs:comment>CoordinatingConjunction originally conflated two different classifications of conjunctions:
(a) according to position and distribution (CoordinatingConjunction_PositionalType)
(b) according to the elements conjoined (CoordinatingConjunction_ConjunctType).</rdfs:comment>
    </owl:Class>
    


    <!-- http://purl.org/olia/mte/multext-east.owl#CoordinatingConjunction_PositionalType -->

    <owl:Class rdf:about="http://purl.org/olia/mte/multext-east.owl#CoordinatingConjunction_PositionalType">
        <rdfs:subClassOf rdf:resource="http://purl.org/olia/mte/multext-east.owl#CoordinatingConjunction"/>
        <rdfs:comment>CoordinatingConjunction originally conflated two different classifications of conjunctions:
(a) according to position and distribution (CoordinatingConjunction_PositionalType)
(b) according to the elements conjoined (CoordinatingConjunction_ConjunctType).</rdfs:comment>
    </owl:Class>
    


    <!-- http://purl.org/olia/mte/multext-east.owl#CopulaVerb -->

    <owl:Class rdf:about="http://purl.org/olia/mte/multext-east.owl#CopulaVerb">
        <rdfs:subClassOf rdf:resource="http://purl.org/olia/mte/multext-east.owl#Verb"/>
        <rdfs:comment>e.g., bejt/být, budete/být, byste/by, jste/být, nebudete/být, nebýt/být, nejste/být, ste/být (cs)</rdfs:comment>
        <rdfs:comment>e.g., bet/bet, bit/bet, biti/bet, mata/mët, ostane/ostät, sta/bet, stè/bet, stö/bet, teita/tët (sl-rozaj)</rdfs:comment>
        <rdfs:comment>e.g., budete/byť, buďte/byť, ste/byť (sk)</rdfs:comment>
        <rdfs:comment>Verb/Type=&quot;copula&quot;&lt;br/&gt;

Depending on the language-specific classification of verbs in terms of their forms or functions, Verb/Type=&quot;copula&quot; is either applied to forms of the verb &quot;to be&quot; in all its functions (e.g., Czech &quot;být&quot;, Slovak &quot;byť&quot;), or restricted to occasions where it serves as a copula (e.g., Resian &quot;byt&quot;). (MTE v4)

Copula verbs are inflected, so that the corresponding Macedonian word bi is considered as particle, rather than verb copula (in contrast to other copula it doesn&apos;t inflect for person / number) (Tomaz Erjavec, email 2010/06/09)</rdfs:comment>
        <owl:versionInfo>The comments on copula indicate a problem: In some schemes, Type=&quot;copula&quot; is assigned to all forms of (the translated forms of) &quot;to be&quot;, and thus to be understood as *potential copula verb*, whereas other schemes classify properly according to functions. However, one cannot tell from MTE tags when which model is applied. The MTE types are thus to be interpreted as *potential* copula, etc., i.e., &quot;olia:CopulaVerb or olia:AuxiliaryVerb or olia:LexicalVerb&quot;.</owl:versionInfo>
    </owl:Class>
    


    <!-- http://purl.org/olia/mte/multext-east.owl#CorrelativeCoordinatingConjunction -->

    <owl:Class rdf:about="http://purl.org/olia/mte/multext-east.owl#CorrelativeCoordinatingConjunction">
        <rdfs:subClassOf rdf:resource="http://purl.org/olia/mte/multext-east.owl#CoordinatingConjunction_PositionalType"/>
        <rdfs:comment>Conjunction/Coord_Type=&quot;correlat&quot; (Romanian).

In Romanian, there are three kinds of conjunctions depending on their usage: as such or together with other conjunctions or adverbs: (1) simple, between conjuncts: Ion ori Maria (John or Mary); (2) repetitive, before each conjunct: fie Ion fie Maria fie... (either John or Mary or...) (3) correlative, before a conjoined phrase, it requires specific coordinators between conjuncts: atât mama cât şi tata (both mother and father). (MTE v4)</rdfs:comment>
    </owl:Class>
    


    <!-- http://purl.org/olia/mte/multext-east.owl#CountNumber -->

    <owl:Class rdf:about="http://purl.org/olia/mte/multext-east.owl#CountNumber">
        <rdfs:subClassOf rdf:resource="http://purl.org/olia/mte/multext-east.owl#Number"/>
        <rdfs:comment>Number=&quot;count&quot; (Nouns in Serbian, Macedonian, Bulgarian), e.g., Bulgarian яка/як, язовира/язовир, яда/яд, юргана/юрган, юбилея/юбилей, ъгъла/ъгъл</rdfs:comment>
    </owl:Class>
    


    <!-- http://purl.org/olia/mte/multext-east.owl#Courtesy -->

    <owl:Class rdf:about="http://purl.org/olia/mte/multext-east.owl#Courtesy">
        <rdfs:subClassOf rdf:resource="http://purl.org/olia/mte/multext-east.owl#MorphosyntacticFeature"/>
        <rdfs:comment>feature &quot;Courtesy&quot;&lt;br/&gt;

In Resian, the attribute Courtesy is relevant for the 2nd person plural, where forms in &apos;-ta&apos; refer to a plural subject and &apos;-të&apos; to a singular subject. For Slovene this attribute is not used, even though the distinction is made in a similar manner. (MTE v4)&lt;br/&gt;

In Persian,  instead of the singular form of the verb, the plural form is used to refer to a singular subject for reasons of couresy. In fact, such attributes for Farsi are not found in traditional grammar books.
(Qasemizadeh and Rahimi 2006)
</rdfs:comment>
    </owl:Class>
    


    <!-- http://purl.org/olia/mte/multext-east.owl#DativeCase -->

    <owl:Class rdf:about="http://purl.org/olia/mte/multext-east.owl#DativeCase">
        <rdfs:subClassOf rdf:resource="http://purl.org/olia/mte/multext-east.owl#Case"/>
        <rdfs:comment>e.g., , drugemu/drug, drugi/drug, drugim/drug, dvema/dva, enemu/en, enim/en, Hrvatoma/Hrvat, jim/on (sl)</rdfs:comment>
        <rdfs:comment>e.g., -, akiknek/aki, amelyeknek/amely, azoknak/az, egyikének/egyik, egyiküknek/egyik, egymásnak/egymás, egytizedének/egytized, egyének/egy (hu)</rdfs:comment>
        <rdfs:comment>e.g., -i/el, -şi/sieşi, i-/el, i/el, le/el, li/el, mi/eu, mie/eu, ne/noi (ro)</rdfs:comment>
        <rdfs:comment>e.g., 0, Аахену/Аахен Аахенові/Аахен Абаю/Абай Абаєві/Абай Абакану/Абакан Абаканові/Абакан Абакану/Абакан Абаканові/Абакан Абіджану/Абіджан Абіджанові/Абіджан Абовяну/Абовян Абовянові/Абовян Авентину/Авентин Авентинові/Авентин Адамстауну/Адамстаун Адамстаунові/Адамстаун Адену/Аден Аденові/Аден Аджаристану/Аджаристан Аджаристанові/Аджаристан, Або/= Абруццо/= Абу-Дабі/= Адріатичному морю/Адріатичне море Азовському морю/Азовське море Айдахо/= Ай-Петрі/= Аконкагуа/= Актау/= Алеппо/= Аліканте/= Алмати/= Альбі/= Андаманському морю/Андаманське море Анжу/= Ані/= Антананаріву/= Антигуа/= Апіа/= Апостоловому/Апостолове, Абіссінії/Абіссінія Абуджі/Абуджа Абхазії/Абхазія Авдіївці/Авдіївка Австралії/Австралія Австрії/Австрія Австро-Угорщині/Австро-Угорщина Аддис-Абебі/Аддис-Абеба Аджарії/Аджарія Адигеї/Адигея Адріатиці/Адріатика Азії/Азія Айові/Айова Аквітанії/Аквітанія Аккрі/Аккра Ак-Мечеті/Ак-Мечеть Акмолі/Акмола акриловій кислоті/акрилова кислота Алабамі/Алабама Албанії/Албанія, Азорським островам/Азорські острови Аландським островам/Аландські острови Алеутським островам/Алеутські острови Андаманським островам/Андаманські острови Антильським островам/Антильські острови Багамським островам/Багамські острови Балеарським островам/Балеарські острови Бельбекам/Бельбек Бермудським островам/Бермудські острови Бугам/Буг Великодням/Великдень Великим Сорочинцям/Великі Сорочинці Віргінським островам/Віргінські острови Гавайським островам/Гавайські острови Гебридським островам/Гебридські острови Драконовим горам/Драконові гори ЖЕКам/ЖЕК Зеленого Мису островам/Зеленого Мису острови Змієвим валам/Змієві вали Зондським островам/Зондські острови, Альпам/Альпи Андам/Анди Апеннінам/Апенніни Аппалачам/Аппалачі Арденнам/Арденни Афінам/Афіни Багамам/Багами Балканам/Балкани Байдарським воротам/Байдарські ворота Барановичам/Барановичі Бендерам/Бендери Березнякам/Березняки Бермудам/Бермуди Бескидам/Бескиди Біличам/Біличі Близнюкам/Близнюки Богородчанам/Богородчани Боровичам/Боровичі Бортничам/Бортничі Броварам/Бровари, Америкам/Америка Андалуським горам/Андалуські гори Атлаським горам/Атлаські гори Бистрицям/Бистриця Держдумам/Держдума Жовтим Водам/Жовті Води Збройним Силам України/Збройні сили України Індіям/Індія Інтернет-газетам/Інтернет-газета Караваєвим дачам/Караваєві дачі Магеллановим хмарам/Магелланові хмари Македоніям/Македонія Мате Залка/= Пасхам/Пасха Пилипівкам/Пилипівка Радам/Рада Родезіям/Родезія Інтернет-технологіям/Інтернет-технологія, Антроповим/Антропов Абакумам/Абакум Абакумовичам/Абакумович Абалкіним/Абалкін Абашидзе/= Аббасам/Аббас Абдулам/Абдула Абдуллоджановим/Абдуллоджанов Абелям/Абель Абовянам/Абовян Абрамам/Абрам Абрамовичам/Абрамович Абрамовичам/Абрамович Абрамчукам/Абрамчук Абуладзе/= Авакумам/Авакум Авакумовичам/Авакумович Августам/Август Августимовим/Августимов Августинам/Августин, Антроповим/Антропов Абакумівнам/Абакумівна Абалкіним/Абалкін Абашидзе/= Абдуллоджановим/Абдуллоджанов Абрамівнам/Абрамівна Абуладзе/= Авакумівнам/Авакумівна Августам/Августа Августимовим/Августимов Августинівнам/Августинівна Авдієвським/Авдієвський Авенірівнам/Авенірівна Аверіним/Аверін Аверкіївнам/Аверкіївна Авер&apos;янівнам/Авер&apos;янівна Авіятам/Авіята Авксентіївнам/Авксентіївна Авогадро/= Аврамівнам/Аврамівна (uk)</rdfs:comment>
        <rdfs:comment>e.g., Bohù/bug, dnej/dän, dnumu/dän, dobrim/dobar, druhemu/drügi, druhomu/drügi, dulsnichen/dužnïk, dušici/dušïca, dužnikaên/dužnïk (sl-rozaj)</rdfs:comment>
        <rdfs:comment>e.g., XXVII/xxvii, Дарданеллам/дарданелла, Двум/два, Иванам/иван, МНЕ/я, Мне/я, НАМ/мы, Нам/мы, Обоим/оба (ru)</rdfs:comment>
        <rdfs:comment>e.g., amerykańskiej/amerykański, amerykańskim/amerykański, awansującym/awansować, całemu/cały, celowi/cel, choremu/chory, ci/ty, czemu/co, czemuś/coś (pl)</rdfs:comment>
        <rdfs:comment>e.g., desaterým/desaterý, devatenácté/devatenáctý, devatenáctému/devatenáctý, devatenáctým/devatenáctý, druhé/druhý, druhému/druhý, druhým/druhý, dvojí, dvěma/dva (cs)</rdfs:comment>
        <rdfs:comment>e.g., druhej/druhý, druhému/druhý, druhým/druhý, dvom/dva, hentej/hentá, hentomu/hento, hentým/hento, hentým/hentá, ich (sk)</rdfs:comment>
        <rdfs:comment>e.g., dvojim/dvoje, grupama/grupa, im/ona, im/one, im/oni, jednoj/jedan, jednom/jedan, jednome/jedan, jednomu/jedan (sr)</rdfs:comment>
        <rdfs:comment>e.g., Вам/Вие, Ви/Вие, вам/вие, ви/вие, и/таа, им/тие, кому/кој, мене/јас, ми/јас (mk)</rdfs:comment>
        <rdfs:comment>e.g., вам, всекиму/всеки, им/те, й/тя, кому/кой, комуто/който, мен/аз, мене/аз, мене_ми (bg)</rdfs:comment>
    </owl:Class>
    


    <!-- http://purl.org/olia/mte/multext-east.owl#Definite -->

    <owl:Class rdf:about="http://purl.org/olia/mte/multext-east.owl#Definite">
        <rdfs:subClassOf rdf:resource="http://purl.org/olia/mte/multext-east.owl#AmbiguousDefinitenessFeature"/>
        <rdfs:subClassOf>
            <owl:Class>
                <owl:unionOf rdf:parseType="Collection">
                    <rdf:Description rdf:about="http://purl.org/olia/mte/multext-east.owl#CliticDefiniteDeterminer"/>
                    <rdf:Description rdf:about="http://purl.org/olia/mte/multext-east.owl#CliticSpecificDeterminer"/>
                    <rdf:Description rdf:about="http://purl.org/olia/mte/multext-east.owl#PersonOfObject"/>
                </owl:unionOf>
            </owl:Class>
        </rdfs:subClassOf>
        <rdfs:comment>e.g., -nsutitelor/însutit, -nsutitului/însutit, -nsutiţilor/însutit, -ntreitelor/întreit, -ntreitului/întreit, -ntreiţilor/întreit, -ntâia/întâi, -ntâiaşi/întâi, -ntâii/întâi (ro)</rdfs:comment>
        <rdfs:comment>e.g., Boshij/böžji, delečni/dalëčnji, dobre/dobar, Erove/jëruw, Rozajanski/rozajanski, sami/sam, shihnani/žignan, Svete/svet, tulste/tulst (sl-rozaj)</rdfs:comment>
        <rdfs:comment>e.g., drugi/drug, dvojni/dvojen (sl)</rdfs:comment>
        <rdfs:comment>e.g., gipsani/gipsan, inkriminisani/inkriminisan, neustrašivi/neustrašiv, omiljeni/omiljen, popravljeni/popravljen, propisani/propisan, rasni/rasan, uobičajeni/uobičajen, ženskog/ženski (sr)</rdfs:comment>
        <rdfs:comment>e.g., lennétek/lesz, továbbtaníttatnátok/továbbtaníttat, tudnátok/tud, uralhatjátok/uralhat, venné/vesz, veszélyeztetné/veszélyeztet, visszakapná/visszakap, visszautazom/visszautaz, visszautazom/visszautazik (hu)</rdfs:comment>
        <rdfs:comment>e.g., БАЛКАНИТЕ, Балканите, Зайченцето, Лудогорието, Филипините, Черноморието, бъдещата/бъда, бъдещите/бъда, бъдещото/бъда (bg)</rdfs:comment>
        <rdfs:comment>e.g., Винстоне/Винстон, Македонецот/Македонец, Македонката/Македонка, Македонките/Македонка, Македонците/Македонец, Македончето/Македонче, Македончињата/Македонче, Мартине/Мартин, Медитеранот/Медитеран (mk)</rdfs:comment>
        <rdfs:comment>e.g., بِ/ب اينگسوسِ/اينگسوس اسميتِ/اسميت, ميني‌ترو سن‌باستين ب-ب, پسرهٔ/پسر (fa)</rdfs:comment>
        <rdfs:comment>Definiteness=&quot;yes&quot; (Noun/Adjective: Romanian, Macedonian, Bulgarian, Persian; Verb: Bulgarian, Hungarian; Pronoun: Resian, Macedonian, Bulgarian)&lt;br/&gt;

In Romanian, nouns can be marked for definiteness with the enclitic definite article. In noun-adjective construction, the definite article may attach enclitically to either adjectives or modified nouns (never to both of them). If present, the definite article attaches to the right of the first word in the sequence, e.g. Bunul om (The kind man) v.s. Omul bun. (The kind man) (MTE v4)&lt;br/&gt;

For Macedonian, the definiteness attributes can take the values: non definite (no), generally definite (yes), definite at short visible distance (proximal), and definite at longer visible distance (distal). (MTE v4)&lt;br/&gt;

Persian does have an article, but it marks specificity rather than definiteness. (Ivan A. Derzhanski, email 2010/06/18) According to Qasemizadeh &amp; Rahimi&apos;s (2006) description of tokenization, Definiteness of Nouns etc. thus refers to an orthographically non-separated definite (specifity-marking) article.</rdfs:comment>
    </owl:Class>
    


    <!-- http://purl.org/olia/mte/multext-east.owl#DefiniteArticle -->

    <owl:Class rdf:about="http://purl.org/olia/mte/multext-east.owl#DefiniteArticle">
        <rdfs:subClassOf rdf:resource="http://purl.org/olia/mte/multext-east.owl#Article"/>
        <rdfs:comment>e.g., -a, -ilor, -istei, -istele, -istelor, -istul, -istului, -iştii, -iştilor (ro)</rdfs:comment>
        <rdfs:comment>e.g., a, az (hu)</rdfs:comment>
        <rdfs:comment>e.g., itoga/te, ta/te, taga/te, te/te, teh/te, temi/te, tey/te, ti/te, tih/te (sl-rozaj)</rdfs:comment>
        <rdfs:comment>Article/Type=&quot;definite&quot; is used in the Romanian, Hungarian and Resian MTE v4 specs.&lt;br/&gt;

Hungarian has tree articles: a, az and egy. a and az are definite. These may not have number and case. The word &apos;az&apos; may have but that is a pronoun in those cases. (MTE v4)&lt;br/&gt;
The definite article in Resian is &apos;te ta tö&apos; and formally distinct from the demonstrative pronoun from which it derived: &apos;jte jta jtö&apos;. (MTE v4)</rdfs:comment>
    </owl:Class>
    


    <!-- http://purl.org/olia/mte/multext-east.owl#Definiteness -->

    <owl:Class rdf:about="http://purl.org/olia/mte/multext-east.owl#Definiteness">
        <rdfs:subClassOf rdf:resource="http://purl.org/olia/mte/multext-east.owl#MorphosyntacticFeature"/>
        <rdfs:comment>Like Cliticness, Definiteness assembles a number of *different* phenomena grouped together under a single MTE attribute.

Definiteness refers to the definite and indefinite article in English, Bulgarian and Romanian, for the difference between long and short adjective inflection in other Slavic languages, for verbal agreement features of the Hungarian verb.

Bulgarian Definiteness attribute: One of the most important grammatical characteristics of the new Bulgarian language which sets it apart from the rest of the Slavic languages is the existence of a definite article. The definite article is a morphological indicator of the grammatical category determination (definiteness). The definite article is not a particle (particles are a separate category of words – parts-of-speech, while the article is not a separate word), nor is it a simple suffix, but a meaningful compound part of the word. It is a word-forming morpheme, which is placed at the end of words in order to express definiteness, familiarity, acquaintance (Bulgarian Grammar, 1993). In Bulgarian, nouns, adjectives, numerals, and full-forms of the possessive pronouns and participles can acquire an article. For the singular masculine article, there are two forms: a full article(f)[l.s.] and a short article(s)[l.s.]. The full article is used when a singular masculine form is the syntactic subject of the clause, otherwise a short one is used – a purely orthographic rule. The distinction of full vs. short is not made for feminine, neuter and plural forms, and we use just the yes(y) or no(n) to mark definiteness or respectively lack thereof. Therefore, the definiteness attribute can take overall 4 different values: indefinite(n), definitive(y), short article(s), full article(f). (Dimitrova et al. 2009)

In Polish, the vocalicity of (a)gglutinated forms like -em vs -m is mapped on the Definiteness attribute with its values &quot;(f)ull-art&quot; and &quot;(s)hort-art&quot; respectively, meaning &quot;full form&quot; and &quot;short form&quot;. The IPIC flexeme winien and predicatives like rad are treated as short adjectives—Definiteness=&quot;short-art&quot;. The terms are very artificial, but this category is used due to the similarity of the phenomenon. (MTE v4)&lt;br/&gt;

One of MTE v.3’s most perplexing choices is that it uses the same binary feature Definiteness of the part of speech Verb to indicate, in Bulgarian, that a participle bears a definite article (говорилите ‘the ones who talked’), and in Hungarian, that a finite form of a transitive verb has a definite 3rd person direct object (tanulom ‘I learn it’). Thus two totally dissimilar (not to mention unrelated) phenomena are handled alike merely because their names in the respective grammatical traditions happen to mean the same. In MTE v.4 the tagset for Persian encodes izafet as Case=genitive (i.e., practically the opposite!) in an effort to avoid introducing a language-specific feature.
(Derzhanski and Kotsyba 2009)&lt;br/&gt;

Hungarian Definiteness (of verbs):
In simple terms, it means that the verb takes a definite object, 
which is reflected in the type of verb conjugation. 
Eg. in Hungarian there will be two forms of the verb &apos;see&apos; here
1. I can see an elephant.
2. I can see the elephant.
depending on the definiteness of the object, &apos;látok&apos; vs. &apos;látom&apos;.
The above 1s2s form of verbs takes a 1st person singular subject and
2nd person definite object (which in actual fact can also be plural not only
singular). Both subject and object can be (pro)dropped. Eg.
I can see you -&gt; (Én) látlak (téged/titeket)
                  I    see     you_sg/you_pl
(Csaba Oravecz, email 2010/06/15)&lt;br/&gt;

Persian:
In Farsi, Nouns are inflected for number and Definiteness. ... Farsi adjectives are inflected for degree and definiteness.
(Qasemizadeh and Rahimi 2006)</rdfs:comment>
        <owl:versionInfo>Definiteness covers a broad variety of phenomena, incl.
- reduction (in Slavic languages without determiner, Serge Sharoff, email 2010/06/09)
- distinction between definite and indefinite article (English)
- distinction between different types (or absence) of cliticized articles (Bulgarian, Macedonian)
- definite and indefinite verbal conjungations (depending on the object of a verb; Hungarian, Csaba Oravecz, http://en.wikipedia.org/wiki/Hungarian_grammar_(verbs)#Definite_and_indefinite_conjugations)
</owl:versionInfo>
    </owl:Class>
    


    <!-- http://purl.org/olia/mte/multext-east.owl#Degree -->

    <owl:Class rdf:about="http://purl.org/olia/mte/multext-east.owl#Degree">
        <rdfs:subClassOf rdf:resource="http://purl.org/olia/mte/multext-east.owl#MorphosyntacticFeature"/>
        <rdfs:comment>A feature of adjectives. In some languages, e.g., Hungarian and Slovak, also some adverbs may have degree. (MTE v4)</rdfs:comment>
    </owl:Class>
    


    <!-- http://purl.org/olia/mte/multext-east.owl#DelativeCase -->

    <owl:Class rdf:about="http://purl.org/olia/mte/multext-east.owl#DelativeCase">
        <rdfs:subClassOf rdf:resource="http://purl.org/olia/mte/multext-east.owl#Case"/>
        <rdfs:comment>e.g., -, akikről/aki, amelyekről/amely, arcodról/arc, arról/az, azokról/az, cselekedeteidről/cselekedet, egyebekről/egyéb, egyikükről/egyik (hu)</rdfs:comment>
        <rdfs:comment>Case=&quot;delative&quot; (Hungarian)</rdfs:comment>
    </owl:Class>
    


    <!-- http://purl.org/olia/mte/multext-east.owl#DemandingClitic -->

    <owl:Class rdf:about="http://purl.org/olia/mte/multext-east.owl#DemandingClitic">
        <rdfs:subClassOf rdf:resource="http://purl.org/olia/mte/multext-east.owl#ElementWithoutClitic"/>
        <rdfs:comment>Clitic=&quot;demanding&quot; (Verb: Polish)&lt;br/&gt;

An element that contains a clitic which is, however, represented as a separate token.&lt;br/&gt;

Polish: Particles were extracted from the IPIC particle-adverbs category manually along with adverbs, pronouns and interjections and a few conjunctions. The Clitic attribute enables differentiating particles that are agglutinated to non-particles (value= &quot;a&quot;), e.g., by, że. The value &quot;y&quot; labels a composite particle such as niechby when treated as one word; alternatively it may be encoded as a aequence of two particles, the optionally demanding niech with Clitic=&quot;d&quot; and the agglutinant by with Clitic=&quot;a&quot;. (MTE v4)&lt;br/&gt;

This can be a subclass of ElementWithoutClitic. They are default though and won&apos;t be encoded in most cases. We only use them in some cases for Polish verbs. (Natalia Kotsyba, email 2010/06/21)
</rdfs:comment>
    </owl:Class>
    


    <!-- http://purl.org/olia/mte/multext-east.owl#DemonstrativeArticle -->

    <owl:Class rdf:about="http://purl.org/olia/mte/multext-east.owl#DemonstrativeArticle">
        <rdfs:subClassOf rdf:resource="http://purl.org/olia/mte/multext-east.owl#Article"/>
        <rdfs:comment>e.g., cea/cel, cei/cel, cel, cele/cel, celei/cel, celor/cel, celui/cel (ro)</rdfs:comment>
        <rdfs:comment>The demonstrative article (Article/Type=&quot;demonstrative&quot;) in Romanian links a definite noun to its determinants, links a numeral or an adjective to a noun, and it is a constituent part of the relative superlative (e.g. fata cea mare (the elder girl), cel lenes, (the lazy), respectively prietenul cel mai bun (the best friend)). (MTE v4)</rdfs:comment>
    </owl:Class>
    


    <!-- http://purl.org/olia/mte/multext-east.owl#DemonstrativeDeterminer -->

    <owl:Class rdf:about="http://purl.org/olia/mte/multext-east.owl#DemonstrativeDeterminer">
        <rdfs:subClassOf rdf:resource="http://purl.org/olia/mte/multext-east.owl#Determiner"/>
        <rdfs:comment>e.g., -acea/acel, -aceasta/acesta, -această/acest, -alea/ăla, -astea/ăsta, -ăia/ăla, -ăla/ăla, cealaltă/celălalt, ceastălaltă/cestălalt (ro)</rdfs:comment>
        <rdfs:comment>e.g., the (en)</rdfs:comment>
        <rdfs:comment>e.g., آن‌نوع آن‌دست آن (fa)</rdfs:comment>
        <rdfs:comment>Determiner/Type=&quot;demonstrative&quot; (English, Romanian, Persian)</rdfs:comment>
    </owl:Class>
    


    <!-- http://purl.org/olia/mte/multext-east.owl#DemonstrativePronoun -->

    <owl:Class rdf:about="http://purl.org/olia/mte/multext-east.owl#DemonstrativePronoun">
        <rdfs:subClassOf rdf:resource="http://purl.org/olia/mte/multext-east.owl#Pronoun"/>
        <rdfs:comment>e.g., -, abba/az, abból/az, addig/az, ahhoz/az, annál/az, arról/az, attól/az, azokban/az (hu)</rdfs:comment>
        <rdfs:comment>e.g., -alea/ăla, -astea/ăsta, -ăia/ăla, -ăla/ăla, -ăştia/ăsta, ast-/ăsta, ast/asta, celorlalte/celălalt, celorlalţi/celălalt (ro)</rdfs:comment>
        <rdfs:comment>e.g., ci/ten, dlatego/dlatego, owa/ów, owe/ów, owego/ów, owej/ów, owo/ów, owych/ów, owym/ów (pl)</rdfs:comment>
        <rdfs:comment>e.g., etej/iti, isa/isi, ise/isi, isi/isi, iso/isi, isà/isi, isè/isi, isó/isi, ite/iti (sl-rozaj)</rdfs:comment>
        <rdfs:comment>e.g., hentej/hentá, henten, hentie/henten, hentie/hento, hentie/hentá, hentoho/henten, hentoho/hento, hentom/hento, hentomu/hento (sk)</rdfs:comment>
        <rdfs:comment>e.g., nendeni/see, nendetagi/see, niisugustena/niisugune, samasugustena/samasugune, selleni/see, selleta/see, selletagi/see, sellistena/selline, teistsugused/teistsugune (et)</rdfs:comment>
        <rdfs:comment>e.g., ona/onaj, one/onaj, ove/ovaj, ovim/ovaj, ta/taj (sr)</rdfs:comment>
        <rdfs:comment>e.g., ti/ta, tistih/tisti, tistim/tisti (sl)</rdfs:comment>
        <rdfs:comment>e.g., tos/ten, týmiž/týž, těmahle/tenhle, těmi/ten, těmito/tento (cs)</rdfs:comment>
        <rdfs:comment>e.g., онака/онакий онакая/онакий она/оний оная/оний отака/отакий отакая/отакий отакісінька/отакісінький отакісінькая/отакісінький ота/отой отая/отой отся/отсей отсяя/отсей оттака/оттакий оттакая/оттакий отта/оттой оттая/оттой отця/отцей отцяя/отцей оця/оцей оцяя/оцей, онаке/онакий онакеє/онакий онеє/оний оне/оний оно/оний отаке/отакий отакеє/отакий отакісіньке/отакісінький отакісінькеє/отакісінький оте/отой отеє/отой отсе/отсей отсеє/отсей оттаке/оттакий оттакеє/оттакий отте/оттой оттеє/оттой отце/отцей отцеє/отцей оце/оцей, онакий/= оний/= отакий/= отакісінький/= отой/= отсей/= оттакий/= оттой/= отцей/= оцей/= перетакий/= позатой/= сей/= стільки/= стільки-то/= сякий/= сякий-такий/= такенний/= такий/= такий-сякий/=, онаким/онакий оним/оний отаким/отакий отакісіньким/отакісінький отим/отой отсим/отсей оттаким/оттакий оттим/оттой отцим/отцей оцим/оцей перетаким/перетакий позатим/позатой сим/сей стількома/стільки стількома-то/стільки-то сяким/сякий сяким-таким/сякий-такий такенним/такенний таким/такий таким-сяким/такий-сякий, онаким/онакий оним/оний отаким/отакий отакісіньким/отакісінький отим/отой отсим/отсей оттаким/оттакий оттим/оттой отцим/отцей оцим/оцей перетаким/перетакий позатим/позатой сим/сей сяким/сякий сяким-таким/сякий-такий такенним/такенний таким/такий таким-сяким/такий-сякий таким-то/такий-то такісіньким/такісінький, онакими/онакий оними/оний отакими/отакий отакісінькими/отакісінький отими/отой отсими/отсей оттакими/оттакий оттими/оттой отцими/отцей оцими/оцей перетакими/перетакий позатими/позатой сими/сей сякими/сякий сякими-такими/сякий-такий такенними/такенний такими/такий такими-сякими/такий-сякий такими-то/такий-то такісінькими/такісінький, онаких/онакий оних/оний отаких/отакий отакісіньких/отакісінький отих/отой отсих/отсей оттаких/оттакий оттих/оттой отцих/отцей оцих/оцей перетаких/перетакий позатих/позатой сих/сей сяких/сякий сяких-таких/сякий-такий такенних/такенний таких/такий таких-сяких/такий-сякий таких-то/такий-то такісіньких/такісінький, онакого/онакий оного/оний отакого/отакий отакісінького/отакісінький отого/отой отсього/отсей оттакого/оттакий оттого/оттой отцього/отцей оцього/оцей перетакого/перетакий позатого/позатой сього/сей стількох/стільки стількох-то/стільки-то сякого/сякий сякого-такого/сякий-такий такенного/такенний такого/такий такого-сякого/такий-сякий, онакого/онакий оного/оний отакого/отакий отакісінького/отакісінький отого/отой отсього/отсей оттакого/оттакий оттого/оттой отцього/отцей оцього/оцей перетакого/перетакий позатого/позатой сього/сей сякого/сякий сякого-такого/сякий-такий такенного/такенний такого/такий такого-сякого/такий-сякий такого-то/такий-то такісінького/такісінький (uk)</rdfs:comment>
        <rdfs:comment>e.g., толкова (bg)</rdfs:comment>
        <rdfs:comment>e.g., آنهايِ/آنها, ش/آن, شون/آنها شان/آنها آنهايي/آنها, همان‌ها/همان آنها, همين‌طور آن‌که آن, همين‌قدر اين‌گونه اين‌طوري/اين‌طور, يش/آن ش/آن اش/آن, يشان/آنها شان/آنها (fa)</rdfs:comment>
        <rdfs:comment>Pronoun/Type=&quot;demonstrative&quot;</rdfs:comment>
    </owl:Class>
    


    <!-- http://purl.org/olia/mte/multext-east.owl#DemonstrativeQuantifier -->

    <owl:Class rdf:about="http://purl.org/olia/mte/multext-east.owl#DemonstrativeQuantifier">
        <rdfs:subClassOf rdf:resource="http://purl.org/olia/mte/multext-east.owl#ProQuantifier"/>
        <rdfs:comment>In the Czech and Slovak MTE v4 specs, Numeral/Class=&quot;demonstrative&quot; are items meaning `this many/much&apos;, etc. Strictly speaking, they are pronumerals (pro-quantifiers), but traditional descriptions don&apos;t recognise such a category, so they are described variously as pronouns (because they contain a demonstrative element) or as numerals (because their syntactic distribution is that of numerals, or very close).&quot; (Ivan A Derzhanski, email 2010/06/11)</rdfs:comment>
    </owl:Class>
    


    <!-- http://purl.org/olia/mte/multext-east.owl#DeterminalPronoun -->

    <owl:Class rdf:about="http://purl.org/olia/mte/multext-east.owl#DeterminalPronoun">
        <rdfs:subClassOf rdf:resource="http://purl.org/olia/mte/multext-east.owl#Pronoun"/>
        <rdfs:comment>e.g., endasse/ise, endil/ise, endilt/ise, endisse/ise, enesesse/ise, igasse/iga, kõigiga/kõik, kõigiks/kõik, kõigil/kõik (et)</rdfs:comment>
        <rdfs:comment>DeterminalPronoun refers to an Estonian intensifier that is formally identical with the reflexive pronoun. Thus, Pronoun/Type=&quot;determinal&quot; in the Estonian MTE v4 specs is used for the emphatic/reflexive pronouns _ise_, _end(a)_ `(one)self&apos;.&quot; &lt;br/&gt;
Note that DeterminalPronoun is not to be confused with English pronominal determiners (attributive pronouns). (Ivan A. Derzhanski, email 2010/06/15; Heiki-Jaan Kaalep, email 2010/06/21; Gülzow 2006, p.258)
&lt;br/&gt;
Insa Gülzow (2006), The acquisition of intensifiers: Emphatic reflexives in English and German child language, Mouton de Gruyter, Berlin, p. 258</rdfs:comment>
        <owl:versionInfo>Heiki-Jaan Kaalep: &quot;When I created the MTE tables, I used &quot;Eesti keele grammatika II. Morfoloogia. Arv- ja asesõna&quot; Tartu, TÜ, 1981 (Grammar of Estonian II. Morphology. Numerals and pronouns. Tartu, Univ. of Tartu, 1981). The types of pronouns in MTE tables originate from p. 35 of this booklet.
However, grammar books of the current century give a different list of types for pronouns, and group the pronouns in somewhat different ways. There is no consensus about the issue at the moment, and no debate on it also, as far as I can tell.
Estonian determinal pronouns are not similar to the English determiners. However, all the determinal pronouns could be classified into other types (if we wanted to...), so we could get rid of this category altogether.&quot;
(Heiki-Jaan Kaalep, email 2010/06/21)</owl:versionInfo>
    </owl:Class>
    


    <!-- http://purl.org/olia/mte/multext-east.owl#Determiner -->

    <owl:Class rdf:about="http://purl.org/olia/mte/multext-east.owl#Determiner">
        <rdfs:subClassOf rdf:resource="http://purl.org/olia/mte/multext-east.owl#MorphosyntacticCategory"/>
        <rdfs:comment>Persian:
In traditional Farsi grammar, the category of determiners is not specified.
Considering morphosyntactic specifications of words and the place of them in phrasal structures, we believe that determiners can be specified as a PoS in Farsi. Moreover, this consideration is more consistent with other languages. Most of the words we have considered as determiners here are categorized as adjectives in traditional grammar. There are different types of determiners namely demonstrative, indefinite, interrogative, exclamative, and article.
(Qasemizadeh and Rahimi 2006)</rdfs:comment>
        <rdfs:comment>e.g., &apos;Er/her, &apos;is/his, a, an/a, her, his, its, my, our (en)</rdfs:comment>
        <rdfs:comment>e.g., -acea/acel, -aceasta/acesta, -această/acest, -alea/ăla, -astea/ăsta, -atât/atât, -atâta/atât, -mea/mea, -meu/meu (ro)</rdfs:comment>
        <rdfs:comment>e.g., آن‌نوع آن‌دست آن, تنها, يکي/يک يک يه/يک, چه‌قدر چه, چه‌مقدار چه‌جور چند, کليهٔ/کليه ساير انواعِ/نوع (fa)</rdfs:comment>
        <owl:versionInfo>Note that here, Articles are not a priori Determiners, but only if they are specified as such, i.e., by Determiner/Type=&quot;article&quot;</owl:versionInfo>
    </owl:Class>
    


    <!-- http://purl.org/olia/mte/multext-east.owl#DigitNumeral -->

    <owl:Class rdf:about="http://purl.org/olia/mte/multext-east.owl#DigitNumeral">
        <rdfs:subClassOf rdf:resource="http://purl.org/olia/mte/multext-east.owl#OrthographicalRepresentationOfNumeral"/>
        <rdfs:comment>e.g., -, 1900-tól/1900, 1970-re/1970, 2050-ig/2050, 2050-re/2050, 2050-től/2050 (hu)</rdfs:comment>
        <rdfs:comment>e.g., 1, 1. (mk)</rdfs:comment>
        <rdfs:comment>e.g., 1, 2, 3, 4 (cs)</rdfs:comment>
        <rdfs:comment>e.g., 1, 2, 3, 4 (sk)</rdfs:comment>
        <rdfs:comment>e.g., 1/1, 2/2, 3/3 (pl)</rdfs:comment>
        <rdfs:comment>e.g., 12/dwanijst, 32/trïstinudwa, 5/pet (sl-rozaj)</rdfs:comment>
        <rdfs:comment>e.g., 248, 59000, 7 (uk)</rdfs:comment>
        <rdfs:comment>Form=&quot;digit&quot;</rdfs:comment>
    </owl:Class>
    


    <!-- http://purl.org/olia/mte/multext-east.owl#Diminuitive -->

    <owl:Class rdf:about="http://purl.org/olia/mte/multext-east.owl#Diminuitive">
        <rdfs:subClassOf rdf:resource="http://purl.org/olia/mte/multext-east.owl#MorphologicalDerivation"/>
        <rdfs:comment>The value &apos;diminutive&apos; for Degree is used in Resian only, for derivated adjectives that end with the suffix &apos;-ić&apos; (MTE v.4). 
            In MTE, diminuitive was modelled as a feature of Degree. This is, however, misplaced, as there are languages where Degree and Diminuitivity are independent. 
            In Latvian, for example, the diminutive suffix may be attached to an adjective,
            not only in the positive but in the comparative and superlative degrees (Ruke-Dravina 1953).
            DiminuitiveDegree was thus renamed to Diminuitive and removed from Degree.
            
            Velta Ruke-Dravina (1953), Adjectival Diminuitives in Latvian. The Slavonic and East European Review  31(77): 452-465
        </rdfs:comment>
    </owl:Class>
    


    <!-- http://purl.org/olia/mte/multext-east.owl#DirectCase -->

    <owl:Class rdf:about="http://purl.org/olia/mte/multext-east.owl#DirectCase">
        <rdfs:subClassOf rdf:resource="http://purl.org/olia/mte/multext-east.owl#Case"/>
        <rdfs:comment>e.g., -acea/acel, -aceasta/acesta, -această/acest, -alea/ăla, -astea/ăsta, -atât/atât, -atâta/atât, -ist, -istele (ro)</rdfs:comment>
        <rdfs:comment>Case=&quot;direct&quot; (Romanian)&lt;br/&gt;

In the Romanian case system the value &apos;direct&apos; conflates &apos;nominative&apos; and &apos;accusative&apos;.</rdfs:comment>
    </owl:Class>
    


    <!-- http://purl.org/olia/mte/multext-east.owl#DistributiveCase -->

    <owl:Class rdf:about="http://purl.org/olia/mte/multext-east.owl#DistributiveCase">
        <rdfs:subClassOf rdf:resource="http://purl.org/olia/mte/multext-east.owl#Case"/>
        <rdfs:comment>e.g., -, egyenként/egy, hetenként/hét, ilyenként/ily, kéthetenként/kéthét, rekordonként/rekord, tömbönként/tömb, vércsoportonként/vércsoport (hu)</rdfs:comment>
        <rdfs:comment>
            The distributive case is used on nouns for the meanings of per or each.
            
            In Hungarian it is -nként and expresses the manner when something happens to each member of a set one by one (e.g., fejenként &quot;per head&quot;, esetenként &quot;in some case&quot;), or the frequency in time (hetenként &quot;once a week&quot;, tízpercenként &quot;every ten minutes&quot;).
            In the Finnish language, this adverb type is rare, even rarer in the singular. Its ending is -ttain/-ttäin. The basic meaning is &quot;separately for each&quot;. For example, maa (&quot;country&quot;) becomes maittain for an expression like Laki ratifioidaan maittain (&quot;The law is ratified separately in each country&quot;). It can be used to distribute the action to frequent points in time, e.g., päivä (day) has the plural distributive päivittäin (each day). It can mean also &quot;in (or with) regard to the (cultural) perspective&quot; when combined with a word referring to an inhabitant (-lais-). Frequently Finns (suomalaiset) say that suomalaisittain tuntuu oudolta, että, or &quot;in the Finnish perspective, it feels strange that&quot;.
            (http://en.wikipedia.org/wiki/Distributive_case)
        </rdfs:comment>
        <rdfs:comment>Case=&quot;distributive&quot; (Hungarian)</rdfs:comment>
    </owl:Class>
    


    <!-- http://purl.org/olia/mte/multext-east.owl#DualNumber -->

    <owl:Class rdf:about="http://purl.org/olia/mte/multext-east.owl#DualNumber">
        <rdfs:subClassOf rdf:resource="http://purl.org/olia/mte/multext-east.owl#Number"/>
        <rdfs:comment>e.g., bodita/biti, bosta/biti, hodita/hoditi, hočeta/hoteti, hočeva/hoteti, Hrvatoma/Hrvat, imata/imeti, nimata/imeti, nočeta/hoteti (sl)</rdfs:comment>
        <rdfs:comment>e.g., hardéhata/tet, mata/mët, Misteriha/mišterih, poznahata/poznät, pravijahata/pravit, prašávahata/pravit, sta/bet, tožna/tožan, ustala/wstät (sl-rozaj)</rdfs:comment>
        <rdfs:comment>e.g., stotine/stotina, ta/taj, tri, trima/tri, četiri (sr)</rdfs:comment>
        <rdfs:comment>e.g., těmahle/tenhle, zamaštěnýma/zamaštěný (cs)</rdfs:comment>
        <rdfs:comment>In Czech, the dual Number manifests itself in the instrumental Case of several Nouns denoting dual parts of the human body. (MTE v4)</rdfs:comment>
    </owl:Class>
    


    <!-- http://purl.org/olia/mte/multext-east.owl#DualQuantifier -->

    <owl:Class rdf:about="http://purl.org/olia/mte/multext-east.owl#DualQuantifier">
        <rdfs:subClassOf rdf:resource="http://purl.org/olia/mte/multext-east.owl#NumeralAgreementClass"/>
        <rdfs:comment>Numeral/Class=&quot;definite2&quot; (Czech)&lt;br/&gt;

Some feminine and neuter body parts in Czech have preserved dual forms, and if the noun is dual, so are its attributes (adjectives, pronouns).  So the agreement of the numeral 2 differs formally from 3-4
(Ivan A. Derzhanski, email 2010/06/16)</rdfs:comment>
        <owl:versionInfo>Numeral/Class=&quot;definite&quot;, Numeral/Class=&quot;definite1&quot;, Numeral/Class=&quot;definite234&quot; etc. refer to specific patterns of congruency with Slavic numerals that originate from the difference between Old Slavic singular (definite1), dual (definite2, definite234) and plural (definite).</owl:versionInfo>
    </owl:Class>
    


    <!-- http://purl.org/olia/mte/multext-east.owl#ElativeCase -->

    <owl:Class rdf:about="http://purl.org/olia/mte/multext-east.owl#ElativeCase">
        <rdfs:subClassOf rdf:resource="http://purl.org/olia/mte/multext-east.owl#Case"/>
        <rdfs:comment>e.g., -, abból/az, amelyekből/amely, azokból/az, dolgozóiból/dolgozó, ebből/ez, egyikéből/egyik, elemzéséből/elemzés, ezekből/ez (hu)</rdfs:comment>
        <rdfs:comment>e.g., endist/ise, esimestest/esimene, meist/mina, meistki/mina, minust/mina, minustki/mina, must/mina, neist/tema, nendest/tema (et)</rdfs:comment>
        <rdfs:comment>Case=&quot;elative&quot; (Estonian, Hungarian)</rdfs:comment>
    </owl:Class>
    


    <!-- http://purl.org/olia/mte/multext-east.owl#ElativeDegree -->

    <owl:Class rdf:about="http://purl.org/olia/mte/multext-east.owl#ElativeDegree">
        <rdfs:subClassOf rdf:resource="http://purl.org/olia/mte/multext-east.owl#Degree"/>
        <rdfs:comment>e.g., predivan, prekasan, premanjeg/premali, premanjega/premali, premanjem/premali, premanjemu/premali, premanji/premali (sr)</rdfs:comment>
        <rdfs:comment>e.g., прешпионска/шпионски, прешпионскава/шпионски, прешпионскана/шпионски, прешпионската/шпионски, прешпионски/шпионски, прешпионскиве/шпионски, прешпионскине/шпионски, прешпионскиов/шпионски, прешпионскион/шпионски (mk)</rdfs:comment>
        <rdfs:comment>Degree=&quot;elative&quot; (Adjective: Resian, Serbian, Macedonian)&lt;br/&gt;

In Semitic languages, ElativeDegree refers to the “adjective of superiority.” In some languages such as Arabic, the concepts of comparative and superlative degree of an adjective are merged into a single form, the elative. How this form is understood or translated depends upon context and definiteness. In the absence of comparison, the elative conveys the notion of “greatest”, “supreme.” The elative of كبير (kabí:r, &quot;big&quot;) is أكبر (’ákbar, “bigger/biggest”, “greater/greatest”). (http://en.wiktionary.org/wiki/elative)

In Slavic languages, as well, it is pretty standard. I do agree with the definition though, that &quot;the elative conveys the notion of “greatest”, “supreme.”&quot; So, Slovene &quot;lep&quot; is beautiful, &quot;prelep&quot; is very (or supremely) beautiful; I guess the &quot;pre-&quot; prefix could be roughly translated as &quot;over-&quot;. Used in Resian, Serbian, Macedonian. In Slovenian, we banished it, as even &quot;ordinary&quot; degrees are borderline inflection / derivation, but, I think, elative is is definitely not inflection. (Tomaž Erjavec, email 2010/06/21)</rdfs:comment>
    </owl:Class>
    


    <!-- http://purl.org/olia/mte/multext-east.owl#ElementWithClitic -->

    <owl:Class rdf:about="http://purl.org/olia/mte/multext-east.owl#ElementWithClitic">
        <rdfs:subClassOf rdf:resource="http://purl.org/olia/mte/multext-east.owl#Cliticness"/>
        <owl:versionInfo>Introduced to designate annotations that mark an element as *cointaining* (being composed of nonclitic and) clitic components, and to distinguish them from elements that *are* clitic elements.</owl:versionInfo>
    </owl:Class>
    


    <!-- http://purl.org/olia/mte/multext-east.owl#ElementWithoutClitic -->

    <owl:Class rdf:about="http://purl.org/olia/mte/multext-east.owl#ElementWithoutClitic">
        <rdfs:subClassOf rdf:resource="http://purl.org/olia/mte/multext-east.owl#Cliticness"/>
    </owl:Class>
    


    <!-- http://purl.org/olia/mte/multext-east.owl#EmphaticDeterminer -->

    <owl:Class rdf:about="http://purl.org/olia/mte/multext-east.owl#EmphaticDeterminer">
        <rdfs:subClassOf rdf:resource="http://purl.org/olia/mte/multext-east.owl#Determiner"/>
        <rdfs:comment>e.g., însele/însumi, însemi/însumi, însene/însumi, însevă/însumi, înseşi/însumi, înseţi/însumi, însumi, însuşi/însumi, însuţi/însumi (ro)</rdfs:comment>
        <rdfs:comment>Determiner/Type=&quot;emphatic&quot; (Romanian)&lt;br/&gt;

In Romanian, there are specific forms for the so-called emphatic determiner, which may accompany both a noun and a personal pronoun: fata însăşi (the girl herself), also ea însăşi (she herself).</rdfs:comment>
    </owl:Class>
    


    <!-- http://purl.org/olia/mte/multext-east.owl#EmphaticPronoun -->

    <owl:Class rdf:about="http://purl.org/olia/mte/multext-east.owl#EmphaticPronoun">
        <rdfs:subClassOf rdf:resource="http://purl.org/olia/mte/multext-east.owl#Pronoun"/>
        <rdfs:comment>e.g., ніким/= ніким/= ніким/нікого ні з ким/нікого, нікого/=, нікому/=, нікому/нікого нікому/= нікому/=, нічим/=, нічого/=, нічому/= (uk)</rdfs:comment>
        <rdfs:comment>In the Ukrainian MTE v4 specs, Pronoun/Type=&quot;emphatic&quot; is used for pronoun forms ні&quot;кому, ні&quot;чому, ні&quot;чим, ні&quot;кого, etc., with complex meanings like &quot;there is nobody/nothing (to do sth/to use for doing sth, etc.)&quot;. Orthographically these are identical forms of negative nominal pronouns ніхто, ніщо &quot;nobody, nothing&quot; in oblique cases, however, with differing accent. They are referred to as either separate pronoun lexemes or predicatives in grammars. All Ukrainian emphatic pronoun forms include negation.
(MTE v4)</rdfs:comment>
    </owl:Class>
    


    <!-- http://purl.org/olia/mte/multext-east.owl#EssiveCase -->

    <owl:Class rdf:about="http://purl.org/olia/mte/multext-east.owl#EssiveCase">
        <rdfs:subClassOf rdf:resource="http://purl.org/olia/mte/multext-east.owl#Case"/>
        <rdfs:comment>e.g., esimestena/esimene, missugustena/missugune, niisugustena/niisugune, samasugustena/samasugune, sellistena/selline, teisena/teine, tootmisvõimsamana/tootmisvõimsam, tüüpilisemana/tüüpilisem, vanematena/vanem (et)</rdfs:comment>
        <rdfs:comment>e.g., feltételéül/feltétel, kamarapartneréül/kamarapartner, zavarodottan/zavarodott, zavartan/zavart (hu)</rdfs:comment>
        <rdfs:comment>Case=&quot;essive&quot; (Hungarian, Estonian)&lt;br/&gt;

In Estonian the essive case means such things as `(I played golf)
as a student&apos;, `(I worked) as a bartender&apos;, `(you look) tired&apos;,
`(he&apos;s very good) as a dancing partner&apos;, `(we parted) as friends&apos;.
This doesn&apos;t sound like the definition you quoted, but is similar
(though not identical) to the meaning of the Hungarian form.
(Ivan A. Derzhanski, email 2010/06/15)&lt;br/&gt;

Hungarian has two essive cases, essive-formalis (formatives, e.g., emberként &quot;as people&quot;) and essive-modalis (essivus-formalis, e.g., emberül from ember &quot;people&quot;)
(Nose 2003, p. 108)&lt;br/&gt;

The essive-modal case in Hungarian language can express the state, capacity, task in which somebody is or which somebody has (Essive case, e.g. &quot;as a reward&quot;, &quot;for example&quot;), or the manner in which an action is carried out, an event happens, or the language which somebody knows (Modal case, e.g. &quot;sloppily&quot;, &quot;unexpectedly&quot;, &quot;speak German&quot;).
An example of this would be in the sentence &quot;Beszélek magyarul.&quot; (I speak Hungarian.) The sentence denotes the ability of being able to speak the Hungarian language. According to vowel harmony rules, ul becomes ül in cases such as &quot;Beszélek németül.&quot; (I speak German.) because the word for &quot;German&quot;, német is composed completely of median and/or frontal vowels.
(http://en.wikipedia.org/wiki/Essive-modal_case)</rdfs:comment>
    </owl:Class>
    


    <!-- http://purl.org/olia/mte/multext-east.owl#EssiveFormalCase -->

    <owl:Class rdf:about="http://purl.org/olia/mte/multext-east.owl#EssiveFormalCase">
        <rdfs:subClassOf rdf:resource="http://purl.org/olia/mte/multext-east.owl#Case"/>
        <rdfs:comment>e.g., amiként/ami, egyikeként/egyik, elsőként/első, gondozóiként/gondozó, ilyenként/ilyen, miként/mi, termelőjeként/termelő, tulajdonképp/tulajdon, tulajdonosaként/tulajdonos (hu)</rdfs:comment>
        <rdfs:comment>Case=&quot;essive-formal&quot; (Hungarian)&lt;br/&gt;

e.g., Hungarian &apos;katonaként&apos; -&gt; [serves] as a soldier. (Csaba Oravecz, email 2010/06/15)&lt;br/&gt;

The Hungarian &quot;formativus, or essivus-formalis `-ként&apos; ... usually expresses a position, task and manner of the person or the thing.&quot; (Nose 2003)&lt;br/&gt;

&quot;Haspelmath &amp; Buchholz (1998:321) explained the function of the essive case as ``role phrases&apos;&apos;. Role phrases represent the role of the function in which a participant appears. They regard the role phrases as adverbial.&quot;
(Nose 2003, p. 117)&lt;br/&gt;

In the Hungarian language this case combines the Essive case and the Formal case, and it can express the position, task, state (e.g. &quot;as a tourist&quot;), or the manner (e.g. &quot;like a hunted animal&quot;). The status of the suffix -ként in the declension system is disputed for several reasons. First, in general, Hungarian case suffixes are absolute word-final, while -ként permits further suffixation by the locative suffix -i. Second, most Hungarian case endings participate in vowel harmony, while -ként does not. For these reasons, many modern analyses of the Hungarian case system, starting with László Antal&apos;s &quot;A magyar esetrendszer&quot; (1961) do not consider the essive/formal to be a case.
(http://en.wikipedia.org/wiki/Essive-formal_case)&lt;br/&gt;

cf. Masahiko Nose (2003), Adverbial Usage of the Hungarian Essive Case</rdfs:comment>
    </owl:Class>
    


    <!-- http://purl.org/olia/mte/multext-east.owl#ExclamativeDeterminer -->

    <owl:Class rdf:about="http://purl.org/olia/mte/multext-east.owl#ExclamativeDeterminer">
        <rdfs:subClassOf rdf:resource="http://purl.org/olia/mte/multext-east.owl#Determiner"/>
        <rdfs:comment>Determiner/Type=&quot;exclamative&quot; was introduced for Persian چه‌قدر چه </rdfs:comment>
    </owl:Class>
    


    <!-- http://purl.org/olia/mte/multext-east.owl#ExclamativePronoun -->

    <owl:Class rdf:about="http://purl.org/olia/mte/multext-east.owl#ExclamativePronoun">
        <rdfs:subClassOf rdf:resource="http://purl.org/olia/mte/multext-east.owl#Pronoun"/>
        <owl:deprecated>The category Pronoun/Type=&quot;exclamative&quot; is specified in MTE v4, but not actually used.</owl:deprecated>
    </owl:Class>
    


    <!-- http://purl.org/olia/mte/multext-east.owl#ExistentialThere -->

    <owl:Class rdf:about="http://purl.org/olia/mte/multext-east.owl#ExistentialThere">
        <rdfs:subClassOf rdf:resource="http://purl.org/olia/mte/multext-east.owl#Pronoun"/>
        <rdfs:comment>English existential there is specified as a subtype of pronoun in MTE v4, i.e., Pronoun/Type=&quot;ex-there&quot;</rdfs:comment>
    </owl:Class>
    


    <!-- http://purl.org/olia/mte/multext-east.owl#FactiveCase -->

    <owl:Class rdf:about="http://purl.org/olia/mte/multext-east.owl#FactiveCase">
        <rdfs:subClassOf rdf:resource="http://purl.org/olia/mte/multext-east.owl#Case"/>
        <rdfs:comment>e.g., -, amilyenné/amilyen, azzá/az, erőddé/erő, jelmezeivé/jelmez, jelükké/jel, kevéssé/kevés, Kissé/Kiss, legjelentéktelenebbekké/jelentéktelen (hu)</rdfs:comment>
        <rdfs:comment>Case=&quot;factive&quot; (Hungarian)</rdfs:comment>
    </owl:Class>
    


    <!-- http://purl.org/olia/mte/multext-east.owl#FeminineGender -->

    <owl:Class rdf:about="http://purl.org/olia/mte/multext-east.owl#FeminineGender">
        <rdfs:subClassOf rdf:resource="http://purl.org/olia/mte/multext-east.owl#Gender"/>
        <rdfs:comment>e.g., -aceasta/acesta, -această/acest, -astea/ăsta, -istei, -istele, -istelor, -istă, -ngrijitoare/îngrijitoare, -nsoţitoare/însoţitoare (ro)</rdfs:comment>
        <rdfs:comment>e.g., akceptowanymi/akceptować, akredytujące/akredytować, akredytujących/akredytować, akredytującą/akredytować, cytowanych/cytować, cztery/cztery, czwartej/czwarty, czwartą/czwarty, debiutująca/debiutować (pl)</rdfs:comment>
        <rdfs:comment>e.g., costi/kust, dobrute/dubruta, Elisabeto/elizabeta, fiesto/fjëšta, ito/iti, kitinami/këtina, nashanà/nistet, Oshtie/oštja, Santissima/šantišim (sl-rozaj)</rdfs:comment>
        <rdfs:comment>e.g., desaterým/desaterý, desátá/desátý, devatenácté/devatenáctý, devatenáctým/devatenáctý, dostala/dostat, dostaly/dostat, dvacátých/dvacátý, kdekterých/kdekterý, kdekterými/kdekterý (cs)</rdfs:comment>
        <rdfs:comment>e.g., hentej/hentá, hentie/hentá, hentou/hentá, hentá, hentú/hentá, hentých/hentá, hentým/hentá, hentými/hentá, koľkátiek/koľkátka (sk)</rdfs:comment>
        <rdfs:comment>e.g., htele/hteti, htjele/htjeti, javnosti/javnost, kategorije/kategorija, najbigotnije/bigotan, najsuštinskija/suštinski, osobenosti/osobenost, poznate/poznat, ratoborna/ratoboran (sr)</rdfs:comment>
        <rdfs:comment>e.g., katere/kateri, katerimi/kateri, ti/ta, treh/trije, trem/trije, tremi/trije, tretjim/tretji, tvoja/tvoj, tvoje/tvoj (sl)</rdfs:comment>
    </owl:Class>
    


    <!-- http://purl.org/olia/mte/multext-east.owl#FirstPerson -->

    <owl:Class rdf:about="http://purl.org/olia/mte/multext-east.owl#FirstPerson">
        <rdfs:subClassOf rdf:resource="http://purl.org/olia/mte/multext-east.owl#Person"/>
        <rdfs:comment>e.g., , bom/biti, bomo/biti, bova/biti, hočem/hoteti, hočeva/hoteti, imam/imeti, imamo/imeti, imava/imeti (sl)</rdfs:comment>
        <rdfs:comment>e.g., -, belém/én, bennem/én, bennünk/mi, bensőnkben/benső, betegségünktől/betegség, borúlátónkat/borúlátó, condráinkban/condra, cselédkönyveinkkel/cselédkönyv (hu)</rdfs:comment>
        <rdfs:comment>e.g., -am/avea, -aş/avea, -mea/mea, -meu/meu, -mii/mea, -miu/meu, -ne/noi, -nzestrarăm/înzestra, -nzestrasem/înzestra (ro)</rdfs:comment>
        <rdfs:comment>e.g., I, my, myself, our, ourselves, us, was/be, wasn&apos;t/be+not, wass/be (en)</rdfs:comment>
        <rdfs:comment>e.g., abych/aby, abychom/aby, budeme/být, budu/být, bych/by, bychom/by, bývám/bývat, chceme/chtít, dejme/dát (cs)</rdfs:comment>
        <rdfs:comment>e.g., accompagnaimu/akompanjät, amai/amät, aman/amät, bogan/bogat, bom/bet, bon/bet, cion/tët, contemplaimo/kontemplät, dílan/dëlat (sl-rozaj)</rdfs:comment>
        <rdfs:comment>e.g., bi&apos;/biti, bi/biti, bih/biti, bismo/biti, bićemo/biti, biću/biti, budimo/biti, htednimo/hteti, htjednimo/htjeti (sr)</rdfs:comment>
        <rdfs:comment>e.g., budem/byť, budeme/byť, buďme/byť, ja, ma/ja, majme/mať, mi/ja, mne/ja, mnou/ja (sk)</rdfs:comment>
        <rdfs:comment>e.g., byliśmy/być, byłam/być, byłem/być, byłybyśmy/być, byłyśmy/być, będziemy/być, będę/być, chciałabym/chcieć, chciałam/chcieć (pl)</rdfs:comment>
        <rdfs:comment>e.g., ma/mina, me/mina, meid/mina, meie/mina, meiega/mina, meiegi/mina, meieni/mina, meil/mina, meile/mina (et)</rdfs:comment>
        <rdfs:comment>e.g., БУДЕМ/быть, БУДУ/быть, Бежим/бежать, Буду/быть, Вернемся/вернуться, Возьмем/взять, Выпьем/выпить, Идемте/идти, МНЕ/я (ru)</rdfs:comment>
        <rdfs:comment>e.g., абеткуватимемо/абеткувати абеткуватимем/абеткувати авізуватимемо/авізувати авізуватимем/авізувати агакатимемо/агакати агакатимем/агакати агітуватимемо/агітувати агітуватимем/агітувати агонізуватимемо/агонізувати агонізуватимем/агонізувати адвокатуватимемо/адвокатувати адвокатуватимем/адвокатувати адмініструватимемо/адмініструвати адмініструватимем/адмініструвати айкатимемо/айкати айкатимем/айкати акатимемо/акати акатимем/акати акомпануватимемо/акомпанувати акомпануватимем/акомпанувати, абеткуватиму/абеткувати авізуватиму/авізувати агакатиму/агакати агітуватиму/агітувати агонізуватиму/агонізувати адвокатуватиму/адвокатувати адмініструватиму/адмініструвати айкатиму/айкати акатиму/акати акомпануватиму/акомпанувати акредитуватимуся/акредитуватися акредитуватимусь/акредитуватися акторствуватиму/акторствувати акторуватиму/акторувати актуватиму/актувати акушеруватиму/акушерувати альокатиму/альокати аналізуватиму/аналізувати анкетуватиму/анкетувати анодуватиму/анодувати, абеткуймо/абеткувати авізуймо/авізувати агакаймо/агакати агітуймо/агітувати агонізуймо/агонізувати адвокатуймо/адвокатувати адмініструймо/адмініструвати айкаймо/айкати акаймо/акати акомпануймо/акомпанувати акредитуймося/акредитуватися акредитуймось/акредитуватися акторствуймо/акторствувати акторуймо/акторувати актуймо/актувати акушеруймо/акушерувати альокаймо/альокати аналізуймо/аналізувати анкетуймо/анкетувати анодуймо/анодувати, абеткую/абеткувати авізую/авізувати агакаю/агакати агітую/агітувати агонізую/агонізувати адвокатую/адвокатувати адмініструю/адмініструвати айкаю/айкати акаю/акати акомпаную/акомпанувати акредитуюся/акредитуватися акредитуюсь/акредитуватися акторствую/акторствувати акторую/акторувати актую/актувати акушерую/акушерувати альокаю/альокати аналізую/аналізувати анкетую/анкетувати анодую/анодувати, абеткуємо/абеткувати абеткуєм/абеткувати авізуємо/авізувати авізуєм/авізувати агакаємо/агакати агакаєм/агакати агітуємо/агітувати агітуєм/агітувати агонізуємо/агонізувати агонізуєм/агонізувати адвокатуємо/адвокатувати адвокатуєм/адвокатувати адмініструємо/адмініструвати адмініструєм/адмініструвати айкаємо/айкати айкаєм/айкати акаємо/акати акаєм/акати акомпануємо/акомпанувати акомпануєм/акомпанувати, аблактуватимемо/аблактувати аблактуватимем/аблактувати абонуватимемо/абонувати абонуватимем/абонувати абонуватимемося/абонуватися абонуватимемось/абонуватися абонуватимемся/абонуватися абордуватимемо/абордувати абордуватимем/абордувати абортуватимемо/абортувати абортуватимем/абортувати абсолютизуватимемо/абсолютизувати абсолютизуватимем/абсолютизувати абстрагуватимемо/абстрагувати абстрагуватимем/абстрагувати абстрагуватимемося/абстрагуватися абстрагуватимемось/абстрагуватися абстрагуватимемся/абстрагуватися абшитуватимемо/абшитувати абшитуватимем/абшитувати, аблактуватиму/аблактувати абонуватиму/абонувати абонуватимуся/абонуватися абонуватимусь/абонуватися абордуватиму/абордувати абортуватиму/абортувати абсолютизуватиму/абсолютизувати абстрагуватиму/абстрагувати абстрагуватимуся/абстрагуватися абстрагуватимусь/абстрагуватися абшитуватиму/абшитувати авансуватиму/авансувати авансуватимуся/авансуватися авансуватимусь/авансуватися автоматизуватиму/автоматизувати авторизуватиму/авторизувати аглютинуватиму/аглютинувати агрегатуватиму/агрегатувати адаптуватиму/адаптувати адаптуватимуся/адаптуватися, аблактуймо/аблактувати абонуймо/абонувати абонуймося/абонуватися абонуймось/абонуватися абордуймо/абордувати абортуймо/абортувати абсолютизуймо/абсолютизувати абстрагуймо/абстрагувати абстрагуймося/абстрагуватися абстрагуймось/абстрагуватися абшитуймо/абшитувати авансуймо/авансувати авансуймося/авансуватися авансуймось/авансуватися автоматизуймо/автоматизувати авторизуймо/авторизувати аглютинуймо/аглютинувати агрегатуймо/агрегатувати адаптуймо/адаптувати адаптуймося/адаптуватися, аблактую/аблактувати абоную/абонувати абонуюся/абонуватися абонуюсь/абонуватися абордую/абордувати абортую/абортувати абсолютизую/абсолютизувати абстрагую/абстрагувати абстрагуюся/абстрагуватися абстрагуюсь/абстрагуватися абшитую/абшитувати авансую/авансувати авансуюся/авансуватися авансуюсь/авансуватися автоматизую/автоматизувати авторизую/авторизувати аглютиную/аглютинувати агрегатую/агрегатувати адаптую/адаптувати адаптуюся/адаптуватися (uk)</rdfs:comment>
        <rdfs:comment>e.g., аз, бих/бъда, бъда, бъдем/бъда, бях/съм, бяхме/съм, ме/аз, мен/аз, мене/аз (bg)</rdfs:comment>
        <rdfs:comment>e.g., бев/сум, бевме/сум, бидам/сум, бидев/сум, бидевме/сум, бидеме/сум, имав/има, имавме/има, имам/има (mk)</rdfs:comment>
        <rdfs:comment>e.g., آمديم/آمد, باشم/باش, باشيم/باش, بتوانم/توان, بتوانيم/توان, بخواهيم/خواه, بدانم/دان بخوابونم/خوابان ببينم/بين, بدهيم/ده بخوانيم/خوان ببينيم/بين, بريم/رو برويم/رو باشيم/باش (fa)</rdfs:comment>
    </owl:Class>
    


    <!-- http://purl.org/olia/mte/multext-east.owl#FirstSgSecondSg -->

    <owl:Class rdf:about="http://purl.org/olia/mte/multext-east.owl#FirstSgSecondSg">
        <rdfs:subClassOf rdf:resource="http://purl.org/olia/mte/multext-east.owl#PersonOfObject"/>
        <rdfs:comment>e.g., -, elárultalak/elárul, figyelmeztettelek/figyelmeztet, megismertelek/megismer, tudnálak/tud (hu)</rdfs:comment>
        <rdfs:comment>Definiteness=&quot;1s2s&quot; (Verb: Hungarian)&lt;br/&gt;

Hungarian: 1s2s is a special form for definitness, in which the speaker&apos;s person is first singular (I) and the target of the transitivity is second singular (you). (MTE v4)&lt;br/&gt;

Hungarian Definiteness (of verbs):
In simple terms, it means that the verb takes a definite object, 
which is reflected in the type of verb conjugation. 
Eg. in Hungarian there will be two forms of the verb &apos;see&apos; here
1. I can see an elephant.
2. I can see the elephant.
depending on the definiteness of the object, &apos;látok&apos; vs. &apos;látom&apos;.
The above 1s2s form of verbs takes a 1st person singular subject and
2nd person definite object (which in actual fact can also be plural not only
singular). Both subject and object can be (pro)dropped. Eg.
I can see you -&gt; (Én) látlak (téged/titeket)
                  I    see     you_sg/you_pl
(Csaba Oravecz, email 2010/06/15)</rdfs:comment>
    </owl:Class>
    


    <!-- http://purl.org/olia/mte/multext-east.owl#Foreign -->

    <owl:Class rdf:about="http://purl.org/olia/mte/multext-east.owl#Foreign">
        <rdfs:subClassOf rdf:resource="http://purl.org/olia/mte/multext-east.owl#Residual"/>
        <rdfs:comment>In the Slovene MTE v4 specs, Residual/Type=&quot;foreign&quot; marks a words in a strech of foreign language text. (MTE v4)</rdfs:comment>
    </owl:Class>
    


    <!-- http://purl.org/olia/mte/multext-east.owl#FormalCase -->

    <owl:Class rdf:about="http://purl.org/olia/mte/multext-east.owl#FormalCase">
        <rdfs:subClassOf rdf:resource="http://purl.org/olia/mte/multext-east.owl#Case"/>
        <rdfs:comment>(from the discussion of [Hungarian] EssiveFormalCase)&lt;br/&gt;

&quot;`formal&apos; in `essive-formal&apos; is not an indication of register: there is another form, which in some descriptions is simply called `formal&apos;, with the affix _-képp(en)_ and a similar meaning (`in
the form of ...&apos;, they probably meant when they came up with the term).
The line between a case ending, an adverb formative and a postposition
is a thin one in Hungarian.&quot;
(Ivan A. Derzhanski, email 2010/06/15)&lt;br/&gt;

http://en.wikipedia.org/wiki/Essive-formal_case (2010/06/15):
&quot;In the Hungarian language this case combines the Essive case and the Formal case, and it can express the position, task, state (e.g. &quot;as a tourist&quot;), or the manner (e.g. &quot;like a hunted animal&quot;).&quot;</rdfs:comment>
        <owl:versionInfo>This concept pertains to a case in Hungarian, but is not actually used in the annotation scheme.</owl:versionInfo>
    </owl:Class>
    


    <!-- http://purl.org/olia/mte/multext-east.owl#Formation -->

    <owl:Class rdf:about="http://purl.org/olia/mte/multext-east.owl#Formation">
        <rdfs:subClassOf rdf:resource="http://purl.org/olia/mte/multext-east.owl#MorphosyntacticFeature"/>
        <rdfs:comment>Formation refers to the graphical components: simple, i.e. consisting of one word; compound, i.e. consisting of more than one word. (MTE v4 on Conjunction/Formation)</rdfs:comment>
    </owl:Class>
    


    <!-- http://purl.org/olia/mte/multext-east.owl#FractalNumeral -->

    <owl:Class rdf:about="http://purl.org/olia/mte/multext-east.owl#FractalNumeral">
        <rdfs:subClassOf rdf:resource="http://purl.org/olia/mte/multext-east.owl#Numeral"/>
        <rdfs:comment>e.g., treisprezecimea/treisprezecime, treisprezecimi/treisprezecime, treisprezecimii/treisprezecime, treisprezecimile/treisprezecime, treisprezecimilor/treisprezecime, unsprezecimea/unsprezecime, unsprezecimi/unsprezecime, unsprezecimii/unsprezecime, unsprezecimile/unsprezecime (ro)</rdfs:comment>
        <rdfs:comment>e.g., يک‌چهارمِ/يک‌چهار يک‌پنجمِ/يک‌پنج (fa)</rdfs:comment>
        <rdfs:comment>Numeral/Form=&quot;fractional&quot; (Romanian)&lt;br/&gt;
In traditional Romanian grammars, FractionalNumeral refers to expressions like treime-one third. (MTE v4)</rdfs:comment>
    </owl:Class>
    


    <!-- http://purl.org/olia/mte/multext-east.owl#FullArticle -->

    <owl:Class rdf:about="http://purl.org/olia/mte/multext-east.owl#FullArticle">
        <rdfs:subClassOf rdf:resource="http://purl.org/olia/mte/multext-east.owl#AmbiguousDefinitenessFeature"/>
        <rdfs:subClassOf>
            <owl:Class>
                <owl:unionOf rdf:parseType="Collection">
                    <rdf:Description rdf:about="http://purl.org/olia/mte/multext-east.owl#CliticDeterminerType"/>
                    <rdf:Description rdf:about="http://purl.org/olia/mte/multext-east.owl#ReductionFeature"/>
                </owl:unionOf>
            </owl:Class>
        </rdfs:subClassOf>
        <rdfs:comment>e.g., 0, абеткованая/абеткований авізованая/авізований акомпанованая/акомпанований актованая/актований аналізованая/аналізований анкетованая/анкетований анодованая/анодований артикульованая/артикульований балотованая/балотований балуваная/балуваний бальзамованая/бальзамований банітованая/банітований багнітованая/багнітований байцьованая/байцьований балаканая/балаканий баченая/бачений белетризованая/белетризований береженая/бережений бетонованая/бетонований бинтованая/бинтований, абеткованеє/абеткований авізованеє/авізований акомпанованеє/акомпанований актованеє/актований аналізованеє/аналізований анкетованеє/анкетований анодованеє/анодований артикульованеє/артикульований балотованеє/балотований балуванеє/балуваний бальзамованеє/бальзамований банітованеє/банітований багнітованеє/багнітований байцьованеє/байцьований балаканеє/балаканий баченеє/бачений белетризованеє/белетризований береженеє/бережений бетонованеє/бетонований бинтованеє/бинтований, абеткований/= авізований/= акомпанований/= актований/= аналізований/= анкетований/= анодований/= артикульований/= балотований/= балуваний/= бальзамований/= банітований/= багнітований/= байцьований/= балаканий/= бачений/= белетризований/= бережений/= бетонований/= бинтований/=, абеткованим/абеткований авізованим/авізований акомпанованим/акомпанований актованим/актований аналізованим/аналізований анкетованим/анкетований анодованим/анодований артикульованим/артикульований балотованим/балотований балуваним/балуваний бальзамованим/бальзамований банітованим/банітований багнітованим/багнітований байцьованим/байцьований балаканим/балаканий баченим/бачений белетризованим/белетризований береженим/бережений бетонованим/бетонований бинтованим/бинтований, абеткованими/абеткований авізованими/авізований акомпанованими/акомпанований актованими/актований аналізованими/аналізований анкетованими/анкетований анодованими/анодований артикульованими/артикульований балотованими/балотований балуваними/балуваний бальзамованими/бальзамований банітованими/банітований багнітованими/багнітований байцьованими/байцьований балаканими/балаканий баченими/бачений белетризованими/белетризований береженими/бережений бетонованими/бетонований бинтованими/бинтований, абеткованих/абеткований авізованих/авізований акомпанованих/акомпанований актованих/актований аналізованих/аналізований анкетованих/анкетований анодованих/анодований артикульованих/артикульований балотованих/балотований балуваних/балуваний бальзамованих/бальзамований банітованих/банітований багнітованих/багнітований байцьованих/байцьований балаканих/балаканий бачених/бачений белетризованих/белетризований бережених/бережений бетонованих/бетонований бинтованих/бинтований, абеткованого/абеткований авізованого/авізований акомпанованого/акомпанований актованого/актований аналізованого/аналізований анкетованого/анкетований анодованого/анодований артикульованого/артикульований балотованого/балотований балуваного/балуваний бальзамованого/бальзамований банітованого/банітований багнітованого/багнітований байцьованого/байцьований балаканого/балаканий баченого/бачений белетризованого/белетризований береженого/бережений бетонованого/бетонований бинтованого/бинтований, абеткованому/абеткований абеткованім/абеткований авізованому/авізований авізованім/авізований акомпанованім/акомпанований акомпанованому/акомпанований актованому/актований актованім/актований аналізованому/аналізований аналізованім/аналізований анкетованім/анкетований анкетованому/анкетований анодованому/анодований анодованім/анодований артикульованому/артикульований артикульованім/артикульований балотованім/балотований балотованому/балотований балуваному/балуваний балуванім/балуваний (uk)</rdfs:comment>
        <rdfs:comment>e.g., ciebie/ty, em/być, eś/być, jego/on, jego/ono, jemu/on, jemu/ono, mnie/ja, niego/on (pl)</rdfs:comment>
        <rdfs:comment>e.g., Заинтригованная/заинтриговывать, Звенящая/звенеть, Разбитая/разбивать, Толпившиеся/толпиться, Трясущейся/трястись, Улыбающаяся/улыбаться, Улыбающиеся/улыбаться, Улыбающийся/улыбаться, Ушибленная/ушибать (ru)</rdfs:comment>
        <rdfs:comment>e.g., бъдещият/бъда, всичкия, всичкият/всичкия, единият/един, моят/мой, нашият/наш, неговият/негов, нейният/неин, своят/свой (bg)</rdfs:comment>
        <rdfs:comment>Definiteness=&quot;full-art&quot; (Noun: Bulgarian; Verb: Polish, Russian, Bulgarian; Adjective: Polish, Russian, Ukrainian, Bulgarian; Pronoun: Polish, Bulgarian)&lt;br/&gt;

In Bulgarian, the singular masculine article has two forms: a full article(f)[l.s.] and a short article(s)[l.s.]. The full article is used when a singular masculine form is the syntactic subject of the clause, otherwise a short one is used – a purely orthographic rule. The distinction of full vs. short is not made for feminine, neuter and plural forms, and we use just the yes(y) or no(n) to mark definiteness or respectively lack thereof. Therefore, the definiteness attribute can take overall 4 different values: indefinite(n), definitive(y), short article(s), full article(f) e.g., мъж, мъжа, мъжът /a man, the man[short], the man [full]/ (Dimitrova et al. 2009)&lt;br/&gt;

For Polish, the Vocalicity of (a)gglutinated forms like -em vs -m is mapped on the Definiteness attribute with its values &quot;(f)ull-art&quot; and &quot;(s)hort-art&quot; respectively, meaning &quot;full form&quot; and &quot;short form&quot;. The terms are very artificial, but this category is used due to the similarity of the phenomenon. The IPIC flexeme winien and predicatives like rad are thus treated as short adjectives—Definiteness=&quot;short-art&quot;. (MTE v4)
</rdfs:comment>
        <owl:versionInfo>For singular masculine, there are two forms: a full article(f)[l.s.] and a short article(s)[l.s.]. The full
article is used when a singular masculine form is the syntactic subject of the clause, otherwise a short one is
used – a purely orthographic rule. The distinction of full vs. short is not made for feminine, neuter and plural
forms, and we use just the yes(y) or no(n) to mark definiteness or respectively lack thereof. Therefore, the
definiteness attribute can take overall 4 different values: indefinite(n), definitive(y), short article(s), full
article(f)
(Dimitrova et al., 2009)</owl:versionInfo>
    </owl:Class>
    


    <!-- http://purl.org/olia/mte/multext-east.owl#FutureParticle -->

    <owl:Class rdf:about="http://purl.org/olia/mte/multext-east.owl#FutureParticle">
        <rdfs:subClassOf rdf:resource="http://purl.org/olia/mte/multext-east.owl#VerbalParticle"/>
        <rdfs:comment>e.g., -o, o (ro)</rdfs:comment>
        <rdfs:comment>Particle/Type=&quot;future&quot; (Romanian)

A verbal particle with Particle/Type=&quot;future&quot; modifies the verbs and carries the information that the verb is in future tense (Dan Tufis, email 2010/06/09)</rdfs:comment>
    </owl:Class>
    


    <!-- http://purl.org/olia/mte/multext-east.owl#FutureTense -->

    <owl:Class rdf:about="http://purl.org/olia/mte/multext-east.owl#FutureTense">
        <rdfs:subClassOf rdf:resource="http://purl.org/olia/mte/multext-east.owl#Tense"/>
        <rdfs:comment>e.g., biće/biti, bićemo/biti, bićete/biti, bićeš/biti, biću/biti, zveknućemo/zveknuti, zveknućete/zveknuti, žmurićemo/žmuriti, žmurićete/žmuriti (sr)</rdfs:comment>
        <rdfs:comment>e.g., bo/bet, bom/bet, bon/bet, bota/bet (sl-rozaj)</rdfs:comment>
        <rdfs:comment>e.g., bude/byť, budem/byť, budeme/byť, budete/byť, budeš/byť, budú/byť, nepostačia/nestačiť, nepostačí/nestačiť, nepostačím/nestačiť (sk)</rdfs:comment>
        <rdfs:comment>e.g., bude/být, budeme/být, budete/být, budeš/být, budou/být, budu/být, nebude/být, nebudem/být, nebudeme/být (cs)</rdfs:comment>
        <rdfs:comment>e.g., będzie/być, będziecie/być, będziemy/być, będziesz/być, będą/być, będę/być, da/dać, donoszą/donosić, odbędą/odbyć (pl)</rdfs:comment>
        <rdfs:comment>e.g., БУДЕМ/быть, БУДЕТ/быть, БУДЕТЕ/быть, БУДЕШЬ/быть, БУДУ/быть, БУДУТ/быть, Будет/быть, Будете/быть, Будешь/быть (ru)</rdfs:comment>
        <rdfs:comment>e.g., абеткуватиме/абеткувати авізуватиме/авізувати агакатиме/агакати агітуватиме/агітувати агонізуватиме/агонізувати адвокатуватиме/адвокатувати адмініструватиме/адмініструвати адоптуватиметься/адоптуватися адсорбуватиметься/адсорбуватися азотуватиметься/азотуватися айкатиме/айкати акатиме/акати акомпануватиме/акомпанувати акредитуватиметься/акредитуватися акторствуватиме/акторствувати акторуватиме/акторувати актуватиме/актувати акушеруватиме/акушерувати акцентуватиметься/акцентуватися альокатиме/альокати, абеткуватимемо/абеткувати абеткуватимем/абеткувати авізуватимемо/авізувати авізуватимем/авізувати агакатимемо/агакати агакатимем/агакати агітуватимемо/агітувати агітуватимем/агітувати агонізуватимемо/агонізувати агонізуватимем/агонізувати адвокатуватимемо/адвокатувати адвокатуватимем/адвокатувати адмініструватимемо/адмініструвати адмініструватимем/адмініструвати айкатимемо/айкати айкатимем/айкати акатимемо/акати акатимем/акати акомпануватимемо/акомпанувати акомпануватимем/акомпанувати, абеткуватимете/абеткувати авізуватимете/авізувати агакатимете/агакати агітуватимете/агітувати агонізуватимете/агонізувати адвокатуватимете/адвокатувати адмініструватимете/адмініструвати айкатимете/айкати акатимете/акати акомпануватимете/акомпанувати акредитуватиметеся/акредитуватися акредитуватиметесь/акредитуватися акторствуватимете/акторствувати акторуватимете/акторувати актуватимете/актувати акушеруватимете/акушерувати альокатимете/альокати аналізуватимете/аналізувати анкетуватимете/анкетувати анодуватимете/анодувати, абеткуватимеш/абеткувати авізуватимеш/авізувати агакатимеш/агакати агітуватимеш/агітувати агонізуватимеш/агонізувати адвокатуватимеш/адвокатувати адмініструватимеш/адмініструвати айкатимеш/айкати акатимеш/акати акомпануватимеш/акомпанувати акредитуватимешся/акредитуватися акторствуватимеш/акторствувати акторуватимеш/акторувати актуватимеш/актувати акушеруватимеш/акушерувати альокатимеш/альокати аналізуватимеш/аналізувати анкетуватимеш/анкетувати анодуватимеш/анодувати аплодуватимеш/аплодувати, абеткуватиму/абеткувати авізуватиму/авізувати агакатиму/агакати агітуватиму/агітувати агонізуватиму/агонізувати адвокатуватиму/адвокатувати адмініструватиму/адмініструвати айкатиму/айкати акатиму/акати акомпануватиму/акомпанувати акредитуватимуся/акредитуватися акредитуватимусь/акредитуватися акторствуватиму/акторствувати акторуватиму/акторувати актуватиму/актувати акушеруватиму/акушерувати альокатиму/альокати аналізуватиму/аналізувати анкетуватиму/анкетувати анодуватиму/анодувати, абеткуватимуть/абеткувати авізуватимуть/авізувати агакатимуть/агакати агітуватимуть/агітувати агонізуватимуть/агонізувати адвокатуватимуть/адвокатувати адмініструватимуть/адмініструвати адоптуватимуться/адоптуватися адсорбуватимуться/адсорбуватися азотуватимуться/азотуватися айкатимуть/айкати акатимуть/акати акомпануватимуть/акомпанувати акредитуватимуться/акредитуватися акторствуватимуть/акторствувати акторуватимуть/акторувати актуватимуть/актувати акушеруватимуть/акушерувати акцентуватимуться/акцентуватися альокатимуть/альокати, аблактуватиме/аблактувати абонуватиме/абонувати абонуватиметься/абонуватися абордуватиме/абордувати абортуватиме/абортувати абсолютизуватиме/абсолютизувати абсолютизуватиметься/абсолютизуватися абсорбуватиме/абсорбувати абсорбуватиметься/абсорбуватися абстрагуватиме/абстрагувати абстрагуватиметься/абстрагуватися абшитуватиме/абшитувати авансуватиме/авансувати авансуватиметься/авансуватися автоматизуватиме/автоматизувати автоматизуватиметься/автоматизуватися авторизуватиме/авторизувати аглютинуватиме/аглютинувати аглютинуватиметься/аглютинуватися агрегатуватиме/агрегатувати, аблактуватимемо/аблактувати аблактуватимем/аблактувати абонуватимемо/абонувати абонуватимем/абонувати абонуватимемося/абонуватися абонуватимемось/абонуватися абонуватимемся/абонуватися абордуватимемо/абордувати абордуватимем/абордувати абортуватимемо/абортувати абортуватимем/абортувати абсолютизуватимемо/абсолютизувати абсолютизуватимем/абсолютизувати абстрагуватимемо/абстрагувати абстрагуватимем/абстрагувати абстрагуватимемося/абстрагуватися абстрагуватимемось/абстрагуватися абстрагуватимемся/абстрагуватися абшитуватимемо/абшитувати абшитуватимем/абшитувати, аблактуватимете/аблактувати абонуватимете/абонувати абонуватиметеся/абонуватися абонуватиметесь/абонуватися абордуватимете/абордувати абортуватимете/абортувати абсолютизуватимете/абсолютизувати абстрагуватимете/абстрагувати абстрагуватиметеся/абстрагуватися абстрагуватиметесь/абстрагуватися абшитуватимете/абшитувати авансуватимете/авансувати авансуватиметеся/авансуватися авансуватиметесь/авансуватися автоматизуватимете/автоматизувати авторизуватимете/авторизувати аглютинуватимете/аглютинувати агрегатуватимете/агрегатувати адаптуватимете/адаптувати адаптуватиметеся/адаптуватися (uk)</rdfs:comment>
        <rdfs:comment>Tense=&quot;future&quot;&lt;br/&gt;

Czech/Slovak verbs normally form the future Tense periphrastically by auxiliary &quot;být&quot; (E. &quot;to be&quot;) plus infinitive of the main Verb. In addition to the copula, there are, however, some Verbs which form future Tense non-periphrastically, i.e. synthetically (Verbs of motion). Such verbal forms are marked as Tense=f. (MTE v4)</rdfs:comment>
        <owl:versionInfo>&quot;future&quot; and &quot;present&quot; were originally represented in VForm but are equivalent to &quot;future&quot; and &quot;present&quot; in Tense.&lt;br/&gt;

The Slovene specs has a convoluted history - there are
substantial differences between V3 in V4. Version 4 was made on the basis of
the JOS specifications http://nl.ijs.si/jos/josMSD-en.html
which are monolingual Slovene, and the linguists preferred to see future and
present as verb forms, as this is traditional in Slovene grammars. Hence
this inconsistency in regard to other languages.
(Tomaž Erjavec, email 2010/06/09)
</owl:versionInfo>
    </owl:Class>
    


    <!-- http://purl.org/olia/mte/multext-east.owl#Gender -->

    <owl:Class rdf:about="http://purl.org/olia/mte/multext-east.owl#Gender">
        <rdfs:subClassOf rdf:resource="http://purl.org/olia/mte/multext-east.owl#MorphosyntacticFeature"/>
        <rdfs:comment>Gender is reduced to the traditional set of &quot;masculine, feminine, neutral&quot; (and mergers between these). Animacy and Humanness that constitute subgenders of masculine accusative forms in Polish and other Slavic languages are represented as individual attributes. (Polish MTE v4) The Gender value &quot;common&quot; is assigned to nouns that can combine with adjectives in either feminine or masculine,e.g. Ukrainian сирота, or either neutral or masculine gender, e.g., Ukrainian Самоа. (Ukrainian MTE v4)
</rdfs:comment>
    </owl:Class>
    


    <!-- http://purl.org/olia/mte/multext-east.owl#GeneralAdjective -->

    <owl:Class rdf:about="http://purl.org/olia/mte/multext-east.owl#GeneralAdjective">
        <rdfs:subClassOf rdf:resource="http://purl.org/olia/mte/multext-east.owl#Adjective"/>
        <rdfs:comment>e.g., največja/velik, največji/velik, slabša/slab, večjih/velik (sl)</rdfs:comment>
        <rdfs:comment>The Slovene MTE (v4), Adjective/Type=&quot;general&quot; conflates qualificative adjectives and ordinal adjectives (distinguished in MTE v3).
(Tomaz Erjavec, email 2010/06/09)</rdfs:comment>
    </owl:Class>
    


    <!-- http://purl.org/olia/mte/multext-east.owl#GeneralAdverb -->

    <owl:Class rdf:about="http://purl.org/olia/mte/multext-east.owl#GeneralAdverb">
        <rdfs:subClassOf rdf:resource="http://purl.org/olia/mte/multext-east.owl#Adverb"/>
        <rdfs:comment>e.g., itu/ito (sl-rozaj)</rdfs:comment>
        <rdfs:comment>e.g., zárásaként/zárás, záróakkordjaként/záróakkord, zászlóként/zászló (hu)</rdfs:comment>
        <rdfs:comment>Adverbials can be sub-classified in different ways, Adverb/Type=&quot;general&quot; refers to the prototypical case of adverbs per language. Its definition, however, depends on the respective (language-specific) taxonomy of adverbs.

For example the distinction proposed for Romanian considers the principal syntactic properties of the adverbs. For Romanian, the general type includes most of the pronominal adverbs (demonstrative: aici (here), indefinite: oriunde (anywhere)). A distinct negative value is needed for adverbs as well (nicăieri - nowhere, niciodată - never). The particle type covers those adverbs which can dislocate verbal compound forms (ex. Ea a tot cântat -- She has ever sung) or mark degrees (ex. circa (about), foarte (very), prea (too)). Such adverbs are cam, mai, prea, şi, tot, foarte etc. A useful distinction in Romanian considers the adverbs which can have predicative role, that is they can govern a subordinate sentence (ex. Fireşte că o ştiu -- Certainly I know it). Here (for uniformity within a multilingual environment), they are squeezed into the modifier class. No formal distinction is made between the interrogative adverbs and the relative ones. The &quot;portmanteau&quot; type of adverb was introduced to cover some few words which can be both adverbs and conjunctions (with adverbial reading more frequent). This was necessary for tagging purposes. (MTE v4)</rdfs:comment>
    </owl:Class>
    


    <!-- http://purl.org/olia/mte/multext-east.owl#GeneralDeterminer -->

    <owl:Class rdf:about="http://purl.org/olia/mte/multext-east.owl#GeneralDeterminer">
        <rdfs:subClassOf rdf:resource="http://purl.org/olia/mte/multext-east.owl#Determiner"/>
        <rdfs:comment>e.g., which, whichever (en)</rdfs:comment>
        <rdfs:comment>Determiner/Type=&quot;general&quot; (English)</rdfs:comment>
    </owl:Class>
    


    <!-- http://purl.org/olia/mte/multext-east.owl#GeneralParticle -->

    <owl:Class rdf:about="http://purl.org/olia/mte/multext-east.owl#GeneralParticle">
        <rdfs:subClassOf rdf:resource="http://purl.org/olia/mte/multext-east.owl#Particle"/>
        <rdfs:comment>e.g., а_бе, ей-сега, ей-тъй (bg)</rdfs:comment>
        <rdfs:comment>In the Bulgarian MTE v4 specs, Particle/Type=&quot;general&quot; is applied for non-specialised particles that do not fall in any of the other classes, i.e., negative, general, comparative, verbal, interrogative, or modal particle. (Dimitrova et al. 2009)
</rdfs:comment>
    </owl:Class>
    


    <!-- http://purl.org/olia/mte/multext-east.owl#GeneralPronoun -->

    <owl:Class rdf:about="http://purl.org/olia/mte/multext-east.owl#GeneralPronoun">
        <rdfs:subClassOf rdf:resource="http://purl.org/olia/mte/multext-east.owl#Pronoun"/>
        <rdfs:comment>e.g., another, others, whatever (en)</rdfs:comment>
        <rdfs:comment>e.g., ishtes/ištës, takaha/itak (sl-rozaj)</rdfs:comment>
        <rdfs:comment>e.g., wsze/wszystek, wszech/wszystek, wszem/wszystek, wszyscy/wszystek, wszystek/wszystek, wszystka/wszystek, wszystkich/wszystek, wszystkie/wszystek, wszystkiego/wszystek (pl)</rdfs:comment>
        <rdfs:comment>Pronoun/Type=&quot;general&quot; in English, and Slavic MTE v4 specs refers to pronouns not grouped together with any of the other subcategories of Pronoun defined for the respective language. In Slovak, for example, &quot;general&quot; pronouns concern the Pronouns like &quot;všetci&quot; [E. &quot;all&quot;], &quot;každý&quot; [E. &quot;every&quot;] etc.) (MTE v4)</rdfs:comment>
    </owl:Class>
    


    <!-- http://purl.org/olia/mte/multext-east.owl#GenitiveCase -->

    <owl:Class rdf:about="http://purl.org/olia/mte/multext-east.owl#GenitiveCase">
        <rdfs:subClassOf rdf:resource="http://purl.org/olia/mte/multext-east.owl#Case"/>
        <rdfs:comment>Persian:
Nouns may also be accompanied by the Ezafe Marker, a suffix that connects the elements in a phrase, and the indefinite marker. Ezafe Marker can appear as ‘‫( ’ﯼ‬ye) when the word ends in certain characters. It can also appear as a short vowel named Kasre which sounds &quot;e&quot;. In this case, according to the Farsi orthography, it can be deleted from the written text. A noun which is accompanied by Ezafe Marker can be considered as the genitive case of the noun. ...
Adjectives, just the same as nouns, may also be accompanied by the Ezafe Marker and in this case we can consider it as a genitive case.
(Qasemizadeh and Rahimi 2006)</rdfs:comment>
        <rdfs:comment>e.g., , drugega/drug, drugih/drug, dveh/dva, dvojnega/dvojen, enega/en, enga/en, enih/en, enojnih/enojen (sl)</rdfs:comment>
        <rdfs:comment>e.g., - (hu)</rdfs:comment>
        <rdfs:comment>e.g., -mpotriva/împotriva, -naintea/înaintea, asupră/asupra (ro)</rdfs:comment>
        <rdfs:comment>e.g., 0, Аахена/Аахен Абая/Абай Абакана/Абакан Абакану/Абакан Абіджана/Абіджан Абовяна/Абовян Авентина/Авентин Адамстауна/Адамстаун Адена/Аден Аджаристану/Аджаристан Адлера/Адлер Адоніса/Адоніс Адріанополя/Адріанополь Азенкура/Азенкур Азербайджану/Азербайджан Азова/Азов Акермана/Акерман Акмолінська/Акмолінськ Акрополя/Акрополь Актюбінська/Актюбінськ, Або/= Абруццо/= Абу-Дабі/= Адріатичного моря/Адріатичне море Азовського моря/Азовське море Айдахо/= Ай-Петрі/= Аконкагуа/= Актау/= Алеппо/= Аліканте/= Алмати/= Альбі/= Андаманського моря/Андаманське море Анжу/= Ані/= Антананаріву/= Антигуа/= Апіа/= Апостолового/Апостолове, Абіссінії/Абіссінія Абуджі/Абуджа Абхазії/Абхазія Авдіївки/Авдіївка Австралії/Австралія Австрії/Австрія Австро-Угорщини/Австро-Угорщина Аддис-Абеби/Аддис-Абеба Аджарії/Аджарія Адигеї/Адигея Адріатики/Адріатика Азії/Азія Айови/Айова Аквітанії/Аквітанія Аккри/Аккра Ак-Мечеті/Ак-Мечеть Акмоли/Акмола акрилової кислоти/акрилова кислота Алабами/Алабама Албанії/Албанія, Азорських островів/Азорські острови Аландських островів/Аландські острови Алеутських островів/Алеутські острови Андаманських островів/Андаманські острови Антильських островів/Антильські острови Багамських островів/Багамські острови Балеарських островів/Балеарські острови Бельбеків/Бельбек Бермудських островів/Бермудські острови Бугів/Буг Великоднів/Великдень Великих Сорочинців/Великі Сорочинці Віргінських островів/Віргінські острови Гавайських островів/Гавайські острови Гебридських островів/Гебридські острови Драконових гір/Драконові гори ЖЕКів/ЖЕК Зеленого Мису островів/Зеленого Мису острови Змієвих валів/Змієві вали Зондських островів/Зондські острови, Альп/Альпи Анд/Анди Апеннін/Апенніни Аппалачів/Аппалачі Арденн/Арденни Афін/Афіни Багам/Багами Балкан/Балкани Байдарських воріт/Байдарські ворота Барановичів/Барановичі Бендер/Бендери Березняків/Березняки Бермуд/Бермуди Бескидів/Бескиди Біличів/Біличі Близнюків/Близнюки Богородчан/Богородчани Боровичів/Боровичі Бортничів/Бортничі Броварів/Бровари, Америк/Америка Андалуських гір/Андалуські гори Атлаських гір/Атлаські гори Бистриць/Бистриця Держдум/Держдума Жовтих Вод/Жовті Води Збройних Сил України/Збройні сили України Індій/Індія Інтернет-газет/Інтернет-газета Караваєвих дач/Караваєві дачі Магелланових хмар/Магелланові хмари Македоній/Македонія Мате Залка/= Пасх/Пасха Пилипівок/Пилипівка Рад/Рада Родезій/Родезія Інтернет-технологій/Інтернет-технологія, Антропова/Антропов Абая/Абай Абакума/Абакум Абакумовича/Абакумович Абалкіна/Абалкін Абашидзе/= Аббаса/Аббас Абдули/Абдула Абдуллоджанова/Абдуллоджанов Абеля/Абель Абовяна/Абовян Абрама/Абрам Абрамовича/Абрамович Абрамовича/Абрамович Абрамчука/Абрамчук Абуладзе/= Авакума/Авакум Авакумовича/Авакумович Августа/Август Августимова/Августимов, Антропових/Антропов Абакумів/Абакум Абакумовичів/Абакумович Абалкіних/Абалкін Абашидзе/= Аббасів/Аббас Абдулів/Абдула Абдуллоджанових/Абдуллоджанов Абелів/Абель Абовянів/Абовян Абрамів/Абрам Абрамовичів/Абрамович Абрамовичів/Абрамович Абрамчуків/Абрамчук Абуладзе/= Авакумів/Авакум Авакумовичів/Авакумович Августів/Август Августимових/Августимов Августинів/Августин (uk)</rdfs:comment>
        <rdfs:comment>e.g., XXIII/xxiii, XXV/xxv, ВАС/вы, Вас/вы, Двух/два, НАС/мы, Нечего/нечего, Обеих/оба, ПЕРВОЙ/первый (ru)</rdfs:comment>
        <rdfs:comment>e.g., absolwentów/absolwent, adoptujących/adoptować, akredytujących/akredytować, autora/autor, badanego/badać, badań/badanie, bieżącego/bieżeć, bliższej/bliski, bliższych/bliski (pl)</rdfs:comment>
        <rdfs:comment>e.g., becew/beč, Bohovaha/böguw, Bohovih/böguw, bögavi/böguw, chrivaha/krïw, Crishtusha/krïštuš, dneha/dan, dní/din, Eve/eva (sl-rozaj)</rdfs:comment>
        <rdfs:comment>e.g., bezbrojnih/bezbrojni, druge/drugi, drveta/drvo, dva, dvojih/dvoje, Englsoca/Englsoc, evroazijske/evroazijska, evroazijskih/evroazijski, evroazijskog/evroazijski (sr)</rdfs:comment>
        <rdfs:comment>e.g., devatenácté/devatenáctý, druhé/druhý, druhého/druhý, druhých/druhý, dvacátých/dvacátý, dvojí, dvou/dva, ho/on, jaké/jaký (cs)</rdfs:comment>
        <rdfs:comment>e.g., druhej/druhý, druhého/druhý, druhých/druhý, dvoch/dva, hentej/hentá, hentoho/hento, hentých/hento, hentých/hentá, ich (sk)</rdfs:comment>
        <rdfs:comment>e.g., me/mina, meie/mina, meiegi/mina, minu/mina, minugi/mina, mu/mina, nende/tema, nendegi/tema, Pauluste/Paulus (et)</rdfs:comment>
        <rdfs:comment>e.g., آنهايِ/آنها, بادِ/باد امتحان‌کردنِ/امتحان‌کردن ارتفاعِ/ارتفاع, بِ/ب اينگسوسِ/اينگسوس اسميتِ/اسميت, تيغ‌هايِ/تيغ الوارهايِ/الوار آموزه‌هايِ/آموزه, خودِ/خود, دوِ/دو دويِ/دو دهِ/ده, رنگيِ/رنگي بي‌امانِ/بي‌امان بوکسورمانندِ/بوکسورمانند, سرگرمِ/سرگرم روانهٔ/روانه حاويِ/حاوي, قوي‌ترِ/قوي بيشترِ/بيش اعظمِ/اعظم (fa)</rdfs:comment>
    </owl:Class>
    


    <!-- http://purl.org/olia/mte/multext-east.owl#Gerund -->

    <owl:Class rdf:about="http://purl.org/olia/mte/multext-east.owl#Gerund">
        <owl:equivalentClass rdf:resource="http://purl.org/olia/mte/multext-east.owl#GerundOrAdverbialParticiple"/>
        <rdfs:subClassOf rdf:resource="http://purl.org/olia/mte/multext-east.owl#VerbForm"/>
        <rdfs:comment>&quot;Gerund&quot; as defined here is fully ambiguous</rdfs:comment>
        <rdfs:comment>e.g., istnienie/istnienie, istnieniu/istnienie, kształtowanie/kształtowanie, kształtowaniu/kształtowanie, niedostosowanie/niedostosowanie, niedostrzeganie/niedostrzeganie, niedotrzymanie/niedotrzymanie, niepostrzeżenie/niepostrzeżenie, nieprzestrzegania/nieprzestrzeganie (pl)</rdfs:comment>
        <rdfs:comment>e.g., paistes/paistma, vundamentides/vundamentima, võttes/võtma (et)</rdfs:comment>
        <rdfs:comment>Gerunds are represented in MTE v4 by Verb/VForm=&quot;gerund&quot; and Noun/Type=&quot;gerund&quot;.
The term _gerund_ is ambiguous: with respect  to Latin, in whose grammatical tradition it originates, it refers to a  deverbal noun, and is needed in this function for Polish as well; in  descriptions of some other languages, however, it has been used for an  adverbial participle.  
The two meanings have nothing in common, except  that the English _ing_-form can translate both. (Ivan A Derzhanski, email 2010/06/09)&lt;br/&gt;

Gerunds as deverbal nouns are represented here as a separate concept GerundProper that is defined by the intersection of Gerund and Noun.

VForm=&quot;Gerund&quot;. For Polish Nouns also Type=&quot;Gerund&quot;, hence &quot;VerbForm and (Noun or VerbForm)&quot; (http://nl.ijs.si/ME/V4/msd/html/msd.N.html).&lt;br/&gt;

Russian: Verb/Type=&quot;gerund&quot;
Russian specification distinguish Type=Gerund, and hence introduce various nominative properties on Verb, i.e. Definiteness, Case.&lt;br/&gt;

Polish Noun/Type=&quot;gerund&quot;: 
# Gerund as a VForm (imiesłów przysłówkowy) is not to be confused with the gerund as a Noun Type (gerundium).
# The gerund, e.g., bieganie, is considered a Type of Nouns. Strictly speaking, gerunds are a subtype of common nouns, but are treated as a type parallel to both common and proper nouns for convenience. (MTE v4)

cf. Czech: Verbal nouns are classified as Nouns.&lt;br/&gt;

Macedonian: Verb forms gerund and adverbial participle are taken to be separate (noun and adverb) lemmas.&lt;br/&gt;

Romanian: The following features are pertinent to those moods which permit an adjectival use, i.e. participle and gerund. However, the adjectival use of gerund is extremely rare (o mână tremurndă - a shaking hand) and therefore gender and number apply mainly for the participle.</rdfs:comment>
        <owl:versionInfo>The problem is that the English term _gerund_ is ambiguous: with respect  
to Latin, in whose grammatical tradition it originates, it refers to a  
deverbal noun, and is needed in this function for Polish as well; in  
descriptions of some other languages, however, it has been used for an  
adverbial participle.  The two meanings have nothing in common, except  
that the English _ing_-form can translate both.
(Ivan A Derzhanski, email 2010/06/09)</owl:versionInfo>
    </owl:Class>
    


    <!-- http://purl.org/olia/mte/multext-east.owl#GerundOrAdverbialParticiple -->

    <owl:Class rdf:about="http://purl.org/olia/mte/multext-east.owl#GerundOrAdverbialParticiple">
        <rdfs:subClassOf rdf:resource="http://purl.org/olia/mte/multext-east.owl#VerbForm"/>
        <rdfs:comment>The problem is that the English term _gerund_ is ambiguous: with respect  
to Latin, in whose grammatical tradition it originates, it refers to a  
deverbal noun, and is needed in this function for Polish as well; in  
descriptions of some other languages, however, it has been used for an  
adverbial participle.  The two meanings have nothing in common, except  
that the English _ing_-form can translate both.
(Ivan A Derzhanski, email 2010/06/09)</rdfs:comment>
        <owl:versionInfo>introduced as a more precise synonym of &quot;Gerund&quot;</owl:versionInfo>
    </owl:Class>
    


    <!-- http://purl.org/olia/mte/multext-east.owl#GerundProper -->

    <owl:Class rdf:about="http://purl.org/olia/mte/multext-east.owl#GerundProper">
        <owl:equivalentClass>
            <owl:Class>
                <owl:intersectionOf rdf:parseType="Collection">
                    <rdf:Description rdf:about="http://purl.org/olia/mte/multext-east.owl#CommonNoun"/>
                    <rdf:Description rdf:about="http://purl.org/olia/mte/multext-east.owl#GerundOrAdverbialParticiple"/>
                </owl:intersectionOf>
            </owl:Class>
        </owl:equivalentClass>
        <rdfs:comment>The concept GerundProper is introduced here to refer to &quot;gerund&quot; in the sense of a deverbal noun. The term _gerund_, however, is ambiguous: with respect  to Latin, in whose grammatical tradition it originates, it refers to a  deverbal noun, and is needed in this function for Polish as well; in  descriptions of some other languages, however, it has been used for an  adverbial participle.  The two meanings have nothing in common, except  that the English _ing_-form can translate both. (Ivan A Derzhanski, email 2010/06/09)&lt;br/&gt;

Polish proper gerunds (deverbal nouns) are encoded as common nouns. Since they are very frequent in Polish, it seems expedient to add a type for them, i.e., Noun/Type=&quot;gerund&quot;. (Derzhanski and Kotsyba 2009)
</rdfs:comment>
    </owl:Class>
    


    <!-- http://purl.org/olia/mte/multext-east.owl#Human -->

    <owl:Class rdf:about="http://purl.org/olia/mte/multext-east.owl#Human">
        <rdfs:subClassOf rdf:resource="http://purl.org/olia/mte/multext-east.owl#Humanness"/>
        <rdfs:comment>Human=&quot;yes&quot;</rdfs:comment>
    </owl:Class>
    


    <!-- http://purl.org/olia/mte/multext-east.owl#Humanness -->

    <owl:Class rdf:about="http://purl.org/olia/mte/multext-east.owl#Humanness">
        <rdfs:subClassOf rdf:resource="http://purl.org/olia/mte/multext-east.owl#MorphosyntacticFeature"/>
        <rdfs:comment>The attribute &quot;Human&quot; is added to express derogativity in Polish. The Polish derogatives are a class of plural forms of nouns which are [−Human] in the nominative but [+Human] in the accusative. (MTE v4)</rdfs:comment>
    </owl:Class>
    


    <!-- http://purl.org/olia/mte/multext-east.owl#IllativeCase -->

    <owl:Class rdf:about="http://purl.org/olia/mte/multext-east.owl#IllativeCase">
        <rdfs:subClassOf rdf:resource="http://purl.org/olia/mte/multext-east.owl#Case"/>
        <rdfs:comment>e.g., -, abba/az, belé/ő, beléje/ő, beléjük/ők, belém/én, bármibe/bármi, csigaformákba/csigaformá, dolgozójukba/dolgozó (hu)</rdfs:comment>
        <rdfs:comment>e.g., aktuaalseimatesse/aktuaalseim, endasse/ise, endisse/ise, enesesse/ise, igasse/iga, igasugustesse/igasugune, iseendasse/iseenese, kellesse/kes, kõigisse/kõik (et)</rdfs:comment>
        <rdfs:comment>Case=&quot;illative&quot; (Estonian, Hungarian)</rdfs:comment>
    </owl:Class>
    


    <!-- http://purl.org/olia/mte/multext-east.owl#Imperative -->

    <owl:Class rdf:about="http://purl.org/olia/mte/multext-east.owl#Imperative">
        <rdfs:subClassOf rdf:resource="http://purl.org/olia/mte/multext-east.owl#VerbForm"/>
        <rdfs:comment>e.g., , bodi/biti, bodita/biti, bodite/biti, hodita/hoditi, pijva/piti, pojdita/iti (sl)</rdfs:comment>
        <rdfs:comment>e.g., -, veszekedjünk/veszekedik, veszítsenek/veszít, vihessenek/vihet, visszaverjenek/visszaver, vitatkozzunk/vitatkozik, zuhanjunk/zuhan (hu)</rdfs:comment>
        <rdfs:comment>e.g., accompagnaimu/akompanjät, amaite/amät, contemplaimo/kontemplät, Dáite/dät, gauo/tet, gauò/tet, hovarnajte/govarnät, hrishi/grišit, lashi/lägat (sl-rozaj)</rdfs:comment>
        <rdfs:comment>e.g., budi/biti, budimo/biti, htedni/hteti, htednimo/hteti, htjedni/htjeti, htjednimo/htjeti (sr)</rdfs:comment>
        <rdfs:comment>e.g., buď/byť, buďme/byť, buďte/byť, maj/mať, majme/mať, majte/mať, nezvestuj/nezvestovať, nezvestujme/nezvestovať, nezvestujte/nezvestovať (sk)</rdfs:comment>
        <rdfs:comment>e.g., buď/být, chtěj/chtít, dejme/dát, dejte/dát, nebraňme/bránit, nebudiž/být, nebuďme/budit, nebuďme/být, nevezme/vézt (cs)</rdfs:comment>
        <rdfs:comment>e.g., chodź/chodzić, chodźmy/chodzić, daj/dać, dajcie/dać, dodajmy/dodać, idź/iść, idźcie/iść, miejmy/mieć, mówmy/mówić (pl)</rdfs:comment>
        <rdfs:comment>e.g., ole/olema, olegi/olema, olge/olema, olgem/olema, olgu/olema, pidage/pidama, pidagem/pidama, saagu/saama, ärge/ära (et)</rdfs:comment>
        <rdfs:comment>e.g., Идемте/идти, Успокойтесь/успокоиться, Устройтесь/устроиться, Цепляйся/цепляться, Шевелись/шевелиться, идемте/идти, успокойтесь/успокоиться, хватайтесь/хвататься, цепляйтесь/цепляться (ru)</rdfs:comment>
        <rdfs:comment>e.g., абеткуй/абеткувати авізуй/авізувати агакай/агакати агітуй/агітувати агонізуй/агонізувати адвокатуй/адвокатувати адмініструй/адмініструвати айкай/айкати акай/акати акомпануй/акомпанувати акредитуйся/акредитуватися акредитуйсь/акредитуватися акторствуй/акторствувати акторуй/акторувати актуй/актувати акушеруй/акушерувати альокай/альокати аналізуй/аналізувати анкетуй/анкетувати анодуй/анодувати, абеткуймо/абеткувати авізуймо/авізувати агакаймо/агакати агітуймо/агітувати агонізуймо/агонізувати адвокатуймо/адвокатувати адмініструймо/адмініструвати айкаймо/айкати акаймо/акати акомпануймо/акомпанувати акредитуймося/акредитуватися акредитуймось/акредитуватися акторствуймо/акторствувати акторуймо/акторувати актуймо/актувати акушеруймо/акушерувати альокаймо/альокати аналізуймо/аналізувати анкетуймо/анкетувати анодуймо/анодувати, абеткуйте/абеткувати авізуйте/авізувати агакайте/агакати агітуйте/агітувати агонізуйте/агонізувати адвокатуйте/адвокатувати адмініструйте/адмініструвати айкайте/айкати акайте/акати акомпануйте/акомпанувати акредитуйтеся/акредитуватися акредитуйтесь/акредитуватися акторствуйте/акторствувати акторуйте/акторувати актуйте/актувати акушеруйте/акушерувати альокайте/альокати аналізуйте/аналізувати анкетуйте/анкетувати анодуйте/анодувати, аблактуй/аблактувати абонуй/абонувати абонуйся/абонуватися абонуйсь/абонуватися абордуй/абордувати абортуй/абортувати абсолютизуй/абсолютизувати абстрагуй/абстрагувати абстрагуйся/абстрагуватися абстрагуйсь/абстрагуватися абшитуй/абшитувати авансуй/авансувати авансуйся/авансуватися авансуйсь/авансуватися автоматизуй/автоматизувати авторизуй/авторизувати аглютинуй/аглютинувати агрегатуй/агрегатувати адаптуй/адаптувати адаптуйся/адаптуватися, аблактуймо/аблактувати абонуймо/абонувати абонуймося/абонуватися абонуймось/абонуватися абордуймо/абордувати абортуймо/абортувати абсолютизуймо/абсолютизувати абстрагуймо/абстрагувати абстрагуймося/абстрагуватися абстрагуймось/абстрагуватися абшитуймо/абшитувати авансуймо/авансувати авансуймося/авансуватися авансуймось/авансуватися автоматизуймо/автоматизувати авторизуймо/авторизувати аглютинуймо/аглютинувати агрегатуймо/агрегатувати адаптуймо/адаптувати адаптуймося/адаптуватися, аблактуйте/аблактувати абонуйте/абонувати абонуйтеся/абонуватися абонуйтесь/абонуватися абордуйте/абордувати абортуйте/абортувати абсолютизуйте/абсолютизувати абстрагуйте/абстрагувати абстрагуйтеся/абстрагуватися абстрагуйтесь/абстрагуватися абшитуйте/абшитувати авансуйте/авансувати авансуйтеся/авансуватися авансуйтесь/авансуватися автоматизуйте/автоматизувати авторизуйте/авторизувати аглютинуйте/аглютинувати агрегатуйте/агрегатувати адаптуйте/адаптувати адаптуйтеся/адаптуватися, агакни/агакнути айкни/айкнути арештуй/арештувати ахни/ахнути бабахни/бабахнути бабахнися/бабахнутися бабахнись/бабахнутися бамкни/бамкнути бахни/бахнути бахнися/бахнутися бахнись/бахнутися бацни/бацнути бебевхни/бебевхнути бебехни/бебехнути бебехнися/бебехнутися бебехнись/бебехнутися бевкни/бевкнути бекни/бекнути белькни/белькнути бемкни/бемкнути, агакнімо/агакнути агакнім/агакнути айкнімо/айкнути айкнім/айкнути арештуймо/арештувати ахнімо/ахнути ахнім/ахнути бабахнімо/бабахнути бабахнім/бабахнути бабахнімося/бабахнутися бабахнімось/бабахнутися бабахнімся/бабахнутися бамкнімо/бамкнути бамкнім/бамкнути бахнімо/бахнути бахнім/бахнути бахнімося/бахнутися бахнімось/бахнутися бахнімся/бахнутися бацнімо/бацнути, агакніть/агакнути айкніть/айкнути арештуйте/арештувати ахніть/ахнути бабахніть/бабахнути бабахніться/бабахнутися бамкніть/бамкнути бахніть/бахнути бахніться/бахнутися бацніть/бацнути бебевхніть/бебевхнути бебехніть/бебехнути бебехніться/бебехнутися бевкніть/бевкнути бекніть/бекнути белькніть/белькнути бемкніть/бемкнути беркицніть/беркицнути беркицніться/беркицнутися беркицьніть/беркицьнути (uk)</rdfs:comment>
        <rdfs:comment>e.g., бидете/сум, биди/сум, имај/има, имајте/има, недај, недајте/недај, недоспиј/недоспие, недоспијте/недоспие, недостасај/недостаса (mk)</rdfs:comment>
        <rdfs:comment>e.g., бъди/бъда, щете/ща (bg)</rdfs:comment>
        <rdfs:comment>e.g., باش, بخواب/خواب بايست/ايست باش, بده/ده ببخشي/بخش ببخش/بخش, بشماريد/شمار بدهيد/ده ببريد/بر, بمانيد/مان بجنبيد/جنب بايستيد/ايست, بگذاريد/گذار ببخشيد/بخش, شو باش, مکن/کن, نباش/باش (fa)</rdfs:comment>
    </owl:Class>
    


    <!-- http://purl.org/olia/mte/multext-east.owl#ImperfectTense -->

    <owl:Class rdf:about="http://purl.org/olia/mte/multext-east.owl#ImperfectTense">
        <rdfs:subClassOf rdf:resource="http://purl.org/olia/mte/multext-east.owl#Tense"/>
        <rdfs:comment>e.g., -nzestraţi/înzestra, -nzideaţi/înzidi, -nzorzonaţi/înzorzona, torceam/toarce (ro)</rdfs:comment>
        <rdfs:comment>e.g., bese/bet, beše/bet, bramase/bramät, bého/bet, běše/bet, daržaho/däržat, hardéhata/tet, hardéše/tet, herdého/tet (sl-rozaj)</rdfs:comment>
        <rdfs:comment>e.g., oldi/olema, oldud/olema, oli/olema, olid/olema, olidki/olema, oligi/olema, olime/olema, olimegi/olema, olin/olema (et)</rdfs:comment>
        <rdfs:comment>e.g., sažvaće/sažvakati, zastrasmo/zastrijeti, zastraste/zastrijeti, žmurasmo/žmuriti, žmuraste/žmuriti, žrtvovasmo/žrtvovati, žrtvovaste/žrtvovati (sr)</rdfs:comment>
        <rdfs:comment>e.g., беа/сум, бев/сум, бевме/сум, бевте/сум, беше/сум, бидеа/сум, бидев/сум, бидевме/сум, бидевте/сум (mk)</rdfs:comment>
        <rdfs:comment>e.g., беше/съм, бил/съм, била/съм, били/съм, било/съм, бъдеха/бъда, бях/съм, бяха/съм, бяхме/съм (bg)</rdfs:comment>
        <rdfs:comment>Tense=&quot;imperfect&quot; (Romanian, Croatian, Serbian, Macedonian, Bulgarian, Estonian)</rdfs:comment>
    </owl:Class>
    


    <!-- http://purl.org/olia/mte/multext-east.owl#Impersonal -->

    <owl:Class rdf:about="http://purl.org/olia/mte/multext-east.owl#Impersonal">
        <rdfs:subClassOf rdf:resource="http://purl.org/olia/mte/multext-east.owl#VerbForm"/>
        <rdfs:comment>e.g., stwierdzono/stwierdzić (pl)</rdfs:comment>
        <rdfs:comment>VForm=&quot;impersonal&quot; (Polish, Ukrainian)&lt;br/&gt;

In Ukrainian, the impersonal VForm (o) is characterized by the ending -то/-но. It exists in other Slavic languages as well, although in most of them it coincides with the neutral form of the passive adjectival participle and is classified as such. In Ukrainian, as well as in Polish, the attributive form is different from the predicative one, cf. in Ukrainian писане правило (a written rule) vs писано правило (a rule was/is written). (MTE v4)</rdfs:comment>
    </owl:Class>
    


    <!-- http://purl.org/olia/mte/multext-east.owl#Inanimate -->

    <owl:Class rdf:about="http://purl.org/olia/mte/multext-east.owl#Inanimate">
        <rdfs:subClassOf rdf:resource="http://purl.org/olia/mte/multext-east.owl#Animacy"/>
        <rdfs:comment>e.g., 0, Аахен/= Абай/= Абакан/= Абакан/= Абіджан/= Абовян/= Авентин/= Адамстаун/= Аден/= Аджаристан/= Адлер/= Адоніс/= Адріанополь/= Азенкур/= Азербайджан/= Азов/= Акерман/= Акмолінськ/= Акрополь/= Актюбінськ/=, Аахена/Аахен Абая/Абай Абакана/Абакан Абакану/Абакан Абіджана/Абіджан Абовяна/Абовян Авентина/Авентин Адамстауна/Адамстаун Адена/Аден Аджаристану/Аджаристан Адлера/Адлер Адоніса/Адоніс Адріанополя/Адріанополь Азенкура/Азенкур Азербайджану/Азербайджан Азова/Азов Акермана/Акерман Акмолінська/Акмолінськ Акрополя/Акрополь Актюбінська/Актюбінськ, Аахене/Аахен Абаю/Абай Абакане/Абакан Абакане/Абакан Абіджане/Абіджан Абовяне/Абовян Авентине/Авентин Адамстауне/Адамстаун Адене/Аден Аджаристане/Аджаристан Адлере/Адлер Адонісе/Адоніс Адріанополю/Адріанополь Азенкуре/Азенкур Азербайджане/Азербайджан Азове/Азов Акермане/Акерман Акмолінську/Акмолінськ Акрополю/Акрополь Актюбінську/Актюбінськ, Аахеном/Аахен Абаєм/Абай Абаканом/Абакан Абаканом/Абакан Абіджаном/Абіджан Абовяном/Абовян Авентином/Авентин Адамстауном/Адамстаун Аденом/Аден Аджаристаном/Аджаристан Адлером/Адлер Адонісом/Адоніс Адріанополем/Адріанополь Азенкуром/Азенкур Азербайджаном/Азербайджан Азовом/Азов Акерманом/Акерман Акмолінськом/Акмолінськ Акрополем/Акрополь Актюбінськом/Актюбінськ, Аахену/Аахен Аахенові/Аахен Абаю/Абай Абаєві/Абай Абакану/Абакан Абаканові/Абакан Абакану/Абакан Абаканові/Абакан Абіджану/Абіджан Абіджанові/Абіджан Абовяну/Абовян Абовянові/Абовян Авентину/Авентин Авентинові/Авентин Адамстауну/Адамстаун Адамстаунові/Адамстаун Адену/Аден Аденові/Аден Аджаристану/Аджаристан Аджаристанові/Аджаристан, Аахені/Аахен Аахену/Аахен Абаї/Абай Абаю/Абай Абакані/Абакан Абакану/Абакан Абакані/Абакан Абакану/Абакан Абіджані/Абіджан Абіджану/Абіджан Абовяні/Абовян Абовяну/Абовян Авентині/Авентин Авентину/Авентин Адамстауні/Адамстаун Адамстауну/Адамстаун Адені/Аден Адену/Аден Аджаристані/Аджаристан Аджаристану/Аджаристан, Абакумів/= Абрамів/= Авакумів/= Августин/= Августинів/= Августів/= Авенірів/= Аверкіїв/= Авер&apos;янів/= Авіятин/= Авксентіїв/= Аврамів/= Авреліїн/= Аврорин/= Автономів/= авторів/= авторчин/= Агапіїв/= Агапіїн/= Агапітів/=, Або/= Абруццо/= Абу-Дабі/= Адріатичне море/= Азовське море/= Айдахо/= Ай-Петрі/= Аконкагуа/= Актау/= Алеппо/= Аліканте/= Алмати/= Альбі/= Андаманське море/= Анжу/= Ані/= Антананаріву/= Антигуа/= Апіа/= Апостолове/= (uk)</rdfs:comment>
        <rdfs:comment>e.g., Bohouv/böguw, dalesgni/dalëčnji, dan/dan, den/dan, dobar/dobar, dobre/dobar, etej/iti, furlanskë/furlanski, isó/isi (sl-rozaj)</rdfs:comment>
        <rdfs:comment>e.g., VX/vx, XVII/xvii, XXIII/xxiii, XXIV/xxiv, XXV/xxv, XXVII/xxvii, Нечем/нечего, Чечне/Чечня, нечем/нечего (ru)</rdfs:comment>
        <rdfs:comment>e.g., badaniem/badanie, brawo/brawo, cały/cały, celowi/cel, chłopaki/chłopak, co/co, cokolwiek/cokolwiek, coś/coś, czasu/czas (pl)</rdfs:comment>
        <rdfs:comment>e.g., belim/beo, bezbrojnih/bezbrojni, Bratstvom/Bratstvo, Bratstvu/Bratstvo, dva, dvoje, evroazijskih/evroazijski, Faroskih/Faroska, francuski (sr)</rdfs:comment>
        <rdfs:comment>e.g., byly/být, bývaly/bývat, daly/dát, devatenácté/devatenáctý, dostaly/dostat, druhej/druhý, druhé/druhý, druhý, dvojí (cs)</rdfs:comment>
        <rdfs:comment>e.g., druhom/druhý, druhé/druhý, druhého/druhý, druhému/druhý, druhý, druhých/druhý, druhým/druhý, druhými/druhý, dva (sk)</rdfs:comment>
        <rdfs:comment>Animate=&quot;no&quot; (Slavic Noun/Pronoun http://nl.ijs.si/ME/V4/msd/html/msd.N.html; Czech verb)&lt;br/&gt;

Slovak (like most other Slavic languages) distinguishes masculine animate (Animate=&quot;yes&quot;) and masculine inanimate (Animate=&quot;no&quot;) gender. Masculine inanimate nouns always have the same form in the nominative and accusative case, whereas masculine animate nouns have predominantly the same form in the genitive and accusative case. Masculine animate nouns and masculine inanimate nouns differ in accusative singular, nominative (vocative) and accusative plural only (Slovak MTE v4). </rdfs:comment>
    </owl:Class>
    


    <!-- http://purl.org/olia/mte/multext-east.owl#Indefinite -->

    <owl:Class rdf:about="http://purl.org/olia/mte/multext-east.owl#Indefinite">
        <rdfs:subClassOf rdf:resource="http://purl.org/olia/mte/multext-east.owl#AmbiguousDefinitenessFeature"/>
        <rdfs:comment>e.g., -, lennétek/lesz, továbbtaníttatnátok/továbbtaníttat, tudnátok/tud, veszekedjünk/veszekedik, veszítsenek/veszít, vihessenek/vihet, visszaemlékszel/visszaemlékszik, visszarettentek/visszaretten (hu)</rdfs:comment>
        <rdfs:comment>e.g., -mpărate/împărat, -ngrijitoare/îngrijitoare, -nsoţitoare/însoţitoare, -ntrebătoare/întrebător, -ntregi/întreg, -ntreprinzătoare/întreprinzător, -ntâi/întâi, -nvingători/învingător, -nvinşi/învins (ro)</rdfs:comment>
        <rdfs:comment>e.g., Bohouv/böguw, dobar/dobar, furlanskë/furlanski, kako/kak, löpu/lip, malu/mäl, moćan/möćan, niškë/niški, oblejan/oblajän (sl-rozaj)</rdfs:comment>
        <rdfs:comment>e.g., Goldštajnov, govornikov, jak, nepuna/nepun, Parsonsovih/Parsonov, predivan, prekasan, rasan, svetu/svet (sr)</rdfs:comment>
        <rdfs:comment>e.g., drug/=, trojen/= (sl)</rdfs:comment>
        <rdfs:comment>e.g., Америки/Америка, Индуси/Индус, Конго, Македонецу/Македонец, Македонки/Македонка, Македонко/Македонка, Македонци/Македонец, Македонче, Македонче/Македонец (mk)</rdfs:comment>
        <rdfs:comment>e.g., бил/бъда, бил/съм, била/бъда, била/съм, били/бъда, били/съм, било/бъда, било/съм, бъдещ/бъда (bg)</rdfs:comment>
        <rdfs:comment>e.g., بلندتري/بلند انساني‌تري/انساني‌ آرام‌تري/آرام, زنگداري/زنگدار تهوع‌آوري/تهوع‌آور برهنه‌اي/برهنه, ساعاتي/ساعت ارقامي/رقم آستين‌هايي/آستين, سومي/سه, يکي/يک نيمي/نيم اندي/اند, گردبادي/گردباد جذابيتي/جذابيت آيينه‌اي/آيينه (fa)</rdfs:comment>
        <rdfs:comment>Definiteness=&quot;no&quot; (Noun/Adjective: Romanian, Macedonian, Bulgarian, Persian; Verb: Bulgarian, Hungarian; Pronoun: Resian, Macedonian, Bulgarian)&lt;br/&gt;

For Bulgarian, Romanian and Macedonian, Definiteness=&quot;no&quot; marks the absence of the definite article at the element in the clause that is expected to carry it (usually the first word of an NP).&lt;br/&gt;

Also, Persian does have an article, but it marks specificity rather than definiteness. (Ivan A. Derzhanski, email 2010/06/18) According to Qasemizadeh &amp; Rahimi&apos;s (2006) description of tokenization, Definiteness of Nouns etc. thus refers to an orthographically non-separated definite (specifity-marking) article.
</rdfs:comment>
    </owl:Class>
    


    <!-- http://purl.org/olia/mte/multext-east.owl#IndefiniteAdjective -->

    <owl:Class rdf:about="http://purl.org/olia/mte/multext-east.owl#IndefiniteAdjective">
        <rdfs:subClassOf rdf:resource="http://purl.org/olia/mte/multext-east.owl#Adjective"/>
        <owl:deprecated>MTE v4 contains Adjective/Type=&quot;indefinite&quot;, although this isn&apos;t actually used for any of the languages.</owl:deprecated>
    </owl:Class>
    


    <!-- http://purl.org/olia/mte/multext-east.owl#IndefiniteArticle -->

    <owl:Class rdf:about="http://purl.org/olia/mte/multext-east.owl#IndefiniteArticle">
        <rdfs:subClassOf rdf:resource="http://purl.org/olia/mte/multext-east.owl#Article"/>
        <rdfs:comment>e.g., -i, -ist, -iste, -istă, -işti, -o/un, -un/un, -uri, o/un (ro)</rdfs:comment>
        <rdfs:comment>e.g., dan/dan, den/dan, dnaha/dan, dneha/dan, dni/dan, dnin/dan, na/dan, naga/dan, nagha/dan (sl-rozaj)</rdfs:comment>
        <rdfs:comment>e.g., egy (hu)</rdfs:comment>
        <rdfs:comment>Article/Type=&quot;indefinite&quot; is used in the Romanian, Resian and Hungarian MTE v4 specs.

Hungarian, for example, has tree articles: a, az and egy. egy is indefinite. These may not have number and case. In Resian, the indefinite pronoun is &apos;din na nö&apos; and formally distinct from the numeral from which it derived: &apos;dyn dnä dnö&apos;. (MTE v4)</rdfs:comment>
    </owl:Class>
    


    <!-- http://purl.org/olia/mte/multext-east.owl#IndefiniteDeterminer -->

    <owl:Class rdf:about="http://purl.org/olia/mte/multext-east.owl#IndefiniteDeterminer">
        <rdfs:subClassOf rdf:resource="http://purl.org/olia/mte/multext-east.owl#Determiner"/>
        <rdfs:comment>e.g., -atât/atât, -atâta/atât, alde, alt, alte/alt, altă/alt, alţi/alt, anumit, anumite/anumit (ro)</rdfs:comment>
        <rdfs:comment>e.g., a, an/a (en)</rdfs:comment>
        <rdfs:comment>e.g., کليهٔ/کليه ساير انواعِ/نوع (fa)</rdfs:comment>
        <rdfs:comment>Determiner/Type=&quot;indefinite&quot; (English, Romanian, Persian)</rdfs:comment>
    </owl:Class>
    


    <!-- http://purl.org/olia/mte/multext-east.owl#IndefinitePronoun -->

    <owl:Class rdf:about="http://purl.org/olia/mte/multext-east.owl#IndefinitePronoun">
        <rdfs:subClassOf rdf:resource="http://purl.org/olia/mte/multext-east.owl#Pronoun"/>
        <rdfs:comment>e.g., -, bármibe/bármi, egyebekről/egyéb, egyike/egyik, egyikeként/egyik, egyikébe/egyik, egyikében/egyik, egyikéből/egyik, egyikén/egyik (hu)</rdfs:comment>
        <rdfs:comment>e.g., a_dreaptă, niscaiva, oarecare (ro)</rdfs:comment>
        <rdfs:comment>e.g., cach/kak, chira/kiri, dan/dän, dnumu/dän, kako/kak, kej/kej, kiri/kiri (sl-rozaj)</rdfs:comment>
        <rdfs:comment>e.g., cokolwiek/cokolwiek, coś/coś, czegokolwiek/cokolwiek, czegoś/coś, czemuś/coś, czyichkolwiek/czyjkolwiek, czyichś/czyjś, czyimikolwiek/czyjkolwiek, czyimiś/czyjś (pl)</rdfs:comment>
        <rdfs:comment>e.g., hocikoľké/hocikoľko, hocikoľkí/hocikoľko, hockoľké/hockoľko, hockoľkí/hockoľko, niekoľké/niekoľko, niekoľkí/niekoľko, niekoľkých/niekoľko, niekoľkým/niekoľko, niekoľkými/niekoľko (sk)</rdfs:comment>
        <rdfs:comment>e.g., igasugustesse/igasugune, muist, muudeks/muu, muudelt/muu, muuta/muu, paljudeks/palju, paljudesse/palju, teisena/teine, teistega/teine (et)</rdfs:comment>
        <rdfs:comment>e.g., kdekoho/kdekdo, kdekterých/kdekterý, kdekterými/kdekterý, komukoliv/kdokoli, kýmkoli/kdokoli, kýmsi/kdosi, málokterých/málokterý, málokterými/málokterý, někoho/někdo (cs)</rdfs:comment>
        <rdfs:comment>e.g., mnogimi/mnog, nekaterim/nekateri (sl)</rdfs:comment>
        <rdfs:comment>e.g., neka/neki, nekoliko/nekolik, nečega/nešto (sr)</rdfs:comment>
        <rdfs:comment>e.g., аби на кому/абихто аби на кім/абихто бозна-кому/бозна-хто бозна-кім/бозна-хто бозна на кому/бозна-хто бозна на кім/бозна-хто будь-кому/будь-хто будь-кім/будь-хто будь на кому/будь-хто будь на кім/будь-хто декому/дехто декім/дехто де на кому/дехто де на кім/дехто казна-кому/казна-хто казна-кім/казна-хто казна на кому/казна-хто казна на кім/казна-хто леда-кому/леда-хто леда-кім/леда-хто, аби на чому/абищо аби на чім/абищо бозна-чому/бозна-що бозна-чім/бозна-що бозна на чому/бозна-що бозна на чім/бозна-що будь-чому/будь-що будь-чім/будь-що будь на чому/будь-що будь на чім/будь-що дечому/дещо дечім/дещо де на чому/дещо де на чім/дещо казна-чому/казна-що казна-чім/казна-що казна на чому/казна-що казна на чім/казна-що леда-чому/леда-що леда-чім/леда-що, абиким/абихто аби з ким/абихто бозна-ким/бозна-хто будь-ким/будь-хто деким/дехто з деким/дехто де з ким/дехто казна-ким/казна-хто леда-ким/леда-хто небагато-ким/небагато-хто невідь-ким/невідь-хто ким-будь/хто-будь хтозна-ким/хтозна-хто ким-небудь/хто-небудь ким-не-ким/хто-не-хто кимось/хтось кимсь/хтось кимось-то/хтось-то кимсь-то/хтось-то чортзна-ким/чортзна-хто, абикого/абихто аби до кого/абихто бозна-кого/бозна-хто будь-кого/будь-хто декого/дехто казна-кого/казна-хто леда-кого/леда-хто небагато-кого/небагато-хто невідь-кого/невідь-хто кого-будь/хто-будь хтозна-кого/хтозна-хто кого-небудь/хто-небудь кого-не-кого/хто-не-хто когось/хтось когось-то/хтось-то чортзна-кого/чортзна-хто, абикого/абихто бозна-кого/бозна-хто будь-кого/будь-хто декого/дехто казна-кого/казна-хто леда-кого/леда-хто небагато-кого/небагато-хто невідь-кого/невідь-хто кого-будь/хто-будь хтозна-кого/хтозна-хто кого-небудь/хто-небудь кого-не-кого/хто-не-хто когось/хтось когось-то/хтось-то чортзна-кого/чортзна-хто, абикому/абихто бозна-кому/бозна-хто будь-кому/будь-хто декому/дехто казна-кому/казна-хто леда-кому/леда-хто небагато-кому/небагато-хто невідь-кому/невідь-хто кому-будь/хто-будь хтозна-кому/хтозна-хто кому-небудь/хто-небудь кому-не-кому/хто-не-хто комусь/хтось комусь-то/хтось-то чортзна-кому/чортзна-хто, абихто/= бозна-хто/= будь-хто/= дехто/= казна-хто/= леда-хто/= небагато-хто/= невідь-хто/= хто-будь/= хтозна-хто/= хто-небудь/= хто-не-хто/= хтось/= хтось-то/= чортзна-хто/=, абичий/= бозна-чий/= будь-чий/= дечий/= хтозна-чий/= чий-будь/= чий-небудь/= чийсь/=, абичийого/абичий аби до чийого/абичий бозна-чийого/бозна-чий будь-чийого/будь-чий дечийого/дечий хтозна-чийого/хтозна-чий чийого-будь/чий-будь чийого-небудь/чий-небудь чийогось/чийсь (uk)</rdfs:comment>
        <rdfs:comment>e.g., еди-кой, еди-кой_си, което_и_да_е, които_и_да_са, който_и_да_е, която_и_да_е, неколцина, нечие, нечие/нечий (bg)</rdfs:comment>
        <rdfs:comment>e.g., некого/некој, некое/некој, некои/некој, некому/некој, некој, некоја/некој, нечие/нечиј, нечии/нечиј, нечиј (mk)</rdfs:comment>
        <rdfs:comment>e.g., بقيه برخي اين‌همه, يکي/يک هرآنچه ديگري (fa)</rdfs:comment>
        <rdfs:comment>Pronoun/Type=&quot;indefinite&quot;&lt;br/&gt;

For some languages, IndefinitePronoun also covers negative pronous. In Romanian, however,  it is worth differentiating the negative pronoun from other indefinite pronouns: a negative pronoun cannot be an argument for a verb unless the verb itself is negated too (e.g. Nu am văzut pe nimeni / *Am văzut pe nimeni). (MTE v4)</rdfs:comment>
    </owl:Class>
    


    <!-- http://purl.org/olia/mte/multext-east.owl#IndefiniteQuantifier -->

    <owl:Class rdf:about="http://purl.org/olia/mte/multext-east.owl#IndefiniteQuantifier">
        <rdfs:subClassOf rdf:resource="http://purl.org/olia/mte/multext-east.owl#ProQuantifier"/>
        <owl:versionInfo>In the Czech and Slovak MTE v4 specs, Numeral/Class=&quot;indefinite&quot; are items meaning `several/some&apos;,  etc. Strictly speaking, they are pronumerals (pro-quantifiers), but traditional descriptions don&apos;t recognise such a category, so they are described variously as pronouns or as numerals (because their syntactic distribution is that of numerals, or very close).&quot; (Ivan A Derzhanski, email 2010/06/11)</owl:versionInfo>
    </owl:Class>
    


    <!-- http://purl.org/olia/mte/multext-east.owl#Indicative -->

    <owl:Class rdf:about="http://purl.org/olia/mte/multext-east.owl#Indicative">
        <rdfs:subClassOf rdf:resource="http://purl.org/olia/mte/multext-east.owl#VerbForm"/>
        <rdfs:comment>e.g., &apos;A/have, daren&apos;t/dare+not, lacquered/lacquer, nose, oughter/have, was/be, wasn&apos;t/be+not, wass/be, were/be (en)</rdfs:comment>
        <rdfs:comment>e.g., -, elárultalak/elárul, figyelmeztettelek/figyelmeztet, megismertelek/megismer, uralhatjátok/uralhat, visszaemlékszel/visszaemlékszik, visszarettentek/visszaretten, visszatérsz/visszatér, visszatértek/visszatér (hu)</rdfs:comment>
        <rdfs:comment>e.g., -nzestrarăm/înzestra, -nzestrarăţi/înzestra, -nzestrasem/înzestra, -nzestraseră/înzestra, -nzestraserăm/înzestra, -nzestraserăţi/înzestra, -nzestraseşi/înzestra, -nzestraţi/înzestra, -nzideaţi/înzidi (ro)</rdfs:comment>
        <rdfs:comment>e.g., aman/amät, bese/bet, beše/bet, bo/bet, bogan/bogat, boijo/bat, bom/bet, bon/bet, bota/bet (sl-rozaj)</rdfs:comment>
        <rdfs:comment>e.g., bałoś/bać, byli/być, byliście/być, byliśmy/być, bywały/bywać, był/być, była/być, byłam/być, byłaś/być (pl)</rdfs:comment>
        <rdfs:comment>e.g., biće/biti, bićemo/biti, bićete/biti, bićeš/biti, biću/biti, sažvaće/sažvakati, zastrasmo/zastrijeti, zastraste/zastrijeti, zveknućemo/zveknuti (sr)</rdfs:comment>
        <rdfs:comment>e.g., bude/být, budeme/být, budete/být, budeš/být, budou/být, budu/být, bývám/bývat, chceme/chtít, chcete/chtít (cs)</rdfs:comment>
        <rdfs:comment>e.g., je/byť, majú/mať, musia/musieť, musí/musieť, musím/musieť, musíš/musieť, má/mať, mám/mať, máme/mať (sk)</rdfs:comment>
        <rdfs:comment>e.g., olda/olema, oldi/olema, oldud/olema, oled/olema, oledki/olema, oleme/olema, olemegi/olema, olen/olema, olengi/olema (et)</rdfs:comment>
        <rdfs:comment>e.g., БУДЕМ/быть, БУДЕТ/быть, БУДЕТЕ/быть, БУДЕШЬ/быть, БУДУ/быть, БУДУТ/быть, Бежим/бежать, Будет/быть, Будете/быть (ru)</rdfs:comment>
        <rdfs:comment>e.g., абеткував/абеткувати авізував/авізувати агакав/агакати агітував/агітувати агонізував/агонізувати адвокатував/адвокатувати адміністрував/адмініструвати адоптувався/адоптуватися адоптувавсь/адоптуватися адсорбувався/адсорбуватися адсорбувавсь/адсорбуватися азотувався/азотуватися азотувавсь/азотуватися айкав/айкати акав/акати акомпанував/акомпанувати акредитувався/акредитуватися акредитувавсь/акредитуватися акторствував/акторствувати акторував/акторувати, абеткувала/абеткувати авізувала/авізувати агакала/агакати агітувала/агітувати агонізувала/агонізувати адвокатувала/адвокатувати адмініструвала/адмініструвати адоптувалася/адоптуватися адоптувалась/адоптуватися адсорбувалася/адсорбуватися адсорбувалась/адсорбуватися азотувалася/азотуватися азотувалась/азотуватися айкала/айкати акала/акати акомпанувала/акомпанувати акредитувалася/акредитуватися акредитувалась/акредитуватися акторствувала/акторствувати акторувала/акторувати, абеткували/абеткувати авізували/авізувати агакали/агакати агітували/агітувати агонізували/агонізувати адвокатували/адвокатувати адміністрували/адмініструвати адоптувалися/адоптуватися адоптувались/адоптуватися адсорбувалися/адсорбуватися адсорбувались/адсорбуватися азотувалися/азотуватися азотувались/азотуватися айкали/айкати акали/акати акомпанували/акомпанувати акредитувалися/акредитуватися акредитувались/акредитуватися акторствували/акторствувати акторували/акторувати, абеткувало/абеткувати авізувало/авізувати агакало/агакати агітувало/агітувати агонізувало/агонізувати адвокатувало/адвокатувати адмініструвало/адмініструвати адоптувалося/адоптуватися адоптувалось/адоптуватися адсорбувалося/адсорбуватися адсорбувалось/адсорбуватися азотувалося/азотуватися азотувалось/азотуватися айкало/айкати акало/акати акомпанувало/акомпанувати акредитувалося/акредитуватися акредитувалось/акредитуватися акторствувало/акторствувати акторувало/акторувати, абеткуватиме/абеткувати авізуватиме/авізувати агакатиме/агакати агітуватиме/агітувати агонізуватиме/агонізувати адвокатуватиме/адвокатувати адмініструватиме/адмініструвати адоптуватиметься/адоптуватися адсорбуватиметься/адсорбуватися азотуватиметься/азотуватися айкатиме/айкати акатиме/акати акомпануватиме/акомпанувати акредитуватиметься/акредитуватися акторствуватиме/акторствувати акторуватиме/акторувати актуватиме/актувати акушеруватиме/акушерувати акцентуватиметься/акцентуватися альокатиме/альокати, абеткуватимемо/абеткувати абеткуватимем/абеткувати авізуватимемо/авізувати авізуватимем/авізувати агакатимемо/агакати агакатимем/агакати агітуватимемо/агітувати агітуватимем/агітувати агонізуватимемо/агонізувати агонізуватимем/агонізувати адвокатуватимемо/адвокатувати адвокатуватимем/адвокатувати адмініструватимемо/адмініструвати адмініструватимем/адмініструвати айкатимемо/айкати айкатимем/айкати акатимемо/акати акатимем/акати акомпануватимемо/акомпанувати акомпануватимем/акомпанувати, абеткуватимете/абеткувати авізуватимете/авізувати агакатимете/агакати агітуватимете/агітувати агонізуватимете/агонізувати адвокатуватимете/адвокатувати адмініструватимете/адмініструвати айкатимете/айкати акатимете/акати акомпануватимете/акомпанувати акредитуватиметеся/акредитуватися акредитуватиметесь/акредитуватися акторствуватимете/акторствувати акторуватимете/акторувати актуватимете/актувати акушеруватимете/акушерувати альокатимете/альокати аналізуватимете/аналізувати анкетуватимете/анкетувати анодуватимете/анодувати, абеткуватимеш/абеткувати авізуватимеш/авізувати агакатимеш/агакати агітуватимеш/агітувати агонізуватимеш/агонізувати адвокатуватимеш/адвокатувати адмініструватимеш/адмініструвати айкатимеш/айкати акатимеш/акати акомпануватимеш/акомпанувати акредитуватимешся/акредитуватися акторствуватимеш/акторствувати акторуватимеш/акторувати актуватимеш/актувати акушеруватимеш/акушерувати альокатимеш/альокати аналізуватимеш/аналізувати анкетуватимеш/анкетувати анодуватимеш/анодувати аплодуватимеш/аплодувати, абеткуватиму/абеткувати авізуватиму/авізувати агакатиму/агакати агітуватиму/агітувати агонізуватиму/агонізувати адвокатуватиму/адвокатувати адмініструватиму/адмініструвати айкатиму/айкати акатиму/акати акомпануватиму/акомпанувати акредитуватимуся/акредитуватися акредитуватимусь/акредитуватися акторствуватиму/акторствувати акторуватиму/акторувати актуватиму/актувати акушеруватиму/акушерувати альокатиму/альокати аналізуватиму/аналізувати анкетуватиму/анкетувати анодуватиму/анодувати (uk)</rdfs:comment>
        <rdfs:comment>e.g., бе/съм, беше/съм, би/бъда, бих/бъда, биха/бъда, бихте/бъда, бъда, бъдат/бъда, бъде/бъда (bg)</rdfs:comment>
        <rdfs:comment>e.g., беа/сум, бев/сум, бевме/сум, бевте/сум, беше/сум, бидам/сум, бидат/сум, биде/сум, бидеа/сум (mk)</rdfs:comment>
        <rdfs:comment>e.g., آمديد/آمد, آمديم/آمد, اند/است, ايد/است, برآورد انداخت انجاميد, برمي‌داشتيد/برداشت, بودي/بود, بوديد/بود, بوديد/بود بودي/بود (fa)</rdfs:comment>
    </owl:Class>
    


    <!-- http://purl.org/olia/mte/multext-east.owl#InessiveCase -->

    <owl:Class rdf:about="http://purl.org/olia/mte/multext-east.owl#InessiveCase">
        <rdfs:subClassOf rdf:resource="http://purl.org/olia/mte/multext-east.owl#Case"/>
        <rdfs:comment>e.g., Baltimaades/Baltimaad, esimestes/esimene, neis/tema, nendes/tema, paistmas/paistma, tas/tema, teis/sina, teistes/teine, temas/tema (et)</rdfs:comment>
        <rdfs:comment>e.g., bennetek/ti, hetekben/hét, kötőjükben/kötő, tulajdonukban/tulajdon, vallatásukban/vallatás, versgyűjteményekben/versgyűjtemény, vitákban/vita, értelemében/értél, útvesztőiben/útvesztő (hu)</rdfs:comment>
        <rdfs:comment>Case=&quot;inessive&quot; (Hungarian, Estonian)</rdfs:comment>
    </owl:Class>
    


    <!-- http://purl.org/olia/mte/multext-east.owl#Infinitive -->

    <owl:Class rdf:about="http://purl.org/olia/mte/multext-east.owl#Infinitive">
        <rdfs:subClassOf rdf:resource="http://purl.org/olia/mte/multext-east.owl#VerbForm"/>
        <rdfs:comment>e.g., -a/a, a, fi (ro)</rdfs:comment>
        <rdfs:comment>e.g., be (en)</rdfs:comment>
        <rdfs:comment>e.g., bejt/být, být, bývat, dostat, mít, nebýt/být, nemít/mít, nezneužívat/zneužívat, neztratit/ztratit (cs)</rdfs:comment>
        <rdfs:comment>e.g., bet/bet, bit/bet, biti/bet, meritat/maratät, moret/morët, prabet/pribet, Spovedat/spovëdat, veruat/vërwat, videt/vïdët (sl-rozaj)</rdfs:comment>
        <rdfs:comment>e.g., biti, hteti, htjeti (sr)</rdfs:comment>
        <rdfs:comment>e.g., być/być, mieć/mieć, mówić/mówić, określić/określić, powiedzieć/powiedzieć, uznać/uznać (pl)</rdfs:comment>
        <rdfs:comment>e.g., byť, mať, musieť, môcť, smieť (sk)</rdfs:comment>
        <rdfs:comment>e.g., olla/olema, ollagi/olema (et)</rdfs:comment>
        <rdfs:comment>e.g., venniük/vesz, visszajuttatniuk/visszajuttat, végigszenvedniük/végigszenved (hu)</rdfs:comment>
        <rdfs:comment>e.g., абеткувати/= абеткувать/абеткувати авізувати/= авізувать/авізувати агакати/= агакать/агакати агітувати/= агітувать/агітувати агонізувати/= агонізувать/агонізувати адвокатувати/= адвокатувать/адвокатувати адмініструвати/= адмініструвать/адмініструвати адоптуватися/= адоптуватись/адоптуватися адсорбуватися/= адсорбуватись/адсорбуватися азотуватися/= азотуватись/азотуватися, аблактувати/= аблактувать/аблактувати абонувати/= абонувать/абонувати абонуватися/= абонуватись/абонуватися абордувати/= абордувать/абордувати абортувати/= абортувать/абортувати абсолютизувати/= абсолютизувать/абсолютизувати абсолютизуватися/= абсолютизуватись/абсолютизуватися абсорбувати/= абсорбувать/абсорбувати абсорбуватися/= абсорбуватись/абсорбуватися абстрагувати/= абстрагувать/абстрагувати, агакнути/= агакнуть/агакнути айкнути/= айкнуть/айкнути арештувати/= арештувать/арештувати ахнути/= ахнуть/ахнути бабахнути/= бабахнуть/бабахнути бабахнутися/= бабахнутись/бабахнутися бамкнути/= бамкнуть/бамкнути бахнути/= бахнуть/бахнути бахнутися/= бахнутись/бахнутися бацнути/= бацнуть/бацнути, бути/= буть/бути (uk)</rdfs:comment>
    </owl:Class>
    


    <!-- http://purl.org/olia/mte/multext-east.owl#InfinitiveParticle -->

    <owl:Class rdf:about="http://purl.org/olia/mte/multext-east.owl#InfinitiveParticle">
        <rdfs:subClassOf rdf:resource="http://purl.org/olia/mte/multext-east.owl#VerbalParticle"/>
        <rdfs:comment>Particle/Type=&quot;infinitive&quot; (Romanian)

A verbal particle with Particle/Type=&quot;future&quot; modifies the verbs and carries the information that the verb is infinite (Dan Tufis, email 2010/06/09)</rdfs:comment>
    </owl:Class>
    


    <!-- http://purl.org/olia/mte/multext-east.owl#InitialCoordinatingConjunction -->

    <owl:Class rdf:about="http://purl.org/olia/mte/multext-east.owl#InitialCoordinatingConjunction">
        <rdfs:subClassOf rdf:resource="http://purl.org/olia/mte/multext-east.owl#CoordinatingConjunction_PositionalType"/>
        <rdfs:comment>In the English MTE v4 specs, Conjunction/Coord_Type=&quot;initial&quot; designates the initial component of a complex conjunction consisting of multiple words (see CorrelativeCoordinatingConjunction), e.g., &quot;neither&quot; in &quot;either ... or ...&quot; and &quot;either&quot; in &quot;neither ... nor ...&quot;.</rdfs:comment>
    </owl:Class>
    


    <!-- http://purl.org/olia/mte/multext-east.owl#InstrumentalCase -->

    <owl:Class rdf:about="http://purl.org/olia/mte/multext-east.owl#InstrumentalCase">
        <rdfs:subClassOf rdf:resource="http://purl.org/olia/mte/multext-east.owl#Case"/>
        <rdfs:comment>e.g., , drugim/drug, drugimi/drug, drugo/drug, dušikovima/dušikov, dvema/dva, dvemi/dva, enim/en, enimi/en (sl)</rdfs:comment>
        <rdfs:comment>e.g., -, akikkel/aki, amelyekkel/amely, barátoddal/barát, botrányoddal/botrány, cselédkönyveinkkel/cselédkönyv, derekukkal/derék, egyikével/egyik, egymással/egymás (hu)</rdfs:comment>
        <rdfs:comment>e.g., 0, Аахеном/Аахен Абаєм/Абай Абаканом/Абакан Абаканом/Абакан Абіджаном/Абіджан Абовяном/Абовян Авентином/Авентин Адамстауном/Адамстаун Аденом/Аден Аджаристаном/Аджаристан Адлером/Адлер Адонісом/Адоніс Адріанополем/Адріанополь Азенкуром/Азенкур Азербайджаном/Азербайджан Азовом/Азов Акерманом/Акерман Акмолінськом/Акмолінськ Акрополем/Акрополь Актюбінськом/Актюбінськ, Або/= Абруццо/= Абу-Дабі/= Адріатичним морем/Адріатичне море Азовським морем/Азовське море Айдахо/= Ай-Петрі/= Аконкагуа/= Актау/= Алеппо/= Аліканте/= Алмати/= Альбі/= Андаманським морем/Андаманське море Анжу/= Ані/= Антананаріву/= Антигуа/= Апіа/= Апостоловим/Апостолове, Абіссінією/Абіссінія Абуджею/Абуджа Абхазією/Абхазія Авдіївкою/Авдіївка Австралією/Австралія Австрією/Австрія Австро-Угорщиною/Австро-Угорщина Аддис-Абебою/Аддис-Абеба Аджарією/Аджарія Адигеєю/Адигея Адріатикою/Адріатика Азією/Азія Айовою/Айова Аквітанією/Аквітанія Аккрою/Аккра Ак-Мечеттю/Ак-Мечеть Акмолою/Акмола акриловою кислотою/акрилова кислота Алабамою/Алабама Албанією/Албанія, Азорськими островами/Азорські острови Аландськими островами/Аландські острови Алеутськими островами/Алеутські острови Андаманськими островами/Андаманські острови Антильськими островами/Антильські острови Багамськими островами/Багамські острови Балеарськими островами/Балеарські острови Бельбеками/Бельбек Бермудськими островами/Бермудські острови Бугами/Буг Великоднями/Великдень Великими Сорочинцями/Великі Сорочинці Віргінськими островами/Віргінські острови Гавайськими островами/Гавайські острови Гебридськими островами/Гебридські острови Драконовими горами/Драконові гори ЖЕКами/ЖЕК Зеленого Мису островами/Зеленого Мису острови Змієвими валами/Змієві вали Зондськими островами/Зондські острови, Альпами/Альпи Андами/Анди Апеннінами/Апенніни Аппалачами/Аппалачі Арденнами/Арденни Афінами/Афіни Багамами/Багами Балканами/Балкани Байдарськими воротами/Байдарські ворота Барановичами/Барановичі Бендерами/Бендери Березняками/Березняки Бермудами/Бермуди Бескидами/Бескиди Біличами/Біличі Близнюками/Близнюки Богородчанами/Богородчани Боровичами/Боровичі Бортничами/Бортничі Броварами/Бровари, Америками/Америка Андалуськими горами/Андалуські гори Атласькими горами/Атлаські гори Бистрицями/Бистриця Держдумами/Держдума Жовтими Водами/Жовті Води Збройними Силами України/Збройні сили України Індіями/Індія Інтернет-газетами/Інтернет-газета Караваєвими дачами/Караваєві дачі Магеллановими хмарами/Магелланові хмари Македоніями/Македонія Мате Залка/= Пасхами/Пасха Пилипівками/Пилипівка Радами/Рада Родезіями/Родезія Інтернет-технологіями/Інтернет-технологія, Антроповим/Антропов Абаєм/Абай Абакумом/Абакум Абакумовичем/Абакумович Абалкіним/Абалкін Абашидзе/= Аббасом/Аббас Абдулою/Абдула Абдуллоджановим/Абдуллоджанов Абелем/Абель Абовяном/Абовян Абрамом/Абрам Абрамовичем/Абрамович Абрамовичем/Абрамович Абрамчуком/Абрамчук Абуладзе/= Авакумом/Авакум Авакумовичем/Авакумович Августом/Август Августимовим/Августимов, Антроповими/Антропов Абакумами/Абакум Абакумовичами/Абакумович Абалкіними/Абалкін Абашидзе/= Аббасами/Аббас Абдулами/Абдула Абдуллоджановими/Абдуллоджанов Абелями/Абель Абовянами/Абовян Абрамами/Абрам Абрамовичами/Абрамович Абрамовичами/Абрамович Абрамчуками/Абрамчук Абуладзе/= Авакумами/Авакум Авакумовичами/Авакумович Августами/Август Августимовими/Августимов Августинами/Августин (uk)</rdfs:comment>
        <rdfs:comment>e.g., Bohon/bug, Christusam/krïštuš, Dapiton/dapit, gardimi/gärd, gnimi/un, hriſsi/grih, imenom/jïmë, istriki/štrïk, judmi/jüdi (sl-rozaj)</rdfs:comment>
        <rdfs:comment>e.g., akceptowanymi/akceptować, akredytującą/akredytować, badaniem/badanie, całą/cały, czterema/cztery, czworgiem/czworo, czyimikolwiek/czyjkolwiek, czyimiś/czyjś, czyimkolwiek/czyjkolwiek (pl)</rdfs:comment>
        <rdfs:comment>e.g., bolom/bol, Bratstvom/Bratstvo, dvojim/dvoje, jednim/jedan, jednom/jedan, Jevrejkama/Jevrejka, mnom/ja, mnome/ja, najponiznijim/ponizan (sr)</rdfs:comment>
        <rdfs:comment>e.g., desaterým/desaterý, devatenáctým/devatenáctý, druhou/druhý, druhým/druhý, druhými/druhý, dvojí, dvěma/dva, jakou/jaký, jakým/jaký (cs)</rdfs:comment>
        <rdfs:comment>e.g., druhou/druhý, druhým/druhý, druhými/druhý, hentou/hentá, hentým/hento, hentými/hento, hentými/hentá, ich, jednou/jeden (sk)</rdfs:comment>
        <rdfs:comment>e.g., ВАМИ/вы, Вами/вы, Двенадцатой/двенадцатый, Двумя/два, НАМИ/мы, Нами/мы, Нечем/нечего, Ним/он, СОБОЙ/себя (ru)</rdfs:comment>
    </owl:Class>
    


    <!-- http://purl.org/olia/mte/multext-east.owl#Interjection -->

    <owl:Class rdf:about="http://purl.org/olia/mte/multext-east.owl#Interjection">
        <rdfs:subClassOf rdf:resource="http://purl.org/olia/mte/multext-east.owl#MorphosyntacticCategory"/>
        <rdfs:subClassOf>
            <owl:Restriction>
                <owl:onProperty rdf:resource="http://purl.org/olia/mte/multext-east.owl#hasInterjectionFormation"/>
                <owl:maxCardinality rdf:datatype="http://www.w3.org/2001/XMLSchema#nonNegativeInteger">1</owl:maxCardinality>
            </owl:Restriction>
        </rdfs:subClassOf>
        <rdfs:comment>e.g., Giò/ǵö, Oh/ö (sl-rozaj)</rdfs:comment>
        <rdfs:comment>e.g., ach/ach, ho/ho, och/och (pl)</rdfs:comment>
        <rdfs:comment>e.g., а ага агей агов агуш агуша агу адзусь адзуськи адіт адіть аж-аж-аж ай ай-ай-ай але алилуя алло амба ані мур-мур анічичирк (uk)</rdfs:comment>
        <rdfs:comment>e.g., مبادا راستي اوه (fa)</rdfs:comment>
    </owl:Class>
    


    <!-- http://purl.org/olia/mte/multext-east.owl#InterjectionFormation -->

    <owl:Class rdf:about="http://purl.org/olia/mte/multext-east.owl#InterjectionFormation">
        <rdfs:subClassOf rdf:resource="http://purl.org/olia/mte/multext-east.owl#Formation"/>
        <rdfs:comment>Interjection/Formation refers to the graphical components: simple, i.e. consisting of one word; compound, i.e. consisting of more than one word. (MTE v4)</rdfs:comment>
    </owl:Class>
    


    <!-- http://purl.org/olia/mte/multext-east.owl#InterrogativeAdverb -->

    <owl:Class rdf:about="http://purl.org/olia/mte/multext-east.owl#InterrogativeAdverb">
        <owl:equivalentClass>
            <owl:Class>
                <owl:intersectionOf rdf:parseType="Collection">
                    <rdf:Description rdf:about="http://purl.org/olia/mte/multext-east.owl#Adverb"/>
                    <owl:Restriction>
                        <owl:onProperty rdf:resource="http://purl.org/olia/mte/multext-east.owl#hasWHType"/>
                        <owl:hasValue rdf:resource="http://purl.org/olia/mte/multext-east.owl#Question"/>
                    </owl:Restriction>
                </owl:intersectionOf>
            </owl:Class>
        </owl:equivalentClass>
        <rdfs:subClassOf rdf:resource="http://purl.org/olia/mte/multext-east.owl#InterrogativeOrRelativeAdverb"/>
        <rdfs:comment>e.g., -e, e (hu)</rdfs:comment>
        <rdfs:comment>e.g., why, where, when (en)</rdfs:comment>
        <rdfs:comment>Adverb/Type=&quot;interrogative&quot; is used in the Hungarian MTE v4 specs. Corresponds to Adverb/Wh_Type=&quot;question&quot; in English MTE v4.</rdfs:comment>
    </owl:Class>
    


    <!-- http://purl.org/olia/mte/multext-east.owl#InterrogativeDeterminer -->

    <owl:Class rdf:about="http://purl.org/olia/mte/multext-east.owl#InterrogativeDeterminer">
        <owl:equivalentClass>
            <owl:Class>
                <owl:intersectionOf rdf:parseType="Collection">
                    <rdf:Description rdf:about="http://purl.org/olia/mte/multext-east.owl#Determiner"/>
                    <owl:Restriction>
                        <owl:onProperty rdf:resource="http://purl.org/olia/mte/multext-east.owl#hasWHType"/>
                        <owl:hasValue rdf:resource="http://purl.org/olia/mte/multext-east.owl#Question"/>
                    </owl:Restriction>
                </owl:intersectionOf>
            </owl:Class>
        </owl:equivalentClass>
        <rdfs:subClassOf rdf:resource="http://purl.org/olia/mte/multext-east.owl#InterrogativeOrRelativeDeterminer"/>
        <rdfs:comment>e.g., whose (en)</rdfs:comment>
        <rdfs:comment>e.g., چه‌مقدار چه‌جور چند (fa)</rdfs:comment>
        <rdfs:comment>Determiner/Type=&quot;interrogative&quot; (Persian MTE v4), corresponds to Determiner/Type=&quot;question&quot; in English MTE v4.</rdfs:comment>
    </owl:Class>
    


    <!-- http://purl.org/olia/mte/multext-east.owl#InterrogativeOrRelativeAdverb -->

    <owl:Class rdf:about="http://purl.org/olia/mte/multext-east.owl#InterrogativeOrRelativeAdverb">
        <rdfs:subClassOf rdf:resource="http://purl.org/olia/mte/multext-east.owl#Adverb"/>
        <rdfs:comment>e.g., cân&apos;/când (ro)</rdfs:comment>
        <rdfs:comment>Adverb/Type=&quot;int-rel&quot; for Romanian applies to interrogative and relative adverbs that are not formally distinguished in Romanian. (MTE v4)
Corresponds to the presence of Adverb/Wh_Type in English MTE v4.</rdfs:comment>
    </owl:Class>
    


    <!-- http://purl.org/olia/mte/multext-east.owl#InterrogativeOrRelativeDeterminer -->

    <owl:Class rdf:about="http://purl.org/olia/mte/multext-east.owl#InterrogativeOrRelativeDeterminer">
        <rdfs:subClassOf rdf:resource="http://purl.org/olia/mte/multext-east.owl#Determiner"/>
        <rdfs:comment>e.g., care, ce, cât, câta/câtelea, câte/cât, câtelea, câtor/cât, câtă/cât, câţi/cât (ro)</rdfs:comment>
        <rdfs:comment>Determiner/Type=&quot;int-rel&quot; (Romanian MTE v4), corresponds to the presence of Determiner/Wh_Type in English MTE v4.</rdfs:comment>
    </owl:Class>
    


    <!-- http://purl.org/olia/mte/multext-east.owl#InterrogativeOrRelativePronoun -->

    <owl:Class rdf:about="http://purl.org/olia/mte/multext-east.owl#InterrogativeOrRelativePronoun">
        <rdfs:subClassOf rdf:resource="http://purl.org/olia/mte/multext-east.owl#Pronoun"/>
        <rdfs:comment>e.g., cui/cine, cât, câta/câtelea, câte/cât, câtelea, câtor/cât, câtă/cât, câţi/cât, cărei/care (ro)</rdfs:comment>
        <rdfs:comment>Pronoun/Type=&quot;int-rel&quot; (Romanian), corresponds to the presence of Pronoun/Wh_Type in English (MTE v4).</rdfs:comment>
    </owl:Class>
    


    <!-- http://purl.org/olia/mte/multext-east.owl#InterrogativeParticle -->

    <owl:Class rdf:about="http://purl.org/olia/mte/multext-east.owl#InterrogativeParticle">
        <rdfs:subClassOf rdf:resource="http://purl.org/olia/mte/multext-east.owl#Particle"/>
        <rdfs:comment>e.g., дали, ли, нима (bg)</rdfs:comment>
        <rdfs:comment>Particle/Type=&quot;interrogative&quot; (Croatian, Serbian, Bulgarian). 

In Bulgarian, this category is applied to particles used to form yes/no-questions or exclamations (ли, дали, нали,
нима, мигар) (Dimitrova et al. 2009)</rdfs:comment>
    </owl:Class>
    


    <!-- http://purl.org/olia/mte/multext-east.owl#InterrogativePronoun -->

    <owl:Class rdf:about="http://purl.org/olia/mte/multext-east.owl#InterrogativePronoun">
        <owl:equivalentClass>
            <owl:Class>
                <owl:intersectionOf rdf:parseType="Collection">
                    <rdf:Description rdf:about="http://purl.org/olia/mte/multext-east.owl#Pronoun"/>
                    <owl:Restriction>
                        <owl:onProperty rdf:resource="http://purl.org/olia/mte/multext-east.owl#hasWHType"/>
                        <owl:hasValue rdf:resource="http://purl.org/olia/mte/multext-east.owl#Question"/>
                    </owl:Restriction>
                </owl:intersectionOf>
            </owl:Class>
        </owl:equivalentClass>
        <rdfs:subClassOf rdf:resource="http://purl.org/olia/mte/multext-east.owl#InterrogativeOrRelativePronoun"/>
        <rdfs:comment>e.g., , kaki/kak, kakšna/kakšen, kakšni/kakšen, katere/kateri, katerih/kateri, katerim/kateri, katerimi/kateri (sl)</rdfs:comment>
        <rdfs:comment>e.g., -, hányad/hány, hányaddal/hány, hánykor/hány, kihez/ki, kiket/ki, kikkel/ki, kimért/ki, kinek/ki (hu)</rdfs:comment>
        <rdfs:comment>e.g., chira/kiri, chire/kiri, Chiri/kiri, chirj/kiri, coga/du, Coj/koj, Du/du, Kaki/kak, ko/koj (sl-rozaj)</rdfs:comment>
        <rdfs:comment>e.g., co/co, czego/co, czemu/co, czym/co, dlaczego/dlaczego, dlaczegóż/dlaczegóż, gdzie/gdzie, jacy/jaki, jaka/jaki (pl)</rdfs:comment>
        <rdfs:comment>e.g., jakou/jaký, jaká/jaký, jaké/jaký, jakého/jaký, jakém/jaký, jakému/jaký, jaký, jakých/jaký, jakým/jaký (cs)</rdfs:comment>
        <rdfs:comment>e.g., kelledega/kes, kellega/kes, kelleks/kes, kellele/kes, kellelt/kes, kellena/kes, kellesse/kes, kelleta/kes, kumba/kumb (et)</rdfs:comment>
        <rdfs:comment>e.g., koho/kto, kom/kto, komu/kto, koľkonásobnej/koľkonásobný, koľkonásobného/koľkonásobný, koľkonásobnému/koľkonásobný, koľkorakej/koľkoraký, koľkorakého/koľkoraký, koľkorakému/koľkoraký (sk)</rdfs:comment>
        <rdfs:comment>e.g., koja/koji, koje/koji, koliko/kolik (sr)</rdfs:comment>
        <rdfs:comment>e.g., who, whoever (en)</rdfs:comment>
        <rdfs:comment>e.g., де/= доки/= звідки/= звідкіля/= коли/= куди/= наскільки/= чому/= як/=, ким/хто, кого/хто, кому/хто, кому/хто кім/хто, котра/котрий котрая/котрий яка/який якая/який, котре/котрий котреє/котрий яке/який якеє/який, котрий/= який/=, котрим/котрий яким/який (uk)</rdfs:comment>
        <rdfs:comment>e.g., каква/какъв, какви/какъв, какво/какъв, какъв, кво, кого/кой, кое/кой, кои/кой, кой (bg)</rdfs:comment>
        <rdfs:comment>e.g., кого/кој, кое/кој, кои/кој, кому/кој, кој, која/кој, чие/чиј, чии/чиј, чиј (mk)</rdfs:comment>
        <rdfs:comment>e.g., کدام‌يک چيکار چه‌طور (fa)</rdfs:comment>
        <rdfs:comment>Pronoun/Wh_Type=&quot;question&quot; (English MTE v4), Pronoun/Type=&quot;interrogative&quot; (other languages).</rdfs:comment>
    </owl:Class>
    


    <!-- http://purl.org/olia/mte/multext-east.owl#InterrogativeQuantifier -->

    <owl:Class rdf:about="http://purl.org/olia/mte/multext-east.owl#InterrogativeQuantifier">
        <owl:equivalentClass>
            <owl:Class>
                <owl:intersectionOf rdf:parseType="Collection">
                    <rdf:Description rdf:about="http://purl.org/olia/mte/multext-east.owl#ProQuantifier"/>
                    <owl:Restriction>
                        <owl:onProperty rdf:resource="http://purl.org/olia/mte/multext-east.owl#hasWHType"/>
                        <owl:hasValue rdf:resource="http://purl.org/olia/mte/multext-east.owl#Question"/>
                    </owl:Restriction>
                </owl:intersectionOf>
            </owl:Class>
        </owl:equivalentClass>
        <rdfs:subClassOf rdf:resource="http://purl.org/olia/mte/multext-east.owl#ProQuantifier"/>
        <owl:versionInfo>In the Czech and Slovak MTE v4 pecs, Numeral/Class=&quot;interrogative&quot; are items meaning `how many/much&apos;, etc. Strictly speaking, they are pronumerals (pro-quantifiers), but traditional descriptions don&apos;t recognise such a category, so they are described variously as pronouns or as numerals (because their syntactic distribution is that of numerals, or very close).&quot; (Ivan A Derzhanski, email 2010/06/11)</owl:versionInfo>
    </owl:Class>
    


    <!-- http://purl.org/olia/mte/multext-east.owl#Intransitive -->

    <owl:Class rdf:about="http://purl.org/olia/mte/multext-east.owl#Intransitive">
        <rdfs:subClassOf rdf:resource="http://purl.org/olia/mte/multext-east.owl#Transitivity"/>
        <rdfs:comment>e.g., آمديد/آمد, آمديم/آمد, باشه/باش باشد/باش آيد/آ, بخواب/خواب بايست/ايست باش, برآورد انداخت انجاميد, بريم/رو برويم/رو باشيم/باش, بمانند/مان بردارند/بردار باشند/باش, بمانيد/مان بجنبيد/جنب بايستيد/ايست, بوديد/بود (fa)</rdfs:comment>
        <rdfs:comment>Transitive=&quot;no&quot; (Persian)</rdfs:comment>
    </owl:Class>
    


    <!-- http://purl.org/olia/mte/multext-east.owl#LetterNumeral -->

    <owl:Class rdf:about="http://purl.org/olia/mte/multext-east.owl#LetterNumeral">
        <rdfs:subClassOf rdf:resource="http://purl.org/olia/mte/multext-east.owl#OrthographicalRepresentationOfNumeral"/>
        <rdfs:comment>e.g., , drug/=, druga/drug, druge/drug, drugega/drug, drugem/drug, drugemu/drug, drugi/drug, drugih/drug (sl)</rdfs:comment>
        <rdfs:comment>e.g., -, egyedei/egyed, egyem/egy, egyenként/egy, egynegyedét/egynegyed, egytizedének/egytized, egytizedére/egytized, egyén/egy, egyének/egy (hu)</rdfs:comment>
        <rdfs:comment>e.g., -ntâi/întâi, -ntâia/întâi, -ntâiaşi/întâi, -ntâii/întâi, -ntâile/întâi, -ntâilor/întâi, -ntâiul/întâi, -ntâiului/întâi, dintâi (ro)</rdfs:comment>
        <rdfs:comment>e.g., czterdziestych/czterdziesty, czterdziestym/czterdziesty, czterech/cztery, czterem/cztery, czterema/cztery, czternaste/czternasty, czternastym/czternasty, cztery/cztery, czwarte/czwarty (pl)</rdfs:comment>
        <rdfs:comment>e.g., dan/dän, dna/dän, dnej/dän, dnohà/dän, dnó/dän, dua/dwa, dvi/dwa, noga/dän, nò/dän (sl-rozaj)</rdfs:comment>
        <rdfs:comment>e.g., desaterý, desaterým/desaterý, desátá/desátý, devatenácté/devatenáctý, devatenáctému/devatenáctý, devatenáctým/devatenáctý, druhej/druhý, druhou/druhý, druhá/druhý (cs)</rdfs:comment>
        <rdfs:comment>e.g., druhej/druhý, druhom/druhý, druhou/druhý, druhá/druhý, druhé/druhý, druhého/druhý, druhému/druhý, druhí/druhý, druhú/druhý (sk)</rdfs:comment>
        <rdfs:comment>e.g., dva, dvadesetora/dvadesetoro, dve/dva, dvoja/dvoje, dvoje, dvoji/dvoje, dvojih/dvoje, dvojim/dvoje, hiljade/hiljada (sr)</rdfs:comment>
        <rdfs:comment>e.g., esimesse/esimene, esimesteks/esimene, esimestele/esimene, esimestena/esimene, esimestes/esimene, esimestest/esimene, kümneteks/kümme, miljonendani/miljones, miljonitesse/miljon (et)</rdfs:comment>
        <rdfs:comment>e.g., багато/= вісім/= вісімдесят/= вісімнадцять/= вісімсот/= восьмеро/= двадцятеро/= двадцять/= дванадцятеро/= дванадцять/= двійко/= двісті/= двоє/= двоєчко/= двойко/= дев&apos;яносто/= дев&apos;ятдесят/= дев&apos;ятеро/= дев&apos;ятнадцятеро/= дев&apos;ятнадцять/=, багато/= вісім/= вісімдесят/= вісімнадцять/= вісімсот/= восьмеро/= двох/два двадцятеро/= двадцять/= дванадцятеро/= дванадцять/= двійко/= двісті/= двоє/= двоєчко/= двойко/= дев&apos;яносто/= дев&apos;ятдесят/= дев&apos;ятеро/= дев&apos;ятнадцятеро/=, багатьма/багато вісьма/вісім вісьмома/вісім вісімдесятьма/вісімдесят вісімдесятьома/вісімдесят вісімнадцятьма/вісімнадцять вісімнадцятьома/вісімнадцять восьмистами/вісімсот вісьмома/восьмеро двома/два двома/два двадцятьма/двадцятеро двадцятьома/двадцятеро двадцятьма/двадцять двадцятьома/двадцять дванадцятьма/дванадцятеро дванадцятьома/дванадцятеро дванадцятьма/дванадцять дванадцятьома/дванадцять двійко/=, багатьом/багато восьми/вісім вісьмом/вісім вісімдесяти/вісімдесят вісімдесятьом/вісімдесят вісімнадцяти/вісімнадцять вісімнадцятьом/вісімнадцять восьмистам/вісімсот вісьмом/восьмеро двом/два двом/два двадцятьом/двадцятеро двадцяти/двадцять двадцятьом/двадцять дванадцятьом/дванадцятеро дванадцяти/дванадцять дванадцятьом/дванадцять двійко/= двомстам/двісті двом/двоє, багатьох/багато восьми/вісім вісьмох/вісім вісімдесяти/вісімдесят вісімдесятьох/вісімдесят вісімнадцяти/вісімнадцять вісімнадцятьох/вісімнадцять восьмисот/вісімсот вісьмох/восьмеро двох/два двох/два двадцятьох/двадцятеро двадцяти/двадцять двадцятьох/двадцять дванадцятьох/дванадцятеро дванадцяти/дванадцять дванадцятьох/дванадцять двійко/= двохсот/двісті двох/двоє, багатьох/багато восьми/вісім вісьмох/вісім вісімдесяти/вісімдесят вісімдесятьох/вісімдесят вісімнадцяти/вісімнадцять вісімнадцятьох/вісімнадцять восьмистах/вісімсот вісьмох/восьмеро двох/два двох/два двадцятьох/двадцятеро двадцяти/двадцять двадцятьох/двадцять дванадцятьох/дванадцятеро дванадцяти/дванадцять дванадцятьох/дванадцять двійко/= двохстах/двісті двох/двоє, багатьох/багато вісьмох/вісім вісімдесятьох/вісімдесят вісімнадцятьох/вісімнадцять вісьмох/восьмеро двох/два двадцятьох/двадцятеро двадцятьох/двадцять дванадцятьох/дванадцятеро дванадцятьох/дванадцять двох/двоє дев&apos;ятдесятьох/дев&apos;ятдесят дев&apos;ятьох/дев&apos;ятеро дев&apos;ятнадцятьох/дев&apos;ятнадцятеро дев&apos;ятнадцятьох/дев&apos;ятнадцять дев&apos;ятьох/дев&apos;ять декількох/декілька декількох/декілько десятьох/десятеро десятьох/десять, вісімдесята/вісімдесятий вісімнадцята/вісімнадцятий восьма/восьмий двадцята/двадцятий дванадцята/дванадцятий двохсота/двохсотий дев&apos;яноста/дев&apos;яностий дев&apos;ята/дев&apos;ятий дев&apos;ятисота/дев&apos;ятисотий дев&apos;ятнадцята/дев&apos;ятнадцятий десята/десятий друга/другий одинадцята/одинадцятий перша/перший п&apos;ятдесята/п&apos;ятдесятий п&apos;ята/п&apos;ятий п&apos;ятисота/п&apos;ятисотий п&apos;ятитисячна/п&apos;ятитисячний п&apos;ятнадцята/п&apos;ятнадцятий семисота/семисотий, вісімдесяте/вісімдесятий вісімнадцяте/вісімнадцятий восьме/восьмий двадцяте/двадцятий дванадцяте/дванадцятий двохсоте/двохсотий дев&apos;яносте/дев&apos;яностий дев&apos;яте/дев&apos;ятий дев&apos;ятисоте/дев&apos;ятисотий дев&apos;ятнадцяте/дев&apos;ятнадцятий десяте/десятий друге/другий одинадцяте/одинадцятий перше/перший п&apos;ятдесяте/п&apos;ятдесятий п&apos;яте/п&apos;ятий п&apos;ятисоте/п&apos;ятисотий п&apos;ятитисячне/п&apos;ятитисячний п&apos;ятнадцяте/п&apos;ятнадцятий семисоте/семисотий (uk)</rdfs:comment>
        <rdfs:comment>e.g., два, двава/два, двана/два, двата/два, две/два, двеве/два, двене/два, двете/два, еден (mk)</rdfs:comment>
        <rdfs:comment>e.g., два, двайсетия/двайсет, двата/два, две, две-три, двете/две, десетия/десет, единият/един, едно (bg)</rdfs:comment>
        <rdfs:comment>Form=&quot;letter&quot;</rdfs:comment>
    </owl:Class>
    


    <!-- http://purl.org/olia/mte/multext-east.owl#LightVerb -->

    <owl:Class rdf:about="http://purl.org/olia/mte/multext-east.owl#LightVerb">
        <rdfs:subClassOf rdf:resource="http://purl.org/olia/mte/multext-east.owl#Verb"/>
        <rdfs:comment>In linguistics, a light verb is a verb participating in complex predication that has little semantic content of its own, but provides through inflection some details on the event semantics, such as aspect, mood, or tense. The semantics of the compound, as well as its argument structure, are determined by the head or primary component of the compound, which may be a verb or noun (V+V or V+N compounds). Other names for &quot;light verb&quot; include: vector verb or explicator verb, emphasising its role within the compound; or thin verb or semantically weak verb, emphasising (as with &quot;light&quot;) its lack of semantics. A &quot;semantically weak&quot; verb is not to be confused with a &quot;weak verb&quot; as in the Germanic weak inflection. Light verbs are similar to auxiliary verbs in some ways.
            
            Most English light verbs occur in V+N forms sometimes called &quot;stretched verbs&quot;: for example, take in take a nap, where the primary sense is provided by &quot;nap&quot;, and &quot;take&quot; is the light verb. The light verbs most common in these constructions are also common in phrasal verbs. A verb which is &quot;light&quot; in one context may be &quot;heavy&quot; in another: as with &quot;take&quot; in I will take a book to read.
            
            Examples in other languages include the Yiddish geb in geb a helf (literally give a help, &quot;help&quot;); the French faire in faire semblant (lit. make seeming, &quot;pretend&quot;); the Hindi nikal paRA (lit. leave fall, &quot;start to leave&quot;); and the bǎ construction in Chinese.[1] Some verbs are found in many such expressions; to reuse an earlier example, take is found in take a nap, take a shower, take a sip, take a bow, take turns, and so on. Light verbs are extremely common in Indo-Iranian languages, Japanese, and other languages in which verb compounding is a primary mechanism for marking aspectual distinctions.
            (http://en.wikipedia.org/wiki/Light_verb)</rdfs:comment>
        <rdfs:comment>e.g., برآورد انداخت انجاميد, بمانند/مان بردارند/بردار باشند/باش, بوديد/بود, بياورند/آور بخورند/خور آورند/آور, بيندازم/انداز بدم/ده بخشد/بخش, بيندازيم/انداز بدهيم/ده ببريم/بر, داده‌/داد برده/برده انداخته/انداخت, دادي/داد خوردي/خورد بودي/بود, داديد/داد (fa)</rdfs:comment>
        <rdfs:comment>Verb/Type=&quot;light&quot; (Persian)

Light verbs in Farsi are used to make a compound verb structure. Compound verb structure consists of one or more preverbal elements which could be a noun, adjective, or a prepositional phrase, followed by a Light verb. The number of Light verbs is limited. The elements of a compound verb construction can be separated by other lexical elements such as the object of the verbal construction or an adjective, adverb, etc. Therefore our suggestion is to analyze compound verb construction only at the syntactic level. We should also note that Light verbs are homographic with Main verbs. (Qasemizadeh and Rahimi 2006)</rdfs:comment>
    </owl:Class>
    


    <!-- http://purl.org/olia/mte/multext-east.owl#LocativeCase -->

    <owl:Class rdf:about="http://purl.org/olia/mte/multext-east.owl#LocativeCase">
        <rdfs:subClassOf rdf:resource="http://purl.org/olia/mte/multext-east.owl#Case"/>
        <rdfs:comment>e.g., , drugem/drug, drugi/drug, drugih/drug, dveh/dva, dvojnem/dvojen, enem/en, enih/en, katerih/kateri (sl)</rdfs:comment>
        <rdfs:comment>e.g., 0, Аахені/Аахен Аахену/Аахен Абаї/Абай Абаю/Абай Абакані/Абакан Абакану/Абакан Абакані/Абакан Абакану/Абакан Абіджані/Абіджан Абіджану/Абіджан Абовяні/Абовян Абовяну/Абовян Авентині/Авентин Авентину/Авентин Адамстауні/Адамстаун Адамстауну/Адамстаун Адені/Аден Адену/Аден Аджаристані/Аджаристан Аджаристану/Аджаристан, Або/= Абруццо/= Абу-Дабі/= Адріатичному морі/Адріатичне море Адріатичнім морі/Адріатичне море Адріатичному морю/Адріатичне море Адріатичнім морю/Адріатичне море Азовському морі/Азовське море Азовськім морі/Азовське море Азовському морю/Азовське море Азовськім морю/Азовське море Айдахо/= Ай-Петрі/= Аконкагуа/= Актау/= Алеппо/= Аліканте/= Алмати/= Альбі/= Андаманському морі/Андаманське море, Абіссінії/Абіссінія Абуджі/Абуджа Абхазії/Абхазія Авдіївці/Авдіївка Австралії/Австралія Австрії/Австрія Австро-Угорщині/Австро-Угорщина Аддис-Абебі/Аддис-Абеба Аджарії/Аджарія Адигеї/Адигея Адріатиці/Адріатика Азії/Азія Айові/Айова Аквітанії/Аквітанія Аккрі/Аккра Ак-Мечеті/Ак-Мечеть Акмолі/Акмола акриловій кислоті/акрилова кислота Алабамі/Алабама Албанії/Албанія, Азорських островах/Азорські острови Аландських островах/Аландські острови Алеутських островах/Алеутські острови Андаманських островах/Андаманські острови Антильських островах/Антильські острови Багамських островах/Багамські острови Балеарських островах/Балеарські острови Бельбеках/Бельбек Бермудських островах/Бермудські острови Бугах/Буг Великоднях/Великдень Великих Сорочинцях/Великі Сорочинці Віргінських островах/Віргінські острови Гавайських островах/Гавайські острови Гебридських островах/Гебридські острови Драконових горах/Драконові гори ЖЕКах/ЖЕК Зеленого Мису островах/Зеленого Мису острови Змієвих валах/Змієві вали Зондських островах/Зондські острови, Альпах/Альпи Андах/Анди Апеннінах/Апенніни Аппалачах/Аппалачі Арденнах/Арденни Афінах/Афіни Багамах/Багами Балканах/Балкани Байдарських воротах/Байдарські ворота Барановичах/Барановичі Бендерах/Бендери Березняках/Березняки Бермудах/Бермуди Бескидах/Бескиди Біличах/Біличі Близнюках/Близнюки Богородчанах/Богородчани Боровичах/Боровичі Бортничах/Бортничі Броварах/Бровари, Америках/Америка Андалуських горах/Андалуські гори Атлаських горах/Атлаські гори Бистрицях/Бистриця Держдумах/Держдума Жовтих Водах/Жовті Води Збройних Силах України/Збройні сили України Індіях/Індія Інтернет-газетах/Інтернет-газета Караваєвих дачах/Караваєві дачі Магелланових хмарах/Магелланові хмари Македоніях/Македонія Мате Залка/= Пасхах/Пасха Пилипівках/Пилипівка Радах/Рада Родезіях/Родезія Інтернет-технологіях/Інтернет-технологія, Антропових/Антропов Абакумах/Абакум Абакумовичах/Абакумович Абалкіних/Абалкін Абашидзе/= Аббасах/Аббас Абдулах/Абдула Абдуллоджанових/Абдуллоджанов Абелях/Абель Абовянах/Абовян Абрамах/Абрам Абрамовичах/Абрамович Абрамовичах/Абрамович Абрамчуках/Абрамчук Абуладзе/= Авакумах/Авакум Авакумовичах/Авакумович Августах/Август Августимових/Августимов Августинах/Августин, Антропових/Антропов Абакумівнах/Абакумівна Абалкіних/Абалкін Абашидзе/= Абдуллоджанових/Абдуллоджанов Абрамівнах/Абрамівна Абуладзе/= Авакумівнах/Авакумівна Августах/Августа Августимових/Августимов Августинівнах/Августинівна Авдієвських/Авдієвський Авенірівнах/Авенірівна Аверіних/Аверін Аверкіївнах/Аверкіївна Авер&apos;янівнах/Авер&apos;янівна Авіятах/Авіята Авксентіївнах/Авксентіївна Авогадро/= Аврамівнах/Аврамівна (uk)</rdfs:comment>
        <rdfs:comment>e.g., VX/vx, Вас/вы, Женечке/женечка, НЕЙ/она, НИХ/они, Ней/она, Нем/оно, Нём/он, Саше/саша (ru)</rdfs:comment>
        <rdfs:comment>e.g., analizowanych/analizować, bieżącym/bieżeć, bieżącym/bieżący, całej/cały, całym/cały, czterdziestym/czterdziesty, czternastym/czternasty, czwartych/czwarty, czwartym/czwarty (pl)</rdfs:comment>
        <rdfs:comment>e.g., belim/beo, Bratstvu/Bratstvo, dvojim/dvoje, Hajd, jednoj/jedan, jednom/jedan, jednome/jedan, jednomu/jedan, Jevrejkama/Jevrejka (sr)</rdfs:comment>
        <rdfs:comment>e.g., besideh/bisida, Bohavei/böguw, Bohovih/böguw, Bohovij/böguw, Bohovin/böguw, Bohuvin/böguw, chirj/kiri, Chrishtianschin/krištijanski, Comandatmiteh/komandament (sl-rozaj)</rdfs:comment>
        <rdfs:comment>e.g., devatenácté/devatenáctý, druhé/druhý, druhém/druhý, druhých/druhý, dvacátých/dvacátý, dvojí, dvou/dva, jaké/jaký, jakém/jaký (cs)</rdfs:comment>
        <rdfs:comment>e.g., druhej/druhý, druhom/druhý, druhých/druhý, dvoch/dva, hentej/hentá, hentom/hento, hentých/hento, hentých/hentá, ich (sk)</rdfs:comment>
    </owl:Class>
    


    <!-- http://purl.org/olia/mte/multext-east.owl#MFormNumeral -->

    <owl:Class rdf:about="http://purl.org/olia/mte/multext-east.owl#MFormNumeral">
        <rdfs:subClassOf rdf:resource="http://purl.org/olia/mte/multext-east.owl#MorphologicalFormOfNumeral"/>
        <rdfs:subClassOf>
            <owl:Class>
                <owl:intersectionOf rdf:parseType="Collection">
                    <rdf:Description rdf:about="http://purl.org/olia/mte/multext-east.owl#Animate"/>
                    <rdf:Description rdf:about="http://purl.org/olia/mte/multext-east.owl#CardinalNumeral"/>
                    <rdf:Description rdf:about="http://purl.org/olia/mte/multext-east.owl#MasculineGender"/>
                </owl:intersectionOf>
            </owl:Class>
        </rdfs:subClassOf>
        <rdfs:subClassOf>
            <owl:Class>
                <owl:intersectionOf rdf:parseType="Collection">
                    <owl:Restriction>
                        <owl:onProperty rdf:resource="http://purl.org/olia/mte/multext-east.owl#hasGender"/>
                        <owl:someValuesFrom rdf:resource="http://purl.org/olia/mte/multext-east.owl#MFormNumeral"/>
                    </owl:Restriction>
                    <owl:Restriction>
                        <owl:onProperty rdf:resource="http://purl.org/olia/mte/multext-east.owl#hasNumber"/>
                        <owl:someValuesFrom rdf:resource="http://purl.org/olia/mte/multext-east.owl#MFormNumeral"/>
                    </owl:Restriction>
                </owl:intersectionOf>
            </owl:Class>
        </rdfs:subClassOf>
        <rdfs:comment>The Bulgarian MTE v4 specs have an additional subtype of Numeral, Numeral/Form=m_form.
This signifies a special form of cardinal numbers for persons of masculine gender for `two&apos;, `three&apos;, `four&apos;, `five&apos; and `six&apos;, formed with suffix -(и)ма: двама, трима, петима /two(people), three(people), five(people)/ 
(Dimitrova et al. 2009; Earl 2000, p. 153). They go beyond six, though the higher the number, the less natural they sound.  `Seven Brides for Seven Brothers&apos; is _Sedem nevesti za sedmina bratja_, always.  Otoh, _The Seven Samurai_ is _Sedemte samurai_, not _Sedminata samurai_.  It&apos;s a stylistic choice. (Ivan A Derzhanski, email 2010/06/20)&lt;br/&gt;

Lily Earl (2000), A comprehensive Bulgarian grammar for foreign learners, Daniela Ubenova, Sofia</rdfs:comment>
        <owl:versionInfo>We have not yet found a language-independent label for the Bulgarian m-form:
The usage of the m-form is similar to Russian collective numbers, but CollectiveNumeral would be a misnomer, because there&apos;s nothing collective about the m-form: `collective&apos; suggests that the so-and-so many entities are viewed as a unit, and the preference for this form in various languages for counting pluralia tantum, human beings etc. is secondary; the m-forms are just masculine human (and are never applied for pluralia tantum, for example).  But the similarity is there, so it wouldn&apos;t be a very incorrect thing to do.  Also there are synonymous numerals in _-ica_ and _-mina_, which are collective historically (though not synchronically).
In particular, there is no relationship to Romanian Numeral/Type=&quot;collect&quot; (CollectiveNumeral). That type covers items meaning `both&apos;, `all three&apos; etc.  (In Slovene _oba_ `both&apos; is treated as a pronoun, not a numeral.)
(Ivan A Derzhanski, email 2010/06/20; cf. http://masterrussian.com/numbers/collective_numbers.php on collective numbers in Russian)&lt;br/&gt;

Assigned hasGender(masculine) and hasAnimacy(animate).</owl:versionInfo>
    </owl:Class>
    


    <!-- http://purl.org/olia/mte/multext-east.owl#MainVerb -->

    <owl:Class rdf:about="http://purl.org/olia/mte/multext-east.owl#MainVerb">
        <rdfs:subClassOf rdf:resource="http://purl.org/olia/mte/multext-east.owl#Verb"/>
        <rdfs:comment>e.g., -nzestrarăm/înzestra, -nzestrarăţi/înzestra, -nzestrasem/înzestra, -nzestraseră/înzestra, -nzestraserăm/înzestra, -nzestraserăţi/înzestra, -nzestraseşi/înzestra, -nzestraţi/înzestra, -nzestreze/înzestra (ro)</rdfs:comment>
        <rdfs:comment>e.g., amaite/amät, bit/bet, contemplaimo/kontemplät, datte/dät, Dáite/dät, gauo/tet, gauò/tet, hardéhata/tet, hardéše/tet (sl-rozaj)</rdfs:comment>
        <rdfs:comment>e.g., biste/biti, okrete/okrenuti, stajala/stajati, zastrasmo/zastrijeti, zastraste/zastrijeti, zaustavila/zaustaviti, zveknućete/zveknuti, žmuraste/žmuriti, žmurićete/žmuriti (sr)</rdfs:comment>
        <rdfs:comment>e.g., daren&apos;t/dare+not, wasn&apos;t/be+not, weren&apos;t/be+not (en)</rdfs:comment>
        <rdfs:comment>e.g., dostaliście/dostać, dostałyśmy/dostać, dotyczyły/dotyczyć, jest/być, jesteś/być, jesteście/być, jesteśmy/być, nastąpił/nastąpić, otrzymali/otrzymać (pl)</rdfs:comment>
        <rdfs:comment>e.g., elárultalak/elárul, figyelmeztettelek/figyelmeztet, lennétek/lesz, megismertelek/megismer, továbbtaníttatnátok/továbbtaníttat, tudnálak/tud, tudnátok/tud, uralhatjátok/uralhat, veszélyeztetné/veszélyeztet (hu)</rdfs:comment>
        <rdfs:comment>e.g., hodita/hoditi, hoče/hoteti, hočejo/hoteti, hočem/hoteti, hočeta/hoteti, hočeva/hoteti, imata/imeti, imate/imeti, nimata/imeti (sl)</rdfs:comment>
        <rdfs:comment>e.g., nepostačia/nestačiť, nepostačí/nestačiť, nepostačím/nestačiť, nepostačíme/nestačiť, nepostačíte/nestačiť, nepostačíš/nestačiť, nepovlečiete/nevliecť, nepožalujete/nežalovať, nepoženiete/nehnať (sk)</rdfs:comment>
        <rdfs:comment>e.g., nestráveno/strávit, nevzpamatuješ/vzpamatovat, nezneužívat/zneužívat, neztratit/ztratit, nezúčastnit/zúčastnit, půjdete/jít (cs)</rdfs:comment>
        <rdfs:comment>e.g., ulatuvat/ulama, volitatuks/volitama, vormistatakse/vormistama, vormitud/vormima, vormituks/vormima, vulkaniseeritud/vulkaniseerima, vundamentides/vundamentima, võisteldakse/võistlema, võrdsustatuks/võrdsustama (et)</rdfs:comment>
        <rdfs:comment>Type=&quot;main&quot;&lt;br/&gt;

Depending to tagging strategy (see AuxiliaryVerb), MainVerb refers to lexical verbs that have neither auxiliary, nor modal, nor copular function, or it refers to verbs other than &quot;to be&quot;, &quot;to have&quot;, etc.</rdfs:comment>
    </owl:Class>
    


    <!-- http://purl.org/olia/mte/multext-east.owl#MasculineGender -->

    <owl:Class rdf:about="http://purl.org/olia/mte/multext-east.owl#MasculineGender">
        <rdfs:subClassOf rdf:resource="http://purl.org/olia/mte/multext-east.owl#Gender"/>
        <rdfs:comment>e.g., -atât/atât, -istul, -istului, -iştii, -iştilor, -mpărate/împărat, -nsutitului/însutit, -nsutiţilor/însutit, -ntreitului/întreit (ro)</rdfs:comment>
        <rdfs:comment>e.g., Hrvatoma/Hrvat, katerih/kateri, katerim/kateri, katerimi/kateri, pilatusema/pilatus, tistih/tisti, treh/trije, trem/trije, tremi/trije (sl)</rdfs:comment>
        <rdfs:comment>e.g., absolwentów/absolwent, autora/autor, autorzy/autor, bogatszych/bogaty, ci/ten, czterdziestym/czterdziesty, czterem/cztery, czterema/cztery, czternaste/czternasty (pl)</rdfs:comment>
        <rdfs:comment>e.g., bit/bet, Christusa/krïštuš, Christusam/krïštuš, Comandatmiteh/komandament, Crishtusha/krïštuš, Dapiton/dapit, dialëte/dijalët, etej/iti, istriki/štrïk (sl-rozaj)</rdfs:comment>
        <rdfs:comment>e.g., desaterý, desaterým/desaterý, devatenácté/devatenáctý, devatenáctému/devatenáctý, devatenáctým/devatenáctý, dostal/dostat, dostali/dostat, dostaly/dostat, dvacátých/dvacátý (cs)</rdfs:comment>
        <rdfs:comment>e.g., devetogodišnji, Goldštajnov, hteo/hteti, htio/htjeti, Ketrin, najjednostavniji/jednostavan, najsitnijih/sitan, neupotrebljena/neupotrebljen, neustrašivi/neustrašiv (sr)</rdfs:comment>
        <rdfs:comment>e.g., henten, hentie/henten, hentoho/henten, hentí/henten, hentých/henten, najžulovitejšie/žulovitý, najžulovitejšieho/žulovitý, najžulovitejšiemu/žulovitý, najžulovitejšom/žulovitý (sk)</rdfs:comment>
        <rdfs:comment>e.g., viscounts/viscount, welterweights/welterweight (en)</rdfs:comment>
    </owl:Class>
    


    <!-- http://purl.org/olia/mte/multext-east.owl#MedialVoice -->

    <owl:Class rdf:about="http://purl.org/olia/mte/multext-east.owl#MedialVoice">
        <rdfs:subClassOf rdf:resource="http://purl.org/olia/mte/multext-east.owl#Voice"/>
        <rdfs:comment>Voice=&quot;medial&quot; (Russian), e.g., спившийся/спиться, создавшихся/создаться, случившихся/случиться</rdfs:comment>
    </owl:Class>
    


    <!-- http://purl.org/olia/mte/multext-east.owl#ModalParticle -->

    <owl:Class rdf:about="http://purl.org/olia/mte/multext-east.owl#ModalParticle">
        <rdfs:subClassOf rdf:resource="http://purl.org/olia/mte/multext-east.owl#Particle"/>
        <rdfs:comment>Particle/Type=&quot;modal&quot; (Croatian, Serbian, Bulgarian).

In the Bulgarian MTE, Type=modal refers to particles that express urge or order, mostly homonymous with other types of particles, for instance да, дано, нека, хайде. (Dimitrova et al. 2009)</rdfs:comment>
    </owl:Class>
    


    <!-- http://purl.org/olia/mte/multext-east.owl#ModalVerb -->

    <owl:Class rdf:about="http://purl.org/olia/mte/multext-east.owl#ModalVerb">
        <rdfs:subClassOf rdf:resource="http://purl.org/olia/mte/multext-east.owl#Verb"/>
        <rdfs:comment>e.g., Ciete/tët, cion/tët, morata/bet, moret/morët, morete/morët, tel/tët, tese/tët, teu/tët, téshe/tët (sl-rozaj)</rdfs:comment>
        <rdfs:comment>e.g., chceme/chtít, chcete/chtít, chceš/chtít, chtěj/chtít, dejte/dát, můžete/moci, nechceš/chtít, nechtělo/chtít, nemůžete/moci (cs)</rdfs:comment>
        <rdfs:comment>e.g., paistes/paistma, paistmas/paistma, peetaks/pidama, peetav/pidama, peetavat/pidama, peeti/pidama, pidamast/pidama, pidamata/pidama, pidite/pidama (et)</rdfs:comment>
        <rdfs:comment>Type=&quot;modal&quot;&lt;br/&gt;

Persian Modal verbs change the aspect of verbs to Subjunctive. Usually they come before Main verbs in present subjunctive form so the Main verb will have normal inflectional attributes. But if the Main verb appears in past 3rd person form, then the construction will be impersonal. Modal verbs usually are not inflected by number and person. However, there is an exception for the verb &apos;‫( &apos;ﺗﻮاﻧﺴﺘﻦ‬tavânestan) that can be inflected for person and number. (Qasemizadeh and Saeed Rahimi 2006)</rdfs:comment>
    </owl:Class>
    


    <!-- http://purl.org/olia/mte/multext-east.owl#ModificationType -->

    <owl:Class rdf:about="http://purl.org/olia/mte/multext-east.owl#ModificationType">
        <rdfs:subClassOf rdf:resource="http://purl.org/olia/mte/multext-east.owl#MorphosyntacticFeature"/>
        <rdfs:comment>Determiner/Modific_Type refers to the prenominal or postnominal positions of Determiners which distinguish different forms in Romanian. (MTE v4)</rdfs:comment>
    </owl:Class>
    


    <!-- http://purl.org/olia/mte/multext-east.owl#ModifierAdverb -->

    <owl:Class rdf:about="http://purl.org/olia/mte/multext-east.owl#ModifierAdverb">
        <rdfs:subClassOf rdf:resource="http://purl.org/olia/mte/multext-east.owl#Adverb"/>
        <rdfs:comment>e.g., better (en)</rdfs:comment>
        <rdfs:comment>Adverb/Type=&quot;modifier&quot; is used in the English, Romanian and Hungarian MTE v4 specs.

For Romanian, Adverb/Type=&quot;modifier&quot; applies to adverbs which can have predicative role, that is they can govern a subordinate sentence (ex. Fireşte că o ştiu -- Certainly I know it). Here (for uniformity within a multilingual environment), they are squeezed into the modifier class. (MTE v4)</rdfs:comment>
    </owl:Class>
    


    <!-- http://purl.org/olia/mte/multext-east.owl#MoodInterjection -->

    <owl:Class rdf:about="http://purl.org/olia/mte/multext-east.owl#MoodInterjection">
        <rdfs:subClassOf rdf:resource="http://purl.org/olia/mte/multext-east.owl#Interjection"/>
        <rdfs:comment>e.g., - (hu)</rdfs:comment>
        <rdfs:comment>Interjection/Type=&quot;mood&quot; (Hungarian)</rdfs:comment>
    </owl:Class>
    


    <!-- http://purl.org/olia/mte/multext-east.owl#MorphologicalDerivation -->

    <owl:Class rdf:about="http://purl.org/olia/mte/multext-east.owl#MorphologicalDerivation">
        <owl:versionInfo>Occasionally, the MTE v.4 specifications employ tag abuse to represent morphological derivations as morphological features. 
To represent the conceptual difference between inflectional (morphosyntactic) and derivational (morphological) features, the concept MorphologicalDerivation is introduced.</owl:versionInfo>
    </owl:Class>
    


    <!-- http://purl.org/olia/mte/multext-east.owl#MorphologicalFormOfNumeral -->

    <owl:Class rdf:about="http://purl.org/olia/mte/multext-east.owl#MorphologicalFormOfNumeral">
        <rdfs:subClassOf rdf:resource="http://purl.org/olia/mte/multext-east.owl#NumeralForm"/>
        <owl:versionInfo>NumeralForm conflates two different aspects that are made explicit here:
- OrthographicRepresentationOfNumeral: the orthographical representation of Numerals, and
- MorphologicalFormOfNumeral: morphological subclasses of Numeral as defined by their derivational morphology</owl:versionInfo>
    </owl:Class>
    


    <!-- http://purl.org/olia/mte/multext-east.owl#MorphosyntacticCategory -->

    <owl:Class rdf:about="http://purl.org/olia/mte/multext-east.owl#MorphosyntacticCategory">
        <rdfs:subClassOf rdf:resource="http://www.w3.org/2002/07/owl#Thing"/>
        <rdfs:subClassOf>
            <owl:Restriction>
                <owl:onProperty rdf:resource="http://purl.org/olia/system.owl#hasTier"/>
                <owl:hasValue>POS</owl:hasValue>
            </owl:Restriction>
        </rdfs:subClassOf>
        <rdfs:comment>Top-level categories as specified under http://nl.ijs.si/ME/V4/msd/html/msd.cats.html.
Subordinate categories reflect &quot;Type&quot; and related attributes.</rdfs:comment>
    </owl:Class>
    


    <!-- http://purl.org/olia/mte/multext-east.owl#MorphosyntacticFeature -->

    <owl:Class rdf:about="http://purl.org/olia/mte/multext-east.owl#MorphosyntacticFeature">
        <rdfs:comment>Morphosyntactic features as specified under http://nl.ijs.si/ME/V4/msd/html. Note that attribute like &quot;type&quot; are represented as subcategories of MorphosyntacticCategory, cf. remarks there.</rdfs:comment>
    </owl:Class>
    


    <!-- http://purl.org/olia/mte/multext-east.owl#MultipleNumeral -->

    <owl:Class rdf:about="http://purl.org/olia/mte/multext-east.owl#MultipleNumeral">
        <rdfs:subClassOf rdf:resource="http://purl.org/olia/mte/multext-east.owl#Numeral"/>
        <rdfs:comment>A Multiple Numeral serves to define a complex whole, with respect to the number of its parts. 
            In English, a Multiple Numeral is formed by adding the syllable &quot;-fold&quot; to the stem of a numeral.
            (Joseph Ghostwick [1878], English language -- Grammar, Historical, London, Longmans, Green, and Co., http://www.archive.org/details/englishgrammarhi00gostrich)
        </rdfs:comment>
        <rdfs:comment>e.g., -nsutitelor/însutit, -nsutitului/însutit, -nsutiţilor/însutit, -ntreitelor/întreit, -ntreitului/întreit, -ntreiţilor/întreit, -nzecitelor/înzecit, -nzecitului/înzecit, -nzeciţilor/înzecit (ro)</rdfs:comment>
        <rdfs:comment>e.g., dvakrát, dvojnásob, jedinkrát, jedinkráte/jedinkrát, jednou, kolikrát, nadvakrát, potřetí, tolikrát (cs)</rdfs:comment>
        <rdfs:comment>e.g., jedenkrát, prvýkrát (sk)</rdfs:comment>
        <rdfs:comment>Numeral/Type=&quot;multiple&quot; (Romanian)&lt;br/&gt;
In traditional Romanian grammars, multiple numerals include expressions like întreit-trine (MTE v4). In other languages, however, these are analysed as adverbs or adjectives: To the Czech tagset a multiple numeral is an adverbial one (dvakrát ‘twice’), whereas to the Slovene tagset it is adjectival (dvojen ‘double’). (Derzhanski and Kotsyba 2009)</rdfs:comment>
    </owl:Class>
    


    <!-- http://purl.org/olia/mte/multext-east.owl#MultiplicativeCase -->

    <owl:Class rdf:about="http://purl.org/olia/mte/multext-east.owl#MultiplicativeCase">
        <rdfs:subClassOf rdf:resource="http://purl.org/olia/mte/multext-east.owl#Case"/>
        <rdfs:comment>
            The multiplicative case is a grammatical case used for marking a number of something (&quot;three times&quot;).
            The case is found in the Hungarian language, for example nyolc (eight), nyolcszor (eight times).
            The case appears also in Finnish as an adverbial (adverb-forming) case. Used with a cardinal number it denotes the number of actions; for example, viisi (five) -&gt; viidesti (five times). Used with adjectives it refers to the mean of the action, corresponding the English suffix -ly: kaunis (beautiful) -&gt; kauniisti (beautifully). It is also used with a small number of nouns: leikki (play) -&gt; leikisti (just kidding, not really). In addition, it acts as an intensifier when used with a swearword: piru -&gt; pirusti.
            (http://en.wikipedia.org/wiki/Multiplicative_case)
        </rdfs:comment>
        <rdfs:comment>e.g., -, tizennegyedszer/tizennegyed, tucatszor/tucat, tízezredszer/tízezred (hu)</rdfs:comment>
        <rdfs:comment>Case=&quot;multiplicative&quot; (Hungarian)</rdfs:comment>
    </owl:Class>
    


    <!-- http://purl.org/olia/mte/multext-east.owl#Negated -->

    <owl:Class rdf:about="http://purl.org/olia/mte/multext-east.owl#Negated">
        <rdfs:subClassOf rdf:resource="http://purl.org/olia/mte/multext-east.owl#Negation"/>
        <rdfs:comment>e.g., , nima/imeti, nimajo/imeti, nimam/imeti, nimamo/imeti, nimata/imeti, nimate/imeti, nimaš/imeti, nisem/biti (sl)</rdfs:comment>
        <rdfs:comment>e.g., ei, eigi/ei, olda/olema, oldud/olema, olevat/olema, olevatki/olema, olge/olema, olgem/olema, olgu/olema (et)</rdfs:comment>
        <rdfs:comment>e.g., nebraňme/bránit, nebude/být, nebudem/být, nebudeme/být, nebudete/být, nebudeš/být, nebudiž/být, nebudou/být, nebudu/být (cs)</rdfs:comment>
        <rdfs:comment>e.g., nepostačia/nestačiť, nepostačí/nestačiť, nepostačím/nestačiť, nepostačíme/nestačiť, nepostačíte/nestačiť, nepostačíš/nestačiť, nepovlečiem/nevliecť, nepovlečieme/nevliecť, nepovlečiete/nevliecť (sk)</rdfs:comment>
        <rdfs:comment>e.g., ni so/bet, ni/bet, nimaio/mët, nimajo/mët, nimate/mët, nisi/bet, niso/bet, ní/bet (sl-rozaj)</rdfs:comment>
        <rdfs:comment>e.g., nieakcentowanymi/akcentować, nieakceptowane/akceptować, nieakceptowanymi/akceptować, niebudzącym/budzić, niebędące/być, niebędącego/być, niebędącej/być, niebędącemu/być, niebędący/być (pl)</rdfs:comment>
        <rdfs:comment>e.g., недај, недајте/недај, недоспаа/недоспие, недоспав/недоспие, недоспавме/недоспие, недоспавте/недоспие, недоспиев/недоспие, недоспиевме/недоспие, недоспиевте/недоспие (mk)</rdfs:comment>
        <rdfs:comment>e.g., مکن/کن, نباش/باش, نباشم/باش, نباشند/باش, نبودم/بود, نبودي/بود, نبوديم/بود, نبينيد/بين, نتواند/توان (fa)</rdfs:comment>
        <rdfs:comment>Negation=&quot;yes&quot;&lt;br/&gt;

Negative=&quot;yes&quot; encodes negative verbal word-forms in Slavic languages and Estonian. (MTE v4) 
In Slovak, for example, verbs form negative by prefix &apos;ne-&apos;, with the exception of the verb &quot;byť&quot; (E. &quot;to be&quot;) which forms the negative in indicative by using separate particle &quot;nie&quot;, e.g. &quot;nie je&quot; (is not). Here, Slovak &quot;je&quot; would be marked as negative, despite having positive form. In Resian, negative is always marked as &apos;n&apos; except for two verbs: &apos;nïman&apos; / not to have, &apos;nïsi&apos; / not to be. (MTE v4)</rdfs:comment>
    </owl:Class>
    


    <!-- http://purl.org/olia/mte/multext-east.owl#Negation -->

    <owl:Class rdf:about="http://purl.org/olia/mte/multext-east.owl#Negation">
        <rdfs:subClassOf rdf:resource="http://purl.org/olia/mte/multext-east.owl#MorphosyntacticFeature"/>
        <rdfs:comment>Negative=&quot;yes&quot; encodes negative verbal word-forms in Slavic languages and Estonian. (MTE v4)</rdfs:comment>
    </owl:Class>
    


    <!-- http://purl.org/olia/mte/multext-east.owl#NegativeAdverb -->

    <owl:Class rdf:about="http://purl.org/olia/mte/multext-east.owl#NegativeAdverb">
        <rdfs:subClassOf rdf:resource="http://purl.org/olia/mte/multext-east.owl#Adverb"/>
        <rdfs:comment>Adverb/Type=&quot;negative&quot; are used in the Serbian and Romanian MTE v4 specs, e.g., for Romanian nicăieri - nowhere, niciodată - never. (MTE v4)</rdfs:comment>
    </owl:Class>
    


    <!-- http://purl.org/olia/mte/multext-east.owl#NegativeDeterminer -->

    <owl:Class rdf:about="http://purl.org/olia/mte/multext-east.owl#NegativeDeterminer">
        <rdfs:subClassOf rdf:resource="http://purl.org/olia/mte/multext-east.owl#Determiner"/>
        <rdfs:comment>e.g., nici-o/nici_un, nici_o/nici_un, nici_un, nici_unei/nici_un, nici_unii/nici_un, nici_unor/nici_un, nici_unui/nici_un (ro)</rdfs:comment>
        <rdfs:comment>Determiner/Type=&quot;negative&quot; (Romanian)&lt;br/&gt;

In Romanian the negative determiner is expressed by the unit nici + indefinite article (e.g. nici un, nici o). (MTE v4)</rdfs:comment>
    </owl:Class>
    


    <!-- http://purl.org/olia/mte/multext-east.owl#NegativeParticle -->

    <owl:Class rdf:about="http://purl.org/olia/mte/multext-east.owl#NegativeParticle">
        <rdfs:subClassOf rdf:resource="http://purl.org/olia/mte/multext-east.owl#Particle"/>
        <rdfs:comment>e.g., n-/nu, nu (ro)</rdfs:comment>
        <rdfs:comment>e.g., не, нито (bg)</rdfs:comment>
        <owl:versionInfo>Particle/Type=&quot;negative&quot; (Romanian, Bulgarian, Serbian, Croatian) is used for particles expressing negation (не, ни, нито) (Dimitrova et al. 2009)</owl:versionInfo>
    </owl:Class>
    


    <!-- http://purl.org/olia/mte/multext-east.owl#NegativePronoun -->

    <owl:Class rdf:about="http://purl.org/olia/mte/multext-east.owl#NegativePronoun">
        <rdfs:subClassOf rdf:resource="http://purl.org/olia/mte/multext-east.owl#Pronoun"/>
        <rdfs:comment>e.g., ni kógor/nišći, nicar/nikar, nikar/nikar, ninega/nidan, nisgi/nišći, nisçhí/nišći (sl-rozaj)</rdfs:comment>
        <rdfs:comment>e.g., nic, nikdo, nikoho/nikdo, nikom/nikdo, nikomu/nikdo, nikým/nikdo, ničeho/nic, ničem/nic, ničemu/nic (cs)</rdfs:comment>
        <rdfs:comment>e.g., nic/nic, niczego/nic, niczemu/nic, niczyi/niczyj, niczyich/niczyj, niczyim/niczyj, niczyimi/niczyj, niczyj/niczyj, niczyja/niczyj (pl)</rdfs:comment>
        <rdfs:comment>e.g., nici_una/nici_unul, nici_uneia/nici_unul, nici_unele/nici_unul, nici_unii/nici_unul, nici_unora/nici_unul, nici_unuia/nici_unul, nici_unul, nimănui/nimeni, nimănuia/nimeni (ro)</rdfs:comment>
        <rdfs:comment>e.g., nijakej/nijaký, nijakou/nijaký, nijaká/nijaký, nijaké/nijaký, nijakého/nijaký, nijakí/nijaký, nijakú/nijaký, nijakých/nijaký, nijakým/nijaký (sk)</rdfs:comment>
        <rdfs:comment>e.g., nikakav, nikakva/nikakav, nikakve/nikakav, nikakvi/nikakav, nikakvih/nikakav, nikakvo/nikakav, nikakvog/nikakav, nikakvom/nikakav, nikakvu/nikakav (sr)</rdfs:comment>
        <rdfs:comment>e.g., nobene/noben, nobenem/noben, nobenih/noben (sl)</rdfs:comment>
        <rdfs:comment>e.g., ані на кому/аніхто ані на кім/аніхто ні на кому/ніхто ні на кім/ніхто, ані на чому/аніщо ані на чім/аніщо ні на чому/ніщо ні на чім/ніщо, ані на яких/аніякий жадних/жаден жадних/жадний жодних/жоден жодних/жодний жоднісіньких/жоднісінький нікоторих/нікоторий нікотрих/нікотрий ніяких/ніякий, ані на якому/аніякий ані на якім/аніякий жадному/жаден жаднім/жаден жадному/жадний жаднім/жадний жодному/жоден жоднім/жоден жодному/жодний жоднім/жодний жоднісінькому/жоднісінький жоднісінькім/жоднісінький нікоторому/нікоторий нікоторім/нікоторий нікотрому/нікотрий нікотрім/нікотрий ніякому/ніякий ніякім/ніякий, ані на якій/аніякий жадній/жаден жадній/жадний жодній/жоден жодній/жодний жоднісінькій/жоднісінький нікоторій/нікоторий нікотрій/нікотрий ніякій/ніякий, аніким/аніхто ані з ким/аніхто ніким/ніхто ні з ким/ніхто, анікогісінько/= анікого/аніхто ані до кого/аніхто нікогісінько/= нікого/ніхто ні до кого/ніхто, анікогісінько/= анікого/аніхто нікогісінько/= нікого/ніхто, анікогісінько/= аніхто/= нікогісінько/= ніхто/= (uk)</rdfs:comment>
        <rdfs:comment>e.g., никаква/никакъв, никакви/никакъв, никакво/никакъв, никакъв, никого/никой, никой, николко, никому/никой, никоя/никой (bg)</rdfs:comment>
        <rdfs:comment>e.g., никого/никој, никое/никој, никои/никој, никому/никој, никој, никоја/никој, ничие/ничиј, ничии/ничиј, ничиј (mk)</rdfs:comment>
        <rdfs:comment>Pronoun/Type=&quot;negative&quot; (Romanian, Slavic)&lt;br/&gt;

Overlap with EmphaticPronoun: In the Ukrainian MTE v4 specs, the emphatic Type of Pronoun is used for pronoun forms ні&quot;кому, ні&quot;чому, ні&quot;чим, ні&quot;кого, etc., with complex meanings like &quot;there is nobody/nothing (to do sth/to use for doing sth, etc.)&quot;. Orthographically these are identical forms of negative nominal pronouns ніхто, ніщо &quot;nobody, nothing&quot; in oblique cases, however, with differing accent. They are referred to as either separate pronoun lexemes or predicatives in grammars. All Ukrainian emphatic pronoun forms include negation.&lt;br/&gt;

Overlap with IndefinitePronoun: In Romanian it is worth differentiating the negative pronoun from other indefinite pronouns: a negative pronoun cannot be an argument for a verb unless the verb itself is negated too (e.g. Nu am văzut pe nimeni / *Am văzut pe nimeni).</rdfs:comment>
    </owl:Class>
    


    <!-- http://purl.org/olia/mte/multext-east.owl#NegativeSubordinatingConjunction -->

    <owl:Class rdf:about="http://purl.org/olia/mte/multext-east.owl#NegativeSubordinatingConjunction">
        <rdfs:subClassOf rdf:resource="http://purl.org/olia/mte/multext-east.owl#SubordinatingConjunction"/>
        <rdfs:comment>Conjunction/Sub_Type=&quot;negative&quot; (Romanian, Serbian, Russian)

In Romanian, each conjunction requires another mood, so that the diversity may be controlled by subcategorisation rules. The attribute Sub_Type distinguishes among the positive and negative conjunctions, providing means to control verbal double negation, (as in case of the negative pronouns, determiners and adverbs): nici NU am venit, nimeni NU vorbeşte, nici_un tren N-a trecut, nicăieri N-am văzut (MTE v4)</rdfs:comment>
    </owl:Class>
    


    <!-- http://purl.org/olia/mte/multext-east.owl#NeuterGender -->

    <owl:Class rdf:about="http://purl.org/olia/mte/multext-east.owl#NeuterGender">
        <rdfs:subClassOf rdf:resource="http://purl.org/olia/mte/multext-east.owl#Gender"/>
        <rdfs:comment>e.g., , bilo/biti, druga/drug, drugega/drug, drugem/drug, drugemu/drug, drugim/drug, drugo/drug, dve/dva (sl)</rdfs:comment>
        <rdfs:comment>e.g., 0, Або/= Абруццо/= Абу-Дабі/= Адріатичне море/= Азовське море/= Айдахо/= Ай-Петрі/= Аконкагуа/= Актау/= Алеппо/= Аліканте/= Алмати/= Альбі/= Андаманське море/= Анжу/= Ані/= Антананаріву/= Антигуа/= Апіа/= Апостолове/=, Або/= Абруццо/= Абу-Дабі/= Адріатичним морем/Адріатичне море Азовським морем/Азовське море Айдахо/= Ай-Петрі/= Аконкагуа/= Актау/= Алеппо/= Аліканте/= Алмати/= Альбі/= Андаманським морем/Андаманське море Анжу/= Ані/= Антананаріву/= Антигуа/= Апіа/= Апостоловим/Апостолове, Або/= Абруццо/= Абу-Дабі/= Адріатичного моря/Адріатичне море Азовського моря/Азовське море Айдахо/= Ай-Петрі/= Аконкагуа/= Актау/= Алеппо/= Аліканте/= Алмати/= Альбі/= Андаманського моря/Андаманське море Анжу/= Ані/= Антананаріву/= Антигуа/= Апіа/= Апостолового/Апостолове, Або/= Абруццо/= Абу-Дабі/= Адріатичному морю/Адріатичне море Азовському морю/Азовське море Айдахо/= Ай-Петрі/= Аконкагуа/= Актау/= Алеппо/= Аліканте/= Алмати/= Альбі/= Андаманському морю/Андаманське море Анжу/= Ані/= Антананаріву/= Антигуа/= Апіа/= Апостоловому/Апостолове, Або/= Абруццо/= Абу-Дабі/= Адріатичному морі/Адріатичне море Адріатичнім морі/Адріатичне море Адріатичному морю/Адріатичне море Адріатичнім морю/Адріатичне море Азовському морі/Азовське море Азовськім морі/Азовське море Азовському морю/Азовське море Азовськім морю/Азовське море Айдахо/= Ай-Петрі/= Аконкагуа/= Актау/= Алеппо/= Аліканте/= Алмати/= Альбі/= Андаманському морі/Андаманське море, Городищ/Городище Джибуті/= Євангелій/Євангеліє Єлисейських полів/Єлисейські Поля Єлисейських піль/Єлисейські Поля Конго/= мальпігієвих тілець/мальпігієві тільця Інтернет-видань/Інтернет-видання Інтернет-кафе/=, Городища/Городище Джибуті/= Євангелія/Євангеліє Єлисейські поля/Єлисейські Поля Конго/= мальпігієві тільця/= Інтернет-видання/= Інтернет-кафе/=, Городищам/Городище Джибуті/= Євангеліям/Євангеліє Єлисейським полям/Єлисейські Поля Конго/= мальпігієвим тільцям/мальпігієві тільця Інтернет-виданням/Інтернет-видання Інтернет-кафе/= (uk)</rdfs:comment>
        <rdfs:comment>e.g., XVII/xvii, XXIII/xxiii, XXIV/xxiv, XXV/xxv, XXVII/xxvii, ДВА/два, Два/два, Двум/два, Двух/два (ru)</rdfs:comment>
        <rdfs:comment>e.g., adoptujących/adoptować, badania/badanie, badaniem/badanie, badań/badanie, bałoś/bać, brawo/brawo, było/być, byłoby/być, były/być (pl)</rdfs:comment>
        <rdfs:comment>e.g., alibi, Angeles, brillská/brillský, byla/být, bylo/být, bývala/bývat, bývalo/bývat, country, desaterým/desaterý (cs)</rdfs:comment>
        <rdfs:comment>e.g., bezbrojnih/bezbrojni, bilo/biti, Bratstvom/Bratstvo, Bratstvu/Bratstvo, crnobrko/crnobrki, derišteta/derište, drveta/drvo, dva, dvadesetora/dvadesetoro (sr)</rdfs:comment>
        <rdfs:comment>e.g., bilo/bet, bilu/bet, bujše/bujši, Chrishtianschin/krištijanski, chrivaha/krïw, colina/kolënu, comsumano/konsumät, delalo/dëlat, delo/dëlu (sl-rozaj)</rdfs:comment>
        <rdfs:comment>e.g., boli/byť, bolo/byť, druhom/druhý, druhé/druhý, druhého/druhý, druhému/druhý, druhých/druhý, druhým/druhý, druhými/druhý (sk)</rdfs:comment>
        <rdfs:comment>e.g., it, its, itself, negroids/negroid, Olympics (en)</rdfs:comment>
        <rdfs:comment>e.g., Винстоне/Винстон, Конго, Македонче, Македончево/Македонче, Македончено/Македонче, Македончето/Македонче, Македончиња/Македонче, Македончињава/Македонче, Македончињана/Македонче (mk)</rdfs:comment>
        <rdfs:comment>e.g., Зайченцето, Лудогорието, Черноморието, било/бъда, било/съм, бъдещо/бъда, бъдещото/бъда, ваше, вашето/ваше (bg)</rdfs:comment>
        <rdfs:comment>In Romanian the declension of a neuter noun always follows in singular a masculine paradigm and in plural a feminine one. Specific implementations could take advantage of this rule and by organizing the paradigmatic space in partial paradigms (masc-sing, masc-pl, fem-sing, fem-pl) to get rid of neuter value for the gender attribute. (MTE v4)</rdfs:comment>
    </owl:Class>
    


    <!-- http://purl.org/olia/mte/multext-east.owl#NoClitic -->

    <owl:Class rdf:about="http://purl.org/olia/mte/multext-east.owl#NoClitic">
        <rdfs:subClassOf rdf:resource="http://purl.org/olia/mte/multext-east.owl#AmbiguousCliticness"/>
        <rdfs:subClassOf>
            <owl:Class>
                <owl:unionOf rdf:parseType="Collection">
                    <rdf:Description rdf:about="http://purl.org/olia/mte/multext-east.owl#ElementWithoutClitic"/>
                    <rdf:Description rdf:about="http://purl.org/olia/mte/multext-east.owl#NoncliticElement"/>
                </owl:unionOf>
            </owl:Class>
        </rdfs:subClassOf>
        <rdfs:comment>e.g., bi&apos;/biti, bi/biti, bih/biti, bila/biti, bile/biti, bilo/biti, bio/biti, bismo/biti, biste/biti (sr)</rdfs:comment>
        <rdfs:comment>e.g., co, jakou/jaký, jaká/jaký, jaké/jaký, jakého/jaký, jakém/jaký, jakému/jaký, jaký, jakých/jaký (cs)</rdfs:comment>
        <rdfs:comment>e.g., g nagn/un, gnagá/un, gnega/un, gnemu/un, gniei/un, gnimi/un, gnimu/un, gnín/un, ja/jä (sl-rozaj)</rdfs:comment>
        <rdfs:comment>e.g., go/on, go/ono, ich/on, ich/ona, ich/ono, im/on, im/ona, im/ono, je/on (pl)</rdfs:comment>
        <rdfs:comment>e.g., hentej/hentá, henten, hentie/henten, hentie/hento, hentie/hentá, hentoho/henten, hentoho/hento, hentom/hento, hentomu/hento (sk)</rdfs:comment>
        <rdfs:comment>e.g., Вам/Вие, Вас/Вие, вам/вие, вас/вие, кого/кој, кому/кој, мене/јас, нам/ние, нас/ние (mk)</rdfs:comment>
        <rdfs:comment>e.g., вам, вас/вие, ваш, ваша, вашата/ваша, ваше, вашето/ваше, ваши, вашите/ваши (bg)</rdfs:comment>
        <rdfs:comment>e.g., آنهايِ/آنها, اونا/آنها آنهايي/آنها آنان, ترا/تو, تو, خودت/خود, خودش/خود, خودشان/خود, خودم/خود, خودمون/خودمان خودمان/خود (fa)</rdfs:comment>
        <rdfs:comment>Clitic=&quot;no&quot; (Noun/Adjective: Romanian; Verb: Romanian, Polish, Serbian, Persian)&lt;br/&gt;

Slovak Pronoun: The Clitic attribute distinguishes clitical vs. nonclitical pronominal forms, e.g. &quot;ti&quot; vs. &quot;tebe&quot;.&lt;br/&gt;

Romanian Verb, Noun, Adjective: The cliticization phenomenon in Romanian is not restricted to verb-pronoun relationship, but may also be observed with the (main) verb and the auxiliary, the noun or adjective with pronoun, with noun or adjective with copula, pronoun with auxiliary, preposition with (indefinite) article, numeral or (indefinite) pronoun, negative adverb with verb, auxiliary or pronoun, and some others (mainly created through the contracted forms of the verb &quot;a fi&quot;-to be). We restrict ourselves to considering only the graphically marked clicitizations. In such cases, the two, three or (sometimes) four constituents of a cliticized word-form are always separated by a hyphen. Omitting the hyphen in such cases is an unacceptable error in written Romanian.&lt;br/&gt;

Romanian Article: Note that the definite article has only enclitic forms, except for one proclitical form (lui + proper noun: lui Ion). The inflected forms of the foreign-origin words (mainly nouns) not fully assimilated, are usually written with a hyphen between the base-form and the inflectional ending. In our encoding, we classified these endings (which are supposed to be split by the segmenter) as clitic articles (clitic attribute is always &quot;y&quot;) which can be either definite (type=f, &quot;-istul&quot;) or indefinite (type=i, &quot;ist&quot;) and are characterised by gender (gender=m, &quot;ist&quot;; gender=f, &quot;istă&quot;), number (number=s, &quot;ist&quot;; number=p, &quot;işti&quot;) and case (case=r, &quot;istul&quot;; case=o, &quot;istului&quot;).</rdfs:comment>
        <owl:versionInfo>Seems to be NoncliticElement in Slovak and Polish, but ElementWithoutClitic in Hungarian and Romanian.</owl:versionInfo>
    </owl:Class>
    


    <!-- http://purl.org/olia/mte/multext-east.owl#NoHuman -->

    <owl:Class rdf:about="http://purl.org/olia/mte/multext-east.owl#NoHuman">
        <rdfs:subClassOf rdf:resource="http://purl.org/olia/mte/multext-east.owl#Humanness"/>
        <rdfs:comment>e.g., czternaste/czternasty, dostałyśmy/dostać, dwudzieste/dwudziesty, dziewięćset/dziewięćset, fakt/fakt, faktem/fakt, interesom/interes, inwestycyjne/inwestycyjny, kosztem/koszt (pl)</rdfs:comment>
        <rdfs:comment>Human=&quot;no&quot;</rdfs:comment>
    </owl:Class>
    


    <!-- http://purl.org/olia/mte/multext-east.owl#Nominal -->

    <owl:Class rdf:about="http://purl.org/olia/mte/multext-east.owl#Nominal">
        <rdfs:subClassOf rdf:resource="http://purl.org/olia/mte/multext-east.owl#SyntacticType"/>
        <rdfs:comment>e.g., hentej/hentá, henten, hentie/henten, hentie/hento, hentie/hentá, hentoho/henten, hentoho/hento, hentom/hento, hentomu/hento (sk)</rdfs:comment>
        <rdfs:comment>e.g., ite/iti, iti/iti, ito/iti, itoha/iti, itën/iti, tabe/tï, takaha/itak, taêbô/tï, te/tï (sl-rozaj)</rdfs:comment>
        <rdfs:comment>e.g., kimkolwiek/ktokolwiek, kimś/ktoś, kogokolwiek/ktokolwiek, kogoś/ktoś, komukolwiek/ktokolwiek, komuś/ktoś, kto/kto, ktokolwiek/ktokolwiek, ktoś/ktoś (pl)</rdfs:comment>
        <rdfs:comment>e.g., kt-ks/kt (et)</rdfs:comment>
        <rdfs:comment>e.g., kterou/který, která/který, které/který, kterého/který, kterém/který, kterému/který, který, kterých/který, kterým/který (cs)</rdfs:comment>
        <rdfs:comment>Pronoun/Syntactic_Type=&quot;nominal&quot; (Slavic), Abbreviation/Syntactic_Type=&quot;nominal&quot;&lt;br/&gt;

Slovak Pronoun: Pronouns are distinguished between having a (syntactically) nominal and (syntactically) adjectival function. All pronominal types except the demonstrative and possessive one can be nominal, and all except for the personal one can be adjectival.</rdfs:comment>
    </owl:Class>
    


    <!-- http://purl.org/olia/mte/multext-east.owl#NominalAdjective -->

    <owl:Class rdf:about="http://purl.org/olia/mte/multext-east.owl#NominalAdjective">
        <owl:equivalentClass>
            <owl:Class>
                <owl:intersectionOf rdf:parseType="Collection">
                    <rdf:Description rdf:about="http://purl.org/olia/mte/multext-east.owl#ReductionFeature"/>
                    <rdf:Description rdf:about="http://purl.org/olia/mte/multext-east.owl#ShortArticle"/>
                </owl:intersectionOf>
            </owl:Class>
        </owl:equivalentClass>
        <rdfs:subClassOf rdf:resource="http://purl.org/olia/mte/multext-east.owl#AdjectiveFormation"/>
        <rdfs:comment>e.g., brillská/brillský, neznámo/neznámý, samo/sám, samy/sám (cs)</rdfs:comment>
        <rdfs:comment>Formation=&quot;nominal&quot; (Czech)</rdfs:comment>
    </owl:Class>
    


    <!-- http://purl.org/olia/mte/multext-east.owl#NominativeCase -->

    <owl:Class rdf:about="http://purl.org/olia/mte/multext-east.owl#NominativeCase">
        <rdfs:subClassOf rdf:resource="http://purl.org/olia/mte/multext-east.owl#Case"/>
        <rdfs:comment>e.g., , drug/=, druga/drug, druge/drug, drugi/drug, drugo/drug, dva/=, dve/dva, dvojna/dvojen (sl)</rdfs:comment>
        <rdfs:comment>e.g., -, amennyije/amennyi, azoké/az, azé/az, Csabák/Csaba, egyedei/egyed, egyem/egy, egyike/egyik, egyikünk/egyik (hu)</rdfs:comment>
        <rdfs:comment>e.g., 0, Аахен/= Абай/= Абакан/= Абакан/= Абіджан/= Абовян/= Авентин/= Адамстаун/= Аден/= Аджаристан/= Адлер/= Адоніс/= Адріанополь/= Азенкур/= Азербайджан/= Азов/= Акерман/= Акмолінськ/= Акрополь/= Актюбінськ/=, Абакуми/Абакум Абакумовичі/Абакумович Аббаси/Аббас Абдули/Абдула Абелі/Абель Абовяни/Абовян Абрами/Абрам Абрамовичі/Абрамович Абрамовичі/Абрамович Абрамчуки/Абрамчук Авакуми/Авакум Авакумовичі/Авакумович Августи/Август Августини/Августин Августиновичі/Августинович Августиновичі/Августинович Августовичі/Августович Авелі/Авель Авенаріуси/Авенаріус Авеніри/Авенір, Абакумів/= Абрамів/= Авакумів/= Августин/= Августинів/= Августів/= Авенірів/= Аверкіїв/= Авер&apos;янів/= Авіятин/= Авксентіїв/= Аврамів/= Авреліїн/= Аврорин/= Автономів/= авторів/= авторчин/= Агапіїв/= Агапіїн/= Агапітів/=, Або/= Абруццо/= Абу-Дабі/= Адріатичне море/= Азовське море/= Айдахо/= Ай-Петрі/= Аконкагуа/= Актау/= Алеппо/= Аліканте/= Алмати/= Альбі/= Андаманське море/= Анжу/= Ані/= Антананаріву/= Антигуа/= Апіа/= Апостолове/=, Абіссінія/= Абуджа/= Абхазія/= Авдіївка/= Австралія/= Австрія/= Австро-Угорщина/= Аддис-Абеба/= Аджарія/= Адигея/= Адріатика/= Азія/= Айова/= Аквітанія/= Аккра/= Ак-Мечеть/= Акмола/= акрилова кислота/= Алабама/= Албанія/=, Азорські острови/= Аландські острови/= Алеутські острови/= Андаманські острови/= Антильські острови/= Багамські острови/= Балеарські острови/= Бельбеки/Бельбек Бермудські острови/= Буги/Буг Великодні/Великдень Великі Сорочинці/= Віргінські острови/= Гавайські острови/= Гебридські острови/= Драконові гори/= ЖЕКи/ЖЕК Зеленого Мису острови/= Змієві вали/= Зондські острови/=, Альпи/= Анди/= Апенніни/= Аппалачі/= Арденни/= Афіни/= Багами/= Балкани/= Байдарські ворота/= Барановичі/= Бендери/= Березняки/= Бермуди/= Бескиди/= Біличі/= Близнюки/= Богородчани/= Боровичі/= Бортничі/= Бровари/=, Америки/Америка Андалуські гори/= Атлаські гори/= Бистриці/Бистриця Держдуми/Держдума Жовті Води/= Збройні Сили України/Збройні сили України Індії/Індія Інтернет-газети/Інтернет-газета Караваєві дачі/= Магелланові хмари/= Македонії/Македонія Мате Залка/= Пасхи/Пасха Пилипівки/Пилипівка Ради/Рада Родезії/Родезія Інтернет-технології/Інтернет-технологія (uk)</rdfs:comment>
        <rdfs:comment>e.g., Cejlon, crnobrko/crnobrki, devetogodišnji, dva, dve/dva, dvoja/dvoje, dvoje, dvoji/dvoje, Englsoc (sr)</rdfs:comment>
        <rdfs:comment>e.g., XVII/xvii, ДВЕ/два, Два/два, Заинтригованная/заинтриговывать, Звенящая/звенеть, МЫ/мы, Мы/мы, ОБА/оба, ОБЕ/оба (ru)</rdfs:comment>
        <rdfs:comment>e.g., a/un, an/un, Boshij/böžji, bujše/bujši, chira/kiri, chire/kiri, Chiri/kiri, costi/kust, dan/dan (sl-rozaj)</rdfs:comment>
        <rdfs:comment>e.g., abdykujący/abdykować, akredytujące/akredytować, amerykański/amerykański, autorzy/autor, badania/badanie, bąk/bąk, ci/ten, co/co, cokolwiek/cokolwiek (pl)</rdfs:comment>
        <rdfs:comment>e.g., desaterý, desátá/desátý, devatenácté/devatenáctý, druhej/druhý, druhá/druhý, druhé/druhý, druhý, druzí/druhý, dva (cs)</rdfs:comment>
        <rdfs:comment>e.g., druhá/druhý, druhé/druhý, druhí/druhý, druhý, dva, dvaja/dva, dve/dva, hentie/henten, hentie/hento (sk)</rdfs:comment>
        <rdfs:comment>e.g., eu, tu (ro)</rdfs:comment>
        <rdfs:comment>e.g., he, I, me, she, they, we (en)</rdfs:comment>
        <rdfs:comment>e.g., ise, ma/mina, me/mina, meie/mina, meiegi/mina, mina, minagi/mina, nad/tema, nemad/tema (et)</rdfs:comment>
        <rdfs:comment>e.g., Америки/Америка, Вие, Индуси/Индус, Конго, Македонецов/Македонец, Македонецон/Македонец, Македонецот/Македонец, Македонкава/Македонка, Македонкана/Македонка (mk)</rdfs:comment>
        <rdfs:comment>e.g., аз, вие, всеки, всякакъв, еди-кой, еди-кой_си, кой, който, неколцина (bg)</rdfs:comment>
    </owl:Class>
    


    <!-- http://purl.org/olia/mte/multext-east.owl#NonInitialCoordinatingConjunction -->

    <owl:Class rdf:about="http://purl.org/olia/mte/multext-east.owl#NonInitialCoordinatingConjunction">
        <rdfs:subClassOf rdf:resource="http://purl.org/olia/mte/multext-east.owl#CoordinatingConjunction_PositionalType"/>
        <rdfs:comment>In the English MTE v4 specs, Conjunction/Coord_Type=&quot;non-initial&quot; designates coordinating conjunctions that are no InitialCoordinatingConjunction, i.e., the second element of a complex conjunction consisting of multiple words (see CorrelativeCoordinatingConjunction), e.g., &quot;or&quot; in &quot;either ... or ...&quot; and &quot;nor&quot; in &quot;neither ... nor ...&quot;, but also single-word conjunctions such as &quot;than&quot;, &quot;but&quot;, and &quot;and&quot;.</rdfs:comment>
    </owl:Class>
    


    <!-- http://purl.org/olia/mte/multext-east.owl#NonNegated -->

    <owl:Class rdf:about="http://purl.org/olia/mte/multext-east.owl#NonNegated">
        <rdfs:subClassOf rdf:resource="http://purl.org/olia/mte/multext-east.owl#Negation"/>
        <rdfs:comment>e.g., , bodo/biti, bojo/biti, bom/biti, bomo/biti, bosta/biti, boste/biti, bova/biti, boš/biti (sl)</rdfs:comment>
        <rdfs:comment>e.g., abdykujący/abdykować, adoptujących/adoptować, akceptowanymi/akceptować, akredytujące/akredytować, akredytujących/akredytować, akredytującą/akredytować, analizowanych/analizować, awansującym/awansować, badanego/badać (pl)</rdfs:comment>
        <rdfs:comment>e.g., aman/amät, boijo/bat, bota/bet, Ciete/tët, cion/tët, datte/dät, giò/tët, idu/tet, intendate/intendät (sl-rozaj)</rdfs:comment>
        <rdfs:comment>e.g., bejt/být, bude/být, budeme/být, budete/být, budeš/být, budou/být, budu/být, buď/být, byl/být (cs)</rdfs:comment>
        <rdfs:comment>e.g., bi&apos;/biti, bi/biti, bih/biti, bila/biti, bile/biti, bilo/biti, bio/biti, bismo/biti, biste/biti (sr)</rdfs:comment>
        <rdfs:comment>e.g., bola/byť, boli/byť, bolo/byť, bude/byť, budem/byť, budeme/byť, budete/byť, budeš/byť, budú/byť (sk)</rdfs:comment>
        <rdfs:comment>e.g., kuulukse/kuuluksema, oldi/olema, ole/olema, oled/olema, oledki/olema, olegi/olema, oleks/olema, oleksime/olema, oleksin/olema (et)</rdfs:comment>
        <rdfs:comment>e.g., آمديد/آمد, آمديم/آمد, باشه/باش باشد/باش آيد/آ, باشي/باش, بتوان/توان, بتواند/توان, بتوانم/توان, بتوانند/توان, بتوانيد/توان (fa)</rdfs:comment>
        <rdfs:comment>Negation=&quot;no&quot;&lt;br/&gt;

Non-negated verbs carry no morphological marks of negation. In Resian, negative is always marked as &apos;no&apos; except for two verbs: &apos;nïman&apos; / not to have, &apos;nïsi&apos; / not to be. In Slovak, verbs form negative by prefix &apos;ne-&apos;, with the exception of the verb &quot;byť&quot; (E. &quot;to be&quot;) which forms the negative in indicative by using separate particle &quot;nie&quot;, e.g. &quot;nie je&quot; (is not). Here, &quot;je&quot; would be marked as negative, despite having positive form. (MTE v4)</rdfs:comment>
    </owl:Class>
    


    <!-- http://purl.org/olia/mte/multext-east.owl#NoncliticElement -->

    <owl:Class rdf:about="http://purl.org/olia/mte/multext-east.owl#NoncliticElement">
        <rdfs:subClassOf rdf:resource="http://purl.org/olia/mte/multext-east.owl#Cliticness"/>
    </owl:Class>
    


    <!-- http://purl.org/olia/mte/multext-east.owl#NonspecificPronoun -->

    <owl:Class rdf:about="http://purl.org/olia/mte/multext-east.owl#NonspecificPronoun">
        <rdfs:subClassOf rdf:resource="http://purl.org/olia/mte/multext-east.owl#Pronoun"/>
        <rdfs:comment>In the Russian MTE v4 specs, Pronoun/Type=&quot;nonspecific&quot; marks the following Russian words: весь &apos;all&apos;, всякий &apos;any, every&apos;, сам &apos;oneself&apos;, самый &apos;the very&apos;, каждый &apos;every, each&apos;, иной &apos;other&apos;, любой &apos;any&apos;, другой &apos;other&apos;. The name &quot;nonspecific&quot; follows Halliday (1985, Section 6.2.1.1). (MTE v4)

A nonspecific pronoun refers to an unidentified or general entity (e.g., &quot;I saw *someone*&quot;, &quot;I saw *everyone*&quot;). A nonspecific pronoun is not, therefore, a personal pronoun, but an indefinite one. (Andrews 2003).

Andrews, Richard J. (2003), Introduction to Classical Nahuatl. University of Oklahoma Press.
Halliday, M.A.K. (1985), An introduction to Functional Grammar, London: Edward Arnold</rdfs:comment>
    </owl:Class>
    


    <!-- http://purl.org/olia/mte/multext-east.owl#Noun -->

    <owl:Class rdf:about="http://purl.org/olia/mte/multext-east.owl#Noun">
        <rdfs:subClassOf rdf:resource="http://purl.org/olia/mte/multext-east.owl#MorphosyntacticCategory"/>
        <rdfs:subClassOf>
            <owl:Class>
                <owl:intersectionOf rdf:parseType="Collection">
                    <owl:Restriction>
                        <owl:onProperty rdf:resource="http://purl.org/olia/mte/multext-east.owl#hasAspect"/>
                        <owl:maxCardinality rdf:datatype="http://www.w3.org/2001/XMLSchema#nonNegativeInteger">1</owl:maxCardinality>
                    </owl:Restriction>
                    <owl:Restriction>
                        <owl:onProperty rdf:resource="http://purl.org/olia/mte/multext-east.owl#hasCase"/>
                        <owl:maxCardinality rdf:datatype="http://www.w3.org/2001/XMLSchema#nonNegativeInteger">1</owl:maxCardinality>
                    </owl:Restriction>
                    <owl:Restriction>
                        <owl:onProperty rdf:resource="http://purl.org/olia/mte/multext-east.owl#hasClitic"/>
                        <owl:maxCardinality rdf:datatype="http://www.w3.org/2001/XMLSchema#nonNegativeInteger">1</owl:maxCardinality>
                    </owl:Restriction>
                    <owl:Restriction>
                        <owl:onProperty rdf:resource="http://purl.org/olia/mte/multext-east.owl#hasDefiniteness"/>
                        <owl:maxCardinality rdf:datatype="http://www.w3.org/2001/XMLSchema#nonNegativeInteger">1</owl:maxCardinality>
                    </owl:Restriction>
                    <owl:Restriction>
                        <owl:onProperty rdf:resource="http://purl.org/olia/mte/multext-east.owl#hasHumanness"/>
                        <owl:maxCardinality rdf:datatype="http://www.w3.org/2001/XMLSchema#nonNegativeInteger">1</owl:maxCardinality>
                    </owl:Restriction>
                    <owl:Restriction>
                        <owl:onProperty rdf:resource="http://purl.org/olia/mte/multext-east.owl#hasOwnedNumber"/>
                        <owl:maxCardinality rdf:datatype="http://www.w3.org/2001/XMLSchema#nonNegativeInteger">1</owl:maxCardinality>
                    </owl:Restriction>
                    <owl:Restriction>
                        <owl:onProperty rdf:resource="http://purl.org/olia/mte/multext-east.owl#hasOwnerNumber"/>
                        <owl:maxCardinality rdf:datatype="http://www.w3.org/2001/XMLSchema#nonNegativeInteger">1</owl:maxCardinality>
                    </owl:Restriction>
                </owl:intersectionOf>
            </owl:Class>
        </rdfs:subClassOf>
        <rdfs:subClassOf>
            <owl:Restriction>
                <owl:onProperty rdf:resource="http://purl.org/olia/mte/multext-east.owl#hasGender"/>
                <owl:cardinality rdf:datatype="http://www.w3.org/2001/XMLSchema#nonNegativeInteger">1</owl:cardinality>
            </owl:Restriction>
        </rdfs:subClassOf>
        <rdfs:subClassOf>
            <owl:Restriction>
                <owl:onProperty rdf:resource="http://purl.org/olia/mte/multext-east.owl#hasNumber"/>
                <owl:cardinality rdf:datatype="http://www.w3.org/2001/XMLSchema#nonNegativeInteger">1</owl:cardinality>
            </owl:Restriction>
        </rdfs:subClassOf>
        <rdfs:subClassOf>
            <owl:Restriction>
                <owl:onProperty rdf:resource="http://purl.org/olia/mte/multext-east.owl#hasAnimacy"/>
                <owl:maxCardinality rdf:datatype="http://www.w3.org/2001/XMLSchema#nonNegativeInteger">1</owl:maxCardinality>
            </owl:Restriction>
        </rdfs:subClassOf>
        <rdfs:subClassOf>
            <owl:Restriction>
                <owl:onProperty rdf:resource="http://purl.org/olia/mte/multext-east.owl#hasOwnerPerson"/>
                <owl:maxCardinality rdf:datatype="http://www.w3.org/2001/XMLSchema#nonNegativeInteger">1</owl:maxCardinality>
            </owl:Restriction>
        </rdfs:subClassOf>
        <rdfs:comment>e.g., -mpărate/împărat, -ngrijitoare/îngrijitoare, -nsoţitoare/însoţitoare, -nvingători/învingător, -nvingătorii/învingător, -nvingătorilor/învingător, -nvingătorului/învingător, -nvăţătoare/învăţătoare, -nvăţători/învăţător (ro)</rdfs:comment>
        <rdfs:comment>e.g., Aladárét/Aladár, barátoddal/barát, betegségedhez/betegség, betegségünktől/betegség, botrányoddal/botrány, cselekedeteidről/cselekedet, cselekedeteiteken/cselekedet, csontjaiig/csont, embereinktől/ember (hu)</rdfs:comment>
        <rdfs:comment>e.g., Baltimaadel/Baltimaad, Baltimaades/Baltimaad, Kallastel/Kallas, Kallastele/Kallas, Kallastelt/Kallas, Kallasteni/Kallas, Pauluste/Paulus, trükivigadeni/trükiviga, tulemusteni/tulemus (et)</rdfs:comment>
        <rdfs:comment>e.g., Bratstvom/Bratstvo, Bratstvu/Bratstvo, derišteta/derište, drveta/drvo, javnosti/javnost, kategorije/kategorija, Ketrin, ministarstva/ministarstvo, Ministarstvu/Ministarstvo (sr)</rdfs:comment>
        <rdfs:comment>e.g., Christusa/krïštuš, Christusam/krïštuš, Comandatmiteh/komandament, costi/kust, Crishtusha/krïštuš, Dapiton/dapit, dialëte/dijalët, dobrute/dubruta, Elisabeto/elizabeta (sl-rozaj)</rdfs:comment>
        <rdfs:comment>e.g., Christusa/krïštuš, Crishtusha/krïštuš, taleta/tale, taléta/tale (sl-rozaj)</rdfs:comment>
        <rdfs:comment>e.g., Hrvatoma/Hrvat, pilatusema/pilatus (sl)</rdfs:comment>
        <rdfs:comment>e.g., absolwentów/absolwent, autora/autor, autorzy/autor, czytelnika/czytelnik, doktor/doktor, doktorowi/doktor, fakt/fakt, faktem/fakt, gospodarstwa/gospodarstwo (pl)</rdfs:comment>
        <rdfs:comment>e.g., absolwentów/absolwent, autora/autor, autorzy/autor, czytelnika/czytelnik, doktor/doktor, doktorowi/doktor, kot/kot, kotku/kotek, kotu/kot (pl)</rdfs:comment>
        <rdfs:comment>e.g., country, kontra, kontras/kontra, turné, ztotožněním/ztotožnění, ztělesněním/ztělesnění, zvyklostem/zvyklost, žurnalisté/žurnalista (cs)</rdfs:comment>
        <rdfs:comment>e.g., derišteta/derište, zlomislitelja/zlomislitelj, zlomislitelje/zlomislitelj, zlomislitelji/zlomislitelj, zlomisliteljima/zlomislitelj, Zlomislitelju/Zlomislitelj (sr)</rdfs:comment>
        <rdfs:comment>e.g., viscounts/viscount, welterweights/welterweight (en)</rdfs:comment>
        <rdfs:comment>e.g., žurnalistiek/žurnalistka, žurnalistikami/žurnalistika, žurnalistike/žurnalistika, žurnalistikou/žurnalistika, žurnalistiku/žurnalistika, žurnalistiky/žurnalistika, žurnalistikách/žurnalistika, žurnalistikám/žurnalistika, žurnalistkami/žurnalistka (sk)</rdfs:comment>
        <rdfs:comment>e.g., žurnalisté/žurnalista (cs)</rdfs:comment>
        <rdfs:comment>Nouns are characterized by features such as gender and number (for all MTE v4 languages, http://nl.ijs.si/ME/V4/msd/html/msd.N.html)&lt;br/&gt;

As for the overlap between Noun and Adjective, Slovak adjectival nouns (gazdiná, hostinský) are classified as nouns. Sometimes the distinction between noun and adjective is not as clear as we want (obchodný cestujúci). (MTE v4)&lt;br/&gt;

As for the overlap between Noun and Verb, Ukrainian gerunds are not differentiated, but could be treated as a special class of nouns, nota bene: they possess aspect. (MTE v4)</rdfs:comment>
    </owl:Class>
    


    <!-- http://purl.org/olia/mte/multext-east.owl#Number -->

    <owl:Class rdf:about="http://purl.org/olia/mte/multext-east.owl#Number">
        <rdfs:subClassOf rdf:resource="http://purl.org/olia/mte/multext-east.owl#MorphosyntacticFeature"/>
        <rdfs:comment>Hungarian has three types of number in the nominal inflection: 1. The number of the noun. 2. The number of owners that own the noun. 3. The number of the context given referent, which is some possession of the noun, i.e. belongs to the noun (anaphoric possessive). (MTE v4)</rdfs:comment>
    </owl:Class>
    


    <!-- http://purl.org/olia/mte/multext-east.owl#Numeral -->

    <owl:Class rdf:about="http://purl.org/olia/mte/multext-east.owl#Numeral">
        <rdfs:subClassOf rdf:resource="http://purl.org/olia/mte/multext-east.owl#Quantifier"/>
        <rdfs:subClassOf>
            <owl:Class>
                <owl:intersectionOf rdf:parseType="Collection">
                    <owl:Restriction>
                        <owl:onProperty rdf:resource="http://purl.org/olia/mte/multext-east.owl#hasAnimacy"/>
                        <owl:maxCardinality rdf:datatype="http://www.w3.org/2001/XMLSchema#nonNegativeInteger">1</owl:maxCardinality>
                    </owl:Restriction>
                    <owl:Restriction>
                        <owl:onProperty rdf:resource="http://purl.org/olia/mte/multext-east.owl#hasClitic"/>
                        <owl:maxCardinality rdf:datatype="http://www.w3.org/2001/XMLSchema#nonNegativeInteger">1</owl:maxCardinality>
                    </owl:Restriction>
                    <owl:Restriction>
                        <owl:onProperty rdf:resource="http://purl.org/olia/mte/multext-east.owl#hasDefiniteness"/>
                        <owl:maxCardinality rdf:datatype="http://www.w3.org/2001/XMLSchema#nonNegativeInteger">1</owl:maxCardinality>
                    </owl:Restriction>
                    <owl:Restriction>
                        <owl:onProperty rdf:resource="http://purl.org/olia/mte/multext-east.owl#hasNumeralForm"/>
                        <owl:maxCardinality rdf:datatype="http://www.w3.org/2001/XMLSchema#nonNegativeInteger">1</owl:maxCardinality>
                    </owl:Restriction>
                    <owl:Restriction>
                        <owl:onProperty rdf:resource="http://purl.org/olia/mte/multext-east.owl#hasOwnerNumber"/>
                        <owl:maxCardinality rdf:datatype="http://www.w3.org/2001/XMLSchema#nonNegativeInteger">1</owl:maxCardinality>
                    </owl:Restriction>
                    <owl:Restriction>
                        <owl:onProperty rdf:resource="http://purl.org/olia/mte/multext-east.owl#hasOwnerPerson"/>
                        <owl:maxCardinality rdf:datatype="http://www.w3.org/2001/XMLSchema#nonNegativeInteger">1</owl:maxCardinality>
                    </owl:Restriction>
                    <owl:Restriction>
                        <owl:onProperty rdf:resource="http://purl.org/olia/mte/multext-east.owl#hasQuantifier"/>
                        <owl:maxCardinality rdf:datatype="http://www.w3.org/2001/XMLSchema#nonNegativeInteger">1</owl:maxCardinality>
                    </owl:Restriction>
                </owl:intersectionOf>
            </owl:Class>
        </rdfs:subClassOf>
        <rdfs:subClassOf>
            <owl:Class>
                <owl:intersectionOf rdf:parseType="Collection">
                    <owl:Restriction>
                        <owl:onProperty rdf:resource="http://purl.org/olia/mte/multext-east.owl#hasCase"/>
                        <owl:maxCardinality rdf:datatype="http://www.w3.org/2001/XMLSchema#nonNegativeInteger">1</owl:maxCardinality>
                    </owl:Restriction>
                    <owl:Restriction>
                        <owl:onProperty rdf:resource="http://purl.org/olia/mte/multext-east.owl#hasGender"/>
                        <owl:maxCardinality rdf:datatype="http://www.w3.org/2001/XMLSchema#nonNegativeInteger">1</owl:maxCardinality>
                    </owl:Restriction>
                    <owl:Restriction>
                        <owl:onProperty rdf:resource="http://purl.org/olia/mte/multext-east.owl#hasNumber"/>
                        <owl:maxCardinality rdf:datatype="http://www.w3.org/2001/XMLSchema#nonNegativeInteger">1</owl:maxCardinality>
                    </owl:Restriction>
                </owl:intersectionOf>
            </owl:Class>
        </rdfs:subClassOf>
        <rdfs:subClassOf>
            <owl:Restriction>
                <owl:onProperty rdf:resource="http://purl.org/olia/mte/multext-east.owl#hasHumanness"/>
                <owl:maxCardinality rdf:datatype="http://www.w3.org/2001/XMLSchema#nonNegativeInteger">1</owl:maxCardinality>
            </owl:Restriction>
        </rdfs:subClassOf>
        <rdfs:subClassOf>
            <owl:Restriction>
                <owl:onProperty rdf:resource="http://purl.org/olia/mte/multext-east.owl#hasOwnedNumber"/>
                <owl:maxCardinality rdf:datatype="http://www.w3.org/2001/XMLSchema#nonNegativeInteger">1</owl:maxCardinality>
            </owl:Restriction>
        </rdfs:subClassOf>
        <rdfs:comment>e.g., -nsutitelor/însutit, -nsutitului/însutit, -nsutiţilor/însutit, -ntreitelor/întreit, -ntreitului/întreit, -ntreiţilor/întreit, -ntâi/întâi, -ntâia/întâi, -ntâiaşi/întâi (ro)</rdfs:comment>
        <rdfs:comment>e.g., 1900-tól/1900, 2050-től/2050, egyenként/egy, egynegyedét/egynegyed, egytizedének/egytized, egytizedére/egytized, elsőként/első, ezerért/ezer, hetekben/hét (hu)</rdfs:comment>
        <rdfs:comment>e.g., 32/trïstinudwa, sehont/sagont, shtiri/štirji, starkrat duísti anu dévatnist/štirkratdwistinudëvatnist, treh/trïji, tretgna/trëtnji, tretgni/trëtnji, tretni/trëtnji, tretnji/trëtnji (sl-rozaj)</rdfs:comment>
        <rdfs:comment>e.g., czterdziestych/czterdziesty, czterdziestym/czterdziesty, czterech/cztery, czterem/cztery, czterema/cztery, czternaste/czternasty, czternastym/czternasty, cztery/cztery, czwarte/czwarty (pl)</rdfs:comment>
        <rdfs:comment>e.g., czwartego/czwarty, dwustu/dwieście, piętnastu/piętnaście, półtora/półtora, trzeci/trzeci, trzej/trzy (pl)</rdfs:comment>
        <rdfs:comment>e.g., desaterý, desaterým/desaterý, desátá/desátý, devatenácté/devatenáctý, devatenáctému/devatenáctý, devatenáctým/devatenáctý, dvacátých/dvacátý, jedenáctém/jedenáctý, jedinkráte/jedinkrát (cs)</rdfs:comment>
        <rdfs:comment>e.g., dvadesetora/dvadesetoro, stotine/stotina, tri, tridesetora/tridesetoro, trima/tri, troja/troje, troje, troji/troje, trojih/troje (sr)</rdfs:comment>
        <rdfs:comment>e.g., esimesteks/esimene, esimestele/esimene, esimestena/esimene, esimestes/esimene, esimestest/esimene, kümneteks/kümme, miljonitesse/miljon, teise/teine, teisega/teine (et)</rdfs:comment>
        <rdfs:comment>e.g., tisícinou/tisícina, traja/tri, tretej/tretí, tretia/tretí, tretie/tretí, tretieho/tretí, tretiemu/tretí, tretinou/tretina, tretiu/tretí (sk)</rdfs:comment>
        <rdfs:comment>e.g., treh/trije, trem/trije, tremi/trije, tretjim/tretji, trojen/=, štiri/štirje, štirih/štirje, štirim/štirje (sl)</rdfs:comment>
        <rdfs:comment>e.g., třetí, třetího/třetí, čtvrtí/čtvrtý, šestnáctého/šestnáctý (cs)</rdfs:comment>
        <rdfs:comment>In Romanian (as in many other languages) several numerals have noun behaviour (some grammarians classify such numerals as nouns) with gender and declension of their own, which they preserve even in the composition of the superior order numerals; these are, for instance, sută (hundred), mie (thousand), milion (million) and miliard (billion). In a sentence most numerals may fulfill the function of other parts of speech like noun, determiner or adverb. (Romanian MTE v.4)&lt;br/&gt;
In some languages, a division of numerals according to their nominal, adjectival or adverbial function is, however, not usual, and numerals have not been subsumed under adjectives, pronouns, determiners, etc. because the internal structure of complex numerals is idiosyncratic and because of their specific syntactic distribution. (Resian, English, Czech, MTE v.4). </rdfs:comment>
        <owl:versionInfo>In many MTE schemes, the class &quot;Numeral&quot; is applied to cover non-numerical quantifiers, as well. The common MTE  category &quot;Numeral&quot; thus fails to distinguish between numeral and non-numeral quantifiers and has thus been renamed to the broader concept &quot;Quantifier&quot;.</owl:versionInfo>
    </owl:Class>
    


    <!-- http://purl.org/olia/mte/multext-east.owl#NumeralAgreementClass -->

    <owl:Class rdf:about="http://purl.org/olia/mte/multext-east.owl#NumeralAgreementClass">
        <rdfs:subClassOf rdf:resource="http://purl.org/olia/mte/multext-east.owl#MorphosyntacticFeature"/>
        <rdfs:subClassOf rdf:resource="http://purl.org/olia/mte/multext-east.owl#Quantifier"/>
        <rdfs:comment>In most Slavic languages, Numerals and Quantifiers involve specific agreement patterns, e.g., in Russian:&lt;br/&gt;

(b) PaucalQuantifier (MTE v4: Numeral/Class=&quot;definite234&quot;): requires noun in genitive singular, e.g., два/три/четыре года &quot;two/three/four years&quot;
(c) PluralQuantifier (MTE v4: Numeral/Class=&quot;definite&quot;):requires noun in genitive plural, e.g., пять/много/сколько/столько лет &quot;five/many/how many/that many years&quot;&lt;br/&gt;

Bulgarian has done away with the distinction between 4 and 5, and generalised the 2-4 form to all numerals (and some other quantifiers), but the others generally keep it.  Also Slovene has a living dual (both Sorbians likewise, but they haven&apos;t been MTEd).&lt;br/&gt;

Some Czech feminine and neuter body parts have preserved dual forms, and if the noun is dual, so are its attributes (adjectives, pronouns).  So 2 differs formally from 3-4. The corresponding agreement pattern is a DualQuantifier (MTE v4: Numeral/Class=&quot;definite2&quot;).
(Ivan A. Derzhanski &amp; Christian Chiarcos)</rdfs:comment>
    </owl:Class>
    


    <!-- http://purl.org/olia/mte/multext-east.owl#NumeralForm -->

    <owl:Class rdf:about="http://purl.org/olia/mte/multext-east.owl#NumeralForm">
        <rdfs:subClassOf rdf:resource="http://purl.org/olia/mte/multext-east.owl#MorphosyntacticFeature"/>
        <rdfs:comment>NumeralForm conflates two different aspects that are made explicit here:
- OrthographicRepresentationOfNumeral: the orthographical representation of Numerals, and
- MorphologicalFormOfNumeral: morphological subclasses of Numeral as defined by their derivational morphology</rdfs:comment>
    </owl:Class>
    


    <!-- http://purl.org/olia/mte/multext-east.owl#NumeralThreeOrFour -->

    <owl:Class rdf:about="http://purl.org/olia/mte/multext-east.owl#NumeralThreeOrFour">
        <rdfs:subClassOf rdf:resource="http://purl.org/olia/mte/multext-east.owl#PaucalQuantifier"/>
        <rdfs:comment>Numeral/Class=&quot;definite34&quot; (Polish, Czech). Agreement pattern as prototypically manifested for numerals &quot;three&quot; and &quot;four&quot; (in Czech and Polish).</rdfs:comment>
        <owl:versionInfo>Numeral/Class=&quot;definite&quot;, Numeral/Class=&quot;definite1&quot;, Numeral/Class=&quot;definite234&quot; etc. refer to specific patterns of congruency with Slavic numerals that originate from the difference between Old Slavic singular (definite1), dual (definite2, definite234) and plural (definite).</owl:versionInfo>
    </owl:Class>
    


    <!-- http://purl.org/olia/mte/multext-east.owl#NumeralTwoToFour -->

    <owl:Class rdf:about="http://purl.org/olia/mte/multext-east.owl#NumeralTwoToFour">
        <rdfs:subClassOf rdf:resource="http://purl.org/olia/mte/multext-east.owl#PaucalQuantifier"/>
        <rdfs:comment>Numeral/Class=&quot;definite234&quot; (Slovak)&lt;br/&gt;
Agreement pattern as prototypically manifested for the numerals two to four.</rdfs:comment>
        <owl:versionInfo>Numeral/Class=&quot;definite&quot;, Numeral/Class=&quot;definite1&quot;, Numeral/Class=&quot;definite234&quot; etc. refer to specific patterns of congruency with Slavic numerals that originate from the difference between Old Slavic singular (definite1), dual (definite2, definite234) and plural (definite).</owl:versionInfo>
    </owl:Class>
    


    <!-- http://purl.org/olia/mte/multext-east.owl#ObliqueCase -->

    <owl:Class rdf:about="http://purl.org/olia/mte/multext-east.owl#ObliqueCase">
        <rdfs:subClassOf rdf:resource="http://purl.org/olia/mte/multext-east.owl#Case"/>
        <rdfs:comment>e.g., -istei, -istelor, -istului, -iştilor, -nsutitelor/însutit, -nsutitului/însutit, -nsutiţilor/însutit, -ntreitelor/întreit, -ntreitului/întreit (ro)</rdfs:comment>
        <rdfs:comment>Case=&quot;oblique&quot; (Romanian, Macedonian)&lt;br/&gt;

In the Romanian case system the value &apos;oblique&apos; conflates &apos;genitive&apos; and &apos;dative&apos;. In the Macedonian case system the value &apos;oblique&apos; conflates archaic forms of &apos;genitive&apos;, &apos;dative&apos; and &apos;accusative&apos;.</rdfs:comment>
    </owl:Class>
    


    <!-- http://purl.org/olia/mte/multext-east.owl#OrdinalAdjective -->

    <owl:Class rdf:about="http://purl.org/olia/mte/multext-east.owl#OrdinalAdjective">
        <rdfs:subClassOf rdf:resource="http://purl.org/olia/mte/multext-east.owl#AmbiguousAdjective"/>
        <rdfs:subClassOf>
            <owl:Class>
                <owl:unionOf rdf:parseType="Collection">
                    <rdf:Description rdf:about="http://purl.org/olia/mte/multext-east.owl#RelationalAdjective"/>
                    <owl:Class>
                        <owl:intersectionOf rdf:parseType="Collection">
                            <rdf:Description rdf:about="http://purl.org/olia/mte/multext-east.owl#Adjective"/>
                            <rdf:Description rdf:about="http://purl.org/olia/mte/multext-east.owl#OrdinalNumeral"/>
                        </owl:intersectionOf>
                    </owl:Class>
                </owl:unionOf>
            </owl:Class>
        </rdfs:subClassOf>
        <rdfs:comment>e.g., Bohavei/böguw, Bohouv/böguw, Bohovaha/böguw, Bohove/böguw, Bohovih/böguw, Bohovij/böguw, Bohovin/böguw, Bohuvin/böguw, Boshij/böžji (sl-rozaj)</rdfs:comment>
        <rdfs:comment>e.g., evroazijskog/evroazijski, Faroskih/Faroska, francuski, gipsani/gipsan, malabarskog/malabarski, malabarskom/malabarski, muzičkog/muzički, novogovorske/novogovorski, okeanijskog/okeanijski (sr)</rdfs:comment>
        <rdfs:comment>e.g., Абакумів/= Абрамів/= Авакумів/= Августин/= Августинів/= Августів/= Авенірів/= Аверкіїв/= Авер&apos;янів/= Авіятин/= Авксентіїв/= Аврамів/= Авреліїн/= Аврорин/= Автономів/= авторів/= авторчин/= Агапіїв/= Агапіїн/= Агапітів/=, антресольна/антресольний антропічна/антропічний антропна/антропний антропогенна/антропогенний антропоїдна/антропоїдний антропологічна/антропологічний абажурна/абажурний абазинська/абазинський абаканська/абаканський Абакумова/Абакумів абатська/абатський абераційна/абераційний абеткова/абетковий абіджанська/абіджанський абіогенна/абіогенний абісальна/абісальний абіссінська/абіссінський абітурієнтська/абітурієнтський аболіціоністська/аболіціоністський абонементна/абонементний, антресольная/антресольний антропічная/антропічний антропная/антропний антропогенная/антропогенний антропоїдная/антропоїдний антропологічная/антропологічний абажурная/абажурний абазинськая/абазинський абаканськая/абаканський Абакумовая/Абакумів абатськая/абатський абераційная/абераційний абетковая/абетковий абіджанськая/абіджанський абіогенная/абіогенний абісальная/абісальний абіссінськая/абіссінський абітурієнтськая/абітурієнтський аболіціоністськая/аболіціоністський абонементная/абонементний, антресольне/антресольний антропічне/антропічний антропне/антропний антропогенне/антропогенний антропоїдне/антропоїдний антропологічне/антропологічний абажурне/абажурний абазинське/абазинський абаканське/абаканський Абакумове/Абакумів абатське/абатський абераційне/абераційний абеткове/абетковий абіджанське/абіджанський абіогенне/абіогенний абісальне/абісальний абіссінське/абіссінський абітурієнтське/абітурієнтський аболіціоністське/аболіціоністський абонементне/абонементний, антресольнеє/антресольний антропічнеє/антропічний антропнеє/антропний антропогеннеє/антропогенний антропоїднеє/антропоїдний антропологічнеє/антропологічний абажурнеє/абажурний абазинськеє/абазинський абаканськеє/абаканський Абакумовеє/Абакумів абатськеє/абатський абераційнеє/абераційний абетковеє/абетковий абіджанськеє/абіджанський абіогеннеє/абіогенний абісальнеє/абісальний абіссінськеє/абіссінський абітурієнтськеє/абітурієнтський аболіціоністськеє/аболіціоністський абонементнеє/абонементний, антресольний/= антропічний/= антропний/= антропогенний/= антропоїдний/= антропологічний/= абажурний/= абазинський/= абаканський/= абатський/= абераційний/= абетковий/= абіджанський/= абіогенний/= абісальний/= абіссінський/= абітурієнтський/= аболіціоністський/= абонементний/= абонентний/=, антресольним/антресольний антропічним/антропічний антропним/антропний антропогенним/антропогенний антропоїдним/антропоїдний антропологічним/антропологічний абажурним/абажурний абазинським/абазинський абаканським/абаканський Абакумовим/Абакумів абатським/абатський абераційним/абераційний абетковим/абетковий абіджанським/абіджанський абіогенним/абіогенний абісальним/абісальний абіссінським/абіссінський абітурієнтським/абітурієнтський аболіціоністським/аболіціоністський абонементним/абонементний, антресольними/антресольний антропічними/антропічний антропними/антропний антропогенними/антропогенний антропоїдними/антропоїдний антропологічними/антропологічний абажурними/абажурний абазинськими/абазинський абаканськими/абаканський Абакумовими/Абакумів абатськими/абатський абераційними/абераційний абетковими/абетковий абіджанськими/абіджанський абіогенними/абіогенний абісальними/абісальний абіссінськими/абіссінський абітурієнтськими/абітурієнтський аболіціоністськими/аболіціоністський абонементними/абонементний, антресольних/антресольний антропічних/антропічний антропних/антропний антропогенних/антропогенний антропоїдних/антропоїдний антропологічних/антропологічний абажурних/абажурний абазинських/абазинський абаканських/абаканський Абакумових/Абакумів абатських/абатський абераційних/абераційний абеткових/абетковий абіджанських/абіджанський абіогенних/абіогенний абісальних/абісальний абіссінських/абіссінський абітурієнтських/абітурієнтський аболіціоністських/аболіціоністський абонементних/абонементний (uk)</rdfs:comment>
        <rdfs:comment>e.g., најшпионска/шпионски, најшпионскава/шпионски, најшпионскана/шпионски, најшпионската/шпионски, најшпионски/шпионски, најшпионскиве/шпионски, најшпионскине/шпионски, најшпионскиов/шпионски, најшпионскион/шпионски (mk)</rdfs:comment>
        <rdfs:comment>&quot;Ordinal adjective&quot; is applied to Slovenian vrstni pridevniki and Ukrainian відносні прикметники. A more appropriate term would be relative adjective (Derzhanski and Kotsyba 2009).
In Macedonian MTE v.4, the term &quot;ordinal adjective&quot; designates ordinal numerals, e.g., prv, vtor (eng. first, second) (note on MTE v4 adjectives).
        This category is thus ambiguous between &quot;RelationalAdjective&quot; and &quot;OrdinalNumeral and Adjective&quot;</rdfs:comment>
    </owl:Class>
    


    <!-- http://purl.org/olia/mte/multext-east.owl#OrdinalNumeral -->

    <owl:Class rdf:about="http://purl.org/olia/mte/multext-east.owl#OrdinalNumeral">
        <rdfs:subClassOf rdf:resource="http://purl.org/olia/mte/multext-east.owl#Numeral"/>
        <rdfs:comment>e.g., -ntâi/întâi, -ntâia/întâi, -ntâiaşi/întâi, -ntâii/întâi, -ntâile/întâi, -ntâilor/întâi, -ntâiul/întâi, -ntâiului/întâi, dintâi (ro)</rdfs:comment>
        <rdfs:comment>e.g., czterdziestych/czterdziesty, czterdziestym/czterdziesty, czternaste/czternasty, czternastym/czternasty, czwarte/czwarty, czwartego/czwarty, czwartej/czwarty, czwartych/czwarty, czwartym/czwarty (pl)</rdfs:comment>
        <rdfs:comment>e.g., desátá/desátý, devatenácté/devatenáctý, devatenáctému/devatenáctý, devatenáctým/devatenáctý, dvacátých/dvacátý, jedenáctém/jedenáctý, miliónté/milióntý, osmatřicátém/osmatřicátý, osmdesátý (cs)</rdfs:comment>
        <rdfs:comment>e.g., esimesteks/esimene, esimestele/esimene, esimestena/esimene, esimestes/esimene, esimestest/esimene, teise/teine, teisega/teine, teisegi/teine, teiselt/teine (et)</rdfs:comment>
        <rdfs:comment>e.g., sehont/sagont, tretgna/trëtnji, tretgni/trëtnji, tretni/trëtnji, tretnji/trëtnji (sl-rozaj)</rdfs:comment>
        <rdfs:comment>e.g., tretej/tretí, tretia/tretí, tretie/tretí, tretieho/tretí, tretiemu/tretí, tretiu/tretí, tretí, tretích/tretí, tretím/tretí (sk)</rdfs:comment>
        <rdfs:comment>e.g., tretjim/tretji (sl)</rdfs:comment>
        <rdfs:comment>Numeral/Type=&quot;ordinal&quot;.

Ordinal (qualitative) numerals have an enumerating property, through which one can determine the consecutive position of an object in an ensemble of homogenous objects, e.g., Slovak prvý deň, druhý mesiac, tretia sekunda; Bulgarian първи ден, втори месец, трета секунда /first day, second month, third second/. (Dimitrova et al. 2009) Ordinal numerals often have the same inflectional characteristics as adjectives (Macedonian MTE v4)</rdfs:comment>
    </owl:Class>
    


    <!-- http://purl.org/olia/mte/multext-east.owl#OrthographicalRepresentationOfNumeral -->

    <owl:Class rdf:about="http://purl.org/olia/mte/multext-east.owl#OrthographicalRepresentationOfNumeral">
        <rdfs:subClassOf rdf:resource="http://purl.org/olia/mte/multext-east.owl#NumeralForm"/>
        <owl:versionInfo>NumeralForm conflates two different aspects that are made explicit here:
- OrthographicRepresentationOfNumeral: the orthographical representation of Numerals, and
- MorphologicalFormOfNumeral: morphological subclasses of Numeral as defined by their derivational morphology</owl:versionInfo>
    </owl:Class>
    


    <!-- http://purl.org/olia/mte/multext-east.owl#OtherInterjection -->

    <owl:Class rdf:about="http://purl.org/olia/mte/multext-east.owl#OtherInterjection">
        <rdfs:subClassOf rdf:resource="http://purl.org/olia/mte/multext-east.owl#Interjection"/>
        <rdfs:comment>Interjection/Type=&quot;other&quot; (Hungarian, as compared to Type=&quot;mood&quot;)</rdfs:comment>
    </owl:Class>
    


    <!-- http://purl.org/olia/mte/multext-east.owl#PartOfFixedExpression -->

    <owl:Class rdf:about="http://purl.org/olia/mte/multext-east.owl#PartOfFixedExpression">
        <rdfs:subClassOf rdf:resource="http://purl.org/olia/mte/multext-east.owl#Collocation"/>
        <rdfs:comment>
Some forms can only be used in a fixed context, e.g., polsku in po polsku. They are classified as special kinds of adjectives in the IPIC. In the MTE version this information is preserved in the status of a &quot;burkinostka&quot;. This term is devised by Magdalena Derwojedowa and refers to dependent words like Burkina which only make sense and can be morphosyntactically identified in a fixed combination (Burkina Faso).</rdfs:comment>
        <owl:versionInfo>Corresponds to MTE Burkinostka (Adverb/Clitic=&quot;burkinostka&quot;; Polish)
&quot;Burkinostka was a local joke :). IsPartOfFixedExpression, to be more precise. Or somehow shorter.&quot;
(Natalia Kotsyba, email 2010/06/21)</owl:versionInfo>
    </owl:Class>
    


    <!-- http://purl.org/olia/mte/multext-east.owl#Participle -->

    <owl:Class rdf:about="http://purl.org/olia/mte/multext-east.owl#Participle">
        <rdfs:subClassOf rdf:resource="http://purl.org/olia/mte/multext-east.owl#Adjective"/>
        <rdfs:subClassOf rdf:resource="http://purl.org/olia/mte/multext-east.owl#VerbForm"/>
        <rdfs:comment>e.g., 0, абеткована/абеткований авізована/авізований акомпанована/акомпанований актована/актований аналізована/аналізований анкетована/анкетований анодована/анодований артикульована/артикульований балотована/балотований балувана/балуваний бальзамована/бальзамований банітована/банітований багнітована/багнітований байцьована/байцьований балакана/балаканий бачена/бачений белетризована/белетризований бережена/бережений бетонована/бетонований бинтована/бинтований, абеткованая/абеткований авізованая/авізований акомпанованая/акомпанований актованая/актований аналізованая/аналізований анкетованая/анкетований анодованая/анодований артикульованая/артикульований балотованая/балотований балуваная/балуваний бальзамованая/бальзамований банітованая/банітований багнітованая/багнітований байцьованая/байцьований балаканая/балаканий баченая/бачений белетризованая/белетризований береженая/бережений бетонованая/бетонований бинтованая/бинтований, абетковане/абеткований авізоване/авізований акомпановане/акомпанований актоване/актований аналізоване/аналізований анкетоване/анкетований анодоване/анодований артикульоване/артикульований балотоване/балотований балуване/балуваний бальзамоване/бальзамований банітоване/банітований багнітоване/багнітований байцьоване/байцьований балакане/балаканий бачене/бачений белетризоване/белетризований бережене/бережений бетоноване/бетонований бинтоване/бинтований, абеткованеє/абеткований авізованеє/авізований акомпанованеє/акомпанований актованеє/актований аналізованеє/аналізований анкетованеє/анкетований анодованеє/анодований артикульованеє/артикульований балотованеє/балотований балуванеє/балуваний бальзамованеє/бальзамований банітованеє/банітований багнітованеє/багнітований байцьованеє/байцьований балаканеє/балаканий баченеє/бачений белетризованеє/белетризований береженеє/бережений бетонованеє/бетонований бинтованеє/бинтований, абеткований/= авізований/= акомпанований/= актований/= аналізований/= анкетований/= анодований/= артикульований/= балотований/= балуваний/= бальзамований/= банітований/= багнітований/= байцьований/= балаканий/= бачений/= белетризований/= бережений/= бетонований/= бинтований/=, абеткованим/абеткований авізованим/авізований акомпанованим/акомпанований актованим/актований аналізованим/аналізований анкетованим/анкетований анодованим/анодований артикульованим/артикульований балотованим/балотований балуваним/балуваний бальзамованим/бальзамований банітованим/банітований багнітованим/багнітований байцьованим/байцьований балаканим/балаканий баченим/бачений белетризованим/белетризований береженим/бережений бетонованим/бетонований бинтованим/бинтований, абеткованими/абеткований авізованими/авізований акомпанованими/акомпанований актованими/актований аналізованими/аналізований анкетованими/анкетований анодованими/анодований артикульованими/артикульований балотованими/балотований балуваними/балуваний бальзамованими/бальзамований банітованими/банітований багнітованими/багнітований байцьованими/байцьований балаканими/балаканий баченими/бачений белетризованими/белетризований береженими/бережений бетонованими/бетонований бинтованими/бинтований, абеткованих/абеткований авізованих/авізований акомпанованих/акомпанований актованих/актований аналізованих/аналізований анкетованих/анкетований анодованих/анодований артикульованих/артикульований балотованих/балотований балуваних/балуваний бальзамованих/бальзамований банітованих/банітований багнітованих/багнітований байцьованих/байцьований балаканих/балаканий бачених/бачений белетризованих/белетризований бережених/бережений бетонованих/бетонований бинтованих/бинтований (uk)</rdfs:comment>
        <rdfs:comment>e.g., abdykujący/abdykować, adoptujących/adoptować, akceptowanymi/akceptować, akredytujące/akredytować, akredytujących/akredytować, akredytującą/akredytować, analizowanych/analizować, awansującym/awansować, badanego/badać (pl)</rdfs:comment>
        <rdfs:comment>e.g., banaden/binidet, benedila/binidet, bil/bet, Bila/bet, bile/bet, bili/bet, bilo/bet, bilu/bet, bit/bet (sl-rozaj)</rdfs:comment>
        <rdfs:comment>e.g., been/be, being/be, doing/do, done/do, having/have (en)</rdfs:comment>
        <rdfs:comment>e.g., bila/biti, bile/biti, bilo/biti, bio/biti, htele/hteti, htelo/hteti, hteo/hteti, htio/htjeti, htjele/htjeti (sr)</rdfs:comment>
        <rdfs:comment>e.g., bila/biti, bilo/biti, navedenih/naveden (sl)</rdfs:comment>
        <rdfs:comment>e.g., bola/byť, boli/byť, bolo/byť, mala/mať, mali/mať, malo/mať, mohli/môcť, museli/musieť, nezvestovali/nezvestovať (sk)</rdfs:comment>
        <rdfs:comment>e.g., byl/být, byla/být, byli/být, bylo/být, byly/být, býval/bývat, bývala/bývat, bývali/bývat, bývalo/bývat (cs)</rdfs:comment>
        <rdfs:comment>e.g., oldud/olema, olev/olema, olnud/olema, olnudki/olema, peetav/pidama, saadav/saama, tunduv/tunduma, vormitud/vormima, vulkaniseeritud/vulkaniseerima (et)</rdfs:comment>
        <rdfs:comment>e.g., Заинтригованная/заинтриговывать, Звенящая/звенеть, Награжден/награждать, Разбитая/разбивать, Трясущейся/трястись, Убит/убивать, видимо/видеть, готовящаяся/готовить, имевшейся/иметься (ru)</rdfs:comment>
        <rdfs:comment>e.g., бидел/сум, бидела/сум, биделе/сум, бидело/сум, бидено/сум, бил/сум, била/сум, биле/сум, било/сум (mk)</rdfs:comment>
        <rdfs:comment>e.g., бил/бъда, бил/съм, била/бъда, била/съм, били/бъда, били/съм, било/бъда, било/съм, бъдещ/бъда (bg)</rdfs:comment>
        <rdfs:comment>e.g., توانسته/توانست, داده‌/داد برده/برده انداخته/انداخت, شده/شد, فروبرده/فروبرد باخته/باخت آراسته/آراست, مي‌جنگيده/جنگيد, مي‌شده/شد, مي‌نوشته/نوشت مي‌دانسته/دانست مي‌داده/داد, مي‌کرده/کرد, مي‌کرده/کرد مي‌داده/داد (fa)</rdfs:comment>
        <rdfs:comment>The concept Participle merges MTE v4 Verb/VForm=&quot;participle&quot; and Adjective/Type=&quot;participle&quot; that are used with partially overlapping extent:&lt;br/&gt;

Overlap with Adjective:
Czech adjectival active and passive participles, e.g. &quot;stojící&quot; (E. &quot;standing&quot;) or &quot;udělaný&quot; (E. &quot;performed&quot; or &quot;done&quot;, cf. Note 4 above) are classified as adjectives. (MTE v4)&lt;br/&gt;

Slovak: The &apos;past participle&apos; in Slovak is used for expressing compound active past Tense and is encoded as: Type=p(articiple), Tense=pa(s)t. (MTE v4)&lt;br/&gt;

Slovak/Bulgarian: Vform=participle(p) corresponds to Slovak L-participle, in Bulgarian called just the participle and is used to form the past tense or the conditional. In Bulgarian, it also includes past participle (говорено) /spoken/). (Dimitrova et al. 2009)&lt;br/&gt;

Macedonian: The passive participle is used in verbal forms with the auxiliary ima / nema (eng. to have, to have not). The verbal adjective, in case it is used out of this construction, is considered as separate lemma. (MTE v4)&lt;br/&gt;

Romanian participle and gerund mood permit an adjectival use. However, the adjectival use of gerund is extremely rare (o mână tremurndă - a shaking hand). (MTE v4)</rdfs:comment>
    </owl:Class>
    


    <!-- http://purl.org/olia/mte/multext-east.owl#ParticipleAdverb -->

    <owl:Class rdf:about="http://purl.org/olia/mte/multext-east.owl#ParticipleAdverb">
        <rdfs:subClassOf rdf:resource="http://purl.org/olia/mte/multext-east.owl#Adverb"/>
        <rdfs:comment>Adverb/Type=&quot;participle&quot; is used in the Slovene MTE v4 specs, e.g., &apos;leže&apos; / lying. Slovenian adverbial participles are, however, not attested for Resian. (MTE v4)</rdfs:comment>
    </owl:Class>
    


    <!-- http://purl.org/olia/mte/multext-east.owl#Particle -->

    <owl:Class rdf:about="http://purl.org/olia/mte/multext-east.owl#Particle">
        <rdfs:subClassOf rdf:resource="http://purl.org/olia/mte/multext-east.owl#MorphosyntacticCategory"/>
        <rdfs:comment>e.g., -a/a, -o, a, n-/nu, nu, o, s-/să, să (ro)</rdfs:comment>
        <rdfs:comment>e.g., -a/a, n-/nu (ro)</rdfs:comment>
        <rdfs:comment>e.g., dret/drët, ni/ni, pa/pa (sl-rozaj)</rdfs:comment>
        <rdfs:comment>e.g., już/już, nie/nie, tylko/tylko (pl)</rdfs:comment>
        <rdfs:comment>e.g., а_бе, дали, ей-сега, ей-тъй, ли, не, нима, нито (bg)</rdfs:comment>
        <rdfs:comment>e.g., або авжеж ага адже адже ж аж ажень але амінь ані ані-ні ато атож ачей аякже б ба бач би бігма (uk)</rdfs:comment>
        <rdfs:comment>Particle has an overlap with Adverb, see Adverb/Type=&quot;particle&quot; as used for Hungarian and Romanian MTE v4. In Slovak MTE v4, however, Particles form a separate part of speech category as is customary in Slovak grammars.

In the Slovak MTE tagset, we simplified our task enormously by resigning the classification attempts
(which can be analysed ad nauseam to an arbitrary precision (Šimková, 2004)), and all the articles have the
same simple tag P. (Dimitrova et al. 2009)</rdfs:comment>
    </owl:Class>
    


    <!-- http://purl.org/olia/mte/multext-east.owl#ParticleAdverb -->

    <owl:Class rdf:about="http://purl.org/olia/mte/multext-east.owl#ParticleAdverb">
        <rdfs:subClassOf rdf:resource="http://purl.org/olia/mte/multext-east.owl#Adverb"/>
        <rdfs:comment>e.g., ma&apos;/mai, to&apos;/tot (ro)</rdfs:comment>
        <rdfs:comment>Adverb/Type=&quot;particle&quot; is used in the Romanian and Hungarian MTE v4 specs.

In Romanian, the particle type covers those adverbs which can dislocate verbal compound forms (ex. Ea a tot cântat -- She has ever sung) or mark degrees (ex. circa (about), foarte (very), prea (too)). Such adverbs are cam, mai, prea, şi, tot, foarte etc. (MTE v4)</rdfs:comment>
    </owl:Class>
    


    <!-- http://purl.org/olia/mte/multext-east.owl#ParticleFormation -->

    <owl:Class rdf:about="http://purl.org/olia/mte/multext-east.owl#ParticleFormation">
        <rdfs:subClassOf rdf:resource="http://purl.org/olia/mte/multext-east.owl#Formation"/>
        <rdfs:comment>Particle/Formation refers to the graphical components: simple, i.e. consisting of one word; compound, i.e. consisting of more than one word. (MTE v4)</rdfs:comment>
    </owl:Class>
    


    <!-- http://purl.org/olia/mte/multext-east.owl#PartitiveCase -->

    <owl:Class rdf:about="http://purl.org/olia/mte/multext-east.owl#PartitiveCase">
        <rdfs:subClassOf rdf:resource="http://purl.org/olia/mte/multext-east.owl#Case"/>
        <rdfs:comment>e.g., endid/ise, meid/mina, mind/mina, neid/tema, neidki/tema, oma, omasid/oma, omi/oma, sind/sina (et)</rdfs:comment>
        <rdfs:comment>Case=&quot;partitive&quot; (Estonian)</rdfs:comment>
    </owl:Class>
    


    <!-- http://purl.org/olia/mte/multext-east.owl#PassiveVoice -->

    <owl:Class rdf:about="http://purl.org/olia/mte/multext-east.owl#PassiveVoice">
        <rdfs:subClassOf rdf:resource="http://purl.org/olia/mte/multext-east.owl#Voice"/>
        <rdfs:comment>e.g., akceptowanymi/akceptować, cytowanych/cytować, dyktowanym/dyktować, emitowanego/emitować, ilustrowanym/ilustrować, interpretowane/interpretować, nieakcentowanymi/akcentować, nieakceptowane/akceptować, nieakceptowanymi/akceptować (pl)</rdfs:comment>
        <rdfs:comment>e.g., bit/bet, nashanà/nistet, nárit/naredit (sl-rozaj)</rdfs:comment>
        <rdfs:comment>e.g., nestráveno/strávit (cs)</rdfs:comment>
        <rdfs:comment>e.g., peetaks/pidama, peetav/pidama, peetavat/pidama, peeti/pidama, saadavat/saama, ulatuvat/ulama, volitatuks/volitama, vormistatakse/vormistama, vormitud/vormima (et)</rdfs:comment>
        <rdfs:comment>Voice=&quot;passive&quot;&lt;br/&gt;

In Macedonian, two types of (adjectival) participles exist: active and passive. Active corresponds to Macedonian L-form and passive to verbal adjective, neuter gender, singular. For example, nosel is encoded as VForm=Participle, Voice=Active, nosen as VForm=participle, Voice=Passive. (MTE v4)</rdfs:comment>
    </owl:Class>
    


    <!-- http://purl.org/olia/mte/multext-east.owl#PastTense -->

    <owl:Class rdf:about="http://purl.org/olia/mte/multext-east.owl#PastTense">
        <rdfs:subClassOf rdf:resource="http://purl.org/olia/mte/multext-east.owl#Tense"/>
        <rdfs:comment>e.g., -nzestrarăm/înzestra, -nzestrarăţi/înzestra, -nzidirăm/înzidi, -nzidirăţi/înzidi, -nzorzonarăm/înzorzona, -nzorzonarăţi/înzorzona (ro)</rdfs:comment>
        <rdfs:comment>e.g., 0, абеткував/абеткувати авізував/авізувати агакав/агакати агітував/агітувати агонізував/агонізувати адвокатував/адвокатувати адміністрував/адмініструвати адоптувався/адоптуватися адоптувавсь/адоптуватися адсорбувався/адсорбуватися адсорбувавсь/адсорбуватися азотувався/азотуватися азотувавсь/азотуватися айкав/айкати акав/акати акомпанував/акомпанувати акредитувався/акредитуватися акредитувавсь/акредитуватися акторствував/акторствувати акторував/акторувати, абеткувавши/абеткувати авізувавши/авізувати агакавши/агакати агітувавши/агітувати агонізувавши/агонізувати адвокатувавши/адвокатувати адмініструвавши/адмініструвати адоптувавшись/адоптуватися адсорбувавшись/адсорбуватися азотувавшись/азотуватися айкавши/айкати акавши/акати акомпанувавши/акомпанувати акредитувавшись/акредитуватися акторствувавши/акторствувати акторувавши/акторувати актувавши/актувати акушерувавши/акушерувати акцентувавшись/акцентуватися альокавши/альокати, абеткувала/абеткувати авізувала/авізувати агакала/агакати агітувала/агітувати агонізувала/агонізувати адвокатувала/адвокатувати адмініструвала/адмініструвати адоптувалася/адоптуватися адоптувалась/адоптуватися адсорбувалася/адсорбуватися адсорбувалась/адсорбуватися азотувалася/азотуватися азотувалась/азотуватися айкала/айкати акала/акати акомпанувала/акомпанувати акредитувалася/акредитуватися акредитувалась/акредитуватися акторствувала/акторствувати акторувала/акторувати, абеткували/абеткувати авізували/авізувати агакали/агакати агітували/агітувати агонізували/агонізувати адвокатували/адвокатувати адміністрували/адмініструвати адоптувалися/адоптуватися адоптувались/адоптуватися адсорбувалися/адсорбуватися адсорбувались/адсорбуватися азотувалися/азотуватися азотувались/азотуватися айкали/айкати акали/акати акомпанували/акомпанувати акредитувалися/акредитуватися акредитувались/акредитуватися акторствували/акторствувати акторували/акторувати, абеткувало/абеткувати авізувало/авізувати агакало/агакати агітувало/агітувати агонізувало/агонізувати адвокатувало/адвокатувати адмініструвало/адмініструвати адоптувалося/адоптуватися адоптувалось/адоптуватися адсорбувалося/адсорбуватися адсорбувалось/адсорбуватися азотувалося/азотуватися азотувалось/азотуватися айкало/айкати акало/акати акомпанувало/акомпанувати акредитувалося/акредитуватися акредитувалось/акредитуватися акторствувало/акторствувати акторувало/акторувати, аблактував/аблактувати абонував/абонувати абонувався/абонуватися абонувавсь/абонуватися абордував/абордувати абортував/абортувати абсолютизував/абсолютизувати абсолютизувався/абсолютизуватися абсолютизувавсь/абсолютизуватися абсорбував/абсорбувати абсорбувався/абсорбуватися абсорбувавсь/абсорбуватися абстрагував/абстрагувати абстрагувався/абстрагуватися абстрагувавсь/абстрагуватися абшитував/абшитувати авансував/авансувати авансувався/авансуватися авансувавсь/авансуватися автоматизував/автоматизувати, аблактувавши/аблактувати абонувавши/абонувати абонувавшись/абонуватися абордувавши/абордувати абортувавши/абортувати абсолютизувавши/абсолютизувати абсолютизувавшись/абсолютизуватися абсорбувавши/абсорбувати абсорбувавшись/абсорбуватися абстрагувавши/абстрагувати абстрагувавшись/абстрагуватися абшитувавши/абшитувати авансувавши/авансувати авансувавшись/авансуватися автоматизувавши/автоматизувати автоматизувавшись/автоматизуватися авторизувавши/авторизувати аглютинувавши/аглютинувати аглютинувавшись/аглютинуватися агрегатувавши/агрегатувати, аблактувала/аблактувати абонувала/абонувати абонувалася/абонуватися абонувалась/абонуватися абордувала/абордувати абортувала/абортувати абсолютизувала/абсолютизувати абсолютизувалася/абсолютизуватися абсолютизувалась/абсолютизуватися абсорбувала/абсорбувати абсорбувалася/абсорбуватися абсорбувалась/абсорбуватися абстрагувала/абстрагувати абстрагувалася/абстрагуватися абстрагувалась/абстрагуватися абшитувала/абшитувати авансувала/авансувати авансувалася/авансуватися авансувалась/авансуватися автоматизувала/автоматизувати (uk)</rdfs:comment>
        <rdfs:comment>e.g., bałoś/bać, byli/być, byliście/być, byliśmy/być, bywały/bywać, był/być, była/być, byłam/być, byłaś/być (pl)</rdfs:comment>
        <rdfs:comment>e.g., been/be, done/do, was/be, wasn&apos;t/be+not, wass/be, were/be, weren&apos;t/be+not (en)</rdfs:comment>
        <rdfs:comment>e.g., benedila/binidet, bil/bet, Bila/bet, bile/bet, bili/bet, bilo/bet, bilu/bet, biu/bet, blíshghnili/blïžnjit (sl-rozaj)</rdfs:comment>
        <rdfs:comment>e.g., bila/biti, bile/biti, bilo/biti, bio/biti, htele/hteti, htelo/hteti, hteo/hteti, htio/htjeti, htjele/htjeti (sr)</rdfs:comment>
        <rdfs:comment>e.g., bola/byť, boli/byť, bolo/byť, mala/mať, mali/mať, malo/mať, mohli/môcť, museli/musieť, nezvestovali/nezvestovať (sk)</rdfs:comment>
        <rdfs:comment>e.g., byl/být, byla/být, byli/být, bylo/být, byly/být, býval/bývat, bývala/bývat, bývali/bývat, bývalo/bývat (cs)</rdfs:comment>
        <rdfs:comment>e.g., elárultalak/elárul, figyelmeztettelek/figyelmeztet, megismertelek/megismer (hu)</rdfs:comment>
        <rdfs:comment>e.g., oldud/olema, olnud/olema, olnudki/olema, olnuks/olema, olnukski/olema, polnuks/olema, ulatuvat/ulama, volitatuks/volitama, vormitud/vormima (et)</rdfs:comment>
        <rdfs:comment>e.g., Заинтригованная/заинтриговывать, Награжден/награждать, Разбитая/разбивать, Толпившиеся/толпиться, Убит/убивать, Ушибленная/ушибать, Уязвленное/уязвлять, Эвакуированные/эвакуировать, Экономила/экономить (ru)</rdfs:comment>
        <rdfs:comment>e.g., централизираното/централизирам, цитираното/цитирам, червеното/червя (bg)</rdfs:comment>
        <rdfs:comment>e.g., آمديد/آمد, آمديم/آمد, برآورد انداخت انجاميد, برمي‌داشتيد/برداشت, بودي/بود, بوديد/بود, بوديد/بود بودي/بود, بوديم/بود, توانست (fa)</rdfs:comment>
        <rdfs:comment>Tense=&quot;past&quot; (Ukrainian also for adjectives)</rdfs:comment>
    </owl:Class>
    


    <!-- http://purl.org/olia/mte/multext-east.owl#PaucalNumber -->

    <owl:Class rdf:about="http://purl.org/olia/mte/multext-east.owl#PaucalNumber">
        <rdfs:subClassOf rdf:resource="http://purl.org/olia/mte/multext-east.owl#Number"/>
        <rdfs:comment>Number=&quot;paucal&quot; (Serbian Verb)&lt;br/&gt;

PaucalNumber is a form used with numerals from 2 to 4 (cf. PaucalQuantifier). (Ivan A. Derzhanski, email 2010/06/16)</rdfs:comment>
    </owl:Class>
    


    <!-- http://purl.org/olia/mte/multext-east.owl#PaucalQuantifier -->

    <owl:Class rdf:about="http://purl.org/olia/mte/multext-east.owl#PaucalQuantifier">
        <rdfs:subClassOf rdf:resource="http://purl.org/olia/mte/multext-east.owl#NumeralAgreementClass"/>
        <rdfs:comment>In many Slavic languages, numerals between 2 and 4 (and some quantifiers) involve a specific agreement patterns that is different from that of smaller and greater numbers. In Russian, for example, genitive singular is requires. These numerals and quantifiers with the same characteristics are referred to here as &quot;paucal quantifiers&quot;.
(cf. David Pesetsky, http://www.uni-leipzig.de/~jtrommer/Harvard/pesetsky.pdf)</rdfs:comment>
        <owl:versionInfo>Introduced as a generalization over MTE Numeral/Class=&quot;definite234&quot; and Numeral/Class=&quot;definite34&quot;. These features are used in Polish, Czech and Slovak, but used differently: Slovak &quot;definite234&quot; and Polish &quot;definite34&quot; are applied to numerals 2,3 and 4 (distinguished from PluralQuantifier and SingularQuantifier), whereas Czech &quot;definite34&quot; is applied to numerals 3 and 4 only (distingushed from PluralQuantifier, SingularQuantifier and DualQuantifier).</owl:versionInfo>
    </owl:Class>
    


    <!-- http://purl.org/olia/mte/multext-east.owl#PerfectiveAspect -->

    <owl:Class rdf:about="http://purl.org/olia/mte/multext-east.owl#PerfectiveAspect">
        <rdfs:subClassOf rdf:resource="http://purl.org/olia/mte/multext-east.owl#Aspect"/>
        <rdfs:comment>e.g., abdykujący/abdykować, adoptujących/adoptować, akredytujące/akredytować, akredytujących/akredytować, akredytującą/akredytować, awansującym/awansować, da/dać, daj/dać, dajcie/dać (pl)</rdfs:comment>
        <rdfs:comment>e.g., accompagnaimu/akompanjät, amai/amät, aman/amät, banaden/binidet, benedila/binidet, bramase/bramät, comsumano/konsumät, contemplaimo/kontemplät, coronana/koronät (sl-rozaj)</rdfs:comment>
        <rdfs:comment>e.g., ispala/ispasti, izdala/izdati, okrete/okrenuti, razdra/razdrati, sažvaće/sažvakati, ukočen/ukočiti, uspeo/uspeti, zastrasmo/zastrijeti, zastraste/zastrijeti (sr)</rdfs:comment>
        <rdfs:comment>e.g., nežmurkneme/nežmurknúť, nežmurknete/nežmurknúť, nežmurknime/nežmurknúť, nežmurknite/nežmurknúť, nežmurknúc/nežmurknúť, nežuchneme/nežuchnúť, nežuchnete/nežuchnúť, nežuchnime/nežuchnúť, nežuchnite/nežuchnúť (sk)</rdfs:comment>
        <rdfs:comment>e.g., Вернемся/вернуться, Возьмем/взять, Выпьем/выпить, Заинтригованная/заинтриговывать, Затошнило/затошнить, Награжден/награждать, Разбитая/разбивать, Убедитесь/убедиться, Убит/убивать (ru)</rdfs:comment>
        <rdfs:comment>e.g., агакне/агакнути айкне/айкнути арештує/арештувати ахне/ахнути бабахне/бабахнути бабахнеться/бабахнутися бамкне/бамкнути бахне/бахнути бахнеться/бахнутися бацне/бацнути бебевхне/бебевхнути бебехне/бебехнути бебехнеться/бебехнутися бевкне/бевкнути бекне/бекнути белькне/белькнути бемкне/бемкнути беркицне/беркицнути беркицнеться/беркицнутися беркицьне/беркицьнути, агакнемо/агакнути агакнем/агакнути айкнемо/айкнути айкнем/айкнути арештуємо/арештувати арештуєм/арештувати ахнемо/ахнути ахнем/ахнути бабахнемо/бабахнути бабахнем/бабахнути бабахнемося/бабахнутися бабахнемось/бабахнутися бабахнемся/бабахнутися бамкнемо/бамкнути бамкнем/бамкнути бахнемо/бахнути бахнем/бахнути бахнемося/бахнутися бахнемось/бахнутися бахнемся/бахнутися, агакнете/агакнути айкнете/айкнути арештуєте/арештувати ахнете/ахнути бабахнете/бабахнути бабахнетеся/бабахнутися бабахнетесь/бабахнутися бамкнете/бамкнути бахнете/бахнути бахнетеся/бахнутися бахнетесь/бахнутися бацнете/бацнути бебевхнете/бебевхнути бебехнете/бебехнути бебехнетеся/бебехнутися бебехнетесь/бебехнутися бевкнете/бевкнути бекнете/бекнути белькнете/белькнути бемкнете/бемкнути, агакнеш/агакнути айкнеш/айкнути арештуєш/арештувати ахнеш/ахнути бабахнеш/бабахнути бабахнешся/бабахнутися бамкнеш/бамкнути бахнеш/бахнути бахнешся/бахнутися бацнеш/бацнути бебевхнеш/бебевхнути бебехнеш/бебехнути бебехнешся/бебехнутися бевкнеш/бевкнути бекнеш/бекнути белькнеш/белькнути бемкнеш/бемкнути беркицнеш/беркицнути беркицнешся/беркицнутися беркицьнеш/беркицьнути, агакни/агакнути айкни/айкнути арештуй/арештувати ахни/ахнути бабахни/бабахнути бабахнися/бабахнутися бабахнись/бабахнутися бамкни/бамкнути бахни/бахнути бахнися/бахнутися бахнись/бахнутися бацни/бацнути бебевхни/бебевхнути бебехни/бебехнути бебехнися/бебехнутися бебехнись/бебехнутися бевкни/бевкнути бекни/бекнути белькни/белькнути бемкни/бемкнути, агакну/агакнути айкну/айкнути арештую/арештувати ахну/ахнути бабахну/бабахнути бабахнуся/бабахнутися бабахнусь/бабахнутися бамкну/бамкнути бахну/бахнути бахнуся/бахнутися бахнусь/бахнутися бацну/бацнути бебевхну/бебевхнути бебехну/бебехнути бебехнуся/бебехнутися бебехнусь/бебехнутися бевкну/бевкнути бекну/бекнути белькну/белькнути бемкну/бемкнути, агакнув/агакнути айкнув/айкнути арештував/арештувати ахнув/ахнути бабахнув/бабахнути бабахнувся/бабахнутися бабахнувсь/бабахнутися бамкнув/бамкнути бахнув/бахнути бахнувся/бахнутися бахнувсь/бахнутися бацнув/бацнути бебевхнув/бебевхнути бебехнув/бебехнути бебехнувся/бебехнутися бебехнувсь/бебехнутися бевкнув/бевкнути бекнув/бекнути белькнув/белькнути бемкнув/бемкнути, агакнувши/агакнути айкнувши/айкнути арештувавши/арештувати ахнувши/ахнути бабахнувши/бабахнути бабахнувшись/бабахнутися бамкнувши/бамкнути бахнувши/бахнути бахнувшись/бахнутися бацнувши/бацнути бебевхнувши/бебевхнути бебехнувши/бебехнути бебехнувшись/бебехнутися бевкнувши/бевкнути бекнувши/бекнути белькнувши/белькнути бемкнувши/бемкнути беркицнувши/беркицнути беркицнувшись/беркицнутися беркицьнувши/беркицьнути, агакнула/агакнути айкнула/айкнути арештувала/арештувати ахнула/ахнути бабахнула/бабахнути бабахнулася/бабахнутися бабахнулась/бабахнутися бамкнула/бамкнути бахнула/бахнути бахнулася/бахнутися бахнулась/бахнутися бацнула/бацнути бебевхнула/бебевхнути бебехнула/бебехнути бебехнулася/бебехнутися бебехнулась/бебехнутися бевкнула/бевкнути бекнула/бекнути белькнула/белькнути бемкнула/бемкнути (uk)</rdfs:comment>
        <rdfs:comment>e.g., недоспаа/недоспие, недоспав/недоспие, недоспавме/недоспие, недоспавте/недоспие, недоспиев/недоспие, недоспиевме/недоспие, недоспиевте/недоспие, недоспиеме/недоспие, недоспиено/недоспие (mk)</rdfs:comment>
        <rdfs:comment>Aspect=&quot;perfective&quot; (Noun: Polish; Verb: Slavic; Adjective: Polish, Ukrainian)

In Slavic aspectology, Russian aspect is usually considered to be a binary category, i.e., every Russian verb form is either perfective or imperfective. Only imperfective verbs can combine with the auxiliary быть &apos;be&apos; in the analytic future construction, e.g. 

(1)  Когда-нибудь я буду писать как Hабоков.
Sometime I will write like Nabokov
&apos;I will write like Nabokov one day.&apos;

The synthetic future tense is restricted to perfective verbs, e.g.

(2) Я позвоню тебе.
I callFUTURE you
&apos;I&apos;ll call you.&apos;

There is the syntactic restriction that only imperfective verbs combine with phase verbs. In Russian, verbs like начинать / начать &apos;begin&apos;, продолжать / продолжить &apos;continue&apos; or кончать / кончить &apos;stop/finish&apos; can only take an imperfective infinitive as a complement. (Feldman &amp; Arshavskaya 2007)

Anna Feldman &amp; Katya Arshavskaya (2007), English and Russian event annotation: A pilot study. Studies in Variation, Contacts and Change in English 1, http://www.helsinki.fi/varieng/journal/volumes/01/feldman_arshavskaya/</rdfs:comment>
    </owl:Class>
    


    <!-- http://purl.org/olia/mte/multext-east.owl#Person -->

    <owl:Class rdf:about="http://purl.org/olia/mte/multext-east.owl#Person">
        <rdfs:subClassOf rdf:resource="http://purl.org/olia/mte/multext-east.owl#MorphosyntacticFeature"/>
    </owl:Class>
    


    <!-- http://purl.org/olia/mte/multext-east.owl#PersonOfObject -->

    <owl:Class rdf:about="http://purl.org/olia/mte/multext-east.owl#PersonOfObject">
        <rdfs:subClassOf rdf:resource="http://purl.org/olia/mte/multext-east.owl#Definiteness"/>
        <rdfs:comment>Hungarian verbs ... [have] two conjugations: definite and indefinite.&lt;br/&gt;

The indefinite conjugation is used:
   1. With an intransitive verb
   2. With an indefinite object including an indefinite pronoun object
   3. With most question words as the object
   4. With a relative pronoun as the object
   5. With a 1st or 2nd person pronoun as the object, whether stated or unstated&lt;br/&gt;

The definite conjugation is used:
   1. With a definite object
   2. With a following clause with hogy (&quot;that&quot;)
   3. With questions with melyik and hányadik (&quot;which&quot;) as the object
   4. With a 3rd person pronoun as the object, whether stated or unstated
(http://en.wikipedia.org/wiki/Hungarian_grammar_(verbs)#Definite_and_indefinite_conjugations, 2010/06/18)&lt;br/&gt;

The term `conjugation&apos;, while traditional, is confusing here:  it normally refers to a paradigmatic class, not to part of a lexeme&apos;s paradigm.
What Hungarian has in fact is limited marking of the person of the direct object (object agreement) in the verb, with the caveat that a 3rd person object is only marked if it is definite, a 2nd person object is only marked if the subject is 1st person singular, and a 1st person object is never marked.
(Ivan A. Derzhanski, email 2010/06/18)</rdfs:comment>
        <owl:versionInfo>The term `conjugation&apos;, while traditional, is confusing here: it normally refers to a paradigmatic class, not to part of a lexeme&apos;s paradigm.
Why not just `object&apos;?  (`person of object&apos; is too verbose.)
(Ivan A. Derzhanski, email 2010/06/18)&lt;br/&gt;

</owl:versionInfo>
        <owl:versionInfo>introduced to distangle the different functions of MTE v4 Definiteness</owl:versionInfo>
    </owl:Class>
    


    <!-- http://purl.org/olia/mte/multext-east.owl#PersonalPronoun -->

    <owl:Class rdf:about="http://purl.org/olia/mte/multext-east.owl#PersonalPronoun">
        <rdfs:subClassOf rdf:resource="http://purl.org/olia/mte/multext-east.owl#Pronoun"/>
        <rdfs:comment>e.g., &apos;Em/them, thee/you, them, they, thou (en)</rdfs:comment>
        <rdfs:comment>e.g., -te/tu, dumitale/dumneata, dumneavoastră, matale/mata, te-/tu, te/tu, tine/tu (ro)</rdfs:comment>
        <rdfs:comment>e.g., bennetek/ti, benneteket/ti, bennünket/ti, engemet/én, minket/mi, nektek/ti, nálatok/ti, Rajta/ő, rajtad/te (hu)</rdfs:comment>
        <rdfs:comment>e.g., meilt/mina, meist/mina, meistki/mina, minult/mina, minust/mina, minustki/mina, minutagi/mina, mult/mina, must/mina (et)</rdfs:comment>
        <rdfs:comment>e.g., tabe/tï, taêbô/tï, te/tï, ti/tï, to/to, tobe/tï, tè/tï, tí/tï (sl-rozaj)</rdfs:comment>
        <rdfs:comment>e.g., te/ti, tebe/ti, tebi/ti, tobom/ti (sr)</rdfs:comment>
        <rdfs:comment>e.g., teba/ty, tebe/ty, tebou/ty, ti/ty (sk)</rdfs:comment>
        <rdfs:comment>e.g., tebe/ty, tebou/ty, ti/ty, tobě/ty, tys/ty, tě/ty (cs)</rdfs:comment>
        <rdfs:comment>e.g., teboj/ti, ti/= (sl)</rdfs:comment>
        <rdfs:comment>e.g., tobie/ty, tobą/ty, ty/ty (pl)</rdfs:comment>
        <rdfs:comment>Pronoun/Type=&quot;personal&quot; and Pronoun/Referent_Type=&quot;personal&quot;</rdfs:comment>
    </owl:Class>
    


    <!-- http://purl.org/olia/mte/multext-east.owl#PluperfectTense -->

    <owl:Class rdf:about="http://purl.org/olia/mte/multext-east.owl#PluperfectTense">
        <rdfs:subClassOf rdf:resource="http://purl.org/olia/mte/multext-east.owl#Tense"/>
        <rdfs:comment>e.g., -nzestrasem/înzestra, -nzestraseră/înzestra, -nzestraserăm/înzestra, -nzestraserăţi/înzestra, -nzestraseşi/înzestra, -nzidisem/înzidi, -nzidiseră/înzidi, -nzidiserăm/înzidi, -nzidiserăţi/înzidi (ro)</rdfs:comment>
        <rdfs:comment>Tense=&quot;pluperfect&quot;</rdfs:comment>
    </owl:Class>
    


    <!-- http://purl.org/olia/mte/multext-east.owl#PluralNumber -->

    <owl:Class rdf:about="http://purl.org/olia/mte/multext-east.owl#PluralNumber">
        <rdfs:subClassOf rdf:resource="http://purl.org/olia/mte/multext-east.owl#Number"/>
        <rdfs:comment>e.g., &apos;Em/them, others, their, theirs, them, themselves, they, thou, viscounts/viscount (en)</rdfs:comment>
        <rdfs:comment>e.g., -astea/ăsta, -istele, -istelor, -iştii, -iştilor, -nsutitelor/însutit, -nsutiţilor/însutit, -ntregi/întreg, -ntreitelor/întreit (ro)</rdfs:comment>
        <rdfs:comment>e.g., absolwentów/absolwent, adoptujących/adoptować, akceptowanymi/akceptować, akredytujące/akredytować, akredytujących/akredytować, autorzy/autor, bogatszych/bogaty, ci/ten, cytowanych/cytować (pl)</rdfs:comment>
        <rdfs:comment>e.g., abyste/aby, budete/být, byste/by, chceme/chtít, chcete/chtít, dejte/dát, desaterým/desaterý, desátá/desátý, devatenácté/devatenáctý (cs)</rdfs:comment>
        <rdfs:comment>e.g., akiktől/aki, amelyekért/amely, azoktól/az, bennetek/ti, benneteket/ti, bennünket/ti, betegségünktől/betegség, borúlátónkat/borúlátó, buktatóin/buktató (hu)</rdfs:comment>
        <rdfs:comment>e.g., aktuaalseimatesse/aktuaalseim, Baltimaadel/Baltimaad, Baltimaades/Baltimaad, endilt/ise, endist/ise, esimesteks/esimene, esimestele/esimene, esimestena/esimene, esimestes/esimene (et)</rdfs:comment>
        <rdfs:comment>e.g., amaite/amät, bodete/bet, bodite/bet, bota/bet, Ciete/tët, Comandatmiteh/komandament, contemplaimo/kontemplät, costi/kust, datte/dät (sl-rozaj)</rdfs:comment>
        <rdfs:comment>e.g., biste/biti, bićete/biti, dvadesetora/dvadesetoro, htednimo/hteti, htele/hteti, htjednimo/htjeti, htjele/htjeti, jeste/jesam, Ketrin (sr)</rdfs:comment>
        <rdfs:comment>e.g., bodite/biti, boste/biti, hočejo/hoteti, imate/imeti, katere/kateri, katerih/kateri, katerim/kateri, katerimi/kateri, nekaterim/nekateri (sl)</rdfs:comment>
        <rdfs:comment>e.g., budete/byť, buďte/byť, hentie/henten, hentie/hento, hentie/hentá, hentí/henten, hentých/henten, hentých/hento, hentých/hentá (sk)</rdfs:comment>
    </owl:Class>
    


    <!-- http://purl.org/olia/mte/multext-east.owl#PluralQuantifier -->

    <owl:Class rdf:about="http://purl.org/olia/mte/multext-east.owl#PluralQuantifier">
        <rdfs:subClassOf rdf:resource="http://purl.org/olia/mte/multext-east.owl#NumeralAgreementClass"/>
        <rdfs:comment>A PluralQuantifier is a Quantifier (or Numeral) that specifies a large multitude of entities. The agreement pattern of a plural quantifier is different from that or an singular quantifier, but as opposed to DualQuantifier and PaucalQuantifier, PluralQuantifier includes quantifiers that denote arbitrarily large sets of entities.
(Chiarcos)

The corresponding category in Czech, Polish and Slovak MTE v4 specs is Numeral/Class=&quot;definite&quot;, that refers to numerals larger than four. (MTE v4)</rdfs:comment>
        <owl:versionInfo>Corresponds to MTE v4 Numeral/Class=&quot;definite&quot;. Renamed in accordance with SingularQuantifier, DualQuantifier and PaucalQuantifier.
After the current &quot;Numeral&quot; is renamed to &quot;Quantifier&quot;, Numeral/Class=&quot;definite&quot;, Numeral/Class=&quot;definite1&quot;, Numeral/Class=&quot;definite234&quot; etc. refer to specific patterns of congruency with Slavic numerals that originate from the difference between Old Slavic singular (definite1), dual (definite2, definite234) and plural (definite).</owl:versionInfo>
    </owl:Class>
    


    <!-- http://purl.org/olia/mte/multext-east.owl#PortmanteauAdverb -->

    <owl:Class rdf:about="http://purl.org/olia/mte/multext-east.owl#PortmanteauAdverb">
        <rdfs:subClassOf rdf:resource="http://purl.org/olia/mte/multext-east.owl#Adverb"/>
        <rdfs:comment>For Romanian, Adverb/Type=&quot;portmanteau&quot; was introduced to cover some few words which can be both adverbs and conjunctions (with adverbial reading more frequent). This was necessary for tagging purposes. (MTE v4)</rdfs:comment>
    </owl:Class>
    


    <!-- http://purl.org/olia/mte/multext-east.owl#PortmanteauConjunction -->

    <owl:Class rdf:about="http://purl.org/olia/mte/multext-east.owl#PortmanteauConjunction">
        <rdfs:subClassOf rdf:resource="http://purl.org/olia/mte/multext-east.owl#CoordinatingConjunction"/>
        <rdfs:comment>Conjunction/Type=&quot;portmanteau&quot; (Romanian)&lt;br/&gt;

Romanian: The &quot;portmanteau&quot; type of conjunction applies only to the word &quot;şi&quot; which can be both a coordonating conjunction and an adverb. The distinction among these interpretations is rather tricky for the average native speaker and was a constant source of noise in automatic tagging. Therefore, for the sake of automatic processing we defined this &quot;portmanteau&quot; type value. (MTE v4)</rdfs:comment>
    </owl:Class>
    


    <!-- http://purl.org/olia/mte/multext-east.owl#PositiveDegree -->

    <owl:Class rdf:about="http://purl.org/olia/mte/multext-east.owl#PositiveDegree">
        <rdfs:subClassOf rdf:resource="http://purl.org/olia/mte/multext-east.owl#Degree"/>
        <rdfs:comment>e.g., &apos;Ow, how, when, where, whereupon, why (en)</rdfs:comment>
        <rdfs:comment>e.g., -, bensőnkben/benső, borúlátónkat/borúlátó, buktatóin/buktató, csigaformákba/csigaformá, derekukkal/derék, derekukra/derék, dolgozóiból/dolgozó, dolgozójukba/dolgozó (hu)</rdfs:comment>
        <rdfs:comment>e.g., -ntrebătoare/întrebător, -ntregi/întreg, -ntreprinzătoare/întreprinzător, -nvăluitoare/învăluitor, -nzestrata/înzestrat, -nzestrate/înzestrat, -nzestratei/înzestrat, -nzestratele/înzestrat, -nzestratelor/înzestrat (ro)</rdfs:comment>
        <rdfs:comment>e.g., amerykański/amerykański, amerykańskiej/amerykański, amerykańskim/amerykański, bardzo/bardzo, bieżącym/bieżący, całego/cały, całej/cały, całemu/cały, cały/cały (pl)</rdfs:comment>
        <rdfs:comment>e.g., belim/beo, bezbrojnih/bezbrojni, devetogodišnji, evroazijskih/evroazijski, evroazijskog/evroazijski, Faroskih/Faroska, francuski, gipsani/gipsan, Goldštajnov (sr)</rdfs:comment>
        <rdfs:comment>e.g., blishgnaha/blïžnji, Bohavei/böguw, Bohouv/böguw, Bohovaha/böguw, Bohove/böguw, Bohovih/böguw, Bohovij/böguw, Bohovin/böguw, Bohuvin/böguw (sl-rozaj)</rdfs:comment>
        <rdfs:comment>e.g., brillská/brillský, neznámo/neznámý, samo/sám, samy/sám, zamaštěnýma/zamaštěný, zavřenýma/zavřený, zkříženýma/zkřížený (cs)</rdfs:comment>
        <rdfs:comment>e.g., dušikovima/dušikov, Marsovi/Marsov, navedenih/naveden (sl)</rdfs:comment>
        <rdfs:comment>e.g., rõivavalmistajateni/rõivavalmistaja, vanadelt/vana, vastastikustelt/vastastikune, veealustena/veealune, veidratesse/veider, vertikaalseina/vertikaalne, vibutajatesse/vibutaja, vokaalsetest/vokaalne, volitavateks/volitav (et)</rdfs:comment>
        <rdfs:comment>e.g., žurnálového/žurnálový, žurnálovému/žurnálový, žuvacieho/žuvací, žuvaciemu/žuvací, žúžoľového/žúžoľový, žúžoľovému/žúžoľový (sk)</rdfs:comment>
        <rdfs:comment>e.g., Чертова/чертовый, Швейцарских/швейцарский, Язвительно/язвительный, га, микро, участковым/участковый, фен, форсированным/форсированный, частным/частный (ru)</rdfs:comment>
        <rdfs:comment>e.g., аварійно небезпечна/аварійно небезпечний азартна/азартний активна/активний актуальна/актуальний амбітна/амбітний амбіційна/амбіційний амбіціозна/амбіціозний апетитна/апетитний ароматна/ароматний багата/багатий багатозначна/багатозначний бадьора/бадьорий бажана/бажаний балаклива/балакливий балакуча/балакучий безпечна/безпечний безумна/безумний бентежна/бентежний бережлива/бережливий бідна/бідний, аварійно небезпечная/аварійно небезпечний азартная/азартний активная/активний актуальная/актуальний амбітная/амбітний амбіційная/амбіційний амбіціозная/амбіціозний апетитная/апетитний ароматная/ароматний багатая/багатий багатозначная/багатозначний бадьорая/бадьорий бажаная/бажаний балакливая/балакливий балакучая/балакучий безпечная/безпечний безумная/безумний бентежная/бентежний бережливая/бережливий бідная/бідний, аварійно небезпечне/аварійно небезпечний азартне/азартний активне/активний актуальне/актуальний амбітне/амбітний амбіційне/амбіційний амбіціозне/амбіціозний апетитне/апетитний ароматне/ароматний багате/багатий багатозначне/багатозначний бадьоре/бадьорий бажане/бажаний балакливе/балакливий балакуче/балакучий безпечне/безпечний безумне/безумний бентежне/бентежний бережливе/бережливий бідне/бідний, аварійно небезпечнеє/аварійно небезпечний азартнеє/азартний активнеє/активний актуальнеє/актуальний амбітнеє/амбітний амбіційнеє/амбіційний амбіціознеє/амбіціозний апетитнеє/апетитний ароматнеє/ароматний багатеє/багатий багатозначнеє/багатозначний бадьореє/бадьорий бажанеє/бажаний балакливеє/балакливий балакучеє/балакучий безпечнеє/безпечний безумнеє/безумний бентежнеє/бентежний бережливеє/бережливий біднеє/бідний, аварійно небезпечний/= азартний/= активний/= актуальний/= амбітний/= амбіційний/= амбіціозний/= апетитний/= ароматний/= багатий/= багатозначний/= бадьорий/= бажаний/= балакливий/= балакучий/= безпечний/= безумний/= бентежний/= бережливий/= бідний/=, аварійно небезпечним/аварійно небезпечний азартним/азартний активним/активний актуальним/актуальний амбітним/амбітний амбіційним/амбіційний амбіціозним/амбіціозний апетитним/апетитний ароматним/ароматний багатим/багатий багатозначним/багатозначний бадьорим/бадьорий бажаним/бажаний балакливим/балакливий балакучим/балакучий безпечним/безпечний безумним/безумний бентежним/бентежний бережливим/бережливий бідним/бідний, аварійно небезпечними/аварійно небезпечний азартними/азартний активними/активний актуальними/актуальний амбітними/амбітний амбіційними/амбіційний амбіціозними/амбіціозний апетитними/апетитний ароматними/ароматний багатими/багатий багатозначними/багатозначний бадьорими/бадьорий бажаними/бажаний балакливими/балакливий балакучими/балакучий безпечними/безпечний безумними/безумний бентежними/бентежний бережливими/бережливий бідними/бідний, аварійно небезпечних/аварійно небезпечний азартних/азартний активних/активний актуальних/актуальний амбітних/амбітний амбіційних/амбіційний амбіціозних/амбіціозний апетитних/апетитний ароматних/ароматний багатих/багатий багатозначних/багатозначний бадьорих/бадьорий бажаних/бажаний балакливих/балакливий балакучих/балакучий безпечних/безпечний безумних/безумний бентежних/бентежний бережливих/бережливий бідних/бідний, аварійно небезпечного/аварійно небезпечний азартного/азартний активного/активний актуального/актуальний амбітного/амбітний амбіційного/амбіційний амбіціозного/амбіціозний апетитного/апетитний ароматного/ароматний багатого/багатий багатозначного/багатозначний бадьорого/бадьорий бажаного/бажаний балакливого/балакливий балакучого/балакучий безпечного/безпечний безумного/безумний бентежного/бентежний бережливого/бережливий бідного/бідний (uk)</rdfs:comment>
        <rdfs:comment>e.g., ски (mk)</rdfs:comment>
        <rdfs:comment>e.g., تازه تار بسيج, خيره تمام‌وقت بي‌شک, رنگيِ/رنگي بي‌امانِ/بي‌امان بوکسورمانندِ/بوکسورمانند, زنگداري/زنگدار تهوع‌آوري/تهوع‌آور برهنه‌اي/برهنه, سرگرمِ/سرگرم روانهٔ/روانه حاويِ/حاوي, موذي عاري سبيلو, پشتِ/پشت صرفِ/صرف جلويِ/جلو (fa)</rdfs:comment>
        <rdfs:comment>Degree=&quot;positive&quot; designates PositiveDegree, but also the absence of morphological degree markers. In English, for example, many comparatives and superlatives are formed with more/most, so that &quot;positive&quot; in this context cannot be interpreted as &quot;neither comparative nor superlative&quot;. (MTE v4)</rdfs:comment>
    </owl:Class>
    


    <!-- http://purl.org/olia/mte/multext-east.owl#PositiveSubordinatingConjunction -->

    <owl:Class rdf:about="http://purl.org/olia/mte/multext-east.owl#PositiveSubordinatingConjunction">
        <rdfs:subClassOf rdf:resource="http://purl.org/olia/mte/multext-east.owl#SubordinatingConjunction"/>
        <rdfs:comment>e.g., aşa_că, va_să_zică (ro)</rdfs:comment>
        <rdfs:comment>Conjunction/Sub_Type=&quot;positive&quot; (Romanian, Serbian, Russian)

In Romanian, each conjunction requires another mood, so that the diversity may be controlled by subcategorisation rules. The attribute Sub_Type distinguishes among the positive and negative conjunctions, providing means to control verbal double negation, (as in case of the negative pronouns, determiners and adverbs): nici NU am venit, nimeni NU vorbeşte, nici_un tren N-a trecut, nicăieri N-am văzut (MTE v4)</rdfs:comment>
    </owl:Class>
    


    <!-- http://purl.org/olia/mte/multext-east.owl#PossessiveAdjective -->

    <owl:Class rdf:about="http://purl.org/olia/mte/multext-east.owl#PossessiveAdjective">
        <rdfs:subClassOf rdf:resource="http://purl.org/olia/mte/multext-east.owl#Adjective"/>
        <rdfs:comment>e.g., Riegrovými/Riegrův, Stradellovými/Stradellův, Tristanovou/Tristanův, Wagnerových/Wagnerův, Wagnerovým/Wagnerův, Weberovi/Weberův, Weberových/Weberův, Wertherovi/Wertherův, Winstonovi/Winstonův (cs)</rdfs:comment>
        <rdfs:comment>e.g., dušikovima/dušikov, Marsovi/Marsov (sl)</rdfs:comment>
        <rdfs:comment>e.g., evroazijske/evroazijska, evroazijskih/evroazijski, Goldštajnov, govornikov, Jehovine/Jehovin, malabarskom/malabarski, O&apos;Brajenov, O&apos;Brajenovog/O&apos;Brajenov, oficirov (sr)</rdfs:comment>
        <rdfs:comment>e.g., vojvodova/vojvodov, vojvodove/vojvodov, vojvodovej/vojvodov, vojvodovho/vojvodov, vojvodovi/vojvodov, vojvodovmu/vojvodov, vojvodovo/vojvodov, vojvodovom/vojvodov, vojvodovou/vojvodov (sk)</rdfs:comment>
        <rdfs:comment>Adjective/Type=&quot;possessive&quot; are denominal, not pronominal expressions of possession (Ivan A Derzhanski, email 2010/06/09). Therefore not to be confused with Pronoun/Type=adjectival(a) (Bulgarian only), for words like умно /cleverly, wisely, sensibly/, which are derived from adjectives. (Dimitrova et al. 2009)
</rdfs:comment>
    </owl:Class>
    


    <!-- http://purl.org/olia/mte/multext-east.owl#PossessiveArticle -->

    <owl:Class rdf:about="http://purl.org/olia/mte/multext-east.owl#PossessiveArticle">
        <rdfs:subClassOf rdf:resource="http://purl.org/olia/mte/multext-east.owl#Article"/>
        <rdfs:comment>e.g., -al/al, a/al, ai/al, al, ale/al, alor/al (ro)</rdfs:comment>
        <rdfs:comment>In Romanian,  the possessive article (also called genitival article) is an element in the structure of the possessive pronoun, of the ordinal numeral (e.g. al meu (mine) and al treilea (the third)), and of the indefinite genitive forms of the nouns (e.g. capitol al cărţii (chapter of the book)). (MTE v4)</rdfs:comment>
    </owl:Class>
    


    <!-- http://purl.org/olia/mte/multext-east.owl#PossessiveDeterminer -->

    <owl:Class rdf:about="http://purl.org/olia/mte/multext-east.owl#PossessiveDeterminer">
        <rdfs:subClassOf rdf:resource="http://purl.org/olia/mte/multext-east.owl#Determiner"/>
        <rdfs:comment>e.g., &apos;Er/her, &apos;is/his, her, his, its, my, our, their, whose (en)</rdfs:comment>
        <rdfs:comment>e.g., -mea/mea, -meu/meu, -mii/mea, -miu/meu, -sa/sa, -sii/sa, -su/său, -său/său, -ta/ta (ro)</rdfs:comment>
        <rdfs:comment>Determiner/Type=&quot;possessive&quot; (English, Romanian, Persian)</rdfs:comment>
    </owl:Class>
    


    <!-- http://purl.org/olia/mte/multext-east.owl#PossessivePronoun -->

    <owl:Class rdf:about="http://purl.org/olia/mte/multext-east.owl#PossessivePronoun">
        <rdfs:subClassOf rdf:resource="http://purl.org/olia/mte/multext-east.owl#Pronoun"/>
        <rdfs:comment>e.g., -tău/tău, noastre/nostru, noastră/nostru, nostru, noştri/nostru, ta/tău, tale/tău, tăi/tău, tău (ro)</rdfs:comment>
        <rdfs:comment>e.g., enyémet/én, tied/te, tiéd/te, övét/ő, övétől/ő (hu)</rdfs:comment>
        <rdfs:comment>e.g., omadest/oma, omalt/oma, omast/oma (et)</rdfs:comment>
        <rdfs:comment>e.g., theirs (en)</rdfs:comment>
        <rdfs:comment>e.g., tiviga/twöj, trivin/twöj, tuoi/twöj, tuvoi/twöj, tuói/twöj, tuö/twöj, tvíga/twöj (sl-rozaj)</rdfs:comment>
        <rdfs:comment>e.g., tvoj, tvoja/tvoj, tvoje/tvoj, tvojej/tvoj, tvojho/tvoj, tvoji/tvoj, tvojich/tvoj, tvojim/tvoj, tvojimi/tvoj (sk)</rdfs:comment>
        <rdfs:comment>e.g., tvoj/=, tvoja/tvoj, tvoje/tvoj, tvojega/tvoj, tvojem/tvoj, tvojemu/tvoj, tvoji/tvoj, tvojih/tvoj, tvojim/tvoj (sl)</rdfs:comment>
        <rdfs:comment>e.g., tvoje/tvůj, tvoji/tvůj, tvou/tvůj, tvá/tvůj, tvé/tvůj, tvého/tvůj, tvém/tvůj, tvým/tvůj, tvůj (cs)</rdfs:comment>
        <rdfs:comment>e.g., twe/twój, twego/twój, twej/twój, twoi/twój, twoich/twój, twoim/twój, twoimi/twój, twoja/twój, twoje/twój (pl)</rdfs:comment>
        <rdfs:comment>Pronoun/Type=&quot;possessive&quot; and Pronoun/Referent_Type=&quot;possessive&quot;, e.g., Macedonian moj, tvoj (eng. my, your). (MTE v4)</rdfs:comment>
    </owl:Class>
    


    <!-- http://purl.org/olia/mte/multext-east.owl#PostnominalModification -->

    <owl:Class rdf:about="http://purl.org/olia/mte/multext-east.owl#PostnominalModification">
        <rdfs:subClassOf rdf:resource="http://purl.org/olia/mte/multext-east.owl#ModificationType"/>
        <rdfs:comment>e.g., -aceasta/acesta, -ăia/ăla, -ăla/ăla (ro)</rdfs:comment>
        <rdfs:comment>Determiner/Modific_Type=&quot;postnomin&quot; (Romanian)&lt;br/&gt;

The Modific_Type attribute is relevant for some Romanian pronouns and determiners. The prenominal determiner always precedes the noun (e.g.acest băiat - this boy), whereas the postnominal determiner appears only after the noun (e.g. băiatul acesta - this boy). (MTE v4)</rdfs:comment>
    </owl:Class>
    


    <!-- http://purl.org/olia/mte/multext-east.owl#Postposition -->

    <owl:Class rdf:about="http://purl.org/olia/mte/multext-east.owl#Postposition">
        <rdfs:subClassOf rdf:resource="http://purl.org/olia/mte/multext-east.owl#Adposition"/>
        <rdfs:comment>e.g., و/را رو/را را (fa)</rdfs:comment>
        <rdfs:comment>Adposition/Type=&quot;postposition&quot;&lt;br/&gt;

English: Postpositions are rare in English. &quot;possessive&quot; &apos;s and &apos; might be considered postpositions, especially if the alternative is to assign them to the unique membership class (where by definition they would be unrelated). (MTE v4)&lt;br/&gt;

Farsi has several prepositions but there is only one postposition &apos;‫( &apos;را‬râ). It is an
overt marker for direct object. (Qasemizadeh and Saeed Rahimi 2006)</rdfs:comment>
    </owl:Class>
    


    <!-- http://purl.org/olia/mte/multext-east.owl#PremodifyingOrdinalNumeral -->

    <owl:Class rdf:about="http://purl.org/olia/mte/multext-east.owl#PremodifyingOrdinalNumeral">
        <rdfs:subClassOf rdf:resource="http://purl.org/olia/mte/multext-east.owl#OrdinalNumeral"/>
        <rdfs:subClassOf rdf:resource="http://purl.org/olia/mte/multext-east.owl#PrenominalModification"/>
        <rdfs:comment>Numeral/Type=&quot;ordinal2&quot; (Persian)&lt;br/&gt;

In Persian, a number can be inflected by two different suffix to express ordinal meaning. These suffixes are &quot;om&quot; and &quot;omin&quot;. They both have more or less the same meaning; however they are different morphosyntactically. For example, the English phrase &quot;first person&quot; can be translated to Persian as follows:

(1) nafar yekom
(2) yekomin nafar

&quot;nafar&quot; in Persian means person, &quot;yek&quot; in Persian means one.
(1)  yek + om = yekom (ordinal)
(2) yek + omin = yekomin (ordinal2)

Ordinal2 refers to the premodifying variant in (2), e.g., هجدهم/هجده نهم/نه دهم/ده (MTE v4; Behrang Qasemizadeh, email 2010/06/26)
</rdfs:comment>
    </owl:Class>
    


    <!-- http://purl.org/olia/mte/multext-east.owl#PrenominalModification -->

    <owl:Class rdf:about="http://purl.org/olia/mte/multext-east.owl#PrenominalModification">
        <rdfs:subClassOf rdf:resource="http://purl.org/olia/mte/multext-east.owl#ModificationType"/>
        <rdfs:comment>e.g., -acea/acel, -această/acest, alde, alt, alte/alt, altă/alt, alţi/alt, care, ce (ro)</rdfs:comment>
        <rdfs:comment>Determiner/Modific_Type=&quot;prenomin&quot; (Romanian)&lt;br/&gt;

The Modific_Type attribute is relevant for some Romanian pronouns and determiners. The prenominal determiner always precedes the noun (e.g.acest băiat - this boy), whereas the postnominal determiner appears only after the noun (e.g. băiatul acesta - this boy). (MTE v4)</rdfs:comment>
    </owl:Class>
    


    <!-- http://purl.org/olia/mte/multext-east.owl#Preposition -->

    <owl:Class rdf:about="http://purl.org/olia/mte/multext-east.owl#Preposition">
        <rdfs:subClassOf rdf:resource="http://purl.org/olia/mte/multext-east.owl#Adposition"/>
        <rdfs:comment>e.g., -mpotriva/împotriva, -naintea/înaintea, asupră/asupra (ro)</rdfs:comment>
        <rdfs:comment>e.g., a незважаючи/=, без біля близько в вві взамін вздовж від вколо внаслідок для до з задля замість заради зверх зверху звиш здовж, в за крізь меж межи на над невважаючи незважаючи о об перед під по повз поза поміж понад понадо поперед, в на о по попри при у ув уві, всупереч завдяки противно уздогін усупереч, з за із меж межи над наді надо перед передо під підо поза помежи поміж понад понадо поперед попід пред, за те за тим з-від з-за з-між з-навпроти з-над з-перед з-під з-поверхні з-поза з-позад з-позаду з-поміж з-понад з-поперед з-попід з-посеред з-проміж з-серед, згідно з, на противагу (uk)</rdfs:comment>
        <rdfs:comment>e.g., dardu/dardu, h/h, na/na, od/od, ot/od, par/par, per/par, po/po, prid/prid (sl-rozaj)</rdfs:comment>
        <rdfs:comment>e.g., dla/dla, do/do, dzięki/dzięki, ku/ku, między/między, na/na, nad/nad, o/o, od/od (pl)</rdfs:comment>
        <rdfs:comment>e.g., از‌لايِ/ازلا ازلحاظِ/ازلحاظ ازجانبِ/ازجانب, پشتِ‌سر طي طرفِ/طرف (fa)</rdfs:comment>
        <rdfs:comment>Type=&quot;preposition&quot;</rdfs:comment>
    </owl:Class>
    


    <!-- http://purl.org/olia/mte/multext-east.owl#PrepositionalCase -->

    <owl:Class rdf:about="http://purl.org/olia/mte/multext-east.owl#PrepositionalCase">
        <rdfs:subClassOf rdf:resource="http://purl.org/olia/mte/multext-east.owl#Case"/>
        <owl:versionInfo>Case=&quot;prepositional&quot; (Russian)</owl:versionInfo>
    </owl:Class>
    


    <!-- http://purl.org/olia/mte/multext-east.owl#PresentTense -->

    <owl:Class rdf:about="http://purl.org/olia/mte/multext-east.owl#PresentTense">
        <rdfs:subClassOf rdf:resource="http://purl.org/olia/mte/multext-east.owl#Tense"/>
        <rdfs:comment>e.g., &apos;A/have, be, being/be, daren&apos;t/dare+not, doing/do, having/have, lacquered/lacquer, nose, oughter/have (en)</rdfs:comment>
        <rdfs:comment>e.g., -, lennétek/lesz, továbbtaníttatnátok/továbbtaníttat, tudnálak/tud, tudnátok/tud, uralhatjátok/uralhat, venniük/vesz, venné/vesz, veszekedjünk/veszekedik (hu)</rdfs:comment>
        <rdfs:comment>e.g., -nzestreze/înzestra, -nzidească/înzidi, -nzorzoneze/înzorzona, fi, fii/fi, fim/fi, fiu/fi, fiţi/fi (ro)</rdfs:comment>
        <rdfs:comment>e.g., accompagnaimu/akompanjät, amai/amät, amaite/amät, aman/amät, Bode/bet, bodete/bet, bodi/bet, bodite/bet, bodê/bet (sl-rozaj)</rdfs:comment>
        <rdfs:comment>e.g., biorąc/brać, byliby/być, byłaby/być, byłby/być, byłbyś/być, byłoby/być, byłyby/być, byłybyście/być, byłybyśmy/być (pl)</rdfs:comment>
        <rdfs:comment>e.g., budi/biti, budimo/biti, htedni/hteti, htednimo/hteti, htjedni/htjeti, htjednimo/htjeti, je/jesam, sam/jesam, si/jesam (sr)</rdfs:comment>
        <rdfs:comment>e.g., buď/byť, buďme/byť, buďte/byť, je/byť, maj/mať, majme/mať, majte/mať, majú/mať, majúc/mať (sk)</rdfs:comment>
        <rdfs:comment>e.g., buď/být, bývám/bývat, chceme/chtít, chcete/chtít, chceš/chtít, chtěj/chtít, dejme/dát, dejte/dát, dostane/dostat (cs)</rdfs:comment>
        <rdfs:comment>e.g., olda/olema, ole/olema, oled/olema, oledki/olema, olegi/olema, oleks/olema, oleksime/olema, oleksin/olema, oleksite/olema (et)</rdfs:comment>
        <rdfs:comment>e.g., Звенящая/звенеть, Поёшь/петь, Си/си, Трясущейся/трястись, Улыбающаяся/улыбаться, Улыбающиеся/улыбаться, Улыбающийся/улыбаться, Хошь/хотеть, видимо/видеть (ru)</rdfs:comment>
        <rdfs:comment>e.g., абеткую/абеткувати авізую/авізувати агакаю/агакати агітую/агітувати агонізую/агонізувати адвокатую/адвокатувати адмініструю/адмініструвати айкаю/айкати акаю/акати акомпаную/акомпанувати акредитуюся/акредитуватися акредитуюсь/акредитуватися акторствую/акторствувати акторую/акторувати актую/актувати акушерую/акушерувати альокаю/альокати аналізую/аналізувати анкетую/анкетувати анодую/анодувати, абеткують/абеткувати авізують/авізувати агакають/агакати агітують/агітувати агонізують/агонізувати адвокатують/адвокатувати адмініструють/адмініструвати адоптуються/адоптуватися адсорбуються/адсорбуватися азотуються/азотуватися айкають/айкати акають/акати акомпанують/акомпанувати акредитуються/акредитуватися акторствують/акторствувати акторують/акторувати актують/актувати акушерують/акушерувати акцентуються/акцентуватися альокають/альокати, абеткуючи/абеткувати авізуючи/авізувати агакаючи/агакати агітуючи/агітувати агонізуючи/агонізувати адвокатуючи/адвокатувати адмініструючи/адмініструвати адоптуючись/адоптуватися адсорбуючись/адсорбуватися азотуючись/азотуватися айкаючи/айкати акаючи/акати акомпануючи/акомпанувати акредитуючись/акредитуватися акторствуючи/акторствувати акторуючи/акторувати актуючи/актувати акушеруючи/акушерувати акцентуючись/акцентуватися альокаючи/альокати, абеткує/абеткувати авізує/авізувати агакає/агакати агака/агакати агітує/агітувати агонізує/агонізувати адвокатує/адвокатувати адмініструє/адмініструвати адоптується/адоптуватися адсорбується/адсорбуватися азотується/азотуватися айкає/айкати айка/айкати акає/акати ака/акати акомпанує/акомпанувати акредитується/акредитуватися акторствує/акторствувати акторує/акторувати актує/актувати, абеткуємо/абеткувати абеткуєм/абеткувати авізуємо/авізувати авізуєм/авізувати агакаємо/агакати агакаєм/агакати агітуємо/агітувати агітуєм/агітувати агонізуємо/агонізувати агонізуєм/агонізувати адвокатуємо/адвокатувати адвокатуєм/адвокатувати адмініструємо/адмініструвати адмініструєм/адмініструвати айкаємо/айкати айкаєм/айкати акаємо/акати акаєм/акати акомпануємо/акомпанувати акомпануєм/акомпанувати, абеткуєте/абеткувати авізуєте/авізувати агакаєте/агакати агітуєте/агітувати агонізуєте/агонізувати адвокатуєте/адвокатувати адмініструєте/адмініструвати айкаєте/айкати акаєте/акати акомпануєте/акомпанувати акредитуєтеся/акредитуватися акредитуєтесь/акредитуватися акторствуєте/акторствувати акторуєте/акторувати актуєте/актувати акушеруєте/акушерувати альокаєте/альокати аналізуєте/аналізувати анкетуєте/анкетувати анодуєте/анодувати, абеткуєш/абеткувати авізуєш/авізувати агакаєш/агакати агітуєш/агітувати агонізуєш/агонізувати адвокатуєш/адвокатувати адмініструєш/адмініструвати айкаєш/айкати акаєш/акати акомпануєш/акомпанувати акредитуєшся/акредитуватися акторствуєш/акторствувати акторуєш/акторувати актуєш/актувати акушеруєш/акушерувати альокаєш/альокати аналізуєш/аналізувати анкетуєш/анкетувати анодуєш/анодувати аплодуєш/аплодувати, аблактую/аблактувати абоную/абонувати абонуюся/абонуватися абонуюсь/абонуватися абордую/абордувати абортую/абортувати абсолютизую/абсолютизувати абстрагую/абстрагувати абстрагуюся/абстрагуватися абстрагуюсь/абстрагуватися абшитую/абшитувати авансую/авансувати авансуюся/авансуватися авансуюсь/авансуватися автоматизую/автоматизувати авторизую/авторизувати аглютиную/аглютинувати агрегатую/агрегатувати адаптую/адаптувати адаптуюся/адаптуватися, аблактують/аблактувати абонують/абонувати абонуються/абонуватися абордують/абордувати абортують/абортувати абсолютизують/абсолютизувати абсолютизуються/абсолютизуватися абсорбують/абсорбувати абсорбуються/абсорбуватися абстрагують/абстрагувати абстрагуються/абстрагуватися абшитують/абшитувати авансують/авансувати авансуються/авансуватися автоматизують/автоматизувати автоматизуються/автоматизуватися авторизують/авторизувати аглютинують/аглютинувати аглютинуються/аглютинуватися агрегатують/агрегатувати (uk)</rdfs:comment>
        <rdfs:comment>e.g., бидам/сум, бидат/сум, биде/сум, бидеме/сум, бидете/сум, бидеш/сум, биди/сум, е/сум, има (mk)</rdfs:comment>
        <rdfs:comment>e.g., бъда, бъдат/бъда, бъде/бъда, бъдем/бъда, бъдете/бъда, бъдеш/бъда, бъдещ/бъда, бъдеща/бъда, бъдещата/бъда (bg)</rdfs:comment>
        <rdfs:comment>e.g., اند/است, ايد/است, باش, باشد/باش, باشم/باش, باشند/باش, باشه/باش باشد/باش آيد/آ, باشي/باش, باشيم/باش (fa)</rdfs:comment>
        <rdfs:comment>Tense=&quot;present&quot; (Ukrainian also for adjectives)</rdfs:comment>
        <owl:versionInfo>Slovene &quot;future&quot; and &quot;present&quot; in VForm are equivalent to &quot;future&quot; and &quot;present&quot; in Tense.&lt;br/&gt;

The Slovene specs has a convoluted history - there are
substantial differences between V3 in V4. Version 4 was made on the basis of
the JOS specifications http://nl.ijs.si/jos/josMSD-en.html
which are monolingual Slovene, and the linguists preferred to see future and
present as verb forms, as this is traditional in Slovene grammars. Hence
this inconsistency in regard to other languages.
(Tomaž Erjavec, email 2010/06/09)
</owl:versionInfo>
    </owl:Class>
    


    <!-- http://purl.org/olia/mte/multext-east.owl#ProQuantifier -->

    <owl:Class rdf:about="http://purl.org/olia/mte/multext-east.owl#ProQuantifier">
        <rdfs:subClassOf rdf:resource="http://purl.org/olia/mte/multext-east.owl#Pronoun"/>
        <rdfs:subClassOf rdf:resource="http://purl.org/olia/mte/multext-east.owl#Quantifier"/>
        <rdfs:comment>ProQuantifier represents Pronoun/Referent_type=&quot;quantitative&quot; and Numeral/Class=&quot;demonstrative&quot; (etc.)&lt;br/&gt;

The MTE v4 categories Numeral/Class=&quot;interrogative&quot;,  Numeral/Class=&quot;demonstrative&quot;, Numeral/Class=&quot;indefinite&quot; and Numeral/Class=&quot;relative&quot; are items meaning `how many/much&apos;, `this many/much&apos;, `several/some&apos;, `as many/much&apos; etc. Strictly speaking, they are pronumerals (pro-quantifiers), but traditional descriptions don&apos;t recognise such a category, so they are described variously as pronouns (because they can be interrogative, demonstrative etc., as proforms other than personal or possessive ones can) or as numerals (because their syntactic distribution is that of numerals, or very close). (Ivan A. Derzhanski, email 2010/06/11)&lt;br/&gt;

The difference between pronouns and these classes of numerals is, however, fuzzy and many are indeed classified as pronouns (Slovak MTE v.4) The Bulgarian equivalents of [Slovak] demonstrative, indefinite, interrogative and relative &quot;numeral&quot; are thus classified as pronouns with Referent_type=&quot;quantitative&quot;, e.g. няколко ученика /a few students/ – indefinite pronoun + noun. or sometimes as adverbs.  (Dimitrova et al. 2009)</rdfs:comment>
        <owl:versionInfo>ProQuantifier is not an original MTE v4 concept, but introduced as a generalization over quantifiers that are derived from pronominal elements and are thus partly characterized as pronoun or quantifier (&quot;numeral&quot;). (Ch. Chiarcos)&lt;br/&gt;

MTE Numeral/Class classifies Quantifiers and Numerals according to two criteria, i.e., morphological/diachronic derivation from a pro-form (see ProQuantifier), and syntactic agreement patterns (singular, plural, dual and paucal quantifiers, see NumeralAgreementClass). The first classification applies to quantifiers that involve an element with pronominal function. The latter classification covers quantifiers (incl. pro-quantifiers) and numerals.</owl:versionInfo>
    </owl:Class>
    


    <!-- http://purl.org/olia/mte/multext-east.owl#Program -->

    <owl:Class rdf:about="http://purl.org/olia/mte/multext-east.owl#Program">
        <rdfs:subClassOf rdf:resource="http://purl.org/olia/mte/multext-east.owl#Residual"/>
        <rdfs:comment>In the Slovene MTE v4 specs, Residual/Type=&quot;program&quot; marks where the tokenisation program made a mistake. (MTE v4)</rdfs:comment>
    </owl:Class>
    


    <!-- http://purl.org/olia/mte/multext-east.owl#ProgressiveAspect -->

    <owl:Class rdf:about="http://purl.org/olia/mte/multext-east.owl#ProgressiveAspect">
        <rdfs:subClassOf rdf:resource="http://purl.org/olia/mte/multext-east.owl#Aspect"/>
        <rdfs:comment>e.g., 0, абеткована/абеткований авізована/авізований акомпанована/акомпанований актована/актований аналізована/аналізований анкетована/анкетований анодована/анодований артикульована/артикульований балотована/балотований балувана/балуваний бальзамована/бальзамований банітована/банітований багнітована/багнітований байцьована/байцьований балакана/балаканий бачена/бачений белетризована/белетризований бережена/бережений бетонована/бетонований бинтована/бинтований, абеткованая/абеткований авізованая/авізований акомпанованая/акомпанований актованая/актований аналізованая/аналізований анкетованая/анкетований анодованая/анодований артикульованая/артикульований балотованая/балотований балуваная/балуваний бальзамованая/бальзамований банітованая/банітований багнітованая/багнітований байцьованая/байцьований балаканая/балаканий баченая/бачений белетризованая/белетризований береженая/бережений бетонованая/бетонований бинтованая/бинтований, абетковане/абеткований авізоване/авізований акомпановане/акомпанований актоване/актований аналізоване/аналізований анкетоване/анкетований анодоване/анодований артикульоване/артикульований балотоване/балотований балуване/балуваний бальзамоване/бальзамований банітоване/банітований багнітоване/багнітований байцьоване/байцьований балакане/балаканий бачене/бачений белетризоване/белетризований бережене/бережений бетоноване/бетонований бинтоване/бинтований, абеткованеє/абеткований авізованеє/авізований акомпанованеє/акомпанований актованеє/актований аналізованеє/аналізований анкетованеє/анкетований анодованеє/анодований артикульованеє/артикульований балотованеє/балотований балуванеє/балуваний бальзамованеє/бальзамований банітованеє/банітований багнітованеє/багнітований байцьованеє/байцьований балаканеє/балаканий баченеє/бачений белетризованеє/белетризований береженеє/бережений бетонованеє/бетонований бинтованеє/бинтований, абеткований/= авізований/= акомпанований/= актований/= аналізований/= анкетований/= анодований/= артикульований/= балотований/= балуваний/= бальзамований/= банітований/= багнітований/= байцьований/= балаканий/= бачений/= белетризований/= бережений/= бетонований/= бинтований/=, абеткованим/абеткований авізованим/авізований акомпанованим/акомпанований актованим/актований аналізованим/аналізований анкетованим/анкетований анодованим/анодований артикульованим/артикульований балотованим/балотований балуваним/балуваний бальзамованим/бальзамований банітованим/банітований багнітованим/багнітований байцьованим/байцьований балаканим/балаканий баченим/бачений белетризованим/белетризований береженим/бережений бетонованим/бетонований бинтованим/бинтований, абеткованими/абеткований авізованими/авізований акомпанованими/акомпанований актованими/актований аналізованими/аналізований анкетованими/анкетований анодованими/анодований артикульованими/артикульований балотованими/балотований балуваними/балуваний бальзамованими/бальзамований банітованими/банітований багнітованими/багнітований байцьованими/байцьований балаканими/балаканий баченими/бачений белетризованими/белетризований береженими/бережений бетонованими/бетонований бинтованими/бинтований, абеткованих/абеткований авізованих/авізований акомпанованих/акомпанований актованих/актований аналізованих/аналізований анкетованих/анкетований анодованих/анодований артикульованих/артикульований балотованих/балотований балуваних/балуваний бальзамованих/бальзамований банітованих/банітований багнітованих/багнітований байцьованих/байцьований балаканих/балаканий бачених/бачений белетризованих/белетризований бережених/бережений бетонованих/бетонований бинтованих/бинтований (uk)</rdfs:comment>
        <rdfs:comment>e.g., akceptowanymi/akceptować, analizowanych/analizować, badanego/badać, badaniem/badanie, bałoś/bać, bieżącego/bieżeć, bieżącym/bieżeć, biorąc/brać, byli/być (pl)</rdfs:comment>
        <rdfs:comment>e.g., amai/amät, amaite/amät, bese/bet, bet/bet, beše/bet, bil/bet, Bila/bet, bile/bet, bili/bet (sl-rozaj)</rdfs:comment>
        <rdfs:comment>e.g., bi&apos;/biti, bi/biti, bih/biti, bila/biti, bile/biti, bilo/biti, bio/biti, bismo/biti, biste/biti (sr)</rdfs:comment>
        <rdfs:comment>e.g., bola/byť, boli/byť, bolo/byť, bude/byť, budem/byť, budeme/byť, budete/byť, budeš/byť, budú/byť (sk)</rdfs:comment>
        <rdfs:comment>e.g., hodita/hoditi, hoče/hoteti, hočejo/hoteti, hočem/hoteti, hočeta/hoteti, hočeva/hoteti, ima/imeti, imajo/imeti, imam/imeti (sl)</rdfs:comment>
        <rdfs:comment>e.g., БУДЕМ/быть, БУДЕТ/быть, БУДЕТЕ/быть, БУДЕШЬ/быть, БУДУ/быть, БУДУТ/быть, Бежим/бежать, Будет/быть, Будете/быть (ru)</rdfs:comment>
        <rdfs:comment>e.g., има, имаа/има, имаат/има, имав/има, имавме/има, имавте/има, имал/има, имала/има, имале/има (mk)</rdfs:comment>
        <rdfs:comment>e.g., برمي‌داشتيد/برداشت, مي‌آمديد/آمد, مي‌توانست/توانست, مي‌توانستم/توانست, مي‌توانستند/توانست, مي‌توانستي/توانست, مي‌جنگيده/جنگيد, مي‌خوانديم/خواند, مي‌داديد/داد (fa)</rdfs:comment>
        <rdfs:comment>Aspect=&quot;progressive&quot; (Noun: Polish; Verb: Slavic and Persian; Adjective: Polish, Ukrainian)

In Slavic aspectology, Russian aspect is usually considered to be a binary category, i.e., every Russian verb form is either perfective or imperfective. Only imperfective verbs can combine with the auxiliary быть &apos;be&apos; in the analytic future construction, e.g. 

(1)  Когда-нибудь я буду писать как Hабоков.
Sometime I will write like Nabokov
&apos;I will write like Nabokov one day.&apos;

The synthetic future tense is restricted to perfective verbs, e.g.

(2) Я позвоню тебе.
I callFUTURE you
&apos;I&apos;ll call you.&apos;

There is the syntactic restriction that only imperfective verbs combine with phase verbs. In Russian, verbs like начинать / начать &apos;begin&apos;, продолжать / продолжить &apos;continue&apos; or кончать / кончить &apos;stop/finish&apos; can only take an imperfective infinitive as a complement. (Feldman &amp; Arshavskaya 2007)

Anna Feldman &amp; Katya Arshavskaya (2007), English and Russian event annotation: A pilot study. Studies in Variation, Contacts and Change in English 1, http://www.helsinki.fi/varieng/journal/volumes/01/feldman_arshavskaya/</rdfs:comment>
    </owl:Class>
    


    <!-- http://purl.org/olia/mte/multext-east.owl#Pronominal -->

    <owl:Class rdf:about="http://purl.org/olia/mte/multext-east.owl#Pronominal">
        <rdfs:subClassOf rdf:resource="http://purl.org/olia/mte/multext-east.owl#SyntacticType"/>
        <rdfs:comment>e.g., d-ta/dumneata, d-tale/dumitale, d-voastră/dumneavoastră, dv./dumneavoastră, dvs./dumneavoastră (ro)</rdfs:comment>
        <rdfs:comment>Abbreviation/Syntactic_Type=&quot;pronominal&quot; (Romanian)</rdfs:comment>
    </owl:Class>
    


    <!-- http://purl.org/olia/mte/multext-east.owl#Pronoun -->

    <owl:Class rdf:about="http://purl.org/olia/mte/multext-east.owl#Pronoun">
        <rdfs:subClassOf rdf:resource="http://purl.org/olia/mte/multext-east.owl#MorphosyntacticCategory"/>
        <rdfs:subClassOf>
            <owl:Class>
                <owl:intersectionOf rdf:parseType="Collection">
                    <owl:Restriction>
                        <owl:onProperty rdf:resource="http://purl.org/olia/mte/multext-east.owl#hasCase"/>
                        <owl:cardinality rdf:datatype="http://www.w3.org/2001/XMLSchema#nonNegativeInteger">1</owl:cardinality>
                    </owl:Restriction>
                    <owl:Restriction>
                        <owl:onProperty rdf:resource="http://purl.org/olia/mte/multext-east.owl#hasNumber"/>
                        <owl:cardinality rdf:datatype="http://www.w3.org/2001/XMLSchema#nonNegativeInteger">1</owl:cardinality>
                    </owl:Restriction>
                </owl:intersectionOf>
            </owl:Class>
        </rdfs:subClassOf>
        <rdfs:subClassOf>
            <owl:Class>
                <owl:intersectionOf rdf:parseType="Collection">
                    <owl:Restriction>
                        <owl:onProperty rdf:resource="http://purl.org/olia/mte/multext-east.owl#hasClitic"/>
                        <owl:maxCardinality rdf:datatype="http://www.w3.org/2001/XMLSchema#nonNegativeInteger">1</owl:maxCardinality>
                    </owl:Restriction>
                    <owl:Restriction>
                        <owl:onProperty rdf:resource="http://purl.org/olia/mte/multext-east.owl#hasDefiniteness"/>
                        <owl:maxCardinality rdf:datatype="http://www.w3.org/2001/XMLSchema#nonNegativeInteger">1</owl:maxCardinality>
                    </owl:Restriction>
                    <owl:Restriction>
                        <owl:onProperty rdf:resource="http://purl.org/olia/mte/multext-east.owl#hasOwnerGender"/>
                        <owl:maxCardinality rdf:datatype="http://www.w3.org/2001/XMLSchema#nonNegativeInteger">1</owl:maxCardinality>
                    </owl:Restriction>
                    <owl:Restriction>
                        <owl:onProperty rdf:resource="http://purl.org/olia/mte/multext-east.owl#hasOwnerNumber"/>
                        <owl:maxCardinality rdf:datatype="http://www.w3.org/2001/XMLSchema#nonNegativeInteger">1</owl:maxCardinality>
                    </owl:Restriction>
                    <owl:Restriction>
                        <owl:onProperty rdf:resource="http://purl.org/olia/mte/multext-east.owl#hasSyntacticType"/>
                        <owl:maxCardinality rdf:datatype="http://www.w3.org/2001/XMLSchema#nonNegativeInteger">1</owl:maxCardinality>
                    </owl:Restriction>
                </owl:intersectionOf>
            </owl:Class>
        </rdfs:subClassOf>
        <rdfs:subClassOf>
            <owl:Restriction>
                <owl:onProperty rdf:resource="http://purl.org/olia/mte/multext-east.owl#hasPerson"/>
                <owl:cardinality rdf:datatype="http://www.w3.org/2001/XMLSchema#nonNegativeInteger">1</owl:cardinality>
            </owl:Restriction>
        </rdfs:subClassOf>
        <rdfs:subClassOf>
            <owl:Restriction>
                <owl:onProperty rdf:resource="http://purl.org/olia/mte/multext-east.owl#hasGender"/>
                <owl:maxCardinality rdf:datatype="http://www.w3.org/2001/XMLSchema#nonNegativeInteger">1</owl:maxCardinality>
            </owl:Restriction>
        </rdfs:subClassOf>
        <rdfs:comment>e.g., &apos;Em/them, another, itself, others, thee/you, theirs, them, themselves, there (en)</rdfs:comment>
        <rdfs:comment>e.g., -astea/ăsta, -te/tu, -tău/tău, -ăştia/ăsta, ast-/ăsta, ast/asta, a_dreaptă, celorlalte/celălalt, cestorlalte/cestălalt (ro)</rdfs:comment>
        <rdfs:comment>e.g., -astea/ăsta, -te/tu, -tău/tău, -ăştia/ăsta, ast-/ăsta, ast/asta, te-/tu (ro)</rdfs:comment>
        <rdfs:comment>e.g., akiktől/aki, akiét/aki, amelyekért/amely, amelytől/amely, amiként/ami, amitől/ami, attól/az, azoktól/az, azét/az (hu)</rdfs:comment>
        <rdfs:comment>e.g., ci/ten, dlatego/dlatego, kimkolwiek/ktokolwiek, kimś/ktoś, kogokolwiek/ktokolwiek, kogoś/ktoś, komukolwiek/ktokolwiek, komuś/ktoś, kto/kto (pl)</rdfs:comment>
        <rdfs:comment>e.g., ci/ten, kimkolwiek/ktokolwiek, kimś/ktoś, kogokolwiek/ktokolwiek, kogoś/ktoś, komukolwiek/ktokolwiek, komuś/ktoś, kto/kto, ktokolwiek/ktokolwiek (pl)</rdfs:comment>
        <rdfs:comment>e.g., endalt/ise, endilt/ise, endist/ise, eneselt/ise, igasugustesse/igasugune, iseenestega/iseenese, kellelt/kes, kelleta/kes, kõigilt/kõik (et)</rdfs:comment>
        <rdfs:comment>e.g., etej/iti, ishtes/ištës, ite/iti, iti/iti, itim/iti, itin/iti, ito/iti, itoga/iti, itoha/iti (sl-rozaj)</rdfs:comment>
        <rdfs:comment>e.g., hentej/hentá, henten, hentie/henten, hentie/hento, hentie/hentá, hentoho/henten, hentoho/hento, hentom/hento, hentomu/hento (sk)</rdfs:comment>
        <rdfs:comment>e.g., katere/kateri, katerih/kateri, katerim/kateri, katerimi/kateri, nekaterim/nekateri, teboj/ti, ti/=, ti/ta, tistih/tisti (sl)</rdfs:comment>
        <rdfs:comment>e.g., kdekterých/kdekterý, kdekterými/kdekterý, kterou/který, která/který, které/který, kterého/který, kterém/který, kterému/který, který (cs)</rdfs:comment>
        <rdfs:comment>e.g., kterého/který, kteří/který, ti/ty, tvoji/tvůj, tvého/tvůj, tě/ty, vašeho/tvůj, vaši/tvůj (cs)</rdfs:comment>
        <rdfs:comment>e.g., ta/taj, take/takav, te/ti, tebe/ti, tebi/ti, tobom/ti (sr)</rdfs:comment>
        <rdfs:comment>e.g., te/tï, ti/tï, tiviga/twöj, to/to, tvíga/twöj, tè/tï (sl-rozaj)</rdfs:comment>
        <rdfs:comment>e.g., ti/ty (sk)</rdfs:comment>
        <rdfs:comment>The English MTE v4 specs distinguish five major classes of Pronoun, i.e., PersonalPronoun, PossessivePronoun, DemonstrativePronoun, ReflexivePronoun and GeneralPronoun. &quot;General&quot; pronouns are those which are not personal, possessive, demonstrative or reflexive. The choice of these four categories is based on distributional facts, though at a rather high level of abstraction. They enter into anaphoric dependencies which are signalled morphosyntactically and are therefore (in principle) more amenable to automatic detection. Most general pronouns do not, although they too sometimes encode number information.
(MTE v4)&lt;br/&gt;

Bulgarian marks definiteness for pronouns, but it is present only for the possessive and reflexive types of pronouns, and for some general pronouns. Examples include: 
Possessive: Мой – моя - моят /my/, Твой - твоя – твоят /your, 2 p. sing/, Негов – неговия – неговият /his/
Reflexive: Свой – своя – своят, своя – своята, свое-своето, свои - своите /his, her, its, their own/
(Dimitrova et al. 2009)</rdfs:comment>
        <owl:versionInfo>
		The original MTE feature Pronoun/Referent_Type covers a subset of Pronoun classes to represent multiple inheritance. Redundant in the ontology.		
		
Referent_Type:
    used to distinguish reflexive personal from reflexive possessive pronouns in the Slavic languages. In Bulgarian, it also describes a subdivision on the basis of semantic features which have effect on the morpho-syntactic paradigm, e.g. quantitative: the pronoun refers to quantity, etc.
(MTE v4)&lt;br/&gt;

Ukrainian: Many pronouns can be assigned to more than one Type. The Referent_Type feature is used to show the additional feature, like possessiveness or personality. The main type is defined according to the grammatical tradition.
(MTE v4)&lt;br/&gt;

Czech: Referent_Type is used to distinguish personal reflexives (which include &quot;se&quot; in all its functions) from the possesive reflexives (&quot;svůj&quot;).
(MTE v4)&lt;br/&gt;

Slovak: Type=reflexive ecompasses all reflexive pronouns (sa, sebe, si, svoj, seba) as well as &quot;sa&quot; in its role as the obligatory particle of reflexive verbs. Personal and possessive reflexives are further distinguished via the Referent_Type attribute. &quot;sa&quot; in all its roles will be marked as the reflexive personal clitic pronoun.
Referent_Type is used to distinguish personal reflexives (which include &quot;sa&quot; in all its functions) from the possesive reflexives (&quot;svoj&quot;).
(MTE v4)&lt;br/&gt;

Referent_Type is personal, possessive, attributive and quantitative in Bulgarian, but only personal and po-
ssessive in Slovak – the rest of pronouns do not have this type set (Referent_Type=-), which is just a deficiency in the Slovak MTE description.
(Dimitrova et al. 2009)
</owl:versionInfo>
    </owl:Class>
    


    <!-- http://purl.org/olia/mte/multext-east.owl#PronounForm -->

    <owl:Class rdf:about="http://purl.org/olia/mte/multext-east.owl#PronounForm">
        <rdfs:subClassOf rdf:resource="http://purl.org/olia/mte/multext-east.owl#MorphosyntacticFeature"/>
        <rdfs:comment>The feature &quot;Pronoun_Form&quot; distinguishes weak and strong pronouns Romanian.&lt;br/&gt;

For Romanian we need an attribute (called Pronoun_Form) to make the distinction between strong and weak forms of the same personal pronoun or reflexive pronoun. All the weak forms can be adjoined to the adjacent words both proclitically or enclitically. In such cases the junction is always graphically marked by a hyphen between the pronoun and the neighboring word. The hyphen also marks possible elisions from either pronoun or the adjacent word. (MTE v4)</rdfs:comment>
    </owl:Class>
    


    <!-- http://purl.org/olia/mte/multext-east.owl#ProperNoun -->

    <owl:Class rdf:about="http://purl.org/olia/mte/multext-east.owl#ProperNoun">
        <rdfs:subClassOf rdf:resource="http://purl.org/olia/mte/multext-east.owl#Noun"/>
        <rdfs:comment>e.g., Aladárét/Aladár, Gyöngyikét/Gyöngyi, Kennedy-testvérekig/Kennedy-testvér, Kossuth-díjaikat/Kossuth-díj, Kossuth-díjakat/Kossuth-díj, Krisztináé/Krisztina, NATO-tagságának/NATO-tagság, Sopronét/Sopron, Szlovákiáért/Szlovákia (hu)</rdfs:comment>
        <rdfs:comment>e.g., Atrizi/Atrid, Statelor_Unite/Statele_Unite, Statelor_Unite_ale_Americii/Statele_Unite_ale_Americii, Washingtonul/Washington, Washingtonului/Washington, Zărneştiul/Zărneşti, Zărneştiului/Zărneşti (ro)</rdfs:comment>
        <rdfs:comment>e.g., Baltimaadel/Baltimaad, Baltimaades/Baltimaad, Kallastel/Kallas, Kallastele/Kallas, Kallastelt/Kallas, Kallasteni/Kallas, Pauluste/Paulus, Vautseliinasse/Vautseliina, Viljandimaalt/Viljandimaa (et)</rdfs:comment>
        <rdfs:comment>e.g., Bratstvom/Bratstvo, Bratstvu/Bratstvo, Ministarstvu/Ministarstvo, Stepni (sr)</rdfs:comment>
        <rdfs:comment>e.g., Christusa/krïštuš, Christusam/krïštuš, Crishtusha/krïštuš, Dapiton/dapit, Elisabeto/elizabeta, Kristušon/krïštuš, Kristušu/krïštuš (sl-rozaj)</rdfs:comment>
        <rdfs:comment>e.g., Hrvatoma/Hrvat, pilatusema/pilatus (sl)</rdfs:comment>
        <rdfs:comment>Noun/Type=Proper</rdfs:comment>
    </owl:Class>
    


    <!-- http://purl.org/olia/mte/multext-east.owl#QualificativeAdjective -->

    <owl:Class rdf:about="http://purl.org/olia/mte/multext-east.owl#QualificativeAdjective">
        <rdfs:subClassOf rdf:resource="http://purl.org/olia/mte/multext-east.owl#GeneralAdjective"/>
        <rdfs:comment>e.g., -, bensőnkben/benső, borúlátónkat/borúlátó, buktatóin/buktató, csigaformákba/csigaformá, derekukkal/derék, derekukra/derék, dolgozóiból/dolgozó, dolgozójukba/dolgozó (hu)</rdfs:comment>
        <rdfs:comment>e.g., -ntrebătoare/întrebător, -ntregi/întreg, -ntreprinzătoare/întreprinzător, -nvăluitoare/învăluitor, -nzestrata/înzestrat, -nzestrate/înzestrat, -nzestratei/înzestrat, -nzestratele/înzestrat, -nzestratelor/înzestrat (ro)</rdfs:comment>
        <rdfs:comment>e.g., belim/beo, bezbrojnih/bezbrojni, crnobrko/crnobrki, devetogodišnji, druge/drugi, gvozdene/gvozden, inkriminisani/inkriminisan, jak, kubnih/kubni (sr)</rdfs:comment>
        <rdfs:comment>e.g., blishgnaha/blïžnji, bujše/bujši, cert/čert, Chrishtianschin/krištijanski, chrivaha/krïw, dalesgni/dalëčnji, delečni/dalëčnji, dobar/dobar, dobre/dobar (sl-rozaj)</rdfs:comment>
        <rdfs:comment>e.g., bliższe/bliski, bliższej/bliski, bliższych/bliski, bogatszych/bogaty, dalsza/daleki, dalsze/daleki, dalszego/daleki, dalszej/daleki, dalszemu/daleki (pl)</rdfs:comment>
        <rdfs:comment>e.g., brillská/brillský, nejubožejšími/ubohý, nejvyspělejších/vyspělý, nejvyšších/vysoký, nejvznešenějšímu/vznešený, nejvážnějšímu/vážný, nejvýznamnějších/významný, nejvýznamnějšími/významný, nejvýznamnějšímu/významný (cs)</rdfs:comment>
        <rdfs:comment>e.g., najžoviálnejšej/žoviálny, najžoviálnejšia/žoviálny, najžoviálnejšie/žoviálny, najžoviálnejšieho/žoviálny, najžoviálnejšiemu/žoviálny, najžoviálnejšiu/žoviálny, najžoviálnejšom/žoviálny, najžoviálnejšou/žoviálny, najžoviálnejší/žoviálny (sk)</rdfs:comment>
        <rdfs:comment>e.g., Чертова/чертовый, Швейцарских/швейцарский, Язвительно/язвительный, га, микро, участковым/участковый, фен, форсированным/форсированный, частным/частный (ru)</rdfs:comment>
        <rdfs:comment>e.g., аварійно небезпечна/аварійно небезпечний азартна/азартний активна/активний актуальна/актуальний амбітна/амбітний амбіційна/амбіційний амбіціозна/амбіціозний апетитна/апетитний ароматна/ароматний багата/багатий багатозначна/багатозначний бадьора/бадьорий бажана/бажаний балаклива/балакливий балакуча/балакучий безпечна/безпечний безумна/безумний бентежна/бентежний бережлива/бережливий бідна/бідний, аварійно небезпечная/аварійно небезпечний азартная/азартний активная/активний актуальная/актуальний амбітная/амбітний амбіційная/амбіційний амбіціозная/амбіціозний апетитная/апетитний ароматная/ароматний багатая/багатий багатозначная/багатозначний бадьорая/бадьорий бажаная/бажаний балакливая/балакливий балакучая/балакучий безпечная/безпечний безумная/безумний бентежная/бентежний бережливая/бережливий бідная/бідний, аварійно небезпечне/аварійно небезпечний азартне/азартний активне/активний актуальне/актуальний амбітне/амбітний амбіційне/амбіційний амбіціозне/амбіціозний апетитне/апетитний ароматне/ароматний багате/багатий багатозначне/багатозначний бадьоре/бадьорий бажане/бажаний балакливе/балакливий балакуче/балакучий безпечне/безпечний безумне/безумний бентежне/бентежний бережливе/бережливий бідне/бідний, аварійно небезпечнеє/аварійно небезпечний азартнеє/азартний активнеє/активний актуальнеє/актуальний амбітнеє/амбітний амбіційнеє/амбіційний амбіціознеє/амбіціозний апетитнеє/апетитний ароматнеє/ароматний багатеє/багатий багатозначнеє/багатозначний бадьореє/бадьорий бажанеє/бажаний балакливеє/балакливий балакучеє/балакучий безпечнеє/безпечний безумнеє/безумний бентежнеє/бентежний бережливеє/бережливий біднеє/бідний, аварійно небезпечний/= азартний/= активний/= актуальний/= амбітний/= амбіційний/= амбіціозний/= апетитний/= ароматний/= багатий/= багатозначний/= бадьорий/= бажаний/= балакливий/= балакучий/= безпечний/= безумний/= бентежний/= бережливий/= бідний/=, аварійно небезпечним/аварійно небезпечний азартним/азартний активним/активний актуальним/актуальний амбітним/амбітний амбіційним/амбіційний амбіціозним/амбіціозний апетитним/апетитний ароматним/ароматний багатим/багатий багатозначним/багатозначний бадьорим/бадьорий бажаним/бажаний балакливим/балакливий балакучим/балакучий безпечним/безпечний безумним/безумний бентежним/бентежний бережливим/бережливий бідним/бідний, аварійно небезпечними/аварійно небезпечний азартними/азартний активними/активний актуальними/актуальний амбітними/амбітний амбіційними/амбіційний амбіціозними/амбіціозний апетитними/апетитний ароматними/ароматний багатими/багатий багатозначними/багатозначний бадьорими/бадьорий бажаними/бажаний балакливими/балакливий балакучими/балакучий безпечними/безпечний безумними/безумний бентежними/бентежний бережливими/бережливий бідними/бідний, аварійно небезпечних/аварійно небезпечний азартних/азартний активних/активний актуальних/актуальний амбітних/амбітний амбіційних/амбіційний амбіціозних/амбіціозний апетитних/апетитний ароматних/ароматний багатих/багатий багатозначних/багатозначний бадьорих/бадьорий бажаних/бажаний балакливих/балакливий балакучих/балакучий безпечних/безпечний безумних/безумний бентежних/бентежний бережливих/бережливий бідних/бідний, аварійно небезпечного/аварійно небезпечний азартного/азартний активного/активний актуального/актуальний амбітного/амбітний амбіційного/амбіційний амбіціозного/амбіціозний апетитного/апетитний ароматного/ароматний багатого/багатий багатозначного/багатозначний бадьорого/бадьорий бажаного/бажаний балакливого/балакливий балакучого/балакучий безпечного/безпечний безумного/безумний бентежного/бентежний бережливого/бережливий бідного/бідний (uk)</rdfs:comment>
        <rdfs:comment>e.g., بلندتري/بلند انساني‌تري/انساني‌ آرام‌تري/آرام, رنگيِ/رنگي بي‌امانِ/بي‌امان بوکسورمانندِ/بوکسورمانند, زنگداري/زنگدار تهوع‌آوري/تهوع‌آور برهنه‌اي/برهنه, قوي‌ترِ/قوي بيشترِ/بيش اعظمِ/اعظم, متعصّب‌ترين/متعصّب قديمي‌ترين/قديمي ترسناک‌ترين/ترسناک, مطمئن‌تر/مطمئن عاقلانه‌تر/عاقلانه بدبوتر/بدبو, موذي عاري سبيلو (fa)</rdfs:comment>
        <rdfs:comment>In Czech and Slovak MTE v4, Adjective/Type=qualificative conflates the deverbative adjectival participles, i.e., past active participle (Czech only), passive participle and present active participle, e.g., Slovak &quot;stojaci&quot; (E. &quot;standing&quot;) or &quot;urobený&quot; (E. &quot;made&quot; or &quot;done&quot;)

For Romanian, one could make the distinction between qualificative and determinative adjectives, although this is not common practice in Romanian linguistics. (MTE v4)</rdfs:comment>
    </owl:Class>
    


    <!-- http://purl.org/olia/mte/multext-east.owl#Quantifier -->

    <owl:Class rdf:about="http://purl.org/olia/mte/multext-east.owl#Quantifier">
        <rdfs:subClassOf rdf:resource="http://purl.org/olia/mte/multext-east.owl#MorphosyntacticCategory"/>
        <rdfs:comment>A quantifier is a pronoun or a determiner that expresses a referent&apos;s definite or indefinite number or amount. (adapted from http://linguistics-ontology.org/gold/2008/Quantifier, quoting Crystal 1997, 317; extended in order to cover ProQuantifier, as suggested by Ivan A Derzhinski).&lt;br/&gt;

In MTE v4, Quantifier corresponds to the top-class Numeral that has been extended to cover non-numerical quantifiers. In Slavic languages, (Pro)Quantifiers and Numerals have a specific syntactic distribution where different quantities are correlated with certain agreement patterns. &lt;br/&gt;

The Slovak MTE, for example, distinguishes the following agreement patterns: definite1 for “one”, definite2 for “two”, definite34 for “three” or “four”, definite for “five or more”. Definite1, definite2, definite34 and definite are separated according to syntactical structures the numerals impose on the governed nouns – definite1 requires the corresponding noun to be in nominative singular, definite2 in nominative plural, definite34 nominative plural, definite genitive plural. (Dimitrova et al. 2009)&lt;br/&gt;

These agreement patterns are specified in the subconcept NumeralAgreementClass. See the subconcepts Numeral and ProQuantifier for their respective semantic sub-classification.&lt;br/&gt;

Overlap with Pronoun: Bulgarian equivalents of [Slovak] demonstrative, indefinite, interrogative numerals (ProQuantifiers) are classified as pronouns of a respective Type (including relative), e.g. няколко ученика /a few students/ – indefinite pronoun + noun. or sometimes as adverbs. (Dimitrova et al. 2009)</rdfs:comment>
        <owl:versionInfo>In many MTE schemes, the class &quot;Numeral&quot; is applied to cover non-numerical quantifiers, as well. The common MTE  category &quot;Numeral&quot; thus fails to distinguish between numeral and non-numeral quantifiers and is thus to be renamed to the broader concept &quot;Quantifier&quot;.
Quantifier is identified with Numeral/Class in MTE v.4 that is also applied to non-numerical quantifiers.
TODO: NumeralAgreementClass is to be distinguished from other Numeral/Class features and Numeral subconcepts and to be represented as an independent MorphosyntacticFeature. However, this requires modifications of the underlying MTE scheme.</owl:versionInfo>
    </owl:Class>
    


    <!-- http://purl.org/olia/mte/multext-east.owl#Question -->

    <owl:Class rdf:about="http://purl.org/olia/mte/multext-east.owl#Question">
        <rdfs:subClassOf rdf:resource="http://purl.org/olia/mte/multext-east.owl#WHType"/>
    </owl:Class>
    


    <!-- http://purl.org/olia/mte/multext-east.owl#Quotative -->

    <owl:Class rdf:about="http://purl.org/olia/mte/multext-east.owl#Quotative">
        <rdfs:subClassOf rdf:resource="http://purl.org/olia/mte/multext-east.owl#VerbForm"/>
        <rdfs:comment>e.g., olevat/olema, olevatki/olema, peetavat/pidama, polevat/olema, saadavat/saama, ulatuvat/ulama (et)</rdfs:comment>
        <rdfs:comment>VForm=&quot;quotative&quot; (Estonian)&lt;br/&gt;

A quotative is grammatical device to mark reported speech in some languages (http://en.wikipedia.org/wiki/Quotative), e.g., in Estonian.&lt;br/&gt;

‘Reportedly, while he was going (in his boat), he turned over.’
 Ta olevat        oma     paadiga   ümber läinud
He was_QUOTATIVE his_own boat_WITH over  gone.&lt;br/&gt;

(Estonian translation of an example given under http://www.sil.org/linguistics/GlossaryOfLinguisticTerms/WhatIsAQuotativeEvidential.htm)
(Heiki-Jaan.Kaalep, email 2010/06/22)</rdfs:comment>
    </owl:Class>
    


    <!-- http://purl.org/olia/mte/multext-east.owl#ReciprocalPronoun -->

    <owl:Class rdf:about="http://purl.org/olia/mte/multext-east.owl#ReciprocalPronoun">
        <rdfs:subClassOf rdf:resource="http://purl.org/olia/mte/multext-east.owl#Pronoun"/>
        <rdfs:comment>e.g., egymást/egymás, egymástól/egymás (hu)</rdfs:comment>
        <rdfs:comment>e.g., teineteise, teineteisega/teineteise, teineteisele/teineteise, teineteiselt/teineteise, teineteisesse/teineteise, teineteisest/teineteise, teineteist/teineteise, üksteise, üksteisega/üksteise (et)</rdfs:comment>
        <rdfs:comment>Pronoun/Type=&quot;reciprocal&quot; (Persian, Estonian, Hungarian)</rdfs:comment>
    </owl:Class>
    


    <!-- http://purl.org/olia/mte/multext-east.owl#ReductionFeature -->

    <owl:Class rdf:about="http://purl.org/olia/mte/multext-east.owl#ReductionFeature">
        <rdfs:subClassOf rdf:resource="http://purl.org/olia/mte/multext-east.owl#Definiteness"/>
        <rdfs:comment>For Polish, the Vocalicity of (a)gglutinated forms like -em vs -m is mapped on the MTE Definiteness attribute with its values &quot;(f)ull-art&quot; and &quot;(s)hort-art&quot; respectively, meaning &quot;full form&quot; and &quot;short form&quot;. The terms are very artificial, but this category is used due to the similarity of the phenomenon. The IPIC flexeme winien and predicatives like rad are treated as short adjectives—Definiteness=&quot;short-art&quot;. (MTE v4)&lt;br/&gt;

Etymologically speaking, CliticDeterminerType and ReductionFeature are the same: the ending of the full form was originally a cliticised demonstrative pronoun (just like the article in Bg or Ro), and the semantic distinction was [+/- definite], but it has shifted to [attributive:predicative] or some such on some occasions.
However, keeping them together wouldn&apos;t be correct: Bulgarian has preserved (to a limited extent) the old long form, and has a fourfold opposition of, say, _nov : novi : novija : novijat_, the first two members of which have counterparts in several Slavic languages (although the functions differ), while the second two are 
restricted to the Balkan sprachbund.  I&apos;d call them [-article short], [-article full], [+article short] and [+article full] respectively. (Ivan A. Derzhanski, emails 2010/06/18)&lt;br/&gt;

[T]he suffixation of an actual pronoun to the adjective ... for the Balto-Slavic definite adjective inflection ... was used with definite nouns ... the Balto-Slavic forms show clear evidence of a well-attested IE pronoun suffixed to the adjective (McFadden 2004)&lt;br/&gt;

ReductionFeature corresponds to AdjectiveFormation in Czech.&lt;br/&gt;

Thomas McFadden (2004), On the pronominal origins of the Germanic strong adjective inflection, http://ifla.uni-stuttgart.de/institut/mitarbeiter/tom/downloads/gmcadj.pdf (to appear in Münchner Studien zur Sprachwissenschaft)</rdfs:comment>
        <owl:versionInfo>In Polish, the MTE feature definiteness is used to distinguish forms with full and reduced inflections.</owl:versionInfo>
    </owl:Class>
    


    <!-- http://purl.org/olia/mte/multext-east.owl#ReflexivePronoun -->

    <owl:Class rdf:about="http://purl.org/olia/mte/multext-east.owl#ReflexivePronoun">
        <rdfs:subClassOf rdf:resource="http://purl.org/olia/mte/multext-east.owl#Pronoun"/>
        <rdfs:comment>e.g., endalt/ise, endilt/ise, endist/ise, eneselt/ise, iseenestega/iseenese, omadest/oma, omalt/oma (et)</rdfs:comment>
        <rdfs:comment>e.g., itself, themselves (en)</rdfs:comment>
        <rdfs:comment>e.g., magadat/maga, magamat/maga, magamét/maga, magatokat/maga, magukat/maga, maguktól/maga, magukéit/maga, magukét/maga, magunkat/maga (hu)</rdfs:comment>
        <rdfs:comment>In the Czech and Slovak MTE v4 specs, Pronoun/Type=&quot;reflexive&quot; ecompasses all reflexive pronouns (Slovak sa, sebe, si, svoj, seba, Czech se, sebe, si, svůj) as well as Slovak &quot;sa&quot; and Czech &quot;se&quot; in its role as the obligatory particle of reflexive verbs. Personal and possessive reflexives are further distinguished via the Referent_Type attribute. &quot;sa&quot; in all its roles will be marked as the reflexive personal clitic pronoun. (MTE v4)</rdfs:comment>
    </owl:Class>
    


    <!-- http://purl.org/olia/mte/multext-east.owl#RelationalAdjective -->

    <owl:Class rdf:about="http://purl.org/olia/mte/multext-east.owl#RelationalAdjective">
        <rdfs:subClassOf rdf:resource="http://purl.org/olia/mte/multext-east.owl#GeneralAdjective"/>
        <rdfs:comment>The Slovene adjective expresses three main ideas: quality (qualitative adjectives, kakovostni pridevniki), relation (relational adjectives, vrstni pridevniki) and possession (possessive adjectives, svojilni pridevniki).
            Relational adjectives express type, class or numerical sequence of a noun. For instance: kemijska in fizikalna sprememba (chemical and physical change), fotografski aparat (photographic device (=camera)). (http://en.wikipedia.org/wiki/Slovene_grammar)</rdfs:comment>
        <rdfs:comment>e.g., Bohavei/böguw, Bohouv/böguw, Bohovaha/böguw, Bohove/böguw, Bohovih/böguw, Bohovij/böguw, Bohovin/böguw, Bohuvin/böguw, Boshij/böžji (sl-rozaj)</rdfs:comment>
        <rdfs:comment>e.g., evroazijskog/evroazijski, Faroskih/Faroska, francuski, gipsani/gipsan, malabarskog/malabarski, malabarskom/malabarski, muzičkog/muzički, novogovorske/novogovorski, okeanijskog/okeanijski (sr)</rdfs:comment>
        <rdfs:comment>e.g., Абакумів/= Абрамів/= Авакумів/= Августин/= Августинів/= Августів/= Авенірів/= Аверкіїв/= Авер&apos;янів/= Авіятин/= Авксентіїв/= Аврамів/= Авреліїн/= Аврорин/= Автономів/= авторів/= авторчин/= Агапіїв/= Агапіїн/= Агапітів/=, антресольна/антресольний антропічна/антропічний антропна/антропний антропогенна/антропогенний антропоїдна/антропоїдний антропологічна/антропологічний абажурна/абажурний абазинська/абазинський абаканська/абаканський Абакумова/Абакумів абатська/абатський абераційна/абераційний абеткова/абетковий абіджанська/абіджанський абіогенна/абіогенний абісальна/абісальний абіссінська/абіссінський абітурієнтська/абітурієнтський аболіціоністська/аболіціоністський абонементна/абонементний, антресольная/антресольний антропічная/антропічний антропная/антропний антропогенная/антропогенний антропоїдная/антропоїдний антропологічная/антропологічний абажурная/абажурний абазинськая/абазинський абаканськая/абаканський Абакумовая/Абакумів абатськая/абатський абераційная/абераційний абетковая/абетковий абіджанськая/абіджанський абіогенная/абіогенний абісальная/абісальний абіссінськая/абіссінський абітурієнтськая/абітурієнтський аболіціоністськая/аболіціоністський абонементная/абонементний, антресольне/антресольний антропічне/антропічний антропне/антропний антропогенне/антропогенний антропоїдне/антропоїдний антропологічне/антропологічний абажурне/абажурний абазинське/абазинський абаканське/абаканський Абакумове/Абакумів абатське/абатський абераційне/абераційний абеткове/абетковий абіджанське/абіджанський абіогенне/абіогенний абісальне/абісальний абіссінське/абіссінський абітурієнтське/абітурієнтський аболіціоністське/аболіціоністський абонементне/абонементний, антресольнеє/антресольний антропічнеє/антропічний антропнеє/антропний антропогеннеє/антропогенний антропоїднеє/антропоїдний антропологічнеє/антропологічний абажурнеє/абажурний абазинськеє/абазинський абаканськеє/абаканський Абакумовеє/Абакумів абатськеє/абатський абераційнеє/абераційний абетковеє/абетковий абіджанськеє/абіджанський абіогеннеє/абіогенний абісальнеє/абісальний абіссінськеє/абіссінський абітурієнтськеє/абітурієнтський аболіціоністськеє/аболіціоністський абонементнеє/абонементний, антресольний/= антропічний/= антропний/= антропогенний/= антропоїдний/= антропологічний/= абажурний/= абазинський/= абаканський/= абатський/= абераційний/= абетковий/= абіджанський/= абіогенний/= абісальний/= абіссінський/= абітурієнтський/= аболіціоністський/= абонементний/= абонентний/=, антресольним/антресольний антропічним/антропічний антропним/антропний антропогенним/антропогенний антропоїдним/антропоїдний антропологічним/антропологічний абажурним/абажурний абазинським/абазинський абаканським/абаканський Абакумовим/Абакумів абатським/абатський абераційним/абераційний абетковим/абетковий абіджанським/абіджанський абіогенним/абіогенний абісальним/абісальний абіссінським/абіссінський абітурієнтським/абітурієнтський аболіціоністським/аболіціоністський абонементним/абонементний, антресольними/антресольний антропічними/антропічний антропними/антропний антропогенними/антропогенний антропоїдними/антропоїдний антропологічними/антропологічний абажурними/абажурний абазинськими/абазинський абаканськими/абаканський Абакумовими/Абакумів абатськими/абатський абераційними/абераційний абетковими/абетковий абіджанськими/абіджанський абіогенними/абіогенний абісальними/абісальний абіссінськими/абіссінський абітурієнтськими/абітурієнтський аболіціоністськими/аболіціоністський абонементними/абонементний, антресольних/антресольний антропічних/антропічний антропних/антропний антропогенних/антропогенний антропоїдних/антропоїдний антропологічних/антропологічний абажурних/абажурний абазинських/абазинський абаканських/абаканський Абакумових/Абакумів абатських/абатський абераційних/абераційний абеткових/абетковий абіджанських/абіджанський абіогенних/абіогенний абісальних/абісальний абіссінських/абіссінський абітурієнтських/абітурієнтський аболіціоністських/аболіціоністський абонементних/абонементний (uk)</rdfs:comment>
        <rdfs:comment>&quot;Ordinal adjective&quot; is applied to Slovenian vrstni pridevniki and Ukrainian відносні прикметники. A more appropriate term would be relative adjective (Derzhanski and Kotsyba 2009).
            However, in other MTE languages (e.g., Macedonian), the term &quot;ordinal adjective&quot; designates ordinal numerals, e.g., Macedonian prv, vtor (eng. first, second) (note on MTE v4 adjectives).</rdfs:comment>
    </owl:Class>
    


    <!-- http://purl.org/olia/mte/multext-east.owl#Relative -->

    <owl:Class rdf:about="http://purl.org/olia/mte/multext-east.owl#Relative">
        <rdfs:subClassOf rdf:resource="http://purl.org/olia/mte/multext-east.owl#WHType"/>
    </owl:Class>
    


    <!-- http://purl.org/olia/mte/multext-east.owl#RelativeAdverb -->

    <owl:Class rdf:about="http://purl.org/olia/mte/multext-east.owl#RelativeAdverb">
        <owl:equivalentClass>
            <owl:Class>
                <owl:intersectionOf rdf:parseType="Collection">
                    <rdf:Description rdf:about="http://purl.org/olia/mte/multext-east.owl#Adverb"/>
                    <owl:Restriction>
                        <owl:onProperty rdf:resource="http://purl.org/olia/mte/multext-east.owl#hasWHType"/>
                        <owl:hasValue rdf:resource="http://purl.org/olia/mte/multext-east.owl#Relative"/>
                    </owl:Restriction>
                </owl:intersectionOf>
            </owl:Class>
        </owl:equivalentClass>
        <rdfs:subClassOf rdf:resource="http://purl.org/olia/mte/multext-east.owl#InterrogativeOrRelativeAdverb"/>
        <rdfs:comment>Adverb/Wh_Type=&quot;relative&quot;, placed here in analogy with Adverb/Wh_Type=&quot;question&quot;.</rdfs:comment>
        <rdfs:comment>e.g., &apos;Ow, &apos;ow, how, where, whereupon, when (en)</rdfs:comment>
    </owl:Class>
    


    <!-- http://purl.org/olia/mte/multext-east.owl#RelativeDeterminer -->

    <owl:Class rdf:about="http://purl.org/olia/mte/multext-east.owl#RelativeDeterminer">
        <owl:equivalentClass>
            <owl:Class>
                <owl:intersectionOf rdf:parseType="Collection">
                    <rdf:Description rdf:about="http://purl.org/olia/mte/multext-east.owl#Determiner"/>
                    <owl:Restriction>
                        <owl:onProperty rdf:resource="http://purl.org/olia/mte/multext-east.owl#hasWHType"/>
                        <owl:hasValue rdf:resource="http://purl.org/olia/mte/multext-east.owl#Relative"/>
                    </owl:Restriction>
                </owl:intersectionOf>
            </owl:Class>
        </owl:equivalentClass>
        <rdfs:subClassOf rdf:resource="http://purl.org/olia/mte/multext-east.owl#InterrogativeOrRelativeDeterminer"/>
        <rdfs:comment>Determiner/Wh_Type=&quot;relative&quot; (English MTE v4)</rdfs:comment>
        <rdfs:comment>e.g., whose (en)</rdfs:comment>
    </owl:Class>
    


    <!-- http://purl.org/olia/mte/multext-east.owl#RelativePronoun -->

    <owl:Class rdf:about="http://purl.org/olia/mte/multext-east.owl#RelativePronoun">
        <owl:equivalentClass>
            <owl:Class>
                <owl:intersectionOf rdf:parseType="Collection">
                    <rdf:Description rdf:about="http://purl.org/olia/mte/multext-east.owl#Pronoun"/>
                    <owl:Restriction>
                        <owl:onProperty rdf:resource="http://purl.org/olia/mte/multext-east.owl#hasWHType"/>
                        <owl:hasValue rdf:resource="http://purl.org/olia/mte/multext-east.owl#Relative"/>
                    </owl:Restriction>
                </owl:intersectionOf>
            </owl:Class>
        </owl:equivalentClass>
        <rdfs:subClassOf rdf:resource="http://purl.org/olia/mte/multext-east.owl#InterrogativeOrRelativePronoun"/>
        <rdfs:comment>e.g., -, akikben/aki, akiken/aki, akikhez/aki, akikkel/aki, akiknek/aki, akikre/aki, akikről/aki, akiktől/aki (hu)</rdfs:comment>
        <rdfs:comment>e.g., ch’/ka, ke/ka, kir/kir, koja/koji (sl-rozaj)</rdfs:comment>
        <rdfs:comment>e.g., co, jaká/jaký, jaké/jaký, jakého/jaký, jakém/jaký, jakému/jaký, jakých/jaký, jakým/jaký, jakými/jaký (cs)</rdfs:comment>
        <rdfs:comment>e.g., co/co, czego/co, czemu/co, czym/co, dlaczego/dlaczego, dlaczegóż/dlaczegóż, gdzie/gdzie, jacy/jaki, jaka/jaki (pl)</rdfs:comment>
        <rdfs:comment>e.g., kakršne/kakršen, kakršni/kakršen, kakršnih/kakršen, čemur/kar, čimer/kar (sl)</rdfs:comment>
        <rdfs:comment>e.g., kelledega/kes, kellega/kes, kelleks/kes, kellele/kes, kellelt/kes, kellena/kes, kellesse/kes, kelleta/kes, kumba/kumb (et)</rdfs:comment>
        <rdfs:comment>e.g., whom (en)</rdfs:comment>
        <rdfs:comment>e.g., де/= доки/= звідки/= звідкіля/= коли/= куди/= наскільки/= чому/= як/=, ким/хто, кого/хто, кому/хто, кому/хто кім/хто, котра/котрий котрая/котрий яка/який якая/який, котре/котрий котреє/котрий яке/який якеє/який, котрий/= який/=, котрим/котрий яким/який (uk)</rdfs:comment>
        <rdfs:comment>e.g., каквато/какъвто, каквито/какъвто, каквото/какъвто, какъвто, когото/който, което/който, които/който, който, колкото (bg)</rdfs:comment>
        <rdfs:comment>e.g., кого/кој, кому/кој, свое/свој, своево/свој, своено/свој, своето/свој, свои/свој, своиве/свој, своине/свој (mk)</rdfs:comment>
        <rdfs:comment>Pronoun/Wh_Type=&quot;relative&quot; (English) or Pronoun/Type=&quot;relative&quot; (other languages).</rdfs:comment>
    </owl:Class>
    


    <!-- http://purl.org/olia/mte/multext-east.owl#RelativeQuantifier -->

    <owl:Class rdf:about="http://purl.org/olia/mte/multext-east.owl#RelativeQuantifier">
        <owl:equivalentClass>
            <owl:Class>
                <owl:intersectionOf rdf:parseType="Collection">
                    <rdf:Description rdf:about="http://purl.org/olia/mte/multext-east.owl#ProQuantifier"/>
                    <owl:Restriction>
                        <owl:onProperty rdf:resource="http://purl.org/olia/mte/multext-east.owl#hasWHType"/>
                        <owl:hasValue rdf:resource="http://purl.org/olia/mte/multext-east.owl#Relative"/>
                    </owl:Restriction>
                </owl:intersectionOf>
            </owl:Class>
        </owl:equivalentClass>
        <rdfs:subClassOf rdf:resource="http://purl.org/olia/mte/multext-east.owl#ProQuantifier"/>
        <owl:versionInfo>In the Czech MTE v4 specs, Numeral/Class=&quot;relative&quot; are items meaning `how many/much&apos;, `as many/much&apos; etc. Strictly speaking, they are pronumerals (pro-quantifiers), but traditional descriptions don&apos;t recognise such a category, so they are described variously as pronouns or as numerals (because their syntactic distribution is that of numerals, or very close).&quot; (Ivan A Derzhanski, email 2010/06/11)</owl:versionInfo>
    </owl:Class>
    


    <!-- http://purl.org/olia/mte/multext-east.owl#RepetitiveCoordinatingConjunction -->

    <owl:Class rdf:about="http://purl.org/olia/mte/multext-east.owl#RepetitiveCoordinatingConjunction">
        <rdfs:subClassOf rdf:resource="http://purl.org/olia/mte/multext-east.owl#CoordinatingConjunction_PositionalType"/>
        <rdfs:comment>Conjunction/Coord_Type=&quot;repetit&quot; (Romanian).

In Romanian, there are three kinds of conjunctions depending on their usage: as such or together with other conjunctions or adverbs: (1) simple, between conjuncts: Ion ori Maria (John or Mary); (2) repetitive, before each conjunct: fie Ion fie Maria fie... (either John or Mary or...) (3) correlative, before a conjoined phrase, it requires specific coordinators between conjuncts: atât mama cât şi tata (both mother and father). (MTE v4)</rdfs:comment>
    </owl:Class>
    


    <!-- http://purl.org/olia/mte/multext-east.owl#Residual -->

    <owl:Class rdf:about="http://purl.org/olia/mte/multext-east.owl#Residual">
        <rdfs:subClassOf rdf:resource="http://purl.org/olia/mte/multext-east.owl#MorphosyntacticCategory"/>
        <rdfs:comment>e.g., deleted-end-of-sentence/deleted-end-of-sentence, deleted-token/deleted-token (pl)</rdfs:comment>
        <rdfs:comment>Residual refers to otherwise non-classified parts of speech.&lt;br/&gt;

In Slovak, special &apos;adverb prepositions&apos; (po, na, do), encountered in expressions like po anglicky, na zeleno,
do modra are classified as residuals. Traditional Slovak grammars do not like to consider them separate words,
but rather see them to be different part-of-speech, mostly an adverb (see interjections above), with a space inside. In corresponding Bulgarian expressions (e.g. на български), the residual will be classified as Sp (preposition). This is however just a difference in grammar description, not an inherent difference in the languages. (Dimitrova et al. 2009)</rdfs:comment>
    </owl:Class>
    


    <!-- http://purl.org/olia/mte/multext-east.owl#RomanNumeral -->

    <owl:Class rdf:about="http://purl.org/olia/mte/multext-east.owl#RomanNumeral">
        <rdfs:subClassOf rdf:resource="http://purl.org/olia/mte/multext-east.owl#OrthographicalRepresentationOfNumeral"/>
        <rdfs:comment>Form=&quot;roman&quot;</rdfs:comment>
    </owl:Class>
    


    <!-- http://purl.org/olia/mte/multext-east.owl#SecondPerson -->

    <owl:Class rdf:about="http://purl.org/olia/mte/multext-east.owl#SecondPerson">
        <rdfs:subClassOf rdf:resource="http://purl.org/olia/mte/multext-east.owl#Person"/>
        <rdfs:comment>e.g., -nzestrarăţi/înzestra, -nzestraserăţi/înzestra, -nzestraseşi/înzestra, -nzestraţi/înzestra, -ta/ta, -te/tu, -tii/ta, -tu/tău, -tău/tău (ro)</rdfs:comment>
        <rdfs:comment>e.g., abyste/aby, budete/být, byste/by, chcete/chtít, chceš/chtít, chtěj/chtít, dejte/dát, jste/být, kdybyste/kdyby (cs)</rdfs:comment>
        <rdfs:comment>e.g., amaite/amät, bodete/bet, bodite/bet, bota/bet, Ciete/tët, datte/dät, Dáite/dät, hovarnajte/govarnät, intendate/intendät (sl-rozaj)</rdfs:comment>
        <rdfs:comment>e.g., barátoddal/barát, bennetek/ti, benneteket/ti, bennünket/ti, betegségedhez/betegség, botrányoddal/botrány, cselekedeteidről/cselekedet, cselekedeteiteken/cselekedet, fiaitoknak/fi (hu)</rdfs:comment>
        <rdfs:comment>e.g., biste/biti, bićete/biti, htedni/hteti, htjedni/htjeti, ste/jesam, te/ti, tebe/ti, tebi/ti, tobom/ti (sr)</rdfs:comment>
        <rdfs:comment>e.g., bodita/biti, bodite/biti, bosta/biti, boste/biti, hodita/hoditi, imate/imeti, nimate/imeti, niste/biti, nočete/hoteti (sl)</rdfs:comment>
        <rdfs:comment>e.g., budete/byť, buďte/byť, majte/mať, máte/mať, nepostačíte/nestačiť, nepostačíš/nestačiť, nepovlečiete/nevliecť, nepožalujete/nežalovať, nepoženiete/nehnať (sk)</rdfs:comment>
        <rdfs:comment>e.g., dostaliście/dostać, jesteś/być, jesteście/być, otworzyłbyś/otworzyć, patrzcie/patrzeć, pozostałoś/pozostać, przestań/przestać, spotkałyście/spotkać, tobie/ty (pl)</rdfs:comment>
        <rdfs:comment>e.g., oleksite/olema, olete/olema, olite/olema, pidite/pidama, saite/saama, sinult/sina, sinust/sina, sinuta/sina, sult/sina (et)</rdfs:comment>
        <rdfs:comment>e.g., thee/you, thou, weren&apos;t/be+not (en)</rdfs:comment>
    </owl:Class>
    


    <!-- http://purl.org/olia/mte/multext-east.owl#SentenceCoordinatingConjunction -->

    <owl:Class rdf:about="http://purl.org/olia/mte/multext-east.owl#SentenceCoordinatingConjunction">
        <rdfs:subClassOf rdf:resource="http://purl.org/olia/mte/multext-east.owl#CoordinatingConjunction_ConjunctType"/>
        <rdfs:comment>Conjunction/Coord_Type=&quot;sentence&quot; (Serbian, Russian, Hungarian).</rdfs:comment>
    </owl:Class>
    


    <!-- http://purl.org/olia/mte/multext-east.owl#ShortArticle -->

    <owl:Class rdf:about="http://purl.org/olia/mte/multext-east.owl#ShortArticle">
        <rdfs:subClassOf rdf:resource="http://purl.org/olia/mte/multext-east.owl#AmbiguousDefinitenessFeature"/>
        <rdfs:subClassOf>
            <owl:Class>
                <owl:unionOf rdf:parseType="Collection">
                    <rdf:Description rdf:about="http://purl.org/olia/mte/multext-east.owl#CliticDeterminerType"/>
                    <rdf:Description rdf:about="http://purl.org/olia/mte/multext-east.owl#ReductionFeature"/>
                </owl:unionOf>
            </owl:Class>
        </rdfs:subClassOf>
        <rdfs:comment>e.g., 0, Абакумів/= Абрамів/= Авакумів/= Августин/= Августинів/= Августів/= Авенірів/= Аверкіїв/= Авер&apos;янів/= Авіятин/= Авксентіїв/= Аврамів/= Авреліїн/= Аврорин/= Автономів/= авторів/= авторчин/= Агапіїв/= Агапіїн/= Агапітів/=, абеткована/абеткований авізована/авізований акомпанована/акомпанований актована/актований аналізована/аналізований анкетована/анкетований анодована/анодований артикульована/артикульований балотована/балотований балувана/балуваний бальзамована/бальзамований банітована/банітований багнітована/багнітований байцьована/байцьований балакана/балаканий бачена/бачений белетризована/белетризований бережена/бережений бетонована/бетонований бинтована/бинтований, абетковане/абеткований авізоване/авізований акомпановане/акомпанований актоване/актований аналізоване/аналізований анкетоване/анкетований анодоване/анодований артикульоване/артикульований балотоване/балотований балуване/балуваний бальзамоване/бальзамований банітоване/банітований багнітоване/багнітований байцьоване/байцьований балакане/балаканий бачене/бачений белетризоване/белетризований бережене/бережений бетоноване/бетонований бинтоване/бинтований, абетковану/абеткований авізовану/авізований акомпановану/акомпанований актовану/актований аналізовану/аналізований анкетовану/анкетований анодовану/анодований артикульовану/артикульований балотовану/балотований балувану/балуваний бальзамовану/бальзамований банітовану/банітований багнітовану/багнітований байцьовану/байцьований балакану/балаканий бачену/бачений белетризовану/белетризований бережену/бережений бетоновану/бетонований бинтовану/бинтований, абетковані/абеткований авізовані/авізований акомпановані/акомпанований актовані/актований аналізовані/аналізований анкетовані/анкетований анодовані/анодований артикульовані/артикульований балотовані/балотований балувані/балуваний бальзамовані/бальзамований банітовані/банітований багнітовані/багнітований байцьовані/байцьований балакані/балаканий бачені/бачений белетризовані/белетризований бережені/бережений бетоновані/бетонований бинтовані/бинтований, аблактована/аблактований абонована/абонований абордована/абордований абортована/абортований абсолютизована/абсолютизований абстрагована/абстрагований абшитована/абшитований авансована/авансований автоматизована/автоматизований авторизована/авторизований агрегатована/агрегатований адаптована/адаптований адоптована/адоптований адресована/адресований адсорбована/адсорбований азотизована/азотизований азотована/азотований акліматизована/акліматизований акомодована/акомодований акредитована/акредитований, аблактоване/аблактований абоноване/абонований абордоване/абордований абортоване/абортований абсолютизоване/абсолютизований абстраговане/абстрагований абшитоване/абшитований авансоване/авансований автоматизоване/автоматизований авторизоване/авторизований агрегатоване/агрегатований адаптоване/адаптований адоптоване/адоптований адресоване/адресований адсорбоване/адсорбований азотизоване/азотизований азотоване/азотований акліматизоване/акліматизований акомодоване/акомодований акредитоване/акредитований, аблактовану/аблактований абоновану/абонований абордовану/абордований абортовану/абортований абсолютизовану/абсолютизований абстраговану/абстрагований абшитовану/абшитований авансовану/авансований автоматизовану/автоматизований авторизовану/авторизований агрегатовану/агрегатований адаптовану/адаптований адоптовану/адоптований адресовану/адресований адсорбовану/адсорбований азотизовану/азотизований азотовану/азотований акліматизовану/акліматизований акомодовану/акомодований акредитовану/акредитований (uk)</rdfs:comment>
        <rdfs:comment>e.g., ci/ty, cię/ty, go/on, go/ono, m/być, mi/ja, mię/ja, mu/on, mu/ono (pl)</rdfs:comment>
        <rdfs:comment>e.g., Награжден/награждать, Убит/убивать, Язвительно/язвительный, видимо/видеть, опровергнута/опровергать, прогнозируемо/прогнозировать, разрешаема/разрешать, реализуема/реализовать, реализуемо/реализовать (ru)</rdfs:comment>
        <rdfs:comment>e.g., бъдещия/бъда, вашия/ваш, всичкия, двайсетия/двайсет, десетия/десет, моя/мой, нашия/наш, неговия/негов, нейния/неин (bg)</rdfs:comment>
        <rdfs:comment>Definiteness=&quot;short-art&quot; (Noun: Bulgarian; Verb: Polish, Russian, Bulgarian; Adjective: : Polish, Russian, Ukrainian, Bulgarian; Pronoun: Polish, Bulgarian)&lt;br/&gt;

The Bulgarian singular masculine article has two forms: a full article(f)[l.s.] and a short article(s)[l.s.]. The full
article is used when a singular masculine form is the syntactic subject of the clause, otherwise a short one is
used – a purely orthographic rule. The distinction of full vs. short is not made for feminine, neuter and plural
forms, and we use just the yes(y) or no(n) to mark definiteness or respectively lack thereof. Therefore, the
definiteness attribute can take overall 4 different values: indefinite(n), definitive(y), short article(s), full
article(f) e.g., мъж, мъжа, мъжът /a man, the man[short], the man [full]/ (Dimitrova et al. 2009)&lt;br/&gt;

For Polish, the Vocalicity of (a)gglutinated forms like -em vs -m is mapped on the Definiteness attribute with its values &quot;(f)ull-art&quot; and &quot;(s)hort-art&quot; respectively, meaning &quot;full form&quot; and &quot;short form&quot;. The terms are very artificial, but this category is used due to the similarity of the phenomenon. The IPIC flexeme winien and predicatives like rad are thus treated as short adjectives—Definiteness=&quot;short-art&quot;. (MTE v.4)</rdfs:comment>
    </owl:Class>
    


    <!-- http://purl.org/olia/mte/multext-east.owl#SimpleAdposition -->

    <owl:Class rdf:about="http://purl.org/olia/mte/multext-east.owl#SimpleAdposition">
        <rdfs:subClassOf rdf:resource="http://purl.org/olia/mte/multext-east.owl#AdpositionFormation"/>
        <rdfs:comment>e.g., -mpotriva/împotriva, -naintea/înaintea, asupră/asupra (ro)</rdfs:comment>
        <rdfs:comment>e.g., dardu/dardu, h/h, na/na, od/od, ot/od, par/par, per/par, po/po, prid/prid (sl-rozaj)</rdfs:comment>
        <rdfs:comment>e.g., без біля близько в вві взамін вздовж від вколо внаслідок для до з задля замість заради зверх зверху звиш здовж, в за крізь меж межи на над невважаючи незважаючи о об перед під по повз поза поміж понад понадо поперед, в на о по попри при у ув уві, всупереч завдяки противно уздогін усупереч, з за із меж межи над наді надо перед передо під підо поза помежи поміж понад понадо поперед попід пред (uk)</rdfs:comment>
        <rdfs:comment>e.g., و/را رو/را را, پشتِ‌سر طي طرفِ/طرف (fa)</rdfs:comment>
        <rdfs:comment>Adposition/Formation=&quot;simple&quot;, i.e., non-compound adposition.</rdfs:comment>
    </owl:Class>
    


    <!-- http://purl.org/olia/mte/multext-east.owl#SimpleConjunction -->

    <owl:Class rdf:about="http://purl.org/olia/mte/multext-east.owl#SimpleConjunction">
        <rdfs:subClassOf rdf:resource="http://purl.org/olia/mte/multext-east.owl#ConjunctionFormation"/>
        <rdfs:comment>e.g., - (hu)</rdfs:comment>
        <rdfs:comment>e.g., ano/anu, anu/anu, k/ka, kir/kir, k’/ka, tácui/takoj (sl-rozaj)</rdfs:comment>
        <rdfs:comment>e.g., а або абощо але ані зате зачим і іно й йно но однак одначе притім притому причім причому проте та, аби адже аж аніж ба бо буцім буцімто все втім гейби доки допіру допоки же заки заким замісто зас коб (uk)</rdfs:comment>
        <rdfs:comment>e.g., حتي اگه/اگر اگر, طيِّ/طيّ ضمناً بلکه (fa)</rdfs:comment>
        <rdfs:comment>Formation=&quot;simple&quot;&lt;br/&gt;

Romanian: As with prepositions, we can distinguish two kinds of conjunctions in Romanian: (1) simple conjunctions: e.g. şi,dar,deşi etc. (2) conjunctions formed periphrastically, with some word/phrase combined by a conjunction: din moment ce, fără să, fat,ă de cum etc. (MTE v4)</rdfs:comment>
    </owl:Class>
    


    <!-- http://purl.org/olia/mte/multext-east.owl#SimpleCoordinatingConjunction -->

    <owl:Class rdf:about="http://purl.org/olia/mte/multext-east.owl#SimpleCoordinatingConjunction">
        <rdfs:subClassOf rdf:resource="http://purl.org/olia/mte/multext-east.owl#CoordinatingConjunction_PositionalType"/>
        <rdfs:comment>e.g., aşa_că, va_să_zică (ro)</rdfs:comment>
        <rdfs:comment>In the Romanian MTE v4 specs, Conjunction/Coord_Type=&quot;simple&quot; is defined in contrast to repetitive and correlative coordinating conjunctions.

In Romanian, there are three kinds of conjunctions depending on their usage: as such or together with other conjunctions or adverbs: (1) simple, between conjuncts: Ion ori Maria (John or Mary); (2) repetitive, before each conjunct: fie Ion fie Maria fie... (either John or Mary or...) (3) correlative, before a conjoined phrase, it requires specific coordinators between conjuncts: atât mama cât şi tata (both mother and father). (MTE v4)</rdfs:comment>
    </owl:Class>
    


    <!-- http://purl.org/olia/mte/multext-east.owl#SimpleInterjection -->

    <owl:Class rdf:about="http://purl.org/olia/mte/multext-east.owl#SimpleInterjection">
        <rdfs:subClassOf rdf:resource="http://purl.org/olia/mte/multext-east.owl#InterjectionFormation"/>
        <rdfs:comment>Interjection/Formation=&quot;simple&quot;</rdfs:comment>
    </owl:Class>
    


    <!-- http://purl.org/olia/mte/multext-east.owl#SimpleParticle -->

    <owl:Class rdf:about="http://purl.org/olia/mte/multext-east.owl#SimpleParticle">
        <rdfs:subClassOf rdf:resource="http://purl.org/olia/mte/multext-east.owl#ParticleFormation"/>
        <rdfs:comment>e.g., дали, ли, не, нима, нито (bg)</rdfs:comment>
        <rdfs:comment>Particle/Formation=&quot;simple&quot;</rdfs:comment>
    </owl:Class>
    


    <!-- http://purl.org/olia/mte/multext-east.owl#SingularNumber -->

    <owl:Class rdf:about="http://purl.org/olia/mte/multext-east.owl#SingularNumber">
        <rdfs:subClassOf rdf:resource="http://purl.org/olia/mte/multext-east.owl#Number"/>
        <rdfs:comment>e.g., -aceasta/acesta, -această/acest, -atât/atât, -atâta/atât, -istei, -istul, -istului, -istă, -mpărate/împărat (ro)</rdfs:comment>
        <rdfs:comment>e.g., 1900-tól/1900, 2050-től/2050, akiét/aki, Aladárét/Aladár, amelytől/amely, amiként/ami, amitől/ami, attól/az, azét/az (hu)</rdfs:comment>
        <rdfs:comment>e.g., Bratstvom/Bratstvo, Bratstvu/Bratstvo, devetogodišnji, drveta/drvo, Goldštajnov, htedni/hteti, htelo/hteti, hteo/hteti, htio/htjeti (sr)</rdfs:comment>
        <rdfs:comment>e.g., akredytującą/akredytować, autora/autor, czterdziestym/czterdziesty, czternastym/czternasty, czwartego/czwarty, czwartej/czwarty, czwartym/czwarty, czwartą/czwarty, czytelnika/czytelnik (pl)</rdfs:comment>
        <rdfs:comment>e.g., another, itself, wasn&apos;t/be+not, weren&apos;t/be+not (en)</rdfs:comment>
        <rdfs:comment>e.g., bit/bet, Chrishtianschin/krištijanski, Christusa/krïštuš, Christusam/krïštuš, cion/tët, Crishtusha/krïštuš, Dapiton/dapit, Elisabeto/elizabeta, etej/iti (sl-rozaj)</rdfs:comment>
        <rdfs:comment>e.g., chceš/chtít, chtěj/chtít, country, desaterý, desaterým/desaterý, desátá/desátý, devatenácté/devatenáctý, devatenáctému/devatenáctý, devatenáctým/devatenáctý (cs)</rdfs:comment>
        <rdfs:comment>e.g., endalt/ise, eneselt/ise, kellelt/kes, kelleta/kes, kt-ks/kt, millelt/mis, milleta/mis, minult/mina, minust/mina (et)</rdfs:comment>
        <rdfs:comment>e.g., hentej/hentá, henten, hentoho/henten, hentoho/hento, hentom/hento, hentomu/hento, hentou/hentá, hentá, hentú/hentá (sk)</rdfs:comment>
        <rdfs:comment>e.g., hoče/hoteti, hočem/hoteti, nočem/hoteti, nočeš/hoteti, teboj/ti, ti/=, tlelevš/=, trojen/=, tvoj/= (sl)</rdfs:comment>
    </owl:Class>
    


    <!-- http://purl.org/olia/mte/multext-east.owl#SingularQuantifier -->

    <owl:Class rdf:about="http://purl.org/olia/mte/multext-east.owl#SingularQuantifier">
        <rdfs:subClassOf rdf:resource="http://purl.org/olia/mte/multext-east.owl#NumeralAgreementClass"/>
        <rdfs:comment>A singular quantifier is a quantifier or a numeral that specifies a single referent from a set. (Chiarcos) 
In Czech and Slovak MTE v4 specs, the corresponding category Numeral/Class=&quot;definite1&quot; is applied to the numeral &quot;one&quot;. (MTE v4)</rdfs:comment>
        <owl:versionInfo>MTE v4 Numeral/Class=&quot;definite1&quot;. Renamed in accordance with PaucalQuantifier.

Numeral/Class=&quot;definite&quot;, Numeral/Class=&quot;definite1&quot;, Numeral/Class=&quot;definite234&quot; etc. refer to specific patterns of congruency with Slavic numerals that originate from the difference between Old Slavic singular (definite1), dual (definite2, definite234) and plural (definite).</owl:versionInfo>
    </owl:Class>
    


    <!-- http://purl.org/olia/mte/multext-east.owl#SociativeCase -->

    <owl:Class rdf:about="http://purl.org/olia/mte/multext-east.owl#SociativeCase">
        <rdfs:subClassOf rdf:resource="http://purl.org/olia/mte/multext-east.owl#Case"/>
        <rdfs:comment>e.g., -, gyökerestül/gyökér, levelestül/levél, mindenestül/minden (hu)</rdfs:comment>
        <rdfs:comment>Case=&quot;sociative&quot; (Hungarian)</rdfs:comment>
    </owl:Class>
    


    <!-- http://purl.org/olia/mte/multext-east.owl#SpecialNumeral -->

    <owl:Class rdf:about="http://purl.org/olia/mte/multext-east.owl#SpecialNumeral">
        <rdfs:subClassOf rdf:resource="http://purl.org/olia/mte/multext-east.owl#Numeral"/>
        <rdfs:comment>e.g., desaterý, desaterým/desaterý (cs)</rdfs:comment>
        <rdfs:comment>e.g., stotine/stotina (sr)</rdfs:comment>
        <rdfs:comment>e.g., trojen/= (sl)</rdfs:comment>
        <rdfs:comment>Numeral/Type=&quot;special&quot;</rdfs:comment>
    </owl:Class>
    


    <!-- http://purl.org/olia/mte/multext-east.owl#SpecifierAdverb -->

    <owl:Class rdf:about="http://purl.org/olia/mte/multext-east.owl#SpecifierAdverb">
        <rdfs:subClassOf rdf:resource="http://purl.org/olia/mte/multext-east.owl#Adverb"/>
        <rdfs:comment>Specifier Adverb: Adverb used to indicate degree. (http://www.unlweb.net/unlarium/dictionary/export_tagset.php)</rdfs:comment>
        <rdfs:comment>Adverb/Type=&quot;specifier&quot; (English)</rdfs:comment>
    </owl:Class>
    


    <!-- http://purl.org/olia/mte/multext-east.owl#StrongPronoun -->

    <owl:Class rdf:about="http://purl.org/olia/mte/multext-east.owl#StrongPronoun">
        <rdfs:subClassOf rdf:resource="http://purl.org/olia/mte/multext-east.owl#PronounForm"/>
        <rdfs:comment>e.g., domnia_sa, dumisale/dumneasa, dumitale/dumneata, dumneaei/dumnealui, dumnealor/dumnealui, dumnealui, dumneasa, dumneata, dumneavoastră (ro)</rdfs:comment>
        <rdfs:comment>Pronoun_form=&quot;strong&quot; (Romanian)&lt;br/&gt;

For Romanian we need an attribute (called Pronoun_Form) to make the distinction between strong and weak forms of the same personal pronoun or reflexive pronoun. All the weak forms can be adjoined to the adjacent words both proclitically or enclitically. In such cases the junction is always graphically marked by a hyphen between the pronoun and the neighboring word. The hyphen also marks possible elisions from either pronoun or the adjacent word. (MTE v4)</rdfs:comment>
    </owl:Class>
    


    <!-- http://purl.org/olia/mte/multext-east.owl#Subjunctive -->

    <owl:Class rdf:about="http://purl.org/olia/mte/multext-east.owl#Subjunctive">
        <rdfs:subClassOf rdf:resource="http://purl.org/olia/mte/multext-east.owl#VerbForm"/>
        <rdfs:comment>e.g., -nzestreze/înzestra, -nzidească/înzidi, -nzorzoneze/înzorzona, fii/fi, fim/fi, fiu/fi, fiţi/fi (ro)</rdfs:comment>
        <rdfs:comment>e.g., amai/amät, Bode/bet, bodete/bet, bodi/bet, bodite/bet, bodê/bet, pidè/pujtet, pride/prït, Prydy/prït (sl-rozaj)</rdfs:comment>
        <rdfs:comment>e.g., باشد/باش, باشم/باش, باشند/باش, باشه/باش باشد/باش آيد/آ, باشي/باش, باشيم/باش, بتوان/توان, بتواند/توان, بتوانم/توان (fa)</rdfs:comment>
        <rdfs:comment>In Resian, the subjunctive is formally identical to the imperative, with one form for the three persons in the singular and the forms for the 2nd and 3rd person plural being identical. (MTE v4)</rdfs:comment>
    </owl:Class>
    


    <!-- http://purl.org/olia/mte/multext-east.owl#SubjunctiveParticle -->

    <owl:Class rdf:about="http://purl.org/olia/mte/multext-east.owl#SubjunctiveParticle">
        <rdfs:subClassOf rdf:resource="http://purl.org/olia/mte/multext-east.owl#VerbalParticle"/>
        <rdfs:comment>e.g., s-/să, să (ro)</rdfs:comment>
        <rdfs:comment>Particle/Type=&quot;subjunctive&quot; (Romanian)

A verbal particle with Particle/Type=&quot;future&quot; modifies the verbs and marks the verb as being subjunctive (Dan Tufis, email 2010/06/09)</rdfs:comment>
    </owl:Class>
    


    <!-- http://purl.org/olia/mte/multext-east.owl#SublativeCase -->

    <owl:Class rdf:about="http://purl.org/olia/mte/multext-east.owl#SublativeCase">
        <rdfs:subClassOf rdf:resource="http://purl.org/olia/mte/multext-east.owl#Case"/>
        <rdfs:comment>e.g., -, 1970-re/1970, 2050-re/2050, akikre/aki, amelyekre/amely, azokra/az, derekukra/derék, egymásra/egymás, egytizedére/egytized (hu)</rdfs:comment>
        <rdfs:comment>Case=&quot;sublative&quot; (Hungarian)</rdfs:comment>
    </owl:Class>
    


    <!-- http://purl.org/olia/mte/multext-east.owl#SubordinatingConjunction -->

    <owl:Class rdf:about="http://purl.org/olia/mte/multext-east.owl#SubordinatingConjunction">
        <rdfs:subClassOf rdf:resource="http://purl.org/olia/mte/multext-east.owl#Conjunction"/>
        <rdfs:comment>e.g., - (hu)</rdfs:comment>
        <rdfs:comment>e.g., aby, abych/aby, abychom/aby, abys/aby, abyste/aby, kdyby, kdybych/kdyby, kdybychom/kdyby, kdybys/kdyby (cs)</rdfs:comment>
        <rdfs:comment>e.g., k/ka, kir/kir, k’/ka, mabej/mabej, sa ito kir/zajtökir, sauvocha/zawojoka (sl-rozaj)</rdfs:comment>
        <rdfs:comment>e.g., аби адже аж аніж ба бо буцім буцімто все втім гейби доки допіру допоки же заки заким замісто зас коб, аби-но аби-то все-таки для того щоб за винятком замість того щоб не вважаючи на те що не зважаючи на те що отож-то тим-то тільки-но тому що усе-таки якби-то (uk)</rdfs:comment>
        <rdfs:comment>e.g., به‌اين‌دليل‌که ازبس‌که ازآنجاکه, حتي اگه/اگر اگر (fa)</rdfs:comment>
        <rdfs:comment>Conjunction/Type=&quot;subordinating&quot;, for Romanian, Serbian and Russian further sub-classified by the Sub_Type attribute.

In Romanian, each conjunction requires another mood, so that the diversity may be controlled by subcategorisation rules. The attribute Sub_Type distinguishes among the positive and negative conjunctions, providing means to control verbal double negation, (as in case of the negative pronouns, determiners and adverbs): nici NU am venit, nimeni NU vorbeşte, nici_un tren N-a trecut, nicăieri N-am văzut (MTE v4)</rdfs:comment>
    </owl:Class>
    


    <!-- http://purl.org/olia/mte/multext-east.owl#SuperessiveCase -->

    <owl:Class rdf:about="http://purl.org/olia/mte/multext-east.owl#SuperessiveCase">
        <rdfs:subClassOf rdf:resource="http://purl.org/olia/mte/multext-east.owl#Case"/>
        <rdfs:comment>e.g., buktatóin/buktató, cselekedeteiteken/cselekedet, heteken/hét, mindkettőjükön/mindkettő, Rajta/ő, rajtad/te, rajtam/én, Rajtuk/ők, Rajtunk/mi (hu)</rdfs:comment>
        <rdfs:comment>Case=&quot;superessive&quot; (Hungarian)</rdfs:comment>
    </owl:Class>
    


    <!-- http://purl.org/olia/mte/multext-east.owl#SuperlativeDegree -->

    <owl:Class rdf:about="http://purl.org/olia/mte/multext-east.owl#SuperlativeDegree">
        <rdfs:subClassOf rdf:resource="http://purl.org/olia/mte/multext-east.owl#Degree"/>
        <rdfs:comment>e.g., -, legalsóból/alsó, legbensejét/benső, legjelentéktelenebbekké/jelentéktelen, legjobbaknak/jó, legjobbjai/jó, legjobbjait/jó, legjobbjaitól/jó, legjobbkor/jó (hu)</rdfs:comment>
        <rdfs:comment>e.g., aktuaalseimatesse/aktuaalseim, kiireimale/kiireim, kõrgeimale/kõrgeim, parimail/parim, parimale/parim, parimalt/parim, parimana/parim, parimateks/parim, parimatele/parim (et)</rdfs:comment>
        <rdfs:comment>e.g., best, least, most, worst (en)</rdfs:comment>
        <rdfs:comment>e.g., extra, preafericita/preafericit, preafericite/preafericit, preafericitei/preafericit, preafericitele/preafericit, preafericitelor/preafericit, preafericitul/preafericit, preafericitule/preafericit, preafericitului/preafericit (ro)</rdfs:comment>
        <rdfs:comment>e.g., najbardziej/bardzo, najbezpieczniejsze/bezpieczny, najbliżsi/bliski, najbliższe/bliski, najbliższego/bliski, najbliższej/bliski, najbliższy/bliski, najbliższych/bliski, najbliższym/bliski (pl)</rdfs:comment>
        <rdfs:comment>e.g., najbigotnije/bigotan, najbolje/dobar, najboljem/dobar, najbolji/dobar, najboljim/dobar, najdubljem/dubok, najgrublje/grub, najjednostavniji/jednostavan, najnevažnijim/nevažan (sr)</rdfs:comment>
        <rdfs:comment>e.g., najlipsi/lip, nej već/najveć, nejveć/najveć, Santissima/šantišim, Santiſshima/šantišim, Santiſsim/šantišim, Santiſsima/šantišim (sl-rozaj)</rdfs:comment>
        <rdfs:comment>e.g., največja/velik, največji/velik (sl)</rdfs:comment>
        <rdfs:comment>e.g., najžobravejšie/žobravo, najžoviálnejšej/žoviálny, najžoviálnejšia/žoviálny, najžoviálnejšie/žoviálne, najžoviálnejšie/žoviálny, najžoviálnejšieho/žoviálny, najžoviálnejšiemu/žoviálny, najžoviálnejšiu/žoviálny, najžoviálnejšom/žoviálny (sk)</rdfs:comment>
        <rdfs:comment>e.g., nejubožejšími/ubohý, nejvyspělejších/vyspělý, nejvyšších/vysoký, nejvznešenějšímu/vznešený, nejvážnějšímu/vážný, nejvýznamnějších/významný, nejvýznamnějšími/významný, nejvýznamnějšímu/významný, největšími/velký (cs)</rdfs:comment>
        <rdfs:comment>e.g., найбезпечніше найбільш найбільше найближче найважче найвишуканіше найвище найвідповідніше найгірш найгірше найглибше найгучніше найдалі найдальше найдетальніше найдешевше найдовше найдорожче найдошкульніше найдрібніше, найголодніша/найголодніший найазартніша/найазартніший найактивніша/найактивніший найактуальніша/найактуальніший найамбітніша/найамбітніший найамбіційніша/найамбіційніший найамбіціозніша/найамбіціозніший найапетитніша/найапетитніший найароматніша/найароматніший найбагатіша/найбагатіший найбагатша/найбагатший найбадьоріша/найбадьоріший найбажаніша/найбажаніший найбалакливіша/найбалакливіший найбалакучіша/найбалакучіший найбезпечніша/найбезпечніший найбентежніша/найбентежніший найбережливіша/найбережливіший найбідніша/найбідніший найбіліша/найбіліший, найголоднішая/найголодніший найазартнішая/найазартніший найактивнішая/найактивніший найактуальнішая/найактуальніший найамбітнішая/найамбітніший найамбіційнішая/найамбіційніший найамбіціознішая/найамбіціозніший найапетитнішая/найапетитніший найароматнішая/найароматніший найбагатішая/найбагатіший найбагатшая/найбагатший найбадьорішая/найбадьоріший найбажанішая/найбажаніший найбалакливішая/найбалакливіший найбалакучішая/найбалакучіший найбезпечнішая/найбезпечніший найбентежнішая/найбентежніший найбережливішая/найбережливіший найбіднішая/найбідніший найбілішая/найбіліший, найголодніше/найголодніший найазартніше/найазартніший найактивніше/найактивніший найактуальніше/найактуальніший найамбітніше/найамбітніший найамбіційніше/найамбіційніший найамбіціозніше/найамбіціозніший найапетитніше/найапетитніший найароматніше/найароматніший найбагатіше/найбагатіший найбагатше/найбагатший найбадьоріше/найбадьоріший найбажаніше/найбажаніший найбалакливіше/найбалакливіший найбалакучіше/найбалакучіший найбезпечніше/найбезпечніший найбентежніше/найбентежніший найбережливіше/найбережливіший найбідніше/найбідніший найбіліше/найбіліший, найголоднішеє/найголодніший найазартнішеє/найазартніший найактивнішеє/найактивніший найактуальнішеє/найактуальніший найамбітнішеє/найамбітніший найамбіційнішеє/найамбіційніший найамбіціознішеє/найамбіціозніший найапетитнішеє/найапетитніший найароматнішеє/найароматніший найбагатішеє/найбагатіший найбагатшеє/найбагатший найбадьорішеє/найбадьоріший найбажанішеє/найбажаніший найбалакливішеє/найбалакливіший найбалакучішеє/найбалакучіший найбезпечнішеє/найбезпечніший найбентежнішеє/найбентежніший найбережливішеє/найбережливіший найбіднішеє/найбідніший найбілішеє/найбіліший, найголодніший/= найазартніший/= найактивніший/= найактуальніший/= найамбітніший/= найамбіційніший/= найамбіціозніший/= найапетитніший/= найароматніший/= найбагатіший/= найбагатший/= найбадьоріший/= найбажаніший/= найбалакливіший/= найбалакучіший/= найбезпечніший/= найбентежніший/= найбережливіший/= найбідніший/= найбіліший/=, найголоднішим/найголодніший найазартнішим/найазартніший найактивнішим/найактивніший найактуальнішим/найактуальніший найамбітнішим/найамбітніший найамбіційнішим/найамбіційніший найамбіціознішим/найамбіціозніший найапетитнішим/найапетитніший найароматнішим/найароматніший найбагатішим/найбагатіший найбагатшим/найбагатший найбадьорішим/найбадьоріший найбажанішим/найбажаніший найбалакливішим/найбалакливіший найбалакучішим/найбалакучіший найбезпечнішим/найбезпечніший найбентежнішим/найбентежніший найбережливішим/найбережливіший найбіднішим/найбідніший найбілішим/найбіліший, найголоднішими/найголодніший найазартнішими/найазартніший найактивнішими/найактивніший найактуальнішими/найактуальніший найамбітнішими/найамбітніший найамбіційнішими/найамбіційніший найамбіціознішими/найамбіціозніший найапетитнішими/найапетитніший найароматнішими/найароматніший найбагатішими/найбагатіший найбагатшими/найбагатший найбадьорішими/найбадьоріший найбажанішими/найбажаніший найбалакливішими/найбалакливіший найбалакучішими/найбалакучіший найбезпечнішими/найбезпечніший найбентежнішими/найбентежніший найбережливішими/найбережливіший найбіднішими/найбідніший найбілішими/найбіліший, найголодніших/найголодніший найазартніших/найазартніший найактивніших/найактивніший найактуальніших/найактуальніший найамбітніших/найамбітніший найамбіційніших/найамбіційніший найамбіціозніших/найамбіціозніший найапетитніших/найапетитніший найароматніших/найароматніший найбагатіших/найбагатіший найбагатших/найбагатший найбадьоріших/найбадьоріший найбажаніших/найбажаніший найбалакливіших/найбалакливіший найбалакучіших/найбалакучіший найбезпечніших/найбезпечніший найбентежніших/найбентежніший найбережливіших/найбережливіший найбідніших/найбідніший найбіліших/найбіліший (uk)</rdfs:comment>
        <rdfs:comment>e.g., најшпионска/шпионски, најшпионскава/шпионски, најшпионскана/шпионски, најшпионската/шпионски, најшпионски/шпионски, најшпионскиве/шпионски, најшпионскине/шпионски, најшпионскиов/шпионски, најшпионскион/шпионски (mk)</rdfs:comment>
        <rdfs:comment>e.g., متعصّب‌ترين/متعصّب قديمي‌ترين/قديمي ترسناک‌ترين/ترسناک (fa)</rdfs:comment>
    </owl:Class>
    


    <!-- http://purl.org/olia/mte/multext-east.owl#Supine -->

    <owl:Class rdf:about="http://purl.org/olia/mte/multext-east.owl#Supine">
        <rdfs:subClassOf rdf:resource="http://purl.org/olia/mte/multext-east.owl#VerbForm"/>
        <rdfs:comment>e.g., olemast/olema, olemata/olema, paistmas/paistma, pidamast/pidama, pidamata/pidama, saamata/saama (et)</rdfs:comment>
        <rdfs:comment>e.g., spat/spät (sl-rozaj)</rdfs:comment>
        <rdfs:comment>VForm=&quot;supine&quot; (Slovene, Estonian)&lt;br/&gt;

In Romanian, Supine appears mostly with a preposition, except for a few intransitive verbs when they are subordinated to the impersonal verb a trebui (must). Only the preposition allows for differentiating a supine from a participle-masculine-singular. It was thus left out from Romanian MTE v4 specs. (MTE v4)</rdfs:comment>
    </owl:Class>
    


    <!-- http://purl.org/olia/mte/multext-east.owl#SyntacticType -->

    <owl:Class rdf:about="http://purl.org/olia/mte/multext-east.owl#SyntacticType">
        <rdfs:subClassOf rdf:resource="http://purl.org/olia/mte/multext-east.owl#MorphosyntacticFeature"/>
        <rdfs:comment>Syntactic_Type is used to distinguish the nominal and adjectival function of Pronouns in Croatian, Slovak, Resian and Czech. In Czech and Slovak, pronouns are distinguished between having a (syntactically) nominal and (syntactically) adjectival function, e.g. Slovak ktorý, môj. All pronominal types except the demonstrative and possessive one can be nominal, and all except for the personal one can be adjectival. Furthermore, in Slovene and Serbian, the adverbial function of certain Pronouns is distinguished. (MTE v4) This distinction is absent in the Bulgarian language (there are no adjectival pronouns of this type). Slovak also has several quasi-adjectival pronouns classified as Syntactic_Type=&quot;adjectival&quot; (e.g. tvoj), equivalents of which do exist in Bulgarian as well, but due to lack of the clear distinction of adjectival paradigm it was not felt unnecessary to introduce this value in Bulgarian MTE (Dimitrova et al. 2009)&lt;br/&gt;

Also used in Abbreviations to signal the Part of Speech of the abbreviation in Romanian and Estonian. Although the values for this attribute could range over the part of speech categories in the language, in Romanian most of the abbreviations falls into noun class. (MTE v4)</rdfs:comment>
        <owl:versionInfo>TODO: Redefine SyntacticType as a property.</owl:versionInfo>
    </owl:Class>
    


    <!-- http://purl.org/olia/mte/multext-east.owl#TemporalisCase -->

    <owl:Class rdf:about="http://purl.org/olia/mte/multext-east.owl#TemporalisCase">
        <rdfs:subClassOf rdf:resource="http://purl.org/olia/mte/multext-east.owl#Case"/>
        <rdfs:comment>The so-called Temporalis Case is formed in Hungarian with -kor. Expresses a point of time or a period. (http://member.melbpc.org.au/~tmajlath/form-suffix.html)</rdfs:comment>
        <rdfs:comment>e.g., lapzártánkkor/lapzárta, megszületésükkor/megszületés, múltkor/múlt, tanulmányozásakor/tanulmányozás, választáskor/választás, változtatásakor/változtatás (hu)</rdfs:comment>
        <rdfs:comment>Case=&quot;temporalis&quot; (Hungarian)</rdfs:comment>
    </owl:Class>
    


    <!-- http://purl.org/olia/mte/multext-east.owl#Tense -->

    <owl:Class rdf:about="http://purl.org/olia/mte/multext-east.owl#Tense">
        <rdfs:subClassOf rdf:resource="http://purl.org/olia/mte/multext-east.owl#MorphosyntacticFeature"/>
    </owl:Class>
    


    <!-- http://purl.org/olia/mte/multext-east.owl#TerminativeCase -->

    <owl:Class rdf:about="http://purl.org/olia/mte/multext-east.owl#TerminativeCase">
        <rdfs:subClassOf rdf:resource="http://purl.org/olia/mte/multext-east.owl#Case"/>
        <rdfs:comment>e.g., -, 2050-ig/2050, addig/az, csontjaiig/csont, eddig/ez, elkészültéig/elkészült, halálodig/halál, halálomig/halál, halálukig/halál (hu)</rdfs:comment>
        <rdfs:comment>e.g., Kallasteni/Kallas, meieni/mina, miljonendani/miljones, milleni/mis, minuni/mina, nendeni/see, nendeni/tema, rõivavalmistajateni/rõivavalmistaja, selleni/see (et)</rdfs:comment>
        <rdfs:comment>Case=&quot;terminative&quot; (Estonian, Hungarian)</rdfs:comment>
    </owl:Class>
    


    <!-- http://purl.org/olia/mte/multext-east.owl#ThirdPerson -->

    <owl:Class rdf:about="http://purl.org/olia/mte/multext-east.owl#ThirdPerson">
        <rdfs:subClassOf rdf:resource="http://purl.org/olia/mte/multext-east.owl#Person"/>
        <rdfs:comment>e.g., &apos;Em/them, another, itself, others, their, theirs, them, themselves, there (en)</rdfs:comment>
        <rdfs:comment>e.g., -aceasta/acesta, -această/acest, -astea/ăsta, -atât/atât, -atâta/atât, -nzestraseră/înzestra, -nzestreze/înzestra, -ăştia/ăsta, alte/alt (ro)</rdfs:comment>
        <rdfs:comment>e.g., akiktől/aki, akiét/aki, amelyekért/amely, amelytől/amely, amiként/ami, amitől/ami, attól/az, azoktól/az, azét/az (hu)</rdfs:comment>
        <rdfs:comment>e.g., bosta/biti, hoče/hoteti, hočejo/hoteti, hočeta/hoteti, imata/imeti, nimata/imeti, nočejo/hoteti, nočeta/hoteti, sta/biti (sl)</rdfs:comment>
        <rdfs:comment>e.g., dostane/dostat, dostanou/dostat, nedostane/dostat, nedostanou/dostat (cs)</rdfs:comment>
        <rdfs:comment>e.g., hardéhata/tet, hardéše/tet, herdého/tet, idu/tet, ostane/ostät, pidè/pujtet, poznahata/poznät, pravijahata/pravit, prašávahata/pravit (sl-rozaj)</rdfs:comment>
        <rdfs:comment>e.g., jest/być, pogniotłyby/pognieść, przedostałyby/przedostać, wystarczy/wystarczyć, wystarczyłoby/wystarczyć, zostanie/zostać, zostaną/zostać, zostałaby/zostać, zostałyby/zostać (pl)</rdfs:comment>
        <rdfs:comment>e.g., jeste/jesam, okrete/okrenuti, će/hteti, će/htjeti (sr)</rdfs:comment>
        <rdfs:comment>e.g., nad/tema, neid/tema, neidki/tema, neile/tema, neilegi/tema, neilt/tema, neis/tema, neisse/tema, neist/tema (et)</rdfs:comment>
        <rdfs:comment>e.g., nepostačia/nestačiť, nepostačí/nestačiť, nezvestuje/nezvestovať, nezvestujú/nezvestovať, postačia/stačiť, postačí/stačiť (sk)</rdfs:comment>
        <rdfs:comment>Although in traditional grammar books the demonstrative, indefinite and int_rel determiners are not characterised by person, in the Romanian MTE dictionaries they are recorded (for reasons beyond morpho-lexical encoding) as 3rd person (the same as nouns). However, for the automatic tagging this value has been marked as irrelevant. (MTE v4)</rdfs:comment>
    </owl:Class>
    


    <!-- http://purl.org/olia/mte/multext-east.owl#Transgressive -->

    <owl:Class rdf:about="http://purl.org/olia/mte/multext-east.owl#Transgressive">
        <owl:equivalentClass>
            <owl:Class>
                <owl:intersectionOf rdf:parseType="Collection">
                    <rdf:Description rdf:about="http://purl.org/olia/mte/multext-east.owl#GerundOrAdverbialParticiple"/>
                    <owl:Class>
                        <owl:complementOf rdf:resource="http://purl.org/olia/mte/multext-east.owl#Noun"/>
                    </owl:Class>
                </owl:intersectionOf>
            </owl:Class>
        </owl:equivalentClass>
        <rdfs:subClassOf rdf:resource="http://purl.org/olia/mte/multext-east.owl#GerundOrAdverbialParticiple"/>
        <rdfs:subClassOf rdf:resource="http://purl.org/olia/mte/multext-east.owl#Participle"/>
        <rdfs:comment>e.g., nezvestujúc/nezvestovať (sk)</rdfs:comment>
        <rdfs:comment>‘Transgressive’ and ‘Gerund’ refer to the same category, but the former is used in the tagsets for Czech and Slovak and the latter for Bulgarian and Serbian (Derzhanski and Kotsyba, 2009). This is just a difference in description (Dimitrova et al. 2009), therefore, both are identified here. (Note: this entails that Transgressive is-a Participle)

Verb/VForm=&quot;gerund&quot; is, however, ambiguous: with respect to Latin, in whose grammatical tradition it originates, it refers to a  deverbal noun, and is needed in this function for Polish as well; in descriptions of some other languages, however, it has been used for an adverbial participle.  The two meanings have nothing in common, except that the English _ing_-form can translate both.
(Ivan A Derzhanski, email 2010/06/09)</rdfs:comment>
        <owl:versionInfo>introduced to account for the term &quot;gerund&quot; if applied to non-nominal participles.</owl:versionInfo>
    </owl:Class>
    


    <!-- http://purl.org/olia/mte/multext-east.owl#Transitive -->

    <owl:Class rdf:about="http://purl.org/olia/mte/multext-east.owl#Transitive">
        <rdfs:subClassOf rdf:resource="http://purl.org/olia/mte/multext-east.owl#Transitivity"/>
        <rdfs:comment>Transitive=&quot;yes&quot; (Persian)</rdfs:comment>
    </owl:Class>
    


    <!-- http://purl.org/olia/mte/multext-east.owl#Transitivity -->

    <owl:Class rdf:about="http://purl.org/olia/mte/multext-east.owl#Transitivity">
        <rdfs:subClassOf rdf:resource="http://purl.org/olia/mte/multext-east.owl#MorphosyntacticFeature"/>
        <rdfs:comment>feature &quot;Transitive&quot;</rdfs:comment>
    </owl:Class>
    


    <!-- http://purl.org/olia/mte/multext-east.owl#TranslativeCase -->

    <owl:Class rdf:about="http://purl.org/olia/mte/multext-east.owl#TranslativeCase">
        <rdfs:subClassOf rdf:resource="http://purl.org/olia/mte/multext-east.owl#Case"/>
        <rdfs:comment>e.g., esimesteks/esimene, kelleks/kes, kt-ks/kt, kõigiks/kõik, kümneteks/kümme, milleks/mis, muudeks/muu, nendeks/tema, nendekski/tema (et)</rdfs:comment>
        <rdfs:comment>Case=&quot;translative&quot; (Estonian)</rdfs:comment>
    </owl:Class>
    


    <!-- http://purl.org/olia/mte/multext-east.owl#Typo -->

    <owl:Class rdf:about="http://purl.org/olia/mte/multext-east.owl#Typo">
        <rdfs:subClassOf rdf:resource="http://purl.org/olia/mte/multext-east.owl#Residual"/>
        <rdfs:comment>In the Slovene MTE v4 specs, Residual/Type=&quot;typo&quot; marks a mis-typed word. (MTE v4)</rdfs:comment>
    </owl:Class>
    


    <!-- http://purl.org/olia/mte/multext-east.owl#UniquitiveDeterminer -->

    <owl:Class rdf:about="http://purl.org/olia/mte/multext-east.owl#UniquitiveDeterminer">
        <rdfs:subClassOf rdf:resource="http://purl.org/olia/mte/multext-east.owl#Determiner"/>
        <rdfs:comment>Determiner/Type=&quot;exceptional&quot; is applied to the Persian uniquitive determiner تنها  i.e., &quot;the only&quot; (MTE v4; Hamidreza Kobdani, email 2010/06/15)</rdfs:comment>
    </owl:Class>
    


    <!-- http://purl.org/olia/mte/multext-east.owl#Verb -->

    <owl:Class rdf:about="http://purl.org/olia/mte/multext-east.owl#Verb">
        <rdfs:subClassOf rdf:resource="http://purl.org/olia/mte/multext-east.owl#MorphosyntacticCategory"/>
        <rdfs:subClassOf>
            <owl:Restriction>
                <owl:onProperty rdf:resource="http://purl.org/olia/mte/multext-east.owl#hasVerbForm"/>
                <owl:cardinality rdf:datatype="http://www.w3.org/2001/XMLSchema#nonNegativeInteger">1</owl:cardinality>
            </owl:Restriction>
        </rdfs:subClassOf>
        <rdfs:subClassOf>
            <owl:Restriction>
                <owl:onProperty rdf:resource="http://purl.org/olia/mte/multext-east.owl#hasAnimacy"/>
                <owl:maxCardinality rdf:datatype="http://www.w3.org/2001/XMLSchema#nonNegativeInteger">1</owl:maxCardinality>
            </owl:Restriction>
        </rdfs:subClassOf>
        <rdfs:subClassOf>
            <owl:Restriction>
                <owl:onProperty rdf:resource="http://purl.org/olia/mte/multext-east.owl#hasAspect"/>
                <owl:maxCardinality rdf:datatype="http://www.w3.org/2001/XMLSchema#nonNegativeInteger">1</owl:maxCardinality>
            </owl:Restriction>
        </rdfs:subClassOf>
        <rdfs:subClassOf>
            <owl:Restriction>
                <owl:onProperty rdf:resource="http://purl.org/olia/mte/multext-east.owl#hasCase"/>
                <owl:maxCardinality rdf:datatype="http://www.w3.org/2001/XMLSchema#nonNegativeInteger">1</owl:maxCardinality>
            </owl:Restriction>
        </rdfs:subClassOf>
        <rdfs:subClassOf>
            <owl:Restriction>
                <owl:onProperty rdf:resource="http://purl.org/olia/mte/multext-east.owl#hasClitic"/>
                <owl:maxCardinality rdf:datatype="http://www.w3.org/2001/XMLSchema#nonNegativeInteger">1</owl:maxCardinality>
            </owl:Restriction>
        </rdfs:subClassOf>
        <rdfs:subClassOf>
            <owl:Restriction>
                <owl:onProperty rdf:resource="http://purl.org/olia/mte/multext-east.owl#hasCourtesy"/>
                <owl:maxCardinality rdf:datatype="http://www.w3.org/2001/XMLSchema#nonNegativeInteger">1</owl:maxCardinality>
            </owl:Restriction>
        </rdfs:subClassOf>
        <rdfs:subClassOf>
            <owl:Restriction>
                <owl:onProperty rdf:resource="http://purl.org/olia/mte/multext-east.owl#hasDefiniteness"/>
                <owl:maxCardinality rdf:datatype="http://www.w3.org/2001/XMLSchema#nonNegativeInteger">1</owl:maxCardinality>
            </owl:Restriction>
        </rdfs:subClassOf>
        <rdfs:subClassOf>
            <owl:Restriction>
                <owl:onProperty rdf:resource="http://purl.org/olia/mte/multext-east.owl#hasGender"/>
                <owl:maxCardinality rdf:datatype="http://www.w3.org/2001/XMLSchema#nonNegativeInteger">1</owl:maxCardinality>
            </owl:Restriction>
        </rdfs:subClassOf>
        <rdfs:subClassOf>
            <owl:Restriction>
                <owl:onProperty rdf:resource="http://purl.org/olia/mte/multext-east.owl#hasHumanness"/>
                <owl:maxCardinality rdf:datatype="http://www.w3.org/2001/XMLSchema#nonNegativeInteger">1</owl:maxCardinality>
            </owl:Restriction>
        </rdfs:subClassOf>
        <rdfs:subClassOf>
            <owl:Restriction>
                <owl:onProperty rdf:resource="http://purl.org/olia/mte/multext-east.owl#hasNegation"/>
                <owl:maxCardinality rdf:datatype="http://www.w3.org/2001/XMLSchema#nonNegativeInteger">1</owl:maxCardinality>
            </owl:Restriction>
        </rdfs:subClassOf>
        <rdfs:subClassOf>
            <owl:Restriction>
                <owl:onProperty rdf:resource="http://purl.org/olia/mte/multext-east.owl#hasNumber"/>
                <owl:maxCardinality rdf:datatype="http://www.w3.org/2001/XMLSchema#nonNegativeInteger">1</owl:maxCardinality>
            </owl:Restriction>
        </rdfs:subClassOf>
        <rdfs:subClassOf>
            <owl:Restriction>
                <owl:onProperty rdf:resource="http://purl.org/olia/mte/multext-east.owl#hasPerson"/>
                <owl:maxCardinality rdf:datatype="http://www.w3.org/2001/XMLSchema#nonNegativeInteger">1</owl:maxCardinality>
            </owl:Restriction>
        </rdfs:subClassOf>
        <rdfs:subClassOf>
            <owl:Restriction>
                <owl:onProperty rdf:resource="http://purl.org/olia/mte/multext-east.owl#hasTense"/>
                <owl:maxCardinality rdf:datatype="http://www.w3.org/2001/XMLSchema#nonNegativeInteger">1</owl:maxCardinality>
            </owl:Restriction>
        </rdfs:subClassOf>
        <rdfs:subClassOf>
            <owl:Restriction>
                <owl:onProperty rdf:resource="http://purl.org/olia/mte/multext-east.owl#hasTransitivity"/>
                <owl:maxCardinality rdf:datatype="http://www.w3.org/2001/XMLSchema#nonNegativeInteger">1</owl:maxCardinality>
            </owl:Restriction>
        </rdfs:subClassOf>
        <rdfs:subClassOf>
            <owl:Restriction>
                <owl:onProperty rdf:resource="http://purl.org/olia/mte/multext-east.owl#hasVoice"/>
                <owl:maxCardinality rdf:datatype="http://www.w3.org/2001/XMLSchema#nonNegativeInteger">1</owl:maxCardinality>
            </owl:Restriction>
        </rdfs:subClassOf>
        <rdfs:comment>e.g., -nzestrarăm/înzestra, -nzestrarăţi/înzestra, -nzestrasem/înzestra, -nzestraseră/înzestra, -nzestraserăm/înzestra, -nzestraserăţi/înzestra, -nzestraseşi/înzestra, -nzestraţi/înzestra, -nzestreze/înzestra (ro)</rdfs:comment>
        <rdfs:comment>e.g., amaite/amät, bet/bet, bit/bet, biti/bet, bodete/bet, bodite/bet, bota/bet, Ciete/tët, cion/tët (sl-rozaj)</rdfs:comment>
        <rdfs:comment>e.g., bejt/být, budete/být, byste/by, chceme/chtít, chcete/chtít, chceš/chtít, chtěj/chtít, dejte/dát, dostal/dostat (cs)</rdfs:comment>
        <rdfs:comment>e.g., biste/biti, bićete/biti, htedni/hteti, htednimo/hteti, htele/hteti, htelo/hteti, hteo/hteti, hteti, htio/htjeti (sr)</rdfs:comment>
        <rdfs:comment>e.g., bodita/biti, bodite/biti, bosta/biti, boste/biti, hodita/hoditi, hoče/hoteti, hočejo/hoteti, hočem/hoteti, hočeta/hoteti (sl)</rdfs:comment>
        <rdfs:comment>e.g., budete/byť, buďte/byť, majte/mať, máte/mať, nepostačia/nestačiť, nepostačí/nestačiť, nepostačím/nestačiť, nepostačíme/nestačiť, nepostačíte/nestačiť (sk)</rdfs:comment>
        <rdfs:comment>e.g., daren&apos;t/dare+not, oughter/have, wasn&apos;t/be+not, weren&apos;t/be+not (en)</rdfs:comment>
        <rdfs:comment>e.g., dostali/dostat (cs)</rdfs:comment>
        <rdfs:comment>e.g., dostaliście/dostać, dostałyśmy/dostać, dotyczyły/dotyczyć, jest/być, jesteś/być, jesteście/być, jesteśmy/być, nastąpił/nastąpić, otrzymali/otrzymać (pl)</rdfs:comment>
        <rdfs:comment>e.g., dostaliście/dostać, dostałyśmy/dostać, otrzymali/otrzymać, otrzymaliśmy/otrzymać, otworzyłbyś/otworzyć, pogniotłyby/pognieść, pozostałoś/pozostać, przedostałyby/przedostać, spotkałyście/spotkać (pl)</rdfs:comment>
        <rdfs:comment>e.g., elárultalak/elárul, figyelmeztettelek/figyelmeztet, lennétek/lesz, megismertelek/megismer, továbbtaníttatnátok/továbbtaníttat, tudnálak/tud, tudnátok/tud, uralhatjátok/uralhat, veszélyeztetné/veszélyeztet (hu)</rdfs:comment>
        <rdfs:comment>e.g., oleksite/olema, olemast/olema, olemata/olema, olete/olema, olevat/olema, olevatki/olema, olite/olema, paistes/paistma, paistmas/paistma (et)</rdfs:comment>
        <rdfs:comment>e.g., ste/jesam, će/hteti, će/htjeti, ćemo/hteti, ćemo/htjeti, ćete/hteti, ćete/htjeti, ćeš/hteti, ćeš/htjeti (sr)</rdfs:comment>
    </owl:Class>
    


    <!-- http://purl.org/olia/mte/multext-east.owl#VerbForm -->

    <owl:Class rdf:about="http://purl.org/olia/mte/multext-east.owl#VerbForm">
        <rdfs:subClassOf rdf:resource="http://purl.org/olia/mte/multext-east.owl#MorphosyntacticFeature"/>
        <rdfs:comment>Feature &quot;VForm&quot; of verbs</rdfs:comment>
    </owl:Class>
    


    <!-- http://purl.org/olia/mte/multext-east.owl#Verbal -->

    <owl:Class rdf:about="http://purl.org/olia/mte/multext-east.owl#Verbal">
        <rdfs:subClassOf rdf:resource="http://purl.org/olia/mte/multext-east.owl#SyntacticType"/>
        <rdfs:comment>Abbreviation/Syntactic_Type=&quot;verbal&quot;</rdfs:comment>
    </owl:Class>
    


    <!-- http://purl.org/olia/mte/multext-east.owl#VerbalAdverb -->

    <owl:Class rdf:about="http://purl.org/olia/mte/multext-east.owl#VerbalAdverb">
        <rdfs:subClassOf rdf:resource="http://purl.org/olia/mte/multext-east.owl#Adverb"/>
        <rdfs:comment>Adverb/Type=&quot;verbal&quot; applies to adverbs derived from from verbs (verbal adverbs) in the Serbian, Macedonian and Hungarian MTE v4 specs. Macedonian verbal adverbs (gerunds) like odejkji are thus not considered as verbal forms, but as Adverb/Type=&quot;verbal&quot;. (MTE v4)</rdfs:comment>
    </owl:Class>
    


    <!-- http://purl.org/olia/mte/multext-east.owl#VerbalParticle -->

    <owl:Class rdf:about="http://purl.org/olia/mte/multext-east.owl#VerbalParticle">
        <rdfs:subClassOf rdf:resource="http://purl.org/olia/mte/multext-east.owl#Particle"/>
        <rdfs:comment>A verbal particle modifies the verb and carries information on the verb form (e.g., finiteness, tense and aspect). (Dimitrova et al. 2009, Dan Tufis, email 2010/06/09).

In the Bulgarian MTE specs, Particle/Type=verbal(v) is used to form different type of verbal syntactical relationships, e.g. to create future tense (ще говориш), or particles like се, да. (Dimitrova et al. 2009) 
The Romanian MTE v4 specs provide a more fine-grained subclassification of (verbal) particles (MTE v4)</rdfs:comment>
        <owl:versionInfo>[Romanian] Particle, as a word class, modifies the verbs and carry information on verb form (negated form, infinitive form, on aspect and subjunctive present or future time) (Dan Tufis, email 2010/06/09)&lt;br/&gt;
=&gt; regrouped under VerbalParticiple.</owl:versionInfo>
    </owl:Class>
    


    <!-- http://purl.org/olia/mte/multext-east.owl#VocativeCase -->

    <owl:Class rdf:about="http://purl.org/olia/mte/multext-east.owl#VocativeCase">
        <rdfs:subClassOf rdf:resource="http://purl.org/olia/mte/multext-east.owl#Case"/>
        <rdfs:comment>e.g., -mpărate/împărat, bătrâne/bătrân, d-le/domnule, d-lor/doamnelor, d-lor/domnilor, dragă/drag, iubite/iubit, liderelor/lideră, mânuitorilor/mânuitor (ro)</rdfs:comment>
        <rdfs:comment>e.g., Jevrejke/Jevrejka, muški/muško, ti, vi, zlomislitelje/zlomislitelj, Zlomislitelju/Zlomislitelj, zločinče/zločinac, železnička/železnički, železničke/železnički (sr)</rdfs:comment>
        <rdfs:comment>e.g., Weberovi/Weberův, Wertherovi/Wertherův, Winstonovi/Winstonův, Winstonovy/Winstonův, zbrojířovy/zbrojířův, Zuzančiny/Zuzančin (cs)</rdfs:comment>
        <rdfs:comment>e.g., boże/bóg, brawo/brawo, chłopaki/chłopak, chłopcy/chłopiec, dobra/dobro, dzieci/dziecko, dziecko/dziecko, izby/izba, kochanie/kochanie (pl)</rdfs:comment>
        <rdfs:comment>e.g., druhá/druhý, druhé/druhý, druhí/druhý, druhý, dva, dvaja/dva, dve/dva, hentie/henten, hentie/hento (sk)</rdfs:comment>
        <rdfs:comment>e.g., Аахене/Аахен Абаю/Абай Абакане/Абакан Абакане/Абакан Абіджане/Абіджан Абовяне/Абовян Авентине/Авентин Адамстауне/Адамстаун Адене/Аден Аджаристане/Аджаристан Адлере/Адлер Адонісе/Адоніс Адріанополю/Адріанополь Азенкуре/Азенкур Азербайджане/Азербайджан Азове/Азов Акермане/Акерман Акмолінську/Акмолінськ Акрополю/Акрополь Актюбінську/Актюбінськ, Або/= Абруццо/= Абу-Дабі/= Адріатичне море/= Азовське море/= Айдахо/= Ай-Петрі/= Аконкагуа/= Актау/= Алеппо/= Аліканте/= Алмати/= Альбі/= Андаманське море/= Анжу/= Ані/= Антананаріву/= Антигуа/= Апіа/= Апостолове/=, Абіссініє/Абіссінія Абудже/Абуджа Абхазіє/Абхазія Авдіївко/Авдіївка Австраліє/Австралія Австріє/Австрія Австро-Угорщино/Австро-Угорщина Аддис-Абебо/Аддис-Абеба Аджаріє/Аджарія Адигеє/Адигея Адріатико/Адріатика Азіє/Азія Айово/Айова Аквітаніє/Аквітанія Аккро/Аккра Ак-Мечете/Ак-Мечеть Акмоло/Акмола акрилова кислото/акрилова кислота Алабамо/Алабама Албаніє/Албанія, Азорські острови/= Аландські острови/= Алеутські острови/= Андаманські острови/= Антильські острови/= Багамські острови/= Балеарські острови/= Бельбеки/Бельбек Бермудські острови/= Буги/Буг Великодні/Великдень Великі Сорочинці/= Віргінські острови/= Гавайські острови/= Гебридські острови/= Драконові гори/= ЖЕКи/ЖЕК Зеленого Мису острови/= Змієві вали/= Зондські острови/=, Альпи/= Анди/= Апенніни/= Аппалачі/= Арденни/= Афіни/= Багами/= Балкани/= Байдарські ворота/= Барановичі/= Бендери/= Березняки/= Бермуди/= Бескиди/= Біличі/= Близнюки/= Богородчани/= Боровичі/= Бортничі/= Бровари/=, Америки/Америка Андалуські гори/= Атлаські гори/= Бистриці/Бистриця Держдуми/Держдума Жовті Води/= Збройні Сили України/Збройні сили України Індії/Індія Інтернет-газети/Інтернет-газета Караваєві дачі/= Магелланові хмари/= Македонії/Македонія Мате Залка/= Пасхи/Пасха Пилипівки/Пилипівка Ради/Рада Родезії/Родезія Інтернет-технології/Інтернет-технологія, Антропова/Антропов Абакумівно/Абакумівна Абалкіна/Абалкін Абашидзе/= Абдуллоджанова/Абдуллоджанов Абрамівно/Абрамівна Абуладзе/= Авакумівно/Авакумівна Августо/Августа Августимова/Августимов Августинівно/Августинівна Авдієвська/Авдієвський Авенірівно/Авенірівна Аверіна/Аверін Аверкіївно/Аверкіївна Авер&apos;янівно/Авер&apos;янівна Авіято/Авіята Авксентіївно/Авксентіївна Авогадро/= Аврамівно/Аврамівна, Антропове/Антропов Антропов/= Абаю/Абай Абакуме/Абакум Абакумовичу/Абакумович Абалкіне/Абалкін Абалкін/= Абашидзе/= Аббасе/Аббас Абдуло/Абдула Абдуллоджанове/Абдуллоджанов Абдуллоджанов/= Абелю/Абель Абель/= Абовяне/Абовян Абовян/= Абраме/Абрам Абрамовичу/Абрамович Абрамовичу/Абрамович Абрамович/=, Антропови/Антропов Абакуми/Абакум Абакумовичі/Абакумович Абалкіни/Абалкін Абашидзе/= Аббаси/Аббас Абдули/Абдула Абдуллоджанови/Абдуллоджанов Абелі/Абель Абовяни/Абовян Абрами/Абрам Абрамовичі/Абрамович Абрамовичі/Абрамович Абрамчуки/Абрамчук Абуладзе/= Авакуми/Авакум Авакумовичі/Авакумович Августи/Август Августимови/Августимов Августини/Августин (uk)</rdfs:comment>
        <rdfs:comment>e.g., Винстоне/Винстон, Македонецу/Македонец, Македонко/Македонка, Македонче/Македонец, Мартине/Мартин, Океанијо/Океанија, проклетињо/проклетиња (mk)</rdfs:comment>
        <rdfs:comment>Macedonian: Two vocative forms exist with same MSD, e.g. narode / narodu (narod) are both Ncmsvn.&lt;br/&gt;

Slovak: Slovak distinguishes 7 cases, the locative case being obligatorily prepositional. Vocative is identical with nominative, with the exception of several nouns and (substandard usage of) some proper names. Here, vocative is marked according to its syntactic role.
&apos;ty&apos; (E. &apos;you&apos;) is usually vocative. Many other pronouns can be marked as vocative because of their syntactical position, e.g. in &apos;môj bože&apos; (E. &apos;my god&apos;), &apos;môj&apos; is vocative.</rdfs:comment>
    </owl:Class>
    


    <!-- http://purl.org/olia/mte/multext-east.owl#Voice -->

    <owl:Class rdf:about="http://purl.org/olia/mte/multext-east.owl#Voice">
        <rdfs:subClassOf rdf:resource="http://purl.org/olia/mte/multext-east.owl#MorphosyntacticFeature"/>
    </owl:Class>
    


    <!-- http://purl.org/olia/mte/multext-east.owl#WHType -->

    <owl:Class rdf:about="http://purl.org/olia/mte/multext-east.owl#WHType">
        <rdfs:subClassOf rdf:resource="http://purl.org/olia/mte/multext-east.owl#MorphosyntacticFeature"/>
    </owl:Class>
    


    <!-- http://purl.org/olia/mte/multext-east.owl#WeakPronoun -->

    <owl:Class rdf:about="http://purl.org/olia/mte/multext-east.owl#WeakPronoun">
        <rdfs:subClassOf rdf:resource="http://purl.org/olia/mte/multext-east.owl#PronounForm"/>
        <rdfs:comment>e.g., -te/tu, te-/tu, te/tu (ro)</rdfs:comment>
        <rdfs:comment>Pronoun_Form=&quot;weak&quot; (Romanian)&lt;br/&gt;

For Romanian we need an attribute (called Pronoun_Form) to make the distinction between strong and weak forms of the same personal pronoun or reflexive pronoun. All the weak forms can be adjoined to the adjacent words both proclitically or enclitically. In such cases the junction is always graphically marked by a hyphen between the pronoun and the neighboring word. The hyphen also marks possible elisions from either pronoun or the adjacent word. (MTE v4)</rdfs:comment>
    </owl:Class>
    


    <!-- http://purl.org/olia/mte/multext-east.owl#WithCliticS -->

    <owl:Class rdf:about="http://purl.org/olia/mte/multext-east.owl#WithCliticS">
        <rdfs:subClassOf rdf:resource="http://purl.org/olia/mte/multext-east.owl#ElementWithClitic"/>
        <rdfs:subClassOf>
            <owl:Class>
                <owl:intersectionOf rdf:parseType="Collection">
                    <rdf:Description rdf:about="http://purl.org/olia/mte/multext-east.owl#PresentTense"/>
                    <rdf:Description rdf:about="http://purl.org/olia/mte/multext-east.owl#SecondPerson"/>
                    <rdf:Description rdf:about="http://purl.org/olia/mte/multext-east.owl#SingularNumber"/>
                </owl:intersectionOf>
            </owl:Class>
        </rdfs:subClassOf>
        <rdfs:comment>e.g., nahlas/nahnout, ohlas/ohnout, ses/se, sis/se, slíbils/slíbit, tos/ten, tys/ty, zapomněls/zapomenout, zapomněls/zapomnět (cs)</rdfs:comment>
        <rdfs:comment>Clitic_s=&quot;yes&quot; (Czech)

In Czech the 2nd Person singular present Tense of the auxiliary Verb &quot;být&quot; (i.e. the form &quot;jsi&quot;) can be cliticised as -s on certain non-finite verb forms and pronouns. There is no intermediate hyphen between the verbal form and the &apos;s&apos; morpheme. Its presence is indicated by the positive value of the binary feature Clitic_s of the parts of speech Verb and Pronoun. The feature Clitic_s=&apos;yes&apos; thus denotes Czech pronouns having the clitic morpheme &apos;s&apos; appended as a suffix. (Derzhanski and Kotsyba 2009; MTE v4)</rdfs:comment>
    </owl:Class>
    


    <!-- http://purl.org/olia/mte/multext-east.owl#WithCourtesy -->

    <owl:Class rdf:about="http://purl.org/olia/mte/multext-east.owl#WithCourtesy">
        <rdfs:subClassOf rdf:resource="http://purl.org/olia/mte/multext-east.owl#Courtesy"/>
        <rdfs:comment>e.g., bodete/bet, bodite/bet, Ciete/tët, datte/dät, Dáite/dät, hovarnajte/govarnät, nimate/mët, prosite/pruset, Ricite/rićet (sl-rozaj)</rdfs:comment>
        <rdfs:comment>e.g., آمديد/آمد, ايد/است, بتوانيد/توان, بخواهيد/خواه, بوديد/بود, بوديم/بود, بيندازيد/انداز بياييد/آ, بگذاريد/گذار ببخشيد/بخش, بگيريد/گير بخواهيد/خواه بخريد/خر (fa)</rdfs:comment>
        <rdfs:comment>Courtesy=&quot;yes&quot; (Slovene/Resian, Persian)</rdfs:comment>
    </owl:Class>
    


    <!-- http://purl.org/olia/mte/multext-east.owl#WithoutCliticS -->

    <owl:Class rdf:about="http://purl.org/olia/mte/multext-east.owl#WithoutCliticS">
        <rdfs:subClassOf rdf:resource="http://purl.org/olia/mte/multext-east.owl#ElementWithoutClitic"/>
        <rdfs:comment>e.g., bejt/být, byl/být, byla/být, byli/být, bylo/být, byly/být, být, býval/bývat, bývala/bývat (cs)</rdfs:comment>
        <rdfs:comment>feature Clitic_s: the &apos;yes&apos; value of the Clitic_s attribute denotes Czech pronouns having the clitic morpheme &apos;s&apos; appended as a suffix.
Czech: The &apos;yes&apos; value of the Clitic_s attribute denotes a verbal form having the clitic morpheme &apos;s&apos; appended as a suffix. This &apos;s&apos; morpheme expresses 2nd Person singular present Tense of the auxiliary Verb &quot;být&quot; (i.e. the form &quot;jsi&quot;). There is no intermediate hyphen between the verbal form and the &apos;s&apos; morpheme.
The Clitic_s attribute is specified for VForm=infinitive (VForm=n) and Vform=p(articiple) only.
(MTE v.4)&lt;br/&gt;

In Czech the 2nd person singular present tense form of the copula jsi
can be cliticised as -s on certain non-finite verb forms and pronouns, and its presence is indicated by
the positive value of the binary feature Clitic_s of the parts of speech Verb and Pronoun. Essentially
the same phenomenon exists in Polish, but it involves four cliticised forms of the copula (1sg -m, 1pl -
śmy, 2sg -ś, 2pl -ście), and they float more freely (the host can be any content word, e.g. świniaś ‘thou
art a pig’, dobryś ‘thou art good’)
(Derzhanski and Kotsyba 2009)&lt;br/&gt;

Therefore modeled here as subClass of Clitic.&lt;br/&gt;

Clitic_s=&quot;no&quot; (Czech)</rdfs:comment>
    </owl:Class>
    


    <!-- http://purl.org/olia/mte/multext-east.owl#WithoutCourtesy -->

    <owl:Class rdf:about="http://purl.org/olia/mte/multext-east.owl#WithoutCourtesy">
        <rdfs:subClassOf rdf:resource="http://purl.org/olia/mte/multext-east.owl#Courtesy"/>
        <rdfs:comment>e.g., amaite/amät, bota/bet, intendate/intendät, mata/mët, morata/bet, morete/morët, Parnisijta/parnistet, poite/pujtet, pošlišata/pušlüšat (sl-rozaj)</rdfs:comment>
        <rdfs:comment>e.g., باش, باشد/باش, باشم/باش, باشه/باش باشد/باش آيد/آ, باشي/باش, بتواند/توان, بتوانم/توان, بخواب/خواب بايست/ايست باش, بدانم/دان بخوابونم/خوابان ببينم/بين (fa)</rdfs:comment>
        <rdfs:comment>Courtesy=&quot;no&quot; (Resian, Persian)</rdfs:comment>
    </owl:Class>
    


    <!-- http://purl.org/olia/mte/multext-east.owl#WordsCoordinatingConjunction -->

    <owl:Class rdf:about="http://purl.org/olia/mte/multext-east.owl#WordsCoordinatingConjunction">
        <rdfs:subClassOf rdf:resource="http://purl.org/olia/mte/multext-east.owl#CoordinatingConjunction_ConjunctType"/>
        <rdfs:comment>Conjunction/Coord_Type=&quot;words&quot; (Serbian, Russian, Hungarian)</rdfs:comment>
    </owl:Class>
    


    <!-- http://www.w3.org/2002/07/owl#Thing -->

    <owl:Class rdf:about="http://www.w3.org/2002/07/owl#Thing"/>
    


    <!-- 
    ///////////////////////////////////////////////////////////////////////////////////////
    //
    // Individuals
    //
    ///////////////////////////////////////////////////////////////////////////////////////
     -->

    


    <!-- http://purl.org/olia/mte/multext-east.owl#Question -->

    <owl:NamedIndividual rdf:about="http://purl.org/olia/mte/multext-east.owl#Question"/>
    


    <!-- http://purl.org/olia/mte/multext-east.owl#Relative -->

    <owl:NamedIndividual rdf:about="http://purl.org/olia/mte/multext-east.owl#Relative"/>
    


    <!-- 
    ///////////////////////////////////////////////////////////////////////////////////////
    //
    // Annotations
    //
    ///////////////////////////////////////////////////////////////////////////////////////
     -->

    <rdf:Description rdf:about="http://purl.org/olia/mte/multext-east.owl#Question">
        <rdfs:comment>WHType=&quot;question&quot; (English)</rdfs:comment>
    </rdf:Description>
    <rdf:Description rdf:about="http://purl.org/olia/mte/multext-east.owl#Relative">
        <rdfs:comment>WHType=&quot;relative&quot; (English)</rdfs:comment>
    </rdf:Description>
</rdf:RDF>



<!-- Generated by the OWL API (version 4.5.25.2023-02-15T19:15:49Z) https://github.com/owlcs/owlapi -->

