<?xml version="1.0"?>
<rdf:RDF xmlns="http://purl.org/olia/russleeds.owl#"
     xml:base="http://purl.org/olia/russleeds.owl"
     xmlns:ms="http://w3id.org/meta-share/meta-share/"
     xmlns:dct="http://purl.org/dc/terms/"
     xmlns:owl="http://www.w3.org/2002/07/owl#"
     xmlns:rdf="http://www.w3.org/1999/02/22-rdf-syntax-ns#"
     xmlns:xml="http://www.w3.org/XML/1998/namespace"
     xmlns:xsd="http://www.w3.org/2001/XMLSchema#"
     xmlns:rdfs="http://www.w3.org/2000/01/rdf-schema#"
     xmlns:olia_system="http://purl.org/olia/system.owl#">
    <owl:Ontology rdf:about="http://purl.org/olia/russleeds.owl">
        <dct:license rdf:resource="https://creativecommons.org/licenses/by/3.0/"/>
        <ms:language rdf:resource="http://lexvo.org/id/iso639-3/rus"/>
        <rdfs:comment>
      Annotation scheme for part of speech annotation used by Serge Sharoff&apos;s
      TreeTagger module, cf. Sharoff et al. (2008).&lt;br/&gt; 
      Sharoff, S. and Kopotev, M.
      and Erjavec, T. and Feldman, A. and Divjak, D. (2008), Designing and evaluating Russian
      tagsets. In Proceedings of the 6th International Conference on Language Resources and
      Evaluation (LREC 2008), Marrakech, Morocco, May 2008
    </rdfs:comment>
        <owl:versionInfo>
      2007 created on the basis of data samples (no other documentation available)
      2010-04-06 updated
      Christian Chiarcos, chiarcos@uni-potsdam.de
    </owl:versionInfo>
    </owl:Ontology>
    


    <!-- 
    ///////////////////////////////////////////////////////////////////////////////////////
    //
    // Annotation properties
    //
    ///////////////////////////////////////////////////////////////////////////////////////
     -->

    


    <!-- http://purl.org/dc/terms/license -->

    <owl:AnnotationProperty rdf:about="http://purl.org/dc/terms/license"/>
    


    <!-- http://w3id.org/meta-share/meta-share/language -->

    <owl:AnnotationProperty rdf:about="http://w3id.org/meta-share/meta-share/language"/>
    


    <!-- 
    ///////////////////////////////////////////////////////////////////////////////////////
    //
    // Data properties
    //
    ///////////////////////////////////////////////////////////////////////////////////////
     -->

    


    <!-- http://purl.org/olia/system.owl#hasTag -->

    <owl:DatatypeProperty rdf:about="http://purl.org/olia/system.owl#hasTag">
        <rdfs:domain rdf:resource="http://purl.org/olia/russleeds.owl#Tag"/>
    </owl:DatatypeProperty>
    


    <!-- http://purl.org/olia/system.owl#hasTier -->

    <owl:DatatypeProperty rdf:about="http://purl.org/olia/system.owl#hasTier"/>
    


    <!-- 
    ///////////////////////////////////////////////////////////////////////////////////////
    //
    // Classes
    //
    ///////////////////////////////////////////////////////////////////////////////////////
     -->

    


    <!-- http://purl.org/olia/russleeds.owl#AdjectivalPronoun -->

    <owl:Class rdf:about="http://purl.org/olia/russleeds.owl#AdjectivalPronoun">
        <rdfs:subClassOf rdf:resource="http://purl.org/olia/russleeds.owl#Pronoun"/>
        <rdfs:comment>These are adjectival
      pronouns, e.g. который (&quot;which&quot;), твой (&quot;your&quot;).</rdfs:comment>
    </owl:Class>
    


    <!-- http://purl.org/olia/russleeds.owl#Adjective -->

    <owl:Class rdf:about="http://purl.org/olia/russleeds.owl#Adjective">
        <rdfs:subClassOf rdf:resource="http://purl.org/olia/russleeds.owl#Tag"/>
        <rdfs:comment>These are adjectives, e.g.
      коричневый (&quot;brown&quot;), таинственный (&quot;mysterious&quot;).</rdfs:comment>
    </owl:Class>
    


    <!-- http://purl.org/olia/russleeds.owl#Adverb -->

    <owl:Class rdf:about="http://purl.org/olia/russleeds.owl#Adverb">
        <rdfs:subClassOf rdf:resource="http://purl.org/olia/russleeds.owl#Tag"/>
        <rdfs:comment>These are adverbs, e.g.
      сгоряча (&quot;in a temper&quot;), очень (&quot;very much&quot;).</rdfs:comment>
    </owl:Class>
    


    <!-- http://purl.org/olia/russleeds.owl#AdverbialPronoun -->

    <owl:Class rdf:about="http://purl.org/olia/russleeds.owl#AdverbialPronoun">
        <rdfs:subClassOf rdf:resource="http://purl.org/olia/russleeds.owl#Pronoun"/>
        <rdfs:comment>These are adverbal
      pronouns, e.g. где (&quot;where; where is&quot;), вот (&quot;there; there is&quot;).</rdfs:comment>
    </owl:Class>
    


    <!-- http://purl.org/olia/russleeds.owl#Conjunction -->

    <owl:Class rdf:about="http://purl.org/olia/russleeds.owl#Conjunction">
        <rdfs:subClassOf rdf:resource="http://purl.org/olia/russleeds.owl#Tag"/>
        <rdfs:comment>These are conjunctions,
      e.g. и (&quot;and&quot;), чтобы (&quot;that&quot;).</rdfs:comment>
    </owl:Class>
    


    <!-- http://purl.org/olia/russleeds.owl#Initials -->

    <owl:Class rdf:about="http://purl.org/olia/russleeds.owl#Initials">
        <rdfs:subClassOf rdf:resource="http://purl.org/olia/russleeds.owl#Tag"/>
        <rdfs:comment>These are initials, e.g.
      (M., P.).</rdfs:comment>
    </owl:Class>
    


    <!-- http://purl.org/olia/russleeds.owl#Interjection -->

    <owl:Class rdf:about="http://purl.org/olia/russleeds.owl#Interjection">
        <rdfs:subClassOf rdf:resource="http://purl.org/olia/russleeds.owl#Tag"/>
        <rdfs:comment>These are interjections,
      e.g. увы (&quot;alas&quot;), Ай (&quot;Aye&quot;), Ой (&quot;Oh&quot;), Ах (&quot;Oh&quot;), Ох (&quot;Oh&quot;), Ух (&quot;Uh&quot;).</rdfs:comment>
    </owl:Class>
    


    <!-- http://purl.org/olia/russleeds.owl#Noun -->

    <owl:Class rdf:about="http://purl.org/olia/russleeds.owl#Noun">
        <rdfs:subClassOf rdf:resource="http://purl.org/olia/russleeds.owl#Tag"/>
        <rdfs:comment>Theses are nouns, e.g.
      яблоня (&quot;an apple tree&quot;), лошадь (&quot;a horse&quot;), корпус (&quot;the case&quot;), вечность
      (&quot;eternity&quot;).</rdfs:comment>
    </owl:Class>
    


    <!-- http://purl.org/olia/russleeds.owl#Numerative -->

    <owl:Class rdf:about="http://purl.org/olia/russleeds.owl#Numerative">
        <rdfs:subClassOf rdf:resource="http://purl.org/olia/russleeds.owl#Tag"/>
        <rdfs:comment>These are numerals, e.g.
      четыре (&quot;four&quot;), десять (&quot;ten&quot;), много (&quot;it is a lot of&quot;).</rdfs:comment>
    </owl:Class>
    


    <!-- http://purl.org/olia/russleeds.owl#OrdinalNumber -->

    <owl:Class rdf:about="http://purl.org/olia/russleeds.owl#OrdinalNumber">
        <rdfs:subClassOf rdf:resource="http://purl.org/olia/russleeds.owl#Tag"/>
        <rdfs:comment>These are ordinal numbers,
      e.g. один (&quot;one&quot;), седьмой (&quot;the seventh&quot;), восьмидесятый (&quot;the eightieth&quot;).</rdfs:comment>
    </owl:Class>
    


    <!-- http://purl.org/olia/russleeds.owl#Parenthetical -->

    <owl:Class rdf:about="http://purl.org/olia/russleeds.owl#Parenthetical">
        <rdfs:subClassOf rdf:resource="http://purl.org/olia/russleeds.owl#Tag"/>
        <rdfs:comment>This is an idiomatic phrase
      marking the beginning of a new turn in a dialog, or a new topic in a discourse, e.g. кстати
      (&quot;by the way&quot;), по-моему (&quot;in my opinion&quot;).</rdfs:comment>
    </owl:Class>
    


    <!-- http://purl.org/olia/russleeds.owl#Particle -->

    <owl:Class rdf:about="http://purl.org/olia/russleeds.owl#Particle">
        <rdfs:subClassOf rdf:resource="http://purl.org/olia/russleeds.owl#Tag"/>
        <rdfs:comment>These are particles, e.g.
      бы, же, пусть.</rdfs:comment>
    </owl:Class>
    


    <!-- http://purl.org/olia/russleeds.owl#PersonalPronoun -->

    <owl:Class rdf:about="http://purl.org/olia/russleeds.owl#PersonalPronoun">
        <rdfs:subClassOf rdf:resource="http://purl.org/olia/russleeds.owl#Pronoun"/>
        <rdfs:comment>These are personal
      pronouns, e.g. она (&quot;she&quot;), что (&quot;what&quot;).</rdfs:comment>
    </owl:Class>
    


    <!-- http://purl.org/olia/russleeds.owl#Predicative -->

    <owl:Class rdf:about="http://purl.org/olia/russleeds.owl#Predicative">
        <rdfs:subClassOf rdf:resource="http://purl.org/olia/russleeds.owl#Tag"/>
        <rdfs:comment></rdfs:comment>
        <rdfs:comment>These are expressions used
      as a predicative, thus are non-inflected, e.g. жаль (&quot;it is a pity&quot;), хорошо (&quot;well&quot;), пора
      (&quot;it is time&quot;).</rdfs:comment>
    </owl:Class>
    


    <!-- http://purl.org/olia/russleeds.owl#PredicativePronoun -->

    <owl:Class rdf:about="http://purl.org/olia/russleeds.owl#PredicativePronoun">
        <rdfs:subClassOf rdf:resource="http://purl.org/olia/russleeds.owl#Pronoun"/>
        <rdfs:comment>These are predicatives
      pronouns, e.g. некого (&quot;noone&quot;), нечего (&quot;nothing&quot;).</rdfs:comment>
    </owl:Class>
    


    <!-- http://purl.org/olia/russleeds.owl#Preposition -->

    <owl:Class rdf:about="http://purl.org/olia/russleeds.owl#Preposition">
        <rdfs:subClassOf rdf:resource="http://purl.org/olia/russleeds.owl#Tag"/>
        <rdfs:comment>These are prepositions,
      e.g. под (&quot;under&quot;), напротив(&quot;opposite&quot;).</rdfs:comment>
    </owl:Class>
    


    <!-- http://purl.org/olia/russleeds.owl#Pronoun -->

    <owl:Class rdf:about="http://purl.org/olia/russleeds.owl#Pronoun">
        <rdfs:subClassOf rdf:resource="http://purl.org/olia/russleeds.owl#Tag"/>
    </owl:Class>
    


    <!-- http://purl.org/olia/russleeds.owl#Punctuation -->

    <owl:Class rdf:about="http://purl.org/olia/russleeds.owl#Punctuation">
        <rdfs:subClassOf rdf:resource="http://purl.org/olia/russleeds.owl#Tag"/>
        <rdfs:comment>These are punctuation
      marks.</rdfs:comment>
    </owl:Class>
    


    <!-- http://purl.org/olia/russleeds.owl#SentenceEnd -->

    <owl:Class rdf:about="http://purl.org/olia/russleeds.owl#SentenceEnd">
        <rdfs:subClassOf rdf:resource="http://purl.org/olia/russleeds.owl#Tag"/>
        <rdfs:comment>These are punctuation marks
      marking sentence ending.</rdfs:comment>
    </owl:Class>
    


    <!-- http://purl.org/olia/russleeds.owl#Tag -->

    <owl:Class rdf:about="http://purl.org/olia/russleeds.owl#Tag">
        <rdfs:subClassOf rdf:resource="http://purl.org/olia/system.owl#LinguisticAnnotation"/>
        <rdfs:subClassOf>
            <owl:Restriction>
                <owl:onProperty rdf:resource="http://purl.org/olia/system.owl#hasTier"/>
                <owl:hasValue>POS</owl:hasValue>
            </owl:Restriction>
        </rdfs:subClassOf>
    </owl:Class>
    


    <!-- http://purl.org/olia/russleeds.owl#Verb -->

    <owl:Class rdf:about="http://purl.org/olia/russleeds.owl#Verb">
        <rdfs:subClassOf rdf:resource="http://purl.org/olia/russleeds.owl#Tag"/>
        <rdfs:comment>These are verbs, e.g.
      пользоваться (&quot;to use&quot;), обрабатывать (&quot;to process&quot;).</rdfs:comment>
    </owl:Class>
    


    <!-- http://purl.org/olia/system.owl#LinguisticAnnotation -->

    <owl:Class rdf:about="http://purl.org/olia/system.owl#LinguisticAnnotation"/>
    


    <!-- 
    ///////////////////////////////////////////////////////////////////////////////////////
    //
    // Individuals
    //
    ///////////////////////////////////////////////////////////////////////////////////////
     -->

    


    <!-- http://purl.org/olia/russleeds.owl#A -->

    <owl:NamedIndividual rdf:about="http://purl.org/olia/russleeds.owl#A">
        <rdf:type rdf:resource="http://purl.org/olia/russleeds.owl#Adjective"/>
        <olia_system:hasTag>A</olia_system:hasTag>
    </owl:NamedIndividual>
    


    <!-- http://purl.org/olia/russleeds.owl#A-NUM -->

    <owl:NamedIndividual rdf:about="http://purl.org/olia/russleeds.owl#A-NUM">
        <rdf:type rdf:resource="http://purl.org/olia/russleeds.owl#OrdinalNumber"/>
        <olia_system:hasTag>A-NUM</olia_system:hasTag>
    </owl:NamedIndividual>
    


    <!-- http://purl.org/olia/russleeds.owl#A-PRO -->

    <owl:NamedIndividual rdf:about="http://purl.org/olia/russleeds.owl#A-PRO">
        <rdf:type rdf:resource="http://purl.org/olia/russleeds.owl#AdjectivalPronoun"/>
        <olia_system:hasTag>A-PRO</olia_system:hasTag>
    </owl:NamedIndividual>
    


    <!-- http://purl.org/olia/russleeds.owl#ADV -->

    <owl:NamedIndividual rdf:about="http://purl.org/olia/russleeds.owl#ADV">
        <rdf:type rdf:resource="http://purl.org/olia/russleeds.owl#Adverb"/>
        <olia_system:hasTag>ADV</olia_system:hasTag>
    </owl:NamedIndividual>
    


    <!-- http://purl.org/olia/russleeds.owl#ADV-PRO -->

    <owl:NamedIndividual rdf:about="http://purl.org/olia/russleeds.owl#ADV-PRO">
        <rdf:type rdf:resource="http://purl.org/olia/russleeds.owl#AdverbialPronoun"/>
        <olia_system:hasTag>ADV-PRO</olia_system:hasTag>
    </owl:NamedIndividual>
    


    <!-- http://purl.org/olia/russleeds.owl#CONJ -->

    <owl:NamedIndividual rdf:about="http://purl.org/olia/russleeds.owl#CONJ">
        <rdf:type rdf:resource="http://purl.org/olia/russleeds.owl#Conjunction"/>
        <olia_system:hasTag>CONJ</olia_system:hasTag>
    </owl:NamedIndividual>
    


    <!-- http://purl.org/olia/russleeds.owl#INIT -->

    <owl:NamedIndividual rdf:about="http://purl.org/olia/russleeds.owl#INIT">
        <rdf:type rdf:resource="http://purl.org/olia/russleeds.owl#Initials"/>
        <olia_system:hasTag>INIT</olia_system:hasTag>
    </owl:NamedIndividual>
    


    <!-- http://purl.org/olia/russleeds.owl#INTJ -->

    <owl:NamedIndividual rdf:about="http://purl.org/olia/russleeds.owl#INTJ">
        <rdf:type rdf:resource="http://purl.org/olia/russleeds.owl#Interjection"/>
        <olia_system:hasTag>INTJ</olia_system:hasTag>
    </owl:NamedIndividual>
    


    <!-- http://purl.org/olia/russleeds.owl#NUM -->

    <owl:NamedIndividual rdf:about="http://purl.org/olia/russleeds.owl#NUM">
        <rdf:type rdf:resource="http://purl.org/olia/russleeds.owl#Numerative"/>
        <olia_system:hasTag>NUM</olia_system:hasTag>
    </owl:NamedIndividual>
    


    <!-- http://purl.org/olia/russleeds.owl#PARENTH -->

    <owl:NamedIndividual rdf:about="http://purl.org/olia/russleeds.owl#PARENTH">
        <rdf:type rdf:resource="http://purl.org/olia/russleeds.owl#Parenthetical"/>
        <olia_system:hasTag>PARENTH</olia_system:hasTag>
    </owl:NamedIndividual>
    


    <!-- http://purl.org/olia/russleeds.owl#PART -->

    <owl:NamedIndividual rdf:about="http://purl.org/olia/russleeds.owl#PART">
        <rdf:type rdf:resource="http://purl.org/olia/russleeds.owl#Particle"/>
        <olia_system:hasTag>PART</olia_system:hasTag>
    </owl:NamedIndividual>
    


    <!-- http://purl.org/olia/russleeds.owl#PR -->

    <owl:NamedIndividual rdf:about="http://purl.org/olia/russleeds.owl#PR">
        <rdf:type rdf:resource="http://purl.org/olia/russleeds.owl#Preposition"/>
        <olia_system:hasTag>PRAEDIC-PRO</olia_system:hasTag>
    </owl:NamedIndividual>
    


    <!-- http://purl.org/olia/russleeds.owl#PRAEDIC -->

    <owl:NamedIndividual rdf:about="http://purl.org/olia/russleeds.owl#PRAEDIC">
        <rdf:type rdf:resource="http://purl.org/olia/russleeds.owl#Predicative"/>
        <olia_system:hasTag>PRAEDIC</olia_system:hasTag>
    </owl:NamedIndividual>
    


    <!-- http://purl.org/olia/russleeds.owl#PRAEDIC-PRO -->

    <owl:NamedIndividual rdf:about="http://purl.org/olia/russleeds.owl#PRAEDIC-PRO">
        <rdf:type rdf:resource="http://purl.org/olia/russleeds.owl#PredicativePronoun"/>
        <olia_system:hasTag>PRAEDIC-PRO</olia_system:hasTag>
    </owl:NamedIndividual>
    


    <!-- http://purl.org/olia/russleeds.owl#PUNCT -->

    <owl:NamedIndividual rdf:about="http://purl.org/olia/russleeds.owl#PUNCT">
        <rdf:type rdf:resource="http://purl.org/olia/russleeds.owl#Punctuation"/>
        <olia_system:hasTag>PUNCT</olia_system:hasTag>
    </owl:NamedIndividual>
    


    <!-- http://purl.org/olia/russleeds.owl#S -->

    <owl:NamedIndividual rdf:about="http://purl.org/olia/russleeds.owl#S">
        <rdf:type rdf:resource="http://purl.org/olia/russleeds.owl#Noun"/>
        <olia_system:hasTag>S</olia_system:hasTag>
    </owl:NamedIndividual>
    


    <!-- http://purl.org/olia/russleeds.owl#S-PRO -->

    <owl:NamedIndividual rdf:about="http://purl.org/olia/russleeds.owl#S-PRO">
        <rdf:type rdf:resource="http://purl.org/olia/russleeds.owl#PersonalPronoun"/>
        <olia_system:hasTag>S-PRO</olia_system:hasTag>
    </owl:NamedIndividual>
    


    <!-- http://purl.org/olia/russleeds.owl#SENT -->

    <owl:NamedIndividual rdf:about="http://purl.org/olia/russleeds.owl#SENT">
        <rdf:type rdf:resource="http://purl.org/olia/russleeds.owl#SentenceEnd"/>
        <olia_system:hasTag>SENT</olia_system:hasTag>
    </owl:NamedIndividual>
    


    <!-- http://purl.org/olia/russleeds.owl#V -->

    <owl:NamedIndividual rdf:about="http://purl.org/olia/russleeds.owl#V">
        <rdf:type rdf:resource="http://purl.org/olia/russleeds.owl#Verb"/>
        <olia_system:hasTag>V</olia_system:hasTag>
    </owl:NamedIndividual>
</rdf:RDF>



<!-- Generated by the OWL API (version 4.5.25.2023-02-15T19:15:49Z) https://github.com/owlcs/owlapi -->

