<?xml version="1.0"?>
<rdf:RDF xmlns="http://purl.org/olia/susa.owl#"
     xml:base="http://purl.org/olia/susa.owl"
     xmlns:ms="http://w3id.org/meta-share/meta-share/"
     xmlns:dct="http://purl.org/dc/terms/"
     xmlns:owl="http://www.w3.org/2002/07/owl#"
     xmlns:rdf="http://www.w3.org/1999/02/22-rdf-syntax-ns#"
     xmlns:xml="http://www.w3.org/XML/1998/namespace"
     xmlns:xsd="http://www.w3.org/2001/XMLSchema#"
     xmlns:rdfs="http://www.w3.org/2000/01/rdf-schema#"
     xmlns:olia_system="http://purl.org/olia/system.owl#">
    <owl:Ontology rdf:about="http://purl.org/olia/susa.owl">
        <dct:license rdf:resource="https://creativecommons.org/licenses/by/3.0/"/>
        <ms:language rdf:resource="http://lexvo.org/id/iso639-3/eng"/>
        <rdfs:comment>
		Annotation Model of the morphosyntactic component of the SUSANNE scheme as 
		applied to the British English SUSANNE corpus (Sampson, 1995), also 
		covering the simplified SUSANNE tag set as used by the TnT Tagger
		(Brants 2000).
		&lt;br/&gt;
		Brants, T. (2000), 
		TnT--a statistical part-of-speech tagger,
		In Proc. ANLP 2000 &lt;br/&gt;
		Sampson, G. (1995), English for the computer: 
		The SUSANNE corpus and analytic scheme, 
		Oxford University Press
	</rdfs:comment>
        <owl:versionInfo>
		2006 created by Christian Chiarcos
		2006-2008 maintained by Christian Chiarcos, Johannes Bubenzer and Angelika Adam
		2010-04-07 updated, 0ld-comments removed, partially proof-read, Christian Chiarcos
    2024-11-29 tier label &quot;pos&quot; changed to &quot;POS&quot;
	</owl:versionInfo>
        <owl:versionInfo>TODO: syntax</owl:versionInfo>
    </owl:Ontology>
    


    <!-- 
    ///////////////////////////////////////////////////////////////////////////////////////
    //
    // Annotation properties
    //
    ///////////////////////////////////////////////////////////////////////////////////////
     -->

    


    <!-- http://purl.org/dc/terms/license -->

    <owl:AnnotationProperty rdf:about="http://purl.org/dc/terms/license"/>
    


    <!-- http://w3id.org/meta-share/meta-share/language -->

    <owl:AnnotationProperty rdf:about="http://w3id.org/meta-share/meta-share/language"/>
    


    <!-- 
    ///////////////////////////////////////////////////////////////////////////////////////
    //
    // Object Properties
    //
    ///////////////////////////////////////////////////////////////////////////////////////
     -->

    


    <!-- http://purl.org/olia/susa.owl#hasCase -->

    <owl:ObjectProperty rdf:about="http://purl.org/olia/susa.owl#hasCase">
        <rdfs:subPropertyOf rdf:resource="http://purl.org/olia/system.owl#hasFeature"/>
        <rdfs:domain>
            <owl:Class>
                <owl:unionOf rdf:parseType="Collection">
                    <rdf:Description rdf:about="http://purl.org/olia/susa.owl#AttributivePronoun"/>
                    <rdf:Description rdf:about="http://purl.org/olia/susa.owl#SubstitutiveFirstPersonPronoun"/>
                    <rdf:Description rdf:about="http://purl.org/olia/susa.owl#SubstitutiveThirdPersonPronoun"/>
                    <rdf:Description rdf:about="http://purl.org/olia/susa.owl#SubstitutiveWHPronoun"/>
                    <rdf:Description rdf:about="http://purl.org/olia/susa.owl#WHDeterminer"/>
                </owl:unionOf>
            </owl:Class>
        </rdfs:domain>
        <rdfs:range rdf:resource="http://purl.org/olia/susa.owl#Case"/>
    </owl:ObjectProperty>
    


    <!-- http://purl.org/olia/susa.owl#hasCountability -->

    <owl:ObjectProperty rdf:about="http://purl.org/olia/susa.owl#hasCountability">
        <rdfs:subPropertyOf rdf:resource="http://purl.org/olia/system.owl#hasFeature"/>
        <rdfs:domain rdf:resource="http://purl.org/olia/susa.owl#CommonNoun"/>
        <rdfs:range rdf:resource="http://purl.org/olia/susa.owl#Countability"/>
    </owl:ObjectProperty>
    


    <!-- http://purl.org/olia/susa.owl#hasDegree -->

    <owl:ObjectProperty rdf:about="http://purl.org/olia/susa.owl#hasDegree">
        <rdfs:subPropertyOf rdf:resource="http://purl.org/olia/system.owl#hasFeature"/>
        <rdfs:domain>
            <owl:Class>
                <owl:unionOf rdf:parseType="Collection">
                    <rdf:Description rdf:about="http://purl.org/olia/susa.owl#Adjective"/>
                    <rdf:Description rdf:about="http://purl.org/olia/susa.owl#Adverb"/>
                </owl:unionOf>
            </owl:Class>
        </rdfs:domain>
    </owl:ObjectProperty>
    


    <!-- http://purl.org/olia/susa.owl#hasForm -->

    <owl:ObjectProperty rdf:about="http://purl.org/olia/susa.owl#hasForm">
        <rdfs:subPropertyOf rdf:resource="http://purl.org/olia/system.owl#hasFeature"/>
        <rdfs:domain rdf:resource="http://purl.org/olia/susa.owl#Verb"/>
        <rdfs:range rdf:resource="http://purl.org/olia/susa.owl#Form"/>
    </owl:ObjectProperty>
    


    <!-- http://purl.org/olia/susa.owl#hasGender -->

    <owl:ObjectProperty rdf:about="http://purl.org/olia/susa.owl#hasGender">
        <rdfs:subPropertyOf rdf:resource="http://purl.org/olia/system.owl#hasFeature"/>
        <rdfs:domain>
            <owl:Class>
                <owl:unionOf rdf:parseType="Collection">
                    <rdf:Description rdf:about="http://purl.org/olia/susa.owl#AttributivePronoun"/>
                    <rdf:Description rdf:about="http://purl.org/olia/susa.owl#Noun"/>
                    <rdf:Description rdf:about="http://purl.org/olia/susa.owl#SubstitutivePersonalPronoun"/>
                </owl:unionOf>
            </owl:Class>
        </rdfs:domain>
        <rdfs:range rdf:resource="http://purl.org/olia/susa.owl#Gender"/>
    </owl:ObjectProperty>
    


    <!-- http://purl.org/olia/susa.owl#hasNumber -->

    <owl:ObjectProperty rdf:about="http://purl.org/olia/susa.owl#hasNumber">
        <rdfs:subPropertyOf rdf:resource="http://purl.org/olia/system.owl#hasFeature"/>
        <rdfs:domain>
            <owl:Class>
                <owl:unionOf rdf:parseType="Collection">
                    <rdf:Description rdf:about="http://purl.org/olia/susa.owl#AttributivePronoun"/>
                    <rdf:Description rdf:about="http://purl.org/olia/susa.owl#Letter"/>
                    <rdf:Description rdf:about="http://purl.org/olia/susa.owl#LexicalVerbThirdPerson"/>
                    <rdf:Description rdf:about="http://purl.org/olia/susa.owl#Noun"/>
                    <rdf:Description rdf:about="http://purl.org/olia/susa.owl#Numeral"/>
                    <rdf:Description rdf:about="http://purl.org/olia/susa.owl#SubstitutivePersonalPronoun"/>
                </owl:unionOf>
            </owl:Class>
        </rdfs:domain>
        <rdfs:range rdf:resource="http://purl.org/olia/susa.owl#Number"/>
    </owl:ObjectProperty>
    


    <!-- http://purl.org/olia/susa.owl#hasPerson -->

    <owl:ObjectProperty rdf:about="http://purl.org/olia/susa.owl#hasPerson">
        <rdfs:subPropertyOf rdf:resource="http://purl.org/olia/system.owl#hasFeature"/>
        <rdfs:domain>
            <owl:Class>
                <owl:unionOf rdf:parseType="Collection">
                    <rdf:Description rdf:about="http://purl.org/olia/susa.owl#AttributivePronoun"/>
                    <rdf:Description rdf:about="http://purl.org/olia/susa.owl#LexicalVerbThirdPerson"/>
                    <rdf:Description rdf:about="http://purl.org/olia/susa.owl#SubstitutivePersonalPronoun"/>
                </owl:unionOf>
            </owl:Class>
        </rdfs:domain>
        <rdfs:range rdf:resource="http://purl.org/olia/susa.owl#Person"/>
    </owl:ObjectProperty>
    


    <!-- http://purl.org/olia/susa.owl#hasTense -->

    <owl:ObjectProperty rdf:about="http://purl.org/olia/susa.owl#hasTense">
        <rdfs:subPropertyOf rdf:resource="http://purl.org/olia/system.owl#hasFeature"/>
        <rdfs:domain rdf:resource="http://purl.org/olia/susa.owl#Verb"/>
        <rdfs:range rdf:resource="http://purl.org/olia/susa.owl#Tense"/>
    </owl:ObjectProperty>
    


    <!-- http://purl.org/olia/susa.owl#hasValency -->

    <owl:ObjectProperty rdf:about="http://purl.org/olia/susa.owl#hasValency">
        <rdfs:subPropertyOf rdf:resource="http://purl.org/olia/system.owl#hasFeature"/>
        <rdfs:domain rdf:resource="http://purl.org/olia/susa.owl#Verb"/>
        <rdfs:range rdf:resource="http://purl.org/olia/susa.owl#Valency"/>
    </owl:ObjectProperty>
    


    <!-- http://purl.org/olia/system.owl#hasFeature -->

    <owl:ObjectProperty rdf:about="http://purl.org/olia/system.owl#hasFeature"/>
    


    <!-- 
    ///////////////////////////////////////////////////////////////////////////////////////
    //
    // Data properties
    //
    ///////////////////////////////////////////////////////////////////////////////////////
     -->

    


    <!-- http://purl.org/olia/system.owl#hasTag -->

    <owl:DatatypeProperty rdf:about="http://purl.org/olia/system.owl#hasTag">
        <rdfs:domain rdf:resource="http://purl.org/olia/susa.owl#Tag"/>
        <rdfs:range rdf:resource="http://www.w3.org/2001/XMLSchema#string"/>
    </owl:DatatypeProperty>
    


    <!-- http://purl.org/olia/system.owl#hasTier -->

    <owl:DatatypeProperty rdf:about="http://purl.org/olia/system.owl#hasTier">
        <rdfs:domain rdf:resource="http://purl.org/olia/susa.owl#Tag"/>
        <rdfs:range rdf:resource="http://www.w3.org/2001/XMLSchema#string"/>
    </owl:DatatypeProperty>
    


    <!-- 
    ///////////////////////////////////////////////////////////////////////////////////////
    //
    // Classes
    //
    ///////////////////////////////////////////////////////////////////////////////////////
     -->

    


    <!-- http://purl.org/olia/susa.owl#Adjective -->

    <owl:Class rdf:about="http://purl.org/olia/susa.owl#Adjective">
        <rdfs:subClassOf rdf:resource="http://purl.org/olia/susa.owl#Tag"/>
        <rdfs:comment>SUSANNE tags begining with J... represent predicative adjectives, attributive adjectives and general adjectives.</rdfs:comment>
    </owl:Class>
    


    <!-- http://purl.org/olia/susa.owl#Adverb -->

    <owl:Class rdf:about="http://purl.org/olia/susa.owl#Adverb">
        <rdfs:subClassOf rdf:resource="http://purl.org/olia/susa.owl#Tag"/>
        <rdfs:comment>SUSANNE tags beginning with R... represent adverbs.</rdfs:comment>
    </owl:Class>
    


    <!-- http://purl.org/olia/susa.owl#Am -->

    <owl:Class rdf:about="http://purl.org/olia/susa.owl#Am">
        <rdfs:subClassOf rdf:resource="http://purl.org/olia/susa.owl#Be"/>
        <rdfs:subClassOf rdf:resource="http://purl.org/olia/susa.owl#Present"/>
        <rdfs:comment>The tag VBM is used for &quot;am&quot;.
(Sampson 1995, p. 118)</rdfs:comment>
    </owl:Class>
    


    <!-- http://purl.org/olia/susa.owl#AppositionIntroducingAdverb -->

    <owl:Class rdf:about="http://purl.org/olia/susa.owl#AppositionIntroducingAdverb">
        <rdfs:subClassOf rdf:resource="http://purl.org/olia/susa.owl#Adverb"/>
        <rdfs:comment>These are apposition-introducing elements e.g. &quot;for example&quot;, &quot;for instance&quot;, &quot;namely&quot;.
(Sampson 1995, p.116)</rdfs:comment>
    </owl:Class>
    


    <!-- http://purl.org/olia/susa.owl#Are -->

    <owl:Class rdf:about="http://purl.org/olia/susa.owl#Are">
        <rdfs:subClassOf rdf:resource="http://purl.org/olia/susa.owl#Be"/>
        <rdfs:comment>The SUSANNE tag VBR is used for &quot;are&quot;.
(Sampson 1995, p. 118)</rdfs:comment>
        <owl:versionInfo>
		added by Johannes Bubenzer (09.09.2006) for a TnT tag used in a data sample from 
		Collaborative Research Center (SFB) 538 &quot;Multilingualism&quot; (Hamburg), project K4
	</owl:versionInfo>
    </owl:Class>
    


    <!-- http://purl.org/olia/susa.owl#Article -->

    <owl:Class rdf:about="http://purl.org/olia/susa.owl#Article">
        <rdfs:subClassOf rdf:resource="http://purl.org/olia/susa.owl#Tag"/>
        <rdfs:comment>SUSANNE tag AT pertains to articles and other determiners, i.e., &quot;every&quot;, the indefinite article, the negative determiner and the definite article.

(Sampson 1995, p.105)</rdfs:comment>
    </owl:Class>
    


    <!-- http://purl.org/olia/susa.owl#AttributiveAdjective -->

    <owl:Class rdf:about="http://purl.org/olia/susa.owl#AttributiveAdjective">
        <rdfs:subClassOf rdf:resource="http://purl.org/olia/susa.owl#Adjective"/>
        <rdfs:comment>SUSANNE tags beginning with JB... represent attributively used adjectives, e.g., &quot;inner&quot;, &quot;interior&quot;, &quot;joint&quot;.
(Sampson 1995, p. 109)</rdfs:comment>
    </owl:Class>
    


    <!-- http://purl.org/olia/susa.owl#AttributivePossessivePronoun -->

    <owl:Class rdf:about="http://purl.org/olia/susa.owl#AttributivePossessivePronoun">
        <rdfs:subClassOf rdf:resource="http://purl.org/olia/susa.owl#AttributivePronoun"/>
        <rdfs:comment>SUSANNE tags beginning with APPG... are used for attributive possessive pronouns (&quot;her&quot;, &quot;his&quot;, &quot;its&quot;, &quot;my&quot;, &quot;our&quot;, &quot;your&quot;, &quot;their&quot;)
(Sampson 1995, p.105)</rdfs:comment>
    </owl:Class>
    


    <!-- http://purl.org/olia/susa.owl#AttributivePronoun -->

    <owl:Class rdf:about="http://purl.org/olia/susa.owl#AttributivePronoun">
        <rdfs:subClassOf rdf:resource="http://purl.org/olia/susa.owl#Tag"/>
        <rdfs:comment>SUSANNE tags beginning with APP represent attributive pronouns.</rdfs:comment>
    </owl:Class>
    


    <!-- http://purl.org/olia/susa.owl#BaseForm -->

    <owl:Class rdf:about="http://purl.org/olia/susa.owl#BaseForm">
        <rdfs:subClassOf rdf:resource="http://purl.org/olia/susa.owl#Verb"/>
        <rdfs:comment>SUSANNE tags beginning with V and containing 0 represent base forms of verbs, i.e., infinitive and identical word forms (indicative, imperative).</rdfs:comment>
        <owl:versionInfo>TODO: check linking</owl:versionInfo>
    </owl:Class>
    


    <!-- http://purl.org/olia/susa.owl#Be -->

    <owl:Class rdf:about="http://purl.org/olia/susa.owl#Be">
        <rdfs:subClassOf rdf:resource="http://purl.org/olia/susa.owl#Verb"/>
        <rdfs:comment>The class Be contains the SUSANNE tags for the forms of &quot;be&quot;.
(Sampson 1995, p. 118)</rdfs:comment>
    </owl:Class>
    


    <!-- http://purl.org/olia/susa.owl#BeBaseForm -->

    <owl:Class rdf:about="http://purl.org/olia/susa.owl#BeBaseForm">
        <rdfs:subClassOf rdf:resource="http://purl.org/olia/susa.owl#BaseForm"/>
        <rdfs:subClassOf rdf:resource="http://purl.org/olia/susa.owl#Be"/>
        <rdfs:comment>The SUSANNE tag VB0 is used for &quot;be&quot;. 
(Sampson 1995, p. 119)</rdfs:comment>
    </owl:Class>
    


    <!-- http://purl.org/olia/susa.owl#BePast -->

    <owl:Class rdf:about="http://purl.org/olia/susa.owl#BePast">
        <rdfs:subClassOf rdf:resource="http://purl.org/olia/susa.owl#Be"/>
        <rdfs:subClassOf rdf:resource="http://purl.org/olia/susa.owl#Past"/>
        <rdfs:comment>Past forms of &quot;be&quot;.</rdfs:comment>
    </owl:Class>
    


    <!-- http://purl.org/olia/susa.owl#BePastParticiple -->

    <owl:Class rdf:about="http://purl.org/olia/susa.owl#BePastParticiple">
        <rdfs:subClassOf rdf:resource="http://purl.org/olia/susa.owl#Be"/>
        <rdfs:comment>This used for the past participle of &quot;be&quot;.</rdfs:comment>
    </owl:Class>
    


    <!-- http://purl.org/olia/susa.owl#BePresentParticiple -->

    <owl:Class rdf:about="http://purl.org/olia/susa.owl#BePresentParticiple">
        <rdfs:subClassOf rdf:resource="http://purl.org/olia/susa.owl#Be"/>
        <rdfs:subClassOf rdf:resource="http://purl.org/olia/susa.owl#PresentParticiple"/>
        <rdfs:comment>The SUSANNE tag VBG is used for the present participle of &quot;be&quot;, i.e., &quot;being&quot;. 
(Sampson 1995, p. 118)</rdfs:comment>
    </owl:Class>
    


    <!-- http://purl.org/olia/susa.owl#CardinalNumber -->

    <owl:Class rdf:about="http://purl.org/olia/susa.owl#CardinalNumber">
        <rdfs:subClassOf rdf:resource="http://purl.org/olia/susa.owl#Numeral"/>
        <rdfs:comment>MC is the SUSANNE tag used for cardinal numbers from  &quot;zero&quot; upwards, spelled out. This includes &quot;umpteen&quot;.
(Sampson 1995, p. 111)</rdfs:comment>
    </owl:Class>
    


    <!-- http://purl.org/olia/susa.owl#Case -->

    <owl:Class rdf:about="http://purl.org/olia/susa.owl#Case">
        <rdfs:subClassOf rdf:resource="http://purl.org/olia/system.owl#Feature"/>
    </owl:Class>
    


    <!-- http://purl.org/olia/susa.owl#CatenativeModalVerb -->

    <owl:Class rdf:about="http://purl.org/olia/susa.owl#CatenativeModalVerb">
        <rdfs:subClassOf rdf:resource="http://purl.org/olia/susa.owl#ModalVerb"/>
        <rdfs:subClassOf rdf:resource="http://purl.org/olia/susa.owl#Past"/>
        <rdfs:comment>The SUSANNE tag VMK is used for &quot;ought&quot; and &quot;used&quot; as modal catenatives.
(Sampson 1995, p. 118)</rdfs:comment>
    </owl:Class>
    


    <!-- http://purl.org/olia/susa.owl#CommonNoun -->

    <owl:Class rdf:about="http://purl.org/olia/susa.owl#CommonNoun">
        <rdfs:subClassOf rdf:resource="http://purl.org/olia/susa.owl#Noun"/>
        <rdfs:comment>SUSANNE tags beginning with NN represent common nouns and direction nouns.
	Also, ND has been included here as it is comparable with temporal situating as in NNa, NNp, NNT....</rdfs:comment>
    </owl:Class>
    


    <!-- http://purl.org/olia/susa.owl#ComparativeAdverb -->

    <owl:Class rdf:about="http://purl.org/olia/susa.owl#ComparativeAdverb">
        <rdfs:subClassOf rdf:resource="http://purl.org/olia/susa.owl#GeneralAdverb"/>
        <rdfs:comment>This is a single-word comparative adverb other than &quot;more&quot; and &quot;less&quot;.
(Sampson 1995, p. 117)</rdfs:comment>
    </owl:Class>
    


    <!-- http://purl.org/olia/susa.owl#Conjunction -->

    <owl:Class rdf:about="http://purl.org/olia/susa.owl#Conjunction">
        <rdfs:subClassOf rdf:resource="http://purl.org/olia/susa.owl#Tag"/>
        <rdfs:comment>The Conjunction class tags conjunctions and subsumes the classes BTO, coordinating conjunctions, subordinating conjunctions and pre-coordinators.
The SUSANNE tags begin with C... . for logical reasons,  pre-coordinator (LE) is added here.</rdfs:comment>
    </owl:Class>
    


    <!-- http://purl.org/olia/susa.owl#CoordinatingConjunction -->

    <owl:Class rdf:about="http://purl.org/olia/susa.owl#CoordinatingConjunction">
        <rdfs:subClassOf rdf:resource="http://purl.org/olia/susa.owl#Conjunction"/>
        <rdfs:comment>SUSANNE tags beginning with CC represent coordinating conjunctions (&quot;and&quot;/CC, &quot;as&quot;/CC31, &quot;but&quot;/CCB).

(Sampson 1995, p. 105)</rdfs:comment>
    </owl:Class>
    


    <!-- http://purl.org/olia/susa.owl#Countability -->

    <owl:Class rdf:about="http://purl.org/olia/susa.owl#Countability">
        <rdfs:subClassOf rdf:resource="http://purl.org/olia/system.owl#Feature"/>
    </owl:Class>
    


    <!-- http://purl.org/olia/susa.owl#DefiniteArticle -->

    <owl:Class rdf:about="http://purl.org/olia/susa.owl#DefiniteArticle">
        <rdfs:subClassOf rdf:resource="http://purl.org/olia/susa.owl#Article"/>
        <rdfs:comment>This is the definite article &quot;the&quot;.
(Sampson 1995, p. 105)</rdfs:comment>
    </owl:Class>
    


    <!-- http://purl.org/olia/susa.owl#Degree -->

    <owl:Class rdf:about="http://purl.org/olia/susa.owl#Degree">
        <rdfs:subClassOf rdf:resource="http://purl.org/olia/system.owl#Feature"/>
    </owl:Class>
    


    <!-- http://purl.org/olia/susa.owl#Demonstrative -->

    <owl:Class rdf:about="http://purl.org/olia/susa.owl#Demonstrative">
        <rdfs:subClassOf rdf:resource="http://purl.org/olia/susa.owl#Determiner"/>
        <rdfs:comment>Demonstratives</rdfs:comment>
    </owl:Class>
    


    <!-- http://purl.org/olia/susa.owl#Determiner -->

    <owl:Class rdf:about="http://purl.org/olia/susa.owl#Determiner">
        <rdfs:subClassOf rdf:resource="http://purl.org/olia/susa.owl#QuantifierDeterminerPronoun"/>
        <rdfs:comment>SUSANNE tag beginning with DD... represent a very heterogeneous group including demonstratives, quantifiers and wh-determiner. 
(Sampson 1995, p. 106)</rdfs:comment>
    </owl:Class>
    


    <!-- http://purl.org/olia/susa.owl#DirectionNoun -->

    <owl:Class rdf:about="http://purl.org/olia/susa.owl#DirectionNoun">
        <rdfs:subClassOf rdf:resource="http://purl.org/olia/susa.owl#CommonNoun"/>
        <rdfs:comment>The SUSANNE tag ND1 is used for direction e.g. &quot;north&quot;, &quot;N&quot;, &quot;southeast&quot;.
(Sampson 1995, p. 111)</rdfs:comment>
    </owl:Class>
    


    <!-- http://purl.org/olia/susa.owl#Distorted -->

    <owl:Class rdf:about="http://purl.org/olia/susa.owl#Distorted">
        <rdfs:subClassOf rdf:resource="http://purl.org/olia/susa.owl#NonPOS"/>
        <rdfs:comment>FD is used for a distorted word, for spoken language only.
(Sampson 1995, p. 107)</rdfs:comment>
    </owl:Class>
    


    <!-- http://purl.org/olia/susa.owl#Do -->

    <owl:Class rdf:about="http://purl.org/olia/susa.owl#Do">
        <rdfs:subClassOf rdf:resource="http://purl.org/olia/susa.owl#Verb"/>
        <rdfs:comment>The class DoType contains the SUSANNE tags for the forms of &quot;do&quot;.
(Sampson 1995, p. 118)</rdfs:comment>
    </owl:Class>
    


    <!-- http://purl.org/olia/susa.owl#DoBaseForm -->

    <owl:Class rdf:about="http://purl.org/olia/susa.owl#DoBaseForm">
        <rdfs:subClassOf rdf:resource="http://purl.org/olia/susa.owl#BaseForm"/>
        <rdfs:subClassOf rdf:resource="http://purl.org/olia/susa.owl#Do"/>
        <rdfs:comment>The SUSANNE tag VD0 is used for &quot;do&quot; as infinitive or as indicative.  
(Sampson 1995, p. 119)</rdfs:comment>
    </owl:Class>
    


    <!-- http://purl.org/olia/susa.owl#DoPast -->

    <owl:Class rdf:about="http://purl.org/olia/susa.owl#DoPast">
        <rdfs:subClassOf rdf:resource="http://purl.org/olia/susa.owl#Do"/>
        <rdfs:subClassOf rdf:resource="http://purl.org/olia/susa.owl#PresentParticiple"/>
        <rdfs:comment>VDD is used for &quot;did&quot;. 
(Sampson 1995, p. 118)</rdfs:comment>
    </owl:Class>
    


    <!-- http://purl.org/olia/susa.owl#DoPastParticiple -->

    <owl:Class rdf:about="http://purl.org/olia/susa.owl#DoPastParticiple">
        <rdfs:subClassOf rdf:resource="http://purl.org/olia/susa.owl#Do"/>
        <rdfs:subClassOf rdf:resource="http://purl.org/olia/susa.owl#PastParticiple"/>
        <rdfs:comment>The VDN tag describes &quot;done&quot;.
(Sampson 1995, p. 118)</rdfs:comment>
    </owl:Class>
    


    <!-- http://purl.org/olia/susa.owl#DoPresentParticiple -->

    <owl:Class rdf:about="http://purl.org/olia/susa.owl#DoPresentParticiple">
        <rdfs:subClassOf rdf:resource="http://purl.org/olia/susa.owl#Do"/>
        <rdfs:comment>Present participle of &quot;to do&quot;.</rdfs:comment>
    </owl:Class>
    


    <!-- http://purl.org/olia/susa.owl#Does -->

    <owl:Class rdf:about="http://purl.org/olia/susa.owl#Does">
        <rdfs:subClassOf rdf:resource="http://purl.org/olia/susa.owl#Do"/>
        <rdfs:subClassOf rdf:resource="http://purl.org/olia/susa.owl#Present"/>
        <rdfs:comment>VDZ is used for &quot;does&quot;.
(Sampson 1995, p. 118)</rdfs:comment>
    </owl:Class>
    


    <!-- http://purl.org/olia/susa.owl#Every -->

    <owl:Class rdf:about="http://purl.org/olia/susa.owl#Every">
        <rdfs:subClassOf rdf:resource="http://purl.org/olia/susa.owl#Article"/>
        <rdfs:comment>SUSANNE tag used for &quot;every&quot; (Sampson 1995, p. 105), according to http://www.ilc.cnr.it/EAGLES96/morphsyn/node454.html#SECTION00084100000000000000, an indefinite determiner</rdfs:comment>
    </owl:Class>
    


    <!-- http://purl.org/olia/susa.owl#ExistentialThere -->

    <owl:Class rdf:about="http://purl.org/olia/susa.owl#ExistentialThere">
        <rdfs:subClassOf rdf:resource="http://purl.org/olia/susa.owl#Unique"/>
        <rdfs:comment>EX is the SUSANNE tag used for existential &quot;there&quot;.
(Sampson 1995, p. 107)</rdfs:comment>
    </owl:Class>
    


    <!-- http://purl.org/olia/susa.owl#ForeignWord -->

    <owl:Class rdf:about="http://purl.org/olia/susa.owl#ForeignWord">
        <rdfs:subClassOf rdf:resource="http://purl.org/olia/susa.owl#NonPOS"/>
        <rdfs:comment>SUSANNE tag beginning with FW... apply to foreign words which are not capable of being allocated a more specific tag by reference to their English context.
(Sampson 1995, p. 108)</rdfs:comment>
    </owl:Class>
    


    <!-- http://purl.org/olia/susa.owl#Form -->

    <owl:Class rdf:about="http://purl.org/olia/susa.owl#Form">
        <rdfs:subClassOf rdf:resource="http://purl.org/olia/system.owl#Feature"/>
    </owl:Class>
    


    <!-- http://purl.org/olia/susa.owl#Formula -->

    <owl:Class rdf:about="http://purl.org/olia/susa.owl#Formula">
        <rdfs:subClassOf rdf:resource="http://purl.org/olia/susa.owl#NonPOS"/>
        <rdfs:comment>The FO class subsumes formulas, mathematical expressions, adresses etc..
(Sampson 1995, p. 107f.)</rdfs:comment>
    </owl:Class>
    


    <!-- http://purl.org/olia/susa.owl#Fraction -->

    <owl:Class rdf:about="http://purl.org/olia/susa.owl#Fraction">
        <rdfs:subClassOf rdf:resource="http://purl.org/olia/susa.owl#Numeral"/>
        <rdfs:comment>MFn is the tag used for fractons written digitally e.g. &quot;2/3&quot;.
(Sampson 1995, p. 111)</rdfs:comment>
    </owl:Class>
    


    <!-- http://purl.org/olia/susa.owl#Gender -->

    <owl:Class rdf:about="http://purl.org/olia/susa.owl#Gender">
        <rdfs:subClassOf rdf:resource="http://purl.org/olia/system.owl#Feature"/>
    </owl:Class>
    


    <!-- http://purl.org/olia/susa.owl#GeneralAdjective -->

    <owl:Class rdf:about="http://purl.org/olia/susa.owl#GeneralAdjective">
        <rdfs:subClassOf rdf:resource="http://purl.org/olia/susa.owl#Adjective"/>
        <rdfs:comment>These are general adjectives.
(Sampson 1995, p. 109)</rdfs:comment>
    </owl:Class>
    


    <!-- http://purl.org/olia/susa.owl#GeneralAdverb -->

    <owl:Class rdf:about="http://purl.org/olia/susa.owl#GeneralAdverb">
        <rdfs:subClassOf rdf:resource="http://purl.org/olia/susa.owl#Adverb"/>
        <rdfs:comment>SUSANNE tags beginning with RR... are general adverbs. 
(Sampson 1995, p.117)</rdfs:comment>
    </owl:Class>
    


    <!-- http://purl.org/olia/susa.owl#GenitiveInflection -->

    <owl:Class rdf:about="http://purl.org/olia/susa.owl#GenitiveInflection">
        <rdfs:subClassOf rdf:resource="http://purl.org/olia/susa.owl#NonPOS"/>
        <rdfs:comment>GG is the SUSANNE tag used for the Germanic genitive inflection +´s, or + ´ after a plural stem and certain other stems ending in -s.
(Sampson 1995, p. 108)</rdfs:comment>
        <owl:versionInfo>
		Germanic genitive &apos;s is modelled as NonPOS here because of its diachronic origin as a morphological element, cf. FA. (Chiarcos)
		Alternatively, &apos;s could be treated as postposition (http://www.ilc.cnr.it/EAGLES96/morphsyn/node56.html#SECTION00044000000000000000, 
		http://www.ilc.cnr.it/EAGLES96/morphsyn/node586.html#SECTION000114100000000000000)</owl:versionInfo>
    </owl:Class>
    


    <!-- http://purl.org/olia/susa.owl#Has -->

    <owl:Class rdf:about="http://purl.org/olia/susa.owl#Has">
        <rdfs:subClassOf rdf:resource="http://purl.org/olia/susa.owl#Have"/>
        <rdfs:subClassOf rdf:resource="http://purl.org/olia/susa.owl#Present"/>
        <rdfs:comment>The SUSANNE tag VHZ is used for &quot;has&quot;. 
(Sampson 1995, p. 119)</rdfs:comment>
    </owl:Class>
    


    <!-- http://purl.org/olia/susa.owl#Have -->

    <owl:Class rdf:about="http://purl.org/olia/susa.owl#Have">
        <rdfs:subClassOf rdf:resource="http://purl.org/olia/susa.owl#Verb"/>
        <rdfs:comment>SUSANNE tags for forms of &quot;to have&quot;.
(Sampson 1995, p. 118)</rdfs:comment>
    </owl:Class>
    


    <!-- http://purl.org/olia/susa.owl#HaveBaseForm -->

    <owl:Class rdf:about="http://purl.org/olia/susa.owl#HaveBaseForm">
        <rdfs:subClassOf rdf:resource="http://purl.org/olia/susa.owl#BaseForm"/>
        <rdfs:subClassOf rdf:resource="http://purl.org/olia/susa.owl#Have"/>
        <rdfs:comment>The SUSANNE VH0 is used for &quot;have&quot;. 
(Sampson 1995, p. 119)</rdfs:comment>
    </owl:Class>
    


    <!-- http://purl.org/olia/susa.owl#HavePast -->

    <owl:Class rdf:about="http://purl.org/olia/susa.owl#HavePast">
        <rdfs:subClassOf rdf:resource="http://purl.org/olia/susa.owl#Have"/>
        <rdfs:subClassOf rdf:resource="http://purl.org/olia/susa.owl#Past"/>
        <rdfs:comment>The tag VHD is used for the past tense form &quot;had&quot;. 
(Sampson 1995, p. 119)</rdfs:comment>
    </owl:Class>
    


    <!-- http://purl.org/olia/susa.owl#HavePastParticiple -->

    <owl:Class rdf:about="http://purl.org/olia/susa.owl#HavePastParticiple">
        <rdfs:subClassOf rdf:resource="http://purl.org/olia/susa.owl#Have"/>
        <rdfs:subClassOf rdf:resource="http://purl.org/olia/susa.owl#PastParticiple"/>
        <rdfs:comment>The SUSANNE tag VHN is used for the past participle form &quot;had&quot;. 
(Sampson 1995, p. 119)</rdfs:comment>
    </owl:Class>
    


    <!-- http://purl.org/olia/susa.owl#HavePresentParticiple -->

    <owl:Class rdf:about="http://purl.org/olia/susa.owl#HavePresentParticiple">
        <rdfs:subClassOf rdf:resource="http://purl.org/olia/susa.owl#Have"/>
        <rdfs:subClassOf rdf:resource="http://purl.org/olia/susa.owl#PresentParticiple"/>
        <rdfs:comment>The SUSANNE tag VHG is used for &quot;having&quot;. 
(Sampson 1995, p. 119)</rdfs:comment>
    </owl:Class>
    


    <!-- http://purl.org/olia/susa.owl#IndefiniteArticle -->

    <owl:Class rdf:about="http://purl.org/olia/susa.owl#IndefiniteArticle">
        <rdfs:subClassOf rdf:resource="http://purl.org/olia/susa.owl#Article"/>
        <rdfs:comment>This is used for the indefinite article &quot;a&quot;, &quot;an&quot;.
(Sampson 1995, p. 105)</rdfs:comment>
    </owl:Class>
    


    <!-- http://purl.org/olia/susa.owl#Interjection -->

    <owl:Class rdf:about="http://purl.org/olia/susa.owl#Interjection">
        <rdfs:subClassOf rdf:resource="http://purl.org/olia/susa.owl#Tag"/>
        <rdfs:comment>These are interjections tagged UH in SUSANNE.
	In the CHRISTINE corpus replaced with a range of different U-tags.
	</rdfs:comment>
    </owl:Class>
    


    <!-- http://purl.org/olia/susa.owl#Is -->

    <owl:Class rdf:about="http://purl.org/olia/susa.owl#Is">
        <rdfs:subClassOf rdf:resource="http://purl.org/olia/susa.owl#Be"/>
        <rdfs:subClassOf rdf:resource="http://purl.org/olia/susa.owl#Present"/>
        <rdfs:comment>The SUSANNE tag VBZ is used for &quot;is&quot;.
(Sampson 1995, p. 118)</rdfs:comment>
    </owl:Class>
    


    <!-- http://purl.org/olia/susa.owl#Letter -->

    <owl:Class rdf:about="http://purl.org/olia/susa.owl#Letter">
        <rdfs:subClassOf rdf:resource="http://purl.org/olia/susa.owl#NonPOS"/>
        <rdfs:comment>ZZ is used for letters and letter names of the (roman or other) alphabet.
(Sampson 1995, p. 120)</rdfs:comment>
    </owl:Class>
    


    <!-- http://purl.org/olia/susa.owl#LexicalVerb -->

    <owl:Class rdf:about="http://purl.org/olia/susa.owl#LexicalVerb">
        <rdfs:subClassOf rdf:resource="http://purl.org/olia/susa.owl#Verb"/>
        <rdfs:comment>These are lexical verbs.</rdfs:comment>
    </owl:Class>
    


    <!-- http://purl.org/olia/susa.owl#LexicalVerbBaseForm -->

    <owl:Class rdf:about="http://purl.org/olia/susa.owl#LexicalVerbBaseForm">
        <rdfs:subClassOf rdf:resource="http://purl.org/olia/susa.owl#BaseForm"/>
        <rdfs:subClassOf rdf:resource="http://purl.org/olia/susa.owl#LexicalVerb"/>
        <rdfs:comment>SUSANNE tags which begin with VV... are used for non-modal/non-auxiliar verbs.
(Sampson 1995, p. 118f)</rdfs:comment>
    </owl:Class>
    


    <!-- http://purl.org/olia/susa.owl#LexicalVerbPastForm -->

    <owl:Class rdf:about="http://purl.org/olia/susa.owl#LexicalVerbPastForm">
        <rdfs:subClassOf rdf:resource="http://purl.org/olia/susa.owl#LexicalVerb"/>
        <rdfs:subClassOf rdf:resource="http://purl.org/olia/susa.owl#Past"/>
        <rdfs:comment>SUSANNE tags beginning with VV... are used for non-modal verbs or non-auxiliary verbs. 
LexicalVerbPastForm is a class for past tense verbforms. 

(Sampson 1995, p. 118f)</rdfs:comment>
    </owl:Class>
    


    <!-- http://purl.org/olia/susa.owl#LexicalVerbPastParticiple -->

    <owl:Class rdf:about="http://purl.org/olia/susa.owl#LexicalVerbPastParticiple">
        <rdfs:subClassOf rdf:resource="http://purl.org/olia/susa.owl#LexicalVerb"/>
        <rdfs:subClassOf rdf:resource="http://purl.org/olia/susa.owl#PastParticiple"/>
        <rdfs:comment>SUSANNE tags beginningwith VVN represent past participles of lexical verbs.</rdfs:comment>
    </owl:Class>
    


    <!-- http://purl.org/olia/susa.owl#LexicalVerbPresentParticiple -->

    <owl:Class rdf:about="http://purl.org/olia/susa.owl#LexicalVerbPresentParticiple">
        <rdfs:subClassOf rdf:resource="http://purl.org/olia/susa.owl#LexicalVerb"/>
        <rdfs:subClassOf rdf:resource="http://purl.org/olia/susa.owl#PresentParticiple"/>
        <rdfs:comment>Tags which begin with VV... are used for non-modal verbs or non-auxiliary verbs.
	 LexicalVerbPresentParticiple is a class for present participle verbforms.
	(Sampson 1995: 118f)</rdfs:comment>
    </owl:Class>
    


    <!-- http://purl.org/olia/susa.owl#LexicalVerbThirdPerson -->

    <owl:Class rdf:about="http://purl.org/olia/susa.owl#LexicalVerbThirdPerson">
        <rdfs:subClassOf rdf:resource="http://purl.org/olia/susa.owl#LexicalVerb"/>
        <rdfs:subClassOf rdf:resource="http://purl.org/olia/susa.owl#Present"/>
        <rdfs:comment>Tags which begin with VV... are used for non-modal verbs or non-auxiliary verbs.
LexicalVerbThirdPerson is used for the third person form of full verbs. 
(Sampson 1995, p. 119)</rdfs:comment>
    </owl:Class>
    


    <!-- http://purl.org/olia/susa.owl#ModalVerb -->

    <owl:Class rdf:about="http://purl.org/olia/susa.owl#ModalVerb">
        <rdfs:subClassOf rdf:resource="http://purl.org/olia/susa.owl#Verb"/>
        <rdfs:comment>The class of ModalVerb contains the SUSANNE tags VMd, VMo and VMK.
</rdfs:comment>
    </owl:Class>
    


    <!-- http://purl.org/olia/susa.owl#ModalVerbBaseForm -->

    <owl:Class rdf:about="http://purl.org/olia/susa.owl#ModalVerbBaseForm">
        <rdfs:subClassOf rdf:resource="http://purl.org/olia/susa.owl#BaseForm"/>
        <rdfs:subClassOf rdf:resource="http://purl.org/olia/susa.owl#ModalVerb"/>
        <rdfs:comment>The SUSANNE tag VMo is used for modals in present form e.g. &quot;can&quot;, &quot;dare&quot;, &quot;may&quot;, &quot;must&quot;, &quot;need&quot;, &quot;shall&quot;, &quot;will&quot;.
(Sampson 1995, p. 118)
	</rdfs:comment>
        <owl:versionInfo>&quot;o&quot; (Sampson 1995, p. 118) is possibly misspelled for &quot;0&quot;.</owl:versionInfo>
    </owl:Class>
    


    <!-- http://purl.org/olia/susa.owl#ModalVerbPast -->

    <owl:Class rdf:about="http://purl.org/olia/susa.owl#ModalVerbPast">
        <rdfs:subClassOf rdf:resource="http://purl.org/olia/susa.owl#ModalVerb"/>
        <rdfs:subClassOf rdf:resource="http://purl.org/olia/susa.owl#Past"/>
        <rdfs:comment>The SUSANNE tag VMd is used for modals in past form e.g. &quot;could&quot;, &quot;might&quot;, &quot;should&quot;, &quot;would&quot;.
(Sampson 1995, p. 118)</rdfs:comment>
        <owl:versionInfo>&quot;d&quot; in the tag name is possibly misspelled for &quot;D&quot;.</owl:versionInfo>
    </owl:Class>
    


    <!-- http://purl.org/olia/susa.owl#NegativeDeterminer -->

    <owl:Class rdf:about="http://purl.org/olia/susa.owl#NegativeDeterminer">
        <rdfs:subClassOf rdf:resource="http://purl.org/olia/susa.owl#Article"/>
        <rdfs:comment>This is used for &quot;no&quot; as determiner or qualifier.
(Sampson 1995, p. 105)</rdfs:comment>
    </owl:Class>
    


    <!-- http://purl.org/olia/susa.owl#NonPOS -->

    <owl:Class rdf:about="http://purl.org/olia/susa.owl#NonPOS">
        <rdfs:subClassOf rdf:resource="http://purl.org/olia/susa.owl#Tag"/>
        <rdfs:comment>The NonPOS class subsumes separated morphological elements, formulae, equations, foreign words etc.
	Also, GG (~ FA) and ZZ (single Letter) are added here
	</rdfs:comment>
    </owl:Class>
    


    <!-- http://purl.org/olia/susa.owl#Not -->

    <owl:Class rdf:about="http://purl.org/olia/susa.owl#Not">
        <rdfs:subClassOf rdf:resource="http://purl.org/olia/susa.owl#Unique"/>
        <rdfs:comment>XX is the SUSANNE tag for the word &quot;not&quot;.
(Sampson 1995, p. 119)</rdfs:comment>
    </owl:Class>
    


    <!-- http://purl.org/olia/susa.owl#Noun -->

    <owl:Class rdf:about="http://purl.org/olia/susa.owl#Noun">
        <rdfs:subClassOf rdf:resource="http://purl.org/olia/susa.owl#Tag"/>
        <rdfs:comment>SUSANNE tags beginning with N... represent nouns (proper nouns and common nouns).</rdfs:comment>
    </owl:Class>
    


    <!-- http://purl.org/olia/susa.owl#Number -->

    <owl:Class rdf:about="http://purl.org/olia/susa.owl#Number">
        <rdfs:subClassOf rdf:resource="http://purl.org/olia/system.owl#Feature"/>
    </owl:Class>
    


    <!-- http://purl.org/olia/susa.owl#Numeral -->

    <owl:Class rdf:about="http://purl.org/olia/susa.owl#Numeral">
        <rdfs:subClassOf rdf:resource="http://purl.org/olia/susa.owl#Tag"/>
        <rdfs:comment>The Numeral class subsumes cardinal numbers, ordinal numbers and fraction numbers. The SUSANNE tags begin with M.. .</rdfs:comment>
    </owl:Class>
    


    <!-- http://purl.org/olia/susa.owl#OrdinalNumber -->

    <owl:Class rdf:about="http://purl.org/olia/susa.owl#OrdinalNumber">
        <rdfs:subClassOf rdf:resource="http://purl.org/olia/susa.owl#Numeral"/>
        <rdfs:comment>MD is the SUSANNE tag used for ordinal numbers, whether used as ordinal adjective or adverb or as fraction e.g. &quot;third&quot;, &quot;fourth&quot;.
(Sampson 1995, p. 111)</rdfs:comment>
    </owl:Class>
    


    <!-- http://purl.org/olia/susa.owl#OrganizationNoun -->

    <owl:Class rdf:about="http://purl.org/olia/susa.owl#OrganizationNoun">
        <rdfs:subClassOf rdf:resource="http://purl.org/olia/susa.owl#CommonNoun"/>
        <rdfs:comment>Organization nouns are common nouns that denote is an organization and that are used as the head word in the name of organizations of that kind. (Sampson 1995, p. 94)</rdfs:comment>
    </owl:Class>
    


    <!-- http://purl.org/olia/susa.owl#Past -->

    <owl:Class rdf:about="http://purl.org/olia/susa.owl#Past">
        <rdfs:subClassOf rdf:resource="http://purl.org/olia/susa.owl#Verb"/>
        <rdfs:comment>SUSANNE tags beginning with V and containing D,d or K represent past tense verbs (VBD, VHD, VMd, VMK and VVD).</rdfs:comment>
    </owl:Class>
    


    <!-- http://purl.org/olia/susa.owl#PastParticiple -->

    <owl:Class rdf:about="http://purl.org/olia/susa.owl#PastParticiple">
        <rdfs:subClassOf rdf:resource="http://purl.org/olia/susa.owl#Verb"/>
        <rdfs:comment>SUSANNE tags beginning with V and containing N (VDN, VHN and VVN) represent past participles.</rdfs:comment>
    </owl:Class>
    


    <!-- http://purl.org/olia/susa.owl#Person -->

    <owl:Class rdf:about="http://purl.org/olia/susa.owl#Person">
        <rdfs:subClassOf rdf:resource="http://purl.org/olia/system.owl#Feature"/>
    </owl:Class>
    


    <!-- http://purl.org/olia/susa.owl#PostmodifyingAdverb -->

    <owl:Class rdf:about="http://purl.org/olia/susa.owl#PostmodifyingAdverb">
        <rdfs:subClassOf rdf:resource="http://purl.org/olia/susa.owl#Adverb"/>
        <rdfs:comment>Postmodifying adverbs and adverb-like phrases.
(Sampson 1995, p.115f.)</rdfs:comment>
    </owl:Class>
    


    <!-- http://purl.org/olia/susa.owl#PreCoordinator -->

    <owl:Class rdf:about="http://purl.org/olia/susa.owl#PreCoordinator">
        <rdfs:subClassOf rdf:resource="http://purl.org/olia/susa.owl#Conjunction"/>
        <rdfs:comment>The SUSANNE tag LE applies to pre-coordinators, i.e., the first element of paired coordination markers (cf. http://www.ilc.cnr.it/EAGLES96/morphsyn/node622.html#SECTION000124200000000000000, §3.71).
In the Susanne Corpus &quot;pre-co-ordinator&quot; means the first part of  paired co-ordinating markers, e.g. in &quot;both... and&quot;, &quot;neither... nor&quot;.
(Sampson 1995, p.110)</rdfs:comment>
    </owl:Class>
    


    <!-- http://purl.org/olia/susa.owl#PredicativeAdjective -->

    <owl:Class rdf:about="http://purl.org/olia/susa.owl#PredicativeAdjective">
        <rdfs:subClassOf rdf:resource="http://purl.org/olia/susa.owl#Adjective"/>
        <rdfs:comment>These are predicatively used adjectives (&quot;akin&quot;, &quot;alike&quot;, &quot;asleep&quot;).
(Sampson 1995, p. 109)</rdfs:comment>
    </owl:Class>
    


    <!-- http://purl.org/olia/susa.owl#Prefix -->

    <owl:Class rdf:about="http://purl.org/olia/susa.owl#Prefix">
        <rdfs:subClassOf rdf:resource="http://purl.org/olia/susa.owl#NonPOS"/>
        <rdfs:comment>FB is the SUSANNE tag used for a prefix which is seperated by a hyphen.
(Sampson 1995, p. 107)</rdfs:comment>
    </owl:Class>
    


    <!-- http://purl.org/olia/susa.owl#Preposition -->

    <owl:Class rdf:about="http://purl.org/olia/susa.owl#Preposition">
        <rdfs:subClassOf rdf:resource="http://purl.org/olia/susa.owl#Tag"/>
        <rdfs:comment>SUSANNE tags beginning with I... represent prepositions, but also PrepositionOrSubordinatingConjunction.</rdfs:comment>
    </owl:Class>
    


    <!-- http://purl.org/olia/susa.owl#PrepositionAsAdverb -->

    <owl:Class rdf:about="http://purl.org/olia/susa.owl#PrepositionAsAdverb">
        <rdfs:subClassOf rdf:resource="http://purl.org/olia/susa.owl#Adverb"/>
        <rdfs:comment>SUSANNE tags beginning with RP... represent prepositions used as adverb.
(Sampson 1995, p.116f)</rdfs:comment>
    </owl:Class>
    


    <!-- http://purl.org/olia/susa.owl#PrepositionOrSubordinatingConjunction -->

    <owl:Class rdf:about="http://purl.org/olia/susa.owl#PrepositionOrSubordinatingConjunction">
        <rdfs:subClassOf rdf:resource="http://purl.org/olia/susa.owl#Preposition"/>
        <rdfs:subClassOf rdf:resource="http://purl.org/olia/susa.owl#SubordinatingConjunction"/>
        <rdfs:comment>SUSANNE tags beginning with ICS apply to prepositions (I) that can also occur as subordinating conjunctions (CS), e.g.,
	&quot;after&quot;, &quot;before&quot;, &quot;since&quot; (ICSt), &quot;considering&quot; (ICS), &quot;save&quot; (ICSx).
	This ambiguity is not resolved in SUSANNE.
(Sampson 1995, p.108f.)</rdfs:comment>
        <owl:versionInfo>TODO: check linking</owl:versionInfo>
    </owl:Class>
    


    <!-- http://purl.org/olia/susa.owl#Present -->

    <owl:Class rdf:about="http://purl.org/olia/susa.owl#Present">
        <rdfs:subClassOf rdf:resource="http://purl.org/olia/susa.owl#Verb"/>
        <rdfs:comment>The Present class contains the SUSANNE tags VBM, VBZ, VDZ, VHZ and VVZ.
	 SUSANNE V...-tags which contain &quot;M&quot; represent first person singular of &quot;be&quot;, those which contain &quot;Z&quot; represent third person singular verbs.
	 Other present verbs are tagged as BaseForm.
	</rdfs:comment>
    </owl:Class>
    


    <!-- http://purl.org/olia/susa.owl#PresentParticiple -->

    <owl:Class rdf:about="http://purl.org/olia/susa.owl#PresentParticiple">
        <rdfs:subClassOf rdf:resource="http://purl.org/olia/susa.owl#Verb"/>
        <rdfs:comment>The PresentParticiple class contains the SUSANNE tags VBG, VDD, VHG and VVG which stand for present participle forms.</rdfs:comment>
    </owl:Class>
    


    <!-- http://purl.org/olia/susa.owl#ProperNoun -->

    <owl:Class rdf:about="http://purl.org/olia/susa.owl#ProperNoun">
        <rdfs:subClassOf rdf:resource="http://purl.org/olia/susa.owl#Noun"/>
        <rdfs:comment>SUSANNE tags beginning with NP... apply to several subtypes of proper nouns. 
(Sampson 1995, p. 113f.)</rdfs:comment>
    </owl:Class>
    


    <!-- http://purl.org/olia/susa.owl#ProperSubordinatingConjunction -->

    <owl:Class rdf:about="http://purl.org/olia/susa.owl#ProperSubordinatingConjunction">
        <rdfs:subClassOf rdf:resource="http://purl.org/olia/susa.owl#SubordinatingConjunction"/>
    </owl:Class>
    


    <!-- http://purl.org/olia/susa.owl#Punctuation -->

    <owl:Class rdf:about="http://purl.org/olia/susa.owl#Punctuation">
        <rdfs:subClassOf rdf:resource="http://purl.org/olia/susa.owl#Tag"/>
        <rdfs:comment>SUSANNE tags beginning with Y represent punctuation, text-structuring symbols, font instructions and pauses.</rdfs:comment>
    </owl:Class>
    


    <!-- http://purl.org/olia/susa.owl#Qualifier -->

    <owl:Class rdf:about="http://purl.org/olia/susa.owl#Qualifier">
        <rdfs:subClassOf rdf:resource="http://purl.org/olia/susa.owl#Adverb"/>
        <rdfs:comment>In SUSANNE terminology, a &quot;qualifier&quot; is an adverb-modifying adjective or adverb.
	 Tags beginning with RG... apply to qualifiers which having no other adverbial use. 
	(Sampson 1995, p.116)</rdfs:comment>
    </owl:Class>
    


    <!-- http://purl.org/olia/susa.owl#Quantifier -->

    <owl:Class rdf:about="http://purl.org/olia/susa.owl#Quantifier">
        <rdfs:subClassOf rdf:resource="http://purl.org/olia/susa.owl#Determiner"/>
        <rdfs:subClassOf rdf:resource="http://purl.org/olia/susa.owl#QuantifierDeterminerPronoun"/>
        <rdfs:comment>SUSANNE tags begin with DA... represent quantifiers (&quot;few&quot;, &quot;little&quot;, &quot;less&quot;, &quot;many&quot;, &quot;several&quot;). 
(Sampson 1995, p. 106)</rdfs:comment>
    </owl:Class>
    


    <!-- http://purl.org/olia/susa.owl#QuantifierDeterminerPronoun -->

    <owl:Class rdf:about="http://purl.org/olia/susa.owl#QuantifierDeterminerPronoun">
        <rdfs:subClassOf rdf:resource="http://purl.org/olia/susa.owl#Tag"/>
        <rdfs:comment>SUSANNE tags beginning with D... form a very heterogeneous class of expressions include quantifiers, DB and determiners. 
	 According to the examples, the prototypical forms which are collected here can be used as determiners. Some have ambiguity with pronouns.</rdfs:comment>
    </owl:Class>
    


    <!-- http://purl.org/olia/susa.owl#QuantifyingPronoun -->

    <owl:Class rdf:about="http://purl.org/olia/susa.owl#QuantifyingPronoun">
        <rdfs:subClassOf rdf:resource="http://purl.org/olia/susa.owl#QuantifierDeterminerPronoun"/>
        <rdfs:comment>The class QuantifyingPronoun subsumes quantifying determiners or pronouns (&quot;all&quot;, &quot;both&quot;, &quot;half&quot;).
(Sampson 1995, p. 106)</rdfs:comment>
    </owl:Class>
    


    <!-- http://purl.org/olia/susa.owl#ReflexivePronoun -->

    <owl:Class rdf:about="http://purl.org/olia/susa.owl#ReflexivePronoun">
        <rdfs:subClassOf rdf:resource="http://purl.org/olia/susa.owl#SubstitutivePersonalPronoun"/>
        <rdfs:comment>These are the reflexive personal pronouns. 
Their tags begin with PPX.. . 
(Sampson 1995, p. 115)</rdfs:comment>
    </owl:Class>
    


    <!-- http://purl.org/olia/susa.owl#SubordinatingConjunction -->

    <owl:Class rdf:about="http://purl.org/olia/susa.owl#SubordinatingConjunction">
        <rdfs:subClassOf rdf:resource="http://purl.org/olia/susa.owl#Conjunction"/>
        <rdfs:comment>SUSANNE tags beginning with CS... represent subcoordinating conjunctions (&quot;although&quot;, &quot;how&quot;, &quot;if&quot;).
(Sampson 1995, p.106)
	The tags BTO and TO are also included here, according to van Valin and Lapolla (1997), English &quot;to&quot; (+infinitive) is a subordinating
	conjunction.
	</rdfs:comment>
    </owl:Class>
    


    <!-- http://purl.org/olia/susa.owl#SubordinatingConjunctionWithInfinitival -->

    <owl:Class rdf:about="http://purl.org/olia/susa.owl#SubordinatingConjunctionWithInfinitival">
        <rdfs:subClassOf rdf:resource="http://purl.org/olia/susa.owl#SubordinatingConjunction"/>
        <rdfs:comment>SUSANNE tag for &quot;in order&quot; introducing infinitive (cf. TO);
	according to http://www.ilc.cnr.it/EAGLES96/morphsyn/node623.html#SECTION000124300000000000000 this is a subordinating conjunction</rdfs:comment>
    </owl:Class>
    


    <!-- http://purl.org/olia/susa.owl#SubstitutiveFirstPersonPronoun -->

    <owl:Class rdf:about="http://purl.org/olia/susa.owl#SubstitutiveFirstPersonPronoun">
        <rdfs:subClassOf rdf:resource="http://purl.org/olia/susa.owl#SubstitutivePersonalPronoun"/>
        <rdfs:comment>SUSANNE tags beginning with PPI... represent first person pronouns.
(Sampson 1995, p. 115)</rdfs:comment>
    </owl:Class>
    


    <!-- http://purl.org/olia/susa.owl#SubstitutiveIndefinitePronoun -->

    <owl:Class rdf:about="http://purl.org/olia/susa.owl#SubstitutiveIndefinitePronoun">
        <rdfs:subClassOf rdf:resource="http://purl.org/olia/susa.owl#SubstitutivePronoun"/>
        <rdfs:comment>The SubstitutiveIndefinitePronoun class subsumes the SUSANNE tags PN1 and PNX1.</rdfs:comment>
    </owl:Class>
    


    <!-- http://purl.org/olia/susa.owl#SubstitutiveIndefiniteReflexive -->

    <owl:Class rdf:about="http://purl.org/olia/susa.owl#SubstitutiveIndefiniteReflexive">
        <rdfs:subClassOf rdf:resource="http://purl.org/olia/susa.owl#SubstitutiveIndefinitePronoun"/>
        <rdfs:comment>PNX1 is the SUSANNE tag used for the singular indefinite reflexive &quot;oneself&quot;. 
(Sampson 1995, p. 115)</rdfs:comment>
    </owl:Class>
    


    <!-- http://purl.org/olia/susa.owl#SubstitutiveInterrogativePronoun -->

    <owl:Class rdf:about="http://purl.org/olia/susa.owl#SubstitutiveInterrogativePronoun">
        <rdfs:subClassOf rdf:resource="http://purl.org/olia/susa.owl#SubstitutiveWHPronoun"/>
        <rdfs:comment>The SubstitutiveInterrogativePronoun class contains the SUSANNE tags PNQOq and PNQSq.</rdfs:comment>
    </owl:Class>
    


    <!-- http://purl.org/olia/susa.owl#SubstitutiveNegativePronoun -->

    <owl:Class rdf:about="http://purl.org/olia/susa.owl#SubstitutiveNegativePronoun">
        <rdfs:subClassOf rdf:resource="http://purl.org/olia/susa.owl#SubstitutivePronoun"/>
        <rdfs:comment>This is the negative substitutive pronoun &quot;none&quot;. 
(Sampson 1995, p. 114)</rdfs:comment>
    </owl:Class>
    


    <!-- http://purl.org/olia/susa.owl#SubstitutivePersonalPronoun -->

    <owl:Class rdf:about="http://purl.org/olia/susa.owl#SubstitutivePersonalPronoun">
        <rdfs:subClassOf rdf:resource="http://purl.org/olia/susa.owl#SubstitutivePronoun"/>
        <rdfs:comment>SUSANNE tags beginning with PP... represent substitutive personal pronouns</rdfs:comment>
    </owl:Class>
    


    <!-- http://purl.org/olia/susa.owl#SubstitutivePossessivePronoun -->

    <owl:Class rdf:about="http://purl.org/olia/susa.owl#SubstitutivePossessivePronoun">
        <rdfs:subClassOf rdf:resource="http://purl.org/olia/susa.owl#SubstitutivePersonalPronoun"/>
        <rdfs:comment>These are substitutive possessive pronouns. The SUSANNE tags begin with PPG... . (G is &quot;genitive&quot;, as English possessives are derived from Genitive forms of personal pronouns)
(Sampson 1995, p. 115)</rdfs:comment>
    </owl:Class>
    


    <!-- http://purl.org/olia/susa.owl#SubstitutivePronoun -->

    <owl:Class rdf:about="http://purl.org/olia/susa.owl#SubstitutivePronoun">
        <rdfs:subClassOf rdf:resource="http://purl.org/olia/susa.owl#Tag"/>
        <rdfs:comment>SUSANNE tags beginning with P... represent substitutive pronouns (EAGLES &quot;pronouns&quot; as opposed to &quot;determiner&quot;).</rdfs:comment>
    </owl:Class>
    


    <!-- http://purl.org/olia/susa.owl#SubstitutiveRelativePronoun -->

    <owl:Class rdf:about="http://purl.org/olia/susa.owl#SubstitutiveRelativePronoun">
        <rdfs:subClassOf rdf:resource="http://purl.org/olia/susa.owl#SubstitutiveWHPronoun"/>
        <rdfs:comment>The SubstitutiveRelativePronoun class contains the SUSANNE tags PNQOr and PNQSr.</rdfs:comment>
    </owl:Class>
    


    <!-- http://purl.org/olia/susa.owl#SubstitutiveSecondPersonPronoun -->

    <owl:Class rdf:about="http://purl.org/olia/susa.owl#SubstitutiveSecondPersonPronoun">
        <rdfs:subClassOf rdf:resource="http://purl.org/olia/susa.owl#SubstitutivePersonalPronoun"/>
        <rdfs:comment>This is the second person personal pronoun &quot;you&quot;.
(Sampson 1995, p. 115)
</rdfs:comment>
    </owl:Class>
    


    <!-- http://purl.org/olia/susa.owl#SubstitutiveThirdPersonPronoun -->

    <owl:Class rdf:about="http://purl.org/olia/susa.owl#SubstitutiveThirdPersonPronoun">
        <rdfs:subClassOf rdf:resource="http://purl.org/olia/susa.owl#SubstitutivePersonalPronoun"/>
        <rdfs:comment>These are third person personal pronouns. 
(Sampson 1995, p. 115)</rdfs:comment>
    </owl:Class>
    


    <!-- http://purl.org/olia/susa.owl#SubstitutiveWHPronoun -->

    <owl:Class rdf:about="http://purl.org/olia/susa.owl#SubstitutiveWHPronoun">
        <rdfs:subClassOf rdf:resource="http://purl.org/olia/susa.owl#SubstitutivePronoun"/>
        <rdfs:comment>SUSANNE tags which begin with PNQ... represent SubstitutiveWHPronouns. This class contains PNQV (&quot;whosever&quot;, &quot;whomever&quot;, &quot;whoever&quot;), SubstitutiveInterrogativePronoun and SubstitutiveRelativePronoun.</rdfs:comment>
    </owl:Class>
    


    <!-- http://purl.org/olia/susa.owl#Suffix -->

    <owl:Class rdf:about="http://purl.org/olia/susa.owl#Suffix">
        <rdfs:subClassOf rdf:resource="http://purl.org/olia/susa.owl#NonPOS"/>
        <rdfs:comment>FA is the SUSANNE tag used for a suffix which is seperated by a hyphen.
(Sampson 1995, p. 107)</rdfs:comment>
    </owl:Class>
    


    <!-- http://purl.org/olia/susa.owl#SuperlativeAdverb -->

    <owl:Class rdf:about="http://purl.org/olia/susa.owl#SuperlativeAdverb">
        <rdfs:subClassOf rdf:resource="http://purl.org/olia/susa.owl#GeneralAdverb"/>
        <rdfs:comment>This is a superlative adverb other than &quot;most&quot; and &quot;least&quot;. 
(Sampson 1995, p. 117)</rdfs:comment>
    </owl:Class>
    


    <!-- http://purl.org/olia/susa.owl#Tag -->

    <owl:Class rdf:about="http://purl.org/olia/susa.owl#Tag">
        <rdfs:subClassOf rdf:resource="http://purl.org/olia/system.owl#LinguisticAnnotation"/>
        <rdfs:subClassOf>
            <owl:Restriction>
                <owl:onProperty rdf:resource="http://purl.org/olia/system.owl#hasTier"/>
                <owl:hasValue>POS</owl:hasValue>
            </owl:Restriction>
        </rdfs:subClassOf>
        <rdfs:comment>SUSANNE TagSet (Sampson 1995) augmented with 
	English examples from the Susanne corpus and from &quot;Morphosyntactic 
	Phenomena Encoded in Lexicons and Corpora A Common Proposal and
	Applications to European Languages EAG---CLWG---MORPHSYN/R
	Version of 31st Aug, 1996&quot;
	(http://www.ilc.cnr.it/EAGLES96/morphsyn/)
	</rdfs:comment>
        <owl:versionInfo>
		The hierarchical structure is inferred from the
		structure of SUSANNE tags: Letters on the left tend
		to represent superconcepts, letters to the right define
		their subclassification. There are, however, some
		deviations to this rule, e.g., APPGf for &quot;her&quot; as 
		a determiner, where 
		the A is a prefix (&quot;attributive&quot;)
		attached to a tag of the PPG family (&quot;possessive
		pronoun&quot;)
	</owl:versionInfo>
    </owl:Class>
    


    <!-- http://purl.org/olia/susa.owl#TemporalAdverb -->

    <owl:Class rdf:about="http://purl.org/olia/susa.owl#TemporalAdverb">
        <rdfs:subClassOf rdf:resource="http://purl.org/olia/susa.owl#Adverb"/>
        <rdfs:comment>SUSANNE tags beginning with RT... are temporal adverbs.
(Sampson 1995, p.118)</rdfs:comment>
    </owl:Class>
    


    <!-- http://purl.org/olia/susa.owl#TemporalNoun -->

    <owl:Class rdf:about="http://purl.org/olia/susa.owl#TemporalNoun">
        <rdfs:subClassOf rdf:resource="http://purl.org/olia/susa.owl#CommonNoun"/>
        <rdfs:comment>These are nouns for time.
(Sampson 1995, p. 113)</rdfs:comment>
    </owl:Class>
    


    <!-- http://purl.org/olia/susa.owl#Tense -->

    <owl:Class rdf:about="http://purl.org/olia/susa.owl#Tense">
        <rdfs:subClassOf rdf:resource="http://purl.org/olia/system.owl#Feature"/>
    </owl:Class>
    


    <!-- http://purl.org/olia/susa.owl#Title -->

    <owl:Class rdf:about="http://purl.org/olia/susa.owl#Title">
        <rdfs:subClassOf rdf:resource="http://purl.org/olia/susa.owl#CommonNoun"/>
        <rdfs:comment>Common nouns of style and title. An S term is a status-indicating item which either accompanies one or more individual names within the full title of a person or is used to addres a person of appropriate status, or both. (Sampson 1995, p. 95, 112-113)</rdfs:comment>
    </owl:Class>
    


    <!-- http://purl.org/olia/susa.owl#TopographicalAdverb -->

    <owl:Class rdf:about="http://purl.org/olia/susa.owl#TopographicalAdverb">
        <rdfs:subClassOf rdf:resource="http://purl.org/olia/susa.owl#Adverb"/>
        <rdfs:comment>SUSANNE tags beginning with RL... represent adverbs of place or direction.
(Sampson 1995, p.116)</rdfs:comment>
    </owl:Class>
    


    <!-- http://purl.org/olia/susa.owl#TopographicalNoun -->

    <owl:Class rdf:about="http://purl.org/olia/susa.owl#TopographicalNoun">
        <rdfs:subClassOf rdf:resource="http://purl.org/olia/susa.owl#CommonNoun"/>
        <rdfs:comment>Common nouns where the meaning of the word is a topographical feature and the noun is used as the head word in a place-name.
(Sampson 1995, p. 94)</rdfs:comment>
    </owl:Class>
    


    <!-- http://purl.org/olia/susa.owl#Unique -->

    <owl:Class rdf:about="http://purl.org/olia/susa.owl#Unique">
        <rdfs:subClassOf rdf:resource="http://purl.org/olia/susa.owl#Tag"/>
        <rdfs:comment>Following the EAGLES recommendations, the Unique class subsumes different &apos;particles&apos;. 
	 These are  isolate forms, uninflectable, which have not been included anwhere else
	(see http://www.ilc.cnr.it/EAGLES96/morphsyn/node700.html#SECTION000153100000000000000 for a list). 
	Includes &quot;to&quot; (+ Infin.) (UI), negative &quot;not&quot;, &quot;n&apos;t&quot; (UN), and existential &quot;there&quot; (UX)
	</rdfs:comment>
    </owl:Class>
    


    <!-- http://purl.org/olia/susa.owl#UnitNoun -->

    <owl:Class rdf:about="http://purl.org/olia/susa.owl#UnitNoun">
        <rdfs:subClassOf rdf:resource="http://purl.org/olia/susa.owl#CommonNoun"/>
        <rdfs:comment>Unit nouns, i.e., units of measurement, wether written in full (&quot;inch&quot;, &quot;kilogramm&quot;) or abbreviated either alphabetically or symbolically, as head of a noun phrase denoting a measured quantity. (Sampson 1995, p. 97)</rdfs:comment>
    </owl:Class>
    


    <!-- http://purl.org/olia/susa.owl#Valency -->

    <owl:Class rdf:about="http://purl.org/olia/susa.owl#Valency">
        <rdfs:subClassOf rdf:resource="http://purl.org/olia/system.owl#Feature"/>
    </owl:Class>
    


    <!-- http://purl.org/olia/susa.owl#Verb -->

    <owl:Class rdf:about="http://purl.org/olia/susa.owl#Verb">
        <rdfs:subClassOf rdf:resource="http://purl.org/olia/susa.owl#Tag"/>
        <rdfs:comment>SUSANNE tags beginning with V... represent verbs.
	Note that the subclassification follows the following EAGLES recommendation:
	
	Since it is impractical, however, given the current capabilities of tagging software, 
	to resolve automatically the ambiguity of these six morphological functions, it is a 
	common practice to assign a single value to the base form, or else to assign two values, 
	one for the finite and one for the non-finite functions. Because of this, the tables below 
	show two tagsets: one tagset representing the 6 attribute-values above, and a reduced tagset 
	(`RTags&apos;), which resembles most tagsets so far used for the English language in reducing the 
	six values to two.
	http://www.ilc.cnr.it/EAGLES96/morphsyn/node150.html#SECTION00054000000000000000
	</rdfs:comment>
    </owl:Class>
    


    <!-- http://purl.org/olia/susa.owl#WHAdverb -->

    <owl:Class rdf:about="http://purl.org/olia/susa.owl#WHAdverb">
        <rdfs:subClassOf rdf:resource="http://purl.org/olia/susa.owl#GeneralAdverb"/>
        <rdfs:comment>SUSANNE tags beginning with RRQ represent interrogative or relative adverbs, e.g., &quot;where&quot;, &quot;how&quot;, &quot;when&quot;. 
(Sampson 1995, p. 117)</rdfs:comment>
    </owl:Class>
    


    <!-- http://purl.org/olia/susa.owl#WHDeterminer -->

    <owl:Class rdf:about="http://purl.org/olia/susa.owl#WHDeterminer">
        <rdfs:subClassOf rdf:resource="http://purl.org/olia/susa.owl#Determiner"/>
        <rdfs:comment>These are interrogative or relative pronouns in attributive use.
(Sampson 1995, p. 107)</rdfs:comment>
    </owl:Class>
    


    <!-- http://purl.org/olia/system.owl#Feature -->

    <owl:Class rdf:about="http://purl.org/olia/system.owl#Feature"/>
    


    <!-- http://purl.org/olia/system.owl#LinguisticAnnotation -->

    <owl:Class rdf:about="http://purl.org/olia/system.owl#LinguisticAnnotation"/>
    


    <!-- 
    ///////////////////////////////////////////////////////////////////////////////////////
    //
    // Individuals
    //
    ///////////////////////////////////////////////////////////////////////////////////////
     -->

    


    <!-- http://purl.org/olia/susa.owl#APPG -->

    <owl:NamedIndividual rdf:about="http://purl.org/olia/susa.owl#APPG">
        <rdf:type rdf:resource="http://purl.org/olia/susa.owl#AttributivePossessivePronoun"/>
        <hasCase rdf:resource="http://purl.org/olia/susa.owl#genitive"/>
        <olia_system:hasTag>APPG</olia_system:hasTag>
        <olia_system:hasTier>POS</olia_system:hasTier>
        <rdfs:comment>APPG is used for attributive possessive pronouns.</rdfs:comment>
    </owl:NamedIndividual>
    


    <!-- http://purl.org/olia/susa.owl#APPGf -->

    <owl:NamedIndividual rdf:about="http://purl.org/olia/susa.owl#APPGf">
        <rdf:type rdf:resource="http://purl.org/olia/susa.owl#AttributivePossessivePronoun"/>
        <hasCase rdf:resource="http://purl.org/olia/susa.owl#genitive"/>
        <hasGender rdf:resource="http://purl.org/olia/susa.owl#feminine"/>
        <hasNumber rdf:resource="http://purl.org/olia/susa.owl#singular"/>
        <hasPerson rdf:resource="http://purl.org/olia/susa.owl#third"/>
        <olia_system:hasTag>APPGf</olia_system:hasTag>
        <olia_system:hasTier>POS</olia_system:hasTier>
        <rdfs:comment>APPGf is used for &quot;her&quot; as possessive.</rdfs:comment>
    </owl:NamedIndividual>
    


    <!-- http://purl.org/olia/susa.owl#APPGh1 -->

    <owl:NamedIndividual rdf:about="http://purl.org/olia/susa.owl#APPGh1">
        <rdf:type rdf:resource="http://purl.org/olia/susa.owl#AttributivePossessivePronoun"/>
        <hasCase rdf:resource="http://purl.org/olia/susa.owl#genitive"/>
        <hasGender rdf:resource="http://purl.org/olia/susa.owl#neutral"/>
        <hasNumber rdf:resource="http://purl.org/olia/susa.owl#singular"/>
        <hasPerson rdf:resource="http://purl.org/olia/susa.owl#third"/>
        <olia_system:hasTag>APPGh1</olia_system:hasTag>
        <olia_system:hasTier>POS</olia_system:hasTier>
        <rdfs:comment>APPGh1 is the tag for &quot;its&quot;.</rdfs:comment>
    </owl:NamedIndividual>
    


    <!-- http://purl.org/olia/susa.owl#APPGh2 -->

    <owl:NamedIndividual rdf:about="http://purl.org/olia/susa.owl#APPGh2">
        <rdf:type rdf:resource="http://purl.org/olia/susa.owl#AttributivePossessivePronoun"/>
        <hasCase rdf:resource="http://purl.org/olia/susa.owl#genitive"/>
        <hasNumber rdf:resource="http://purl.org/olia/susa.owl#plural"/>
        <hasPerson rdf:resource="http://purl.org/olia/susa.owl#third"/>
        <olia_system:hasTag>APPGh2</olia_system:hasTag>
        <olia_system:hasTier>POS</olia_system:hasTier>
        <rdfs:comment>APPGh2 for &quot;their&quot;.</rdfs:comment>
    </owl:NamedIndividual>
    


    <!-- http://purl.org/olia/susa.owl#APPGi1 -->

    <owl:NamedIndividual rdf:about="http://purl.org/olia/susa.owl#APPGi1">
        <rdf:type rdf:resource="http://purl.org/olia/susa.owl#AttributivePossessivePronoun"/>
        <hasCase rdf:resource="http://purl.org/olia/susa.owl#genitive"/>
        <hasNumber rdf:resource="http://purl.org/olia/susa.owl#singular"/>
        <hasPerson rdf:resource="http://purl.org/olia/susa.owl#first"/>
        <olia_system:hasTag>APPGi1</olia_system:hasTag>
        <olia_system:hasTier>POS</olia_system:hasTier>
        <rdfs:comment>APPGi1 is the tag for &quot;my&quot; as possessive.</rdfs:comment>
    </owl:NamedIndividual>
    


    <!-- http://purl.org/olia/susa.owl#APPGi2 -->

    <owl:NamedIndividual rdf:about="http://purl.org/olia/susa.owl#APPGi2">
        <rdf:type rdf:resource="http://purl.org/olia/susa.owl#AttributivePossessivePronoun"/>
        <hasCase rdf:resource="http://purl.org/olia/susa.owl#genitive"/>
        <hasNumber rdf:resource="http://purl.org/olia/susa.owl#plural"/>
        <hasPerson rdf:resource="http://purl.org/olia/susa.owl#first"/>
        <olia_system:hasTag>APPGi2</olia_system:hasTag>
        <olia_system:hasTier>POS</olia_system:hasTier>
        <rdfs:comment>APPGi2 is used for &quot;our&quot;.</rdfs:comment>
    </owl:NamedIndividual>
    


    <!-- http://purl.org/olia/susa.owl#APPGm -->

    <owl:NamedIndividual rdf:about="http://purl.org/olia/susa.owl#APPGm">
        <rdf:type rdf:resource="http://purl.org/olia/susa.owl#AttributivePossessivePronoun"/>
        <hasCase rdf:resource="http://purl.org/olia/susa.owl#genitive"/>
        <hasGender rdf:resource="http://purl.org/olia/susa.owl#masculine"/>
        <hasNumber rdf:resource="http://purl.org/olia/susa.owl#singular"/>
        <hasPerson rdf:resource="http://purl.org/olia/susa.owl#third"/>
        <olia_system:hasTag>APPGm</olia_system:hasTag>
        <olia_system:hasTier>POS</olia_system:hasTier>
        <rdfs:comment>APPGm is used for &quot;his&quot; except as pronoun.</rdfs:comment>
    </owl:NamedIndividual>
    


    <!-- http://purl.org/olia/susa.owl#APPGy -->

    <owl:NamedIndividual rdf:about="http://purl.org/olia/susa.owl#APPGy">
        <rdf:type rdf:resource="http://purl.org/olia/susa.owl#AttributivePossessivePronoun"/>
        <hasCase rdf:resource="http://purl.org/olia/susa.owl#genitive"/>
        <hasPerson rdf:resource="http://purl.org/olia/susa.owl#second"/>
        <olia_system:hasTag>APPGy</olia_system:hasTag>
        <olia_system:hasTier>POS</olia_system:hasTier>
        <rdfs:comment>APPGy is used for &quot;your&quot;.</rdfs:comment>
    </owl:NamedIndividual>
    


    <!-- http://purl.org/olia/susa.owl#AT -->

    <owl:NamedIndividual rdf:about="http://purl.org/olia/susa.owl#AT">
        <rdf:type rdf:resource="http://purl.org/olia/susa.owl#DefiniteArticle"/>
        <olia_system:hasTag>AT</olia_system:hasTag>
        <olia_system:hasTier>POS</olia_system:hasTier>
        <rdfs:comment>The SUSANNE tag AT is used for &quot;the&quot;.</rdfs:comment>
    </owl:NamedIndividual>
    


    <!-- http://purl.org/olia/susa.owl#AT1 -->

    <owl:NamedIndividual rdf:about="http://purl.org/olia/susa.owl#AT1">
        <rdf:type rdf:resource="http://purl.org/olia/susa.owl#IndefiniteArticle"/>
        <olia_system:hasTag>AT1</olia_system:hasTag>
        <olia_system:hasTier>POS</olia_system:hasTier>
        <rdfs:comment>AT1 is used for the indefinite article &quot;a&quot;, &quot;an&quot;.</rdfs:comment>
    </owl:NamedIndividual>
    


    <!-- http://purl.org/olia/susa.owl#AT1e -->

    <owl:NamedIndividual rdf:about="http://purl.org/olia/susa.owl#AT1e">
        <rdf:type rdf:resource="http://purl.org/olia/susa.owl#Every"/>
        <olia_system:hasTag>AT1e</olia_system:hasTag>
        <olia_system:hasTier>POS</olia_system:hasTier>
        <rdfs:comment>AT1e is used for &quot;every&quot;.</rdfs:comment>
    </owl:NamedIndividual>
    


    <!-- http://purl.org/olia/susa.owl#ATn -->

    <owl:NamedIndividual rdf:about="http://purl.org/olia/susa.owl#ATn">
        <rdf:type rdf:resource="http://purl.org/olia/susa.owl#NegativeDeterminer"/>
        <olia_system:hasTag>ATn</olia_system:hasTag>
        <olia_system:hasTier>POS</olia_system:hasTier>
        <rdfs:comment>ATn stands for &quot;no&quot; as determiner or qualifier.</rdfs:comment>
    </owl:NamedIndividual>
    


    <!-- http://purl.org/olia/susa.owl#BTO -->

    <owl:NamedIndividual rdf:about="http://purl.org/olia/susa.owl#BTO">
        <rdf:type rdf:resource="http://purl.org/olia/susa.owl#SubordinatingConjunctionWithInfinitival"/>
        <olia_system:hasTag>BTO</olia_system:hasTag>
        <olia_system:hasTier>POS</olia_system:hasTier>
        <rdfs:comment>BTO stands for &quot; in order&quot; and occurs within a infinitival clause as a left sister of an infinitival verb/ verb group. 
(Sampson 1995, p.105, 268)</rdfs:comment>
    </owl:NamedIndividual>
    


    <!-- http://purl.org/olia/susa.owl#CC -->

    <owl:NamedIndividual rdf:about="http://purl.org/olia/susa.owl#CC">
        <rdf:type rdf:resource="http://purl.org/olia/susa.owl#CoordinatingConjunction"/>
        <olia_system:hasTag>CC</olia_system:hasTag>
        <olia_system:hasTier>POS</olia_system:hasTier>
        <rdfs:comment>CC is used for coordinating conjunctions &quot;and&quot;, &quot;and/or&quot;, &quot;as well as&quot;, &quot;plus&quot;</rdfs:comment>
    </owl:NamedIndividual>
    


    <!-- http://purl.org/olia/susa.owl#CCB -->

    <owl:NamedIndividual rdf:about="http://purl.org/olia/susa.owl#CCB">
        <rdf:type rdf:resource="http://purl.org/olia/susa.owl#CoordinatingConjunction"/>
        <olia_system:hasTag>CCB</olia_system:hasTag>
        <olia_system:hasTier>POS</olia_system:hasTier>
        <rdfs:comment>CCB is used for &quot;but&quot; as coordinating conjunction.</rdfs:comment>
    </owl:NamedIndividual>
    


    <!-- http://purl.org/olia/susa.owl#CCn -->

    <owl:NamedIndividual rdf:about="http://purl.org/olia/susa.owl#CCn">
        <rdf:type rdf:resource="http://purl.org/olia/susa.owl#CoordinatingConjunction"/>
        <olia_system:hasTag>CCn</olia_system:hasTag>
        <olia_system:hasTier>POS</olia_system:hasTier>
        <rdfs:comment>CCn is used for &quot;nor&quot;.</rdfs:comment>
    </owl:NamedIndividual>
    


    <!-- http://purl.org/olia/susa.owl#CCr -->

    <owl:NamedIndividual rdf:about="http://purl.org/olia/susa.owl#CCr">
        <rdf:type rdf:resource="http://purl.org/olia/susa.owl#CoordinatingConjunction"/>
        <olia_system:hasTag>CCr</olia_system:hasTag>
        <olia_system:hasTier>POS</olia_system:hasTier>
        <rdfs:comment>CCr is the tag for &quot;or&quot;.</rdfs:comment>
    </owl:NamedIndividual>
    


    <!-- http://purl.org/olia/susa.owl#CS -->

    <owl:NamedIndividual rdf:about="http://purl.org/olia/susa.owl#CS">
        <rdf:type rdf:resource="http://purl.org/olia/susa.owl#ProperSubordinatingConjunction"/>
        <olia_system:hasTag>CS</olia_system:hasTag>
        <olia_system:hasTier>POS</olia_system:hasTier>
        <rdfs:comment>These are subordinating conjunctions.</rdfs:comment>
    </owl:NamedIndividual>
    


    <!-- http://purl.org/olia/susa.owl#CSA -->

    <owl:NamedIndividual rdf:about="http://purl.org/olia/susa.owl#CSA">
        <rdf:type rdf:resource="http://purl.org/olia/susa.owl#ProperSubordinatingConjunction"/>
        <olia_system:hasTag>CSA</olia_system:hasTag>
        <olia_system:hasTier>POS</olia_system:hasTier>
        <rdfs:comment>CSA is the SUSANNE tag for &quot;as&quot; as subordinating conjunction or as preposition in comparative sense.</rdfs:comment>
    </owl:NamedIndividual>
    


    <!-- http://purl.org/olia/susa.owl#CSN -->

    <owl:NamedIndividual rdf:about="http://purl.org/olia/susa.owl#CSN">
        <rdf:type rdf:resource="http://purl.org/olia/susa.owl#ProperSubordinatingConjunction"/>
        <olia_system:hasTag>CSN</olia_system:hasTag>
        <olia_system:hasTier>POS</olia_system:hasTier>
        <rdfs:comment>CSN is used for &quot;than&quot; in all uses.</rdfs:comment>
    </owl:NamedIndividual>
    


    <!-- http://purl.org/olia/susa.owl#CST -->

    <owl:NamedIndividual rdf:about="http://purl.org/olia/susa.owl#CST">
        <rdf:type rdf:resource="http://purl.org/olia/susa.owl#ProperSubordinatingConjunction"/>
        <olia_system:hasTag>CST</olia_system:hasTag>
        <olia_system:hasTier>POS</olia_system:hasTier>
        <rdfs:comment>CST is the tag for &quot;that&quot; as subordinating conjunction, including in its use in introducing relative clauses.</rdfs:comment>
    </owl:NamedIndividual>
    


    <!-- http://purl.org/olia/susa.owl#CSW -->

    <owl:NamedIndividual rdf:about="http://purl.org/olia/susa.owl#CSW">
        <rdf:type rdf:resource="http://purl.org/olia/susa.owl#ProperSubordinatingConjunction"/>
        <olia_system:hasTag>CSW</olia_system:hasTag>
        <olia_system:hasTier>POS</olia_system:hasTier>
        <rdfs:comment>CSW  is used for &quot;whether&quot; in all uses.</rdfs:comment>
    </owl:NamedIndividual>
    


    <!-- http://purl.org/olia/susa.owl#CSf -->

    <owl:NamedIndividual rdf:about="http://purl.org/olia/susa.owl#CSf">
        <rdf:type rdf:resource="http://purl.org/olia/susa.owl#ProperSubordinatingConjunction"/>
        <olia_system:hasTag>CSf</olia_system:hasTag>
        <olia_system:hasTier>POS</olia_system:hasTier>
        <rdfs:comment>CSf is used for &quot;for&quot; as conjunction.</rdfs:comment>
    </owl:NamedIndividual>
    


    <!-- http://purl.org/olia/susa.owl#CSg -->

    <owl:NamedIndividual rdf:about="http://purl.org/olia/susa.owl#CSg">
        <rdf:type rdf:resource="http://purl.org/olia/susa.owl#ProperSubordinatingConjunction"/>
        <olia_system:hasTag>CSg</olia_system:hasTag>
        <olia_system:hasTier>POS</olia_system:hasTier>
        <rdfs:comment>CSg is used for &quot;though&quot; as subordinating conjunction.</rdfs:comment>
    </owl:NamedIndividual>
    


    <!-- http://purl.org/olia/susa.owl#CSi -->

    <owl:NamedIndividual rdf:about="http://purl.org/olia/susa.owl#CSi">
        <rdf:type rdf:resource="http://purl.org/olia/susa.owl#ProperSubordinatingConjunction"/>
        <olia_system:hasTag>CSi</olia_system:hasTag>
        <olia_system:hasTier>POS</olia_system:hasTier>
        <rdfs:comment>CSi is used for &quot;if&quot;.</rdfs:comment>
    </owl:NamedIndividual>
    


    <!-- http://purl.org/olia/susa.owl#CSk -->

    <owl:NamedIndividual rdf:about="http://purl.org/olia/susa.owl#CSk">
        <rdf:type rdf:resource="http://purl.org/olia/susa.owl#ProperSubordinatingConjunction"/>
        <olia_system:hasTag>CSk</olia_system:hasTag>
        <olia_system:hasTier>POS</olia_system:hasTier>
        <rdfs:comment>CSk is used for &quot;as if&quot;, &quot;as though&quot;.</rdfs:comment>
    </owl:NamedIndividual>
    


    <!-- http://purl.org/olia/susa.owl#CSn -->

    <owl:NamedIndividual rdf:about="http://purl.org/olia/susa.owl#CSn">
        <rdf:type rdf:resource="http://purl.org/olia/susa.owl#ProperSubordinatingConjunction"/>
        <olia_system:hasTag>CSn</olia_system:hasTag>
        <olia_system:hasTier>POS</olia_system:hasTier>
        <rdfs:comment>CSn is used for &quot;when&quot; as subordinating conjunction.</rdfs:comment>
    </owl:NamedIndividual>
    


    <!-- http://purl.org/olia/susa.owl#CSr -->

    <owl:NamedIndividual rdf:about="http://purl.org/olia/susa.owl#CSr">
        <rdf:type rdf:resource="http://purl.org/olia/susa.owl#ProperSubordinatingConjunction"/>
        <olia_system:hasTag>CSr</olia_system:hasTag>
        <olia_system:hasTier>POS</olia_system:hasTier>
        <rdfs:comment>CSr is used for &quot;where&quot; as subordinating conjunction.</rdfs:comment>
    </owl:NamedIndividual>
    


    <!-- http://purl.org/olia/susa.owl#DA -->

    <owl:NamedIndividual rdf:about="http://purl.org/olia/susa.owl#DA">
        <rdf:type rdf:resource="http://purl.org/olia/susa.owl#Quantifier"/>
        <olia_system:hasTag>DA</olia_system:hasTag>
        <olia_system:hasTier>POS</olia_system:hasTier>
        <rdfs:comment>DA is used for quantifiers.</rdfs:comment>
    </owl:NamedIndividual>
    


    <!-- http://purl.org/olia/susa.owl#DA1 -->

    <owl:NamedIndividual rdf:about="http://purl.org/olia/susa.owl#DA1">
        <rdf:type rdf:resource="http://purl.org/olia/susa.owl#Quantifier"/>
        <olia_system:hasTag>DA1</olia_system:hasTag>
        <olia_system:hasTier>POS</olia_system:hasTier>
        <rdfs:comment>DA1 is used for &quot;much&quot;, &quot;little&quot;.</rdfs:comment>
    </owl:NamedIndividual>
    


    <!-- http://purl.org/olia/susa.owl#DA2 -->

    <owl:NamedIndividual rdf:about="http://purl.org/olia/susa.owl#DA2">
        <rdf:type rdf:resource="http://purl.org/olia/susa.owl#Quantifier"/>
        <olia_system:hasTag>DA2</olia_system:hasTag>
        <olia_system:hasTier>POS</olia_system:hasTier>
        <rdfs:comment>DA2 is the SUSANNE tag used for &quot;few&quot; and &quot;many&quot;.</rdfs:comment>
    </owl:NamedIndividual>
    


    <!-- http://purl.org/olia/susa.owl#DA2R -->

    <owl:NamedIndividual rdf:about="http://purl.org/olia/susa.owl#DA2R">
        <rdf:type rdf:resource="http://purl.org/olia/susa.owl#Quantifier"/>
        <olia_system:hasTag>DA2R</olia_system:hasTag>
        <olia_system:hasTier>POS</olia_system:hasTier>
        <rdfs:comment>DA2R is the SUSANNE tag used for &quot;fewer&quot;.</rdfs:comment>
    </owl:NamedIndividual>
    


    <!-- http://purl.org/olia/susa.owl#DA2T -->

    <owl:NamedIndividual rdf:about="http://purl.org/olia/susa.owl#DA2T">
        <rdf:type rdf:resource="http://purl.org/olia/susa.owl#Quantifier"/>
        <olia_system:hasTag>DA2T</olia_system:hasTag>
        <olia_system:hasTier>POS</olia_system:hasTier>
        <rdfs:comment>DA2T is used for &quot;fewest&quot;.</rdfs:comment>
    </owl:NamedIndividual>
    


    <!-- http://purl.org/olia/susa.owl#DA2q -->

    <owl:NamedIndividual rdf:about="http://purl.org/olia/susa.owl#DA2q">
        <rdf:type rdf:resource="http://purl.org/olia/susa.owl#Quantifier"/>
        <olia_system:hasTag>DA2q</olia_system:hasTag>
        <olia_system:hasTier>POS</olia_system:hasTier>
        <rdfs:comment>DA2q is used for &quot;several&quot;.</rdfs:comment>
    </owl:NamedIndividual>
    


    <!-- http://purl.org/olia/susa.owl#DAR -->

    <owl:NamedIndividual rdf:about="http://purl.org/olia/susa.owl#DAR">
        <rdf:type rdf:resource="http://purl.org/olia/susa.owl#Quantifier"/>
        <olia_system:hasTag>DAR</olia_system:hasTag>
        <olia_system:hasTier>POS</olia_system:hasTier>
        <rdfs:comment>DAR is used for &quot;less&quot; or &quot;more&quot;.</rdfs:comment>
    </owl:NamedIndividual>
    


    <!-- http://purl.org/olia/susa.owl#DAT -->

    <owl:NamedIndividual rdf:about="http://purl.org/olia/susa.owl#DAT">
        <rdf:type rdf:resource="http://purl.org/olia/susa.owl#Quantifier"/>
        <olia_system:hasTag>DAT</olia_system:hasTag>
        <olia_system:hasTier>POS</olia_system:hasTier>
        <rdfs:comment>DAT is used for &quot;least&quot; and &quot;most&quot; in all uses.</rdfs:comment>
    </owl:NamedIndividual>
    


    <!-- http://purl.org/olia/susa.owl#DAg -->

    <owl:NamedIndividual rdf:about="http://purl.org/olia/susa.owl#DAg">
        <rdf:type rdf:resource="http://purl.org/olia/susa.owl#Quantifier"/>
        <olia_system:hasTag>DAg</olia_system:hasTag>
        <olia_system:hasTier>POS</olia_system:hasTier>
        <rdfs:comment>DAg is used for &quot;own&quot; as part of a genitive construction.</rdfs:comment>
    </owl:NamedIndividual>
    


    <!-- http://purl.org/olia/susa.owl#DAr -->

    <owl:NamedIndividual rdf:about="http://purl.org/olia/susa.owl#DAr">
        <rdf:type rdf:resource="http://purl.org/olia/susa.owl#Quantifier"/>
        <olia_system:hasTag>DAr</olia_system:hasTag>
        <olia_system:hasTier>POS</olia_system:hasTier>
        <rdfs:comment>DAr is used for &quot;former&quot;/ &quot; latter&quot; in all uses.</rdfs:comment>
    </owl:NamedIndividual>
    


    <!-- http://purl.org/olia/susa.owl#DAy -->

    <owl:NamedIndividual rdf:about="http://purl.org/olia/susa.owl#DAy">
        <rdf:type rdf:resource="http://purl.org/olia/susa.owl#Quantifier"/>
        <olia_system:hasTag>DAy</olia_system:hasTag>
        <olia_system:hasTier>POS</olia_system:hasTier>
        <rdfs:comment>DAy is the tag for &quot;same&quot; / &quot;selfsame&quot;.</rdfs:comment>
    </owl:NamedIndividual>
    


    <!-- http://purl.org/olia/susa.owl#DAz -->

    <owl:NamedIndividual rdf:about="http://purl.org/olia/susa.owl#DAz">
        <rdf:type rdf:resource="http://purl.org/olia/susa.owl#Quantifier"/>
        <olia_system:hasTag>DAz</olia_system:hasTag>
        <olia_system:hasTier>POS</olia_system:hasTier>
        <rdfs:comment>DAz is used for &quot;such&quot;.</rdfs:comment>
    </owl:NamedIndividual>
    


    <!-- http://purl.org/olia/susa.owl#DB -->

    <owl:NamedIndividual rdf:about="http://purl.org/olia/susa.owl#DB">
        <rdf:type rdf:resource="http://purl.org/olia/susa.owl#QuantifyingPronoun"/>
        <olia_system:hasTag>DB</olia_system:hasTag>
        <olia_system:hasTier>POS</olia_system:hasTier>
        <rdfs:comment>DB is used for &quot;all&quot;, &quot;both&quot; or &quot;half&quot; as pronoun or determiner.</rdfs:comment>
    </owl:NamedIndividual>
    


    <!-- http://purl.org/olia/susa.owl#DB2 -->

    <owl:NamedIndividual rdf:about="http://purl.org/olia/susa.owl#DB2">
        <rdf:type rdf:resource="http://purl.org/olia/susa.owl#QuantifyingPronoun"/>
        <olia_system:hasTag>DB2</olia_system:hasTag>
        <olia_system:hasTier>POS</olia_system:hasTier>
        <rdfs:comment>DB2 is used for &quot;both&quot; as determiner or pronoun.</rdfs:comment>
    </owl:NamedIndividual>
    


    <!-- http://purl.org/olia/susa.owl#DBa -->

    <owl:NamedIndividual rdf:about="http://purl.org/olia/susa.owl#DBa">
        <rdf:type rdf:resource="http://purl.org/olia/susa.owl#QuantifyingPronoun"/>
        <olia_system:hasTag>DBa</olia_system:hasTag>
        <olia_system:hasTier>POS</olia_system:hasTier>
        <rdfs:comment>DBa is used for &quot;all&quot; as determiner or pronoun.</rdfs:comment>
    </owl:NamedIndividual>
    


    <!-- http://purl.org/olia/susa.owl#DBh -->

    <owl:NamedIndividual rdf:about="http://purl.org/olia/susa.owl#DBh">
        <rdf:type rdf:resource="http://purl.org/olia/susa.owl#QuantifyingPronoun"/>
        <olia_system:hasTag>DBh</olia_system:hasTag>
        <olia_system:hasTier>POS</olia_system:hasTier>
        <rdfs:comment>DBh is used for &quot;half&quot; as determiner or pronoun.</rdfs:comment>
    </owl:NamedIndividual>
    


    <!-- http://purl.org/olia/susa.owl#DD -->

    <owl:NamedIndividual rdf:about="http://purl.org/olia/susa.owl#DD">
        <rdf:type rdf:resource="http://purl.org/olia/susa.owl#Determiner"/>
        <olia_system:hasTag>DD</olia_system:hasTag>
        <olia_system:hasTier>POS</olia_system:hasTier>
        <rdfs:comment>DD is used for &quot;yon&quot;, &quot;yonder&quot; as determiner, &quot;somesuch&quot;, &quot;the rest&quot;.</rdfs:comment>
    </owl:NamedIndividual>
    


    <!-- http://purl.org/olia/susa.owl#DD1 -->

    <owl:NamedIndividual rdf:about="http://purl.org/olia/susa.owl#DD1">
        <rdf:type rdf:resource="http://purl.org/olia/susa.owl#Determiner"/>
        <olia_system:hasTag>DD1</olia_system:hasTag>
        <olia_system:hasTier>POS</olia_system:hasTier>
        <rdfs:comment>DD1 is used for determiner in singular.</rdfs:comment>
        <owl:versionInfo>added by Johannes Bubenzer (2006-09-09) in accordance to a
	TnT-tagged data set provided by SFB 538 (Hamburg), project K4</owl:versionInfo>
    </owl:NamedIndividual>
    


    <!-- http://purl.org/olia/susa.owl#DD1a -->

    <owl:NamedIndividual rdf:about="http://purl.org/olia/susa.owl#DD1a">
        <rdf:type rdf:resource="http://purl.org/olia/susa.owl#Determiner"/>
        <olia_system:hasTag>DD1a</olia_system:hasTag>
        <olia_system:hasTier>POS</olia_system:hasTier>
        <rdfs:comment>DD1a is used for &quot;that&quot; as determiner, demonstrative pronoun, or qualifier (e.g. that slowly).</rdfs:comment>
    </owl:NamedIndividual>
    


    <!-- http://purl.org/olia/susa.owl#DD1b -->

    <owl:NamedIndividual rdf:about="http://purl.org/olia/susa.owl#DD1b">
        <rdf:type rdf:resource="http://purl.org/olia/susa.owl#Quantifier"/>
        <olia_system:hasTag>DD1b</olia_system:hasTag>
        <olia_system:hasTier>POS</olia_system:hasTier>
        <rdfs:comment>DD1b is used for &quot;a bit&quot;.</rdfs:comment>
    </owl:NamedIndividual>
    


    <!-- http://purl.org/olia/susa.owl#DD1e -->

    <owl:NamedIndividual rdf:about="http://purl.org/olia/susa.owl#DD1e">
        <rdf:type rdf:resource="http://purl.org/olia/susa.owl#Quantifier"/>
        <olia_system:hasTag>DD1e</olia_system:hasTag>
        <olia_system:hasTier>POS</olia_system:hasTier>
        <rdfs:comment>DD1e is used for &quot;either&quot; as determiner or pronoun.</rdfs:comment>
    </owl:NamedIndividual>
    


    <!-- http://purl.org/olia/susa.owl#DD1i -->

    <owl:NamedIndividual rdf:about="http://purl.org/olia/susa.owl#DD1i">
        <rdf:type rdf:resource="http://purl.org/olia/susa.owl#Demonstrative"/>
        <olia_system:hasTag>DD1i</olia_system:hasTag>
        <olia_system:hasTier>POS</olia_system:hasTier>
        <rdfs:comment>DD1i is used for &quot;this&quot; in al uses including as qualifier.</rdfs:comment>
    </owl:NamedIndividual>
    


    <!-- http://purl.org/olia/susa.owl#DD1n -->

    <owl:NamedIndividual rdf:about="http://purl.org/olia/susa.owl#DD1n">
        <rdf:type rdf:resource="http://purl.org/olia/susa.owl#Quantifier"/>
        <olia_system:hasTag>DD1n</olia_system:hasTag>
        <olia_system:hasTier>POS</olia_system:hasTier>
        <rdfs:comment>DD1n is used for &quot;neither&quot; as determiner or pronoun.</rdfs:comment>
    </owl:NamedIndividual>
    


    <!-- http://purl.org/olia/susa.owl#DD1q -->

    <owl:NamedIndividual rdf:about="http://purl.org/olia/susa.owl#DD1q">
        <rdf:type rdf:resource="http://purl.org/olia/susa.owl#Quantifier"/>
        <olia_system:hasTag>DD1q</olia_system:hasTag>
        <olia_system:hasTier>POS</olia_system:hasTier>
        <rdfs:comment>DD1q is used for &quot;another&quot;, &quot;each&quot;, &quot;one and the same&quot; as determiner or pronoun.</rdfs:comment>
    </owl:NamedIndividual>
    


    <!-- http://purl.org/olia/susa.owl#DD1t -->

    <owl:NamedIndividual rdf:about="http://purl.org/olia/susa.owl#DD1t">
        <rdf:type rdf:resource="http://purl.org/olia/susa.owl#Determiner"/>
        <olia_system:hasTag>DD1t</olia_system:hasTag>
        <olia_system:hasTier>POS</olia_system:hasTier>
        <rdfs:comment>DD1t is used for &quot;a little&quot;.</rdfs:comment>
    </owl:NamedIndividual>
    


    <!-- http://purl.org/olia/susa.owl#DD2 -->

    <owl:NamedIndividual rdf:about="http://purl.org/olia/susa.owl#DD2">
        <rdf:type rdf:resource="http://purl.org/olia/susa.owl#Quantifier"/>
        <olia_system:hasTag>DD2</olia_system:hasTag>
        <olia_system:hasTier>POS</olia_system:hasTier>
        <rdfs:comment>DD2 is used for &quot;a few&quot;, &quot;a good few&quot;, &quot;a good many&quot;, &quot;a good great&quot;.</rdfs:comment>
    </owl:NamedIndividual>
    


    <!-- http://purl.org/olia/susa.owl#DD2a -->

    <owl:NamedIndividual rdf:about="http://purl.org/olia/susa.owl#DD2a">
        <rdf:type rdf:resource="http://purl.org/olia/susa.owl#Demonstrative"/>
        <olia_system:hasTag>DD2a</olia_system:hasTag>
        <olia_system:hasTier>POS</olia_system:hasTier>
        <rdfs:comment>DD2a is used for &quot;those&quot;.</rdfs:comment>
    </owl:NamedIndividual>
    


    <!-- http://purl.org/olia/susa.owl#DD2i -->

    <owl:NamedIndividual rdf:about="http://purl.org/olia/susa.owl#DD2i">
        <rdf:type rdf:resource="http://purl.org/olia/susa.owl#Demonstrative"/>
        <olia_system:hasTag>DD2i</olia_system:hasTag>
        <olia_system:hasTier>POS</olia_system:hasTier>
        <rdfs:comment>DD2i is used for &quot;these&quot;.</rdfs:comment>
    </owl:NamedIndividual>
    


    <!-- http://purl.org/olia/susa.owl#DDQ -->

    <owl:NamedIndividual rdf:about="http://purl.org/olia/susa.owl#DDQ">
        <rdf:type rdf:resource="http://purl.org/olia/susa.owl#WHDeterminer"/>
        <olia_system:hasTag>DDQ</olia_system:hasTag>
        <olia_system:hasTier>POS</olia_system:hasTier>
        <rdfs:comment>DDQ is the SUSANNE tag used for &quot;what&quot;.</rdfs:comment>
    </owl:NamedIndividual>
    


    <!-- http://purl.org/olia/susa.owl#DDQG -->

    <owl:NamedIndividual rdf:about="http://purl.org/olia/susa.owl#DDQG">
        <rdf:type rdf:resource="http://purl.org/olia/susa.owl#WHDeterminer"/>
        <hasCase rdf:resource="http://purl.org/olia/susa.owl#genitive"/>
        <olia_system:hasTag>DDQG</olia_system:hasTag>
        <olia_system:hasTier>POS</olia_system:hasTier>
        <rdfs:comment>&quot;Whose&quot; without a specification of its use.</rdfs:comment>
    </owl:NamedIndividual>
    


    <!-- http://purl.org/olia/susa.owl#DDQGq -->

    <owl:NamedIndividual rdf:about="http://purl.org/olia/susa.owl#DDQGq">
        <rdf:type rdf:resource="http://purl.org/olia/susa.owl#WHDeterminer"/>
        <hasCase rdf:resource="http://purl.org/olia/susa.owl#genitive"/>
        <olia_system:hasTag>DDQGq</olia_system:hasTag>
        <olia_system:hasTier>POS</olia_system:hasTier>
        <rdfs:comment>DDQGq is the tag for &quot;whose&quot; in interrogative uses.</rdfs:comment>
    </owl:NamedIndividual>
    


    <!-- http://purl.org/olia/susa.owl#DDQGr -->

    <owl:NamedIndividual rdf:about="http://purl.org/olia/susa.owl#DDQGr">
        <rdf:type rdf:resource="http://purl.org/olia/susa.owl#WHDeterminer"/>
        <hasCase rdf:resource="http://purl.org/olia/susa.owl#genitive"/>
        <olia_system:hasTag>DDQGr</olia_system:hasTag>
        <olia_system:hasTier>POS</olia_system:hasTier>
        <rdfs:comment>DDQGr for &quot;whose&quot; in relative uses.</rdfs:comment>
    </owl:NamedIndividual>
    


    <!-- http://purl.org/olia/susa.owl#DDQV -->

    <owl:NamedIndividual rdf:about="http://purl.org/olia/susa.owl#DDQV">
        <rdf:type rdf:resource="http://purl.org/olia/susa.owl#WHDeterminer"/>
        <olia_system:hasTag>DDQV</olia_system:hasTag>
        <olia_system:hasTier>POS</olia_system:hasTier>
        <rdfs:comment>The SUSANNE tag DDQV describes e.g. &quot;whatever&quot;, &quot;whichever&quot;, &quot;whichsever&quot;, &quot;no matter which&quot;.</rdfs:comment>
    </owl:NamedIndividual>
    


    <!-- http://purl.org/olia/susa.owl#DDQq -->

    <owl:NamedIndividual rdf:about="http://purl.org/olia/susa.owl#DDQq">
        <rdf:type rdf:resource="http://purl.org/olia/susa.owl#WHDeterminer"/>
        <olia_system:hasTag>RAh</olia_system:hasTag>
        <olia_system:hasTier>POS</olia_system:hasTier>
        <rdfs:comment>DDQq for &quot;which&quot; in interrogative uses.</rdfs:comment>
    </owl:NamedIndividual>
    


    <!-- http://purl.org/olia/susa.owl#DDQr -->

    <owl:NamedIndividual rdf:about="http://purl.org/olia/susa.owl#DDQr">
        <rdf:type rdf:resource="http://purl.org/olia/susa.owl#WHDeterminer"/>
        <olia_system:hasTag>DDQr</olia_system:hasTag>
        <olia_system:hasTier>POS</olia_system:hasTier>
        <rdfs:comment>DDQr for &quot;which&quot; in relative uses.</rdfs:comment>
    </owl:NamedIndividual>
    


    <!-- http://purl.org/olia/susa.owl#DDf -->

    <owl:NamedIndividual rdf:about="http://purl.org/olia/susa.owl#DDf">
        <rdf:type rdf:resource="http://purl.org/olia/susa.owl#Quantifier"/>
        <olia_system:hasTag>DDf</olia_system:hasTag>
        <olia_system:hasTier>POS</olia_system:hasTier>
        <rdfs:comment>DDf is used for &quot;enough&quot; as pronoun or pre- or postmodifying a noun.</rdfs:comment>
    </owl:NamedIndividual>
    


    <!-- http://purl.org/olia/susa.owl#DDi -->

    <owl:NamedIndividual rdf:about="http://purl.org/olia/susa.owl#DDi">
        <rdf:type rdf:resource="http://purl.org/olia/susa.owl#Quantifier"/>
        <olia_system:hasTag>DDi</olia_system:hasTag>
        <olia_system:hasTier>POS</olia_system:hasTier>
        <rdfs:comment>DDi is used for &quot;some&quot; as determiner or pronoun.</rdfs:comment>
    </owl:NamedIndividual>
    


    <!-- http://purl.org/olia/susa.owl#DDo -->

    <owl:NamedIndividual rdf:about="http://purl.org/olia/susa.owl#DDo">
        <rdf:type rdf:resource="http://purl.org/olia/susa.owl#Quantifier"/>
        <olia_system:hasTag>DDo</olia_system:hasTag>
        <olia_system:hasTier>POS</olia_system:hasTier>
        <rdfs:comment>DDo is used for &quot;a lot&quot;.</rdfs:comment>
    </owl:NamedIndividual>
    


    <!-- http://purl.org/olia/susa.owl#DDy -->

    <owl:NamedIndividual rdf:about="http://purl.org/olia/susa.owl#DDy">
        <rdf:type rdf:resource="http://purl.org/olia/susa.owl#Quantifier"/>
        <olia_system:hasTag>DDy</olia_system:hasTag>
        <olia_system:hasTier>POS</olia_system:hasTier>
        <rdfs:comment>DDy is used for &quot;any&quot; as determiner or pronoun.</rdfs:comment>
    </owl:NamedIndividual>
    


    <!-- http://purl.org/olia/susa.owl#EX-Tag -->

    <owl:NamedIndividual rdf:about="http://purl.org/olia/susa.owl#EX-Tag">
        <rdf:type rdf:resource="http://purl.org/olia/susa.owl#ExistentialThere"/>
        <olia_system:hasTag>EX</olia_system:hasTag>
        <olia_system:hasTier>POS</olia_system:hasTier>
        <rdfs:comment>EX is the SUSANNE tag used for the existential &quot;there&quot;.</rdfs:comment>
    </owl:NamedIndividual>
    


    <!-- http://purl.org/olia/susa.owl#FA -->

    <owl:NamedIndividual rdf:about="http://purl.org/olia/susa.owl#FA">
        <rdf:type rdf:resource="http://purl.org/olia/susa.owl#Suffix"/>
        <olia_system:hasTag>FA</olia_system:hasTag>
        <olia_system:hasTier>POS</olia_system:hasTier>
        <rdfs:comment>FA is the SUSANNE tag used for a suffix which is seperated by a hyphen.</rdfs:comment>
    </owl:NamedIndividual>
    


    <!-- http://purl.org/olia/susa.owl#FB -->

    <owl:NamedIndividual rdf:about="http://purl.org/olia/susa.owl#FB">
        <rdf:type rdf:resource="http://purl.org/olia/susa.owl#Prefix"/>
        <olia_system:hasTag>FB</olia_system:hasTag>
        <olia_system:hasTier>POS</olia_system:hasTier>
        <rdfs:comment>FB is the SUSANNE tag used for a prefix which is seperated by a hyphen.</rdfs:comment>
    </owl:NamedIndividual>
    


    <!-- http://purl.org/olia/susa.owl#FD -->

    <owl:NamedIndividual rdf:about="http://purl.org/olia/susa.owl#FD">
        <rdf:type rdf:resource="http://purl.org/olia/susa.owl#Distorted"/>
        <olia_system:hasTag>FD</olia_system:hasTag>
        <olia_system:hasTier>POS</olia_system:hasTier>
        <rdfs:comment>FD is the SUSANNE tag used for a distorted word. It is only used in speech analysis.</rdfs:comment>
    </owl:NamedIndividual>
    


    <!-- http://purl.org/olia/susa.owl#FO -->

    <owl:NamedIndividual rdf:about="http://purl.org/olia/susa.owl#FO">
        <rdf:type rdf:resource="http://purl.org/olia/susa.owl#Formula"/>
        <olia_system:hasTag>FO</olia_system:hasTag>
        <olia_system:hasTier>POS</olia_system:hasTier>
        <rdfs:comment>FO is the SUSANNE tag used for a determinate formula.</rdfs:comment>
    </owl:NamedIndividual>
    


    <!-- http://purl.org/olia/susa.owl#FOc -->

    <owl:NamedIndividual rdf:about="http://purl.org/olia/susa.owl#FOc">
        <rdf:type rdf:resource="http://purl.org/olia/susa.owl#Formula"/>
        <olia_system:hasTag>FOc</olia_system:hasTag>
        <olia_system:hasTier>POS</olia_system:hasTier>
        <rdfs:comment>FOc tags a formula or an acronym for chemical substances, molecules or subatomic particles e.g. &quot;TNT&quot;, &quot;DDT&quot;.</rdfs:comment>
    </owl:NamedIndividual>
    


    <!-- http://purl.org/olia/susa.owl#FOp -->

    <owl:NamedIndividual rdf:about="http://purl.org/olia/susa.owl#FOp">
        <rdf:type rdf:resource="http://purl.org/olia/susa.owl#Formula"/>
        <olia_system:hasTag>FOp</olia_system:hasTag>
        <olia_system:hasTier>POS</olia_system:hasTier>
        <rdfs:comment>FOp is used for a London postal district, the British post-code, teh American &apos;Zip-code&apos; e.g. &quot;W.C.2&quot;, &quot;LA6 3AN&quot;.</rdfs:comment>
    </owl:NamedIndividual>
    


    <!-- http://purl.org/olia/susa.owl#FOqc -->

    <owl:NamedIndividual rdf:about="http://purl.org/olia/susa.owl#FOqc">
        <rdf:type rdf:resource="http://purl.org/olia/susa.owl#Formula"/>
        <olia_system:hasTag>FOqc</olia_system:hasTag>
        <olia_system:hasTier>POS</olia_system:hasTier>
        <rdfs:comment>FOqc is the tag fora chemical equation, when it is analysed as a single word.</rdfs:comment>
    </owl:NamedIndividual>
    


    <!-- http://purl.org/olia/susa.owl#FOqx -->

    <owl:NamedIndividual rdf:about="http://purl.org/olia/susa.owl#FOqx">
        <rdf:type rdf:resource="http://purl.org/olia/susa.owl#Formula"/>
        <olia_system:hasTag>FOqx</olia_system:hasTag>
        <olia_system:hasTier>POS</olia_system:hasTier>
        <rdfs:comment>FOqx is used for a algebraic equation, when it is analysed as a single word.</rdfs:comment>
    </owl:NamedIndividual>
    


    <!-- http://purl.org/olia/susa.owl#FOr -->

    <owl:NamedIndividual rdf:about="http://purl.org/olia/susa.owl#FOr">
        <rdf:type rdf:resource="http://purl.org/olia/susa.owl#Formula"/>
        <olia_system:hasTag>FOr</olia_system:hasTag>
        <olia_system:hasTier>POS</olia_system:hasTier>
        <rdfs:comment>FOr is the tag for a road name e.g. &quot;M6 B6480 I-95&quot;.</rdfs:comment>
    </owl:NamedIndividual>
    


    <!-- http://purl.org/olia/susa.owl#FOs -->

    <owl:NamedIndividual rdf:about="http://purl.org/olia/susa.owl#FOs">
        <rdf:type rdf:resource="http://purl.org/olia/susa.owl#Formula"/>
        <olia_system:hasTag>FOs</olia_system:hasTag>
        <olia_system:hasTier>POS</olia_system:hasTier>
        <rdfs:comment>FOs is the tag for registrtation/ reference/ serial/ model number.</rdfs:comment>
    </owl:NamedIndividual>
    


    <!-- http://purl.org/olia/susa.owl#FOt -->

    <owl:NamedIndividual rdf:about="http://purl.org/olia/susa.owl#FOt">
        <rdf:type rdf:resource="http://purl.org/olia/susa.owl#Formula"/>
        <olia_system:hasTag>FOt</olia_system:hasTag>
        <olia_system:hasTier>POS</olia_system:hasTier>
        <rdfs:comment>FOt is used for a telephone number.</rdfs:comment>
    </owl:NamedIndividual>
    


    <!-- http://purl.org/olia/susa.owl#FOx -->

    <owl:NamedIndividual rdf:about="http://purl.org/olia/susa.owl#FOx">
        <rdf:type rdf:resource="http://purl.org/olia/susa.owl#Formula"/>
        <olia_system:hasTag>FOx</olia_system:hasTag>
        <olia_system:hasTier>POS</olia_system:hasTier>
        <rdfs:comment>FOx is the tag for an algebraic expression with nominal as opposed to equative function e.g. &quot;a&quot;, &quot;pi&quot;.</rdfs:comment>
    </owl:NamedIndividual>
    


    <!-- http://purl.org/olia/susa.owl#FW -->

    <owl:NamedIndividual rdf:about="http://purl.org/olia/susa.owl#FW">
        <rdf:type rdf:resource="http://purl.org/olia/susa.owl#ForeignWord"/>
        <olia_system:hasTag>FW</olia_system:hasTag>
        <olia_system:hasTier>POS</olia_system:hasTier>
        <rdfs:comment>FW is the SUSANNE tag used for a foreign word which is not capable of being allocated a more specific tag by reference to its English context.</rdfs:comment>
    </owl:NamedIndividual>
    


    <!-- http://purl.org/olia/susa.owl#FWg -->

    <owl:NamedIndividual rdf:about="http://purl.org/olia/susa.owl#FWg">
        <rdf:type rdf:resource="http://purl.org/olia/susa.owl#ForeignWord"/>
        <olia_system:hasTag>FWg</olia_system:hasTag>
        <olia_system:hasTier>POS</olia_system:hasTier>
        <rdfs:comment>FWg is used for a biological Latin name of genus or other rank higherthan species e.g. &quot;Equus Umbelliferae&quot;.</rdfs:comment>
    </owl:NamedIndividual>
    


    <!-- http://purl.org/olia/susa.owl#FWs -->

    <owl:NamedIndividual rdf:about="http://purl.org/olia/susa.owl#FWs">
        <rdf:type rdf:resource="http://purl.org/olia/susa.owl#ForeignWord"/>
        <olia_system:hasTag>FWs</olia_system:hasTag>
        <olia_system:hasTier>POS</olia_system:hasTier>
        <rdfs:comment>FWs is the tag for a biological Latin species (or lower rank) name e.g.  &quot;sapiens officinale&quot;.</rdfs:comment>
    </owl:NamedIndividual>
    


    <!-- http://purl.org/olia/susa.owl#GG -->

    <owl:NamedIndividual rdf:about="http://purl.org/olia/susa.owl#GG">
        <rdf:type rdf:resource="http://purl.org/olia/susa.owl#GenitiveInflection"/>
        <olia_system:hasTag>GG</olia_system:hasTag>
        <olia_system:hasTier>POS</olia_system:hasTier>
        <rdfs:comment>GG is the SUSANNE tag used for the Germanic genitive inflection +´s, or + ´ after a plural stem and certain other stems ending in -s.</rdfs:comment>
    </owl:NamedIndividual>
    


    <!-- http://purl.org/olia/susa.owl#ICS -->

    <owl:NamedIndividual rdf:about="http://purl.org/olia/susa.owl#ICS">
        <rdf:type rdf:resource="http://purl.org/olia/susa.owl#PrepositionOrSubordinatingConjunction"/>
        <olia_system:hasTag>ICS</olia_system:hasTag>
        <olia_system:hasTier>POS</olia_system:hasTier>
        <rdfs:comment>ICS is used for &quot;considering&quot;, &quot;notwithstanding&quot;.</rdfs:comment>
    </owl:NamedIndividual>
    


    <!-- http://purl.org/olia/susa.owl#ICSk -->

    <owl:NamedIndividual rdf:about="http://purl.org/olia/susa.owl#ICSk">
        <rdf:type rdf:resource="http://purl.org/olia/susa.owl#PrepositionOrSubordinatingConjunction"/>
        <olia_system:hasTag>ICSk</olia_system:hasTag>
        <olia_system:hasTier>POS</olia_system:hasTier>
        <rdfs:comment>ICSk is the tag for &quot;like&quot; as preposition, subordinating conjunction, or in a relative use.</rdfs:comment>
    </owl:NamedIndividual>
    


    <!-- http://purl.org/olia/susa.owl#ICSt -->

    <owl:NamedIndividual rdf:about="http://purl.org/olia/susa.owl#ICSt">
        <rdf:type rdf:resource="http://purl.org/olia/susa.owl#PrepositionOrSubordinatingConjunction"/>
        <olia_system:hasTag>ICSt</olia_system:hasTag>
        <olia_system:hasTier>POS</olia_system:hasTier>
        <rdfs:comment>ISCt describes &quot;after&quot;, &quot;before&quot;, &quot;ere&quot;, &quot;since&quot;, &quot;until&quot;, &quot;til&quot; as prepositions (with a complement) or subordinating conjunctions.</rdfs:comment>
    </owl:NamedIndividual>
    


    <!-- http://purl.org/olia/susa.owl#ICSx -->

    <owl:NamedIndividual rdf:about="http://purl.org/olia/susa.owl#ICSx">
        <rdf:type rdf:resource="http://purl.org/olia/susa.owl#PrepositionOrSubordinatingConjunction"/>
        <olia_system:hasTag>ICSx</olia_system:hasTag>
        <olia_system:hasTier>POS</olia_system:hasTier>
        <rdfs:comment>ISCx is the SUSANNE tag used for &quot;but&quot;, &quot;except&quot;, &quot;save&quot; as prepositions or subordinating conjunctions.</rdfs:comment>
    </owl:NamedIndividual>
    


    <!-- http://purl.org/olia/susa.owl#IF -->

    <owl:NamedIndividual rdf:about="http://purl.org/olia/susa.owl#IF">
        <rdf:type rdf:resource="http://purl.org/olia/susa.owl#Preposition"/>
        <olia_system:hasTag>IF</olia_system:hasTag>
        <olia_system:hasTier>POS</olia_system:hasTier>
        <rdfs:comment>IF is the SUSANNE tag used for &quot;for&quot; as preposition.
(Sampson 1995, p. 109)</rdfs:comment>
    </owl:NamedIndividual>
    


    <!-- http://purl.org/olia/susa.owl#II -->

    <owl:NamedIndividual rdf:about="http://purl.org/olia/susa.owl#II">
        <rdf:type rdf:resource="http://purl.org/olia/susa.owl#Preposition"/>
        <olia_system:hasTag>II</olia_system:hasTag>
        <olia_system:hasTier>POS</olia_system:hasTier>
        <rdfs:comment>II is the SUSANNE tag used for general prepositions, including prepositional use of words which can function either as preposition or as adverb. e.g. &quot;into&quot;, &quot;near&quot;, &quot;off&quot;, &quot;on&quot;, &quot;onto&quot;, &quot;opposite&quot;, &quot;outside&quot;, &quot;over&quot;, &quot;past&quot;, &quot;through&quot;.
(Sampson 1995, p. 109)</rdfs:comment>
    </owl:NamedIndividual>
    


    <!-- http://purl.org/olia/susa.owl#IIa -->

    <owl:NamedIndividual rdf:about="http://purl.org/olia/susa.owl#IIa">
        <rdf:type rdf:resource="http://purl.org/olia/susa.owl#Preposition"/>
        <olia_system:hasTag>IIa</olia_system:hasTag>
        <olia_system:hasTier>POS</olia_system:hasTier>
        <rdfs:comment>IIa is the SUSANNE tag used for &quot;as&quot;.</rdfs:comment>
    </owl:NamedIndividual>
    


    <!-- http://purl.org/olia/susa.owl#IIb -->

    <owl:NamedIndividual rdf:about="http://purl.org/olia/susa.owl#IIb">
        <rdf:type rdf:resource="http://purl.org/olia/susa.owl#Preposition"/>
        <olia_system:hasTag>IIb</olia_system:hasTag>
        <olia_system:hasTier>POS</olia_system:hasTier>
        <rdfs:comment>IIb is used for &quot;by&quot;.</rdfs:comment>
    </owl:NamedIndividual>
    


    <!-- http://purl.org/olia/susa.owl#IIg -->

    <owl:NamedIndividual rdf:about="http://purl.org/olia/susa.owl#IIg">
        <rdf:type rdf:resource="http://purl.org/olia/susa.owl#Preposition"/>
        <olia_system:hasTag>IIg</olia_system:hasTag>
        <olia_system:hasTier>POS</olia_system:hasTier>
        <rdfs:comment>IIg is the tag for  &quot;aged&quot; as a pseudo-preposition.</rdfs:comment>
    </owl:NamedIndividual>
    


    <!-- http://purl.org/olia/susa.owl#IIp -->

    <owl:NamedIndividual rdf:about="http://purl.org/olia/susa.owl#IIp">
        <rdf:type rdf:resource="http://purl.org/olia/susa.owl#Preposition"/>
        <olia_system:hasTag>IIp</olia_system:hasTag>
        <olia_system:hasTier>POS</olia_system:hasTier>
        <rdfs:comment>IIp is used for &quot;per&quot;.</rdfs:comment>
    </owl:NamedIndividual>
    


    <!-- http://purl.org/olia/susa.owl#IIt -->

    <owl:NamedIndividual rdf:about="http://purl.org/olia/susa.owl#IIt">
        <rdf:type rdf:resource="http://purl.org/olia/susa.owl#Preposition"/>
        <olia_system:hasTag>IIt</olia_system:hasTag>
        <olia_system:hasTier>POS</olia_system:hasTier>
        <rdfs:comment>IIt is used for &quot;to&quot; as preposition.</rdfs:comment>
    </owl:NamedIndividual>
    


    <!-- http://purl.org/olia/susa.owl#IIx -->

    <owl:NamedIndividual rdf:about="http://purl.org/olia/susa.owl#IIx">
        <rdf:type rdf:resource="http://purl.org/olia/susa.owl#Preposition"/>
        <olia_system:hasTag>IIx</olia_system:hasTag>
        <olia_system:hasTier>POS</olia_system:hasTier>
        <rdfs:comment>IIx is used for mathematical infix operators e.g. &quot;+&quot;, &quot;&gt;&quot;, &quot;=&quot;, etc. .</rdfs:comment>
    </owl:NamedIndividual>
    


    <!-- http://purl.org/olia/susa.owl#IO -->

    <owl:NamedIndividual rdf:about="http://purl.org/olia/susa.owl#IO">
        <rdf:type rdf:resource="http://purl.org/olia/susa.owl#Preposition"/>
        <olia_system:hasTag>IO</olia_system:hasTag>
        <olia_system:hasTier>POS</olia_system:hasTier>
        <rdfs:comment>IO is the SUSANNE tag used for &quot;of&quot;.
(Sampson 1995, p. 109)</rdfs:comment>
    </owl:NamedIndividual>
    


    <!-- http://purl.org/olia/susa.owl#IW -->

    <owl:NamedIndividual rdf:about="http://purl.org/olia/susa.owl#IW">
        <rdf:type rdf:resource="http://purl.org/olia/susa.owl#Preposition"/>
        <olia_system:hasTag>IW</olia_system:hasTag>
        <olia_system:hasTier>POS</olia_system:hasTier>
        <rdfs:comment>IW is the SUSANNE tag used for &quot;with&quot; in all uses, &quot;without&quot; as preposition, &quot;what with&quot;.
(Sampson 1995, p. 109)</rdfs:comment>
    </owl:NamedIndividual>
    


    <!-- http://purl.org/olia/susa.owl#JA -->

    <owl:NamedIndividual rdf:about="http://purl.org/olia/susa.owl#JA">
        <rdf:type rdf:resource="http://purl.org/olia/susa.owl#PredicativeAdjective"/>
        <olia_system:hasTag>JA</olia_system:hasTag>
        <olia_system:hasTier>POS</olia_system:hasTier>
        <rdfs:comment>JA is used for predicatively used adjectives e.g. &quot;ablaze&quot;, &quot;alone&quot;.</rdfs:comment>
    </owl:NamedIndividual>
    


    <!-- http://purl.org/olia/susa.owl#JB -->

    <owl:NamedIndividual rdf:about="http://purl.org/olia/susa.owl#JB">
        <rdf:type rdf:resource="http://purl.org/olia/susa.owl#AttributiveAdjective"/>
        <olia_system:hasTag>JB</olia_system:hasTag>
        <olia_system:hasTier>POS</olia_system:hasTier>
        <rdfs:comment>JB is used for attributively used adjectives e.g. &quot;chief&quot;, &quot;entire&quot;, &quot;future&quot;, &quot;inverse&quot;, &quot;major&quot;.</rdfs:comment>
    </owl:NamedIndividual>
    


    <!-- http://purl.org/olia/susa.owl#JBR -->

    <owl:NamedIndividual rdf:about="http://purl.org/olia/susa.owl#JBR">
        <rdf:type rdf:resource="http://purl.org/olia/susa.owl#AttributiveAdjective"/>
        <olia_system:hasTag>JBR</olia_system:hasTag>
        <olia_system:hasTier>POS</olia_system:hasTier>
        <rdfs:comment>JBR is used for e.g. &quot;inner&quot;, &quot;lesser&quot;, &quot;nether&quot;, &quot;outer&quot;, &quot;upper&quot;.</rdfs:comment>
    </owl:NamedIndividual>
    


    <!-- http://purl.org/olia/susa.owl#JBT -->

    <owl:NamedIndividual rdf:about="http://purl.org/olia/susa.owl#JBT">
        <rdf:type rdf:resource="http://purl.org/olia/susa.owl#AttributiveAdjective"/>
        <olia_system:hasTag>JBT</olia_system:hasTag>
        <olia_system:hasTier>POS</olia_system:hasTier>
        <rdfs:comment>JBT is the SUSANNE tag used for e.g. &quot;utmost&quot;, &quot;uttermost&quot;.</rdfs:comment>
    </owl:NamedIndividual>
    


    <!-- http://purl.org/olia/susa.owl#JBo -->

    <owl:NamedIndividual rdf:about="http://purl.org/olia/susa.owl#JBo">
        <rdf:type rdf:resource="http://purl.org/olia/susa.owl#AttributiveAdjective"/>
        <olia_system:hasTag>JBo</olia_system:hasTag>
        <olia_system:hasTier>POS</olia_system:hasTier>
        <rdfs:comment>JBo is used for &quot;other&quot; in all uses.</rdfs:comment>
    </owl:NamedIndividual>
    


    <!-- http://purl.org/olia/susa.owl#JBy -->

    <owl:NamedIndividual rdf:about="http://purl.org/olia/susa.owl#JBy">
        <rdf:type rdf:resource="http://purl.org/olia/susa.owl#AttributiveAdjective"/>
        <olia_system:hasTag>JBy</olia_system:hasTag>
        <olia_system:hasTier>POS</olia_system:hasTier>
        <rdfs:comment>JBy is used for &quot;only&quot; as an adjective like in the example &quot;the only thing&quot;.</rdfs:comment>
    </owl:NamedIndividual>
    


    <!-- http://purl.org/olia/susa.owl#JJ -->

    <owl:NamedIndividual rdf:about="http://purl.org/olia/susa.owl#JJ">
        <rdf:type rdf:resource="http://purl.org/olia/susa.owl#GeneralAdjective"/>
        <hasDegree rdf:resource="http://purl.org/olia/susa.owl#positive"/>
        <olia_system:hasTag>JJ</olia_system:hasTag>
        <olia_system:hasTier>POS</olia_system:hasTier>
        <rdfs:comment>JJ is used for general adjectives e.g. &quot;blue&quot;, &quot;English&quot;.</rdfs:comment>
    </owl:NamedIndividual>
    


    <!-- http://purl.org/olia/susa.owl#JJR -->

    <owl:NamedIndividual rdf:about="http://purl.org/olia/susa.owl#JJR">
        <rdf:type rdf:resource="http://purl.org/olia/susa.owl#GeneralAdjective"/>
        <hasDegree rdf:resource="http://purl.org/olia/susa.owl#comparative"/>
        <olia_system:hasTag>JJR</olia_system:hasTag>
        <olia_system:hasTier>POS</olia_system:hasTier>
        <rdfs:comment>JJRis used for comparative adjectives, including &quot;elder&quot; and &quot;further&quot;.</rdfs:comment>
    </owl:NamedIndividual>
    


    <!-- http://purl.org/olia/susa.owl#JJT -->

    <owl:NamedIndividual rdf:about="http://purl.org/olia/susa.owl#JJT">
        <rdf:type rdf:resource="http://purl.org/olia/susa.owl#GeneralAdjective"/>
        <hasDegree rdf:resource="http://purl.org/olia/susa.owl#superlative"/>
        <olia_system:hasTag>JJT</olia_system:hasTag>
        <olia_system:hasTier>POS</olia_system:hasTier>
        <rdfs:comment>JJT is used for superlative adjectives, including &quot;eldest&quot; and &quot;furthest&quot;.</rdfs:comment>
    </owl:NamedIndividual>
    


    <!-- http://purl.org/olia/susa.owl#JJh -->

    <owl:NamedIndividual rdf:about="http://purl.org/olia/susa.owl#JJh">
        <rdf:type rdf:resource="http://purl.org/olia/susa.owl#GeneralAdjective"/>
        <hasDegree rdf:resource="http://purl.org/olia/susa.owl#positive"/>
        <olia_system:hasTag>JJh</olia_system:hasTag>
        <olia_system:hasTier>POS</olia_system:hasTier>
        <rdfs:comment>JJh is used for pseudo-adjectives formed by suffixing &quot;-ed&quot; to the last word of a nominal compound.</rdfs:comment>
    </owl:NamedIndividual>
    


    <!-- http://purl.org/olia/susa.owl#JJj -->

    <owl:NamedIndividual rdf:about="http://purl.org/olia/susa.owl#JJj">
        <rdf:type rdf:resource="http://purl.org/olia/susa.owl#GeneralAdjective"/>
        <hasDegree rdf:resource="http://purl.org/olia/susa.owl#positive"/>
        <olia_system:hasTag>JJj</olia_system:hasTag>
        <olia_system:hasTier>POS</olia_system:hasTier>
        <rdfs:comment>JJj is the tag for abbreviated adjectives appended to organization names to identify it legal status e.g. &quot;Ltd Inc Pty&quot; and counterparts in other jurisdictions.</rdfs:comment>
    </owl:NamedIndividual>
    


    <!-- http://purl.org/olia/susa.owl#JJs -->

    <owl:NamedIndividual rdf:about="http://purl.org/olia/susa.owl#JJs">
        <rdf:type rdf:resource="http://purl.org/olia/susa.owl#GeneralAdjective"/>
        <hasDegree rdf:resource="http://purl.org/olia/susa.owl#positive"/>
        <olia_system:hasTag>JJs</olia_system:hasTag>
        <olia_system:hasTier>POS</olia_system:hasTier>
        <rdfs:comment>JJs is used for adjectives in -most orther than &quot;utmost/ uttermost&quot; e.g. &quot;backmost&quot;, &quot;inmost&quot;, &quot;lowermost&quot;, &quot;midmost&quot;.</rdfs:comment>
    </owl:NamedIndividual>
    


    <!-- http://purl.org/olia/susa.owl#LE -->

    <owl:NamedIndividual rdf:about="http://purl.org/olia/susa.owl#LE">
        <rdf:type rdf:resource="http://purl.org/olia/susa.owl#PreCoordinator"/>
        <olia_system:hasTag>LE</olia_system:hasTag>
        <olia_system:hasTier>POS</olia_system:hasTier>
        <rdfs:comment>LE is used for &quot;both&quot;, &quot;not only&quot; as pre-co-ordinator.</rdfs:comment>
    </owl:NamedIndividual>
    


    <!-- http://purl.org/olia/susa.owl#LEe -->

    <owl:NamedIndividual rdf:about="http://purl.org/olia/susa.owl#LEe">
        <rdf:type rdf:resource="http://purl.org/olia/susa.owl#PreCoordinator"/>
        <olia_system:hasTag>LEe</olia_system:hasTag>
        <olia_system:hasTier>POS</olia_system:hasTier>
        <rdfs:comment>LEe is used for &quot;either&quot; as pre-co-ordinator.</rdfs:comment>
    </owl:NamedIndividual>
    


    <!-- http://purl.org/olia/susa.owl#LEn -->

    <owl:NamedIndividual rdf:about="http://purl.org/olia/susa.owl#LEn">
        <rdf:type rdf:resource="http://purl.org/olia/susa.owl#PreCoordinator"/>
        <olia_system:hasTag>LEn</olia_system:hasTag>
        <olia_system:hasTier>POS</olia_system:hasTier>
        <rdfs:comment>LEn is used for &quot;neither&quot; as pre-co-ordinator.</rdfs:comment>
    </owl:NamedIndividual>
    


    <!-- http://purl.org/olia/susa.owl#MC -->

    <owl:NamedIndividual rdf:about="http://purl.org/olia/susa.owl#MC">
        <rdf:type rdf:resource="http://purl.org/olia/susa.owl#CardinalNumber"/>
        <hasNumber rdf:resource="http://purl.org/olia/susa.owl#singular"/>
        <olia_system:hasTag>MC</olia_system:hasTag>
        <olia_system:hasTier>POS</olia_system:hasTier>
        <rdfs:comment>MC is the SUSANNE tag used for cardinal numbers from  &quot;zero&quot; upwards, spelled out. This includes &quot;umpteen&quot;.</rdfs:comment>
    </owl:NamedIndividual>
    


    <!-- http://purl.org/olia/susa.owl#MC1 -->

    <owl:NamedIndividual rdf:about="http://purl.org/olia/susa.owl#MC1">
        <rdf:type rdf:resource="http://purl.org/olia/susa.owl#CardinalNumber"/>
        <olia_system:hasTag>MC1</olia_system:hasTag>
        <olia_system:hasTier>POS</olia_system:hasTier>
        <rdfs:comment>MC1 is used for &quot;one&quot; as numeral.</rdfs:comment>
    </owl:NamedIndividual>
    


    <!-- http://purl.org/olia/susa.owl#MC1n -->

    <owl:NamedIndividual rdf:about="http://purl.org/olia/susa.owl#MC1n">
        <rdf:type rdf:resource="http://purl.org/olia/susa.owl#CardinalNumber"/>
        <olia_system:hasTag>MC1n</olia_system:hasTag>
        <olia_system:hasTier>POS</olia_system:hasTier>
        <rdfs:comment>MC1n is the tag for 1 written digitally, including uses as ordinal e.g. &quot;February 1&quot;.</rdfs:comment>
    </owl:NamedIndividual>
    


    <!-- http://purl.org/olia/susa.owl#MC2 -->

    <owl:NamedIndividual rdf:about="http://purl.org/olia/susa.owl#MC2">
        <rdf:type rdf:resource="http://purl.org/olia/susa.owl#CardinalNumber"/>
        <hasNumber rdf:resource="http://purl.org/olia/susa.owl#plural"/>
        <olia_system:hasTag>MC2</olia_system:hasTag>
        <olia_system:hasTier>POS</olia_system:hasTier>
        <rdfs:comment>MC2 tags the plural of cardinals.</rdfs:comment>
    </owl:NamedIndividual>
    


    <!-- http://purl.org/olia/susa.owl#MC2n -->

    <owl:NamedIndividual rdf:about="http://purl.org/olia/susa.owl#MC2n">
        <rdf:type rdf:resource="http://purl.org/olia/susa.owl#CardinalNumber"/>
        <hasNumber rdf:resource="http://purl.org/olia/susa.owl#plural"/>
        <olia_system:hasTag>MC2n</olia_system:hasTag>
        <olia_system:hasTier>POS</olia_system:hasTier>
        <rdfs:comment>MC2n is used for the plural of cardinals written digitally.</rdfs:comment>
    </owl:NamedIndividual>
    


    <!-- http://purl.org/olia/susa.owl#MC2r -->

    <owl:NamedIndividual rdf:about="http://purl.org/olia/susa.owl#MC2r">
        <rdf:type rdf:resource="http://purl.org/olia/susa.owl#CardinalNumber"/>
        <hasNumber rdf:resource="http://purl.org/olia/susa.owl#plural"/>
        <olia_system:hasTag>MC2r</olia_system:hasTag>
        <olia_system:hasTier>POS</olia_system:hasTier>
        <rdfs:comment>MC2r decribes the plural of roman numerals.</rdfs:comment>
    </owl:NamedIndividual>
    


    <!-- http://purl.org/olia/susa.owl#MC2y -->

    <owl:NamedIndividual rdf:about="http://purl.org/olia/susa.owl#MC2y">
        <rdf:type rdf:resource="http://purl.org/olia/susa.owl#CardinalNumber"/>
        <hasNumber rdf:resource="http://purl.org/olia/susa.owl#plural"/>
        <olia_system:hasTag>MC2y</olia_system:hasTag>
        <olia_system:hasTier>POS</olia_system:hasTier>
        <rdfs:comment>MC2y is used for the plural of year names e.g. &quot;1960s&quot;.</rdfs:comment>
    </owl:NamedIndividual>
    


    <!-- http://purl.org/olia/susa.owl#MCb -->

    <owl:NamedIndividual rdf:about="http://purl.org/olia/susa.owl#MCb">
        <rdf:type rdf:resource="http://purl.org/olia/susa.owl#CardinalNumber"/>
        <olia_system:hasTag>vMCb</olia_system:hasTag>
        <olia_system:hasTier>POS</olia_system:hasTier>
        <rdfs:comment>MCb is used for &apos;labels&apos; for cross-reference within and between texts, comprising combinations of digits, letters and/ or non-alphanumeric characters.</rdfs:comment>
    </owl:NamedIndividual>
    


    <!-- http://purl.org/olia/susa.owl#MCd -->

    <owl:NamedIndividual rdf:about="http://purl.org/olia/susa.owl#MCd">
        <rdf:type rdf:resource="http://purl.org/olia/susa.owl#CardinalNumber"/>
        <olia_system:hasTag>MCd</olia_system:hasTag>
        <olia_system:hasTier>POS</olia_system:hasTier>
        <rdfs:comment>MCd is the tag for numerals including decimal points.</rdfs:comment>
    </owl:NamedIndividual>
    


    <!-- http://purl.org/olia/susa.owl#MCe -->

    <owl:NamedIndividual rdf:about="http://purl.org/olia/susa.owl#MCe">
        <rdf:type rdf:resource="http://purl.org/olia/susa.owl#CardinalNumber"/>
        <olia_system:hasTag>MCe</olia_system:hasTag>
        <olia_system:hasTier>POS</olia_system:hasTier>
        <rdfs:comment>MCe is for numbers containing a non-decimal separator, other than a time-of-day expression, e.g. &quot;4:11&quot;, &quot;4.11&quot;(stands for four years and 11 months), &quot;3.4.93&quot;.</rdfs:comment>
    </owl:NamedIndividual>
    


    <!-- http://purl.org/olia/susa.owl#MCn -->

    <owl:NamedIndividual rdf:about="http://purl.org/olia/susa.owl#MCn">
        <rdf:type rdf:resource="http://purl.org/olia/susa.owl#CardinalNumber"/>
        <hasNumber rdf:resource="http://purl.org/olia/susa.owl#singular"/>
        <olia_system:hasTag>MCn</olia_system:hasTag>
        <olia_system:hasTier>POS</olia_system:hasTier>
        <rdfs:comment>MCn is used for cardinal numerals written in digits, e.g &quot;February 28&quot;.</rdfs:comment>
    </owl:NamedIndividual>
    


    <!-- http://purl.org/olia/susa.owl#MCo -->

    <owl:NamedIndividual rdf:about="http://purl.org/olia/susa.owl#MCo">
        <rdf:type rdf:resource="http://purl.org/olia/susa.owl#CardinalNumber"/>
        <olia_system:hasTag>MCo</olia_system:hasTag>
        <olia_system:hasTier>POS</olia_system:hasTier>
        <rdfs:comment>MCo is the tag for &quot;0&quot; written as digit.</rdfs:comment>
    </owl:NamedIndividual>
    


    <!-- http://purl.org/olia/susa.owl#MCr -->

    <owl:NamedIndividual rdf:about="http://purl.org/olia/susa.owl#MCr">
        <rdf:type rdf:resource="http://purl.org/olia/susa.owl#CardinalNumber"/>
        <hasNumber rdf:resource="http://purl.org/olia/susa.owl#singular"/>
        <olia_system:hasTag>MCr</olia_system:hasTag>
        <olia_system:hasTier>POS</olia_system:hasTier>
        <rdfs:comment>MCr is used for roman numerals from &quot; I &quot;  upwards.</rdfs:comment>
    </owl:NamedIndividual>
    


    <!-- http://purl.org/olia/susa.owl#MCs -->

    <owl:NamedIndividual rdf:about="http://purl.org/olia/susa.owl#MCs">
        <rdf:type rdf:resource="http://purl.org/olia/susa.owl#CardinalNumber"/>
        <olia_system:hasTag>MCs</olia_system:hasTag>
        <olia_system:hasTier>POS</olia_system:hasTier>
        <rdfs:comment>MCs is the desciption for integers written digitally with a leading zero e.g. &quot;007&quot;.</rdfs:comment>
    </owl:NamedIndividual>
    


    <!-- http://purl.org/olia/susa.owl#MCy -->

    <owl:NamedIndividual rdf:about="http://purl.org/olia/susa.owl#MCy">
        <rdf:type rdf:resource="http://purl.org/olia/susa.owl#CardinalNumber"/>
        <hasNumber rdf:resource="http://purl.org/olia/susa.owl#singular"/>
        <olia_system:hasTag>MCy</olia_system:hasTag>
        <olia_system:hasTier>POS</olia_system:hasTier>
        <rdfs:comment>MCy stands for the year name written digitally (full or with apostrophe) e.g. &quot;1987&quot;, &quot; `99&quot;.</rdfs:comment>
    </owl:NamedIndividual>
    


    <!-- http://purl.org/olia/susa.owl#MD -->

    <owl:NamedIndividual rdf:about="http://purl.org/olia/susa.owl#MD">
        <rdf:type rdf:resource="http://purl.org/olia/susa.owl#OrdinalNumber"/>
        <olia_system:hasTag>MD</olia_system:hasTag>
        <olia_system:hasTier>POS</olia_system:hasTier>
        <rdfs:comment>MD is the SUSANNE tag used for ordinal numbers, whether used as ordinal adjective or adverb or as fraction e.g. &quot;third&quot;, &quot;fourth&quot;.</rdfs:comment>
    </owl:NamedIndividual>
    


    <!-- http://purl.org/olia/susa.owl#MDn -->

    <owl:NamedIndividual rdf:about="http://purl.org/olia/susa.owl#MDn">
        <rdf:type rdf:resource="http://purl.org/olia/susa.owl#OrdinalNumber"/>
        <olia_system:hasTag>MDn</olia_system:hasTag>
        <olia_system:hasTier>POS</olia_system:hasTier>
        <rdfs:comment>MDn are ordinal numbers written digitally e.g.  &quot;1 st&quot;, &quot;2 nd&quot;.</rdfs:comment>
    </owl:NamedIndividual>
    


    <!-- http://purl.org/olia/susa.owl#MDo -->

    <owl:NamedIndividual rdf:about="http://purl.org/olia/susa.owl#MDo">
        <rdf:type rdf:resource="http://purl.org/olia/susa.owl#OrdinalNumber"/>
        <olia_system:hasTag>MDo</olia_system:hasTag>
        <olia_system:hasTier>POS</olia_system:hasTier>
        <rdfs:comment>MDo is the tag for &quot;first&quot;, &quot;second&quot;.</rdfs:comment>
    </owl:NamedIndividual>
    


    <!-- http://purl.org/olia/susa.owl#MDt -->

    <owl:NamedIndividual rdf:about="http://purl.org/olia/susa.owl#MDt">
        <rdf:type rdf:resource="http://purl.org/olia/susa.owl#OrdinalNumber"/>
        <olia_system:hasTag>MDt</olia_system:hasTag>
        <olia_system:hasTier>POS</olia_system:hasTier>
        <rdfs:comment>MDt is used for &quot;next&quot;, &quot;last&quot;.</rdfs:comment>
    </owl:NamedIndividual>
    


    <!-- http://purl.org/olia/susa.owl#MF -->

    <owl:NamedIndividual rdf:about="http://purl.org/olia/susa.owl#MF">
        <rdf:type rdf:resource="http://purl.org/olia/susa.owl#Fraction"/>
        <olia_system:hasTag>MF</olia_system:hasTag>
        <olia_system:hasTier>POS</olia_system:hasTier>
        <rdfs:comment>MF is used  for fraction numerals.</rdfs:comment>
    </owl:NamedIndividual>
    


    <!-- http://purl.org/olia/susa.owl#MFn -->

    <owl:NamedIndividual rdf:about="http://purl.org/olia/susa.owl#MFn">
        <rdf:type rdf:resource="http://purl.org/olia/susa.owl#Fraction"/>
        <olia_system:hasTag>MFn</olia_system:hasTag>
        <olia_system:hasTier>POS</olia_system:hasTier>
        <rdfs:comment>MFn is the SUSANNE tag used for fractions written digitally e.g. &quot;2/3&quot;.</rdfs:comment>
    </owl:NamedIndividual>
    


    <!-- http://purl.org/olia/susa.owl#ND -->

    <owl:NamedIndividual rdf:about="http://purl.org/olia/susa.owl#ND">
        <rdf:type rdf:resource="http://purl.org/olia/susa.owl#DirectionNoun"/>
        <olia_system:hasTag>ND</olia_system:hasTag>
        <olia_system:hasTier>POS</olia_system:hasTier>
        <rdfs:comment>ND is used for direction nouns.</rdfs:comment>
    </owl:NamedIndividual>
    


    <!-- http://purl.org/olia/susa.owl#ND1 -->

    <owl:NamedIndividual rdf:about="http://purl.org/olia/susa.owl#ND1">
        <rdf:type rdf:resource="http://purl.org/olia/susa.owl#DirectionNoun"/>
        <hasNumber rdf:resource="http://purl.org/olia/susa.owl#singular"/>
        <olia_system:hasTag>ND1</olia_system:hasTag>
        <olia_system:hasTier>POS</olia_system:hasTier>
        <rdfs:comment>ND1 is used for direction e.g. &quot;north&quot;, &quot;N&quot;, &quot;southeast&quot;.</rdfs:comment>
    </owl:NamedIndividual>
    


    <!-- http://purl.org/olia/susa.owl#NN -->

    <owl:NamedIndividual rdf:about="http://purl.org/olia/susa.owl#NN">
        <rdf:type rdf:resource="http://purl.org/olia/susa.owl#CommonNoun"/>
        <olia_system:hasTag>NN</olia_system:hasTag>
        <olia_system:hasTier>POS</olia_system:hasTier>
        <rdfs:comment>This is a common noun.</rdfs:comment>
    </owl:NamedIndividual>
    


    <!-- http://purl.org/olia/susa.owl#NN1 -->

    <owl:NamedIndividual rdf:about="http://purl.org/olia/susa.owl#NN1">
        <rdf:type rdf:resource="http://purl.org/olia/susa.owl#CommonNoun"/>
        <hasNumber rdf:resource="http://purl.org/olia/susa.owl#singular"/>
        <olia_system:hasTag>NN1</olia_system:hasTag>
        <olia_system:hasTier>POS</olia_system:hasTier>
        <rdfs:comment>This is a common noun in singular.</rdfs:comment>
    </owl:NamedIndividual>
    


    <!-- http://purl.org/olia/susa.owl#NN1c -->

    <owl:NamedIndividual rdf:about="http://purl.org/olia/susa.owl#NN1c">
        <rdf:type rdf:resource="http://purl.org/olia/susa.owl#CommonNoun"/>
        <hasCountability rdf:resource="http://purl.org/olia/susa.owl#countable"/>
        <hasNumber rdf:resource="http://purl.org/olia/susa.owl#singular"/>
        <olia_system:hasTag>NN1c</olia_system:hasTag>
        <olia_system:hasTier>POS</olia_system:hasTier>
        <rdfs:comment>This is a countable singular noun, e.g. &quot;clock&quot;, &quot;crowd&quot;, &quot;Buddhist&quot;.</rdfs:comment>
    </owl:NamedIndividual>
    


    <!-- http://purl.org/olia/susa.owl#NN1m -->

    <owl:NamedIndividual rdf:about="http://purl.org/olia/susa.owl#NN1m">
        <rdf:type rdf:resource="http://purl.org/olia/susa.owl#CommonNoun"/>
        <hasNumber rdf:resource="http://purl.org/olia/susa.owl#singular"/>
        <olia_system:hasTag>NN1m</olia_system:hasTag>
        <olia_system:hasTier>POS</olia_system:hasTier>
        <rdfs:comment>This is a noun which beginns with &quot;mid-&quot; other than time noun, e.g. &quot;midstream&quot;, &quot;midfield&quot;.</rdfs:comment>
    </owl:NamedIndividual>
    


    <!-- http://purl.org/olia/susa.owl#NN1n -->

    <owl:NamedIndividual rdf:about="http://purl.org/olia/susa.owl#NN1n">
        <rdf:type rdf:resource="http://purl.org/olia/susa.owl#CommonNoun"/>
        <hasNumber rdf:resource="http://purl.org/olia/susa.owl#singular"/>
        <olia_system:hasTag>NN1n</olia_system:hasTag>
        <olia_system:hasTier>POS</olia_system:hasTier>
        <rdfs:comment>This is a noun which can be used in a countable singular or as uncountable/ mass noun.</rdfs:comment>
    </owl:NamedIndividual>
    


    <!-- http://purl.org/olia/susa.owl#NN1u -->

    <owl:NamedIndividual rdf:about="http://purl.org/olia/susa.owl#NN1u">
        <rdf:type rdf:resource="http://purl.org/olia/susa.owl#CommonNoun"/>
        <hasCountability rdf:resource="http://purl.org/olia/susa.owl#uncountable"/>
        <olia_system:hasTag>NN1u</olia_system:hasTag>
        <olia_system:hasTier>POS</olia_system:hasTier>
        <rdfs:comment>This is a uncountable/ mass noun, e.g. &quot;snow&quot;, &quot;Buddhism&quot;.</rdfs:comment>
    </owl:NamedIndividual>
    


    <!-- http://purl.org/olia/susa.owl#NN1ux -->

    <owl:NamedIndividual rdf:about="http://purl.org/olia/susa.owl#NN1ux">
        <rdf:type rdf:resource="http://purl.org/olia/susa.owl#CommonNoun"/>
        <hasCountability rdf:resource="http://purl.org/olia/susa.owl#uncountable"/>
        <olia_system:hasTag>NN1ux</olia_system:hasTag>
        <olia_system:hasTier>POS</olia_system:hasTier>
        <rdfs:comment>This is a uncountable/ mass noun whch is ending on &quot;-ics&quot;, e.g. &quot;athletics&quot;, &quot;thermodynamics&quot;.</rdfs:comment>
    </owl:NamedIndividual>
    


    <!-- http://purl.org/olia/susa.owl#NN2 -->

    <owl:NamedIndividual rdf:about="http://purl.org/olia/susa.owl#NN2">
        <rdf:type rdf:resource="http://purl.org/olia/susa.owl#CommonNoun"/>
        <hasNumber rdf:resource="http://purl.org/olia/susa.owl#plural"/>
        <olia_system:hasTag>NN2</olia_system:hasTag>
        <olia_system:hasTier>POS</olia_system:hasTier>
        <rdfs:comment>This is a common noun in plural.</rdfs:comment>
    </owl:NamedIndividual>
    


    <!-- http://purl.org/olia/susa.owl#NNJ -->

    <owl:NamedIndividual rdf:about="http://purl.org/olia/susa.owl#NNJ">
        <rdf:type rdf:resource="http://purl.org/olia/susa.owl#OrganizationNoun"/>
        <olia_system:hasTag>NNJ</olia_system:hasTag>
        <olia_system:hasTier>POS</olia_system:hasTier>
        <rdfs:comment>NNJ is used for a noun which appears only as a desciptive head of an organisation name, e.g. &quot;Corp&quot;, &quot;Bros&quot;. Singular or plural is possible.</rdfs:comment>
    </owl:NamedIndividual>
    


    <!-- http://purl.org/olia/susa.owl#NNJ1 -->

    <owl:NamedIndividual rdf:about="http://purl.org/olia/susa.owl#NNJ1">
        <rdf:type rdf:resource="http://purl.org/olia/susa.owl#OrganizationNoun"/>
        <hasNumber rdf:resource="http://purl.org/olia/susa.owl#singular"/>
        <olia_system:hasTag>NNJ1</olia_system:hasTag>
        <olia_system:hasTier>POS</olia_system:hasTier>
        <rdfs:comment>NNJ1 is used for organization nouns in singular.</rdfs:comment>
        <owl:versionInfo>added by Johannes Bubenzer (2006-09-09) in accordance to a
	TnT-tagged data set provided by SFB 538 (Hamburg), project K4</owl:versionInfo>
    </owl:NamedIndividual>
    


    <!-- http://purl.org/olia/susa.owl#NNJ1c -->

    <owl:NamedIndividual rdf:about="http://purl.org/olia/susa.owl#NNJ1c">
        <rdf:type rdf:resource="http://purl.org/olia/susa.owl#OrganizationNoun"/>
        <hasCountability rdf:resource="http://purl.org/olia/susa.owl#countable"/>
        <hasNumber rdf:resource="http://purl.org/olia/susa.owl#singular"/>
        <olia_system:hasTag>NNJ1c</olia_system:hasTag>
        <olia_system:hasTier>POS</olia_system:hasTier>
        <rdfs:comment>This is a noun which appears as a countable singular and is a desciptive head of an organisation name</rdfs:comment>
    </owl:NamedIndividual>
    


    <!-- http://purl.org/olia/susa.owl#NNJ1n -->

    <owl:NamedIndividual rdf:about="http://purl.org/olia/susa.owl#NNJ1n">
        <rdf:type rdf:resource="http://purl.org/olia/susa.owl#OrganizationNoun"/>
        <hasNumber rdf:resource="http://purl.org/olia/susa.owl#singular"/>
        <olia_system:hasTag>NNJ1n</olia_system:hasTag>
        <olia_system:hasTier>POS</olia_system:hasTier>
        <rdfs:comment>NNJ1n is used for nouns which can be uncountable (&quot;mass&quot;), a countable singular and a descriptive head of an organisation name, e.g. &quot;company&quot;, &quot;organization&quot;.</rdfs:comment>
    </owl:NamedIndividual>
    


    <!-- http://purl.org/olia/susa.owl#NNJ2 -->

    <owl:NamedIndividual rdf:about="http://purl.org/olia/susa.owl#NNJ2">
        <rdf:type rdf:resource="http://purl.org/olia/susa.owl#OrganizationNoun"/>
        <hasNumber rdf:resource="http://purl.org/olia/susa.owl#plural"/>
        <olia_system:hasTag>NNJ2</olia_system:hasTag>
        <olia_system:hasTier>POS</olia_system:hasTier>
        <rdfs:comment>NNJ2 is used for plural descriptive heads of an organisation name, e.g. &quot;associates&quot;.</rdfs:comment>
    </owl:NamedIndividual>
    


    <!-- http://purl.org/olia/susa.owl#NNL -->

    <owl:NamedIndividual rdf:about="http://purl.org/olia/susa.owl#NNL">
        <rdf:type rdf:resource="http://purl.org/olia/susa.owl#TopographicalNoun"/>
        <olia_system:hasTag>NNL</olia_system:hasTag>
        <olia_system:hasTier>POS</olia_system:hasTier>
        <rdfs:comment>NNL is used for descriptive head of place-name items in singular or plural, e.g. &quot;Rd&quot;, &quot;Is&quot;.</rdfs:comment>
    </owl:NamedIndividual>
    


    <!-- http://purl.org/olia/susa.owl#NNL1 -->

    <owl:NamedIndividual rdf:about="http://purl.org/olia/susa.owl#NNL1">
        <rdf:type rdf:resource="http://purl.org/olia/susa.owl#TopographicalNoun"/>
        <hasNumber rdf:resource="http://purl.org/olia/susa.owl#singular"/>
        <olia_system:hasTag>NNL1</olia_system:hasTag>
        <olia_system:hasTier>POS</olia_system:hasTier>
        <rdfs:comment>NNL1 is used for topographical nouns in singular.</rdfs:comment>
        <owl:versionInfo>added by Johannes Bubenzer (2006-09-09) according to a TnT-tagged 
	dataset provided by SFB 538 (Hamburg), project K4.</owl:versionInfo>
    </owl:NamedIndividual>
    


    <!-- http://purl.org/olia/susa.owl#NNL1c -->

    <owl:NamedIndividual rdf:about="http://purl.org/olia/susa.owl#NNL1c">
        <rdf:type rdf:resource="http://purl.org/olia/susa.owl#TopographicalNoun"/>
        <hasCountability rdf:resource="http://purl.org/olia/susa.owl#countable"/>
        <hasNumber rdf:resource="http://purl.org/olia/susa.owl#singular"/>
        <olia_system:hasTag>NNL1c</olia_system:hasTag>
        <olia_system:hasTier>POS</olia_system:hasTier>
        <rdfs:comment>NNL1c is used for descriptive heads of place-name in countable singular, e.g. &quot;road&quot;, &quot;island&quot;.</rdfs:comment>
    </owl:NamedIndividual>
    


    <!-- http://purl.org/olia/susa.owl#NNL1cb -->

    <owl:NamedIndividual rdf:about="http://purl.org/olia/susa.owl#NNL1cb">
        <rdf:type rdf:resource="http://purl.org/olia/susa.owl#TopographicalNoun"/>
        <hasCountability rdf:resource="http://purl.org/olia/susa.owl#countable"/>
        <hasNumber rdf:resource="http://purl.org/olia/susa.owl#singular"/>
        <olia_system:hasTag>NNL1cb</olia_system:hasTag>
        <olia_system:hasTier>POS</olia_system:hasTier>
        <rdfs:comment>NNL1cb is used for descriptive heads of place-name in countable singular with tendency to precede the specific name, e.g. &quot;camp&quot;, &quot;lake&quot;, &quot;mount&quot;.</rdfs:comment>
    </owl:NamedIndividual>
    


    <!-- http://purl.org/olia/susa.owl#NNL1n -->

    <owl:NamedIndividual rdf:about="http://purl.org/olia/susa.owl#NNL1n">
        <rdf:type rdf:resource="http://purl.org/olia/susa.owl#TopographicalNoun"/>
        <hasNumber rdf:resource="http://purl.org/olia/susa.owl#singular"/>
        <olia_system:hasTag>NNL1n</olia_system:hasTag>
        <olia_system:hasTier>POS</olia_system:hasTier>
        <rdfs:comment>NNL1n  is used for descriptive heads of place-name in countable singular or uncountable mass nouns, e.g. &quot;drive&quot;, &quot;water&quot;, &quot;green&quot;.</rdfs:comment>
    </owl:NamedIndividual>
    


    <!-- http://purl.org/olia/susa.owl#NNL2 -->

    <owl:NamedIndividual rdf:about="http://purl.org/olia/susa.owl#NNL2">
        <rdf:type rdf:resource="http://purl.org/olia/susa.owl#TopographicalNoun"/>
        <hasNumber rdf:resource="http://purl.org/olia/susa.owl#plural"/>
        <olia_system:hasTag>NNL2</olia_system:hasTag>
        <olia_system:hasTier>POS</olia_system:hasTier>
        <rdfs:comment>NNL2 is used for descriptive heads of place-name in plural, e.g. &quot;buildings&quot;, &quot;montains&quot;.</rdfs:comment>
    </owl:NamedIndividual>
    


    <!-- http://purl.org/olia/susa.owl#NNLb -->

    <owl:NamedIndividual rdf:about="http://purl.org/olia/susa.owl#NNLb">
        <rdf:type rdf:resource="http://purl.org/olia/susa.owl#TopographicalNoun"/>
        <olia_system:hasTag>NNLb</olia_system:hasTag>
        <olia_system:hasTier>POS</olia_system:hasTier>
        <rdfs:comment>NNLb are descriptive heads of place-name nouns with tendency to precede the specific name &quot;Costa&quot;.</rdfs:comment>
    </owl:NamedIndividual>
    


    <!-- http://purl.org/olia/susa.owl#NNLc -->

    <owl:NamedIndividual rdf:about="http://purl.org/olia/susa.owl#NNLc">
        <rdf:type rdf:resource="http://purl.org/olia/susa.owl#TopographicalNoun"/>
        <hasCountability rdf:resource="http://purl.org/olia/susa.owl#countable"/>
        <olia_system:hasTag>NNLc</olia_system:hasTag>
        <olia_system:hasTier>POS</olia_system:hasTier>
        <rdfs:comment>NNLc is used for descriptive heads of place-name in countable singular or plural, e.g. &quot;barracks&quot;, &quot;links&quot;.</rdfs:comment>
    </owl:NamedIndividual>
    


    <!-- http://purl.org/olia/susa.owl#NNO -->

    <owl:NamedIndividual rdf:about="http://purl.org/olia/susa.owl#NNO">
        <rdf:type rdf:resource="http://purl.org/olia/susa.owl#CommonNoun"/>
        <olia_system:hasTag>NNO</olia_system:hasTag>
        <olia_system:hasTier>POS</olia_system:hasTier>
    </owl:NamedIndividual>
    


    <!-- http://purl.org/olia/susa.owl#NNOc -->

    <owl:NamedIndividual rdf:about="http://purl.org/olia/susa.owl#NNOc">
        <rdf:type rdf:resource="http://purl.org/olia/susa.owl#CommonNoun"/>
        <olia_system:hasTag>NNOc</olia_system:hasTag>
        <olia_system:hasTier>POS</olia_system:hasTier>
        <rdfs:comment>NNOc is used for e.g. &quot;dozen&quot;, &quot;score&quot;, &quot;gross&quot; etc. .</rdfs:comment>
    </owl:NamedIndividual>
    


    <!-- http://purl.org/olia/susa.owl#NNOn -->

    <owl:NamedIndividual rdf:about="http://purl.org/olia/susa.owl#NNOn">
        <rdf:type rdf:resource="http://purl.org/olia/susa.owl#CommonNoun"/>
        <olia_system:hasTag>NNOn</olia_system:hasTag>
        <olia_system:hasTier>POS</olia_system:hasTier>
        <rdfs:comment>NNOn is used for abbreviated NNOc words and is ambiguous between singular and plural, e.g. &quot;m&quot; for million(s).</rdfs:comment>
    </owl:NamedIndividual>
    


    <!-- http://purl.org/olia/susa.owl#NNS -->

    <owl:NamedIndividual rdf:about="http://purl.org/olia/susa.owl#NNS">
        <rdf:type rdf:resource="http://purl.org/olia/susa.owl#Title"/>
        <hasNumber rdf:resource="http://purl.org/olia/susa.owl#singular"/>
        <olia_system:hasTag>NNS</olia_system:hasTag>
        <olia_system:hasTier>POS</olia_system:hasTier>
        <rdfs:comment>NNS is used for nouns of style or title in singular, e.g. &quot;Mr&quot;, &quot;Mrs&quot;, &quot;Dr&quot;.</rdfs:comment>
    </owl:NamedIndividual>
    


    <!-- http://purl.org/olia/susa.owl#NNS1 -->

    <owl:NamedIndividual rdf:about="http://purl.org/olia/susa.owl#NNS1">
        <rdf:type rdf:resource="http://purl.org/olia/susa.owl#Title"/>
        <hasNumber rdf:resource="http://purl.org/olia/susa.owl#singular"/>
        <olia_system:hasTag>NNS1</olia_system:hasTag>
        <olia_system:hasTier>POS</olia_system:hasTier>
        <rdfs:comment>NNS1 is used for title nouns in singular.</rdfs:comment>
    </owl:NamedIndividual>
    


    <!-- http://purl.org/olia/susa.owl#NNS1c -->

    <owl:NamedIndividual rdf:about="http://purl.org/olia/susa.owl#NNS1c">
        <rdf:type rdf:resource="http://purl.org/olia/susa.owl#Title"/>
        <hasCountability rdf:resource="http://purl.org/olia/susa.owl#countable"/>
        <hasNumber rdf:resource="http://purl.org/olia/susa.owl#singular"/>
        <olia_system:hasTag>NNS1c</olia_system:hasTag>
        <olia_system:hasTier>POS</olia_system:hasTier>
        <rdfs:comment>NNS1c is used for nouns of style or title in countable singular &quot;doctor&quot;, &quot;miss&quot;, &quot;madam&quot;.</rdfs:comment>
    </owl:NamedIndividual>
    


    <!-- http://purl.org/olia/susa.owl#NNS1n -->

    <owl:NamedIndividual rdf:about="http://purl.org/olia/susa.owl#NNS1n">
        <rdf:type rdf:resource="http://purl.org/olia/susa.owl#Title"/>
        <hasNumber rdf:resource="http://purl.org/olia/susa.owl#singular"/>
        <olia_system:hasTag>NNS1n</olia_system:hasTag>
        <olia_system:hasTier>POS</olia_system:hasTier>
        <rdfs:comment>NNS1n is used for nouns of style or title in countable singular or uncountable mass noun, e.g. &quot;justice&quot;.</rdfs:comment>
    </owl:NamedIndividual>
    


    <!-- http://purl.org/olia/susa.owl#NNS2 -->

    <owl:NamedIndividual rdf:about="http://purl.org/olia/susa.owl#NNS2">
        <rdf:type rdf:resource="http://purl.org/olia/susa.owl#Title"/>
        <hasNumber rdf:resource="http://purl.org/olia/susa.owl#plural"/>
        <olia_system:hasTag>NNS2</olia_system:hasTag>
        <olia_system:hasTier>POS</olia_system:hasTier>
        <rdfs:comment>NNS2  is used for nouns of style or title in plural, e.g. &quot;doctors&quot;.</rdfs:comment>
    </owl:NamedIndividual>
    


    <!-- http://purl.org/olia/susa.owl#NNSA -->

    <owl:NamedIndividual rdf:about="http://purl.org/olia/susa.owl#NNSA">
        <rdf:type rdf:resource="http://purl.org/olia/susa.owl#Title"/>
        <olia_system:hasTag>NNSA</olia_system:hasTag>
        <olia_system:hasTier>POS</olia_system:hasTier>
        <rdfs:comment>NNSA is used for an item of style or title fllowing name, with or without a countable singular use, e.g. &quot;Jr&quot;, &quot;Sr&quot;.</rdfs:comment>
    </owl:NamedIndividual>
    


    <!-- http://purl.org/olia/susa.owl#NNSS -->

    <owl:NamedIndividual rdf:about="http://purl.org/olia/susa.owl#NNSS">
        <rdf:type rdf:resource="http://purl.org/olia/susa.owl#Title"/>
        <hasNumber rdf:resource="http://purl.org/olia/susa.owl#plural"/>
        <olia_system:hasTag>NNSS</olia_system:hasTag>
        <olia_system:hasTier>POS</olia_system:hasTier>
        <rdfs:comment>NNSS is used for style or title-only adjectival items in plural, e.g. &quot;Messrs&quot;, &quot;Mmes&quot;.</rdfs:comment>
    </owl:NamedIndividual>
    


    <!-- http://purl.org/olia/susa.owl#NNSj -->

    <owl:NamedIndividual rdf:about="http://purl.org/olia/susa.owl#NNSj">
        <rdf:type rdf:resource="http://purl.org/olia/susa.owl#Title"/>
        <olia_system:hasTag>NNSj</olia_system:hasTag>
        <olia_system:hasTier>POS</olia_system:hasTier>
        <rdfs:comment>NNSj is used for style or title-only adjectival items, e.g &quot;Rev&quot;, &quot;Very Rev&quot;.</rdfs:comment>
    </owl:NamedIndividual>
    


    <!-- http://purl.org/olia/susa.owl#NNT1 -->

    <owl:NamedIndividual rdf:about="http://purl.org/olia/susa.owl#NNT1">
        <rdf:type rdf:resource="http://purl.org/olia/susa.owl#TemporalNoun"/>
        <hasNumber rdf:resource="http://purl.org/olia/susa.owl#singular"/>
        <olia_system:hasTag>NNT1</olia_system:hasTag>
        <olia_system:hasTier>POS</olia_system:hasTier>
        <rdfs:comment>NNT1 is sued for temporal nouns in singular.</rdfs:comment>
        <owl:versionInfo>added by Johannes Bubenzer (2006-09-09) in accordance to a
	TnT-tagged data set provided by SFB 538 (Hamburg), project K4</owl:versionInfo>
    </owl:NamedIndividual>
    


    <!-- http://purl.org/olia/susa.owl#NNT1c -->

    <owl:NamedIndividual rdf:about="http://purl.org/olia/susa.owl#NNT1c">
        <rdf:type rdf:resource="http://purl.org/olia/susa.owl#TemporalNoun"/>
        <hasNumber rdf:resource="http://purl.org/olia/susa.owl#singular"/>
        <olia_system:hasTag>NNT1c</olia_system:hasTag>
        <olia_system:hasTier>POS</olia_system:hasTier>
        <rdfs:comment>NNT1c is for a singular time noun that can head a noun phrase functioning adverbially, e.g. &quot;hour&quot;, &quot;day&quot;, &quot;evening&quot;.</rdfs:comment>
    </owl:NamedIndividual>
    


    <!-- http://purl.org/olia/susa.owl#NNT1h -->

    <owl:NamedIndividual rdf:about="http://purl.org/olia/susa.owl#NNT1h">
        <rdf:type rdf:resource="http://purl.org/olia/susa.owl#TemporalNoun"/>
        <hasNumber rdf:resource="http://purl.org/olia/susa.owl#singular"/>
        <olia_system:hasTag>NNT1h</olia_system:hasTag>
        <olia_system:hasTier>POS</olia_system:hasTier>
        <rdfs:comment>NNT1h is the tag for holiday or season, e.g. &quot;Christmas&quot;, &quot;Boxing Day&quot;.</rdfs:comment>
    </owl:NamedIndividual>
    


    <!-- http://purl.org/olia/susa.owl#NNT1m -->

    <owl:NamedIndividual rdf:about="http://purl.org/olia/susa.owl#NNT1m">
        <rdf:type rdf:resource="http://purl.org/olia/susa.owl#TemporalNoun"/>
        <hasNumber rdf:resource="http://purl.org/olia/susa.owl#singular"/>
        <olia_system:hasTag>NNT1m</olia_system:hasTag>
        <olia_system:hasTier>POS</olia_system:hasTier>
        <rdfs:comment>NNT1m is used for a point-of-time noun, which cannot head a noun phrase functioning adverbially, e.g. &quot;noon&quot;, &quot;midnight&quot;, &quot;midyear&quot;.</rdfs:comment>
    </owl:NamedIndividual>
    


    <!-- http://purl.org/olia/susa.owl#NNT2 -->

    <owl:NamedIndividual rdf:about="http://purl.org/olia/susa.owl#NNT2">
        <rdf:type rdf:resource="http://purl.org/olia/susa.owl#TemporalNoun"/>
        <hasNumber rdf:resource="http://purl.org/olia/susa.owl#plural"/>
        <olia_system:hasTag>NNT2</olia_system:hasTag>
        <olia_system:hasTier>POS</olia_system:hasTier>
        <rdfs:comment>NNT2 stands for the plural of NNT1.. nouns.</rdfs:comment>
    </owl:NamedIndividual>
    


    <!-- http://purl.org/olia/susa.owl#NNU -->

    <owl:NamedIndividual rdf:about="http://purl.org/olia/susa.owl#NNU">
        <rdf:type rdf:resource="http://purl.org/olia/susa.owl#UnitNoun"/>
        <hasNumber rdf:resource="http://purl.org/olia/susa.owl#plural"/>
        <hasNumber rdf:resource="http://purl.org/olia/susa.owl#singular"/>
        <olia_system:hasTag>NNU</olia_system:hasTag>
        <olia_system:hasTier>POS</olia_system:hasTier>
        <rdfs:comment>NNU is used for unit-only nouns in singular, plural, or neutral.</rdfs:comment>
    </owl:NamedIndividual>
    


    <!-- http://purl.org/olia/susa.owl#NNU1 -->

    <owl:NamedIndividual rdf:about="http://purl.org/olia/susa.owl#NNU1">
        <rdf:type rdf:resource="http://purl.org/olia/susa.owl#UnitNoun"/>
        <hasNumber rdf:resource="http://purl.org/olia/susa.owl#singular"/>
        <olia_system:hasTag>NNU1</olia_system:hasTag>
        <olia_system:hasTier>POS</olia_system:hasTier>
        <rdfs:comment>NNU1 is used for unit nouns in singular.</rdfs:comment>
    </owl:NamedIndividual>
    


    <!-- http://purl.org/olia/susa.owl#NNU1c -->

    <owl:NamedIndividual rdf:about="http://purl.org/olia/susa.owl#NNU1c">
        <rdf:type rdf:resource="http://purl.org/olia/susa.owl#UnitNoun"/>
        <hasCountability rdf:resource="http://purl.org/olia/susa.owl#countable"/>
        <hasNumber rdf:resource="http://purl.org/olia/susa.owl#singular"/>
        <olia_system:hasTag>NNU1c</olia_system:hasTag>
        <olia_system:hasTier>POS</olia_system:hasTier>
        <rdfs:comment>NNU1c is the tag for unit countable nouns in singular e.g. &quot;inch&quot;, &quot;kilogram&quot;.</rdfs:comment>
    </owl:NamedIndividual>
    


    <!-- http://purl.org/olia/susa.owl#NNU1n -->

    <owl:NamedIndividual rdf:about="http://purl.org/olia/susa.owl#NNU1n">
        <rdf:type rdf:resource="http://purl.org/olia/susa.owl#UnitNoun"/>
        <hasNumber rdf:resource="http://purl.org/olia/susa.owl#singular"/>
        <olia_system:hasTag>NNU1n</olia_system:hasTag>
        <olia_system:hasTier>POS</olia_system:hasTier>
        <rdfs:comment>NNU1n is used for unit nouns which can be used in countable singular or as uncountable  mass noun e.g. &quot;metre&quot;.</rdfs:comment>
    </owl:NamedIndividual>
    


    <!-- http://purl.org/olia/susa.owl#NNU2 -->

    <owl:NamedIndividual rdf:about="http://purl.org/olia/susa.owl#NNU2">
        <rdf:type rdf:resource="http://purl.org/olia/susa.owl#UnitNoun"/>
        <hasNumber rdf:resource="http://purl.org/olia/susa.owl#plural"/>
        <olia_system:hasTag>NNU2</olia_system:hasTag>
        <olia_system:hasTier>POS</olia_system:hasTier>
        <rdfs:comment>NNU2 is the tag for unit  nouns in plural, e.g. &quot;inches&quot;.</rdfs:comment>
    </owl:NamedIndividual>
    


    <!-- http://purl.org/olia/susa.owl#NNUb -->

    <owl:NamedIndividual rdf:about="http://purl.org/olia/susa.owl#NNUb">
        <rdf:type rdf:resource="http://purl.org/olia/susa.owl#UnitNoun"/>
        <olia_system:hasTag>NNUb</olia_system:hasTag>
        <olia_system:hasTier>POS</olia_system:hasTier>
        <rdfs:comment>NNUb is used for a unit symbol which precedes numerals, e.g. &quot;$&quot;.</rdfs:comment>
    </owl:NamedIndividual>
    


    <!-- http://purl.org/olia/susa.owl#NNUc -->

    <owl:NamedIndividual rdf:about="http://purl.org/olia/susa.owl#NNUc">
        <rdf:type rdf:resource="http://purl.org/olia/susa.owl#UnitNoun"/>
        <hasCountability rdf:resource="http://purl.org/olia/susa.owl#countable"/>
        <olia_system:hasTag>NNUc</olia_system:hasTag>
        <olia_system:hasTier>POS</olia_system:hasTier>
        <rdfs:comment>NNUc is used for unit nouns which can stand in countable singular or in plural, e.g. &quot;hertz&quot;, &quot;yen&quot;.</rdfs:comment>
    </owl:NamedIndividual>
    


    <!-- http://purl.org/olia/susa.owl#NNUn -->

    <owl:NamedIndividual rdf:about="http://purl.org/olia/susa.owl#NNUn">
        <rdf:type rdf:resource="http://purl.org/olia/susa.owl#UnitNoun"/>
        <olia_system:hasTag>NNUn</olia_system:hasTag>
        <olia_system:hasTier>POS</olia_system:hasTier>
        <rdfs:comment>NNUn is used unit nouns which can be used as countable singular,  plural or as uncountable mass noun.</rdfs:comment>
    </owl:NamedIndividual>
    


    <!-- http://purl.org/olia/susa.owl#NNUp -->

    <owl:NamedIndividual rdf:about="http://purl.org/olia/susa.owl#NNUp">
        <rdf:type rdf:resource="http://purl.org/olia/susa.owl#UnitNoun"/>
        <olia_system:hasTag>NNUp</olia_system:hasTag>
        <olia_system:hasTier>POS</olia_system:hasTier>
        <rdfs:comment>NNUp is used for &quot;%&quot;, &quot;percent&quot;, &quot;per cent&quot;.</rdfs:comment>
    </owl:NamedIndividual>
    


    <!-- http://purl.org/olia/susa.owl#NNa -->

    <owl:NamedIndividual rdf:about="http://purl.org/olia/susa.owl#NNa">
        <rdf:type rdf:resource="http://purl.org/olia/susa.owl#CommonNoun"/>
        <olia_system:hasTag>NNa</olia_system:hasTag>
        <olia_system:hasTier>POS</olia_system:hasTier>
        <rdfs:comment>This is the time of the day written digitally, e.g. &quot;10:30&quot;, &quot;10.30&quot;.</rdfs:comment>
    </owl:NamedIndividual>
    


    <!-- http://purl.org/olia/susa.owl#NNb -->

    <owl:NamedIndividual rdf:about="http://purl.org/olia/susa.owl#NNb">
        <rdf:type rdf:resource="http://purl.org/olia/susa.owl#CommonNoun"/>
        <olia_system:hasTag>NNb</olia_system:hasTag>
        <olia_system:hasTier>POS</olia_system:hasTier>
        <rdfs:comment>THis is an attributive common noun, e.g. &quot;scissor&quot;, &quot;trouser&quot;</rdfs:comment>
    </owl:NamedIndividual>
    


    <!-- http://purl.org/olia/susa.owl#NNc -->

    <owl:NamedIndividual rdf:about="http://purl.org/olia/susa.owl#NNc">
        <rdf:type rdf:resource="http://purl.org/olia/susa.owl#CommonNoun"/>
        <hasCountability rdf:resource="http://purl.org/olia/susa.owl#countable"/>
        <olia_system:hasTag>NNc</olia_system:hasTag>
        <olia_system:hasTier>POS</olia_system:hasTier>
        <rdfs:comment>This is a noun which can appear in a countable singular or in plural, e.g. &quot;sheep&quot;, &quot;species&quot;, &quot;people&quot;.</rdfs:comment>
    </owl:NamedIndividual>
    


    <!-- http://purl.org/olia/susa.owl#NNm -->

    <owl:NamedIndividual rdf:about="http://purl.org/olia/susa.owl#NNm">
        <rdf:type rdf:resource="http://purl.org/olia/susa.owl#CommonNoun"/>
        <hasNumber rdf:resource="http://purl.org/olia/susa.owl#singular"/>
        <olia_system:hasTag>NNm</olia_system:hasTag>
        <olia_system:hasTier>POS</olia_system:hasTier>
        <rdfs:comment>NNm is the tag for a singular abbreviation normally followed by a numeral functioning as a proper name e.g. &quot;Fig.&quot;, &quot;No.&quot;.</rdfs:comment>
    </owl:NamedIndividual>
    


    <!-- http://purl.org/olia/susa.owl#NNmm -->

    <owl:NamedIndividual rdf:about="http://purl.org/olia/susa.owl#NNmm">
        <rdf:type rdf:resource="http://purl.org/olia/susa.owl#CommonNoun"/>
        <hasNumber rdf:resource="http://purl.org/olia/susa.owl#plural"/>
        <olia_system:hasTag>NNmm</olia_system:hasTag>
        <olia_system:hasTier>POS</olia_system:hasTier>
        <rdfs:comment>NNmm stands for the plural of NNm abbreviation, e.g. &quot;Figs.&quot;, &quot;Nos.&quot;.</rdfs:comment>
    </owl:NamedIndividual>
    


    <!-- http://purl.org/olia/susa.owl#NNn -->

    <owl:NamedIndividual rdf:about="http://purl.org/olia/susa.owl#NNn">
        <rdf:type rdf:resource="http://purl.org/olia/susa.owl#CommonNoun"/>
        <olia_system:hasTag>NNn</olia_system:hasTag>
        <olia_system:hasTier>POS</olia_system:hasTier>
        <rdfs:comment>NNn is used  for nouns which can be uncountable (&quot;mass&quot;), countable singular or plural, e.g &quot;fish&quot; (a fish, three fish, a piece of fish), &quot;Chinese (a Chinese, three Chinese, Chinese is tonal)&quot; .</rdfs:comment>
    </owl:NamedIndividual>
    


    <!-- http://purl.org/olia/susa.owl#NNp -->

    <owl:NamedIndividual rdf:about="http://purl.org/olia/susa.owl#NNp">
        <rdf:type rdf:resource="http://purl.org/olia/susa.owl#CommonNoun"/>
        <olia_system:hasTag>NNp</olia_system:hasTag>
        <olia_system:hasTier>POS</olia_system:hasTier>
        <rdfs:comment>NNp is the tag for the time of a day written digitally in 24-hour notation from 13:00 on, e.g. &quot;13:30&quot;.</rdfs:comment>
    </owl:NamedIndividual>
    


    <!-- http://purl.org/olia/susa.owl#NNu -->

    <owl:NamedIndividual rdf:about="http://purl.org/olia/susa.owl#NNu">
        <rdf:type rdf:resource="http://purl.org/olia/susa.owl#CommonNoun"/>
        <hasCountability rdf:resource="http://purl.org/olia/susa.owl#uncountable"/>
        <hasNumber rdf:resource="http://purl.org/olia/susa.owl#plural"/>
        <olia_system:hasTag>NNu</olia_system:hasTag>
        <olia_system:hasTier>POS</olia_system:hasTier>
        <rdfs:comment>NNu is the tag for plural mass nouns e.g. &quot;data&quot;, &quot;measles&quot;.</rdfs:comment>
    </owl:NamedIndividual>
    


    <!-- http://purl.org/olia/susa.owl#NNux -->

    <owl:NamedIndividual rdf:about="http://purl.org/olia/susa.owl#NNux">
        <rdf:type rdf:resource="http://purl.org/olia/susa.owl#CommonNoun"/>
        <hasCountability rdf:resource="http://purl.org/olia/susa.owl#uncountable"/>
        <hasNumber rdf:resource="http://purl.org/olia/susa.owl#plural"/>
        <olia_system:hasTag>NNux</olia_system:hasTag>
        <olia_system:hasTier>POS</olia_system:hasTier>
        <rdfs:comment>NNux is used for plural mass nouns in &quot;-ics&quot;, e.g. &quot;mechanics&quot;.</rdfs:comment>
    </owl:NamedIndividual>
    


    <!-- http://purl.org/olia/susa.owl#NP -->

    <owl:NamedIndividual rdf:about="http://purl.org/olia/susa.owl#NP">
        <rdf:type rdf:resource="http://purl.org/olia/susa.owl#ProperNoun"/>
        <olia_system:hasTag>NP</olia_system:hasTag>
        <olia_system:hasTier>POS</olia_system:hasTier>
        <rdfs:comment>These are proper nouns.</rdfs:comment>
    </owl:NamedIndividual>
    


    <!-- http://purl.org/olia/susa.owl#NP1 -->

    <owl:NamedIndividual rdf:about="http://purl.org/olia/susa.owl#NP1">
        <rdf:type rdf:resource="http://purl.org/olia/susa.owl#ProperNoun"/>
        <hasNumber rdf:resource="http://purl.org/olia/susa.owl#singular"/>
        <olia_system:hasTag>NP1</olia_system:hasTag>
        <olia_system:hasTier>POS</olia_system:hasTier>
        <rdfs:comment>These are singular proper names.</rdfs:comment>
    </owl:NamedIndividual>
    


    <!-- http://purl.org/olia/susa.owl#NP1c -->

    <owl:NamedIndividual rdf:about="http://purl.org/olia/susa.owl#NP1c">
        <rdf:type rdf:resource="http://purl.org/olia/susa.owl#ProperNoun"/>
        <hasNumber rdf:resource="http://purl.org/olia/susa.owl#singular"/>
        <olia_system:hasTag>NP1c</olia_system:hasTag>
        <olia_system:hasTier>POS</olia_system:hasTier>
        <rdfs:comment>NP1c is the used special tag for country names.</rdfs:comment>
    </owl:NamedIndividual>
    


    <!-- http://purl.org/olia/susa.owl#NP1f -->

    <owl:NamedIndividual rdf:about="http://purl.org/olia/susa.owl#NP1f">
        <rdf:type rdf:resource="http://purl.org/olia/susa.owl#ProperNoun"/>
        <hasGender rdf:resource="http://purl.org/olia/susa.owl#feminine"/>
        <hasNumber rdf:resource="http://purl.org/olia/susa.owl#singular"/>
        <olia_system:hasTag>NP1f</olia_system:hasTag>
        <olia_system:hasTier>POS</olia_system:hasTier>
        <rdfs:comment>NP1f tags a feminine forename.</rdfs:comment>
    </owl:NamedIndividual>
    


    <!-- http://purl.org/olia/susa.owl#NP1g -->

    <owl:NamedIndividual rdf:about="http://purl.org/olia/susa.owl#NP1g">
        <rdf:type rdf:resource="http://purl.org/olia/susa.owl#ProperNoun"/>
        <hasNumber rdf:resource="http://purl.org/olia/susa.owl#singular"/>
        <olia_system:hasTag>NP1g</olia_system:hasTag>
        <olia_system:hasTier>POS</olia_system:hasTier>
        <rdfs:comment>NP1g is used for miscellaneous singular geographical proper names, e.g. &quot;Adriatic&quot;, &quot;America&quot;, &quot;Sherwood&quot;.</rdfs:comment>
    </owl:NamedIndividual>
    


    <!-- http://purl.org/olia/susa.owl#NP1i -->

    <owl:NamedIndividual rdf:about="http://purl.org/olia/susa.owl#NP1i">
        <rdf:type rdf:resource="http://purl.org/olia/susa.owl#ProperNoun"/>
        <hasNumber rdf:resource="http://purl.org/olia/susa.owl#singular"/>
        <olia_system:hasTag>NP1i</olia_system:hasTag>
        <olia_system:hasTier>POS</olia_system:hasTier>
        <rdfs:comment>NP1i is the tag for intitials of personal names.</rdfs:comment>
    </owl:NamedIndividual>
    


    <!-- http://purl.org/olia/susa.owl#NP1j -->

    <owl:NamedIndividual rdf:about="http://purl.org/olia/susa.owl#NP1j">
        <rdf:type rdf:resource="http://purl.org/olia/susa.owl#ProperNoun"/>
        <hasNumber rdf:resource="http://purl.org/olia/susa.owl#singular"/>
        <olia_system:hasTag>NP1j</olia_system:hasTag>
        <olia_system:hasTier>POS</olia_system:hasTier>
        <rdfs:comment>NP1j stands for organization names, e.g. &quot;Unilever&quot;, &quot;Kiwanis&quot;.</rdfs:comment>
    </owl:NamedIndividual>
    


    <!-- http://purl.org/olia/susa.owl#NP1m -->

    <owl:NamedIndividual rdf:about="http://purl.org/olia/susa.owl#NP1m">
        <rdf:type rdf:resource="http://purl.org/olia/susa.owl#ProperNoun"/>
        <hasGender rdf:resource="http://purl.org/olia/susa.owl#masculine"/>
        <hasNumber rdf:resource="http://purl.org/olia/susa.owl#singular"/>
        <olia_system:hasTag>NP1m</olia_system:hasTag>
        <olia_system:hasTier>POS</olia_system:hasTier>
        <rdfs:comment>NP1m NP1f tags a masculine forename.</rdfs:comment>
    </owl:NamedIndividual>
    


    <!-- http://purl.org/olia/susa.owl#NP1p -->

    <owl:NamedIndividual rdf:about="http://purl.org/olia/susa.owl#NP1p">
        <rdf:type rdf:resource="http://purl.org/olia/susa.owl#ProperNoun"/>
        <hasNumber rdf:resource="http://purl.org/olia/susa.owl#singular"/>
        <olia_system:hasTag>NP1p</olia_system:hasTag>
        <olia_system:hasTier>POS</olia_system:hasTier>
        <rdfs:comment>NP1p is the SUSANNE tag used for &apos;province&apos; name, name of an US state, an English county etc. .</rdfs:comment>
    </owl:NamedIndividual>
    


    <!-- http://purl.org/olia/susa.owl#NP1s -->

    <owl:NamedIndividual rdf:about="http://purl.org/olia/susa.owl#NP1s">
        <rdf:type rdf:resource="http://purl.org/olia/susa.owl#ProperNoun"/>
        <hasNumber rdf:resource="http://purl.org/olia/susa.owl#singular"/>
        <olia_system:hasTag>NP1s</olia_system:hasTag>
        <olia_system:hasTier>POS</olia_system:hasTier>
        <rdfs:comment>NP1s is used for surnames.</rdfs:comment>
    </owl:NamedIndividual>
    


    <!-- http://purl.org/olia/susa.owl#NP1t -->

    <owl:NamedIndividual rdf:about="http://purl.org/olia/susa.owl#NP1t">
        <rdf:type rdf:resource="http://purl.org/olia/susa.owl#ProperNoun"/>
        <hasNumber rdf:resource="http://purl.org/olia/susa.owl#singular"/>
        <olia_system:hasTag>NP1t</olia_system:hasTag>
        <olia_system:hasTier>POS</olia_system:hasTier>
        <rdfs:comment>NP1t is the tag for a town name.</rdfs:comment>
    </owl:NamedIndividual>
    


    <!-- http://purl.org/olia/susa.owl#NP1x -->

    <owl:NamedIndividual rdf:about="http://purl.org/olia/susa.owl#NP1x">
        <rdf:type rdf:resource="http://purl.org/olia/susa.owl#ProperNoun"/>
        <hasNumber rdf:resource="http://purl.org/olia/susa.owl#singular"/>
        <olia_system:hasTag>NP1x</olia_system:hasTag>
        <olia_system:hasTier>POS</olia_system:hasTier>
        <rdfs:comment>NP1x  is used for miscellaneous singular proper name, e.g. &quot;Parthenon&quot;, &quot;Persil&quot;.</rdfs:comment>
    </owl:NamedIndividual>
    


    <!-- http://purl.org/olia/susa.owl#NP1z -->

    <owl:NamedIndividual rdf:about="http://purl.org/olia/susa.owl#NP1z">
        <rdf:type rdf:resource="http://purl.org/olia/susa.owl#ProperNoun"/>
        <hasNumber rdf:resource="http://purl.org/olia/susa.owl#singular"/>
        <olia_system:hasTag>NP1z</olia_system:hasTag>
        <olia_system:hasTier>POS</olia_system:hasTier>
        <rdfs:comment>NP1z is used for a &apos;code name&apos;, an acronym or arbitrary alphanumeric expression functioning as countable noun.</rdfs:comment>
    </owl:NamedIndividual>
    


    <!-- http://purl.org/olia/susa.owl#NP2 -->

    <owl:NamedIndividual rdf:about="http://purl.org/olia/susa.owl#NP2">
        <rdf:type rdf:resource="http://purl.org/olia/susa.owl#ProperNoun"/>
        <hasNumber rdf:resource="http://purl.org/olia/susa.owl#plural"/>
        <olia_system:hasTag>NP2</olia_system:hasTag>
        <olia_system:hasTier>POS</olia_system:hasTier>
        <rdfs:comment>These are plural proper names.</rdfs:comment>
    </owl:NamedIndividual>
    


    <!-- http://purl.org/olia/susa.owl#NP2c -->

    <owl:NamedIndividual rdf:about="http://purl.org/olia/susa.owl#NP2c">
        <rdf:type rdf:resource="http://purl.org/olia/susa.owl#ProperNoun"/>
        <hasNumber rdf:resource="http://purl.org/olia/susa.owl#plural"/>
        <olia_system:hasTag>NP2c</olia_system:hasTag>
        <olia_system:hasTier>POS</olia_system:hasTier>
        <rdfs:comment>NP2c stands for the plural of country names, e.g. &quot;the Philippines&quot;.</rdfs:comment>
    </owl:NamedIndividual>
    


    <!-- http://purl.org/olia/susa.owl#NP2f -->

    <owl:NamedIndividual rdf:about="http://purl.org/olia/susa.owl#NP2f">
        <rdf:type rdf:resource="http://purl.org/olia/susa.owl#ProperNoun"/>
        <hasGender rdf:resource="http://purl.org/olia/susa.owl#feminine"/>
        <hasNumber rdf:resource="http://purl.org/olia/susa.owl#plural"/>
        <olia_system:hasTag>NP2f</olia_system:hasTag>
        <olia_system:hasTier>POS</olia_system:hasTier>
        <rdfs:comment>NP2f is used for plural feminine forenames.</rdfs:comment>
    </owl:NamedIndividual>
    


    <!-- http://purl.org/olia/susa.owl#NP2g -->

    <owl:NamedIndividual rdf:about="http://purl.org/olia/susa.owl#NP2g">
        <rdf:type rdf:resource="http://purl.org/olia/susa.owl#ProperNoun"/>
        <hasNumber rdf:resource="http://purl.org/olia/susa.owl#plural"/>
        <olia_system:hasTag>NP2g</olia_system:hasTag>
        <olia_system:hasTier>POS</olia_system:hasTier>
        <rdfs:comment>NP2g is used for miscellaneous plural geographical proper names, e.g. &quot;Alps&quot;, &quot;Americas&quot;, &quot;Antilles&quot;.</rdfs:comment>
    </owl:NamedIndividual>
    


    <!-- http://purl.org/olia/susa.owl#NP2j -->

    <owl:NamedIndividual rdf:about="http://purl.org/olia/susa.owl#NP2j">
        <rdf:type rdf:resource="http://purl.org/olia/susa.owl#ProperNoun"/>
        <hasNumber rdf:resource="http://purl.org/olia/susa.owl#plural"/>
        <olia_system:hasTag>NP2j</olia_system:hasTag>
        <olia_system:hasTier>POS</olia_system:hasTier>
        <rdfs:comment>NP2j is the SUSANNE tag used for plural organization names, e.g. &quot;ICP&apos;s&quot;, &quot;Unilevers&quot;.</rdfs:comment>
    </owl:NamedIndividual>
    


    <!-- http://purl.org/olia/susa.owl#NP2m -->

    <owl:NamedIndividual rdf:about="http://purl.org/olia/susa.owl#NP2m">
        <rdf:type rdf:resource="http://purl.org/olia/susa.owl#ProperNoun"/>
        <hasGender rdf:resource="http://purl.org/olia/susa.owl#masculine"/>
        <hasNumber rdf:resource="http://purl.org/olia/susa.owl#plural"/>
        <olia_system:hasTag>NP2m</olia_system:hasTag>
        <olia_system:hasTier>POS</olia_system:hasTier>
        <rdfs:comment>NP2m tags plural masculine forenames.</rdfs:comment>
    </owl:NamedIndividual>
    


    <!-- http://purl.org/olia/susa.owl#NP2p -->

    <owl:NamedIndividual rdf:about="http://purl.org/olia/susa.owl#NP2p">
        <rdf:type rdf:resource="http://purl.org/olia/susa.owl#ProperNoun"/>
        <hasNumber rdf:resource="http://purl.org/olia/susa.owl#plural"/>
        <olia_system:hasTag>NP2p</olia_system:hasTag>
        <olia_system:hasTier>POS</olia_system:hasTier>
        <rdfs:comment>NP2p is the SUSANNE tag used for plural province names, e.g. &quot;Carolinas&quot;.</rdfs:comment>
    </owl:NamedIndividual>
    


    <!-- http://purl.org/olia/susa.owl#NP2s -->

    <owl:NamedIndividual rdf:about="http://purl.org/olia/susa.owl#NP2s">
        <rdf:type rdf:resource="http://purl.org/olia/susa.owl#ProperNoun"/>
        <hasNumber rdf:resource="http://purl.org/olia/susa.owl#plural"/>
        <olia_system:hasTag>NP2s</olia_system:hasTag>
        <olia_system:hasTier>POS</olia_system:hasTier>
        <rdfs:comment>NP2s describes plural surnames, as in the &quot;Robinsons&quot;.</rdfs:comment>
    </owl:NamedIndividual>
    


    <!-- http://purl.org/olia/susa.owl#NP2t -->

    <owl:NamedIndividual rdf:about="http://purl.org/olia/susa.owl#NP2t">
        <rdf:type rdf:resource="http://purl.org/olia/susa.owl#ProperNoun"/>
        <hasNumber rdf:resource="http://purl.org/olia/susa.owl#plural"/>
        <olia_system:hasTag>NP2t</olia_system:hasTag>
        <olia_system:hasTier>POS</olia_system:hasTier>
        <rdfs:comment>NP2t is used for plural town names.</rdfs:comment>
    </owl:NamedIndividual>
    


    <!-- http://purl.org/olia/susa.owl#NP2x -->

    <owl:NamedIndividual rdf:about="http://purl.org/olia/susa.owl#NP2x">
        <rdf:type rdf:resource="http://purl.org/olia/susa.owl#ProperNoun"/>
        <hasNumber rdf:resource="http://purl.org/olia/susa.owl#plural"/>
        <olia_system:hasTag>NP2x</olia_system:hasTag>
        <olia_system:hasTier>POS</olia_system:hasTier>
        <rdfs:comment>NP2x are miscellaneous plural proper names.</rdfs:comment>
    </owl:NamedIndividual>
    


    <!-- http://purl.org/olia/susa.owl#NP2z -->

    <owl:NamedIndividual rdf:about="http://purl.org/olia/susa.owl#NP2z">
        <rdf:type rdf:resource="http://purl.org/olia/susa.owl#ProperNoun"/>
        <hasNumber rdf:resource="http://purl.org/olia/susa.owl#plural"/>
        <olia_system:hasTag>NP2z</olia_system:hasTag>
        <olia_system:hasTier>POS</olia_system:hasTier>
        <rdfs:comment>NP2z is used for the pluralized form of a &apos;code name&apos; functioning as countable noun, e.g. &quot;1-11´s&quot;.</rdfs:comment>
    </owl:NamedIndividual>
    


    <!-- http://purl.org/olia/susa.owl#NPD -->

    <owl:NamedIndividual rdf:about="http://purl.org/olia/susa.owl#NPD">
        <rdf:type rdf:resource="http://purl.org/olia/susa.owl#ProperNoun"/>
        <olia_system:hasTag>NPD</olia_system:hasTag>
        <olia_system:hasTier>POS</olia_system:hasTier>
        <rdfs:comment>NPD is the SUSANNE tag for an abbreviated day of the week, e.g. &quot;Tues&quot;.</rdfs:comment>
    </owl:NamedIndividual>
    


    <!-- http://purl.org/olia/susa.owl#NPD1 -->

    <owl:NamedIndividual rdf:about="http://purl.org/olia/susa.owl#NPD1">
        <rdf:type rdf:resource="http://purl.org/olia/susa.owl#ProperNoun"/>
        <hasNumber rdf:resource="http://purl.org/olia/susa.owl#singular"/>
        <olia_system:hasTag>NPD1</olia_system:hasTag>
        <olia_system:hasTier>POS</olia_system:hasTier>
        <rdfs:comment>NPD1 is the SUSANNE tag used for a day of the week e.g. &quot;Monday&quot;.</rdfs:comment>
    </owl:NamedIndividual>
    


    <!-- http://purl.org/olia/susa.owl#NPD2 -->

    <owl:NamedIndividual rdf:about="http://purl.org/olia/susa.owl#NPD2">
        <rdf:type rdf:resource="http://purl.org/olia/susa.owl#ProperNoun"/>
        <hasNumber rdf:resource="http://purl.org/olia/susa.owl#plural"/>
        <olia_system:hasTag>NPD2</olia_system:hasTag>
        <olia_system:hasTier>POS</olia_system:hasTier>
        <rdfs:comment>NPD2 is the SUSANNE tag used for a day of the week in plural, e.g. &quot;Tuesdays&quot;.</rdfs:comment>
    </owl:NamedIndividual>
    


    <!-- http://purl.org/olia/susa.owl#NPM -->

    <owl:NamedIndividual rdf:about="http://purl.org/olia/susa.owl#NPM">
        <rdf:type rdf:resource="http://purl.org/olia/susa.owl#ProperNoun"/>
        <olia_system:hasTag>NPM</olia_system:hasTag>
        <olia_system:hasTier>POS</olia_system:hasTier>
        <rdfs:comment>NPM is the tag for an abbreviated month name, e.g. &quot;Oct&quot;.</rdfs:comment>
    </owl:NamedIndividual>
    


    <!-- http://purl.org/olia/susa.owl#NPM1 -->

    <owl:NamedIndividual rdf:about="http://purl.org/olia/susa.owl#NPM1">
        <rdf:type rdf:resource="http://purl.org/olia/susa.owl#ProperNoun"/>
        <hasNumber rdf:resource="http://purl.org/olia/susa.owl#singular"/>
        <olia_system:hasTag>NPM1</olia_system:hasTag>
        <olia_system:hasTier>POS</olia_system:hasTier>
        <rdfs:comment>NPM1 is the SUSANNE tag used for a month name, e.g. &quot;October&quot;</rdfs:comment>
    </owl:NamedIndividual>
    


    <!-- http://purl.org/olia/susa.owl#NPM2 -->

    <owl:NamedIndividual rdf:about="http://purl.org/olia/susa.owl#NPM2">
        <rdf:type rdf:resource="http://purl.org/olia/susa.owl#ProperNoun"/>
        <hasNumber rdf:resource="http://purl.org/olia/susa.owl#plural"/>
        <olia_system:hasTag>NPM2</olia_system:hasTag>
        <olia_system:hasTier>POS</olia_system:hasTier>
        <rdfs:comment>NPM2 is the SUSANNE tag used for plural of month names, e.g. &quot;Octobers&quot;.</rdfs:comment>
    </owl:NamedIndividual>
    


    <!-- http://purl.org/olia/susa.owl#PN -->

    <owl:NamedIndividual rdf:about="http://purl.org/olia/susa.owl#PN">
        <rdf:type rdf:resource="http://purl.org/olia/susa.owl#SubstitutiveNegativePronoun"/>
        <olia_system:hasTag>PN</olia_system:hasTag>
        <olia_system:hasTier>POS</olia_system:hasTier>
        <rdfs:comment>PN is the SUSANNE tag used for the negative substitutive pronoun &quot;none&quot; in all uses. 
(Sampson 1995, p. 114)</rdfs:comment>
    </owl:NamedIndividual>
    


    <!-- http://purl.org/olia/susa.owl#PN1 -->

    <owl:NamedIndividual rdf:about="http://purl.org/olia/susa.owl#PN1">
        <rdf:type rdf:resource="http://purl.org/olia/susa.owl#SubstitutiveIndefinitePronoun"/>
        <olia_system:hasTag>PN1</olia_system:hasTag>
        <olia_system:hasTier>POS</olia_system:hasTier>
        <rdfs:comment>PN1 is used for e.g. &quot;anybody&quot;, &quot;anyone&quot;, &quot;anything&quot;, &quot;everybody&quot;, &quot;everything&quot;, &quot;naught&quot;, &quot;nobody&quot;, &quot;no one&quot;, &quot;nothing&quot;.
(Sampson 1995, p. 114)</rdfs:comment>
    </owl:NamedIndividual>
    


    <!-- http://purl.org/olia/susa.owl#PN1o -->

    <owl:NamedIndividual rdf:about="http://purl.org/olia/susa.owl#PN1o">
        <rdf:type rdf:resource="http://purl.org/olia/susa.owl#SubstitutiveIndefinitePronoun"/>
        <olia_system:hasTag>PN1o</olia_system:hasTag>
        <olia_system:hasTier>POS</olia_system:hasTier>
        <rdfs:comment>PN1o is the SUSANNE tag usedfor the singular indefinite pronoun (&quot;one&quot;).
(Sampson 1995, p. 114)</rdfs:comment>
    </owl:NamedIndividual>
    


    <!-- http://purl.org/olia/susa.owl#PN1z -->

    <owl:NamedIndividual rdf:about="http://purl.org/olia/susa.owl#PN1z">
        <rdf:type rdf:resource="http://purl.org/olia/susa.owl#SubstitutiveIndefinitePronoun"/>
        <olia_system:hasTag>PN1z</olia_system:hasTag>
        <olia_system:hasTier>POS</olia_system:hasTier>
        <rdfs:comment>PN1z is used for &quot;so&quot; as a pro-form, for instance in the &quot;do so&quot;- construction.
(Sampson 1995, p. 114)</rdfs:comment>
    </owl:NamedIndividual>
    


    <!-- http://purl.org/olia/susa.owl#PNQOq -->

    <owl:NamedIndividual rdf:about="http://purl.org/olia/susa.owl#PNQOq">
        <rdf:type rdf:resource="http://purl.org/olia/susa.owl#SubstitutiveInterrogativePronoun"/>
        <hasCase rdf:resource="http://purl.org/olia/susa.owl#objective"/>
        <olia_system:hasTag>PNQOq</olia_system:hasTag>
        <olia_system:hasTier>POS</olia_system:hasTier>
        <rdfs:comment>This tag is used for the interrogative &quot;whom&quot;.
(Sampson 1995, p. 115)</rdfs:comment>
    </owl:NamedIndividual>
    


    <!-- http://purl.org/olia/susa.owl#PNQOr -->

    <owl:NamedIndividual rdf:about="http://purl.org/olia/susa.owl#PNQOr">
        <rdf:type rdf:resource="http://purl.org/olia/susa.owl#SubstitutiveRelativePronoun"/>
        <hasCase rdf:resource="http://purl.org/olia/susa.owl#objective"/>
        <olia_system:hasTag>PNQOr</olia_system:hasTag>
        <olia_system:hasTier>POS</olia_system:hasTier>
        <rdfs:comment>This tag is used for the relative &quot;whom&quot;.
(Sampson 1995, p. 115)</rdfs:comment>
    </owl:NamedIndividual>
    


    <!-- http://purl.org/olia/susa.owl#PNQS -->

    <owl:NamedIndividual rdf:about="http://purl.org/olia/susa.owl#PNQS">
        <rdf:type rdf:resource="http://purl.org/olia/susa.owl#SubstitutiveWHPronoun"/>
        <olia_system:hasTag>PNQS</olia_system:hasTag>
        <olia_system:hasTier>POS</olia_system:hasTier>
        <rdfs:comment>PNQS is used for &quot;who&quot;. This tag is taken from the reduced TnT tagset.</rdfs:comment>
    </owl:NamedIndividual>
    


    <!-- http://purl.org/olia/susa.owl#PNQSq -->

    <owl:NamedIndividual rdf:about="http://purl.org/olia/susa.owl#PNQSq">
        <rdf:type rdf:resource="http://purl.org/olia/susa.owl#SubstitutiveInterrogativePronoun"/>
        <hasCase rdf:resource="http://purl.org/olia/susa.owl#subjective"/>
        <olia_system:hasTag>PNQSq</olia_system:hasTag>
        <olia_system:hasTier>POS</olia_system:hasTier>
        <rdfs:comment>This tag is used for the interrogative &quot;who&quot;.
(Sampson 1995, p. 115)</rdfs:comment>
    </owl:NamedIndividual>
    


    <!-- http://purl.org/olia/susa.owl#PNQSr -->

    <owl:NamedIndividual rdf:about="http://purl.org/olia/susa.owl#PNQSr">
        <rdf:type rdf:resource="http://purl.org/olia/susa.owl#SubstitutiveRelativePronoun"/>
        <hasCase rdf:resource="http://purl.org/olia/susa.owl#subjective"/>
        <olia_system:hasTag>PNQSr</olia_system:hasTag>
        <olia_system:hasTier>POS</olia_system:hasTier>
        <rdfs:comment>This tag is used for the relative &quot;who&quot;.
(Sampson 1995, p. 115)</rdfs:comment>
    </owl:NamedIndividual>
    


    <!-- http://purl.org/olia/susa.owl#PNQV -->

    <owl:NamedIndividual rdf:about="http://purl.org/olia/susa.owl#PNQV">
        <rdf:type rdf:resource="http://purl.org/olia/susa.owl#SubstitutiveWHPronoun"/>
        <olia_system:hasTag>PNQV</olia_system:hasTag>
        <olia_system:hasTier>POS</olia_system:hasTier>
        <rdfs:comment>PNQV is used for substitutive wh pronouns without a specification of case.</rdfs:comment>
    </owl:NamedIndividual>
    


    <!-- http://purl.org/olia/susa.owl#PNQVG -->

    <owl:NamedIndividual rdf:about="http://purl.org/olia/susa.owl#PNQVG">
        <rdf:type rdf:resource="http://purl.org/olia/susa.owl#SubstitutiveWHPronoun"/>
        <hasCase rdf:resource="http://purl.org/olia/susa.owl#genitive"/>
        <olia_system:hasTag>PNQVG</olia_system:hasTag>
        <olia_system:hasTier>POS</olia_system:hasTier>
        <rdfs:comment>This tag is used for &quot;no matter whose&quot;, &quot;whosever&quot;.</rdfs:comment>
    </owl:NamedIndividual>
    


    <!-- http://purl.org/olia/susa.owl#PNQVO -->

    <owl:NamedIndividual rdf:about="http://purl.org/olia/susa.owl#PNQVO">
        <rdf:type rdf:resource="http://purl.org/olia/susa.owl#SubstitutiveWHPronoun"/>
        <hasCase rdf:resource="http://purl.org/olia/susa.owl#objective"/>
        <olia_system:hasTag>PNQVO</olia_system:hasTag>
        <olia_system:hasTier>POS</olia_system:hasTier>
        <rdfs:comment>This tag is used for &quot;no matter whom&quot;, &quot;whomever&quot;.</rdfs:comment>
    </owl:NamedIndividual>
    


    <!-- http://purl.org/olia/susa.owl#PNQVS -->

    <owl:NamedIndividual rdf:about="http://purl.org/olia/susa.owl#PNQVS">
        <rdf:type rdf:resource="http://purl.org/olia/susa.owl#SubstitutiveWHPronoun"/>
        <hasCase rdf:resource="http://purl.org/olia/susa.owl#subjective"/>
        <olia_system:hasTag>PNQVS</olia_system:hasTag>
        <olia_system:hasTier>POS</olia_system:hasTier>
        <rdfs:comment>This tag is used for &quot;no matter who&quot;, &quot;whoever&quot;, &quot;whosever&quot;.</rdfs:comment>
    </owl:NamedIndividual>
    


    <!-- http://purl.org/olia/susa.owl#PNX1 -->

    <owl:NamedIndividual rdf:about="http://purl.org/olia/susa.owl#PNX1">
        <rdf:type rdf:resource="http://purl.org/olia/susa.owl#SubstitutiveIndefiniteReflexive"/>
        <olia_system:hasTag>PNX1</olia_system:hasTag>
        <olia_system:hasTier>POS</olia_system:hasTier>
        <rdfs:comment>PNX1 is the SUSANNE tag used for the singular indefinite reflexive &quot;oneself&quot;.</rdfs:comment>
    </owl:NamedIndividual>
    


    <!-- http://purl.org/olia/susa.owl#PPG -->

    <owl:NamedIndividual rdf:about="http://purl.org/olia/susa.owl#PPG">
        <rdf:type rdf:resource="http://purl.org/olia/susa.owl#SubstitutivePossessivePronoun"/>
        <olia_system:hasTag>PPG</olia_system:hasTag>
        <olia_system:hasTier>POS</olia_system:hasTier>
        <rdfs:comment>These are substitutive possessive pronouns.</rdfs:comment>
    </owl:NamedIndividual>
    


    <!-- http://purl.org/olia/susa.owl#PPGf -->

    <owl:NamedIndividual rdf:about="http://purl.org/olia/susa.owl#PPGf">
        <rdf:type rdf:resource="http://purl.org/olia/susa.owl#SubstitutivePossessivePronoun"/>
        <hasGender rdf:resource="http://purl.org/olia/susa.owl#feminine"/>
        <hasNumber rdf:resource="http://purl.org/olia/susa.owl#singular"/>
        <hasPerson rdf:resource="http://purl.org/olia/susa.owl#third"/>
        <olia_system:hasTag>PPGf</olia_system:hasTag>
        <olia_system:hasTier>POS</olia_system:hasTier>
        <rdfs:comment>PPGf is used for &quot;hers&quot;.</rdfs:comment>
    </owl:NamedIndividual>
    


    <!-- http://purl.org/olia/susa.owl#PPGh2 -->

    <owl:NamedIndividual rdf:about="http://purl.org/olia/susa.owl#PPGh2">
        <rdf:type rdf:resource="http://purl.org/olia/susa.owl#SubstitutivePossessivePronoun"/>
        <hasNumber rdf:resource="http://purl.org/olia/susa.owl#plural"/>
        <hasPerson rdf:resource="http://purl.org/olia/susa.owl#third"/>
        <olia_system:hasTag>PPGh2</olia_system:hasTag>
        <olia_system:hasTier>POS</olia_system:hasTier>
        <rdfs:comment>PPGh2 is used for &quot;theirs&quot;.</rdfs:comment>
    </owl:NamedIndividual>
    


    <!-- http://purl.org/olia/susa.owl#PPGi1 -->

    <owl:NamedIndividual rdf:about="http://purl.org/olia/susa.owl#PPGi1">
        <rdf:type rdf:resource="http://purl.org/olia/susa.owl#SubstitutivePossessivePronoun"/>
        <hasNumber rdf:resource="http://purl.org/olia/susa.owl#singular"/>
        <hasPerson rdf:resource="http://purl.org/olia/susa.owl#first"/>
        <olia_system:hasTag>PPGi1</olia_system:hasTag>
        <olia_system:hasTier>POS</olia_system:hasTier>
        <rdfs:comment>PPGi1 is used for &quot;mine&quot;.</rdfs:comment>
    </owl:NamedIndividual>
    


    <!-- http://purl.org/olia/susa.owl#PPGi2 -->

    <owl:NamedIndividual rdf:about="http://purl.org/olia/susa.owl#PPGi2">
        <rdf:type rdf:resource="http://purl.org/olia/susa.owl#SubstitutivePossessivePronoun"/>
        <hasNumber rdf:resource="http://purl.org/olia/susa.owl#singular"/>
        <hasPerson rdf:resource="http://purl.org/olia/susa.owl#first"/>
        <olia_system:hasTag>PPGi2</olia_system:hasTag>
        <olia_system:hasTier>POS</olia_system:hasTier>
        <rdfs:comment>PPGi2 is used &quot;ours&quot;.</rdfs:comment>
    </owl:NamedIndividual>
    


    <!-- http://purl.org/olia/susa.owl#PPGm -->

    <owl:NamedIndividual rdf:about="http://purl.org/olia/susa.owl#PPGm">
        <rdf:type rdf:resource="http://purl.org/olia/susa.owl#SubstitutivePossessivePronoun"/>
        <hasGender rdf:resource="http://purl.org/olia/susa.owl#masculine"/>
        <hasNumber rdf:resource="http://purl.org/olia/susa.owl#singular"/>
        <hasPerson rdf:resource="http://purl.org/olia/susa.owl#third"/>
        <olia_system:hasTag>PPGm</olia_system:hasTag>
        <olia_system:hasTier>POS</olia_system:hasTier>
        <rdfs:comment>PPGm is used for &quot;his&quot;.</rdfs:comment>
    </owl:NamedIndividual>
    


    <!-- http://purl.org/olia/susa.owl#PPGy -->

    <owl:NamedIndividual rdf:about="http://purl.org/olia/susa.owl#PPGy">
        <rdf:type rdf:resource="http://purl.org/olia/susa.owl#SubstitutivePossessivePronoun"/>
        <hasPerson rdf:resource="http://purl.org/olia/susa.owl#second"/>
        <olia_system:hasTag>NPM</olia_system:hasTag>
        <olia_system:hasTier>POS</olia_system:hasTier>
        <rdfs:comment>PPGy is used for &quot;yours&quot;in singular or plural.</rdfs:comment>
    </owl:NamedIndividual>
    


    <!-- http://purl.org/olia/susa.owl#PPH -->

    <owl:NamedIndividual rdf:about="http://purl.org/olia/susa.owl#PPH">
        <rdf:type rdf:resource="http://purl.org/olia/susa.owl#SubstitutiveThirdPersonPronoun"/>
        <olia_system:hasTag>PPH</olia_system:hasTag>
        <olia_system:hasTier>POS</olia_system:hasTier>
        <rdfs:comment>These are third person pronouns.</rdfs:comment>
    </owl:NamedIndividual>
    


    <!-- http://purl.org/olia/susa.owl#PPH1 -->

    <owl:NamedIndividual rdf:about="http://purl.org/olia/susa.owl#PPH1">
        <rdf:type rdf:resource="http://purl.org/olia/susa.owl#SubstitutiveThirdPersonPronoun"/>
        <hasGender rdf:resource="http://purl.org/olia/susa.owl#neutral"/>
        <hasNumber rdf:resource="http://purl.org/olia/susa.owl#singular"/>
        <hasPerson rdf:resource="http://purl.org/olia/susa.owl#third"/>
        <olia_system:hasTag>PPH1</olia_system:hasTag>
        <olia_system:hasTier>POS</olia_system:hasTier>
        <rdfs:comment>PPH1 is used for &quot;it&quot;.</rdfs:comment>
    </owl:NamedIndividual>
    


    <!-- http://purl.org/olia/susa.owl#PPHO1 -->

    <owl:NamedIndividual rdf:about="http://purl.org/olia/susa.owl#PPHO1">
        <rdf:type rdf:resource="http://purl.org/olia/susa.owl#SubstitutiveThirdPersonPronoun"/>
        <hasCase rdf:resource="http://purl.org/olia/susa.owl#objective"/>
        <hasNumber rdf:resource="http://purl.org/olia/susa.owl#singular"/>
        <olia_system:hasTag>PPHO1</olia_system:hasTag>
        <olia_system:hasTier>POS</olia_system:hasTier>
        <rdfs:comment>PPHO1 ia used for objective third person pronouns in singular.</rdfs:comment>
    </owl:NamedIndividual>
    


    <!-- http://purl.org/olia/susa.owl#PPHO1f -->

    <owl:NamedIndividual rdf:about="http://purl.org/olia/susa.owl#PPHO1f">
        <rdf:type rdf:resource="http://purl.org/olia/susa.owl#SubstitutiveThirdPersonPronoun"/>
        <hasCase rdf:resource="http://purl.org/olia/susa.owl#objective"/>
        <hasGender rdf:resource="http://purl.org/olia/susa.owl#feminine"/>
        <hasNumber rdf:resource="http://purl.org/olia/susa.owl#singular"/>
        <hasPerson rdf:resource="http://purl.org/olia/susa.owl#third"/>
        <olia_system:hasTag>PPHO1f</olia_system:hasTag>
        <olia_system:hasTier>POS</olia_system:hasTier>
        <rdfs:comment>PPHO1f is the SUSANNE tag used for &quot;her&quot; as pronoun.</rdfs:comment>
    </owl:NamedIndividual>
    


    <!-- http://purl.org/olia/susa.owl#PPHO1m -->

    <owl:NamedIndividual rdf:about="http://purl.org/olia/susa.owl#PPHO1m">
        <rdf:type rdf:resource="http://purl.org/olia/susa.owl#SubstitutiveThirdPersonPronoun"/>
        <hasCase rdf:resource="http://purl.org/olia/susa.owl#objective"/>
        <hasGender rdf:resource="http://purl.org/olia/susa.owl#masculine"/>
        <hasNumber rdf:resource="http://purl.org/olia/susa.owl#singular"/>
        <hasPerson rdf:resource="http://purl.org/olia/susa.owl#third"/>
        <olia_system:hasTag>PPHO1m</olia_system:hasTag>
        <olia_system:hasTier>POS</olia_system:hasTier>
        <rdfs:comment>PPHO1m  for &quot;him&quot;.</rdfs:comment>
    </owl:NamedIndividual>
    


    <!-- http://purl.org/olia/susa.owl#PPHO2 -->

    <owl:NamedIndividual rdf:about="http://purl.org/olia/susa.owl#PPHO2">
        <rdf:type rdf:resource="http://purl.org/olia/susa.owl#SubstitutiveThirdPersonPronoun"/>
        <hasCase rdf:resource="http://purl.org/olia/susa.owl#objective"/>
        <hasNumber rdf:resource="http://purl.org/olia/susa.owl#plural"/>
        <hasPerson rdf:resource="http://purl.org/olia/susa.owl#third"/>
        <olia_system:hasTag>PPHO2</olia_system:hasTag>
        <olia_system:hasTier>POS</olia_system:hasTier>
        <rdfs:comment>PPHO2 is used for &quot;them&quot;.</rdfs:comment>
    </owl:NamedIndividual>
    


    <!-- http://purl.org/olia/susa.owl#PPHS1 -->

    <owl:NamedIndividual rdf:about="http://purl.org/olia/susa.owl#PPHS1">
        <rdf:type rdf:resource="http://purl.org/olia/susa.owl#SubstitutiveThirdPersonPronoun"/>
        <hasCase rdf:resource="http://purl.org/olia/susa.owl#subjective"/>
        <hasNumber rdf:resource="http://purl.org/olia/susa.owl#singular"/>
        <olia_system:hasTag>PPHS1</olia_system:hasTag>
        <olia_system:hasTier>POS</olia_system:hasTier>
        <rdfs:comment>PPHS1 ia used for subjective third person pronouns in singular.</rdfs:comment>
    </owl:NamedIndividual>
    


    <!-- http://purl.org/olia/susa.owl#PPHS1f -->

    <owl:NamedIndividual rdf:about="http://purl.org/olia/susa.owl#PPHS1f">
        <rdf:type rdf:resource="http://purl.org/olia/susa.owl#SubstitutiveThirdPersonPronoun"/>
        <hasCase rdf:resource="http://purl.org/olia/susa.owl#subjective"/>
        <hasGender rdf:resource="http://purl.org/olia/susa.owl#feminine"/>
        <hasNumber rdf:resource="http://purl.org/olia/susa.owl#singular"/>
        <hasPerson rdf:resource="http://purl.org/olia/susa.owl#third"/>
        <olia_system:hasTag>PPHS1f</olia_system:hasTag>
        <olia_system:hasTier>POS</olia_system:hasTier>
        <rdfs:comment>PPHS1f describes &quot;she&quot;.</rdfs:comment>
    </owl:NamedIndividual>
    


    <!-- http://purl.org/olia/susa.owl#PPHS1m -->

    <owl:NamedIndividual rdf:about="http://purl.org/olia/susa.owl#PPHS1m">
        <rdf:type rdf:resource="http://purl.org/olia/susa.owl#SubstitutiveThirdPersonPronoun"/>
        <hasCase rdf:resource="http://purl.org/olia/susa.owl#subjective"/>
        <hasGender rdf:resource="http://purl.org/olia/susa.owl#masculine"/>
        <hasNumber rdf:resource="http://purl.org/olia/susa.owl#singular"/>
        <hasPerson rdf:resource="http://purl.org/olia/susa.owl#third"/>
        <olia_system:hasTag>PPHS1m</olia_system:hasTag>
        <olia_system:hasTier>POS</olia_system:hasTier>
        <rdfs:comment>PPHS1m id used for &quot;he&quot;.</rdfs:comment>
    </owl:NamedIndividual>
    


    <!-- http://purl.org/olia/susa.owl#PPHS2 -->

    <owl:NamedIndividual rdf:about="http://purl.org/olia/susa.owl#PPHS2">
        <rdf:type rdf:resource="http://purl.org/olia/susa.owl#SubstitutiveThirdPersonPronoun"/>
        <hasCase rdf:resource="http://purl.org/olia/susa.owl#subjective"/>
        <hasNumber rdf:resource="http://purl.org/olia/susa.owl#plural"/>
        <olia_system:hasTag>PPHS2</olia_system:hasTag>
        <olia_system:hasTier>POS</olia_system:hasTier>
        <rdfs:comment>PPHS2 is used for &quot;they&quot;.</rdfs:comment>
    </owl:NamedIndividual>
    


    <!-- http://purl.org/olia/susa.owl#PPI -->

    <owl:NamedIndividual rdf:about="http://purl.org/olia/susa.owl#PPI">
        <rdf:type rdf:resource="http://purl.org/olia/susa.owl#SubstitutiveFirstPersonPronoun"/>
        <olia_system:hasTag>PPI</olia_system:hasTag>
        <olia_system:hasTier>POS</olia_system:hasTier>
        <rdfs:comment>PPI is used for substitutive first person pronouns.</rdfs:comment>
    </owl:NamedIndividual>
    


    <!-- http://purl.org/olia/susa.owl#PPIO1 -->

    <owl:NamedIndividual rdf:about="http://purl.org/olia/susa.owl#PPIO1">
        <rdf:type rdf:resource="http://purl.org/olia/susa.owl#SubstitutiveFirstPersonPronoun"/>
        <hasCase rdf:resource="http://purl.org/olia/susa.owl#objective"/>
        <hasNumber rdf:resource="http://purl.org/olia/susa.owl#singular"/>
        <hasPerson rdf:resource="http://purl.org/olia/susa.owl#first"/>
        <olia_system:hasTag>PPIO1</olia_system:hasTag>
        <olia_system:hasTier>POS</olia_system:hasTier>
        <rdfs:comment>PPIO1 is used for &quot;me&quot;.</rdfs:comment>
    </owl:NamedIndividual>
    


    <!-- http://purl.org/olia/susa.owl#PPIO2 -->

    <owl:NamedIndividual rdf:about="http://purl.org/olia/susa.owl#PPIO2">
        <rdf:type rdf:resource="http://purl.org/olia/susa.owl#SubstitutiveFirstPersonPronoun"/>
        <hasCase rdf:resource="http://purl.org/olia/susa.owl#objective"/>
        <hasNumber rdf:resource="http://purl.org/olia/susa.owl#plural"/>
        <hasPerson rdf:resource="http://purl.org/olia/susa.owl#first"/>
        <olia_system:hasTag>PPIO2</olia_system:hasTag>
        <olia_system:hasTier>POS</olia_system:hasTier>
        <rdfs:comment>PPIO2 is the SUSANNE tag used for &quot;us&quot;.</rdfs:comment>
    </owl:NamedIndividual>
    


    <!-- http://purl.org/olia/susa.owl#PPIS1 -->

    <owl:NamedIndividual rdf:about="http://purl.org/olia/susa.owl#PPIS1">
        <rdf:type rdf:resource="http://purl.org/olia/susa.owl#SubstitutiveFirstPersonPronoun"/>
        <hasCase rdf:resource="http://purl.org/olia/susa.owl#subjective"/>
        <hasNumber rdf:resource="http://purl.org/olia/susa.owl#singular"/>
        <hasPerson rdf:resource="http://purl.org/olia/susa.owl#first"/>
        <olia_system:hasTag>PPIS1</olia_system:hasTag>
        <olia_system:hasTier>POS</olia_system:hasTier>
        <rdfs:comment>This is the tag for &apos; I &apos; as personal pronoun.</rdfs:comment>
    </owl:NamedIndividual>
    


    <!-- http://purl.org/olia/susa.owl#PPIS2 -->

    <owl:NamedIndividual rdf:about="http://purl.org/olia/susa.owl#PPIS2">
        <rdf:type rdf:resource="http://purl.org/olia/susa.owl#SubstitutiveFirstPersonPronoun"/>
        <hasCase rdf:resource="http://purl.org/olia/susa.owl#subjective"/>
        <hasNumber rdf:resource="http://purl.org/olia/susa.owl#plural"/>
        <hasPerson rdf:resource="http://purl.org/olia/susa.owl#first"/>
        <olia_system:hasTag>PPIS2</olia_system:hasTag>
        <olia_system:hasTier>POS</olia_system:hasTier>
        <rdfs:comment>This is the tag for &quot;we&quot;.</rdfs:comment>
    </owl:NamedIndividual>
    


    <!-- http://purl.org/olia/susa.owl#PPX -->

    <owl:NamedIndividual rdf:about="http://purl.org/olia/susa.owl#PPX">
        <rdf:type rdf:resource="http://purl.org/olia/susa.owl#ReflexivePronoun"/>
        <olia_system:hasTag>PPX</olia_system:hasTag>
        <olia_system:hasTier>POS</olia_system:hasTier>
        <rdfs:comment>PPX are reflexive personal pronouns.</rdfs:comment>
    </owl:NamedIndividual>
    


    <!-- http://purl.org/olia/susa.owl#PPX1 -->

    <owl:NamedIndividual rdf:about="http://purl.org/olia/susa.owl#PPX1">
        <rdf:type rdf:resource="http://purl.org/olia/susa.owl#ReflexivePronoun"/>
        <hasNumber rdf:resource="http://purl.org/olia/susa.owl#singular"/>
        <olia_system:hasTag>PPX1</olia_system:hasTag>
        <olia_system:hasTier>POS</olia_system:hasTier>
        <rdfs:comment>These are the singular forms of the reflexive personal pronouns.</rdfs:comment>
    </owl:NamedIndividual>
    


    <!-- http://purl.org/olia/susa.owl#PPX1f -->

    <owl:NamedIndividual rdf:about="http://purl.org/olia/susa.owl#PPX1f">
        <rdf:type rdf:resource="http://purl.org/olia/susa.owl#ReflexivePronoun"/>
        <hasGender rdf:resource="http://purl.org/olia/susa.owl#feminine"/>
        <hasNumber rdf:resource="http://purl.org/olia/susa.owl#singular"/>
        <hasPerson rdf:resource="http://purl.org/olia/susa.owl#third"/>
        <olia_system:hasTag>PPX1f</olia_system:hasTag>
        <olia_system:hasTier>POS</olia_system:hasTier>
        <rdfs:comment>PPX1f is the SUSANNE tag used for &quot;herself&quot;.</rdfs:comment>
    </owl:NamedIndividual>
    


    <!-- http://purl.org/olia/susa.owl#PPX1h -->

    <owl:NamedIndividual rdf:about="http://purl.org/olia/susa.owl#PPX1h">
        <rdf:type rdf:resource="http://purl.org/olia/susa.owl#ReflexivePronoun"/>
        <hasGender rdf:resource="http://purl.org/olia/susa.owl#neutral"/>
        <hasNumber rdf:resource="http://purl.org/olia/susa.owl#singular"/>
        <hasPerson rdf:resource="http://purl.org/olia/susa.owl#third"/>
        <olia_system:hasTag>PPX1h</olia_system:hasTag>
        <olia_system:hasTier>POS</olia_system:hasTier>
        <rdfs:comment>PPX1h tags &quot;itself&quot;.</rdfs:comment>
    </owl:NamedIndividual>
    


    <!-- http://purl.org/olia/susa.owl#PPX1i -->

    <owl:NamedIndividual rdf:about="http://purl.org/olia/susa.owl#PPX1i">
        <rdf:type rdf:resource="http://purl.org/olia/susa.owl#ReflexivePronoun"/>
        <hasNumber rdf:resource="http://purl.org/olia/susa.owl#singular"/>
        <hasPerson rdf:resource="http://purl.org/olia/susa.owl#first"/>
        <olia_system:hasTag>PPX1i</olia_system:hasTag>
        <olia_system:hasTier>POS</olia_system:hasTier>
        <rdfs:comment>PPX1i is used for &quot;myself&quot;.</rdfs:comment>
    </owl:NamedIndividual>
    


    <!-- http://purl.org/olia/susa.owl#PPX1m -->

    <owl:NamedIndividual rdf:about="http://purl.org/olia/susa.owl#PPX1m">
        <rdf:type rdf:resource="http://purl.org/olia/susa.owl#ReflexivePronoun"/>
        <hasGender rdf:resource="http://purl.org/olia/susa.owl#masculine"/>
        <hasNumber rdf:resource="http://purl.org/olia/susa.owl#singular"/>
        <hasPerson rdf:resource="http://purl.org/olia/susa.owl#third"/>
        <olia_system:hasTag>PPX1m</olia_system:hasTag>
        <olia_system:hasTier>POS</olia_system:hasTier>
        <rdfs:comment>PPX1m is used for &quot;himself&quot;.</rdfs:comment>
    </owl:NamedIndividual>
    


    <!-- http://purl.org/olia/susa.owl#PPX1y -->

    <owl:NamedIndividual rdf:about="http://purl.org/olia/susa.owl#PPX1y">
        <rdf:type rdf:resource="http://purl.org/olia/susa.owl#ReflexivePronoun"/>
        <hasNumber rdf:resource="http://purl.org/olia/susa.owl#singular"/>
        <hasPerson rdf:resource="http://purl.org/olia/susa.owl#second"/>
        <olia_system:hasTag>PPX1y</olia_system:hasTag>
        <olia_system:hasTier>POS</olia_system:hasTier>
        <rdfs:comment>PPX1y  for &quot;yourselves&quot;.</rdfs:comment>
    </owl:NamedIndividual>
    


    <!-- http://purl.org/olia/susa.owl#PPX2 -->

    <owl:NamedIndividual rdf:about="http://purl.org/olia/susa.owl#PPX2">
        <rdf:type rdf:resource="http://purl.org/olia/susa.owl#ReflexivePronoun"/>
        <hasNumber rdf:resource="http://purl.org/olia/susa.owl#plural"/>
        <olia_system:hasTag>PPX2</olia_system:hasTag>
        <olia_system:hasTier>POS</olia_system:hasTier>
        <rdfs:comment>These are the plural forms of the reflexive personal pronouns.</rdfs:comment>
    </owl:NamedIndividual>
    


    <!-- http://purl.org/olia/susa.owl#PPX2h -->

    <owl:NamedIndividual rdf:about="http://purl.org/olia/susa.owl#PPX2h">
        <rdf:type rdf:resource="http://purl.org/olia/susa.owl#ReflexivePronoun"/>
        <hasNumber rdf:resource="http://purl.org/olia/susa.owl#plural"/>
        <hasPerson rdf:resource="http://purl.org/olia/susa.owl#third"/>
        <olia_system:hasTag>PPX2h</olia_system:hasTag>
        <olia_system:hasTier>POS</olia_system:hasTier>
        <rdfs:comment>PPX2h is the SUSANNE tag used for &quot;themselves&quot;, &quot;each other&quot; or &quot;one another&quot;.</rdfs:comment>
    </owl:NamedIndividual>
    


    <!-- http://purl.org/olia/susa.owl#PPX2i -->

    <owl:NamedIndividual rdf:about="http://purl.org/olia/susa.owl#PPX2i">
        <rdf:type rdf:resource="http://purl.org/olia/susa.owl#ReflexivePronoun"/>
        <hasNumber rdf:resource="http://purl.org/olia/susa.owl#plural"/>
        <hasPerson rdf:resource="http://purl.org/olia/susa.owl#first"/>
        <olia_system:hasTag>PPX2i</olia_system:hasTag>
        <olia_system:hasTier>POS</olia_system:hasTier>
        <rdfs:comment>PPX2i describes &quot;ourselves&quot;/ &quot;ourself&quot;.</rdfs:comment>
    </owl:NamedIndividual>
    


    <!-- http://purl.org/olia/susa.owl#PPX2y -->

    <owl:NamedIndividual rdf:about="http://purl.org/olia/susa.owl#PPX2y">
        <rdf:type rdf:resource="http://purl.org/olia/susa.owl#ReflexivePronoun"/>
        <hasNumber rdf:resource="http://purl.org/olia/susa.owl#plural"/>
        <hasPerson rdf:resource="http://purl.org/olia/susa.owl#second"/>
        <olia_system:hasTag>PPX2y</olia_system:hasTag>
        <olia_system:hasTier>POS</olia_system:hasTier>
        <rdfs:comment>PPX2y tags &quot;yourselves&quot;.</rdfs:comment>
    </owl:NamedIndividual>
    


    <!-- http://purl.org/olia/susa.owl#PPY -->

    <owl:NamedIndividual rdf:about="http://purl.org/olia/susa.owl#PPY">
        <rdf:type rdf:resource="http://purl.org/olia/susa.owl#SubstitutiveSecondPersonPronoun"/>
        <hasPerson rdf:resource="http://purl.org/olia/susa.owl#second"/>
        <olia_system:hasTag>PPY</olia_system:hasTag>
        <olia_system:hasTier>POS</olia_system:hasTier>
        <rdfs:comment>This tag is used for &quot;you&quot; in singular or plural.</rdfs:comment>
    </owl:NamedIndividual>
    


    <!-- http://purl.org/olia/susa.owl#RA -->

    <owl:NamedIndividual rdf:about="http://purl.org/olia/susa.owl#RA">
        <rdf:type rdf:resource="http://purl.org/olia/susa.owl#PostmodifyingAdverb"/>
        <olia_system:hasTag>RA</olia_system:hasTag>
        <olia_system:hasTier>POS</olia_system:hasTier>
        <rdfs:comment>These are adverbs.</rdfs:comment>
    </owl:NamedIndividual>
    


    <!-- http://purl.org/olia/susa.owl#RAa -->

    <owl:NamedIndividual rdf:about="http://purl.org/olia/susa.owl#RAa">
        <rdf:type rdf:resource="http://purl.org/olia/susa.owl#PostmodifyingAdverb"/>
        <olia_system:hasTag>RAa</olia_system:hasTag>
        <olia_system:hasTier>POS</olia_system:hasTier>
        <rdfs:comment>RAa is the SUSANNE tag used for &quot;ago&quot;, &quot;since&quot; as synonym for age.</rdfs:comment>
    </owl:NamedIndividual>
    


    <!-- http://purl.org/olia/susa.owl#RAb -->

    <owl:NamedIndividual rdf:about="http://purl.org/olia/susa.owl#RAb">
        <rdf:type rdf:resource="http://purl.org/olia/susa.owl#PostmodifyingAdverb"/>
        <olia_system:hasTag>RAb</olia_system:hasTag>
        <olia_system:hasTier>POS</olia_system:hasTier>
        <rdfs:comment>RAb is used for &quot;A.D./ Anno Domini&quot; and  for counterparts used in the pre-date position in other calendars.</rdfs:comment>
    </owl:NamedIndividual>
    


    <!-- http://purl.org/olia/susa.owl#RAc -->

    <owl:NamedIndividual rdf:about="http://purl.org/olia/susa.owl#RAc">
        <rdf:type rdf:resource="http://purl.org/olia/susa.owl#PostmodifyingAdverb"/>
        <olia_system:hasTag>RAc</olia_system:hasTag>
        <olia_system:hasTier>POS</olia_system:hasTier>
        <rdfs:comment>RAc stands for a cocordinationg element e.g. &quot;etc&quot;, &quot;f&quot; or &quot;ff&quot; (means &apos;following&apos;).</rdfs:comment>
    </owl:NamedIndividual>
    


    <!-- http://purl.org/olia/susa.owl#RAe -->

    <owl:NamedIndividual rdf:about="http://purl.org/olia/susa.owl#RAe">
        <rdf:type rdf:resource="http://purl.org/olia/susa.owl#PostmodifyingAdverb"/>
        <olia_system:hasTag>RAe</olia_system:hasTag>
        <olia_system:hasTier>POS</olia_system:hasTier>
        <rdfs:comment>RAe is the tag for &quot;else&quot; in all uses.</rdfs:comment>
    </owl:NamedIndividual>
    


    <!-- http://purl.org/olia/susa.owl#RAh -->

    <owl:NamedIndividual rdf:about="http://purl.org/olia/susa.owl#RAh">
        <rdf:type rdf:resource="http://purl.org/olia/susa.owl#PostmodifyingAdverb"/>
        <olia_system:hasTag>RAh</olia_system:hasTag>
        <olia_system:hasTier>POS</olia_system:hasTier>
        <rdfs:comment>RAh is used &quot;am&quot; (for &apos;ante meridiem&apos;), &quot;pm&quot; o`clock.</rdfs:comment>
    </owl:NamedIndividual>
    


    <!-- http://purl.org/olia/susa.owl#RAi -->

    <owl:NamedIndividual rdf:about="http://purl.org/olia/susa.owl#RAi">
        <rdf:type rdf:resource="http://purl.org/olia/susa.owl#PostmodifyingAdverb"/>
        <olia_system:hasTag>RAi</olia_system:hasTag>
        <olia_system:hasTier>POS</olia_system:hasTier>
        <rdfs:comment>RAi is the tag for &quot;inst&quot;, &quot;ult&quot; etc. .</rdfs:comment>
    </owl:NamedIndividual>
    


    <!-- http://purl.org/olia/susa.owl#RAj -->

    <owl:NamedIndividual rdf:about="http://purl.org/olia/susa.owl#RAj">
        <rdf:type rdf:resource="http://purl.org/olia/susa.owl#PostmodifyingAdverb"/>
        <olia_system:hasTag>RAj</olia_system:hasTag>
        <olia_system:hasTier>POS</olia_system:hasTier>
        <rdfs:comment>RAj is used for postnomianl adjectives e.g. &quot;destinate&quot;, &quot;centigrade&quot;, &quot;elect&quot;, &quot;galore&quot;.</rdfs:comment>
    </owl:NamedIndividual>
    


    <!-- http://purl.org/olia/susa.owl#RAn -->

    <owl:NamedIndividual rdf:about="http://purl.org/olia/susa.owl#RAn">
        <rdf:type rdf:resource="http://purl.org/olia/susa.owl#PostmodifyingAdverb"/>
        <olia_system:hasTag>RAn</olia_system:hasTag>
        <olia_system:hasTier>POS</olia_system:hasTier>
        <rdfs:comment>RAn is used for &quot;whatever&quot;, &quot;whatsever&quot; after a negative or non-assertive nominal head.</rdfs:comment>
    </owl:NamedIndividual>
    


    <!-- http://purl.org/olia/susa.owl#RAp -->

    <owl:NamedIndividual rdf:about="http://purl.org/olia/susa.owl#RAp">
        <rdf:type rdf:resource="http://purl.org/olia/susa.owl#PostmodifyingAdverb"/>
        <olia_system:hasTag>RAp</olia_system:hasTag>
        <olia_system:hasTier>POS</olia_system:hasTier>
        <rdfs:comment>RAp is used for &quot;per annum&quot;, &quot;pa&quot;, &quot;per diem&quot; etc. .</rdfs:comment>
    </owl:NamedIndividual>
    


    <!-- http://purl.org/olia/susa.owl#RAq -->

    <owl:NamedIndividual rdf:about="http://purl.org/olia/susa.owl#RAq">
        <rdf:type rdf:resource="http://purl.org/olia/susa.owl#PostmodifyingAdverb"/>
        <olia_system:hasTag>RAq</olia_system:hasTag>
        <olia_system:hasTier>POS</olia_system:hasTier>
        <rdfs:comment>RAq is the SUSANNE tag used for &quot;apiece&quot;, distributive uses for &quot;each&quot;.</rdfs:comment>
    </owl:NamedIndividual>
    


    <!-- http://purl.org/olia/susa.owl#RAx -->

    <owl:NamedIndividual rdf:about="http://purl.org/olia/susa.owl#RAx">
        <rdf:type rdf:resource="http://purl.org/olia/susa.owl#PostmodifyingAdverb"/>
        <olia_system:hasTag>RAx</olia_system:hasTag>
        <olia_system:hasTier>POS</olia_system:hasTier>
        <rdfs:comment>RAx is used for a mathematical postfix operator e.g. &quot;!&quot; for factorial.</rdfs:comment>
    </owl:NamedIndividual>
    


    <!-- http://purl.org/olia/susa.owl#RAy -->

    <owl:NamedIndividual rdf:about="http://purl.org/olia/susa.owl#RAy">
        <rdf:type rdf:resource="http://purl.org/olia/susa.owl#PostmodifyingAdverb"/>
        <olia_system:hasTag>RAy</olia_system:hasTag>
        <olia_system:hasTier>POS</olia_system:hasTier>
        <rdfs:comment>RAy describes &quot;B.C.&quot;  and counterparts following dates in other calendars.</rdfs:comment>
    </owl:NamedIndividual>
    


    <!-- http://purl.org/olia/susa.owl#RAz -->

    <owl:NamedIndividual rdf:about="http://purl.org/olia/susa.owl#RAz">
        <rdf:type rdf:resource="http://purl.org/olia/susa.owl#PostmodifyingAdverb"/>
        <olia_system:hasTag>RAz</olia_system:hasTag>
        <olia_system:hasTier>POS</olia_system:hasTier>
        <rdfs:comment>RAz tags &quot;or so&quot; as in &quot;fifty or so&quot;.</rdfs:comment>
    </owl:NamedIndividual>
    


    <!-- http://purl.org/olia/susa.owl#REX -->

    <owl:NamedIndividual rdf:about="http://purl.org/olia/susa.owl#REX">
        <rdf:type rdf:resource="http://purl.org/olia/susa.owl#AppositionIntroducingAdverb"/>
        <olia_system:hasTag>REX</olia_system:hasTag>
        <olia_system:hasTier>POS</olia_system:hasTier>
        <rdfs:comment>REX is the SUSANNE tag used for an apposition-introducing element e.g. &quot;for example&quot;, &quot;for instance&quot;, &quot;namely&quot;.</rdfs:comment>
    </owl:NamedIndividual>
    


    <!-- http://purl.org/olia/susa.owl#RG -->

    <owl:NamedIndividual rdf:about="http://purl.org/olia/susa.owl#RG">
        <rdf:type rdf:resource="http://purl.org/olia/susa.owl#Qualifier"/>
        <olia_system:hasTag>RG</olia_system:hasTag>
        <olia_system:hasTier>POS</olia_system:hasTier>
        <rdfs:comment>RG is the SUSANNE tag used for a qualifier which having no other adverbial use e.g. &quot;very&quot;, &quot;jolly&quot;, &quot;mighty&quot;, &quot;stark&quot;.</rdfs:comment>
    </owl:NamedIndividual>
    


    <!-- http://purl.org/olia/susa.owl#RGA -->

    <owl:NamedIndividual rdf:about="http://purl.org/olia/susa.owl#RGA">
        <rdf:type rdf:resource="http://purl.org/olia/susa.owl#Qualifier"/>
        <olia_system:hasTag>RGA</olia_system:hasTag>
        <olia_system:hasTier>POS</olia_system:hasTier>
        <rdfs:comment>RGA is the SUSANNE tag for &quot;indeed&quot; as qualifier.</rdfs:comment>
    </owl:NamedIndividual>
    


    <!-- http://purl.org/olia/susa.owl#RGAf -->

    <owl:NamedIndividual rdf:about="http://purl.org/olia/susa.owl#RGAf">
        <rdf:type rdf:resource="http://purl.org/olia/susa.owl#Qualifier"/>
        <olia_system:hasTag>RGAf</olia_system:hasTag>
        <olia_system:hasTier>POS</olia_system:hasTier>
        <rdfs:comment>RGAf for &quot;enough&quot; as qualifier.</rdfs:comment>
    </owl:NamedIndividual>
    


    <!-- http://purl.org/olia/susa.owl#RGQ -->

    <owl:NamedIndividual rdf:about="http://purl.org/olia/susa.owl#RGQ">
        <rdf:type rdf:resource="http://purl.org/olia/susa.owl#Qualifier"/>
        <olia_system:hasTag>RGQ</olia_system:hasTag>
        <olia_system:hasTier>POS</olia_system:hasTier>
        <rdfs:comment>RGQ is used for question qualifiers.</rdfs:comment>
    </owl:NamedIndividual>
    


    <!-- http://purl.org/olia/susa.owl#RGQV -->

    <owl:NamedIndividual rdf:about="http://purl.org/olia/susa.owl#RGQV">
        <rdf:type rdf:resource="http://purl.org/olia/susa.owl#Qualifier"/>
        <olia_system:hasTag>RGQV</olia_system:hasTag>
        <olia_system:hasTier>POS</olia_system:hasTier>
        <rdfs:comment>RGQV is the tag for &quot;however&quot;, &quot;no matter how&quot; as qualifier.</rdfs:comment>
    </owl:NamedIndividual>
    


    <!-- http://purl.org/olia/susa.owl#RGQq -->

    <owl:NamedIndividual rdf:about="http://purl.org/olia/susa.owl#RGQq">
        <rdf:type rdf:resource="http://purl.org/olia/susa.owl#Qualifier"/>
        <olia_system:hasTag>RGQq</olia_system:hasTag>
        <olia_system:hasTier>POS</olia_system:hasTier>
        <rdfs:comment>RGQq for &quot;how&quot; as qualifier.</rdfs:comment>
    </owl:NamedIndividual>
    


    <!-- http://purl.org/olia/susa.owl#RGa -->

    <owl:NamedIndividual rdf:about="http://purl.org/olia/susa.owl#RGa">
        <rdf:type rdf:resource="http://purl.org/olia/susa.owl#Qualifier"/>
        <olia_system:hasTag>RGa</olia_system:hasTag>
        <olia_system:hasTier>POS</olia_system:hasTier>
        <rdfs:comment>Rga is used for &quot;as&quot; as qualifier. RGb is the tag for &quot;quite&quot; as qualifier or before an article e.g. in &quot;quite a good idea&quot;. RGf stands for &quot;too&quot; as qualifier.</rdfs:comment>
    </owl:NamedIndividual>
    


    <!-- http://purl.org/olia/susa.owl#RGb -->

    <owl:NamedIndividual rdf:about="http://purl.org/olia/susa.owl#RGb">
        <rdf:type rdf:resource="http://purl.org/olia/susa.owl#Qualifier"/>
        <olia_system:hasTag>RGb</olia_system:hasTag>
        <olia_system:hasTier>POS</olia_system:hasTier>
        <rdfs:comment>RGb is the tag for &quot;quite&quot; as qualifier or before an article e.g. in &quot;quite a good idea&quot;.</rdfs:comment>
    </owl:NamedIndividual>
    


    <!-- http://purl.org/olia/susa.owl#RGf -->

    <owl:NamedIndividual rdf:about="http://purl.org/olia/susa.owl#RGf">
        <rdf:type rdf:resource="http://purl.org/olia/susa.owl#Qualifier"/>
        <olia_system:hasTag>RGf</olia_system:hasTag>
        <olia_system:hasTier>POS</olia_system:hasTier>
        <rdfs:comment>RGf stands for &quot;too&quot; as qualifier.</rdfs:comment>
    </owl:NamedIndividual>
    


    <!-- http://purl.org/olia/susa.owl#RGi -->

    <owl:NamedIndividual rdf:about="http://purl.org/olia/susa.owl#RGi">
        <rdf:type rdf:resource="http://purl.org/olia/susa.owl#Qualifier"/>
        <olia_system:hasTag>RGi</olia_system:hasTag>
        <olia_system:hasTier>POS</olia_system:hasTier>
        <rdfs:comment>The SUSANNE tag RGi is used for &quot;about&quot;, &quot;around&quot;, &quot;circa&quot;, &quot;getting on for&quot; etc..</rdfs:comment>
    </owl:NamedIndividual>
    


    <!-- http://purl.org/olia/susa.owl#RGr -->

    <owl:NamedIndividual rdf:about="http://purl.org/olia/susa.owl#RGr">
        <rdf:type rdf:resource="http://purl.org/olia/susa.owl#Qualifier"/>
        <olia_system:hasTag>RGr</olia_system:hasTag>
        <olia_system:hasTier>POS</olia_system:hasTier>
        <rdfs:comment>RGr is used for &quot;rather&quot; as qualifier or before an article. RGz for &quot;so&quot; as qualifier.</rdfs:comment>
    </owl:NamedIndividual>
    


    <!-- http://purl.org/olia/susa.owl#RGz -->

    <owl:NamedIndividual rdf:about="http://purl.org/olia/susa.owl#RGz">
        <rdf:type rdf:resource="http://purl.org/olia/susa.owl#Qualifier"/>
        <olia_system:hasTag>RGz</olia_system:hasTag>
        <olia_system:hasTier>POS</olia_system:hasTier>
        <rdfs:comment>RGz for &quot;so&quot; as qualifier.</rdfs:comment>
    </owl:NamedIndividual>
    


    <!-- http://purl.org/olia/susa.owl#RL -->

    <owl:NamedIndividual rdf:about="http://purl.org/olia/susa.owl#RL">
        <rdf:type rdf:resource="http://purl.org/olia/susa.owl#TopographicalAdverb"/>
        <olia_system:hasTag>RL</olia_system:hasTag>
        <olia_system:hasTier>POS</olia_system:hasTier>
        <rdfs:comment>RL is the SUSANNE tag used for an adverb of place or direction e.g. &quot;along&quot;, &quot;back&quot;, &quot;outside&quot;.</rdfs:comment>
    </owl:NamedIndividual>
    


    <!-- http://purl.org/olia/susa.owl#RLe -->

    <owl:NamedIndividual rdf:about="http://purl.org/olia/susa.owl#RLe">
        <rdf:type rdf:resource="http://purl.org/olia/susa.owl#TopographicalAdverb"/>
        <olia_system:hasTag>RLe</olia_system:hasTag>
        <olia_system:hasTier>POS</olia_system:hasTier>
        <rdfs:comment>RLe is used for &quot;elsewhere&quot;.</rdfs:comment>
    </owl:NamedIndividual>
    


    <!-- http://purl.org/olia/susa.owl#RLh -->

    <owl:NamedIndividual rdf:about="http://purl.org/olia/susa.owl#RLh">
        <rdf:type rdf:resource="http://purl.org/olia/susa.owl#TopographicalAdverb"/>
        <olia_system:hasTag>RLh</olia_system:hasTag>
        <olia_system:hasTier>POS</olia_system:hasTier>
        <rdfs:comment>RLh is used for &quot;here&quot;, &quot;there&quot; as adverbs of place</rdfs:comment>
    </owl:NamedIndividual>
    


    <!-- http://purl.org/olia/susa.owl#RLn -->

    <owl:NamedIndividual rdf:about="http://purl.org/olia/susa.owl#RLn">
        <rdf:type rdf:resource="http://purl.org/olia/susa.owl#TopographicalAdverb"/>
        <olia_system:hasTag>RLn</olia_system:hasTag>
        <olia_system:hasTier>POS</olia_system:hasTier>
        <rdfs:comment>RLn is used for &quot;downstairs&quot;, &quot;upstairs&quot; .</rdfs:comment>
    </owl:NamedIndividual>
    


    <!-- http://purl.org/olia/susa.owl#RLw -->

    <owl:NamedIndividual rdf:about="http://purl.org/olia/susa.owl#RLw">
        <rdf:type rdf:resource="http://purl.org/olia/susa.owl#TopographicalAdverb"/>
        <olia_system:hasTag>RLw</olia_system:hasTag>
        <olia_system:hasTier>POS</olia_system:hasTier>
        <rdfs:comment>RLw is used for &quot;somewhere&quot;, &quot;someplace&quot;, &quot;anywhere&quot;, &quot;anyplace&quot;, &quot;everywhere&quot;, &quot;nowhere&quot; are adverbs of place or direction.</rdfs:comment>
    </owl:NamedIndividual>
    


    <!-- http://purl.org/olia/susa.owl#RP -->

    <owl:NamedIndividual rdf:about="http://purl.org/olia/susa.owl#RP">
        <rdf:type rdf:resource="http://purl.org/olia/susa.owl#PrepositionAsAdverb"/>
        <olia_system:hasTag>RP</olia_system:hasTag>
        <olia_system:hasTier>POS</olia_system:hasTier>
        <rdfs:comment>RP is used for &quot;across&quot;, &quot;down&quot;, &quot;in&quot;, &quot;off&quot;, &quot;on&quot;, &quot;out&quot;, &quot;over&quot;, &quot;through&quot;, &quot;up&quot; in adverberbial uses.</rdfs:comment>
    </owl:NamedIndividual>
    


    <!-- http://purl.org/olia/susa.owl#RPK -->

    <owl:NamedIndividual rdf:about="http://purl.org/olia/susa.owl#RPK">
        <rdf:type rdf:resource="http://purl.org/olia/susa.owl#PrepositionAsAdverb"/>
        <olia_system:hasTag>RPK</olia_system:hasTag>
        <olia_system:hasTier>POS</olia_system:hasTier>
        <rdfs:comment>RPK is used for &quot;about&quot; in adverbial and catenative use.</rdfs:comment>
    </owl:NamedIndividual>
    


    <!-- http://purl.org/olia/susa.owl#RR -->

    <owl:NamedIndividual rdf:about="http://purl.org/olia/susa.owl#RR">
        <rdf:type rdf:resource="http://purl.org/olia/susa.owl#GeneralAdverb"/>
        <olia_system:hasTag>RR</olia_system:hasTag>
        <olia_system:hasTier>POS</olia_system:hasTier>
        <rdfs:comment>RR is used for general adverbs.</rdfs:comment>
        <owl:versionInfo>added by Johannes Bubenzer (2006-09-09) in accordance to a
	TnT-tagged data set provided by SFB 538 (Hamburg), project K4</owl:versionInfo>
    </owl:NamedIndividual>
    


    <!-- http://purl.org/olia/susa.owl#RRQ -->

    <owl:NamedIndividual rdf:about="http://purl.org/olia/susa.owl#RRQ">
        <rdf:type rdf:resource="http://purl.org/olia/susa.owl#WHAdverb"/>
        <olia_system:hasTag>RRQ</olia_system:hasTag>
        <olia_system:hasTier>POS</olia_system:hasTier>
        <rdfs:comment>These are wh-adverbs.</rdfs:comment>
    </owl:NamedIndividual>
    


    <!-- http://purl.org/olia/susa.owl#RRQV -->

    <owl:NamedIndividual rdf:about="http://purl.org/olia/susa.owl#RRQV">
        <rdf:type rdf:resource="http://purl.org/olia/susa.owl#WHAdverb"/>
        <olia_system:hasTag>RRQV</olia_system:hasTag>
        <olia_system:hasTier>POS</olia_system:hasTier>
        <rdfs:comment>RRQV is used for wh-...-ever adverbs, e.g. &quot;however&quot;, &quot;no matter how&quot;, &quot;whenever&quot;, &quot;wherever&quot;, &quot;wheresoever&quot;.</rdfs:comment>
    </owl:NamedIndividual>
    


    <!-- http://purl.org/olia/susa.owl#RRQq -->

    <owl:NamedIndividual rdf:about="http://purl.org/olia/susa.owl#RRQq">
        <rdf:type rdf:resource="http://purl.org/olia/susa.owl#WHAdverb"/>
        <olia_system:hasTag>RRQq</olia_system:hasTag>
        <olia_system:hasTier>POS</olia_system:hasTier>
        <rdfs:comment>These are interrogative (RRQq) wh- adverbs e.g. &quot;how&quot;, &quot;when&quot;, &quot;where&quot;.</rdfs:comment>
    </owl:NamedIndividual>
    


    <!-- http://purl.org/olia/susa.owl#RRQr -->

    <owl:NamedIndividual rdf:about="http://purl.org/olia/susa.owl#RRQr">
        <rdf:type rdf:resource="http://purl.org/olia/susa.owl#WHAdverb"/>
        <olia_system:hasTag>RRQr</olia_system:hasTag>
        <olia_system:hasTier>POS</olia_system:hasTier>
        <rdfs:comment>RRQr is used for relative wh- adverbs (having overt antecedent - not &quot;fused&quot; relative) e.g. &quot;when&quot;, &quot;where&quot;, &quot;whereat&quot;, &quot;whereby&quot;.</rdfs:comment>
    </owl:NamedIndividual>
    


    <!-- http://purl.org/olia/susa.owl#RRR -->

    <owl:NamedIndividual rdf:about="http://purl.org/olia/susa.owl#RRR">
        <rdf:type rdf:resource="http://purl.org/olia/susa.owl#ComparativeAdverb"/>
        <hasDegree rdf:resource="http://purl.org/olia/susa.owl#comparative"/>
        <olia_system:hasTag>RRR</olia_system:hasTag>
        <olia_system:hasTier>POS</olia_system:hasTier>
        <rdfs:comment>RRR is used for a single-word comparative adverb other than &quot;more&quot;, e.g. &quot; better&quot;, &quot;closer&quot;, &quot;deeper&quot;, &quot;earlier&quot; and so on.</rdfs:comment>
    </owl:NamedIndividual>
    


    <!-- http://purl.org/olia/susa.owl#RRT -->

    <owl:NamedIndividual rdf:about="http://purl.org/olia/susa.owl#RRT">
        <rdf:type rdf:resource="http://purl.org/olia/susa.owl#SuperlativeAdverb"/>
        <hasDegree rdf:resource="http://purl.org/olia/susa.owl#superlative"/>
        <olia_system:hasTag>RRT</olia_system:hasTag>
        <olia_system:hasTier>POS</olia_system:hasTier>
        <rdfs:comment>RRT is used for a superlative adverb other than &quot;most&quot;, e.g. &quot;best&quot;, &quot;brightest&quot;, &quot;closest&quot;, &quot;earliest&quot;, &quot;fastest&quot; and so on.</rdfs:comment>
    </owl:NamedIndividual>
    


    <!-- http://purl.org/olia/susa.owl#RRe -->

    <owl:NamedIndividual rdf:about="http://purl.org/olia/susa.owl#RRe">
        <rdf:type rdf:resource="http://purl.org/olia/susa.owl#GeneralAdverb"/>
        <olia_system:hasTag>RRe</olia_system:hasTag>
        <olia_system:hasTier>POS</olia_system:hasTier>
        <rdfs:comment>RRe is the tag for &quot;enough&quot; as clause adverb.</rdfs:comment>
    </owl:NamedIndividual>
    


    <!-- http://purl.org/olia/susa.owl#RRf -->

    <owl:NamedIndividual rdf:about="http://purl.org/olia/susa.owl#RRf">
        <rdf:type rdf:resource="http://purl.org/olia/susa.owl#GeneralAdverb"/>
        <olia_system:hasTag>RRf</olia_system:hasTag>
        <olia_system:hasTier>POS</olia_system:hasTier>
        <rdfs:comment>RRf is used for &quot;far&quot; as adverb.</rdfs:comment>
    </owl:NamedIndividual>
    


    <!-- http://purl.org/olia/susa.owl#RRg -->

    <owl:NamedIndividual rdf:about="http://purl.org/olia/susa.owl#RRg">
        <rdf:type rdf:resource="http://purl.org/olia/susa.owl#GeneralAdverb"/>
        <olia_system:hasTag>RRg</olia_system:hasTag>
        <olia_system:hasTier>POS</olia_system:hasTier>
        <rdfs:comment>RRg is used for &quot;long&quot; as adverb.</rdfs:comment>
    </owl:NamedIndividual>
    


    <!-- http://purl.org/olia/susa.owl#RRs -->

    <owl:NamedIndividual rdf:about="http://purl.org/olia/susa.owl#RRs">
        <rdf:type rdf:resource="http://purl.org/olia/susa.owl#GeneralAdverb"/>
        <olia_system:hasTag>RRs</olia_system:hasTag>
        <olia_system:hasTier>POS</olia_system:hasTier>
        <rdfs:comment>RRs describes &quot;otherwise&quot;, &quot;yet&quot;.</rdfs:comment>
    </owl:NamedIndividual>
    


    <!-- http://purl.org/olia/susa.owl#RRx -->

    <owl:NamedIndividual rdf:about="http://purl.org/olia/susa.owl#RRx">
        <rdf:type rdf:resource="http://purl.org/olia/susa.owl#GeneralAdverb"/>
        <olia_system:hasTag>RRx</olia_system:hasTag>
        <olia_system:hasTier>POS</olia_system:hasTier>
        <rdfs:comment>RRx stands for &quot;only&quot; as adverb.</rdfs:comment>
    </owl:NamedIndividual>
    


    <!-- http://purl.org/olia/susa.owl#RRy -->

    <owl:NamedIndividual rdf:about="http://purl.org/olia/susa.owl#RRy">
        <rdf:type rdf:resource="http://purl.org/olia/susa.owl#GeneralAdverb"/>
        <olia_system:hasTag>RRy</olia_system:hasTag>
        <olia_system:hasTier>POS</olia_system:hasTier>
        <rdfs:comment>RRy is used for &quot;any&quot; as qualifier with comparative.</rdfs:comment>
    </owl:NamedIndividual>
    


    <!-- http://purl.org/olia/susa.owl#RRz -->

    <owl:NamedIndividual rdf:about="http://purl.org/olia/susa.owl#RRz">
        <rdf:type rdf:resource="http://purl.org/olia/susa.owl#GeneralAdverb"/>
        <olia_system:hasTag>RRz</olia_system:hasTag>
        <olia_system:hasTier>POS</olia_system:hasTier>
        <rdfs:comment>RRz is used for &quot;so&quot; introducing a main clause or a clause of purpose or result, or as an adverb of manner or degree.</rdfs:comment>
    </owl:NamedIndividual>
    


    <!-- http://purl.org/olia/susa.owl#RT -->

    <owl:NamedIndividual rdf:about="http://purl.org/olia/susa.owl#RT">
        <rdf:type rdf:resource="http://purl.org/olia/susa.owl#TemporalAdverb"/>
        <olia_system:hasTag>RT</olia_system:hasTag>
        <olia_system:hasTier>POS</olia_system:hasTier>
        <rdfs:comment>RT is the SUSANNE tag used for &quot;again&quot;, &quot;hereafter&quot;, &quot;overnight&quot;.</rdfs:comment>
    </owl:NamedIndividual>
    


    <!-- http://purl.org/olia/susa.owl#RTn -->

    <owl:NamedIndividual rdf:about="http://purl.org/olia/susa.owl#RTn">
        <rdf:type rdf:resource="http://purl.org/olia/susa.owl#TemporalAdverb"/>
        <olia_system:hasTag>RTn</olia_system:hasTag>
        <olia_system:hasTier>POS</olia_system:hasTier>
        <rdfs:comment>RTn is used for &quot;then&quot;.</rdfs:comment>
    </owl:NamedIndividual>
    


    <!-- http://purl.org/olia/susa.owl#RTo -->

    <owl:NamedIndividual rdf:about="http://purl.org/olia/susa.owl#RTo">
        <rdf:type rdf:resource="http://purl.org/olia/susa.owl#TemporalAdverb"/>
        <olia_system:hasTag>RTo</olia_system:hasTag>
        <olia_system:hasTier>POS</olia_system:hasTier>
        <rdfs:comment>RTo is used for &quot;now&quot;.</rdfs:comment>
    </owl:NamedIndividual>
    


    <!-- http://purl.org/olia/susa.owl#RTt -->

    <owl:NamedIndividual rdf:about="http://purl.org/olia/susa.owl#RTt">
        <rdf:type rdf:resource="http://purl.org/olia/susa.owl#TemporalAdverb"/>
        <olia_system:hasTag>RTt</olia_system:hasTag>
        <olia_system:hasTier>POS</olia_system:hasTier>
        <rdfs:comment>RTt is used for &quot;today&quot;, &quot;tomorrow&quot;, &quot;tonight&quot;, &quot;yesterday&quot;.</rdfs:comment>
    </owl:NamedIndividual>
    


    <!-- http://purl.org/olia/susa.owl#TO -->

    <owl:NamedIndividual rdf:about="http://purl.org/olia/susa.owl#TO">
        <rdf:type rdf:resource="http://purl.org/olia/susa.owl#SubordinatingConjunctionWithInfinitival"/>
        <olia_system:hasTag>TO</olia_system:hasTag>
        <olia_system:hasTier>POS</olia_system:hasTier>
        <rdfs:comment>TO is the SUSANNE tag used for the infinitival &quot;to&quot;. It could be analyzed as a sub-type of subordination.
(Sampson 1995, p. 118)</rdfs:comment>
    </owl:NamedIndividual>
    


    <!-- http://purl.org/olia/susa.owl#UH -->

    <owl:NamedIndividual rdf:about="http://purl.org/olia/susa.owl#UH">
        <rdf:type rdf:resource="http://purl.org/olia/susa.owl#Interjection"/>
        <olia_system:hasTag>UH</olia_system:hasTag>
        <olia_system:hasTier>POS</olia_system:hasTier>
        <rdfs:comment>UH is the SUSANNE tag used for an interjection e.g. &quot;blimey&quot;, &quot;hello&quot;, &quot;please&quot;, &quot;well&quot;, &quot;yes&quot;.</rdfs:comment>
    </owl:NamedIndividual>
    


    <!-- http://purl.org/olia/susa.owl#VB0 -->

    <owl:NamedIndividual rdf:about="http://purl.org/olia/susa.owl#VB0">
        <rdf:type rdf:resource="http://purl.org/olia/susa.owl#BeBaseForm"/>
        <hasForm rdf:resource="http://purl.org/olia/susa.owl#base_form"/>
        <olia_system:hasTag>VB0</olia_system:hasTag>
        <olia_system:hasTier>POS</olia_system:hasTier>
        <rdfs:comment>VB0 is used for &quot;be&quot;.</rdfs:comment>
    </owl:NamedIndividual>
    


    <!-- http://purl.org/olia/susa.owl#VBD -->

    <owl:NamedIndividual rdf:about="http://purl.org/olia/susa.owl#VBD">
        <rdf:type rdf:resource="http://purl.org/olia/susa.owl#BePast"/>
        <hasForm rdf:resource="http://purl.org/olia/susa.owl#inflected_form"/>
        <hasTense rdf:resource="http://purl.org/olia/susa.owl#past"/>
        <olia_system:hasTag>VBD</olia_system:hasTag>
        <olia_system:hasTier>POS</olia_system:hasTier>
        <rdfs:comment>VBD is used for the past forms of be.</rdfs:comment>
    </owl:NamedIndividual>
    


    <!-- http://purl.org/olia/susa.owl#VBDR -->

    <owl:NamedIndividual rdf:about="http://purl.org/olia/susa.owl#VBDR">
        <rdf:type rdf:resource="http://purl.org/olia/susa.owl#BePast"/>
        <hasForm rdf:resource="http://purl.org/olia/susa.owl#inflected_form"/>
        <hasTense rdf:resource="http://purl.org/olia/susa.owl#past"/>
        <olia_system:hasTag>VBDR</olia_system:hasTag>
        <olia_system:hasTier>POS</olia_system:hasTier>
        <rdfs:comment>VBDR is used for &quot;were&quot;.</rdfs:comment>
    </owl:NamedIndividual>
    


    <!-- http://purl.org/olia/susa.owl#VBDZ -->

    <owl:NamedIndividual rdf:about="http://purl.org/olia/susa.owl#VBDZ">
        <rdf:type rdf:resource="http://purl.org/olia/susa.owl#BePast"/>
        <hasForm rdf:resource="http://purl.org/olia/susa.owl#inflected_form"/>
        <hasTense rdf:resource="http://purl.org/olia/susa.owl#past"/>
        <olia_system:hasTag>VBDZ</olia_system:hasTag>
        <olia_system:hasTier>POS</olia_system:hasTier>
        <rdfs:comment>VBDZ is used for &quot;was&quot;.</rdfs:comment>
    </owl:NamedIndividual>
    


    <!-- http://purl.org/olia/susa.owl#VBG -->

    <owl:NamedIndividual rdf:about="http://purl.org/olia/susa.owl#VBG">
        <rdf:type rdf:resource="http://purl.org/olia/susa.owl#BePresentParticiple"/>
        <hasForm rdf:resource="http://purl.org/olia/susa.owl#inflected_form"/>
        <olia_system:hasTag>VBG</olia_system:hasTag>
        <olia_system:hasTier>POS</olia_system:hasTier>
        <rdfs:comment>VBG is used for &quot;being&quot;.</rdfs:comment>
    </owl:NamedIndividual>
    


    <!-- http://purl.org/olia/susa.owl#VBM -->

    <owl:NamedIndividual rdf:about="http://purl.org/olia/susa.owl#VBM">
        <rdf:type rdf:resource="http://purl.org/olia/susa.owl#Am"/>
        <hasForm rdf:resource="http://purl.org/olia/susa.owl#inflected_form"/>
        <hasTense rdf:resource="http://purl.org/olia/susa.owl#present"/>
        <olia_system:hasTag>VBM</olia_system:hasTag>
        <olia_system:hasTier>POS</olia_system:hasTier>
        <rdfs:comment>The SUSANNE tag VBM is used for &quot;am&quot;.</rdfs:comment>
    </owl:NamedIndividual>
    


    <!-- http://purl.org/olia/susa.owl#VBN -->

    <owl:NamedIndividual rdf:about="http://purl.org/olia/susa.owl#VBN">
        <rdf:type rdf:resource="http://purl.org/olia/susa.owl#BePastParticiple"/>
        <hasForm rdf:resource="http://purl.org/olia/susa.owl#inflected_form"/>
        <olia_system:hasTag>VBN</olia_system:hasTag>
        <olia_system:hasTier>POS</olia_system:hasTier>
        <rdfs:comment>This is the SUSANNE tag used for &quot;been&quot;.</rdfs:comment>
    </owl:NamedIndividual>
    


    <!-- http://purl.org/olia/susa.owl#VBR -->

    <owl:NamedIndividual rdf:about="http://purl.org/olia/susa.owl#VBR">
        <rdf:type rdf:resource="http://purl.org/olia/susa.owl#Are"/>
        <hasForm rdf:resource="http://purl.org/olia/susa.owl#inflected_form"/>
        <olia_system:hasTag>VBR</olia_system:hasTag>
        <olia_system:hasTier>POS</olia_system:hasTier>
        <rdfs:comment>VBR is used for &quot;are&quot;.</rdfs:comment>
    </owl:NamedIndividual>
    


    <!-- http://purl.org/olia/susa.owl#VBZ -->

    <owl:NamedIndividual rdf:about="http://purl.org/olia/susa.owl#VBZ">
        <rdf:type rdf:resource="http://purl.org/olia/susa.owl#Is"/>
        <hasForm rdf:resource="http://purl.org/olia/susa.owl#inflected_form"/>
        <hasTense rdf:resource="http://purl.org/olia/susa.owl#present"/>
        <olia_system:hasTag>VBZ</olia_system:hasTag>
        <olia_system:hasTier>POS</olia_system:hasTier>
        <rdfs:comment>The SUSANNE tag VBZ is used for &quot;is&quot;.</rdfs:comment>
    </owl:NamedIndividual>
    


    <!-- http://purl.org/olia/susa.owl#VD0 -->

    <owl:NamedIndividual rdf:about="http://purl.org/olia/susa.owl#VD0">
        <rdf:type rdf:resource="http://purl.org/olia/susa.owl#DoBaseForm"/>
        <hasForm rdf:resource="http://purl.org/olia/susa.owl#base_form"/>
        <hasTense rdf:resource="http://purl.org/olia/susa.owl#present"/>
        <olia_system:hasTag>VD0</olia_system:hasTag>
        <olia_system:hasTier>POS</olia_system:hasTier>
        <rdfs:comment>The SUSANNE tag VD0 is used for &quot;do&quot; as infinitive or as indicative.</rdfs:comment>
    </owl:NamedIndividual>
    


    <!-- http://purl.org/olia/susa.owl#VDD -->

    <owl:NamedIndividual rdf:about="http://purl.org/olia/susa.owl#VDD">
        <rdf:type rdf:resource="http://purl.org/olia/susa.owl#DoPast"/>
        <hasForm rdf:resource="http://purl.org/olia/susa.owl#inflected_form"/>
        <hasTense rdf:resource="http://purl.org/olia/susa.owl#past"/>
        <olia_system:hasTag>VDD</olia_system:hasTag>
        <olia_system:hasTier>POS</olia_system:hasTier>
        <rdfs:comment>VDD is used for &quot;did&quot;.</rdfs:comment>
    </owl:NamedIndividual>
    


    <!-- http://purl.org/olia/susa.owl#VDG -->

    <owl:NamedIndividual rdf:about="http://purl.org/olia/susa.owl#VDG">
        <rdf:type rdf:resource="http://purl.org/olia/susa.owl#DoPresentParticiple"/>
        <hasForm rdf:resource="http://purl.org/olia/susa.owl#inflected_form"/>
        <olia_system:hasTag>VDG</olia_system:hasTag>
        <olia_system:hasTier>POS</olia_system:hasTier>
        <rdfs:comment>This is the SUSANNE tag used for &quot;doing&quot;.</rdfs:comment>
    </owl:NamedIndividual>
    


    <!-- http://purl.org/olia/susa.owl#VDN -->

    <owl:NamedIndividual rdf:about="http://purl.org/olia/susa.owl#VDN">
        <rdf:type rdf:resource="http://purl.org/olia/susa.owl#DoPastParticiple"/>
        <hasForm rdf:resource="http://purl.org/olia/susa.owl#inflected_form"/>
        <hasTense rdf:resource="http://purl.org/olia/susa.owl#past"/>
        <olia_system:hasTag>VDN</olia_system:hasTag>
        <olia_system:hasTier>POS</olia_system:hasTier>
        <rdfs:comment>The VDN tag describes &quot;done&quot;.</rdfs:comment>
    </owl:NamedIndividual>
    


    <!-- http://purl.org/olia/susa.owl#VDZ -->

    <owl:NamedIndividual rdf:about="http://purl.org/olia/susa.owl#VDZ">
        <rdf:type rdf:resource="http://purl.org/olia/susa.owl#Does"/>
        <hasForm rdf:resource="http://purl.org/olia/susa.owl#inflected_form"/>
        <hasTense rdf:resource="http://purl.org/olia/susa.owl#present"/>
        <olia_system:hasTag>VDZ</olia_system:hasTag>
        <olia_system:hasTier>POS</olia_system:hasTier>
        <rdfs:comment>VDZ is used for &quot;does&quot;.</rdfs:comment>
    </owl:NamedIndividual>
    


    <!-- http://purl.org/olia/susa.owl#VH0 -->

    <owl:NamedIndividual rdf:about="http://purl.org/olia/susa.owl#VH0">
        <rdf:type rdf:resource="http://purl.org/olia/susa.owl#HaveBaseForm"/>
        <hasForm rdf:resource="http://purl.org/olia/susa.owl#base_form"/>
        <hasTense rdf:resource="http://purl.org/olia/susa.owl#present"/>
        <olia_system:hasTag>VH0</olia_system:hasTag>
        <olia_system:hasTier>POS</olia_system:hasTier>
        <rdfs:comment>The SUSANNE tag VH0 is used for &quot;have&quot;.</rdfs:comment>
    </owl:NamedIndividual>
    


    <!-- http://purl.org/olia/susa.owl#VHD -->

    <owl:NamedIndividual rdf:about="http://purl.org/olia/susa.owl#VHD">
        <rdf:type rdf:resource="http://purl.org/olia/susa.owl#HavePast"/>
        <hasForm rdf:resource="http://purl.org/olia/susa.owl#inflected_form"/>
        <hasTense rdf:resource="http://purl.org/olia/susa.owl#past"/>
        <olia_system:hasTag>VHD</olia_system:hasTag>
        <olia_system:hasTier>POS</olia_system:hasTier>
        <rdfs:comment>The SUSANNE tag VHD is used for the past tense form &quot;had&quot;.</rdfs:comment>
    </owl:NamedIndividual>
    


    <!-- http://purl.org/olia/susa.owl#VHG -->

    <owl:NamedIndividual rdf:about="http://purl.org/olia/susa.owl#VHG">
        <rdf:type rdf:resource="http://purl.org/olia/susa.owl#HavePresentParticiple"/>
        <hasForm rdf:resource="http://purl.org/olia/susa.owl#inflected_form"/>
        <olia_system:hasTag>VHG</olia_system:hasTag>
        <olia_system:hasTier>POS</olia_system:hasTier>
        <rdfs:comment>The SUSANNE tag VHG is used for &quot;having&quot;.</rdfs:comment>
    </owl:NamedIndividual>
    


    <!-- http://purl.org/olia/susa.owl#VHN -->

    <owl:NamedIndividual rdf:about="http://purl.org/olia/susa.owl#VHN">
        <rdf:type rdf:resource="http://purl.org/olia/susa.owl#HavePastParticiple"/>
        <hasForm rdf:resource="http://purl.org/olia/susa.owl#inflected_form"/>
        <hasTense rdf:resource="http://purl.org/olia/susa.owl#past"/>
        <olia_system:hasTag>VHN</olia_system:hasTag>
        <olia_system:hasTier>POS</olia_system:hasTier>
        <rdfs:comment>The SUSANNE tag VHN is used for the past participle form &quot;had&quot;.</rdfs:comment>
    </owl:NamedIndividual>
    


    <!-- http://purl.org/olia/susa.owl#VHZ -->

    <owl:NamedIndividual rdf:about="http://purl.org/olia/susa.owl#VHZ">
        <rdf:type rdf:resource="http://purl.org/olia/susa.owl#Has"/>
        <hasForm rdf:resource="http://purl.org/olia/susa.owl#inflected_form"/>
        <hasTense rdf:resource="http://purl.org/olia/susa.owl#present"/>
        <olia_system:hasTag>VHZ</olia_system:hasTag>
        <olia_system:hasTier>POS</olia_system:hasTier>
        <rdfs:comment>The SUSANNE tag VHZ is used for &quot;has&quot;.</rdfs:comment>
    </owl:NamedIndividual>
    


    <!-- http://purl.org/olia/susa.owl#VM -->

    <owl:NamedIndividual rdf:about="http://purl.org/olia/susa.owl#VM">
        <rdf:type rdf:resource="http://purl.org/olia/susa.owl#ModalVerbPast"/>
        <hasForm rdf:resource="http://purl.org/olia/susa.owl#inflected_form"/>
        <hasTense rdf:resource="http://purl.org/olia/susa.owl#past"/>
        <olia_system:hasTag>VM</olia_system:hasTag>
        <olia_system:hasTier>POS</olia_system:hasTier>
        <rdfs:comment>VM  is used for modal verbforms.</rdfs:comment>
        <owl:versionInfo>added by Johannes Bubenzer (2006-09-09) in accordance to a
	TnT-tagged data set provided by SFB 538 (Hamburg), project K4</owl:versionInfo>
    </owl:NamedIndividual>
    


    <!-- http://purl.org/olia/susa.owl#VMK -->

    <owl:NamedIndividual rdf:about="http://purl.org/olia/susa.owl#VMK">
        <rdf:type rdf:resource="http://purl.org/olia/susa.owl#CatenativeModalVerb"/>
        <hasForm rdf:resource="http://purl.org/olia/susa.owl#inflected_form"/>
        <hasTense rdf:resource="http://purl.org/olia/susa.owl#past"/>
        <olia_system:hasTag>VMK</olia_system:hasTag>
        <olia_system:hasTier>POS</olia_system:hasTier>
        <rdfs:comment>The SUSANNE tag VMK is used for &quot;ought used&quot; as modal catenative.</rdfs:comment>
    </owl:NamedIndividual>
    


    <!-- http://purl.org/olia/susa.owl#VMd -->

    <owl:NamedIndividual rdf:about="http://purl.org/olia/susa.owl#VMd">
        <rdf:type rdf:resource="http://purl.org/olia/susa.owl#ModalVerbPast"/>
        <hasForm rdf:resource="http://purl.org/olia/susa.owl#inflected_form"/>
        <hasTense rdf:resource="http://purl.org/olia/susa.owl#past"/>
        <olia_system:hasTag>VMd</olia_system:hasTag>
        <olia_system:hasTier>POS</olia_system:hasTier>
        <rdfs:comment>The SUSANNE tag VMd is used for modals in past form e.g. &quot;could&quot;, &quot;might&quot;, &quot;should&quot;, &quot;would&quot;.</rdfs:comment>
    </owl:NamedIndividual>
    


    <!-- http://purl.org/olia/susa.owl#VMo -->

    <owl:NamedIndividual rdf:about="http://purl.org/olia/susa.owl#VMo">
        <rdf:type rdf:resource="http://purl.org/olia/susa.owl#ModalVerbBaseForm"/>
        <hasForm rdf:resource="http://purl.org/olia/susa.owl#base_form"/>
        <olia_system:hasTag>VMo</olia_system:hasTag>
        <olia_system:hasTier>POS</olia_system:hasTier>
        <rdfs:comment>The SUSANNE tag VMo is used for modals in present form e.g. &quot;can&quot;, &quot;dare&quot;, &quot;may&quot;, &quot;must&quot;, &quot;need&quot;, &quot;shall&quot;, &quot;will&quot;.</rdfs:comment>
    </owl:NamedIndividual>
    


    <!-- http://purl.org/olia/susa.owl#VV0 -->

    <owl:NamedIndividual rdf:about="http://purl.org/olia/susa.owl#VV0">
        <rdf:type rdf:resource="http://purl.org/olia/susa.owl#LexicalVerbBaseForm"/>
        <hasForm rdf:resource="http://purl.org/olia/susa.owl#base_form"/>
        <olia_system:hasTag>VV0</olia_system:hasTag>
        <olia_system:hasTier>POS</olia_system:hasTier>
        <rdfs:comment>These are base form of verbs.</rdfs:comment>
    </owl:NamedIndividual>
    


    <!-- http://purl.org/olia/susa.owl#VV0i -->

    <owl:NamedIndividual rdf:about="http://purl.org/olia/susa.owl#VV0i">
        <rdf:type rdf:resource="http://purl.org/olia/susa.owl#LexicalVerbBaseForm"/>
        <hasForm rdf:resource="http://purl.org/olia/susa.owl#base_form"/>
        <olia_system:hasTag>VV0i</olia_system:hasTag>
        <olia_system:hasTier>POS</olia_system:hasTier>
        <rdfs:comment>VV0i is used for the base form of intransitive verbs.</rdfs:comment>
    </owl:NamedIndividual>
    


    <!-- http://purl.org/olia/susa.owl#VV0t -->

    <owl:NamedIndividual rdf:about="http://purl.org/olia/susa.owl#VV0t">
        <rdf:type rdf:resource="http://purl.org/olia/susa.owl#LexicalVerbBaseForm"/>
        <hasForm rdf:resource="http://purl.org/olia/susa.owl#base_form"/>
        <olia_system:hasTag>VV0t</olia_system:hasTag>
        <olia_system:hasTier>POS</olia_system:hasTier>
        <rdfs:comment>The base form of transitive verbs is tagged with VV0t.</rdfs:comment>
    </owl:NamedIndividual>
    


    <!-- http://purl.org/olia/susa.owl#VV0v -->

    <owl:NamedIndividual rdf:about="http://purl.org/olia/susa.owl#VV0v">
        <rdf:type rdf:resource="http://purl.org/olia/susa.owl#LexicalVerbBaseForm"/>
        <hasForm rdf:resource="http://purl.org/olia/susa.owl#base_form"/>
        <olia_system:hasTag>VV0v</olia_system:hasTag>
        <olia_system:hasTier>POS</olia_system:hasTier>
        <rdfs:comment>VV0v is used for the base form of verbs which have transitive and intransitive uses.</rdfs:comment>
    </owl:NamedIndividual>
    


    <!-- http://purl.org/olia/susa.owl#VVD -->

    <owl:NamedIndividual rdf:about="http://purl.org/olia/susa.owl#VVD">
        <rdf:type rdf:resource="http://purl.org/olia/susa.owl#LexicalVerbPastForm"/>
        <hasForm rdf:resource="http://purl.org/olia/susa.owl#inflected_form"/>
        <hasTense rdf:resource="http://purl.org/olia/susa.owl#past"/>
        <olia_system:hasTag>VVD</olia_system:hasTag>
        <olia_system:hasTier>POS</olia_system:hasTier>
        <rdfs:comment>VVD is used for past tense verbforms.</rdfs:comment>
    </owl:NamedIndividual>
    


    <!-- http://purl.org/olia/susa.owl#VVDi -->

    <owl:NamedIndividual rdf:about="http://purl.org/olia/susa.owl#VVDi">
        <rdf:type rdf:resource="http://purl.org/olia/susa.owl#LexicalVerbPastForm"/>
        <hasForm rdf:resource="http://purl.org/olia/susa.owl#inflected_form"/>
        <hasTense rdf:resource="http://purl.org/olia/susa.owl#past"/>
        <hasValency rdf:resource="http://purl.org/olia/susa.owl#intransitive"/>
        <olia_system:hasTag>VVDi</olia_system:hasTag>
        <olia_system:hasTier>POS</olia_system:hasTier>
        <rdfs:comment>VVDi is used for the past tense form of intransitive verbs.</rdfs:comment>
    </owl:NamedIndividual>
    


    <!-- http://purl.org/olia/susa.owl#VVDt -->

    <owl:NamedIndividual rdf:about="http://purl.org/olia/susa.owl#VVDt">
        <rdf:type rdf:resource="http://purl.org/olia/susa.owl#LexicalVerbPastForm"/>
        <hasForm rdf:resource="http://purl.org/olia/susa.owl#inflected_form"/>
        <hasTense rdf:resource="http://purl.org/olia/susa.owl#past"/>
        <hasValency rdf:resource="http://purl.org/olia/susa.owl#transitive"/>
        <olia_system:hasTag>VVDt</olia_system:hasTag>
        <olia_system:hasTier>POS</olia_system:hasTier>
        <rdfs:comment>The past tense form of transitive verbs is tagged with VVDt.</rdfs:comment>
    </owl:NamedIndividual>
    


    <!-- http://purl.org/olia/susa.owl#VVDv -->

    <owl:NamedIndividual rdf:about="http://purl.org/olia/susa.owl#VVDv">
        <rdf:type rdf:resource="http://purl.org/olia/susa.owl#LexicalVerbPastForm"/>
        <hasForm rdf:resource="http://purl.org/olia/susa.owl#inflected_form"/>
        <hasTense rdf:resource="http://purl.org/olia/susa.owl#past"/>
        <olia_system:hasTag>VVDv</olia_system:hasTag>
        <olia_system:hasTier>POS</olia_system:hasTier>
        <rdfs:comment>VVDv describes the past tense form of verbs which have transitive and intransitive uses.</rdfs:comment>
    </owl:NamedIndividual>
    


    <!-- http://purl.org/olia/susa.owl#VVG -->

    <owl:NamedIndividual rdf:about="http://purl.org/olia/susa.owl#VVG">
        <rdf:type rdf:resource="http://purl.org/olia/susa.owl#LexicalVerbPresentParticiple"/>
        <hasForm rdf:resource="http://purl.org/olia/susa.owl#inflected_form"/>
        <hasTense rdf:resource="http://purl.org/olia/susa.owl#present"/>
        <olia_system:hasTag>VVG</olia_system:hasTag>
        <olia_system:hasTier>POS</olia_system:hasTier>
        <rdfs:comment>VVG is used for present participle verbforms.</rdfs:comment>
    </owl:NamedIndividual>
    


    <!-- http://purl.org/olia/susa.owl#VVGK -->

    <owl:NamedIndividual rdf:about="http://purl.org/olia/susa.owl#VVGK">
        <rdf:type rdf:resource="http://purl.org/olia/susa.owl#LexicalVerbPresentParticiple"/>
        <hasForm rdf:resource="http://purl.org/olia/susa.owl#inflected_form"/>
        <hasTense rdf:resource="http://purl.org/olia/susa.owl#present"/>
        <olia_system:hasTag>VVGK</olia_system:hasTag>
        <olia_system:hasTier>POS</olia_system:hasTier>
        <rdfs:comment>VVGK is used for &quot;going&quot; as catenative (in BE &quot;going to&quot;).</rdfs:comment>
    </owl:NamedIndividual>
    


    <!-- http://purl.org/olia/susa.owl#VVGi -->

    <owl:NamedIndividual rdf:about="http://purl.org/olia/susa.owl#VVGi">
        <rdf:type rdf:resource="http://purl.org/olia/susa.owl#LexicalVerbPresentParticiple"/>
        <hasForm rdf:resource="http://purl.org/olia/susa.owl#inflected_form"/>
        <hasTense rdf:resource="http://purl.org/olia/susa.owl#present"/>
        <hasValency rdf:resource="http://purl.org/olia/susa.owl#intransitive"/>
        <olia_system:hasTag>VVGi</olia_system:hasTag>
        <olia_system:hasTier>POS</olia_system:hasTier>
        <rdfs:comment>VVGi is used for present participle intransitive verbforms.</rdfs:comment>
    </owl:NamedIndividual>
    


    <!-- http://purl.org/olia/susa.owl#VVGt -->

    <owl:NamedIndividual rdf:about="http://purl.org/olia/susa.owl#VVGt">
        <rdf:type rdf:resource="http://purl.org/olia/susa.owl#LexicalVerbPresentParticiple"/>
        <hasForm rdf:resource="http://purl.org/olia/susa.owl#inflected_form"/>
        <hasTense rdf:resource="http://purl.org/olia/susa.owl#present"/>
        <hasValency rdf:resource="http://purl.org/olia/susa.owl#transitive"/>
        <olia_system:hasTag>VVGt</olia_system:hasTag>
        <olia_system:hasTier>POS</olia_system:hasTier>
        <rdfs:comment>The present participle form of transitive verbs is tagged with VVGt.</rdfs:comment>
    </owl:NamedIndividual>
    


    <!-- http://purl.org/olia/susa.owl#VVGv -->

    <owl:NamedIndividual rdf:about="http://purl.org/olia/susa.owl#VVGv">
        <rdf:type rdf:resource="http://purl.org/olia/susa.owl#LexicalVerbPresentParticiple"/>
        <hasForm rdf:resource="http://purl.org/olia/susa.owl#inflected_form"/>
        <hasTense rdf:resource="http://purl.org/olia/susa.owl#present"/>
        <olia_system:hasTag>VVGv</olia_system:hasTag>
        <olia_system:hasTier>POS</olia_system:hasTier>
        <rdfs:comment>VVGv describes the present participle form of verbs which have transitive and intransitive uses.</rdfs:comment>
    </owl:NamedIndividual>
    


    <!-- http://purl.org/olia/susa.owl#VVN -->

    <owl:NamedIndividual rdf:about="http://purl.org/olia/susa.owl#VVN">
        <rdf:type rdf:resource="http://purl.org/olia/susa.owl#LexicalVerbPastParticiple"/>
        <hasForm rdf:resource="http://purl.org/olia/susa.owl#inflected_form"/>
        <hasTense rdf:resource="http://purl.org/olia/susa.owl#past"/>
        <olia_system:hasTag>VVN</olia_system:hasTag>
        <olia_system:hasTier>POS</olia_system:hasTier>
        <rdfs:comment>VVN iS used for the past participle verbforms.</rdfs:comment>
    </owl:NamedIndividual>
    


    <!-- http://purl.org/olia/susa.owl#VVNi -->

    <owl:NamedIndividual rdf:about="http://purl.org/olia/susa.owl#VVNi">
        <rdf:type rdf:resource="http://purl.org/olia/susa.owl#LexicalVerbPastParticiple"/>
        <hasForm rdf:resource="http://purl.org/olia/susa.owl#inflected_form"/>
        <hasTense rdf:resource="http://purl.org/olia/susa.owl#past"/>
        <hasValency rdf:resource="http://purl.org/olia/susa.owl#intransitive"/>
        <olia_system:hasTag>VVNi</olia_system:hasTag>
        <olia_system:hasTier>POS</olia_system:hasTier>
        <rdfs:comment>VVNi used for the past participle of intransitive verbs</rdfs:comment>
    </owl:NamedIndividual>
    


    <!-- http://purl.org/olia/susa.owl#VVNt -->

    <owl:NamedIndividual rdf:about="http://purl.org/olia/susa.owl#VVNt">
        <rdf:type rdf:resource="http://purl.org/olia/susa.owl#LexicalVerbPastParticiple"/>
        <hasForm rdf:resource="http://purl.org/olia/susa.owl#inflected_form"/>
        <hasTense rdf:resource="http://purl.org/olia/susa.owl#past"/>
        <hasValency rdf:resource="http://purl.org/olia/susa.owl#transitive"/>
        <olia_system:hasTag>VVNt</olia_system:hasTag>
        <olia_system:hasTier>POS</olia_system:hasTier>
        <rdfs:comment>VVNt used for the past participle of transitive verbs.</rdfs:comment>
    </owl:NamedIndividual>
    


    <!-- http://purl.org/olia/susa.owl#VVNv -->

    <owl:NamedIndividual rdf:about="http://purl.org/olia/susa.owl#VVNv">
        <rdf:type rdf:resource="http://purl.org/olia/susa.owl#LexicalVerbPastParticiple"/>
        <hasForm rdf:resource="http://purl.org/olia/susa.owl#inflected_form"/>
        <hasTense rdf:resource="http://purl.org/olia/susa.owl#past"/>
        <olia_system:hasTag>VVNv</olia_system:hasTag>
        <olia_system:hasTier>POS</olia_system:hasTier>
        <rdfs:comment>VVNv for the past participle of verbs having transitive and intransitive uses.</rdfs:comment>
    </owl:NamedIndividual>
    


    <!-- http://purl.org/olia/susa.owl#VVZ -->

    <owl:NamedIndividual rdf:about="http://purl.org/olia/susa.owl#VVZ">
        <rdf:type rdf:resource="http://purl.org/olia/susa.owl#LexicalVerbThirdPerson"/>
        <hasForm rdf:resource="http://purl.org/olia/susa.owl#inflected_form"/>
        <hasNumber rdf:resource="http://purl.org/olia/susa.owl#singular"/>
        <hasPerson rdf:resource="http://purl.org/olia/susa.owl#third"/>
        <hasTense rdf:resource="http://purl.org/olia/susa.owl#present"/>
        <olia_system:hasTag>VVZ</olia_system:hasTag>
        <olia_system:hasTier>POS</olia_system:hasTier>
        <rdfs:comment>VVZ is used  for the third person singular verbforms.</rdfs:comment>
    </owl:NamedIndividual>
    


    <!-- http://purl.org/olia/susa.owl#VVZi -->

    <owl:NamedIndividual rdf:about="http://purl.org/olia/susa.owl#VVZi">
        <rdf:type rdf:resource="http://purl.org/olia/susa.owl#LexicalVerbThirdPerson"/>
        <hasForm rdf:resource="http://purl.org/olia/susa.owl#inflected_form"/>
        <hasNumber rdf:resource="http://purl.org/olia/susa.owl#singular"/>
        <hasPerson rdf:resource="http://purl.org/olia/susa.owl#third"/>
        <hasTense rdf:resource="http://purl.org/olia/susa.owl#present"/>
        <hasValency rdf:resource="http://purl.org/olia/susa.owl#intransitive"/>
        <olia_system:hasTag>VVZi</olia_system:hasTag>
        <olia_system:hasTier>POS</olia_system:hasTier>
        <rdfs:comment>VVZi is used for the third person singular form of intransitive verbs.</rdfs:comment>
    </owl:NamedIndividual>
    


    <!-- http://purl.org/olia/susa.owl#VVZt -->

    <owl:NamedIndividual rdf:about="http://purl.org/olia/susa.owl#VVZt">
        <rdf:type rdf:resource="http://purl.org/olia/susa.owl#LexicalVerbThirdPerson"/>
        <hasForm rdf:resource="http://purl.org/olia/susa.owl#inflected_form"/>
        <hasNumber rdf:resource="http://purl.org/olia/susa.owl#singular"/>
        <hasPerson rdf:resource="http://purl.org/olia/susa.owl#third"/>
        <hasTense rdf:resource="http://purl.org/olia/susa.owl#present"/>
        <hasValency rdf:resource="http://purl.org/olia/susa.owl#transitive"/>
        <olia_system:hasTag>VVZt</olia_system:hasTag>
        <olia_system:hasTier>POS</olia_system:hasTier>
        <rdfs:comment>The third person singular form of transitive verbs is tagged with VVZt.</rdfs:comment>
    </owl:NamedIndividual>
    


    <!-- http://purl.org/olia/susa.owl#VVZv -->

    <owl:NamedIndividual rdf:about="http://purl.org/olia/susa.owl#VVZv">
        <rdf:type rdf:resource="http://purl.org/olia/susa.owl#LexicalVerbThirdPerson"/>
        <hasForm rdf:resource="http://purl.org/olia/susa.owl#inflected_form"/>
        <hasNumber rdf:resource="http://purl.org/olia/susa.owl#singular"/>
        <hasPerson rdf:resource="http://purl.org/olia/susa.owl#third"/>
        <hasTense rdf:resource="http://purl.org/olia/susa.owl#present"/>
        <olia_system:hasTag>VVZv</olia_system:hasTag>
        <olia_system:hasTier>POS</olia_system:hasTier>
        <rdfs:comment>VVZv describes the third person singular form of verbs which have transitive and intransitive uses.</rdfs:comment>
    </owl:NamedIndividual>
    


    <!-- http://purl.org/olia/susa.owl#XX-Tag -->

    <owl:NamedIndividual rdf:about="http://purl.org/olia/susa.owl#XX-Tag">
        <rdf:type rdf:resource="http://purl.org/olia/susa.owl#Not"/>
        <olia_system:hasTag>XX</olia_system:hasTag>
        <olia_system:hasTag>XX-Tag</olia_system:hasTag>
        <olia_system:hasTier>POS</olia_system:hasTier>
        <rdfs:comment>XX is the SUSANNE tag used for &quot;not&quot;.</rdfs:comment>
    </owl:NamedIndividual>
    


    <!-- http://purl.org/olia/susa.owl#YB -->

    <owl:NamedIndividual rdf:about="http://purl.org/olia/susa.owl#YB">
        <rdf:type rdf:resource="http://purl.org/olia/susa.owl#Punctuation"/>
        <olia_system:hasTag>YB</olia_system:hasTag>
        <olia_system:hasTier>POS</olia_system:hasTier>
        <rdfs:comment>YB is the SUSANNE tag used for text devisions of a paragraph or a higher rank which do not have a heading: &lt;majbrk&gt; &lt;minbrk&gt;.</rdfs:comment>
    </owl:NamedIndividual>
    


    <!-- http://purl.org/olia/susa.owl#YBL -->

    <owl:NamedIndividual rdf:about="http://purl.org/olia/susa.owl#YBL">
        <rdf:type rdf:resource="http://purl.org/olia/susa.owl#Punctuation"/>
        <olia_system:hasTag>YBL</olia_system:hasTag>
        <olia_system:hasTier>POS</olia_system:hasTier>
        <rdfs:comment>YBL describes the beginning of  heading: &lt;bmajhd&gt; &lt;bminhd&gt;.</rdfs:comment>
    </owl:NamedIndividual>
    


    <!-- http://purl.org/olia/susa.owl#YBR -->

    <owl:NamedIndividual rdf:about="http://purl.org/olia/susa.owl#YBR">
        <rdf:type rdf:resource="http://purl.org/olia/susa.owl#Punctuation"/>
        <olia_system:hasTag>YBR</olia_system:hasTag>
        <olia_system:hasTier>POS</olia_system:hasTier>
        <rdfs:comment>YBR tags the end of heading &lt;emajhd&gt; &lt;eminhd&gt;.</rdfs:comment>
    </owl:NamedIndividual>
    


    <!-- http://purl.org/olia/susa.owl#YC -->

    <owl:NamedIndividual rdf:about="http://purl.org/olia/susa.owl#YC">
        <rdf:type rdf:resource="http://purl.org/olia/susa.owl#Punctuation"/>
        <olia_system:hasTag>YC</olia_system:hasTag>
        <olia_system:hasTier>POS</olia_system:hasTier>
        <rdfs:comment>YC is the SUSANNE tag used for comma.</rdfs:comment>
    </owl:NamedIndividual>
    


    <!-- http://purl.org/olia/susa.owl#YD -->

    <owl:NamedIndividual rdf:about="http://purl.org/olia/susa.owl#YD">
        <rdf:type rdf:resource="http://purl.org/olia/susa.owl#Punctuation"/>
        <olia_system:hasTag>YD</olia_system:hasTag>
        <olia_system:hasTier>POS</olia_system:hasTier>
        <rdfs:comment>YD is the SUSANNE tag used for dash (em-dash or larger).</rdfs:comment>
    </owl:NamedIndividual>
    


    <!-- http://purl.org/olia/susa.owl#YE -->

    <owl:NamedIndividual rdf:about="http://purl.org/olia/susa.owl#YE">
        <rdf:type rdf:resource="http://purl.org/olia/susa.owl#Punctuation"/>
        <olia_system:hasTag>YE</olia_system:hasTag>
        <olia_system:hasTier>POS</olia_system:hasTier>
        <rdfs:comment>YE is the SUSANNE tag used for the ellipsis mark &quot;...&quot;.</rdfs:comment>
    </owl:NamedIndividual>
    


    <!-- http://purl.org/olia/susa.owl#YF -->

    <owl:NamedIndividual rdf:about="http://purl.org/olia/susa.owl#YF">
        <rdf:type rdf:resource="http://purl.org/olia/susa.owl#Punctuation"/>
        <olia_system:hasTag>YF</olia_system:hasTag>
        <olia_system:hasTier>POS</olia_system:hasTier>
        <rdfs:comment>YF is the SUSANNE tag used for the full stop, American &quot;period&quot;, &quot;.&quot;.</rdfs:comment>
    </owl:NamedIndividual>
    


    <!-- http://purl.org/olia/susa.owl#YG -->

    <owl:NamedIndividual rdf:about="http://purl.org/olia/susa.owl#YG">
        <rdf:type rdf:resource="http://purl.org/olia/susa.owl#Punctuation"/>
        <olia_system:hasTag>YG</olia_system:hasTag>
        <olia_system:hasTier>POS</olia_system:hasTier>
        <rdfs:comment>YG is the SUSANNE tag used for a logical position of a transformationally moved/deleted item.</rdfs:comment>
    </owl:NamedIndividual>
    


    <!-- http://purl.org/olia/susa.owl#YH -->

    <owl:NamedIndividual rdf:about="http://purl.org/olia/susa.owl#YH">
        <rdf:type rdf:resource="http://purl.org/olia/susa.owl#Punctuation"/>
        <olia_system:hasTag>YH</olia_system:hasTag>
        <olia_system:hasTier>POS</olia_system:hasTier>
        <rdfs:comment>YH is the SUSANNE tag used for a hyphen, &quot;-&quot; dash.</rdfs:comment>
    </owl:NamedIndividual>
    


    <!-- http://purl.org/olia/susa.owl#YIL -->

    <owl:NamedIndividual rdf:about="http://purl.org/olia/susa.owl#YIL">
        <rdf:type rdf:resource="http://purl.org/olia/susa.owl#Punctuation"/>
        <olia_system:hasTag>YIL</olia_system:hasTag>
        <olia_system:hasTier>POS</olia_system:hasTier>
        <rdfs:comment>YIL is the SUSANNE tag used for left quotes, opening (single or double) inverted commas.</rdfs:comment>
    </owl:NamedIndividual>
    


    <!-- http://purl.org/olia/susa.owl#YIR -->

    <owl:NamedIndividual rdf:about="http://purl.org/olia/susa.owl#YIR">
        <rdf:type rdf:resource="http://purl.org/olia/susa.owl#Punctuation"/>
        <olia_system:hasTag>YIR</olia_system:hasTag>
        <olia_system:hasTier>POS</olia_system:hasTier>
        <rdfs:comment>YIR is the SUSANNE tag used for closing (single or double) inverted commas.</rdfs:comment>
    </owl:NamedIndividual>
    


    <!-- http://purl.org/olia/susa.owl#YM -->

    <owl:NamedIndividual rdf:about="http://purl.org/olia/susa.owl#YM">
        <rdf:type rdf:resource="http://purl.org/olia/susa.owl#Punctuation"/>
        <olia_system:hasTag>YM</olia_system:hasTag>
        <olia_system:hasTier>POS</olia_system:hasTier>
        <rdfs:comment>YM is the SUSANNE tag used for a filled pause. Its only used in speech analysis.</rdfs:comment>
    </owl:NamedIndividual>
    


    <!-- http://purl.org/olia/susa.owl#YN -->

    <owl:NamedIndividual rdf:about="http://purl.org/olia/susa.owl#YN">
        <rdf:type rdf:resource="http://purl.org/olia/susa.owl#Punctuation"/>
        <olia_system:hasTag>YN</olia_system:hasTag>
        <olia_system:hasTier>POS</olia_system:hasTier>
        <rdfs:comment>YN is the SUSANNE tag used for colon.</rdfs:comment>
    </owl:NamedIndividual>
    


    <!-- http://purl.org/olia/susa.owl#YND -->

    <owl:NamedIndividual rdf:about="http://purl.org/olia/susa.owl#YND">
        <rdf:type rdf:resource="http://purl.org/olia/susa.owl#Punctuation"/>
        <olia_system:hasTag>YND</olia_system:hasTag>
        <olia_system:hasTier>POS</olia_system:hasTier>
        <rdfs:comment>YND for the colon-dash &quot;:&quot;.</rdfs:comment>
    </owl:NamedIndividual>
    


    <!-- http://purl.org/olia/susa.owl#YO -->

    <owl:NamedIndividual rdf:about="http://purl.org/olia/susa.owl#YO">
        <rdf:type rdf:resource="http://purl.org/olia/susa.owl#Punctuation"/>
        <olia_system:hasTag>YO</olia_system:hasTag>
        <olia_system:hasTier>POS</olia_system:hasTier>
        <rdfs:comment>YO is the SUSANNE tag used for bullet, pilcrom, or other special symbol visually marking a text division.</rdfs:comment>
    </owl:NamedIndividual>
    


    <!-- http://purl.org/olia/susa.owl#YP -->

    <owl:NamedIndividual rdf:about="http://purl.org/olia/susa.owl#YP">
        <rdf:type rdf:resource="http://purl.org/olia/susa.owl#Punctuation"/>
        <olia_system:hasTag>YP</olia_system:hasTag>
        <olia_system:hasTier>POS</olia_system:hasTier>
        <rdfs:comment>YP is the SUSANNE tag used for the silent pause. It is used only in speech analysis.</rdfs:comment>
    </owl:NamedIndividual>
    


    <!-- http://purl.org/olia/susa.owl#YPL -->

    <owl:NamedIndividual rdf:about="http://purl.org/olia/susa.owl#YPL">
        <rdf:type rdf:resource="http://purl.org/olia/susa.owl#Punctuation"/>
        <olia_system:hasTag>YPL</olia_system:hasTag>
        <olia_system:hasTier>POS</olia_system:hasTier>
        <rdfs:comment>YPL is the SUSANNE tag used for the opening bracket &quot;(&quot;.</rdfs:comment>
    </owl:NamedIndividual>
    


    <!-- http://purl.org/olia/susa.owl#YPR -->

    <owl:NamedIndividual rdf:about="http://purl.org/olia/susa.owl#YPR">
        <rdf:type rdf:resource="http://purl.org/olia/susa.owl#Punctuation"/>
        <olia_system:hasTag>YPR</olia_system:hasTag>
        <olia_system:hasTier>POS</olia_system:hasTier>
        <rdfs:comment>YPR is the SUSANNE tag used for the closing bracket &quot;)&quot;.</rdfs:comment>
    </owl:NamedIndividual>
    


    <!-- http://purl.org/olia/susa.owl#YQ -->

    <owl:NamedIndividual rdf:about="http://purl.org/olia/susa.owl#YQ">
        <rdf:type rdf:resource="http://purl.org/olia/susa.owl#Punctuation"/>
        <olia_system:hasTag>YQ</olia_system:hasTag>
        <olia_system:hasTier>POS</olia_system:hasTier>
        <rdfs:comment>YQ is the SUSANNE tag used for the question mark &quot;?&quot;.</rdfs:comment>
    </owl:NamedIndividual>
    


    <!-- http://purl.org/olia/susa.owl#YR -->

    <owl:NamedIndividual rdf:about="http://purl.org/olia/susa.owl#YR">
        <rdf:type rdf:resource="http://purl.org/olia/susa.owl#Punctuation"/>
        <olia_system:hasTag>YR</olia_system:hasTag>
        <olia_system:hasTier>POS</olia_system:hasTier>
        <rdfs:comment>YR is the SUSANNE tag used for an interruption point. It is only used in speech analysis.</rdfs:comment>
    </owl:NamedIndividual>
    


    <!-- http://purl.org/olia/susa.owl#YS -->

    <owl:NamedIndividual rdf:about="http://purl.org/olia/susa.owl#YS">
        <rdf:type rdf:resource="http://purl.org/olia/susa.owl#Punctuation"/>
        <olia_system:hasTag>YS</olia_system:hasTag>
        <olia_system:hasTier>POS</olia_system:hasTier>
        <rdfs:comment>YS is the SUSANNE tag used for a semicolon.</rdfs:comment>
    </owl:NamedIndividual>
    


    <!-- http://purl.org/olia/susa.owl#YT -->

    <owl:NamedIndividual rdf:about="http://purl.org/olia/susa.owl#YT">
        <rdf:type rdf:resource="http://purl.org/olia/susa.owl#Punctuation"/>
        <olia_system:hasTag>YT</olia_system:hasTag>
        <olia_system:hasTier>POS</olia_system:hasTier>
        <rdfs:comment>YT is used for bolds.</rdfs:comment>
    </owl:NamedIndividual>
    


    <!-- http://purl.org/olia/susa.owl#YTL -->

    <owl:NamedIndividual rdf:about="http://purl.org/olia/susa.owl#YTL">
        <rdf:type rdf:resource="http://purl.org/olia/susa.owl#Punctuation"/>
        <olia_system:hasTag>YTL</olia_system:hasTag>
        <olia_system:hasTier>POS</olia_system:hasTier>
        <rdfs:comment>YTL is used for a begin bold.</rdfs:comment>
    </owl:NamedIndividual>
    


    <!-- http://purl.org/olia/susa.owl#YTR -->

    <owl:NamedIndividual rdf:about="http://purl.org/olia/susa.owl#YTR">
        <rdf:type rdf:resource="http://purl.org/olia/susa.owl#Punctuation"/>
        <olia_system:hasTag>YTR</olia_system:hasTag>
        <olia_system:hasTier>POS</olia_system:hasTier>
        <rdfs:comment>YTR is used for an end bold.</rdfs:comment>
    </owl:NamedIndividual>
    


    <!-- http://purl.org/olia/susa.owl#YX -->

    <owl:NamedIndividual rdf:about="http://purl.org/olia/susa.owl#YX">
        <rdf:type rdf:resource="http://purl.org/olia/susa.owl#Punctuation"/>
        <olia_system:hasTag>YX</olia_system:hasTag>
        <olia_system:hasTier>POS</olia_system:hasTier>
        <rdfs:comment>YX is the SUSANNE tag used for the exclamation mark &quot;!&quot;.</rdfs:comment>
    </owl:NamedIndividual>
    


    <!-- http://purl.org/olia/susa.owl#ZZ -->

    <owl:NamedIndividual rdf:about="http://purl.org/olia/susa.owl#ZZ">
        <rdf:type rdf:resource="http://purl.org/olia/susa.owl#Letter"/>
        <olia_system:hasTag>ZZ</olia_system:hasTag>
        <olia_system:hasTier>POS</olia_system:hasTier>
        <rdfs:comment>ZZ is used for letters of the (roman or other) alphabet.</rdfs:comment>
    </owl:NamedIndividual>
    


    <!-- http://purl.org/olia/susa.owl#ZZ1 -->

    <owl:NamedIndividual rdf:about="http://purl.org/olia/susa.owl#ZZ1">
        <rdf:type rdf:resource="http://purl.org/olia/susa.owl#Letter"/>
        <hasNumber rdf:resource="http://purl.org/olia/susa.owl#singular"/>
        <olia_system:hasTag>ZZ1</olia_system:hasTag>
        <olia_system:hasTier>POS</olia_system:hasTier>
        <rdfs:comment>ZZ1 is the SUSANNE tag used for a singular letter of the (roman or other) alphabet.</rdfs:comment>
    </owl:NamedIndividual>
    


    <!-- http://purl.org/olia/susa.owl#ZZ2 -->

    <owl:NamedIndividual rdf:about="http://purl.org/olia/susa.owl#ZZ2">
        <rdf:type rdf:resource="http://purl.org/olia/susa.owl#Letter"/>
        <hasNumber rdf:resource="http://purl.org/olia/susa.owl#plural"/>
        <olia_system:hasTag>ZZ2</olia_system:hasTag>
        <olia_system:hasTier>POS</olia_system:hasTier>
        <rdfs:comment>ZZ2 which is used for a letter of the alphabet with plural inflexion.</rdfs:comment>
    </owl:NamedIndividual>
    


    <!-- http://purl.org/olia/susa.owl#base_form -->

    <owl:NamedIndividual rdf:about="http://purl.org/olia/susa.owl#base_form">
        <rdf:type rdf:resource="http://purl.org/olia/susa.owl#Form"/>
    </owl:NamedIndividual>
    


    <!-- http://purl.org/olia/susa.owl#comparative -->

    <owl:NamedIndividual rdf:about="http://purl.org/olia/susa.owl#comparative">
        <rdf:type rdf:resource="http://purl.org/olia/susa.owl#Degree"/>
    </owl:NamedIndividual>
    


    <!-- http://purl.org/olia/susa.owl#countable -->

    <owl:NamedIndividual rdf:about="http://purl.org/olia/susa.owl#countable">
        <rdf:type rdf:resource="http://purl.org/olia/susa.owl#Countability"/>
    </owl:NamedIndividual>
    


    <!-- http://purl.org/olia/susa.owl#feminine -->

    <owl:NamedIndividual rdf:about="http://purl.org/olia/susa.owl#feminine">
        <rdf:type rdf:resource="http://purl.org/olia/susa.owl#Gender"/>
    </owl:NamedIndividual>
    


    <!-- http://purl.org/olia/susa.owl#first -->

    <owl:NamedIndividual rdf:about="http://purl.org/olia/susa.owl#first">
        <rdf:type rdf:resource="http://purl.org/olia/susa.owl#Person"/>
    </owl:NamedIndividual>
    


    <!-- http://purl.org/olia/susa.owl#genitive -->

    <owl:NamedIndividual rdf:about="http://purl.org/olia/susa.owl#genitive">
        <rdf:type rdf:resource="http://purl.org/olia/susa.owl#Case"/>
    </owl:NamedIndividual>
    


    <!-- http://purl.org/olia/susa.owl#inflected_form -->

    <owl:NamedIndividual rdf:about="http://purl.org/olia/susa.owl#inflected_form">
        <rdf:type rdf:resource="http://purl.org/olia/susa.owl#Form"/>
    </owl:NamedIndividual>
    


    <!-- http://purl.org/olia/susa.owl#intransitive -->

    <owl:NamedIndividual rdf:about="http://purl.org/olia/susa.owl#intransitive">
        <rdf:type rdf:resource="http://purl.org/olia/susa.owl#Valency"/>
    </owl:NamedIndividual>
    


    <!-- http://purl.org/olia/susa.owl#masculine -->

    <owl:NamedIndividual rdf:about="http://purl.org/olia/susa.owl#masculine">
        <rdf:type rdf:resource="http://purl.org/olia/susa.owl#Gender"/>
    </owl:NamedIndividual>
    


    <!-- http://purl.org/olia/susa.owl#neutral -->

    <owl:NamedIndividual rdf:about="http://purl.org/olia/susa.owl#neutral">
        <rdf:type rdf:resource="http://purl.org/olia/susa.owl#Gender"/>
    </owl:NamedIndividual>
    


    <!-- http://purl.org/olia/susa.owl#objective -->

    <owl:NamedIndividual rdf:about="http://purl.org/olia/susa.owl#objective">
        <rdf:type rdf:resource="http://purl.org/olia/susa.owl#Case"/>
    </owl:NamedIndividual>
    


    <!-- http://purl.org/olia/susa.owl#past -->

    <owl:NamedIndividual rdf:about="http://purl.org/olia/susa.owl#past">
        <rdf:type rdf:resource="http://purl.org/olia/susa.owl#Tense"/>
    </owl:NamedIndividual>
    


    <!-- http://purl.org/olia/susa.owl#plural -->

    <owl:NamedIndividual rdf:about="http://purl.org/olia/susa.owl#plural">
        <rdf:type rdf:resource="http://purl.org/olia/susa.owl#Number"/>
    </owl:NamedIndividual>
    


    <!-- http://purl.org/olia/susa.owl#positive -->

    <owl:NamedIndividual rdf:about="http://purl.org/olia/susa.owl#positive">
        <rdf:type rdf:resource="http://purl.org/olia/susa.owl#Degree"/>
    </owl:NamedIndividual>
    


    <!-- http://purl.org/olia/susa.owl#present -->

    <owl:NamedIndividual rdf:about="http://purl.org/olia/susa.owl#present">
        <rdf:type rdf:resource="http://purl.org/olia/susa.owl#Tense"/>
    </owl:NamedIndividual>
    


    <!-- http://purl.org/olia/susa.owl#second -->

    <owl:NamedIndividual rdf:about="http://purl.org/olia/susa.owl#second">
        <rdf:type rdf:resource="http://purl.org/olia/susa.owl#Person"/>
    </owl:NamedIndividual>
    


    <!-- http://purl.org/olia/susa.owl#singular -->

    <owl:NamedIndividual rdf:about="http://purl.org/olia/susa.owl#singular">
        <rdf:type rdf:resource="http://purl.org/olia/susa.owl#Number"/>
    </owl:NamedIndividual>
    


    <!-- http://purl.org/olia/susa.owl#subjective -->

    <owl:NamedIndividual rdf:about="http://purl.org/olia/susa.owl#subjective">
        <rdf:type rdf:resource="http://purl.org/olia/susa.owl#Case"/>
    </owl:NamedIndividual>
    


    <!-- http://purl.org/olia/susa.owl#superlative -->

    <owl:NamedIndividual rdf:about="http://purl.org/olia/susa.owl#superlative">
        <rdf:type rdf:resource="http://purl.org/olia/susa.owl#Degree"/>
    </owl:NamedIndividual>
    


    <!-- http://purl.org/olia/susa.owl#third -->

    <owl:NamedIndividual rdf:about="http://purl.org/olia/susa.owl#third">
        <rdf:type rdf:resource="http://purl.org/olia/susa.owl#Person"/>
    </owl:NamedIndividual>
    


    <!-- http://purl.org/olia/susa.owl#transitive -->

    <owl:NamedIndividual rdf:about="http://purl.org/olia/susa.owl#transitive">
        <rdf:type rdf:resource="http://purl.org/olia/susa.owl#Valency"/>
    </owl:NamedIndividual>
    


    <!-- http://purl.org/olia/susa.owl#uncountable -->

    <owl:NamedIndividual rdf:about="http://purl.org/olia/susa.owl#uncountable">
        <rdf:type rdf:resource="http://purl.org/olia/susa.owl#Countability"/>
    </owl:NamedIndividual>
</rdf:RDF>



<!-- Generated by the OWL API (version 4.5.25.2023-02-15T19:15:49Z) https://github.com/owlcs/owlapi -->

