<?xml version="1.0"?>
<rdf:RDF xmlns="http://purl.org/olia/tcodex.owl#"
     xml:base="http://purl.org/olia/tcodex.owl"
     xmlns:ms="http://w3id.org/meta-share/meta-share/"
     xmlns:dct="http://purl.org/dc/terms/"
     xmlns:owl="http://www.w3.org/2002/07/owl#"
     xmlns:rdf="http://www.w3.org/1999/02/22-rdf-syntax-ns#"
     xmlns:xml="http://www.w3.org/XML/1998/namespace"
     xmlns:xsd="http://www.w3.org/2001/XMLSchema#"
     xmlns:rdfs="http://www.w3.org/2000/01/rdf-schema#"
     xmlns:system="http://purl.org/olia/system.owl#"
     xmlns:protege="http://protege.stanford.edu/plugins/owl/protege#">
    <owl:Ontology rdf:about="http://purl.org/olia/tcodex.owl">
        <owl:imports rdf:resource="http://purl.org/olia/system.owl"/>
        <dct:license rdf:resource="https://creativecommons.org/licenses/by/3.0/"/>
        <ms:language rdf:resource="http://lexvo.org/id/iso639-3/goh"/>
        <rdfs:comment>OLiA Annotation Model for the Tatian Corpus of Deviating Examples (T-CODEX, Petrova et al. 2009) and other resources for Old High German (OHG) assembled by project B4 of the Collaborative Research Center (SFB) 632 &quot;Information Structure&quot; (2003-2015), Universität Potsdam, HU Berlin.

The present corpus, the Tatian Corpus of Deviating Examples T-CODEX 2.0, provides morpho-syntactic and information structural annotation of parts of the Old High German translation attested in the MS St. Gallen Cod. 56, traditionally called the OHG Tatian, one of the largest prose texts from the classical OHG period. This corpus was designed and annotated by Project B4 of Collaborative Research Center on Information Structure at Humboldt University Berlin. (Petrova and Odebrecht 2011)

Unless marked otherwise, all comments are authored by Svetlana Petrova from the 2008 edition of this ontology. Additional resources consulted for the development of this ontology include Petrova and Odebrecht (2011).

References:

Svetlana Petrova and Carolin Odebrecht (2011), Tatian Corpus of Deviating Examples. T-CODEX 2.1 Corpus Description (version of 21-Mar-2011). Technical Report, HU Berlin, https://korpling.german.hu-berlin.de/~annis/T-CODEX/corpus_description_tatian2.1.pdf

Petrova, Svetlana, Solf, Michael, Ritz, Julia, Chiarcos, Christian, Zeldes, Amir (2009) Building and using a richly annotated interlinear diachronic corpus: the case of Old High German Tatian. Traitement Automatique des Langues 50 (2): 47-71.</rdfs:comment>
        <owl:versionInfo>2008-10-14 created by Svetlana Petrova (content) and Angelika Adam (OWL modelling)
2011-08-12 updated to T-CODEX v. 2.1, Christian Chiarcos (Note: naming conventions for tags have been changed, the naming conventions of the individuals follow the *original* naming conventions for tags)
      
Christian Chiarcos, chiarcos@uni-potsdam.de</owl:versionInfo>
    </owl:Ontology>
    


    <!-- 
    ///////////////////////////////////////////////////////////////////////////////////////
    //
    // Annotation properties
    //
    ///////////////////////////////////////////////////////////////////////////////////////
     -->

    


    <!-- http://purl.org/olia/system.owl#hasTagMatching -->

    <owl:AnnotationProperty rdf:about="http://purl.org/olia/system.owl#hasTagMatching"/>
    


    <!-- http://w3id.org/meta-share/meta-share/language -->

    <owl:AnnotationProperty rdf:about="http://w3id.org/meta-share/meta-share/language"/>
    


    <!-- 
    ///////////////////////////////////////////////////////////////////////////////////////
    //
    // Data properties
    //
    ///////////////////////////////////////////////////////////////////////////////////////
     -->

    


    <!-- http://purl.org/olia/system.owl#hasTag -->

    <owl:DatatypeProperty rdf:about="http://purl.org/olia/system.owl#hasTag"/>
    


    <!-- http://purl.org/olia/system.owl#hasTier -->

    <owl:DatatypeProperty rdf:about="http://purl.org/olia/system.owl#hasTier"/>
    


    <!-- 
    ///////////////////////////////////////////////////////////////////////////////////////
    //
    // Classes
    //
    ///////////////////////////////////////////////////////////////////////////////////////
     -->

    


    <!-- http://purl.org/olia/system.owl#UnitOfAnnotation -->

    <owl:Class rdf:about="http://purl.org/olia/system.owl#UnitOfAnnotation"/>
    


    <!-- http://purl.org/olia/tcodex.owl#Aboutness -->

    <owl:Class rdf:about="http://purl.org/olia/tcodex.owl#Aboutness">
        <rdfs:subClassOf rdf:resource="http://purl.org/olia/tcodex.owl#TopicComment"/>
        <rdfs:subClassOf>
            <owl:Restriction>
                <owl:onProperty rdf:resource="http://purl.org/olia/system.owl#hasTier"/>
                <owl:hasValue>ABOUTNESS</owl:hasValue>
            </owl:Restriction>
        </rdfs:subClassOf>
        <rdfs:comment>This tag is given to phrases that are potential candidates for topics in the clause.</rdfs:comment>
    </owl:Class>
    


    <!-- http://purl.org/olia/tcodex.owl#AccessibleInformation -->

    <owl:Class rdf:about="http://purl.org/olia/tcodex.owl#AccessibleInformation">
        <rdfs:subClassOf rdf:resource="http://purl.org/olia/tcodex.owl#Givenness"/>
        <rdfs:comment>This tag is given to expressions that are accessible via contextual reference to a given entitiy or to the assumed world knowledge of the interlocutors.</rdfs:comment>
    </owl:Class>
    


    <!-- http://purl.org/olia/tcodex.owl#Adjective -->

    <owl:Class rdf:about="http://purl.org/olia/tcodex.owl#Adjective">
        <rdfs:subClassOf rdf:resource="http://purl.org/olia/tcodex.owl#InflectedPOS"/>
        <rdfs:comment></rdfs:comment>
    </owl:Class>
    


    <!-- http://purl.org/olia/tcodex.owl#AdjectivialPhrase -->

    <owl:Class rdf:about="http://purl.org/olia/tcodex.owl#AdjectivialPhrase">
        <rdfs:subClassOf rdf:resource="http://purl.org/olia/tcodex.owl#SyntacticalCategory"/>
        <rdfs:comment>A adjectival  phrase  is a phrase whose head is a adjective.</rdfs:comment>
    </owl:Class>
    


    <!-- http://purl.org/olia/tcodex.owl#Adverb -->

    <owl:Class rdf:about="http://purl.org/olia/tcodex.owl#Adverb">
        <rdfs:subClassOf rdf:resource="http://purl.org/olia/tcodex.owl#NonInflectedPOS"/>
        <rdfs:comment>This tag is assigned to adverbs of all kinds, i.e. to adverbs of time, place, incl. location and direction, and to adverbs of cause and manner. (Petrova and Odebrecht 2011).</rdfs:comment>
        <owl:versionInfo>The original T-CODEX tagset distinguished five subtypes of Adverbs, CausalAdverb, DirectionalAdverb, LocalAdverb, ModalAdverb, TemporalAdverb. In T-CODEX 2.1, these are conflated into a single Adverb category, tagged ADV.
These are now represented only in the GrammaticalFunction layer.</owl:versionInfo>
    </owl:Class>
    


    <!-- http://purl.org/olia/tcodex.owl#AdverbalPhrase -->

    <owl:Class rdf:about="http://purl.org/olia/tcodex.owl#AdverbalPhrase">
        <rdfs:subClassOf rdf:resource="http://purl.org/olia/tcodex.owl#SyntacticalCategory"/>
        <rdfs:comment>An adverbial or adverbial phrase is a linguistic term for a single adverb or a group of more than one word operating adverbially, when viewed in terms of their syntactic function.
An adverbial phrase can modify a verb phrase, an adjectival phrase or an entire clause.
(http://en.wikipedia.org/wiki/Adverbial_phrase 23.07.08)</rdfs:comment>
    </owl:Class>
    


    <!-- http://purl.org/olia/tcodex.owl#Adverbial -->

    <owl:Class rdf:about="http://purl.org/olia/tcodex.owl#Adverbial">
        <rdfs:subClassOf rdf:resource="http://purl.org/olia/tcodex.owl#GrammaticalFunction"/>
        <rdfs:comment>An adverbial is a nonobligatory adjunct position which can be further specified according to its semantic function. The tag adv is given incase the interpretation of the adjunct is ambigious or impossible for particular reasons.</rdfs:comment>
    </owl:Class>
    


    <!-- http://purl.org/olia/tcodex.owl#AnaphoricReference -->

    <owl:Class rdf:about="http://purl.org/olia/tcodex.owl#AnaphoricReference">
        <rdfs:subClassOf rdf:resource="http://purl.org/olia/tcodex.owl#Context"/>
        <rdfs:comment>Context: Here, we annotate the relation of the clause with respect to the preceding context, especially in terms of discourse organization. We mainly distinguish between “situation shift” (Situationswechsel) und “anaphoric reference” (“AR”). Situationswechsel involves a change of time, place, speaker/narrator and participants. (Petrova and Odebrecht 2011)</rdfs:comment>
    </owl:Class>
    


    <!-- http://purl.org/olia/tcodex.owl#Apposition -->

    <owl:Class rdf:about="http://purl.org/olia/tcodex.owl#Apposition">
        <rdfs:subClassOf rdf:resource="http://purl.org/olia/tcodex.owl#GrammaticalFunction"/>
        <rdfs:comment>An apposition is a repetition of an argument expression which provides further information, eg.
&quot;zacharîas sin fater&quot; (Zacharia, his father).</rdfs:comment>
    </owl:Class>
    


    <!-- http://purl.org/olia/tcodex.owl#Attrbute_to_Object -->

    <owl:Class rdf:about="http://purl.org/olia/tcodex.owl#Attrbute_to_Object">
        <rdfs:subClassOf rdf:resource="http://purl.org/olia/tcodex.owl#Attribute"/>
        <rdfs:comment>This attribute modifies the object.</rdfs:comment>
        <owl:deprecated>Removed from T-CODEX 2.1</owl:deprecated>
    </owl:Class>
    


    <!-- http://purl.org/olia/tcodex.owl#Attribute -->

    <owl:Class rdf:about="http://purl.org/olia/tcodex.owl#Attribute">
        <rdfs:subClassOf rdf:resource="http://purl.org/olia/tcodex.owl#GrammaticalFunction"/>
        <rdfs:comment>An attribute is a modifier to a noun.</rdfs:comment>
    </owl:Class>
    


    <!-- http://purl.org/olia/tcodex.owl#Attribute_to_PredicateNoun -->

    <owl:Class rdf:about="http://purl.org/olia/tcodex.owl#Attribute_to_PredicateNoun">
        <rdfs:subClassOf rdf:resource="http://purl.org/olia/tcodex.owl#Attribute"/>
        <rdfs:comment>This attribute modifies a predicate noun.</rdfs:comment>
    </owl:Class>
    


    <!-- http://purl.org/olia/tcodex.owl#Attribute_to_Subject -->

    <owl:Class rdf:about="http://purl.org/olia/tcodex.owl#Attribute_to_Subject">
        <rdfs:subClassOf rdf:resource="http://purl.org/olia/tcodex.owl#Attribute"/>
        <rdfs:comment>This attribute modifies the subject.</rdfs:comment>
        <owl:deprecated>Removed from T-CODEX 2.1</owl:deprecated>
    </owl:Class>
    


    <!-- http://purl.org/olia/tcodex.owl#AttributiveSubordinateClause -->

    <owl:Class rdf:about="http://purl.org/olia/tcodex.owl#AttributiveSubordinateClause">
        <rdfs:subClassOf rdf:resource="http://purl.org/olia/tcodex.owl#SubordinateClause"/>
        <rdfs:comment>This tag is given to argument clauses which modify an argument of the matrix clause.</rdfs:comment>
    </owl:Class>
    


    <!-- http://purl.org/olia/tcodex.owl#AuxiliaryVerb -->

    <owl:Class rdf:about="http://purl.org/olia/tcodex.owl#AuxiliaryVerb">
        <rdfs:subClassOf rdf:resource="http://purl.org/olia/tcodex.owl#Verb"/>
        <rdfs:comment>An auxiliary verb is a verb which accompanies the lexical verb of a verb phrase, and expresses grammatical distinctions not carried by the lexical verb, such as person, number, tense aspect, and voice. (http://www.sil.org/linguistics/GlossaryOfLinguisticTerms/WhatIsAnAuxiliaryVerb.htm 19.09.06)</rdfs:comment>
    </owl:Class>
    


    <!-- http://purl.org/olia/tcodex.owl#Causal -->

    <owl:Class rdf:about="http://purl.org/olia/tcodex.owl#Causal">
        <rdfs:subClassOf rdf:resource="http://purl.org/olia/tcodex.owl#ClauseStatus"/>
        <rdfs:comment>Clauses introduced by the causal conjunctions &quot;uuanta&quot;  or &quot;bithiu uuanta&quot; (because) in Old High German are ambigious between main and subordinate clauses. For this reason, they are classified as causal uniformly.</rdfs:comment>
    </owl:Class>
    


    <!-- http://purl.org/olia/tcodex.owl#CausalAdverb -->

    <owl:Class rdf:about="http://purl.org/olia/tcodex.owl#CausalAdverb">
        <rdfs:subClassOf rdf:resource="http://purl.org/olia/tcodex.owl#Adverb"/>
        <rdfs:comment>This tag is given to adverbs of cause.</rdfs:comment>
        <owl:deprecated>Removed from T-CODEX 2.1</owl:deprecated>
    </owl:Class>
    


    <!-- http://purl.org/olia/tcodex.owl#CausalAdverbial -->

    <owl:Class rdf:about="http://purl.org/olia/tcodex.owl#CausalAdverbial">
        <rdfs:subClassOf rdf:resource="http://purl.org/olia/tcodex.owl#Adverbial"/>
        <rdfs:comment>This is an adverbial of cause.</rdfs:comment>
    </owl:Class>
    


    <!-- http://purl.org/olia/tcodex.owl#ClauseStatus -->

    <owl:Class rdf:about="http://purl.org/olia/tcodex.owl#ClauseStatus">
        <rdfs:subClassOf rdf:resource="http://purl.org/olia/tcodex.owl#Morpho-Syntactic"/>
        <rdfs:subClassOf>
            <owl:Restriction>
                <owl:onProperty rdf:resource="http://purl.org/olia/system.owl#hasTier"/>
                <owl:hasValue>CLAUSE_STATUS</owl:hasValue>
            </owl:Restriction>
        </rdfs:subClassOf>
    </owl:Class>
    


    <!-- http://purl.org/olia/tcodex.owl#ComitativeAdverbial -->

    <owl:Class rdf:about="http://purl.org/olia/tcodex.owl#ComitativeAdverbial">
        <rdfs:subClassOf rdf:resource="http://purl.org/olia/tcodex.owl#Adverbial"/>
        <rdfs:comment>comitative adverbial: This is an adverbial denoting an accompanying
person. (Petrova and Odebrecht 2011)</rdfs:comment>
        <owl:versionInfo>added in T-CODEX 2.1</owl:versionInfo>
    </owl:Class>
    


    <!-- http://purl.org/olia/tcodex.owl#Comment -->

    <owl:Class rdf:about="http://purl.org/olia/tcodex.owl#Comment">
        <rdfs:subClassOf rdf:resource="http://purl.org/olia/tcodex.owl#TopicComment"/>
        <rdfs:subClassOf>
            <owl:Restriction>
                <owl:onProperty rdf:resource="http://purl.org/olia/system.owl#hasTier"/>
                <owl:hasValue>TOPIC_COMMENT</owl:hasValue>
            </owl:Restriction>
        </rdfs:subClassOf>
        <rdfs:comment>The rest of a clause with a topic is annotated for comment. If the entire clause is annotated for comment, this implies that a topic-comment division applies but there is no overt topic phrase (e.g., due to topic-drop etc.).</rdfs:comment>
    </owl:Class>
    


    <!-- http://purl.org/olia/tcodex.owl#ComparativeSubordinateClause -->

    <owl:Class rdf:about="http://purl.org/olia/tcodex.owl#ComparativeSubordinateClause">
        <rdfs:subClassOf rdf:resource="http://purl.org/olia/tcodex.owl#SubordinateClause"/>
        <rdfs:comment>This type of subclause expresses comparison.</rdfs:comment>
    </owl:Class>
    


    <!-- http://purl.org/olia/tcodex.owl#ComplementizerPhrase -->

    <owl:Class rdf:about="http://purl.org/olia/tcodex.owl#ComplementizerPhrase">
        <rdfs:subClassOf rdf:resource="http://purl.org/olia/tcodex.owl#SyntacticalCategory"/>
        <rdfs:comment>The complementizer is widely held to be the syntactic head of a full clause, which is therefore often represented by the abbreviation CP (for complementizer phrase). 
(http://en.wikipedia.org/wiki/Complementizer 23.07.08)</rdfs:comment>
        <rdfs:label>sentential complementizer</rdfs:label>
    </owl:Class>
    


    <!-- http://purl.org/olia/tcodex.owl#ConcessiveSubordinateClause -->

    <owl:Class rdf:about="http://purl.org/olia/tcodex.owl#ConcessiveSubordinateClause">
        <rdfs:subClassOf rdf:resource="http://purl.org/olia/tcodex.owl#SubordinateClause"/>
        <rdfs:comment>This type of subclause expresses a concessive relation to the matrix clause.
In modern German these clauses are introduced by &quot;obwohl&quot;, &quot;obschon&quot; or &quot;auch wenn&quot;.</rdfs:comment>
    </owl:Class>
    


    <!-- http://purl.org/olia/tcodex.owl#ConditionalAdverb -->

    <owl:Class rdf:about="http://purl.org/olia/tcodex.owl#ConditionalAdverb">
        <rdfs:subClassOf rdf:resource="http://purl.org/olia/tcodex.owl#Adverbial"/>
        <rdfs:comment>conditional adverb: this adverbial denotes a condition. (Petrova and Odebrecht 2011)</rdfs:comment>
        <owl:versionInfo>Added with T-CODEX 2.1</owl:versionInfo>
    </owl:Class>
    


    <!-- http://purl.org/olia/tcodex.owl#ConditionalSubordinateClause -->

    <owl:Class rdf:about="http://purl.org/olia/tcodex.owl#ConditionalSubordinateClause">
        <rdfs:subClassOf rdf:resource="http://purl.org/olia/tcodex.owl#SubordinateClause"/>
        <rdfs:comment>This type of subclause expresses conditions.</rdfs:comment>
    </owl:Class>
    


    <!-- http://purl.org/olia/tcodex.owl#Conjunction -->

    <owl:Class rdf:about="http://purl.org/olia/tcodex.owl#Conjunction">
        <rdfs:subClassOf rdf:resource="http://purl.org/olia/tcodex.owl#NonInflectedPOS"/>
        <rdfs:comment>This tag is given to conjunctions in general. We do not differentiate at this level between coordinating and subordinating conjunctions.</rdfs:comment>
    </owl:Class>
    


    <!-- http://purl.org/olia/tcodex.owl#ConsecutiveSubordinateClause -->

    <owl:Class rdf:about="http://purl.org/olia/tcodex.owl#ConsecutiveSubordinateClause">
        <rdfs:subClassOf rdf:resource="http://purl.org/olia/tcodex.owl#SubordinateClause"/>
        <rdfs:comment>This type of subclause expresses consequences.</rdfs:comment>
    </owl:Class>
    


    <!-- http://purl.org/olia/tcodex.owl#Context -->

    <owl:Class rdf:about="http://purl.org/olia/tcodex.owl#Context">
        <rdfs:subClassOf rdf:resource="http://purl.org/olia/tcodex.owl#InformationStructure"/>
        <rdfs:subClassOf>
            <owl:Restriction>
                <owl:onProperty rdf:resource="http://purl.org/olia/system.owl#hasTier"/>
                <owl:hasValue>CONTEXT</owl:hasValue>
            </owl:Restriction>
        </rdfs:subClassOf>
        <rdfs:comment>Context: Here, we annotate the relation of the clause with respect to the preceding context, especially in terms of discourse organization. We mainly distinguish between “situation shift” (Situationswechsel) und “anaphoric reference” (“AR”). Situationswechsel involves a change of time, place, speaker/narrator and participants. (Petrova and Odebrecht 2011)</rdfs:comment>
        <owl:versionInfo>Added with T-CODEX 2.1</owl:versionInfo>
    </owl:Class>
    


    <!-- http://purl.org/olia/tcodex.owl#ContrastFocus -->

    <owl:Class rdf:about="http://purl.org/olia/tcodex.owl#ContrastFocus">
        <rdfs:subClassOf rdf:resource="http://purl.org/olia/tcodex.owl#FocusBackground"/>
        <rdfs:subClassOf>
            <owl:Restriction>
                <owl:onProperty rdf:resource="http://purl.org/olia/system.owl#hasTier"/>
                <owl:hasValue>FOCUS_BACKGROUND</owl:hasValue>
            </owl:Restriction>
        </rdfs:subClassOf>
    </owl:Class>
    


    <!-- http://purl.org/olia/tcodex.owl#CopulaVerb -->

    <owl:Class rdf:about="http://purl.org/olia/tcodex.owl#CopulaVerb">
        <rdfs:subClassOf rdf:resource="http://purl.org/olia/tcodex.owl#Verb"/>
        <rdfs:comment>A copula is a verb that links the subject or an object to another phrase, adjective etc. which is part of a complex predicate. The complement of a copula is annotated as PredicateNoun.</rdfs:comment>
    </owl:Class>
    


    <!-- http://purl.org/olia/tcodex.owl#DeclarativeMainClause -->

    <owl:Class rdf:about="http://purl.org/olia/tcodex.owl#DeclarativeMainClause">
        <rdfs:subClassOf rdf:resource="http://purl.org/olia/tcodex.owl#MainClause"/>
        <rdfs:comment>This tag is given to main declarative sentences.</rdfs:comment>
    </owl:Class>
    


    <!-- http://purl.org/olia/tcodex.owl#Definite -->

    <owl:Class rdf:about="http://purl.org/olia/tcodex.owl#Definite">
        <rdfs:subClassOf rdf:resource="http://purl.org/olia/tcodex.owl#Definiteness"/>
    </owl:Class>
    


    <!-- http://purl.org/olia/tcodex.owl#Definiteness -->

    <owl:Class rdf:about="http://purl.org/olia/tcodex.owl#Definiteness">
        <rdfs:subClassOf rdf:resource="http://purl.org/olia/tcodex.owl#TopicComment"/>
        <rdfs:subClassOf>
            <owl:Restriction>
                <owl:onProperty rdf:resource="http://purl.org/olia/system.owl#hasTier"/>
                <owl:hasValue>DEFINITENESS</owl:hasValue>
            </owl:Restriction>
        </rdfs:subClassOf>
        <rdfs:comment>At this level, we annotate the semantic properties of phrases with respect to the definite/indefinite distinction. In OHG, the system of definite determiners is not developed yet. Therefore, we annotate the semantic interpretation of the phrase despite of the presence of a definite or indefinite marker.</rdfs:comment>
    </owl:Class>
    


    <!-- http://purl.org/olia/tcodex.owl#DemonstrativePronoun -->

    <owl:Class rdf:about="http://purl.org/olia/tcodex.owl#DemonstrativePronoun">
        <rdfs:subClassOf rdf:resource="http://purl.org/olia/tcodex.owl#Pronoun"/>
        <rdfs:comment>In OHG, the demonstrative pronouns are also used as articles (definite determiners).</rdfs:comment>
    </owl:Class>
    


    <!-- http://purl.org/olia/tcodex.owl#DirectObject -->

    <owl:Class rdf:about="http://purl.org/olia/tcodex.owl#DirectObject">
        <rdfs:subClassOf rdf:resource="http://purl.org/olia/tcodex.owl#GrammaticalFunction"/>
    </owl:Class>
    


    <!-- http://purl.org/olia/tcodex.owl#Directional -->

    <owl:Class rdf:about="http://purl.org/olia/tcodex.owl#Directional">
        <rdfs:subClassOf rdf:resource="http://purl.org/olia/tcodex.owl#GrammaticalFunction"/>
        <rdfs:comment>This is given to the directional arguments of verbs of movement, e.g. &quot;in b&amp;hleem&quot; in &quot;santa sie in b&amp;hleem&quot; (And sent them to Bethlehem.) (T_040_02)</rdfs:comment>
    </owl:Class>
    


    <!-- http://purl.org/olia/tcodex.owl#DirectionalAdverb -->

    <owl:Class rdf:about="http://purl.org/olia/tcodex.owl#DirectionalAdverb">
        <rdfs:subClassOf rdf:resource="http://purl.org/olia/tcodex.owl#Adverb"/>
        <rdfs:comment>This tag is given to adverbs of direction. In some cases, they can be potentially interpreted as separable verb prefixes which are formally identical with directional adverbs in OHG. See “zuo” in “gieng tho zuo/ ein buochari” (One of the learned man approached) (T__085_21-22). If you want to search for potential prefixes that are stranded from the finite verb, look for entities that are annotated as “adv:dir” at the level of “pos” and “dir” at the level of “gf”.</rdfs:comment>
        <owl:deprecated>Removed from T-CODEX 2.1</owl:deprecated>
    </owl:Class>
    


    <!-- http://purl.org/olia/tcodex.owl#FinalSubordinateClause -->

    <owl:Class rdf:about="http://purl.org/olia/tcodex.owl#FinalSubordinateClause">
        <rdfs:subClassOf rdf:resource="http://purl.org/olia/tcodex.owl#SubordinateClause"/>
        <rdfs:comment>This type of subclause expresses intentions.</rdfs:comment>
    </owl:Class>
    


    <!-- http://purl.org/olia/tcodex.owl#FiniteVerb -->

    <owl:Class rdf:about="http://purl.org/olia/tcodex.owl#FiniteVerb">
        <rdfs:subClassOf rdf:resource="http://purl.org/olia/tcodex.owl#GrammaticalFunction"/>
        <rdfs:comment>This tag at the level of grammatical function is forced by the subject matter of the project B4, namely to investigate verb-object orders in Old High German. It is of utmost importances to distinguish between tensed and untensed verb forms and to have a quick access to the finite verb in the annotation. 
(Pintzuk, Susann: Phrase Structures in Competition. Variation in change in old english word order, Garland New York 1999)</rdfs:comment>
    </owl:Class>
    


    <!-- http://purl.org/olia/tcodex.owl#FocusBackground -->

    <owl:Class rdf:about="http://purl.org/olia/tcodex.owl#FocusBackground">
        <rdfs:subClassOf rdf:resource="http://purl.org/olia/tcodex.owl#InformationStructure"/>
        <rdfs:comment>For more information</rdfs:comment>
    </owl:Class>
    


    <!-- http://purl.org/olia/tcodex.owl#FocusMarker -->

    <owl:Class rdf:about="http://purl.org/olia/tcodex.owl#FocusMarker">
        <rdfs:subClassOf rdf:resource="http://purl.org/olia/tcodex.owl#FocusBackground"/>
        <rdfs:subClassOf>
            <owl:Restriction>
                <owl:onProperty rdf:resource="http://purl.org/olia/system.owl#hasTier"/>
                <owl:hasValue>FOCUS_MARKER</owl:hasValue>
            </owl:Restriction>
        </rdfs:subClassOf>
    </owl:Class>
    


    <!-- http://purl.org/olia/tcodex.owl#FocusSensitiveOperator -->

    <owl:Class rdf:about="http://purl.org/olia/tcodex.owl#FocusSensitiveOperator">
        <rdfs:subClassOf rdf:resource="http://purl.org/olia/tcodex.owl#FocusMarker"/>
        <rdfs:label>focus-sensitive operator</rdfs:label>
        <owl:versionInfo>Added in T-CODEX 2.1</owl:versionInfo>
    </owl:Class>
    


    <!-- http://purl.org/olia/tcodex.owl#Frame -->

    <owl:Class rdf:about="http://purl.org/olia/tcodex.owl#Frame">
        <rdfs:subClassOf rdf:resource="http://purl.org/olia/tcodex.owl#Aboutness"/>
        <rdfs:comment>This tag is given to frame-setting topics, i.e. to expressions that reflect identifiable time spans and locations within which the predication holds. For more details, see SFB-Guildelines, Sec. 4.2.3.</rdfs:comment>
    </owl:Class>
    


    <!-- http://purl.org/olia/tcodex.owl#GermanVorfeld -->

    <owl:Class rdf:about="http://purl.org/olia/tcodex.owl#GermanVorfeld">
        <rdfs:subClassOf rdf:resource="http://purl.org/olia/tcodex.owl#InitionalPosition"/>
        <rdfs:comment>German Vorfeld: This tag is assigned to the clause-initial
constituent of a V2 main clause. (Petrova and Odebrecht 2011)</rdfs:comment>
        <owl:versionInfo>Addd with T-CODEX 2.1</owl:versionInfo>
    </owl:Class>
    


    <!-- http://purl.org/olia/tcodex.owl#Gerund -->

    <owl:Class rdf:about="http://purl.org/olia/tcodex.owl#Gerund">
        <rdfs:subClassOf rdf:resource="http://purl.org/olia/tcodex.owl#GrammaticalFunction"/>
        <rdfs:comment>This tag at the level of grammatical function is forced by the subject matter of the project B4, namely to investigate verb-object orders in Old High German. It is of utmost importances to distinguish between tensed and untensed verb forms and to have a quick access to these categories in the annotation. 
(Pintzuk, Susann: Phrase Structures in Competition. Variation in change in old english word order, Garland New York 1999)</rdfs:comment>
    </owl:Class>
    


    <!-- http://purl.org/olia/tcodex.owl#GivenInformation -->

    <owl:Class rdf:about="http://purl.org/olia/tcodex.owl#GivenInformation">
        <rdfs:subClassOf rdf:resource="http://purl.org/olia/tcodex.owl#Givenness"/>
        <rdfs:comment>This tag is given to expressions that refer to entities with a given antecedent in the context.</rdfs:comment>
    </owl:Class>
    


    <!-- http://purl.org/olia/tcodex.owl#Givenness -->

    <owl:Class rdf:about="http://purl.org/olia/tcodex.owl#Givenness">
        <rdfs:subClassOf rdf:resource="http://purl.org/olia/tcodex.owl#InformationStructure"/>
        <rdfs:subClassOf>
            <owl:Restriction>
                <owl:onProperty rdf:resource="http://purl.org/olia/system.owl#hasTier"/>
                <owl:hasValue>GIVENNESS</owl:hasValue>
            </owl:Restriction>
        </rdfs:subClassOf>
        <rdfs:comment>The following tags are given to discourse refernts only. For more details on entities that have to be annotated at this level, see the SFB-Guildelines.</rdfs:comment>
    </owl:Class>
    


    <!-- http://purl.org/olia/tcodex.owl#GrammaticalFunction -->

    <owl:Class rdf:about="http://purl.org/olia/tcodex.owl#GrammaticalFunction">
        <rdfs:subClassOf rdf:resource="http://purl.org/olia/tcodex.owl#Morpho-Syntactic"/>
        <rdfs:subClassOf>
            <owl:Restriction>
                <owl:onProperty rdf:resource="http://purl.org/olia/system.owl#hasTier"/>
                <owl:hasValue>EDGE</owl:hasValue>
            </owl:Restriction>
        </rdfs:subClassOf>
    </owl:Class>
    


    <!-- http://purl.org/olia/tcodex.owl#HangingTopic -->

    <owl:Class rdf:about="http://purl.org/olia/tcodex.owl#HangingTopic">
        <rdfs:subClassOf rdf:resource="http://purl.org/olia/tcodex.owl#InitionalPosition"/>
        <rdfs:comment>hanging topic: In this construction, a dislocated element and its
resuming pronoun do not necessarily agree in
case, number and gender. (Petrova and Odebrecht 2011)</rdfs:comment>
        <owl:versionInfo>Added in T-CODEX 2.1</owl:versionInfo>
    </owl:Class>
    


    <!-- http://purl.org/olia/tcodex.owl#ImperativeMainClause -->

    <owl:Class rdf:about="http://purl.org/olia/tcodex.owl#ImperativeMainClause">
        <rdfs:subClassOf rdf:resource="http://purl.org/olia/tcodex.owl#MainClause"/>
        <rdfs:comment>This tag is given to main sentences which use the imperative mood to utter requests.</rdfs:comment>
    </owl:Class>
    


    <!-- http://purl.org/olia/tcodex.owl#Indefinite -->

    <owl:Class rdf:about="http://purl.org/olia/tcodex.owl#Indefinite">
        <rdfs:subClassOf rdf:resource="http://purl.org/olia/tcodex.owl#Definiteness"/>
    </owl:Class>
    


    <!-- http://purl.org/olia/tcodex.owl#IndefinitePronoun -->

    <owl:Class rdf:about="http://purl.org/olia/tcodex.owl#IndefinitePronoun">
        <rdfs:subClassOf rdf:resource="http://purl.org/olia/tcodex.owl#Pronoun"/>
        <rdfs:comment>This is a cover term for indefinites and quantifiers in OHG including items like &quot;many&quot;, &quot;all&quot;, &quot;some&quot; etc.</rdfs:comment>
    </owl:Class>
    


    <!-- http://purl.org/olia/tcodex.owl#IndirectObject -->

    <owl:Class rdf:about="http://purl.org/olia/tcodex.owl#IndirectObject">
        <rdfs:subClassOf rdf:resource="http://purl.org/olia/tcodex.owl#GrammaticalFunction"/>
    </owl:Class>
    


    <!-- http://purl.org/olia/tcodex.owl#InfinitivalClause -->

    <owl:Class rdf:about="http://purl.org/olia/tcodex.owl#InfinitivalClause">
        <rdfs:subClassOf rdf:resource="http://purl.org/olia/tcodex.owl#ClauseStatus"/>
        <rdfs:comment>This tag is given to nonfinite complement clauses.</rdfs:comment>
    </owl:Class>
    


    <!-- http://purl.org/olia/tcodex.owl#Infinitive -->

    <owl:Class rdf:about="http://purl.org/olia/tcodex.owl#Infinitive">
        <rdfs:subClassOf rdf:resource="http://purl.org/olia/tcodex.owl#GrammaticalFunction"/>
        <rdfs:comment>This tag at the level of grammatical function is forced by the subject matter of the project B4, namely to investigate verb-object orders in Old High German. It is of utmost importances to distinguish between tensed and untensed verb forms and to have a quick access to these categories in the annotation. 
(Pintzuk, Susann: Phrase Structures in Competition. Variation in change in old english word order, Garland New York 1999)</rdfs:comment>
    </owl:Class>
    


    <!-- http://purl.org/olia/tcodex.owl#InflectedPOS -->

    <owl:Class rdf:about="http://purl.org/olia/tcodex.owl#InflectedPOS">
        <rdfs:subClassOf rdf:resource="http://purl.org/olia/tcodex.owl#POS"/>
        <rdfs:comment>inflected part of speech</rdfs:comment>
        <owl:versionInfo>Category inserted in accordance with Petrova and Odebrecht (2011).</owl:versionInfo>
    </owl:Class>
    


    <!-- http://purl.org/olia/tcodex.owl#InformationStructure -->

    <owl:Class rdf:about="http://purl.org/olia/tcodex.owl#InformationStructure">
        <rdfs:subClassOf rdf:resource="http://purl.org/olia/system.owl#UnitOfAnnotation"/>
        <owl:versionInfo>T-CODEX annotation was done using with a tool that requires for every annotation to establish its own markable (Exmaralda, http://www.exmaralda.org). Thus, every annotation is a UnitOfAnnotation.</owl:versionInfo>
    </owl:Class>
    


    <!-- http://purl.org/olia/tcodex.owl#InitionalPosition -->

    <owl:Class rdf:about="http://purl.org/olia/tcodex.owl#InitionalPosition">
        <rdfs:subClassOf rdf:resource="http://purl.org/olia/tcodex.owl#Position"/>
        <rdfs:comment>This tag is given to the first constituent before the finite verb in a declarative main clause.</rdfs:comment>
        <owl:versionInfo>In the original T-CODEX scheme, only a differentiation between initial and non-initial position were annotated. T-CODEX 2.1 has a more fine-grained subclassification of InitialPosition.</owl:versionInfo>
    </owl:Class>
    


    <!-- http://purl.org/olia/tcodex.owl#InstrumentalAdverbial -->

    <owl:Class rdf:about="http://purl.org/olia/tcodex.owl#InstrumentalAdverbial">
        <rdfs:subClassOf rdf:resource="http://purl.org/olia/tcodex.owl#Adverbial"/>
        <rdfs:comment>instrumental adverbial: This is an adverbial of instrument. (Petrova and Odebrecht 2011)</rdfs:comment>
        <owl:versionInfo>Added with T-CODEX 2.1</owl:versionInfo>
    </owl:Class>
    


    <!-- http://purl.org/olia/tcodex.owl#Interjection -->

    <owl:Class rdf:about="http://purl.org/olia/tcodex.owl#Interjection">
        <rdfs:subClassOf rdf:resource="http://purl.org/olia/tcodex.owl#NonInflectedPOS"/>
    </owl:Class>
    


    <!-- http://purl.org/olia/tcodex.owl#InterrogativeMainClause -->

    <owl:Class rdf:about="http://purl.org/olia/tcodex.owl#InterrogativeMainClause">
        <rdfs:subClassOf rdf:resource="http://purl.org/olia/tcodex.owl#MainClause"/>
        <rdfs:comment>This tag is given to main interrogative sentences. No further distinction is made between constituent (wh) and propositional questions.</rdfs:comment>
    </owl:Class>
    


    <!-- http://purl.org/olia/tcodex.owl#InterrogativePronoun -->

    <owl:Class rdf:about="http://purl.org/olia/tcodex.owl#InterrogativePronoun">
        <rdfs:subClassOf rdf:resource="http://purl.org/olia/tcodex.owl#Pronoun"/>
        <rdfs:comment>A interrogative pronoun is a pro-form that is used in questions to stand for the item questioned.
(http://www.sil.org/linguistics/GlossaryOfLinguisticTerms/WhatIsAnInterrogativeProForm.htm 19.09.06)</rdfs:comment>
    </owl:Class>
    


    <!-- http://purl.org/olia/tcodex.owl#InterrogativeSubordinateClause -->

    <owl:Class rdf:about="http://purl.org/olia/tcodex.owl#InterrogativeSubordinateClause">
        <rdfs:subClassOf rdf:resource="http://purl.org/olia/tcodex.owl#SubordinateClause"/>
        <rdfs:comment>This type of subclause expresses embedded questions.</rdfs:comment>
        <owl:deprecated>Removed from T-CODEX 2.1</owl:deprecated>
    </owl:Class>
    


    <!-- http://purl.org/olia/tcodex.owl#LeftDislocation -->

    <owl:Class rdf:about="http://purl.org/olia/tcodex.owl#LeftDislocation">
        <rdfs:subClassOf rdf:resource="http://purl.org/olia/tcodex.owl#InitionalPosition"/>
        <rdfs:comment>Added in T-CODEX 2.1</rdfs:comment>
        <rdfs:comment>left dislocation: In this construction, a left dislocated element is
resumed by a pronoun in the prefield of the main
clause. Note that the pronoun and the left
dislocated element agree in case, gender and
number. (Petrova and Odebrecht 2011)</rdfs:comment>
    </owl:Class>
    


    <!-- http://purl.org/olia/tcodex.owl#LocalAdverb -->

    <owl:Class rdf:about="http://purl.org/olia/tcodex.owl#LocalAdverb">
        <rdfs:subClassOf rdf:resource="http://purl.org/olia/tcodex.owl#Adverb"/>
        <rdfs:comment>This tag is given to adverbs of location.</rdfs:comment>
        <owl:deprecated>Removed from T-CODEX 2.1</owl:deprecated>
    </owl:Class>
    


    <!-- http://purl.org/olia/tcodex.owl#LocalAdverbial -->

    <owl:Class rdf:about="http://purl.org/olia/tcodex.owl#LocalAdverbial">
        <rdfs:subClassOf rdf:resource="http://purl.org/olia/tcodex.owl#Adverbial"/>
        <rdfs:comment>This is an adverbial of location.</rdfs:comment>
    </owl:Class>
    


    <!-- http://purl.org/olia/tcodex.owl#LocalSubordinateClause -->

    <owl:Class rdf:about="http://purl.org/olia/tcodex.owl#LocalSubordinateClause">
        <rdfs:subClassOf rdf:resource="http://purl.org/olia/tcodex.owl#SubordinateClause"/>
        <rdfs:comment>This type of subclause expresses embedded locations.</rdfs:comment>
    </owl:Class>
    


    <!-- http://purl.org/olia/tcodex.owl#MainClause -->

    <owl:Class rdf:about="http://purl.org/olia/tcodex.owl#MainClause">
        <rdfs:subClassOf rdf:resource="http://purl.org/olia/tcodex.owl#ClauseStatus"/>
        <rdfs:comment>This tag is given to independent root clauses with a finite verb. Normally we distinguish between declarative and different types of nondeclarative main clauses, but if a clear-cut distinction is not possible, we use the tag main.</rdfs:comment>
    </owl:Class>
    


    <!-- http://purl.org/olia/tcodex.owl#MainVerb -->

    <owl:Class rdf:about="http://purl.org/olia/tcodex.owl#MainVerb">
        <rdfs:subClassOf rdf:resource="http://purl.org/olia/tcodex.owl#Verb"/>
        <rdfs:comment>This tag is given to the main lexical verb in the clause.</rdfs:comment>
    </owl:Class>
    


    <!-- http://purl.org/olia/tcodex.owl#MixedFocusForm -->

    <owl:Class rdf:about="http://purl.org/olia/tcodex.owl#MixedFocusForm">
        <rdfs:subClassOf rdf:resource="http://purl.org/olia/tcodex.owl#FocusBackground"/>
        <rdfs:subClassOf>
            <owl:Restriction>
                <owl:onProperty rdf:resource="http://purl.org/olia/system.owl#hasTier"/>
                <owl:hasValue>FOCUS_BACKGROUND</owl:hasValue>
            </owl:Restriction>
        </rdfs:subClassOf>
        <rdfs:comment>The categories of „nif“ and „cf“ are not mutually exclusive. If they (partially) overplap, i.e. if a contrastive feature is included in nif, then we use a slash to mark this relation.</rdfs:comment>
    </owl:Class>
    


    <!-- http://purl.org/olia/tcodex.owl#ModalAdverb -->

    <owl:Class rdf:about="http://purl.org/olia/tcodex.owl#ModalAdverb">
        <rdfs:subClassOf rdf:resource="http://purl.org/olia/tcodex.owl#Adverb"/>
        <rdfs:comment>This tag is given to adverbs of manner.</rdfs:comment>
        <owl:deprecated>Removed from T-CODEX 2.1</owl:deprecated>
    </owl:Class>
    


    <!-- http://purl.org/olia/tcodex.owl#ModalAdverbial -->

    <owl:Class rdf:about="http://purl.org/olia/tcodex.owl#ModalAdverbial">
        <rdfs:subClassOf rdf:resource="http://purl.org/olia/tcodex.owl#Adverbial"/>
        <rdfs:comment>This is an adverbial of manner.</rdfs:comment>
    </owl:Class>
    


    <!-- http://purl.org/olia/tcodex.owl#ModalSubordinateClause -->

    <owl:Class rdf:about="http://purl.org/olia/tcodex.owl#ModalSubordinateClause">
        <rdfs:subClassOf rdf:resource="http://purl.org/olia/tcodex.owl#SubordinateClause"/>
        <rdfs:comment>This type of subclause expresses manner.</rdfs:comment>
    </owl:Class>
    


    <!-- http://purl.org/olia/tcodex.owl#ModalVerb -->

    <owl:Class rdf:about="http://purl.org/olia/tcodex.owl#ModalVerb">
        <rdfs:subClassOf rdf:resource="http://purl.org/olia/tcodex.owl#Verb"/>
        <rdfs:comment>Modals are a class of verbs that are used most often with an infinitive to express ability, possibility, disposition or obligation. Pay attention to the fact that the list of modal verbs in OHG is larger than in modern German.</rdfs:comment>
    </owl:Class>
    


    <!-- http://purl.org/olia/tcodex.owl#Morpho-Syntactic -->

    <owl:Class rdf:about="http://purl.org/olia/tcodex.owl#Morpho-Syntactic">
        <rdfs:subClassOf rdf:resource="http://purl.org/olia/system.owl#UnitOfAnnotation"/>
        <owl:versionInfo>T-CODEX annotation was done using with a tool that requires for every annotation to establish its own markable (Exmaralda, http://www.exmaralda.org). Thus, every annotation is a UnitOfAnnotation.</owl:versionInfo>
    </owl:Class>
    


    <!-- http://purl.org/olia/tcodex.owl#NegationWord -->

    <owl:Class rdf:about="http://purl.org/olia/tcodex.owl#NegationWord">
        <rdfs:subClassOf rdf:resource="http://purl.org/olia/tcodex.owl#NonInflectedPOS"/>
        <rdfs:comment>In this category we subsume words that express sentence negation in Old High German:for example the negative particle &quot;ni/ ne&quot; which cliticizes on the finite verb, like in &quot;Ni quam ih&quot; (I didn&apos;t come) or words like &quot;nalles&quot; (and not), &quot;noh&quot; (neither).</rdfs:comment>
    </owl:Class>
    


    <!-- http://purl.org/olia/tcodex.owl#NewInformation -->

    <owl:Class rdf:about="http://purl.org/olia/tcodex.owl#NewInformation">
        <rdfs:subClassOf rdf:resource="http://purl.org/olia/tcodex.owl#Givenness"/>
        <rdfs:comment>This tag is given to expressions that refer to entities with no antecedent in the context.</rdfs:comment>
    </owl:Class>
    


    <!-- http://purl.org/olia/tcodex.owl#NewInformationFocus -->

    <owl:Class rdf:about="http://purl.org/olia/tcodex.owl#NewInformationFocus">
        <rdfs:subClassOf rdf:resource="http://purl.org/olia/tcodex.owl#FocusBackground"/>
        <rdfs:subClassOf>
            <owl:Restriction>
                <owl:onProperty rdf:resource="http://purl.org/olia/system.owl#hasTier"/>
                <owl:hasValue>FOCUS_BACKGROUND</owl:hasValue>
            </owl:Restriction>
        </rdfs:subClassOf>
    </owl:Class>
    


    <!-- http://purl.org/olia/tcodex.owl#NonInflectedPOS -->

    <owl:Class rdf:about="http://purl.org/olia/tcodex.owl#NonInflectedPOS">
        <rdfs:subClassOf rdf:resource="http://purl.org/olia/tcodex.owl#POS"/>
        <rdfs:comment>non-inflected part of speech</rdfs:comment>
        <owl:versionInfo>Category inserted in accordance with Petrova and Odebrecht (2011).</owl:versionInfo>
    </owl:Class>
    


    <!-- http://purl.org/olia/tcodex.owl#NonInitionalPosition -->

    <owl:Class rdf:about="http://purl.org/olia/tcodex.owl#NonInitionalPosition">
        <rdfs:subClassOf rdf:resource="http://purl.org/olia/tcodex.owl#Position"/>
        <rdfs:comment>This tag refers to all non-initial constituents in main declarative clauses.</rdfs:comment>
        <owl:deprecated>Removed from T-CODEX 2.1</owl:deprecated>
    </owl:Class>
    


    <!-- http://purl.org/olia/tcodex.owl#Noun -->

    <owl:Class rdf:about="http://purl.org/olia/tcodex.owl#Noun">
        <rdfs:subClassOf rdf:resource="http://purl.org/olia/tcodex.owl#InflectedPOS"/>
    </owl:Class>
    


    <!-- http://purl.org/olia/tcodex.owl#NounPhrase -->

    <owl:Class rdf:about="http://purl.org/olia/tcodex.owl#NounPhrase">
        <rdfs:subClassOf rdf:resource="http://purl.org/olia/tcodex.owl#SyntacticalCategory"/>
        <rdfs:comment>A noun phrase is a phrase whose head is a noun or a pronoun.</rdfs:comment>
    </owl:Class>
    


    <!-- http://purl.org/olia/tcodex.owl#Numeral -->

    <owl:Class rdf:about="http://purl.org/olia/tcodex.owl#Numeral">
        <rdfs:subClassOf rdf:resource="http://purl.org/olia/tcodex.owl#InflectedPOS"/>
        <rdfs:comment>Numeral is a cover term for cardinal numers, ordinal numbers and some special classes like &apos;both&apos;, &apos;lots of&apos;, &apos;half&apos;. 
(Helbig, G., Buscha J., Deutsche Grammatik, Leipzig Enzyklopädie 10. edition, 1987, page 320 f.) 

Example: &quot;zuelif iaro&quot; (twelve years) (T_096_31-32)</rdfs:comment>
    </owl:Class>
    


    <!-- http://purl.org/olia/tcodex.owl#ObjectFunctionRelativeClause -->

    <owl:Class rdf:about="http://purl.org/olia/tcodex.owl#ObjectFunctionRelativeClause">
        <rdfs:subClassOf rdf:resource="http://purl.org/olia/tcodex.owl#RelativeClause"/>
        <rdfs:comment>These are relative clauses which function as object.</rdfs:comment>
        <owl:deprecated>Removed from T-CODEX 2.1</owl:deprecated>
    </owl:Class>
    


    <!-- http://purl.org/olia/tcodex.owl#ObjectSubordinateClause -->

    <owl:Class rdf:about="http://purl.org/olia/tcodex.owl#ObjectSubordinateClause">
        <rdfs:subClassOf rdf:resource="http://purl.org/olia/tcodex.owl#SubordinateClause"/>
        <rdfs:comment>This tag is given to argument clauses which provide the object of the matrix clause.</rdfs:comment>
        <owl:deprecated>Removed from T-CODEX 2.1</owl:deprecated>
    </owl:Class>
    


    <!-- http://purl.org/olia/tcodex.owl#OptativeMainClause -->

    <owl:Class rdf:about="http://purl.org/olia/tcodex.owl#OptativeMainClause">
        <rdfs:subClassOf rdf:resource="http://purl.org/olia/tcodex.owl#MainClause"/>
        <rdfs:comment>This tag is given to main optative sentences which contain the verb in the subjunctive mood.</rdfs:comment>
    </owl:Class>
    


    <!-- http://purl.org/olia/tcodex.owl#POS -->

    <owl:Class rdf:about="http://purl.org/olia/tcodex.owl#POS">
        <rdfs:subClassOf rdf:resource="http://purl.org/olia/tcodex.owl#Morpho-Syntactic"/>
        <rdfs:subClassOf>
            <owl:Restriction>
                <owl:onProperty rdf:resource="http://purl.org/olia/system.owl#hasTier"/>
                <owl:hasValue>POS</owl:hasValue>
            </owl:Restriction>
        </rdfs:subClassOf>
    </owl:Class>
    


    <!-- http://purl.org/olia/tcodex.owl#ParticipialConstruction -->

    <owl:Class rdf:about="http://purl.org/olia/tcodex.owl#ParticipialConstruction">
        <rdfs:subClassOf rdf:resource="http://purl.org/olia/tcodex.owl#ClauseStatus"/>
        <rdfs:comment>Participial constructions are used as adjunct clauses in Old High German. As they lack a finite verb form they are kept separately from finite subordinate clauses.</rdfs:comment>
    </owl:Class>
    


    <!-- http://purl.org/olia/tcodex.owl#Participle -->

    <owl:Class rdf:about="http://purl.org/olia/tcodex.owl#Participle">
        <rdfs:subClassOf rdf:resource="http://purl.org/olia/tcodex.owl#GrammaticalFunction"/>
        <rdfs:comment>strukturelle Klasse, nicht in Tagset enthalten</rdfs:comment>
    </owl:Class>
    


    <!-- http://purl.org/olia/tcodex.owl#Particle -->

    <owl:Class rdf:about="http://purl.org/olia/tcodex.owl#Particle">
        <rdfs:subClassOf rdf:resource="http://purl.org/olia/tcodex.owl#NonInflectedPOS"/>
        <rdfs:comment>Noninflected parts of speech with no proper denotation, but special functions which contribute to the truth value of the sentence. 
Examples: &quot;uuârlihho&quot;, &quot;ía&quot;, &quot;enu&quot;</rdfs:comment>
    </owl:Class>
    


    <!-- http://purl.org/olia/tcodex.owl#PastParticiple -->

    <owl:Class rdf:about="http://purl.org/olia/tcodex.owl#PastParticiple">
        <rdfs:subClassOf rdf:resource="http://purl.org/olia/tcodex.owl#Participle"/>
        <rdfs:comment>This tag at the level of grammatical function is forced by the subject matter of the project B4, namely to investigate verb-object orders in Old High German. It is of utmost importances to distinguish between tensed and untensed verb forms and to have a quick access to these categories in the annotation. 
(Pintzuk, Susann: Phrase Structures in Competition. Variation in change in old english word order, Garland New York 1999)</rdfs:comment>
    </owl:Class>
    


    <!-- http://purl.org/olia/tcodex.owl#PersonalPronoun -->

    <owl:Class rdf:about="http://purl.org/olia/tcodex.owl#PersonalPronoun">
        <rdfs:subClassOf rdf:resource="http://purl.org/olia/tcodex.owl#Pronoun"/>
        <rdfs:comment>A personal pronoun is a pronoun that expresses a distinction of person deixis. (http://www.sil.org/linguistics/GlossaryOfLinguisticTerms/WhatIsAPersonalPronoun.htm 19.09.06)</rdfs:comment>
    </owl:Class>
    


    <!-- http://purl.org/olia/tcodex.owl#Position -->

    <owl:Class rdf:about="http://purl.org/olia/tcodex.owl#Position">
        <rdfs:subClassOf rdf:resource="http://purl.org/olia/tcodex.owl#TopicComment"/>
        <rdfs:subClassOf>
            <owl:Restriction>
                <owl:onProperty rdf:resource="http://purl.org/olia/system.owl#hasTier"/>
                <owl:hasValue>POSITION</owl:hasValue>
            </owl:Restriction>
        </rdfs:subClassOf>
        <rdfs:comment>This distinction mainly concerns root declaratives. An consistent extension over subclauses will be provided in future.</rdfs:comment>
    </owl:Class>
    


    <!-- http://purl.org/olia/tcodex.owl#PossessivePronoun -->

    <owl:Class rdf:about="http://purl.org/olia/tcodex.owl#PossessivePronoun">
        <rdfs:subClassOf rdf:resource="http://purl.org/olia/tcodex.owl#Pronoun"/>
        <rdfs:comment>In OHG, there is no formal class of possessive pronouns. We give this tag to the genitive form of personal pronouns used to express possessive relations.</rdfs:comment>
    </owl:Class>
    


    <!-- http://purl.org/olia/tcodex.owl#PredicateNoun -->

    <owl:Class rdf:about="http://purl.org/olia/tcodex.owl#PredicateNoun">
        <rdfs:subClassOf rdf:resource="http://purl.org/olia/tcodex.owl#GrammaticalFunction"/>
        <rdfs:comment>The predicate noun (Deutsch: Prädikatsnomen) is a term used in classical philology to describe  the obligatory argument of copula verbs, like &apos;to be&apos;, &apos;to become&apos;, &apos;to call&apos;,  etc.
The predicate noun can be a noun, an adjective, a prepositional phrase and even a whole sentence.

Example: &quot;uuituua&quot; in &quot;thiu uuas uuituua&quot; (She was a widow.) , &quot;cephas&quot; in &quot;thu bist giheizzan cephas&quot; (Your name will be Cephas.)</rdfs:comment>
    </owl:Class>
    


    <!-- http://purl.org/olia/tcodex.owl#PredicativeAttribute -->

    <owl:Class rdf:about="http://purl.org/olia/tcodex.owl#PredicativeAttribute">
        <rdfs:subClassOf rdf:resource="http://purl.org/olia/tcodex.owl#GrammaticalFunction"/>
        <rdfs:comment>A traditional term which expresses secondary predication.
Example: &quot;blint&quot; in &quot;thaz her blint uuvrdi geboran&quot; (That he was born as a blind man.) (T_220_ 17)</rdfs:comment>
    </owl:Class>
    


    <!-- http://purl.org/olia/tcodex.owl#Preposition -->

    <owl:Class rdf:about="http://purl.org/olia/tcodex.owl#Preposition">
        <rdfs:subClassOf rdf:resource="http://purl.org/olia/tcodex.owl#NonInflectedPOS"/>
    </owl:Class>
    


    <!-- http://purl.org/olia/tcodex.owl#PrepositionalObject -->

    <owl:Class rdf:about="http://purl.org/olia/tcodex.owl#PrepositionalObject">
        <rdfs:subClassOf rdf:resource="http://purl.org/olia/tcodex.owl#GrammaticalFunction"/>
        <rdfs:comment>A prepositional phrase which is selected as an argument of a verb or an adjective.
Examples: &quot;in inan&quot; in &quot;giloubtun in inan thó sine iungiron&quot; (His disciples started to believe in Him.) 	                  (T_056_10)
                 &quot;fora gote&quot; in &quot;siu uuarun rehtiu beidu fora gote&quot; (They were both rightious before God.) 	                  (T_026_3)</rdfs:comment>
    </owl:Class>
    


    <!-- http://purl.org/olia/tcodex.owl#PrepositionalPhrase -->

    <owl:Class rdf:about="http://purl.org/olia/tcodex.owl#PrepositionalPhrase">
        <rdfs:subClassOf rdf:resource="http://purl.org/olia/tcodex.owl#SyntacticalCategory"/>
        <rdfs:comment>A prepositional phrase is a phrase whose head is a preposition.</rdfs:comment>
    </owl:Class>
    


    <!-- http://purl.org/olia/tcodex.owl#PresentParticiple -->

    <owl:Class rdf:about="http://purl.org/olia/tcodex.owl#PresentParticiple">
        <rdfs:subClassOf rdf:resource="http://purl.org/olia/tcodex.owl#Participle"/>
        <rdfs:comment>This tag at the level of grammatical function is forced by the subject matter of the project B4, namely to investigate verb-object orders in Old High German. It is of utmost importances to distinguish between tensed and untensed verb forms and to have a quick access to these categories in the annotation. 
(Pintzuk, Susann: Phrase Structures in Competition. Variation in change in old english word order, Garland New York 1999)</rdfs:comment>
    </owl:Class>
    


    <!-- http://purl.org/olia/tcodex.owl#Pronoun -->

    <owl:Class rdf:about="http://purl.org/olia/tcodex.owl#Pronoun">
        <rdfs:subClassOf rdf:resource="http://purl.org/olia/tcodex.owl#InflectedPOS"/>
        <owl:versionInfo>Added for structural reasons, not a tag.</owl:versionInfo>
    </owl:Class>
    


    <!-- http://purl.org/olia/tcodex.owl#QuestionWord -->

    <owl:Class rdf:about="http://purl.org/olia/tcodex.owl#QuestionWord">
        <rdfs:subClassOf rdf:resource="http://purl.org/olia/tcodex.owl#FocusMarker"/>
    </owl:Class>
    


    <!-- http://purl.org/olia/tcodex.owl#ReciprocalPronoun -->

    <owl:Class rdf:about="http://purl.org/olia/tcodex.owl#ReciprocalPronoun">
        <rdfs:subClassOf rdf:resource="http://purl.org/olia/tcodex.owl#Pronoun"/>
        <rdfs:comment>A reciprocal pronoun is a pronoun that expresses a mutual feeling or action among the referents of a plural subject.
(http://www.sil.org/linguistics/GlossaryOfLinguisticTerms/WhatIsAReciprocalPronoun.htm 19.09.06)</rdfs:comment>
    </owl:Class>
    


    <!-- http://purl.org/olia/tcodex.owl#Referent -->

    <owl:Class rdf:about="http://purl.org/olia/tcodex.owl#Referent">
        <rdfs:subClassOf rdf:resource="http://purl.org/olia/tcodex.owl#Aboutness"/>
        <rdfs:comment>This tag is given to expressions that are possible aboutness topics of the clause. For more information on the notion of aboutness, see SFB-Guideline 4.2.2.</rdfs:comment>
    </owl:Class>
    


    <!-- http://purl.org/olia/tcodex.owl#ReflexivePronoun -->

    <owl:Class rdf:about="http://purl.org/olia/tcodex.owl#ReflexivePronoun">
        <rdfs:subClassOf rdf:resource="http://purl.org/olia/tcodex.owl#Pronoun"/>
        <rdfs:comment>A reflexive pronoun is a pronoun that has coreference with the subject.
(http://www.sil.org/linguistics/GlossaryOfLinguisticTerms/WhatIsAReflexivePronoun.htm 19.09.06)</rdfs:comment>
    </owl:Class>
    


    <!-- http://purl.org/olia/tcodex.owl#RelativeClause -->

    <owl:Class rdf:about="http://purl.org/olia/tcodex.owl#RelativeClause">
        <rdfs:subClassOf rdf:resource="http://purl.org/olia/tcodex.owl#ClauseStatus"/>
        <rdfs:comment>Clauses introduced by the demonstrative pronouns in relative function in Old High German are ambigious between main and subordinate clauses. For this reason, they are classified as relative uniformly.
Headless relative clauses are further specified according to their function in the clause, e.g. relative subject or relative object.</rdfs:comment>
    </owl:Class>
    


    <!-- http://purl.org/olia/tcodex.owl#RelativePronoun -->

    <owl:Class rdf:about="http://purl.org/olia/tcodex.owl#RelativePronoun">
        <rdfs:subClassOf rdf:resource="http://purl.org/olia/tcodex.owl#Pronoun"/>
        <rdfs:comment>In OHG, there is no formal class of relative pronouns. We give this tag to different demonstrative pronouns used to introduce a relative clause.</rdfs:comment>
    </owl:Class>
    


    <!-- http://purl.org/olia/tcodex.owl#RequestMainClause -->

    <owl:Class rdf:about="http://purl.org/olia/tcodex.owl#RequestMainClause">
        <rdfs:subClassOf rdf:resource="http://purl.org/olia/tcodex.owl#MainClause"/>
        <rdfs:comment>This tag is given to main sentences which use the subjunctive mood to utter requests.</rdfs:comment>
    </owl:Class>
    


    <!-- http://purl.org/olia/tcodex.owl#SententialAdverbial -->

    <owl:Class rdf:about="http://purl.org/olia/tcodex.owl#SententialAdverbial">
        <rdfs:subClassOf rdf:resource="http://purl.org/olia/tcodex.owl#Adverbial"/>
        <rdfs:comment>sentential adverb This kind of adverbial relates to the entire
proposition. (Petrova and Odebrecht 2011)</rdfs:comment>
        <owl:versionInfo>Added with T-CODEX 2.1</owl:versionInfo>
    </owl:Class>
    


    <!-- http://purl.org/olia/tcodex.owl#SituationShift -->

    <owl:Class rdf:about="http://purl.org/olia/tcodex.owl#SituationShift">
        <rdfs:subClassOf rdf:resource="http://purl.org/olia/tcodex.owl#Context"/>
        <rdfs:comment>Context: Here, we annotate the relation of the clause with respect to the preceding context, especially in terms of discourse organization. We mainly distinguish between “situation shift” (Situationswechsel) und “anaphoric reference” (“AR”). Situationswechsel involves a change of time, place, speaker/narrator and participants. (Petrova and Odebrecht 2011)</rdfs:comment>
    </owl:Class>
    


    <!-- http://purl.org/olia/tcodex.owl#Subject -->

    <owl:Class rdf:about="http://purl.org/olia/tcodex.owl#Subject">
        <rdfs:subClassOf rdf:resource="http://purl.org/olia/tcodex.owl#GrammaticalFunction"/>
    </owl:Class>
    


    <!-- http://purl.org/olia/tcodex.owl#SubjectFunctionRelativeClause -->

    <owl:Class rdf:about="http://purl.org/olia/tcodex.owl#SubjectFunctionRelativeClause">
        <rdfs:subClassOf rdf:resource="http://purl.org/olia/tcodex.owl#RelativeClause"/>
        <rdfs:comment>These are relative clauses which function as subject.</rdfs:comment>
        <owl:deprecated>Removed from T-CODEX 2.1</owl:deprecated>
    </owl:Class>
    


    <!-- http://purl.org/olia/tcodex.owl#SubjectSubordinateClause -->

    <owl:Class rdf:about="http://purl.org/olia/tcodex.owl#SubjectSubordinateClause">
        <rdfs:subClassOf rdf:resource="http://purl.org/olia/tcodex.owl#SubordinateClause"/>
        <rdfs:comment>This tag is given to argument clauses which provide the subject of the matrix clause.</rdfs:comment>
        <owl:deprecated>Removed from T-CODEX 2.1</owl:deprecated>
    </owl:Class>
    


    <!-- http://purl.org/olia/tcodex.owl#SubordinateClause -->

    <owl:Class rdf:about="http://purl.org/olia/tcodex.owl#SubordinateClause">
        <rdfs:subClassOf rdf:resource="http://purl.org/olia/tcodex.owl#ClauseStatus"/>
        <rdfs:comment>This category comprises all finite dependent clauses introduced by a subordinative conjunction except of causal clauses which are kept separately.</rdfs:comment>
    </owl:Class>
    


    <!-- http://purl.org/olia/tcodex.owl#SyntacticalCategory -->

    <owl:Class rdf:about="http://purl.org/olia/tcodex.owl#SyntacticalCategory">
        <rdfs:subClassOf rdf:resource="http://purl.org/olia/tcodex.owl#Morpho-Syntactic"/>
        <rdfs:subClassOf>
            <owl:Restriction>
                <owl:onProperty rdf:resource="http://purl.org/olia/system.owl#hasTier"/>
                <owl:hasValue>CAT</owl:hasValue>
            </owl:Restriction>
        </rdfs:subClassOf>
    </owl:Class>
    


    <!-- http://purl.org/olia/tcodex.owl#TemporalAdverb -->

    <owl:Class rdf:about="http://purl.org/olia/tcodex.owl#TemporalAdverb">
        <rdfs:subClassOf rdf:resource="http://purl.org/olia/tcodex.owl#Adverb"/>
        <rdfs:comment>This is an adverbial of temporal location and extension.</rdfs:comment>
        <owl:deprecated>Removed from T-CODEX 2.1</owl:deprecated>
    </owl:Class>
    


    <!-- http://purl.org/olia/tcodex.owl#TemporalAdverbial -->

    <owl:Class rdf:about="http://purl.org/olia/tcodex.owl#TemporalAdverbial">
        <rdfs:subClassOf rdf:resource="http://purl.org/olia/tcodex.owl#Adverbial"/>
        <rdfs:comment>This is an adverbial of temporal location and extension.</rdfs:comment>
    </owl:Class>
    


    <!-- http://purl.org/olia/tcodex.owl#TemporalSubordinateClause -->

    <owl:Class rdf:about="http://purl.org/olia/tcodex.owl#TemporalSubordinateClause">
        <rdfs:subClassOf rdf:resource="http://purl.org/olia/tcodex.owl#SubordinateClause"/>
        <rdfs:comment>This type of subclause expresses temporal location or extension.</rdfs:comment>
    </owl:Class>
    


    <!-- http://purl.org/olia/tcodex.owl#Topic -->

    <owl:Class rdf:about="http://purl.org/olia/tcodex.owl#Topic">
        <rdfs:subClassOf rdf:resource="http://purl.org/olia/tcodex.owl#TopicComment"/>
        <rdfs:subClassOf>
            <owl:Restriction>
                <owl:onProperty rdf:resource="http://purl.org/olia/system.owl#hasTier"/>
                <owl:hasValue>TOPIC_COMMENT</owl:hasValue>
            </owl:Restriction>
        </rdfs:subClassOf>
        <rdfs:comment>If the sentence favours a topic-comment reading as describe below 5., we mark the constituent that is put in A for topic.</rdfs:comment>
    </owl:Class>
    


    <!-- http://purl.org/olia/tcodex.owl#TopicComment -->

    <owl:Class rdf:about="http://purl.org/olia/tcodex.owl#TopicComment">
        <rdfs:subClassOf rdf:resource="http://purl.org/olia/tcodex.owl#InformationStructure"/>
        <rdfs:comment>Anntoation at this level applies if the sentence favours an unambiguous topic-comment reding, i.e., if the utterance allows for any of the types of canonical tests for topics like “As for X, A says that X…” or “ A says about X that X….”</rdfs:comment>
    </owl:Class>
    


    <!-- http://purl.org/olia/tcodex.owl#TopicMarker -->

    <owl:Class rdf:about="http://purl.org/olia/tcodex.owl#TopicMarker">
        <rdfs:subClassOf rdf:resource="http://purl.org/olia/tcodex.owl#TopicComment"/>
        <rdfs:subClassOf>
            <owl:Restriction>
                <owl:onProperty rdf:resource="http://purl.org/olia/system.owl#hasTier"/>
                <owl:hasValue>TOPIC_MARKER</owl:hasValue>
            </owl:Restriction>
        </rdfs:subClassOf>
        <rdfs:comment>das entsprechende Wort, was einen Topic markiert kein; Tag</rdfs:comment>
    </owl:Class>
    


    <!-- http://purl.org/olia/tcodex.owl#Verb -->

    <owl:Class rdf:about="http://purl.org/olia/tcodex.owl#Verb">
        <rdfs:subClassOf rdf:resource="http://purl.org/olia/tcodex.owl#InflectedPOS"/>
        <owl:versionInfo>Added for structural reasons, not a tag.</owl:versionInfo>
    </owl:Class>
    


    <!-- http://purl.org/olia/tcodex.owl#VerbalNoun -->

    <owl:Class rdf:about="http://purl.org/olia/tcodex.owl#VerbalNoun">
        <rdfs:subClassOf rdf:resource="http://purl.org/olia/tcodex.owl#Verb"/>
        <rdfs:comment>According to the standard literature the category of VerbalNoun in Old High German is a cover term that comprises the noninflected and the inflected infinitives (gerund) and the two participles, the present and the past participle.
(Braune, Wilhelm Althochdeutsche Grammatik I - Laut- und Formenlehre, 15. edition by Reiffenstein, Ingo; Tübingen NIemeyer 2004, §301.5, p.257)

Examples:
noninflected infinitive: &quot;ziohan&quot;  (to draw, to pull)
inflected infinitive after a preposition (zi) which selects the dative case (gerund): &quot;zigebanne&quot; (T_031_23)
present participle: &quot;sehenti&quot; (seeing/ looking) (T_026_21)
past  participle: &quot;gitruobet&quot; (aggrieved, saddened) (T_026_20)</rdfs:comment>
    </owl:Class>
    


    <!-- http://purl.org/olia/tcodex.owl#VerbalPhrase -->

    <owl:Class rdf:about="http://purl.org/olia/tcodex.owl#VerbalPhrase">
        <rdfs:subClassOf rdf:resource="http://purl.org/olia/tcodex.owl#SyntacticalCategory"/>
    </owl:Class>
    


    <!-- http://purl.org/olia/tcodex.owl#VocativeForm -->

    <owl:Class rdf:about="http://purl.org/olia/tcodex.owl#VocativeForm">
        <rdfs:subClassOf rdf:resource="http://purl.org/olia/tcodex.owl#GrammaticalFunction"/>
        <rdfs:comment>An expression referring to a person to which the utterance is addressed, e.g. &quot;truhtin&quot;,  &quot;meistar&quot; or &quot;fater&quot;. The vocative expression typically occurs outside of the clause and not in an argument position selected by the predicate.</rdfs:comment>
    </owl:Class>
    


    <!-- 
    ///////////////////////////////////////////////////////////////////////////////////////
    //
    // Individuals
    //
    ///////////////////////////////////////////////////////////////////////////////////////
     -->

    


    <!-- http://purl.org/olia/tcodex.owl#ADVCOM -->

    <owl:NamedIndividual rdf:about="http://purl.org/olia/tcodex.owl#ADVCOM">
        <rdf:type rdf:resource="http://purl.org/olia/tcodex.owl#ComitativeAdverbial"/>
        <system:hasTag>ADVCOM</system:hasTag>
    </owl:NamedIndividual>
    


    <!-- http://purl.org/olia/tcodex.owl#ADVCOND -->

    <owl:NamedIndividual rdf:about="http://purl.org/olia/tcodex.owl#ADVCOND">
        <rdf:type rdf:resource="http://purl.org/olia/tcodex.owl#ConditionalAdverb"/>
        <system:hasTag>ADVCOND</system:hasTag>
    </owl:NamedIndividual>
    


    <!-- http://purl.org/olia/tcodex.owl#ADVINSTR -->

    <owl:NamedIndividual rdf:about="http://purl.org/olia/tcodex.owl#ADVINSTR">
        <rdf:type rdf:resource="http://purl.org/olia/tcodex.owl#InstrumentalAdverbial"/>
        <system:hasTag>ADVINSTR</system:hasTag>
    </owl:NamedIndividual>
    


    <!-- http://purl.org/olia/tcodex.owl#ADVSENT -->

    <owl:NamedIndividual rdf:about="http://purl.org/olia/tcodex.owl#ADVSENT">
        <rdf:type rdf:resource="http://purl.org/olia/tcodex.owl#SententialAdverbial"/>
        <system:hasTag>ADVSENT</system:hasTag>
    </owl:NamedIndividual>
    


    <!-- http://purl.org/olia/tcodex.owl#AR -->

    <owl:NamedIndividual rdf:about="http://purl.org/olia/tcodex.owl#AR">
        <rdf:type rdf:resource="http://purl.org/olia/tcodex.owl#AnaphoricReference"/>
        <system:hasTag>AR</system:hasTag>
    </owl:NamedIndividual>
    


    <!-- http://purl.org/olia/tcodex.owl#CF_index -->

    <owl:NamedIndividual rdf:about="http://purl.org/olia/tcodex.owl#CF_index">
        <rdf:type rdf:resource="http://purl.org/olia/tcodex.owl#ContrastFocus"/>
        <system:hasTagMatching>^CF_[0-9]*$</system:hasTagMatching>
        <rdfs:comment>CF_01: In cases of multiple foci, we assign indices to the foci belonging to different contrastive pairs. (Petrova and Odebrecht 2011)</rdfs:comment>
    </owl:NamedIndividual>
    


    <!-- http://purl.org/olia/tcodex.owl#FOPR -->

    <owl:NamedIndividual rdf:about="http://purl.org/olia/tcodex.owl#FOPR">
        <rdf:type rdf:resource="http://purl.org/olia/tcodex.owl#FocusSensitiveOperator"/>
        <system:hasTag>FOPR</system:hasTag>
    </owl:NamedIndividual>
    


    <!-- http://purl.org/olia/tcodex.owl#GV -->

    <owl:NamedIndividual rdf:about="http://purl.org/olia/tcodex.owl#GV">
        <rdf:type rdf:resource="http://purl.org/olia/tcodex.owl#GermanVorfeld"/>
        <system:hasTag>GV</system:hasTag>
    </owl:NamedIndividual>
    


    <!-- http://purl.org/olia/tcodex.owl#HT -->

    <owl:NamedIndividual rdf:about="http://purl.org/olia/tcodex.owl#HT">
        <rdf:type rdf:resource="http://purl.org/olia/tcodex.owl#HangingTopic"/>
        <system:hasTag>HT</system:hasTag>
    </owl:NamedIndividual>
    


    <!-- http://purl.org/olia/tcodex.owl#LD -->

    <owl:NamedIndividual rdf:about="http://purl.org/olia/tcodex.owl#LD">
        <rdf:type rdf:resource="http://purl.org/olia/tcodex.owl#LeftDislocation"/>
        <system:hasTag>LD</system:hasTag>
    </owl:NamedIndividual>
    


    <!-- http://purl.org/olia/tcodex.owl#PRD -->

    <owl:NamedIndividual rdf:about="http://purl.org/olia/tcodex.owl#PRD">
        <rdf:type rdf:resource="http://purl.org/olia/tcodex.owl#PredicativeAttribute"/>
        <system:hasTag>PRD</system:hasTag>
    </owl:NamedIndividual>
    


    <!-- http://purl.org/olia/tcodex.owl#Situationswechsel -->

    <owl:NamedIndividual rdf:about="http://purl.org/olia/tcodex.owl#Situationswechsel">
        <rdf:type rdf:resource="http://purl.org/olia/tcodex.owl#SituationShift"/>
        <system:hasTag>Situationswechsel</system:hasTag>
    </owl:NamedIndividual>
    


    <!-- http://purl.org/olia/tcodex.owl#acc -->

    <owl:NamedIndividual rdf:about="http://purl.org/olia/tcodex.owl#acc">
        <rdf:type rdf:resource="http://purl.org/olia/tcodex.owl#AccessibleInformation"/>
        <system:hasTag>ACC</system:hasTag>
    </owl:NamedIndividual>
    


    <!-- http://purl.org/olia/tcodex.owl#adj -->

    <owl:NamedIndividual rdf:about="http://purl.org/olia/tcodex.owl#adj">
        <rdf:type rdf:resource="http://purl.org/olia/tcodex.owl#Adjective"/>
        <system:hasTag>A</system:hasTag>
    </owl:NamedIndividual>
    


    <!-- http://purl.org/olia/tcodex.owl#adjp -->

    <owl:NamedIndividual rdf:about="http://purl.org/olia/tcodex.owl#adjp">
        <rdf:type rdf:resource="http://purl.org/olia/tcodex.owl#AdjectivialPhrase"/>
        <system:hasTag>adjp</system:hasTag>
    </owl:NamedIndividual>
    


    <!-- http://purl.org/olia/tcodex.owl#adv -->

    <owl:NamedIndividual rdf:about="http://purl.org/olia/tcodex.owl#adv">
        <rdf:type rdf:resource="http://purl.org/olia/tcodex.owl#Adverb"/>
        <system:hasTag>ADV</system:hasTag>
    </owl:NamedIndividual>
    


    <!-- http://purl.org/olia/tcodex.owl#adv_caus -->

    <owl:NamedIndividual rdf:about="http://purl.org/olia/tcodex.owl#adv_caus">
        <rdf:type rdf:resource="http://purl.org/olia/tcodex.owl#CausalAdverb"/>
        <system:hasTag>adv:caus</system:hasTag>
    </owl:NamedIndividual>
    


    <!-- http://purl.org/olia/tcodex.owl#adv_dir -->

    <owl:NamedIndividual rdf:about="http://purl.org/olia/tcodex.owl#adv_dir">
        <rdf:type rdf:resource="http://purl.org/olia/tcodex.owl#DirectionalAdverb"/>
        <system:hasTag>adv:dir</system:hasTag>
    </owl:NamedIndividual>
    


    <!-- http://purl.org/olia/tcodex.owl#adv_loc -->

    <owl:NamedIndividual rdf:about="http://purl.org/olia/tcodex.owl#adv_loc">
        <rdf:type rdf:resource="http://purl.org/olia/tcodex.owl#LocalAdverb"/>
        <system:hasTag>adv:loc</system:hasTag>
    </owl:NamedIndividual>
    


    <!-- http://purl.org/olia/tcodex.owl#adv_mod -->

    <owl:NamedIndividual rdf:about="http://purl.org/olia/tcodex.owl#adv_mod">
        <rdf:type rdf:resource="http://purl.org/olia/tcodex.owl#ModalAdverb"/>
        <system:hasTag>adv:mod</system:hasTag>
    </owl:NamedIndividual>
    


    <!-- http://purl.org/olia/tcodex.owl#adv_temp -->

    <owl:NamedIndividual rdf:about="http://purl.org/olia/tcodex.owl#adv_temp">
        <rdf:type rdf:resource="http://purl.org/olia/tcodex.owl#TemporalAdverb"/>
        <system:hasTag>adv:temp</system:hasTag>
    </owl:NamedIndividual>
    


    <!-- http://purl.org/olia/tcodex.owl#adverbial -->

    <owl:NamedIndividual rdf:about="http://purl.org/olia/tcodex.owl#adverbial">
        <rdf:type rdf:resource="http://purl.org/olia/tcodex.owl#Adverbial"/>
        <system:hasTag>adv</system:hasTag>
    </owl:NamedIndividual>
    


    <!-- http://purl.org/olia/tcodex.owl#advp -->

    <owl:NamedIndividual rdf:about="http://purl.org/olia/tcodex.owl#advp">
        <rdf:type rdf:resource="http://purl.org/olia/tcodex.owl#AdverbalPhrase"/>
        <system:hasTag>ADVP</system:hasTag>
    </owl:NamedIndividual>
    


    <!-- http://purl.org/olia/tcodex.owl#appos -->

    <owl:NamedIndividual rdf:about="http://purl.org/olia/tcodex.owl#appos">
        <rdf:type rdf:resource="http://purl.org/olia/tcodex.owl#Apposition"/>
        <system:hasTag>APPOS</system:hasTag>
    </owl:NamedIndividual>
    


    <!-- http://purl.org/olia/tcodex.owl#attr -->

    <owl:NamedIndividual rdf:about="http://purl.org/olia/tcodex.owl#attr">
        <rdf:type rdf:resource="http://purl.org/olia/tcodex.owl#Attribute"/>
        <system:hasTag>ATTR</system:hasTag>
    </owl:NamedIndividual>
    


    <!-- http://purl.org/olia/tcodex.owl#attr_do -->

    <owl:NamedIndividual rdf:about="http://purl.org/olia/tcodex.owl#attr_do">
        <rdf:type rdf:resource="http://purl.org/olia/tcodex.owl#Attrbute_to_Object"/>
        <system:hasTag>attr/do</system:hasTag>
    </owl:NamedIndividual>
    


    <!-- http://purl.org/olia/tcodex.owl#attr_predn -->

    <owl:NamedIndividual rdf:about="http://purl.org/olia/tcodex.owl#attr_predn">
        <rdf:type rdf:resource="http://purl.org/olia/tcodex.owl#Attribute_to_PredicateNoun"/>
        <system:hasTag>ATTRPRDNOM</system:hasTag>
    </owl:NamedIndividual>
    


    <!-- http://purl.org/olia/tcodex.owl#attr_su -->

    <owl:NamedIndividual rdf:about="http://purl.org/olia/tcodex.owl#attr_su">
        <rdf:type rdf:resource="http://purl.org/olia/tcodex.owl#Attribute_to_Subject"/>
        <system:hasTag>attr/su</system:hasTag>
    </owl:NamedIndividual>
    


    <!-- http://purl.org/olia/tcodex.owl#aux -->

    <owl:NamedIndividual rdf:about="http://purl.org/olia/tcodex.owl#aux">
        <rdf:type rdf:resource="http://purl.org/olia/tcodex.owl#AuxiliaryVerb"/>
        <system:hasTag>VAUX</system:hasTag>
    </owl:NamedIndividual>
    


    <!-- http://purl.org/olia/tcodex.owl#caus_adverbial -->

    <owl:NamedIndividual rdf:about="http://purl.org/olia/tcodex.owl#caus_adverbial">
        <rdf:type rdf:resource="http://purl.org/olia/tcodex.owl#CausalAdverbial"/>
        <system:hasTag>ADVCAUS</system:hasTag>
    </owl:NamedIndividual>
    


    <!-- http://purl.org/olia/tcodex.owl#causal -->

    <owl:NamedIndividual rdf:about="http://purl.org/olia/tcodex.owl#causal">
        <rdf:type rdf:resource="http://purl.org/olia/tcodex.owl#Causal"/>
        <system:hasTag>CAUSAL</system:hasTag>
    </owl:NamedIndividual>
    


    <!-- http://purl.org/olia/tcodex.owl#cf -->

    <owl:NamedIndividual rdf:about="http://purl.org/olia/tcodex.owl#cf">
        <rdf:type rdf:resource="http://purl.org/olia/tcodex.owl#ContrastFocus"/>
        <system:hasTag>CF</system:hasTag>
    </owl:NamedIndividual>
    


    <!-- http://purl.org/olia/tcodex.owl#comm -->

    <owl:NamedIndividual rdf:about="http://purl.org/olia/tcodex.owl#comm">
        <rdf:type rdf:resource="http://purl.org/olia/tcodex.owl#Comment"/>
        <system:hasTag>COMM</system:hasTag>
    </owl:NamedIndividual>
    


    <!-- http://purl.org/olia/tcodex.owl#conj -->

    <owl:NamedIndividual rdf:about="http://purl.org/olia/tcodex.owl#conj">
        <rdf:type rdf:resource="http://purl.org/olia/tcodex.owl#Conjunction"/>
        <system:hasTag>CONJ</system:hasTag>
    </owl:NamedIndividual>
    


    <!-- http://purl.org/olia/tcodex.owl#cop -->

    <owl:NamedIndividual rdf:about="http://purl.org/olia/tcodex.owl#cop">
        <rdf:type rdf:resource="http://purl.org/olia/tcodex.owl#CopulaVerb"/>
        <system:hasTag>VCOP</system:hasTag>
    </owl:NamedIndividual>
    


    <!-- http://purl.org/olia/tcodex.owl#cp -->

    <owl:NamedIndividual rdf:about="http://purl.org/olia/tcodex.owl#cp">
        <rdf:type rdf:resource="http://purl.org/olia/tcodex.owl#ComplementizerPhrase"/>
        <system:hasTag>CP</system:hasTag>
    </owl:NamedIndividual>
    


    <!-- http://purl.org/olia/tcodex.owl#def -->

    <owl:NamedIndividual rdf:about="http://purl.org/olia/tcodex.owl#def">
        <rdf:type rdf:resource="http://purl.org/olia/tcodex.owl#Definite"/>
        <system:hasTag>DEF</system:hasTag>
    </owl:NamedIndividual>
    


    <!-- http://purl.org/olia/tcodex.owl#dir -->

    <owl:NamedIndividual rdf:about="http://purl.org/olia/tcodex.owl#dir">
        <rdf:type rdf:resource="http://purl.org/olia/tcodex.owl#Directional"/>
        <system:hasTag>DIR</system:hasTag>
    </owl:NamedIndividual>
    


    <!-- http://purl.org/olia/tcodex.owl#do -->

    <owl:NamedIndividual rdf:about="http://purl.org/olia/tcodex.owl#do">
        <rdf:type rdf:resource="http://purl.org/olia/tcodex.owl#DirectObject"/>
        <system:hasTag>DO</system:hasTag>
    </owl:NamedIndividual>
    


    <!-- http://purl.org/olia/tcodex.owl#frame -->

    <owl:NamedIndividual rdf:about="http://purl.org/olia/tcodex.owl#frame">
        <rdf:type rdf:resource="http://purl.org/olia/tcodex.owl#Frame"/>
        <system:hasTag>FRAME</system:hasTag>
    </owl:NamedIndividual>
    


    <!-- http://purl.org/olia/tcodex.owl#gerund -->

    <owl:NamedIndividual rdf:about="http://purl.org/olia/tcodex.owl#gerund">
        <rdf:type rdf:resource="http://purl.org/olia/tcodex.owl#Gerund"/>
        <system:hasTag>GERUND</system:hasTag>
    </owl:NamedIndividual>
    


    <!-- http://purl.org/olia/tcodex.owl#giv -->

    <owl:NamedIndividual rdf:about="http://purl.org/olia/tcodex.owl#giv">
        <rdf:type rdf:resource="http://purl.org/olia/tcodex.owl#GivenInformation"/>
        <system:hasTag>GIV</system:hasTag>
    </owl:NamedIndividual>
    


    <!-- http://purl.org/olia/tcodex.owl#indef -->

    <owl:NamedIndividual rdf:about="http://purl.org/olia/tcodex.owl#indef">
        <rdf:type rdf:resource="http://purl.org/olia/tcodex.owl#Indefinite"/>
        <system:hasTag>INDEF</system:hasTag>
    </owl:NamedIndividual>
    


    <!-- http://purl.org/olia/tcodex.owl#inf -->

    <owl:NamedIndividual rdf:about="http://purl.org/olia/tcodex.owl#inf">
        <rdf:type rdf:resource="http://purl.org/olia/tcodex.owl#Infinitive"/>
        <system:hasTag>INF</system:hasTag>
    </owl:NamedIndividual>
    


    <!-- http://purl.org/olia/tcodex.owl#infinitival_clause -->

    <owl:NamedIndividual rdf:about="http://purl.org/olia/tcodex.owl#infinitival_clause">
        <rdf:type rdf:resource="http://purl.org/olia/tcodex.owl#InfinitivalClause"/>
        <system:hasTag>INFCLAUSE</system:hasTag>
    </owl:NamedIndividual>
    


    <!-- http://purl.org/olia/tcodex.owl#init -->

    <owl:NamedIndividual rdf:about="http://purl.org/olia/tcodex.owl#init">
        <rdf:type rdf:resource="http://purl.org/olia/tcodex.owl#InitionalPosition"/>
        <system:hasTag>init</system:hasTag>
    </owl:NamedIndividual>
    


    <!-- http://purl.org/olia/tcodex.owl#interj -->

    <owl:NamedIndividual rdf:about="http://purl.org/olia/tcodex.owl#interj">
        <rdf:type rdf:resource="http://purl.org/olia/tcodex.owl#Interjection"/>
        <system:hasTag>INTERJ</system:hasTag>
    </owl:NamedIndividual>
    


    <!-- http://purl.org/olia/tcodex.owl#io -->

    <owl:NamedIndividual rdf:about="http://purl.org/olia/tcodex.owl#io">
        <rdf:type rdf:resource="http://purl.org/olia/tcodex.owl#IndirectObject"/>
        <system:hasTag>IO</system:hasTag>
    </owl:NamedIndividual>
    


    <!-- http://purl.org/olia/tcodex.owl#loc_adverbial -->

    <owl:NamedIndividual rdf:about="http://purl.org/olia/tcodex.owl#loc_adverbial">
        <rdf:type rdf:resource="http://purl.org/olia/tcodex.owl#LocalAdverbial"/>
        <system:hasTag>ADVLOC</system:hasTag>
    </owl:NamedIndividual>
    


    <!-- http://purl.org/olia/tcodex.owl#main -->

    <owl:NamedIndividual rdf:about="http://purl.org/olia/tcodex.owl#main">
        <rdf:type rdf:resource="http://purl.org/olia/tcodex.owl#MainClause"/>
    </owl:NamedIndividual>
    


    <!-- http://purl.org/olia/tcodex.owl#main_declarative -->

    <owl:NamedIndividual rdf:about="http://purl.org/olia/tcodex.owl#main_declarative">
        <rdf:type rdf:resource="http://purl.org/olia/tcodex.owl#DeclarativeMainClause"/>
        <system:hasTag>MAINDECL</system:hasTag>
    </owl:NamedIndividual>
    


    <!-- http://purl.org/olia/tcodex.owl#main_imperative -->

    <owl:NamedIndividual rdf:about="http://purl.org/olia/tcodex.owl#main_imperative">
        <rdf:type rdf:resource="http://purl.org/olia/tcodex.owl#ImperativeMainClause"/>
        <system:hasTag>MAINIMPER</system:hasTag>
    </owl:NamedIndividual>
    


    <!-- http://purl.org/olia/tcodex.owl#main_interrogative -->

    <owl:NamedIndividual rdf:about="http://purl.org/olia/tcodex.owl#main_interrogative">
        <rdf:type rdf:resource="http://purl.org/olia/tcodex.owl#InterrogativeMainClause"/>
        <system:hasTag>MAININTERR</system:hasTag>
    </owl:NamedIndividual>
    


    <!-- http://purl.org/olia/tcodex.owl#main_optative -->

    <owl:NamedIndividual rdf:about="http://purl.org/olia/tcodex.owl#main_optative">
        <rdf:type rdf:resource="http://purl.org/olia/tcodex.owl#OptativeMainClause"/>
        <system:hasTag>MAINOPTAT</system:hasTag>
    </owl:NamedIndividual>
    


    <!-- http://purl.org/olia/tcodex.owl#main_request -->

    <owl:NamedIndividual rdf:about="http://purl.org/olia/tcodex.owl#main_request">
        <rdf:type rdf:resource="http://purl.org/olia/tcodex.owl#RequestMainClause"/>
        <system:hasTag>MAINREQUEST</system:hasTag>
    </owl:NamedIndividual>
    


    <!-- http://purl.org/olia/tcodex.owl#modal -->

    <owl:NamedIndividual rdf:about="http://purl.org/olia/tcodex.owl#modal">
        <rdf:type rdf:resource="http://purl.org/olia/tcodex.owl#ModalVerb"/>
        <system:hasTag>VMOD</system:hasTag>
    </owl:NamedIndividual>
    


    <!-- http://purl.org/olia/tcodex.owl#modal_adverbial -->

    <owl:NamedIndividual rdf:about="http://purl.org/olia/tcodex.owl#modal_adverbial">
        <rdf:type rdf:resource="http://purl.org/olia/tcodex.owl#ModalAdverbial"/>
        <system:hasTag>ADVMOD</system:hasTag>
    </owl:NamedIndividual>
    


    <!-- http://purl.org/olia/tcodex.owl#n -->

    <owl:NamedIndividual rdf:about="http://purl.org/olia/tcodex.owl#n">
        <rdf:type rdf:resource="http://purl.org/olia/tcodex.owl#Noun"/>
        <system:hasTag>N</system:hasTag>
    </owl:NamedIndividual>
    


    <!-- http://purl.org/olia/tcodex.owl#neg -->

    <owl:NamedIndividual rdf:about="http://purl.org/olia/tcodex.owl#neg">
        <rdf:type rdf:resource="http://purl.org/olia/tcodex.owl#NegationWord"/>
        <system:hasTag>NEG</system:hasTag>
    </owl:NamedIndividual>
    


    <!-- http://purl.org/olia/tcodex.owl#new -->

    <owl:NamedIndividual rdf:about="http://purl.org/olia/tcodex.owl#new">
        <rdf:type rdf:resource="http://purl.org/olia/tcodex.owl#NewInformation"/>
        <system:hasTag>NEW</system:hasTag>
    </owl:NamedIndividual>
    


    <!-- http://purl.org/olia/tcodex.owl#nif -->

    <owl:NamedIndividual rdf:about="http://purl.org/olia/tcodex.owl#nif">
        <rdf:type rdf:resource="http://purl.org/olia/tcodex.owl#NewInformationFocus"/>
        <system:hasTag>NIF</system:hasTag>
    </owl:NamedIndividual>
    


    <!-- http://purl.org/olia/tcodex.owl#nif-cf -->

    <owl:NamedIndividual rdf:about="http://purl.org/olia/tcodex.owl#nif-cf">
        <rdf:type rdf:resource="http://purl.org/olia/tcodex.owl#MixedFocusForm"/>
        <system:hasTag>NIFCF</system:hasTag>
    </owl:NamedIndividual>
    


    <!-- http://purl.org/olia/tcodex.owl#noninit -->

    <owl:NamedIndividual rdf:about="http://purl.org/olia/tcodex.owl#noninit">
        <rdf:type rdf:resource="http://purl.org/olia/tcodex.owl#NonInitionalPosition"/>
        <system:hasTag>noninit</system:hasTag>
    </owl:NamedIndividual>
    


    <!-- http://purl.org/olia/tcodex.owl#np -->

    <owl:NamedIndividual rdf:about="http://purl.org/olia/tcodex.owl#np">
        <rdf:type rdf:resource="http://purl.org/olia/tcodex.owl#NounPhrase"/>
        <system:hasTag>NP</system:hasTag>
    </owl:NamedIndividual>
    


    <!-- http://purl.org/olia/tcodex.owl#num -->

    <owl:NamedIndividual rdf:about="http://purl.org/olia/tcodex.owl#num">
        <rdf:type rdf:resource="http://purl.org/olia/tcodex.owl#Numeral"/>
        <system:hasTag>NUM</system:hasTag>
    </owl:NamedIndividual>
    


    <!-- http://purl.org/olia/tcodex.owl#participial_construction -->

    <owl:NamedIndividual rdf:about="http://purl.org/olia/tcodex.owl#participial_construction">
        <rdf:type rdf:resource="http://purl.org/olia/tcodex.owl#ParticipialConstruction"/>
        <system:hasTag>PARTCONSTR</system:hasTag>
    </owl:NamedIndividual>
    


    <!-- http://purl.org/olia/tcodex.owl#particle -->

    <owl:NamedIndividual rdf:about="http://purl.org/olia/tcodex.owl#particle">
        <rdf:type rdf:resource="http://purl.org/olia/tcodex.owl#Particle"/>
        <system:hasTag>PTC</system:hasTag>
    </owl:NamedIndividual>
    


    <!-- http://purl.org/olia/tcodex.owl#partpf -->

    <owl:NamedIndividual rdf:about="http://purl.org/olia/tcodex.owl#partpf">
        <rdf:type rdf:resource="http://purl.org/olia/tcodex.owl#PastParticiple"/>
        <system:hasTag>PARTPF</system:hasTag>
    </owl:NamedIndividual>
    


    <!-- http://purl.org/olia/tcodex.owl#partpr -->

    <owl:NamedIndividual rdf:about="http://purl.org/olia/tcodex.owl#partpr">
        <rdf:type rdf:resource="http://purl.org/olia/tcodex.owl#PresentParticiple"/>
        <system:hasTag>PARTPR</system:hasTag>
    </owl:NamedIndividual>
    


    <!-- http://purl.org/olia/tcodex.owl#pp -->

    <owl:NamedIndividual rdf:about="http://purl.org/olia/tcodex.owl#pp">
        <rdf:type rdf:resource="http://purl.org/olia/tcodex.owl#PrepositionalPhrase"/>
        <system:hasTag>PP</system:hasTag>
    </owl:NamedIndividual>
    


    <!-- http://purl.org/olia/tcodex.owl#prdem -->

    <owl:NamedIndividual rdf:about="http://purl.org/olia/tcodex.owl#prdem">
        <rdf:type rdf:resource="http://purl.org/olia/tcodex.owl#DemonstrativePronoun"/>
        <system:hasTag>PRONDEM</system:hasTag>
    </owl:NamedIndividual>
    


    <!-- http://purl.org/olia/tcodex.owl#pred -->

    <owl:NamedIndividual rdf:about="http://purl.org/olia/tcodex.owl#pred">
        <rdf:type rdf:resource="http://purl.org/olia/tcodex.owl#PrepositionalObject"/>
        <system:hasTag>PO</system:hasTag>
    </owl:NamedIndividual>
    


    <!-- http://purl.org/olia/tcodex.owl#predn -->

    <owl:NamedIndividual rdf:about="http://purl.org/olia/tcodex.owl#predn">
        <rdf:type rdf:resource="http://purl.org/olia/tcodex.owl#PredicateNoun"/>
        <system:hasTag>PRDNOM</system:hasTag>
    </owl:NamedIndividual>
    


    <!-- http://purl.org/olia/tcodex.owl#prep -->

    <owl:NamedIndividual rdf:about="http://purl.org/olia/tcodex.owl#prep">
        <rdf:type rdf:resource="http://purl.org/olia/tcodex.owl#Preposition"/>
        <system:hasTag>AP</system:hasTag>
    </owl:NamedIndividual>
    


    <!-- http://purl.org/olia/tcodex.owl#prindef -->

    <owl:NamedIndividual rdf:about="http://purl.org/olia/tcodex.owl#prindef">
        <rdf:type rdf:resource="http://purl.org/olia/tcodex.owl#IndefinitePronoun"/>
        <system:hasTag>PRONINTERR</system:hasTag>
    </owl:NamedIndividual>
    


    <!-- http://purl.org/olia/tcodex.owl#printerr -->

    <owl:NamedIndividual rdf:about="http://purl.org/olia/tcodex.owl#printerr">
        <rdf:type rdf:resource="http://purl.org/olia/tcodex.owl#InterrogativePronoun"/>
        <system:hasTag>printerr</system:hasTag>
    </owl:NamedIndividual>
    


    <!-- http://purl.org/olia/tcodex.owl#prpers -->

    <owl:NamedIndividual rdf:about="http://purl.org/olia/tcodex.owl#prpers">
        <rdf:type rdf:resource="http://purl.org/olia/tcodex.owl#PersonalPronoun"/>
        <system:hasTag>PRONPRS</system:hasTag>
    </owl:NamedIndividual>
    


    <!-- http://purl.org/olia/tcodex.owl#prposs -->

    <owl:NamedIndividual rdf:about="http://purl.org/olia/tcodex.owl#prposs">
        <rdf:type rdf:resource="http://purl.org/olia/tcodex.owl#PossessivePronoun"/>
        <system:hasTag>PRONPOS</system:hasTag>
    </owl:NamedIndividual>
    


    <!-- http://purl.org/olia/tcodex.owl#prref -->

    <owl:NamedIndividual rdf:about="http://purl.org/olia/tcodex.owl#prref">
        <rdf:type rdf:resource="http://purl.org/olia/tcodex.owl#ReflexivePronoun"/>
        <system:hasTag>PRONRFL</system:hasTag>
    </owl:NamedIndividual>
    


    <!-- http://purl.org/olia/tcodex.owl#prrel -->

    <owl:NamedIndividual rdf:about="http://purl.org/olia/tcodex.owl#prrel">
        <rdf:type rdf:resource="http://purl.org/olia/tcodex.owl#RelativePronoun"/>
        <system:hasTag>PRONREL</system:hasTag>
    </owl:NamedIndividual>
    


    <!-- http://purl.org/olia/tcodex.owl#prrez -->

    <owl:NamedIndividual rdf:about="http://purl.org/olia/tcodex.owl#prrez">
        <rdf:type rdf:resource="http://purl.org/olia/tcodex.owl#ReciprocalPronoun"/>
        <system:hasTag>PRONREZ</system:hasTag>
    </owl:NamedIndividual>
    


    <!-- http://purl.org/olia/tcodex.owl#ref -->

    <owl:NamedIndividual rdf:about="http://purl.org/olia/tcodex.owl#ref">
        <rdf:type rdf:resource="http://purl.org/olia/tcodex.owl#Referent"/>
        <system:hasTag>AB</system:hasTag>
    </owl:NamedIndividual>
    


    <!-- http://purl.org/olia/tcodex.owl#relative -->

    <owl:NamedIndividual rdf:about="http://purl.org/olia/tcodex.owl#relative">
        <rdf:type rdf:resource="http://purl.org/olia/tcodex.owl#RelativeClause"/>
        <system:hasTag>REL</system:hasTag>
    </owl:NamedIndividual>
    


    <!-- http://purl.org/olia/tcodex.owl#relative_obj -->

    <owl:NamedIndividual rdf:about="http://purl.org/olia/tcodex.owl#relative_obj">
        <rdf:type rdf:resource="http://purl.org/olia/tcodex.owl#ObjectFunctionRelativeClause"/>
        <system:hasTag>relative:obj</system:hasTag>
    </owl:NamedIndividual>
    


    <!-- http://purl.org/olia/tcodex.owl#relative_su -->

    <owl:NamedIndividual rdf:about="http://purl.org/olia/tcodex.owl#relative_su">
        <rdf:type rdf:resource="http://purl.org/olia/tcodex.owl#SubjectFunctionRelativeClause"/>
        <system:hasTag>relative:su</system:hasTag>
    </owl:NamedIndividual>
    


    <!-- http://purl.org/olia/tcodex.owl#su -->

    <owl:NamedIndividual rdf:about="http://purl.org/olia/tcodex.owl#su">
        <rdf:type rdf:resource="http://purl.org/olia/tcodex.owl#Subject"/>
        <system:hasTag>SUBJ</system:hasTag>
    </owl:NamedIndividual>
    


    <!-- http://purl.org/olia/tcodex.owl#subordinate -->

    <owl:NamedIndividual rdf:about="http://purl.org/olia/tcodex.owl#subordinate">
        <rdf:type rdf:resource="http://purl.org/olia/tcodex.owl#SubordinateClause"/>
        <system:hasTag>SUB</system:hasTag>
    </owl:NamedIndividual>
    


    <!-- http://purl.org/olia/tcodex.owl#subordinate_attributive -->

    <owl:NamedIndividual rdf:about="http://purl.org/olia/tcodex.owl#subordinate_attributive">
        <rdf:type rdf:resource="http://purl.org/olia/tcodex.owl#AttributiveSubordinateClause"/>
        <system:hasTag>subordinate:attributive</system:hasTag>
    </owl:NamedIndividual>
    


    <!-- http://purl.org/olia/tcodex.owl#subordinate_comparative -->

    <owl:NamedIndividual rdf:about="http://purl.org/olia/tcodex.owl#subordinate_comparative">
        <rdf:type rdf:resource="http://purl.org/olia/tcodex.owl#ComparativeSubordinateClause"/>
        <system:hasTag>SUBCOMPAR</system:hasTag>
    </owl:NamedIndividual>
    


    <!-- http://purl.org/olia/tcodex.owl#subordinate_concessive -->

    <owl:NamedIndividual rdf:about="http://purl.org/olia/tcodex.owl#subordinate_concessive">
        <rdf:type rdf:resource="http://purl.org/olia/tcodex.owl#ConcessiveSubordinateClause"/>
        <system:hasTag>SUBCONC</system:hasTag>
    </owl:NamedIndividual>
    


    <!-- http://purl.org/olia/tcodex.owl#subordinate_conditional -->

    <owl:NamedIndividual rdf:about="http://purl.org/olia/tcodex.owl#subordinate_conditional">
        <rdf:type rdf:resource="http://purl.org/olia/tcodex.owl#ConditionalSubordinateClause"/>
        <system:hasTag>SUBCOND</system:hasTag>
    </owl:NamedIndividual>
    


    <!-- http://purl.org/olia/tcodex.owl#subordinate_consecutive -->

    <owl:NamedIndividual rdf:about="http://purl.org/olia/tcodex.owl#subordinate_consecutive">
        <rdf:type rdf:resource="http://purl.org/olia/tcodex.owl#ConsecutiveSubordinateClause"/>
        <system:hasTag>SUBCONS</system:hasTag>
    </owl:NamedIndividual>
    


    <!-- http://purl.org/olia/tcodex.owl#subordinate_final -->

    <owl:NamedIndividual rdf:about="http://purl.org/olia/tcodex.owl#subordinate_final">
        <rdf:type rdf:resource="http://purl.org/olia/tcodex.owl#FinalSubordinateClause"/>
        <system:hasTag>SUBFINAL</system:hasTag>
    </owl:NamedIndividual>
    


    <!-- http://purl.org/olia/tcodex.owl#subordinate_interrogative -->

    <owl:NamedIndividual rdf:about="http://purl.org/olia/tcodex.owl#subordinate_interrogative">
        <rdf:type rdf:resource="http://purl.org/olia/tcodex.owl#InterrogativeSubordinateClause"/>
        <system:hasTag>subordinate:interrogative</system:hasTag>
    </owl:NamedIndividual>
    


    <!-- http://purl.org/olia/tcodex.owl#subordinate_local -->

    <owl:NamedIndividual rdf:about="http://purl.org/olia/tcodex.owl#subordinate_local">
        <rdf:type rdf:resource="http://purl.org/olia/tcodex.owl#LocalSubordinateClause"/>
        <system:hasTag>SUBLOCAL</system:hasTag>
    </owl:NamedIndividual>
    


    <!-- http://purl.org/olia/tcodex.owl#subordinate_modal -->

    <owl:NamedIndividual rdf:about="http://purl.org/olia/tcodex.owl#subordinate_modal">
        <rdf:type rdf:resource="http://purl.org/olia/tcodex.owl#ModalSubordinateClause"/>
        <system:hasTag>SUBMODAL</system:hasTag>
    </owl:NamedIndividual>
    


    <!-- http://purl.org/olia/tcodex.owl#subordinate_object -->

    <owl:NamedIndividual rdf:about="http://purl.org/olia/tcodex.owl#subordinate_object">
        <rdf:type rdf:resource="http://purl.org/olia/tcodex.owl#ObjectSubordinateClause"/>
        <system:hasTag>subordinate:object</system:hasTag>
    </owl:NamedIndividual>
    


    <!-- http://purl.org/olia/tcodex.owl#subordinate_subject -->

    <owl:NamedIndividual rdf:about="http://purl.org/olia/tcodex.owl#subordinate_subject">
        <rdf:type rdf:resource="http://purl.org/olia/tcodex.owl#SubjectSubordinateClause"/>
        <system:hasTag>subordinate:su</system:hasTag>
    </owl:NamedIndividual>
    


    <!-- http://purl.org/olia/tcodex.owl#subordinate_temporal -->

    <owl:NamedIndividual rdf:about="http://purl.org/olia/tcodex.owl#subordinate_temporal">
        <rdf:type rdf:resource="http://purl.org/olia/tcodex.owl#TemporalSubordinateClause"/>
        <system:hasTag>SUBTEMP</system:hasTag>
    </owl:NamedIndividual>
    


    <!-- http://purl.org/olia/tcodex.owl#temporal_adverbial -->

    <owl:NamedIndividual rdf:about="http://purl.org/olia/tcodex.owl#temporal_adverbial">
        <rdf:type rdf:resource="http://purl.org/olia/tcodex.owl#TemporalAdverbial"/>
        <system:hasTag>ADVTEMP</system:hasTag>
    </owl:NamedIndividual>
    


    <!-- http://purl.org/olia/tcodex.owl#top -->

    <owl:NamedIndividual rdf:about="http://purl.org/olia/tcodex.owl#top">
        <rdf:type rdf:resource="http://purl.org/olia/tcodex.owl#Topic"/>
        <system:hasTag>TOP</system:hasTag>
    </owl:NamedIndividual>
    


    <!-- http://purl.org/olia/tcodex.owl#v -->

    <owl:NamedIndividual rdf:about="http://purl.org/olia/tcodex.owl#v">
        <rdf:type rdf:resource="http://purl.org/olia/tcodex.owl#MainVerb"/>
        <system:hasTag>V</system:hasTag>
    </owl:NamedIndividual>
    


    <!-- http://purl.org/olia/tcodex.owl#vfin -->

    <owl:NamedIndividual rdf:about="http://purl.org/olia/tcodex.owl#vfin">
        <rdf:type rdf:resource="http://purl.org/olia/tcodex.owl#FiniteVerb"/>
        <system:hasTag>VFIN</system:hasTag>
    </owl:NamedIndividual>
    


    <!-- http://purl.org/olia/tcodex.owl#vn -->

    <owl:NamedIndividual rdf:about="http://purl.org/olia/tcodex.owl#vn">
        <rdf:type rdf:resource="http://purl.org/olia/tcodex.owl#VerbalNoun"/>
        <system:hasTag>VN</system:hasTag>
    </owl:NamedIndividual>
    


    <!-- http://purl.org/olia/tcodex.owl#voc -->

    <owl:NamedIndividual rdf:about="http://purl.org/olia/tcodex.owl#voc">
        <rdf:type rdf:resource="http://purl.org/olia/tcodex.owl#VocativeForm"/>
        <system:hasTag>VOC</system:hasTag>
    </owl:NamedIndividual>
    


    <!-- http://purl.org/olia/tcodex.owl#vp -->

    <owl:NamedIndividual rdf:about="http://purl.org/olia/tcodex.owl#vp">
        <rdf:type rdf:resource="http://purl.org/olia/tcodex.owl#VerbalPhrase"/>
        <system:hasTag>VP</system:hasTag>
    </owl:NamedIndividual>
    


    <!-- http://purl.org/olia/tcodex.owl#wh -->

    <owl:NamedIndividual rdf:about="http://purl.org/olia/tcodex.owl#wh">
        <rdf:type rdf:resource="http://purl.org/olia/tcodex.owl#QuestionWord"/>
        <system:hasTag>WH</system:hasTag>
    </owl:NamedIndividual>
</rdf:RDF>



<!-- Generated by the OWL API (version 4.5.25.2023-02-15T19:15:49Z) https://github.com/owlcs/owlapi -->

