<?xml version="1.0"?>
<rdf:RDF xmlns="http://purl.org/olia/urdu.owl#"
     xml:base="http://purl.org/olia/urdu.owl"
     xmlns:ms="http://w3id.org/meta-share/meta-share/"
     xmlns:dct="http://purl.org/dc/terms/"
     xmlns:owl="http://www.w3.org/2002/07/owl#"
     xmlns:rdf="http://www.w3.org/1999/02/22-rdf-syntax-ns#"
     xmlns:xml="http://www.w3.org/XML/1998/namespace"
     xmlns:xsd="http://www.w3.org/2001/XMLSchema#"
     xmlns:rdfs="http://www.w3.org/2000/01/rdf-schema#"
     xmlns:urdu="http://purl.org/olia/urdu.owl#"
     xmlns:system="http://purl.org/olia/system.owl#">
    <owl:Ontology rdf:about="http://purl.org/olia/urdu.owl">
        <owl:imports rdf:resource="http://purl.org/olia/system.owl"/>
        <dct:license rdf:resource="https://creativecommons.org/licenses/by/3.0/"/>
        <ms:language rdf:resource="http://lexvo.org/id/iso639-3/urd"/>
        <rdfs:comment>OLiA annotation model for morphosyntactic and morphological annotations of Urdu following Sajjad (2007). Unless marked otherwise, all coments are quoted from this document.

Hassan Sajjad (2007), Urdu Part of Speech Tagset, version 1.0.0.0, 07-12-2007, Center for research in Urdu Language Processing. National University of Computer and Emerging Sciences, Lahore, Pakistan, http://www.crulp.org/Downloads/langproc/UrduPOStagger/UrduPOStagset.pdf</rdfs:comment>
        <rdfs:isDefinedBy>http://www.crulp.org/Downloads/langproc/UrduPOStagger/UrduPOStagset.pdf</rdfs:isDefinedBy>
        <owl:versionInfo>2011-07-28 created

Note: encoding errors when copying Arabic letters from PDF, hence, no examples.

Christian Chiarcos, chiarcos@uni-potsdam.de</owl:versionInfo>
    </owl:Ontology>
    


    <!-- 
    ///////////////////////////////////////////////////////////////////////////////////////
    //
    // Annotation properties
    //
    ///////////////////////////////////////////////////////////////////////////////////////
     -->

    


    <!-- http://w3id.org/meta-share/meta-share/language -->

    <owl:AnnotationProperty rdf:about="http://w3id.org/meta-share/meta-share/language"/>
    


    <!-- 
    ///////////////////////////////////////////////////////////////////////////////////////
    //
    // Classes
    //
    ///////////////////////////////////////////////////////////////////////////////////////
     -->

    


    <!-- http://purl.org/olia/urdu.owl#AdjectivalParticle -->

    <owl:Class rdf:about="http://purl.org/olia/urdu.owl#AdjectivalParticle">
        <rdfs:subClassOf rdf:resource="http://purl.org/olia/urdu.owl#PartOfSpeech"/>
        <rdfs:comment>Adjectival particle (A):
This category includes only one word sa with its two inflection forms. This particle is normally
used for comparison.</rdfs:comment>
    </owl:Class>
    


    <!-- http://purl.org/olia/urdu.owl#Adjective -->

    <owl:Class rdf:about="http://purl.org/olia/urdu.owl#Adjective">
        <rdfs:subClassOf rdf:resource="http://purl.org/olia/urdu.owl#PartOfSpeech"/>
        <rdfs:comment>Adjective (ADJ):
Adjectives are catered as one category. The information related to the degree of adjective is not
taken into account.</rdfs:comment>
    </owl:Class>
    


    <!-- http://purl.org/olia/urdu.owl#Adverb -->

    <owl:Class rdf:about="http://purl.org/olia/urdu.owl#Adverb">
        <rdfs:subClassOf rdf:resource="http://purl.org/olia/urdu.owl#PartOfSpeech"/>
        <rdfs:comment>Adverb (ADV):
Adverbs are handled as one category in the tagset. Consider the following examples of adverbs.</rdfs:comment>
    </owl:Class>
    


    <!-- http://purl.org/olia/urdu.owl#AdverbialDemonstrative -->

    <owl:Class rdf:about="http://purl.org/olia/urdu.owl#AdverbialDemonstrative">
        <rdfs:subClassOf rdf:resource="http://purl.org/olia/urdu.owl#Demonstrative"/>
    </owl:Class>
    


    <!-- http://purl.org/olia/urdu.owl#AdverbialKafPronoun -->

    <owl:Class rdf:about="http://purl.org/olia/urdu.owl#AdverbialKafPronoun">
        <rdfs:subClassOf rdf:resource="http://purl.org/olia/urdu.owl#Pronoun"/>
        <rdfs:comment>Kaf pronouns add interrogative property in the sentence. They are divided into two categories.
Kaf pronouns, represented by KP, are used to ask question about a noun. The second category
includes adverbial kaf pronouns which are used at the place of nouns with adverbial nature.</rdfs:comment>
    </owl:Class>
    


    <!-- http://purl.org/olia/urdu.owl#AdverbialPronoun -->

    <owl:Class rdf:about="http://purl.org/olia/urdu.owl#AdverbialPronoun">
        <rdfs:subClassOf rdf:resource="http://purl.org/olia/urdu.owl#Pronoun"/>
        <rdfs:comment>The adverbial pronouns occur at the place of nouns with adverbial nature and show the property
of time, place, manner, etc. They are represented by AP in the tagset.</rdfs:comment>
    </owl:Class>
    


    <!-- http://purl.org/olia/urdu.owl#AspectualAuxiliary -->

    <owl:Class rdf:about="http://purl.org/olia/urdu.owl#AspectualAuxiliary">
        <rdfs:subClassOf rdf:resource="http://purl.org/olia/urdu.owl#Auxiliary"/>
    </owl:Class>
    


    <!-- http://purl.org/olia/urdu.owl#Auxiliary -->

    <owl:Class rdf:about="http://purl.org/olia/urdu.owl#Auxiliary">
        <rdfs:subClassOf rdf:resource="http://purl.org/olia/urdu.owl#PartOfSpeech"/>
        <rdfs:comment>Auxiliaries:
Based on the syntactic nature of language, auxiliaries are divided into two categories. Aspectual
auxiliaries always occur after main verb of the sentence. Tense auxiliaries are used to show the
time of the action. They occurred at the end of the verb phrase.</rdfs:comment>
    </owl:Class>
    


    <!-- http://purl.org/olia/urdu.owl#CardinalNumeral -->

    <owl:Class rdf:about="http://purl.org/olia/urdu.owl#CardinalNumeral">
        <rdfs:subClassOf rdf:resource="http://purl.org/olia/urdu.owl#Numeral"/>
    </owl:Class>
    


    <!-- http://purl.org/olia/urdu.owl#Conjunction -->

    <owl:Class rdf:about="http://purl.org/olia/urdu.owl#Conjunction">
        <rdfs:subClassOf rdf:resource="http://purl.org/olia/urdu.owl#PartOfSpeech"/>
        <rdfs:comment>Conjunction:
Conjunctions are divided into coordinating and subordinating conjunctions.</rdfs:comment>
    </owl:Class>
    


    <!-- http://purl.org/olia/urdu.owl#CoordinatingConjunction -->

    <owl:Class rdf:about="http://purl.org/olia/urdu.owl#CoordinatingConjunction">
        <rdfs:subClassOf rdf:resource="http://purl.org/olia/urdu.owl#Conjunction"/>
    </owl:Class>
    


    <!-- http://purl.org/olia/urdu.owl#Date -->

    <owl:Class rdf:about="http://purl.org/olia/urdu.owl#Date">
        <rdfs:subClassOf rdf:resource="http://purl.org/olia/urdu.owl#PartOfSpeech"/>
        <rdfs:comment>Date, e.g., 2007, 1999</rdfs:comment>
    </owl:Class>
    


    <!-- http://purl.org/olia/urdu.owl#Demonstrative -->

    <owl:Class rdf:about="http://purl.org/olia/urdu.owl#Demonstrative">
        <rdfs:subClassOf rdf:resource="http://purl.org/olia/urdu.owl#PartOfSpeech"/>
        <rdfs:comment>Demonstratives are divided into four categories. All four categories of demonstratives have
ambiguity with four categories of pronoun. Phrase level analysis was done to distinguish
between demonstrative and pronoun.</rdfs:comment>
    </owl:Class>
    


    <!-- http://purl.org/olia/urdu.owl#Expression -->

    <owl:Class rdf:about="http://purl.org/olia/urdu.owl#Expression">
        <rdfs:subClassOf rdf:resource="http://purl.org/olia/urdu.owl#PartOfSpeech"/>
        <rdfs:comment>Expression (Exp):
Any word or symbol which is not handled in this tagset will be catered under expression. It can
be mathematical symbols, digits, etc.</rdfs:comment>
    </owl:Class>
    


    <!-- http://purl.org/olia/urdu.owl#FractionalNumeral -->

    <owl:Class rdf:about="http://purl.org/olia/urdu.owl#FractionalNumeral">
        <rdfs:subClassOf rdf:resource="http://purl.org/olia/urdu.owl#Numeral"/>
    </owl:Class>
    


    <!-- http://purl.org/olia/urdu.owl#Genitive -->

    <owl:Class rdf:about="http://purl.org/olia/urdu.owl#Genitive">
        <rdfs:subClassOf rdf:resource="http://purl.org/olia/urdu.owl#PartOfSpeech"/>
    </owl:Class>
    


    <!-- http://purl.org/olia/urdu.owl#GenitiveReflexive -->

    <owl:Class rdf:about="http://purl.org/olia/urdu.owl#GenitiveReflexive">
        <rdfs:subClassOf rdf:resource="http://purl.org/olia/urdu.owl#PartOfSpeech"/>
    </owl:Class>
    


    <!-- http://purl.org/olia/urdu.owl#Intensifier -->

    <owl:Class rdf:about="http://purl.org/olia/urdu.owl#Intensifier">
        <rdfs:subClassOf rdf:resource="http://purl.org/olia/urdu.owl#PartOfSpeech"/>
        <rdfs:comment>Intensifier (I):
There are only three words in this category</rdfs:comment>
    </owl:Class>
    


    <!-- http://purl.org/olia/urdu.owl#Interjection -->

    <owl:Class rdf:about="http://purl.org/olia/urdu.owl#Interjection">
        <rdfs:subClassOf rdf:resource="http://purl.org/olia/urdu.owl#PartOfSpeech"/>
        <rdfs:comment>Interjection (INT):
Interjections normally occur at the start of the sentence. They are kept as separate category in
the tagset.</rdfs:comment>
    </owl:Class>
    


    <!-- http://purl.org/olia/urdu.owl#KERParticle -->

    <owl:Class rdf:about="http://purl.org/olia/urdu.owl#KERParticle">
        <rdfs:subClassOf rdf:resource="http://purl.org/olia/urdu.owl#PartOfSpeech"/>
        <rdfs:comment>KER particle (KER):
These particles normally occur in verb phrase. There are only two entities in this class.</rdfs:comment>
    </owl:Class>
    


    <!-- http://purl.org/olia/urdu.owl#KafDemonstrative -->

    <owl:Class rdf:about="http://purl.org/olia/urdu.owl#KafDemonstrative">
        <rdfs:subClassOf rdf:resource="http://purl.org/olia/urdu.owl#Demonstrative"/>
    </owl:Class>
    


    <!-- http://purl.org/olia/urdu.owl#KafPronoun -->

    <owl:Class rdf:about="http://purl.org/olia/urdu.owl#KafPronoun">
        <rdfs:subClassOf rdf:resource="http://purl.org/olia/urdu.owl#Pronoun"/>
        <rdfs:comment>Kaf pronouns add interrogative property in the sentence. They are divided into two categories.
Kaf pronouns, represented by KP, are used to ask question about a noun. The second category
includes adverbial kaf pronouns which are used at the place of nouns with adverbial nature.</rdfs:comment>
    </owl:Class>
    


    <!-- http://purl.org/olia/urdu.owl#MeasuringUnit -->

    <owl:Class rdf:about="http://purl.org/olia/urdu.owl#MeasuringUnit">
        <rdfs:subClassOf rdf:resource="http://purl.org/olia/urdu.owl#PartOfSpeech"/>
        <rdfs:comment>Measuring unit (U):
They are frequently used with numerals. However, they have a different syntactic structure than
numerals.</rdfs:comment>
    </owl:Class>
    


    <!-- http://purl.org/olia/urdu.owl#MultiplicativeNumeral -->

    <owl:Class rdf:about="http://purl.org/olia/urdu.owl#MultiplicativeNumeral">
        <rdfs:subClassOf rdf:resource="http://purl.org/olia/urdu.owl#Numeral"/>
    </owl:Class>
    


    <!-- http://purl.org/olia/urdu.owl#Negation -->

    <owl:Class rdf:about="http://purl.org/olia/urdu.owl#Negation">
        <rdfs:subClassOf rdf:resource="http://purl.org/olia/urdu.owl#PartOfSpeech"/>
    </owl:Class>
    


    <!-- http://purl.org/olia/urdu.owl#Noun -->

    <owl:Class rdf:about="http://purl.org/olia/urdu.owl#Noun">
        <rdfs:subClassOf rdf:resource="http://purl.org/olia/urdu.owl#PartOfSpeech"/>
        <rdfs:comment>Nouns are divided into two categories. First category consists of simple nouns which are
represented by NN in the tagset. However, there are other nouns that show adverbial nature like
time, place, manner, etc. These are also catered under noun. The proper nouns are kept in a
separate category.</rdfs:comment>
    </owl:Class>
    


    <!-- http://purl.org/olia/urdu.owl#Numeral -->

    <owl:Class rdf:about="http://purl.org/olia/urdu.owl#Numeral">
        <rdfs:subClassOf rdf:resource="http://purl.org/olia/urdu.owl#PartOfSpeech"/>
        <rdfs:comment>Numerals:
Numerals are divided into four categories based on their syntactic structure. Cardinal (CA),
ordinal (OR), fractional (FR) and multiplicative (MUL) are types included in the tagset. Following
are the examples of each category.</rdfs:comment>
    </owl:Class>
    


    <!-- http://purl.org/olia/urdu.owl#OrdinalNumeral -->

    <owl:Class rdf:about="http://purl.org/olia/urdu.owl#OrdinalNumeral">
        <rdfs:subClassOf rdf:resource="http://purl.org/olia/urdu.owl#Numeral"/>
    </owl:Class>
    


    <!-- http://purl.org/olia/urdu.owl#PartOfSpeech -->

    <owl:Class rdf:about="http://purl.org/olia/urdu.owl#PartOfSpeech">
        <rdfs:subClassOf rdf:resource="http://purl.org/olia/system.owl#UnitOfAnnotation"/>
        <rdfs:subClassOf>
            <owl:Restriction>
                <owl:onProperty rdf:resource="http://purl.org/olia/system.owl#hasTier"/>
                <owl:hasValue>POS</owl:hasValue>
            </owl:Restriction>
        </rdfs:subClassOf>
    </owl:Class>
    


    <!-- http://purl.org/olia/urdu.owl#PersonalDemonstrative -->

    <owl:Class rdf:about="http://purl.org/olia/urdu.owl#PersonalDemonstrative">
        <rdfs:subClassOf rdf:resource="http://purl.org/olia/urdu.owl#Demonstrative"/>
        <rdfs:comment>Personal demonstrative (PD)
This category includes the elements of demonstrative and personal demonstratives. </rdfs:comment>
    </owl:Class>
    


    <!-- http://purl.org/olia/urdu.owl#PersonalPronoun -->

    <owl:Class rdf:about="http://purl.org/olia/urdu.owl#PersonalPronoun">
        <rdfs:subClassOf rdf:resource="http://purl.org/olia/urdu.owl#Pronoun"/>
    </owl:Class>
    


    <!-- http://purl.org/olia/urdu.owl#PhraseMarker -->

    <owl:Class rdf:about="http://purl.org/olia/urdu.owl#PhraseMarker">
        <rdfs:subClassOf rdf:resource="http://purl.org/olia/urdu.owl#Punctuation"/>
    </owl:Class>
    


    <!-- http://purl.org/olia/urdu.owl#PostTitle -->

    <owl:Class rdf:about="http://purl.org/olia/urdu.owl#PostTitle">
        <rdfs:subClassOf rdf:resource="http://purl.org/olia/urdu.owl#Title"/>
        <rdfs:comment>Post-title</rdfs:comment>
    </owl:Class>
    


    <!-- http://purl.org/olia/urdu.owl#PreTitle -->

    <owl:Class rdf:about="http://purl.org/olia/urdu.owl#PreTitle">
        <rdfs:subClassOf rdf:resource="http://purl.org/olia/urdu.owl#Title"/>
        <rdfs:comment>Pre-title</rdfs:comment>
    </owl:Class>
    


    <!-- http://purl.org/olia/urdu.owl#Pronoun -->

    <owl:Class rdf:about="http://purl.org/olia/urdu.owl#Pronoun">
        <rdfs:subClassOf rdf:resource="http://purl.org/olia/urdu.owl#PartOfSpeech"/>
        <rdfs:comment>Pronouns are divided into six categories based on their syntactic structure. Most of the
categories are consistent with the types provided by Urdu grammarians. </rdfs:comment>
    </owl:Class>
    


    <!-- http://purl.org/olia/urdu.owl#ProperNoun -->

    <owl:Class rdf:about="http://purl.org/olia/urdu.owl#ProperNoun">
        <rdfs:subClassOf rdf:resource="http://purl.org/olia/urdu.owl#Noun"/>
    </owl:Class>
    


    <!-- http://purl.org/olia/urdu.owl#Punctuation -->

    <owl:Class rdf:about="http://purl.org/olia/urdu.owl#Punctuation">
        <rdfs:subClassOf rdf:resource="http://purl.org/olia/urdu.owl#PartOfSpeech"/>
        <rdfs:comment>Punctuation marks: In this tagset, punctuation marks are divided into two categories. Sentence
markers mark the boundary of the sentence. Phrase markers are used inside the sentence but
never used at the end of sentence.</rdfs:comment>
    </owl:Class>
    


    <!-- http://purl.org/olia/urdu.owl#Quantifier -->

    <owl:Class rdf:about="http://purl.org/olia/urdu.owl#Quantifier">
        <rdfs:subClassOf rdf:resource="http://purl.org/olia/urdu.owl#PartOfSpeech"/>
    </owl:Class>
    


    <!-- http://purl.org/olia/urdu.owl#QuestionWord -->

    <owl:Class rdf:about="http://purl.org/olia/urdu.owl#QuestionWord">
        <rdfs:subClassOf rdf:resource="http://purl.org/olia/urdu.owl#PartOfSpeech"/>
        <rdfs:comment>Question words (QW):
There are some words instead of kaf pronouns that are used for the interrogation in the sentence.
However, these words cannot be replaced by a noun or pronoun. A separate category of question
words has been formed for these words.</rdfs:comment>
    </owl:Class>
    


    <!-- http://purl.org/olia/urdu.owl#ReflexivePronoun -->

    <owl:Class rdf:about="http://purl.org/olia/urdu.owl#ReflexivePronoun">
        <rdfs:subClassOf rdf:resource="http://purl.org/olia/urdu.owl#Pronoun"/>
    </owl:Class>
    


    <!-- http://purl.org/olia/urdu.owl#RelativeDemonstrative -->

    <owl:Class rdf:about="http://purl.org/olia/urdu.owl#RelativeDemonstrative">
        <rdfs:subClassOf rdf:resource="http://purl.org/olia/urdu.owl#Demonstrative"/>
    </owl:Class>
    


    <!-- http://purl.org/olia/urdu.owl#RelativePronoun -->

    <owl:Class rdf:about="http://purl.org/olia/urdu.owl#RelativePronoun">
        <rdfs:subClassOf rdf:resource="http://purl.org/olia/urdu.owl#Pronoun"/>
    </owl:Class>
    


    <!-- http://purl.org/olia/urdu.owl#SemanticMarker -->

    <owl:Class rdf:about="http://purl.org/olia/urdu.owl#SemanticMarker">
        <rdfs:subClassOf rdf:resource="http://purl.org/olia/urdu.owl#PartOfSpeech"/>
        <rdfs:comment>Semantic Marker (P):
Following are the list of particles included into this category. The tag SE is applied to an ambiguous category.</rdfs:comment>
    </owl:Class>
    


    <!-- http://purl.org/olia/urdu.owl#SentenceMarker -->

    <owl:Class rdf:about="http://purl.org/olia/urdu.owl#SentenceMarker">
        <rdfs:subClassOf rdf:resource="http://purl.org/olia/urdu.owl#Punctuation"/>
    </owl:Class>
    


    <!-- http://purl.org/olia/urdu.owl#SimpleNoun -->

    <owl:Class rdf:about="http://purl.org/olia/urdu.owl#SimpleNoun">
        <rdfs:subClassOf rdf:resource="http://purl.org/olia/urdu.owl#Noun"/>
    </owl:Class>
    


    <!-- http://purl.org/olia/urdu.owl#SubordinatingConjunction -->

    <owl:Class rdf:about="http://purl.org/olia/urdu.owl#SubordinatingConjunction">
        <rdfs:subClassOf rdf:resource="http://purl.org/olia/urdu.owl#Conjunction"/>
    </owl:Class>
    


    <!-- http://purl.org/olia/urdu.owl#TenseAuxiliary -->

    <owl:Class rdf:about="http://purl.org/olia/urdu.owl#TenseAuxiliary">
        <rdfs:subClassOf rdf:resource="http://purl.org/olia/urdu.owl#Auxiliary"/>
    </owl:Class>
    


    <!-- http://purl.org/olia/urdu.owl#Title -->

    <owl:Class rdf:about="http://purl.org/olia/urdu.owl#Title">
        <rdfs:subClassOf rdf:resource="http://purl.org/olia/urdu.owl#PartOfSpeech"/>
        <rdfs:comment>Title:
Titles are divided into two categories based on their pre and post occurrence around a proper
noun.</rdfs:comment>
    </owl:Class>
    


    <!-- http://purl.org/olia/urdu.owl#Verb -->

    <owl:Class rdf:about="http://purl.org/olia/urdu.owl#Verb">
        <rdfs:subClassOf rdf:resource="http://purl.org/olia/urdu.owl#PartOfSpeech"/>
        <rdfs:comment>Verb (VB): At sentence level, any word showing action in any form is considered as verb. No
further categorization is done.</rdfs:comment>
    </owl:Class>
    


    <!-- http://purl.org/olia/urdu.owl#Wala -->

    <owl:Class rdf:about="http://purl.org/olia/urdu.owl#Wala">
        <rdfs:subClassOf rdf:resource="http://purl.org/olia/urdu.owl#PartOfSpeech"/>
        <rdfs:comment>Wala (WALA):
        This category contains one word wala and its inflections</rdfs:comment>
        <rdfs:comment>wala expresses generalized possession of the noun it follows.
            
            H والا वाला wālā = H وال वाल wāl [prob. Prk. वालो and वालओ; S. पालः and पालकः; but often confounded with the primary suff. 
            hārā and wālā in ani-hārā or ane-wālā = Ap. Prk. अणिअअडं or अणिअअडअ (with euphonic h or w inserted)=S. अनीय+क+रं, or
            र+कं], suff. (f. -ī), added to subst. to derive nouns implying possession or relation generally;—e.g. go-wāl, or 
            go-wālā, s.m. cow-keeper, cow-herd (fr. go, &apos;cow&apos;);—ghaṭ-wāl, s.m. wharf-keeper, wharfinger (fr. ghāṭ, &apos;landing-place&apos;);
            —nāʼo-wālā, s.m. boat-keeper, boatman (fr. nāʼo, &apos;boat&apos;);—ghar-wālā, s.m. master or owner of the house (fr. ghar, 
            &apos;house&apos;);—kapṛā-wālā, s.m. cloth-man, cloth-merchant (fr. kapṛā, &apos;cloth&apos;);—roṭī-wālā, s.m. bread-man, baker (fr. roṭī, 
            &apos;bread&apos;);—dillī-wālā, belonging to, or a native of, Delhi;—it is even suffixed to foreign words, e.g. bakas-wālā, box-man, 
            pedlar (fr. bakas, &apos;a box&apos;);—it is sometimes used to form adj. fr. subst., e.g. kifāyat-wālā, &apos;economical&apos; (fr. kifāyat, 
            &apos;economy&apos;);—gunjāʼish-wālā, &apos;capacious, spacious, roomy&apos; (fr. gunjāʼish, &apos;capacity&apos;):—The suff. (a)ne-wālā (or ani-hārā) 
            is added to the roots of verbs to form fut. act. part., or nouns of agency, e.g. paṛh-ne-wālā, &apos;one who is going (or is 
            about) to read&apos;; &apos;a reader&apos;;—de-ne-wālā, &apos;who is about to give&apos;; &apos;a giver&apos;;—ho-ne-wālā, &apos;that is about to happen&apos;; &apos;that 
            has yet to come to pass&apos;; &apos;which is yet possible.&apos; 
            
            (Platts, John T. (John Thompson). A dictionary of Urdu, classical Hindi, and English. London: W. H. Allen &amp; Co., 1884, http://dsal.uchicago.edu/cgi-bin/philologic/contextualize.pl?p.9.platts.538398)</rdfs:comment>
    </owl:Class>
    


    <!-- 
    ///////////////////////////////////////////////////////////////////////////////////////
    //
    // Individuals
    //
    ///////////////////////////////////////////////////////////////////////////////////////
     -->

    


    <!-- http://purl.org/olia/urdu.owl#A -->

    <owl:NamedIndividual rdf:about="http://purl.org/olia/urdu.owl#A">
        <rdf:type rdf:resource="http://purl.org/olia/urdu.owl#AdjectivalParticle"/>
        <system:hasTag>A</system:hasTag>
    </owl:NamedIndividual>
    


    <!-- http://purl.org/olia/urdu.owl#AA -->

    <owl:NamedIndividual rdf:about="http://purl.org/olia/urdu.owl#AA">
        <rdf:type rdf:resource="http://purl.org/olia/urdu.owl#AspectualAuxiliary"/>
        <system:hasTag>AA</system:hasTag>
    </owl:NamedIndividual>
    


    <!-- http://purl.org/olia/urdu.owl#AD -->

    <owl:NamedIndividual rdf:about="http://purl.org/olia/urdu.owl#AD">
        <rdf:type rdf:resource="http://purl.org/olia/urdu.owl#AdverbialDemonstrative"/>
        <system:hasTag>KD</system:hasTag>
    </owl:NamedIndividual>
    


    <!-- http://purl.org/olia/urdu.owl#ADJ -->

    <owl:NamedIndividual rdf:about="http://purl.org/olia/urdu.owl#ADJ">
        <rdf:type rdf:resource="http://purl.org/olia/urdu.owl#Adjective"/>
        <system:hasTag>ADJ</system:hasTag>
    </owl:NamedIndividual>
    


    <!-- http://purl.org/olia/urdu.owl#ADV -->

    <owl:NamedIndividual rdf:about="http://purl.org/olia/urdu.owl#ADV">
        <rdf:type rdf:resource="http://purl.org/olia/urdu.owl#Adverb"/>
        <system:hasTag>ADV</system:hasTag>
    </owl:NamedIndividual>
    


    <!-- http://purl.org/olia/urdu.owl#AKP -->

    <owl:NamedIndividual rdf:about="http://purl.org/olia/urdu.owl#AKP">
        <rdf:type rdf:resource="http://purl.org/olia/urdu.owl#AdverbialKafPronoun"/>
        <system:hasTag>AKP</system:hasTag>
    </owl:NamedIndividual>
    


    <!-- http://purl.org/olia/urdu.owl#AP -->

    <owl:NamedIndividual rdf:about="http://purl.org/olia/urdu.owl#AP">
        <rdf:type rdf:resource="http://purl.org/olia/urdu.owl#AdverbialPronoun"/>
        <system:hasTag>AP</system:hasTag>
    </owl:NamedIndividual>
    


    <!-- http://purl.org/olia/urdu.owl#CA -->

    <owl:NamedIndividual rdf:about="http://purl.org/olia/urdu.owl#CA">
        <rdf:type rdf:resource="http://purl.org/olia/urdu.owl#CardinalNumeral"/>
        <system:hasTag>CA</system:hasTag>
    </owl:NamedIndividual>
    


    <!-- http://purl.org/olia/urdu.owl#CC -->

    <owl:NamedIndividual rdf:about="http://purl.org/olia/urdu.owl#CC">
        <rdf:type rdf:resource="http://purl.org/olia/urdu.owl#CoordinatingConjunction"/>
        <system:hasTag>CC</system:hasTag>
    </owl:NamedIndividual>
    


    <!-- http://purl.org/olia/urdu.owl#DATE -->

    <owl:NamedIndividual rdf:about="http://purl.org/olia/urdu.owl#DATE">
        <rdf:type rdf:resource="http://purl.org/olia/urdu.owl#Date"/>
        <system:hasTag>DATE</system:hasTag>
    </owl:NamedIndividual>
    


    <!-- http://purl.org/olia/urdu.owl#Exp -->

    <owl:NamedIndividual rdf:about="http://purl.org/olia/urdu.owl#Exp">
        <rdf:type rdf:resource="http://purl.org/olia/urdu.owl#Expression"/>
        <system:hasTag>Exp</system:hasTag>
    </owl:NamedIndividual>
    


    <!-- http://purl.org/olia/urdu.owl#FR -->

    <owl:NamedIndividual rdf:about="http://purl.org/olia/urdu.owl#FR">
        <rdf:type rdf:resource="http://purl.org/olia/urdu.owl#FractionalNumeral"/>
        <system:hasTag>FR</system:hasTag>
    </owl:NamedIndividual>
    


    <!-- http://purl.org/olia/urdu.owl#G -->

    <owl:NamedIndividual rdf:about="http://purl.org/olia/urdu.owl#G">
        <rdf:type rdf:resource="http://purl.org/olia/urdu.owl#Genitive"/>
        <system:hasTag>G</system:hasTag>
    </owl:NamedIndividual>
    


    <!-- http://purl.org/olia/urdu.owl#GR -->

    <owl:NamedIndividual rdf:about="http://purl.org/olia/urdu.owl#GR">
        <rdf:type rdf:resource="http://purl.org/olia/urdu.owl#GenitiveReflexive"/>
        <system:hasTag>GR</system:hasTag>
    </owl:NamedIndividual>
    


    <!-- http://purl.org/olia/urdu.owl#I -->

    <owl:NamedIndividual rdf:about="http://purl.org/olia/urdu.owl#I">
        <rdf:type rdf:resource="http://purl.org/olia/urdu.owl#Intensifier"/>
        <system:hasTag>I</system:hasTag>
    </owl:NamedIndividual>
    


    <!-- http://purl.org/olia/urdu.owl#INT -->

    <owl:NamedIndividual rdf:about="http://purl.org/olia/urdu.owl#INT">
        <rdf:type rdf:resource="http://purl.org/olia/urdu.owl#Interjection"/>
        <system:hasTag>INT</system:hasTag>
    </owl:NamedIndividual>
    


    <!-- http://purl.org/olia/urdu.owl#KD -->

    <owl:NamedIndividual rdf:about="http://purl.org/olia/urdu.owl#KD">
        <rdf:type rdf:resource="http://purl.org/olia/urdu.owl#KafDemonstrative"/>
        <system:hasTag>AD</system:hasTag>
    </owl:NamedIndividual>
    


    <!-- http://purl.org/olia/urdu.owl#KER -->

    <owl:NamedIndividual rdf:about="http://purl.org/olia/urdu.owl#KER">
        <rdf:type rdf:resource="http://purl.org/olia/urdu.owl#KERParticle"/>
        <system:hasTag>KER</system:hasTag>
    </owl:NamedIndividual>
    


    <!-- http://purl.org/olia/urdu.owl#KP -->

    <owl:NamedIndividual rdf:about="http://purl.org/olia/urdu.owl#KP">
        <rdf:type rdf:resource="http://purl.org/olia/urdu.owl#KafPronoun"/>
        <system:hasTag>KP</system:hasTag>
    </owl:NamedIndividual>
    


    <!-- http://purl.org/olia/urdu.owl#MUL -->

    <owl:NamedIndividual rdf:about="http://purl.org/olia/urdu.owl#MUL">
        <rdf:type rdf:resource="http://purl.org/olia/urdu.owl#MultiplicativeNumeral"/>
        <system:hasTag>MUL</system:hasTag>
    </owl:NamedIndividual>
    


    <!-- http://purl.org/olia/urdu.owl#NEG -->

    <owl:NamedIndividual rdf:about="http://purl.org/olia/urdu.owl#NEG">
        <rdf:type rdf:resource="http://purl.org/olia/urdu.owl#Negation"/>
        <system:hasTag>NEG</system:hasTag>
    </owl:NamedIndividual>
    


    <!-- http://purl.org/olia/urdu.owl#NN -->

    <owl:NamedIndividual rdf:about="http://purl.org/olia/urdu.owl#NN">
        <rdf:type rdf:resource="http://purl.org/olia/urdu.owl#SimpleNoun"/>
        <system:hasTag>NN</system:hasTag>
    </owl:NamedIndividual>
    


    <!-- http://purl.org/olia/urdu.owl#OR -->

    <owl:NamedIndividual rdf:about="http://purl.org/olia/urdu.owl#OR">
        <rdf:type rdf:resource="http://purl.org/olia/urdu.owl#OrdinalNumeral"/>
        <system:hasTag>OR</system:hasTag>
    </owl:NamedIndividual>
    


    <!-- http://purl.org/olia/urdu.owl#P -->

    <owl:NamedIndividual rdf:about="http://purl.org/olia/urdu.owl#P">
        <rdf:type rdf:resource="http://purl.org/olia/urdu.owl#SemanticMarker"/>
        <system:hasTag>P</system:hasTag>
    </owl:NamedIndividual>
    


    <!-- http://purl.org/olia/urdu.owl#PD -->

    <owl:NamedIndividual rdf:about="http://purl.org/olia/urdu.owl#PD">
        <rdf:type rdf:resource="http://purl.org/olia/urdu.owl#PersonalDemonstrative"/>
        <system:hasTag>PD</system:hasTag>
    </owl:NamedIndividual>
    


    <!-- http://purl.org/olia/urdu.owl#PM -->

    <owl:NamedIndividual rdf:about="http://purl.org/olia/urdu.owl#PM">
        <rdf:type rdf:resource="http://purl.org/olia/urdu.owl#PhraseMarker"/>
        <system:hasTag>PM</system:hasTag>
    </owl:NamedIndividual>
    


    <!-- http://purl.org/olia/urdu.owl#PN -->

    <owl:NamedIndividual rdf:about="http://purl.org/olia/urdu.owl#PN">
        <rdf:type rdf:resource="http://purl.org/olia/urdu.owl#ProperNoun"/>
        <system:hasTag>PN</system:hasTag>
    </owl:NamedIndividual>
    


    <!-- http://purl.org/olia/urdu.owl#POT -->

    <owl:NamedIndividual rdf:about="http://purl.org/olia/urdu.owl#POT">
        <rdf:type rdf:resource="http://purl.org/olia/urdu.owl#PostTitle"/>
        <system:hasTag>POT</system:hasTag>
    </owl:NamedIndividual>
    


    <!-- http://purl.org/olia/urdu.owl#PP -->

    <owl:NamedIndividual rdf:about="http://purl.org/olia/urdu.owl#PP">
        <rdf:type rdf:resource="http://purl.org/olia/urdu.owl#PersonalPronoun"/>
        <system:hasTag>PP</system:hasTag>
    </owl:NamedIndividual>
    


    <!-- http://purl.org/olia/urdu.owl#PRT -->

    <owl:NamedIndividual rdf:about="http://purl.org/olia/urdu.owl#PRT">
        <rdf:type rdf:resource="http://purl.org/olia/urdu.owl#PreTitle"/>
        <system:hasTag>PRT</system:hasTag>
    </owl:NamedIndividual>
    


    <!-- http://purl.org/olia/urdu.owl#Q -->

    <owl:NamedIndividual rdf:about="http://purl.org/olia/urdu.owl#Q">
        <rdf:type rdf:resource="http://purl.org/olia/urdu.owl#Quantifier"/>
        <system:hasTag>Q</system:hasTag>
    </owl:NamedIndividual>
    


    <!-- http://purl.org/olia/urdu.owl#QW -->

    <owl:NamedIndividual rdf:about="http://purl.org/olia/urdu.owl#QW">
        <rdf:type rdf:resource="http://purl.org/olia/urdu.owl#QuestionWord"/>
        <system:hasTag>QW</system:hasTag>
    </owl:NamedIndividual>
    


    <!-- http://purl.org/olia/urdu.owl#RD -->

    <owl:NamedIndividual rdf:about="http://purl.org/olia/urdu.owl#RD">
        <rdf:type rdf:resource="http://purl.org/olia/urdu.owl#RelativeDemonstrative"/>
        <system:hasTag>RD</system:hasTag>
    </owl:NamedIndividual>
    


    <!-- http://purl.org/olia/urdu.owl#REP -->

    <owl:NamedIndividual rdf:about="http://purl.org/olia/urdu.owl#REP">
        <rdf:type rdf:resource="http://purl.org/olia/urdu.owl#RelativePronoun"/>
        <system:hasTag>REP</system:hasTag>
    </owl:NamedIndividual>
    


    <!-- http://purl.org/olia/urdu.owl#RP -->

    <owl:NamedIndividual rdf:about="http://purl.org/olia/urdu.owl#RP">
        <rdf:type rdf:resource="http://purl.org/olia/urdu.owl#ReflexivePronoun"/>
        <system:hasTag>RP</system:hasTag>
    </owl:NamedIndividual>
    


    <!-- http://purl.org/olia/urdu.owl#SC -->

    <owl:NamedIndividual rdf:about="http://purl.org/olia/urdu.owl#SC">
        <rdf:type rdf:resource="http://purl.org/olia/urdu.owl#SubordinatingConjunction"/>
        <system:hasTag>SC</system:hasTag>
    </owl:NamedIndividual>
    


    <!-- http://purl.org/olia/urdu.owl#SE -->

    <owl:NamedIndividual rdf:about="http://purl.org/olia/urdu.owl#SE">
        <rdf:type rdf:resource="http://purl.org/olia/urdu.owl#SemanticMarker"/>
        <system:hasTag>SE</system:hasTag>
    </owl:NamedIndividual>
    


    <!-- http://purl.org/olia/urdu.owl#SM -->

    <owl:NamedIndividual rdf:about="http://purl.org/olia/urdu.owl#SM">
        <rdf:type rdf:resource="http://purl.org/olia/urdu.owl#SentenceMarker"/>
        <system:hasTag>SM</system:hasTag>
    </owl:NamedIndividual>
    


    <!-- http://purl.org/olia/urdu.owl#TA -->

    <owl:NamedIndividual rdf:about="http://purl.org/olia/urdu.owl#TA">
        <rdf:type rdf:resource="http://purl.org/olia/urdu.owl#TenseAuxiliary"/>
        <system:hasTag>TA</system:hasTag>
    </owl:NamedIndividual>
    


    <!-- http://purl.org/olia/urdu.owl#U -->

    <owl:NamedIndividual rdf:about="http://purl.org/olia/urdu.owl#U">
        <rdf:type rdf:resource="http://purl.org/olia/urdu.owl#MeasuringUnit"/>
        <system:hasTag>U</system:hasTag>
    </owl:NamedIndividual>
    


    <!-- http://purl.org/olia/urdu.owl#VB -->

    <owl:NamedIndividual rdf:about="http://purl.org/olia/urdu.owl#VB">
        <rdf:type rdf:resource="http://purl.org/olia/urdu.owl#Verb"/>
        <system:hasTag>VB</system:hasTag>
    </owl:NamedIndividual>
    


    <!-- http://purl.org/olia/urdu.owl#WALA -->

    <owl:NamedIndividual rdf:about="http://purl.org/olia/urdu.owl#WALA">
        <rdf:type rdf:resource="http://purl.org/olia/urdu.owl#Wala"/>
        <system:hasTag>WALA</system:hasTag>
    </owl:NamedIndividual>
</rdf:RDF>



<!-- Generated by the OWL API (version 4.5.25.2023-02-15T19:15:49Z) https://github.com/owlcs/owlapi -->

